@prefix dc: <http://purl.org/dc/elements/1.1/> .
@prefix : <http://iflastandards.info/ns/fr/frbr/frbrer/frbrer.rdf#> .
@prefix rdfs: <http://www.w3.org/2000/01/rdf-schema#> .
@prefix publications: <http://www.ifla.org/en/publications/> .
@prefix foaf: <http://xmlns.com/foaf/0.1/> .
@prefix xsd: <http://www.w3.org/2001/XMLSchema#> .
@prefix owl: <http://www.w3.org/2002/07/owl#> .
@prefix rdf: <http://www.w3.org/1999/02/22-rdf-syntax-ns#> .
@prefix frbrer: <http://iflastandards.info/ns/fr/frbr/frbrer/> .
@prefix RegAp: <http://metadataregistry.org/uri/profile/RegAp/> .
@prefix skos: <http://www.w3.org/2004/02/skos/core#> .

<http://iflastandards.info/ns/fr/frbr/frbrer/frbrer.rdf> a owl:Ontology ;
	dc:date "2011-03-23"^^xsd:date ;
	dc:contributor "IFLA. FRBR Review Group"^^xsd:token ;
	rdfs:comment "This ontology is based on Functional requirements for bibliographic records, current text, February 2009."^^xsd:string ;
	owl:versionInfo "Version 1.0"^^xsd:string ;
	dc:creator "http://viaf.org/viaf/21647077/"^^xsd:anyURI ;
	owl:versionIRI <http://iflastandards.info/ns/fr/frbr/frbrer/20110323/frbrer.rdf> .

dc:creator a owl:AnnotationProperty .

owl:versionInfo a owl:AnnotationProperty .

dc:contributor a owl:AnnotationProperty .

rdfs:isDefinedBy a owl:AnnotationProperty .

dc:date a owl:AnnotationProperty .

rdfs:label a owl:AnnotationProperty .

rdfs:comment a owl:AnnotationProperty .

dc:title a owl:AnnotationProperty .

frbrer:P2001 a owl:ObjectProperty ;
	rdfs:label "is realized through"@en ;
	rdfs:isDefinedBy <http://iflastandards.info/ns/fr/frbr/frbrer/> ;
	rdfs:domain frbrer:C1001 ;
	rdfs:range frbrer:C1002 ;
	owl:inverseOf frbrer:P2002 ;
	owl:propertyDisjointWith frbrer:P2037 , frbrer:P2096 , frbrer:P2100 , frbrer:P2102 , frbrer:P2104 , frbrer:P2106 , frbrer:P2108 , frbrer:P3001 , frbrer:P3002 , frbrer:P3003 , frbrer:P3004 , frbrer:P3005 , frbrer:P3006 , frbrer:P3007 .

frbrer:P2002 a owl:ObjectProperty ;
	rdfs:label "is realization of"@en ;
	rdfs:isDefinedBy <http://iflastandards.info/ns/fr/frbr/frbrer/> ;
	rdfs:range frbrer:C1001 ;
	rdfs:domain frbrer:C1002 ;
	owl:propertyDisjointWith frbrer:P2038 , frbrer:P2095 , frbrer:P2097 , frbrer:P2099 , frbrer:P2101 , frbrer:P2103 , frbrer:P2105 , frbrer:P2107 , frbrer:P3008 , frbrer:P3009 , frbrer:P3010 , frbrer:P3011 , frbrer:P3012 , frbrer:P3013 , frbrer:P3014 , frbrer:P3015 , frbrer:P3016 , frbrer:P3017 , frbrer:P3018 , frbrer:P3019 .

frbrer:P2003 a owl:ObjectProperty ;
	rdfs:label "is embodied in"@en ;
	rdfs:isDefinedBy <http://iflastandards.info/ns/fr/frbr/frbrer/> ;
	rdfs:domain frbrer:C1002 ;
	rdfs:range frbrer:C1003 ;
	owl:inverseOf frbrer:P2004 ;
	owl:propertyDisjointWith frbrer:P3008 , frbrer:P3009 , frbrer:P3010 , frbrer:P3011 , frbrer:P3012 , frbrer:P3013 , frbrer:P3014 , frbrer:P3015 , frbrer:P3016 , frbrer:P3017 , frbrer:P3018 , frbrer:P3019 .

frbrer:P2004 a owl:ObjectProperty ;
	rdfs:label "is embodiment of"@en ;
	rdfs:isDefinedBy <http://iflastandards.info/ns/fr/frbr/frbrer/> ;
	rdfs:range frbrer:C1002 ;
	rdfs:domain frbrer:C1003 ;
	owl:propertyDisjointWith frbrer:P3020 , frbrer:P3021 , frbrer:P3022 , frbrer:P3023 , frbrer:P3024 , frbrer:P3025 , frbrer:P3026 , frbrer:P3027 , frbrer:P3028 , frbrer:P3029 , frbrer:P3030 , frbrer:P3053 , frbrer:P3054 , frbrer:P3055 , frbrer:P3056 , frbrer:P3057 , frbrer:P3058 .

frbrer:P2005 a owl:ObjectProperty ;
	rdfs:label "is exemplified by"@en ;
	rdfs:isDefinedBy <http://iflastandards.info/ns/fr/frbr/frbrer/> ;
	rdfs:domain frbrer:C1003 ;
	rdfs:range frbrer:C1004 ;
	owl:inverseOf frbrer:P2006 ;
	owl:propertyDisjointWith frbrer:P2094 , frbrer:P3020 , frbrer:P3021 , frbrer:P3022 , frbrer:P3023 , frbrer:P3024 , frbrer:P3025 , frbrer:P3026 , frbrer:P3027 , frbrer:P3028 , frbrer:P3029 , frbrer:P3030 , frbrer:P3053 , frbrer:P3054 , frbrer:P3055 , frbrer:P3056 , frbrer:P3057 , frbrer:P3058 .

frbrer:P2006 a owl:ObjectProperty ;
	rdfs:label "is exemplar of"@en ;
	rdfs:isDefinedBy <http://iflastandards.info/ns/fr/frbr/frbrer/> ;
	rdfs:range frbrer:C1003 ;
	rdfs:domain frbrer:C1004 ;
	owl:propertyDisjointWith frbrer:P3031 , frbrer:P3032 , frbrer:P3033 , frbrer:P3034 , frbrer:P3035 , frbrer:P3036 , frbrer:P3037 , frbrer:P3038 , frbrer:P3052 .

frbrer:P2007 a owl:ObjectProperty ;
	rdfs:label "is created by (corporate body)"@en ;
	rdfs:isDefinedBy <http://iflastandards.info/ns/fr/frbr/frbrer/> ;
	rdfs:domain frbrer:C1001 ;
	rdfs:range frbrer:C1006 ;
	owl:inverseOf frbrer:P2008 ;
	owl:propertyDisjointWith frbrer:P2059 , frbrer:P2060 , frbrer:P2061 , frbrer:P2062 , frbrer:P2063 , frbrer:P2064 , frbrer:P2065 , frbrer:P2066 , frbrer:P2067 , frbrer:P2068 , frbrer:P2069 , frbrer:P2071 , frbrer:P2072 , frbrer:P2073 , frbrer:P2074 , frbrer:P2075 , frbrer:P2076 , frbrer:P2077 , frbrer:P2078 , frbrer:P2079 , frbrer:P2080 , frbrer:P2109 , frbrer:P2110 , frbrer:P3001 , frbrer:P3002 , frbrer:P3003 , frbrer:P3004 , frbrer:P3005 , frbrer:P3006 , frbrer:P3007 , frbrer:P3008 , frbrer:P3009 , frbrer:P3010 , frbrer:P3011 , frbrer:P3012 , frbrer:P3013 , frbrer:P3014 , frbrer:P3015 , frbrer:P3016 , frbrer:P3017 , frbrer:P3018 , frbrer:P3019 .

frbrer:P2008 a owl:ObjectProperty ;
	rdfs:label "is creator (corporate body) of"@en ;
	rdfs:isDefinedBy <http://iflastandards.info/ns/fr/frbr/frbrer/> ;
	rdfs:range frbrer:C1001 ;
	rdfs:domain frbrer:C1006 ;
	owl:propertyDisjointWith frbrer:P3043 , frbrer:P3044 , frbrer:P3045 , frbrer:P3046 , frbrer:P3047 .

frbrer:P2009 a owl:ObjectProperty ;
	rdfs:label "is created by (person)"@en ;
	rdfs:isDefinedBy <http://iflastandards.info/ns/fr/frbr/frbrer/> ;
	rdfs:domain frbrer:C1001 ;
	rdfs:range frbrer:C1005 ;
	owl:inverseOf frbrer:P2010 .

frbrer:P2010 a owl:ObjectProperty ;
	rdfs:label "is creator (person) of"@en ;
	rdfs:isDefinedBy <http://iflastandards.info/ns/fr/frbr/frbrer/> ;
	rdfs:range frbrer:C1001 ;
	rdfs:domain frbrer:C1005 ;
	owl:propertyDisjointWith frbrer:P3039 , frbrer:P3040 , frbrer:P3041 , frbrer:P3042 .

frbrer:P2011 a owl:ObjectProperty ;
	rdfs:label "is realized by (corporate body)"@en ;
	rdfs:isDefinedBy <http://iflastandards.info/ns/fr/frbr/frbrer/> ;
	rdfs:domain frbrer:C1002 ;
	rdfs:range frbrer:C1006 ;
	owl:inverseOf frbrer:P2012 ;
	owl:propertyDisjointWith frbrer:P3008 , frbrer:P3009 , frbrer:P3010 , frbrer:P3011 , frbrer:P3012 , frbrer:P3013 , frbrer:P3014 , frbrer:P3015 , frbrer:P3016 , frbrer:P3017 , frbrer:P3018 , frbrer:P3019 .

frbrer:P2012 a owl:ObjectProperty ;
	rdfs:label "is realizer (corporate body) of"@en ;
	rdfs:isDefinedBy <http://iflastandards.info/ns/fr/frbr/frbrer/> ;
	rdfs:range frbrer:C1002 ;
	rdfs:domain frbrer:C1006 ;
	owl:propertyDisjointWith frbrer:P3043 , frbrer:P3044 , frbrer:P3045 , frbrer:P3046 , frbrer:P3047 .

frbrer:P2013 a owl:ObjectProperty ;
	rdfs:label "is realized by (person)"@en ;
	rdfs:isDefinedBy <http://iflastandards.info/ns/fr/frbr/frbrer/> ;
	rdfs:domain frbrer:C1002 ;
	rdfs:range frbrer:C1005 ;
	owl:inverseOf frbrer:P2014 ;
	owl:propertyDisjointWith frbrer:P3008 , frbrer:P3009 , frbrer:P3010 , frbrer:P3011 , frbrer:P3012 , frbrer:P3013 , frbrer:P3014 , frbrer:P3015 , frbrer:P3016 , frbrer:P3017 , frbrer:P3018 , frbrer:P3019 .

frbrer:P2014 a owl:ObjectProperty ;
	rdfs:label "is realizer (person) of"@en ;
	rdfs:isDefinedBy <http://iflastandards.info/ns/fr/frbr/frbrer/> ;
	rdfs:range frbrer:C1002 ;
	rdfs:domain frbrer:C1005 ;
	owl:propertyDisjointWith frbrer:P3039 , frbrer:P3040 , frbrer:P3041 , frbrer:P3042 .

frbrer:P2015 a owl:ObjectProperty ;
	rdfs:label "is produced by (corporate body)"@en ;
	rdfs:isDefinedBy <http://iflastandards.info/ns/fr/frbr/frbrer/> ;
	rdfs:domain frbrer:C1003 ;
	rdfs:range frbrer:C1006 ;
	owl:inverseOf frbrer:P2016 ;
	owl:propertyDisjointWith frbrer:P3020 , frbrer:P3021 , frbrer:P3022 , frbrer:P3023 , frbrer:P3024 , frbrer:P3025 , frbrer:P3026 , frbrer:P3027 , frbrer:P3028 , frbrer:P3029 , frbrer:P3030 , frbrer:P3053 , frbrer:P3054 , frbrer:P3055 , frbrer:P3056 , frbrer:P3057 , frbrer:P3058 .

frbrer:P2016 a owl:ObjectProperty ;
	rdfs:label "is producer (corporate body) of"@en ;
	rdfs:isDefinedBy <http://iflastandards.info/ns/fr/frbr/frbrer/> ;
	rdfs:range frbrer:C1003 ;
	rdfs:domain frbrer:C1006 ;
	owl:propertyDisjointWith frbrer:P3043 , frbrer:P3044 , frbrer:P3045 , frbrer:P3046 , frbrer:P3047 .

frbrer:P2017 a owl:ObjectProperty ;
	rdfs:label "is produced by (person)"@en ;
	rdfs:isDefinedBy <http://iflastandards.info/ns/fr/frbr/frbrer/> ;
	rdfs:domain frbrer:C1003 ;
	rdfs:range frbrer:C1005 ;
	owl:inverseOf frbrer:P2018 ;
	owl:propertyDisjointWith frbrer:P3020 , frbrer:P3021 , frbrer:P3022 , frbrer:P3023 , frbrer:P3024 , frbrer:P3025 , frbrer:P3026 , frbrer:P3027 , frbrer:P3028 , frbrer:P3029 , frbrer:P3030 , frbrer:P3053 , frbrer:P3054 , frbrer:P3055 , frbrer:P3056 , frbrer:P3057 , frbrer:P3058 .

frbrer:P2018 a owl:ObjectProperty ;
	rdfs:label "is producer (person) of"@en ;
	rdfs:isDefinedBy <http://iflastandards.info/ns/fr/frbr/frbrer/> ;
	rdfs:range frbrer:C1003 ;
	rdfs:domain frbrer:C1005 ;
	owl:propertyDisjointWith frbrer:P3039 , frbrer:P3040 , frbrer:P3041 , frbrer:P3042 .

frbrer:P2019 a owl:ObjectProperty ;
	rdfs:label "is owned by (corporate body)"@en ;
	rdfs:isDefinedBy <http://iflastandards.info/ns/fr/frbr/frbrer/> ;
	rdfs:domain frbrer:C1004 ;
	rdfs:range frbrer:C1006 ;
	owl:inverseOf frbrer:P2020 ;
	owl:propertyDisjointWith frbrer:P3031 , frbrer:P3032 , frbrer:P3033 , frbrer:P3034 , frbrer:P3035 , frbrer:P3036 , frbrer:P3037 , frbrer:P3038 , frbrer:P3052 .

frbrer:P2020 a owl:ObjectProperty ;
	rdfs:label "is owner (corporate body) of"@en ;
	rdfs:isDefinedBy <http://iflastandards.info/ns/fr/frbr/frbrer/> ;
	rdfs:range frbrer:C1004 ;
	rdfs:domain frbrer:C1006 ;
	owl:propertyDisjointWith frbrer:P3043 , frbrer:P3044 , frbrer:P3045 , frbrer:P3046 , frbrer:P3047 .

frbrer:P2021 a owl:ObjectProperty ;
	rdfs:label "is owned by (person)"@en ;
	rdfs:isDefinedBy <http://iflastandards.info/ns/fr/frbr/frbrer/> ;
	rdfs:domain frbrer:C1004 ;
	rdfs:range frbrer:C1005 ;
	owl:inverseOf frbrer:P2022 ;
	owl:propertyDisjointWith frbrer:P3031 , frbrer:P3032 , frbrer:P3033 , frbrer:P3034 , frbrer:P3035 , frbrer:P3036 , frbrer:P3037 , frbrer:P3038 , frbrer:P3052 .

frbrer:P2022 a owl:ObjectProperty ;
	rdfs:label "is owner (person) of"@en ;
	rdfs:isDefinedBy <http://iflastandards.info/ns/fr/frbr/frbrer/> ;
	rdfs:range frbrer:C1004 ;
	rdfs:domain frbrer:C1005 ;
	owl:propertyDisjointWith frbrer:P3039 , frbrer:P3040 , frbrer:P3041 , frbrer:P3042 .

frbrer:P2023 a owl:ObjectProperty ;
	rdfs:label "has as subject (concept)"@en ;
	rdfs:isDefinedBy <http://iflastandards.info/ns/fr/frbr/frbrer/> ;
	rdfs:domain frbrer:C1001 ;
	rdfs:range frbrer:C1007 ;
	owl:inverseOf frbrer:P2024 ;
	owl:propertyDisjointWith frbrer:P3001 , frbrer:P3002 , frbrer:P3003 , frbrer:P3004 , frbrer:P3005 , frbrer:P3006 , frbrer:P3007 .

frbrer:P2024 a owl:ObjectProperty ;
	rdfs:label "is subject (concept) of"@en ;
	rdfs:isDefinedBy <http://iflastandards.info/ns/fr/frbr/frbrer/> ;
	rdfs:range frbrer:C1001 ;
	rdfs:domain frbrer:C1007 .

frbrer:P2025 a owl:ObjectProperty ;
	rdfs:label "has as subject (object)"@en ;
	rdfs:isDefinedBy <http://iflastandards.info/ns/fr/frbr/frbrer/> ;
	rdfs:domain frbrer:C1001 ;
	rdfs:range frbrer:C1008 ;
	owl:inverseOf frbrer:P2026 ;
	owl:propertyDisjointWith frbrer:P3001 , frbrer:P3002 , frbrer:P3003 , frbrer:P3004 , frbrer:P3005 , frbrer:P3006 , frbrer:P3007 .

frbrer:P2026 a owl:ObjectProperty ;
	rdfs:label "is subject (object) of"@en ;
	rdfs:isDefinedBy <http://iflastandards.info/ns/fr/frbr/frbrer/> ;
	rdfs:range frbrer:C1001 ;
	rdfs:domain frbrer:C1008 .

frbrer:P2027 a owl:ObjectProperty ;
	rdfs:label "has as subject (event)"@en ;
	rdfs:isDefinedBy <http://iflastandards.info/ns/fr/frbr/frbrer/> ;
	rdfs:domain frbrer:C1001 ;
	rdfs:range frbrer:C1009 ;
	owl:inverseOf frbrer:P2028 ;
	owl:propertyDisjointWith frbrer:P3001 , frbrer:P3002 , frbrer:P3003 , frbrer:P3004 , frbrer:P3005 , frbrer:P3006 , frbrer:P3007 .

frbrer:P2028 a owl:ObjectProperty ;
	rdfs:label "is subject (event) of"@en ;
	rdfs:isDefinedBy <http://iflastandards.info/ns/fr/frbr/frbrer/> ;
	rdfs:range frbrer:C1001 ;
	rdfs:domain frbrer:C1009 .

frbrer:P2029 a owl:ObjectProperty ;
	rdfs:label "has as subject (place)"@en ;
	rdfs:isDefinedBy <http://iflastandards.info/ns/fr/frbr/frbrer/> ;
	rdfs:domain frbrer:C1001 ;
	rdfs:range frbrer:C1010 ;
	owl:inverseOf frbrer:P2030 ;
	owl:propertyDisjointWith frbrer:P3001 , frbrer:P3002 , frbrer:P3003 , frbrer:P3004 , frbrer:P3005 , frbrer:P3006 , frbrer:P3007 .

frbrer:P2030 a owl:ObjectProperty ;
	rdfs:label "is subject (place) of"@en ;
	rdfs:isDefinedBy <http://iflastandards.info/ns/fr/frbr/frbrer/> ;
	rdfs:range frbrer:C1001 ;
	rdfs:domain frbrer:C1010 .

frbrer:P2031 a owl:ObjectProperty ;
	rdfs:label "has as subject (corporate body)"@en ;
	rdfs:isDefinedBy <http://iflastandards.info/ns/fr/frbr/frbrer/> ;
	rdfs:domain frbrer:C1001 ;
	rdfs:range frbrer:C1006 ;
	owl:inverseOf frbrer:P2032 ;
	owl:propertyDisjointWith frbrer:P3001 , frbrer:P3002 , frbrer:P3003 , frbrer:P3004 , frbrer:P3005 , frbrer:P3006 , frbrer:P3007 .

frbrer:P2032 a owl:ObjectProperty ;
	rdfs:label "is subject (corporate body) of"@en ;
	rdfs:isDefinedBy <http://iflastandards.info/ns/fr/frbr/frbrer/> ;
	rdfs:range frbrer:C1001 ;
	rdfs:domain frbrer:C1006 ;
	owl:propertyDisjointWith frbrer:P3043 , frbrer:P3044 , frbrer:P3045 , frbrer:P3046 , frbrer:P3047 .

frbrer:P2033 a owl:ObjectProperty ;
	rdfs:label "has as subject (person)"@en ;
	rdfs:isDefinedBy <http://iflastandards.info/ns/fr/frbr/frbrer/> ;
	rdfs:domain frbrer:C1001 ;
	rdfs:range frbrer:C1005 ;
	owl:inverseOf frbrer:P2034 ;
	owl:propertyDisjointWith frbrer:P3001 , frbrer:P3002 , frbrer:P3003 , frbrer:P3004 , frbrer:P3005 , frbrer:P3006 , frbrer:P3007 .

frbrer:P2034 a owl:ObjectProperty ;
	rdfs:label "is subject (person) of"@en ;
	rdfs:isDefinedBy <http://iflastandards.info/ns/fr/frbr/frbrer/> ;
	rdfs:range frbrer:C1001 ;
	rdfs:domain frbrer:C1005 ;
	owl:propertyDisjointWith frbrer:P3039 , frbrer:P3040 , frbrer:P3041 , frbrer:P3042 .

frbrer:P2035 a owl:ObjectProperty , owl:AsymmetricProperty ;
	rdfs:label "has as subject (work)"@en ;
	rdfs:isDefinedBy <http://iflastandards.info/ns/fr/frbr/frbrer/> ;
	rdfs:range frbrer:C1001 ;
	rdfs:domain frbrer:C1001 ;
	owl:inverseOf frbrer:P2036 ;
	owl:propertyDisjointWith frbrer:P2036 , frbrer:P2043 , frbrer:P2044 , frbrer:P2045 , frbrer:P2046 , frbrer:P2047 , frbrer:P2049 , frbrer:P2050 , frbrer:P2052 , frbrer:P2053 , frbrer:P2054 , frbrer:P2056 , frbrer:P2057 , frbrer:P2058 , frbrer:P2098 , frbrer:P3001 , frbrer:P3002 , frbrer:P3003 , frbrer:P3004 , frbrer:P3005 , frbrer:P3006 , frbrer:P3007 .

frbrer:P2036 a owl:ObjectProperty , owl:AsymmetricProperty ;
	rdfs:label "is subject (work) of"@en ;
	rdfs:isDefinedBy <http://iflastandards.info/ns/fr/frbr/frbrer/> ;
	rdfs:domain frbrer:C1001 ;
	rdfs:range frbrer:C1001 ;
	owl:propertyDisjointWith frbrer:P2043 , frbrer:P2044 , frbrer:P2045 , frbrer:P2046 , frbrer:P2047 , frbrer:P2049 , frbrer:P2050 , frbrer:P2052 , frbrer:P2053 , frbrer:P2054 , frbrer:P2056 , frbrer:P2057 , frbrer:P2058 , frbrer:P2098 , frbrer:P3001 , frbrer:P3002 , frbrer:P3003 , frbrer:P3004 , frbrer:P3005 , frbrer:P3006 , frbrer:P3007 .

frbrer:P2037 a owl:ObjectProperty ;
	rdfs:label "has as subject (expression)"@en ;
	rdfs:isDefinedBy <http://iflastandards.info/ns/fr/frbr/frbrer/> ;
	rdfs:domain frbrer:C1001 ;
	rdfs:range frbrer:C1002 ;
	owl:inverseOf frbrer:P2038 ;
	owl:propertyDisjointWith frbrer:P2096 , frbrer:P2100 , frbrer:P2102 , frbrer:P2104 , frbrer:P2106 , frbrer:P2108 , frbrer:P3001 , frbrer:P3002 , frbrer:P3003 , frbrer:P3004 , frbrer:P3005 , frbrer:P3006 , frbrer:P3007 .

frbrer:P2038 a owl:ObjectProperty ;
	rdfs:label "is subject (expression) of"@en ;
	rdfs:isDefinedBy <http://iflastandards.info/ns/fr/frbr/frbrer/> ;
	rdfs:range frbrer:C1001 ;
	rdfs:domain frbrer:C1002 ;
	owl:propertyDisjointWith frbrer:P2095 , frbrer:P2097 , frbrer:P2099 , frbrer:P2101 , frbrer:P2103 , frbrer:P2105 , frbrer:P2107 , frbrer:P3008 , frbrer:P3009 , frbrer:P3010 , frbrer:P3011 , frbrer:P3012 , frbrer:P3013 , frbrer:P3014 , frbrer:P3015 , frbrer:P3016 , frbrer:P3017 , frbrer:P3018 , frbrer:P3019 .

frbrer:P2039 a owl:ObjectProperty ;
	rdfs:label "has as subject (manifestation)"@en ;
	rdfs:isDefinedBy <http://iflastandards.info/ns/fr/frbr/frbrer/> ;
	rdfs:domain frbrer:C1001 ;
	rdfs:range frbrer:C1003 ;
	owl:inverseOf frbrer:P2040 ;
	owl:propertyDisjointWith frbrer:P3001 , frbrer:P3002 , frbrer:P3003 , frbrer:P3004 , frbrer:P3005 , frbrer:P3006 , frbrer:P3007 .

frbrer:P2040 a owl:ObjectProperty ;
	rdfs:label "is subject (manifestation) of"@en ;
	rdfs:isDefinedBy <http://iflastandards.info/ns/fr/frbr/frbrer/> ;
	rdfs:range frbrer:C1001 ;
	rdfs:domain frbrer:C1003 ;
	owl:propertyDisjointWith frbrer:P3020 , frbrer:P3021 , frbrer:P3022 , frbrer:P3023 , frbrer:P3024 , frbrer:P3025 , frbrer:P3026 , frbrer:P3027 , frbrer:P3028 , frbrer:P3029 , frbrer:P3030 , frbrer:P3053 , frbrer:P3054 , frbrer:P3055 , frbrer:P3056 , frbrer:P3057 , frbrer:P3058 .

frbrer:P2041 a owl:ObjectProperty ;
	rdfs:label "has as subject (item)"@en ;
	rdfs:isDefinedBy <http://iflastandards.info/ns/fr/frbr/frbrer/> ;
	rdfs:domain frbrer:C1001 ;
	rdfs:range frbrer:C1004 ;
	owl:inverseOf frbrer:P2042 ;
	owl:propertyDisjointWith frbrer:P3001 , frbrer:P3002 , frbrer:P3003 , frbrer:P3004 , frbrer:P3005 , frbrer:P3006 , frbrer:P3007 .

frbrer:P2042 a owl:ObjectProperty ;
	rdfs:label "is subject (item) of"@en ;
	rdfs:isDefinedBy <http://iflastandards.info/ns/fr/frbr/frbrer/> ;
	rdfs:range frbrer:C1001 ;
	rdfs:domain frbrer:C1004 ;
	owl:propertyDisjointWith frbrer:P3031 , frbrer:P3032 , frbrer:P3033 , frbrer:P3034 , frbrer:P3035 , frbrer:P3036 , frbrer:P3037 , frbrer:P3038 , frbrer:P3052 .

frbrer:P2043 a owl:ObjectProperty , owl:AsymmetricProperty , owl:TransitiveProperty ;
	rdfs:label "has a successor (work) (from work)"@en ;
	rdfs:isDefinedBy <http://iflastandards.info/ns/fr/frbr/frbrer/> ;
	rdfs:range frbrer:C1001 ;
	rdfs:domain frbrer:C1001 ;
	owl:inverseOf frbrer:P2044 ;
	owl:propertyDisjointWith frbrer:P2044 , frbrer:P2045 , frbrer:P2046 , frbrer:P2047 , frbrer:P2049 , frbrer:P2050 , frbrer:P2052 , frbrer:P2053 , frbrer:P2054 , frbrer:P2056 , frbrer:P2057 , frbrer:P2058 , frbrer:P2098 , frbrer:P3001 , frbrer:P3002 , frbrer:P3003 , frbrer:P3004 , frbrer:P3005 , frbrer:P3006 , frbrer:P3007 .

frbrer:P2044 a owl:ObjectProperty , owl:AsymmetricProperty , owl:TransitiveProperty ;
	rdfs:label "is a successor (work) to (work)"@en ;
	rdfs:isDefinedBy <http://iflastandards.info/ns/fr/frbr/frbrer/> ;
	rdfs:range frbrer:C1001 ;
	rdfs:domain frbrer:C1001 ;
	owl:propertyDisjointWith frbrer:P2045 , frbrer:P2046 , frbrer:P2047 , frbrer:P2049 , frbrer:P2050 , frbrer:P2052 , frbrer:P2053 , frbrer:P2054 , frbrer:P2056 , frbrer:P2057 , frbrer:P2058 , frbrer:P2098 , frbrer:P3001 , frbrer:P3002 , frbrer:P3003 , frbrer:P3004 , frbrer:P3005 , frbrer:P3006 , frbrer:P3007 .

frbrer:P2045 a owl:ObjectProperty , owl:AsymmetricProperty ;
	rdfs:label "has a supplement (work) (from work)"@en ;
	rdfs:isDefinedBy <http://iflastandards.info/ns/fr/frbr/frbrer/> ;
	rdfs:domain frbrer:C1001 ;
	rdfs:range frbrer:C1001 ;
	owl:propertyDisjointWith frbrer:P2046 ;
	owl:inverseOf frbrer:P2046 ;
	owl:propertyDisjointWith frbrer:P2047 , frbrer:P2049 , frbrer:P2050 , frbrer:P2052 , frbrer:P2053 , frbrer:P2054 , frbrer:P2056 , frbrer:P2057 , frbrer:P2058 , frbrer:P2098 , frbrer:P3001 , frbrer:P3002 , frbrer:P3003 , frbrer:P3004 , frbrer:P3005 , frbrer:P3006 , frbrer:P3007 .

frbrer:P2046 a owl:ObjectProperty , owl:AsymmetricProperty ;
	rdfs:label "supplements (work) (from work)"@en ;
	rdfs:isDefinedBy <http://iflastandards.info/ns/fr/frbr/frbrer/> ;
	rdfs:domain frbrer:C1001 ;
	rdfs:range frbrer:C1001 ;
	owl:propertyDisjointWith frbrer:P2047 , frbrer:P2049 , frbrer:P2050 , frbrer:P2052 , frbrer:P2053 , frbrer:P2054 , frbrer:P2056 , frbrer:P2057 , frbrer:P2058 , frbrer:P2098 .

frbrer:P2047 a owl:ObjectProperty ;
	rdfs:label "has a complement (work) (from work)"@en ;
	rdfs:isDefinedBy <http://iflastandards.info/ns/fr/frbr/frbrer/> ;
	rdfs:range frbrer:C1001 ;
	rdfs:domain frbrer:C1001 ;
	owl:inverseOf frbrer:P2048 ;
	owl:propertyDisjointWith frbrer:P2049 , frbrer:P2050 , frbrer:P2052 , frbrer:P2053 , frbrer:P2054 , frbrer:P2056 , frbrer:P2057 , frbrer:P2058 , frbrer:P2098 , frbrer:P3001 , frbrer:P3002 , frbrer:P3003 , frbrer:P3004 , frbrer:P3005 , frbrer:P3006 , frbrer:P3007 .

frbrer:P2048 a owl:ObjectProperty ;
	rdfs:label "complements (work) (from work)"@en ;
	rdfs:isDefinedBy <http://iflastandards.info/ns/fr/frbr/frbrer/> ;
	rdfs:domain frbrer:C1001 ;
	rdfs:range frbrer:C1001 ;
	owl:propertyDisjointWith frbrer:P3001 , frbrer:P3002 , frbrer:P3003 , frbrer:P3004 , frbrer:P3005 , frbrer:P3006 , frbrer:P3007 .

frbrer:P2049 a owl:ObjectProperty , owl:AsymmetricProperty ;
	rdfs:label "has a summary (work) (from work)"@en ;
	rdfs:isDefinedBy <http://iflastandards.info/ns/fr/frbr/frbrer/> ;
	rdfs:domain frbrer:C1001 ;
	rdfs:range frbrer:C1001 ;
	owl:inverseOf frbrer:P2050 ;
	owl:propertyDisjointWith frbrer:P2050 , frbrer:P2052 , frbrer:P2053 , frbrer:P2054 , frbrer:P2056 , frbrer:P2057 , frbrer:P2058 , frbrer:P2098 , frbrer:P3001 , frbrer:P3002 , frbrer:P3003 , frbrer:P3004 , frbrer:P3005 , frbrer:P3006 , frbrer:P3007 .

frbrer:P2050 a owl:ObjectProperty , owl:AsymmetricProperty ;
	rdfs:label "is a summary (work) of (work)"@en ;
	rdfs:isDefinedBy <http://iflastandards.info/ns/fr/frbr/frbrer/> ;
	rdfs:domain frbrer:C1001 ;
	rdfs:range frbrer:C1001 ;
	owl:propertyDisjointWith frbrer:P2052 , frbrer:P2053 , frbrer:P2054 , frbrer:P2056 , frbrer:P2057 , frbrer:P2058 , frbrer:P2098 , frbrer:P3001 , frbrer:P3002 , frbrer:P3003 , frbrer:P3004 , frbrer:P3005 , frbrer:P3006 , frbrer:P3007 .

frbrer:P2051 a owl:ObjectProperty , owl:AsymmetricProperty ;
	rdfs:label "has an adaptation (work) (from work)"@en ;
	rdfs:comment "Source documentation has label \"has adaptation\"; amended to improve consistency."@en ;
	rdfs:isDefinedBy <http://iflastandards.info/ns/fr/frbr/frbrer/> ;
	rdfs:range frbrer:C1001 ;
	rdfs:domain frbrer:C1001 ;
	owl:inverseOf frbrer:P2052 ;
	owl:propertyDisjointWith frbrer:P3001 , frbrer:P3002 , frbrer:P3003 , frbrer:P3004 , frbrer:P3005 , frbrer:P3006 , frbrer:P3007 .

frbrer:P2052 a owl:ObjectProperty , owl:AsymmetricProperty ;
	rdfs:label "is an adaptation (work) of (work)"@en ;
	rdfs:isDefinedBy <http://iflastandards.info/ns/fr/frbr/frbrer/> ;
	rdfs:range frbrer:C1001 ;
	rdfs:domain frbrer:C1001 ;
	owl:propertyDisjointWith frbrer:P2053 , frbrer:P2054 , frbrer:P2056 , frbrer:P2057 , frbrer:P2058 , frbrer:P2098 , frbrer:P3001 , frbrer:P3002 , frbrer:P3003 , frbrer:P3004 , frbrer:P3005 , frbrer:P3006 , frbrer:P3007 .

frbrer:P2053 a owl:ObjectProperty , owl:AsymmetricProperty , owl:TransitiveProperty ;
	rdfs:label "has a transformation (work) (from work)"@en ;
	rdfs:comment "Source documentation has \"literary genre\", but other genres allowed."@en ;
	rdfs:isDefinedBy <http://iflastandards.info/ns/fr/frbr/frbrer/> ;
	rdfs:domain frbrer:C1001 ;
	rdfs:range frbrer:C1001 ;
	owl:inverseOf frbrer:P2054 ;
	owl:propertyDisjointWith frbrer:P2054 , frbrer:P2056 , frbrer:P2057 , frbrer:P2058 , frbrer:P2098 , frbrer:P3001 , frbrer:P3002 , frbrer:P3003 , frbrer:P3004 , frbrer:P3005 , frbrer:P3006 , frbrer:P3007 .

frbrer:P2054 a owl:ObjectProperty , owl:AsymmetricProperty , owl:TransitiveProperty ;
	rdfs:label "is a transformation (work) of (work)"@en ;
	rdfs:comment "Source documentation has \"literary genre\", but other genres allowed."@en ;
	rdfs:isDefinedBy <http://iflastandards.info/ns/fr/frbr/frbrer/> ;
	rdfs:range frbrer:C1001 ;
	rdfs:domain frbrer:C1001 ;
	owl:propertyDisjointWith frbrer:P2056 , frbrer:P2057 , frbrer:P2058 , frbrer:P2098 , frbrer:P3001 , frbrer:P3002 , frbrer:P3003 , frbrer:P3004 , frbrer:P3005 , frbrer:P3006 , frbrer:P3007 .

frbrer:P2055 a owl:ObjectProperty , owl:AsymmetricProperty ;
	rdfs:label "has an imitation (work) (from work)"@en ;
	rdfs:isDefinedBy <http://iflastandards.info/ns/fr/frbr/frbrer/> ;
	rdfs:domain frbrer:C1001 ;
	rdfs:range frbrer:C1001 ;
	owl:inverseOf frbrer:P2056 ;
	owl:propertyDisjointWith frbrer:P3001 , frbrer:P3002 , frbrer:P3003 , frbrer:P3004 , frbrer:P3005 , frbrer:P3006 , frbrer:P3007 .

frbrer:P2056 a owl:ObjectProperty , owl:AsymmetricProperty ;
	rdfs:label "is an imitation (work) of (work)"@en ;
	rdfs:isDefinedBy <http://iflastandards.info/ns/fr/frbr/frbrer/> ;
	rdfs:range frbrer:C1001 ;
	rdfs:domain frbrer:C1001 ;
	owl:propertyDisjointWith frbrer:P2057 , frbrer:P2058 , frbrer:P2098 , frbrer:P3001 , frbrer:P3002 , frbrer:P3003 , frbrer:P3004 , frbrer:P3005 , frbrer:P3006 , frbrer:P3007 .

frbrer:P2057 a owl:ObjectProperty , owl:AsymmetricProperty , owl:TransitiveProperty ;
	rdfs:label "has part (work)"@en ;
	rdfs:isDefinedBy <http://iflastandards.info/ns/fr/frbr/frbrer/> ;
	rdfs:range frbrer:C1001 ;
	rdfs:domain frbrer:C1001 ;
	owl:propertyDisjointWith frbrer:P2058 ;
	owl:inverseOf frbrer:P2058 ;
	owl:propertyDisjointWith frbrer:P2098 , frbrer:P3001 , frbrer:P3002 , frbrer:P3003 , frbrer:P3004 , frbrer:P3005 , frbrer:P3006 , frbrer:P3007 .

frbrer:P2058 a owl:ObjectProperty , owl:AsymmetricProperty , owl:TransitiveProperty ;
	rdfs:label "is part (work) of"@en ;
	rdfs:isDefinedBy <http://iflastandards.info/ns/fr/frbr/frbrer/> ;
	rdfs:domain frbrer:C1001 ;
	rdfs:range frbrer:C1001 ;
	owl:propertyDisjointWith frbrer:P2098 , frbrer:P3001 , frbrer:P3002 , frbrer:P3003 , frbrer:P3004 , frbrer:P3005 , frbrer:P3006 , frbrer:P3007 .

frbrer:P2059 a owl:ObjectProperty , owl:AsymmetricProperty ;
	rdfs:label "has an abridgement (expression)"@en ;
	rdfs:isDefinedBy <http://iflastandards.info/ns/fr/frbr/frbrer/> ;
	rdfs:domain frbrer:C1002 ;
	rdfs:range frbrer:C1002 ;
	owl:inverseOf frbrer:P2060 ;
	owl:propertyDisjointWith frbrer:P2060 , frbrer:P2061 , frbrer:P2062 , frbrer:P2063 , frbrer:P2064 , frbrer:P2065 , frbrer:P2066 , frbrer:P2067 , frbrer:P2068 , frbrer:P2069 , frbrer:P2071 , frbrer:P2072 , frbrer:P2073 , frbrer:P2074 , frbrer:P2075 , frbrer:P2076 , frbrer:P2077 , frbrer:P2078 , frbrer:P2079 , frbrer:P2080 , frbrer:P2109 , frbrer:P2110 , frbrer:P3008 , frbrer:P3009 , frbrer:P3010 , frbrer:P3011 , frbrer:P3012 , frbrer:P3013 , frbrer:P3014 , frbrer:P3015 , frbrer:P3016 , frbrer:P3017 , frbrer:P3018 , frbrer:P3019 .

frbrer:P2060 a owl:ObjectProperty , owl:AsymmetricProperty ;
	rdfs:label "is an abridgement (expression) of"@en ;
	rdfs:isDefinedBy <http://iflastandards.info/ns/fr/frbr/frbrer/> ;
	rdfs:range frbrer:C1002 ;
	rdfs:domain frbrer:C1002 ;
	owl:propertyDisjointWith frbrer:P2061 , frbrer:P2062 , frbrer:P2063 , frbrer:P2064 , frbrer:P2065 , frbrer:P2066 , frbrer:P2067 , frbrer:P2068 , frbrer:P2069 , frbrer:P2071 , frbrer:P2072 , frbrer:P2073 , frbrer:P2074 , frbrer:P2075 , frbrer:P2076 , frbrer:P2077 , frbrer:P2078 , frbrer:P2079 , frbrer:P2080 , frbrer:P2109 , frbrer:P2110 , frbrer:P3008 , frbrer:P3009 , frbrer:P3010 , frbrer:P3011 , frbrer:P3012 , frbrer:P3013 , frbrer:P3014 , frbrer:P3015 , frbrer:P3016 , frbrer:P3017 , frbrer:P3018 , frbrer:P3019 .

frbrer:P2061 a owl:ObjectProperty , owl:AsymmetricProperty ;
	rdfs:label "has a revision (expression)"@en ;
	rdfs:isDefinedBy <http://iflastandards.info/ns/fr/frbr/frbrer/> ;
	rdfs:domain frbrer:C1002 ;
	rdfs:range frbrer:C1002 ;
	owl:propertyDisjointWith frbrer:P2062 ;
	owl:inverseOf frbrer:P2062 ;
	owl:propertyDisjointWith frbrer:P2063 , frbrer:P2064 , frbrer:P2065 , frbrer:P2066 , frbrer:P2067 , frbrer:P2068 , frbrer:P2069 , frbrer:P2071 , frbrer:P2072 , frbrer:P2073 , frbrer:P2074 , frbrer:P2075 , frbrer:P2076 , frbrer:P2077 , frbrer:P2078 , frbrer:P2079 , frbrer:P2080 , frbrer:P2109 , frbrer:P2110 , frbrer:P3008 , frbrer:P3009 , frbrer:P3010 , frbrer:P3011 , frbrer:P3012 , frbrer:P3013 , frbrer:P3014 , frbrer:P3015 , frbrer:P3016 , frbrer:P3017 , frbrer:P3018 , frbrer:P3019 .

frbrer:P2062 a owl:ObjectProperty , owl:AsymmetricProperty ;
	rdfs:label "is a revision (expression) of"@en ;
	rdfs:isDefinedBy <http://iflastandards.info/ns/fr/frbr/frbrer/> ;
	rdfs:domain frbrer:C1002 ;
	rdfs:range frbrer:C1002 ;
	owl:propertyDisjointWith frbrer:P2063 , frbrer:P2064 , frbrer:P2065 , frbrer:P2066 , frbrer:P2067 , frbrer:P2068 , frbrer:P2069 , frbrer:P2071 , frbrer:P2072 , frbrer:P2073 , frbrer:P2074 , frbrer:P2075 , frbrer:P2076 , frbrer:P2077 , frbrer:P2078 , frbrer:P2079 , frbrer:P2080 , frbrer:P2109 , frbrer:P2110 , frbrer:P3008 , frbrer:P3009 , frbrer:P3010 , frbrer:P3011 , frbrer:P3012 , frbrer:P3013 , frbrer:P3014 , frbrer:P3015 , frbrer:P3016 , frbrer:P3017 , frbrer:P3018 , frbrer:P3019 .

frbrer:P2063 a owl:ObjectProperty , owl:AsymmetricProperty , owl:TransitiveProperty ;
	rdfs:label "has a translation (expression)"@en ;
	rdfs:isDefinedBy <http://iflastandards.info/ns/fr/frbr/frbrer/> ;
	rdfs:domain frbrer:C1002 ;
	rdfs:range frbrer:C1002 ;
	owl:inverseOf frbrer:P2064 ;
	owl:propertyDisjointWith frbrer:P2064 , frbrer:P2065 , frbrer:P2066 , frbrer:P2067 , frbrer:P2068 , frbrer:P2069 , frbrer:P2071 , frbrer:P2072 , frbrer:P2073 , frbrer:P2074 , frbrer:P2075 , frbrer:P2076 , frbrer:P2077 , frbrer:P2078 , frbrer:P2079 , frbrer:P2080 , frbrer:P2109 , frbrer:P2110 , frbrer:P3008 , frbrer:P3009 , frbrer:P3010 , frbrer:P3011 , frbrer:P3012 , frbrer:P3013 , frbrer:P3014 , frbrer:P3015 , frbrer:P3016 , frbrer:P3017 , frbrer:P3018 , frbrer:P3019 .

frbrer:P2064 a owl:ObjectProperty , owl:AsymmetricProperty , owl:TransitiveProperty ;
	rdfs:label "is a translation (expression) of"@en ;
	rdfs:isDefinedBy <http://iflastandards.info/ns/fr/frbr/frbrer/> ;
	rdfs:domain frbrer:C1002 ;
	rdfs:range frbrer:C1002 ;
	owl:propertyDisjointWith frbrer:P2065 , frbrer:P2066 , frbrer:P2067 , frbrer:P2068 , frbrer:P2069 , frbrer:P2071 , frbrer:P2072 , frbrer:P2073 , frbrer:P2074 , frbrer:P2075 , frbrer:P2076 , frbrer:P2077 , frbrer:P2078 , frbrer:P2079 , frbrer:P2080 , frbrer:P2109 , frbrer:P2110 , frbrer:P3008 , frbrer:P3009 , frbrer:P3010 , frbrer:P3011 , frbrer:P3012 , frbrer:P3013 , frbrer:P3014 , frbrer:P3015 , frbrer:P3016 , frbrer:P3017 , frbrer:P3018 , frbrer:P3019 .

frbrer:P2065 a owl:ObjectProperty , owl:AsymmetricProperty ;
	rdfs:label "has an arrangement (expression)"@en ;
	rdfs:isDefinedBy <http://iflastandards.info/ns/fr/frbr/frbrer/> ;
	rdfs:domain frbrer:C1002 ;
	rdfs:range frbrer:C1002 ;
	owl:inverseOf frbrer:P2066 ;
	owl:propertyDisjointWith frbrer:P2066 , frbrer:P2067 , frbrer:P2068 , frbrer:P2069 , frbrer:P2071 , frbrer:P2072 , frbrer:P2073 , frbrer:P2074 , frbrer:P2075 , frbrer:P2076 , frbrer:P2077 , frbrer:P2078 , frbrer:P2079 , frbrer:P2080 , frbrer:P2109 , frbrer:P2110 , frbrer:P3008 , frbrer:P3009 , frbrer:P3010 , frbrer:P3011 , frbrer:P3012 , frbrer:P3013 , frbrer:P3014 , frbrer:P3015 , frbrer:P3016 , frbrer:P3017 , frbrer:P3018 , frbrer:P3019 .

frbrer:P2066 a owl:ObjectProperty , owl:AsymmetricProperty ;
	rdfs:label "is an arrangement (expression) of"@en ;
	rdfs:isDefinedBy <http://iflastandards.info/ns/fr/frbr/frbrer/> ;
	rdfs:domain frbrer:C1002 ;
	rdfs:range frbrer:C1002 ;
	owl:propertyDisjointWith frbrer:P2067 , frbrer:P2068 , frbrer:P2069 , frbrer:P2071 , frbrer:P2072 , frbrer:P2073 , frbrer:P2074 , frbrer:P2075 , frbrer:P2076 , frbrer:P2077 , frbrer:P2078 , frbrer:P2079 , frbrer:P2080 , frbrer:P2109 , frbrer:P2110 , frbrer:P3008 , frbrer:P3009 , frbrer:P3010 , frbrer:P3011 , frbrer:P3012 , frbrer:P3013 , frbrer:P3014 , frbrer:P3015 , frbrer:P3016 , frbrer:P3017 , frbrer:P3018 , frbrer:P3019 .

frbrer:P2067 a owl:ObjectProperty , owl:AsymmetricProperty , owl:TransitiveProperty ;
	rdfs:label "has a successor (expression) (from expression)"@en ;
	rdfs:isDefinedBy <http://iflastandards.info/ns/fr/frbr/frbrer/> ;
	rdfs:range frbrer:C1002 ;
	rdfs:domain frbrer:C1002 ;
	owl:propertyDisjointWith frbrer:P2068 ;
	owl:inverseOf frbrer:P2068 ;
	owl:propertyDisjointWith frbrer:P2069 , frbrer:P2071 , frbrer:P2072 , frbrer:P2073 , frbrer:P2074 , frbrer:P2075 , frbrer:P2076 , frbrer:P2077 , frbrer:P2078 , frbrer:P2079 , frbrer:P2080 , frbrer:P2109 , frbrer:P2110 , frbrer:P3008 , frbrer:P3009 , frbrer:P3010 , frbrer:P3011 , frbrer:P3012 , frbrer:P3013 , frbrer:P3014 , frbrer:P3015 , frbrer:P3016 , frbrer:P3017 , frbrer:P3018 , frbrer:P3019 .

frbrer:P2068 a owl:ObjectProperty , owl:AsymmetricProperty , owl:TransitiveProperty ;
	rdfs:label "is a successor (expression) to (expression)"@en ;
	rdfs:isDefinedBy <http://iflastandards.info/ns/fr/frbr/frbrer/> ;
	rdfs:range frbrer:C1002 ;
	rdfs:domain frbrer:C1002 ;
	owl:propertyDisjointWith frbrer:P2069 , frbrer:P2071 , frbrer:P2072 , frbrer:P2073 , frbrer:P2074 , frbrer:P2075 , frbrer:P2076 , frbrer:P2077 , frbrer:P2078 , frbrer:P2079 , frbrer:P2080 , frbrer:P2109 , frbrer:P2110 , frbrer:P3008 , frbrer:P3009 , frbrer:P3010 , frbrer:P3011 , frbrer:P3012 , frbrer:P3013 , frbrer:P3014 , frbrer:P3015 , frbrer:P3016 , frbrer:P3017 , frbrer:P3018 , frbrer:P3019 .

frbrer:P2069 a owl:ObjectProperty ;
	rdfs:label "has a complement (expression) (from expression)"@en ;
	rdfs:isDefinedBy <http://iflastandards.info/ns/fr/frbr/frbrer/> ;
	rdfs:range frbrer:C1002 ;
	rdfs:domain frbrer:C1002 ;
	owl:inverseOf frbrer:P2070 ;
	owl:propertyDisjointWith frbrer:P2071 , frbrer:P2072 , frbrer:P2073 , frbrer:P2074 , frbrer:P2075 , frbrer:P2076 , frbrer:P2077 , frbrer:P2078 , frbrer:P2079 , frbrer:P2080 , frbrer:P2109 , frbrer:P2110 , frbrer:P3008 , frbrer:P3009 , frbrer:P3010 , frbrer:P3011 , frbrer:P3012 , frbrer:P3013 , frbrer:P3014 , frbrer:P3015 , frbrer:P3016 , frbrer:P3017 , frbrer:P3018 , frbrer:P3019 .

frbrer:P2070 a owl:ObjectProperty ;
	rdfs:label "complements (expression) (from expression)"@en ;
	rdfs:isDefinedBy <http://iflastandards.info/ns/fr/frbr/frbrer/> ;
	rdfs:domain frbrer:C1002 ;
	rdfs:range frbrer:C1002 .

frbrer:P2071 a owl:ObjectProperty , owl:AsymmetricProperty ;
	rdfs:label "has a summary (expression) (from expression)"@en ;
	rdfs:isDefinedBy <http://iflastandards.info/ns/fr/frbr/frbrer/> ;
	rdfs:domain frbrer:C1002 ;
	rdfs:range frbrer:C1002 ;
	owl:propertyDisjointWith frbrer:P2072 ;
	owl:inverseOf frbrer:P2072 ;
	owl:propertyDisjointWith frbrer:P2073 , frbrer:P2074 , frbrer:P2075 , frbrer:P2076 , frbrer:P2077 , frbrer:P2078 , frbrer:P2079 , frbrer:P2080 , frbrer:P2109 , frbrer:P2110 , frbrer:P3008 , frbrer:P3009 , frbrer:P3010 , frbrer:P3011 , frbrer:P3012 , frbrer:P3013 , frbrer:P3014 , frbrer:P3015 , frbrer:P3016 , frbrer:P3017 , frbrer:P3018 , frbrer:P3019 .

frbrer:P2072 a owl:ObjectProperty , owl:AsymmetricProperty ;
	rdfs:label "is a summary (expression) of (expression)"@en ;
	rdfs:isDefinedBy <http://iflastandards.info/ns/fr/frbr/frbrer/> ;
	rdfs:domain frbrer:C1002 ;
	rdfs:range frbrer:C1002 ;
	owl:propertyDisjointWith frbrer:P2073 , frbrer:P2074 , frbrer:P2075 , frbrer:P2076 , frbrer:P2077 , frbrer:P2078 , frbrer:P2079 , frbrer:P2080 , frbrer:P2109 , frbrer:P2110 , frbrer:P3008 , frbrer:P3009 , frbrer:P3010 , frbrer:P3011 , frbrer:P3012 , frbrer:P3013 , frbrer:P3014 , frbrer:P3015 , frbrer:P3016 , frbrer:P3017 , frbrer:P3018 , frbrer:P3019 .

frbrer:P2073 a owl:ObjectProperty , owl:AsymmetricProperty ;
	rdfs:label "has an adaptation (expression) (from expression)"@en ;
	rdfs:isDefinedBy <http://iflastandards.info/ns/fr/frbr/frbrer/> ;
	rdfs:range frbrer:C1002 ;
	rdfs:domain frbrer:C1002 ;
	owl:inverseOf frbrer:P2074 ;
	owl:propertyDisjointWith frbrer:P2074 , frbrer:P2075 , frbrer:P2076 , frbrer:P2077 , frbrer:P2078 , frbrer:P2079 , frbrer:P2080 , frbrer:P2109 , frbrer:P2110 , frbrer:P3008 , frbrer:P3009 , frbrer:P3010 , frbrer:P3011 , frbrer:P3012 , frbrer:P3013 , frbrer:P3014 , frbrer:P3015 , frbrer:P3016 , frbrer:P3017 , frbrer:P3018 , frbrer:P3019 .

frbrer:P2074 a owl:ObjectProperty , owl:AsymmetricProperty ;
	rdfs:label "is an adaptation (expression) of (expression)"@en ;
	rdfs:isDefinedBy <http://iflastandards.info/ns/fr/frbr/frbrer/> ;
	rdfs:range frbrer:C1002 ;
	rdfs:domain frbrer:C1002 ;
	owl:propertyDisjointWith frbrer:P2075 , frbrer:P2076 , frbrer:P2077 , frbrer:P2078 , frbrer:P2079 , frbrer:P2080 , frbrer:P2109 , frbrer:P2110 , frbrer:P3008 , frbrer:P3009 , frbrer:P3010 , frbrer:P3011 , frbrer:P3012 , frbrer:P3013 , frbrer:P3014 , frbrer:P3015 , frbrer:P3016 , frbrer:P3017 , frbrer:P3018 , frbrer:P3019 .

frbrer:P2075 a owl:ObjectProperty , owl:AsymmetricProperty , owl:TransitiveProperty ;
	rdfs:label "has a transformation (expression) (from expression)"@en ;
	rdfs:comment "Source documentation has \"literary genre\", but other genres allowed."@en ;
	rdfs:isDefinedBy <http://iflastandards.info/ns/fr/frbr/frbrer/> ;
	rdfs:range frbrer:C1002 ;
	rdfs:domain frbrer:C1002 ;
	owl:inverseOf frbrer:P2076 ;
	owl:propertyDisjointWith frbrer:P2076 , frbrer:P2077 , frbrer:P2078 , frbrer:P2079 , frbrer:P2080 , frbrer:P2109 , frbrer:P2110 , frbrer:P3008 , frbrer:P3009 , frbrer:P3010 , frbrer:P3011 , frbrer:P3012 , frbrer:P3013 , frbrer:P3014 , frbrer:P3015 , frbrer:P3016 , frbrer:P3017 , frbrer:P3018 , frbrer:P3019 .

frbrer:P2076 a owl:ObjectProperty , owl:AsymmetricProperty , owl:TransitiveProperty ;
	rdfs:label "is a transformation (expression) of (expression)"@en ;
	rdfs:comment "Source documentation has \"literary genre\", but other genres allowed."@en ;
	rdfs:isDefinedBy <http://iflastandards.info/ns/fr/frbr/frbrer/> ;
	rdfs:domain frbrer:C1002 ;
	rdfs:range frbrer:C1002 ;
	owl:propertyDisjointWith frbrer:P2077 , frbrer:P2078 , frbrer:P2079 , frbrer:P2080 , frbrer:P2109 , frbrer:P2110 , frbrer:P3008 , frbrer:P3009 , frbrer:P3010 , frbrer:P3011 , frbrer:P3012 , frbrer:P3013 , frbrer:P3014 , frbrer:P3015 , frbrer:P3016 , frbrer:P3017 , frbrer:P3018 , frbrer:P3019 .

frbrer:P2077 a owl:ObjectProperty , owl:AsymmetricProperty ;
	rdfs:label "has an imitation (expression) (from expression)"@en ;
	rdfs:isDefinedBy <http://iflastandards.info/ns/fr/frbr/frbrer/> ;
	rdfs:domain frbrer:C1002 ;
	rdfs:range frbrer:C1002 ;
	owl:inverseOf frbrer:P2078 ;
	owl:propertyDisjointWith frbrer:P2078 , frbrer:P2079 , frbrer:P2080 , frbrer:P2109 , frbrer:P2110 , frbrer:P3008 , frbrer:P3009 , frbrer:P3010 , frbrer:P3011 , frbrer:P3012 , frbrer:P3013 , frbrer:P3014 , frbrer:P3015 , frbrer:P3016 , frbrer:P3017 , frbrer:P3018 , frbrer:P3019 .

frbrer:P2078 a owl:ObjectProperty , owl:AsymmetricProperty ;
	rdfs:label "is an imitation (expression) of (expression)"@en ;
	rdfs:isDefinedBy <http://iflastandards.info/ns/fr/frbr/frbrer/> ;
	rdfs:range frbrer:C1002 ;
	rdfs:domain frbrer:C1002 ;
	owl:propertyDisjointWith frbrer:P2079 , frbrer:P2080 , frbrer:P2109 , frbrer:P2110 , frbrer:P3008 , frbrer:P3009 , frbrer:P3010 , frbrer:P3011 , frbrer:P3012 , frbrer:P3013 , frbrer:P3014 , frbrer:P3015 , frbrer:P3016 , frbrer:P3017 , frbrer:P3018 , frbrer:P3019 .

frbrer:P2079 a owl:ObjectProperty , owl:AsymmetricProperty , owl:TransitiveProperty ;
	rdfs:label "has part (expression)"@en ;
	rdfs:isDefinedBy <http://iflastandards.info/ns/fr/frbr/frbrer/> ;
	rdfs:range frbrer:C1002 ;
	rdfs:domain frbrer:C1002 ;
	owl:propertyDisjointWith frbrer:P2080 ;
	owl:inverseOf frbrer:P2080 ;
	owl:propertyDisjointWith frbrer:P2109 , frbrer:P2110 , frbrer:P3008 , frbrer:P3009 , frbrer:P3010 , frbrer:P3011 , frbrer:P3012 , frbrer:P3013 , frbrer:P3014 , frbrer:P3015 , frbrer:P3016 , frbrer:P3017 , frbrer:P3018 , frbrer:P3019 .

frbrer:P2080 a owl:ObjectProperty , owl:AsymmetricProperty , owl:TransitiveProperty ;
	rdfs:label "is part (expression) of"@en ;
	rdfs:isDefinedBy <http://iflastandards.info/ns/fr/frbr/frbrer/> ;
	rdfs:domain frbrer:C1002 ;
	rdfs:range frbrer:C1002 ;
	owl:propertyDisjointWith frbrer:P2109 , frbrer:P2110 , frbrer:P3008 , frbrer:P3009 , frbrer:P3010 , frbrer:P3011 , frbrer:P3012 , frbrer:P3013 , frbrer:P3014 , frbrer:P3015 , frbrer:P3016 , frbrer:P3017 , frbrer:P3018 , frbrer:P3019 .

frbrer:P2081 a owl:ObjectProperty , owl:AsymmetricProperty , owl:TransitiveProperty ;
	rdfs:label "has a reproduction (manifestation) (from manifestation)"@en ;
	rdfs:isDefinedBy <http://iflastandards.info/ns/fr/frbr/frbrer/> ;
	rdfs:range frbrer:C1003 ;
	rdfs:domain frbrer:C1003 ;
	owl:propertyDisjointWith frbrer:P2082 ;
	owl:inverseOf frbrer:P2082 ;
	owl:propertyDisjointWith frbrer:P2083 , frbrer:P2085 , frbrer:P2086 , frbrer:P3020 , frbrer:P3021 , frbrer:P3022 , frbrer:P3023 , frbrer:P3024 , frbrer:P3025 , frbrer:P3026 , frbrer:P3027 , frbrer:P3028 , frbrer:P3029 , frbrer:P3030 , frbrer:P3053 , frbrer:P3054 , frbrer:P3055 , frbrer:P3056 , frbrer:P3057 , frbrer:P3058 .

frbrer:P2082 a owl:ObjectProperty , owl:AsymmetricProperty , owl:TransitiveProperty ;
	rdfs:label "is a reproduction (manifestation) of (manifestation)"@en ;
	rdfs:isDefinedBy <http://iflastandards.info/ns/fr/frbr/frbrer/> ;
	rdfs:range frbrer:C1003 ;
	rdfs:domain frbrer:C1003 ;
	owl:propertyDisjointWith frbrer:P2083 , frbrer:P2085 , frbrer:P2086 , frbrer:P3020 , frbrer:P3021 , frbrer:P3022 , frbrer:P3023 , frbrer:P3024 , frbrer:P3025 , frbrer:P3026 , frbrer:P3027 , frbrer:P3028 , frbrer:P3029 , frbrer:P3030 , frbrer:P3053 , frbrer:P3054 , frbrer:P3055 , frbrer:P3056 , frbrer:P3057 , frbrer:P3058 .

frbrer:P2083 a owl:ObjectProperty , owl:SymmetricProperty ;
	rdfs:label "has an alternate"@en ;
	rdfs:isDefinedBy <http://iflastandards.info/ns/fr/frbr/frbrer/> ;
	rdfs:domain frbrer:C1003 ;
	rdfs:range frbrer:C1003 ;
	owl:propertyDisjointWith frbrer:P2085 , frbrer:P2086 , frbrer:P3020 , frbrer:P3021 , frbrer:P3022 , frbrer:P3023 , frbrer:P3024 , frbrer:P3025 , frbrer:P3026 , frbrer:P3027 , frbrer:P3028 , frbrer:P3029 , frbrer:P3030 , frbrer:P3053 , frbrer:P3054 , frbrer:P3055 , frbrer:P3056 , frbrer:P3057 , frbrer:P3058 .

frbrer:P2085 a owl:ObjectProperty , owl:AsymmetricProperty , owl:TransitiveProperty ;
	rdfs:label "has part (manifestation)"@en ;
	rdfs:isDefinedBy <http://iflastandards.info/ns/fr/frbr/frbrer/> ;
	rdfs:domain frbrer:C1003 ;
	rdfs:range frbrer:C1003 ;
	owl:propertyDisjointWith frbrer:P2086 ;
	owl:inverseOf frbrer:P2086 ;
	owl:propertyDisjointWith frbrer:P3020 , frbrer:P3021 , frbrer:P3022 , frbrer:P3023 , frbrer:P3024 , frbrer:P3025 , frbrer:P3026 , frbrer:P3027 , frbrer:P3028 , frbrer:P3029 , frbrer:P3030 , frbrer:P3053 , frbrer:P3054 , frbrer:P3055 , frbrer:P3056 , frbrer:P3057 , frbrer:P3058 .

frbrer:P2086 a owl:ObjectProperty , owl:AsymmetricProperty , owl:TransitiveProperty ;
	rdfs:label "is part (manifestation) of"@en ;
	rdfs:isDefinedBy <http://iflastandards.info/ns/fr/frbr/frbrer/> ;
	rdfs:range frbrer:C1003 ;
	rdfs:domain frbrer:C1003 ;
	owl:propertyDisjointWith frbrer:P3020 , frbrer:P3021 , frbrer:P3022 , frbrer:P3023 , frbrer:P3024 , frbrer:P3025 , frbrer:P3026 , frbrer:P3027 , frbrer:P3028 , frbrer:P3029 , frbrer:P3030 , frbrer:P3053 , frbrer:P3054 , frbrer:P3055 , frbrer:P3056 , frbrer:P3057 , frbrer:P3058 .

frbrer:P2087 a owl:ObjectProperty , owl:AsymmetricProperty ;
	rdfs:label "has a reconfiguration"@en ;
	rdfs:comment "Source documentation has label \"has reconfiguration\", amended to improve consistency."@en ;
	rdfs:isDefinedBy <http://iflastandards.info/ns/fr/frbr/frbrer/> ;
	rdfs:domain frbrer:C1004 ;
	rdfs:range frbrer:C1004 ;
	owl:propertyDisjointWith frbrer:P2088 ;
	owl:inverseOf frbrer:P2088 ;
	owl:propertyDisjointWith frbrer:P2089 , frbrer:P2090 , frbrer:P2091 , frbrer:P2092 , frbrer:P3031 , frbrer:P3032 , frbrer:P3033 , frbrer:P3034 , frbrer:P3035 , frbrer:P3036 , frbrer:P3037 , frbrer:P3038 , frbrer:P3052 .

frbrer:P2088 a owl:ObjectProperty , owl:AsymmetricProperty ;
	rdfs:label "is a reconfiguration of"@en ;
	rdfs:isDefinedBy <http://iflastandards.info/ns/fr/frbr/frbrer/> ;
	rdfs:domain frbrer:C1004 ;
	rdfs:range frbrer:C1004 ;
	owl:propertyDisjointWith frbrer:P2089 , frbrer:P2090 , frbrer:P2091 , frbrer:P2092 , frbrer:P3031 , frbrer:P3032 , frbrer:P3033 , frbrer:P3034 , frbrer:P3035 , frbrer:P3036 , frbrer:P3037 , frbrer:P3038 , frbrer:P3052 .

frbrer:P2089 a owl:ObjectProperty , owl:AsymmetricProperty , owl:TransitiveProperty ;
	rdfs:label "has a reproduction (item) (from item)"@en ;
	rdfs:comment "Source documentation has label \"has reproduction\"; amended to improve consistency."@en ;
	rdfs:isDefinedBy <http://iflastandards.info/ns/fr/frbr/frbrer/> ;
	rdfs:domain frbrer:C1004 ;
	rdfs:range frbrer:C1004 ;
	owl:propertyDisjointWith frbrer:P2090 ;
	owl:inverseOf frbrer:P2090 ;
	owl:propertyDisjointWith frbrer:P2091 , frbrer:P2092 , frbrer:P3031 , frbrer:P3032 , frbrer:P3033 , frbrer:P3034 , frbrer:P3035 , frbrer:P3036 , frbrer:P3037 , frbrer:P3038 , frbrer:P3052 .

frbrer:P2090 a owl:ObjectProperty , owl:AsymmetricProperty , owl:TransitiveProperty ;
	rdfs:label "is a reproduction (item) of (item)"@en ;
	rdfs:isDefinedBy <http://iflastandards.info/ns/fr/frbr/frbrer/> ;
	rdfs:range frbrer:C1004 ;
	rdfs:domain frbrer:C1004 ;
	owl:propertyDisjointWith frbrer:P2091 , frbrer:P2092 , frbrer:P3031 , frbrer:P3032 , frbrer:P3033 , frbrer:P3034 , frbrer:P3035 , frbrer:P3036 , frbrer:P3037 , frbrer:P3038 , frbrer:P3052 .

frbrer:P2091 a owl:ObjectProperty , owl:AsymmetricProperty , owl:TransitiveProperty ;
	rdfs:label "has part (item)"@en ;
	rdfs:isDefinedBy <http://iflastandards.info/ns/fr/frbr/frbrer/> ;
	rdfs:range frbrer:C1004 ;
	rdfs:domain frbrer:C1004 ;
	owl:propertyDisjointWith frbrer:P2092 ;
	owl:inverseOf frbrer:P2092 ;
	owl:propertyDisjointWith frbrer:P3031 , frbrer:P3032 , frbrer:P3033 , frbrer:P3034 , frbrer:P3035 , frbrer:P3036 , frbrer:P3037 , frbrer:P3038 , frbrer:P3052 .

frbrer:P2092 a owl:ObjectProperty , owl:AsymmetricProperty , owl:TransitiveProperty ;
	rdfs:label "is part (item) of"@en ;
	rdfs:isDefinedBy <http://iflastandards.info/ns/fr/frbr/frbrer/> ;
	rdfs:range frbrer:C1004 ;
	rdfs:domain frbrer:C1004 ;
	owl:propertyDisjointWith frbrer:P3031 , frbrer:P3032 , frbrer:P3033 , frbrer:P3034 , frbrer:P3035 , frbrer:P3036 , frbrer:P3037 , frbrer:P3038 , frbrer:P3052 .

frbrer:P2093 a owl:ObjectProperty ;
	rdfs:label "has a reproduction (manifestation) (from item)"@en ;
	rdfs:isDefinedBy <http://iflastandards.info/ns/fr/frbr/frbrer/> ;
	rdfs:range frbrer:C1003 ;
	rdfs:domain frbrer:C1004 ;
	owl:inverseOf frbrer:P2094 ;
	owl:propertyDisjointWith frbrer:P3031 , frbrer:P3032 , frbrer:P3033 , frbrer:P3034 , frbrer:P3035 , frbrer:P3036 , frbrer:P3037 , frbrer:P3038 , frbrer:P3052 .

frbrer:P2094 a owl:ObjectProperty ;
	rdfs:label "is a reproduction (manifestation) of (item)"@en ;
	rdfs:isDefinedBy <http://iflastandards.info/ns/fr/frbr/frbrer/> ;
	rdfs:domain frbrer:C1003 ;
	rdfs:range frbrer:C1004 ;
	owl:propertyDisjointWith frbrer:P3020 , frbrer:P3021 , frbrer:P3022 , frbrer:P3023 , frbrer:P3024 , frbrer:P3025 , frbrer:P3026 , frbrer:P3027 , frbrer:P3028 , frbrer:P3029 , frbrer:P3030 , frbrer:P3053 , frbrer:P3054 , frbrer:P3055 , frbrer:P3056 , frbrer:P3057 , frbrer:P3058 .

frbrer:P2095 a owl:ObjectProperty ;
	rdfs:label "has a successor (work) (from expression)"@en ;
	rdfs:isDefinedBy <http://iflastandards.info/ns/fr/frbr/frbrer/> ;
	rdfs:range frbrer:C1001 ;
	rdfs:domain frbrer:C1002 ;
	owl:inverseOf frbrer:P2096 ;
	owl:propertyDisjointWith frbrer:P2097 , frbrer:P2099 , frbrer:P2101 , frbrer:P2103 , frbrer:P2105 , frbrer:P2107 , frbrer:P3008 , frbrer:P3009 , frbrer:P3010 , frbrer:P3011 , frbrer:P3012 , frbrer:P3013 , frbrer:P3014 , frbrer:P3015 , frbrer:P3016 , frbrer:P3017 , frbrer:P3018 , frbrer:P3019 .

frbrer:P2096 a owl:ObjectProperty ;
	rdfs:label "is a successor (work) to (expression)"@en ;
	rdfs:isDefinedBy <http://iflastandards.info/ns/fr/frbr/frbrer/> ;
	rdfs:domain frbrer:C1001 ;
	rdfs:range frbrer:C1002 ;
	owl:propertyDisjointWith frbrer:P2100 , frbrer:P2102 , frbrer:P2104 , frbrer:P2106 , frbrer:P2108 , frbrer:P3001 , frbrer:P3002 , frbrer:P3003 , frbrer:P3004 , frbrer:P3005 , frbrer:P3006 , frbrer:P3007 .

frbrer:P2097 a owl:ObjectProperty ;
	rdfs:label "has a supplement (work) (from expression)"@en ;
	rdfs:isDefinedBy <http://iflastandards.info/ns/fr/frbr/frbrer/> ;
	rdfs:range frbrer:C1001 ;
	rdfs:domain frbrer:C1002 ;
	owl:inverseOf frbrer:P2098 ;
	owl:propertyDisjointWith frbrer:P2099 , frbrer:P2101 , frbrer:P2103 , frbrer:P2105 , frbrer:P2107 , frbrer:P3008 , frbrer:P3009 , frbrer:P3010 , frbrer:P3011 , frbrer:P3012 , frbrer:P3013 , frbrer:P3014 , frbrer:P3015 , frbrer:P3016 , frbrer:P3017 , frbrer:P3018 , frbrer:P3019 .

frbrer:P2098 a owl:ObjectProperty ;
	rdfs:label "supplements (expression) (from work)"@en ;
	rdfs:isDefinedBy <http://iflastandards.info/ns/fr/frbr/frbrer/> ;
	rdfs:domain frbrer:C1001 ;
	rdfs:range frbrer:C1002 ;
	owl:propertyDisjointWith frbrer:P3001 , frbrer:P3002 , frbrer:P3003 , frbrer:P3004 , frbrer:P3005 , frbrer:P3006 , frbrer:P3007 .

frbrer:P2099 a owl:ObjectProperty ;
	rdfs:label "has a complement (work) (from expression)"@en ;
	rdfs:isDefinedBy <http://iflastandards.info/ns/fr/frbr/frbrer/> ;
	rdfs:range frbrer:C1001 ;
	rdfs:domain frbrer:C1002 ;
	owl:inverseOf frbrer:P2100 ;
	owl:propertyDisjointWith frbrer:P2101 , frbrer:P2103 , frbrer:P2105 , frbrer:P2107 , frbrer:P3008 , frbrer:P3009 , frbrer:P3010 , frbrer:P3011 , frbrer:P3012 , frbrer:P3013 , frbrer:P3014 , frbrer:P3015 , frbrer:P3016 , frbrer:P3017 , frbrer:P3018 , frbrer:P3019 .

frbrer:P2100 a owl:ObjectProperty ;
	rdfs:label "complements (work) (from expression)"@en ;
	rdfs:isDefinedBy <http://iflastandards.info/ns/fr/frbr/frbrer/> ;
	rdfs:domain frbrer:C1001 ;
	rdfs:range frbrer:C1002 ;
	owl:propertyDisjointWith frbrer:P2102 , frbrer:P2104 , frbrer:P2106 , frbrer:P2108 , frbrer:P3001 , frbrer:P3002 , frbrer:P3003 , frbrer:P3004 , frbrer:P3005 , frbrer:P3006 , frbrer:P3007 .

frbrer:P2101 a owl:ObjectProperty ;
	rdfs:label "has a summary (work) (from expression)"@en ;
	rdfs:isDefinedBy <http://iflastandards.info/ns/fr/frbr/frbrer/> ;
	rdfs:range frbrer:C1001 ;
	rdfs:domain frbrer:C1002 ;
	owl:inverseOf frbrer:P2102 ;
	owl:propertyDisjointWith frbrer:P2103 , frbrer:P2105 , frbrer:P2107 , frbrer:P3008 , frbrer:P3009 , frbrer:P3010 , frbrer:P3011 , frbrer:P3012 , frbrer:P3013 , frbrer:P3014 , frbrer:P3015 , frbrer:P3016 , frbrer:P3017 , frbrer:P3018 , frbrer:P3019 .

frbrer:P2102 a owl:ObjectProperty ;
	rdfs:label "is a summary (work) of (expression)"@en ;
	rdfs:isDefinedBy <http://iflastandards.info/ns/fr/frbr/frbrer/> ;
	rdfs:domain frbrer:C1001 ;
	rdfs:range frbrer:C1002 ;
	owl:propertyDisjointWith frbrer:P2104 , frbrer:P2106 , frbrer:P2108 , frbrer:P3001 , frbrer:P3002 , frbrer:P3003 , frbrer:P3004 , frbrer:P3005 , frbrer:P3006 , frbrer:P3007 .

frbrer:P2103 a owl:ObjectProperty ;
	rdfs:label "has an adaptation (work) (from expression)"@en ;
	rdfs:isDefinedBy <http://iflastandards.info/ns/fr/frbr/frbrer/> ;
	rdfs:range frbrer:C1001 ;
	rdfs:domain frbrer:C1002 ;
	owl:inverseOf frbrer:P2104 ;
	owl:propertyDisjointWith frbrer:P2105 , frbrer:P2107 , frbrer:P3008 , frbrer:P3009 , frbrer:P3010 , frbrer:P3011 , frbrer:P3012 , frbrer:P3013 , frbrer:P3014 , frbrer:P3015 , frbrer:P3016 , frbrer:P3017 , frbrer:P3018 , frbrer:P3019 .

frbrer:P2104 a owl:ObjectProperty ;
	rdfs:label "is an adaptation (work) of (expression)"@en ;
	rdfs:isDefinedBy <http://iflastandards.info/ns/fr/frbr/frbrer/> ;
	rdfs:domain frbrer:C1001 ;
	rdfs:range frbrer:C1002 ;
	owl:propertyDisjointWith frbrer:P2106 , frbrer:P2108 , frbrer:P3001 , frbrer:P3002 , frbrer:P3003 , frbrer:P3004 , frbrer:P3005 , frbrer:P3006 , frbrer:P3007 .

frbrer:P2105 a owl:ObjectProperty ;
	rdfs:label "has a transformation (work) (from expression)"@en ;
	rdfs:comment "Source documentation has \"literary genre\", but other genres allowed."@en ;
	rdfs:isDefinedBy <http://iflastandards.info/ns/fr/frbr/frbrer/> ;
	rdfs:range frbrer:C1001 ;
	rdfs:domain frbrer:C1002 ;
	owl:inverseOf frbrer:P2106 ;
	owl:propertyDisjointWith frbrer:P2107 , frbrer:P3008 , frbrer:P3009 , frbrer:P3010 , frbrer:P3011 , frbrer:P3012 , frbrer:P3013 , frbrer:P3014 , frbrer:P3015 , frbrer:P3016 , frbrer:P3017 , frbrer:P3018 , frbrer:P3019 .

frbrer:P2106 a owl:ObjectProperty ;
	rdfs:label "is a transformation (work) of (expression)"@en ;
	rdfs:comment "Source documentation has \"literary genre\", but other genres allowed."@en ;
	rdfs:isDefinedBy <http://iflastandards.info/ns/fr/frbr/frbrer/> ;
	rdfs:domain frbrer:C1001 ;
	rdfs:range frbrer:C1002 ;
	owl:propertyDisjointWith frbrer:P2108 , frbrer:P3001 , frbrer:P3002 , frbrer:P3003 , frbrer:P3004 , frbrer:P3005 , frbrer:P3006 , frbrer:P3007 .

frbrer:P2107 a owl:ObjectProperty ;
	rdfs:label "has an imitation (work) (from expression)"@en ;
	rdfs:isDefinedBy <http://iflastandards.info/ns/fr/frbr/frbrer/> ;
	rdfs:range frbrer:C1001 ;
	rdfs:domain frbrer:C1002 ;
	owl:inverseOf frbrer:P2108 ;
	owl:propertyDisjointWith frbrer:P3008 , frbrer:P3009 , frbrer:P3010 , frbrer:P3011 , frbrer:P3012 , frbrer:P3013 , frbrer:P3014 , frbrer:P3015 , frbrer:P3016 , frbrer:P3017 , frbrer:P3018 , frbrer:P3019 .

frbrer:P2108 a owl:ObjectProperty ;
	rdfs:label "is an imitation (work) of (expression)"@en ;
	rdfs:isDefinedBy <http://iflastandards.info/ns/fr/frbr/frbrer/> ;
	rdfs:domain frbrer:C1001 ;
	rdfs:range frbrer:C1002 ;
	owl:propertyDisjointWith frbrer:P3001 , frbrer:P3002 , frbrer:P3003 , frbrer:P3004 , frbrer:P3005 , frbrer:P3006 , frbrer:P3007 .

frbrer:P2109 a owl:ObjectProperty , owl:AsymmetricProperty ;
	rdfs:label "has a supplement (expression) (from expression)"@en ;
	rdfs:isDefinedBy <http://iflastandards.info/ns/fr/frbr/frbrer/> ;
	rdfs:domain frbrer:C1002 ;
	rdfs:range frbrer:C1002 ;
	owl:inverseOf frbrer:P2110 ;
	owl:propertyDisjointWith frbrer:P2110 , frbrer:P3008 , frbrer:P3009 , frbrer:P3010 , frbrer:P3011 , frbrer:P3012 , frbrer:P3013 , frbrer:P3014 , frbrer:P3015 , frbrer:P3016 , frbrer:P3017 , frbrer:P3018 , frbrer:P3019 .

frbrer:P2110 a owl:ObjectProperty , owl:AsymmetricProperty ;
	rdfs:label "supplements (expression) (from expression)"@en ;
	rdfs:isDefinedBy <http://iflastandards.info/ns/fr/frbr/frbrer/> ;
	rdfs:domain frbrer:C1002 ;
	rdfs:range frbrer:C1002 ;
	owl:propertyDisjointWith frbrer:P3008 , frbrer:P3009 , frbrer:P3010 , frbrer:P3011 , frbrer:P3012 , frbrer:P3013 , frbrer:P3014 , frbrer:P3015 , frbrer:P3016 , frbrer:P3017 , frbrer:P3018 , frbrer:P3019 .

frbrer:P3001 a owl:ObjectProperty ;
	rdfs:label "has title of the work"@en ;
	rdfs:isDefinedBy <http://iflastandards.info/ns/fr/frbr/frbrer/> ;
	rdfs:domain frbrer:C1001 ;
	owl:propertyDisjointWith frbrer:P3002 , frbrer:P3003 , frbrer:P3004 , frbrer:P3005 , frbrer:P3006 , frbrer:P3007 .

frbrer:P3002 a owl:ObjectProperty ;
	rdfs:label "has form of work"@en ;
	rdfs:isDefinedBy <http://iflastandards.info/ns/fr/frbr/frbrer/> ;
	rdfs:domain frbrer:C1001 ;
	owl:propertyDisjointWith frbrer:P3003 , frbrer:P3004 , frbrer:P3005 , frbrer:P3006 , frbrer:P3007 .

frbrer:P3003 a owl:ObjectProperty ;
	rdfs:label "has date of the work"@en ;
	rdfs:isDefinedBy <http://iflastandards.info/ns/fr/frbr/frbrer/> ;
	rdfs:domain frbrer:C1001 ;
	owl:propertyDisjointWith frbrer:P3004 , frbrer:P3005 , frbrer:P3006 , frbrer:P3007 .

frbrer:P3004 a owl:ObjectProperty ;
	rdfs:label "has other distinguishing characteristic of work"@en ;
	rdfs:comment "Source documentation has label \"Other Distinguishing Characteristic\", used also for an Expression attribute."@en ;
	rdfs:isDefinedBy <http://iflastandards.info/ns/fr/frbr/frbrer/> ;
	rdfs:domain frbrer:C1001 ;
	owl:propertyDisjointWith frbrer:P3005 , frbrer:P3006 , frbrer:P3007 .

frbrer:P3005 a owl:ObjectProperty ;
	rdfs:label "has intended termination"@en ;
	rdfs:isDefinedBy <http://iflastandards.info/ns/fr/frbr/frbrer/> ;
	rdfs:domain frbrer:C1001 ;
	owl:propertyDisjointWith frbrer:P3006 , frbrer:P3007 .

frbrer:P3006 a owl:ObjectProperty ;
	rdfs:label "has intended audience"@en ;
	rdfs:isDefinedBy <http://iflastandards.info/ns/fr/frbr/frbrer/> ;
	rdfs:domain frbrer:C1001 ;
	owl:propertyDisjointWith frbrer:P3007 .

frbrer:P3007 a owl:ObjectProperty ;
	rdfs:label "has context for the work"@en ;
	rdfs:isDefinedBy <http://iflastandards.info/ns/fr/frbr/frbrer/> ;
	rdfs:domain frbrer:C1001 .

frbrer:P3008 a owl:ObjectProperty ;
	rdfs:label "has title of the expression"@en ;
	rdfs:isDefinedBy <http://iflastandards.info/ns/fr/frbr/frbrer/> ;
	rdfs:domain frbrer:C1002 ;
	owl:propertyDisjointWith frbrer:P3009 , frbrer:P3010 , frbrer:P3011 , frbrer:P3012 , frbrer:P3013 , frbrer:P3014 , frbrer:P3015 , frbrer:P3016 , frbrer:P3017 , frbrer:P3018 , frbrer:P3019 .

frbrer:P3009 a owl:ObjectProperty ;
	rdfs:label "has form of expression"@en ;
	rdfs:isDefinedBy <http://iflastandards.info/ns/fr/frbr/frbrer/> ;
	rdfs:domain frbrer:C1002 ;
	owl:propertyDisjointWith frbrer:P3010 , frbrer:P3011 , frbrer:P3012 , frbrer:P3013 , frbrer:P3014 , frbrer:P3015 , frbrer:P3016 , frbrer:P3017 , frbrer:P3018 , frbrer:P3019 .

frbrer:P3010 a owl:ObjectProperty ;
	rdfs:label "has date of expression"@en ;
	rdfs:isDefinedBy <http://iflastandards.info/ns/fr/frbr/frbrer/> ;
	rdfs:domain frbrer:C1002 ;
	owl:propertyDisjointWith frbrer:P3011 , frbrer:P3012 , frbrer:P3013 , frbrer:P3014 , frbrer:P3015 , frbrer:P3016 , frbrer:P3017 , frbrer:P3018 , frbrer:P3019 .

frbrer:P3011 a owl:ObjectProperty ;
	rdfs:label "has language of expression"@en ;
	rdfs:isDefinedBy <http://iflastandards.info/ns/fr/frbr/frbrer/> ;
	rdfs:domain frbrer:C1002 ;
	owl:propertyDisjointWith frbrer:P3012 , frbrer:P3013 , frbrer:P3014 , frbrer:P3015 , frbrer:P3016 , frbrer:P3017 , frbrer:P3018 , frbrer:P3019 .

frbrer:P3012 a owl:ObjectProperty ;
	rdfs:label "has other distinguishing characteristic of expression"@en ;
	rdfs:comment "Source document has label \"Other Distinguishing Characteristic\" used also for a Work attribute."@en ;
	rdfs:isDefinedBy <http://iflastandards.info/ns/fr/frbr/frbrer/> ;
	rdfs:domain frbrer:C1002 ;
	owl:propertyDisjointWith frbrer:P3013 , frbrer:P3014 , frbrer:P3015 , frbrer:P3016 , frbrer:P3017 , frbrer:P3018 , frbrer:P3019 .

frbrer:P3013 a owl:ObjectProperty ;
	rdfs:label "has extensibility of expression"@en ;
	rdfs:isDefinedBy <http://iflastandards.info/ns/fr/frbr/frbrer/> ;
	rdfs:domain frbrer:C1002 ;
	owl:propertyDisjointWith frbrer:P3014 , frbrer:P3015 , frbrer:P3016 , frbrer:P3017 , frbrer:P3018 , frbrer:P3019 .

frbrer:P3014 a owl:ObjectProperty ;
	rdfs:label "has revisability of expression"@en ;
	rdfs:isDefinedBy <http://iflastandards.info/ns/fr/frbr/frbrer/> ;
	rdfs:domain frbrer:C1002 ;
	owl:propertyDisjointWith frbrer:P3015 , frbrer:P3016 , frbrer:P3017 , frbrer:P3018 , frbrer:P3019 .

frbrer:P3015 a owl:ObjectProperty ;
	rdfs:label "has extent of the expression"@en ;
	rdfs:isDefinedBy <http://iflastandards.info/ns/fr/frbr/frbrer/> ;
	rdfs:domain frbrer:C1002 ;
	owl:propertyDisjointWith frbrer:P3016 , frbrer:P3017 , frbrer:P3018 , frbrer:P3019 .

frbrer:P3016 a owl:ObjectProperty ;
	rdfs:label "has summarization of content"@en ;
	rdfs:isDefinedBy <http://iflastandards.info/ns/fr/frbr/frbrer/> ;
	rdfs:domain frbrer:C1002 ;
	owl:propertyDisjointWith frbrer:P3017 , frbrer:P3018 , frbrer:P3019 .

frbrer:P3017 a owl:ObjectProperty ;
	rdfs:label "has context for the expression"@en ;
	rdfs:isDefinedBy <http://iflastandards.info/ns/fr/frbr/frbrer/> ;
	rdfs:domain frbrer:C1002 ;
	owl:propertyDisjointWith frbrer:P3018 , frbrer:P3019 .

frbrer:P3018 a owl:ObjectProperty ;
	rdfs:label "has critical response to the expression"@en ;
	rdfs:isDefinedBy <http://iflastandards.info/ns/fr/frbr/frbrer/> ;
	rdfs:domain frbrer:C1002 ;
	owl:propertyDisjointWith frbrer:P3019 .

frbrer:P3019 a owl:ObjectProperty ;
	rdfs:label "has use restrictions on the expression"@en ;
	rdfs:isDefinedBy <http://iflastandards.info/ns/fr/frbr/frbrer/> ;
	rdfs:domain frbrer:C1002 .

frbrer:P3020 a owl:ObjectProperty ;
	rdfs:label "has title of the manifestation"@en ;
	rdfs:isDefinedBy <http://iflastandards.info/ns/fr/frbr/frbrer/> ;
	rdfs:domain frbrer:C1003 ;
	owl:propertyDisjointWith frbrer:P3021 , frbrer:P3022 , frbrer:P3023 , frbrer:P3024 , frbrer:P3025 , frbrer:P3026 , frbrer:P3027 , frbrer:P3028 , frbrer:P3029 , frbrer:P3030 , frbrer:P3053 , frbrer:P3054 , frbrer:P3055 , frbrer:P3056 , frbrer:P3057 , frbrer:P3058 .

frbrer:P3021 a owl:ObjectProperty ;
	rdfs:label "has statement of responsibility"@en ;
	rdfs:isDefinedBy <http://iflastandards.info/ns/fr/frbr/frbrer/> ;
	rdfs:domain frbrer:C1003 ;
	owl:propertyDisjointWith frbrer:P3022 , frbrer:P3023 , frbrer:P3024 , frbrer:P3025 , frbrer:P3026 , frbrer:P3027 , frbrer:P3028 , frbrer:P3029 , frbrer:P3030 , frbrer:P3053 , frbrer:P3054 , frbrer:P3055 , frbrer:P3056 , frbrer:P3057 , frbrer:P3058 .

frbrer:P3022 a owl:ObjectProperty ;
	rdfs:label "has series statement"@en ;
	rdfs:isDefinedBy <http://iflastandards.info/ns/fr/frbr/frbrer/> ;
	rdfs:domain frbrer:C1003 ;
	owl:propertyDisjointWith frbrer:P3023 , frbrer:P3024 , frbrer:P3025 , frbrer:P3026 , frbrer:P3027 , frbrer:P3028 , frbrer:P3029 , frbrer:P3030 , frbrer:P3053 , frbrer:P3054 , frbrer:P3055 , frbrer:P3056 , frbrer:P3057 , frbrer:P3058 .

frbrer:P3023 a owl:ObjectProperty ;
	rdfs:label "has form of carrier"@en ;
	rdfs:isDefinedBy <http://iflastandards.info/ns/fr/frbr/frbrer/> ;
	rdfs:domain frbrer:C1003 ;
	owl:propertyDisjointWith frbrer:P3053 , frbrer:P3054 , frbrer:P3056 .

frbrer:P3024 a owl:ObjectProperty ;
	rdfs:label "has extent of the carrier"@en ;
	rdfs:isDefinedBy <http://iflastandards.info/ns/fr/frbr/frbrer/> ;
	rdfs:domain frbrer:C1003 ;
	owl:propertyDisjointWith frbrer:P3025 , frbrer:P3026 , frbrer:P3027 , frbrer:P3028 , frbrer:P3029 , frbrer:P3030 , frbrer:P3053 , frbrer:P3054 , frbrer:P3055 , frbrer:P3056 , frbrer:P3057 , frbrer:P3058 .

frbrer:P3025 a owl:ObjectProperty ;
	rdfs:label "has physical medium"@en ;
	rdfs:isDefinedBy <http://iflastandards.info/ns/fr/frbr/frbrer/> ;
	rdfs:domain frbrer:C1003 ;
	owl:propertyDisjointWith frbrer:P3026 , frbrer:P3027 , frbrer:P3028 , frbrer:P3029 , frbrer:P3030 , frbrer:P3053 , frbrer:P3054 , frbrer:P3055 , frbrer:P3056 , frbrer:P3057 , frbrer:P3058 .

frbrer:P3026 a owl:ObjectProperty ;
	rdfs:label "has capture mode"@en ;
	rdfs:isDefinedBy <http://iflastandards.info/ns/fr/frbr/frbrer/> ;
	rdfs:domain frbrer:C1003 ;
	owl:propertyDisjointWith frbrer:P3027 , frbrer:P3028 , frbrer:P3029 , frbrer:P3030 , frbrer:P3053 , frbrer:P3054 , frbrer:P3055 , frbrer:P3056 , frbrer:P3057 , frbrer:P3058 .

frbrer:P3027 a owl:ObjectProperty ;
	rdfs:label "has dimensions of the carrier"@en ;
	rdfs:isDefinedBy <http://iflastandards.info/ns/fr/frbr/frbrer/> ;
	rdfs:domain frbrer:C1003 ;
	owl:propertyDisjointWith frbrer:P3028 , frbrer:P3029 , frbrer:P3030 , frbrer:P3053 , frbrer:P3054 , frbrer:P3055 , frbrer:P3056 , frbrer:P3057 , frbrer:P3058 .

frbrer:P3028 a owl:ObjectProperty ;
	rdfs:label "has manifestation identifier"@en ;
	rdfs:isDefinedBy <http://iflastandards.info/ns/fr/frbr/frbrer/> ;
	rdfs:domain frbrer:C1003 ;
	owl:propertyDisjointWith frbrer:P3029 , frbrer:P3030 , frbrer:P3053 , frbrer:P3054 , frbrer:P3055 , frbrer:P3056 , frbrer:P3057 , frbrer:P3058 .

frbrer:P3029 a owl:ObjectProperty ;
	rdfs:label "has terms of availability"@en ;
	rdfs:isDefinedBy <http://iflastandards.info/ns/fr/frbr/frbrer/> ;
	rdfs:domain frbrer:C1003 ;
	owl:propertyDisjointWith frbrer:P3030 , frbrer:P3053 , frbrer:P3054 , frbrer:P3055 , frbrer:P3056 , frbrer:P3057 , frbrer:P3058 .

frbrer:P3030 a owl:ObjectProperty ;
	rdfs:label "has access restrictions on the manifestation"@en ;
	rdfs:isDefinedBy <http://iflastandards.info/ns/fr/frbr/frbrer/> ;
	rdfs:domain frbrer:C1003 ;
	owl:propertyDisjointWith frbrer:P3053 , frbrer:P3054 , frbrer:P3055 , frbrer:P3056 , frbrer:P3057 , frbrer:P3058 .

frbrer:P3031 a owl:ObjectProperty ;
	rdfs:label "has item identifier"@en ;
	rdfs:isDefinedBy <http://iflastandards.info/ns/fr/frbr/frbrer/> ;
	rdfs:domain frbrer:C1004 ;
	owl:propertyDisjointWith frbrer:P3032 , frbrer:P3033 , frbrer:P3034 , frbrer:P3035 , frbrer:P3036 , frbrer:P3037 , frbrer:P3038 , frbrer:P3052 .

frbrer:P3032 a owl:ObjectProperty ;
	rdfs:label "has fingerprint"@en ;
	rdfs:isDefinedBy <http://iflastandards.info/ns/fr/frbr/frbrer/> ;
	rdfs:domain frbrer:C1004 ;
	owl:propertyDisjointWith frbrer:P3033 , frbrer:P3034 , frbrer:P3035 , frbrer:P3036 , frbrer:P3037 , frbrer:P3038 , frbrer:P3052 .

frbrer:P3033 a owl:ObjectProperty ;
	rdfs:label "has provenance of the item"@en ;
	rdfs:isDefinedBy <http://iflastandards.info/ns/fr/frbr/frbrer/> ;
	rdfs:domain frbrer:C1004 ;
	owl:propertyDisjointWith frbrer:P3034 , frbrer:P3035 , frbrer:P3036 , frbrer:P3037 , frbrer:P3038 , frbrer:P3052 .

frbrer:P3034 a owl:ObjectProperty ;
	rdfs:label "has exhibition history"@en ;
	rdfs:isDefinedBy <http://iflastandards.info/ns/fr/frbr/frbrer/> ;
	rdfs:domain frbrer:C1004 ;
	owl:propertyDisjointWith frbrer:P3035 , frbrer:P3036 , frbrer:P3037 , frbrer:P3038 , frbrer:P3052 .

frbrer:P3035 a owl:ObjectProperty ;
	rdfs:label "has condition of the item"@en ;
	rdfs:isDefinedBy <http://iflastandards.info/ns/fr/frbr/frbrer/> ;
	rdfs:domain frbrer:C1004 ;
	owl:propertyDisjointWith frbrer:P3036 , frbrer:P3037 , frbrer:P3038 , frbrer:P3052 .

frbrer:P3036 a owl:ObjectProperty ;
	rdfs:label "has treatment history"@en ;
	rdfs:isDefinedBy <http://iflastandards.info/ns/fr/frbr/frbrer/> ;
	rdfs:domain frbrer:C1004 ;
	owl:propertyDisjointWith frbrer:P3037 , frbrer:P3038 , frbrer:P3052 .

frbrer:P3037 a owl:ObjectProperty ;
	rdfs:label "has scheduled treatment"@en ;
	rdfs:isDefinedBy <http://iflastandards.info/ns/fr/frbr/frbrer/> ;
	rdfs:domain frbrer:C1004 ;
	owl:propertyDisjointWith frbrer:P3038 , frbrer:P3052 .

frbrer:P3038 a owl:ObjectProperty ;
	rdfs:label "has access restrictions on the item"@en ;
	rdfs:isDefinedBy <http://iflastandards.info/ns/fr/frbr/frbrer/> ;
	rdfs:domain frbrer:C1004 ;
	owl:propertyDisjointWith frbrer:P3052 .

frbrer:P3039 a owl:ObjectProperty ;
	rdfs:label "has name of person"@en ;
	rdfs:isDefinedBy <http://iflastandards.info/ns/fr/frbr/frbrer/> ;
	rdfs:domain frbrer:C1005 ;
	owl:propertyDisjointWith frbrer:P3040 , frbrer:P3041 , frbrer:P3042 .

frbrer:P3040 a owl:ObjectProperty ;
	rdfs:label "has dates of person"@en ;
	rdfs:comment "Source documentation has \"includes\" prefixing the definition, interpreted as \"and other dates\" in the property description."@en ;
	rdfs:isDefinedBy <http://iflastandards.info/ns/fr/frbr/frbrer/> ;
	rdfs:domain frbrer:C1005 ;
	owl:propertyDisjointWith frbrer:P3041 , frbrer:P3042 .

frbrer:P3041 a owl:ObjectProperty ;
	rdfs:label "has title of person"@en ;
	rdfs:isDefinedBy <http://iflastandards.info/ns/fr/frbr/frbrer/> ;
	rdfs:domain frbrer:C1005 ;
	owl:propertyDisjointWith frbrer:P3042 .

frbrer:P3042 a owl:ObjectProperty ;
	rdfs:label "has other designation associated with the person"@en ;
	rdfs:isDefinedBy <http://iflastandards.info/ns/fr/frbr/frbrer/> ;
	rdfs:domain frbrer:C1005 .

frbrer:P3043 a owl:ObjectProperty ;
	rdfs:label "has name of the corporate body"@en ;
	rdfs:isDefinedBy <http://iflastandards.info/ns/fr/frbr/frbrer/> ;
	rdfs:domain frbrer:C1006 ;
	owl:propertyDisjointWith frbrer:P3044 , frbrer:P3045 , frbrer:P3046 , frbrer:P3047 .

frbrer:P3044 a owl:ObjectProperty ;
	rdfs:label "has number associated with the corporate body"@en ;
	rdfs:isDefinedBy <http://iflastandards.info/ns/fr/frbr/frbrer/> ;
	rdfs:domain frbrer:C1006 ;
	owl:propertyDisjointWith frbrer:P3045 , frbrer:P3046 , frbrer:P3047 .

frbrer:P3045 a owl:ObjectProperty ;
	rdfs:label "has place associated with the corporate body"@en ;
	rdfs:isDefinedBy <http://iflastandards.info/ns/fr/frbr/frbrer/> ;
	rdfs:domain frbrer:C1006 ;
	owl:propertyDisjointWith frbrer:P3046 , frbrer:P3047 .

frbrer:P3046 a owl:ObjectProperty ;
	rdfs:label "has date associated with the corporate body"@en ;
	rdfs:isDefinedBy <http://iflastandards.info/ns/fr/frbr/frbrer/> ;
	rdfs:domain frbrer:C1006 ;
	owl:propertyDisjointWith frbrer:P3047 .

frbrer:P3047 a owl:ObjectProperty ;
	rdfs:label "has other designation associated with the corporate body"@en ;
	rdfs:isDefinedBy <http://iflastandards.info/ns/fr/frbr/frbrer/> ;
	rdfs:domain frbrer:C1006 .

frbrer:P3048 a owl:ObjectProperty ;
	rdfs:label "has term for the concept"@en ;
	rdfs:isDefinedBy <http://iflastandards.info/ns/fr/frbr/frbrer/> ;
	rdfs:domain frbrer:C1007 .

frbrer:P3049 a owl:ObjectProperty ;
	rdfs:label "has term for the object"@en ;
	rdfs:isDefinedBy <http://iflastandards.info/ns/fr/frbr/frbrer/> ;
	rdfs:domain frbrer:C1008 .

frbrer:P3050 a owl:ObjectProperty ;
	rdfs:label "has term for the event"@en ;
	rdfs:isDefinedBy <http://iflastandards.info/ns/fr/frbr/frbrer/> ;
	rdfs:domain frbrer:C1009 .

frbrer:P3051 a owl:ObjectProperty ;
	rdfs:label "has term for the place"@en ;
	rdfs:isDefinedBy <http://iflastandards.info/ns/fr/frbr/frbrer/> ;
	rdfs:domain frbrer:C1010 .

frbrer:P3052 a owl:ObjectProperty ;
	rdfs:label "has marks or inscriptions"@en ;
	rdfs:comment "Source documentation has \"marks/inscriptions\"; slash character replaced with \"or\" to improve clarity."@en ;
	rdfs:isDefinedBy <http://iflastandards.info/ns/fr/frbr/frbrer/> ;
	rdfs:domain frbrer:C1004 .

frbrer:P3053 a owl:ObjectProperty ;
	rdfs:label "has source for acquisition or access authorization"@en ;
	rdfs:comment "Source documentation has \"acquisition/access\"; slash character replaced with \"or\" to improve clarity."@en ;
	rdfs:isDefinedBy <http://iflastandards.info/ns/fr/frbr/frbrer/> ;
	rdfs:domain frbrer:C1003 ;
	owl:propertyDisjointWith frbrer:P3054 , frbrer:P3055 , frbrer:P3057 , frbrer:P3058 .

frbrer:P3054 a owl:ObjectProperty ;
	rdfs:label "has fabricator or manufacturer"@en ;
	rdfs:comment "Source documentation has \"fabricator/manufacturer\"; slash character replaced with \"or\" to improve clarity."@en ;
	rdfs:isDefinedBy <http://iflastandards.info/ns/fr/frbr/frbrer/> ;
	rdfs:domain frbrer:C1003 ;
	owl:propertyDisjointWith frbrer:P3055 , frbrer:P3056 , frbrer:P3057 , frbrer:P3058 .

_:node18r56emdgx1 a owl:AllDisjointProperties ;
	owl:members _:node18r56emdgx2 .

_:node18r56emdgx2 rdf:first frbrer:P3054 ;
	rdf:rest rdf:nil .

frbrer:P3055 a owl:ObjectProperty ;
	rdfs:label "has date of publication or distribution"@en ;
	rdfs:comment "Source documentation has \"publication/distribution\"; slash character replaced with \"or\" to improve clarity."@en ;
	rdfs:isDefinedBy <http://iflastandards.info/ns/fr/frbr/frbrer/> ;
	rdfs:domain frbrer:C1003 ;
	owl:propertyDisjointWith frbrer:P3056 , frbrer:P3057 , frbrer:P3058 .

frbrer:P3056 a owl:ObjectProperty ;
	rdfs:label "has publisher or distributor"@en ;
	rdfs:comment "Source documentation has \"publisher/distributor\"; slash character replaced with \"or\" to improve clarity."@en ;
	rdfs:isDefinedBy <http://iflastandards.info/ns/fr/frbr/frbrer/> ;
	rdfs:domain frbrer:C1003 ;
	owl:propertyDisjointWith frbrer:P3057 , frbrer:P3058 .

frbrer:P3057 a owl:ObjectProperty ;
	rdfs:label "has place of publication or distribution"@en ;
	rdfs:comment "Source documentation has \"publication/distribution\"; slash character replaced with \"or\" to improve clarity."@en ;
	rdfs:isDefinedBy <http://iflastandards.info/ns/fr/frbr/frbrer/> ;
	rdfs:domain frbrer:C1003 ;
	owl:propertyDisjointWith frbrer:P3058 .

frbrer:P3058 a owl:ObjectProperty ;
	rdfs:label "has edition or issue designation"@en ;
	rdfs:comment "Source documentation has \"edition/issue\"; slash character replaced with \"or\" to improve clarity."@en ;
	rdfs:isDefinedBy <http://iflastandards.info/ns/fr/frbr/frbrer/> ;
	rdfs:domain frbrer:C1003 .

frbrer:P3059 a owl:ObjectProperty ;
	rdfs:label "has medium of performance (musical work)"@en ;
	rdfs:isDefinedBy <http://iflastandards.info/ns/fr/frbr/frbrer/> ;
	rdfs:domain frbrer:C1001 .

frbrer:P3060 a owl:ObjectProperty ;
	rdfs:label "has numeric designation (musical work)"@en ;
	rdfs:isDefinedBy <http://iflastandards.info/ns/fr/frbr/frbrer/> ;
	rdfs:domain frbrer:C1001 .

frbrer:P3061 a owl:ObjectProperty ;
	rdfs:label "has key (musical work)"@en ;
	rdfs:isDefinedBy <http://iflastandards.info/ns/fr/frbr/frbrer/> ;
	rdfs:domain frbrer:C1001 .

frbrer:P3062 a owl:ObjectProperty ;
	rdfs:label "has coordinates (cartographic work)"@en ;
	rdfs:isDefinedBy <http://iflastandards.info/ns/fr/frbr/frbrer/> ;
	rdfs:domain frbrer:C1001 .

frbrer:P3063 a owl:ObjectProperty ;
	rdfs:label "has equinox (cartographic work)"@en ;
	rdfs:isDefinedBy <http://iflastandards.info/ns/fr/frbr/frbrer/> ;
	rdfs:domain frbrer:C1001 .

frbrer:P3064 a owl:ObjectProperty ;
	rdfs:label "has sequencing pattern (serial)"@en ;
	rdfs:isDefinedBy <http://iflastandards.info/ns/fr/frbr/frbrer/> ;
	rdfs:domain frbrer:C1002 .

frbrer:P3065 a owl:ObjectProperty ;
	rdfs:label "has expected regularity of issue (serial)"@en ;
	rdfs:isDefinedBy <http://iflastandards.info/ns/fr/frbr/frbrer/> ;
	rdfs:domain frbrer:C1002 .

frbrer:P3066 a owl:ObjectProperty ;
	rdfs:label "has expected frequency of issue (serial)"@en ;
	rdfs:isDefinedBy <http://iflastandards.info/ns/fr/frbr/frbrer/> ;
	rdfs:domain frbrer:C1002 .

frbrer:P3067 a owl:ObjectProperty ;
	rdfs:label "has type of score (musical notation)"@en ;
	rdfs:isDefinedBy <http://iflastandards.info/ns/fr/frbr/frbrer/> ;
	rdfs:domain frbrer:C1002 .

frbrer:P3068 a owl:ObjectProperty ;
	rdfs:label "has medium of performance (musical notation or recorded sound)"@en ;
	rdfs:isDefinedBy <http://iflastandards.info/ns/fr/frbr/frbrer/> ;
	rdfs:domain frbrer:C1002 .

frbrer:P3070 a owl:ObjectProperty ;
	rdfs:label "has recording technique (remote sensing image)"@en ;
	rdfs:isDefinedBy <http://iflastandards.info/ns/fr/frbr/frbrer/> ;
	rdfs:domain frbrer:C1002 .

frbrer:P3071 a owl:ObjectProperty ;
	rdfs:label "has special characteristic (remote sensing image)"@en ;
	rdfs:isDefinedBy <http://iflastandards.info/ns/fr/frbr/frbrer/> ;
	rdfs:domain frbrer:C1002 .

frbrer:P3072 a owl:ObjectProperty ;
	rdfs:label "has technique (graphic or projected image)"@en ;
	rdfs:isDefinedBy <http://iflastandards.info/ns/fr/frbr/frbrer/> ;
	rdfs:domain frbrer:C1002 .

frbrer:P3074 a owl:ObjectProperty ;
	rdfs:label "has typeface (printed book)"@en ;
	rdfs:isDefinedBy <http://iflastandards.info/ns/fr/frbr/frbrer/> ;
	rdfs:domain frbrer:C1003 .

frbrer:P3075 a owl:ObjectProperty ;
	rdfs:label "has type size (printed book)"@en ;
	rdfs:isDefinedBy <http://iflastandards.info/ns/fr/frbr/frbrer/> ;
	rdfs:domain frbrer:C1003 .

frbrer:P3076 a owl:ObjectProperty ;
	rdfs:label "has foliation (hand-printed book)"@en ;
	rdfs:isDefinedBy <http://iflastandards.info/ns/fr/frbr/frbrer/> ;
	rdfs:domain frbrer:C1003 .

frbrer:P3077 a owl:ObjectProperty ;
	rdfs:label "has collation (hand-printed book)"@en ;
	rdfs:isDefinedBy <http://iflastandards.info/ns/fr/frbr/frbrer/> ;
	rdfs:domain frbrer:C1003 .

frbrer:P3078 a owl:ObjectProperty ;
	rdfs:label "has publication status (serial)"@en ;
	rdfs:isDefinedBy <http://iflastandards.info/ns/fr/frbr/frbrer/> ;
	rdfs:domain frbrer:C1003 .

frbrer:P3079 a owl:ObjectProperty ;
	rdfs:label "has numbering (serial)"@en ;
	rdfs:isDefinedBy <http://iflastandards.info/ns/fr/frbr/frbrer/> ;
	rdfs:domain frbrer:C1003 .

frbrer:P3080 a owl:ObjectProperty ;
	rdfs:label "has playing speed (sound recording)"@en ;
	rdfs:isDefinedBy <http://iflastandards.info/ns/fr/frbr/frbrer/> ;
	rdfs:domain frbrer:C1003 .

frbrer:P3081 a owl:ObjectProperty ;
	rdfs:label "has groove width"@en ;
	rdfs:isDefinedBy <http://iflastandards.info/ns/fr/frbr/frbrer/> ;
	rdfs:domain frbrer:C1003 .

frbrer:P3082 a owl:ObjectProperty ;
	rdfs:label "has kind of cutting (sound recording)"@en ;
	rdfs:isDefinedBy <http://iflastandards.info/ns/fr/frbr/frbrer/> ;
	rdfs:domain frbrer:C1003 .

frbrer:P3083 a owl:ObjectProperty ;
	rdfs:label "has tape configuration (sound recording)"@en ;
	rdfs:isDefinedBy <http://iflastandards.info/ns/fr/frbr/frbrer/> ;
	rdfs:domain frbrer:C1003 .

frbrer:P3084 a owl:ObjectProperty ;
	rdfs:label "has kind of sound (sound recording)"@en ;
	rdfs:isDefinedBy <http://iflastandards.info/ns/fr/frbr/frbrer/> ;
	rdfs:domain frbrer:C1003 .

frbrer:P3085 a owl:ObjectProperty ;
	rdfs:label "has special reproduction characteristic (sound recording)"@en ;
	rdfs:isDefinedBy <http://iflastandards.info/ns/fr/frbr/frbrer/> ;
	rdfs:domain frbrer:C1003 .

frbrer:P3086 a owl:ObjectProperty ;
	rdfs:label "has colour (image)"@en ;
	rdfs:isDefinedBy <http://iflastandards.info/ns/fr/frbr/frbrer/> ;
	rdfs:domain frbrer:C1003 .

frbrer:P3087 a owl:ObjectProperty ;
	rdfs:label "has reduction ratio (microform)"@en ;
	rdfs:isDefinedBy <http://iflastandards.info/ns/fr/frbr/frbrer/> ;
	rdfs:domain frbrer:C1003 .

frbrer:P3088 a owl:ObjectProperty ;
	rdfs:label "has polarity (microform or visual projection)"@en ;
	rdfs:isDefinedBy <http://iflastandards.info/ns/fr/frbr/frbrer/> ;
	rdfs:domain frbrer:C1003 .

frbrer:P3089 a owl:ObjectProperty ;
	rdfs:label "has generation (microform or visual projection)"@en ;
	rdfs:isDefinedBy <http://iflastandards.info/ns/fr/frbr/frbrer/> ;
	rdfs:domain frbrer:C1003 .

frbrer:P3090 a owl:ObjectProperty ;
	rdfs:label "has presentation format (visual projection)"@en ;
	rdfs:isDefinedBy <http://iflastandards.info/ns/fr/frbr/frbrer/> ;
	rdfs:domain frbrer:C1003 .

frbrer:P3093 a owl:ObjectProperty ;
	rdfs:label "has system requirements (electronic resource)"@en ;
	rdfs:comment "Source documentation has \"includes\" prefixing the definition, interpreted as \"and other system components\" in the property description."@en ;
	rdfs:isDefinedBy <http://iflastandards.info/ns/fr/frbr/frbrer/> ;
	rdfs:domain frbrer:C1003 .

frbrer:P3094 a owl:ObjectProperty ;
	rdfs:label "has file characteristics (electronic resource)"@en ;
	rdfs:comment "Source documentation has \"include\" prefixing the definition, removed for being redundant with respect to \"and other characteristics\" in the property description."@en ;
	rdfs:isDefinedBy <http://iflastandards.info/ns/fr/frbr/frbrer/> ;
	rdfs:domain frbrer:C1003 .

frbrer:P3095 a owl:ObjectProperty ;
	rdfs:label "has mode of access (remote electronic resource)"@en ;
	rdfs:isDefinedBy <http://iflastandards.info/ns/fr/frbr/frbrer/> ;
	rdfs:domain frbrer:C1003 .

frbrer:P3096 a owl:ObjectProperty ;
	rdfs:label "has access address (remote electronic resource)"@en ;
	rdfs:isDefinedBy <http://iflastandards.info/ns/fr/frbr/frbrer/> ;
	rdfs:domain frbrer:C1003 .

frbrer:P3097 a owl:ObjectProperty ;
	rdfs:label "has scale (cartographic image or object)"@en ;
	rdfs:isDefinedBy <http://iflastandards.info/ns/fr/frbr/frbrer/> ;
	rdfs:domain frbrer:C1002 .

frbrer:P3098 a owl:ObjectProperty ;
	rdfs:label "has projection (cartographic image or object)"@en ;
	rdfs:isDefinedBy <http://iflastandards.info/ns/fr/frbr/frbrer/> ;
	rdfs:domain frbrer:C1002 .

frbrer:P3099 a owl:ObjectProperty ;
	rdfs:label "has presentation technique (cartographic image or object)"@en ;
	rdfs:isDefinedBy <http://iflastandards.info/ns/fr/frbr/frbrer/> ;
	rdfs:domain frbrer:C1002 .

frbrer:P3100 a owl:ObjectProperty ;
	rdfs:label "has representation of relief (cartographic image or object)"@en ;
	rdfs:isDefinedBy <http://iflastandards.info/ns/fr/frbr/frbrer/> ;
	rdfs:domain frbrer:C1002 .

frbrer:P3101 a owl:ObjectProperty ;
	rdfs:label "has geodetic, grid and vertical measurement (cartographic image or object)"@en ;
	rdfs:comment "Source documentation has \"includes\" prefixing the definition, interpreted as \"and other geodetic, grid and vertical measurements\" in the property description."@en ;
	rdfs:isDefinedBy <http://iflastandards.info/ns/fr/frbr/frbrer/> ;
	rdfs:domain frbrer:C1002 .

RegAp:status a owl:ObjectProperty .

foaf:homepage a owl:ObjectProperty .

RegAp:name a owl:DatatypeProperty .

skos:altLabel a owl:DatatypeProperty .

skos:definition a owl:DatatypeProperty .

skos:note a owl:DatatypeProperty .

skos:prefLabel a owl:DatatypeProperty .

skos:scopeNote a owl:DatatypeProperty .

frbrer:C1001 a owl:Class ;
	rdfs:label "Work"@en ;
	owl:disjointWith frbrer:C1002 , frbrer:C1003 , frbrer:C1004 , frbrer:C1005 , frbrer:C1006 , frbrer:C1007 , frbrer:C1008 , frbrer:C1009 , frbrer:C1010 ;
	rdfs:isDefinedBy <http://iflastandards.info/ns/fr/frbr/frbrer/> .

frbrer:C1002 a owl:Class ;
	rdfs:label "Expression"@en ;
	rdfs:subClassOf _:node18r56emdgx3 .

_:node18r56emdgx3 a owl:Restriction ;
	owl:onProperty frbrer:P2002 ;
	owl:onClass frbrer:C1001 ;
	owl:qualifiedCardinality "1"^^xsd:nonNegativeInteger .

frbrer:C1002 owl:disjointWith frbrer:C1003 , frbrer:C1004 , frbrer:C1005 , frbrer:C1006 , frbrer:C1007 , frbrer:C1008 , frbrer:C1009 , frbrer:C1010 ;
	rdfs:isDefinedBy <http://iflastandards.info/ns/fr/frbr/frbrer/> .

frbrer:C1003 a owl:Class ;
	rdfs:label "Manifestation"@en ;
	rdfs:subClassOf _:node18r56emdgx4 .

_:node18r56emdgx4 a owl:Restriction ;
	owl:onProperty frbrer:P2004 ;
	owl:onClass frbrer:C1002 ;
	owl:minQualifiedCardinality "1"^^xsd:nonNegativeInteger .

frbrer:C1003 owl:disjointWith frbrer:C1004 , frbrer:C1005 , frbrer:C1006 , frbrer:C1007 , frbrer:C1008 , frbrer:C1009 , frbrer:C1010 ;
	rdfs:isDefinedBy <http://iflastandards.info/ns/fr/frbr/frbrer/> .

frbrer:C1004 a owl:Class ;
	rdfs:label "Item"@en ;
	rdfs:subClassOf _:node18r56emdgx5 .

_:node18r56emdgx5 a owl:Restriction ;
	owl:onProperty frbrer:P2006 ;
	owl:onClass frbrer:C1003 ;
	owl:qualifiedCardinality "1"^^xsd:nonNegativeInteger .

frbrer:C1004 owl:disjointWith frbrer:C1005 , frbrer:C1006 , frbrer:C1007 , frbrer:C1008 , frbrer:C1009 , frbrer:C1010 ;
	rdfs:isDefinedBy <http://iflastandards.info/ns/fr/frbr/frbrer/> .

frbrer:C1005 a owl:Class ;
	rdfs:label "Person"@en ;
	owl:disjointWith frbrer:C1006 , frbrer:C1007 , frbrer:C1008 , frbrer:C1009 , frbrer:C1010 ;
	rdfs:isDefinedBy <http://iflastandards.info/ns/fr/frbr/frbrer/> .

frbrer:C1006 a owl:Class ;
	rdfs:label "Corporate Body"@en ;
	owl:disjointWith frbrer:C1007 , frbrer:C1008 , frbrer:C1009 , frbrer:C1010 ;
	rdfs:isDefinedBy <http://iflastandards.info/ns/fr/frbr/frbrer/> .

frbrer:C1007 a owl:Class ;
	rdfs:label "Concept"@en ;
	owl:disjointWith frbrer:C1008 , frbrer:C1009 , frbrer:C1010 ;
	rdfs:isDefinedBy <http://iflastandards.info/ns/fr/frbr/frbrer/> .

frbrer:C1008 a owl:Class ;
	rdfs:label "Object"@en ;
	owl:disjointWith frbrer:C1009 , frbrer:C1010 ;
	rdfs:isDefinedBy <http://iflastandards.info/ns/fr/frbr/frbrer/> .

frbrer:C1009 a owl:Class ;
	rdfs:label "Event"@en ;
	owl:disjointWith frbrer:C1010 ;
	rdfs:isDefinedBy <http://iflastandards.info/ns/fr/frbr/frbrer/> .

frbrer:C1010 a owl:Class ;
	rdfs:label "Place"@en ;
	rdfs:isDefinedBy <http://iflastandards.info/ns/fr/frbr/frbrer/> .

skos:Concept a owl:Class .

<http://iflastandards.info/ns/fr/frbr/frbrer/> a owl:NamedIndividual ;
	skos:note "Based on the current text, Feb 2009."@en ;
	dc:title "FRBRer model"@en ;
	foaf:homepage publications:functional-requirements-for-bibliographic-records .

frbrer:C1001 a owl:NamedIndividual ;
	skos:definition "A distinct intellectual or artistic creation."@en ;
	skos:scopeNote "A work is an abstract entity; there is no single material object one can point to as the work. We recognize the work through individual realizations or expressions of the work, but the work itself exists only in the commonality of content between and among the various expressions of the work. Because the notion of a work is abstract, it is difficult to define precise boundaries for the entity. The concept of what constitutes a work and where the line of demarcation lies between one work and another may in fact be viewed differently from one culture to another. Consequently the bibliographic conventions established by various cultures or national groups may differ in terms of the criteria they use for determining the boundaries between one work and another. For the purposes of this model variant texts incorporating revisions or updates to an earlier text are viewed simply as expressions of the same work (i.e., the variant texts are not viewed as separate works). Similarly, abridgements or enlargements of an existing text, or the addition of parts or an accompaniment to a musical composition are considered to be different expressions of the same work. Translations from one language to another, musical transcriptions and arrangements, and dubbed or subtitled versions of a film are also considered simply as different expressions of the same original work. By contrast, when the modification of a work involves a significant degree of independent intellectual or artistic effort, the result is viewed, for the purpose of this model, as a new work. Thus paraphrases, rewritings, adaptations for children, parodies, musical variations on a theme and free transcriptions of a musical composition are considered to represent new works. Similarly, adaptations of a work from one literary or art form to another (e.g., dramatizations, adaptations from one medium of the graphic arts to another, etc.) are considered to represent new works. Abstracts, digests and summaries are also considered to represent new works."@en ;
	RegAp:name "Work"@en ;
	RegAp:status <http://metadataregistry.org/uri/RegStatus/1001> .

frbrer:C1002 a owl:NamedIndividual ;
	skos:scopeNote "An expression is the specific intellectual or artistic form that a work takes each time it is \"realized\". Expression encompasses, for example, the specific words, sentences, paragraphs, etc. that result from the realization of a work in the form of a text, or the particular sounds, phrasing, etc. resulting from the realization of a musical work. The boundaries of the entity expression are defined, however, so as to exclude aspects of physical form, such as typeface and page layout, that are not integral to the intellectual or artistic realization of the work as such. Inasmuch as the form of expression is an inherent characteristic of the expression, any change in form (e.g., from alpha-numeric notation to spoken word) results in a new expression. Similarly, changes in the intellectual conventions or instruments that are employed to express a work (e.g., translation from one language to another) result in the production of a new expression. If a text is revised or modified, the resulting expression is considered to be a new expression. The degree to which bibliographic distinctions are made between variant expressions of a work will depend to some extent on the nature of the work itself, on the anticipated needs of users and on what the cataloguer can reasonably be expected to recognize from the manifestation being described. Differences in form of expression (e.g., the differences between the expression of a work in the form of musical notation and the expression of the same work in the form of recorded sound) will normally be reflected in the bibliographic record, no matter what the nature of the work itself may be. Variant expressions in the same form (e.g., revised versions of a text) will often be indirectly identified as different expressions because the variation is apparent from the data associated with an attribute used to identify the manifestation in which the expression is embodied (e.g., an edition statement). Variations that would be evident only from a more detailed analysis and comparison of expressions (e.g., variations between several of the early texts of Shakespeare's Hamlet) would normally be reflected in the data only if the nature or stature of the work warranted such analysis, and only if it was anticipated that the distinction would be important to users."@en ;
	RegAp:name "Expression"@en ;
	skos:definition "The intellectual or artistic realization of a work in the form of alpha-numeric, musical, or choreographic notation, sound, image, object, movement, etc., or any combination of such forms."@en ;
	RegAp:status <http://metadataregistry.org/uri/RegStatus/1001> .

frbrer:C1003 a owl:NamedIndividual ;
	RegAp:name "Manifestation"@en ;
	skos:scopeNote "The entity defined as manifestation encompasses a wide range of materials, including manuscripts, books, periodicals, maps, posters, sound recordings, films, video recordings, CD-ROMs, multimedia kits, etc. As an entity, manifestation represents all the physical objects that bear the same characteristics, in respect to both intellectual content and physical form. When a work is realized, the resulting expression of the work may be physically embodied on or in a medium such as paper, audio tape, video tape, canvas, plaster, etc. That physical embodiment constitutes a manifestation of the work. In some cases there may be only a single physical exemplar produced of that manifestation of the work (e.g., an author's manuscript, a tape recorded for an oral history archive, an original oil painting, etc.). In other cases there are multiple copies produced in order to facilitate public dissemination or distribution. In those cases there is normally a more formal production process involved, and a publisher, producer, or distributor takes responsibility for the process. In other cases there may be only a limited number of copies made of an original exemplar for purposes such as private study (e.g., a dubbing of an original recording of a piece of music), or preservation (e.g., a photocopy produced on permanent paper of an author's original typescript). Whether the scope of production is broad (e.g., in the case of publication, etc.) or limited (e.g., in the case of copies made for private study, etc.), the set of copies produced in each case constitutes a manifestation. All copies produced that form part of the same set are considered to be copies of the same manifestation. The boundaries between one manifestation and another are drawn on the basis of both intellectual content and physical form. When the production process involves changes in physical form the resulting product is considered a new manifestation. Changes in physical form include changes affecting display characteristics (e.g., a change in typeface, size of font, page layout, etc.), changes in physical medium (e.g., a change from paper to microfilm as the medium of conveyance), and changes in the container (e.g., a change from cassette to cartridge as the container for a tape). Where the production process involves a publisher, producer, distributor, etc., and there are changes signalled in the product that are related to publication, marketing, etc. (e.g., a change in publisher, repackaging, etc.), the resulting product may be considered a new manifestation. Whenever the production process involves modifications, additions, deletions, etc. that affect the intellectual or artistic content, the result is a new manifestation embodying a new expression of the work. Changes that occur deliberately or even inadvertently in the production process that affect the copies result, strictly speaking, in a new manifestation. A manifestation resulting from such a change may be identified as a particular \"state\" or \"issue\" of the publication. Changes that occur to an individual copy after the production process is complete (e.g., the loss of a page, rebinding, etc.) are not considered to result in a new manifestation. That copy is simply considered to be an exemplar (or item) of the manifestation that deviates from the copy as produced."@en ;
	skos:definition "The physical embodiment of an expression of a work."@en ;
	RegAp:status <http://metadataregistry.org/uri/RegStatus/1001> .

frbrer:C1004 a owl:NamedIndividual ;
	skos:definition "A single exemplar of a manifestation."@en ;
	RegAp:name "Item"@en ;
	skos:scopeNote "The entity defined as item is a concrete entity. It is in many instances a single physical object (e.g., a copy of a one-volume monograph, a single audio cassette, etc.). There are instances, however, where the entity defined as item comprises more than one physical object (e.g., a monograph issued as two separately bound volumes, a recording issued on three separate compact discs, etc.). In terms of intellectual content and physical form, an item exemplifying a manifestation is normally the same as the manifestation itself. However, variations may occur from one item to another, even when the items exemplify the same manifestation, where those variations are the result of actions external to the intent of the producer of the manifestation (e.g., damage occurring after the item was produced, binding performed by a library, etc.)."@en ;
	RegAp:status <http://metadataregistry.org/uri/RegStatus/1001> .

frbrer:C1005 a owl:NamedIndividual ;
	skos:definition "An individual."@en ;
	RegAp:name "Person"@en ;
	skos:scopeNote "The entity defined as person encompasses individuals that are deceased as well as those that are living. For the purposes of this model persons are treated as entities only to the extent that they are involved in the creation or realization of a work (e.g., as authors, composers, artists, editors, translators, directors, performers, etc.), or are the subject of a work (e.g., as the subject of a biographical or autobiographical work, of a history, etc.)."@en ;
	RegAp:status <http://metadataregistry.org/uri/RegStatus/1001> .

frbrer:C1006 a owl:NamedIndividual ;
	skos:definition "An organization or group of individuals and/or organizations acting as a unit."@en ;
	RegAp:name "CorporateBody"@en ;
	skos:scopeNote "The entity defined as corporate body encompasses organizations and groups of individuals and-or organizations that are identified by a particular name, including occasional groups and groups that are constituted as meetings, conferences, congresses, expeditions, exhibitions, festivals, fairs, etc. The entity also encompasses organizations that act as territorial authorities, exercising or claiming to exercise government functions over a certain territory, such as a federation, a state, a region, a local municipality, etc. The entity encompasses organizations and groups that are defunct as well as those that continue to operate.  For the purposes of this model corporate bodies are treated as entities only to the extent that they are involved in the creation or realization of a work (e.g., as the sponsors or endorsers of a work, etc.), or are the subject of a work (e.g., as the subject of a history, etc.)."@en ;
	RegAp:status <http://metadataregistry.org/uri/RegStatus/1001> .

frbrer:C1007 a owl:NamedIndividual ;
	skos:definition "An abstract notion or idea."@en ;
	RegAp:name "Concept"@en ;
	skos:scopeNote "The entity defined as concept encompasses a comprehensive range of abstractions that may be the subject of a work: fields of knowledge, disciplines, schools of thought (philosophies, religions, political ideologies, etc.), theories, processes, techniques, practices, etc. A concept may be broad in nature or narrowly defined and precise. For the purposes of this model concepts are treated as entities only to the extent that they are the subject of a work (e.g., as the subject of a philosophical treatise, of a critique of a school of thought, etc.)."@en ;
	RegAp:status <http://metadataregistry.org/uri/RegStatus/1001> .

frbrer:C1008 a owl:NamedIndividual ;
	skos:definition "A material thing."@en ;
	RegAp:name "Object"@en ;
	skos:scopeNote "The entity defined as object encompasses a comprehensive range of material things that may be the subject of a work: animate and inanimate objects occurring in nature; fixed, movable, and moving objects that are the product of human creation; objects that no longer exist. For the purposes of this model objects are treated as entities only to the extent that they are the subject of a work (e.g., as the subject of a scientific study, etc.)."@en ;
	RegAp:status <http://metadataregistry.org/uri/RegStatus/1001> .

frbrer:C1009 a owl:NamedIndividual ;
	skos:definition "An action or occurrence."@en ;
	RegAp:name "Event"@en ;
	skos:scopeNote "The entity defined as event encompasses a comprehensive range of actions and occurrences that may be the subject of a work: historical events, epochs, periods of time, etc. For the purposes of this model events are treated as entities only to the extent that they are the subject of a work (e.g., the subject of an historical treatise, of a painting, etc.)."@en ;
	RegAp:status <http://metadataregistry.org/uri/RegStatus/1001> .

frbrer:C1010 a owl:NamedIndividual ;
	skos:definition "A location."@en ;
	RegAp:name "Place"@en ;
	skos:scopeNote "The entity defined as place encompasses a comprehensive range of locations: terrestrial and extra-terrestrial; historical and contemporary; geographic features and geo-political jurisdictions. For the purposes of this model places are treated as entities only to the extent that they are the subject of a work (e.g., the subject of a map or atlas, or of a travel guide, etc.)."@en ;
	RegAp:status <http://metadataregistry.org/uri/RegStatus/1001> .

frbrer:P2001 a owl:NamedIndividual ;
	skos:definition "Relates a work to an expression that is the realization of the work."@en ;
	RegAp:name "isRealizedThrough"@en ;
	RegAp:status <http://metadataregistry.org/uri/RegStatus/1001> .

frbrer:P2002 a owl:NamedIndividual ;
	skos:definition "Relates an expression to the work that is realized through the expression."@en ;
	RegAp:name "isRealizationOf"@en ;
	RegAp:status <http://metadataregistry.org/uri/RegStatus/1001> .

frbrer:P2003 a owl:NamedIndividual ;
	skos:definition "Relates an expression to a manifestation that is the embodiment of the expression."@en ;
	RegAp:name "isEmbodiedIn"@en ;
	RegAp:status <http://metadataregistry.org/uri/RegStatus/1001> .

frbrer:P2004 a owl:NamedIndividual ;
	skos:definition "Relates a manifestation to an expression that is embodied in the manifestation."@en ;
	RegAp:name "isEmbodimentOf"@en ;
	RegAp:status <http://metadataregistry.org/uri/RegStatus/1001> .

frbrer:P2005 a owl:NamedIndividual ;
	skos:definition "Relates a manifestation to an item that is a single exemplar of the manifestation."@en ;
	RegAp:name "isExemplifiedBy"@en ;
	RegAp:status <http://metadataregistry.org/uri/RegStatus/1001> .

frbrer:P2006 a owl:NamedIndividual ;
	skos:definition "Relates an item to the manifestation that is exemplified by the item."@en ;
	RegAp:name "isExemplarOf"@en ;
	RegAp:status <http://metadataregistry.org/uri/RegStatus/1001> .

frbrer:P2007 a owl:NamedIndividual ;
	skos:definition "Relates a work to a corporate body that is responsible for the creation of the intellectual or artistic content of the work."@en ;
	RegAp:name "isCreatedByCorporateBody"@en ;
	RegAp:status <http://metadataregistry.org/uri/RegStatus/1001> .

frbrer:P2008 a owl:NamedIndividual ;
	skos:definition "Relates a corporate body to a work of which it is responsible for the creation of the intellectual or artistic content."@en ;
	RegAp:name "isCreatorCorporateBodyOf"@en ;
	RegAp:status <http://metadataregistry.org/uri/RegStatus/1001> .

frbrer:P2009 a owl:NamedIndividual ;
	skos:definition "Relates a work to a person who is responsible for the creation of the intellectual or artistic content of the work."@en ;
	RegAp:name "isCreatedByPerson"@en ;
	RegAp:status <http://metadataregistry.org/uri/RegStatus/1001> .

frbrer:P2010 a owl:NamedIndividual ;
	skos:definition "Relates a person to a work of which they are responsible for the creation of the intellectual or artistic content."@en ;
	RegAp:name "isCreatorPersonOf"@en ;
	RegAp:status <http://metadataregistry.org/uri/RegStatus/1001> .

frbrer:P2011 a owl:NamedIndividual ;
	skos:definition "Relates an expression to a corporate body that is responsible for the specifics of the intellectual or artistic realization or execution of the expression."@en ;
	RegAp:name "isRealizedByCorporateBody"@en ;
	RegAp:status <http://metadataregistry.org/uri/RegStatus/1001> .

frbrer:P2012 a owl:NamedIndividual ;
	skos:definition "Relates a corporate body to an expression of which it is responsible for the specifics of the intellectual or artistic realization or execution."@en ;
	RegAp:name "isRealizerCorporateBodyOf"@en ;
	RegAp:status <http://metadataregistry.org/uri/RegStatus/1001> .

frbrer:P2013 a owl:NamedIndividual ;
	skos:definition "Relates an expression to a person who is responsible for the specifics of the intellectual or artistic realization or execution of the expression."@en ;
	RegAp:name "isRealizedByPerson"@en ;
	RegAp:status <http://metadataregistry.org/uri/RegStatus/1001> .

frbrer:P2014 a owl:NamedIndividual ;
	skos:definition "Relates a person to an expression of which they are responsible for the specifics of the intellectual or artistic realization or execution."@en ;
	RegAp:name "isRealizerPersonOf"@en ;
	RegAp:status <http://metadataregistry.org/uri/RegStatus/1001> .

frbrer:P2015 a owl:NamedIndividual ;
	skos:definition "Relates a manifestation to a corporate body that is responsible for publishing, distributing, fabricating or manufacturing the manifestation."@en ;
	RegAp:name "isProducedByCorporateBody"@en ;
	RegAp:status <http://metadataregistry.org/uri/RegStatus/1001> .

frbrer:P2016 a owl:NamedIndividual ;
	skos:definition "Relates a corporate body to a manifestation of which it is responsible for publishing, distributing, fabricating or manufacturing."@en ;
	RegAp:name "isProducerCorporateBodyOf"@en ;
	RegAp:status <http://metadataregistry.org/uri/RegStatus/1001> .

frbrer:P2017 a owl:NamedIndividual ;
	skos:definition "Relates a manifestation to a person who is responsible for publishing, distributing, fabricating or manufacturing the manifestation."@en ;
	RegAp:name "isProducedByPerson"@en ;
	RegAp:status <http://metadataregistry.org/uri/RegStatus/1001> .

frbrer:P2018 a owl:NamedIndividual ;
	skos:definition "Relates a person to a manifestation of which they are responsible for publishing, distributing, fabricating or manufacturing."@en ;
	RegAp:name "isProducerPersonOf"@en ;
	RegAp:status <http://metadataregistry.org/uri/RegStatus/1001> .

frbrer:P2019 a owl:NamedIndividual ;
	skos:definition "Relates an item to a corporate body that is the owner or custodian of the item."@en ;
	RegAp:name "isOwnedByCorporateBody"@en ;
	RegAp:status <http://metadataregistry.org/uri/RegStatus/1001> .

frbrer:P2020 a owl:NamedIndividual ;
	skos:definition "Relates a corporate body to an item of which it is the owner or custodian."@en ;
	RegAp:name "isOwnerCorporateBodyOf"@en ;
	RegAp:status <http://metadataregistry.org/uri/RegStatus/1001> .

frbrer:P2021 a owl:NamedIndividual ;
	skos:definition "Relates an item to a person who is the owner or custodian of the item."@en ;
	RegAp:name "isOwnedByPerson"@en ;
	RegAp:status <http://metadataregistry.org/uri/RegStatus/1001> .

frbrer:P2022 a owl:NamedIndividual ;
	skos:definition "Relates a person to an item of which they are the owner or custodian."@en ;
	RegAp:name "isOwnerPersonOf"@en ;
	RegAp:status <http://metadataregistry.org/uri/RegStatus/1001> .

frbrer:P2023 a owl:NamedIndividual ;
	skos:definition "Relates a work to a concept that is the subject of the work."@en ;
	RegAp:name "hasAsSubjectConcept"@en ;
	RegAp:status <http://metadataregistry.org/uri/RegStatus/1001> .

frbrer:P2024 a owl:NamedIndividual ;
	skos:definition "Relates a concept to a work of which it is the subject."@en ;
	RegAp:name "isSubjectConceptOf"@en ;
	RegAp:status <http://metadataregistry.org/uri/RegStatus/1001> .

frbrer:P2025 a owl:NamedIndividual ;
	skos:definition "Relates a work to an object that is the subject of the work."@en ;
	RegAp:name "hasAsSubjectObject"@en ;
	RegAp:status <http://metadataregistry.org/uri/RegStatus/1001> .

frbrer:P2026 a owl:NamedIndividual ;
	skos:definition "Relates an object to a work of which it is the subject."@en ;
	RegAp:name "isSubjectObjectOf"@en ;
	RegAp:status <http://metadataregistry.org/uri/RegStatus/1001> .

frbrer:P2027 a owl:NamedIndividual ;
	skos:definition "Relates a work to an event that is the subject of the work."@en ;
	RegAp:name "hasAsSubjectEvent"@en ;
	RegAp:status <http://metadataregistry.org/uri/RegStatus/1001> .

frbrer:P2028 a owl:NamedIndividual ;
	skos:definition "Relates an event to a work of which it is the subject."@en ;
	RegAp:name "isSubjectEventOf"@en ;
	RegAp:status <http://metadataregistry.org/uri/RegStatus/1001> .

frbrer:P2029 a owl:NamedIndividual ;
	skos:definition "Relates a work to a place that is the subject of the work."@en ;
	RegAp:name "hasAsSubjectPlace"@en ;
	RegAp:status <http://metadataregistry.org/uri/RegStatus/1001> .

frbrer:P2030 a owl:NamedIndividual ;
	skos:definition "Relates a place to a work of which it is the subject."@en ;
	RegAp:name "isSubjectPlaceOf"@en ;
	RegAp:status <http://metadataregistry.org/uri/RegStatus/1001> .

frbrer:P2031 a owl:NamedIndividual ;
	skos:definition "Relates a work to a corporate body that is the subject of the work."@en ;
	RegAp:name "hasAsSubjectCorporateBody"@en ;
	RegAp:status <http://metadataregistry.org/uri/RegStatus/1001> .

frbrer:P2032 a owl:NamedIndividual ;
	skos:definition "Relates a corporate body to a work of which it is the subject."@en ;
	RegAp:name "isSubjectCorporateBodyOf"@en ;
	RegAp:status <http://metadataregistry.org/uri/RegStatus/1001> .

frbrer:P2033 a owl:NamedIndividual ;
	skos:definition "Relates a work to a person that is the subject of the work."@en ;
	RegAp:name "hasAsSubjectPerson"@en ;
	RegAp:status <http://metadataregistry.org/uri/RegStatus/1001> .

frbrer:P2034 a owl:NamedIndividual ;
	skos:definition "Relates a person to a work of which it is the subject."@en ;
	RegAp:name "isSubjectPersonOf"@en ;
	RegAp:status <http://metadataregistry.org/uri/RegStatus/1001> .

frbrer:P2035 a owl:NamedIndividual ;
	skos:definition "Relates a work to a prior work that is the subject of the work."@en ;
	RegAp:name "hasAsSubjectWork"@en ;
	RegAp:status <http://metadataregistry.org/uri/RegStatus/1001> .

frbrer:P2036 a owl:NamedIndividual ;
	skos:definition "Relates a prior work to another work of which it is the subject."@en ;
	RegAp:name "isSubjectWorkOf"@en ;
	RegAp:status <http://metadataregistry.org/uri/RegStatus/1001> .

frbrer:P2037 a owl:NamedIndividual ;
	skos:definition "Relates a work to an expression that is the subject of the work."@en ;
	RegAp:name "hasAsSubjectExpression"@en ;
	RegAp:status <http://metadataregistry.org/uri/RegStatus/1001> .

frbrer:P2038 a owl:NamedIndividual ;
	skos:definition "Relates an expression to a work of which it is the subject."@en ;
	RegAp:name "isSubjectExpressionOf"@en ;
	RegAp:status <http://metadataregistry.org/uri/RegStatus/1001> .

frbrer:P2039 a owl:NamedIndividual ;
	skos:definition "Relates a work to a manifestation that is the subject of the work."@en ;
	RegAp:name "hasAsSubjectManifestation"@en ;
	RegAp:status <http://metadataregistry.org/uri/RegStatus/1001> .

frbrer:P2040 a owl:NamedIndividual ;
	skos:definition "Relates a manifestation to a work of which it is the subject."@en ;
	RegAp:name "isSubjectManifestationOf"@en ;
	RegAp:status <http://metadataregistry.org/uri/RegStatus/1001> .

frbrer:P2041 a owl:NamedIndividual ;
	skos:definition "Relates a work to an item that is the subject of the work."@en ;
	RegAp:name "hasAsSubjectItem"@en ;
	RegAp:status <http://metadataregistry.org/uri/RegStatus/1001> .

frbrer:P2042 a owl:NamedIndividual ;
	skos:definition "Relates an item to a work of which it is the subject."@en ;
	RegAp:name "isSubjectItemOf"@en ;
	RegAp:status <http://metadataregistry.org/uri/RegStatus/1001> .

frbrer:P2043 a owl:NamedIndividual ;
	skos:definition "Relates a prior work to another work, the content of which represents a linear progression from that of the prior work. The content may be closely or loosely connected, so the successor work may be referential or autonomous with respect to the prior work."@en ;
	RegAp:name "hasASuccessorWorkFromWork"@en ;
	RegAp:status <http://metadataregistry.org/uri/RegStatus/1001> .

frbrer:P2044 a owl:NamedIndividual ;
	skos:definition "Relates a work to a prior work, the content of which represents the basis of a linear progression to that of the successor work. The content may be closely or loosely connected, so the successor work may be referential or autonomous with respect to the prior work."@en ;
	RegAp:name "isASuccessorWorkToWork"@en ;
	RegAp:status <http://metadataregistry.org/uri/RegStatus/1001> .

frbrer:P2045 a owl:NamedIndividual ;
	skos:definition "Relates a prior work to another work that is intended to be used in conjunction with the prior work. The content may be closely or loosely associatedd, so the supplementary work may be referential or autonomous with respect to the prior work."@en ;
	RegAp:name "hasASupplementWorkFromWork"@en ;
	RegAp:status <http://metadataregistry.org/uri/RegStatus/1001> .

frbrer:P2046 a owl:NamedIndividual ;
	skos:definition "Relates a work to a prior work with which it is intended to be used in conjunction. The content may be closely or loosely associated, so the supplementary work may be referential or autonomous with respect to the prior work."@en ;
	RegAp:name "supplementsWorkFromWork"@en ;
	RegAp:status <http://metadataregistry.org/uri/RegStatus/1001> .

frbrer:P2047 a owl:NamedIndividual ;
	skos:definition "Relates a prior work to another work that is intended to be combined with or inserted into the prior work, but was not part of the original conception of the prior work. The content may be closely or loosely connected, so the complementary work may be referential or autonomous with respect to the prior work."@en ;
	RegAp:name "hasAComplementWorkFromWork"@en ;
	RegAp:status <http://metadataregistry.org/uri/RegStatus/1001> .

frbrer:P2048 a owl:NamedIndividual ;
	skos:definition "Relates a work to a prior work that it is intended to be combined with or inserted into, but was not part of the original conception of the prior work. The content may be closely or loosely connected, so the complementary work may be referential or autonomous with respect to the prior work."@en ;
	RegAp:name "complementsWorkFromWork"@en ;
	RegAp:status <http://metadataregistry.org/uri/RegStatus/1001> .

frbrer:P2049 a owl:NamedIndividual ;
	skos:definition "Relates a prior work to another work that represents a brief recapitulation of the content of the prior work. The modification of the content of the prior work must be sufficient in degree to warrant the summary work being considered as a new work autonomous with respect to the prior work."@en ;
	RegAp:name "hasASummaryWorkFromWork"@en ;
	RegAp:status <http://metadataregistry.org/uri/RegStatus/1001> .

frbrer:P2050 a owl:NamedIndividual ;
	skos:definition "Relates a work to a prior work of which it represents a brief recapitulation. The modification of the content of the prior work must be sufficient in degree to warrant the summary work being considered as a new work autonomous with respect to the prior work."@en ;
	RegAp:name "isASummaryWorkOfWork"@en ;
	RegAp:status <http://metadataregistry.org/uri/RegStatus/1001> .

frbrer:P2051 a owl:NamedIndividual ;
	skos:definition "Relates a prior work to another work that represents a modification of the content of the prior work for a purpose, use, or medium other than that for which it was originally intended. The modification of the content of the prior work must be sufficient in degree to warrant the adaptation work being considered as a new work autonomous with respect to the prior work."@en ;
	RegAp:name "hasAnAdaptationWorkFromWork"@en ;
	RegAp:status <http://metadataregistry.org/uri/RegStatus/1001> .

frbrer:P2052 a owl:NamedIndividual ;
	skos:definition "Relates a work to a prior work of which it represents a modification of the content for a purpose, use, or medium other than that for which it was originally intended.The modification of the content of the prior work must be sufficient in degree to warrant the adaptation work being considered as a new work autonomous with respect to the prior work."@en ;
	RegAp:name "isAnAdaptationWorkOfWork"@en ;
	RegAp:status <http://metadataregistry.org/uri/RegStatus/1001> .

frbrer:P2053 a owl:NamedIndividual ;
	skos:definition "Relates a prior work to another work that represents a transformation of the content of the prior work in a different genre. The modification of the content of the prior work must be sufficient in degree to warrant the transformation work being considered as a new work autonomous with respect to the prior work."@en ;
	RegAp:name "hasATransformationWorkFromWork"@en ;
	RegAp:status <http://metadataregistry.org/uri/RegStatus/1001> .

frbrer:P2054 a owl:NamedIndividual ;
	skos:definition "Relates a work to a prior work of which it represents a transformation of the content in a different genre. The modification of the content of the prior work must be sufficient in degree to warrant the adaptation work being considered as a new work autonomous with respect to the prior work."@en ;
	RegAp:name "isATransformationWorkOfWork"@en ;
	RegAp:status <http://metadataregistry.org/uri/RegStatus/1001> .

frbrer:P2055 a owl:NamedIndividual ;
	skos:definition "Relates a prior work to another work that that copies the style of the content of the prior work. The modification of the content of the prior work must be sufficient in degree to warrant the imitation work being considered as a new work autonomous with respect to the prior work."@en ;
	RegAp:name "hasAnImitationWorkFromWork"@en ;
	RegAp:status <http://metadataregistry.org/uri/RegStatus/1001> .

frbrer:P2056 a owl:NamedIndividual ;
	skos:definition "Relates a work to a prior work of which it copies the style of the content. The modification of the content of the prior work must be sufficient in degree to warrant the imitation work being considered as a new work autonomous with respect to the prior work."@en ;
	RegAp:name "isAnImitationWorkOfWork"@en ;
	RegAp:status <http://metadataregistry.org/uri/RegStatus/1001> .

frbrer:P2057 a owl:NamedIndividual ;
	skos:definition "Relates a work to another work that is a component of the work."@en ;
	skos:scopeNote "The component work may be intended to be used in the context of the prior work or may not depend to any significant extent on the context provided by the prior work."@en ;
	RegAp:name "hasPartWork"@en ;
	RegAp:status <http://metadataregistry.org/uri/RegStatus/1001> .

frbrer:P2058 a owl:NamedIndividual ;
	skos:definition "Relates a work to another work of which it is a component."@en ;
	skos:scopeNote "The component work may be intended to be used in the context of the prior work or may not depend to any significant extent on the context provided by the prior work."@en ;
	RegAp:name "isPartWorkOf"@en ;
	RegAp:status <http://metadataregistry.org/uri/RegStatus/1001> .

frbrer:P2059 a owl:NamedIndividual ;
	skos:definition "Relates an expression to another expression of the same work that represents an abridgement, in which some content of the prior expression is removed, but the result does not alter the content to the extent that it becomes a new work."@en ;
	RegAp:name "hasAnAbridgementExpression"@en ;
	RegAp:status <http://metadataregistry.org/uri/RegStatus/1001> .

frbrer:P2060 a owl:NamedIndividual ;
	skos:definition "Relates an expression to a prior expression of the same work of which it represents an abridgement, in which some content of the prior expression is removed, but the result does not alter the content to the extent that it becomes a new work."@en ;
	RegAp:name "isAnAbridgementExpressionOf"@en ;
	RegAp:status <http://metadataregistry.org/uri/RegStatus/1001> .

frbrer:P2061 a owl:NamedIndividual ;
	skos:definition "Relates an expression to another expression of the same work that represents a revision, in which the intent is to alter or update the content of the prior expression, but without changing the content so much that it becomes a new work."@en ;
	RegAp:name "hasARevisionExpression"@en ;
	RegAp:status <http://metadataregistry.org/uri/RegStatus/1001> .

frbrer:P2062 a owl:NamedIndividual ;
	skos:definition "Relates an expression to a prior expression of the same work of which it represents a revision, in which the intent is to alter or update the content of the prior expression, but without changing the content so much that it becomes a new work."@en ;
	RegAp:name "isARevisionExpressionOf"@en ;
	RegAp:status <http://metadataregistry.org/uri/RegStatus/1001> .

frbrer:P2063 a owl:NamedIndividual ;
	skos:scopeNote "Free translations are treated in the model as new works."@en ;
	skos:definition "Relates an expression to another expression of the same work that represents a literal translation, in which the intent is to render the intellectual content of the previous expression as accurately as possible."@en ;
	RegAp:name "hasATranslationExpression"@en ;
	RegAp:status <http://metadataregistry.org/uri/RegStatus/1001> .

frbrer:P2064 a owl:NamedIndividual ;
	skos:scopeNote "Free translations are treated in the model as new works."@en ;
	skos:definition "Relates an expression to a prior expression of the same work of which it represents a literal translation, in which the intent is to render the intellectual content of the previous expression as accurately as possible."@en ;
	RegAp:name "isATranslationExpressionOf"@en ;
	RegAp:status <http://metadataregistry.org/uri/RegStatus/1001> .

frbrer:P2065 a owl:NamedIndividual ;
	skos:definition "Relates an expression to another expression that represents an arrangement of the same musical composition work."@en ;
	RegAp:name "hasAnArrangementExpression"@en ;
	RegAp:status <http://metadataregistry.org/uri/RegStatus/1001> .

frbrer:P2066 a owl:NamedIndividual ;
	skos:definition "Relates an expression to a prior expression of which it represents an arrangement of the same musical composition work."@en ;
	RegAp:name "isAnArrangementExpressionOf"@en ;
	RegAp:status <http://metadataregistry.org/uri/RegStatus/1001> .

frbrer:P2067 a owl:NamedIndividual ;
	skos:definition "Relates an expression of a prior work to an expression of another work, the content of which represents a linear progression from that of the prior work. The content may be closely or loosely connected, so the successor work may be referential or autonomous with respect to the prior work."@en ;
	RegAp:name "hasASuccessorExpressionFromExpression"@en ;
	RegAp:status <http://metadataregistry.org/uri/RegStatus/1001> .

frbrer:P2068 a owl:NamedIndividual ;
	skos:definition "Relates an expression of a work to an expression of a prior work, the content of which represents the basis of a linear progression to that of the successor work. The content may be closely or loosely connected, so the successor work may be referential or autonomous with respect to the prior work."@en ;
	RegAp:name "isASuccessorExpressionToExpression"@en ;
	RegAp:status <http://metadataregistry.org/uri/RegStatus/1001> .

frbrer:P2069 a owl:NamedIndividual ;
	skos:definition "Relates an expression of a prior work to an expression of another work that is intended to be combined with or inserted into the prior work, but was not part of the original conception of the prior work. The content may be closely or loosely connected, so the complementary work may be referential or autonomous with respect to the prior work."@en ;
	RegAp:name "hasAComplementExpressionFromExpression"@en ;
	RegAp:status <http://metadataregistry.org/uri/RegStatus/1001> .

frbrer:P2070 a owl:NamedIndividual ;
	skos:definition "Relates an expression of a work to an expression of a prior work that it is intended to be combined with or inserted into, but was not part of the original conception of the prior work. The content may be closely or loosely connected, so the complementary work may be referential or autonomous with respect to the prior work."@en ;
	RegAp:name "complementsExpressionFromExpression"@en ;
	RegAp:status <http://metadataregistry.org/uri/RegStatus/1001> .

frbrer:P2071 a owl:NamedIndividual ;
	skos:definition "Relates an expression of a prior work to an expression of another work that represents a brief recapitulation of the content of the prior work. The modification of the content of the prior work must be sufficient in degree to warrant the summary work being considered as a new work autonomous with respect to the prior work."@en ;
	RegAp:name "hasASummaryExpressionFromExpression"@en ;
	RegAp:status <http://metadataregistry.org/uri/RegStatus/1001> .

frbrer:P2072 a owl:NamedIndividual ;
	skos:definition "Relates an expression of a work to an expression of a prior work of which it represents a brief recapitulation. The modification of the content of the prior work must be sufficient in degree to warrant the summary work being considered as a new work autonomous with respect to the prior work."@en ;
	RegAp:name "isASummaryExpressionOfExpression"@en ;
	RegAp:status <http://metadataregistry.org/uri/RegStatus/1001> .

frbrer:P2073 a owl:NamedIndividual ;
	skos:definition "Relates an expression of a prior work to an expression of another work that represents a modification of the content of the prior work for a purpose, use, or medium other than that for which it was originally intended. The modification of the content of the prior work must be sufficient in degree to warrant the adaptation work being considered as a new work autonomous with respect to the prior work."@en ;
	RegAp:name "hasAnAdaptationExpressionFromExpression"@en ;
	RegAp:status <http://metadataregistry.org/uri/RegStatus/1001> .

frbrer:P2074 a owl:NamedIndividual ;
	skos:definition "Relates an expression of a work to an expression of a prior work of which it represents a modification of the content for a purpose, use, or medium other than that for which it was originally intended. The modification of the content of the prior work must be sufficient in degree to warrant the adaptation work being considered as a new work autonomous with respect to the prior work."@en ;
	RegAp:name "isAnAdaptationExpressionOfExpression"@en ;
	RegAp:status <http://metadataregistry.org/uri/RegStatus/1001> .

frbrer:P2075 a owl:NamedIndividual ;
	skos:definition "Relates an expression of a prior work to an expression of another work that represents a transformation of the content of the prior work in a different genre. The modification of the content of the prior work must be sufficient in degree to warrant the transformation work being considered as a new work autonomous with respect to the prior work."@en ;
	RegAp:name "hasATransformationExpressionFromExpression"@en ;
	RegAp:status <http://metadataregistry.org/uri/RegStatus/1001> .

frbrer:P2076 a owl:NamedIndividual ;
	skos:definition "Relates an expression of a work to an expression of a prior work of which it represents a transformation of the content in a different genre. The modification of the content of the prior work must be sufficient in degree to warrant the adaptation work being considered as a new work autonomous with respect to the prior work."@en ;
	RegAp:name "isATransformationExpressionOfExpression"@en ;
	RegAp:status <http://metadataregistry.org/uri/RegStatus/1001> .

frbrer:P2077 a owl:NamedIndividual ;
	skos:definition "Relates an expression of a prior work to an expression of another work that copies the style of the content of the prior work. The modification of the content of the prior work must be sufficient in degree to warrant the imitation work being considered as a new work autonomous with respect to the prior work."@en ;
	RegAp:name "hasAnImitationExpressionFromExpression"@en ;
	RegAp:status <http://metadataregistry.org/uri/RegStatus/1001> .

frbrer:P2078 a owl:NamedIndividual ;
	skos:definition "Relates an expression of a work to an expression of a prior work of which it copies the style of the content. The modification of the content of the prior work must be sufficient in degree to warrant the imitation work being considered as a new work autonomous with respect to the prior work."@en ;
	RegAp:name "isAnImitationExpressionOfExpression"@en ;
	RegAp:status <http://metadataregistry.org/uri/RegStatus/1001> .

frbrer:P2079 a owl:NamedIndividual ;
	skos:definition "Relates an expression to another expression that is a component of the expression."@en ;
	skos:scopeNote "The component expression may be intended to be used in the context of the prior expression or may not depend to any significant extent on the context provided by the prior expression."@en ;
	RegAp:name "hasPartExpression"@en ;
	RegAp:status <http://metadataregistry.org/uri/RegStatus/1001> .

frbrer:P2080 a owl:NamedIndividual ;
	skos:definition "Relates an expression to another expression of which it is a component."@en ;
	skos:scopeNote "The component expression may be intended to be used in the context of the prior expression or may not depend to any significant extent on the context provided by the prior expression."@en ;
	RegAp:name "isPartExpressionOf"@en ;
	RegAp:status <http://metadataregistry.org/uri/RegStatus/1001> .

frbrer:P2081 a owl:NamedIndividual ;
	skos:definition "Relates a manifestation to another manifestation, usually of the same expression, that represents the same intellectual or artistic content as the prior manifestation. The reproduction manifestation may or may not replicate the look and feel or other physical characteristics of the prior manifestation."@en ;
	RegAp:name "hasAReproductionManifestationFromManifestation"@en ;
	RegAp:status <http://metadataregistry.org/uri/RegStatus/1001> .

frbrer:P2082 a owl:NamedIndividual ;
	skos:definition "Relates a manifestation to a prior manifestation, usually of the same expression, of which it represents the same intellectual or artistic content as the prior manifestation. The reproduction manifestation may or may not replicate the look and feel or other physical characteristics of the prior manifestation."@en ;
	RegAp:name "isAReproductionManifestationOfManifestation"@en ;
	RegAp:status <http://metadataregistry.org/uri/RegStatus/1001> .

frbrer:P2083 a owl:NamedIndividual ;
	skos:definition "Relates a manifestation to another manifestation, usually of the same expression, that effectively serves as an alternate manifestation."@en ;
	skos:scopeNote "The alternate relationship obtains, for example, when a publication, sound recording, video, etc. is issued in more than one format or when it is released simultaneously by different publishers in different countries."@en ;
	RegAp:name "hasAnAlternate"@en ;
	skos:altLabel "is an alternate to"@en ;
	RegAp:status <http://metadataregistry.org/uri/RegStatus/1001> .

frbrer:P2085 a owl:NamedIndividual ;
	skos:definition "Relates a manifestation to another manifestation that is a component of the manifestation."@en ;
	skos:scopeNote "The component manifestation may be a discrete physical unit of the prior manifestation or may be an integral part that is physically inseparable from the whole of the prior expression."@en ;
	RegAp:name "hasPartManifestation"@en ;
	RegAp:status <http://metadataregistry.org/uri/RegStatus/1001> .

frbrer:P2086 a owl:NamedIndividual ;
	skos:definition "Relates a manifestation to another manifestation of which it is a component."@en ;
	skos:scopeNote "The component manifestation may be a discrete physical unit of the prior manifestation or may be an integral part that is physically inseparable from the whole of the prior manifestation."@en ;
	RegAp:name "isPartManifestationOf"@en ;
	RegAp:status <http://metadataregistry.org/uri/RegStatus/1001> .

frbrer:P2087 a owl:NamedIndividual ;
	skos:scopeNote "Most commonly, an item of one manifestation is bound with an item of a different manifestation to make a new item."@en ;
	skos:definition "Relates an item to another item that is the result of a change to the prior item. The reconfiguration item may be the result of changes to more than one prior item."@en ;
	RegAp:name "hasAReconfiguration"@en ;
	RegAp:status <http://metadataregistry.org/uri/RegStatus/1001> .

frbrer:P2088 a owl:NamedIndividual ;
	skos:scopeNote "Most commonly, an item of one manifestation is bound with an item of a different manifestation to make a new item."@en ;
	skos:definition "Relates an item to another item to which it is the result of a change. The reconfiguration item may be the result of changes to more than one prior item."@en ;
	RegAp:name "isAReconfigurationOf"@en ;
	RegAp:status <http://metadataregistry.org/uri/RegStatus/1001> .

frbrer:P2089 a owl:NamedIndividual ;
	skos:definition "Relates an item to another item that has been derived in some way from the prior item. There can be varying levels of fidelity of the reproduction item to the prior item. The reproduction item must replicate the type of carrier and other physical characteristics of the prior item."@en ;
	RegAp:name "hasAReproductionItemFromItem"@en ;
	RegAp:status <http://metadataregistry.org/uri/RegStatus/1001> .

frbrer:P2090 a owl:NamedIndividual ;
	skos:definition "Relates an item to a prior item from which it has been derived in some way. There can be varying levels of fidelity of the reproduction item to the prior item. The reproduction item must replicate the type of carrier and other physical characteristics of the prior item."@en ;
	RegAp:name "isAReproductionItemOfItem"@en ;
	RegAp:status <http://metadataregistry.org/uri/RegStatus/1001> .

frbrer:P2091 a owl:NamedIndividual ;
	skos:definition "Relates an item to another item that is a component of the item."@en ;
	skos:scopeNote "The component item may be a discrete physical unit of the prior item or may be an integral part that is physically inseparable from the whole of the prior item."@en ;
	RegAp:name "hasPartItem"@en ;
	RegAp:status <http://metadataregistry.org/uri/RegStatus/1001> .

frbrer:P2092 a owl:NamedIndividual ;
	skos:definition "Relates an item to another item of which it is a component."@en ;
	RegAp:name "isPartItemOf"@en ;
	RegAp:status <http://metadataregistry.org/uri/RegStatus/1001> .

frbrer:P2093 a owl:NamedIndividual ;
	skos:definition "Relates an item to a manifestation that has been derived in some way from the prior item. There can be varying levels of fidelity of the reproduction manifestation to the prior item."@en ;
	skos:scopeNote "The reproduction relationship will be stated at this level when it is useful to indicate the specific item used, as opposed to stating the relationship at the more general level of manifestation-to-manifestation."@en ;
	RegAp:name "hasAReproductionManifestationFromItem"@en ;
	RegAp:status <http://metadataregistry.org/uri/RegStatus/1001> .

frbrer:P2094 a owl:NamedIndividual ;
	skos:definition "Relates a manifestation to an item from which it has been derived in some way. There can be varying levels of fidelity of the reproduction manifestation to the prior item."@en ;
	skos:scopeNote "The reproduction relationship will be stated at this level when it is useful to indicate the specific item used, as opposed to stating the relationship at the more general level of manifestation-to-manifestation."@en ;
	RegAp:name "isAReproductionManifestationOfItem"@en ;
	RegAp:status <http://metadataregistry.org/uri/RegStatus/1001> .

frbrer:P2095 a owl:NamedIndividual ;
	skos:definition "Relates an expression of a prior work to another work, the content of which represents a linear progression from that of the prior work. The content may be closely or loosely connected, so the successor work may be referential or autonomous with respect to the prior work."@en ;
	RegAp:name "hasASuccessorWorkFromExpression"@en ;
	RegAp:status <http://metadataregistry.org/uri/RegStatus/1001> .

frbrer:P2096 a owl:NamedIndividual ;
	skos:definition "Relates a work to an expression of a prior work, the content of which represents the basis of a linear progression to that of the successor work. The content may be closely or loosely connected, so the successor work may be referential or autonomous with respect to the prior work."@en ;
	RegAp:name "isASuccessorWorkToExpression"@en ;
	RegAp:status <http://metadataregistry.org/uri/RegStatus/1001> .

frbrer:P2097 a owl:NamedIndividual ;
	skos:definition "Relates an expression of a prior work to another work that is intended to be used in conjunction with the prior work. The content may be closely or loosely associated, so the supplementary work may be referential or autonomous with respect to the prior work."@en ;
	RegAp:name "hasASupplementWorkFromExpression"@en ;
	RegAp:status <http://metadataregistry.org/uri/RegStatus/1001> .

frbrer:P2098 a owl:NamedIndividual ;
	skos:definition "Relates a work to an expression of a prior work with which it is intended to be used in conjunction. The content may be closely or loosely associated, so the supplementary work may be referential or autonomous with respect to the prior work."@en ;
	RegAp:name "supplementsExpressionFromWork"@en ;
	RegAp:status <http://metadataregistry.org/uri/RegStatus/1001> .

frbrer:P2099 a owl:NamedIndividual ;
	skos:definition "Relates an expression of a prior work to another work that is intended to be combined with or inserted into the prior work, but was not part of the original conception of the prior work. The content may be closely or loosely connected, so the complementary work may be referential or autonomous with respect to the prior work."@en ;
	RegAp:name "hasAComplementWorkFromExpression"@en ;
	RegAp:status <http://metadataregistry.org/uri/RegStatus/1001> .

frbrer:P2100 a owl:NamedIndividual ;
	skos:definition "Relates a work to an expression of a prior work that it is intended to be combined with or inserted into, but was not part of the original conception of the prior work. The content may be closely or loosely connected, so the complementary work may be referential or autonomous with respect to the prior work."@en ;
	RegAp:name "complementsWorkFromExpression"@en ;
	RegAp:status <http://metadataregistry.org/uri/RegStatus/1001> .

frbrer:P2101 a owl:NamedIndividual ;
	skos:definition "Relates an expression of a prior work to another work that represents a brief recapitulation of the content of the prior work. The modification of the content of the prior work must be sufficient in degree to warrant the summary work being considered as a new work autonomous with respect to the prior work."@en ;
	RegAp:name "hasASummaryWorkFromExpression"@en ;
	RegAp:status <http://metadataregistry.org/uri/RegStatus/1001> .

frbrer:P2102 a owl:NamedIndividual ;
	skos:definition "Relates a work to an expression of a prior work of which it represents a brief recapitulation. The modification of the content of the prior work must be sufficient in degree to warrant the summary work being considered as a new work autonomous with respect to the prior work."@en ;
	RegAp:name "isASummaryWorkOfExpression"@en ;
	RegAp:status <http://metadataregistry.org/uri/RegStatus/1001> .

frbrer:P2103 a owl:NamedIndividual ;
	skos:definition "Relates an expression of a prior work to another work that represents a modification of the content of the prior work for a purpose, use, or medium other than that for which it was originally intended. The modification of the content of the prior work must be sufficient in degree to warrant the adaption work being considered as a new work autonomous with respect to the prior work."@en ;
	RegAp:name "hasAnAdaptationWorkFromExpression"@en ;
	RegAp:status <http://metadataregistry.org/uri/RegStatus/1001> .

frbrer:P2104 a owl:NamedIndividual ;
	skos:definition "Relates a work to an expression of a prior work of which it represents a modification of the content for a purpose, use, or medium other than that for which it was originally intended. The modification of the content of the prior work must be sufficient in degree to warrant the adaptation work being considered as a new work autonomous with respect to the prior work."@en ;
	RegAp:name "isAnAdaptationWorkOfExpression"@en ;
	RegAp:status <http://metadataregistry.org/uri/RegStatus/1001> .

frbrer:P2105 a owl:NamedIndividual ;
	skos:definition "Relates an expression of a prior work to another work that represents a transformation of the content of the prior work in a different genre. The modification of the content of the prior work must be sufficient in degree to warrant the transformation work being considered as a new work autonomous with respect to the prior work."@en ;
	RegAp:name "hasATransformationWorkFromExpression"@en ;
	RegAp:status <http://metadataregistry.org/uri/RegStatus/1001> .

frbrer:P2106 a owl:NamedIndividual ;
	skos:definition "Relates a work to an expression of a prior work of which it represents a transformation of the content in a different genre. The modification of the content of the prior work must be sufficient in degree to warrant the adaptation work being considered as a new work autonomous with respect to the prior work."@en ;
	RegAp:name "isATransformationWorkOfExpression"@en ;
	RegAp:status <http://metadataregistry.org/uri/RegStatus/1001> .

frbrer:P2107 a owl:NamedIndividual ;
	skos:definition "Relates an expression of a prior work to another work that copies the style of the content of the prior work. The modification of the content of the prior work must be sufficient in degree to warrant the imitation work being considered as a new work autonomous with respect to the prior work."@en ;
	RegAp:name "hasAnImitationWorkFromExpression"@en ;
	RegAp:status <http://metadataregistry.org/uri/RegStatus/1001> .

frbrer:P2108 a owl:NamedIndividual ;
	skos:definition "Relates a work to an expression of a prior work of which it copies the style of the content. The modification of the content of the prior work must be sufficient in degree to warrant the imitation work being considered as a new work autonomous with respect to the prior work."@en ;
	RegAp:name "isAnImitationWorkOfExpression"@en ;
	RegAp:status <http://metadataregistry.org/uri/RegStatus/1001> .

frbrer:P2109 a owl:NamedIndividual ;
	skos:definition "Relates an expression of a prior work to an expression of another work that is intended to be used in conjunction with the prior work. The content may be closely or loosely associated, so the supplementary work may be referential or autonomous with respect to the prior work."@en ;
	RegAp:name "hasASupplementExpressionFromExpression"@en ;
	RegAp:status <http://metadataregistry.org/uri/RegStatus/1001> .

frbrer:P2110 a owl:NamedIndividual ;
	skos:definition "Relates an expression of a work to an expression of a prior work with which it is intended to be used in conjunction. The content may be closely or loosely associated, so the supplementary work may be referential or autonomous with respect to the prior work."@en ;
	RegAp:name "supplementsExpressionFromExpression"@en ;
	RegAp:status <http://metadataregistry.org/uri/RegStatus/1001> .

frbrer:P3001 a owl:NamedIndividual ;
	skos:definition "Relates a work to the word, phrase, or group of characters naming the work."@en ;
	skos:scopeNote "There may be one or more titles associated with a work. If the work has appeared under varying titles (differing in form, language, etc.), a bibliographic agency normally selects one of those titles as the basis of a \"uniform title\" for purposes of consistency in naming and referencing the work. Other titles under which the work has appeared may be treated as variant titles for the work, or in some cases as a parallel uniform title. The title of a work that forms part of a larger work may consist solely of a number or other generic designation that is dependent on the title of the larger work."@en ;
	RegAp:name "hasTitleOfTheWork"@en ;
	RegAp:status <http://metadataregistry.org/uri/RegStatus/1001> .

frbrer:P3002 a owl:NamedIndividual ;
	skos:scopeNote "E.g., novel, play, poem, essay, biography, symphony, concerto, sonata, map, drawing, painting, photograph, etc."@en ;
	skos:definition "Relates a work to the class to which the work belongs."@en ;
	RegAp:name "hasFormOfWork"@en ;
	RegAp:status <http://metadataregistry.org/uri/RegStatus/1001> .

frbrer:P3003 a owl:NamedIndividual ;
	skos:definition "Relates a work to the date the work was originally created."@en ;
	skos:scopeNote "The date (normally the year) may be a single date or a range of dates. In the absence of an ascertainable date of creation, the date of the work may be associated with the date of its first publication or release."@en ;
	RegAp:name "hasDateOfTheWork"@en ;
	RegAp:status <http://metadataregistry.org/uri/RegStatus/1001> .

frbrer:P3004 a owl:NamedIndividual ;
	skos:definition "Relates a work to any characteristic that serves to differentiate the work from another work with the same title."@en ;
	RegAp:name "hasOtherDistinguishingCharacteristicOfWork"@en ;
	RegAp:status <http://metadataregistry.org/uri/RegStatus/1001> .

frbrer:P3005 a owl:NamedIndividual ;
	skos:definition "Relates a work to a reflection of whether the work has been conceived as having a finite end or whether it is intended to continue indefinitely."@en ;
	RegAp:name "hasIntendedTermination"@en ;
	RegAp:status <http://metadataregistry.org/uri/RegStatus/1001> .

frbrer:P3006 a owl:NamedIndividual ;
	skos:definition "Relates a work to the class of user for which the work is intended, as defined by age group, educational level, or other categorization."@en ;
	RegAp:name "hasIntendedAudience"@en ;
	RegAp:status <http://metadataregistry.org/uri/RegStatus/1001> .

frbrer:P3007 a owl:NamedIndividual ;
	skos:definition "Relates a work to the historical, social, intellectual, artistic, or other context within which the work was originally conceived."@en ;
	RegAp:name "hasContextForTheWork"@en ;
	RegAp:status <http://metadataregistry.org/uri/RegStatus/1001> .

frbrer:P3008 a owl:NamedIndividual ;
	skos:definition "Relates an expression to a word, phrase, or group of characters naming the expression."@en ;
	skos:scopeNote "There may be one or more titles associated with an expression. The title of an expression that forms part of a larger expression may consist solely of a number or other generic designation that is dependent on the title of the larger expression."@en ;
	RegAp:name "hasTitleOfTheExpression"@en ;
	RegAp:status <http://metadataregistry.org/uri/RegStatus/1001> .

frbrer:P3009 a owl:NamedIndividual ;
	skos:scopeNote "E.g., through alpha-numeric notation, musical notation, spoken word, musical sound, cartographic image, photographic image, sculpture, dance, mime, etc."@en ;
	skos:definition "Relates an expression to the means by which the work is realized."@en ;
	RegAp:name "hasFormOfExpression"@en ;
	RegAp:status <http://metadataregistry.org/uri/RegStatus/1001> .

frbrer:P3010 a owl:NamedIndividual ;
	skos:scopeNote "E.g., the date the particular text of a work was written or revised, the date a song was performed, etc. The date may be a single date or a range of dates. In the absence of an ascertainable date of expression, the date of the expression may be associated with the date of its publication or release."@en ;
	skos:definition "Relates an expression to the date the expression was created."@en ;
	RegAp:name "hasDateOfExpression"@en ;
	RegAp:status <http://metadataregistry.org/uri/RegStatus/1001> .

frbrer:P3011 a owl:NamedIndividual ;
	skos:definition "Relates an expression to the language in which the work is expressed."@en ;
	skos:scopeNote "The language of the expression may comprise a number of languages, each pertaining to an individual component of the expression."@en ;
	RegAp:name "hasLanguageOfExpression"@en ;
	RegAp:status <http://metadataregistry.org/uri/RegStatus/1001> .

frbrer:P3012 a owl:NamedIndividual ;
	skos:scopeNote "E.g., the names used to differentiate the various versions of the English text of the Bible, or an \"edition\" or version designation relating to the intellectual content of the expression such as \"2nd revision\"."@en ;
	skos:definition "Relates an expression to any characteristic of the expression that serves to differentiate the expression from another expression of the same work."@en ;
	RegAp:name "hasOtherDistinguishingCharacteristicOfExpression"@en ;
	RegAp:status <http://metadataregistry.org/uri/RegStatus/1001> .

frbrer:P3013 a owl:NamedIndividual ;
	skos:scopeNote "E.g., an expression that is completed one part at a time, segment by segment, issue by issue, etc."@en ;
	skos:definition "Relates an expression to a reflection of the expectation that the expression will have additional intellectual or artistic content added to it."@en ;
	RegAp:name "hasExtensibilityOfExpression"@en ;
	RegAp:status <http://metadataregistry.org/uri/RegStatus/1001> .

frbrer:P3014 a owl:NamedIndividual ;
	skos:scopeNote "E.g., a draft or interim report, a directory that is expected to be updated periodically."@en ;
	skos:definition "Relates an expression to a reflection of the expectation that the intellectual or artistic content of the expression will be revised."@en ;
	RegAp:name "hasRevisabilityOfExpression"@en ;
	RegAp:status <http://metadataregistry.org/uri/RegStatus/1001> .

frbrer:P3015 a owl:NamedIndividual ;
	skos:scopeNote "E.g., number of words in a text, statements in a computer program, images in a comic strip, etc. For works expressed as sound and, or, motion the extent may be a measure of duration; e.g., playing time."@en ;
	skos:definition "Relates an expression to a quantification of the intellectual content of the expression."@en ;
	RegAp:name "hasExtentOfTheExpression"@en ;
	RegAp:status <http://metadataregistry.org/uri/RegStatus/1001> .

frbrer:P3016 a owl:NamedIndividual ;
	skos:definition "Relates an expression to an abstract, summary, synopsis, etc., or a list of chapter headings, songs, parts, etc. included in the expression."@en ;
	RegAp:name "hasSummarizationOfContent"@en ;
	RegAp:status <http://metadataregistry.org/uri/RegStatus/1001> .

frbrer:P3017 a owl:NamedIndividual ;
	skos:definition "Relates an expression to the historical, social, intellectual, artistic, or other context within which the expression was realized."@en ;
	RegAp:name "hasContextForTheExpression"@en ;
	RegAp:status <http://metadataregistry.org/uri/RegStatus/1001> .

frbrer:P3018 a owl:NamedIndividual ;
	skos:definition "Relates an expression to the reception given to the expression by reviewers, critics, etc., as encapsulated in an annotation."@en ;
	RegAp:name "hasCriticalResponseToTheExpression"@en ;
	RegAp:status <http://metadataregistry.org/uri/RegStatus/1001> .

frbrer:P3019 a owl:NamedIndividual ;
	skos:definition "Relates an expression to restrictions on access to and use of an expression."@en ;
	skos:scopeNote "Use restrictions may be based in copyright, or they may extend beyond the protections guaranteed in law to the owner of the copyright."@en ;
	RegAp:name "hasUseRestrictionsOnTheExpression"@en ;
	RegAp:status <http://metadataregistry.org/uri/RegStatus/1001> .

frbrer:P3020 a owl:NamedIndividual ;
	skos:definition "Relates a manifestation to the word, phrase, or group of characters naming the manifestation."@en ;
	skos:scopeNote "There may be one or more titles associated with a manifestation. Titles associated with a manifestation include all those that appear in the manifestation itself (e.g., the title on the title page, title frame, etc., a cover title, added title-page title, caption title, running title, spine title, etc., the title in a colophon, explicit, etc., the title on a container, on a microfiche header, etc.), as well as those that have been assigned to the manifestation for purposes of bibliographic control (e.g., key title, expanded title, translated title, supplied title, etc.)."@en ;
	RegAp:name "hasTitleOfTheManifestation"@en ;
	RegAp:status <http://metadataregistry.org/uri/RegStatus/1001> .

frbrer:P3021 a owl:NamedIndividual ;
	skos:scopeNote "An individual or group named may be directly responsible for the work embodied in the manifestation (e.g., the author, composer, etc.), or indirectly responsible (e.g., the author of a novel on which a film script is based). Other individuals or groups named in the statement may include those responsible for the expression of the work contained in the manifestation (e.g., translators, performers, etc.), or those responsible for the compilation of works contained in the manifestation (e.g., the editor, compiler, etc.). A statement of responsibility may name an organization responsible for sponsoring or issuing the work contained in the manifestation. The statement may also indicate the role or function performed by each of the individuals, groups, or organizations responsible. The names appearing in the statement of responsibility in the manifestation may or may not be those of the persons and corporate bodies actually responsible for the creation or realization of the intellectual or artistic content embodied in the manifestation. Similarly, the stated functions may or may not reflect the actual relationship that exists between the individuals and groups named and the intellectual or artistic content."@en ;
	skos:definition "Relates a manifestation to a statement appearing in the manifestation (normally in conjunction with the title) that names one or more individuals or groups responsible for the creation or realization of the intellectual or artistic content embodied in the manifestation."@en ;
	RegAp:name "hasStatementOfResponsibility"@en ;
	RegAp:status <http://metadataregistry.org/uri/RegStatus/1001> .

frbrer:P3022 a owl:NamedIndividual ;
	skos:scopeNote "A series statement may also include a number designating the sequential position of the manifestation within the series. There may be one or more series and, or, subseries named in the manifestation."@en ;
	skos:definition "Relates a manifestation to the word, phrase, or group of characters appearing in the manifestation naming the series to which the manifestation belongs."@en ;
	RegAp:name "hasSeriesStatement"@en ;
	RegAp:status <http://metadataregistry.org/uri/RegStatus/1001> .

frbrer:P3023 a owl:NamedIndividual ;
	skos:scopeNote "E.g., sound cassette, videodisc, microfilm cartridge, transparency, etc. The carrier for a manifestation comprising multiple physical components may include more than one form (e.g., a filmstrip with an accompanying booklet, a separate sound disc carrying the sound track for a film, etc.)."@en ;
	skos:definition "Relates a manifestation to the specific class of material to which the physical carrier of the manifestation belongs."@en ;
	RegAp:name "hasFormOfCarrier"@en ;
	RegAp:status <http://metadataregistry.org/uri/RegStatus/1001> .

frbrer:P3024 a owl:NamedIndividual ;
	skos:scopeNote "E.g., number of sheets, discs, reels, etc."@en ;
	skos:definition "Relates a manifestation to a quantification of the number of physical units making up the carrier."@en ;
	RegAp:name "hasExtentOfTheCarrier"@en ;
	RegAp:status <http://metadataregistry.org/uri/RegStatus/1001> .

frbrer:P3025 a owl:NamedIndividual ;
	skos:scopeNote "E.g., paper, wood, plastic, metal, etc. The physical medium may include in addition to the base material any material that is applied to the base (e.g., oil paint applied to canvas, a chemical emulsion applied to a film base, etc.). Each component of a manifestation comprising multiple physical components may be produced from a different type of material."@en ;
	skos:definition "Relates a manifestation to the type of material from which the carrier is produced."@en ;
	RegAp:name "hasPhysicalMedium"@en ;
	RegAp:status <http://metadataregistry.org/uri/RegStatus/1001> .

frbrer:P3026 a owl:NamedIndividual ;
	skos:scopeNote "E.g., analogue, acoustic, electric, digital, optical etc."@en ;
	skos:definition "Relates a manifestation to the means used to record notation, sound, or images in the production of a manifestation."@en ;
	RegAp:name "hasCaptureMode"@en ;
	RegAp:status <http://metadataregistry.org/uri/RegStatus/1001> .

frbrer:P3027 a owl:NamedIndividual ;
	skos:definition "Relates a manifestation to the measurements of the physical components and, or, the container of the manifestation."@en ;
	skos:scopeNote "The dimensions may comprise measurements of height (e.g., 18 cm bound volume), width (e.g., 8mm film), height x width (e.g., 5 x 5 cm slide), height x width x depth (e.g., 9 x 30 x 20 cm model), or diameter (e.g., 30 cm disc)."@en ;
	RegAp:name "hasDimensionsOfTheCarrier"@en ;
	RegAp:status <http://metadataregistry.org/uri/RegStatus/1001> .

frbrer:P3028 a owl:NamedIndividual ;
	skos:scopeNote "A manifestation may have one or more identifiers associated with it. The identifier may be assigned as part of an international numbering or coding system (e.g., ISBN, etc.), as part of a national system (e.g., legal deposit number), or it may be assigned independently by the publisher or distributor of the manifestation (e.g., government publication number, music publisher's number, clearinghouse inventory number, etc.). A manifestation identifier may also be assigned by a bibliographer, musicologist, etc. The manifestation identifier may comprise both a numeric component and a textual or coded component identifying the system under which it was assigned and, or, the agency or individual that assigned the number, so as to render the identifier unique to the manifestation."@en ;
	skos:definition "Relates a manifestation to a number or code uniquely associated with the manifestation that serves to differentiate that manifestation from any other manifestation."@en ;
	RegAp:name "hasManifestationIdentifier"@en ;
	RegAp:status <http://metadataregistry.org/uri/RegStatus/1001> .

frbrer:P3029 a owl:NamedIndividual ;
	skos:scopeNote "E.g., free to members of a particular association."@en ;
	skos:definition "Relates a manifestation to the terms indicated in the manifestation under which the supplier (i.e., the source for acquisition or access authorization) will normally make the manifestation available, or the price for which the manifestation sells."@en ;
	RegAp:name "hasTermsOfAvailability"@en ;
	RegAp:status <http://metadataregistry.org/uri/RegStatus/1001> .

frbrer:P3030 a owl:NamedIndividual ;
	skos:scopeNote "Access restrictions may be based in copyright, or they may extend beyond the protections guaranteed in law to the owner of the copyright."@en ;
	skos:definition "Relates a manifestation to restrictions on access to and use of a manifestation."@en ;
	RegAp:name "hasAccessRestrictionsOnTheManifestation"@en ;
	RegAp:status <http://metadataregistry.org/uri/RegStatus/1001> .

frbrer:P3031 a owl:NamedIndividual ;
	skos:scopeNote "E.g., call number, accession number, bar code, etc. The number is normally assigned by the institution that holds the item. The item identifier may also include a name or code identifying the institution or repository in which the item is housed, and a name or code identifying a particular collection or sub-unit within the institution (e.g., a rare book collection, a branch library, etc.)."@en ;
	skos:definition "Relates an item to a number or code that is uniquely associated with the item, and serves to differentiate that item from any other item in the same collection and, or, institution."@en ;
	RegAp:name "hasItemIdentifier"@en ;
	RegAp:status <http://metadataregistry.org/uri/RegStatus/1001> .

frbrer:P3032 a owl:NamedIndividual ;
	skos:definition "Relates an item to an identifier constructed by combining groups of characters transcribed from specified pages of a printed item."@en ;
	skos:scopeNote "The technique is used primarily to signal differences between individual copies of early printed books. There are various formulae for constructing the fingerprint (e.g., the one specified in Fingerprints = Empreintes = Impronte, published by the Institut de Recherche et dHistoire des Textes in Paris)."@en ;
	RegAp:name "hasFingerprint"@en ;
	RegAp:status <http://metadataregistry.org/uri/RegStatus/1001> .

frbrer:P3033 a owl:NamedIndividual ;
	skos:definition "Relates an item to a record of previous ownership or custodianship of the item."@en ;
	RegAp:name "hasProvenanceOfTheItem"@en ;
	RegAp:status <http://metadataregistry.org/uri/RegStatus/1001> .

frbrer:P3034 a owl:NamedIndividual ;
	skos:definition "Relates an item to a record of public exhibitions of an item, including dates, venues, etc."@en ;
	RegAp:name "hasExhibitionHistory"@en ;
	RegAp:status <http://metadataregistry.org/uri/RegStatus/1001> .

frbrer:P3035 a owl:NamedIndividual ;
	skos:scopeNote "E.g., missing pages, plates, etc. Condition may reflect other aspects of the physical condition of the item as well (e.g., brittleness, faded images, etc.)."@en ;
	skos:definition "Relates an item to the physical condition of the item, particularly any variances between the physical makeup of the item and that of the manifestation it exemplifies."@en ;
	RegAp:name "hasConditionOfTheItem"@en ;
	RegAp:status <http://metadataregistry.org/uri/RegStatus/1001> .

frbrer:P3036 a owl:NamedIndividual ;
	skos:scopeNote "E.g., deacidification, restoration, etc. Treatment history may also comprise details of the treatment process (e.g., chemical solutions used, techniques applied, etc.), the date the treatment was applied, etc."@en ;
	skos:definition "Relates an item to a record of the treatment the item has undergone."@en ;
	RegAp:name "hasTreatmentHistory"@en ;
	RegAp:status <http://metadataregistry.org/uri/RegStatus/1001> .

frbrer:P3037 a owl:NamedIndividual ;
	skos:scopeNote "E.g., chemical wash. Scheduled treatment may also comprise details of the planned treatment process and the scheduled date of application."@en ;
	skos:definition "Relates an item to a plan for future treatment of the item."@en ;
	RegAp:name "hasScheduledTreatment"@en ;
	RegAp:status <http://metadataregistry.org/uri/RegStatus/1001> .

frbrer:P3038 a owl:NamedIndividual ;
	skos:scopeNote "E.g., restricted to supervised on-site use, etc."@en ;
	skos:definition "Relates an item to any limitations placed on physical access to the item."@en ;
	RegAp:name "hasAccessRestrictionsOnTheItem"@en ;
	RegAp:status <http://metadataregistry.org/uri/RegStatus/1001> .

frbrer:P3039 a owl:NamedIndividual ;
	skos:scopeNote "E.g., Donald Horne, A. A. Milne, Ellery Queen, etc. A name may include one or more forenames (or given names), matronymics, patronymics, family names (or surnames), sobriquets, dynastic names, etc. A person may be known by more than one name, or by more than one form of the same name. A bibliographic agency normally selects one of those names as the uniform heading for purposes of consistency in naming and referencing the person. The other names or forms of name may be treated as variant names for the person. In some cases (e.g., in the case of a person who writes under more than one pseudonym, or a person who writes both in an official capacity and as an individual) the bibliographic agency may establish more than one uniform heading for the person."@en ;
	skos:definition "Relates a person to the word, character, or group of words and, or, characters by which the person is known."@en ;
	RegAp:name "hasNameOfPerson"@en ;
	RegAp:status <http://metadataregistry.org/uri/RegStatus/1001> .

frbrer:P3040 a owl:NamedIndividual ;
	skos:definition "Relates a person to the precise or approximate date of the person's birth and, or, death, or dates indicating the period in which the person was known to be active in a given field of endeavour, and other dates."@en ;
	RegAp:name "hasDatesOfPerson"@en ;
	RegAp:status <http://metadataregistry.org/uri/RegStatus/1001> .

frbrer:P3041 a owl:NamedIndividual ;
	skos:scopeNote "E.g., Major, Premier, Duke, etc.; Sir, Mrs., etc."@en ;
	skos:definition "Relates a person to a word or phrase indicative of rank, office, nobility, honour, etc., or a term of address associated with the person."@en ;
	RegAp:name "hasTitleOfPerson"@en ;
	RegAp:status <http://metadataregistry.org/uri/RegStatus/1001> .

frbrer:P3042 a owl:NamedIndividual ;
	skos:scopeNote "E.g., III, Jr., etc.; the Brave, Professional Engineer, etc."@en ;
	skos:definition "Relates a person to a numeral, word, or abbreviation indicating succession within a family or dynasty, or an epithet or other word or phrase associated with the person."@en ;
	RegAp:name "hasOtherDesignationAssociatedWithThePerson"@en ;
	RegAp:status <http://metadataregistry.org/uri/RegStatus/1001> .

frbrer:P3043 a owl:NamedIndividual ;
	skos:scopeNote "E.g., Royal Aeronautical Society, IBM, Sminaire europen sur la recherche en ducation, Friedrich Witte, etc. A corporate body may be known by more than one name, or more than one form of the same name. A bibliographic agency normally selects one of those names as the uniform heading for purposes of consistency in naming and referencing the corporate body. The other names or forms of name may be treated as variant names for the corporate body. In some cases (e.g., in the case where a corporate body is known by different names at different periods in its history) the bibliographic agency may establish more than one uniform heading for the corporate body."@en ;
	skos:definition "Relates a corporate body to the word, phrase, character, or group of words and, or, characters by which the body is known."@en ;
	RegAp:name "hasNameOfTheCorporateBody"@en ;
	RegAp:status <http://metadataregistry.org/uri/RegStatus/1001> .

frbrer:P3044 a owl:NamedIndividual ;
	skos:definition "Relates a corporate body to the numerical designation sequencing a meeting, conference, exhibition, fair, etc. that constitutes one of a series of related meetings, conferences, exhibitions, fairs, etc., or any other numerical designation associated with a corporate body."@en ;
	RegAp:name "hasNumberAssociatedWithTheCorporateBody"@en ;
	RegAp:status <http://metadataregistry.org/uri/RegStatus/1001> .

frbrer:P3045 a owl:NamedIndividual ;
	skos:scopeNote "E.g., Los Angeles, Bretton Woods, Oxford University, etc. The place may comprise the name of the state, province, territory, and, or, country as well as the local place name."@en ;
	skos:definition "Relates a corporate body to the city, town, or other designation of location in which a meeting, conference, exhibition, fair, etc. was held, or the location with which the corporate body is otherwise associated."@en ;
	RegAp:name "hasPlaceAssociatedWithTheCorporateBody"@en ;
	RegAp:status <http://metadataregistry.org/uri/RegStatus/1001> .

frbrer:P3046 a owl:NamedIndividual ;
	skos:scopeNote "E.g., the date of incorporation."@en ;
	skos:definition "Relates a corporate body to the date or range of dates on which a meeting, conference, exhibition, fair, etc. was held, or a date with which the corporate body is otherwise associated."@en ;
	RegAp:name "hasDateAssociatedWithTheCorporateBody"@en ;
	RegAp:status <http://metadataregistry.org/uri/RegStatus/1001> .

frbrer:P3047 a owl:NamedIndividual ;
	skos:scopeNote "E.g., Inc., Ltd., etc.; firm, musical group, etc."@en ;
	skos:definition "Relates a corporate body to a word, phrase, or abbreviation indicating incorporation or legal status of the body, or any term serving to differentiate the body from other corporate bodies, persons, etc."@en ;
	RegAp:name "hasOtherDesignationAssociatedWithTheCorporateBody"@en ;
	RegAp:status <http://metadataregistry.org/uri/RegStatus/1001> .

frbrer:P3048 a owl:NamedIndividual ;
	skos:scopeNote "E.g., economics, existentialism, radioactivity, etc. A concept may be designated by more than one term, or by more than one form of the term. A bibliographic agency normally selects one of those terms as the uniform heading for purposes of consistency in naming and referencing the concept. The other terms or forms of term may be treated as variant terms for the concept."@en ;
	skos:definition "Relates a concept to the word, phrase, or group of characters used to name or designate the concept."@en ;
	RegAp:name "hasTermForTheConcept"@en ;
	RegAp:status <http://metadataregistry.org/uri/RegStatus/1001> .

frbrer:P3049 a owl:NamedIndividual ;
	skos:scopeNote "E.g., a building, a ship, etc. An object may be designated by more than one term, or by more than one form of the term. A bibliographic agency normally selects one of those terms as the uniform heading for purposes of consistency in naming and referencing the object. The other terms or forms of term may be treated as variant terms for the object."@en ;
	skos:definition "Relates an object to the word, phrase, or group of characters used to name or designate the object."@en ;
	RegAp:name "hasTermForTheObject"@en ;
	RegAp:status <http://metadataregistry.org/uri/RegStatus/1001> .

frbrer:P3050 a owl:NamedIndividual ;
	skos:scopeNote "E.g., Battle of Hastings, Tour de France, etc. An event may be designated by more than one term, or by more than one form of the term. A bibliographic agency normally selects one of those terms as the uniform heading for purposes of consistency in naming and referencing the event. The other terms or forms of term may be treated as variant terms for the event."@en ;
	skos:definition "Relates an event to the word, phrase, or group of characters used to name or designate the event."@en ;
	RegAp:name "hasTermForTheEvent"@en ;
	RegAp:status <http://metadataregistry.org/uri/RegStatus/1001> .

frbrer:P3051 a owl:NamedIndividual ;
	skos:scopeNote "E.g., London, St. Lawrence River, etc. A place may be designated by more than one term, or by more than one form of the term. A bibliographic agency normally selects one of those terms as the uniform heading for purposes of consistency in naming and referencing the place. The other terms or forms of term may be treated as variant terms for the place."@en ;
	skos:definition "Relates a place to the word, phrase, or group of characters used to name or designate the place."@en ;
	RegAp:name "hasTermForThePlace"@en ;
	RegAp:status <http://metadataregistry.org/uri/RegStatus/1001> .

frbrer:P3052 a owl:NamedIndividual ;
	skos:definition "Relates an item to any signatures, numbering, annotations, etc. that have been applied uniquely to the item by the artist, fabricator, owner, etc., and other marks and inscriptions."@en ;
	RegAp:name "hasMarksOrInscriptions"@en ;
	RegAp:status <http://metadataregistry.org/uri/RegStatus/1001> .

frbrer:P3053 a owl:NamedIndividual ;
	skos:definition "Relates a manifestation to the name of a publisher, distributor, etc. indicated in the manifestation as the source from which the manifestation may be acquired or through whom access may be authorized."@en ;
	skos:scopeNote "The source for acquisition/access authorization will normally also include an address for the publisher, distributor, etc. A manifestation may be associated with one or more sources."@en ;
	RegAp:name "hasSourceForAcquisitionOrAccessAuthorization"@en ;
	RegAp:status <http://metadataregistry.org/uri/RegStatus/1001> .

frbrer:P3054 a owl:NamedIndividual ;
	skos:scopeNote "A manifestation may be associated with one or more fabricators or manufacturers."@en ;
	skos:definition "Relates a manifestation to the individual, group, or organization named in the manifestation as being responsible for the fabrication or manufacture of the manifestation."@en ;
	RegAp:name "hasFabricatorOrManufacturer"@en ;
	RegAp:status <http://metadataregistry.org/uri/RegStatus/1001> .

frbrer:P3055 a owl:NamedIndividual ;
	skos:definition "Relates a manifestation to the date of public release of the manifestation."@en ;
	skos:scopeNote "The date (normally a year) may be a single date of publication or release, or a range of dates (e.g., in the case of a serial publication). In the absence of a date designated as the date of publication or release, a copyright date or a date of printing or manufacture may serve as a substitute."@en ;
	RegAp:name "hasDateOfPublicationOrDistribution"@en ;
	RegAp:status <http://metadataregistry.org/uri/RegStatus/1001> .

frbrer:P3056 a owl:NamedIndividual ;
	skos:scopeNote "A manifestation may be associated with one or more publishers or distributors."@en ;
	skos:definition "Relates a manifestation to the individual, group, or organization named in the manifestation as being responsible for the publication, distribution, issuing, or release of the manifestation."@en ;
	RegAp:name "hasPublisherOrDistributor"@en ;
	RegAp:status <http://metadataregistry.org/uri/RegStatus/1001> .

frbrer:P3057 a owl:NamedIndividual ;
	skos:definition "Relates a manifestation to the city, town, or other locality associated in the manifestation with the name of the publisher or distributor."@en ;
	skos:scopeNote "The place of publication may comprise the name of the state, province, territory, and/or country as well as the local place name. A manifestation may be associated with one or more places of publication or distribution."@en ;
	RegAp:name "hasPlaceOfPublicationOrDistribution"@en ;
	RegAp:status <http://metadataregistry.org/uri/RegStatus/1001> .

frbrer:P3058 a owl:NamedIndividual ;
	skos:definition "Relates a manifestation to a word or phrase appearing in the manifestation that normally indicates a difference in either content or form between the manifestation and a related manifestation previously issued by the same publisher/distributor, or simultaneously issued by either the same publisher/distributor or another publisher/distributor."@en ;
	skos:scopeNote "The edition/issue designation pertains to all copies of a manifestation produced from substantially the same master and issued by the same publisher/distributor or group of publishers/distributors."@en ;
	RegAp:name "hasEditionOrIssueDesignation"@en ;
	RegAp:status <http://metadataregistry.org/uri/RegStatus/1001> .

frbrer:P3059 a owl:NamedIndividual ;
	skos:scopeNote "E.g., piano, violin, orchestra, men's voices, etc."@en ;
	skos:definition "Relates a work that is musical to the instrumental, vocal, and, or, other medium of performance for which the work was originally intended."@en ;
	RegAp:name "hasMediumOfPerformanceMusicalWork"@en ;
	RegAp:status <http://metadataregistry.org/uri/RegStatus/1001> .

frbrer:P3060 a owl:NamedIndividual ;
	skos:definition "Relates a work that is musical to a serial number, opus number, or thematic index number assigned to thel work by the composer, publisher, or a musicologist."@en ;
	RegAp:name "hasNumericDesignationMusicalWork"@en ;
	RegAp:status <http://metadataregistry.org/uri/RegStatus/1001> .

frbrer:P3061 a owl:NamedIndividual ;
	skos:definition "Relates a work that is musical to the set of pitch relationships that establishes a single pitch class as a tonal centre."@en ;
	skos:scopeNote "The key for a musical work is the key in which the work is originally composed."@en ;
	RegAp:name "hasKeyMusicalWork"@en ;
	RegAp:status <http://metadataregistry.org/uri/RegStatus/1001> .

frbrer:P3062 a owl:NamedIndividual ;
	skos:definition "Relates a work that is cartographic to the degrees, minutes, and seconds of longitude and latitude, or the angles of declination and ascension that form the outer boundaries for the area represented in the cartographic image or object."@en ;
	RegAp:name "hasCoordinatesCartographicWork"@en ;
	RegAp:status <http://metadataregistry.org/uri/RegStatus/1001> .

frbrer:P3063 a owl:NamedIndividual ;
	skos:definition "Relates a work that is cartographic to the year that serves as the point of reference for a celestial chart or model."@en ;
	RegAp:name "hasEquinoxCartographicWork"@en ;
	RegAp:status <http://metadataregistry.org/uri/RegStatus/1001> .

frbrer:P3064 a owl:NamedIndividual ;
	skos:definition "Relates an expression issued as a serial to the form anticipated to be used in designating volumes, issues, etc. and, or, dates for the individual units of the serial."@en ;
	RegAp:name "hasSequencingPatternSerial"@en ;
	RegAp:status <http://metadataregistry.org/uri/RegStatus/1001> .

frbrer:P3065 a owl:NamedIndividual ;
	skos:definition "Relates an expression issued as a serial to the anticipated regularity of release of individual issues (i.e., whether the release is expected to be regular or irregular)."@en ;
	RegAp:name "hasExpectedRegularityOfIssueSerial"@en ;
	RegAp:status <http://metadataregistry.org/uri/RegStatus/1001> .

frbrer:P3066 a owl:NamedIndividual ;
	skos:scopeNote "E.g., weekly, monthly, quarterly, annually, etc."@en ;
	skos:definition "Relates an expression issued as a serial to the interval at which individual issues of the serial are anticipated to be released."@en ;
	RegAp:name "hasExpectedFrequencyOfIssueSerial"@en ;
	RegAp:status <http://metadataregistry.org/uri/RegStatus/1001> .

frbrer:P3067 a owl:NamedIndividual ;
	skos:scopeNote "E.g., short score, full score, condensed score, close score, etc."@en ;
	skos:definition "Relates an expression that is a musical notation to the format used to represent a musical composition."@en ;
	RegAp:name "hasTypeOfScoreMusicalNotation"@en ;
	RegAp:status <http://metadataregistry.org/uri/RegStatus/1001> .

frbrer:P3068 a owl:NamedIndividual ;
	skos:scopeNote "E.g., two pianos, soprano and alto, etc."@en ;
	skos:definition "Relates an expression that is a musical notation or recorded sound to the instrumental and, or, vocal medium of performance of a musical work represented in the expression. The instruments and, or, voices represented in a particular expression of a work may differ from the medium of performance for which the work was originally intended."@en ;
	RegAp:name "hasMediumOfPerformanceMusicalNotationExpressionOrRecordedSound"@en ;
	RegAp:status <http://metadataregistry.org/uri/RegStatus/1001> .

frbrer:P3070 a owl:NamedIndividual ;
	skos:scopeNote "E.g., multispectral photography, infrared line scanning, SLAR, passive microwave mapping, etc."@en ;
	skos:definition "Relates an expression that is a remote sensing image to the technique used to capture the image through remote sensing."@en ;
	RegAp:name "hasRecordingTechniqueRemoteSensingImage"@en ;
	RegAp:status <http://metadataregistry.org/uri/RegStatus/1001> .

frbrer:P3071 a owl:NamedIndividual ;
	skos:definition "Relates an expression that is a remote sensing image to the altitude and attitude of the sensor, the position of the platform, the category and name of the satellite, the number of spectral bands involved, the quality of the image, the extent of cloud cover, or the mean value of the ground resolution."@en ;
	RegAp:name "hasSpecialCharacteristicRemoteSensingImage"@en ;
	RegAp:status <http://metadataregistry.org/uri/RegStatus/1001> .

frbrer:P3072 a owl:NamedIndividual ;
	skos:scopeNote "E.g., engraving, etc."@en ;
	skos:definition "Relates an expression that is a graphic or projected image to the method used to create it."@en ;
	RegAp:name "hasTechniqueGraphicOrProjectedImage"@en ;
	RegAp:status <http://metadataregistry.org/uri/RegStatus/1001> .

frbrer:P3074 a owl:NamedIndividual ;
	skos:scopeNote "E.g., Baskerville, Times New Roman, etc."@en ;
	skos:definition "Relates a manifestation that is a printed book to the style of type used to print it."@en ;
	RegAp:name "hasTypefacePrintedBook"@en ;
	RegAp:status <http://metadataregistry.org/uri/RegStatus/1001> .

frbrer:P3075 a owl:NamedIndividual ;
	skos:definition "Relates a manifestation that is a printed book to the size of the characters in it."@en ;
	RegAp:name "hasTypeSizePrintedBook"@en ;
	RegAp:status <http://metadataregistry.org/uri/RegStatus/1001> .

frbrer:P3076 a owl:NamedIndividual ;
	skos:scopeNote "E.g., a sheet folded twice to form a quarto, three times to form an octavo, etc."@en ;
	skos:definition "Relates a manifestation that is a hand-printed book to a reflection of the number of folds made in a printed sheet to form a gathering of leaves."@en ;
	RegAp:name "hasFoliationHandPrintedBook"@en ;
	RegAp:status <http://metadataregistry.org/uri/RegStatus/1001> .

frbrer:P3077 a owl:NamedIndividual ;
	skos:scopeNote "E.g., four gatherings bearing signatures A through D."@en ;
	skos:definition "Relates a manifestation that is a hand-printed book to a reflection of the sequence of gatherings in the book as indicated by signatures on each gathering."@en ;
	RegAp:name "hasCollationHandPrintedBook"@en ;
	RegAp:status <http://metadataregistry.org/uri/RegStatus/1001> .

frbrer:P3078 a owl:NamedIndividual ;
	skos:definition "Relates a manifestation that is a serial to its status with respect to its continuing publication (i.e., whether it is currently published or has ceased publication)."@en ;
	RegAp:name "hasPublicationStatusSerial"@en ;
	RegAp:status <http://metadataregistry.org/uri/RegStatus/1001> .

frbrer:P3079 a owl:NamedIndividual ;
	skos:definition "Relates a manifestation that is a serial to the designation of volume, issue, etc. and, or, date appearing in it."@en ;
	skos:scopeNote "The numbering may comprise a numeric, alphabetic and, or, a date component (e.g., Volume 1, number 1 (January 1971))."@en ;
	RegAp:name "hasNumberingSerial"@en ;
	RegAp:status <http://metadataregistry.org/uri/RegStatus/1001> .

frbrer:P3080 a owl:NamedIndividual ;
	skos:scopeNote "E.g., 33 1/3 rpm, 19 cm/s, etc."@en ;
	skos:definition "Relates a manifestation that is a sound recording to the speed at which the carrier must be operated to produce the sound intended."@en ;
	RegAp:name "hasPlayingSpeedSoundRecording"@en ;
	RegAp:status <http://metadataregistry.org/uri/RegStatus/1001> .

frbrer:P3081 a owl:NamedIndividual ;
	skos:scopeNote "E.g., microgroove--i.e., 200 grooves per inch."@en ;
	skos:definition "Relates a manifestation that is a sound recording to an indication of the number of grooves per inch cut on a disc or cylinder."@en ;
	RegAp:name "hasGrooveWidth"@en ;
	RegAp:status <http://metadataregistry.org/uri/RegStatus/1001> .

frbrer:P3082 a owl:NamedIndividual ;
	skos:scopeNote "E.g., lateral, vertical, etc."@en ;
	skos:definition "Relates a manifestation that is a sound recording to the direction in which the grooves are cut on a disc or cylinder."@en ;
	RegAp:name "hasKindOfCuttingSoundRecording"@en ;
	RegAp:status <http://metadataregistry.org/uri/RegStatus/1001> .

frbrer:P3083 a owl:NamedIndividual ;
	skos:scopeNote "E.g., eight track, twelve track."@en ;
	skos:definition "Relates a manifestation that is a sound recording to the number of tracks on a sound tape."@en ;
	RegAp:name "hasTapeConfigurationSoundRecording"@en ;
	RegAp:status <http://metadataregistry.org/uri/RegStatus/1001> .

frbrer:P3084 a owl:NamedIndividual ;
	skos:scopeNote "E.g., Monaural, stereophonic, quadraphonic, etc."@en ;
	skos:definition "Relates a manifestation that is a sound recording to a reflection of the number of sound channels used to make the recording."@en ;
	RegAp:name "hasKindOfSoundSoundRecording"@en ;
	RegAp:status <http://metadataregistry.org/uri/RegStatus/1001> .

frbrer:P3085 a owl:NamedIndividual ;
	skos:scopeNote "E.g., NAB, DBX, Dolby, etc."@en ;
	skos:definition "Relates a manifestation that is a sound recording to the equalization system, noise reduction system, etc. used in making the recording."@en ;
	RegAp:name "hasSpecialReproductionCharacteristicSoundRecording"@en ;
	RegAp:status <http://metadataregistry.org/uri/RegStatus/1001> .

frbrer:P3086 a owl:NamedIndividual ;
	skos:definition "Relates a manifestation that is an image to the colour(s), tone(s), etc. (including black and white) used in the production of the image."@en ;
	RegAp:name "hasColourImage"@en ;
	RegAp:status <http://metadataregistry.org/uri/RegStatus/1001> .

frbrer:P3087 a owl:NamedIndividual ;
	skos:scopeNote "E.g., 42x, etc. Reduction ratio may also be indicated as a range (e.g., very high reduction indicates a reduction in the range of 61x to 90x)."@en ;
	skos:definition "Relates a manifestation that is a microform to the degree to which a text or image has been reduced in the process of microfilming."@en ;
	RegAp:name "hasReductionRatioMicroform"@en ;
	RegAp:status <http://metadataregistry.org/uri/RegStatus/1001> .

frbrer:P3088 a owl:NamedIndividual ;
	skos:definition "Relates a manifestation that is a microform or visual projection to the relationship of the colours and tones in the image on film to the colours and tones of the object filmed."@en ;
	skos:scopeNote "When the colours and tones in the film image reflect directly the colour and tones of the object filmed, the polarity is positive. When they are the reverse of the object the polarity is negative. The polarity of images in a manifestation comprising more than one image may be mixed."@en ;
	RegAp:name "hasPolarityMicroformOrVisualProjection"@en ;
	RegAp:status <http://metadataregistry.org/uri/RegStatus/1001> .

frbrer:P3089 a owl:NamedIndividual ;
	skos:scopeNote "E.g., a first generation camera master, a second generation printing master, a third generation service copy, etc."@en ;
	skos:definition "Relates a manifestation that is a microform or visual projection to a reflection of the number of times the image on film has been transferred from one carrier to another."@en ;
	RegAp:name "hasGenerationMicroformOrVisualProjection"@en ;
	RegAp:status <http://metadataregistry.org/uri/RegStatus/1001> .

frbrer:P3090 a owl:NamedIndividual ;
	skos:scopeNote "E.g., wide screen, Beta, VHS, etc."@en ;
	skos:definition "Relates a manifestation that is a visual projection to the format used in the production of the projected image."@en ;
	RegAp:name "hasPresentationFormatVisualProjection"@en ;
	RegAp:status <http://metadataregistry.org/uri/RegStatus/1001> .

frbrer:P3093 a owl:NamedIndividual ;
	skos:scopeNote "E.g., machine make and model, RAM capacity, etc. E.g., operating systems, programming language, supporting software, etc. Peripherals include monitor, printer, mouse, etc."@en ;
	skos:definition "Relates a manifestation that is an electronic resource to requirements related to hardware, software, and peripherals, and other system components."@en ;
	RegAp:name "hasSystemRequirementsElectronicResource"@en ;
	RegAp:status <http://metadataregistry.org/uri/RegStatus/1001> .

frbrer:P3094 a owl:NamedIndividual ;
	skos:scopeNote "E.g., ASCII, SGML, etc. E.g., recording density, parity, blocking, etc."@en ;
	skos:definition "Relates a manifestation that is an electronic resource to standards or schemes used to encode the file, physical characteristics of the file, and other characteristics that have a bearing on how the file can be processed."@en ;
	RegAp:name "hasFileCharacteristicsElectronicResource"@en ;
	RegAp:status <http://metadataregistry.org/uri/RegStatus/1001> .

frbrer:P3095 a owl:NamedIndividual ;
	skos:scopeNote "E.g., Internet, World Wide Web, etc."@en ;
	skos:definition "Relates a manifestation that is a remote electronic resource to the means of accessing it."@en ;
	RegAp:name "hasModeOfAccessRemoteElectronicResource"@en ;
	RegAp:status <http://metadataregistry.org/uri/RegStatus/1001> .

frbrer:P3096 a owl:NamedIndividual ;
	skos:scopeNote "E.g., universal resource locator  URL."@en ;
	skos:definition "Relates a manifestation that is a remote electronic resource to an alpha-numeric code used to facilitate remote access to it."@en ;
	RegAp:name "hasAccessAddressRemoteElectronicResource"@en ;
	RegAp:status <http://metadataregistry.org/uri/RegStatus/1001> .

frbrer:P3097 a owl:NamedIndividual ;
	skos:definition "Relates an expression that is cartographic to the ratio of distances in the expression to the actual distances they represent."@en ;
	skos:scopeNote "Scale may apply to horizontal, vertical, angular, and, or, other distances represented in the expression."@en ;
	RegAp:name "hasScaleCartographicImageOrObject"@en ;
	RegAp:status <http://metadataregistry.org/uri/RegStatus/1001> .

frbrer:P3098 a owl:NamedIndividual ;
	skos:scopeNote "E.g., transverse Mercator, azimuthal equidistant, etc."@en ;
	skos:definition "Relates an expression that is cartographic to the method or system used to represent the surface of the Earth or of a celestial sphere on a plane."@en ;
	RegAp:name "hasProjectionCartographicImageOrObject"@en ;
	RegAp:status <http://metadataregistry.org/uri/RegStatus/1001> .

frbrer:P3099 a owl:NamedIndividual ;
	skos:scopeNote "E.g., anaglyphic, diagrammatic, pictorial, etc."@en ;
	skos:definition "Relates an expression that is cartographic to the method used to represent geographic or other features in a cartographic image."@en ;
	RegAp:name "hasPresentationTechniqueCartographicImageOrObject"@en ;
	RegAp:status <http://metadataregistry.org/uri/RegStatus/1001> .

frbrer:P3100 a owl:NamedIndividual ;
	skos:scopeNote "E.g., contours, shading, hachures, spot heights, bathymetric tints, etc."@en ;
	skos:definition "Relates an expression that is cartographic to the technique used to depict the elevations or the inequalities of a land surface or of the bed of a body of water in a cartographic image."@en ;
	RegAp:name "hasRepresentationOfReliefCartographicImageOrObject"@en ;
	RegAp:status <http://metadataregistry.org/uri/RegStatus/1001> .

frbrer:P3101 a owl:NamedIndividual ;
	skos:definition "Relates an expression that is cartographic to information on the spheroid used to construct the cartographic image, the grid or referencing systems used in the image, horizontal datum, vertical datum, mathematical data on contour intervals, bathymetric intervals, etc., and other geodetic, grid and vertical measurements."@en ;
	RegAp:name "hasGeodeticGridAndVerticalMeasurementCartographicImageOrObject"@en ;
	RegAp:status <http://metadataregistry.org/uri/RegStatus/1001> .

<http://metadataregistry.org/uri/RegStatus/1001> a skos:Concept , owl:NamedIndividual ;
	skos:prefLabel "Published"@en .

publications:functional-requirements-for-bibliographic-records a owl:NamedIndividual .

owl:genid1 rdfs:comment "stuff" .

_:node18r56emdgx6 a owl:AllDisjointProperties ;
	owl:members _:node18r56emdgx7 .

_:node18r56emdgx7 rdf:first frbrer:P3054 ;
	rdf:rest rdf:nil .

frbrer:C1002 rdfs:subClassOf _:node18r56emdgx8 .

_:node18r56emdgx8 a owl:Restriction ;
	owl:onProperty frbrer:P2002 ;
	owl:onClass frbrer:C1001 ;
	owl:qualifiedCardinality "1"^^xsd:nonNegativeInteger .

frbrer:C1003 rdfs:subClassOf _:node18r56emdgx9 .

_:node18r56emdgx9 a owl:Restriction ;
	owl:onProperty frbrer:P2004 ;
	owl:onClass frbrer:C1002 ;
	owl:minQualifiedCardinality "1"^^xsd:nonNegativeInteger .

frbrer:C1004 rdfs:subClassOf _:node18r56emdgx10 .

_:node18r56emdgx10 a owl:Restriction ;
	owl:onProperty frbrer:P2006 ;
	owl:onClass frbrer:C1003 ;
	owl:qualifiedCardinality "1"^^xsd:nonNegativeInteger .
