<http://vcharpenay.github.io/hto/hto.xml> <http://www.w3.org/1999/02/22-rdf-syntax-ns#type> <http://www.w3.org/2002/07/owl#Ontology> .
<http://vcharpenay.github.io/hto/hto.xml> <http://purl.org/dc/terms/modified> "2015-10-19"^^<http://www.w3.org/2001/XMLSchema#date> .
<http://vcharpenay.github.io/hto/hto.xml> <http://www.w3.org/2000/01/rdf-schema#seeAlso> "http://project-haystack.org"^^<http://www.w3.org/2001/XMLSchema#anyURI> .
<http://vcharpenay.github.io/hto/hto.xml> <http://creativecommons.org/ns#license> "Academic Free License (\"AFL\") 3.0" .
<http://vcharpenay.github.io/hto/hto.xml> <http://purl.org/dc/elements/1.1/title> "Haystack Tagging Ontology" .
<http://vcharpenay.github.io/hto/hto.xml> <http://purl.org/dc/elements/1.1/creator> "Victor Charpenay <victor.charpenay[at]siemens.com>" .
<http://vcharpenay.github.io/hto/hto.xml> <http://www.w3.org/2000/01/rdf-schema#comment> "The Haystack Tagging Ontology is an OWL ontology for Project Haystack, a domain vocabulary for Building Automation Systems." .
<http://vcharpenay.github.io/hto/hto.xml> <http://www.w3.org/2002/07/owl#versionInfo> "0.1.0" .
<http://vcharpenay.github.io/hto/hto.xml> <http://www.w3.org/2002/07/owl#imports> <http://purl.oclc.org/NET/ssnx/ssn> .
<http://vcharpenay.github.io/hto/hto.xml#associatedTo> <http://www.w3.org/1999/02/22-rdf-syntax-ns#type> <http://www.w3.org/2002/07/owl#AnnotationProperty> .
<http://vcharpenay.github.io/hto/hto.xml#associatedTo> <http://www.w3.org/2000/01/rdf-schema#comment> "gives the OWL class defined in the present ontology that should be associated to the individual defined as subject." .
<http://vcharpenay.github.io/hto/hto.xml#associatedTo> <http://www.w3.org/2000/01/rdf-schema#domain> <http://vcharpenay.github.io/hto/hto.xml#HTag> .
<http://vcharpenay.github.io/hto/hto.xml#belongsTo> <http://www.w3.org/1999/02/22-rdf-syntax-ns#type> <http://www.w3.org/2002/07/owl#ObjectProperty> .
<http://vcharpenay.github.io/hto/hto.xml#belongsTo> <http://www.w3.org/2000/01/rdf-schema#subPropertyOf> <http://purl.oclc.org/NET/ssnx/ssn#onPlatform> .
<http://vcharpenay.github.io/hto/hto.xml#belongsTo> <http://www.w3.org/2000/01/rdf-schema#range> <http://vcharpenay.github.io/hto/hto.xml#Equipment> .
<http://vcharpenay.github.io/hto/hto.xml#belongsTo> <http://www.w3.org/2000/01/rdf-schema#domain> <http://vcharpenay.github.io/hto/hto.xml#Point> .
<http://vcharpenay.github.io/hto/hto.xml#hasRef> <http://www.w3.org/1999/02/22-rdf-syntax-ns#type> <http://www.w3.org/2002/07/owl#ObjectProperty> .
<http://vcharpenay.github.io/hto/hto.xml#hasRef> <http://www.w3.org/2002/07/owl#inverseOf> <http://vcharpenay.github.io/hto/hto.xml#isRefedBy> .
<http://vcharpenay.github.io/hto/hto.xml#hasRef> <http://www.w3.org/2000/01/rdf-schema#subPropertyOf> <http://www.w3.org/2002/07/owl#topObjectProperty> .
<http://vcharpenay.github.io/hto/hto.xml#hasSection> <http://www.w3.org/1999/02/22-rdf-syntax-ns#type> <http://www.w3.org/2002/07/owl#ObjectProperty> .
<http://vcharpenay.github.io/hto/hto.xml#hasSection> <http://www.w3.org/2000/01/rdf-schema#domain> <http://vcharpenay.github.io/hto/hto.xml#Equipment> .
<http://vcharpenay.github.io/hto/hto.xml#hasSection> <http://www.w3.org/2000/01/rdf-schema#range> <http://vcharpenay.github.io/hto/hto.xml#Section> .
<http://vcharpenay.github.io/hto/hto.xml#hasTag> <http://www.w3.org/1999/02/22-rdf-syntax-ns#type> <http://www.w3.org/2002/07/owl#ObjectProperty> .
<http://vcharpenay.github.io/hto/hto.xml#isRefedBy> <http://www.w3.org/1999/02/22-rdf-syntax-ns#type> <http://www.w3.org/2002/07/owl#ObjectProperty> .
<http://vcharpenay.github.io/hto/hto.xml#locatedOn> <http://www.w3.org/1999/02/22-rdf-syntax-ns#type> <http://www.w3.org/2002/07/owl#ObjectProperty> .
<http://vcharpenay.github.io/hto/hto.xml#locatedOn> <http://www.w3.org/2000/01/rdf-schema#subPropertyOf> <http://purl.oclc.org/NET/ssnx/ssn#isPropertyOf> .
<http://vcharpenay.github.io/hto/hto.xml#locatedOn> <http://www.w3.org/2000/01/rdf-schema#domain> <http://vcharpenay.github.io/hto/hto.xml#Point> .
<http://vcharpenay.github.io/hto/hto.xml#locatedOn> <http://www.w3.org/2000/01/rdf-schema#range> <http://vcharpenay.github.io/hto/hto.xml#Section> .
<http://vcharpenay.github.io/hto/hto.xml#measuredOn> <http://www.w3.org/1999/02/22-rdf-syntax-ns#type> <http://www.w3.org/2002/07/owl#ObjectProperty> .
<http://vcharpenay.github.io/hto/hto.xml#measuredOn> <http://www.w3.org/2000/01/rdf-schema#domain> <http://vcharpenay.github.io/hto/hto.xml#Measurement> .
<http://vcharpenay.github.io/hto/hto.xml#measuredOn> <http://www.w3.org/2000/01/rdf-schema#range> <http://vcharpenay.github.io/hto/hto.xml#PhysicalBody> .
<http://vcharpenay.github.io/hto/hto.xml#quantifies> <http://www.w3.org/1999/02/22-rdf-syntax-ns#type> <http://www.w3.org/2002/07/owl#ObjectProperty> .
<http://vcharpenay.github.io/hto/hto.xml#quantifies> <http://www.w3.org/2000/01/rdf-schema#subPropertyOf> <http://purl.oclc.org/NET/ssnx/ssn#observes> .
<http://vcharpenay.github.io/hto/hto.xml#quantifies> <http://www.w3.org/2000/01/rdf-schema#range> <http://vcharpenay.github.io/hto/hto.xml#Measurement> .
<http://vcharpenay.github.io/hto/hto.xml#quantifies> <http://www.w3.org/2000/01/rdf-schema#domain> <http://vcharpenay.github.io/hto/hto.xml#Point> .
<http://vcharpenay.github.io/hto/hto.xml#dis> <http://www.w3.org/1999/02/22-rdf-syntax-ns#type> <http://www.w3.org/2002/07/owl#DatatypeProperty> .
<http://vcharpenay.github.io/hto/hto.xml#dis> <http://www.w3.org/2000/01/rdf-schema#domain> <http://vcharpenay.github.io/hto/hto.xml#HEntity> .
<http://vcharpenay.github.io/hto/hto.xml#AHU> <http://www.w3.org/1999/02/22-rdf-syntax-ns#type> <http://www.w3.org/2002/07/owl#Class> .
<http://vcharpenay.github.io/hto/hto.xml#AHU> <http://www.w3.org/2000/01/rdf-schema#label> "AHU" .
<http://vcharpenay.github.io/hto/hto.xml#AHU> <http://www.w3.org/2000/01/rdf-schema#subClassOf> <http://vcharpenay.github.io/hto/hto.xml#HVAC> .
<http://vcharpenay.github.io/hto/hto.xml#Air> <http://www.w3.org/1999/02/22-rdf-syntax-ns#type> <http://www.w3.org/2002/07/owl#Class> .
<http://vcharpenay.github.io/hto/hto.xml#Air> <http://www.w3.org/2000/01/rdf-schema#label> "Air" .
<http://vcharpenay.github.io/hto/hto.xml#Air> <http://www.w3.org/2000/01/rdf-schema#subClassOf> <http://vcharpenay.github.io/hto/hto.xml#PhysicalBody> .
<http://vcharpenay.github.io/hto/hto.xml#Boiler> <http://www.w3.org/1999/02/22-rdf-syntax-ns#type> <http://www.w3.org/2002/07/owl#Class> .
<http://vcharpenay.github.io/hto/hto.xml#Boiler> <http://www.w3.org/2000/01/rdf-schema#label> "Boiler" .
<http://vcharpenay.github.io/hto/hto.xml#Boiler> <http://www.w3.org/2000/01/rdf-schema#subClassOf> <http://vcharpenay.github.io/hto/hto.xml#HVAC> .
<http://vcharpenay.github.io/hto/hto.xml#CO2> <http://www.w3.org/1999/02/22-rdf-syntax-ns#type> <http://www.w3.org/2002/07/owl#Class> .
<http://vcharpenay.github.io/hto/hto.xml#CO2> <http://www.w3.org/2000/01/rdf-schema#label> "CO2" .
<http://vcharpenay.github.io/hto/hto.xml#CO2> <http://www.w3.org/2000/01/rdf-schema#subClassOf> <http://vcharpenay.github.io/hto/hto.xml#Measurement> .
<http://vcharpenay.github.io/hto/hto.xml#ChilledSystem> <http://www.w3.org/1999/02/22-rdf-syntax-ns#type> <http://www.w3.org/2002/07/owl#Class> .
<http://vcharpenay.github.io/hto/hto.xml#ChilledSystem> <http://www.w3.org/2000/01/rdf-schema#label> "Chilled System" .
<http://vcharpenay.github.io/hto/hto.xml#ChilledSystem> <http://www.w3.org/2000/01/rdf-schema#subClassOf> <http://vcharpenay.github.io/hto/hto.xml#Section> .
<http://vcharpenay.github.io/hto/hto.xml#Chiller> <http://www.w3.org/1999/02/22-rdf-syntax-ns#type> <http://www.w3.org/2002/07/owl#Class> .
<http://vcharpenay.github.io/hto/hto.xml#Chiller> <http://www.w3.org/2000/01/rdf-schema#label> "Chiller" .
<http://vcharpenay.github.io/hto/hto.xml#Chiller> <http://www.w3.org/2000/01/rdf-schema#subClassOf> <http://vcharpenay.github.io/hto/hto.xml#HVAC> .
<http://vcharpenay.github.io/hto/hto.xml#Command> <http://www.w3.org/1999/02/22-rdf-syntax-ns#type> <http://www.w3.org/2002/07/owl#Class> .
<http://vcharpenay.github.io/hto/hto.xml#Command> <http://www.w3.org/2000/01/rdf-schema#label> "Command" .
<http://vcharpenay.github.io/hto/hto.xml#Command> <http://www.w3.org/2000/01/rdf-schema#subClassOf> <http://vcharpenay.github.io/hto/hto.xml#Point> .
<http://vcharpenay.github.io/hto/hto.xml#CondenserSystem> <http://www.w3.org/1999/02/22-rdf-syntax-ns#type> <http://www.w3.org/2002/07/owl#Class> .
<http://vcharpenay.github.io/hto/hto.xml#CondenserSystem> <http://www.w3.org/2000/01/rdf-schema#label> "Condenser System" .
<http://vcharpenay.github.io/hto/hto.xml#CondenserSystem> <http://www.w3.org/2000/01/rdf-schema#subClassOf> <http://vcharpenay.github.io/hto/hto.xml#Section> .
<http://vcharpenay.github.io/hto/hto.xml#CoolingCoil> <http://www.w3.org/1999/02/22-rdf-syntax-ns#type> <http://www.w3.org/2002/07/owl#Class> .
<http://vcharpenay.github.io/hto/hto.xml#CoolingCoil> <http://www.w3.org/2000/01/rdf-schema#label> "Cooling Coil" .
<http://vcharpenay.github.io/hto/hto.xml#CoolingCoil> <http://www.w3.org/2000/01/rdf-schema#subClassOf> <http://vcharpenay.github.io/hto/hto.xml#Section> .
<http://vcharpenay.github.io/hto/hto.xml#Discharge> <http://www.w3.org/1999/02/22-rdf-syntax-ns#type> <http://www.w3.org/2002/07/owl#Class> .
<http://vcharpenay.github.io/hto/hto.xml#Discharge> <http://www.w3.org/2000/01/rdf-schema#label> "Discharge" .
<http://vcharpenay.github.io/hto/hto.xml#Discharge> <http://www.w3.org/2000/01/rdf-schema#subClassOf> <http://vcharpenay.github.io/hto/hto.xml#Section> .
<http://vcharpenay.github.io/hto/hto.xml#Efficiency> <http://www.w3.org/1999/02/22-rdf-syntax-ns#type> <http://www.w3.org/2002/07/owl#Class> .
<http://vcharpenay.github.io/hto/hto.xml#Efficiency> <http://www.w3.org/2000/01/rdf-schema#label> "Efficiency" .
<http://vcharpenay.github.io/hto/hto.xml#Efficiency> <http://www.w3.org/2000/01/rdf-schema#subClassOf> <http://vcharpenay.github.io/hto/hto.xml#Measurement> .
<http://vcharpenay.github.io/hto/hto.xml#Entering> <http://www.w3.org/1999/02/22-rdf-syntax-ns#type> <http://www.w3.org/2002/07/owl#Class> .
<http://vcharpenay.github.io/hto/hto.xml#Entering> <http://www.w3.org/2000/01/rdf-schema#label> "Entering" .
<http://vcharpenay.github.io/hto/hto.xml#Entering> <http://www.w3.org/2000/01/rdf-schema#subClassOf> <http://vcharpenay.github.io/hto/hto.xml#Section> .
<http://vcharpenay.github.io/hto/hto.xml#Equipment> <http://www.w3.org/1999/02/22-rdf-syntax-ns#type> <http://www.w3.org/2002/07/owl#Class> .
<http://vcharpenay.github.io/hto/hto.xml#Equipment> <http://www.w3.org/2000/01/rdf-schema#label> "Equipment" .
<http://vcharpenay.github.io/hto/hto.xml#Equipment> <http://www.w3.org/2000/01/rdf-schema#subClassOf> <http://purl.oclc.org/NET/ssnx/ssn#Platform> .
<http://vcharpenay.github.io/hto/hto.xml#Equipment> <http://www.w3.org/2000/01/rdf-schema#subClassOf> <http://vcharpenay.github.io/hto/hto.xml#HEntity> .
<http://vcharpenay.github.io/hto/hto.xml#Exhaust> <http://www.w3.org/1999/02/22-rdf-syntax-ns#type> <http://www.w3.org/2002/07/owl#Class> .
<http://vcharpenay.github.io/hto/hto.xml#Exhaust> <http://www.w3.org/2000/01/rdf-schema#label> "Exhaust" .
<http://vcharpenay.github.io/hto/hto.xml#Exhaust> <http://www.w3.org/2000/01/rdf-schema#subClassOf> <http://vcharpenay.github.io/hto/hto.xml#Section> .
<http://vcharpenay.github.io/hto/hto.xml#Fan> <http://www.w3.org/1999/02/22-rdf-syntax-ns#type> <http://www.w3.org/2002/07/owl#Class> .
<http://vcharpenay.github.io/hto/hto.xml#Fan> <http://www.w3.org/2000/01/rdf-schema#label> "Fan" .
<http://vcharpenay.github.io/hto/hto.xml#Fan> <http://www.w3.org/2000/01/rdf-schema#subClassOf> <http://vcharpenay.github.io/hto/hto.xml#Section> .
<http://vcharpenay.github.io/hto/hto.xml#Flow> <http://www.w3.org/1999/02/22-rdf-syntax-ns#type> <http://www.w3.org/2002/07/owl#Class> .
<http://vcharpenay.github.io/hto/hto.xml#Flow> <http://www.w3.org/2000/01/rdf-schema#label> "Flow" .
<http://vcharpenay.github.io/hto/hto.xml#Flow> <http://www.w3.org/2000/01/rdf-schema#subClassOf> <http://vcharpenay.github.io/hto/hto.xml#Measurement> .
<http://vcharpenay.github.io/hto/hto.xml#Frequency> <http://www.w3.org/1999/02/22-rdf-syntax-ns#type> <http://www.w3.org/2002/07/owl#Class> .
<http://vcharpenay.github.io/hto/hto.xml#Frequency> <http://www.w3.org/2000/01/rdf-schema#label> "Frequency" .
<http://vcharpenay.github.io/hto/hto.xml#Frequency> <http://www.w3.org/2000/01/rdf-schema#subClassOf> <http://vcharpenay.github.io/hto/hto.xml#Measurement> .
<http://vcharpenay.github.io/hto/hto.xml#Gas> <http://www.w3.org/1999/02/22-rdf-syntax-ns#type> <http://www.w3.org/2002/07/owl#Class> .
<http://vcharpenay.github.io/hto/hto.xml#Gas> <http://www.w3.org/2000/01/rdf-schema#label> "Gas" .
<http://vcharpenay.github.io/hto/hto.xml#Gas> <http://www.w3.org/2000/01/rdf-schema#subClassOf> <http://vcharpenay.github.io/hto/hto.xml#PhysicalBody> .
<http://vcharpenay.github.io/hto/hto.xml#HEntity> <http://www.w3.org/1999/02/22-rdf-syntax-ns#type> <http://www.w3.org/2002/07/owl#Class> .
<http://vcharpenay.github.io/hto/hto.xml#HEntity> <http://www.w3.org/2000/01/rdf-schema#label> "HEntity" .
<http://vcharpenay.github.io/hto/hto.xml#HTag> <http://www.w3.org/1999/02/22-rdf-syntax-ns#type> <http://www.w3.org/2002/07/owl#Class> .
<http://vcharpenay.github.io/hto/hto.xml#HTag> <http://www.w3.org/2000/01/rdf-schema#label> "HTag" .
<http://vcharpenay.github.io/hto/hto.xml#HVAC> <http://www.w3.org/1999/02/22-rdf-syntax-ns#type> <http://www.w3.org/2002/07/owl#Class> .
<http://vcharpenay.github.io/hto/hto.xml#HVAC> <http://www.w3.org/2000/01/rdf-schema#label> "HVAC" .
<http://vcharpenay.github.io/hto/hto.xml#HVAC> <http://www.w3.org/2000/01/rdf-schema#subClassOf> <http://vcharpenay.github.io/hto/hto.xml#Equipment> .
<http://vcharpenay.github.io/hto/hto.xml#HeatingCoil> <http://www.w3.org/1999/02/22-rdf-syntax-ns#type> <http://www.w3.org/2002/07/owl#Class> .
<http://vcharpenay.github.io/hto/hto.xml#HeatingCoil> <http://www.w3.org/2000/01/rdf-schema#label> "Heating Coil" .
<http://vcharpenay.github.io/hto/hto.xml#HeatingCoil> <http://www.w3.org/2000/01/rdf-schema#subClassOf> <http://vcharpenay.github.io/hto/hto.xml#Section> .
<http://vcharpenay.github.io/hto/hto.xml#Historized> <http://www.w3.org/1999/02/22-rdf-syntax-ns#type> <http://www.w3.org/2002/07/owl#Class> .
<http://vcharpenay.github.io/hto/hto.xml#Historized> <http://www.w3.org/2000/01/rdf-schema#label> "Historized" .
<http://vcharpenay.github.io/hto/hto.xml#Historized> <http://www.w3.org/2000/01/rdf-schema#subClassOf> <http://vcharpenay.github.io/hto/hto.xml#PointProperty> .
<http://vcharpenay.github.io/hto/hto.xml#Humidity> <http://www.w3.org/1999/02/22-rdf-syntax-ns#type> <http://www.w3.org/2002/07/owl#Class> .
<http://vcharpenay.github.io/hto/hto.xml#Humidity> <http://www.w3.org/2000/01/rdf-schema#label> "Humidity" .
<http://vcharpenay.github.io/hto/hto.xml#Humidity> <http://www.w3.org/2000/01/rdf-schema#subClassOf> <http://vcharpenay.github.io/hto/hto.xml#Measurement> .
<http://vcharpenay.github.io/hto/hto.xml#IsolationValve> <http://www.w3.org/1999/02/22-rdf-syntax-ns#type> <http://www.w3.org/2002/07/owl#Class> .
<http://vcharpenay.github.io/hto/hto.xml#IsolationValve> <http://www.w3.org/2000/01/rdf-schema#label> "Isolation Valve" .
<http://vcharpenay.github.io/hto/hto.xml#IsolationValve> <http://www.w3.org/2000/01/rdf-schema#subClassOf> <http://vcharpenay.github.io/hto/hto.xml#Valve> .
<http://vcharpenay.github.io/hto/hto.xml#Leaving> <http://www.w3.org/1999/02/22-rdf-syntax-ns#type> <http://www.w3.org/2002/07/owl#Class> .
<http://vcharpenay.github.io/hto/hto.xml#Leaving> <http://www.w3.org/2000/01/rdf-schema#label> "Leaving" .
<http://vcharpenay.github.io/hto/hto.xml#Leaving> <http://www.w3.org/2000/01/rdf-schema#subClassOf> <http://vcharpenay.github.io/hto/hto.xml#Section> .
<http://vcharpenay.github.io/hto/hto.xml#LightLevel> <http://www.w3.org/1999/02/22-rdf-syntax-ns#type> <http://www.w3.org/2002/07/owl#Class> .
<http://vcharpenay.github.io/hto/hto.xml#LightLevel> <http://www.w3.org/2000/01/rdf-schema#label> "Light Level" .
<http://vcharpenay.github.io/hto/hto.xml#LightLevel> <http://www.w3.org/2000/01/rdf-schema#subClassOf> <http://vcharpenay.github.io/hto/hto.xml#Measurement> .
<http://vcharpenay.github.io/hto/hto.xml#LightsGroup> <http://www.w3.org/1999/02/22-rdf-syntax-ns#type> <http://www.w3.org/2002/07/owl#Class> .
<http://vcharpenay.github.io/hto/hto.xml#LightsGroup> <http://www.w3.org/2000/01/rdf-schema#label> "Lights Group" .
<http://vcharpenay.github.io/hto/hto.xml#LightsGroup> <http://www.w3.org/2000/01/rdf-schema#subClassOf> <http://vcharpenay.github.io/hto/hto.xml#Equipment> .
<http://vcharpenay.github.io/hto/hto.xml#Measurement> <http://www.w3.org/1999/02/22-rdf-syntax-ns#type> <http://www.w3.org/2002/07/owl#Class> .
<http://vcharpenay.github.io/hto/hto.xml#Measurement> <http://www.w3.org/2000/01/rdf-schema#label> "Measurement" .
<http://vcharpenay.github.io/hto/hto.xml#Meter> <http://www.w3.org/1999/02/22-rdf-syntax-ns#type> <http://www.w3.org/2002/07/owl#Class> .
<http://vcharpenay.github.io/hto/hto.xml#Meter> <http://www.w3.org/2000/01/rdf-schema#label> "Meter" .
<http://vcharpenay.github.io/hto/hto.xml#Meter> <http://www.w3.org/2000/01/rdf-schema#subClassOf> <http://vcharpenay.github.io/hto/hto.xml#Equipment> .
<http://vcharpenay.github.io/hto/hto.xml#Mixed> <http://www.w3.org/1999/02/22-rdf-syntax-ns#type> <http://www.w3.org/2002/07/owl#Class> .
<http://vcharpenay.github.io/hto/hto.xml#Mixed> <http://www.w3.org/2000/01/rdf-schema#label> "Mixed" .
<http://vcharpenay.github.io/hto/hto.xml#Mixed> <http://www.w3.org/2000/01/rdf-schema#subClassOf> <http://vcharpenay.github.io/hto/hto.xml#Section> .
<http://vcharpenay.github.io/hto/hto.xml#OnOff> <http://www.w3.org/1999/02/22-rdf-syntax-ns#type> <http://www.w3.org/2002/07/owl#Class> .
<http://vcharpenay.github.io/hto/hto.xml#OnOff> <http://www.w3.org/2000/01/rdf-schema#label> "On/Off" .
<http://vcharpenay.github.io/hto/hto.xml#OnOff> <http://www.w3.org/2000/01/rdf-schema#subClassOf> <http://vcharpenay.github.io/hto/hto.xml#Measurement> .
<http://vcharpenay.github.io/hto/hto.xml#Percentage> <http://www.w3.org/1999/02/22-rdf-syntax-ns#type> <http://www.w3.org/2002/07/owl#Class> .
<http://vcharpenay.github.io/hto/hto.xml#Percentage> <http://www.w3.org/2000/01/rdf-schema#label> "Percentage" .
<http://vcharpenay.github.io/hto/hto.xml#Percentage> <http://www.w3.org/2000/01/rdf-schema#subClassOf> <http://vcharpenay.github.io/hto/hto.xml#Measurement> .
<http://vcharpenay.github.io/hto/hto.xml#PerimeterHeat> <http://www.w3.org/1999/02/22-rdf-syntax-ns#type> <http://www.w3.org/2002/07/owl#Class> .
<http://vcharpenay.github.io/hto/hto.xml#PerimeterHeat> <http://www.w3.org/2000/01/rdf-schema#label> "Perimeter Heat" .
<http://vcharpenay.github.io/hto/hto.xml#PerimeterHeat> <http://www.w3.org/2000/01/rdf-schema#subClassOf> <http://vcharpenay.github.io/hto/hto.xml#Section> .
<http://vcharpenay.github.io/hto/hto.xml#PhysicalBody> <http://www.w3.org/1999/02/22-rdf-syntax-ns#type> <http://www.w3.org/2002/07/owl#Class> .
<http://vcharpenay.github.io/hto/hto.xml#PhysicalBody> <http://www.w3.org/2000/01/rdf-schema#label> "Physical Body" .
<http://vcharpenay.github.io/hto/hto.xml#Point> <http://www.w3.org/1999/02/22-rdf-syntax-ns#type> <http://www.w3.org/2002/07/owl#Class> .
<http://vcharpenay.github.io/hto/hto.xml#Point> <http://www.w3.org/2000/01/rdf-schema#label> "Point" .
<http://vcharpenay.github.io/hto/hto.xml#Point> <http://www.w3.org/2000/01/rdf-schema#subClassOf> <http://vcharpenay.github.io/hto/hto.xml#HEntity> .
<http://vcharpenay.github.io/hto/hto.xml#PointProperty> <http://www.w3.org/1999/02/22-rdf-syntax-ns#type> <http://www.w3.org/2002/07/owl#Class> .
<http://vcharpenay.github.io/hto/hto.xml#PointProperty> <http://www.w3.org/2000/01/rdf-schema#label> "Point Property" .
<http://vcharpenay.github.io/hto/hto.xml#Power> <http://www.w3.org/1999/02/22-rdf-syntax-ns#type> <http://www.w3.org/2002/07/owl#Class> .
<http://vcharpenay.github.io/hto/hto.xml#Power> <http://www.w3.org/2000/01/rdf-schema#label> "Power" .
<http://vcharpenay.github.io/hto/hto.xml#Power> <http://www.w3.org/2000/01/rdf-schema#subClassOf> <http://vcharpenay.github.io/hto/hto.xml#Measurement> .
<http://vcharpenay.github.io/hto/hto.xml#Pressure> <http://www.w3.org/1999/02/22-rdf-syntax-ns#type> <http://www.w3.org/2002/07/owl#Class> .
<http://vcharpenay.github.io/hto/hto.xml#Pressure> <http://www.w3.org/2000/01/rdf-schema#label> "Pressure" .
<http://vcharpenay.github.io/hto/hto.xml#Pressure> <http://www.w3.org/2000/01/rdf-schema#subClassOf> <http://vcharpenay.github.io/hto/hto.xml#Measurement> .
<http://vcharpenay.github.io/hto/hto.xml#Pump> <http://www.w3.org/1999/02/22-rdf-syntax-ns#type> <http://www.w3.org/2002/07/owl#Class> .
<http://vcharpenay.github.io/hto/hto.xml#Pump> <http://www.w3.org/2000/01/rdf-schema#label> "Pump" .
<http://vcharpenay.github.io/hto/hto.xml#Pump> <http://www.w3.org/2000/01/rdf-schema#subClassOf> <http://vcharpenay.github.io/hto/hto.xml#VFD> .
<http://vcharpenay.github.io/hto/hto.xml#RTU> <http://www.w3.org/1999/02/22-rdf-syntax-ns#type> <http://www.w3.org/2002/07/owl#Class> .
<http://vcharpenay.github.io/hto/hto.xml#RTU> <http://www.w3.org/2000/01/rdf-schema#label> "RTU" .
<http://vcharpenay.github.io/hto/hto.xml#RTU> <http://www.w3.org/2000/01/rdf-schema#subClassOf> <http://vcharpenay.github.io/hto/hto.xml#AHU> .
<http://vcharpenay.github.io/hto/hto.xml#RealTime> <http://www.w3.org/1999/02/22-rdf-syntax-ns#type> <http://www.w3.org/2002/07/owl#Class> .
<http://vcharpenay.github.io/hto/hto.xml#RealTime> <http://www.w3.org/2000/01/rdf-schema#label> "Real time" .
<http://vcharpenay.github.io/hto/hto.xml#RealTime> <http://www.w3.org/2000/01/rdf-schema#subClassOf> <http://vcharpenay.github.io/hto/hto.xml#PointProperty> .
<http://vcharpenay.github.io/hto/hto.xml#RefrigerantSubstance> <http://www.w3.org/1999/02/22-rdf-syntax-ns#type> <http://www.w3.org/2002/07/owl#Class> .
<http://vcharpenay.github.io/hto/hto.xml#RefrigerantSubstance> <http://www.w3.org/2000/01/rdf-schema#label> "Refrigirant Substance" .
<http://vcharpenay.github.io/hto/hto.xml#RefrigerantSubstance> <http://www.w3.org/2000/01/rdf-schema#subClassOf> <http://vcharpenay.github.io/hto/hto.xml#PhysicalBody> .
<http://vcharpenay.github.io/hto/hto.xml#Return> <http://www.w3.org/1999/02/22-rdf-syntax-ns#type> <http://www.w3.org/2002/07/owl#Class> .
<http://vcharpenay.github.io/hto/hto.xml#Return> <http://www.w3.org/2000/01/rdf-schema#label> "Return" .
<http://vcharpenay.github.io/hto/hto.xml#Return> <http://www.w3.org/2000/01/rdf-schema#subClassOf> <http://vcharpenay.github.io/hto/hto.xml#Section> .
<http://vcharpenay.github.io/hto/hto.xml#Section> <http://www.w3.org/1999/02/22-rdf-syntax-ns#type> <http://www.w3.org/2002/07/owl#Class> .
<http://vcharpenay.github.io/hto/hto.xml#Section> <http://www.w3.org/2000/01/rdf-schema#label> "Section" .
<http://vcharpenay.github.io/hto/hto.xml#Section> <http://www.w3.org/2000/01/rdf-schema#subClassOf> <http://purl.oclc.org/NET/ssnx/ssn#FeatureOfInterest> .
<http://vcharpenay.github.io/hto/hto.xml#Sensor> <http://www.w3.org/1999/02/22-rdf-syntax-ns#type> <http://www.w3.org/2002/07/owl#Class> .
<http://vcharpenay.github.io/hto/hto.xml#Sensor> <http://www.w3.org/2000/01/rdf-schema#label> "Sensor" .
<http://vcharpenay.github.io/hto/hto.xml#Sensor> <http://www.w3.org/2000/01/rdf-schema#subClassOf> <http://purl.oclc.org/NET/ssnx/ssn#SensingDevice> .
<http://vcharpenay.github.io/hto/hto.xml#Sensor> <http://www.w3.org/2000/01/rdf-schema#subClassOf> <http://vcharpenay.github.io/hto/hto.xml#Point> .
<http://vcharpenay.github.io/hto/hto.xml#Sensor> <http://vcharpenay.github.io/hto/hto.xml#associatedTo> <http://vcharpenay.github.io/hto/hto.xml#sensor> .
<http://vcharpenay.github.io/hto/hto.xml#SetPoint> <http://www.w3.org/1999/02/22-rdf-syntax-ns#type> <http://www.w3.org/2002/07/owl#Class> .
<http://vcharpenay.github.io/hto/hto.xml#SetPoint> <http://www.w3.org/2000/01/rdf-schema#label> "Set Point" .
<http://vcharpenay.github.io/hto/hto.xml#SetPoint> <http://www.w3.org/2000/01/rdf-schema#subClassOf> <http://vcharpenay.github.io/hto/hto.xml#Point> .
<http://vcharpenay.github.io/hto/hto.xml#Site> <http://www.w3.org/1999/02/22-rdf-syntax-ns#type> <http://www.w3.org/2002/07/owl#Class> .
<http://vcharpenay.github.io/hto/hto.xml#Site> <http://www.w3.org/2000/01/rdf-schema#label> "Site" .
<http://vcharpenay.github.io/hto/hto.xml#Site> <http://www.w3.org/2000/01/rdf-schema#subClassOf> <http://vcharpenay.github.io/hto/hto.xml#HEntity> .
<http://vcharpenay.github.io/hto/hto.xml#Speed> <http://www.w3.org/1999/02/22-rdf-syntax-ns#type> <http://www.w3.org/2002/07/owl#Class> .
<http://vcharpenay.github.io/hto/hto.xml#Speed> <http://www.w3.org/2000/01/rdf-schema#label> "Speed" .
<http://vcharpenay.github.io/hto/hto.xml#Speed> <http://www.w3.org/2000/01/rdf-schema#subClassOf> <http://vcharpenay.github.io/hto/hto.xml#Measurement> .
<http://vcharpenay.github.io/hto/hto.xml#Steam> <http://www.w3.org/1999/02/22-rdf-syntax-ns#type> <http://www.w3.org/2002/07/owl#Class> .
<http://vcharpenay.github.io/hto/hto.xml#Steam> <http://www.w3.org/2000/01/rdf-schema#label> "Steam" .
<http://vcharpenay.github.io/hto/hto.xml#Steam> <http://www.w3.org/2000/01/rdf-schema#subClassOf> <http://vcharpenay.github.io/hto/hto.xml#PhysicalBody> .
<http://vcharpenay.github.io/hto/hto.xml#Temperature> <http://www.w3.org/1999/02/22-rdf-syntax-ns#type> <http://www.w3.org/2002/07/owl#Class> .
<http://vcharpenay.github.io/hto/hto.xml#Temperature> <http://www.w3.org/2000/01/rdf-schema#label> "Temperature" .
<http://vcharpenay.github.io/hto/hto.xml#Temperature> <http://www.w3.org/2000/01/rdf-schema#subClassOf> <http://vcharpenay.github.io/hto/hto.xml#Measurement> .
<http://vcharpenay.github.io/hto/hto.xml#VAV> <http://www.w3.org/1999/02/22-rdf-syntax-ns#type> <http://www.w3.org/2002/07/owl#Class> .
<http://vcharpenay.github.io/hto/hto.xml#VAV> <http://www.w3.org/2000/01/rdf-schema#label> "VAV" .
<http://vcharpenay.github.io/hto/hto.xml#VAV> <http://www.w3.org/2000/01/rdf-schema#subClassOf> <http://vcharpenay.github.io/hto/hto.xml#HVAC> .
<http://vcharpenay.github.io/hto/hto.xml#VFD> <http://www.w3.org/1999/02/22-rdf-syntax-ns#type> <http://www.w3.org/2002/07/owl#Class> .
<http://vcharpenay.github.io/hto/hto.xml#VFD> <http://www.w3.org/2000/01/rdf-schema#label> "VFD" .
<http://vcharpenay.github.io/hto/hto.xml#VFD> <http://www.w3.org/2000/01/rdf-schema#subClassOf> <http://vcharpenay.github.io/hto/hto.xml#Equipment> .
<http://vcharpenay.github.io/hto/hto.xml#VFDFan> <http://www.w3.org/1999/02/22-rdf-syntax-ns#type> <http://www.w3.org/2002/07/owl#Class> .
<http://vcharpenay.github.io/hto/hto.xml#VFDFan> <http://www.w3.org/2000/01/rdf-schema#label> "VFD Fan" .
<http://vcharpenay.github.io/hto/hto.xml#VFDFan> <http://www.w3.org/2000/01/rdf-schema#subClassOf> <http://vcharpenay.github.io/hto/hto.xml#VFD> .
<http://vcharpenay.github.io/hto/hto.xml#Valve> <http://www.w3.org/1999/02/22-rdf-syntax-ns#type> <http://www.w3.org/2002/07/owl#Class> .
<http://vcharpenay.github.io/hto/hto.xml#Valve> <http://www.w3.org/2000/01/rdf-schema#label> "Valve" .
<http://vcharpenay.github.io/hto/hto.xml#Valve> <http://www.w3.org/2000/01/rdf-schema#subClassOf> <http://vcharpenay.github.io/hto/hto.xml#Section> .
<http://vcharpenay.github.io/hto/hto.xml#Water> <http://www.w3.org/1999/02/22-rdf-syntax-ns#type> <http://www.w3.org/2002/07/owl#Class> .
<http://vcharpenay.github.io/hto/hto.xml#Water> <http://www.w3.org/2000/01/rdf-schema#label> "Water" .
<http://vcharpenay.github.io/hto/hto.xml#Water> <http://www.w3.org/2000/01/rdf-schema#subClassOf> <http://vcharpenay.github.io/hto/hto.xml#PhysicalBody> .
<http://vcharpenay.github.io/hto/hto.xml#Writable> <http://www.w3.org/1999/02/22-rdf-syntax-ns#type> <http://www.w3.org/2002/07/owl#Class> .
<http://vcharpenay.github.io/hto/hto.xml#Writable> <http://www.w3.org/2000/01/rdf-schema#label> "Writable" .
<http://vcharpenay.github.io/hto/hto.xml#Writable> <http://www.w3.org/2000/01/rdf-schema#subClassOf> <http://vcharpenay.github.io/hto/hto.xml#PointProperty> .
<http://vcharpenay.github.io/hto/hto.xml#Zone> <http://www.w3.org/1999/02/22-rdf-syntax-ns#type> <http://www.w3.org/2002/07/owl#Class> .
<http://vcharpenay.github.io/hto/hto.xml#Zone> <http://www.w3.org/2000/01/rdf-schema#label> "Zone" .
<http://vcharpenay.github.io/hto/hto.xml#Zone> <http://www.w3.org/2000/01/rdf-schema#subClassOf> <http://vcharpenay.github.io/hto/hto.xml#Section> .
<http://vcharpenay.github.io/hto/hto.xml#ahu> <http://www.w3.org/1999/02/22-rdf-syntax-ns#type> <http://www.w3.org/2002/07/owl#NamedIndividual> .
<http://vcharpenay.github.io/hto/hto.xml#ahu> <http://www.w3.org/1999/02/22-rdf-syntax-ns#type> <http://vcharpenay.github.io/hto/hto.xml#HTag> .
<http://vcharpenay.github.io/hto/hto.xml#ahu> <http://www.w3.org/2000/01/rdf-schema#comment> "  Air Handler Unit which heats and/or cools air."^^<http://www.w3.org/2001/XMLSchema#string> .
<http://vcharpenay.github.io/hto/hto.xml#ahu> <http://vcharpenay.github.io/hto/hto.xml#associatedTo> <http://vcharpenay.github.io/hto/hto.xml#AHU> .
<http://vcharpenay.github.io/hto/hto.xml#air> <http://www.w3.org/1999/02/22-rdf-syntax-ns#type> <http://www.w3.org/2002/07/owl#NamedIndividual> .
<http://vcharpenay.github.io/hto/hto.xml#air> <http://www.w3.org/1999/02/22-rdf-syntax-ns#type> <http://vcharpenay.github.io/hto/hto.xml#HTag> .
<http://vcharpenay.github.io/hto/hto.xml#air> <http://www.w3.org/2000/01/rdf-schema#comment> "  Point associated with the measurement or control of air. In regards to `wetBulb`, points with the 'air' tag are associated with dry bulb."^^<http://www.w3.org/2001/XMLSchema#string> .
<http://vcharpenay.github.io/hto/hto.xml#air> <http://vcharpenay.github.io/hto/hto.xml#associatedTo> <http://vcharpenay.github.io/hto/hto.xml#Air> .
<http://vcharpenay.github.io/hto/hto.xml#boiler> <http://www.w3.org/1999/02/22-rdf-syntax-ns#type> <http://www.w3.org/2002/07/owl#NamedIndividual> .
<http://vcharpenay.github.io/hto/hto.xml#boiler> <http://www.w3.org/1999/02/22-rdf-syntax-ns#type> <http://vcharpenay.github.io/hto/hto.xml#HTag> .
<http://vcharpenay.github.io/hto/hto.xml#boiler> <http://www.w3.org/2000/01/rdf-schema#comment> "  Boiler `equip` used to generate hot water or steam for heating."^^<http://www.w3.org/2001/XMLSchema#string> .
<http://vcharpenay.github.io/hto/hto.xml#boiler> <http://www.w3.org/2000/01/rdf-schema#comment> "note: does not fully implement specification (no boilerPlant). However, is still a TODO in project Haystack." .
<http://vcharpenay.github.io/hto/hto.xml#boiler> <http://vcharpenay.github.io/hto/hto.xml#associatedTo> <http://vcharpenay.github.io/hto/hto.xml#Boiler> .
<http://vcharpenay.github.io/hto/hto.xml#bypass> <http://www.w3.org/1999/02/22-rdf-syntax-ns#type> <http://www.w3.org/2002/07/owl#NamedIndividual> .
<http://vcharpenay.github.io/hto/hto.xml#bypass> <http://www.w3.org/1999/02/22-rdf-syntax-ns#type> <http://vcharpenay.github.io/hto/hto.xml#HTag> .
<http://vcharpenay.github.io/hto/hto.xml#bypass> <http://www.w3.org/2000/01/rdf-schema#comment> "  If used with `valve` indicates a by-pass in a piping system. If used in combination with the `damper` tag on an `ahu` to indicate a damper in the ductwork to by-pass the VAV boxs and create a direct circuit between the discharge and return of the unit."^^<http://www.w3.org/2001/XMLSchema#string> .
<http://vcharpenay.github.io/hto/hto.xml#chilled> <http://www.w3.org/1999/02/22-rdf-syntax-ns#type> <http://www.w3.org/2002/07/owl#NamedIndividual> .
<http://vcharpenay.github.io/hto/hto.xml#chilled> <http://www.w3.org/1999/02/22-rdf-syntax-ns#type> <http://vcharpenay.github.io/hto/hto.xml#HTag> .
<http://vcharpenay.github.io/hto/hto.xml#chilled> <http://www.w3.org/2000/01/rdf-schema#comment> "  Marker tag used with `water` for the chilled water system between `chiller` and `ahu`."^^<http://www.w3.org/2001/XMLSchema#string> .
<http://vcharpenay.github.io/hto/hto.xml#chilled> <http://vcharpenay.github.io/hto/hto.xml#associatedTo> <http://vcharpenay.github.io/hto/hto.xml#ChilledSystem> .
<http://vcharpenay.github.io/hto/hto.xml#chiller> <http://www.w3.org/1999/02/22-rdf-syntax-ns#type> <http://www.w3.org/2002/07/owl#NamedIndividual> .
<http://vcharpenay.github.io/hto/hto.xml#chiller> <http://www.w3.org/1999/02/22-rdf-syntax-ns#type> <http://vcharpenay.github.io/hto/hto.xml#HTag> .
<http://vcharpenay.github.io/hto/hto.xml#chiller> <http://www.w3.org/2000/01/rdf-schema#comment> "  Chillers remove heat from a liquid via a vapor compression or an absorption refrigeration cycle."^^<http://www.w3.org/2001/XMLSchema#string> .
<http://vcharpenay.github.io/hto/hto.xml#chiller> <http://www.w3.org/2000/01/rdf-schema#comment> "note: does not fully implement specification (no chillerPlant, no CoolingTower)." .
<http://vcharpenay.github.io/hto/hto.xml#chiller> <http://vcharpenay.github.io/hto/hto.xml#associatedTo> <http://vcharpenay.github.io/hto/hto.xml#Chiller> .
<http://vcharpenay.github.io/hto/hto.xml#cmd> <http://www.w3.org/1999/02/22-rdf-syntax-ns#type> <http://www.w3.org/2002/07/owl#NamedIndividual> .
<http://vcharpenay.github.io/hto/hto.xml#cmd> <http://www.w3.org/1999/02/22-rdf-syntax-ns#type> <http://vcharpenay.github.io/hto/hto.xml#HTag> .
<http://vcharpenay.github.io/hto/hto.xml#cmd> <http://www.w3.org/2000/01/rdf-schema#comment> "  Classifies a `point` as an output, AO/BO, command, or actuator."^^<http://www.w3.org/2001/XMLSchema#string> .
<http://vcharpenay.github.io/hto/hto.xml#cmd> <http://vcharpenay.github.io/hto/hto.xml#associatedTo> <http://vcharpenay.github.io/hto/hto.xml#Command> .
<http://vcharpenay.github.io/hto/hto.xml#co2> <http://www.w3.org/1999/02/22-rdf-syntax-ns#type> <http://www.w3.org/2002/07/owl#NamedIndividual> .
<http://vcharpenay.github.io/hto/hto.xml#co2> <http://www.w3.org/1999/02/22-rdf-syntax-ns#type> <http://vcharpenay.github.io/hto/hto.xml#HTag> .
<http://vcharpenay.github.io/hto/hto.xml#co2> <http://www.w3.org/2000/01/rdf-schema#comment> "  Carbon dioxide level `point` measured in \"ppm\"."^^<http://www.w3.org/2001/XMLSchema#string> .
<http://vcharpenay.github.io/hto/hto.xml#co2> <http://vcharpenay.github.io/hto/hto.xml#associatedTo> <http://vcharpenay.github.io/hto/hto.xml#CO2> .
<http://vcharpenay.github.io/hto/hto.xml#condenser> <http://www.w3.org/1999/02/22-rdf-syntax-ns#type> <http://www.w3.org/2002/07/owl#NamedIndividual> .
<http://vcharpenay.github.io/hto/hto.xml#condenser> <http://www.w3.org/1999/02/22-rdf-syntax-ns#type> <http://vcharpenay.github.io/hto/hto.xml#HTag> .
<http://vcharpenay.github.io/hto/hto.xml#condenser> <http://www.w3.org/2000/01/rdf-schema#comment> "  When combined with the `water` tag, this indicates points in a condenser water system between a `chiller` and `coolingTower`. When used with the `refrig` tag, this indicates points on the condenser mechanism used to convert a refrigerant from its gaseous to liquid state. If paired with the `cmd` tag this tag indicates the command status of a condensor in a `chiller` modeled as true/false (on/off) or 0% to 100%."^^<http://www.w3.org/2001/XMLSchema#string> .
<http://vcharpenay.github.io/hto/hto.xml#condenser> <http://vcharpenay.github.io/hto/hto.xml#associatedTo> <http://vcharpenay.github.io/hto/hto.xml#CondenserSystem> .
<http://vcharpenay.github.io/hto/hto.xml#cool> <http://www.w3.org/1999/02/22-rdf-syntax-ns#type> <http://www.w3.org/2002/07/owl#NamedIndividual> .
<http://vcharpenay.github.io/hto/hto.xml#cool> <http://www.w3.org/1999/02/22-rdf-syntax-ns#type> <http://vcharpenay.github.io/hto/hto.xml#HTag> .
<http://vcharpenay.github.io/hto/hto.xml#cool> <http://www.w3.org/2000/01/rdf-schema#comment> "  Cooling coil as bool or numeric `point` used with `ahu` equip.  If multiple stages are used, then also specify the `stage` tag. If the cooling coil is controlled by a valve, then this point is mesaured from 0% to 100%, otherwise it should be a boolean point."^^<http://www.w3.org/2001/XMLSchema#string> .
<http://vcharpenay.github.io/hto/hto.xml#cool> <http://vcharpenay.github.io/hto/hto.xml#associatedTo> <http://vcharpenay.github.io/hto/hto.xml#CoolingCoil> .
<http://vcharpenay.github.io/hto/hto.xml#cooling> <http://www.w3.org/1999/02/22-rdf-syntax-ns#type> <http://www.w3.org/2002/07/owl#NamedIndividual> .
<http://vcharpenay.github.io/hto/hto.xml#cooling> <http://www.w3.org/1999/02/22-rdf-syntax-ns#type> <http://vcharpenay.github.io/hto/hto.xml#HTag> .
<http://vcharpenay.github.io/hto/hto.xml#cooling> <http://www.w3.org/2000/01/rdf-schema#comment> "  Associated with the cooling mode of an HVAC system."^^<http://www.w3.org/2001/XMLSchema#string> .
<http://vcharpenay.github.io/hto/hto.xml#damper> <http://www.w3.org/1999/02/22-rdf-syntax-ns#type> <http://www.w3.org/2002/07/owl#NamedIndividual> .
<http://vcharpenay.github.io/hto/hto.xml#damper> <http://www.w3.org/1999/02/22-rdf-syntax-ns#type> <http://vcharpenay.github.io/hto/hto.xml#HTag> .
<http://vcharpenay.github.io/hto/hto.xml#damper> <http://www.w3.org/2000/01/rdf-schema#comment> "  Damper position measured from 0% (fully closed) to 100% (fully open)."^^<http://www.w3.org/2001/XMLSchema#string> .
<http://vcharpenay.github.io/hto/hto.xml#damper> <http://www.w3.org/2000/01/rdf-schema#comment> "note: indicates the measurement of how open the damper of a AHU is (0-100%)" .
<http://vcharpenay.github.io/hto/hto.xml#damper> <http://vcharpenay.github.io/hto/hto.xml#associatedTo> <http://vcharpenay.github.io/hto/hto.xml#Percentage> .
<http://vcharpenay.github.io/hto/hto.xml#delta> <http://www.w3.org/1999/02/22-rdf-syntax-ns#type> <http://www.w3.org/2002/07/owl#NamedIndividual> .
<http://vcharpenay.github.io/hto/hto.xml#delta> <http://www.w3.org/1999/02/22-rdf-syntax-ns#type> <http://vcharpenay.github.io/hto/hto.xml#HTag> .
<http://vcharpenay.github.io/hto/hto.xml#delta> <http://www.w3.org/2000/01/rdf-schema#comment> "  Indicates a differential of `air`, `water`, or `steam` between the `entering` and `leaving` sensors."^^<http://www.w3.org/2001/XMLSchema#string> .
<http://vcharpenay.github.io/hto/hto.xml#discharge> <http://www.w3.org/1999/02/22-rdf-syntax-ns#type> <http://www.w3.org/2002/07/owl#NamedIndividual> .
<http://vcharpenay.github.io/hto/hto.xml#discharge> <http://www.w3.org/1999/02/22-rdf-syntax-ns#type> <http://vcharpenay.github.io/hto/hto.xml#HTag> .
<http://vcharpenay.github.io/hto/hto.xml#discharge> <http://www.w3.org/2000/01/rdf-schema#comment> "  Associated with the discharge air an `ahu` or `vav`."^^<http://www.w3.org/2001/XMLSchema#string> .
<http://vcharpenay.github.io/hto/hto.xml#discharge> <http://vcharpenay.github.io/hto/hto.xml#associatedTo> <http://vcharpenay.github.io/hto/hto.xml#Discharge> .
<http://vcharpenay.github.io/hto/hto.xml#effective> <http://www.w3.org/1999/02/22-rdf-syntax-ns#type> <http://www.w3.org/2002/07/owl#NamedIndividual> .
<http://vcharpenay.github.io/hto/hto.xml#effective> <http://www.w3.org/1999/02/22-rdf-syntax-ns#type> <http://vcharpenay.github.io/hto/hto.xml#HTag> .
<http://vcharpenay.github.io/hto/hto.xml#effective> <http://www.w3.org/2000/01/rdf-schema#comment> "  Used to indicate the effective setpoint which takes into account various other mode based setpoints the equip might define.  See [zone setpoints]`Zones#zonePoints` for complete example of how this tag is used."^^<http://www.w3.org/2001/XMLSchema#string> .
<http://vcharpenay.github.io/hto/hto.xml#efficiency> <http://www.w3.org/1999/02/22-rdf-syntax-ns#type> <http://www.w3.org/2002/07/owl#NamedIndividual> .
<http://vcharpenay.github.io/hto/hto.xml#efficiency> <http://www.w3.org/1999/02/22-rdf-syntax-ns#type> <http://vcharpenay.github.io/hto/hto.xml#HTag> .
<http://vcharpenay.github.io/hto/hto.xml#efficiency> <http://www.w3.org/2000/01/rdf-schema#comment> "  Efficiency point of a `chiller` measured in \"COP\" or \"kW/ton\"."^^<http://www.w3.org/2001/XMLSchema#string> .
<http://vcharpenay.github.io/hto/hto.xml#efficiency> <http://vcharpenay.github.io/hto/hto.xml#associatedTo> <http://vcharpenay.github.io/hto/hto.xml#Efficiency> .
<http://vcharpenay.github.io/hto/hto.xml#elec> <http://www.w3.org/1999/02/22-rdf-syntax-ns#type> <http://www.w3.org/2002/07/owl#NamedIndividual> .
<http://vcharpenay.github.io/hto/hto.xml#elec> <http://www.w3.org/1999/02/22-rdf-syntax-ns#type> <http://vcharpenay.github.io/hto/hto.xml#HTag> .
<http://vcharpenay.github.io/hto/hto.xml#elec> <http://www.w3.org/2000/01/rdf-schema#comment> "  Used on `point` or `equip` entities relating to electricity. When paried with `meter` indicates a electric meter."^^<http://www.w3.org/2001/XMLSchema#string> .
<http://vcharpenay.github.io/hto/hto.xml#elec> <http://www.w3.org/2000/01/rdf-schema#comment> "note: according to the documentation, is assocated to either point or equip" .
<http://vcharpenay.github.io/hto/hto.xml#enable> <http://www.w3.org/1999/02/22-rdf-syntax-ns#type> <http://www.w3.org/2002/07/owl#NamedIndividual> .
<http://vcharpenay.github.io/hto/hto.xml#enable> <http://www.w3.org/1999/02/22-rdf-syntax-ns#type> <http://vcharpenay.github.io/hto/hto.xml#HTag> .
<http://vcharpenay.github.io/hto/hto.xml#enable> <http://www.w3.org/2000/01/rdf-schema#comment> "  Secondary on/off `point` of an `equip` especially used with a `vfd`. Enable is used with Bool points where true indicates on and false indicates off.  Equip with an enable should always also define a `run` point which indicates the primary on/off state of the equipment."^^<http://www.w3.org/2001/XMLSchema#string> .
<http://vcharpenay.github.io/hto/hto.xml#enable> <http://vcharpenay.github.io/hto/hto.xml#associatedTo> <http://vcharpenay.github.io/hto/hto.xml#OnOff> .
<http://vcharpenay.github.io/hto/hto.xml#energy> <http://www.w3.org/1999/02/22-rdf-syntax-ns#type> <http://www.w3.org/2002/07/owl#NamedIndividual> .
<http://vcharpenay.github.io/hto/hto.xml#energy> <http://www.w3.org/1999/02/22-rdf-syntax-ns#type> <http://vcharpenay.github.io/hto/hto.xml#HTag> .
<http://vcharpenay.github.io/hto/hto.xml#energy> <http://www.w3.org/2000/01/rdf-schema#comment> "  Applied to `point` entities which measure energy consumption:   - Electric meters: \"kWh\"   - Thermal meters: \"BTU\"   - Gas meters: \"m\u00C2\u00B3_gas\"   - Chillers: \"tonrefh\""^^<http://www.w3.org/2001/XMLSchema#string> .
<http://vcharpenay.github.io/hto/hto.xml#entering> <http://www.w3.org/1999/02/22-rdf-syntax-ns#type> <http://www.w3.org/2002/07/owl#NamedIndividual> .
<http://vcharpenay.github.io/hto/hto.xml#entering> <http://www.w3.org/1999/02/22-rdf-syntax-ns#type> <http://vcharpenay.github.io/hto/hto.xml#HTag> .
<http://vcharpenay.github.io/hto/hto.xml#entering> <http://www.w3.org/2000/01/rdf-schema#comment> "  Indicates `water` or `steam` entering a piece of equipment like a `boiler` or `chiller`.  Used with `vav` for air flow into the unit from the AHU."^^<http://www.w3.org/2001/XMLSchema#string> .
<http://vcharpenay.github.io/hto/hto.xml#entering> <http://vcharpenay.github.io/hto/hto.xml#associatedTo> <http://vcharpenay.github.io/hto/hto.xml#Entering> .
<http://vcharpenay.github.io/hto/hto.xml#evaporator> <http://www.w3.org/1999/02/22-rdf-syntax-ns#type> <http://www.w3.org/2002/07/owl#NamedIndividual> .
<http://vcharpenay.github.io/hto/hto.xml#evaporator> <http://www.w3.org/1999/02/22-rdf-syntax-ns#type> <http://vcharpenay.github.io/hto/hto.xml#HTag> .
<http://vcharpenay.github.io/hto/hto.xml#evaporator> <http://www.w3.org/2000/01/rdf-schema#comment> "  Indicates points on the evaporator mechanism used to convert a refrigerant from its liquid to gageous state.  It is often paired with the `refrig` marker tag."^^<http://www.w3.org/2001/XMLSchema#string> .
<http://vcharpenay.github.io/hto/hto.xml#exhaust> <http://www.w3.org/1999/02/22-rdf-syntax-ns#type> <http://www.w3.org/2002/07/owl#NamedIndividual> .
<http://vcharpenay.github.io/hto/hto.xml#exhaust> <http://www.w3.org/1999/02/22-rdf-syntax-ns#type> <http://vcharpenay.github.io/hto/hto.xml#HTag> .
<http://vcharpenay.github.io/hto/hto.xml#exhaust> <http://www.w3.org/2000/01/rdf-schema#comment> "  Associated with the exhaust air an `ahu`."^^<http://www.w3.org/2001/XMLSchema#string> .
<http://vcharpenay.github.io/hto/hto.xml#exhaust> <http://vcharpenay.github.io/hto/hto.xml#associatedTo> <http://vcharpenay.github.io/hto/hto.xml#Exhaust> .
<http://vcharpenay.github.io/hto/hto.xml#faceBypass> <http://www.w3.org/1999/02/22-rdf-syntax-ns#type> <http://www.w3.org/2002/07/owl#NamedIndividual> .
<http://vcharpenay.github.io/hto/hto.xml#faceBypass> <http://www.w3.org/1999/02/22-rdf-syntax-ns#type> <http://vcharpenay.github.io/hto/hto.xml#HTag> .
<http://vcharpenay.github.io/hto/hto.xml#faceBypass> <http://www.w3.org/2000/01/rdf-schema#comment> "  A `point` of an `ahu` indicating air flow is by-passing the heating/cooling elements. If a boolean point, then true indicates the unit is in by-pass mode and false indicates by-pass is disabled.  If the point is an analog point then 100% indicates full by-pass mode and 0% that by-pass is completely disabled."^^<http://www.w3.org/2001/XMLSchema#string> .
<http://vcharpenay.github.io/hto/hto.xml#fan> <http://www.w3.org/1999/02/22-rdf-syntax-ns#type> <http://www.w3.org/2002/07/owl#NamedIndividual> .
<http://vcharpenay.github.io/hto/hto.xml#fan> <http://www.w3.org/1999/02/22-rdf-syntax-ns#type> <http://vcharpenay.github.io/hto/hto.xml#HTag> .
<http://vcharpenay.github.io/hto/hto.xml#fan> <http://www.w3.org/2000/01/rdf-schema#comment> "  Fan `point` or `equip` associated with an `ahu`, `vav`, or `coolingTower`."^^<http://www.w3.org/2001/XMLSchema#string> .
<http://vcharpenay.github.io/hto/hto.xml#fan> <http://www.w3.org/2000/01/rdf-schema#comment> "note: according to the documentation, is assocated to either point or equip. Should use reasoning to choose the right one for a given HEntity" .
<http://vcharpenay.github.io/hto/hto.xml#filter> <http://www.w3.org/1999/02/22-rdf-syntax-ns#type> <http://www.w3.org/2002/07/owl#NamedIndividual> .
<http://vcharpenay.github.io/hto/hto.xml#filter> <http://www.w3.org/1999/02/22-rdf-syntax-ns#type> <http://vcharpenay.github.io/hto/hto.xml#HTag> .
<http://vcharpenay.github.io/hto/hto.xml#filter> <http://www.w3.org/2000/01/rdf-schema#comment> "  Differential pressure across the filter of an `ahu`.  If a boolean point then true indicates successful airflow and false indicates a clogged filter.  If a numeric then the pressure differential should be measured in \"inH\u00E2\u201A\u201AO\" or \"kPa\""^^<http://www.w3.org/2001/XMLSchema#string> .
<http://vcharpenay.github.io/hto/hto.xml#filter> <http://vcharpenay.github.io/hto/hto.xml#associatedTo> <http://vcharpenay.github.io/hto/hto.xml#Pressure> .
<http://vcharpenay.github.io/hto/hto.xml#flow> <http://www.w3.org/1999/02/22-rdf-syntax-ns#type> <http://www.w3.org/2002/07/owl#NamedIndividual> .
<http://vcharpenay.github.io/hto/hto.xml#flow> <http://www.w3.org/1999/02/22-rdf-syntax-ns#type> <http://vcharpenay.github.io/hto/hto.xml#HTag> .
<http://vcharpenay.github.io/hto/hto.xml#flow> <http://www.w3.org/2000/01/rdf-schema#comment> "  Marker tag on a `point` which measures rate of volume currently flowing through a flow meter, duct, or pipe .   - Air flow: \"cfm\" or \"L/s\"   - Gas/water flow: \"gal/min\" or \"m\u00C2\u00B3/s\""^^<http://www.w3.org/2001/XMLSchema#string> .
<http://vcharpenay.github.io/hto/hto.xml#flow> <http://vcharpenay.github.io/hto/hto.xml#associatedTo> <http://vcharpenay.github.io/hto/hto.xml#Flow> .
<http://vcharpenay.github.io/hto/hto.xml#freezeStat> <http://www.w3.org/1999/02/22-rdf-syntax-ns#type> <http://www.w3.org/2002/07/owl#NamedIndividual> .
<http://vcharpenay.github.io/hto/hto.xml#freezeStat> <http://www.w3.org/1999/02/22-rdf-syntax-ns#type> <http://vcharpenay.github.io/hto/hto.xml#HTag> .
<http://vcharpenay.github.io/hto/hto.xml#freezeStat> <http://www.w3.org/2000/01/rdf-schema#comment> "  A boolean `point` of an `ahu` indicating a freezing condition which might require a control sequence to protect the equipment. If true then a freeze condition is deteted, or false if not."^^<http://www.w3.org/2001/XMLSchema#string> .
<http://vcharpenay.github.io/hto/hto.xml#freezeStat> <http://vcharpenay.github.io/hto/hto.xml#associatedTo> <http://vcharpenay.github.io/hto/hto.xml#OnOff> .
<http://vcharpenay.github.io/hto/hto.xml#freq> <http://www.w3.org/1999/02/22-rdf-syntax-ns#type> <http://www.w3.org/2002/07/owl#NamedIndividual> .
<http://vcharpenay.github.io/hto/hto.xml#freq> <http://www.w3.org/1999/02/22-rdf-syntax-ns#type> <http://vcharpenay.github.io/hto/hto.xml#HTag> .
<http://vcharpenay.github.io/hto/hto.xml#freq> <http://www.w3.org/2000/01/rdf-schema#comment> "  Electrical A/C frequency `point` measured in \"Hz\" for `elec` `meter` or a `vfd`."^^<http://www.w3.org/2001/XMLSchema#string> .
<http://vcharpenay.github.io/hto/hto.xml#freq> <http://vcharpenay.github.io/hto/hto.xml#associatedTo> <http://vcharpenay.github.io/hto/hto.xml#Frequency> .
<http://vcharpenay.github.io/hto/hto.xml#gas> <http://www.w3.org/1999/02/22-rdf-syntax-ns#type> <http://www.w3.org/2002/07/owl#NamedIndividual> .
<http://vcharpenay.github.io/hto/hto.xml#gas> <http://www.w3.org/1999/02/22-rdf-syntax-ns#type> <http://vcharpenay.github.io/hto/hto.xml#HTag> .
<http://vcharpenay.github.io/hto/hto.xml#gas> <http://www.w3.org/2000/01/rdf-schema#comment> "  Used on `point` or `equip` entities relating to natural gas. When paried with `meter` indicates a gas meter."^^<http://www.w3.org/2001/XMLSchema#string> .
<http://vcharpenay.github.io/hto/hto.xml#gas> <http://vcharpenay.github.io/hto/hto.xml#associatedTo> <http://vcharpenay.github.io/hto/hto.xml#Gas> .
<http://vcharpenay.github.io/hto/hto.xml#heat> <http://www.w3.org/1999/02/22-rdf-syntax-ns#type> <http://www.w3.org/2002/07/owl#NamedIndividual> .
<http://vcharpenay.github.io/hto/hto.xml#heat> <http://www.w3.org/1999/02/22-rdf-syntax-ns#type> <http://vcharpenay.github.io/hto/hto.xml#HTag> .
<http://vcharpenay.github.io/hto/hto.xml#heat> <http://www.w3.org/2000/01/rdf-schema#comment> "  Heating coil as bool or float point on an `ahu` or `vav`. If multiple stages are used, then also specify the `stage` tag. If the heating coil is controlled by a valve, then this point is mesaured from 0% to 100%, otherwise it should be a boolean point."^^<http://www.w3.org/2001/XMLSchema#string> .
<http://vcharpenay.github.io/hto/hto.xml#heat> <http://vcharpenay.github.io/hto/hto.xml#associatedTo> <http://vcharpenay.github.io/hto/hto.xml#HeatingCoil> .
<http://vcharpenay.github.io/hto/hto.xml#heatWheel> <http://www.w3.org/1999/02/22-rdf-syntax-ns#type> <http://www.w3.org/2002/07/owl#NamedIndividual> .
<http://vcharpenay.github.io/hto/hto.xml#heatWheel> <http://www.w3.org/1999/02/22-rdf-syntax-ns#type> <http://vcharpenay.github.io/hto/hto.xml#HTag> .
<http://vcharpenay.github.io/hto/hto.xml#heatWheel> <http://www.w3.org/2000/01/rdf-schema#comment> "  Bool `point` which models the on or off state of an `ahu` heat wheel."^^<http://www.w3.org/2001/XMLSchema#string> .
<http://vcharpenay.github.io/hto/hto.xml#heatWheel> <http://vcharpenay.github.io/hto/hto.xml#associatedTo> <http://vcharpenay.github.io/hto/hto.xml#OnOff> .
<http://vcharpenay.github.io/hto/hto.xml#heating> <http://www.w3.org/1999/02/22-rdf-syntax-ns#type> <http://www.w3.org/2002/07/owl#NamedIndividual> .
<http://vcharpenay.github.io/hto/hto.xml#heating> <http://www.w3.org/1999/02/22-rdf-syntax-ns#type> <http://vcharpenay.github.io/hto/hto.xml#HTag> .
<http://vcharpenay.github.io/hto/hto.xml#heating> <http://www.w3.org/2000/01/rdf-schema#comment> "  Associated with the heating mode of an HVAC system."^^<http://www.w3.org/2001/XMLSchema#string> .
<http://vcharpenay.github.io/hto/hto.xml#humidifier> <http://www.w3.org/1999/02/22-rdf-syntax-ns#type> <http://www.w3.org/2002/07/owl#NamedIndividual> .
<http://vcharpenay.github.io/hto/hto.xml#humidifier> <http://www.w3.org/1999/02/22-rdf-syntax-ns#type> <http://vcharpenay.github.io/hto/hto.xml#HTag> .
<http://vcharpenay.github.io/hto/hto.xml#humidifier> <http://www.w3.org/2000/01/rdf-schema#comment> "  Boolean or numeric `point` of an `ahu` used to indicate if if the humidifier is on or off."^^<http://www.w3.org/2001/XMLSchema#string> .
<http://vcharpenay.github.io/hto/hto.xml#humidifier> <http://vcharpenay.github.io/hto/hto.xml#associatedTo> <http://vcharpenay.github.io/hto/hto.xml#OnOff> .
<http://vcharpenay.github.io/hto/hto.xml#humidity> <http://www.w3.org/1999/02/22-rdf-syntax-ns#type> <http://www.w3.org/2002/07/owl#NamedIndividual> .
<http://vcharpenay.github.io/hto/hto.xml#humidity> <http://www.w3.org/1999/02/22-rdf-syntax-ns#type> <http://vcharpenay.github.io/hto/hto.xml#HTag> .
<http://vcharpenay.github.io/hto/hto.xml#humidity> <http://www.w3.org/2000/01/rdf-schema#comment> "  Humidity measured from 0% to 100%."^^<http://www.w3.org/2001/XMLSchema#string> .
<http://vcharpenay.github.io/hto/hto.xml#humidity> <http://vcharpenay.github.io/hto/hto.xml#associatedTo> <http://vcharpenay.github.io/hto/hto.xml#Humidity> .
<http://vcharpenay.github.io/hto/hto.xml#hvac> <http://www.w3.org/1999/02/22-rdf-syntax-ns#type> <http://www.w3.org/2002/07/owl#NamedIndividual> .
<http://vcharpenay.github.io/hto/hto.xml#hvac> <http://www.w3.org/1999/02/22-rdf-syntax-ns#type> <http://vcharpenay.github.io/hto/hto.xml#HTag> .
<http://vcharpenay.github.io/hto/hto.xml#hvac> <http://www.w3.org/2000/01/rdf-schema#comment> "  Associated with HVAC (Heating, Ventilating, Air Conditioning)"^^<http://www.w3.org/2001/XMLSchema#string> .
<http://vcharpenay.github.io/hto/hto.xml#hvac> <http://vcharpenay.github.io/hto/hto.xml#associatedTo> <http://vcharpenay.github.io/hto/hto.xml#HVAC> .
<http://vcharpenay.github.io/hto/hto.xml#isolation> <http://www.w3.org/1999/02/22-rdf-syntax-ns#type> <http://www.w3.org/2002/07/owl#NamedIndividual> .
<http://vcharpenay.github.io/hto/hto.xml#isolation> <http://www.w3.org/1999/02/22-rdf-syntax-ns#type> <http://vcharpenay.github.io/hto/hto.xml#HTag> .
<http://vcharpenay.github.io/hto/hto.xml#isolation> <http://www.w3.org/2000/01/rdf-schema#comment> "  Indicates a `valve` used to isolate a piece of equipment from a piping system."^^<http://www.w3.org/2001/XMLSchema#string> .
<http://vcharpenay.github.io/hto/hto.xml#isolation> <http://vcharpenay.github.io/hto/hto.xml#associatedTo> <http://vcharpenay.github.io/hto/hto.xml#IsolationValve> .
<http://vcharpenay.github.io/hto/hto.xml#leaving> <http://www.w3.org/1999/02/22-rdf-syntax-ns#type> <http://www.w3.org/2002/07/owl#NamedIndividual> .
<http://vcharpenay.github.io/hto/hto.xml#leaving> <http://www.w3.org/1999/02/22-rdf-syntax-ns#type> <http://vcharpenay.github.io/hto/hto.xml#HTag> .
<http://vcharpenay.github.io/hto/hto.xml#leaving> <http://www.w3.org/2000/01/rdf-schema#comment> "  Indicates `water` or `steam` exiting a piece of equipment like a `boiler` or `chiller`."^^<http://www.w3.org/2001/XMLSchema#string> .
<http://vcharpenay.github.io/hto/hto.xml#leaving> <http://vcharpenay.github.io/hto/hto.xml#associatedTo> <http://vcharpenay.github.io/hto/hto.xml#Leaving> .
<http://vcharpenay.github.io/hto/hto.xml#lightLevel> <http://www.w3.org/1999/02/22-rdf-syntax-ns#type> <http://www.w3.org/2002/07/owl#NamedIndividual> .
<http://vcharpenay.github.io/hto/hto.xml#lightLevel> <http://www.w3.org/1999/02/22-rdf-syntax-ns#type> <http://vcharpenay.github.io/hto/hto.xml#HTag> .
<http://vcharpenay.github.io/hto/hto.xml#lightLevel> <http://www.w3.org/2000/01/rdf-schema#comment> "  Light level sensor point under `lightsGroup` measured in \"lux\" or \"lumen\"."^^<http://www.w3.org/2001/XMLSchema#string> .
<http://vcharpenay.github.io/hto/hto.xml#lightLevel> <http://vcharpenay.github.io/hto/hto.xml#associatedTo> <http://vcharpenay.github.io/hto/hto.xml#LightLevel> .
<http://vcharpenay.github.io/hto/hto.xml#lights> <http://www.w3.org/1999/02/22-rdf-syntax-ns#type> <http://www.w3.org/2002/07/owl#NamedIndividual> .
<http://vcharpenay.github.io/hto/hto.xml#lights> <http://www.w3.org/1999/02/22-rdf-syntax-ns#type> <http://vcharpenay.github.io/hto/hto.xml#HTag> .
<http://vcharpenay.github.io/hto/hto.xml#lights> <http://www.w3.org/2000/01/rdf-schema#comment> "  Lighting on/off status as a boolean or if dimmable a numeric between 0% and 100%."^^<http://www.w3.org/2001/XMLSchema#string> .
<http://vcharpenay.github.io/hto/hto.xml#lights> <http://www.w3.org/2000/01/rdf-schema#comment> "note: according to the documentation, subsumes sensor. But associated here to a Measurement type and redundant with the tag lightLevel." .
<http://vcharpenay.github.io/hto/hto.xml#lights> <http://vcharpenay.github.io/hto/hto.xml#associatedTo> <http://vcharpenay.github.io/hto/hto.xml#LightLevel> .
<http://vcharpenay.github.io/hto/hto.xml#lightsGroup> <http://www.w3.org/1999/02/22-rdf-syntax-ns#type> <http://www.w3.org/2002/07/owl#NamedIndividual> .
<http://vcharpenay.github.io/hto/hto.xml#lightsGroup> <http://www.w3.org/1999/02/22-rdf-syntax-ns#type> <http://vcharpenay.github.io/hto/hto.xml#HTag> .
<http://vcharpenay.github.io/hto/hto.xml#lightsGroup> <http://www.w3.org/2000/01/rdf-schema#comment> "  Equip level of the lighting system which is a group of one or more `lights` points."^^<http://www.w3.org/2001/XMLSchema#string> .
<http://vcharpenay.github.io/hto/hto.xml#lightsGroup> <http://vcharpenay.github.io/hto/hto.xml#associatedTo> <http://vcharpenay.github.io/hto/hto.xml#LightsGroup> .
<http://vcharpenay.github.io/hto/hto.xml#load> <http://www.w3.org/1999/02/22-rdf-syntax-ns#type> <http://www.w3.org/2002/07/owl#NamedIndividual> .
<http://vcharpenay.github.io/hto/hto.xml#load> <http://www.w3.org/1999/02/22-rdf-syntax-ns#type> <http://vcharpenay.github.io/hto/hto.xml#HTag> .
<http://vcharpenay.github.io/hto/hto.xml#load> <http://www.w3.org/2000/01/rdf-schema#comment> "  Models a `point` on a `chiller` used to command or measure the chiller's load as a percentage from \"0%\" to \"100%\".  When paired with `cmd` this models the chiller's load limit.  When paired with `sensor` this models the chiller's current load factor."^^<http://www.w3.org/2001/XMLSchema#string> .
<http://vcharpenay.github.io/hto/hto.xml#load> <http://vcharpenay.github.io/hto/hto.xml#associatedTo> <http://vcharpenay.github.io/hto/hto.xml#Percentage> .
<http://vcharpenay.github.io/hto/hto.xml#meter> <http://www.w3.org/1999/02/22-rdf-syntax-ns#type> <http://www.w3.org/2002/07/owl#NamedIndividual> .
<http://vcharpenay.github.io/hto/hto.xml#meter> <http://www.w3.org/1999/02/22-rdf-syntax-ns#type> <http://vcharpenay.github.io/hto/hto.xml#HTag> .
<http://vcharpenay.github.io/hto/hto.xml#meter> <http://www.w3.org/2000/01/rdf-schema#comment> "  Equip which meters usage of `elec` energy, thermal energy, `gas`, `water` or `steam`."^^<http://www.w3.org/2001/XMLSchema#string> .
<http://vcharpenay.github.io/hto/hto.xml#meter> <http://vcharpenay.github.io/hto/hto.xml#associatedTo> <http://vcharpenay.github.io/hto/hto.xml#Meter> .
<http://vcharpenay.github.io/hto/hto.xml#mixed> <http://www.w3.org/1999/02/22-rdf-syntax-ns#type> <http://www.w3.org/2002/07/owl#NamedIndividual> .
<http://vcharpenay.github.io/hto/hto.xml#mixed> <http://www.w3.org/1999/02/22-rdf-syntax-ns#type> <http://vcharpenay.github.io/hto/hto.xml#HTag> .
<http://vcharpenay.github.io/hto/hto.xml#mixed> <http://www.w3.org/2000/01/rdf-schema#comment> "  Associated with the mixed air of an `ahu`."^^<http://www.w3.org/2001/XMLSchema#string> .
<http://vcharpenay.github.io/hto/hto.xml#mixed> <http://vcharpenay.github.io/hto/hto.xml#associatedTo> <http://vcharpenay.github.io/hto/hto.xml#Mixed> .
<http://vcharpenay.github.io/hto/hto.xml#occupancyIndicator> <http://www.w3.org/1999/02/22-rdf-syntax-ns#type> <http://www.w3.org/2002/07/owl#NamedIndividual> .
<http://vcharpenay.github.io/hto/hto.xml#occupancyIndicator> <http://www.w3.org/1999/02/22-rdf-syntax-ns#type> <http://vcharpenay.github.io/hto/hto.xml#HTag> .
<http://vcharpenay.github.io/hto/hto.xml#occupancyIndicator> <http://www.w3.org/2000/01/rdf-schema#comment> "  Occupancy sensor under `lightsGroup`.  Point must be Bool where true indicates occupied and false indicates unoccupied"^^<http://www.w3.org/2001/XMLSchema#string> .
<http://vcharpenay.github.io/hto/hto.xml#occupancyIndicator> <http://www.w3.org/2000/01/rdf-schema#seeAlso> "http://project-haystack.org/tag/lights" .
<http://vcharpenay.github.io/hto/hto.xml#occupancyIndicator> <http://www.w3.org/2000/01/rdf-schema#comment> "note: according to the documentation, subsumes sensor. But associated here to a Measurement type. Similarly, lights and lightLevel tags both refer to the class LightLevel." .
<http://vcharpenay.github.io/hto/hto.xml#occupancyIndicator> <http://vcharpenay.github.io/hto/hto.xml#associatedTo> <http://vcharpenay.github.io/hto/hto.xml#OnOff> .
<http://vcharpenay.github.io/hto/hto.xml#perimeterHeat> <http://www.w3.org/1999/02/22-rdf-syntax-ns#type> <http://www.w3.org/2002/07/owl#NamedIndividual> .
<http://vcharpenay.github.io/hto/hto.xml#perimeterHeat> <http://www.w3.org/1999/02/22-rdf-syntax-ns#type> <http://vcharpenay.github.io/hto/hto.xml#HTag> .
<http://vcharpenay.github.io/hto/hto.xml#perimeterHeat> <http://www.w3.org/2000/01/rdf-schema#comment> "  Auxiliary heating points associated with a `vav`."^^<http://www.w3.org/2001/XMLSchema#string> .
<http://vcharpenay.github.io/hto/hto.xml#perimeterHeat> <http://vcharpenay.github.io/hto/hto.xml#associatedTo> <http://vcharpenay.github.io/hto/hto.xml#PerimeterHeat> .
<http://vcharpenay.github.io/hto/hto.xml#point> <http://www.w3.org/1999/02/22-rdf-syntax-ns#type> <http://www.w3.org/2002/07/owl#NamedIndividual> .
<http://vcharpenay.github.io/hto/hto.xml#point> <http://www.w3.org/1999/02/22-rdf-syntax-ns#type> <http://vcharpenay.github.io/hto/hto.xml#HTag> .
<http://vcharpenay.github.io/hto/hto.xml#point> <http://www.w3.org/2000/01/rdf-schema#comment> "  Data point such as a sensor or actuator."^^<http://www.w3.org/2001/XMLSchema#string> .
<http://vcharpenay.github.io/hto/hto.xml#point> <http://vcharpenay.github.io/hto/hto.xml#associatedTo> <http://vcharpenay.github.io/hto/hto.xml#Point> .
<http://vcharpenay.github.io/hto/hto.xml#power> <http://www.w3.org/1999/02/22-rdf-syntax-ns#type> <http://www.w3.org/2002/07/owl#NamedIndividual> .
<http://vcharpenay.github.io/hto/hto.xml#power> <http://www.w3.org/1999/02/22-rdf-syntax-ns#type> <http://vcharpenay.github.io/hto/hto.xml#HTag> .
<http://vcharpenay.github.io/hto/hto.xml#power> <http://www.w3.org/2000/01/rdf-schema#comment> "  Applied to `point` entities which measure energy consumed per unit time. For 'elec meter' this is the electrical demand.   - Electric meters: \"kW\"   - Thermal meters: \"BTU/h\"   - Chillers: \"tonref\" or \"kW\" refrigeration"^^<http://www.w3.org/2001/XMLSchema#string> .
<http://vcharpenay.github.io/hto/hto.xml#power> <http://vcharpenay.github.io/hto/hto.xml#associatedTo> <http://vcharpenay.github.io/hto/hto.xml#Power> .
<http://vcharpenay.github.io/hto/hto.xml#pressure> <http://www.w3.org/1999/02/22-rdf-syntax-ns#type> <http://www.w3.org/2002/07/owl#NamedIndividual> .
<http://vcharpenay.github.io/hto/hto.xml#pressure> <http://www.w3.org/1999/02/22-rdf-syntax-ns#type> <http://vcharpenay.github.io/hto/hto.xml#HTag> .
<http://vcharpenay.github.io/hto/hto.xml#pressure> <http://www.w3.org/2000/01/rdf-schema#comment> "  Static pressure associated with the measurement or control of fluids such as air, oxygen, water, steam, gas, oil, etc."^^<http://www.w3.org/2001/XMLSchema#string> .
<http://vcharpenay.github.io/hto/hto.xml#pressure> <http://vcharpenay.github.io/hto/hto.xml#associatedTo> <http://vcharpenay.github.io/hto/hto.xml#Pressure> .
<http://vcharpenay.github.io/hto/hto.xml#refrig> <http://www.w3.org/1999/02/22-rdf-syntax-ns#type> <http://www.w3.org/2002/07/owl#NamedIndividual> .
<http://vcharpenay.github.io/hto/hto.xml#refrig> <http://www.w3.org/1999/02/22-rdf-syntax-ns#type> <http://vcharpenay.github.io/hto/hto.xml#HTag> .
<http://vcharpenay.github.io/hto/hto.xml#refrig> <http://www.w3.org/2000/01/rdf-schema#comment> "  Indicates points associated with the measurment or control of the refrigerant substance in a cooling system like a `chiller`."^^<http://www.w3.org/2001/XMLSchema#string> .
<http://vcharpenay.github.io/hto/hto.xml#refrig> <http://vcharpenay.github.io/hto/hto.xml#associatedTo> <http://vcharpenay.github.io/hto/hto.xml#RefrigerantSubstance> .
<http://vcharpenay.github.io/hto/hto.xml#return> <http://www.w3.org/1999/02/22-rdf-syntax-ns#type> <http://www.w3.org/2002/07/owl#NamedIndividual> .
<http://vcharpenay.github.io/hto/hto.xml#return> <http://www.w3.org/1999/02/22-rdf-syntax-ns#type> <http://vcharpenay.github.io/hto/hto.xml#HTag> .
<http://vcharpenay.github.io/hto/hto.xml#return> <http://www.w3.org/2000/01/rdf-schema#comment> "  Associated with the return air an `ahu`."^^<http://www.w3.org/2001/XMLSchema#string> .
<http://vcharpenay.github.io/hto/hto.xml#return> <http://vcharpenay.github.io/hto/hto.xml#associatedTo> <http://vcharpenay.github.io/hto/hto.xml#Return> .
<http://vcharpenay.github.io/hto/hto.xml#rooftop> <http://www.w3.org/1999/02/22-rdf-syntax-ns#type> <http://www.w3.org/2002/07/owl#NamedIndividual> .
<http://vcharpenay.github.io/hto/hto.xml#rooftop> <http://www.w3.org/1999/02/22-rdf-syntax-ns#type> <http://vcharpenay.github.io/hto/hto.xml#HTag> .
<http://vcharpenay.github.io/hto/hto.xml#rooftop> <http://www.w3.org/2000/01/rdf-schema#comment> "  Used with `ahu` to mark an AHU as a packaged rooftop unit (RTU)."^^<http://www.w3.org/2001/XMLSchema#string> .
<http://vcharpenay.github.io/hto/hto.xml#rooftop> <http://vcharpenay.github.io/hto/hto.xml#associatedTo> <http://vcharpenay.github.io/hto/hto.xml#RTU> .
<http://vcharpenay.github.io/hto/hto.xml#run> <http://www.w3.org/1999/02/22-rdf-syntax-ns#type> <http://www.w3.org/2002/07/owl#NamedIndividual> .
<http://vcharpenay.github.io/hto/hto.xml#run> <http://www.w3.org/1999/02/22-rdf-syntax-ns#type> <http://vcharpenay.github.io/hto/hto.xml#HTag> .
<http://vcharpenay.github.io/hto/hto.xml#run> <http://www.w3.org/2000/01/rdf-schema#comment> "  Primary on/off `point` of an `equip` especially used with a `vfd`. Run is used with Bool points where true indicates on and false indicates off. When paired with `cmd` this is the commanded state of the equipment. When paired with `sensor` this is the actual status of the equip.  If the equipment also defines an `enable` point then both must be commanded on in order to run the equipment."^^<http://www.w3.org/2001/XMLSchema#string> .
<http://vcharpenay.github.io/hto/hto.xml#run> <http://www.w3.org/2000/01/rdf-schema#comment> "note: according to the documentation, subsumes sensor. But associated here to a Measurement type." .
<http://vcharpenay.github.io/hto/hto.xml#run> <http://vcharpenay.github.io/hto/hto.xml#associatedTo> <http://vcharpenay.github.io/hto/hto.xml#OnOff> .
<http://vcharpenay.github.io/hto/hto.xml#sensor> <http://www.w3.org/1999/02/22-rdf-syntax-ns#type> <http://www.w3.org/2002/07/owl#NamedIndividual> .
<http://vcharpenay.github.io/hto/hto.xml#sensor> <http://www.w3.org/1999/02/22-rdf-syntax-ns#type> <http://vcharpenay.github.io/hto/hto.xml#HTag> .
<http://vcharpenay.github.io/hto/hto.xml#sensor> <http://www.w3.org/2000/01/rdf-schema#comment> "  Classifies a `point` as an input, AI/BI, or sensor."^^<http://www.w3.org/2001/XMLSchema#string> .
<http://vcharpenay.github.io/hto/hto.xml#sensor> <http://vcharpenay.github.io/hto/hto.xml#associatedTo> <http://vcharpenay.github.io/hto/hto.xml#Sensor> .
<http://vcharpenay.github.io/hto/hto.xml#sp> <http://www.w3.org/1999/02/22-rdf-syntax-ns#type> <http://www.w3.org/2002/07/owl#NamedIndividual> .
<http://vcharpenay.github.io/hto/hto.xml#sp> <http://www.w3.org/1999/02/22-rdf-syntax-ns#type> <http://vcharpenay.github.io/hto/hto.xml#HTag> .
<http://vcharpenay.github.io/hto/hto.xml#sp> <http://www.w3.org/2000/01/rdf-schema#comment> "  Classifies a `point` as a setpoint, soft point, or process control variable."^^<http://www.w3.org/2001/XMLSchema#string> .
<http://vcharpenay.github.io/hto/hto.xml#sp> <http://vcharpenay.github.io/hto/hto.xml#associatedTo> <http://vcharpenay.github.io/hto/hto.xml#SetPoint> .
<http://vcharpenay.github.io/hto/hto.xml#speed> <http://www.w3.org/1999/02/22-rdf-syntax-ns#type> <http://www.w3.org/2002/07/owl#NamedIndividual> .
<http://vcharpenay.github.io/hto/hto.xml#speed> <http://www.w3.org/1999/02/22-rdf-syntax-ns#type> <http://vcharpenay.github.io/hto/hto.xml#HTag> .
<http://vcharpenay.github.io/hto/hto.xml#speed> <http://www.w3.org/2000/01/rdf-schema#comment> "  Speed `point` of a `vfd` measured in \"%\" where 0% is off and 100% is the fastest speed."^^<http://www.w3.org/2001/XMLSchema#string> .
<http://vcharpenay.github.io/hto/hto.xml#speed> <http://vcharpenay.github.io/hto/hto.xml#associatedTo> <http://vcharpenay.github.io/hto/hto.xml#Speed> .
<http://vcharpenay.github.io/hto/hto.xml#steam> <http://www.w3.org/1999/02/22-rdf-syntax-ns#type> <http://www.w3.org/2002/07/owl#NamedIndividual> .
<http://vcharpenay.github.io/hto/hto.xml#steam> <http://www.w3.org/1999/02/22-rdf-syntax-ns#type> <http://vcharpenay.github.io/hto/hto.xml#HTag> .
<http://vcharpenay.github.io/hto/hto.xml#steam> <http://www.w3.org/2000/01/rdf-schema#comment> "  Point associated with the measurement or control of steam. This tag is often paired with `entering` versus `leaving` versus `delta`. It may also be paired with `meter` to indicate a steam meter."^^<http://www.w3.org/2001/XMLSchema#string> .
<http://vcharpenay.github.io/hto/hto.xml#steam> <http://vcharpenay.github.io/hto/hto.xml#associatedTo> <http://vcharpenay.github.io/hto/hto.xml#Steam> .
<http://vcharpenay.github.io/hto/hto.xml#temp> <http://www.w3.org/1999/02/22-rdf-syntax-ns#type> <http://www.w3.org/2002/07/owl#NamedIndividual> .
<http://vcharpenay.github.io/hto/hto.xml#temp> <http://www.w3.org/1999/02/22-rdf-syntax-ns#type> <http://vcharpenay.github.io/hto/hto.xml#HTag> .
<http://vcharpenay.github.io/hto/hto.xml#temp> <http://www.w3.org/2000/01/rdf-schema#comment> "  Temperature measured in \u00C2\u00B0C or \u00C2\u00B0F."^^<http://www.w3.org/2001/XMLSchema#string> .
<http://vcharpenay.github.io/hto/hto.xml#temp> <http://vcharpenay.github.io/hto/hto.xml#associatedTo> <http://vcharpenay.github.io/hto/hto.xml#Temperature> .
<http://vcharpenay.github.io/hto/hto.xml#valve> <http://www.w3.org/1999/02/22-rdf-syntax-ns#type> <http://www.w3.org/2002/07/owl#NamedIndividual> .
<http://vcharpenay.github.io/hto/hto.xml#valve> <http://www.w3.org/1999/02/22-rdf-syntax-ns#type> <http://vcharpenay.github.io/hto/hto.xml#HTag> .
<http://vcharpenay.github.io/hto/hto.xml#valve> <http://www.w3.org/2000/01/rdf-schema#comment> "  Marker tag on `point` which indicates a valve used to regulate or control the flow or pressure of a fluid.  It is used with `cmd` to indicate the valve command: true/false (open/close) or 0% to 100%.  It may also be used with `sensor` to indicate a feedback sensor such as a voltage giving exact position between 0% and 100%."^^<http://www.w3.org/2001/XMLSchema#string> .
<http://vcharpenay.github.io/hto/hto.xml#valve> <http://vcharpenay.github.io/hto/hto.xml#associatedTo> <http://vcharpenay.github.io/hto/hto.xml#Valve> .
<http://vcharpenay.github.io/hto/hto.xml#vav> <http://www.w3.org/1999/02/22-rdf-syntax-ns#type> <http://www.w3.org/2002/07/owl#NamedIndividual> .
<http://vcharpenay.github.io/hto/hto.xml#vav> <http://www.w3.org/1999/02/22-rdf-syntax-ns#type> <http://vcharpenay.github.io/hto/hto.xml#HTag> .
<http://vcharpenay.github.io/hto/hto.xml#vav> <http://www.w3.org/2000/01/rdf-schema#comment> "  Variable Volume Volume supply duct `equip`."^^<http://www.w3.org/2001/XMLSchema#string> .
<http://vcharpenay.github.io/hto/hto.xml#vav> <http://vcharpenay.github.io/hto/hto.xml#associatedTo> <http://vcharpenay.github.io/hto/hto.xml#VAV> .
<http://vcharpenay.github.io/hto/hto.xml#vfd> <http://www.w3.org/1999/02/22-rdf-syntax-ns#type> <http://www.w3.org/2002/07/owl#NamedIndividual> .
<http://vcharpenay.github.io/hto/hto.xml#vfd> <http://www.w3.org/1999/02/22-rdf-syntax-ns#type> <http://vcharpenay.github.io/hto/hto.xml#HTag> .
<http://vcharpenay.github.io/hto/hto.xml#vfd> <http://www.w3.org/2000/01/rdf-schema#comment> "  Marker for a motor `equip` with variable frequency drive.  Commonly used in combination with `fan` and `pump`."^^<http://www.w3.org/2001/XMLSchema#string> .
<http://vcharpenay.github.io/hto/hto.xml#vfd> <http://vcharpenay.github.io/hto/hto.xml#associatedTo> <http://vcharpenay.github.io/hto/hto.xml#VFD> .
<http://vcharpenay.github.io/hto/hto.xml#water> <http://www.w3.org/1999/02/22-rdf-syntax-ns#type> <http://www.w3.org/2002/07/owl#NamedIndividual> .
<http://vcharpenay.github.io/hto/hto.xml#water> <http://www.w3.org/1999/02/22-rdf-syntax-ns#type> <http://vcharpenay.github.io/hto/hto.xml#HTag> .
<http://vcharpenay.github.io/hto/hto.xml#water> <http://www.w3.org/2000/01/rdf-schema#comment> "  Point associated with the measurement or control of water.  This tag is often paired:   - `entering` versus `leaving` versus `delta`   - `chilled` versus `condenser` It may also be paired with `meter` to indicate a water meter."^^<http://www.w3.org/2001/XMLSchema#string> .
<http://vcharpenay.github.io/hto/hto.xml#water> <http://vcharpenay.github.io/hto/hto.xml#associatedTo> <http://vcharpenay.github.io/hto/hto.xml#Water> .
<http://vcharpenay.github.io/hto/hto.xml#zone> <http://www.w3.org/1999/02/22-rdf-syntax-ns#type> <http://www.w3.org/2002/07/owl#NamedIndividual> .
<http://vcharpenay.github.io/hto/hto.xml#zone> <http://www.w3.org/1999/02/22-rdf-syntax-ns#type> <http://vcharpenay.github.io/hto/hto.xml#HTag> .
<http://vcharpenay.github.io/hto/hto.xml#zone> <http://www.w3.org/2000/01/rdf-schema#comment> "  Associated with a conditioned [zone]`Zones` of a building."^^<http://www.w3.org/2001/XMLSchema#string> .
<http://vcharpenay.github.io/hto/hto.xml#zone> <http://vcharpenay.github.io/hto/hto.xml#associatedTo> <http://vcharpenay.github.io/hto/hto.xml#Zone> .
_:genid1 <http://www.w3.org/1999/02/22-rdf-syntax-ns#type> <http://www.w3.org/2002/07/owl#AllDisjointClasses> .
_:genid2 <http://www.w3.org/1999/02/22-rdf-syntax-ns#first> <http://vcharpenay.github.io/hto/hto.xml#Equipment> .
_:genid3 <http://www.w3.org/1999/02/22-rdf-syntax-ns#first> <http://vcharpenay.github.io/hto/hto.xml#Point> .
_:genid2 <http://www.w3.org/1999/02/22-rdf-syntax-ns#rest> _:genid3 .
_:genid4 <http://www.w3.org/1999/02/22-rdf-syntax-ns#first> <http://vcharpenay.github.io/hto/hto.xml#Site> .
_:genid3 <http://www.w3.org/1999/02/22-rdf-syntax-ns#rest> _:genid4 .
_:genid4 <http://www.w3.org/1999/02/22-rdf-syntax-ns#rest> <http://www.w3.org/1999/02/22-rdf-syntax-ns#nil> .
_:genid1 <http://www.w3.org/2002/07/owl#members> _:genid2 .
