@prefix :      <https://w3id.org/eepsa#> .
@prefix dc:    <http://purl.org/dc/elements/1.1/> .
@prefix ns:    <http://creativecommons.org/ns#> .
@prefix eepsa: <https://w3id.org/eepsa#> .
@prefix prov:  <http://www.w3.org/ns/prov#> .
@prefix bim4eepsa: <https://w3id.org/bim4eepsa#> .
@prefix wgs84_pos: <http://www.w3.org/2003/01/geo/wgs84_pos#> .
@prefix DUL:   <http://www.ontologydesignpatterns.org/ont/dul/DUL.owl#> .
@prefix foaf:  <http://xmlns.com/foaf/0.1/> .
@prefix terms: <http://purl.org/dc/terms/> .
@prefix iot-lite: <http://purl.oclc.org/NET/UNIS/iot-lite/iot-lite#> .
@prefix ssn:   <http://www.w3.org/ns/ssn/> .
@prefix vann:  <http://purl.org/vocab/vann/> .
@prefix schema: <http://schema.org/> .
@prefix ns1:   <http://www.w3.org/2003/06/sw-vocab-status/ns#> .
@prefix rdfs:  <http://www.w3.org/2000/01/rdf-schema#> .
@prefix bot:   <https://w3id.org/bot#> .
@prefix bibo:  <http://purl.org/ontology/bibo/> .
@prefix xsd:   <http://www.w3.org/2001/XMLSchema#> .
@prefix owl:   <http://www.w3.org/2002/07/owl#> .
@prefix rdf:   <http://www.w3.org/1999/02/22-rdf-syntax-ns#> .
@prefix skos:  <http://www.w3.org/2004/02/skos/core#> .
@prefix m4eepsa: <https://w3id.org/measurements4eepsa#> .

eepsa:SolarIrradiance
        a                owl:Class ;
        rdfs:subClassOf  eepsa:MeteorologicalProperty .

eepsa:periodMarchSW  a      owl:NamedIndividual ;
        rdfs:comment        "Individual representing sun exposure period in March for objects oriented towards the South West."@en ;
        eepsa:endingTime    "20:00:00" ;
        eepsa:hasMonth      3 ;
        eepsa:startingTime  "13:00:00" .

eepsa:OutlierCausedByExternalConditions
        a                owl:Class ;
        rdfs:comment     "An erroneous observation (e.g. temperature, illuminance) caused by external factors. For example for being next to a source of radiant heat or cold such as windows and poorly insulated outside walls."@en ;
        rdfs:label       "Outlier caused by External Conditions"@en ;
        rdfs:subClassOf  eepsa:OutlierCausedByDeviceLocation .

eepsa:periodAugustNE  a     owl:NamedIndividual ;
        rdfs:comment        "Individual representing sun exposure period in August for objects oriented towards the North East."@en ;
        eepsa:endingTime    "13:00:00" ;
        eepsa:hasMonth      8 ;
        eepsa:startingTime  "7:00:00" .

eepsa:periodFebruarySE
        a                   owl:NamedIndividual ;
        rdfs:comment        "Individual representing sun exposure period in February for objects oriented towards the South East."@en ;
        eepsa:hasMonth      2 ;
        eepsa:startingTime  "8:00:00" , "19:00:00" .

eepsa:startingTime  a  owl:DatatypeProperty ;
        rdfs:comment  "Determines the Starting time of a temporal entity."@en ;
        rdfs:label    "starting time"@en ;
        rdfs:range    xsd:time .

m4eepsa:southEastOrientation
        a       owl:NamedIndividual .

bot:Space  a             owl:Class ;
        rdfs:subClassOf  [ a                   owl:Class ;
                           owl:intersectionOf  ( [ a               owl:Restriction ;
                                                   owl:hasValue    eepsa:SpaceOccupancy ;
                                                   owl:onProperty  eepsa:isAffectedBy
                                                 ] [ a               owl:Restriction ;
                                                     owl:hasValue    m4eepsa:IndoorRelativeHumidity ;
                                                     owl:onProperty  eepsa:isAffectedBy
                                                   ] [ a               owl:Restriction ;
                                                       owl:hasValue    m4eepsa:IndoorTemperature ;
                                                       owl:onProperty  eepsa:isAffectedBy
                                                     ] )
                         ] .

<http://purl.org/iot/vocab/m3-lite#WindChill>
        rdfs:subClassOf  eepsa:MeteorologicalProperty .

eepsa:ComfortableThermalSituation
        a                owl:Class ;
        rdfs:comment     "A set of circumstances that ensures a comfortable thermal situation. Themal comfort is understood as that condition of mind that express satisfaction with the thermal environment and is assessed by subjective evaluation. (Source: ANSI/ASHRAE Standard 55-2017)"@en ;
        rdfs:label       "Comfortable Thermal Situation"@en ;
        rdfs:subClassOf  eepsa:Situation .

[ owl:minQualifiedCardinality  "1"^^xsd:nonNegativeInteger ] .

eepsa:providesWeatherService
        a             owl:ObjectProperty ;
        rdfs:comment  "Relation between a Weather Station and the Weather Service it provides (weather report, weather forecast,...)"@en ;
        rdfs:label    "provides weather service"@en ;
        rdfs:range    eepsa:WeatherService .

eepsa:isForecastedToProduceSituation
        a             owl:ObjectProperty ;
        rdfs:comment  "A property that links a Thing, with a Situation that is forecasted to produce"@en ;
        rdfs:label    "is forecasted to produce situation"@en ;
        rdfs:range    eepsa:Situation .

eepsa:periodJulySW  a       owl:NamedIndividual ;
        rdfs:comment        "Individual representing sun exposure period in July for objects oriented towards the North West."@en ;
        eepsa:endingTime    "22:00:00" ;
        eepsa:hasMonth      7 ;
        eepsa:startingTime  "14:00:00" .

eepsa:OutlierCausedByDeviceMalfunction
        a                owl:Class ;
        rdfs:comment     "An erroneous observation caused by a malfunction suffered by the device, which might have been transient."@en ;
        rdfs:label       "Outlier caused by Device Malfunction"@en ;
        rdfs:subClassOf  eepsa:OutlierCausedByDeviceError ;
        rdfs:subClassOf  [ a                   owl:Restriction ;
                           owl:onProperty      eepsa:hasSolvingMethod ;
                           owl:someValuesFrom  eepsa:DeviceReplacement
                         ] .

m4eepsa:westOrientation
        a       owl:NamedIndividual .

<http://purl.org/iot/vocab/m3-lite#LeafWetness>
        rdfs:subClassOf  eepsa:MeteorologicalProperty .

eepsa:hasDataSource  a  owl:ObjectProperty ;
        rdfs:comment  "Relation between a Thing and a data source where values can be retrieved."@en ;
        rdfs:label    "has data source"@en .

m4eepsa:southOrientation
        a       owl:NamedIndividual .

DUL:Method  a             owl:Class ;
        rdfs:comment      "A method is a Description that defines or uses concepts in order to guide carrying out actions aimed at a solution with respect to a problem. It is different from a Plan, because plans could be carried out in order to follow a method, but a method can be followed by executing alternative plans." ;
        rdfs:isDefinedBy  <http://www.ontologydesignpatterns.org/ont/dul/DUL.owl> .

eepsa:periodNovemberSE
        a                   owl:NamedIndividual ;
        rdfs:comment        "Individual representing sun exposure period in November for objects oriented towards the South East."@en ;
        eepsa:endingTime    "18:00:00" ;
        eepsa:hasMonth      11 ;
        eepsa:startingTime  "8:00:00" .

eepsa:periodMayNE  a        owl:NamedIndividual ;
        rdfs:comment        "Individual representing sun exposure period in May for objects oriented towards the North East."@en ;
        eepsa:endingTime    "13:00:00" ;
        eepsa:hasMonth      5 ;
        eepsa:startingTime  "7:00:00" .

[ owl:minQualifiedCardinality  "1"^^xsd:nonNegativeInteger ] .

eepsa:periodDecemberSW
        a                   owl:NamedIndividual ;
        rdfs:comment        "Individual representing sun exposure period in December for objects oriented towards the South West."@en ;
        eepsa:endingTime    "18:00:00" ;
        eepsa:hasMonth      12 ;
        eepsa:startingTime  "12:00:00" .

eepsa:WeatherForecasting
        a                owl:Class ;
        rdfs:comment     "Predicted meteorological conditions for an area"@en ;
        rdfs:label       "Weather Forecasting"@en ;
        rdfs:subClassOf  eepsa:WeatherService .

eepsa:hasMonth  a   owl:DatatypeProperty ;
        rdfs:label  "has month"@en .

eepsa:Situation  a    owl:Class ;
        rdfs:comment  "Relative to a set of circumstances."@en ;
        rdfs:label    "Situation"@en .

eepsa:periodAprilNE  a      owl:NamedIndividual ;
        rdfs:comment        "Individual representing sun exposure period in April for objects oriented towards the North East."@en ;
        eepsa:endingTime    "13:00:00" ;
        eepsa:hasMonth      4 ;
        eepsa:startingTime  "7:00:00" .

eepsa:obsDate  a      owl:DatatypeProperty ;
        rdfs:comment  "Determines the Date (e.g. yyyy-MM-dd) of an observation." ;
        rdfs:label    "observation date"@en ;
        skos:example  "Example:\nmyOnto:obs1 eepsa:observationDate \"2017-02-15\"."@en .

eepsa:WestOrientedObject
        a                    owl:Class ;
        rdfs:comment         "Object oriented towards the West"@en ;
        rdfs:label           "West Oriented Object"@en ;
        rdfs:subClassOf      bim4eepsa:PhysicalObject ;
        owl:equivalentClass  [ a                   owl:Class ;
                               owl:intersectionOf  ( [ a               owl:Restriction ;
                                                       owl:hasValue    m4eepsa:westOrientation ;
                                                       owl:onProperty  <http://purl.org/iot/vocab/m3-lite#hasDirection>
                                                     ] [ a               owl:Restriction ;
                                                         owl:hasValue    <http://es.dbpedia.org/resource/Spain> ;
                                                         owl:onProperty  wgs84_pos:location
                                                       ] )
                             ] .

<http://purl.org/iot/vocab/m3-lite#CO2>
        rdfs:subClassOf  eepsa:MeteorologicalProperty .

owl:minQualifiedCardinality
        a       owl:AnnotationProperty .

eepsa:periodJanuaryNE
        a                   owl:NamedIndividual ;
        rdfs:comment        "Individual representing sun exposure period in January for objects oriented towards the North East."@en ;
        eepsa:endingTime    "11:00:00" ;
        eepsa:hasMonth      1 ;
        eepsa:startingTime  "8:00:00" .

eepsa:periodOctoberSW
        a                   owl:NamedIndividual ;
        rdfs:comment        "Individual representing sun exposure period in October for objects oriented towards the South West."@en ;
        eepsa:endingTime    "20:00:00" ;
        eepsa:hasMonth      10 ;
        eepsa:startingTime  "14:00:00" .

eepsa:OutlierCausedByBeamSpotlight
        a                owl:Class ;
        rdfs:comment     "An erroneous observation (e.g. temperature, illuminance) caused by a beam spotlight. For example, an observation made by a sensing device located under a light bulb"@en ;
        rdfs:label       "Outlier caused by Beam Spotlight"@en ;
        rdfs:subClassOf  eepsa:OutlierCausedByDeviceLocation .

dc:title  a     owl:AnnotationProperty .

<http://www.w3.org/ns/sosa/Sensor>
        rdfs:subClassOf  [ a                   owl:Restriction ;
                           owl:onProperty      <http://qudt.org/schema/qudt#unit> ;
                           owl:someValuesFrom  <http://qudt.org/schema/qudt#Unit>
                         ] .

eepsa:isHighlyAffectedBy
        a                   owl:ObjectProperty ;
        rdfs:comment        "Relationship between a space and the Quantity Kind that is affects its indoor conditions with a higher degree"@en ;
        rdfs:label          "is highly affected by"@en ;
        rdfs:range          ssn:Property ;
        rdfs:subPropertyOf  eepsa:isAffectedBy .

eepsa:periodJuneSW  a       owl:NamedIndividual ;
        rdfs:comment        "Individual representing sun exposure period in June for objects oriented towards the South West."@en ;
        eepsa:endingTime    "14:00:00" ;
        eepsa:hasMonth      6 ;
        eepsa:startingTime  "14:00:00" .

eepsa:SpaceOccupancy  a  owl:NamedIndividual .

<http://purl.org/iot/vocab/m3-lite#Precipitation>
        rdfs:subClassOf  eepsa:MeteorologicalProperty .

bim4eepsa:ExternalDoor
        rdfs:label  "External door"@en .

eepsa:NorthWestOrientedObject
        a                    owl:Class ;
        rdfs:comment         "Object oriented towards the North West"@en ;
        rdfs:label           "North West Oriented Object"@en ;
        rdfs:subClassOf      bim4eepsa:PhysicalObject ;
        rdfs:subClassOf      [ a                   owl:Class ;
                               owl:intersectionOf  ( [ a               owl:Restriction ;
                                                       owl:hasValue    eepsa:periodAprilNW ;
                                                       owl:onProperty  eepsa:hasSunExposurePeriod
                                                     ] [ a               owl:Restriction ;
                                                         owl:hasValue    eepsa:periodAugustNW ;
                                                         owl:onProperty  eepsa:hasSunExposurePeriod
                                                       ] [ a               owl:Restriction ;
                                                           owl:hasValue    eepsa:periodFebruaryNW ;
                                                           owl:onProperty  eepsa:hasSunExposurePeriod
                                                         ] [ a               owl:Restriction ;
                                                             owl:hasValue    eepsa:periodJulyNW ;
                                                             owl:onProperty  eepsa:hasSunExposurePeriod
                                                           ] [ a               owl:Restriction ;
                                                               owl:hasValue    eepsa:periodJuneNW ;
                                                               owl:onProperty  eepsa:hasSunExposurePeriod
                                                             ] [ a               owl:Restriction ;
                                                                 owl:hasValue    eepsa:periodMarchNW ;
                                                                 owl:onProperty  eepsa:hasSunExposurePeriod
                                                               ] [ a               owl:Restriction ;
                                                                   owl:hasValue    eepsa:periodMayNW ;
                                                                   owl:onProperty  eepsa:hasSunExposurePeriod
                                                                 ] [ a               owl:Restriction ;
                                                                     owl:hasValue    eepsa:periodOctoberNW ;
                                                                     owl:onProperty  eepsa:hasSunExposurePeriod
                                                                   ] [ a               owl:Restriction ;
                                                                       owl:hasValue    eepsa:periodSeptemberNW ;
                                                                       owl:onProperty  eepsa:hasSunExposurePeriod
                                                                     ] )
                             ] ;
        owl:equivalentClass  [ a                   owl:Class ;
                               owl:intersectionOf  ( [ a               owl:Restriction ;
                                                       owl:hasValue    m4eepsa:northWestOrientation ;
                                                       owl:onProperty  <http://purl.org/iot/vocab/m3-lite#hasDirection>
                                                     ] [ a               owl:Restriction ;
                                                         owl:hasValue    <http://es.dbpedia.org/resource/Spain> ;
                                                         owl:onProperty  wgs84_pos:location
                                                       ] )
                             ] .

[ owl:minQualifiedCardinality  "1"^^xsd:nonNegativeInteger ] .

<http://qudt.org/schema/qudt#numericValue>
        a           owl:DatatypeProperty ;
        rdfs:range  xsd:double .

eepsa:periodAugustNW  a     owl:NamedIndividual ;
        rdfs:comment        "Individual representing sun exposure period in August for objects oriented towards the North West."@en ;
        eepsa:endingTime    "22:00:00" ;
        eepsa:hasMonth      8 ;
        eepsa:startingTime  "18:00:00" .

eepsa:isAffectedBy  a  owl:ObjectProperty ;
        rdfs:comment  "Relationship between a space and the Quantity Kind that is affects its indoor conditions"@en ;
        rdfs:domain   bot:Space ;
        rdfs:label    "is affected by"@en ;
        rdfs:range    ssn:Property .

<http://purl.org/iot/vocab/m3-lite#CloudCover>
        a                owl:NamedIndividual ;
        rdfs:subClassOf  eepsa:MeteorologicalProperty .

eepsa:periodFebruarySW
        a                   owl:NamedIndividual ;
        rdfs:comment        "Individual representing sun exposure period in February for objects oriented towards the South West."@en ;
        eepsa:endingTime    "19:00:00" ;
        eepsa:hasMonth      2 ;
        eepsa:startingTime  "13:00:00" .

m4eepsa:OutdoorTemperature
        a                owl:NamedIndividual , owl:Class ;
        rdfs:subClassOf  eepsa:MeteorologicalProperty .

eepsa:periodAugustSE  a     owl:NamedIndividual ;
        rdfs:comment        "Individual representing sun exposure period in August for objects oriented towards the South East."@en ;
        eepsa:endingTime    "17:00:00" ;
        eepsa:hasMonth      8 ;
        eepsa:startingTime  "7:00:00" .

eepsa:OutlierCausedByDeviceLocation
        a                owl:Class ;
        rdfs:comment     "Outlier caused by the poor location of the device"@en ;
        rdfs:label       "Outlier caused by Device Location"@en ;
        rdfs:subClassOf  eepsa:Outlier ;
        rdfs:subClassOf  [ a                   owl:Restriction ;
                           owl:onProperty      eepsa:hasSolvingMethod ;
                           owl:someValuesFrom  eepsa:DeviceRelocation
                         ] .

eepsa:EastOrientedObject
        a                    owl:Class ;
        rdfs:comment         "Object oriented towards the East"@en ;
        rdfs:label           "East Oriented Object"@en ;
        rdfs:subClassOf      bim4eepsa:PhysicalObject ;
        owl:equivalentClass  [ a                   owl:Class ;
                               owl:intersectionOf  ( [ a               owl:Restriction ;
                                                       owl:hasValue    m4eepsa:eastOrientation ;
                                                       owl:onProperty  <http://purl.org/iot/vocab/m3-lite#hasDirection>
                                                     ] [ a               owl:Restriction ;
                                                         owl:hasValue    <http://es.dbpedia.org/resource/Spain> ;
                                                         owl:onProperty  wgs84_pos:location
                                                       ] )
                             ] .

eepsa:periodSeptemberNE
        a                   owl:NamedIndividual ;
        rdfs:comment        "Individual representing sun exposure period in September for objects oriented towards the North East."@en ;
        eepsa:endingTime    "13:00:00" ;
        eepsa:hasMonth      9 ;
        eepsa:startingTime  "7:00:00" .

eepsa:INSHTForSedentarySituation
        a                owl:Class ;
        rdfs:comment     "A situation that meets themal requirements defined by Spanish INSHT (Instituto Nacional de Seguridad e Higiene en el Trabajo) guidelines for sedentary workplaces."@en ;
        rdfs:label       "INSHT for Sedentary Situation"@en ;
        rdfs:subClassOf  eepsa:ComfortableThermalSituation .

bim4eepsa:WeatherStation
        rdfs:subClassOf  [ a                   owl:Restriction ;
                           owl:onProperty      eepsa:providesWeatherService ;
                           owl:someValuesFrom  eepsa:WeatherService
                         ] .

eepsa:WaterConductivity
        a                owl:Class ;
        rdfs:subClassOf  <http://purl.org/iot/vocab/m3-lite#Conductivity> .

eepsa:periodMarchNE  a      owl:NamedIndividual ;
        rdfs:comment        "Individual representing sun exposure period in March for objects oriented towards the North East."@en ;
        eepsa:endingTime    "12:00:00" ;
        eepsa:hasMonth      3 ;
        eepsa:startingTime  "7:00:00" .

wgs84_pos:lat_long  rdfs:comment  "A comma-separated representation of a latitude, longitude coordinate." ;
        rdfs:label    "lat/long" .

eepsa:NorthEastOrientedObject
        a                    owl:Class ;
        rdfs:comment         "Object oriented towards the North East"@en ;
        rdfs:label           "North East Oriented Object"@en ;
        rdfs:subClassOf      bim4eepsa:PhysicalObject ;
        rdfs:subClassOf      [ a                   owl:Class ;
                               owl:intersectionOf  ( [ a               owl:Restriction ;
                                                       owl:hasValue    eepsa:periodAprilNE ;
                                                       owl:onProperty  eepsa:hasSunExposurePeriod
                                                     ] [ a               owl:Restriction ;
                                                         owl:hasValue    eepsa:periodAugustNE ;
                                                         owl:onProperty  eepsa:hasSunExposurePeriod
                                                       ] [ a               owl:Restriction ;
                                                           owl:hasValue    eepsa:periodDecemberNE ;
                                                           owl:onProperty  eepsa:hasSunExposurePeriod
                                                         ] [ a               owl:Restriction ;
                                                             owl:hasValue    eepsa:periodFebruaryNE ;
                                                             owl:onProperty  eepsa:hasSunExposurePeriod
                                                           ] [ a               owl:Restriction ;
                                                               owl:hasValue    eepsa:periodJanuaryNE ;
                                                               owl:onProperty  eepsa:hasSunExposurePeriod
                                                             ] [ a               owl:Restriction ;
                                                                 owl:hasValue    eepsa:periodJulyNE ;
                                                                 owl:onProperty  eepsa:hasSunExposurePeriod
                                                               ] [ a               owl:Restriction ;
                                                                   owl:hasValue    eepsa:periodJuneNE ;
                                                                   owl:onProperty  eepsa:hasSunExposurePeriod
                                                                 ] [ a               owl:Restriction ;
                                                                     owl:hasValue    eepsa:periodMarchNE ;
                                                                     owl:onProperty  eepsa:hasSunExposurePeriod
                                                                   ] [ a               owl:Restriction ;
                                                                       owl:hasValue    eepsa:periodMayNE ;
                                                                       owl:onProperty  eepsa:hasSunExposurePeriod
                                                                     ] [ a               owl:Restriction ;
                                                                         owl:hasValue    eepsa:periodNovemberNE ;
                                                                         owl:onProperty  eepsa:hasSunExposurePeriod
                                                                       ] [ a               owl:Restriction ;
                                                                           owl:hasValue    eepsa:periodOctoberNE ;
                                                                           owl:onProperty  eepsa:hasSunExposurePeriod
                                                                         ] [ a               owl:Restriction ;
                                                                             owl:hasValue    eepsa:periodSeptemberNE ;
                                                                             owl:onProperty  eepsa:hasSunExposurePeriod
                                                                           ] )
                             ] ;
        owl:equivalentClass  [ a                   owl:Class ;
                               owl:intersectionOf  ( [ a               owl:Restriction ;
                                                       owl:hasValue    m4eepsa:northEastOrientation ;
                                                       owl:onProperty  <http://purl.org/iot/vocab/m3-lite#hasDirection>
                                                     ] [ a               owl:Restriction ;
                                                         owl:hasValue    <http://es.dbpedia.org/resource/Spain> ;
                                                         owl:onProperty  wgs84_pos:location
                                                       ] )
                             ] .

wgs84_pos:location  a  owl:ObjectProperty , owl:AnnotationProperty .

eepsa:OutlierCausedByDeviceError
        a                owl:Class ;
        rdfs:comment     "Outliers caused by an error on the device itself"@en ;
        rdfs:label       "Outlier caused by Device Error"@en ;
        rdfs:subClassOf  eepsa:Outlier .

[ owl:minQualifiedCardinality  "1"^^xsd:nonNegativeInteger ] .

eepsa:periodNovemberSW
        a                   owl:NamedIndividual ;
        rdfs:comment        "Individual representing sun exposure period in November for objects oriented towards the South West."@en ;
        eepsa:endingTime    "18:00:00" ;
        eepsa:hasMonth      11 ;
        eepsa:startingTime  "13:00:00" .

eepsa:MeteorologicalProperty
        a                owl:Class ;
        rdfs:comment     "Meteorological Variables that can be measured by weather stations (this means that they are outdoors. Maybe the name has to be changed)"@en ;
        rdfs:subClassOf  ssn:Property ;
        rdfs:subClassOf  [ a                   owl:Restriction ;
                           owl:onProperty      eepsa:hasDataSource ;
                           owl:someValuesFrom  eepsa:WeatherService
                         ] .

eepsa:periodMayNW  a        owl:NamedIndividual ;
        rdfs:comment        "Individual representing sun exposure period in May for objects oriented towards the North West."@en ;
        eepsa:endingTime    "22:00:00" ;
        eepsa:hasMonth      5 ;
        eepsa:startingTime  "17:00:00" .

eepsa:OutlierCausedBySolarRadiation
        a                owl:Class ;
        rdfs:comment     "An erroneous observation (e.g. temperature, illuminance) caused by direct sunlight."@en ;
        rdfs:label       "Outlier caused by Solar Radiation"@en ;
        rdfs:subClassOf  eepsa:OutlierCausedByDeviceLocation ;
        rdfs:subClassOf  [ a                   owl:Restriction ;
                           owl:onProperty      eepsa:hasSolvingMethod ;
                           owl:someValuesFrom  eepsa:DeviceShelter
                         ] .

eepsa:endingTime  a   owl:DatatypeProperty ;
        rdfs:comment  "Determines the Ending Time of a temporal entity."@en ;
        rdfs:label    "ending time"@en ;
        rdfs:range    xsd:time .

m4eepsa:southWestOrientation
        a       owl:NamedIndividual .

eepsa:SouthOrientedObject
        a                    owl:Class ;
        rdfs:comment         "Object oriented towards the South"@en ;
        rdfs:label           "South Oriented Object"@en ;
        rdfs:subClassOf      bim4eepsa:PhysicalObject ;
        owl:equivalentClass  [ a                   owl:Class ;
                               owl:intersectionOf  ( [ a               owl:Restriction ;
                                                       owl:hasValue    m4eepsa:southOrientation ;
                                                       owl:onProperty  <http://purl.org/iot/vocab/m3-lite#hasDirection>
                                                     ] [ a               owl:Restriction ;
                                                         owl:hasValue    <http://es.dbpedia.org/resource/Spain> ;
                                                         owl:onProperty  wgs84_pos:location
                                                       ] )
                             ] .

eepsa:periodAprilNW  a      owl:NamedIndividual ;
        rdfs:comment        "Individual representing sun exposure period in April for objects oriented towards the North West."@en ;
        eepsa:endingTime    "21:00:00" ;
        eepsa:hasMonth      4 ;
        eepsa:startingTime  "17:00:00" .

xsd:time  a     rdfs:Datatype .

eepsa:obsTime  a      owl:DatatypeProperty ;
        rdfs:comment  "Determines the Time (e.g. hh:mm:ss) of an observation." ;
        rdfs:label    "observation time"@en ;
        skos:example  "Example:\nmyOnto:obs1 eepsa:observationTime \"12:00:00\"."@en .

DUL:Agent  rdfs:isDefinedBy  <http://www.ontologydesignpatterns.org/ont/dul/DUL.owl> .

<http://purl.org/iot/vocab/m3-lite#ChemicalAgentAtmosphericConcentration>
        rdfs:subClassOf  eepsa:MeteorologicalProperty .

eepsa:periodMaySE  a        owl:NamedIndividual ;
        rdfs:comment        "Individual representing sun exposure period in May for objects oriented towards the South East."@en ;
        eepsa:endingTime    "17:00:00" ;
        eepsa:hasMonth      5 ;
        eepsa:startingTime  "7:00:00" .

m4eepsa:northWestOrientation
        a       owl:NamedIndividual .

eepsa:INSHTForLightSituation
        a                owl:Class ;
        rdfs:comment     "A situation that meets themal requirements defined by Spanish INSHT (Instituto Nacional de Seguridad e Higiene en el Trabajo) guidelines for light workplaces."@en ;
        rdfs:label       "INSHT for Light Situation"@en ;
        rdfs:subClassOf  eepsa:ComfortableThermalSituation .

<http://purl.org/iot/vocab/m3-lite#WindDirection>
        rdfs:subClassOf  eepsa:MeteorologicalProperty .

bibo:status  a  owl:AnnotationProperty .

eepsa:periodJulyNE  a       owl:NamedIndividual ;
        rdfs:comment        "Individual representing sun exposure period in July for objects oriented towards the North East."@en ;
        eepsa:endingTime    "14:00:00" ;
        eepsa:hasMonth      7 ;
        eepsa:startingTime  "7:00:00" .

eepsa:periodAprilSE  a      owl:NamedIndividual ;
        rdfs:comment        "Individual representing sun exposure period in April for objects oriented towards the South East."@en ;
        eepsa:endingTime    "18:00:00" ;
        eepsa:hasMonth      4 ;
        eepsa:startingTime  "7:00:00" .

eepsa:hasSolvingMethod
        a             owl:ObjectProperty ;
        rdfs:comment  "A relation between a Thing (mainly an Outlier) and a Method proposed to solve it" ;
        rdfs:label    "has solving method"@en ;
        rdfs:range    DUL:Method .

eepsa:periodJanuarySE
        a                   owl:NamedIndividual ;
        rdfs:comment        "Individual representing sun exposure period in January for objects oriented towards the South East."@en ;
        eepsa:endingTime    "18:00:00" ;
        eepsa:hasMonth      1 ;
        eepsa:startingTime  "8:00:00" .

eepsa:TemperatureSensor
        a                owl:Class ;
        rdfs:subClassOf  <http://www.w3.org/ns/sosa/Sensor> ;
        rdfs:subClassOf  [ a                   owl:Class ;
                           owl:intersectionOf  ( [ a               owl:Restriction ;
                                                   owl:hasValue    <http://purl.org/iot/vocab/m3-lite#Illuminance> ;
                                                   owl:onProperty  eepsa:susceptibleToOutliersCausedBy
                                                 ] [ a               owl:Restriction ;
                                                     owl:hasValue    <http://purl.org/iot/vocab/m3-lite#Rainfall> ;
                                                     owl:onProperty  eepsa:susceptibleToOutliersCausedBy
                                                   ] [ a               owl:Restriction ;
                                                       owl:hasValue    <http://purl.org/iot/vocab/m3-lite#SolarRadiation> ;
                                                       owl:onProperty  eepsa:susceptibleToOutliersCausedBy
                                                     ] )
                         ] .

<http://purl.org/iot/vocab/m3-lite#DewPoint>
        rdfs:subClassOf  eepsa:MeteorologicalProperty .

eepsa:NorthOrientedObject
        a                    owl:Class ;
        rdfs:comment         "Object oriented towards the North"@en ;
        rdfs:label           "North Oriented Object"@en ;
        rdfs:subClassOf      bim4eepsa:PhysicalObject ;
        owl:equivalentClass  [ a                   owl:Class ;
                               owl:intersectionOf  ( [ a               owl:Restriction ;
                                                       owl:hasValue    m4eepsa:northOrientation ;
                                                       owl:onProperty  <http://purl.org/iot/vocab/m3-lite#hasDirection>
                                                     ] [ a               owl:Restriction ;
                                                         owl:hasValue    <http://es.dbpedia.org/resource/Spain> ;
                                                         owl:onProperty  wgs84_pos:location
                                                       ] )
                             ] .

<http://purl.org/iot/vocab/m3-lite#DegreeCelsius>
        a       owl:NamedIndividual .

<http://purl.org/iot/vocab/m3-lite#AirTemperature>
        rdfs:subClassOf  eepsa:MeteorologicalProperty .

eepsa:Outlier  a         owl:Class ;
        rdfs:comment     "Observations that stand out and do not conform to the expected behaviour"@en ;
        rdfs:label       "Outlier"@en ;
        rdfs:subClassOf  <http://www.w3.org/ns/sosa/Observation> .

wgs84_pos:  rdfs:comment  "\nRecent changes to this namespace:\n$Log: wgs84_pos.rdf,v $\nRevision 1.22  2009/04/20 15:00:30  timbl\nRemove the time bits which have been deal with elsewhere eg in iCal.\n\nRevision 1.21  2009/04/20 12:52:47  timbl\ntry again\n\nRevision 1.20  2009/04/20 12:42:11  timbl\nAdd Event (edited ages ago and never checked in), and location (following discussion http://chatlogs.planetrdf.com/swig/2009-04-20#T12-36-09)\n\nRevision 1.19  2009/04/20 12:36:31  timbl\nAdd Event (edited ages ago and never checked in), and location (following discussion http://chatlogs.planetrdf.com/swig/2009-04-20#T12-36-09)\n\nRevision 1.18  2006/02/01 22:01:04  danbri\nClarified that lat and long are decimal degrees, and that alt is decimal metres about local reference ellipsoid\n\nRevision 1.17  2004/02/06 17:38:12  danbri\nFixed a bad commit screwup\n\nRevision 1.15  2003/04/19 11:24:08  danbri\nFixed the typo even more.\n\nRevision 1.14  2003/04/19 11:16:56  danbri\nfixed a typo\n\nRevision 1.13  2003/02/19 22:27:27  connolly\nrelaxed domain constraints on lat/long/alt from Point to SpatialThing\n\nRevision 1.12  2003/01/12 01:41:41  danbri\nTrying local copy of XSLT doc.\n\nRevision 1.11  2003/01/12 01:20:18  danbri\nadded a link to morten's xslt rdfs viewer.\n\nRevision 1.10  2003/01/11 18:56:49  danbri\nRemoved datatype range from lat and long properties, since they would\nhave required each occurance of the property to mention the datatype.\n\nRevision 1.9  2003/01/11 11:41:31  danbri\nAnother typo; repaired rdfs:Property to rdf:Property x4\n\nRevision 1.8  2003/01/11 11:05:02  danbri\nAdded an rdfs:range for each lat/long/alt property,\nhttp://www.w3.org/2001/XMLSchema#float\n\nRevision 1.7  2003/01/10 20:25:16  danbri\nLonger rdfs:comment for Point, trying to be Earth-centric and neutral about\ncoordinate system(s) at the same time. Feedback welcomed.\n\nRevision 1.6  2003/01/10 20:18:30  danbri\nAdded CVS log comments into the RDF/XML as an rdfs:comment property of the\nvocabulary. Note that this is not common practice (but seems both harmless\nand potentially useful).\n\n\nrevision 1.5\ndate: 2003/01/10 20:14:31;  author: danbri;  state: Exp;  lines: +16 -5\nUpdated schema:\nAdded a dc:date, added url for more info. Changed the rdfs:label of the\nnamespace from gp to geo. Added a class Point, set as the rdfs:domain of\neach property. Added XML comment on the lat_long property suggesting that\nwe might not need it (based on #rdfig commentary from implementors).\n\nrevision 1.4\ndate: 2003/01/10 20:01:07;  author: danbri;  state: Exp;  lines: +6 -5\nFixed typo; several rdfs:about attributes are now rdf:about. Thanks to MortenF in\n#rdfig for catching this error.\n\nrevision 1.3\ndate: 2003/01/10 11:59:03;  author: danbri;  state: Exp;  lines: +4 -3\nfixed buglet in vocab, added more wgs links\n\nrevision 1.2\ndate: 2003/01/10 11:01:11;  author: danbri;  state: Exp;  lines: +4 -4\nRemoved alt from the as-a-flat-string property, and switched from\nspace separated to comma separated.\n\nrevision 1.1\ndate: 2003/01/10 10:53:23;  author: danbri;  state: Exp;\nbasic geo vocab\n\n" ;
        rdfs:label      "geo" ;
        dc:date         "$Date: 2009/04/20 15:00:30 $" ;
        dc:description  "A vocabulary for representing latitude, longitude and \n altitude information in the WGS84 geodetic reference datum. \n Version $Id$. See http://www.w3.org/2003/01/geo/ for more details." ;
        dc:title        "WGS84 Geo Positioning: an RDF vocabulary" .

eepsa:periodDecemberNE
        a                   owl:NamedIndividual ;
        rdfs:comment        "Individual representing sun exposure period in December for objects oriented towards the North East."@en ;
        eepsa:endingTime    "11:00:00" ;
        eepsa:hasMonth      12 ;
        eepsa:startingTime  "8:00:00" .

m4eepsa:northOrientation
        a       owl:NamedIndividual .

foaf:name  a        owl:DatatypeProperty ;
        rdfs:range  rdfs:Literal .

eepsa:BadInsulatedSpace
        a                owl:Class ;
        rdfs:comment     "A space with bad insulation."@en ;
        rdfs:label       "Bad Insulated Space"@en ;
        rdfs:subClassOf  bot:Space ;
        rdfs:subClassOf  [ a                   owl:Class ;
                           owl:intersectionOf  ( [ a               owl:Restriction ;
                                                   owl:hasValue    m4eepsa:OutdoorRelativeHumidity ;
                                                   owl:onProperty  eepsa:isHighlyAffectedBy
                                                 ] [ a               owl:Restriction ;
                                                     owl:hasValue    m4eepsa:OutdoorTemperature ;
                                                     owl:onProperty  eepsa:isHighlyAffectedBy
                                                   ] )
                         ] .

eepsa:periodOctoberNE
        a                   owl:NamedIndividual ;
        rdfs:comment        "Individual representing sun exposure period in October for objects oriented towards the North East."@en ;
        eepsa:endingTime    "12:00:00" ;
        eepsa:hasMonth      10 ;
        eepsa:startingTime  "8:00:00" .

<http://purl.org/iot/vocab/m3-lite#AirQuality>
        rdfs:subClassOf  eepsa:MeteorologicalProperty .

eepsa:periodAugustSW  a     owl:NamedIndividual ;
        rdfs:comment        "Individual representing sun exposure period in August for objects oriented towards the South West."@en ;
        eepsa:endingTime    "21:00:00" ;
        eepsa:hasMonth      8 ;
        eepsa:startingTime  "14:00:00" .

[ owl:minQualifiedCardinality  "1"^^xsd:nonNegativeInteger ] .

eepsa:NaturallyEnlightenedSpace
        a                    owl:Class ;
        rdfs:comment         "A space enlightened with a source of light from the exterior (and not enlightened by a source of light inside the space)."@en ;
        rdfs:label           "Naturally Enlightened Space"@en ;
        rdfs:subClassOf      bot:Space ;
        rdfs:subClassOf      [ a                   owl:Class ;
                               owl:intersectionOf  ( [ a               owl:Restriction ;
                                                       owl:hasValue    <http://purl.org/iot/vocab/m3-lite#CloudCover> ;
                                                       owl:onProperty  eepsa:isHighlyAffectedBy
                                                     ] [ a               owl:Restriction ;
                                                         owl:hasValue    <http://purl.org/iot/vocab/m3-lite#SolarRadiation> ;
                                                         owl:onProperty  eepsa:isHighlyAffectedBy
                                                       ] [ a               owl:Restriction ;
                                                           owl:hasValue    <http://purl.org/iot/vocab/m3-lite#SunPositionDirection> ;
                                                           owl:onProperty  eepsa:isHighlyAffectedBy
                                                         ] [ a               owl:Restriction ;
                                                             owl:hasValue    <http://purl.org/iot/vocab/m3-lite#SunPositionElevation> ;
                                                             owl:onProperty  eepsa:isHighlyAffectedBy
                                                           ] )
                             ] ;
        owl:equivalentClass  [ a                   owl:Class ;
                               owl:intersectionOf  ( bot:Space [ a            owl:Class ;
                                                                 owl:unionOf  ( [ a                   owl:Restriction ;
                                                                                  owl:onProperty      bot:containsElement ;
                                                                                  owl:someValuesFrom  bim4eepsa:ExternalWindow
                                                                                ] [ a                   owl:Restriction ;
                                                                                    owl:onProperty      bot:containsElement ;
                                                                                    owl:someValuesFrom  bim4eepsa:Skylight
                                                                                  ] )
                                                               ] )
                             ] .

eepsa:periodSeptemberNW
        a                   owl:NamedIndividual ;
        rdfs:comment        "Individual representing sun exposure period in September for objects oriented towards the North West."@en ;
        eepsa:endingTime    "21:00:00" ;
        eepsa:hasMonth      9 ;
        eepsa:startingTime  "18:00:00" .

eepsa:periodJuneNE  a       owl:NamedIndividual ;
        rdfs:comment        "Individual representing sun exposure period in June for objects oriented towards the North East."@en ;
        eepsa:endingTime    "14:00:00" ;
        eepsa:hasMonth      6 ;
        eepsa:startingTime  "7:00:00" .

eepsa:hasSunExposurePeriod
        a             owl:ObjectProperty ;
        rdfs:comment  "Determines the period to which it is exposed to sun" ;
        rdfs:label    "has sun exposure period"@en .

<http://purl.org/iot/vocab/m3-lite#AirPollution>
        rdfs:subClassOf  eepsa:MeteorologicalProperty .

dc:date  a      owl:AnnotationProperty .

eepsa:periodSeptemberSE
        a                   owl:NamedIndividual ;
        rdfs:comment        "Individual representing sun exposure period in September for objects oriented towards the South East."@en ;
        eepsa:endingTime    "17:00:00" ;
        eepsa:hasMonth      9 ;
        eepsa:startingTime  "7:00:00" .

eepsa:DeviceRelocation
        a                owl:Class ;
        rdfs:comment     "A method that consists in placing the sensing device in an adequate location. Following guides can be followed:\n\nhttps://www.rmets.org/sites/default/files/pdf/guidelines/aws-guide.pdf\n\nhttp://weatherfaqs.org.uk/node/124\n\nhttp://www.conservationphysics.org/datalog/datlog6.php\n\nhttp://www.weatherstations.co.uk/gooddata.htm"@en ;
        rdfs:label       "Device Relocation"@en ;
        rdfs:subClassOf  DUL:Method .

eepsa:BelowGroundLevelSpace
        a                owl:Class ;
        rdfs:comment     "A space located in a storey below ground."@en ;
        rdfs:label       "Below Ground Level Space"@en ;
        rdfs:subClassOf  bot:Space .

eepsa:capturedIn  a             owl:ObjectProperty ;
        rdfs:comment            "Relation between an Observation and the Spatial Thing (Building, Space) where it has been captured"@en ;
        rdfs:label              "captured in"@en ;
        owl:inverseOf           eepsa:captures ;
        owl:propertyChainAxiom  ( bot:containsElement [ owl:inverseOf
                          <http://www.w3.org/ns/sosa/isObservedBy> ] ) .

eepsa:SouthWestOrientedObject
        a                    owl:Class ;
        rdfs:comment         "Object oriented towards the South West"@en ;
        rdfs:label           "South West Oriented Object"@en ;
        rdfs:subClassOf      bim4eepsa:PhysicalObject ;
        rdfs:subClassOf      [ a                   owl:Class ;
                               owl:intersectionOf  ( [ a               owl:Restriction ;
                                                       owl:hasValue    eepsa:periodAprilSW ;
                                                       owl:onProperty  eepsa:hasSunExposurePeriod
                                                     ] [ a               owl:Restriction ;
                                                         owl:hasValue    eepsa:periodAugustSW ;
                                                         owl:onProperty  eepsa:hasSunExposurePeriod
                                                       ] [ a               owl:Restriction ;
                                                           owl:hasValue    eepsa:periodDecemberSW ;
                                                           owl:onProperty  eepsa:hasSunExposurePeriod
                                                         ] [ a               owl:Restriction ;
                                                             owl:hasValue    eepsa:periodFebruarySW ;
                                                             owl:onProperty  eepsa:hasSunExposurePeriod
                                                           ] [ a               owl:Restriction ;
                                                               owl:hasValue    eepsa:periodJanuarySW ;
                                                               owl:onProperty  eepsa:hasSunExposurePeriod
                                                             ] [ a               owl:Restriction ;
                                                                 owl:hasValue    eepsa:periodJulySW ;
                                                                 owl:onProperty  eepsa:hasSunExposurePeriod
                                                               ] [ a               owl:Restriction ;
                                                                   owl:hasValue    eepsa:periodJuneSW ;
                                                                   owl:onProperty  eepsa:hasSunExposurePeriod
                                                                 ] [ a               owl:Restriction ;
                                                                     owl:hasValue    eepsa:periodMarchSW ;
                                                                     owl:onProperty  eepsa:hasSunExposurePeriod
                                                                   ] [ a               owl:Restriction ;
                                                                       owl:hasValue    eepsa:periodMaySW ;
                                                                       owl:onProperty  eepsa:hasSunExposurePeriod
                                                                     ] [ a               owl:Restriction ;
                                                                         owl:hasValue    eepsa:periodNovemberSW ;
                                                                         owl:onProperty  eepsa:hasSunExposurePeriod
                                                                       ] [ a               owl:Restriction ;
                                                                           owl:hasValue    eepsa:periodOctoberSW ;
                                                                           owl:onProperty  eepsa:hasSunExposurePeriod
                                                                         ] [ a               owl:Restriction ;
                                                                             owl:hasValue    eepsa:periodSeptemberSW ;
                                                                             owl:onProperty  eepsa:hasSunExposurePeriod
                                                                           ] )
                             ] ;
        owl:equivalentClass  [ a                   owl:Class ;
                               owl:intersectionOf  ( [ a               owl:Restriction ;
                                                       owl:hasValue    m4eepsa:southWestOrientation ;
                                                       owl:onProperty  <http://purl.org/iot/vocab/m3-lite#hasDirection>
                                                     ] [ a               owl:Restriction ;
                                                         owl:hasValue    <http://es.dbpedia.org/resource/Spain> ;
                                                         owl:onProperty  wgs84_pos:location
                                                       ] )
                             ] .

<http://purl.org/iot/vocab/m3-lite#Thermometer>
        owl:equivalentClass  eepsa:TemperatureSensor .

eepsa:periodMarchNW  a      owl:NamedIndividual ;
        rdfs:comment        "Individual representing sun exposure period in March for objects oriented towards the North West."@en ;
        eepsa:endingTime    "20:00:00" ;
        eepsa:hasMonth      3 ;
        eepsa:startingTime  "17:00:00" .

eepsa:periodFebruaryNE
        a                   owl:NamedIndividual ;
        rdfs:comment        "Individual representing sun exposure period in February for objects oriented towards the North East."@en ;
        eepsa:endingTime    "11:00:00" ;
        eepsa:hasMonth      2 ;
        eepsa:startingTime  "8:00:00" .

m4eepsa:eastOrientation
        a       owl:NamedIndividual .

<http://qudt.org/schema/qudt#unit>
        a       owl:ObjectProperty .

eepsa:periodMarchSE  a      owl:NamedIndividual ;
        rdfs:comment        "Individual representing sun exposure period in March for objects oriented towards the South East."@en ;
        eepsa:endingTime    "18:00:00" ;
        eepsa:hasMonth      3 ;
        eepsa:startingTime  "7:00:00" .

wgs84_pos:alt  a      owl:AnnotationProperty ;
        rdfs:comment  "The WGS84 altitude of a SpatialThing (decimal meters \nabove the local reference ellipsoid)." ;
        rdfs:domain   wgs84_pos:SpatialThing ;
        rdfs:label    "altitude" .

eepsa:HSESituation  a    owl:Class ;
        rdfs:comment     "A situation that meets themal requirements defined by UK's HSE (Health and Safety Execution) guidelines."@en ;
        rdfs:label       "HSE Situation"@en ;
        rdfs:subClassOf  eepsa:ComfortableThermalSituation .

wgs84_pos:lat  a      owl:AnnotationProperty ;
        rdfs:comment  "The WGS84 latitude of a SpatialThing (decimal degrees)." ;
        rdfs:label    "latitude" .

wgs84_pos:long  a     owl:AnnotationProperty ;
        rdfs:comment  "The WGS84 longitude of a SpatialThing (decimal degrees)." ;
        rdfs:label    "longitude" .

eepsa:OutlierCausedByRain
        a                owl:Class ;
        rdfs:comment     "An erroneous observation caused by rainfall."@en ;
        rdfs:label       "Outlier caused by Rain"@en ;
        rdfs:subClassOf  eepsa:OutlierCausedByDeviceLocation ;
        rdfs:subClassOf  [ a                   owl:Restriction ;
                           owl:onProperty      eepsa:hasSolvingMethod ;
                           owl:someValuesFrom  eepsa:DeviceShelter
                         ] .

eepsa:model  a        owl:DatatypeProperty ;
        rdfs:comment  "Model of a Thing (normally a Physical Object)" ;
        rdfs:label    "model"@en ;
        rdfs:range    xsd:string ;
        skos:example  "Example:\nmyOnto:Vehicle1 eepsa:model xsd:string(\"Golf GTI\")."@en .

m4eepsa:IndoorTemperature
        a       owl:NamedIndividual .

eepsa:periodMaySW  a        owl:NamedIndividual ;
        rdfs:comment        "Individual representing sun exposure period in May for objects oriented towards the South West."@en ;
        eepsa:endingTime    "21:00:00" ;
        eepsa:hasMonth      5 ;
        eepsa:startingTime  "14:00:00" .

<https://w3id.org/eepsa>
        a                              owl:Ontology ;
        rdfs:comment                   "The ontology is documented in:\n\nIker Esnaola-Gonzalez, Jess Bermdez, Izaskun Fernandez, Aitor Arnaiz, (2017) Semantic Prediction Assistant Approach applied to Energy Efficiency in Tertiary Buildings http://www.semantic-web-journal.net/content/semantic-prediction-assistant-approach-applied-energy-efficiency-tertiary-buildings-0"^^xsd:string , "Information about changes compared to version 1.2\n*********************************************************\n\tThe classes and properties related to the building modelling (imported from bim4EEPSA) are now described using the BOT Ontology.\n\tThe f4EEPSA (Forecasting for EEPSA) module is now imported."^^xsd:string ;
        dc:publisher                   "IK4-TEKNIKER (http://www.tekniker.es)" ;
        dc:title                       "EEPSA (Energy Efficiency Prediction Semantic Assistant) Ontology" ;
        terms:created                  "2016-02-20" ;
        terms:creator                  "Iker Esnaola-Gonzalez <mailto:iker.esnaola@tekniker.es>\nJess Bermdez <mailto:jesus.bermudez@ehu.eus>"@en ;
        terms:issued                   "2017-07-21" ;
        terms:license                  "This work is licensed under the Creative Commons Attribution-NonCommercial 4.0 International License. To view a copy of this license, visit http://creativecommons.org/licenses/by-nc/4.0/."@en ;
        terms:modified                 "2018-01-02"^^xsd:string ;
        bibo:status                    "Work in progress"@en ;
        vann:preferredNamespacePrefix  "eepsa" ;
        owl:imports                    <https://w3id.org/bim4eepsa> , <https://w3id.org/forecasting4eepsa> , <http://www.w3.org/2006/time> , <https://w3id.org/measurements4eepsa> , ssn: ;
        owl:versionIRI                 <https://raw.githubusercontent.com/iesnaola/eepsa/master/eepsa-1.3> ;
        owl:versionInfo                1.3 .

eepsa:periodJulyNW  a       owl:NamedIndividual ;
        rdfs:comment        "Individual representing sun exposure period in July for objects oriented towards the North West."@en ;
        eepsa:endingTime    "22:00:00" ;
        eepsa:hasMonth      7 ;
        eepsa:startingTime  "16:00:00" .

eepsa:periodAprilSW  a      owl:NamedIndividual ;
        rdfs:comment        "Individual representing sun exposure period in April for objects oriented towards the South West."@en ;
        eepsa:endingTime    "21:00:00" ;
        eepsa:hasMonth      4 ;
        eepsa:startingTime  "14:00:00" .

<http://purl.org/iot/vocab/m3-lite#SunPositionDirection>
        a                owl:NamedIndividual ;
        rdfs:subClassOf  eepsa:MeteorologicalProperty .

eepsa:susceptibleToOutliersCausedBy
        a             owl:ObjectProperty ;
        rdfs:comment  "Determines the cause that makes a sensing devices susceptible to suffer from Outliers."@en ;
        rdfs:label    "susceptible to outliers caused by"@en .

eepsa:WeatherService  a  owl:Class ;
        rdfs:label  "Weather Service"@en .

[ owl:minQualifiedCardinality  "1"^^xsd:nonNegativeInteger ] .

foaf:based_near  a  owl:AnnotationProperty .

eepsa:periodJanuarySW
        a                   owl:NamedIndividual ;
        rdfs:comment        "Individual representing sun exposure period in January for objects oriented towards the South West."@en ;
        eepsa:endingTime    "18:00:00" ;
        eepsa:hasMonth      1 ;
        eepsa:startingTime  "12:00:00" .

eepsa:periodJulySE  a       owl:NamedIndividual ;
        rdfs:comment        "Individual representing sun exposure period in July for objects oriented towards the South East."@en ;
        eepsa:endingTime    "17:00:00" ;
        eepsa:hasMonth      7 ;
        eepsa:startingTime  "7:00:00" .

m4eepsa:northEastOrientation
        a       owl:NamedIndividual .

eepsa:SouthEastOrientedObject
        a                    owl:Class ;
        rdfs:comment         "Object oriented towards the South East"@en ;
        rdfs:label           "South East Oriented Object"@en ;
        rdfs:subClassOf      bim4eepsa:PhysicalObject ;
        rdfs:subClassOf      [ a                   owl:Class ;
                               owl:intersectionOf  ( [ a               owl:Restriction ;
                                                       owl:hasValue    eepsa:periodAprilSE ;
                                                       owl:onProperty  eepsa:hasSunExposurePeriod
                                                     ] [ a               owl:Restriction ;
                                                         owl:hasValue    eepsa:periodAugustSE ;
                                                         owl:onProperty  eepsa:hasSunExposurePeriod
                                                       ] [ a               owl:Restriction ;
                                                           owl:hasValue    eepsa:periodDecemberSE ;
                                                           owl:onProperty  eepsa:hasSunExposurePeriod
                                                         ] [ a               owl:Restriction ;
                                                             owl:hasValue    eepsa:periodFebruarySE ;
                                                             owl:onProperty  eepsa:hasSunExposurePeriod
                                                           ] [ a               owl:Restriction ;
                                                               owl:hasValue    eepsa:periodJanuarySE ;
                                                               owl:onProperty  eepsa:hasSunExposurePeriod
                                                             ] [ a               owl:Restriction ;
                                                                 owl:hasValue    eepsa:periodJulySE ;
                                                                 owl:onProperty  eepsa:hasSunExposurePeriod
                                                               ] [ a               owl:Restriction ;
                                                                   owl:hasValue    eepsa:periodJuneSE ;
                                                                   owl:onProperty  eepsa:hasSunExposurePeriod
                                                                 ] [ a               owl:Restriction ;
                                                                     owl:hasValue    eepsa:periodMarchSE ;
                                                                     owl:onProperty  eepsa:hasSunExposurePeriod
                                                                   ] [ a               owl:Restriction ;
                                                                       owl:hasValue    eepsa:periodMaySE ;
                                                                       owl:onProperty  eepsa:hasSunExposurePeriod
                                                                     ] [ a               owl:Restriction ;
                                                                         owl:hasValue    eepsa:periodNovemberSE ;
                                                                         owl:onProperty  eepsa:hasSunExposurePeriod
                                                                       ] [ a               owl:Restriction ;
                                                                           owl:hasValue    eepsa:periodOctoberSE ;
                                                                           owl:onProperty  eepsa:hasSunExposurePeriod
                                                                         ] [ a               owl:Restriction ;
                                                                             owl:hasValue    eepsa:periodSeptemberSE ;
                                                                             owl:onProperty  eepsa:hasSunExposurePeriod
                                                                           ] )
                             ] ;
        owl:equivalentClass  [ a                   owl:Class ;
                               owl:intersectionOf  ( [ a               owl:Restriction ;
                                                       owl:hasValue    m4eepsa:southEastOrientation ;
                                                       owl:onProperty  <http://purl.org/iot/vocab/m3-lite#hasDirection>
                                                     ] [ a               owl:Restriction ;
                                                         owl:hasValue    <http://es.dbpedia.org/resource/Spain> ;
                                                         owl:onProperty  wgs84_pos:location
                                                       ] )
                             ] .

eepsa:periodNovemberNE
        a                   owl:NamedIndividual ;
        rdfs:comment        "Individual representing sun exposure period in November for objects oriented towards the North East."@en ;
        eepsa:endingTime    "11:00:00" ;
        eepsa:hasMonth      11 ;
        eepsa:startingTime  "8:00:00" .

<http://purl.org/iot/vocab/m3-lite#SunPositionElevation>
        a                owl:NamedIndividual ;
        rdfs:subClassOf  eepsa:MeteorologicalProperty .

eepsa:OutlierCausedByHVAC
        a                owl:Class ;
        rdfs:comment     "An erroneous observation (e.g. temperature) caused by its placement next to an activated HVAC system (whether it was heating or cooling)"@en ;
        rdfs:label       "Outlier caused by HVAC"@en ;
        rdfs:subClassOf  eepsa:OutlierCausedByDeviceLocation .

m4eepsa:IndoorRelativeHumidity
        a       owl:NamedIndividual .

iot-lite:relativeLocation
        a                 owl:AnnotationProperty ;
        rdfs:comment      "A location not provided by geo-coordinates (i.e. building A, city of Aarhus)."@en ;
        rdfs:domain       wgs84_pos:Point ;
        rdfs:isDefinedBy  <http://purl.oclc.org/NET/UNIS/fiware/iot-lite#> .

eepsa:AdjacentToOutdoorSpace
        a                    owl:Class ;
        rdfs:comment         "A space in contact with the exterior by means of at least one building element."@en ;
        rdfs:label           "Adjacent to Outdoor Space"@en ;
        rdfs:subClassOf      bot:Space ;
        rdfs:subClassOf      [ a                   owl:Class ;
                               owl:intersectionOf  ( [ a               owl:Restriction ;
                                                       owl:hasValue    <http://purl.org/iot/vocab/m3-lite#CloudCover> ;
                                                       owl:onProperty  eepsa:isAffectedBy
                                                     ] [ a               owl:Restriction ;
                                                         owl:hasValue    <http://purl.org/iot/vocab/m3-lite#SolarRadiation> ;
                                                         owl:onProperty  eepsa:isAffectedBy
                                                       ] [ a               owl:Restriction ;
                                                           owl:hasValue    <http://purl.org/iot/vocab/m3-lite#SunPositionDirection> ;
                                                           owl:onProperty  eepsa:isAffectedBy
                                                         ] [ a               owl:Restriction ;
                                                             owl:hasValue    <http://purl.org/iot/vocab/m3-lite#SunPositionElevation> ;
                                                             owl:onProperty  eepsa:isAffectedBy
                                                           ] [ a               owl:Restriction ;
                                                               owl:hasValue    <http://purl.org/iot/vocab/m3-lite#WindSpeed> ;
                                                               owl:onProperty  eepsa:isAffectedBy
                                                             ] [ a               owl:Restriction ;
                                                                 owl:hasValue    m4eepsa:OutdoorRelativeHumidity ;
                                                                 owl:onProperty  eepsa:isAffectedBy
                                                               ] [ a               owl:Restriction ;
                                                                   owl:hasValue    m4eepsa:OutdoorTemperature ;
                                                                   owl:onProperty  eepsa:isAffectedBy
                                                                 ] )
                             ] ;
        owl:equivalentClass  [ a                   owl:Class ;
                               owl:intersectionOf  ( bot:Space [ a                   owl:Restriction ;
                                                                 owl:onProperty      bot:containsElement ;
                                                                 owl:someValuesFrom  bim4eepsa:ExternalBuildingElement
                                                               ] )
                             ] .

eepsa:DeviceReplacement
        a                owl:Class ;
        rdfs:comment     "A method that consists in replacing the sensing device for another one."@en ;
        rdfs:label       "Device Replacement"@en ;
        rdfs:subClassOf  DUL:Method .

<http://purl.org/iot/vocab/m3-lite#HumiditySensor>
        rdfs:subClassOf  [ a               owl:Restriction ;
                           owl:hasValue    <http://purl.org/iot/vocab/m3-lite#Rainfall> ;
                           owl:onProperty  eepsa:susceptibleToOutliersCausedBy
                         ] .

<http://es.dbpedia.org/resource/Spain>
        a       owl:NamedIndividual .

<http://purl.org/iot/vocab/m3-lite#SolarRadiation>
        a                owl:NamedIndividual ;
        rdfs:subClassOf  eepsa:MeteorologicalProperty .

eepsa:periodDecemberSE
        a                   owl:NamedIndividual ;
        rdfs:comment        "Individual representing sun exposure period in December for objects oriented towards the South East."@en ;
        eepsa:endingTime    "18:00:00" ;
        eepsa:hasMonth      12 ;
        eepsa:startingTime  "8:00:00" .

eepsa:OutlierCausedByDeviceLowBattery
        a                owl:Class ;
        rdfs:comment     "An erroneous observation caused by the low battery of the device."@en ;
        rdfs:label       "Outlier caused by Device Low Battery"@en ;
        rdfs:subClassOf  eepsa:OutlierCausedByDeviceError .

<http://purl.org/iot/vocab/m3-lite#WindSpeed>
        a                owl:NamedIndividual ;
        rdfs:subClassOf  eepsa:MeteorologicalProperty .

[ owl:minQualifiedCardinality  "1"^^xsd:nonNegativeInteger ] .

eepsa:RITESituation  a   owl:Class ;
        rdfs:comment     "A situation that meets themal requirements defined by Spanish RITE (Reglamento de Instalaciones Trmicas en los Edificios) guidelines."@en ;
        rdfs:label       "RITE Situation"@en ;
        rdfs:subClassOf  eepsa:ComfortableThermalSituation .

eepsa:periodOctoberNW
        a                   owl:NamedIndividual ;
        rdfs:comment        "Individual representing sun exposure period in October for objects oriented towards the North West."@en ;
        eepsa:endingTime    "20:00:00" ;
        eepsa:hasMonth      10 ;
        eepsa:startingTime  "18:00:00" .

bim4eepsa:ExternalWall
        rdfs:label  "External wall"@en .

<http://purl.org/iot/vocab/m3-lite#Illuminance>
        a                owl:NamedIndividual ;
        rdfs:subClassOf  eepsa:MeteorologicalProperty .

eepsa:captures  a     owl:ObjectProperty ;
        rdfs:comment  "Relation between a Spatial Thing (Building, Space) and the Observation that has been captured"@en ;
        rdfs:label    "captures"@en .

eepsa:periodJuneNW  a       owl:NamedIndividual ;
        rdfs:comment        "Individual representing sun exposure period in June for objects oriented towards the North West."@en ;
        eepsa:endingTime    "22:00:00" ;
        eepsa:hasMonth      6 ;
        eepsa:startingTime  "16:00:00" .

eepsa:periodOctoberSE
        a                   owl:NamedIndividual ;
        rdfs:comment        "Individual representing sun exposure period in October for objects oriented towards the South East."@en ;
        eepsa:endingTime    "18:00:00" ;
        eepsa:hasMonth      10 ;
        eepsa:startingTime  "8:00:00" .

dc:description  a  owl:AnnotationProperty .

<http://purl.org/iot/vocab/m3-lite#Rainfall>
        a                owl:NamedIndividual ;
        rdfs:subClassOf  eepsa:MeteorologicalProperty .

foaf:depiction  a  owl:AnnotationProperty .

eepsa:periodSeptemberSW
        a                   owl:NamedIndividual ;
        rdfs:comment        "Individual representing sun exposure period in September for objects oriented towards the South West."@en ;
        eepsa:endingTime    "21:00:00" ;
        eepsa:hasMonth      9 ;
        eepsa:startingTime  "14:00:00" .

eepsa:periodJuneSE  a       owl:NamedIndividual ;
        rdfs:comment        "Individual representing sun exposure period in June for objects oriented towards the South East."@en ;
        eepsa:endingTime    "17:00:00" ;
        eepsa:hasMonth      6 ;
        eepsa:startingTime  "7:00:00" .

eepsa:manufacturedBy  a  owl:DatatypeProperty ;
        rdfs:comment  "Determines the manufacturer of a Thing"@en ;
        rdfs:label    "manufactured by"@en ;
        rdfs:range    xsd:string ;
        skos:example  "Example:\nmyOnto:Vehicle1 eepsa:manufacturedBy xsd:string(\"Volkswagen\")."@en .

eepsa:DeviceShelter  a   owl:Class ;
        rdfs:comment     "A method that consists in covering the sensing device adequately to avoid erroneous observations. For example, Stevenson Screen to shield the sensing device against direct precipitation or direct sunlight."@en ;
        rdfs:label       "Device Shelter"@en ;
        rdfs:subClassOf  DUL:Method .

eepsa:WeatherReport  a   owl:Class ;
        rdfs:comment     "A summary of weather conditions for an area"@en ;
        rdfs:label       "Weather Report"@en ;
        rdfs:subClassOf  eepsa:WeatherService .

m4eepsa:OutdoorRelativeHumidity
        a                owl:NamedIndividual , owl:Class ;
        rdfs:subClassOf  eepsa:MeteorologicalProperty .

[ owl:minQualifiedCardinality  "1"^^xsd:nonNegativeInteger ] .

eepsa:periodFebruaryNW
        a                   owl:NamedIndividual ;
        rdfs:comment        "Individual representing sun exposure period in February for objects oriented towards the North West."@en ;
        eepsa:endingTime    "19:00:00" ;
        eepsa:hasMonth      2 ;
        eepsa:startingTime  "18:00:00" .
