@prefix schema: <http://schema.org/> .
@prefix dc: <http://purl.org/dc/terms/> .
@prefix rdfs: <http://www.w3.org/2000/01/rdf-schema#> .
@prefix rdf: <http://www.w3.org/1999/02/22-rdf-syntax-ns#> .

schema:APIReference a rdfs:Class ;
	rdfs:label "APIReference" ;
	rdfs:comment "Reference documentation for application programming interfaces (APIs)." ;
	rdfs:subClassOf schema:TechArticle .

schema:AboutPage a rdfs:Class ;
	rdfs:label "AboutPage" ;
	rdfs:comment "Web page type: About page." ;
	rdfs:subClassOf schema:WebPage .

schema:AcceptAction a rdfs:Class ;
	rdfs:label "AcceptAction" ;
	rdfs:comment "The act of committing to/adopting an object.<p>Related actions:</p><ul><li><a href=\"http://schema.org/RejectAction\">RejectAction</a>: The antagonym of AcceptAction.</li></ul>" ;
	rdfs:subClassOf schema:AllocateAction .

schema:AccountingService a rdfs:Class ;
	rdfs:label "AccountingService" ;
	rdfs:comment "Accountancy business." ;
	rdfs:subClassOf schema:FinancialService , schema:ProfessionalService .

schema:AchieveAction a rdfs:Class ;
	rdfs:label "AchieveAction" ;
	rdfs:comment "The act of accomplishing something via     previous efforts. It is an instantaneous action rather than an ongoing     process." ;
	rdfs:subClassOf schema:Action .

schema:Action a rdfs:Class ;
	rdfs:label "Action" ;
	rdfs:comment "An action performed by a direct agent and indirect     participants upon a direct object. Optionally happens at a location     with the help of an inanimate instrument. The execution of the action     may produce a result. Specific action sub-type documentation specifies     the exact expectation of each argument/role." ;
	rdfs:subClassOf schema:Thing .

schema:AddAction a rdfs:Class ;
	rdfs:label "AddAction" ;
	rdfs:comment "The act of editing by adding an object to a collection." ;
	rdfs:subClassOf schema:UpdateAction .

schema:AdministrativeArea a rdfs:Class ;
	rdfs:label "AdministrativeArea" ;
	rdfs:comment "A geographical region under the jurisdiction of a particular government." ;
	rdfs:subClassOf schema:Place .

schema:AdultEntertainment a rdfs:Class ;
	rdfs:label "AdultEntertainment" ;
	rdfs:comment "An adult entertainment establishment." ;
	rdfs:subClassOf schema:EntertainmentBusiness .

schema:AggregateOffer a rdfs:Class ;
	rdfs:label "AggregateOffer" ;
	rdfs:comment "When a single product that has different offers (for example, the same pair of shoes is offered by different merchants), then AggregateOffer can be used." ;
	rdfs:subClassOf schema:Offer .

schema:AggregateRating a rdfs:Class ;
	rdfs:label "AggregateRating" ;
	rdfs:comment "The average rating based on multiple ratings or reviews." ;
	rdfs:subClassOf schema:Rating .

schema:AgreeAction a rdfs:Class ;
	rdfs:label "AgreeAction" ;
	rdfs:comment "The act of expressing a consistency of opinion with the object. An agent agrees to/about an object (a proposition, topic or theme) with participants." ;
	rdfs:subClassOf schema:ReactAction .

schema:Airport a rdfs:Class ;
	rdfs:label "Airport" ;
	rdfs:comment "An airport." ;
	rdfs:subClassOf schema:CivicStructure .

schema:AlignmentObject a rdfs:Class ;
	rdfs:label "AlignmentObject" ;
	dc:source <http://www.w3.org/wiki/WebSchemas/SchemaDotOrgSources#source_LRMIClass> ;
	rdfs:comment "An intangible item that describes an alignment between a learning resource and a node in an educational framework." ;
	rdfs:subClassOf schema:Intangible .

schema:AllocateAction a rdfs:Class ;
	rdfs:label "AllocateAction" ;
	rdfs:comment "The act of organizing tasks/objects/events by associating resources to it." ;
	rdfs:subClassOf schema:OrganizeAction .

schema:AmusementPark a rdfs:Class ;
	rdfs:label "AmusementPark" ;
	rdfs:comment "An amusement park." ;
	rdfs:subClassOf schema:EntertainmentBusiness .

schema:AnatomicalStructure a rdfs:Class ;
	rdfs:label "AnatomicalStructure" ;
	dc:source <http://www.w3.org/wiki/WebSchemas/SchemaDotOrgSources#source_WikiDoc> ;
	rdfs:comment "Any part of the human body, typically a component of an anatomical system. Organs, tissues, and cells are all anatomical structures." ;
	rdfs:subClassOf schema:MedicalEntity .

schema:AnatomicalSystem a rdfs:Class ;
	rdfs:label "AnatomicalSystem" ;
	dc:source <http://www.w3.org/wiki/WebSchemas/SchemaDotOrgSources#source_WikiDoc> ;
	rdfs:comment "An anatomical system is a group of anatomical structures that work together to perform a certain task. Anatomical systems, such as organ systems, are one organizing principle of anatomy, and can includes circulatory, digestive, endocrine, integumentary, immune, lymphatic, muscular, nervous, reproductive, respiratory, skeletal, urinary, vestibular, and other systems." ;
	rdfs:subClassOf schema:MedicalEntity .

schema:AnimalShelter a rdfs:Class ;
	rdfs:label "AnimalShelter" ;
	rdfs:comment "Animal shelter." ;
	rdfs:subClassOf schema:LocalBusiness .

schema:ApartmentComplex a rdfs:Class ;
	rdfs:label "ApartmentComplex" ;
	rdfs:comment "Residence type: Apartment complex." ;
	rdfs:subClassOf schema:Residence .

schema:AppendAction a rdfs:Class ;
	rdfs:label "AppendAction" ;
	rdfs:comment "The act of inserting at the end if an ordered collection." ;
	rdfs:subClassOf schema:InsertAction .

schema:ApplyAction a rdfs:Class ;
	rdfs:label "ApplyAction" ;
	rdfs:comment "The act of registering to an organization/service without the guarantee to receive it. NOTE(goto): should this be under InteractAction instead?<p>Related actions:</p><ul><li><a href=\"http://schema.org/RegisterAction\">RegisterAction</a>: Unlike RegisterAction, ApplyAction has no guarantees that the application will be accepted.</li></ul>" ;
	rdfs:subClassOf schema:OrganizeAction .

schema:ApprovedIndication a rdfs:Class ;
	rdfs:label "ApprovedIndication" ;
	dc:source <http://www.w3.org/wiki/WebSchemas/SchemaDotOrgSources#source_WikiDoc> ;
	rdfs:comment "An indication for a medical therapy that has been formally specified or approved by a regulatory body that regulates use of the therapy; for example, the US FDA approves indications for most drugs in the US." ;
	rdfs:subClassOf schema:MedicalIndication .

schema:Aquarium a rdfs:Class ;
	rdfs:label "Aquarium" ;
	rdfs:comment "Aquarium." ;
	rdfs:subClassOf schema:CivicStructure .

schema:ArriveAction a rdfs:Class ;
	rdfs:label "ArriveAction" ;
	rdfs:comment "The act of arriving at a place. An agent arrives at a destination from an fromLocation, optionally with participants." ;
	rdfs:subClassOf schema:MoveAction .

schema:ArtGallery a rdfs:Class ;
	rdfs:label "ArtGallery" ;
	rdfs:comment "An art gallery." ;
	rdfs:subClassOf schema:EntertainmentBusiness .

schema:Artery a rdfs:Class ;
	rdfs:label "Artery" ;
	dc:source <http://www.w3.org/wiki/WebSchemas/SchemaDotOrgSources#source_WikiDoc> ;
	rdfs:comment "A type of blood vessel that specifically carries blood away from the heart." ;
	rdfs:subClassOf schema:Vessel .

schema:Article a rdfs:Class ;
	rdfs:label "Article" ;
	dc:source <http://www.w3.org/wiki/WebSchemas/SchemaDotOrgSources#source_rNews> ;
	rdfs:comment "An article, such as a news article or piece of investigative report. Newspapers and magazines have articles of many different types and this is intended to cover them all." ;
	rdfs:subClassOf schema:CreativeWork .

schema:AskAction a rdfs:Class ;
	rdfs:label "AskAction" ;
	rdfs:comment "The act of posing a question / favor to someone.<p>Related actions:</p><ul><li><a href=\"http://schema.org/ReplyAction\">ReplyAction</a>: Appears generally as a response to AskAction.</li></ul>" ;
	rdfs:subClassOf schema:CommunicateAction .

schema:AssessAction a rdfs:Class ;
	rdfs:label "AssessAction" ;
	rdfs:comment "The act of forming one's opinion, reaction or sentiment." ;
	rdfs:subClassOf schema:Action .

schema:AssignAction a rdfs:Class ;
	rdfs:label "AssignAction" ;
	rdfs:comment "The act of allocating an action/event/task to some destination (someone or something)." ;
	rdfs:subClassOf schema:AllocateAction .

schema:Attorney a rdfs:Class ;
	rdfs:label "Attorney" ;
	rdfs:comment "Professional service: Attorney." ;
	rdfs:subClassOf schema:ProfessionalService .

schema:Audience a rdfs:Class ;
	rdfs:label "Audience" ;
	rdfs:comment "Intended audience for an item, i.e. the group for whom the item was created." ;
	rdfs:subClassOf schema:Intangible .

schema:AudioObject a rdfs:Class ;
	rdfs:label "AudioObject" ;
	dc:source <http://www.w3.org/wiki/WebSchemas/SchemaDotOrgSources#source_rNews> ;
	rdfs:comment "An audio file." ;
	rdfs:subClassOf schema:MediaObject .

schema:AuthorizeAction a rdfs:Class ;
	rdfs:label "AuthorizeAction" ;
	rdfs:comment "The act of granting permission to an object." ;
	rdfs:subClassOf schema:AllocateAction .

schema:AutoBodyShop a rdfs:Class ;
	rdfs:label "AutoBodyShop" ;
	rdfs:comment "Auto body shop." ;
	rdfs:subClassOf schema:AutomotiveBusiness .

schema:AutoDealer a rdfs:Class ;
	rdfs:label "AutoDealer" ;
	rdfs:comment "An car dealership." ;
	rdfs:subClassOf schema:AutomotiveBusiness .

schema:AutoPartsStore a rdfs:Class ;
	rdfs:label "AutoPartsStore" ;
	rdfs:comment "An auto parts store." ;
	rdfs:subClassOf schema:AutomotiveBusiness , schema:Store .

schema:AutoRental a rdfs:Class ;
	rdfs:label "AutoRental" ;
	rdfs:comment "A car rental business." ;
	rdfs:subClassOf schema:AutomotiveBusiness .

schema:AutoRepair a rdfs:Class ;
	rdfs:label "AutoRepair" ;
	rdfs:comment "Car repair business." ;
	rdfs:subClassOf schema:AutomotiveBusiness .

schema:AutoWash a rdfs:Class ;
	rdfs:label "AutoWash" ;
	rdfs:comment "A car wash business." ;
	rdfs:subClassOf schema:AutomotiveBusiness .

schema:AutomatedTeller a rdfs:Class ;
	rdfs:label "AutomatedTeller" ;
	rdfs:comment "ATM/cash machine." ;
	rdfs:subClassOf schema:FinancialService .

schema:AutomotiveBusiness a rdfs:Class ;
	rdfs:label "AutomotiveBusiness" ;
	rdfs:comment "Car repair, sales, or parts." ;
	rdfs:subClassOf schema:LocalBusiness .

schema:Bakery a rdfs:Class ;
	rdfs:label "Bakery" ;
	rdfs:comment "A bakery." ;
	rdfs:subClassOf schema:FoodEstablishment .

schema:BankOrCreditUnion a rdfs:Class ;
	rdfs:label "BankOrCreditUnion" ;
	rdfs:comment "Bank or credit union." ;
	rdfs:subClassOf schema:FinancialService .

schema:BarOrPub a rdfs:Class ;
	rdfs:label "BarOrPub" ;
	rdfs:comment "A bar or pub." ;
	rdfs:subClassOf schema:FoodEstablishment .

schema:Beach a rdfs:Class ;
	rdfs:label "Beach" ;
	rdfs:comment "Beach." ;
	rdfs:subClassOf schema:CivicStructure .

schema:BeautySalon a rdfs:Class ;
	rdfs:label "BeautySalon" ;
	rdfs:comment "Beauty salon." ;
	rdfs:subClassOf schema:HealthAndBeautyBusiness .

schema:BedAndBreakfast a rdfs:Class ;
	rdfs:label "BedAndBreakfast" ;
	rdfs:comment "Bed and breakfast." ;
	rdfs:subClassOf schema:LodgingBusiness .

schema:BefriendAction a rdfs:Class ;
	rdfs:label "BefriendAction" ;
	rdfs:comment "The act of forming a personal connection with someone (object) mutually/bidirectionally/symmetrically.<p>Related actions:</p><ul><li><a href=\"http://schema.org/FollowAction\">FollowAction</a>: Unlike FollowAction, BefriendAction implies that the connection is reciprocal.</li></ul>" ;
	rdfs:subClassOf schema:InteractAction .

schema:BikeStore a rdfs:Class ;
	rdfs:label "BikeStore" ;
	rdfs:comment "A bike store." ;
	rdfs:subClassOf schema:Store .

schema:Blog a rdfs:Class ;
	rdfs:label "Blog" ;
	rdfs:comment "A blog" ;
	rdfs:subClassOf schema:CreativeWork .

schema:BlogPosting a rdfs:Class ;
	rdfs:label "BlogPosting" ;
	rdfs:comment "A blog post." ;
	rdfs:subClassOf schema:Article .

schema:BloodTest a rdfs:Class ;
	rdfs:label "BloodTest" ;
	dc:source <http://www.w3.org/wiki/WebSchemas/SchemaDotOrgSources#source_WikiDoc> ;
	rdfs:comment "A medical test performed on a sample of a patient's blood." ;
	rdfs:subClassOf schema:MedicalTest .

schema:BodyOfWater a rdfs:Class ;
	rdfs:label "BodyOfWater" ;
	rdfs:comment "A body of water, such as a sea, ocean, or lake." ;
	rdfs:subClassOf schema:Landform .

schema:Bone a rdfs:Class ;
	rdfs:label "Bone" ;
	dc:source <http://www.w3.org/wiki/WebSchemas/SchemaDotOrgSources#source_WikiDoc> ;
	rdfs:comment "Rigid connective tissue that comprises up the skeletal structure of the human body." ;
	rdfs:subClassOf schema:AnatomicalStructure .

schema:Book a rdfs:Class ;
	rdfs:label "Book" ;
	rdfs:comment "A book." ;
	rdfs:subClassOf schema:CreativeWork .

schema:BookFormatType a rdfs:Class ;
	rdfs:label "BookFormatType" ;
	rdfs:comment "The publication format of the book." ;
	rdfs:subClassOf schema:Enumeration .

schema:BookStore a rdfs:Class ;
	rdfs:label "BookStore" ;
	rdfs:comment "A bookstore." ;
	rdfs:subClassOf schema:Store .

schema:BookmarkAction a rdfs:Class ;
	rdfs:label "BookmarkAction" ;
	rdfs:comment "An agent bookmarks/flags/labels/tags/marks an object." ;
	rdfs:subClassOf schema:OrganizeAction .

schema:Boolean a rdfs:Class ;
	rdfs:label "Boolean" ;
	rdfs:comment "Boolean: True or False." ;
	rdfs:subClassOf schema:DataType .

schema:BorrowAction a rdfs:Class ;
	rdfs:label "BorrowAction" ;
	rdfs:comment "The act of obtaining an object under an agreement to return it at a later date. Reciprocal of LendAction.<p>Related actions:</p><ul><li><a href=\"http://schema.org/LendAction\">LendAction</a>: Reciprocal of BorrowAction.</li></ul>" ;
	rdfs:subClassOf schema:TransferAction .

schema:BowlingAlley a rdfs:Class ;
	rdfs:label "BowlingAlley" ;
	rdfs:comment "A bowling alley." ;
	rdfs:subClassOf schema:SportsActivityLocation .

schema:BrainStructure a rdfs:Class ;
	rdfs:label "BrainStructure" ;
	dc:source <http://www.w3.org/wiki/WebSchemas/SchemaDotOrgSources#source_WikiDoc> ;
	rdfs:comment "Any anatomical structure which pertains to the soft nervous tissue functioning as the coordinating center of sensation and intellectual and nervous activity." ;
	rdfs:subClassOf schema:AnatomicalStructure .

schema:Brand a rdfs:Class ;
	rdfs:label "Brand" ;
	dc:source <http://www.w3.org/wiki/WebSchemas/SchemaDotOrgSources#source_GoodRelationsClass> ;
	rdfs:comment "A brand is a name used by an organization or business person for labeling a product, product group, or similar." ;
	rdfs:subClassOf schema:Intangible .

schema:Brewery a rdfs:Class ;
	rdfs:label "Brewery" ;
	rdfs:comment "Brewery." ;
	rdfs:subClassOf schema:FoodEstablishment .

schema:BuddhistTemple a rdfs:Class ;
	rdfs:label "BuddhistTemple" ;
	rdfs:comment "A Buddhist temple." ;
	rdfs:subClassOf schema:PlaceOfWorship .

schema:BusStation a rdfs:Class ;
	rdfs:label "BusStation" ;
	rdfs:comment "A bus station." ;
	rdfs:subClassOf schema:CivicStructure .

schema:BusStop a rdfs:Class ;
	rdfs:label "BusStop" ;
	rdfs:comment "A bus stop." ;
	rdfs:subClassOf schema:CivicStructure .

schema:BusinessEntityType a rdfs:Class ;
	rdfs:label "BusinessEntityType" ;
	dc:source <http://www.w3.org/wiki/WebSchemas/SchemaDotOrgSources#source_GoodRelationsClass> ;
	rdfs:comment """A business entity type is a conceptual entity representing the legal form, the size, the main line of business, the position in the value chain, or any combination thereof, of an organization or business person.

    Commonly used values:

    http://purl.org/goodrelations/v1#Business
    http://purl.org/goodrelations/v1#Enduser
    http://purl.org/goodrelations/v1#PublicInstitution
    http://purl.org/goodrelations/v1#Reseller

    		""" ;
	rdfs:subClassOf schema:Enumeration .

schema:BusinessEvent a rdfs:Class ;
	rdfs:label "BusinessEvent" ;
	rdfs:comment "Event type: Business event." ;
	rdfs:subClassOf schema:Event .

schema:BusinessFunction a rdfs:Class ;
	rdfs:label "BusinessFunction" ;
	dc:source <http://www.w3.org/wiki/WebSchemas/SchemaDotOrgSources#source_GoodRelationsClass> ;
	rdfs:comment """The business function specifies the type of activity or access (i.e., the bundle of rights) offered by the organization or business person through the offer. Typical are sell, rental or lease, maintenance or repair, manufacture / produce, recycle / dispose, engineering / construction, or installation. Proprietary specifications of access rights are also instances of this class.

    Commonly used values:

    http://purl.org/goodrelations/v1#ConstructionInstallation
    http://purl.org/goodrelations/v1#Dispose
    http://purl.org/goodrelations/v1#LeaseOut
    http://purl.org/goodrelations/v1#Maintain
    http://purl.org/goodrelations/v1#ProvideService
    http://purl.org/goodrelations/v1#Repair
    http://purl.org/goodrelations/v1#Sell
    http://purl.org/goodrelations/v1#Buy
    		""" ;
	rdfs:subClassOf schema:Enumeration .

schema:BuyAction a rdfs:Class ;
	rdfs:label "BuyAction" ;
	rdfs:comment "The act of giving money to a seller in exchange for goods or services rendered. An agent buys an object, product, or service from a seller for a price. Reciprocal of SellAction." ;
	rdfs:subClassOf schema:TradeAction .

schema:CafeOrCoffeeShop a rdfs:Class ;
	rdfs:label "CafeOrCoffeeShop" ;
	rdfs:comment "A cafe or coffee shop." ;
	rdfs:subClassOf schema:FoodEstablishment .

schema:Campground a rdfs:Class ;
	rdfs:label "Campground" ;
	rdfs:comment "A campground." ;
	rdfs:subClassOf schema:CivicStructure .

schema:Canal a rdfs:Class ;
	rdfs:label "Canal" ;
	rdfs:comment "A canal, like the Panama Canal" ;
	rdfs:subClassOf schema:BodyOfWater .

schema:CancelAction a rdfs:Class ;
	rdfs:label "CancelAction" ;
	rdfs:comment "The act of asserting that a future event/action is no longer going to happen.<p>Related actions:</p><ul><li><a href=\"http://schema.org/ConfirmAction\">ConfirmAction</a>: The antagonym of CancelAction.</li></ul>" ;
	rdfs:subClassOf schema:PlanAction .

schema:Casino a rdfs:Class ;
	rdfs:label "Casino" ;
	rdfs:comment "A casino." ;
	rdfs:subClassOf schema:EntertainmentBusiness .

schema:CatholicChurch a rdfs:Class ;
	rdfs:label "CatholicChurch" ;
	rdfs:comment "A Catholic church." ;
	rdfs:subClassOf schema:PlaceOfWorship .

schema:Cemetery a rdfs:Class ;
	rdfs:label "Cemetery" ;
	rdfs:comment "A graveyard." ;
	rdfs:subClassOf schema:CivicStructure .

schema:CheckAction a rdfs:Class ;
	rdfs:label "CheckAction" ;
	rdfs:comment "An agent inspects/determines/investigates/inquire or examine an object's accuracy/quality/condition or state." ;
	rdfs:subClassOf schema:FindAction .

schema:CheckInAction a rdfs:Class ;
	rdfs:label "CheckInAction" ;
	rdfs:comment "The act of an agent communicating (service provider, social media, etc) their arrival by registering/confirming for a previously reserved service (e.g. flight check in) or at a place (e.g. hotel), possibly resulting in a result (boarding pass, etc).<p>Related actions:</p><ul><li><a href=\"http://schema.org/CheckOutAction\">CheckOutAction</a>: The antagonym of CheckInAction.</li><li><a href=\"http://schema.org/ArriveAction\">ArriveAction</a>: Unlike ArriveAction, CheckInAction implies that the agent is informing/confirming the start of a previously reserved service.</li><li><a href=\"http://schema.org/ConfirmAction\">ConfirmAction</a>: Unlike ConfirmAction, CheckInAction implies that the agent is informing/confirming the *start* of a previously reserved service rather than its validity/existance.</li></ul>" ;
	rdfs:subClassOf schema:CommunicateAction .

schema:CheckOutAction a rdfs:Class ;
	rdfs:label "CheckOutAction" ;
	rdfs:comment "The act of an agent communicating (service provider, social media, etc) their departure of a previously reserved service (e.g. flight check in) or place (e.g. hotel).<p>Related actions:</p><ul><li><a href=\"http://schema.org/CheckInAction\">CheckInAction</a>: The antagonym of CheckOutAction.</li><li><a href=\"http://schema.org/DepartAction\">DepartAction</a>: Unlike DepartAction, CheckOutAction implies that the agent is informing/confirming the end of a previously reserved service.</li><li><a href=\"http://schema.org/CancelAction\">CancelAction</a>: Unlike CancelAction, CheckOutAction implies that the agent is informing/confirming the end of a previously reserved service.</li></ul>" ;
	rdfs:subClassOf schema:CommunicateAction .

schema:CheckoutPage a rdfs:Class ;
	rdfs:label "CheckoutPage" ;
	rdfs:comment "Web page type: Checkout page." ;
	rdfs:subClassOf schema:WebPage .

schema:ChildCare a rdfs:Class ;
	rdfs:label "ChildCare" ;
	rdfs:comment "A Childcare center." ;
	rdfs:subClassOf schema:LocalBusiness .

schema:ChildrensEvent a rdfs:Class ;
	rdfs:label "ChildrensEvent" ;
	rdfs:comment "Event type: Children's event." ;
	rdfs:subClassOf schema:Event .

schema:ChooseAction a rdfs:Class ;
	rdfs:label "ChooseAction" ;
	rdfs:comment "The act of expressing a preference from a set of options or a large or unbounded set of choices/options." ;
	rdfs:subClassOf schema:AssessAction .

schema:Church a rdfs:Class ;
	rdfs:label "Church" ;
	rdfs:comment "A church." ;
	rdfs:subClassOf schema:PlaceOfWorship .

schema:City a rdfs:Class ;
	rdfs:label "City" ;
	rdfs:comment "A city or town." ;
	rdfs:subClassOf schema:AdministrativeArea .

schema:CityHall a rdfs:Class ;
	rdfs:label "CityHall" ;
	rdfs:comment "A city hall." ;
	rdfs:subClassOf schema:GovernmentBuilding .

schema:CivicStructure a rdfs:Class ;
	rdfs:label "CivicStructure" ;
	rdfs:comment "A public structure, such as a town hall or concert hall." ;
	rdfs:subClassOf schema:Place .

schema:Class a rdfs:Class ;
	rdfs:label "Class" ;
	rdfs:comment "A class, also often called a 'Type'; equivalent to rdfs:Class." ;
	rdfs:subClassOf schema:Thing .

schema:ClothingStore a rdfs:Class ;
	rdfs:label "ClothingStore" ;
	rdfs:comment "A clothing store." ;
	rdfs:subClassOf schema:Store .

schema:Code a rdfs:Class ;
	rdfs:label "Code" ;
	rdfs:comment "Computer programming source code. Example: Full (compile ready) solutions, code snippet samples, scripts, templates." ;
	rdfs:subClassOf schema:CreativeWork .

schema:CollectionPage a rdfs:Class ;
	rdfs:label "CollectionPage" ;
	rdfs:comment "Web page type: Collection page." ;
	rdfs:subClassOf schema:WebPage .

schema:CollegeOrUniversity a rdfs:Class ;
	rdfs:label "CollegeOrUniversity" ;
	rdfs:comment "A college, university, or other third-level educational institution." ;
	rdfs:subClassOf schema:EducationalOrganization .

schema:ComedyClub a rdfs:Class ;
	rdfs:label "ComedyClub" ;
	rdfs:comment "A comedy club." ;
	rdfs:subClassOf schema:EntertainmentBusiness .

schema:ComedyEvent a rdfs:Class ;
	rdfs:label "ComedyEvent" ;
	rdfs:comment "Event type: Comedy event." ;
	rdfs:subClassOf schema:Event .

schema:Comment a rdfs:Class ;
	rdfs:label "Comment" ;
	rdfs:comment "A comment on an item - for example, a comment on a blog post. The comment's content is expressed via the \"text\" property, and its topic via \"about\", properties shared with all CreativeWorks." ;
	rdfs:subClassOf schema:CreativeWork .

schema:CommentAction a rdfs:Class ;
	rdfs:label "CommentAction" ;
	rdfs:comment "The act of generating a comment about a subject." ;
	rdfs:subClassOf schema:CommunicateAction .

schema:CommunicateAction a rdfs:Class ;
	rdfs:label "CommunicateAction" ;
	rdfs:comment "The act of conveying information to another person via a communication medium (instrument) such as speech, email, or telephone conversation." ;
	rdfs:subClassOf schema:InteractAction .

schema:ComputerStore a rdfs:Class ;
	rdfs:label "ComputerStore" ;
	rdfs:comment "A computer store." ;
	rdfs:subClassOf schema:Store .

schema:ConfirmAction a rdfs:Class ;
	rdfs:label "ConfirmAction" ;
	rdfs:comment "The act of notifying someone that a future event/action is going to happen as expected.<p>Related actions:</p><ul><li><a href=\"http://schema.org/CancelAction\">CancelAction</a>: The antagonym of ConfirmAction.</li></ul>" ;
	rdfs:subClassOf schema:InformAction .

schema:ConsumeAction a rdfs:Class ;
	rdfs:label "ConsumeAction" ;
	rdfs:comment "The act of ingesting information/resources/food." ;
	rdfs:subClassOf schema:Action .

schema:ContactPage a rdfs:Class ;
	rdfs:label "ContactPage" ;
	rdfs:comment "Web page type: Contact page." ;
	rdfs:subClassOf schema:WebPage .

schema:ContactPoint a rdfs:Class ;
	rdfs:label "ContactPoint" ;
	rdfs:comment "A contact point&#x2014;for example, a Customer Complaints department." ;
	rdfs:subClassOf schema:StructuredValue .

schema:Continent a rdfs:Class ;
	rdfs:label "Continent" ;
	rdfs:comment "One of the continents (for example, Europe or Africa)." ;
	rdfs:subClassOf schema:Landform .

schema:ConvenienceStore a rdfs:Class ;
	rdfs:label "ConvenienceStore" ;
	rdfs:comment "A convenience store." ;
	rdfs:subClassOf schema:Store .

schema:CookAction a rdfs:Class ;
	rdfs:label "CookAction" ;
	rdfs:comment "The act of producing/preparing food." ;
	rdfs:subClassOf schema:CreateAction .

schema:Corporation a rdfs:Class ;
	rdfs:label "Corporation" ;
	dc:source <http://www.w3.org/wiki/WebSchemas/SchemaDotOrgSources#source_rNews> ;
	rdfs:comment "Organization: A business corporation." ;
	rdfs:subClassOf schema:Organization .

schema:Country a rdfs:Class ;
	rdfs:label "Country" ;
	rdfs:comment "A country." ;
	rdfs:subClassOf schema:AdministrativeArea .

schema:Courthouse a rdfs:Class ;
	rdfs:label "Courthouse" ;
	rdfs:comment "A courthouse." ;
	rdfs:subClassOf schema:GovernmentBuilding .

schema:CreateAction a rdfs:Class ;
	rdfs:label "CreateAction" ;
	rdfs:comment "The act of deliberately creating/producing/generating/building a result out of the agent." ;
	rdfs:subClassOf schema:Action .

schema:CreativeWork a rdfs:Class ;
	rdfs:label "CreativeWork" ;
	dc:source <http://www.w3.org/wiki/WebSchemas/SchemaDotOrgSources#source_rNews> ;
	rdfs:comment "The most generic kind of creative work, including books, movies, photographs, software programs, etc." ;
	rdfs:subClassOf schema:Thing .

schema:CreditCard a rdfs:Class ;
	rdfs:label "CreditCard" ;
	dc:source <http://www.w3.org/wiki/WebSchemas/SchemaDotOrgSources#source_GoodRelationsClass> ;
	rdfs:comment """A credit or debit card type as a standardized procedure for transferring the monetary amount for a purchase.

    Commonly used values:

    http://purl.org/goodrelations/v1#AmericanExpress
    http://purl.org/goodrelations/v1#DinersClub
    http://purl.org/goodrelations/v1#Discover
    http://purl.org/goodrelations/v1#JCB
    http://purl.org/goodrelations/v1#MasterCard
    http://purl.org/goodrelations/v1#VISA
    		""" ;
	rdfs:subClassOf schema:PaymentMethod .

schema:Crematorium a rdfs:Class ;
	rdfs:label "Crematorium" ;
	rdfs:comment "A crematorium." ;
	rdfs:subClassOf schema:CivicStructure .

schema:DDxElement a rdfs:Class ;
	rdfs:label "DDxElement" ;
	dc:source <http://www.w3.org/wiki/WebSchemas/SchemaDotOrgSources#source_WikiDoc> ;
	rdfs:comment "An alternative, closely-related condition typically considered later in the differential diagnosis process along with the signs that are used to distinguish it." ;
	rdfs:subClassOf schema:MedicalIntangible .

schema:DanceEvent a rdfs:Class ;
	rdfs:label "DanceEvent" ;
	rdfs:comment "Event type: A social dance." ;
	rdfs:subClassOf schema:Event .

schema:DanceGroup a rdfs:Class ;
	rdfs:label "DanceGroup" ;
	rdfs:comment "A dance group&#x2014;for example, the Alvin Ailey Dance Theater or Riverdance." ;
	rdfs:subClassOf schema:PerformingGroup .

schema:DataCatalog a rdfs:Class ;
	rdfs:label "DataCatalog" ;
	dc:source <http://www.w3.org/wiki/WebSchemas/SchemaDotOrgSources#source_DatasetClass> ;
	rdfs:comment "A collection of datasets." ;
	rdfs:subClassOf schema:CreativeWork .

schema:DataDownload a rdfs:Class ;
	rdfs:label "DataDownload" ;
	dc:source <http://www.w3.org/wiki/WebSchemas/SchemaDotOrgSources#source_DatasetClass> ;
	rdfs:comment "A dataset in downloadable form." ;
	rdfs:subClassOf schema:MediaObject .

schema:DataType a rdfs:Class ;
	rdfs:label "DataType" ;
	rdfs:comment "The basic data types such as Integers, Strings, etc." .

schema:Dataset a rdfs:Class ;
	rdfs:label "Dataset" ;
	dc:source <http://www.w3.org/wiki/WebSchemas/SchemaDotOrgSources#source_DatasetClass> ;
	rdfs:comment "A body of structured information describing some topic(s) of interest." ;
	rdfs:subClassOf schema:CreativeWork .

schema:Date a rdfs:Class ;
	rdfs:label "Date" ;
	rdfs:comment "A date value in <a href='http://en.wikipedia.org/wiki/ISO_8601'>ISO 8601 date format</a>." ;
	rdfs:subClassOf schema:DataType .

schema:DateTime a rdfs:Class ;
	rdfs:label "DateTime" ;
	rdfs:comment "A combination of date and time of day in the form [-]CCYY-MM-DDThh:mm:ss[Z|(+|-)hh:mm] (see Chapter 5.4 of ISO 8601)." ;
	rdfs:subClassOf schema:DataType .

schema:DayOfWeek a rdfs:Class ;
	rdfs:label "DayOfWeek" ;
	dc:source <http://www.w3.org/wiki/WebSchemas/SchemaDotOrgSources#source_GoodRelationsClass> ;
	rdfs:comment """The day of the week, e.g. used to specify to which day the opening hours of an OpeningHoursSpecification refer.

    Commonly used values:

    http://purl.org/goodrelations/v1#Monday
    http://purl.org/goodrelations/v1#Tuesday
    http://purl.org/goodrelations/v1#Wednesday
    http://purl.org/goodrelations/v1#Thursday
    http://purl.org/goodrelations/v1#Friday
    http://purl.org/goodrelations/v1#Saturday
    http://purl.org/goodrelations/v1#Sunday
    http://purl.org/goodrelations/v1#PublicHolidays
    		""" ;
	rdfs:subClassOf schema:Enumeration .

schema:DaySpa a rdfs:Class ;
	rdfs:label "DaySpa" ;
	rdfs:comment "A day spa." ;
	rdfs:subClassOf schema:HealthAndBeautyBusiness .

schema:DefenceEstablishment a rdfs:Class ;
	rdfs:label "DefenceEstablishment" ;
	rdfs:comment "A defence establishment, such as an army or navy base." ;
	rdfs:subClassOf schema:GovernmentBuilding .

schema:DeleteAction a rdfs:Class ;
	rdfs:label "DeleteAction" ;
	rdfs:comment "The act of editing a recipient by removing one of its objects." ;
	rdfs:subClassOf schema:UpdateAction .

schema:DeliveryChargeSpecification a rdfs:Class ;
	rdfs:label "DeliveryChargeSpecification" ;
	dc:source <http://www.w3.org/wiki/WebSchemas/SchemaDotOrgSources#source_GoodRelationsClass> ;
	rdfs:comment "The price for the delivery of an offer using a particular delivery method." ;
	rdfs:subClassOf schema:PriceSpecification .

schema:DeliveryMethod a rdfs:Class ;
	rdfs:label "DeliveryMethod" ;
	dc:source <http://www.w3.org/wiki/WebSchemas/SchemaDotOrgSources#source_GoodRelationsClass> ;
	rdfs:comment """A delivery method is a standardized procedure for transferring the product or service to the destination of fulfilment chosen by the customer. Delivery methods are characterized by the means of transportation used, and by the organization or group that is the contracting party for the sending organization or person.

    Commonly used values:

    http://purl.org/goodrelations/v1#DeliveryModeDirectDownload
    http://purl.org/goodrelations/v1#DeliveryModeFreight
    http://purl.org/goodrelations/v1#DeliveryModeMail
    http://purl.org/goodrelations/v1#DeliveryModeOwnFleet
    http://purl.org/goodrelations/v1#DeliveryModePickUp
    http://purl.org/goodrelations/v1#DHL
    http://purl.org/goodrelations/v1#FederalExpress
    http://purl.org/goodrelations/v1#UPS
    		""" ;
	rdfs:subClassOf schema:Enumeration .

schema:Demand a rdfs:Class ;
	rdfs:label "Demand" ;
	dc:source <http://www.w3.org/wiki/WebSchemas/SchemaDotOrgSources#source_GoodRelationsClass> ;
	rdfs:comment "A demand entity represents the public, not necessarily binding, not necessarily exclusive, announcement by an organization or person to seek a certain type of goods or services. For describing demand using this type, the very same properties used for Offer apply." ;
	rdfs:subClassOf schema:Intangible .

schema:Dentist a rdfs:Class ;
	rdfs:label "Dentist" ;
	rdfs:comment "A dentist." ;
	rdfs:subClassOf schema:MedicalOrganization , schema:ProfessionalService .

schema:DepartAction a rdfs:Class ;
	rdfs:label "DepartAction" ;
	rdfs:comment "The act of  departing from a place. An agent departs from an fromLocation for a destination, optionally with participants." ;
	rdfs:subClassOf schema:MoveAction .

schema:DepartmentStore a rdfs:Class ;
	rdfs:label "DepartmentStore" ;
	rdfs:comment "A department store." ;
	rdfs:subClassOf schema:Store .

schema:DiagnosticLab a rdfs:Class ;
	rdfs:label "DiagnosticLab" ;
	rdfs:comment "A medical laboratory that offers on-site or off-site diagnostic services." ;
	rdfs:subClassOf schema:MedicalOrganization .

schema:DiagnosticProcedure a rdfs:Class ;
	rdfs:label "DiagnosticProcedure" ;
	dc:source <http://www.w3.org/wiki/WebSchemas/SchemaDotOrgSources#source_WikiDoc> ;
	rdfs:comment "A medical procedure intended primarly for diagnostic, as opposed to therapeutic, purposes." ;
	rdfs:subClassOf schema:MedicalProcedure , schema:MedicalTest .

schema:Diet a rdfs:Class ;
	rdfs:label "Diet" ;
	dc:source <http://www.w3.org/wiki/WebSchemas/SchemaDotOrgSources#source_WikiDoc> ;
	rdfs:comment "A strategy of regulating the intake of food to achieve or maintain a specific health-related goal." ;
	rdfs:subClassOf schema:CreativeWork , schema:LifestyleModification .

schema:DietarySupplement a rdfs:Class ;
	rdfs:label "DietarySupplement" ;
	dc:source <http://www.w3.org/wiki/WebSchemas/SchemaDotOrgSources#source_WikiDoc> ;
	rdfs:comment "A product taken by mouth that contains a dietary ingredient intended to supplement the diet. Dietary ingredients may include vitamins, minerals, herbs or other botanicals, amino acids, and substances such as enzymes, organ tissues, glandulars and metabolites." ;
	rdfs:subClassOf schema:MedicalTherapy .

schema:DisagreeAction a rdfs:Class ;
	rdfs:label "DisagreeAction" ;
	rdfs:comment "The act of expressing a difference of opinion with the object. An agent disagrees to/about an object (a proposition, topic or theme) with participants." ;
	rdfs:subClassOf schema:ReactAction .

schema:DiscoverAction a rdfs:Class ;
	rdfs:label "DiscoverAction" ;
	rdfs:comment "The act of discovering/finding an object." ;
	rdfs:subClassOf schema:FindAction .

schema:DislikeAction a rdfs:Class ;
	rdfs:label "DislikeAction" ;
	rdfs:comment "The act of expressing a negative sentiment about the object. An agent dislikes an object (a proposition, topic or theme) with participants." ;
	rdfs:subClassOf schema:ReactAction .

schema:Distance a rdfs:Class ;
	rdfs:label "Distance" ;
	rdfs:comment "Properties that take Distances as values are of the form '&lt;Number&gt; &lt;Length unit of measure&gt;'. E.g., '7 ft'" ;
	rdfs:subClassOf schema:Quantity .

schema:DonateAction a rdfs:Class ;
	rdfs:label "DonateAction" ;
	rdfs:comment "The act of providing goods, services, or money without compensation, often for philanthropic reasons." ;
	rdfs:subClassOf schema:TradeAction .

schema:DoseSchedule a rdfs:Class ;
	rdfs:label "DoseSchedule" ;
	rdfs:comment "A specific dosing schedule for a drug or supplement." ;
	rdfs:subClassOf schema:MedicalIntangible .

schema:DownloadAction a rdfs:Class ;
	rdfs:label "DownloadAction" ;
	rdfs:comment "The act of downloading an object." ;
	rdfs:subClassOf schema:TransferAction .

schema:DrawAction a rdfs:Class ;
	rdfs:label "DrawAction" ;
	rdfs:comment "The act of producing a visual/graphical representation of an object, typically with a pen/pencil and paper as instruments." ;
	rdfs:subClassOf schema:CreateAction .

schema:DrinkAction a rdfs:Class ;
	rdfs:label "DrinkAction" ;
	rdfs:comment "The act of swallowing liquids." ;
	rdfs:subClassOf schema:ConsumeAction .

schema:Drug a rdfs:Class ;
	rdfs:label "Drug" ;
	dc:source <http://www.w3.org/wiki/WebSchemas/SchemaDotOrgSources#source_WikiDoc> ;
	rdfs:comment "A chemical or biologic substance, used as a medical therapy, that has a physiological effect on an organism." ;
	rdfs:subClassOf schema:MedicalTherapy .

schema:DrugClass a rdfs:Class ;
	rdfs:label "DrugClass" ;
	dc:source <http://www.w3.org/wiki/WebSchemas/SchemaDotOrgSources#source_WikiDoc> ;
	rdfs:comment "A class of medical drugs, e.g., statins. Classes can represent general pharmacological class, common mechanisms of action, common physiological effects, etc." ;
	rdfs:subClassOf schema:MedicalTherapy .

schema:DrugCost a rdfs:Class ;
	rdfs:label "DrugCost" ;
	rdfs:comment "The cost per unit of a medical drug. Note that this type is not meant to represent the price in an offer of a drug for sale; see the Offer type for that. This type will typically be used to tag wholesale or average retail cost of a drug, or maximum reimbursable cost. Costs of medical drugs vary widely depending on how and where they are paid for, so while this type captures some of the variables, costs should be used with caution by consumers of this schema's markup." ;
	rdfs:subClassOf schema:MedicalIntangible .

schema:DrugCostCategory a rdfs:Class ;
	rdfs:label "DrugCostCategory" ;
	rdfs:comment "Enumerated categories of medical drug costs." ;
	rdfs:subClassOf schema:MedicalEnumeration .

schema:DrugLegalStatus a rdfs:Class ;
	rdfs:label "DrugLegalStatus" ;
	dc:source <http://www.w3.org/wiki/WebSchemas/SchemaDotOrgSources#source_WikiDoc> ;
	rdfs:comment "The legal availability status of a medical drug." ;
	rdfs:subClassOf schema:MedicalIntangible .

schema:DrugPregnancyCategory a rdfs:Class ;
	rdfs:label "DrugPregnancyCategory" ;
	rdfs:comment "Categories that represent an assessment of the risk of fetal injury due to a drug or pharmaceutical used as directed by the mother during pregnancy." ;
	rdfs:subClassOf schema:MedicalEnumeration .

schema:DrugPrescriptionStatus a rdfs:Class ;
	rdfs:label "DrugPrescriptionStatus" ;
	rdfs:comment "Indicates whether this drug is available by prescription or over-the-counter." ;
	rdfs:subClassOf schema:MedicalEnumeration .

schema:DrugStrength a rdfs:Class ;
	rdfs:label "DrugStrength" ;
	dc:source <http://www.w3.org/wiki/WebSchemas/SchemaDotOrgSources#source_WikiDoc> ;
	rdfs:comment "A specific strength in which a medical drug is available in a specific country." ;
	rdfs:subClassOf schema:MedicalIntangible .

schema:DryCleaningOrLaundry a rdfs:Class ;
	rdfs:label "DryCleaningOrLaundry" ;
	rdfs:comment "A dry-cleaning business." ;
	rdfs:subClassOf schema:LocalBusiness .

schema:Duration a rdfs:Class ;
	rdfs:label "Duration" ;
	rdfs:comment "Quantity: Duration (use  <a href='http://en.wikipedia.org/wiki/ISO_8601'>ISO 8601 duration format</a>)." ;
	rdfs:subClassOf schema:Quantity .

schema:EatAction a rdfs:Class ;
	rdfs:label "EatAction" ;
	rdfs:comment "The act of swallowing solid objects." ;
	rdfs:subClassOf schema:ConsumeAction .

schema:EducationEvent a rdfs:Class ;
	rdfs:label "EducationEvent" ;
	rdfs:comment "Event type: Education event." ;
	rdfs:subClassOf schema:Event .

schema:EducationalAudience a rdfs:Class ;
	rdfs:label "EducationalAudience" ;
	dc:source <http://www.w3.org/wiki/WebSchemas/SchemaDotOrgSources#source_LRMIClass> ;
	rdfs:comment "An EducationalAudience" ;
	rdfs:subClassOf schema:Audience .

schema:EducationalOrganization a rdfs:Class ;
	rdfs:label "EducationalOrganization" ;
	rdfs:comment "An educational organization." ;
	rdfs:subClassOf schema:Organization .

schema:Electrician a rdfs:Class ;
	rdfs:label "Electrician" ;
	rdfs:comment "An electrician." ;
	rdfs:subClassOf schema:HomeAndConstructionBusiness , schema:ProfessionalService .

schema:ElectronicsStore a rdfs:Class ;
	rdfs:label "ElectronicsStore" ;
	rdfs:comment "An electronics store." ;
	rdfs:subClassOf schema:Store .

schema:ElementarySchool a rdfs:Class ;
	rdfs:label "ElementarySchool" ;
	rdfs:comment "An elementary school." ;
	rdfs:subClassOf schema:EducationalOrganization .

schema:Embassy a rdfs:Class ;
	rdfs:label "Embassy" ;
	rdfs:comment "An embassy." ;
	rdfs:subClassOf schema:GovernmentBuilding .

schema:EmergencyService a rdfs:Class ;
	rdfs:label "EmergencyService" ;
	rdfs:comment "An emergency service, such as a fire station or ER." ;
	rdfs:subClassOf schema:LocalBusiness .

schema:EmploymentAgency a rdfs:Class ;
	rdfs:label "EmploymentAgency" ;
	rdfs:comment "An employment agency." ;
	rdfs:subClassOf schema:LocalBusiness .

schema:EndorseAction a rdfs:Class ;
	rdfs:label "EndorseAction" ;
	rdfs:comment "An agent approves/certifies/likes/supports/sanction an object." ;
	rdfs:subClassOf schema:ReactAction .

schema:Energy a rdfs:Class ;
	rdfs:label "Energy" ;
	rdfs:comment "Properties that take Enerygy as values are of the form '&lt;Number&gt; &lt;Energy unit of measure&gt;'" ;
	rdfs:subClassOf schema:Quantity .

schema:EntertainmentBusiness a rdfs:Class ;
	rdfs:label "EntertainmentBusiness" ;
	rdfs:comment "A business providing entertainment." ;
	rdfs:subClassOf schema:LocalBusiness .

schema:Enumeration a rdfs:Class ;
	rdfs:label "Enumeration" ;
	rdfs:comment "Lists or enumerations&#x2014;for example, a list of cuisines or music genres, etc." ;
	rdfs:subClassOf schema:Intangible .

schema:Event a rdfs:Class ;
	rdfs:label "Event" ;
	rdfs:comment "An event happening at a certain time at a certain location." ;
	rdfs:subClassOf schema:Thing .

schema:EventVenue a rdfs:Class ;
	rdfs:label "EventVenue" ;
	rdfs:comment "An event venue." ;
	rdfs:subClassOf schema:CivicStructure .

schema:ExerciseAction a rdfs:Class ;
	rdfs:label "ExerciseAction" ;
	rdfs:comment "The act of participating in exertive activity for the purposes of improving health and fitness" ;
	rdfs:subClassOf schema:PlayAction .

schema:ExerciseGym a rdfs:Class ;
	rdfs:label "ExerciseGym" ;
	rdfs:comment "A gym." ;
	rdfs:subClassOf schema:SportsActivityLocation .

schema:ExercisePlan a rdfs:Class ;
	rdfs:label "ExercisePlan" ;
	dc:source <http://www.w3.org/wiki/WebSchemas/SchemaDotOrgSources#source_WikiDoc> ;
	rdfs:comment "Fitness-related activity designed for a specific health-related purpose, including defined exercise routines as well as activity prescribed by a clinician." ;
	rdfs:subClassOf schema:CreativeWork , schema:PhysicalActivity .

schema:FastFoodRestaurant a rdfs:Class ;
	rdfs:label "FastFoodRestaurant" ;
	rdfs:comment "A fast-food restaurant." ;
	rdfs:subClassOf schema:FoodEstablishment .

schema:Festival a rdfs:Class ;
	rdfs:label "Festival" ;
	rdfs:comment "Event type: Festival." ;
	rdfs:subClassOf schema:Event .

schema:FilmAction a rdfs:Class ;
	rdfs:label "FilmAction" ;
	rdfs:comment "The act of capturing sound and moving images on film, video, or digitally." ;
	rdfs:subClassOf schema:CreateAction .

schema:FinancialService a rdfs:Class ;
	rdfs:label "FinancialService" ;
	rdfs:comment "Financial services business." ;
	rdfs:subClassOf schema:LocalBusiness .

schema:FindAction a rdfs:Class ;
	rdfs:label "FindAction" ;
	rdfs:comment "The act of finding an object.<p>Related actions:</p><ul><li><a href=\"http://schema.org/SearchAction\">SearchAction</a>: FindAction is generally lead by a SearchAction, but not necessarily.</li></ul>" ;
	rdfs:subClassOf schema:Action .

schema:FireStation a rdfs:Class ;
	rdfs:label "FireStation" ;
	rdfs:comment "A fire station. With firemen." ;
	rdfs:subClassOf schema:CivicStructure , schema:EmergencyService .

schema:Float a rdfs:Class ;
	rdfs:label "Float" ;
	rdfs:comment "Data type: Floating number." ;
	rdfs:subClassOf schema:Number .

schema:Florist a rdfs:Class ;
	rdfs:label "Florist" ;
	rdfs:comment "A florist." ;
	rdfs:subClassOf schema:Store .

schema:FollowAction a rdfs:Class ;
	rdfs:label "FollowAction" ;
	rdfs:comment "The act of forming a personal connection with someone/something (object) unidirectionally/asymmetrically to get updates polled from.<p>Related actions:</p><ul><li><a href=\"http://schema.org/BefriendAction\">BefriendAction</a>: Unlike BefriendAction, FollowAction implies that the connection is *not* necessarily reciprocal.</li><li><a href=\"http://schema.org/SubscribeAction\">SubscribeAction</a>: Unlike SubscribeAction, FollowAction implies that the follower acts as an active agent constantly/actively polling for updates.</li><li><a href=\"http://schema.org/RegisterAction\">RegisterAction</a>: Unlike RegisterAction, FollowAction implies that the agent is interested in continuing receiving updates from the object.</li><li><a href=\"http://schema.org/JoinAction\">JoinAction</a>: Unlike JoinAction, FollowAction implies that the agent is interested in getting updates from the object.</li><li><a href=\"http://schema.org/TrackAction\">TrackAction</a>: Unlike TrackAction, FollowAction refers to the polling of updates of all aspects of animate objects rather than the location of inanimate objects (e.g. you track a package, but you don't follow it).</li></ul>" ;
	rdfs:subClassOf schema:InteractAction .

schema:FoodEstablishment a rdfs:Class ;
	rdfs:label "FoodEstablishment" ;
	rdfs:comment "A food-related business." ;
	rdfs:subClassOf schema:LocalBusiness .

schema:FoodEvent a rdfs:Class ;
	rdfs:label "FoodEvent" ;
	rdfs:comment "Event type: Food event." ;
	rdfs:subClassOf schema:Event .

schema:FurnitureStore a rdfs:Class ;
	rdfs:label "FurnitureStore" ;
	rdfs:comment "A furniture store." ;
	rdfs:subClassOf schema:Store .

schema:GardenStore a rdfs:Class ;
	rdfs:label "GardenStore" ;
	rdfs:comment "A garden store." ;
	rdfs:subClassOf schema:Store .

schema:GasStation a rdfs:Class ;
	rdfs:label "GasStation" ;
	rdfs:comment "A gas station." ;
	rdfs:subClassOf schema:AutomotiveBusiness .

schema:GatedResidenceCommunity a rdfs:Class ;
	rdfs:label "GatedResidenceCommunity" ;
	rdfs:comment "Residence type: Gated community." ;
	rdfs:subClassOf schema:Residence .

schema:GeneralContractor a rdfs:Class ;
	rdfs:label "GeneralContractor" ;
	rdfs:comment "A general contractor." ;
	rdfs:subClassOf schema:HomeAndConstructionBusiness , schema:ProfessionalService .

schema:GeoCoordinates a rdfs:Class ;
	rdfs:label "GeoCoordinates" ;
	rdfs:comment "The geographic coordinates of a place or event." ;
	rdfs:subClassOf schema:StructuredValue .

schema:GeoShape a rdfs:Class ;
	rdfs:label "GeoShape" ;
	dc:source <http://www.w3.org/wiki/WebSchemas/SchemaDotOrgSources#source_rNews> ;
	rdfs:comment "The geographic shape of a place." ;
	rdfs:subClassOf schema:StructuredValue .

schema:GiveAction a rdfs:Class ;
	rdfs:label "GiveAction" ;
	rdfs:comment "The act of transferring ownership of an object to a destination. Reciprocal of TakeAction.<p>Related actions:</p><ul><li><a href=\"http://schema.org/TakeAction\">TakeAction</a>: Reciprocal of GiveAction.</li><li><a href=\"http://schema.org/SendAction\">SendAction</a>: Unlike SendAction, GiveAction implies that ownership is being transferred (e.g. I may send my laptop to you, but that doesn't mean I'm giving it to you).</li></ul>" ;
	rdfs:subClassOf schema:TransferAction .

schema:GolfCourse a rdfs:Class ;
	rdfs:label "GolfCourse" ;
	rdfs:comment "A golf course." ;
	rdfs:subClassOf schema:SportsActivityLocation .

schema:GovernmentBuilding a rdfs:Class ;
	rdfs:label "GovernmentBuilding" ;
	rdfs:comment "A government building." ;
	rdfs:subClassOf schema:CivicStructure .

schema:GovernmentOffice a rdfs:Class ;
	rdfs:label "GovernmentOffice" ;
	rdfs:comment "A government office&#x2014;for example, an IRS or DMV office." ;
	rdfs:subClassOf schema:LocalBusiness .

schema:GovernmentOrganization a rdfs:Class ;
	rdfs:label "GovernmentOrganization" ;
	rdfs:comment "A governmental organization or agency." ;
	rdfs:subClassOf schema:Organization .

schema:GroceryStore a rdfs:Class ;
	rdfs:label "GroceryStore" ;
	rdfs:comment "A grocery store." ;
	rdfs:subClassOf schema:Store .

schema:HVACBusiness a rdfs:Class ;
	rdfs:label "HVACBusiness" ;
	rdfs:comment "An HVAC service." ;
	rdfs:subClassOf schema:HomeAndConstructionBusiness .

schema:HairSalon a rdfs:Class ;
	rdfs:label "HairSalon" ;
	rdfs:comment "A hair salon." ;
	rdfs:subClassOf schema:HealthAndBeautyBusiness .

schema:HardwareStore a rdfs:Class ;
	rdfs:label "HardwareStore" ;
	rdfs:comment "A hardware store." ;
	rdfs:subClassOf schema:Store .

schema:HealthAndBeautyBusiness a rdfs:Class ;
	rdfs:label "HealthAndBeautyBusiness" ;
	rdfs:comment "Health and beauty." ;
	rdfs:subClassOf schema:LocalBusiness .

schema:HealthClub a rdfs:Class ;
	rdfs:label "HealthClub" ;
	rdfs:comment "A health club." ;
	rdfs:subClassOf schema:HealthAndBeautyBusiness , schema:SportsActivityLocation .

schema:HighSchool a rdfs:Class ;
	rdfs:label "HighSchool" ;
	rdfs:comment "A high school." ;
	rdfs:subClassOf schema:EducationalOrganization .

schema:HinduTemple a rdfs:Class ;
	rdfs:label "HinduTemple" ;
	rdfs:comment "A Hindu temple." ;
	rdfs:subClassOf schema:PlaceOfWorship .

schema:HobbyShop a rdfs:Class ;
	rdfs:label "HobbyShop" ;
	rdfs:comment "A hobby store." ;
	rdfs:subClassOf schema:Store .

schema:HomeAndConstructionBusiness a rdfs:Class ;
	rdfs:label "HomeAndConstructionBusiness" ;
	rdfs:comment "A construction business." ;
	rdfs:subClassOf schema:LocalBusiness .

schema:HomeGoodsStore a rdfs:Class ;
	rdfs:label "HomeGoodsStore" ;
	rdfs:comment "A home goods store." ;
	rdfs:subClassOf schema:Store .

schema:Hospital a rdfs:Class ;
	rdfs:label "Hospital" ;
	rdfs:comment "A hospital." ;
	rdfs:subClassOf schema:CivicStructure , schema:EmergencyService , schema:MedicalOrganization .

schema:Hostel a rdfs:Class ;
	rdfs:label "Hostel" ;
	rdfs:comment "A hostel." ;
	rdfs:subClassOf schema:LodgingBusiness .

schema:Hotel a rdfs:Class ;
	rdfs:label "Hotel" ;
	rdfs:comment "A hotel." ;
	rdfs:subClassOf schema:LodgingBusiness .

schema:HousePainter a rdfs:Class ;
	rdfs:label "HousePainter" ;
	rdfs:comment "A house painting service." ;
	rdfs:subClassOf schema:HomeAndConstructionBusiness , schema:ProfessionalService .

schema:IceCreamShop a rdfs:Class ;
	rdfs:label "IceCreamShop" ;
	rdfs:comment "An ice cream shop" ;
	rdfs:subClassOf schema:FoodEstablishment .

schema:IgnoreAction a rdfs:Class ;
	rdfs:label "IgnoreAction" ;
	rdfs:comment "The act of intentionally disregarding the object. An agent ignores an object." ;
	rdfs:subClassOf schema:AssessAction .

schema:ImageGallery a rdfs:Class ;
	rdfs:label "ImageGallery" ;
	rdfs:comment "Web page type: Image gallery page." ;
	rdfs:subClassOf schema:CollectionPage .

schema:ImageObject a rdfs:Class ;
	rdfs:label "ImageObject" ;
	rdfs:comment "An image file." ;
	rdfs:subClassOf schema:MediaObject .

schema:ImagingTest a rdfs:Class ;
	rdfs:label "ImagingTest" ;
	dc:source <http://www.w3.org/wiki/WebSchemas/SchemaDotOrgSources#source_WikiDoc> ;
	rdfs:comment "Any medical imaging modality typically used for diagnostic purposes." ;
	rdfs:subClassOf schema:MedicalTest .

schema:IndividualProduct a rdfs:Class ;
	rdfs:label "IndividualProduct" ;
	dc:source <http://www.w3.org/wiki/WebSchemas/SchemaDotOrgSources#source_GoodRelationsClass> ;
	rdfs:comment "A single, identifiable product instance (e.g. a laptop with a particular serial number)." ;
	rdfs:subClassOf schema:Product .

schema:InfectiousAgentClass a rdfs:Class ;
	rdfs:label "InfectiousAgentClass" ;
	dc:source <http://www.w3.org/wiki/WebSchemas/SchemaDotOrgSources#source_WikiDoc> ;
	rdfs:comment "Classes of agents or pathogens that transmit infectious diseases. Enumerated type." ;
	rdfs:subClassOf schema:MedicalEnumeration .

schema:InfectiousDisease a rdfs:Class ;
	rdfs:label "InfectiousDisease" ;
	dc:source <http://www.w3.org/wiki/WebSchemas/SchemaDotOrgSources#source_WikiDoc> ;
	rdfs:comment "An infectious disease is a clinically evident human disease resulting from the presence of pathogenic microbial agents, like pathogenic viruses, pathogenic bacteria, fungi, protozoa, multicellular parasites, and prions. To be considered an infectious disease, such pathogens are known to be able to cause this disease." ;
	rdfs:subClassOf schema:MedicalCondition .

schema:InformAction a rdfs:Class ;
	rdfs:label "InformAction" ;
	rdfs:comment "The act of notifying someone of information pertinent to them, with no expectation of a response." ;
	rdfs:subClassOf schema:CommunicateAction .

schema:InsertAction a rdfs:Class ;
	rdfs:label "InsertAction" ;
	rdfs:comment "The act of adding at a specific location in an ordered collection." ;
	rdfs:subClassOf schema:AddAction .

schema:InstallAction a rdfs:Class ;
	rdfs:label "InstallAction" ;
	rdfs:comment "The act of installing an application." ;
	rdfs:subClassOf schema:ConsumeAction .

schema:InsuranceAgency a rdfs:Class ;
	rdfs:label "InsuranceAgency" ;
	rdfs:comment "Insurance agency." ;
	rdfs:subClassOf schema:FinancialService .

schema:Intangible a rdfs:Class ;
	rdfs:label "Intangible" ;
	rdfs:comment "A utility class that serves as the umbrella for a number of 'intangible' things such as quantities, structured values, etc." ;
	rdfs:subClassOf schema:Thing .

schema:Integer a rdfs:Class ;
	rdfs:label "Integer" ;
	rdfs:comment "Data type: Integer." ;
	rdfs:subClassOf schema:Number .

schema:InteractAction a rdfs:Class ;
	rdfs:label "InteractAction" ;
	rdfs:comment "The act of interacting with another person or organization." ;
	rdfs:subClassOf schema:Action .

schema:InternetCafe a rdfs:Class ;
	rdfs:label "InternetCafe" ;
	rdfs:comment "An internet cafe." ;
	rdfs:subClassOf schema:LocalBusiness .

schema:InviteAction a rdfs:Class ;
	rdfs:label "InviteAction" ;
	rdfs:comment "The act of asking someone to attend an event. Reciprocal of RsvpAction." ;
	rdfs:subClassOf schema:CommunicateAction .

schema:ItemAvailability a rdfs:Class ;
	rdfs:label "ItemAvailability" ;
	rdfs:comment "A list of possible product availablity options." ;
	rdfs:subClassOf schema:Enumeration .

schema:ItemList a rdfs:Class ;
	rdfs:label "ItemList" ;
	rdfs:comment "A list of items of any sort&#x2014;for example, Top 10 Movies About Weathermen, or Top 100 Party Songs. Not to be confused with HTML lists, which are often used only for formatting." ;
	rdfs:subClassOf schema:CreativeWork .

schema:ItemPage a rdfs:Class ;
	rdfs:label "ItemPage" ;
	rdfs:comment "A page devoted to a single item, such as a particular product or hotel." ;
	rdfs:subClassOf schema:WebPage .

schema:JewelryStore a rdfs:Class ;
	rdfs:label "JewelryStore" ;
	rdfs:comment "A jewelry store." ;
	rdfs:subClassOf schema:Store .

schema:JobPosting a rdfs:Class ;
	rdfs:label "JobPosting" ;
	rdfs:comment "A listing that describes a job opening in a certain organization." ;
	rdfs:subClassOf schema:Intangible .

schema:JoinAction a rdfs:Class ;
	rdfs:label "JoinAction" ;
	rdfs:comment "An agent joins an event/group with participants/friends at a location.<p>Related actions:</p><ul><li><a href=\"http://schema.org/RegisterAction\">RegisterAction</a>: Unlike RegisterAction, JoinAction refers to joining a group/team of people.</li><li><a href=\"http://schema.org/SubscribeAction\">SubscribeAction</a>: Unlike SubscribeAction, JoinAction does not imply that you'll be receiving updates.</li><li><a href=\"http://schema.org/FollowAction\">FollowAction</a>: Unlike FollowAction, JoinAction does not imply that you'll be polling for updates.</li></ul>" ;
	rdfs:subClassOf schema:InteractAction .

schema:Joint a rdfs:Class ;
	rdfs:label "Joint" ;
	dc:source <http://www.w3.org/wiki/WebSchemas/SchemaDotOrgSources#source_WikiDoc> ;
	rdfs:comment "The anatomical location at which two or more bones make contact." ;
	rdfs:subClassOf schema:AnatomicalStructure .

schema:LakeBodyOfWater a rdfs:Class ;
	rdfs:label "LakeBodyOfWater" ;
	rdfs:comment "A lake (for example, Lake Pontrachain)." ;
	rdfs:subClassOf schema:BodyOfWater .

schema:Landform a rdfs:Class ;
	rdfs:label "Landform" ;
	rdfs:comment "A landform or physical feature.  Landform elements include mountains, plains, lakes, rivers, seascape and oceanic waterbody interface features such as bays, peninsulas, seas and so forth, including sub-aqueous terrain features such as submersed mountain ranges, volcanoes, and the great ocean basins." ;
	rdfs:subClassOf schema:Place .

schema:LandmarksOrHistoricalBuildings a rdfs:Class ;
	rdfs:label "LandmarksOrHistoricalBuildings" ;
	rdfs:comment "An historical landmark or building." ;
	rdfs:subClassOf schema:Place .

schema:Language a rdfs:Class ;
	rdfs:label "Language" ;
	rdfs:comment "Natural languages such as Spanish, Tamil, Hindi, English, etc. and programming languages such as Scheme and Lisp." ;
	rdfs:subClassOf schema:Intangible .

schema:LeaveAction a rdfs:Class ;
	rdfs:label "LeaveAction" ;
	rdfs:comment "An agent leaves an event / group with participants/friends at a location.<p>Related actions:</p><ul><li><a href=\"http://schema.org/JoinAction\">JoinAction</a>: The antagonym of LeaveAction.</li><li><a href=\"http://schema.org/UnRegisterAction\">UnRegisterAction</a>: Unlike UnRegisterAction, LeaveAction implies leaving a group/team of people rather than a service.</li></ul>" ;
	rdfs:subClassOf schema:InteractAction .

schema:LegislativeBuilding a rdfs:Class ;
	rdfs:label "LegislativeBuilding" ;
	rdfs:comment "A legislative building&#x2014;for example, the state capitol." ;
	rdfs:subClassOf schema:GovernmentBuilding .

schema:LendAction a rdfs:Class ;
	rdfs:label "LendAction" ;
	rdfs:comment "The act of providing an object under an agreement that it will be returned at a later date. Reciprocal of BorrowAction.<p>Related actions:</p><ul><li><a href=\"http://schema.org/BorrowAction\">BorrowAction</a>: Reciprocal of LendAction.</li></ul>" ;
	rdfs:subClassOf schema:TransferAction .

schema:Library a rdfs:Class ;
	rdfs:label "Library" ;
	rdfs:comment "A library." ;
	rdfs:subClassOf schema:LocalBusiness .

schema:LifestyleModification a rdfs:Class ;
	rdfs:label "LifestyleModification" ;
	dc:source <http://www.w3.org/wiki/WebSchemas/SchemaDotOrgSources#source_WikiDoc> ;
	rdfs:comment "A process of care involving exercise, changes to diet, fitness routines, and other lifestyle changes aimed at improving a health condition." ;
	rdfs:subClassOf schema:MedicalTherapy .

schema:Ligament a rdfs:Class ;
	rdfs:label "Ligament" ;
	dc:source <http://www.w3.org/wiki/WebSchemas/SchemaDotOrgSources#source_WikiDoc> ;
	rdfs:comment "A short band of tough, flexible, fibrous connective tissue that functions to connect multiple bones, cartilages, and structurally support joints." ;
	rdfs:subClassOf schema:AnatomicalStructure .

schema:LikeAction a rdfs:Class ;
	rdfs:label "LikeAction" ;
	rdfs:comment "The act of expressing a positive sentiment about the object. An agent likes an object (a proposition, topic or theme) with participants." ;
	rdfs:subClassOf schema:ReactAction .

schema:LiquorStore a rdfs:Class ;
	rdfs:label "LiquorStore" ;
	rdfs:comment "A liquor store." ;
	rdfs:subClassOf schema:Store .

schema:ListenAction a rdfs:Class ;
	rdfs:label "ListenAction" ;
	rdfs:comment "The act of consuming audio content." ;
	rdfs:subClassOf schema:ConsumeAction .

schema:LiteraryEvent a rdfs:Class ;
	rdfs:label "LiteraryEvent" ;
	rdfs:comment "Event type: Literary event." ;
	rdfs:subClassOf schema:Event .

schema:LocalBusiness a rdfs:Class ;
	rdfs:label "LocalBusiness" ;
	rdfs:comment "A particular physical business or branch of an organization. Examples of LocalBusiness include a restaurant, a particular branch of a restaurant chain, a branch of a bank, a medical practice, a club, a bowling alley, etc." ;
	rdfs:subClassOf schema:Organization , schema:Place .

schema:Locksmith a rdfs:Class ;
	rdfs:label "Locksmith" ;
	rdfs:comment "A locksmith." ;
	rdfs:subClassOf schema:HomeAndConstructionBusiness , schema:ProfessionalService .

schema:LodgingBusiness a rdfs:Class ;
	rdfs:label "LodgingBusiness" ;
	rdfs:comment "A lodging business, such as a motel, hotel, or inn." ;
	rdfs:subClassOf schema:LocalBusiness .

schema:LoseAction a rdfs:Class ;
	rdfs:label "LoseAction" ;
	rdfs:comment "The act of being defeated in a competitive activity." ;
	rdfs:subClassOf schema:AchieveAction .

schema:LymphaticVessel a rdfs:Class ;
	rdfs:label "LymphaticVessel" ;
	dc:source <http://www.w3.org/wiki/WebSchemas/SchemaDotOrgSources#source_WikiDoc> ;
	rdfs:comment "A type of blood vessel that specifically carries lymph fluid unidirectionally toward the heart." ;
	rdfs:subClassOf schema:Vessel .

schema:Map a rdfs:Class ;
	rdfs:label "Map" ;
	rdfs:comment "A map." ;
	rdfs:subClassOf schema:CreativeWork .

schema:MarryAction a rdfs:Class ;
	rdfs:label "MarryAction" ;
	rdfs:comment "The act of marrying a person." ;
	rdfs:subClassOf schema:InteractAction .

schema:Mass a rdfs:Class ;
	rdfs:label "Mass" ;
	rdfs:comment "Properties that take Mass as values are of the form '&lt;Number&gt; &lt;Mass unit of measure&gt;'. E.g., '7 kg'" ;
	rdfs:subClassOf schema:Quantity .

schema:MaximumDoseSchedule a rdfs:Class ;
	rdfs:label "MaximumDoseSchedule" ;
	rdfs:comment "The maximum dosing schedule considered safe for a drug or supplement as recommended by an authority or by the drug/supplement's manufacturer. Capture the recommending authority in the recognizingAuthority property of MedicalEntity." ;
	rdfs:subClassOf schema:DoseSchedule .

schema:MediaObject a rdfs:Class ;
	rdfs:label "MediaObject" ;
	rdfs:comment "An image, video, or audio object embedded in a web page. Note that a creative work may have many media objects associated with it on the same web page. For example, a page about a single song (MusicRecording) may have a music video (VideoObject), and a high and low bandwidth audio stream (2 AudioObject's)." ;
	rdfs:subClassOf schema:CreativeWork .

schema:MedicalAudience a rdfs:Class ;
	rdfs:label "MedicalAudience" ;
	dc:source <http://www.w3.org/wiki/WebSchemas/SchemaDotOrgSources#source_WikiDoc> ;
	rdfs:comment "Target audiences for medical web pages. Enumerated type." ;
	rdfs:subClassOf schema:Audience , schema:MedicalEnumeration , schema:PeopleAudience .

schema:MedicalCause a rdfs:Class ;
	rdfs:label "MedicalCause" ;
	dc:source <http://www.w3.org/wiki/WebSchemas/SchemaDotOrgSources#source_WikiDoc> ;
	rdfs:comment "The causative agent(s) that are responsible for the pathophysiologic process that eventually results in a medical condition, symptom or sign. In this schema, unless otherwise specified this is meant to be the proximate cause of the medical condition, symptom or sign. The proximate cause is defined as the causative agent that most directly results in the medical condition, symptom or sign. For example, the HIV virus could be considered a cause of AIDS. Or in a diagnostic context, if a patient fell and sustained a hip fracture and two days later sustained a pulmonary embolism which eventuated in a cardiac arrest, the cause of the cardiac arrest (the proximate cause) would be the pulmonary embolism and not the fall. <p>Medical causes can include cardiovascular, chemical, dermatologic, endocrine, environmental, gastroenterologic, genetic, hematologic, gynecologic, iatrogenic, infectious, musculoskeletal, neurologic, nutritional, obstetric, oncologic, otolaryngologic, pharmacologic, psychiatric, pulmonary, renal, rheumatologic, toxic, traumatic, or urologic causes; medical conditions can be causes as well." ;
	rdfs:subClassOf schema:MedicalEntity .

schema:MedicalClinic a rdfs:Class ;
	rdfs:label "MedicalClinic" ;
	rdfs:comment "A medical clinic." ;
	rdfs:subClassOf schema:MedicalOrganization .

schema:MedicalCode a rdfs:Class ;
	rdfs:label "MedicalCode" ;
	dc:source <http://www.w3.org/wiki/WebSchemas/SchemaDotOrgSources#source_WikiDoc> ;
	rdfs:comment "A code for a medical entity." ;
	rdfs:subClassOf schema:MedicalIntangible .

schema:MedicalCondition a rdfs:Class ;
	rdfs:label "MedicalCondition" ;
	dc:source <http://www.w3.org/wiki/WebSchemas/SchemaDotOrgSources#source_WikiDoc> ;
	rdfs:comment "Any condition of the human body that affects the normal functioning of a person, whether physically or mentally. Includes diseases, injuries, disabilities, disorders, syndromes, etc." ;
	rdfs:subClassOf schema:MedicalEntity .

schema:MedicalConditionStage a rdfs:Class ;
	rdfs:label "MedicalConditionStage" ;
	dc:source <http://www.w3.org/wiki/WebSchemas/SchemaDotOrgSources#source_WikiDoc> ;
	rdfs:comment "A stage of a medical condition, such as 'Stage IIIa'." ;
	rdfs:subClassOf schema:MedicalIntangible .

schema:MedicalContraindication a rdfs:Class ;
	rdfs:label "MedicalContraindication" ;
	dc:source <http://www.w3.org/wiki/WebSchemas/SchemaDotOrgSources#source_WikiDoc> ;
	rdfs:comment "A condition or factor that serves as a reason to withhold a certain medical therapy. Contraindications can be absolute (there are no reasonable circumstances for undertaking a course of action) or relative (the patient is at higher risk of complications, but that these risks may be outweighed by other considerations or mitigated by other measures)." ;
	rdfs:subClassOf schema:MedicalEntity .

schema:MedicalDevice a rdfs:Class ;
	rdfs:label "MedicalDevice" ;
	dc:source <http://www.w3.org/wiki/WebSchemas/SchemaDotOrgSources#source_WikiDoc> ;
	rdfs:comment "Any object used in a medical capacity, such as to diagnose or treat a patient." ;
	rdfs:subClassOf schema:MedicalEntity .

schema:MedicalDevicePurpose a rdfs:Class ;
	rdfs:label "MedicalDevicePurpose" ;
	dc:source <http://www.w3.org/wiki/WebSchemas/SchemaDotOrgSources#source_WikiDoc> ;
	rdfs:comment "Categories of medical devices, organized by the purpose or intended use of the device." ;
	rdfs:subClassOf schema:MedicalEnumeration .

schema:MedicalEntity a rdfs:Class ;
	rdfs:label "MedicalEntity" ;
	dc:source <http://www.w3.org/wiki/WebSchemas/SchemaDotOrgSources#source_WikiDoc> ;
	rdfs:comment "The most generic type of entity related to health and the practice of medicine." ;
	rdfs:subClassOf schema:Thing .

schema:MedicalEnumeration a rdfs:Class ;
	rdfs:label "MedicalEnumeration" ;
	rdfs:comment "Enumerations related to health and the practice of medicine." ;
	rdfs:subClassOf schema:MedicalIntangible .

schema:MedicalEvidenceLevel a rdfs:Class ;
	rdfs:label "MedicalEvidenceLevel" ;
	dc:source <http://www.w3.org/wiki/WebSchemas/SchemaDotOrgSources#source_WikiDoc> ;
	rdfs:comment "Level of evidence for a medical guideline. Enumerated type." ;
	rdfs:subClassOf schema:MedicalEnumeration .

schema:MedicalGuideline a rdfs:Class ;
	rdfs:label "MedicalGuideline" ;
	dc:source <http://www.w3.org/wiki/WebSchemas/SchemaDotOrgSources#source_WikiDoc> ;
	rdfs:comment "Any recommendation made by a standard society (e.g. ACC/AHA) or consensus statement that denotes how to diagnose and treat a particular condition. Note: this type should be used to tag the actual guideline recommendation; if the guideline recommendation occurs in a larger scholarly article, use MedicalScholarlyArticle to tag the overall article, not this type. Note also: the organization making the recommendation should be captured in the recognizingAuthority base property of MedicalEntity." ;
	rdfs:subClassOf schema:MedicalEntity .

schema:MedicalGuidelineContraindication a rdfs:Class ;
	rdfs:label "MedicalGuidelineContraindication" ;
	dc:source <http://www.w3.org/wiki/WebSchemas/SchemaDotOrgSources#source_WikiDoc> ;
	rdfs:comment "A guideline contraindication that designates a process as harmful and where quality of the data supporting the contraindication is sound." ;
	rdfs:subClassOf schema:MedicalGuideline .

schema:MedicalGuidelineRecommendation a rdfs:Class ;
	rdfs:label "MedicalGuidelineRecommendation" ;
	dc:source <http://www.w3.org/wiki/WebSchemas/SchemaDotOrgSources#source_WikiDoc> ;
	rdfs:comment "A guideline recommendation that is regarded as efficacious and where quality of the data supporting the recommendation is sound." ;
	rdfs:subClassOf schema:MedicalGuideline .

schema:MedicalImagingTechnique a rdfs:Class ;
	rdfs:label "MedicalImagingTechnique" ;
	dc:source <http://www.w3.org/wiki/WebSchemas/SchemaDotOrgSources#source_WikiDoc> ;
	rdfs:comment "Any medical imaging modality typically used for diagnostic purposes. Enumerated type." ;
	rdfs:subClassOf schema:MedicalEnumeration .

schema:MedicalIndication a rdfs:Class ;
	rdfs:label "MedicalIndication" ;
	dc:source <http://www.w3.org/wiki/WebSchemas/SchemaDotOrgSources#source_WikiDoc> ;
	rdfs:comment "A condition or factor that indicates use of a medical therapy, including signs, symptoms, risk factors, anatomical states, etc." ;
	rdfs:subClassOf schema:MedicalEntity .

schema:MedicalIntangible a rdfs:Class ;
	rdfs:label "MedicalIntangible" ;
	rdfs:comment "A utility class that serves as the umbrella for a number of 'intangible' things in the medical space." ;
	rdfs:subClassOf schema:MedicalEntity .

schema:MedicalObservationalStudy a rdfs:Class ;
	rdfs:label "MedicalObservationalStudy" ;
	dc:source <http://www.w3.org/wiki/WebSchemas/SchemaDotOrgSources#source_WikiDoc> ;
	rdfs:comment "An observational study is a type of medical study that attempts to infer the possible effect of a treatment through observation of a cohort of subjects over a period of time. In an observational study, the assignment of subjects into treatment groups versus control groups is outside the control of the investigator. This is in contrast with controlled studies, such as the randomized controlled trials represented by MedicalTrial, where each subject is randomly assigned to a treatment group or a control group before the start of the treatment." ;
	rdfs:subClassOf schema:MedicalStudy .

schema:MedicalObservationalStudyDesign a rdfs:Class ;
	rdfs:label "MedicalObservationalStudyDesign" ;
	dc:source <http://www.w3.org/wiki/WebSchemas/SchemaDotOrgSources#source_WikiDoc> ;
	rdfs:comment "Design models for observational medical studies. Enumerated type." ;
	rdfs:subClassOf schema:MedicalEnumeration .

schema:MedicalOrganization a rdfs:Class ;
	rdfs:label "MedicalOrganization" ;
	rdfs:comment "A medical organization, such as a doctor's office or clinic." ;
	rdfs:subClassOf schema:LocalBusiness .

schema:MedicalProcedure a rdfs:Class ;
	rdfs:label "MedicalProcedure" ;
	dc:source <http://www.w3.org/wiki/WebSchemas/SchemaDotOrgSources#source_WikiDoc> ;
	rdfs:comment "A process of care used in either a diagnostic, therapeutic, or palliative capacity that relies on invasive (surgical), non-invasive, or percutaneous techniques." ;
	rdfs:subClassOf schema:MedicalEntity .

schema:MedicalProcedureType a rdfs:Class ;
	rdfs:label "MedicalProcedureType" ;
	dc:source <http://www.w3.org/wiki/WebSchemas/SchemaDotOrgSources#source_WikiDoc> ;
	rdfs:comment "An enumeration that describes different types of medical procedures." ;
	rdfs:subClassOf schema:MedicalEnumeration .

schema:MedicalRiskCalculator a rdfs:Class ;
	rdfs:label "MedicalRiskCalculator" ;
	dc:source <http://www.w3.org/wiki/WebSchemas/SchemaDotOrgSources#source_WikiDoc> ;
	rdfs:comment "A complex mathematical calculation requiring an online calculator, used to assess prognosis. Note: use the url property of Thing to record any URLs for online calculators." ;
	rdfs:subClassOf schema:MedicalRiskEstimator .

schema:MedicalRiskEstimator a rdfs:Class ;
	rdfs:label "MedicalRiskEstimator" ;
	dc:source <http://www.w3.org/wiki/WebSchemas/SchemaDotOrgSources#source_WikiDoc> ;
	rdfs:comment "Any rule set or interactive tool for estimating the risk of developing a complication or condition." ;
	rdfs:subClassOf schema:MedicalEntity .

schema:MedicalRiskFactor a rdfs:Class ;
	rdfs:label "MedicalRiskFactor" ;
	dc:source <http://www.w3.org/wiki/WebSchemas/SchemaDotOrgSources#source_WikiDoc> ;
	rdfs:comment "A risk factor is anything that increases a person's likelihood of developing or contracting a disease, medical condition, or complication." ;
	rdfs:subClassOf schema:MedicalEntity .

schema:MedicalRiskScore a rdfs:Class ;
	rdfs:label "MedicalRiskScore" ;
	dc:source <http://www.w3.org/wiki/WebSchemas/SchemaDotOrgSources#source_WikiDoc> ;
	rdfs:comment "A simple system that adds up the number of risk factors to yield a score that is associated with prognosis, e.g. CHAD score, TIMI risk score." ;
	rdfs:subClassOf schema:MedicalRiskEstimator .

schema:MedicalScholarlyArticle a rdfs:Class ;
	rdfs:label "MedicalScholarlyArticle" ;
	rdfs:comment "A scholarly article in the medical domain." ;
	rdfs:subClassOf schema:ScholarlyArticle .

schema:MedicalSign a rdfs:Class ;
	rdfs:label "MedicalSign" ;
	dc:source <http://www.w3.org/wiki/WebSchemas/SchemaDotOrgSources#source_WikiDoc> ;
	rdfs:comment "Any physical manifestation of a person's medical condition discoverable by objective diagnostic tests or physical examination." ;
	rdfs:subClassOf schema:MedicalSignOrSymptom .

schema:MedicalSignOrSymptom a rdfs:Class ;
	rdfs:label "MedicalSignOrSymptom" ;
	dc:source <http://www.w3.org/wiki/WebSchemas/SchemaDotOrgSources#source_WikiDoc> ;
	rdfs:comment "Any indication of the existence of a medical condition or disease." ;
	rdfs:subClassOf schema:MedicalEntity .

schema:MedicalSpecialty a rdfs:Class ;
	rdfs:label "MedicalSpecialty" ;
	dc:source <http://www.w3.org/wiki/WebSchemas/SchemaDotOrgSources#source_WikiDoc> ;
	rdfs:comment "Any specific branch of medical science or practice. Medical specialities include clinical specialties that pertain to particular organ systems and their respective disease states, as well as allied health specialties. Enumerated type." ;
	rdfs:subClassOf schema:MedicalEnumeration , schema:Specialty .

schema:MedicalStudy a rdfs:Class ;
	rdfs:label "MedicalStudy" ;
	dc:source <http://www.w3.org/wiki/WebSchemas/SchemaDotOrgSources#source_WikiDoc> ;
	rdfs:comment "A medical study is an umbrella type covering all kinds of research studies relating to human medicine or health, including observational studies and interventional trials and registries, randomized, controlled or not. When the specific type of study is known, use one of the extensions of this type, such as MedicalTrial or MedicalObservationalStudy. Also, note that this type should be used to mark up data that describes the study itself; to tag an article that publishes the results of a study, use MedicalScholarlyArticle. Note: use the code property of MedicalEntity to store study IDs, e.g. clinicaltrials.gov ID." ;
	rdfs:subClassOf schema:MedicalEntity .

schema:MedicalStudyStatus a rdfs:Class ;
	rdfs:label "MedicalStudyStatus" ;
	dc:source <http://www.w3.org/wiki/WebSchemas/SchemaDotOrgSources#source_WikiDoc> ;
	rdfs:comment "The status of a medical study. Enumerated type." ;
	rdfs:subClassOf schema:MedicalEnumeration .

schema:MedicalSymptom a rdfs:Class ;
	rdfs:label "MedicalSymptom" ;
	dc:source <http://www.w3.org/wiki/WebSchemas/SchemaDotOrgSources#source_WikiDoc> ;
	rdfs:comment "Any indication of the existence of a medical condition or disease that is apparent to the patient." ;
	rdfs:subClassOf schema:MedicalSignOrSymptom .

schema:MedicalTest a rdfs:Class ;
	rdfs:label "MedicalTest" ;
	dc:source <http://www.w3.org/wiki/WebSchemas/SchemaDotOrgSources#source_WikiDoc> ;
	rdfs:comment "Any medical test, typically performed for diagnostic purposes." ;
	rdfs:subClassOf schema:MedicalEntity .

schema:MedicalTestPanel a rdfs:Class ;
	rdfs:label "MedicalTestPanel" ;
	dc:source <http://www.w3.org/wiki/WebSchemas/SchemaDotOrgSources#source_WikiDoc> ;
	rdfs:comment "Any collection of tests commonly ordered together." ;
	rdfs:subClassOf schema:MedicalTest .

schema:MedicalTherapy a rdfs:Class ;
	rdfs:label "MedicalTherapy" ;
	dc:source <http://www.w3.org/wiki/WebSchemas/SchemaDotOrgSources#source_WikiDoc> ;
	rdfs:comment "Any medical intervention designed to prevent, treat, and cure human diseases and medical conditions, including both curative and palliative therapies. Medical therapies are typically processes of care relying upon pharmacotherapy, behavioral therapy, supportive therapy (with fluid or nutrition for example), or detoxification (e.g. hemodialysis) aimed at improving or preventing a health condition." ;
	rdfs:subClassOf schema:MedicalEntity .

schema:MedicalTrial a rdfs:Class ;
	rdfs:label "MedicalTrial" ;
	dc:source <http://www.w3.org/wiki/WebSchemas/SchemaDotOrgSources#source_WikiDoc> ;
	rdfs:comment "A medical trial is a type of medical study that uses scientific process used to compare the safety and efficacy of medical therapies or medical procedures. In general, medical trials are controlled and subjects are allocated at random to the different treatment and/or control groups." ;
	rdfs:subClassOf schema:MedicalStudy .

schema:MedicalTrialDesign a rdfs:Class ;
	rdfs:label "MedicalTrialDesign" ;
	dc:source <http://www.w3.org/wiki/WebSchemas/SchemaDotOrgSources#source_WikiDoc> ;
	rdfs:comment "Design models for medical trials. Enumerated type." ;
	rdfs:subClassOf schema:MedicalEnumeration .

schema:MedicalWebPage a rdfs:Class ;
	rdfs:label "MedicalWebPage" ;
	rdfs:comment "A web page that provides medical information." ;
	rdfs:subClassOf schema:WebPage .

schema:MedicineSystem a rdfs:Class ;
	rdfs:label "MedicineSystem" ;
	rdfs:comment "Systems of medical practice." ;
	rdfs:subClassOf schema:MedicalEnumeration .

schema:MensClothingStore a rdfs:Class ;
	rdfs:label "MensClothingStore" ;
	rdfs:comment "A men's clothing store." ;
	rdfs:subClassOf schema:Store .

schema:MiddleSchool a rdfs:Class ;
	rdfs:label "MiddleSchool" ;
	rdfs:comment "A middle school." ;
	rdfs:subClassOf schema:EducationalOrganization .

schema:MobileApplication a rdfs:Class ;
	rdfs:label "MobileApplication" ;
	rdfs:comment "A mobile software application." ;
	rdfs:subClassOf schema:SoftwareApplication .

schema:MobilePhoneStore a rdfs:Class ;
	rdfs:label "MobilePhoneStore" ;
	rdfs:comment "A mobile-phone store." ;
	rdfs:subClassOf schema:Store .

schema:Mosque a rdfs:Class ;
	rdfs:label "Mosque" ;
	rdfs:comment "A mosque." ;
	rdfs:subClassOf schema:PlaceOfWorship .

schema:Motel a rdfs:Class ;
	rdfs:label "Motel" ;
	rdfs:comment "A motel." ;
	rdfs:subClassOf schema:LodgingBusiness .

schema:MotorcycleDealer a rdfs:Class ;
	rdfs:label "MotorcycleDealer" ;
	rdfs:comment "A motorcycle dealer." ;
	rdfs:subClassOf schema:AutomotiveBusiness .

schema:MotorcycleRepair a rdfs:Class ;
	rdfs:label "MotorcycleRepair" ;
	rdfs:comment "A motorcycle repair shop." ;
	rdfs:subClassOf schema:AutomotiveBusiness .

schema:Mountain a rdfs:Class ;
	rdfs:label "Mountain" ;
	rdfs:comment "A mountain, like Mount Whitney or Mount Everest" ;
	rdfs:subClassOf schema:Landform .

schema:MoveAction a rdfs:Class ;
	rdfs:label "MoveAction" ;
	rdfs:comment "The act of an agent relocating to a place.<p>Related actions:</p><ul><li><a href=\"http://schema.org/TransferAction\">TransferAction</a>: Unlike TransferAction, the subject of the move is a living Person or Organization rather than an inanimate object.</li></ul>" ;
	rdfs:subClassOf schema:Action .

schema:Movie a rdfs:Class ;
	rdfs:label "Movie" ;
	rdfs:comment "A movie." ;
	rdfs:subClassOf schema:CreativeWork .

schema:MovieRentalStore a rdfs:Class ;
	rdfs:label "MovieRentalStore" ;
	rdfs:comment "A movie rental store." ;
	rdfs:subClassOf schema:Store .

schema:MovieTheater a rdfs:Class ;
	rdfs:label "MovieTheater" ;
	rdfs:comment "A movie theater." ;
	rdfs:subClassOf schema:CivicStructure , schema:EntertainmentBusiness .

schema:MovingCompany a rdfs:Class ;
	rdfs:label "MovingCompany" ;
	rdfs:comment "A moving company." ;
	rdfs:subClassOf schema:HomeAndConstructionBusiness .

schema:Muscle a rdfs:Class ;
	rdfs:label "Muscle" ;
	dc:source <http://www.w3.org/wiki/WebSchemas/SchemaDotOrgSources#source_WikiDoc> ;
	rdfs:comment "A muscle is an anatomical structure consisting of a contractile form of tissue that animals use to effect movement." ;
	rdfs:subClassOf schema:AnatomicalStructure .

schema:Museum a rdfs:Class ;
	rdfs:label "Museum" ;
	rdfs:comment "A museum." ;
	rdfs:subClassOf schema:CivicStructure .

schema:MusicAlbum a rdfs:Class ;
	rdfs:label "MusicAlbum" ;
	rdfs:comment "A collection of music tracks." ;
	rdfs:subClassOf schema:MusicPlaylist .

schema:MusicEvent a rdfs:Class ;
	rdfs:label "MusicEvent" ;
	rdfs:comment "Event type: Music event." ;
	rdfs:subClassOf schema:Event .

schema:MusicGroup a rdfs:Class ;
	rdfs:label "MusicGroup" ;
	rdfs:comment "A musical group, such as a band, an orchestra, or a choir. Can also be a solo musician." ;
	rdfs:subClassOf schema:PerformingGroup .

schema:MusicPlaylist a rdfs:Class ;
	rdfs:label "MusicPlaylist" ;
	rdfs:comment "A collection of music tracks in playlist form." ;
	rdfs:subClassOf schema:CreativeWork .

schema:MusicRecording a rdfs:Class ;
	rdfs:label "MusicRecording" ;
	rdfs:comment "A music recording (track), usually a single song." ;
	rdfs:subClassOf schema:CreativeWork .

schema:MusicStore a rdfs:Class ;
	rdfs:label "MusicStore" ;
	rdfs:comment "A music store." ;
	rdfs:subClassOf schema:Store .

schema:MusicVenue a rdfs:Class ;
	rdfs:label "MusicVenue" ;
	rdfs:comment "A music venue." ;
	rdfs:subClassOf schema:CivicStructure .

schema:MusicVideoObject a rdfs:Class ;
	rdfs:label "MusicVideoObject" ;
	rdfs:comment "A music video file." ;
	rdfs:subClassOf schema:MediaObject .

schema:NGO a rdfs:Class ;
	rdfs:label "NGO" ;
	rdfs:comment "Organization: Non-governmental Organization." ;
	rdfs:subClassOf schema:Organization .

schema:NailSalon a rdfs:Class ;
	rdfs:label "NailSalon" ;
	rdfs:comment "A nail salon." ;
	rdfs:subClassOf schema:HealthAndBeautyBusiness .

schema:Nerve a rdfs:Class ;
	rdfs:label "Nerve" ;
	dc:source <http://www.w3.org/wiki/WebSchemas/SchemaDotOrgSources#source_WikiDoc> ;
	rdfs:comment "A common pathway for the electrochemical nerve impulses that are transmitted along each of the axons." ;
	rdfs:subClassOf schema:AnatomicalStructure .

schema:NewsArticle a rdfs:Class ;
	rdfs:label "NewsArticle" ;
	dc:source <http://www.w3.org/wiki/WebSchemas/SchemaDotOrgSources#source_rNews> ;
	rdfs:comment "A news article" ;
	rdfs:subClassOf schema:Article .

schema:NightClub a rdfs:Class ;
	rdfs:label "NightClub" ;
	rdfs:comment "A nightclub or discotheque." ;
	rdfs:subClassOf schema:EntertainmentBusiness .

schema:Notary a rdfs:Class ;
	rdfs:label "Notary" ;
	rdfs:comment "A notary." ;
	rdfs:subClassOf schema:ProfessionalService .

schema:Number a rdfs:Class ;
	rdfs:label "Number" ;
	rdfs:comment "Data type: Number." ;
	rdfs:subClassOf schema:DataType .

schema:NutritionInformation a rdfs:Class ;
	rdfs:label "NutritionInformation" ;
	rdfs:comment "Nutritional information about the recipe." ;
	rdfs:subClassOf schema:StructuredValue .

schema:OceanBodyOfWater a rdfs:Class ;
	rdfs:label "OceanBodyOfWater" ;
	rdfs:comment "An ocean (for example, the Pacific)." ;
	rdfs:subClassOf schema:BodyOfWater .

schema:Offer a rdfs:Class ;
	rdfs:label "Offer" ;
	dc:source <http://www.w3.org/wiki/WebSchemas/SchemaDotOrgSources#source_GoodRelationsProperties> ;
	rdfs:comment "An offer to sell an item&#x2014;for example, an offer to sell a product, the DVD of a movie, or tickets to an event." ;
	rdfs:subClassOf schema:Intangible .

schema:OfferItemCondition a rdfs:Class ;
	rdfs:label "OfferItemCondition" ;
	rdfs:comment "A list of possible conditions for the item for sale." ;
	rdfs:subClassOf schema:Enumeration .

schema:OfficeEquipmentStore a rdfs:Class ;
	rdfs:label "OfficeEquipmentStore" ;
	rdfs:comment "An office equipment store." ;
	rdfs:subClassOf schema:Store .

schema:OpeningHoursSpecification a rdfs:Class ;
	rdfs:label "OpeningHoursSpecification" ;
	dc:source <http://www.w3.org/wiki/WebSchemas/SchemaDotOrgSources#source_GoodRelationsClass> ;
	rdfs:comment "A structured value providing information about the opening hours of a place or a certain service inside a place." ;
	rdfs:subClassOf schema:StructuredValue .

schema:Optician a rdfs:Class ;
	rdfs:label "Optician" ;
	rdfs:comment "An optician's store." ;
	rdfs:subClassOf schema:MedicalOrganization .

schema:OrderAction a rdfs:Class ;
	rdfs:label "OrderAction" ;
	rdfs:comment "An agent orders an object/product/service to be delivered/sent." ;
	rdfs:subClassOf schema:TradeAction .

schema:Organization a rdfs:Class ;
	rdfs:label "Organization" ;
	rdfs:comment "An organization such as a school, NGO, corporation, club, etc." ;
	rdfs:subClassOf schema:Thing .

schema:OrganizeAction a rdfs:Class ;
	rdfs:label "OrganizeAction" ;
	rdfs:comment "The act of manipulating/administering/supervising/controlling one or more objects." ;
	rdfs:subClassOf schema:Action .

schema:OutletStore a rdfs:Class ;
	rdfs:label "OutletStore" ;
	rdfs:comment "An outlet store." ;
	rdfs:subClassOf schema:Store .

schema:OwnershipInfo a rdfs:Class ;
	rdfs:label "OwnershipInfo" ;
	dc:source <http://www.w3.org/wiki/WebSchemas/SchemaDotOrgSources#source_GoodRelationsClass> ;
	rdfs:comment "A structured value providing information about when a certain organization or person owned a certain product." ;
	rdfs:subClassOf schema:StructuredValue .

schema:PaintAction a rdfs:Class ;
	rdfs:label "PaintAction" ;
	rdfs:comment "The act of producing a painting, typically with paint and canvas as instruments." ;
	rdfs:subClassOf schema:CreateAction .

schema:Painting a rdfs:Class ;
	rdfs:label "Painting" ;
	rdfs:comment "A painting." ;
	rdfs:subClassOf schema:CreativeWork .

schema:PalliativeProcedure a rdfs:Class ;
	rdfs:label "PalliativeProcedure" ;
	dc:source <http://www.w3.org/wiki/WebSchemas/SchemaDotOrgSources#source_WikiDoc> ;
	rdfs:comment "A medical procedure intended primarly for palliative purposes, aimed at relieving the symptoms of an underlying health condition." ;
	rdfs:subClassOf schema:MedicalProcedure , schema:MedicalTherapy .

schema:ParcelService a rdfs:Class ;
	rdfs:label "ParcelService" ;
	dc:source <http://www.w3.org/wiki/WebSchemas/SchemaDotOrgSources#source_GoodRelationsClass> ;
	rdfs:comment """A private parcel service as the delivery mode available for a certain offer.

    Commonly used values:

    http://purl.org/goodrelations/v1#DHL
    http://purl.org/goodrelations/v1#FederalExpress
    http://purl.org/goodrelations/v1#UPS
    	""" ;
	rdfs:subClassOf schema:DeliveryMethod .

schema:ParentAudience a rdfs:Class ;
	rdfs:label "ParentAudience" ;
	rdfs:comment "A set of characteristics describing parents, who can be interested in viewing some content" ;
	rdfs:subClassOf schema:PeopleAudience .

schema:Park a rdfs:Class ;
	rdfs:label "Park" ;
	rdfs:comment "A park." ;
	rdfs:subClassOf schema:CivicStructure .

schema:ParkingFacility a rdfs:Class ;
	rdfs:label "ParkingFacility" ;
	rdfs:comment "A parking lot or other parking facility." ;
	rdfs:subClassOf schema:CivicStructure .

schema:PathologyTest a rdfs:Class ;
	rdfs:label "PathologyTest" ;
	dc:source <http://www.w3.org/wiki/WebSchemas/SchemaDotOrgSources#source_WikiDoc> ;
	rdfs:comment "A medical test performed by a laboratory that typically involves examination of a tissue sample by a pathologist." ;
	rdfs:subClassOf schema:MedicalTest .

schema:PawnShop a rdfs:Class ;
	rdfs:label "PawnShop" ;
	rdfs:comment "A pawnstore." ;
	rdfs:subClassOf schema:Store .

schema:PayAction a rdfs:Class ;
	rdfs:label "PayAction" ;
	rdfs:comment "An agent pays a price to a participant." ;
	rdfs:subClassOf schema:TradeAction .

schema:PaymentChargeSpecification a rdfs:Class ;
	rdfs:label "PaymentChargeSpecification" ;
	dc:source <http://www.w3.org/wiki/WebSchemas/SchemaDotOrgSources#source_GoodRelationsClass> ;
	rdfs:comment "The costs of settling the payment using a particular payment method." ;
	rdfs:subClassOf schema:PriceSpecification .

schema:PaymentMethod a rdfs:Class ;
	rdfs:label "PaymentMethod" ;
	dc:source <http://www.w3.org/wiki/WebSchemas/SchemaDotOrgSources#source_GoodRelationsClass> ;
	rdfs:comment """A payment method is a standardized procedure for transferring the monetary amount for a purchase. Payment methods are characterized by the legal and technical structures used, and by the organization or group carrying out the transaction.

    Commonly used values:

    http://purl.org/goodrelations/v1#ByBankTransferInAdvance
    http://purl.org/goodrelations/v1#ByInvoice
    http://purl.org/goodrelations/v1#Cash
    http://purl.org/goodrelations/v1#CheckInAdvance
    http://purl.org/goodrelations/v1#COD
    http://purl.org/goodrelations/v1#DirectDebit
    http://purl.org/goodrelations/v1#GoogleCheckout
    http://purl.org/goodrelations/v1#PayPal
    http://purl.org/goodrelations/v1#PaySwarm
    		""" ;
	rdfs:subClassOf schema:Enumeration .

schema:PeopleAudience a rdfs:Class ;
	rdfs:label "PeopleAudience" ;
	rdfs:comment "A set of characteristics belonging to people, e.g. who compose an item's target audience." ;
	rdfs:subClassOf schema:Audience .

schema:PerformAction a rdfs:Class ;
	rdfs:label "PerformAction" ;
	rdfs:comment "The act of participating in performance arts." ;
	rdfs:subClassOf schema:PlayAction .

schema:PerformingArtsTheater a rdfs:Class ;
	rdfs:label "PerformingArtsTheater" ;
	rdfs:comment "A theatre or other performing art center." ;
	rdfs:subClassOf schema:CivicStructure .

schema:PerformingGroup a rdfs:Class ;
	rdfs:label "PerformingGroup" ;
	rdfs:comment "A performance group, such as a band, an orchestra, or a circus." ;
	rdfs:subClassOf schema:Organization .

schema:Person a rdfs:Class ;
	rdfs:label "Person" ;
	dc:source <http://www.w3.org/wiki/WebSchemas/SchemaDotOrgSources#source_rNews> ;
	rdfs:comment "A person (alive, dead, undead, or fictional)." ;
	rdfs:subClassOf schema:Thing .

schema:PetStore a rdfs:Class ;
	rdfs:label "PetStore" ;
	rdfs:comment "A pet store." ;
	rdfs:subClassOf schema:Store .

schema:Pharmacy a rdfs:Class ;
	rdfs:label "Pharmacy" ;
	rdfs:comment "A pharmacy or drugstore." ;
	rdfs:subClassOf schema:MedicalOrganization .

schema:Photograph a rdfs:Class ;
	rdfs:label "Photograph" ;
	rdfs:comment "A photograph." ;
	rdfs:subClassOf schema:CreativeWork .

schema:PhotographAction a rdfs:Class ;
	rdfs:label "PhotographAction" ;
	rdfs:comment "The act of capturing still images of objects using a camera." ;
	rdfs:subClassOf schema:CreateAction .

schema:PhysicalActivity a rdfs:Class ;
	rdfs:label "PhysicalActivity" ;
	dc:source <http://www.w3.org/wiki/WebSchemas/SchemaDotOrgSources#source_WikiDoc> ;
	rdfs:comment "Any bodily activity that enhances or maintains physical fitness and overall health and wellness. Includes activity that is part of daily living and routine, structured exercise, and exercise prescribed as part of a medical treatment or recovery plan." ;
	rdfs:subClassOf schema:LifestyleModification .

schema:PhysicalActivityCategory a rdfs:Class ;
	rdfs:label "PhysicalActivityCategory" ;
	dc:source <http://www.w3.org/wiki/WebSchemas/SchemaDotOrgSources#source_WikiDoc> ;
	rdfs:comment "Categories of physical activity, organized by physiologic classification." ;
	rdfs:subClassOf schema:MedicalEnumeration .

schema:PhysicalExam a rdfs:Class ;
	rdfs:label "PhysicalExam" ;
	dc:source <http://www.w3.org/wiki/WebSchemas/SchemaDotOrgSources#source_WikiDoc> ;
	rdfs:comment "A type of physical examination of a patient performed by a physician. Enumerated type." ;
	rdfs:subClassOf schema:MedicalEnumeration .

schema:PhysicalTherapy a rdfs:Class ;
	rdfs:label "PhysicalTherapy" ;
	dc:source <http://www.w3.org/wiki/WebSchemas/SchemaDotOrgSources#source_WikiDoc> ;
	rdfs:comment "A process of progressive physical care and rehabilitation aimed at improving a health condition." ;
	rdfs:subClassOf schema:MedicalTherapy .

schema:Physician a rdfs:Class ;
	rdfs:label "Physician" ;
	rdfs:comment "A doctor's office." ;
	rdfs:subClassOf schema:MedicalOrganization .

schema:Place a rdfs:Class ;
	rdfs:label "Place" ;
	rdfs:comment "Entities that have a somewhat fixed, physical extension." ;
	rdfs:subClassOf schema:Thing .

schema:PlaceOfWorship a rdfs:Class ;
	rdfs:label "PlaceOfWorship" ;
	rdfs:comment "Place of worship, such as a church, synagogue, or mosque." ;
	rdfs:subClassOf schema:CivicStructure .

schema:PlanAction a rdfs:Class ;
	rdfs:label "PlanAction" ;
	rdfs:comment "The act of planning the execution of an event/task/action/reservation/plan to a future date." ;
	rdfs:subClassOf schema:OrganizeAction .

schema:PlayAction a rdfs:Class ;
	rdfs:label "PlayAction" ;
	rdfs:comment "The act of playing/exercising/training/performing for enjoyment, leisure, recreation, competion or exercise.<p>Related actions:</p><ul><li><a href=\"http://schema.org/ListenAction\">ListenAction</a>: Unlike ListenAction (which is under ConsumeAction), PlayAction refers to performing for an audience or at an event, rather than consuming music.</li><li><a href=\"http://schema.org/WatchAction\">WatchAction</a>: Unlike WatchAction (which is under ConsumeAction), PlayAction refers to showing/displaying for an audience or at an event, rather than consuming visual content.</li></ul>" ;
	rdfs:subClassOf schema:Action .

schema:Playground a rdfs:Class ;
	rdfs:label "Playground" ;
	rdfs:comment "A playground." ;
	rdfs:subClassOf schema:CivicStructure .

schema:Plumber a rdfs:Class ;
	rdfs:label "Plumber" ;
	rdfs:comment "A plumbing service." ;
	rdfs:subClassOf schema:HomeAndConstructionBusiness , schema:ProfessionalService .

schema:PoliceStation a rdfs:Class ;
	rdfs:label "PoliceStation" ;
	rdfs:comment "A police station." ;
	rdfs:subClassOf schema:CivicStructure , schema:EmergencyService .

schema:Pond a rdfs:Class ;
	rdfs:label "Pond" ;
	rdfs:comment "A pond" ;
	rdfs:subClassOf schema:BodyOfWater .

schema:PostOffice a rdfs:Class ;
	rdfs:label "PostOffice" ;
	rdfs:comment "A post office." ;
	rdfs:subClassOf schema:GovernmentOffice .

schema:PostalAddress a rdfs:Class ;
	rdfs:label "PostalAddress" ;
	rdfs:comment "The mailing address." ;
	rdfs:subClassOf schema:ContactPoint .

schema:PrependAction a rdfs:Class ;
	rdfs:label "PrependAction" ;
	rdfs:comment "The act of inserting at the beginning if an ordered collection." ;
	rdfs:subClassOf schema:InsertAction .

schema:Preschool a rdfs:Class ;
	rdfs:label "Preschool" ;
	rdfs:comment "A preschool." ;
	rdfs:subClassOf schema:EducationalOrganization .

schema:PreventionIndication a rdfs:Class ;
	rdfs:label "PreventionIndication" ;
	dc:source <http://www.w3.org/wiki/WebSchemas/SchemaDotOrgSources#source_WikiDoc> ;
	rdfs:comment "An indication for preventing an underlying condition, symptom, etc." ;
	rdfs:subClassOf schema:MedicalIndication .

schema:PriceSpecification a rdfs:Class ;
	rdfs:label "PriceSpecification" ;
	dc:source <http://www.w3.org/wiki/WebSchemas/SchemaDotOrgSources#source_GoodRelationsClass> ;
	rdfs:comment "A structured value representing a monetary amount. Typically, only the subclasses of this type are used for markup." ;
	rdfs:subClassOf schema:StructuredValue .

schema:Product a rdfs:Class ;
	rdfs:label "Product" ;
	dc:source <http://www.w3.org/wiki/WebSchemas/SchemaDotOrgSources#source_GoodRelationsProperties> ;
	rdfs:comment "A product is anything that is made available for salefor example, a pair of shoes, a concert ticket, or a car. Commodity services, like haircuts, can also be represented using this type." ;
	rdfs:subClassOf schema:Thing .

schema:ProductModel a rdfs:Class ;
	rdfs:label "ProductModel" ;
	dc:source <http://www.w3.org/wiki/WebSchemas/SchemaDotOrgSources#source_GoodRelationsClass> ;
	rdfs:comment "A datasheet or vendor specification of a product (in the sense of a prototypical description)." ;
	rdfs:subClassOf schema:Product .

schema:ProfessionalService a rdfs:Class ;
	rdfs:label "ProfessionalService" ;
	rdfs:comment "Provider of professional services." ;
	rdfs:subClassOf schema:LocalBusiness .

schema:ProfilePage a rdfs:Class ;
	rdfs:label "ProfilePage" ;
	rdfs:comment "Web page type: Profile page." ;
	rdfs:subClassOf schema:WebPage .

schema:Property a rdfs:Class ;
	rdfs:label "Property" ;
	rdfs:comment "A property, used to indicate attributes and relationships of some Thing; equivalent to rdf:Property." ;
	rdfs:subClassOf schema:Thing .

schema:PsychologicalTreatment a rdfs:Class ;
	rdfs:label "PsychologicalTreatment" ;
	dc:source <http://www.w3.org/wiki/WebSchemas/SchemaDotOrgSources#source_WikiDoc> ;
	rdfs:comment "A process of care relying upon counseling, dialogue, communication, verbalization aimed at improving a mental health condition." ;
	rdfs:subClassOf schema:MedicalTherapy .

schema:PublicSwimmingPool a rdfs:Class ;
	rdfs:label "PublicSwimmingPool" ;
	rdfs:comment "A public swimming pool." ;
	rdfs:subClassOf schema:SportsActivityLocation .

schema:QualitativeValue a rdfs:Class ;
	rdfs:label "QualitativeValue" ;
	dc:source <http://www.w3.org/wiki/WebSchemas/SchemaDotOrgSources#source_GoodRelationsClass> ;
	rdfs:comment "A predefined value for a product characteristic, e.g. the the power cord plug type \"US\" or the garment sizes \"S\", \"M\", \"L\", and \"XL\"" ;
	rdfs:subClassOf schema:Enumeration .

schema:QuantitativeValue a rdfs:Class ;
	rdfs:label "QuantitativeValue" ;
	dc:source <http://www.w3.org/wiki/WebSchemas/SchemaDotOrgSources#source_GoodRelationsClass> ;
	rdfs:comment " A point value or interval for product characteristics and other purposes." ;
	rdfs:subClassOf schema:StructuredValue .

schema:Quantity a rdfs:Class ;
	rdfs:label "Quantity" ;
	rdfs:comment "Quantities such as distance, time, mass, weight, etc. Particular instances of say Mass are entities like '3 Kg' or '4 milligrams'." ;
	rdfs:subClassOf schema:Intangible .

schema:QuoteAction a rdfs:Class ;
	rdfs:label "QuoteAction" ;
	rdfs:comment "An agent quotes/estimates/appraises an object/product/service with a price at a location/store." ;
	rdfs:subClassOf schema:TradeAction .

schema:RVPark a rdfs:Class ;
	rdfs:label "RVPark" ;
	rdfs:comment "An RV park." ;
	rdfs:subClassOf schema:CivicStructure .

schema:RadiationTherapy a rdfs:Class ;
	rdfs:label "RadiationTherapy" ;
	dc:source <http://www.w3.org/wiki/WebSchemas/SchemaDotOrgSources#source_WikiDoc> ;
	rdfs:comment "A process of care using radiation aimed at improving a health condition." ;
	rdfs:subClassOf schema:MedicalTherapy .

schema:RadioStation a rdfs:Class ;
	rdfs:label "RadioStation" ;
	rdfs:comment "A radio station." ;
	rdfs:subClassOf schema:LocalBusiness .

schema:Rating a rdfs:Class ;
	rdfs:label "Rating" ;
	rdfs:comment "The rating of the video." ;
	rdfs:subClassOf schema:Intangible .

schema:ReactAction a rdfs:Class ;
	rdfs:label "ReactAction" ;
	rdfs:comment "The act of responding instinctively and emotionally to an object, expressing a sentiment." ;
	rdfs:subClassOf schema:AssessAction .

schema:ReadAction a rdfs:Class ;
	rdfs:label "ReadAction" ;
	rdfs:comment "The act of consuming written content." ;
	rdfs:subClassOf schema:ConsumeAction .

schema:RealEstateAgent a rdfs:Class ;
	rdfs:label "RealEstateAgent" ;
	rdfs:comment "A real-estate agent." ;
	rdfs:subClassOf schema:LocalBusiness .

schema:ReceiveAction a rdfs:Class ;
	rdfs:label "ReceiveAction" ;
	rdfs:comment "The act of physically/electronically taking delivery of an object thathas been transferred from an origin to a destination. Reciprocal of SendAction.<p>Related actions:</p><ul><li><a href=\"http://schema.org/SendAction\">SendAction</a>: The reciprocal of ReceiveAction.</li><li><a href=\"http://schema.org/TakeAction\">TakeAction</a>: Unlike TakeAction, ReceiveAction does not imply that the ownership has been transfered (e.g. I can receive a package, but it does not mean the package is now mine).</li></ul>" ;
	rdfs:subClassOf schema:TransferAction .

schema:Recipe a rdfs:Class ;
	rdfs:label "Recipe" ;
	rdfs:comment "A recipe." ;
	rdfs:subClassOf schema:CreativeWork .

schema:RecommendedDoseSchedule a rdfs:Class ;
	rdfs:label "RecommendedDoseSchedule" ;
	rdfs:comment "A recommended dosing schedule for a drug or supplement as prescribed or recommended by an authority or by the drug/supplement's manufacturer. Capture the recommending authority in the recognizingAuthority property of MedicalEntity." ;
	rdfs:subClassOf schema:DoseSchedule .

schema:RecyclingCenter a rdfs:Class ;
	rdfs:label "RecyclingCenter" ;
	rdfs:comment "A recycling center." ;
	rdfs:subClassOf schema:LocalBusiness .

schema:RegisterAction a rdfs:Class ;
	rdfs:label "RegisterAction" ;
	rdfs:comment "The act of registering to be a user of a service, product or web page.<p>Related actions:</p><ul><li><a href=\"http://schema.org/JoinAction\">JoinAction</a>: Unlike JoinAction, RegisterAction implies you are registering to be a user of a service, *not* a group/team of people.</li><li><a href=\"http://schema.org/FollowAction\">FollowAction</a>: Unlike FollowAction, RegisterAction doesn't imply that the agent is expecting to poll for updates from the object.</li><li><a href=\"http://schema.org/SubscribeAction\">SubscribeAction</a>: Unlike SubscribeAction, RegisterAction doesn't imply that the agent is expecting updates from the object.</li></ul>" ;
	rdfs:subClassOf schema:InteractAction .

schema:RejectAction a rdfs:Class ;
	rdfs:label "RejectAction" ;
	rdfs:comment "The act of rejecting to/adopting an object.<p>Related actions:</p><ul><li><a href=\"http://schema.org/AcceptAction\">AcceptAction</a>: The antagonym of RejectAction.</li></ul>" ;
	rdfs:subClassOf schema:AllocateAction .

schema:RentAction a rdfs:Class ;
	rdfs:label "RentAction" ;
	rdfs:comment "The act of giving money in return for temporary use, but not ownership, of an object such as a vehicle or property. For example, an agent rents a property from a landlord in exchange for a periodic payment." ;
	rdfs:subClassOf schema:TradeAction .

schema:ReplaceAction a rdfs:Class ;
	rdfs:label "ReplaceAction" ;
	rdfs:comment "The act of editing a recipient by replacing an old object with a new object." ;
	rdfs:subClassOf schema:UpdateAction .

schema:ReplyAction a rdfs:Class ;
	rdfs:label "ReplyAction" ;
	rdfs:comment "The act of responding to a question/message asked/sent by the object. Related to <a href=\"AskAction\">AskAction</a>.<p>Related actions:</p><ul><li><a href=\"http://schema.org/AskAction\">AskAction</a>: Appears generally as an origin of a ReplyAction.</li></ul>" ;
	rdfs:subClassOf schema:CommunicateAction .

schema:ReportedDoseSchedule a rdfs:Class ;
	rdfs:label "ReportedDoseSchedule" ;
	rdfs:comment "A patient-reported or observed dosing schedule for a drug or supplement." ;
	rdfs:subClassOf schema:DoseSchedule .

schema:ReserveAction a rdfs:Class ;
	rdfs:label "ReserveAction" ;
	rdfs:comment "Reserving a concrete object.<p>Related actions:</p><ul><li><a href=\"http://schema.org/ScheduleAction\">ScheduleAction</a>: Unlike ScheduleAction, ReserveAction reserves concrete objects (e.g. a table, a hotel) towards a time slot / spatial allocation.</li></ul>" ;
	rdfs:subClassOf schema:PlanAction .

schema:Reservoir a rdfs:Class ;
	rdfs:label "Reservoir" ;
	rdfs:comment "A reservoir, like the Lake Kariba reservoir." ;
	rdfs:subClassOf schema:BodyOfWater .

schema:Residence a rdfs:Class ;
	rdfs:label "Residence" ;
	rdfs:comment "The place where a person lives." ;
	rdfs:subClassOf schema:Place .

schema:Restaurant a rdfs:Class ;
	rdfs:label "Restaurant" ;
	rdfs:comment "A restaurant." ;
	rdfs:subClassOf schema:FoodEstablishment .

schema:ReturnAction a rdfs:Class ;
	rdfs:label "ReturnAction" ;
	rdfs:comment "The act of returning to the origin that which was previously received (concrete objects) or taken (ownership)." ;
	rdfs:subClassOf schema:TransferAction .

schema:Review a rdfs:Class ;
	rdfs:label "Review" ;
	rdfs:comment "A review of an item - for example, a restaurant, movie, or store." ;
	rdfs:subClassOf schema:CreativeWork .

schema:ReviewAction a rdfs:Class ;
	rdfs:label "ReviewAction" ;
	rdfs:comment "The act of producing a balanced opinion about the object for an audience. An agent reviews an object with participants resulting in a review." ;
	rdfs:subClassOf schema:AssessAction .

schema:RiverBodyOfWater a rdfs:Class ;
	rdfs:label "RiverBodyOfWater" ;
	rdfs:comment "A river (for example, the broad majestic Shannon)." ;
	rdfs:subClassOf schema:BodyOfWater .

schema:RoofingContractor a rdfs:Class ;
	rdfs:label "RoofingContractor" ;
	rdfs:comment "A roofing contractor." ;
	rdfs:subClassOf schema:HomeAndConstructionBusiness , schema:ProfessionalService .

schema:RsvpAction a rdfs:Class ;
	rdfs:label "RsvpAction" ;
	rdfs:comment "The act of notifying an event organiser as to whether you expect to attend the event." ;
	rdfs:subClassOf schema:InformAction .

schema:SaleEvent a rdfs:Class ;
	rdfs:label "SaleEvent" ;
	rdfs:comment "Event type: Sales event." ;
	rdfs:subClassOf schema:Event .

schema:ScheduleAction a rdfs:Class ;
	rdfs:label "ScheduleAction" ;
	rdfs:comment "Scheduling future actions, events, or tasks.<p>Related actions:</p><ul><li><a href=\"http://schema.org/ReserveAction\">ReserveAction</a>: Unlike ReserveAction, ScheduleAction allocates future actions (e.g. an event, a task, etc) towards a time slot / spatial allocation.</li></ul>" ;
	rdfs:subClassOf schema:PlanAction .

schema:ScholarlyArticle a rdfs:Class ;
	rdfs:label "ScholarlyArticle" ;
	rdfs:comment "A scholarly article." ;
	rdfs:subClassOf schema:Article .

schema:School a rdfs:Class ;
	rdfs:label "School" ;
	rdfs:comment "A school." ;
	rdfs:subClassOf schema:EducationalOrganization .

schema:Sculpture a rdfs:Class ;
	rdfs:label "Sculpture" ;
	rdfs:comment "A piece of sculpture." ;
	rdfs:subClassOf schema:CreativeWork .

schema:SeaBodyOfWater a rdfs:Class ;
	rdfs:label "SeaBodyOfWater" ;
	rdfs:comment "A sea (for example, the Caspian sea)." ;
	rdfs:subClassOf schema:BodyOfWater .

schema:SearchAction a rdfs:Class ;
	rdfs:label "SearchAction" ;
	rdfs:comment "The act of searching for an object.<p>Related actions:</p><ul><li><a href=\"http://schema.org/FindAction\">FindAction</a>: SearchAction generally leads to a FindAction, but not necessarily.</li></ul>" ;
	rdfs:subClassOf schema:Action .

schema:SearchResultsPage a rdfs:Class ;
	rdfs:label "SearchResultsPage" ;
	rdfs:comment "Web page type: Search results page." ;
	rdfs:subClassOf schema:WebPage .

schema:SelfStorage a rdfs:Class ;
	rdfs:label "SelfStorage" ;
	rdfs:comment "Self-storage facility." ;
	rdfs:subClassOf schema:LocalBusiness .

schema:SellAction a rdfs:Class ;
	rdfs:label "SellAction" ;
	rdfs:comment "The act of taking money from a buyer in exchange for goods or services rendered. An agent sells an object, product, or service to a buyer for a price. Reciprocal of BuyAction." ;
	rdfs:subClassOf schema:TradeAction .

schema:SendAction a rdfs:Class ;
	rdfs:label "SendAction" ;
	rdfs:comment "The act of physically/electronically dispatching an object for transfer from an origin to a destination.<p>Related actions:</p><ul><li><a href=\"http://schema.org/ReceiveAction\">ReceiveAction</a>: The reciprocal of SendAction.</li><li><a href=\"http://schema.org/GiveAction\">GiveAction</a>: Unlike GiveAction, SendAction does not imply the transfer of ownership (e.g. I can send you my laptop, but I'm not necessarily giving it to you).</li></ul>" ;
	rdfs:subClassOf schema:TransferAction .

schema:ShareAction a rdfs:Class ;
	rdfs:label "ShareAction" ;
	rdfs:comment "The act of distributing content to people for their amusement or edification." ;
	rdfs:subClassOf schema:CommunicateAction .

schema:ShoeStore a rdfs:Class ;
	rdfs:label "ShoeStore" ;
	rdfs:comment "A shoe store." ;
	rdfs:subClassOf schema:Store .

schema:ShoppingCenter a rdfs:Class ;
	rdfs:label "ShoppingCenter" ;
	rdfs:comment "A shopping center or mall." ;
	rdfs:subClassOf schema:LocalBusiness .

schema:SingleFamilyResidence a rdfs:Class ;
	rdfs:label "SingleFamilyResidence" ;
	rdfs:comment "Residence type: Single-family home." ;
	rdfs:subClassOf schema:Residence .

schema:SiteNavigationElement a rdfs:Class ;
	rdfs:label "SiteNavigationElement" ;
	rdfs:comment "A navigation element of the page." ;
	rdfs:subClassOf schema:WebPageElement .

schema:SkiResort a rdfs:Class ;
	rdfs:label "SkiResort" ;
	rdfs:comment "A ski resort." ;
	rdfs:subClassOf schema:SportsActivityLocation .

schema:SocialEvent a rdfs:Class ;
	rdfs:label "SocialEvent" ;
	rdfs:comment "Event type: Social event." ;
	rdfs:subClassOf schema:Event .

schema:SoftwareApplication a rdfs:Class ;
	rdfs:label "SoftwareApplication" ;
	rdfs:comment "A software application." ;
	rdfs:subClassOf schema:CreativeWork .

schema:SomeProducts a rdfs:Class ;
	rdfs:label "SomeProducts" ;
	dc:source <http://www.w3.org/wiki/WebSchemas/SchemaDotOrgSources#source_GoodRelationsClass> ;
	rdfs:comment "A placeholder for multiple similar products of the same kind." ;
	rdfs:subClassOf schema:Product .

schema:Specialty a rdfs:Class ;
	rdfs:label "Specialty" ;
	rdfs:comment "Any branch of a field in which people typically develop specific expertise, usually after significant study, time, and effort." ;
	rdfs:subClassOf schema:Enumeration .

schema:SportingGoodsStore a rdfs:Class ;
	rdfs:label "SportingGoodsStore" ;
	rdfs:comment "A sporting goods store." ;
	rdfs:subClassOf schema:Store .

schema:SportsActivityLocation a rdfs:Class ;
	rdfs:label "SportsActivityLocation" ;
	rdfs:comment "A sports location, such as a playing field." ;
	rdfs:subClassOf schema:LocalBusiness .

schema:SportsClub a rdfs:Class ;
	rdfs:label "SportsClub" ;
	rdfs:comment "A sports club." ;
	rdfs:subClassOf schema:SportsActivityLocation .

schema:SportsEvent a rdfs:Class ;
	rdfs:label "SportsEvent" ;
	rdfs:comment "Event type: Sports event." ;
	rdfs:subClassOf schema:Event .

schema:SportsTeam a rdfs:Class ;
	rdfs:label "SportsTeam" ;
	rdfs:comment "Organization: Sports team." ;
	rdfs:subClassOf schema:Organization .

schema:StadiumOrArena a rdfs:Class ;
	rdfs:label "StadiumOrArena" ;
	rdfs:comment "A stadium." ;
	rdfs:subClassOf schema:CivicStructure , schema:SportsActivityLocation .

schema:State a rdfs:Class ;
	rdfs:label "State" ;
	rdfs:comment "A state or province." ;
	rdfs:subClassOf schema:AdministrativeArea .

schema:Store a rdfs:Class ;
	rdfs:label "Store" ;
	rdfs:comment "A retail good store." ;
	rdfs:subClassOf schema:LocalBusiness .

schema:StructuredValue a rdfs:Class ;
	rdfs:label "StructuredValue" ;
	rdfs:comment "Structured values are strings&#x2014;for example, addresses&#x2014;that have certain constraints on their structure." ;
	rdfs:subClassOf schema:Intangible .

schema:SubscribeAction a rdfs:Class ;
	rdfs:label "SubscribeAction" ;
	rdfs:comment "The act of forming a personal connection with someone/something (object) unidirectionally/asymmetrically to get updates pushed to.<p>Related actions:</p><ul><li><a href=\"http://schema.org/FollowAction\">FollowAction</a>: Unlike FollowAction, SubscribeAction implies that the subscriber acts as a passive agent being constantly/actively pushed for updates.</li><li><a href=\"http://schema.org/RegisterAction\">RegisterAction</a>: Unlike RegisterAction, SubscribeAction implies that the agent is interested in continuing receiving updates from the object.</li><li><a href=\"http://schema.org/JoinAction\">JoinAction</a>: Unlike JoinAction, SubscribeAction implies that the agent is interested in continuing receiving updates from the object.</li></ul>" ;
	rdfs:subClassOf schema:InteractAction .

schema:SubwayStation a rdfs:Class ;
	rdfs:label "SubwayStation" ;
	rdfs:comment "A subway station." ;
	rdfs:subClassOf schema:CivicStructure .

schema:SuperficialAnatomy a rdfs:Class ;
	rdfs:label "SuperficialAnatomy" ;
	dc:source <http://www.w3.org/wiki/WebSchemas/SchemaDotOrgSources#source_WikiDoc> ;
	rdfs:comment "Anatomical features that can be observed by sight (without dissection), including the form and proportions of the human body as well as surface landmarks that correspond to deeper subcutaneous structures. Superficial anatomy plays an important role in sports medicine, phlebotomy, and other medical specialties as underlying anatomical structures can be identified through surface palpation. For example, during back surgery, superficial anatomy can be used to palpate and count vertebrae to find the site of incision. Or in phlebotomy, superficial anatomy can be used to locate an underlying vein; for example, the median cubital vein can be located by palpating the borders of the cubital fossa (such as the epicondyles of the humerus) and then looking for the superficial signs of the vein, such as size, prominence, ability to refill after depression, and feel of surrounding tissue support. As another example, in a subluxation (dislocation) of the glenohumeral joint, the bony structure becomes pronounced with the deltoid muscle failing to cover the glenohumeral joint allowing the edges of the scapula to be superficially visible. Here, the superficial anatomy is the visible edges of the scapula, implying the underlying dislocation of the joint (the related anatomical structure)." ;
	rdfs:subClassOf schema:MedicalEntity .

schema:Synagogue a rdfs:Class ;
	rdfs:label "Synagogue" ;
	rdfs:comment "A synagogue." ;
	rdfs:subClassOf schema:PlaceOfWorship .

schema:TVEpisode a rdfs:Class ;
	rdfs:label "TVEpisode" ;
	rdfs:comment "An episode of a TV series or season." ;
	rdfs:subClassOf schema:CreativeWork .

schema:TVSeason a rdfs:Class ;
	rdfs:label "TVSeason" ;
	rdfs:comment "A TV season." ;
	rdfs:subClassOf schema:CreativeWork .

schema:TVSeries a rdfs:Class ;
	rdfs:label "TVSeries" ;
	rdfs:comment "A television series." ;
	rdfs:subClassOf schema:CreativeWork .

schema:Table a rdfs:Class ;
	rdfs:label "Table" ;
	rdfs:comment "A table on the page." ;
	rdfs:subClassOf schema:WebPageElement .

schema:TakeAction a rdfs:Class ;
	rdfs:label "TakeAction" ;
	rdfs:comment "The act of gaining ownership of an object from an origin. Reciprocal of GiveAction.<p>Related actions:</p><ul><li><a href=\"http://schema.org/GiveAction\">GiveAction</a>: The reciprocal of TakeAction.</li><li><a href=\"http://schema.org/ReceiveAction\">ReceiveAction</a>: Unlike ReceiveAction, TakeAction implies that ownership has been transfered.</li></ul>" ;
	rdfs:subClassOf schema:TransferAction .

schema:TattooParlor a rdfs:Class ;
	rdfs:label "TattooParlor" ;
	rdfs:comment "A tattoo parlor." ;
	rdfs:subClassOf schema:HealthAndBeautyBusiness .

schema:TaxiStand a rdfs:Class ;
	rdfs:label "TaxiStand" ;
	rdfs:comment "A taxi stand." ;
	rdfs:subClassOf schema:CivicStructure .

schema:TechArticle a rdfs:Class ;
	rdfs:label "TechArticle" ;
	rdfs:comment "A technical article - Example: How-to (task) topics, step-by-step, procedural troubleshooting, specifications, etc." ;
	rdfs:subClassOf schema:Article .

schema:TelevisionStation a rdfs:Class ;
	rdfs:label "TelevisionStation" ;
	rdfs:comment "A television station." ;
	rdfs:subClassOf schema:LocalBusiness .

schema:TennisComplex a rdfs:Class ;
	rdfs:label "TennisComplex" ;
	rdfs:comment "A tennis complex." ;
	rdfs:subClassOf schema:SportsActivityLocation .

schema:Text a rdfs:Class ;
	rdfs:label "Text" ;
	rdfs:comment "Data type: Text." ;
	rdfs:subClassOf schema:DataType .

schema:TheaterEvent a rdfs:Class ;
	rdfs:label "TheaterEvent" ;
	rdfs:comment "Event type: Theater performance." ;
	rdfs:subClassOf schema:Event .

schema:TheaterGroup a rdfs:Class ;
	rdfs:label "TheaterGroup" ;
	rdfs:comment "A theater group or company&#x2014;for example, the Royal Shakespeare Company or Druid Theatre." ;
	rdfs:subClassOf schema:PerformingGroup .

schema:TherapeuticProcedure a rdfs:Class ;
	rdfs:label "TherapeuticProcedure" ;
	dc:source <http://www.w3.org/wiki/WebSchemas/SchemaDotOrgSources#source_WikiDoc> ;
	rdfs:comment "A medical procedure intended primarly for therapeutic purposes, aimed at improving a health condition." ;
	rdfs:subClassOf schema:MedicalProcedure , schema:MedicalTherapy .

schema:Thing a rdfs:Class ;
	rdfs:label "Thing" ;
	rdfs:comment "The most generic type of item." .

schema:TieAction a rdfs:Class ;
	rdfs:label "TieAction" ;
	rdfs:comment "The act of reaching a draw in a competitive activity." ;
	rdfs:subClassOf schema:AchieveAction .

schema:Time a rdfs:Class ;
	rdfs:label "Time" ;
	rdfs:comment "A point in time recurring on multiple days in the form hh:mm:ss[Z|(+|-)hh:mm] (see <a href=\"http://www.w3.org/TR/xmlschema-2/#time\">XML schema for details</a>)." ;
	rdfs:subClassOf schema:DataType .

schema:TipAction a rdfs:Class ;
	rdfs:label "TipAction" ;
	rdfs:comment "The act of giving money voluntarily to a beneficiary in recognition of services rendered." ;
	rdfs:subClassOf schema:TradeAction .

schema:TireShop a rdfs:Class ;
	rdfs:label "TireShop" ;
	rdfs:comment "A tire shop." ;
	rdfs:subClassOf schema:Store .

schema:TouristAttraction a rdfs:Class ;
	rdfs:label "TouristAttraction" ;
	rdfs:comment "A tourist attraction." ;
	rdfs:subClassOf schema:Place .

schema:TouristInformationCenter a rdfs:Class ;
	rdfs:label "TouristInformationCenter" ;
	rdfs:comment "A tourist information center." ;
	rdfs:subClassOf schema:LocalBusiness .

schema:ToyStore a rdfs:Class ;
	rdfs:label "ToyStore" ;
	rdfs:comment "A toystore." ;
	rdfs:subClassOf schema:Store .

schema:TrackAction a rdfs:Class ;
	rdfs:label "TrackAction" ;
	rdfs:comment "An agent tracks an object for updates.<p>Related actions:</p><ul><li><a href=\"http://schema.org/FollowAction\">FollowAction</a>: Unlike FollowAction, TrackAction refers to the interest on the location of innanimates objects.</li><li><a href=\"http://schema.org/SubscribeAction\">SubscribeAction</a>: Unlike SubscribeAction, TrackAction refers to  the interest on the location of innanimate objects.</li></ul>" ;
	rdfs:subClassOf schema:FindAction .

schema:TradeAction a rdfs:Class ;
	rdfs:label "TradeAction" ;
	rdfs:comment "The act of participating in an exchange of goods and services for monetary compensation. An agent trades an object, product or service with a participant in exchange for a one time or periodic payment." ;
	rdfs:subClassOf schema:Action .

schema:TrainStation a rdfs:Class ;
	rdfs:label "TrainStation" ;
	rdfs:comment "A train station." ;
	rdfs:subClassOf schema:CivicStructure .

schema:TransferAction a rdfs:Class ;
	rdfs:label "TransferAction" ;
	rdfs:comment "The act of transferring/moving (abstract or concrete) animate or inanimate objects from one place to another." ;
	rdfs:subClassOf schema:Action .

schema:TravelAction a rdfs:Class ;
	rdfs:label "TravelAction" ;
	rdfs:comment "The act of traveling from an fromLocation to a destination by a specified mode of transport, optionally with participants." ;
	rdfs:subClassOf schema:MoveAction .

schema:TravelAgency a rdfs:Class ;
	rdfs:label "TravelAgency" ;
	rdfs:comment "A travel agency." ;
	rdfs:subClassOf schema:LocalBusiness .

schema:TreatmentIndication a rdfs:Class ;
	rdfs:label "TreatmentIndication" ;
	dc:source <http://www.w3.org/wiki/WebSchemas/SchemaDotOrgSources#source_WikiDoc> ;
	rdfs:comment "An indication for treating an underlying condition, symptom, etc." ;
	rdfs:subClassOf schema:MedicalIndication .

schema:TypeAndQuantityNode a rdfs:Class ;
	rdfs:label "TypeAndQuantityNode" ;
	dc:source <http://www.w3.org/wiki/WebSchemas/SchemaDotOrgSources#source_GoodRelationsClass> ;
	rdfs:comment "A structured value indicating the quantity, unit of measurement, and business function of goods included in a bundle offer." ;
	rdfs:subClassOf schema:StructuredValue .

schema:URL a rdfs:Class ;
	rdfs:label "URL" ;
	rdfs:comment "Data type: URL." ;
	rdfs:subClassOf schema:Text .

schema:UnRegisterAction a rdfs:Class ;
	rdfs:label "UnRegisterAction" ;
	rdfs:comment "The act of un-registering from a service.<p>Related actions:</p><ul><li><a href=\"http://schema.org/RegisterAction\">RegisterAction</a>: Antagonym of UnRegisterAction.</li><li><a href=\"http://schema.org/Leave\">Leave</a>: Unlike LeaveAction, UnRegisterAction implies that you are unregistering from a service you werer previously registered, rather than leaving a team/group of people.</li></ul>" ;
	rdfs:subClassOf schema:InteractAction .

schema:UnitPriceSpecification a rdfs:Class ;
	rdfs:label "UnitPriceSpecification" ;
	dc:source <http://www.w3.org/wiki/WebSchemas/SchemaDotOrgSources#source_GoodRelationsClass> ;
	rdfs:comment "The price asked for a given offer by the respective organization or person." ;
	rdfs:subClassOf schema:PriceSpecification .

schema:UpdateAction a rdfs:Class ;
	rdfs:label "UpdateAction" ;
	rdfs:comment "The act of managing by changing/editing the state of the object." ;
	rdfs:subClassOf schema:Action .

schema:UseAction a rdfs:Class ;
	rdfs:label "UseAction" ;
	rdfs:comment "The act of applying an object to its intended purpose." ;
	rdfs:subClassOf schema:ConsumeAction .

schema:UserBlocks a rdfs:Class ;
	rdfs:label "UserBlocks" ;
	rdfs:comment "User interaction: Block this content." ;
	rdfs:subClassOf schema:UserInteraction .

schema:UserCheckins a rdfs:Class ;
	rdfs:label "UserCheckins" ;
	rdfs:comment "User interaction: Check-in at a place." ;
	rdfs:subClassOf schema:UserInteraction .

schema:UserComments a rdfs:Class ;
	rdfs:label "UserComments" ;
	dc:source <http://www.w3.org/wiki/WebSchemas/SchemaDotOrgSources#source_rNews> ;
	rdfs:comment "The UserInteraction event in which a user comments on an item." ;
	rdfs:subClassOf schema:UserInteraction .

schema:UserDownloads a rdfs:Class ;
	rdfs:label "UserDownloads" ;
	rdfs:comment "User interaction: Download of an item." ;
	rdfs:subClassOf schema:UserInteraction .

schema:UserInteraction a rdfs:Class ;
	rdfs:label "UserInteraction" ;
	rdfs:comment "A user interacting with a page" ;
	rdfs:subClassOf schema:Event .

schema:UserLikes a rdfs:Class ;
	rdfs:label "UserLikes" ;
	rdfs:comment "User interaction: Like an item." ;
	rdfs:subClassOf schema:UserInteraction .

schema:UserPageVisits a rdfs:Class ;
	rdfs:label "UserPageVisits" ;
	rdfs:comment "User interaction: Visit to a web page." ;
	rdfs:subClassOf schema:UserInteraction .

schema:UserPlays a rdfs:Class ;
	rdfs:label "UserPlays" ;
	rdfs:comment "User interaction: Play count of an item, for example a video or a song." ;
	rdfs:subClassOf schema:UserInteraction .

schema:UserPlusOnes a rdfs:Class ;
	rdfs:label "UserPlusOnes" ;
	rdfs:comment "User interaction: +1." ;
	rdfs:subClassOf schema:UserInteraction .

schema:UserTweets a rdfs:Class ;
	rdfs:label "UserTweets" ;
	rdfs:comment "User interaction: Tweets." ;
	rdfs:subClassOf schema:UserInteraction .

schema:Vein a rdfs:Class ;
	rdfs:label "Vein" ;
	dc:source <http://www.w3.org/wiki/WebSchemas/SchemaDotOrgSources#source_WikiDoc> ;
	rdfs:comment "A type of blood vessel that specifically carries blood to the heart." ;
	rdfs:subClassOf schema:Vessel .

schema:Vessel a rdfs:Class ;
	rdfs:label "Vessel" ;
	dc:source <http://www.w3.org/wiki/WebSchemas/SchemaDotOrgSources#source_WikiDoc> ;
	rdfs:comment "A component of the human body circulatory system comprised of an intricate network of hollow tubes that transport blood throughout the entire body." ;
	rdfs:subClassOf schema:AnatomicalStructure .

schema:VeterinaryCare a rdfs:Class ;
	rdfs:label "VeterinaryCare" ;
	rdfs:comment "A vet's office." ;
	rdfs:subClassOf schema:MedicalOrganization .

schema:VideoGallery a rdfs:Class ;
	rdfs:label "VideoGallery" ;
	rdfs:comment "Web page type: Video gallery page." ;
	rdfs:subClassOf schema:CollectionPage .

schema:VideoObject a rdfs:Class ;
	rdfs:label "VideoObject" ;
	dc:source <http://www.w3.org/wiki/WebSchemas/SchemaDotOrgSources#source_rNews> ;
	rdfs:comment "A video file." ;
	rdfs:subClassOf schema:MediaObject .

schema:ViewAction a rdfs:Class ;
	rdfs:label "ViewAction" ;
	rdfs:comment "The act of consuming static visual content." ;
	rdfs:subClassOf schema:ConsumeAction .

schema:VisualArtsEvent a rdfs:Class ;
	rdfs:label "VisualArtsEvent" ;
	rdfs:comment "Event type: Visual arts event." ;
	rdfs:subClassOf schema:Event .

schema:Volcano a rdfs:Class ;
	rdfs:label "Volcano" ;
	rdfs:comment "A volcano, like Fuji san" ;
	rdfs:subClassOf schema:Landform .

schema:VoteAction a rdfs:Class ;
	rdfs:label "VoteAction" ;
	rdfs:comment "The act of expressing a preference from a fixed/finite/structured set of choices/options." ;
	rdfs:subClassOf schema:ChooseAction .

schema:WPAdBlock a rdfs:Class ;
	rdfs:label "WPAdBlock" ;
	rdfs:comment "An advertising section of the page." ;
	rdfs:subClassOf schema:WebPageElement .

schema:WPFooter a rdfs:Class ;
	rdfs:label "WPFooter" ;
	rdfs:comment "The footer section of the page." ;
	rdfs:subClassOf schema:WebPageElement .

schema:WPHeader a rdfs:Class ;
	rdfs:label "WPHeader" ;
	rdfs:comment "The header section of the page." ;
	rdfs:subClassOf schema:WebPageElement .

schema:WPSideBar a rdfs:Class ;
	rdfs:label "WPSideBar" ;
	rdfs:comment "A sidebar section of the page." ;
	rdfs:subClassOf schema:WebPageElement .

schema:WantAction a rdfs:Class ;
	rdfs:label "WantAction" ;
	rdfs:comment "The act of expressing a desire about the object. An agent wants an object." ;
	rdfs:subClassOf schema:ReactAction .

schema:WarrantyPromise a rdfs:Class ;
	rdfs:label "WarrantyPromise" ;
	dc:source <http://www.w3.org/wiki/WebSchemas/SchemaDotOrgSources#source_GoodRelationsClass> ;
	rdfs:comment "A structured value representing the duration and scope of services that will be provided to a customer free of charge in case of a defect or malfunction of a product." ;
	rdfs:subClassOf schema:StructuredValue .

schema:WarrantyScope a rdfs:Class ;
	rdfs:label "WarrantyScope" ;
	dc:source <http://www.w3.org/wiki/WebSchemas/SchemaDotOrgSources#source_GoodRelationsClass> ;
	rdfs:comment """A range of of services that will be provided to a customer free of charge in case of a defect or malfunction of a product.

    Commonly used values:

    http://purl.org/goodrelations/v1#Labor-BringIn
    http://purl.org/goodrelations/v1#PartsAndLabor-BringIn
    http://purl.org/goodrelations/v1#PartsAndLabor-PickUp
    	""" ;
	rdfs:subClassOf schema:Enumeration .

schema:WatchAction a rdfs:Class ;
	rdfs:label "WatchAction" ;
	rdfs:comment "The act of consuming dynamic/moving visual content." ;
	rdfs:subClassOf schema:ConsumeAction .

schema:Waterfall a rdfs:Class ;
	rdfs:label "Waterfall" ;
	rdfs:comment "A waterfall, like Niagara" ;
	rdfs:subClassOf schema:BodyOfWater .

schema:WearAction a rdfs:Class ;
	rdfs:label "WearAction" ;
	rdfs:comment "The act of dressing oneself in clothing." ;
	rdfs:subClassOf schema:UseAction .

schema:WebApplication a rdfs:Class ;
	rdfs:label "WebApplication" ;
	rdfs:comment "Web applications." ;
	rdfs:subClassOf schema:SoftwareApplication .

schema:WebPage a rdfs:Class ;
	rdfs:label "WebPage" ;
	rdfs:comment "A web page. Every web page is implicitly assumed to be declared to be of type WebPage, so the various properties about that webpage, such as <code>breadcrumb</code> may be used. We recommend explicit declaration if these properties are specified, but if they are found outside of an itemscope, they will be assumed to be about the page" ;
	rdfs:subClassOf schema:CreativeWork .

schema:WebPageElement a rdfs:Class ;
	rdfs:label "WebPageElement" ;
	rdfs:comment "A web page element, like a table or an image" ;
	rdfs:subClassOf schema:CreativeWork .

schema:WholesaleStore a rdfs:Class ;
	rdfs:label "WholesaleStore" ;
	rdfs:comment "A wholesale store." ;
	rdfs:subClassOf schema:Store .

schema:WinAction a rdfs:Class ;
	rdfs:label "WinAction" ;
	rdfs:comment "The act of achieving victory in a competitive activity." ;
	rdfs:subClassOf schema:AchieveAction .

schema:Winery a rdfs:Class ;
	rdfs:label "Winery" ;
	rdfs:comment "A winery." ;
	rdfs:subClassOf schema:FoodEstablishment .

schema:WriteAction a rdfs:Class ;
	rdfs:label "WriteAction" ;
	rdfs:comment "The act of authoring written creative content." ;
	rdfs:subClassOf schema:CreateAction .

schema:Zoo a rdfs:Class ;
	rdfs:label "Zoo" ;
	rdfs:comment "A zoo." ;
	rdfs:subClassOf schema:CivicStructure .

schema:Abdomen a schema:PhysicalExam ;
	rdfs:label "Abdomen" ;
	rdfs:comment "Abdomen" .

schema:ActiveNotRecruiting a schema:MedicalStudyStatus ;
	rdfs:label "ActiveNotRecruiting" ;
	rdfs:comment "Active, but not recruiting new participants." .

schema:AerobicActivity a schema:PhysicalActivityCategory ;
	rdfs:label "AerobicActivity" ;
	rdfs:comment "Physical activity of relatively low intensity that depends primarily on the aerobic energy-generating process; during activity, the aerobic metabolism uses oxygen to adequately meet energy demands during exercise." .

schema:AnaerobicActivity a schema:PhysicalActivityCategory ;
	rdfs:label "AnaerobicActivity" ;
	rdfs:comment "Physical activity that is of high-intensity which utilizes the anaerobic metabolism of the body." .

schema:Anesthesia a schema:MedicalSpecialty ;
	rdfs:label "Anesthesia" ;
	rdfs:comment "A specific branch of medical science that pertains to study of anesthetics and their application." .

schema:Appearance a schema:PhysicalExam ;
	rdfs:label "Appearance" ;
	rdfs:comment "Appearance" .

schema:Ayurvedic a schema:MedicineSystem ;
	rdfs:label "Ayurvedic" ;
	rdfs:comment "A system of medicine that originated in India over thousands of years and that focuses on integrating and balancing the body, mind, and spirit." .

schema:Bacteria a schema:InfectiousAgentClass ;
	rdfs:label "Bacteria" ;
	rdfs:comment "Pathogenic bacteria that cause bacterial infection." .

schema:Balance a schema:PhysicalActivityCategory ;
	rdfs:label "Balance" ;
	rdfs:comment "Physical activity that is engaged to help maintain posture and balance." .

schema:CT a schema:MedicalImagingTechnique ;
	rdfs:label "CT" ;
	rdfs:comment "X-ray computed tomography imaging." .

schema:Cardiovascular a schema:MedicalSpecialty ;
	rdfs:label "Cardiovascular" ;
	rdfs:comment "A specific branch of medical science that pertains to diagnosis and treatment of disorders of heart and vasculature." .

schema:CardiovascularExam a schema:PhysicalExam ;
	rdfs:label "CardiovascularExam" ;
	rdfs:comment "Cardiovascular" .

schema:CaseSeries a schema:MedicalObservationalStudyDesign ;
	rdfs:label "CaseSeries" ;
	rdfs:comment "A case series (also known as a clinical series) is a medical research study that tracks patients with a known exposure given similar treatment or examines their medical records for exposure and outcome. A case series can be retrospective or prospective and usually involves a smaller number of patients than the more powerful case-control studies or randomized controlled trials. Case series may be consecutive or non-consecutive, depending on whether all cases presenting to the reporting authors over a period of time were included, or only a selection." .

schema:Chiropractic a schema:MedicineSystem ;
	rdfs:label "Chiropractic" ;
	rdfs:comment "A system of medicine focused on the relationship between the body's structure, mainly the spine, and its functioning." .

schema:Clinician a schema:MedicalAudience ;
	rdfs:label "Clinician" ;
	rdfs:comment "Medical clinicians, including practicing physicians and other medical professionals involved in clinical practice." .

schema:CohortStudy a schema:MedicalObservationalStudyDesign ;
	rdfs:label "CohortStudy" ;
	rdfs:comment "Also known as a panel study. A cohort study is a form of longitudinal study used in medicine and social science. It is one type of study design and should be compared with a cross-sectional study.  A cohort is a group of people who share a common characteristic or experience within a defined period (e.g., are born, leave school, lose their job, are exposed to a drug or a vaccine, etc.). The comparison group may be the general population from which the cohort is drawn, or it may be another cohort of persons thought to have had little or no exposure to the substance under investigation, but otherwise similar. Alternatively, subgroups within the cohort may be compared with each other." .

schema:CommunityHealth a schema:MedicalSpecialty ;
	rdfs:label "CommunityHealth" ;
	rdfs:comment "Community health." .

schema:Completed a schema:MedicalStudyStatus ;
	rdfs:label "Completed" ;
	rdfs:comment "Completed." .

schema:CrossSectional a schema:MedicalObservationalStudyDesign ;
	rdfs:label "CrossSectional" ;
	rdfs:comment "Studies carried out on pre-existing data (usually from 'snapshot' surveys), such as that collected by the Census Bureau. Sometimes called Prevalence Studies." .

schema:DamagedCondition a schema:OfferItemCondition ;
	rdfs:label "DamagedCondition" ;
	rdfs:comment "Indicates that the item for sale is damaged." .

schema:Dentistry a schema:MedicalSpecialty ;
	rdfs:label "Dentistry" ;
	rdfs:comment "Dentistry." .

schema:Dermatologic a schema:MedicalSpecialty ;
	rdfs:label "Dermatologic" ;
	rdfs:comment "A specific branch of medical science that pertains to diagnosis and treatment of disorders of skin." .

schema:Diagnostic a schema:MedicalDevicePurpose ;
	rdfs:label "Diagnostic" ;
	rdfs:comment "A medical device used for diagnostic purposes." .

schema:DietNutrition a schema:MedicalSpecialty ;
	rdfs:label "DietNutrition" ;
	rdfs:comment "Diet and nutrition." .

schema:Discontinued a schema:ItemAvailability ;
	rdfs:label "Discontinued" ;
	rdfs:comment "Indicates that the item for sale has been discontinued." .

schema:DoubleBlindedTrial a schema:MedicalTrialDesign ;
	rdfs:label "DoubleBlindedTrial" ;
	rdfs:comment "A trial design in which neither the researcher nor the patient knows the details of the treatment the patient was randomly assigned to." .

schema:EBook a schema:BookFormatType ;
	rdfs:label "EBook" ;
	rdfs:comment "Book format: Ebook." .

schema:Ear a schema:PhysicalExam ;
	rdfs:label "Ear" ;
	rdfs:comment "Ear" .

schema:Emergency a schema:MedicalSpecialty ;
	rdfs:label "Emergency" ;
	rdfs:comment "A specific branch of medical science that is deals with the evaluation and initial treatment of medical conditions caused by trauma or sudden illness." .

schema:Endocrine a schema:MedicalSpecialty ;
	rdfs:label "Endocrine" ;
	rdfs:comment "A specific branch of medical science that pertains to diagnosis and treatment of disorders of endocrine glands and their secretions." .

schema:EnrollingByInvitation a schema:MedicalStudyStatus ;
	rdfs:label "EnrollingByInvitation" ;
	rdfs:comment "Enrolling participants by invitation only." .

schema:EvidenceLevelA a schema:MedicalEvidenceLevel ;
	rdfs:label "EvidenceLevelA" ;
	rdfs:comment "Data derived from multiple randomized clinical trials or meta-analyses." .

schema:EvidenceLevelB a schema:MedicalEvidenceLevel ;
	rdfs:label "EvidenceLevelB" ;
	rdfs:comment "Data derived from a single randomized trial, or nonrandomized studies." .

schema:EvidenceLevelC a schema:MedicalEvidenceLevel ;
	rdfs:label "EvidenceLevelC" ;
	rdfs:comment "Only consensus opinion of experts, case studies, or standard-of-care." .

schema:Eye a schema:PhysicalExam ;
	rdfs:label "Eye" ;
	rdfs:comment "Eye" .

schema:FDAcategoryA a schema:DrugPregnancyCategory ;
	rdfs:label "FDAcategoryA" ;
	rdfs:comment "A designation by the US FDA signifying that adequate and well-controlled studies have failed to demonstrate a risk to the fetus in the first trimester of pregnancy (and there is no evidence of risk in later trimesters)." .

schema:FDAcategoryB a schema:DrugPregnancyCategory ;
	rdfs:label "FDAcategoryB" ;
	rdfs:comment "A designation by the US FDA signifying that animal reproduction studies have failed to demonstrate a risk to the fetus and there are no adequate and well-controlled studies in pregnant women." .

schema:FDAcategoryC a schema:DrugPregnancyCategory ;
	rdfs:label "FDAcategoryC" ;
	rdfs:comment "A designation by the US FDA signifying that animal reproduction studies have shown an adverse effect on the fetus and there are no adequate and well-controlled studies in humans, but potential benefits may warrant use of the drug in pregnant women despite potential risks." .

schema:FDAcategoryD a schema:DrugPregnancyCategory ;
	rdfs:label "FDAcategoryD" ;
	rdfs:comment "A designation by the US FDA signifying that there is positive evidence of human fetal risk based on adverse reaction data from investigational or marketing experience or studies in humans, but potential benefits may warrant use of the drug in pregnant women despite potential risks." .

schema:FDAcategoryX a schema:DrugPregnancyCategory ;
	rdfs:label "FDAcategoryX" ;
	rdfs:comment "A designation by the US FDA signifying that studies in animals or humans have demonstrated fetal abnormalities and/or there is positive evidence of human fetal risk based on adverse reaction data from investigational or marketing experience, and the risks involved in use of the drug in pregnant women clearly outweigh potential benefits." .

schema:FDAnotEvaluated a schema:DrugPregnancyCategory ;
	rdfs:label "FDAnotEvaluated" ;
	rdfs:comment "A designation that the drug in question has not been assigned a pregnancy category designation by the US FDA." .

schema:False a schema:Boolean ;
	rdfs:label "False" ;
	rdfs:comment "The boolean value false" .

schema:Flexibility a schema:PhysicalActivityCategory ;
	rdfs:label "Flexibility" ;
	rdfs:comment "Physical activity that is engaged in to improve joint and muscle flexibility." .

schema:Fungus a schema:InfectiousAgentClass ;
	rdfs:label "Fungus" ;
	rdfs:comment "Pathogenic fungus." .

schema:Gastroenterologic a schema:MedicalSpecialty ;
	rdfs:label "Gastroenterologic" ;
	rdfs:comment "A specific branch of medical science that pertains to diagnosis and treatment of disorders of digestive system." .

schema:Genetic a schema:MedicalSpecialty ;
	rdfs:label "Genetic" ;
	rdfs:comment "A specific branch of medical science that pertains to hereditary transmission and the variation of inherited characteristics and disorders." .

schema:Genitourinary a schema:PhysicalExam ;
	rdfs:label "Genitourinary" ;
	rdfs:comment "Genitourinary" .

schema:Geriatric a schema:MedicalSpecialty ;
	rdfs:label "Geriatric" ;
	rdfs:comment "A specific branch of medical science that is concerned with the diagnosis and treatment of diseases, debilities and provision of care to the aged." .

schema:Gynecologic a schema:MedicalSpecialty ;
	rdfs:label "Gynecologic" ;
	rdfs:comment "A specific branch of medical science that pertains to the health care of women, particularly in the diagnosis and treatment of disorders affecting the female reproductive system." .

schema:Hardcover a schema:BookFormatType ;
	rdfs:label "Hardcover" ;
	rdfs:comment "Book format: Hardcover." .

schema:Head a schema:PhysicalExam ;
	rdfs:label "Head" ;
	rdfs:comment "Head" .

schema:Hematologic a schema:MedicalSpecialty ;
	rdfs:label "Hematologic" ;
	rdfs:comment "A specific branch of medical science that pertains to diagnosis and treatment of disorders of blood and blood producing organs." .

schema:Homeopathic a schema:MedicineSystem ;
	rdfs:label "Homeopathic" ;
	rdfs:comment "A system of medicine based on the principle that a disease can be cured by a substance that produces similar symptoms in healthy people." .

schema:InStock a schema:ItemAvailability ;
	rdfs:label "InStock" ;
	rdfs:comment "Indicates that the item for sale is in stock." .

schema:InStoreOnly a schema:ItemAvailability ;
	rdfs:label "InStoreOnly" ;
	rdfs:comment "Indicates that the item for sale is available only in brick-and-mortar stores." .

schema:Infectious a schema:MedicalSpecialty ;
	rdfs:label "Infectious" ;
	rdfs:comment "A specific branch of medical science that pertains to diagnosis and treatment of bacterial, viral, fungal and parasitic infections." .

schema:InternationalTrial a schema:MedicalTrialDesign ;
	rdfs:label "InternationalTrial" ;
	rdfs:comment "An international trial." .

schema:LaboratoryScience a schema:MedicalSpecialty ;
	rdfs:label "LaboratoryScience" ;
	rdfs:comment "Laboratory science." .

schema:LeisureTimeActivity a schema:PhysicalActivityCategory ;
	rdfs:label "LeisureTimeActivity" ;
	rdfs:comment "Any physical activity engaged in for recreational purposes. Examples may include ballroom dancing, roller skating, canoeing, fishing, etc." .

schema:Longitudinal a schema:MedicalObservationalStudyDesign ;
	rdfs:label "Longitudinal" ;
	rdfs:comment "Unlike cross-sectional studies, longitudinal studies track the same people, and therefore the differences observed in those people are less likely to be the result of cultural differences across generations. Longitudinal studies are also used in medicine to uncover predictors of certain diseases." .

schema:Lung a schema:PhysicalExam ;
	rdfs:label "Lung" ;
	rdfs:comment "Lung" .

schema:MRI a schema:MedicalImagingTechnique ;
	rdfs:label "MRI" ;
	rdfs:comment "Magnetic resonance imaging." .

schema:MedicalResearcher a schema:MedicalAudience ;
	rdfs:label "MedicalResearcher" ;
	rdfs:comment "Medical researchers." .

schema:Midwifery a schema:MedicalSpecialty ;
	rdfs:label "Midwifery" ;
	rdfs:comment "Midwifery." .

schema:MultiCenterTrial a schema:MedicalTrialDesign ;
	rdfs:label "MultiCenterTrial" ;
	rdfs:comment "A trial that takes place at multiple centers." .

schema:MulticellularParasite a schema:InfectiousAgentClass ;
	rdfs:label "MulticellularParasite" ;
	rdfs:comment "Multicellular parasite that causes an infection." .

schema:Musculoskeletal a schema:MedicalSpecialty ;
	rdfs:label "Musculoskeletal" ;
	rdfs:comment "A specific branch of medical science that pertains to diagnosis and treatment of disorders of muscles, ligaments and skeletal system." .

schema:MusculoskeletalExam a schema:PhysicalExam ;
	rdfs:label "MusculoskeletalExam" ;
	rdfs:comment "Musculoskeletal" .

schema:Neck a schema:PhysicalExam ;
	rdfs:label "Neck" ;
	rdfs:comment "Neck" .

schema:Neuro a schema:PhysicalExam ;
	rdfs:label "Neuro" ;
	rdfs:comment "Neuro" .

schema:Neurologic a schema:MedicalSpecialty ;
	rdfs:label "Neurologic" ;
	rdfs:comment "A specific branch of medical science that studies the nerves and nervous system and its respective disease states." .

schema:NewCondition a schema:OfferItemCondition ;
	rdfs:label "NewCondition" ;
	rdfs:comment "Indicates that the item for sale is new." .

schema:NoninvasiveProcedure a schema:MedicalProcedureType ;
	rdfs:label "NoninvasiveProcedure" ;
	rdfs:comment "A type of medical procedure that involves noninvasive techniques." .

schema:Nose a schema:PhysicalExam ;
	rdfs:label "Nose" ;
	rdfs:comment "Nose" .

schema:NotYetRecruiting a schema:MedicalStudyStatus ;
	rdfs:label "NotYetRecruiting" ;
	rdfs:comment "Not yet recruiting." .

schema:Nursing a schema:MedicalSpecialty ;
	rdfs:label "Nursing" ;
	rdfs:comment "Nursing." .

schema:OTC a schema:DrugPrescriptionStatus ;
	rdfs:label "OTC" ;
	rdfs:comment "Available over the counter." .

schema:Observational a schema:MedicalObservationalStudyDesign ;
	rdfs:label "Observational" ;
	rdfs:comment "An observational study design." .

schema:Obstetric a schema:MedicalSpecialty ;
	rdfs:label "Obstetric" ;
	rdfs:comment "A specific branch of medical science that specializes in the care of women during the prenatal and postnatal care and with the delivery of the child." .

schema:OccupationalActivity a schema:PhysicalActivityCategory ;
	rdfs:label "OccupationalActivity" ;
	rdfs:comment "Any physical activity engaged in for job-related purposes. Examples may include waiting tables, maid service, carrying a mailbag, picking fruits or vegetables, construction work, etc." .

schema:OccupationalTherapy a schema:MedicalSpecialty ;
	rdfs:label "OccupationalTherapy" ;
	rdfs:comment "Occupational therapy." .

schema:Oncologic a schema:MedicalSpecialty ;
	rdfs:label "Oncologic" ;
	rdfs:comment "A specific branch of medical science that deals with benign and malignant tumors, including the study of their development, diagnosis, treatment and prevention." .

schema:OnlineOnly a schema:ItemAvailability ;
	rdfs:label "OnlineOnly" ;
	rdfs:comment "Indicates that the item for sale is available only online." .

schema:OpenTrial a schema:MedicalTrialDesign ;
	rdfs:label "OpenTrial" ;
	rdfs:comment "A trial design in which the researcher knows the full details of the treatment, and so does the patient." .

schema:Optometic a schema:MedicalSpecialty ;
	rdfs:label "Optometic" ;
	rdfs:comment "Optometry." .

schema:Osteopathic a schema:MedicineSystem ;
	rdfs:label "Osteopathic" ;
	rdfs:comment "A system of medicine focused on promoting the body's innate ability to heal itself." .

schema:Otolaryngologic a schema:MedicalSpecialty ;
	rdfs:label "Otolaryngologic" ;
	rdfs:comment "A specific branch of medical science that is concerned with the ear, nose and throat and their respective disease states." .

schema:OutOfStock a schema:ItemAvailability ;
	rdfs:label "OutOfStock" ;
	rdfs:comment "Indicates that the item for sale is out of stock." .

schema:PET a schema:MedicalImagingTechnique ;
	rdfs:label "PET" ;
	rdfs:comment "Positron emission tomography imaging." .

schema:Paperback a schema:BookFormatType ;
	rdfs:label "Paperback" ;
	rdfs:comment "Book format: Paperback." .

schema:Pathology a schema:MedicalSpecialty ;
	rdfs:label "Pathology" ;
	rdfs:comment "A specific branch of medical science that is concerned with the study of the cause, origin and nature of a disease state, including its consequences as a result of manifestation of the disease. In clinical care, the term is used to designate a branch of medicine using laboratory tests to diagnose and determine the prognostic significance of illness." .

schema:Patient a schema:MedicalAudience ;
	rdfs:label "Patient" ;
	rdfs:comment "Patients." .

schema:Pediatric a schema:MedicalSpecialty ;
	rdfs:label "Pediatric" ;
	rdfs:comment "A specific branch of medical science that specializes in the care of infants, children and adolescents." .

schema:PercutaneousProcedure a schema:MedicalProcedureType ;
	rdfs:label "PercutaneousProcedure" ;
	rdfs:comment "A type of medical procedure that involves percutaneous techniques, where access to organs or tissue is achieved via needle-puncture of the skin. For example, catheter-based procedures like stent delivery." .

schema:PharmacySpecialty a schema:MedicalSpecialty ;
	rdfs:label "PharmacySpecialty" ;
	rdfs:comment "Pharmacy." .

schema:Physiotherapy a schema:MedicalSpecialty ;
	rdfs:label "Physiotherapy" ;
	rdfs:comment "Physiotherapy." .

schema:PlaceboControlledTrial a schema:MedicalTrialDesign ;
	rdfs:label "PlaceboControlledTrial" ;
	rdfs:comment "A placebo-controlled trial design." .

schema:PlasticSurgery a schema:MedicalSpecialty ;
	rdfs:label "PlasticSurgery" ;
	rdfs:comment "A specific branch of medical science that pertains to therapeutic or cosmetic repair or re-formation of missing, injured or malformed tissues or body parts by manual and instrumental means." .

schema:Podiatric a schema:MedicalSpecialty ;
	rdfs:label "Podiatric" ;
	rdfs:comment "Podiatry." .

schema:PreOrder a schema:ItemAvailability ;
	rdfs:label "PreOrder" ;
	rdfs:comment "Indicates that the item for sale is available for pre-order." .

schema:PrescriptionOnly a schema:DrugPrescriptionStatus ;
	rdfs:label "PrescriptionOnly" ;
	rdfs:comment "Available by prescription only." .

schema:PrimaryCare a schema:MedicalSpecialty ;
	rdfs:label "PrimaryCare" ;
	rdfs:comment "Primary care." .

schema:Prion a schema:InfectiousAgentClass ;
	rdfs:label "Prion" ;
	rdfs:comment "A prion is an infectious agent composed of protein in a misfolded form." .

schema:Protozoa a schema:InfectiousAgentClass ;
	rdfs:label "Protozoa" ;
	rdfs:comment "Single-celled organism that causes an infection." .

schema:Psychiatric a schema:MedicalSpecialty ;
	rdfs:label "Psychiatric" ;
	rdfs:comment "A specific branch of medical science that is concerned with the study, treatment, and prevention of mental illness, using both medical and psychological therapies." .

schema:PublicHealth a schema:MedicalSpecialty ;
	rdfs:label "PublicHealth" ;
	rdfs:comment "Environment and public health." .

schema:Pulmonary a schema:MedicalSpecialty ;
	rdfs:label "Pulmonary" ;
	rdfs:comment "A specific branch of medical science that pertains to the study of the respiratory system and its respective disease states." .

schema:Radiograpy a schema:MedicalSpecialty ;
	rdfs:label "Radiograpy" ;
	rdfs:comment "Radiography." .

schema:RandomizedTrial a schema:MedicalTrialDesign ;
	rdfs:label "RandomizedTrial" ;
	rdfs:comment "A randomized trial design." .

schema:Recruiting a schema:MedicalStudyStatus ;
	rdfs:label "Recruiting" ;
	rdfs:comment "Recruiting participants." .

schema:RefurbishedCondition a schema:OfferItemCondition ;
	rdfs:label "RefurbishedCondition" ;
	rdfs:comment "Indicates that the item for sale is refurbished." .

schema:Registry a schema:MedicalObservationalStudyDesign ;
	rdfs:label "Registry" ;
	rdfs:comment "A registry-based study design." .

schema:ReimbursementCap a schema:DrugCostCategory ;
	rdfs:label "ReimbursementCap" ;
	rdfs:comment "The drug's cost represents the maximum reimbursement paid by an insurer for the drug." .

schema:Renal a schema:MedicalSpecialty ;
	rdfs:label "Renal" ;
	rdfs:comment "A specific branch of medical science that pertains to the study of the kidneys and its respective disease states." .

schema:Researcher a schema:Audience ;
	rdfs:label "Researcher" ;
	rdfs:comment "Researchers." .

schema:RespiratoryTherapy a schema:MedicalSpecialty ;
	rdfs:label "RespiratoryTherapy" ;
	rdfs:comment "Respiratory therapy." .

schema:ResultsAvailable a schema:MedicalStudyStatus ;
	rdfs:label "ResultsAvailable" ;
	rdfs:comment "Results are available." .

schema:ResultsNotAvailable a schema:MedicalStudyStatus ;
	rdfs:label "ResultsNotAvailable" ;
	rdfs:comment "Results are not available." .

schema:Retail a schema:DrugCostCategory ;
	rdfs:label "Retail" ;
	rdfs:comment "The drug's cost represents the retail cost of the drug." .

schema:Rheumatologic a schema:MedicalSpecialty ;
	rdfs:label "Rheumatologic" ;
	rdfs:comment "A specific branch of medical science that deals with the study and treatment of rheumatic, automimmune or joint diseases." .

schema:SingleBlindedTrial a schema:MedicalTrialDesign ;
	rdfs:label "SingleBlindedTrial" ;
	rdfs:comment "A trial design in which the researcher knows which treatment the patient was randomly assigned to but the patient does not." .

schema:SingleCenterTrial a schema:MedicalTrialDesign ;
	rdfs:label "SingleCenterTrial" ;
	rdfs:comment "A trial that takes place at a single center." .

schema:Skin a schema:PhysicalExam ;
	rdfs:label "Skin" ;
	rdfs:comment "Skin" .

schema:SpeechPathology a schema:MedicalSpecialty ;
	rdfs:label "SpeechPathology" ;
	rdfs:comment "Speech pathology." .

schema:StrengthTraining a schema:PhysicalActivityCategory ;
	rdfs:label "StrengthTraining" ;
	rdfs:comment "Physical activity that is engaged in to improve muscle and bone strength. Also referred to as resistance training." .

schema:Surgical a schema:MedicalSpecialty ;
	rdfs:label "Surgical" ;
	rdfs:comment "A specific branch of medical science that pertains to treating diseases, injuries and deformities by manual and instrumental means." .

schema:SurgicalProcedure a schema:MedicalProcedureType ;
	rdfs:label "SurgicalProcedure" ;
	rdfs:comment "A type of medical procedure that involves invasive surgical techniques." .

schema:Suspended a schema:MedicalStudyStatus ;
	rdfs:label "Suspended" ;
	rdfs:comment "Suspended." .

schema:Terminated a schema:MedicalStudyStatus ;
	rdfs:label "Terminated" ;
	rdfs:comment "Terminated." .

schema:Therapeutic a schema:MedicalDevicePurpose ;
	rdfs:label "Therapeutic" ;
	rdfs:comment "A medical device used for therapeutic purposes." .

schema:Throat a schema:PhysicalExam ;
	rdfs:label "Throat" ;
	rdfs:comment "Throat" .

schema:Toxicologic a schema:MedicalSpecialty ;
	rdfs:label "Toxicologic" ;
	rdfs:comment "A specific branch of medical science that is concerned with poisons, their nature, effects and detection and involved in the treatment of poisoning." .

schema:TraditionalChinese a schema:MedicineSystem ;
	rdfs:label "TraditionalChinese" ;
	rdfs:comment "A system of medicine based on common theoretical concepts that originated in China and evolved over thousands of years, that uses herbs, acupuncture, exercise, massage, dietary therapy, and other methods to treat a wide range of conditions." .

schema:TripleBlindedTrial a schema:MedicalTrialDesign ;
	rdfs:label "TripleBlindedTrial" ;
	rdfs:comment "A trial design in which neither the researcher, the person administering the therapy nor the patient knows the details of the treatment the patient was randomly assigned to." .

schema:True a schema:Boolean ;
	rdfs:label "True" ;
	rdfs:comment "The boolean value true" .

schema:Ultrasound a schema:MedicalImagingTechnique ;
	rdfs:label "Ultrasound" ;
	rdfs:comment "Ultrasound imaging." .

schema:Urologic a schema:MedicalSpecialty ;
	rdfs:label "Urologic" ;
	rdfs:comment "A specific branch of medical science that is concerned with the diagnosis and treatment of diseases pertaining to the urinary tract and the urogenital system." .

schema:UsedCondition a schema:OfferItemCondition ;
	rdfs:label "UsedCondition" ;
	rdfs:comment "Indicates that the item for sale is used." .

schema:Virus a schema:InfectiousAgentClass ;
	rdfs:label "Virus" ;
	rdfs:comment "Pathogenic virus that causes viral infection." .

schema:VitalSign a schema:PhysicalExam ;
	rdfs:label "VitalSign" ;
	rdfs:comment "VitalSign" .

schema:WesternConventional a schema:MedicineSystem ;
	rdfs:label "WesternConventional" ;
	rdfs:comment "The conventional Western system of medicine, that aims to apply the best available evidence gained from the scientific method to clinical decision making. Also known as conventional or Western medicine." .

schema:Wholesale a schema:DrugCostCategory ;
	rdfs:label "Wholesale" ;
	rdfs:comment "The drug's cost represents the wholesale acquisition cost of the drug." .

schema:Withdrawn a schema:MedicalStudyStatus ;
	rdfs:label "Withdrawn" ;
	rdfs:comment "Withdrawn." .

schema:XRay a schema:MedicalImagingTechnique ;
	rdfs:label "XRay" ;
	rdfs:comment "X-ray imaging." .

schema:about a rdf:Property ;
	rdfs:label "about" ;
	schema:domainIncludes schema:CommunicateAction , schema:CreativeWork ;
	schema:rangeIncludes schema:Thing ;
	rdfs:comment "The subject matter of the content." .

schema:acceptedPaymentMethod a rdf:Property ;
	rdfs:label "acceptedPaymentMethod" ;
	schema:domainIncludes schema:Demand , schema:Offer ;
	schema:rangeIncludes schema:PaymentMethod ;
	rdfs:comment "The payment method(s) accepted by seller for this offer." .

schema:acceptsReservations a rdf:Property ;
	rdfs:label "acceptsReservations" ;
	schema:domainIncludes schema:FoodEstablishment ;
	schema:rangeIncludes schema:Text , schema:URL ;
	rdfs:comment "Either <code>Yes/No</code>, or a URL at which reservations can be made." .

schema:accountablePerson a rdf:Property ;
	rdfs:label "accountablePerson" ;
	schema:domainIncludes schema:CreativeWork ;
	schema:rangeIncludes schema:Person ;
	rdfs:comment "Specifies the Person that is legally accountable for the CreativeWork." .

schema:acquiredFrom a rdf:Property ;
	rdfs:label "acquiredFrom" ;
	schema:domainIncludes schema:OwnershipInfo ;
	schema:rangeIncludes schema:Organization , schema:Person ;
	rdfs:comment "The organization or person from which the product was acquired." .

schema:action a rdf:Property ;
	rdfs:label "action" ;
	schema:domainIncludes schema:Muscle ;
	schema:rangeIncludes schema:Text ;
	rdfs:comment "The movement the muscle generates." .

schema:activeIngredient a rdf:Property ;
	rdfs:label "activeIngredient" ;
	schema:domainIncludes schema:DietarySupplement , schema:Drug , schema:DrugStrength ;
	schema:rangeIncludes schema:Text ;
	rdfs:comment "An active ingredient, typically chemical compounds and/or biologic substances." .

schema:activityDuration a rdf:Property ;
	rdfs:label "activityDuration" ;
	schema:domainIncludes schema:ExercisePlan ;
	schema:rangeIncludes schema:Duration ;
	rdfs:comment "Length of time to engage in the activity." .

schema:activityFrequency a rdf:Property ;
	rdfs:label "activityFrequency" ;
	schema:domainIncludes schema:ExercisePlan ;
	schema:rangeIncludes schema:Text ;
	rdfs:comment "How often one should engage in the activity." .

schema:actor a rdf:Property ;
	rdfs:label "actor" ;
	schema:domainIncludes schema:Movie , schema:TVEpisode , schema:TVSeries ;
	schema:rangeIncludes schema:Person ;
	rdfs:comment "A cast member of the movie, TV series, season, or episode, or video." .

schema:actors a rdf:Property ;
	rdfs:label "actors" ;
	schema:domainIncludes schema:Movie , schema:TVEpisode , schema:TVSeries ;
	schema:rangeIncludes schema:Person ;
	rdfs:comment "A cast member of the movie, TV series, season, or episode, or video. (legacy spelling; see singular form, actor)" .

schema:addOn a rdf:Property ;
	rdfs:label "addOn" ;
	schema:domainIncludes schema:Offer ;
	schema:rangeIncludes schema:Offer ;
	rdfs:comment "An additional offer that can only be obtained in combination with the first base offer (e.g. supplements and extensions that are available for a surcharge)." .

schema:additionalName a rdf:Property ;
	rdfs:label "additionalName" ;
	schema:domainIncludes schema:Person ;
	schema:rangeIncludes schema:Text ;
	rdfs:comment "An additional name for a Person, can be used for a middle name." .

schema:additionalType a rdf:Property ;
	rdfs:label "additionalType" ;
	schema:domainIncludes schema:Thing ;
	schema:rangeIncludes schema:URL ;
	rdfs:comment "An additional type for the item, typically used for adding more specific types from external vocabularies in microdata syntax. This is a relationship between something and a class that the thing is in. In RDFa syntax, it is better to use the native RDFa syntax - the 'typeof' attribute - for multiple types. Schema.org tools may have only weaker understanding of extra types, in particular those defined externally." .

schema:additionalVariable a rdf:Property ;
	rdfs:label "additionalVariable" ;
	schema:domainIncludes schema:ExercisePlan ;
	schema:rangeIncludes schema:Text ;
	rdfs:comment "Any additional component of the exercise prescription that may need to be articulated to the patient. This may include the order of exercises, the number of repetitions of movement, quantitative distance, progressions over time, etc." .

schema:address a rdf:Property ;
	rdfs:label "address" ;
	schema:domainIncludes schema:Organization , schema:Person , schema:Place ;
	schema:rangeIncludes schema:PostalAddress ;
	rdfs:comment "Physical address of the item." .

schema:addressCountry a rdf:Property ;
	rdfs:label "addressCountry" ;
	schema:domainIncludes schema:PostalAddress ;
	schema:rangeIncludes schema:Country ;
	rdfs:comment "The country. For example, USA. You can also provide the two-letter <a href='http://en.wikipedia.org/wiki/ISO_3166-1'>ISO 3166-1 alpha-2 country code</a>." .

schema:addressLocality a rdf:Property ;
	rdfs:label "addressLocality" ;
	schema:domainIncludes schema:PostalAddress ;
	schema:rangeIncludes schema:Text ;
	rdfs:comment "The locality. For example, Mountain View." .

schema:addressRegion a rdf:Property ;
	rdfs:label "addressRegion" ;
	schema:domainIncludes schema:PostalAddress ;
	schema:rangeIncludes schema:Text ;
	rdfs:comment "The region. For example, CA." .

schema:administrationRoute a rdf:Property ;
	rdfs:label "administrationRoute" ;
	schema:domainIncludes schema:Drug ;
	schema:rangeIncludes schema:Text ;
	rdfs:comment "A route by which this drug may be administered, e.g. 'oral'." .

schema:advanceBookingRequirement a rdf:Property ;
	rdfs:label "advanceBookingRequirement" ;
	schema:domainIncludes schema:Demand , schema:Offer ;
	schema:rangeIncludes schema:QuantitativeValue ;
	rdfs:comment "The amount of time that is required between accepting the offer and the actual usage of the resource or service." .

schema:adverseOutcome a rdf:Property ;
	rdfs:label "adverseOutcome" ;
	schema:domainIncludes schema:MedicalDevice , schema:MedicalTherapy ;
	schema:rangeIncludes schema:MedicalEntity ;
	rdfs:comment "A possible complication and/or side effect of this therapy. If it is known that an adverse outcome is serious (resulting in death, disability, or permanent damage; requiring hospitalization; or is otherwise life-threatening or requires immediate medical attention), tag it as a seriouseAdverseOutcome instead." .

schema:affectedBy a rdf:Property ;
	rdfs:label "affectedBy" ;
	schema:domainIncludes schema:MedicalTest ;
	schema:rangeIncludes schema:Drug ;
	rdfs:comment "Drugs that affect the test's results." .

schema:affiliation a rdf:Property ;
	rdfs:label "affiliation" ;
	schema:domainIncludes schema:Person ;
	schema:rangeIncludes schema:Organization ;
	rdfs:comment "An organization that this person is affiliated with. For example, a school/university, a club, or a team." .

schema:agent a rdf:Property ;
	rdfs:label "agent" ;
	schema:domainIncludes schema:Action ;
	schema:rangeIncludes schema:Organization , schema:Person ;
	rdfs:comment "The direct performer or driver of the action (animate or inanimate). e.g. *John* wrote a book." .

schema:aggregateRating a rdf:Property ;
	rdfs:label "aggregateRating" ;
	schema:domainIncludes schema:CreativeWork , schema:Offer , schema:Organization , schema:Place , schema:Product ;
	schema:rangeIncludes schema:AggregateRating ;
	rdfs:comment "The overall rating, based on a collection of reviews or ratings, of the item." .

schema:album a rdf:Property ;
	rdfs:label "album" ;
	schema:domainIncludes schema:MusicGroup ;
	schema:rangeIncludes schema:MusicAlbum ;
	rdfs:comment "A music album." .

schema:albums a rdf:Property ;
	rdfs:label "albums" ;
	schema:domainIncludes schema:MusicGroup ;
	schema:rangeIncludes schema:MusicAlbum ;
	rdfs:comment "A collection of music albums (legacy spelling; see singular form, album)." .

schema:alcoholWarning a rdf:Property ;
	rdfs:label "alcoholWarning" ;
	schema:domainIncludes schema:Drug ;
	schema:rangeIncludes schema:Text ;
	rdfs:comment "Any precaution, guidance, contraindication, etc. related to consumption of alcohol while taking this drug." .

schema:algorithm a rdf:Property ;
	rdfs:label "algorithm" ;
	schema:domainIncludes schema:MedicalRiskScore ;
	schema:rangeIncludes schema:Text ;
	rdfs:comment "The algorithm or rules to follow to compute the score." .

schema:alignmentType a rdf:Property ;
	rdfs:label "alignmentType" ;
	schema:domainIncludes schema:AlignmentObject ;
	schema:rangeIncludes schema:Text ;
	rdfs:comment "A category of alignment between the learning resource and the framework node. Recommended values include: 'assesses', 'teaches', 'requires', 'textComplexity', 'readingLevel', 'educationalSubject', and 'educationLevel'." .

schema:alternateName a rdf:Property ;
	rdfs:label "alternateName" ;
	schema:domainIncludes schema:MedicalEntity ;
	schema:rangeIncludes schema:Text ;
	rdfs:comment "Any alternate name for this medical entity." .

schema:alternativeHeadline a rdf:Property ;
	rdfs:label "alternativeHeadline" ;
	schema:domainIncludes schema:CreativeWork ;
	schema:rangeIncludes schema:Text ;
	rdfs:comment "A secondary title of the CreativeWork." .

schema:alumni a rdf:Property ;
	rdfs:label "alumni" ;
	schema:domainIncludes schema:EducationalOrganization ;
	schema:rangeIncludes schema:Person ;
	rdfs:comment "Alumni of educational organization." .

schema:alumniOf a rdf:Property ;
	rdfs:label "alumniOf" ;
	schema:domainIncludes schema:Person ;
	schema:rangeIncludes schema:EducationalOrganization ;
	rdfs:comment "An educational organizations that the person is an alumni of." .

schema:amountOfThisGood a rdf:Property ;
	rdfs:label "amountOfThisGood" ;
	schema:domainIncludes schema:TypeAndQuantityNode ;
	schema:rangeIncludes schema:Number ;
	rdfs:comment "The quantity of the goods included in the offer." .

schema:antagonist a rdf:Property ;
	rdfs:label "antagonist" ;
	schema:domainIncludes schema:Muscle ;
	schema:rangeIncludes schema:Muscle ;
	rdfs:comment "The muscle whose action counteracts the specified muscle." .

schema:applicableLocation a rdf:Property ;
	rdfs:label "applicableLocation" ;
	schema:domainIncludes schema:DrugCost , schema:DrugLegalStatus ;
	schema:rangeIncludes schema:AdministrativeArea ;
	rdfs:comment "The location in which the status applies." .

schema:applicationCategory a rdf:Property ;
	rdfs:label "applicationCategory" ;
	schema:domainIncludes schema:SoftwareApplication ;
	schema:rangeIncludes schema:Text , schema:URL ;
	rdfs:comment "Type of software application, e.g. \"Game, Multimedia\"." .

schema:applicationSubCategory a rdf:Property ;
	rdfs:label "applicationSubCategory" ;
	schema:domainIncludes schema:SoftwareApplication ;
	schema:rangeIncludes schema:Text , schema:URL ;
	rdfs:comment "Subcategory of the application, e.g. \"Arcade Game\"." .

schema:applicationSuite a rdf:Property ;
	rdfs:label "applicationSuite" ;
	schema:domainIncludes schema:SoftwareApplication ;
	schema:rangeIncludes schema:Text ;
	rdfs:comment "The name of the application suite to which the application belongs (e.g. Excel belongs to Office)" .

schema:appliesToDeliveryMethod a rdf:Property ;
	rdfs:label "appliesToDeliveryMethod" ;
	schema:domainIncludes schema:DeliveryChargeSpecification , schema:PaymentChargeSpecification ;
	schema:rangeIncludes schema:DeliveryMethod ;
	rdfs:comment "The delivery method(s) to which the delivery charge or payment charge specification applies." .

schema:appliesToPaymentMethod a rdf:Property ;
	rdfs:label "appliesToPaymentMethod" ;
	schema:domainIncludes schema:PaymentChargeSpecification ;
	schema:rangeIncludes schema:PaymentMethod ;
	rdfs:comment "The payment method(s) to which the payment charge specification applies." .

schema:arterialBranch a rdf:Property ;
	rdfs:label "arterialBranch" ;
	schema:domainIncludes schema:Artery ;
	schema:rangeIncludes schema:AnatomicalStructure ;
	rdfs:comment "The branches that comprise the arterial structure." .

schema:articleBody a rdf:Property ;
	rdfs:label "articleBody" ;
	schema:domainIncludes schema:Article ;
	schema:rangeIncludes schema:Text ;
	rdfs:comment "The actual body of the article." .

schema:articleSection a rdf:Property ;
	rdfs:label "articleSection" ;
	schema:domainIncludes schema:Article ;
	schema:rangeIncludes schema:Text ;
	rdfs:comment "Articles may belong to one or more 'sections' in a magazine or newspaper, such as Sports, Lifestyle, etc." .

schema:aspect a rdf:Property ;
	rdfs:label "aspect" ;
	schema:domainIncludes schema:MedicalWebPage ;
	schema:rangeIncludes schema:Text ;
	rdfs:comment "An aspect of medical practice that is considered on the page, such as 'diagnosis', 'treatment', 'causes', 'prognosis', 'etiology', 'epidemiology', etc." .

schema:assembly a rdf:Property ;
	rdfs:label "assembly" ;
	schema:domainIncludes schema:APIReference ;
	schema:rangeIncludes schema:Text ;
	rdfs:comment "Library file name e.g., mscorlib.dll, system.web.dll" .

schema:assemblyVersion a rdf:Property ;
	rdfs:label "assemblyVersion" ;
	schema:domainIncludes schema:APIReference ;
	schema:rangeIncludes schema:Text ;
	rdfs:comment "Associated product/technology version. e.g., .NET Framework 4.5" .

schema:associatedAnatomy a rdf:Property ;
	rdfs:label "associatedAnatomy" ;
	schema:domainIncludes schema:MedicalCondition , schema:PhysicalActivity ;
	schema:rangeIncludes schema:AnatomicalStructure , schema:AnatomicalSystem , schema:SuperficialAnatomy ;
	rdfs:comment "The anatomy of the underlying organ system or structures associated with this entity." .

schema:associatedArticle a rdf:Property ;
	rdfs:label "associatedArticle" ;
	schema:domainIncludes schema:MediaObject ;
	schema:rangeIncludes schema:NewsArticle ;
	rdfs:comment "A NewsArticle associated with the Media Object." .

schema:associatedMedia a rdf:Property ;
	rdfs:label "associatedMedia" ;
	schema:domainIncludes schema:CreativeWork ;
	schema:rangeIncludes schema:MediaObject ;
	rdfs:comment "The media objects that encode this creative work. This property is a synonym for encodings." .

schema:associatedPathophysiology a rdf:Property ;
	rdfs:label "associatedPathophysiology" ;
	schema:domainIncludes schema:AnatomicalStructure , schema:AnatomicalSystem , schema:SuperficialAnatomy ;
	schema:rangeIncludes schema:Text ;
	rdfs:comment "If applicable, a description of the pathophysiology associated with the anatomical system, including potential abnormal changes in the mechanical, physical, and biochemical functions of the system." .

schema:attendee a rdf:Property ;
	rdfs:label "attendee" ;
	schema:domainIncludes schema:Event ;
	schema:rangeIncludes schema:Organization , schema:Person ;
	rdfs:comment "A person or organization attending the event." .

schema:attendees a rdf:Property ;
	rdfs:label "attendees" ;
	schema:domainIncludes schema:Event ;
	schema:rangeIncludes schema:Organization , schema:Person ;
	rdfs:comment "A person attending the event (legacy spelling; see singular form, attendee)." .

schema:audience a rdf:Property ;
	rdfs:label "audience" ;
	schema:domainIncludes schema:CreativeWork , schema:PlayAction , schema:Product ;
	schema:rangeIncludes schema:Audience ;
	rdfs:comment "The intended audience of the item, i.e. the group for whom the item was created." .

schema:audio a rdf:Property ;
	rdfs:label "audio" ;
	schema:domainIncludes schema:CreativeWork ;
	schema:rangeIncludes schema:AudioObject ;
	rdfs:comment "An embedded audio object." .

schema:author a rdf:Property ;
	rdfs:label "author" ;
	schema:domainIncludes schema:CreativeWork ;
	schema:rangeIncludes schema:Organization , schema:Person ;
	rdfs:comment "The author of this content. Please note that author is special in that HTML 5 provides a special mechanism for indicating authorship via the rel tag. That is equivalent to this and may be used interchangeably." .

schema:availability a rdf:Property ;
	rdfs:label "availability" ;
	schema:domainIncludes schema:Demand , schema:Offer ;
	schema:rangeIncludes schema:ItemAvailability ;
	rdfs:comment "The availability of this item&#x2014;for example In stock, Out of stock, Pre-order, etc." .

schema:availabilityEnds a rdf:Property ;
	rdfs:label "availabilityEnds" ;
	schema:domainIncludes schema:Demand , schema:Offer ;
	schema:rangeIncludes schema:DateTime ;
	rdfs:comment "The end of the availability of the product or service included in the offer." .

schema:availabilityStarts a rdf:Property ;
	rdfs:label "availabilityStarts" ;
	schema:domainIncludes schema:Demand , schema:Offer ;
	schema:rangeIncludes schema:DateTime ;
	rdfs:comment "The beginning of the availability of the product or service included in the offer." .

schema:availableAtOrFrom a rdf:Property ;
	rdfs:label "availableAtOrFrom" ;
	schema:domainIncludes schema:Demand , schema:Offer ;
	schema:rangeIncludes schema:Place ;
	rdfs:comment "The place(s) from which the offer can be obtained (e.g. store locations)." .

schema:availableDeliveryMethod a rdf:Property ;
	rdfs:label "availableDeliveryMethod" ;
	schema:domainIncludes schema:Demand , schema:Offer ;
	schema:rangeIncludes schema:DeliveryMethod ;
	rdfs:comment "The delivery method(s) available for this offer." .

schema:availableIn a rdf:Property ;
	rdfs:label "availableIn" ;
	schema:domainIncludes schema:DrugStrength ;
	schema:rangeIncludes schema:AdministrativeArea ;
	rdfs:comment "The location in which the strength is available." .

schema:availableService a rdf:Property ;
	rdfs:label "availableService" ;
	schema:domainIncludes schema:Hospital , schema:MedicalClinic , schema:Physician ;
	schema:rangeIncludes schema:MedicalProcedure , schema:MedicalTest , schema:MedicalTherapy ;
	rdfs:comment "A medical service available from this provider." .

schema:availableStrength a rdf:Property ;
	rdfs:label "availableStrength" ;
	schema:domainIncludes schema:Drug ;
	schema:rangeIncludes schema:DrugStrength ;
	rdfs:comment "An available dosage strength for the drug." .

schema:availableTest a rdf:Property ;
	rdfs:label "availableTest" ;
	schema:domainIncludes schema:DiagnosticLab ;
	schema:rangeIncludes schema:MedicalTest ;
	rdfs:comment "A diagnostic test or procedure offered by this lab." .

schema:award a rdf:Property ;
	rdfs:label "award" ;
	schema:domainIncludes schema:CreativeWork , schema:Person ;
	schema:rangeIncludes schema:Text ;
	rdfs:comment "An award won by this person or for this creative work." .

schema:awards a rdf:Property ;
	rdfs:label "awards" ;
	schema:domainIncludes schema:CreativeWork , schema:Person ;
	schema:rangeIncludes schema:Text ;
	rdfs:comment "Awards won by this person or for this creative work. (legacy spelling; see singular form, award)" .

schema:background a rdf:Property ;
	rdfs:label "background" ;
	schema:domainIncludes schema:DietarySupplement ;
	schema:rangeIncludes schema:Text ;
	rdfs:comment "Descriptive information establishing a historical perspective on the supplement. May include the rationale for the name, the population where the supplement first came to prominence, etc." .

schema:baseSalary a rdf:Property ;
	rdfs:label "baseSalary" ;
	schema:domainIncludes schema:JobPosting ;
	schema:rangeIncludes schema:Number ;
	rdfs:comment "The base salary of the job." .

schema:benefits a rdf:Property ;
	rdfs:label "benefits" ;
	schema:domainIncludes schema:JobPosting ;
	schema:rangeIncludes schema:Text ;
	rdfs:comment "Description of benefits associated with the job." .

schema:bestRating a rdf:Property ;
	rdfs:label "bestRating" ;
	schema:domainIncludes schema:Rating ;
	schema:rangeIncludes schema:Number , schema:Text ;
	rdfs:comment "The highest value allowed in this rating system. If bestRating is omitted, 5 is assumed." .

schema:billingIncrement a rdf:Property ;
	rdfs:label "billingIncrement" ;
	schema:domainIncludes schema:UnitPriceSpecification ;
	schema:rangeIncludes schema:Number ;
	rdfs:comment "This property specifies the minimal quantity and rounding increment that will be the basis for the billing. The unit of measurement is specified by the unitCode property." .

schema:biomechnicalClass a rdf:Property ;
	rdfs:label "biomechnicalClass" ;
	schema:domainIncludes schema:Joint ;
	schema:rangeIncludes schema:Text ;
	rdfs:comment "The biomechanical properties of the bone." .

schema:birthDate a rdf:Property ;
	rdfs:label "birthDate" ;
	schema:domainIncludes schema:Person ;
	schema:rangeIncludes schema:Date ;
	rdfs:comment "Date of birth." .

schema:bitrate a rdf:Property ;
	rdfs:label "bitrate" ;
	schema:domainIncludes schema:MediaObject ;
	schema:rangeIncludes schema:Text ;
	rdfs:comment "The bitrate of the media object." .

schema:blogPost a rdf:Property ;
	rdfs:label "blogPost" ;
	schema:domainIncludes schema:Blog ;
	schema:rangeIncludes schema:BlogPosting ;
	rdfs:comment "A posting that is part of this blog." .

schema:blogPosts a rdf:Property ;
	rdfs:label "blogPosts" ;
	schema:domainIncludes schema:Blog ;
	schema:rangeIncludes schema:BlogPosting ;
	rdfs:comment "The postings that are part of this blog (legacy spelling; see singular form, blogPost)." .

schema:bloodSupply a rdf:Property ;
	rdfs:label "bloodSupply" ;
	schema:domainIncludes schema:Muscle ;
	schema:rangeIncludes schema:Vessel ;
	rdfs:comment "The blood vessel that carries blood from the heart to the muscle." .

schema:bodyLocation a rdf:Property ;
	rdfs:label "bodyLocation" ;
	schema:domainIncludes schema:AnatomicalStructure ;
	schema:rangeIncludes schema:Text ;
	rdfs:comment "Location in the body of the anatomical structure." .

schema:bookEdition a rdf:Property ;
	rdfs:label "bookEdition" ;
	schema:domainIncludes schema:Book ;
	schema:rangeIncludes schema:Text ;
	rdfs:comment "The edition of the book." .

schema:bookFormat a rdf:Property ;
	rdfs:label "bookFormat" ;
	schema:domainIncludes schema:Book ;
	schema:rangeIncludes schema:BookFormatType ;
	rdfs:comment "The format of the book." .

schema:borrower a rdf:Property ;
	rdfs:label "borrower" ;
	schema:domainIncludes schema:LendAction ;
	schema:rangeIncludes schema:Person ;
	rdfs:comment "A sub property of participant. The person that borrows the object being lent." .

schema:box a rdf:Property ;
	rdfs:label "box" ;
	schema:domainIncludes schema:GeoShape ;
	schema:rangeIncludes schema:Text ;
	rdfs:comment "A polygon is the area enclosed by a point-to-point path for which the starting and ending points are the same. A polygon is expressed as a series of four or more spacedelimited points where the first and final points are identical." .

schema:branch a rdf:Property ;
	rdfs:label "branch" ;
	schema:domainIncludes schema:Nerve ;
	schema:rangeIncludes schema:AnatomicalStructure , schema:Nerve ;
	rdfs:comment "The branches that delineate from the nerve bundle." .

schema:branchOf a rdf:Property ;
	rdfs:label "branchOf" ;
	schema:domainIncludes schema:LocalBusiness ;
	schema:rangeIncludes schema:Organization ;
	rdfs:comment "The larger organization that this local business is a branch of, if any." .

schema:brand a rdf:Property ;
	rdfs:label "brand" ;
	schema:domainIncludes schema:Organization , schema:Person , schema:Product ;
	schema:rangeIncludes schema:Brand , schema:Organization ;
	rdfs:comment "The brand(s) associated with a product or service, or the brand(s) maintained by an organization or business person." .

schema:breadcrumb a rdf:Property ;
	rdfs:label "breadcrumb" ;
	schema:domainIncludes schema:WebPage ;
	schema:rangeIncludes schema:Text ;
	rdfs:comment "A set of links that can help a user understand and navigate a website hierarchy." .

schema:breastfeedingWarning a rdf:Property ;
	rdfs:label "breastfeedingWarning" ;
	schema:domainIncludes schema:Drug ;
	schema:rangeIncludes schema:Text ;
	rdfs:comment "Any precaution, guidance, contraindication, etc. related to this drug's use by breastfeeding mothers." .

schema:browserRequirements a rdf:Property ;
	rdfs:label "browserRequirements" ;
	schema:domainIncludes schema:WebApplication ;
	schema:rangeIncludes schema:Text ;
	rdfs:comment "Specifies browser requirements in human-readable text. For example,\"requires HTML5 support\"." .

schema:businessFunction a rdf:Property ;
	rdfs:label "businessFunction" ;
	schema:domainIncludes schema:Demand , schema:Offer , schema:TypeAndQuantityNode ;
	schema:rangeIncludes schema:BusinessFunction ;
	rdfs:comment "The business function (e.g. sell, lease, repair, dispose) of the offer or component of a bundle (TypeAndQuantityNode). The default is http://purl.org/goodrelations/v1#Sell." .

schema:buyer a rdf:Property ;
	rdfs:label "buyer" ;
	schema:domainIncludes schema:SellAction ;
	schema:rangeIncludes schema:Person ;
	rdfs:comment "A sub property of participant. The participant/person/organization that bought the object." .

schema:byArtist a rdf:Property ;
	rdfs:label "byArtist" ;
	schema:domainIncludes schema:MusicAlbum , schema:MusicRecording ;
	schema:rangeIncludes schema:MusicGroup ;
	rdfs:comment "The artist that performed this album or recording." .

schema:calories a rdf:Property ;
	rdfs:label "calories" ;
	schema:domainIncludes schema:NutritionInformation ;
	schema:rangeIncludes schema:Energy ;
	rdfs:comment "The number of calories" .

schema:candidate a rdf:Property ;
	rdfs:label "candidate" ;
	schema:domainIncludes schema:VoteAction ;
	schema:rangeIncludes schema:Person ;
	rdfs:comment "A sub property of object. The candidate subject of this action." .

schema:caption a rdf:Property ;
	rdfs:label "caption" ;
	schema:domainIncludes schema:ImageObject , schema:VideoObject ;
	schema:rangeIncludes schema:Text ;
	rdfs:comment "The caption for this object." .

schema:carbohydrateContent a rdf:Property ;
	rdfs:label "carbohydrateContent" ;
	schema:domainIncludes schema:NutritionInformation ;
	schema:rangeIncludes schema:Mass ;
	rdfs:comment "The number of grams of carbohydrates." .

schema:carrierRequirements a rdf:Property ;
	rdfs:label "carrierRequirements" ;
	schema:domainIncludes schema:MobileApplication ;
	schema:rangeIncludes schema:Text ;
	rdfs:comment "Specifies specific carrier(s) requirements for the application (e.g. an application may only work on a specific carrier network)." .

schema:catalog a rdf:Property ;
	rdfs:label "catalog" ;
	schema:domainIncludes schema:Dataset ;
	schema:rangeIncludes schema:DataCatalog ;
	rdfs:comment "A data catalog which contains a dataset." .

schema:category a rdf:Property ;
	rdfs:label "category" ;
	schema:domainIncludes schema:Offer , schema:PhysicalActivity ;
	schema:rangeIncludes schema:PhysicalActivityCategory , schema:Text , schema:Thing ;
	rdfs:comment "A category for the item. Greater signs or slashes can be used to informally indicate a category hierarchy." .

schema:cause a rdf:Property ;
	rdfs:label "cause" ;
	schema:domainIncludes schema:MedicalCondition , schema:MedicalSignOrSymptom ;
	schema:rangeIncludes schema:MedicalCause ;
	rdfs:comment "An underlying cause. More specifically, one of the causative agent(s) that are most directly responsible for the pathophysiologic process that eventually results in the occurrence." .

schema:causeOf a rdf:Property ;
	rdfs:label "causeOf" ;
	schema:domainIncludes schema:MedicalCause ;
	schema:rangeIncludes schema:MedicalEntity ;
	rdfs:comment "The condition, complication, symptom, sign, etc. caused." .

schema:childMaxAge a rdf:Property ;
	rdfs:label "childMaxAge" ;
	schema:domainIncludes schema:ParentAudience ;
	schema:rangeIncludes schema:Number ;
	rdfs:comment "Maximal age of the child" .

schema:childMinAge a rdf:Property ;
	rdfs:label "childMinAge" ;
	schema:domainIncludes schema:ParentAudience ;
	schema:rangeIncludes schema:Number ;
	rdfs:comment "Minimal age of the child" .

schema:children a rdf:Property ;
	rdfs:label "children" ;
	schema:domainIncludes schema:Person ;
	schema:rangeIncludes schema:Person ;
	rdfs:comment "A child of the person." .

schema:cholesterolContent a rdf:Property ;
	rdfs:label "cholesterolContent" ;
	schema:domainIncludes schema:NutritionInformation ;
	schema:rangeIncludes schema:Mass ;
	rdfs:comment "The number of milligrams of cholesterol." .

schema:circle a rdf:Property ;
	rdfs:label "circle" ;
	schema:domainIncludes schema:GeoShape ;
	schema:rangeIncludes schema:Text ;
	rdfs:comment "A circle is the circular region of a specified radius centered at a specified latitude and longitude. A circle is expressed as a pair followed by a radius in meters." .

schema:citation a rdf:Property ;
	rdfs:label "citation" ;
	schema:domainIncludes schema:CreativeWork ;
	schema:rangeIncludes schema:CreativeWork , schema:Text ;
	rdfs:comment "A citation or reference to another creative work, such as another publication, web page, scholarly article, etc. NOTE: Candidate for promotion to ScholarlyArticle." .

schema:clincalPharmacology a rdf:Property ;
	rdfs:label "clincalPharmacology" ;
	schema:domainIncludes schema:Drug ;
	schema:rangeIncludes schema:Text ;
	rdfs:comment "Description of the absorption and elimination of drugs, including their concentration (pharmacokinetics, pK) and biological effects (pharmacodynamics, pD)." .

schema:closes a rdf:Property ;
	rdfs:label "closes" ;
	schema:domainIncludes schema:OpeningHoursSpecification ;
	schema:rangeIncludes schema:Time ;
	rdfs:comment "The closing hour of the place or service on the given day(s) of the week." .

schema:code a rdf:Property ;
	rdfs:label "code" ;
	schema:domainIncludes schema:MedicalEntity ;
	schema:rangeIncludes schema:MedicalCode ;
	rdfs:comment "A medical code for the entity, taken from a controlled vocabulary or ontology such as ICD-9, DiseasesDB, MeSH, SNOMED-CT, RxNorm, etc." .

schema:codeRepository a rdf:Property ;
	rdfs:label "codeRepository" ;
	schema:domainIncludes schema:Code ;
	schema:rangeIncludes schema:URL ;
	rdfs:comment "Link to the repository where the un-compiled, human readable code and related code is located (SVN, github, CodePlex)" .

schema:codeValue a rdf:Property ;
	rdfs:label "codeValue" ;
	schema:domainIncludes schema:MedicalCode ;
	schema:rangeIncludes schema:Text ;
	rdfs:comment "The actual code." .

schema:codingSystem a rdf:Property ;
	rdfs:label "codingSystem" ;
	schema:domainIncludes schema:MedicalCode ;
	schema:rangeIncludes schema:Text ;
	rdfs:comment "The coding system, e.g. 'ICD-10'." .

schema:colleague a rdf:Property ;
	rdfs:label "colleague" ;
	schema:domainIncludes schema:Person ;
	schema:rangeIncludes schema:Person ;
	rdfs:comment "A colleague of the person." .

schema:colleagues a rdf:Property ;
	rdfs:label "colleagues" ;
	schema:domainIncludes schema:Person ;
	schema:rangeIncludes schema:Person ;
	rdfs:comment "A colleague of the person (legacy spelling; see singular form, colleague)." .

schema:collection a rdf:Property ;
	rdfs:label "collection" ;
	schema:domainIncludes schema:UpdateAction ;
	schema:rangeIncludes schema:Thing ;
	rdfs:comment "A sub property of object. The collection target of the action." .

schema:color a rdf:Property ;
	rdfs:label "color" ;
	schema:domainIncludes schema:Product ;
	schema:rangeIncludes schema:Text ;
	rdfs:comment "The color of the product." .

schema:comment a rdf:Property ;
	rdfs:label "comment" ;
	schema:domainIncludes schema:CreativeWork ;
	schema:rangeIncludes schema:UserComments ;
	rdfs:comment "Comments, typically from users, on this CreativeWork." .

schema:commentText a rdf:Property ;
	rdfs:label "commentText" ;
	schema:domainIncludes schema:UserComments ;
	schema:rangeIncludes schema:Text ;
	rdfs:comment "The text of the UserComment." .

schema:commentTime a rdf:Property ;
	rdfs:label "commentTime" ;
	schema:domainIncludes schema:UserComments ;
	schema:rangeIncludes schema:Date ;
	rdfs:comment "The time at which the UserComment was made." .

schema:comprisedOf a rdf:Property ;
	rdfs:label "comprisedOf" ;
	schema:domainIncludes schema:AnatomicalSystem ;
	schema:rangeIncludes schema:AnatomicalStructure , schema:AnatomicalSystem ;
	rdfs:comment "The underlying anatomical structures, such as organs, that comprise the anatomical system." .

schema:connectedTo a rdf:Property ;
	rdfs:label "connectedTo" ;
	schema:domainIncludes schema:AnatomicalStructure ;
	schema:rangeIncludes schema:AnatomicalStructure ;
	rdfs:comment "Other anatomical structures to which this structure is connected." .

schema:contactPoint a rdf:Property ;
	rdfs:label "contactPoint" ;
	schema:domainIncludes schema:Organization , schema:Person ;
	schema:rangeIncludes schema:ContactPoint ;
	rdfs:comment "A contact point for a person or organization." .

schema:contactPoints a rdf:Property ;
	rdfs:label "contactPoints" ;
	schema:domainIncludes schema:Organization , schema:Person ;
	schema:rangeIncludes schema:ContactPoint ;
	rdfs:comment "A contact point for a person or organization (legacy spelling; see singular form, contactPoint)." .

schema:contactType a rdf:Property ;
	rdfs:label "contactType" ;
	schema:domainIncludes schema:ContactPoint ;
	schema:rangeIncludes schema:Text ;
	rdfs:comment "A person or organization can have different contact points, for different purposes. For example, a sales contact point, a PR contact point and so on. This property is used to specify the kind of contact point." .

schema:containedIn a rdf:Property ;
	rdfs:label "containedIn" ;
	schema:domainIncludes schema:Place ;
	schema:rangeIncludes schema:Place ;
	rdfs:comment "The basic containment relation between places." .

schema:contentLocation a rdf:Property ;
	rdfs:label "contentLocation" ;
	schema:domainIncludes schema:CreativeWork ;
	schema:rangeIncludes schema:Place ;
	rdfs:comment "The location of the content." .

schema:contentRating a rdf:Property ;
	rdfs:label "contentRating" ;
	schema:domainIncludes schema:CreativeWork ;
	schema:rangeIncludes schema:Text ;
	rdfs:comment "Official rating of a piece of content&#x2014;for example,'MPAA PG-13'." .

schema:contentSize a rdf:Property ;
	rdfs:label "contentSize" ;
	schema:domainIncludes schema:MediaObject ;
	schema:rangeIncludes schema:Text ;
	rdfs:comment "File size in (mega/kilo) bytes." .

schema:contentUrl a rdf:Property ;
	rdfs:label "contentUrl" ;
	schema:domainIncludes schema:MediaObject ;
	schema:rangeIncludes schema:URL ;
	rdfs:comment "Actual bytes of the media object, for example the image file or video file. (previous spelling: contentURL)" .

schema:contraindication a rdf:Property ;
	rdfs:label "contraindication" ;
	schema:domainIncludes schema:MedicalDevice , schema:MedicalTherapy ;
	schema:rangeIncludes schema:MedicalContraindication ;
	rdfs:comment "A contraindication for this therapy." .

schema:contributor a rdf:Property ;
	rdfs:label "contributor" ;
	schema:domainIncludes schema:CreativeWork ;
	schema:rangeIncludes schema:Organization , schema:Person ;
	rdfs:comment "A secondary contributor to the CreativeWork." .

schema:cookTime a rdf:Property ;
	rdfs:label "cookTime" ;
	schema:domainIncludes schema:Recipe ;
	schema:rangeIncludes schema:Duration ;
	rdfs:comment "The time it takes to actually cook the dish, in <a href='http://en.wikipedia.org/wiki/ISO_8601'>ISO 8601 duration format</a>." .

schema:cookingMethod a rdf:Property ;
	rdfs:label "cookingMethod" ;
	schema:domainIncludes schema:Recipe ;
	schema:rangeIncludes schema:Text ;
	rdfs:comment "The method of cooking, such as Frying, Steaming, ..." .

schema:copyrightHolder a rdf:Property ;
	rdfs:label "copyrightHolder" ;
	schema:domainIncludes schema:CreativeWork ;
	schema:rangeIncludes schema:Organization , schema:Person ;
	rdfs:comment "The party holding the legal copyright to the CreativeWork." .

schema:copyrightYear a rdf:Property ;
	rdfs:label "copyrightYear" ;
	schema:domainIncludes schema:CreativeWork ;
	schema:rangeIncludes schema:Number ;
	rdfs:comment "The year during which the claimed copyright for the CreativeWork was first asserted." .

schema:cost a rdf:Property ;
	rdfs:label "cost" ;
	schema:domainIncludes schema:Drug ;
	schema:rangeIncludes schema:DrugCost ;
	rdfs:comment "Cost per unit of the drug, as reported by the source being tagged." .

schema:costCategory a rdf:Property ;
	rdfs:label "costCategory" ;
	schema:domainIncludes schema:DrugCost ;
	schema:rangeIncludes schema:DrugCostCategory ;
	rdfs:comment "The category of cost, such as wholesale, retail, reimbursement cap, etc." .

schema:costCurrency a rdf:Property ;
	rdfs:label "costCurrency" ;
	schema:domainIncludes schema:DrugCost ;
	schema:rangeIncludes schema:Text ;
	rdfs:comment "The currency (in 3-letter <a href=http://en.wikipedia.org/wiki/ISO_4217>ISO 4217 format</a>) of the drug cost." .

schema:costOrigin a rdf:Property ;
	rdfs:label "costOrigin" ;
	schema:domainIncludes schema:DrugCost ;
	schema:rangeIncludes schema:Text ;
	rdfs:comment "Additional details to capture the origin of the cost data. For example, 'Medicare Part B'." .

schema:costPerUnit a rdf:Property ;
	rdfs:label "costPerUnit" ;
	schema:domainIncludes schema:DrugCost ;
	schema:rangeIncludes schema:Number , schema:Text ;
	rdfs:comment "The cost per unit of the drug." .

schema:countriesNotSupported a rdf:Property ;
	rdfs:label "countriesNotSupported" ;
	schema:domainIncludes schema:SoftwareApplication ;
	schema:rangeIncludes schema:Text ;
	rdfs:comment "Countries for which the application is not supported. You can also provide the two-letter ISO 3166-1 alpha-2 country code." .

schema:countriesSupported a rdf:Property ;
	rdfs:label "countriesSupported" ;
	schema:domainIncludes schema:SoftwareApplication ;
	schema:rangeIncludes schema:Text ;
	rdfs:comment "Countries for which the application is supported. You can also provide the two-letter ISO 3166-1 alpha-2 country code." .

schema:course a rdf:Property ;
	rdfs:label "course" ;
	schema:domainIncludes schema:ExerciseAction ;
	schema:rangeIncludes schema:Place ;
	rdfs:comment "A sub property of location. The course where this action was taken." .

schema:creator a rdf:Property ;
	rdfs:label "creator" ;
	schema:domainIncludes schema:CreativeWork , schema:UserComments ;
	schema:rangeIncludes schema:Organization , schema:Person ;
	rdfs:comment "The creator/author of this CreativeWork or UserComments. This is the same as the Author property for CreativeWork." .

schema:currenciesAccepted a rdf:Property ;
	rdfs:label "currenciesAccepted" ;
	schema:domainIncludes schema:LocalBusiness ;
	schema:rangeIncludes schema:Text ;
	rdfs:comment "The currency accepted (in <a href='http://en.wikipedia.org/wiki/ISO_4217'>ISO 4217 currency format</a>)." .

schema:dataset a rdf:Property ;
	rdfs:label "dataset" ;
	schema:domainIncludes schema:DataCatalog ;
	schema:rangeIncludes schema:Dataset ;
	rdfs:comment "A dataset contained in a catalog." .

schema:dateCreated a rdf:Property ;
	rdfs:label "dateCreated" ;
	schema:domainIncludes schema:CreativeWork ;
	schema:rangeIncludes schema:Date ;
	rdfs:comment "The date on which the CreativeWork was created." .

schema:dateModified a rdf:Property ;
	rdfs:label "dateModified" ;
	schema:domainIncludes schema:CreativeWork ;
	schema:rangeIncludes schema:Date ;
	rdfs:comment "The date on which the CreativeWork was most recently modified." .

schema:datePosted a rdf:Property ;
	rdfs:label "datePosted" ;
	schema:domainIncludes schema:JobPosting ;
	schema:rangeIncludes schema:Date ;
	rdfs:comment "Publication date for the job posting." .

schema:datePublished a rdf:Property ;
	rdfs:label "datePublished" ;
	schema:domainIncludes schema:CreativeWork ;
	schema:rangeIncludes schema:Date ;
	rdfs:comment "Date of first broadcast/publication." .

schema:dateline a rdf:Property ;
	rdfs:label "dateline" ;
	schema:domainIncludes schema:NewsArticle ;
	schema:rangeIncludes schema:Text ;
	rdfs:comment "The location where the NewsArticle was produced." .

schema:dayOfWeek a rdf:Property ;
	rdfs:label "dayOfWeek" ;
	schema:domainIncludes schema:OpeningHoursSpecification ;
	schema:rangeIncludes schema:DayOfWeek ;
	rdfs:comment "The day of the week for which these opening hours are valid." .

schema:deathDate a rdf:Property ;
	rdfs:label "deathDate" ;
	schema:domainIncludes schema:Person ;
	schema:rangeIncludes schema:Date ;
	rdfs:comment "Date of death." .

schema:deliveryLeadTime a rdf:Property ;
	rdfs:label "deliveryLeadTime" ;
	schema:domainIncludes schema:Demand , schema:Offer ;
	schema:rangeIncludes schema:QuantitativeValue ;
	rdfs:comment "The typical delay between the receipt of the order and the goods leaving the warehouse." .

schema:deliveryMethod a rdf:Property ;
	rdfs:label "deliveryMethod" ;
	schema:domainIncludes schema:ReceiveAction , schema:SendAction , schema:TrackAction ;
	schema:rangeIncludes schema:DeliveryMethod ;
	rdfs:comment "A sub property of instrument. The method of delivery" .

schema:dependencies a rdf:Property ;
	rdfs:label "dependencies" ;
	schema:domainIncludes schema:TechArticle ;
	schema:rangeIncludes schema:Text ;
	rdfs:comment "Prerequisites needed to fulfill steps in article." .

schema:depth a rdf:Property ;
	rdfs:label "depth" ;
	schema:domainIncludes schema:Product ;
	schema:rangeIncludes schema:Distance , schema:QuantitativeValue ;
	rdfs:comment "The depth of the product." .

schema:description a rdf:Property ;
	rdfs:label "description" ;
	schema:domainIncludes schema:Thing ;
	schema:rangeIncludes schema:Text ;
	rdfs:comment "A short description of the item." .

schema:device a rdf:Property ;
	rdfs:label "device" ;
	schema:domainIncludes schema:SoftwareApplication ;
	schema:rangeIncludes schema:Text ;
	rdfs:comment "Device required to run the application. Used in cases where a specific make/model is required to run the application." .

schema:diagnosis a rdf:Property ;
	rdfs:label "diagnosis" ;
	schema:domainIncludes schema:DDxElement ;
	schema:rangeIncludes schema:MedicalCondition ;
	rdfs:comment "One or more alternative conditions considered in the differential diagnosis process." .

schema:diagram a rdf:Property ;
	rdfs:label "diagram" ;
	schema:domainIncludes schema:AnatomicalStructure ;
	schema:rangeIncludes schema:ImageObject ;
	rdfs:comment "An image containing a diagram that illustrates the structure and/or its component substructures and/or connections with other structures." .

schema:diet a rdf:Property ;
	rdfs:label "diet" ;
	schema:domainIncludes schema:ExerciseAction ;
	schema:rangeIncludes schema:Diet ;
	rdfs:comment "A sub property of instrument. The died used in this action." .

schema:dietFeatures a rdf:Property ;
	rdfs:label "dietFeatures" ;
	schema:domainIncludes schema:Diet ;
	schema:rangeIncludes schema:Text ;
	rdfs:comment "Nutritional information specific to the dietary plan. May include dietary recommendations on what foods to avoid, what foods to consume, and specific alterations/deviations from the USDA or other regulatory body's approved dietary guidelines." .

schema:differentialDiagnosis a rdf:Property ;
	rdfs:label "differentialDiagnosis" ;
	schema:domainIncludes schema:MedicalCondition ;
	schema:rangeIncludes schema:DDxElement ;
	rdfs:comment "One of a set of differential diagnoses for the condition. Specifically, a closely-related or competing diagnosis typically considered later in the cognitive process whereby this medical condition is distinguished from others most likely responsible for a similar collection of signs and symptoms to reach the most parsimonious diagnosis or diagnoses in a patient." .

schema:director a rdf:Property ;
	rdfs:label "director" ;
	schema:domainIncludes schema:Movie , schema:TVEpisode , schema:TVSeries ;
	schema:rangeIncludes schema:Person ;
	rdfs:comment "The director of the movie, TV episode, or series." .

schema:discusses a rdf:Property ;
	rdfs:label "discusses" ;
	schema:domainIncludes schema:UserComments ;
	schema:rangeIncludes schema:CreativeWork ;
	rdfs:comment "Specifies the CreativeWork associated with the UserComment." .

schema:discussionUrl a rdf:Property ;
	rdfs:label "discussionUrl" ;
	schema:domainIncludes schema:CreativeWork ;
	schema:rangeIncludes schema:URL ;
	rdfs:comment "A link to the page containing the comments of the CreativeWork." .

schema:distance a rdf:Property ;
	rdfs:label "distance" ;
	schema:domainIncludes schema:ExerciseAction , schema:TravelAction ;
	schema:rangeIncludes schema:Distance ;
	rdfs:comment "A sub property of asset. The distance travelled." .

schema:distinguishingSign a rdf:Property ;
	rdfs:label "distinguishingSign" ;
	schema:domainIncludes schema:DDxElement ;
	schema:rangeIncludes schema:MedicalSignOrSymptom ;
	rdfs:comment "One of a set of signs and symptoms that can be used to distinguish this diagnosis from others in the differential diagnosis." .

schema:distribution a rdf:Property ;
	rdfs:label "distribution" ;
	schema:domainIncludes schema:Dataset ;
	schema:rangeIncludes schema:DataDownload ;
	rdfs:comment "A downloadable form of this dataset, at a specific location, in a specific format." .

schema:domainIncludes a rdf:Property ;
	rdfs:label "domainIncludes" ;
	schema:domainIncludes schema:Property ;
	schema:rangeIncludes schema:Class ;
	rdfs:comment "Relates a property to a class that is (one of) the type(s) the property is expected to be used on." .

schema:dosageForm a rdf:Property ;
	rdfs:label "dosageForm" ;
	schema:domainIncludes schema:DietarySupplement , schema:Drug ;
	schema:rangeIncludes schema:Text ;
	rdfs:comment "A dosage form in which this drug/supplement is available, e.g. 'tablet', 'suspension', 'injection'." .

schema:doseSchedule a rdf:Property ;
	rdfs:label "doseSchedule" ;
	schema:domainIncludes schema:Drug ;
	schema:rangeIncludes schema:DoseSchedule ;
	rdfs:comment "A dosing schedule for the drug for a given population, either observed, recommended, or maximum dose based on the type used." .

schema:doseUnit a rdf:Property ;
	rdfs:label "doseUnit" ;
	schema:domainIncludes schema:DoseSchedule ;
	schema:rangeIncludes schema:Text ;
	rdfs:comment "The unit of the dose, e.g. 'mg'." .

schema:doseValue a rdf:Property ;
	rdfs:label "doseValue" ;
	schema:domainIncludes schema:DoseSchedule ;
	schema:rangeIncludes schema:Number ;
	rdfs:comment "The value of the dose, e.g. 500." .

schema:downloadUrl a rdf:Property ;
	rdfs:label "downloadUrl" ;
	schema:domainIncludes schema:SoftwareApplication ;
	schema:rangeIncludes schema:URL ;
	rdfs:comment "If the file can be downloaded, URL to download the binary." .

schema:drainsTo a rdf:Property ;
	rdfs:label "drainsTo" ;
	schema:domainIncludes schema:Vein ;
	schema:rangeIncludes schema:Vessel ;
	rdfs:comment "The vasculature that the vein drains into." .

schema:drug a rdf:Property ;
	rdfs:label "drug" ;
	schema:domainIncludes schema:DrugClass ;
	schema:rangeIncludes schema:Drug ;
	rdfs:comment "A drug in this drug class." .

schema:drugClass a rdf:Property ;
	rdfs:label "drugClass" ;
	schema:domainIncludes schema:Drug ;
	schema:rangeIncludes schema:DrugClass ;
	rdfs:comment "The class of drug this belongs to (e.g., statins)." .

schema:drugUnit a rdf:Property ;
	rdfs:label "drugUnit" ;
	schema:domainIncludes schema:DrugCost ;
	schema:rangeIncludes schema:Text ;
	rdfs:comment "The unit in which the drug is measured, e.g. '5 mg tablet'." .

schema:duns a rdf:Property ;
	rdfs:label "duns" ;
	schema:domainIncludes schema:Organization , schema:Person ;
	schema:rangeIncludes schema:Text ;
	rdfs:comment "The Dun & Bradstreet DUNS number for identifying an organization or business person." .

schema:duplicateTherapy a rdf:Property ;
	rdfs:label "duplicateTherapy" ;
	schema:domainIncludes schema:MedicalTherapy ;
	schema:rangeIncludes schema:MedicalTherapy ;
	rdfs:comment "A therapy that duplicates or overlaps this one." .

schema:duration a rdf:Property ;
	rdfs:label "duration" ;
	schema:domainIncludes schema:Event , schema:MediaObject , schema:Movie , schema:MusicRecording ;
	schema:rangeIncludes schema:Duration ;
	rdfs:comment "The duration of the item (movie, audio recording, event, etc.) in <a href='http://en.wikipedia.org/wiki/ISO_8601'>ISO 8601 date format</a>." .

schema:durationOfWarranty a rdf:Property ;
	rdfs:label "durationOfWarranty" ;
	schema:domainIncludes schema:WarrantyPromise ;
	schema:rangeIncludes schema:QuantitativeValue ;
	rdfs:comment "The duration of the warranty promise. Common unitCode values are ANN for year, MON for months, or DAY for days." .

schema:editor a rdf:Property ;
	rdfs:label "editor" ;
	schema:domainIncludes schema:CreativeWork ;
	schema:rangeIncludes schema:Person ;
	rdfs:comment "Specifies the Person who edited the CreativeWork." .

schema:educationRequirements a rdf:Property ;
	rdfs:label "educationRequirements" ;
	schema:domainIncludes schema:JobPosting ;
	schema:rangeIncludes schema:Text ;
	rdfs:comment "Educational background needed for the position." .

schema:educationalAlignment a rdf:Property ;
	rdfs:label "educationalAlignment" ;
	schema:domainIncludes schema:CreativeWork ;
	schema:rangeIncludes schema:AlignmentObject ;
	rdfs:comment "An alignment to an established educational framework." .

schema:educationalFramework a rdf:Property ;
	rdfs:label "educationalFramework" ;
	schema:domainIncludes schema:AlignmentObject ;
	schema:rangeIncludes schema:Text ;
	rdfs:comment "The framework to which the resource being described is aligned." .

schema:educationalRole a rdf:Property ;
	rdfs:label "educationalRole" ;
	schema:domainIncludes schema:EducationalAudience ;
	schema:rangeIncludes schema:Text ;
	rdfs:comment "An educationalRole of an EducationalAudience" .

schema:educationalUse a rdf:Property ;
	rdfs:label "educationalUse" ;
	schema:domainIncludes schema:CreativeWork ;
	schema:rangeIncludes schema:Text ;
	rdfs:comment "The purpose of a work in the context of education; for example, 'assignment', 'group work'." .

schema:elevation a rdf:Property ;
	rdfs:label "elevation" ;
	schema:domainIncludes schema:GeoCoordinates , schema:GeoShape ;
	schema:rangeIncludes schema:Number , schema:Text ;
	rdfs:comment "The elevation of a location." .

schema:eligibleCustomerType a rdf:Property ;
	rdfs:label "eligibleCustomerType" ;
	schema:domainIncludes schema:Demand , schema:Offer ;
	schema:rangeIncludes schema:BusinessEntityType ;
	rdfs:comment "The type(s) of customers for which the given offer is valid." .

schema:eligibleDuration a rdf:Property ;
	rdfs:label "eligibleDuration" ;
	schema:domainIncludes schema:Demand , schema:Offer ;
	schema:rangeIncludes schema:QuantitativeValue ;
	rdfs:comment "The duration for which the given offer is valid." .

schema:eligibleQuantity a rdf:Property ;
	rdfs:label "eligibleQuantity" ;
	schema:domainIncludes schema:Demand , schema:Offer , schema:PriceSpecification ;
	schema:rangeIncludes schema:QuantitativeValue ;
	rdfs:comment "The interval and unit of measurement of ordering quantities for which the offer or price specification is valid. This allows e.g. specifying that a certain freight charge is valid only for a certain quantity." .

schema:eligibleRegion a rdf:Property ;
	rdfs:label "eligibleRegion" ;
	schema:domainIncludes schema:DeliveryChargeSpecification , schema:Demand , schema:Offer ;
	schema:rangeIncludes schema:GeoShape , schema:Text ;
	rdfs:comment "The ISO 3166-1 (ISO 3166-1 alpha-2) or ISO 3166-2 code, or the GeoShape for the geo-political region(s) for which the offer or delivery charge specification is valid." .

schema:eligibleTransactionVolume a rdf:Property ;
	rdfs:label "eligibleTransactionVolume" ;
	schema:domainIncludes schema:Demand , schema:Offer , schema:PriceSpecification ;
	schema:rangeIncludes schema:PriceSpecification ;
	rdfs:comment "The transaction volume, in a monetary unit, for which the offer or price specification is valid, e.g. for indicating a minimal purchasing volume, to express free shipping above a certain order volume, or to limit the acceptance of credit cards to purchases to a certain minimal amount." .

schema:email a rdf:Property ;
	rdfs:label "email" ;
	schema:domainIncludes schema:ContactPoint , schema:Organization , schema:Person ;
	schema:rangeIncludes schema:Text ;
	rdfs:comment "Email address." .

schema:embedUrl a rdf:Property ;
	rdfs:label "embedUrl" ;
	schema:domainIncludes schema:MediaObject ;
	schema:rangeIncludes schema:URL ;
	rdfs:comment "A URL pointing to a player for a specific video. In general, this is the information in the <code>src</code> element of an <code>embed</code> tag and should not be the same as the content of the <code>loc</code> tag. (previous spelling: embedURL)" .

schema:employee a rdf:Property ;
	rdfs:label "employee" ;
	schema:domainIncludes schema:Organization ;
	schema:rangeIncludes schema:Person ;
	rdfs:comment "Someone working for this organization." .

schema:employees a rdf:Property ;
	rdfs:label "employees" ;
	schema:domainIncludes schema:Organization ;
	schema:rangeIncludes schema:Person ;
	rdfs:comment "People working for this organization. (legacy spelling; see singular form, employee)" .

schema:employmentType a rdf:Property ;
	rdfs:label "employmentType" ;
	schema:domainIncludes schema:JobPosting ;
	schema:rangeIncludes schema:Text ;
	rdfs:comment "Type of employment (e.g. full-time, part-time, contract, temporary, seasonal, internship)." .

schema:encodesCreativeWork a rdf:Property ;
	rdfs:label "encodesCreativeWork" ;
	schema:domainIncludes schema:MediaObject ;
	schema:rangeIncludes schema:CreativeWork ;
	rdfs:comment "The creative work encoded by this media object" .

schema:encoding a rdf:Property ;
	rdfs:label "encoding" ;
	schema:domainIncludes schema:CreativeWork ;
	schema:rangeIncludes schema:MediaObject ;
	rdfs:comment "A media object that encode this CreativeWork." .

schema:encodingFormat a rdf:Property ;
	rdfs:label "encodingFormat" ;
	schema:domainIncludes schema:MediaObject ;
	schema:rangeIncludes schema:Text ;
	rdfs:comment "mp3, mpeg4, etc." .

schema:encodings a rdf:Property ;
	rdfs:label "encodings" ;
	schema:domainIncludes schema:CreativeWork ;
	schema:rangeIncludes schema:MediaObject ;
	rdfs:comment "The media objects that encode this creative work (legacy spelling; see singular form, encoding)." .

schema:endDate a rdf:Property ;
	rdfs:label "endDate" ;
	schema:domainIncludes schema:Event , schema:TVSeason , schema:TVSeries ;
	schema:rangeIncludes schema:Date ;
	rdfs:comment "The end date and time of the event (in <a href='http://en.wikipedia.org/wiki/ISO_8601'>ISO 8601 date format</a>)." .

schema:endTime a rdf:Property ;
	rdfs:label "endTime" ;
	schema:domainIncludes schema:Action ;
	schema:rangeIncludes schema:DateTime ;
	rdfs:comment "When the Action was performed: end time. This is for actions that span a period of time. e.g. John wrote a book from January to *December*." .

schema:endorsee a rdf:Property ;
	rdfs:label "endorsee" ;
	schema:domainIncludes schema:EndorseAction ;
	schema:rangeIncludes schema:Organization , schema:Person ;
	rdfs:comment "A sub property of participant. The person/organization being supported." .

schema:endorsers a rdf:Property ;
	rdfs:label "endorsers" ;
	schema:domainIncludes schema:Diet ;
	schema:rangeIncludes schema:Organization , schema:Person ;
	rdfs:comment "People or organizations that endorse the plan." .

schema:entertainmentBusiness a rdf:Property ;
	rdfs:label "entertainmentBusiness" ;
	schema:domainIncludes schema:PerformAction ;
	schema:rangeIncludes schema:EntertainmentBusiness ;
	rdfs:comment "A sub property of location. The entertainment business where the action occurred." .

schema:epidemiology a rdf:Property ;
	rdfs:label "epidemiology" ;
	schema:domainIncludes schema:MedicalCondition , schema:PhysicalActivity ;
	schema:rangeIncludes schema:Text ;
	rdfs:comment "The characteristics of associated patients, such as age, gender, race etc." .

schema:episode a rdf:Property ;
	rdfs:label "episode" ;
	schema:domainIncludes schema:TVSeason , schema:TVSeries ;
	schema:rangeIncludes schema:TVEpisode ;
	rdfs:comment "An episode of a TV series or season." .

schema:episodeNumber a rdf:Property ;
	rdfs:label "episodeNumber" ;
	schema:domainIncludes schema:TVEpisode ;
	schema:rangeIncludes schema:Number ;
	rdfs:comment "The episode number." .

schema:episodes a rdf:Property ;
	rdfs:label "episodes" ;
	schema:domainIncludes schema:TVSeason , schema:TVSeries ;
	schema:rangeIncludes schema:TVEpisode ;
	rdfs:comment "The episode of a TV series or season (legacy spelling; see singular form, episode)." .

schema:equal a rdf:Property ;
	rdfs:label "equal" ;
	schema:domainIncludes schema:QualitativeValue ;
	schema:rangeIncludes schema:QualitativeValue ;
	rdfs:comment "This ordering relation for qualitative values indicates that the subject is equal to the object." .

schema:estimatesRiskOf a rdf:Property ;
	rdfs:label "estimatesRiskOf" ;
	schema:domainIncludes schema:MedicalRiskEstimator ;
	schema:rangeIncludes schema:MedicalEntity ;
	rdfs:comment "The condition, complication, or symptom whose risk is being estimated." .

schema:event a rdf:Property ;
	rdfs:label "event" ;
	schema:domainIncludes schema:InformAction , schema:InviteAction , schema:JoinAction , schema:LeaveAction , schema:Organization , schema:Place , schema:PlayAction ;
	schema:rangeIncludes schema:Event ;
	rdfs:comment "Upcoming or past event associated with this place or organization." .

schema:events a rdf:Property ;
	rdfs:label "events" ;
	schema:domainIncludes schema:Organization , schema:Place ;
	schema:rangeIncludes schema:Event ;
	rdfs:comment "Upcoming or past events associated with this place or organization (legacy spelling; see singular form, event)." .

schema:evidenceLevel a rdf:Property ;
	rdfs:label "evidenceLevel" ;
	schema:domainIncludes schema:MedicalGuideline ;
	schema:rangeIncludes schema:MedicalEvidenceLevel ;
	rdfs:comment "Strength of evidence of the data used to formulate the guideline (enumerated)." .

schema:evidenceOrigin a rdf:Property ;
	rdfs:label "evidenceOrigin" ;
	schema:domainIncludes schema:MedicalGuideline ;
	schema:rangeIncludes schema:Text ;
	rdfs:comment "Source of the data used to formulate the guidance, e.g. RCT, consensus opinion, etc." .

schema:exercisePlan a rdf:Property ;
	rdfs:label "exercisePlan" ;
	schema:domainIncludes schema:ExerciseAction ;
	schema:rangeIncludes schema:ExercisePlan ;
	rdfs:comment "A sub property of instrument. The exercise plan used on this action." .

schema:exerciseType a rdf:Property ;
	rdfs:label "exerciseType" ;
	schema:domainIncludes schema:ExerciseAction , schema:ExercisePlan ;
	schema:rangeIncludes schema:Text ;
	rdfs:comment "Type(s) of exercise or activity, such as strength training, flexibility training, aerobics, cardiac rehabilitation, etc." .

schema:exifData a rdf:Property ;
	rdfs:label "exifData" ;
	schema:domainIncludes schema:ImageObject ;
	schema:rangeIncludes schema:Text ;
	rdfs:comment "exif data for this object." .

schema:expectedPrognosis a rdf:Property ;
	rdfs:label "expectedPrognosis" ;
	schema:domainIncludes schema:MedicalCondition ;
	schema:rangeIncludes schema:Text ;
	rdfs:comment "The likely outcome in either the short term or long term of the medical condition." .

schema:experienceRequirements a rdf:Property ;
	rdfs:label "experienceRequirements" ;
	schema:domainIncludes schema:JobPosting ;
	schema:rangeIncludes schema:Text ;
	rdfs:comment "Description of skills and experience needed for the position." .

schema:expertConsiderations a rdf:Property ;
	rdfs:label "expertConsiderations" ;
	schema:domainIncludes schema:Diet ;
	schema:rangeIncludes schema:Text ;
	rdfs:comment "Medical expert advice related to the plan." .

schema:expires a rdf:Property ;
	rdfs:label "expires" ;
	schema:domainIncludes schema:MediaObject ;
	schema:rangeIncludes schema:Date ;
	rdfs:comment "Date the content expires and is no longer useful or available. Useful for videos." .

schema:familyName a rdf:Property ;
	rdfs:label "familyName" ;
	schema:domainIncludes schema:Person ;
	schema:rangeIncludes schema:Text ;
	rdfs:comment "Family name. In the U.S., the last name of an Person. This can be used along with givenName instead of the Name property." .

schema:fatContent a rdf:Property ;
	rdfs:label "fatContent" ;
	schema:domainIncludes schema:NutritionInformation ;
	schema:rangeIncludes schema:Mass ;
	rdfs:comment "The number of grams of fat." .

schema:faxNumber a rdf:Property ;
	rdfs:label "faxNumber" ;
	schema:domainIncludes schema:ContactPoint , schema:Organization , schema:Person , schema:Place ;
	schema:rangeIncludes schema:Text ;
	rdfs:comment "The fax number." .

schema:featureList a rdf:Property ;
	rdfs:label "featureList" ;
	schema:domainIncludes schema:SoftwareApplication ;
	schema:rangeIncludes schema:Text , schema:URL ;
	rdfs:comment "Features or modules provided by this application (and possibly required by other applications)." .

schema:fiberContent a rdf:Property ;
	rdfs:label "fiberContent" ;
	schema:domainIncludes schema:NutritionInformation ;
	schema:rangeIncludes schema:Mass ;
	rdfs:comment "The number of grams of fiber." .

schema:fileFormat a rdf:Property ;
	rdfs:label "fileFormat" ;
	schema:domainIncludes schema:SoftwareApplication ;
	schema:rangeIncludes schema:Text ;
	rdfs:comment "MIME format of the binary (e.g. application/zip)." .

schema:fileSize a rdf:Property ;
	rdfs:label "fileSize" ;
	schema:domainIncludes schema:SoftwareApplication ;
	schema:rangeIncludes schema:Integer ;
	rdfs:comment "Size of the application / package (e.g. 18MB). In the absence of a unit (MB, KB etc.), KB will be assumed." .

schema:followee a rdf:Property ;
	rdfs:label "followee" ;
	schema:domainIncludes schema:FollowAction ;
	schema:rangeIncludes schema:Organization , schema:Person ;
	rdfs:comment "A sub property of object. The person or organization being followed." .

schema:follows a rdf:Property ;
	rdfs:label "follows" ;
	schema:domainIncludes schema:Person ;
	schema:rangeIncludes schema:Person ;
	rdfs:comment "The most generic uni-directional social relation." .

schema:followup a rdf:Property ;
	rdfs:label "followup" ;
	schema:domainIncludes schema:MedicalProcedure ;
	schema:rangeIncludes schema:Text ;
	rdfs:comment "Typical or recommended followup care after the procedure is performed." .

schema:foodEstablishment a rdf:Property ;
	rdfs:label "foodEstablishment" ;
	schema:domainIncludes schema:CookAction ;
	schema:rangeIncludes schema:FoodEstablishment , schema:Place ;
	rdfs:comment "A sub property of location. The specific food establishment where the action occurreed." .

schema:foodEvent a rdf:Property ;
	rdfs:label "foodEvent" ;
	schema:domainIncludes schema:CookAction ;
	schema:rangeIncludes schema:FoodEvent ;
	rdfs:comment "A sub property of location. The specific food event where the action occurred." .

schema:foodWarning a rdf:Property ;
	rdfs:label "foodWarning" ;
	schema:domainIncludes schema:Drug ;
	schema:rangeIncludes schema:Text ;
	rdfs:comment "Any precaution, guidance, contraindication, etc. related to consumption of specific foods while taking this drug." .

schema:founder a rdf:Property ;
	rdfs:label "founder" ;
	schema:domainIncludes schema:Organization ;
	schema:rangeIncludes schema:Person ;
	rdfs:comment "A person who founded this organization." .

schema:founders a rdf:Property ;
	rdfs:label "founders" ;
	schema:domainIncludes schema:Organization ;
	schema:rangeIncludes schema:Person ;
	rdfs:comment "A person who founded this organization (legacy spelling; see singular form, founder)." .

schema:foundingDate a rdf:Property ;
	rdfs:label "foundingDate" ;
	schema:domainIncludes schema:Organization ;
	schema:rangeIncludes schema:Date ;
	rdfs:comment "The date that this organization was founded." .

schema:frequency a rdf:Property ;
	rdfs:label "frequency" ;
	schema:domainIncludes schema:DoseSchedule ;
	schema:rangeIncludes schema:Text ;
	rdfs:comment "How often the dose is taken, e.g. 'daily'." .

schema:fromLocation a rdf:Property ;
	rdfs:label "fromLocation" ;
	schema:domainIncludes schema:ExerciseAction , schema:MoveAction , schema:TransferAction ;
	schema:rangeIncludes schema:Number , schema:Place ;
	rdfs:comment "A sub property of location. The original location of the object or the agent before the action." .

schema:function a rdf:Property ;
	rdfs:label "function" ;
	schema:domainIncludes schema:AnatomicalStructure ;
	schema:rangeIncludes schema:Text ;
	rdfs:comment "Function of the anatomical structure." .

schema:functionalClass a rdf:Property ;
	rdfs:label "functionalClass" ;
	schema:domainIncludes schema:Joint ;
	schema:rangeIncludes schema:Text ;
	rdfs:comment "The degree of mobility the joint allows." .

schema:gender a rdf:Property ;
	rdfs:label "gender" ;
	schema:domainIncludes schema:Person ;
	schema:rangeIncludes schema:Text ;
	rdfs:comment "Gender of the person." .

schema:genre a rdf:Property ;
	rdfs:label "genre" ;
	schema:domainIncludes schema:CreativeWork ;
	schema:rangeIncludes schema:Text ;
	rdfs:comment "Genre of the creative work" .

schema:geo a rdf:Property ;
	rdfs:label "geo" ;
	schema:domainIncludes schema:Place ;
	schema:rangeIncludes schema:GeoCoordinates , schema:GeoShape ;
	rdfs:comment "The geo coordinates of the place." .

schema:givenName a rdf:Property ;
	rdfs:label "givenName" ;
	schema:domainIncludes schema:Person ;
	schema:rangeIncludes schema:Text ;
	rdfs:comment "Given name. In the U.S., the first name of a Person. This can be used along with familyName instead of the Name property." .

schema:globalLocationNumber a rdf:Property ;
	rdfs:label "globalLocationNumber" ;
	schema:domainIncludes schema:Organization , schema:Person , schema:Place ;
	schema:rangeIncludes schema:Text ;
	rdfs:comment "The Global Location Number (GLN, sometimes also referred to as International Location Number or ILN) of the respective organization, person, or place. The GLN is a 13-digit number used to identify parties and physical locations." .

schema:greater a rdf:Property ;
	rdfs:label "greater" ;
	schema:domainIncludes schema:QualitativeValue ;
	schema:rangeIncludes schema:QualitativeValue ;
	rdfs:comment "This ordering relation for qualitative values indicates that the subject is greater than the object." .

schema:greaterOrEqual a rdf:Property ;
	rdfs:label "greaterOrEqual" ;
	schema:domainIncludes schema:QualitativeValue ;
	schema:rangeIncludes schema:QualitativeValue ;
	rdfs:comment "This ordering relation for qualitative values indicates that the subject is greater than or equal to the object." .

schema:gtin13 a rdf:Property ;
	rdfs:label "gtin13" ;
	schema:domainIncludes schema:Demand , schema:Offer , schema:Product ;
	schema:rangeIncludes schema:Text ;
	rdfs:comment "The GTIN-13 code of the product, or the product to which the offer refers. This is equivalent to 13-digit ISBN codes and EAN UCC-13. Former 12-digit UPC codes can be converted into a GTIN-13 code by simply adding a preceeding zero." .

schema:gtin14 a rdf:Property ;
	rdfs:label "gtin14" ;
	schema:domainIncludes schema:Demand , schema:Offer , schema:Product ;
	schema:rangeIncludes schema:Text ;
	rdfs:comment "The GTIN-14 code of the product, or the product to which the offer refers." .

schema:gtin8 a rdf:Property ;
	rdfs:label "gtin8" ;
	schema:domainIncludes schema:Demand , schema:Offer , schema:Product ;
	schema:rangeIncludes schema:Text ;
	rdfs:comment "The GTIN-8 code of the product, or the product to which the offer refers. This code is also known as EAN/UCC-8 or 8-digit EAN." .

schema:guideline a rdf:Property ;
	rdfs:label "guideline" ;
	schema:domainIncludes schema:MedicalEntity ;
	schema:rangeIncludes schema:MedicalGuideline ;
	rdfs:comment "A medical guideline related to this entity." .

schema:guidelineDate a rdf:Property ;
	rdfs:label "guidelineDate" ;
	schema:domainIncludes schema:MedicalGuideline ;
	schema:rangeIncludes schema:Date ;
	rdfs:comment "Date on which this guideline's recommendation was made." .

schema:guidelineSubject a rdf:Property ;
	rdfs:label "guidelineSubject" ;
	schema:domainIncludes schema:MedicalGuideline ;
	schema:rangeIncludes schema:MedicalEntity ;
	rdfs:comment "The medical conditions, treatments, etc. that are the subject of the guideline." .

schema:hasPOS a rdf:Property ;
	rdfs:label "hasPOS" ;
	schema:domainIncludes schema:Organization , schema:Person ;
	schema:rangeIncludes schema:Place ;
	rdfs:comment "Points-of-Sales operated by the organization or person." .

schema:headline a rdf:Property ;
	rdfs:label "headline" ;
	schema:domainIncludes schema:CreativeWork ;
	schema:rangeIncludes schema:Text ;
	rdfs:comment "Headline of the article" .

schema:healthCondition a rdf:Property ;
	rdfs:label "healthCondition" ;
	schema:domainIncludes schema:PeopleAudience ;
	schema:rangeIncludes schema:MedicalCondition ;
	rdfs:comment "Expectations for health conditions of target audience" .

schema:height a rdf:Property ;
	rdfs:label "height" ;
	schema:domainIncludes schema:MediaObject , schema:Product ;
	schema:rangeIncludes schema:Distance , schema:QuantitativeValue ;
	rdfs:comment "The height of the item." .

schema:highPrice a rdf:Property ;
	rdfs:label "highPrice" ;
	schema:domainIncludes schema:AggregateOffer ;
	schema:rangeIncludes schema:Number , schema:Text ;
	rdfs:comment "The highest price of all offers available." .

schema:hiringOrganization a rdf:Property ;
	rdfs:label "hiringOrganization" ;
	schema:domainIncludes schema:JobPosting ;
	schema:rangeIncludes schema:Organization ;
	rdfs:comment "Organization offering the job position." .

schema:homeLocation a rdf:Property ;
	rdfs:label "homeLocation" ;
	schema:domainIncludes schema:Person ;
	schema:rangeIncludes schema:ContactPoint , schema:Place ;
	rdfs:comment "A contact location for a person's residence." .

schema:honorificPrefix a rdf:Property ;
	rdfs:label "honorificPrefix" ;
	schema:domainIncludes schema:Person ;
	schema:rangeIncludes schema:Text ;
	rdfs:comment "An honorific prefix preceding a Person's name such as Dr/Mrs/Mr." .

schema:honorificSuffix a rdf:Property ;
	rdfs:label "honorificSuffix" ;
	schema:domainIncludes schema:Person ;
	schema:rangeIncludes schema:Text ;
	rdfs:comment "An honorific suffix preceding a Person's name such as M.D. /PhD/MSCSW." .

schema:hospitalAffiliation a rdf:Property ;
	rdfs:label "hospitalAffiliation" ;
	schema:domainIncludes schema:Physician ;
	schema:rangeIncludes schema:Hospital ;
	rdfs:comment "A hospital with which the physician or office is affiliated." .

schema:howPerformed a rdf:Property ;
	rdfs:label "howPerformed" ;
	schema:domainIncludes schema:MedicalProcedure ;
	schema:rangeIncludes schema:Text ;
	rdfs:comment "How the procedure is performed." .

schema:identifyingExam a rdf:Property ;
	rdfs:label "identifyingExam" ;
	schema:domainIncludes schema:MedicalSign ;
	schema:rangeIncludes schema:PhysicalExam ;
	rdfs:comment "A physical examination that can identify this sign." .

schema:identifyingTest a rdf:Property ;
	rdfs:label "identifyingTest" ;
	schema:domainIncludes schema:MedicalSign ;
	schema:rangeIncludes schema:MedicalTest ;
	rdfs:comment "A diagnostic test that can identify this sign." .

schema:illustrator a rdf:Property ;
	rdfs:label "illustrator" ;
	schema:domainIncludes schema:Book ;
	schema:rangeIncludes schema:Person ;
	rdfs:comment "The illustrator of the book." .

schema:image a rdf:Property ;
	rdfs:label "image" ;
	schema:domainIncludes schema:Thing ;
	schema:rangeIncludes schema:URL ;
	rdfs:comment "URL of an image of the item." .

schema:imagingTechnique a rdf:Property ;
	rdfs:label "imagingTechnique" ;
	schema:domainIncludes schema:ImagingTest ;
	schema:rangeIncludes schema:MedicalImagingTechnique ;
	rdfs:comment "Imaging technique used." .

schema:inAlbum a rdf:Property ;
	rdfs:label "inAlbum" ;
	schema:domainIncludes schema:MusicRecording ;
	schema:rangeIncludes schema:MusicAlbum ;
	rdfs:comment "The album to which this recording belongs." .

schema:inLanguage a rdf:Property ;
	rdfs:label "inLanguage" ;
	schema:domainIncludes schema:CreativeWork ;
	schema:rangeIncludes schema:Text ;
	rdfs:comment "The language of the content. please use one of the language codes from the <a href='http://tools.ietf.org/html/bcp47'>IETF BCP 47 standard.</a>" .

schema:inPlaylist a rdf:Property ;
	rdfs:label "inPlaylist" ;
	schema:domainIncludes schema:MusicRecording ;
	schema:rangeIncludes schema:MusicPlaylist ;
	rdfs:comment "The playlist to which this recording belongs." .

schema:incentives a rdf:Property ;
	rdfs:label "incentives" ;
	schema:domainIncludes schema:JobPosting ;
	schema:rangeIncludes schema:Text ;
	rdfs:comment "Description of bonus and commission compensation aspects of the job." .

schema:includedRiskFactor a rdf:Property ;
	rdfs:label "includedRiskFactor" ;
	schema:domainIncludes schema:MedicalRiskEstimator ;
	schema:rangeIncludes schema:MedicalRiskFactor ;
	rdfs:comment "A modifiable or non-modifiable risk factor included in the calculation, e.g. age, coexisting condition." .

schema:includesObject a rdf:Property ;
	rdfs:label "includesObject" ;
	schema:domainIncludes schema:Demand , schema:Offer ;
	schema:rangeIncludes schema:TypeAndQuantityNode ;
	rdfs:comment "This links to a node or nodes indicating the exact quantity of the products included in the offer." .

schema:increasesRiskOf a rdf:Property ;
	rdfs:label "increasesRiskOf" ;
	schema:domainIncludes schema:MedicalRiskFactor ;
	schema:rangeIncludes schema:MedicalEntity ;
	rdfs:comment "The condition, complication, etc. influenced by this factor." .

schema:indication a rdf:Property ;
	rdfs:label "indication" ;
	schema:domainIncludes schema:MedicalDevice , schema:MedicalTherapy ;
	schema:rangeIncludes schema:MedicalIndication ;
	rdfs:comment "A factor that indicates use of this therapy for treatment and/or prevention of a condition, symptom, etc. For therapies such as drugs, indications can include both officially-approved indications as well as off-label uses. These can be distinguished by using the ApprovedIndication subtype of MedicalIndication." .

schema:industry a rdf:Property ;
	rdfs:label "industry" ;
	schema:domainIncludes schema:JobPosting ;
	schema:rangeIncludes schema:Text ;
	rdfs:comment "The industry associated with the job position." .

schema:infectiousAgent a rdf:Property ;
	rdfs:label "infectiousAgent" ;
	schema:domainIncludes schema:InfectiousDisease ;
	schema:rangeIncludes schema:Text ;
	rdfs:comment "The actual infectious agent, such as a specific bacterium." .

schema:infectiousAgentClass a rdf:Property ;
	rdfs:label "infectiousAgentClass" ;
	schema:domainIncludes schema:InfectiousDisease ;
	schema:rangeIncludes schema:InfectiousAgentClass ;
	rdfs:comment "The class of infectious agent (bacteria, prion, etc.) that causes the disease." .

schema:ingredients a rdf:Property ;
	rdfs:label "ingredients" ;
	schema:domainIncludes schema:Recipe ;
	schema:rangeIncludes schema:Text ;
	rdfs:comment "An ingredient used in the recipe." .

schema:insertion a rdf:Property ;
	rdfs:label "insertion" ;
	schema:domainIncludes schema:Muscle ;
	schema:rangeIncludes schema:AnatomicalStructure ;
	rdfs:comment "The place of attachment of a muscle, or what the muscle moves." .

schema:installUrl a rdf:Property ;
	rdfs:label "installUrl" ;
	schema:domainIncludes schema:SoftwareApplication ;
	schema:rangeIncludes schema:URL ;
	rdfs:comment "URL at which the app may be installed, if different from the URL of the item." .

schema:instrument a rdf:Property ;
	rdfs:label "instrument" ;
	schema:domainIncludes schema:Action ;
	schema:rangeIncludes schema:Thing ;
	rdfs:comment "The object that helped the agent perform the action. e.g. John wrote a book with *a pen*." .

schema:intensity a rdf:Property ;
	rdfs:label "intensity" ;
	schema:domainIncludes schema:ExercisePlan ;
	schema:rangeIncludes schema:Text ;
	rdfs:comment "Quantitative measure gauging the degree of force involved in the exercise, for example, heartbeats per minute. May include the velocity of the movement." .

schema:interactingDrug a rdf:Property ;
	rdfs:label "interactingDrug" ;
	schema:domainIncludes schema:Drug ;
	schema:rangeIncludes schema:Drug ;
	rdfs:comment "Another drug that is known to interact with this drug in a way that impacts the effect of this drug or causes a risk to the patient. Note: disease interactions are typically captured as contraindications." .

schema:interactionCount a rdf:Property ;
	rdfs:label "interactionCount" ;
	schema:domainIncludes schema:CreativeWork , schema:MediaObject , schema:Organization , schema:Person , schema:Place ;
	schema:rangeIncludes schema:Text ;
	rdfs:comment "A count of a specific user interactions with this item&#x2014;for example, <code>20 UserLikes</code>, <code>5 UserComments</code>, or <code>300 UserDownloads</code>. The user interaction type should be one of the sub types of <a href='UserInteraction'>UserInteraction</a>." .

schema:interactivityType a rdf:Property ;
	rdfs:label "interactivityType" ;
	schema:domainIncludes schema:CreativeWork ;
	schema:rangeIncludes schema:Text ;
	rdfs:comment "The predominant mode of learning supported by the learning resource. Acceptable values are 'active', 'expositive', or 'mixed'." .

schema:inventoryLevel a rdf:Property ;
	rdfs:label "inventoryLevel" ;
	schema:domainIncludes schema:Demand , schema:Offer , schema:SomeProducts ;
	schema:rangeIncludes schema:QuantitativeValue ;
	rdfs:comment "The current approximate inventory level for the item or items." .

schema:isAccessoryOrSparePartFor a rdf:Property ;
	rdfs:label "isAccessoryOrSparePartFor" ;
	schema:domainIncludes schema:Product ;
	schema:rangeIncludes schema:Product ;
	rdfs:comment "A pointer to another product (or multiple products) for which this product is an accessory or spare part." .

schema:isAvailableGenerically a rdf:Property ;
	rdfs:label "isAvailableGenerically" ;
	schema:domainIncludes schema:Drug ;
	schema:rangeIncludes schema:Boolean ;
	rdfs:comment "True if the drug is available in a generic form (regardless of name)." .

schema:isBasedOnUrl a rdf:Property ;
	rdfs:label "isBasedOnUrl" ;
	schema:domainIncludes schema:CreativeWork ;
	schema:rangeIncludes schema:URL ;
	rdfs:comment "A resource that was used in the creation of this resource. This term can be repeated for multiple sources. For example, http://example.com/great-multiplication-intro.html" .

schema:isConsumableFor a rdf:Property ;
	rdfs:label "isConsumableFor" ;
	schema:domainIncludes schema:Product ;
	schema:rangeIncludes schema:Product ;
	rdfs:comment "A pointer to another product (or multiple products) for which this product is a consumable." .

schema:isFamilyFriendly a rdf:Property ;
	rdfs:label "isFamilyFriendly" ;
	schema:domainIncludes schema:CreativeWork ;
	schema:rangeIncludes schema:Boolean ;
	rdfs:comment "Indicates whether this content is family friendly." .

schema:isPartOf a rdf:Property ;
	rdfs:label "isPartOf" ;
	schema:domainIncludes schema:WebPage ;
	schema:rangeIncludes schema:CollectionPage ;
	rdfs:comment "Indicates the collection or gallery to which the item belongs." .

schema:isProprietary a rdf:Property ;
	rdfs:label "isProprietary" ;
	schema:domainIncludes schema:DietarySupplement , schema:Drug ;
	schema:rangeIncludes schema:Boolean ;
	rdfs:comment "True if this item's name is a proprietary/brand name (vs. generic name)." .

schema:isRelatedTo a rdf:Property ;
	rdfs:label "isRelatedTo" ;
	schema:domainIncludes schema:Product ;
	schema:rangeIncludes schema:Product ;
	rdfs:comment "A pointer to another, somehow related product (or multiple products)." .

schema:isSimilarTo a rdf:Property ;
	rdfs:label "isSimilarTo" ;
	schema:domainIncludes schema:Product ;
	schema:rangeIncludes schema:Product ;
	rdfs:comment "A pointer to another, functionally similar product (or multiple products)." .

schema:isVariantOf a rdf:Property ;
	rdfs:label "isVariantOf" ;
	schema:domainIncludes schema:ProductModel ;
	schema:rangeIncludes schema:ProductModel ;
	rdfs:comment "A pointer to a base product from which this product is a variant. It is safe to infer that the variant inherits all product features from the base model, unless defined locally. This is not transitive." .

schema:isbn a rdf:Property ;
	rdfs:label "isbn" ;
	schema:domainIncludes schema:Book ;
	schema:rangeIncludes schema:Text ;
	rdfs:comment "The ISBN of the book." .

schema:isicV4 a rdf:Property ;
	rdfs:label "isicV4" ;
	schema:domainIncludes schema:Organization , schema:Person , schema:Place ;
	schema:rangeIncludes schema:Text ;
	rdfs:comment "The International Standard of Industrial Classification of All Economic Activities (ISIC), Revision 4 code for a particular organization, business person, or place." .

schema:itemCondition a rdf:Property ;
	rdfs:label "itemCondition" ;
	schema:domainIncludes schema:Demand , schema:Offer , schema:Product ;
	schema:rangeIncludes schema:OfferItemCondition ;
	rdfs:comment "A predefined value from OfferItemCondition or a textual description of the condition of the product or service, or the products or services included in the offer." .

schema:itemListElement a rdf:Property ;
	rdfs:label "itemListElement" ;
	schema:domainIncludes schema:ItemList ;
	schema:rangeIncludes schema:Text ;
	rdfs:comment "A single list item." .

schema:itemListOrder a rdf:Property ;
	rdfs:label "itemListOrder" ;
	schema:domainIncludes schema:ItemList ;
	schema:rangeIncludes schema:Text ;
	rdfs:comment "Type of ordering (e.g. Ascending, Descending, Unordered)." .

schema:itemOffered a rdf:Property ;
	rdfs:label "itemOffered" ;
	schema:domainIncludes schema:Demand , schema:Offer ;
	schema:rangeIncludes schema:Product ;
	rdfs:comment "The item being sold." .

schema:itemReviewed a rdf:Property ;
	rdfs:label "itemReviewed" ;
	schema:domainIncludes schema:AggregateRating , schema:Review ;
	schema:rangeIncludes schema:Thing ;
	rdfs:comment "The item that is being reviewed/rated." .

schema:jobLocation a rdf:Property ;
	rdfs:label "jobLocation" ;
	schema:domainIncludes schema:JobPosting ;
	schema:rangeIncludes schema:Place ;
	rdfs:comment "A (typically single) geographic location associated with the job position." .

schema:jobTitle a rdf:Property ;
	rdfs:label "jobTitle" ;
	schema:domainIncludes schema:Person ;
	schema:rangeIncludes schema:Text ;
	rdfs:comment "The job title of the person (for example, Financial Manager)." .

schema:keywords a rdf:Property ;
	rdfs:label "keywords" ;
	schema:domainIncludes schema:CreativeWork ;
	schema:rangeIncludes schema:Text ;
	rdfs:comment "The keywords/tags used to describe this content." .

schema:knows a rdf:Property ;
	rdfs:label "knows" ;
	schema:domainIncludes schema:Person ;
	schema:rangeIncludes schema:Person ;
	rdfs:comment "The most generic bi-directional social/work relation." .

schema:labelDetails a rdf:Property ;
	rdfs:label "labelDetails" ;
	schema:domainIncludes schema:Drug ;
	schema:rangeIncludes schema:URL ;
	rdfs:comment "Link to the drug's label details." .

schema:landlord a rdf:Property ;
	rdfs:label "landlord" ;
	schema:domainIncludes schema:RentAction ;
	schema:rangeIncludes schema:Organization , schema:Person ;
	rdfs:comment "A sub property of participant. The owner of the real estate property. Sub property of destination or participant?" .

schema:language a rdf:Property ;
	rdfs:label "language" ;
	schema:domainIncludes schema:CommunicateAction , schema:WriteAction ;
	schema:rangeIncludes schema:Language ;
	rdfs:comment "A sub property of instrument. The languaged used on this action." .

schema:lastReviewed a rdf:Property ;
	rdfs:label "lastReviewed" ;
	schema:domainIncludes schema:WebPage ;
	schema:rangeIncludes schema:Date ;
	rdfs:comment "Date on which the content on this web page was last reviewed for accuracy and/or completeness." .

schema:latitude a rdf:Property ;
	rdfs:label "latitude" ;
	schema:domainIncludes schema:GeoCoordinates ;
	schema:rangeIncludes schema:Number , schema:Text ;
	rdfs:comment "The latitude of a location. For example <code>37.42242</code>." .

schema:learningResourceType a rdf:Property ;
	rdfs:label "learningResourceType" ;
	schema:domainIncludes schema:CreativeWork ;
	schema:rangeIncludes schema:Text ;
	rdfs:comment "The predominant type or kind characterizing the learning resource. For example, 'presentation', 'handout'." .

schema:legalName a rdf:Property ;
	rdfs:label "legalName" ;
	schema:domainIncludes schema:Organization ;
	schema:rangeIncludes schema:Text ;
	rdfs:comment "The official name of the organization, e.g. the registered company name." .

schema:legalStatus a rdf:Property ;
	rdfs:label "legalStatus" ;
	schema:domainIncludes schema:DietarySupplement , schema:Drug ;
	schema:rangeIncludes schema:DrugLegalStatus ;
	rdfs:comment "The drug or supplement's legal status, including any controlled substance schedules that apply." .

schema:lender a rdf:Property ;
	rdfs:label "lender" ;
	schema:domainIncludes schema:BorrowAction ;
	schema:rangeIncludes schema:Person ;
	rdfs:comment "A sub property of participant. The person that lends the object being borrowed." .

schema:lesser a rdf:Property ;
	rdfs:label "lesser" ;
	schema:domainIncludes schema:QualitativeValue ;
	schema:rangeIncludes schema:QualitativeValue ;
	rdfs:comment "This ordering relation for qualitative values indicates that the subject is lesser than the object." .

schema:lesserOrEqual a rdf:Property ;
	rdfs:label "lesserOrEqual" ;
	schema:domainIncludes schema:QualitativeValue ;
	schema:rangeIncludes schema:QualitativeValue ;
	rdfs:comment "This ordering relation for qualitative values indicates that the subject is lesser than or equal to the object." .

schema:line a rdf:Property ;
	rdfs:label "line" ;
	schema:domainIncludes schema:GeoShape ;
	schema:rangeIncludes schema:Text ;
	rdfs:comment "A line is a point-to-point path consisting of two or more points. A line is expressed as a series of two or more point objects separated by space." .

schema:location a rdf:Property ;
	rdfs:label "location" ;
	schema:domainIncludes schema:Action , schema:Event , schema:Organization ;
	schema:rangeIncludes schema:Place , schema:PostalAddress ;
	rdfs:comment "The location of the event, organization or action." .

schema:logo a rdf:Property ;
	rdfs:label "logo" ;
	schema:domainIncludes schema:Brand , schema:Organization , schema:Place , schema:Product ;
	schema:rangeIncludes schema:ImageObject , schema:URL ;
	rdfs:comment "URL of an image for the logo of the item." .

schema:longitude a rdf:Property ;
	rdfs:label "longitude" ;
	schema:domainIncludes schema:GeoCoordinates ;
	schema:rangeIncludes schema:Number , schema:Text ;
	rdfs:comment "The longitude of a location. For example <code>-122.08585</code>." .

schema:loser a rdf:Property ;
	rdfs:label "loser" ;
	schema:domainIncludes schema:WinAction ;
	schema:rangeIncludes schema:Person ;
	rdfs:comment "A sub property of participant. The loser of the action." .

schema:lowPrice a rdf:Property ;
	rdfs:label "lowPrice" ;
	schema:domainIncludes schema:AggregateOffer ;
	schema:rangeIncludes schema:Number , schema:Text ;
	rdfs:comment "The lowest price of all offers available." .

schema:mainContentOfPage a rdf:Property ;
	rdfs:label "mainContentOfPage" ;
	schema:domainIncludes schema:WebPage ;
	schema:rangeIncludes schema:WebPageElement ;
	rdfs:comment "Indicates if this web page element is the main subject of the page." .

schema:makesOffer a rdf:Property ;
	rdfs:label "makesOffer" ;
	schema:domainIncludes schema:Organization , schema:Person ;
	schema:rangeIncludes schema:Offer ;
	rdfs:comment "A pointer to products or services offered by the organization or person." .

schema:manufacturer a rdf:Property ;
	rdfs:label "manufacturer" ;
	schema:domainIncludes schema:DietarySupplement , schema:Drug , schema:Product ;
	schema:rangeIncludes schema:Organization ;
	rdfs:comment "The manufacturer of the product." .

schema:map a rdf:Property ;
	rdfs:label "map" ;
	schema:domainIncludes schema:Place ;
	schema:rangeIncludes schema:URL ;
	rdfs:comment "A URL to a map of the place." .

schema:maps a rdf:Property ;
	rdfs:label "maps" ;
	schema:domainIncludes schema:Place ;
	schema:rangeIncludes schema:URL ;
	rdfs:comment "A URL to a map of the place (legacy spelling; see singular form, map)." .

schema:maxPrice a rdf:Property ;
	rdfs:label "maxPrice" ;
	schema:domainIncludes schema:PriceSpecification ;
	schema:rangeIncludes schema:Number ;
	rdfs:comment "The highest price if the price is a range." .

schema:maxValue a rdf:Property ;
	rdfs:label "maxValue" ;
	schema:domainIncludes schema:QuantitativeValue ;
	schema:rangeIncludes schema:Number ;
	rdfs:comment "The upper of the product characteristic." .

schema:maximumIntake a rdf:Property ;
	rdfs:label "maximumIntake" ;
	schema:domainIncludes schema:DietarySupplement ;
	schema:rangeIncludes schema:MaximumDoseSchedule ;
	rdfs:comment "Recommended intake of this supplement for a given population as defined by a specific recommending authority." .

schema:mechanismOfAction a rdf:Property ;
	rdfs:label "mechanismOfAction" ;
	schema:domainIncludes schema:DietarySupplement , schema:Drug ;
	schema:rangeIncludes schema:Text ;
	rdfs:comment "The specific biochemical interaction through which this drug or supplement produces its pharmacological effect." .

schema:medicalSpecialty a rdf:Property ;
	rdfs:label "medicalSpecialty" ;
	schema:domainIncludes schema:Hospital , schema:MedicalClinic , schema:Physician ;
	schema:rangeIncludes schema:MedicalSpecialty ;
	rdfs:comment "A medical specialty of the provider." .

schema:medicineSystem a rdf:Property ;
	rdfs:label "medicineSystem" ;
	schema:domainIncludes schema:MedicalEntity ;
	schema:rangeIncludes schema:MedicineSystem ;
	rdfs:comment "The system of medicine that includes this MedicalEntity, for example 'evidence-based', 'homeopathic', 'chiropractic', etc." .

schema:member a rdf:Property ;
	rdfs:label "member" ;
	schema:domainIncludes schema:Organization ;
	schema:rangeIncludes schema:Organization , schema:Person ;
	rdfs:comment "A member of this organization." .

schema:memberOf a rdf:Property ;
	rdfs:label "memberOf" ;
	schema:domainIncludes schema:Person ;
	schema:rangeIncludes schema:Organization ;
	rdfs:comment "An organization to which the person belongs." .

schema:members a rdf:Property ;
	rdfs:label "members" ;
	schema:domainIncludes schema:Organization ;
	schema:rangeIncludes schema:Organization , schema:Person ;
	rdfs:comment "A member of this organization (legacy spelling; see singular form, member)." .

schema:memoryRequirements a rdf:Property ;
	rdfs:label "memoryRequirements" ;
	schema:domainIncludes schema:SoftwareApplication ;
	schema:rangeIncludes schema:Text , schema:URL ;
	rdfs:comment "Minimum memory requirements." .

schema:mentions a rdf:Property ;
	rdfs:label "mentions" ;
	schema:domainIncludes schema:CreativeWork ;
	schema:rangeIncludes schema:Thing ;
	rdfs:comment "Indicates that the CreativeWork contains a reference to, but is not necessarily about a concept." .

schema:menu a rdf:Property ;
	rdfs:label "menu" ;
	schema:domainIncludes schema:FoodEstablishment ;
	schema:rangeIncludes schema:Text , schema:URL ;
	rdfs:comment "Either the actual menu or a URL of the menu." .

schema:minPrice a rdf:Property ;
	rdfs:label "minPrice" ;
	schema:domainIncludes schema:PriceSpecification ;
	schema:rangeIncludes schema:Number ;
	rdfs:comment "The lowest price if the price is a range." .

schema:minValue a rdf:Property ;
	rdfs:label "minValue" ;
	schema:domainIncludes schema:QuantitativeValue ;
	schema:rangeIncludes schema:Number ;
	rdfs:comment "The lower value of the product characteristic." .

schema:model a rdf:Property ;
	rdfs:label "model" ;
	schema:domainIncludes schema:Product ;
	schema:rangeIncludes schema:ProductModel , schema:Text ;
	rdfs:comment "The model of the product. Use with the URL of a ProductModel or a textual representation of the model identifier. The URL of the ProductModel can be from an external source. It is recommended to additionally provide strong product identifiers via the gtin8/gtin13/gtin14 and mpn properties." .

schema:mpn a rdf:Property ;
	rdfs:label "mpn" ;
	schema:domainIncludes schema:Demand , schema:Offer , schema:Product ;
	schema:rangeIncludes schema:Text ;
	rdfs:comment "The Manufacturer Part Number (MPN) of the product, or the product to which the offer refers." .

schema:musicBy a rdf:Property ;
	rdfs:label "musicBy" ;
	schema:domainIncludes schema:Movie , schema:TVEpisode , schema:TVSeries ;
	schema:rangeIncludes schema:MusicGroup , schema:Person ;
	rdfs:comment "The composer of the movie or TV soundtrack." .

schema:musicGroupMember a rdf:Property ;
	rdfs:label "musicGroupMember" ;
	schema:domainIncludes schema:MusicGroup ;
	schema:rangeIncludes schema:Person ;
	rdfs:comment "A member of the music group&#x2014;for example, John, Paul, George, or Ringo." .

schema:naics a rdf:Property ;
	rdfs:label "naics" ;
	schema:domainIncludes schema:Organization , schema:Person ;
	schema:rangeIncludes schema:Text ;
	rdfs:comment "The North American Industry Classification System (NAICS) code for a particular organization or business person." .

schema:name a rdf:Property ;
	rdfs:label "name" ;
	schema:domainIncludes schema:Thing ;
	schema:rangeIncludes schema:Text ;
	rdfs:comment "The name of the item." .

schema:nationality a rdf:Property ;
	rdfs:label "nationality" ;
	schema:domainIncludes schema:Person ;
	schema:rangeIncludes schema:Country ;
	rdfs:comment "Nationality of the person." .

schema:naturalProgression a rdf:Property ;
	rdfs:label "naturalProgression" ;
	schema:domainIncludes schema:MedicalCondition ;
	schema:rangeIncludes schema:Text ;
	rdfs:comment "The expected progression of the condition if it is not treated and allowed to progress naturally." .

schema:nerve a rdf:Property ;
	rdfs:label "nerve" ;
	schema:domainIncludes schema:Muscle ;
	schema:rangeIncludes schema:Nerve ;
	rdfs:comment "The underlying innervation associated with the muscle." .

schema:nerveMotor a rdf:Property ;
	rdfs:label "nerveMotor" ;
	schema:domainIncludes schema:Nerve ;
	schema:rangeIncludes schema:Muscle ;
	rdfs:comment "The neurological pathway extension that involves muscle control." .

schema:nonEqual a rdf:Property ;
	rdfs:label "nonEqual" ;
	schema:domainIncludes schema:QualitativeValue ;
	schema:rangeIncludes schema:QualitativeValue ;
	rdfs:comment "This ordering relation for qualitative values indicates that the subject is not equal to the object." .

schema:nonProprietaryName a rdf:Property ;
	rdfs:label "nonProprietaryName" ;
	schema:domainIncludes schema:DietarySupplement , schema:Drug ;
	schema:rangeIncludes schema:Text ;
	rdfs:comment "The generic name of this drug or supplement." .

schema:normalRange a rdf:Property ;
	rdfs:label "normalRange" ;
	schema:domainIncludes schema:MedicalTest ;
	schema:rangeIncludes schema:Text ;
	rdfs:comment "Range of acceptable values for a typical patient, when applicable." .

schema:numTracks a rdf:Property ;
	rdfs:label "numTracks" ;
	schema:domainIncludes schema:MusicPlaylist ;
	schema:rangeIncludes schema:Integer ;
	rdfs:comment "The number of tracks in this album or playlist." .

schema:numberOfEpisodes a rdf:Property ;
	rdfs:label "numberOfEpisodes" ;
	schema:domainIncludes schema:TVSeason , schema:TVSeries ;
	schema:rangeIncludes schema:Number ;
	rdfs:comment "The number of episodes in this season or series." .

schema:numberOfPages a rdf:Property ;
	rdfs:label "numberOfPages" ;
	schema:domainIncludes schema:Book ;
	schema:rangeIncludes schema:Integer ;
	rdfs:comment "The number of pages in the book." .

schema:nutrition a rdf:Property ;
	rdfs:label "nutrition" ;
	schema:domainIncludes schema:Recipe ;
	schema:rangeIncludes schema:NutritionInformation ;
	rdfs:comment "Nutrition information about the recipe." .

schema:object a rdf:Property ;
	rdfs:label "object" ;
	schema:domainIncludes schema:Action ;
	schema:rangeIncludes schema:Thing ;
	rdfs:comment "The object upon the action is carried out, whose state is kept intact or changed. Also known as the semantic roles patient, affected or undergoer (which change their state) or theme (which doesn't). e.g. John read *a book*." .

schema:occupationalCategory a rdf:Property ;
	rdfs:label "occupationalCategory" ;
	schema:domainIncludes schema:JobPosting ;
	schema:rangeIncludes schema:Text ;
	rdfs:comment "Category or categories describing the job. Use BLS O*NET-SOC taxonomy: http://www.onetcenter.org/taxonomy.html. Ideally includes textual label and formal code, with the property repeated for each applicable value." .

schema:offerCount a rdf:Property ;
	rdfs:label "offerCount" ;
	schema:domainIncludes schema:AggregateOffer ;
	schema:rangeIncludes schema:Integer ;
	rdfs:comment "The number of offers for the product." .

schema:offers a rdf:Property ;
	rdfs:label "offers" ;
	schema:domainIncludes schema:CreativeWork , schema:Event , schema:MediaObject , schema:Product ;
	schema:rangeIncludes schema:Offer ;
	rdfs:comment "An offer to sell this item&#x2014;for example, an offer to sell a product, the DVD of a movie, or tickets to an event." .

schema:openingHours a rdf:Property ;
	rdfs:label "openingHours" ;
	schema:domainIncludes schema:CivicStructure , schema:LocalBusiness ;
	schema:rangeIncludes schema:Duration ;
	rdfs:comment "The opening hours for a business. Opening hours can be specified as a weekly time range, starting with days, then times per day. Multiple days can be listed with commas ',' separating each day. Day or time ranges are specified using a hyphen '-'.<br />- Days are specified using the following two-letter combinations: <code>Mo</code>, <code>Tu</code>, <code>We</code>, <code>Th</code>, <code>Fr</code>, <code>Sa</code>, <code>Su</code>.<br />- Times are specified using 24:00 time. For example, 3pm is specified as <code>15:00</code>. <br />- Here is an example: <code>&lt;time itemprop=&quot;openingHours&quot; datetime=&quot;Tu,Th 16:00-20:00&quot;&gt;Tuesdays and Thursdays 4-8pm&lt;/time&gt;</code>. <br />- If a business is open 7 days a week, then it can be specified as <code>&lt;time itemprop=&quot;openingHours&quot; datetime=&quot;Mo-Su&quot;&gt;Monday through Sunday, all day&lt;/time&gt;</code>." .

schema:openingHoursSpecification a rdf:Property ;
	rdfs:label "openingHoursSpecification" ;
	schema:domainIncludes schema:Place ;
	schema:rangeIncludes schema:OpeningHoursSpecification ;
	rdfs:comment "The opening hours of a certain place." .

schema:opens a rdf:Property ;
	rdfs:label "opens" ;
	schema:domainIncludes schema:OpeningHoursSpecification ;
	schema:rangeIncludes schema:Time ;
	rdfs:comment "The opening hour of the place or service on the given day(s) of the week." .

schema:operatingSystem a rdf:Property ;
	rdfs:label "operatingSystem" ;
	schema:domainIncludes schema:SoftwareApplication ;
	schema:rangeIncludes schema:Text ;
	rdfs:comment "Operating systems supported (Windows 7, OSX 10.6, Android 1.6)." .

schema:oponent a rdf:Property ;
	rdfs:label "oponent" ;
	schema:domainIncludes schema:ExerciseAction ;
	schema:rangeIncludes schema:Person ;
	rdfs:comment "A sub property of participant. The oponent on this action." .

schema:option a rdf:Property ;
	rdfs:label "option" ;
	schema:domainIncludes schema:ChooseAction ;
	schema:rangeIncludes schema:Text , schema:Thing ;
	rdfs:comment "A sub property of object. The options subject to this action." .

schema:origin a rdf:Property ;
	rdfs:label "origin" ;
	schema:domainIncludes schema:Muscle ;
	schema:rangeIncludes schema:AnatomicalStructure ;
	rdfs:comment "The place or point where a muscle arises." .

schema:originatesFrom a rdf:Property ;
	rdfs:label "originatesFrom" ;
	schema:domainIncludes schema:LymphaticVessel ;
	schema:rangeIncludes schema:Vessel ;
	rdfs:comment "The vasculature the lymphatic structure originates, or afferents, from." .

schema:outcome a rdf:Property ;
	rdfs:label "outcome" ;
	schema:domainIncludes schema:MedicalStudy ;
	schema:rangeIncludes schema:Text ;
	rdfs:comment "Expected or actual outcomes of the study." .

schema:overdosage a rdf:Property ;
	rdfs:label "overdosage" ;
	schema:domainIncludes schema:Drug ;
	schema:rangeIncludes schema:Text ;
	rdfs:comment "Any information related to overdose on a drug, including signs or symptoms, treatments, contact information for emergency response." .

schema:overview a rdf:Property ;
	rdfs:label "overview" ;
	schema:domainIncludes schema:Diet ;
	schema:rangeIncludes schema:Text ;
	rdfs:comment "Descriptive information establishing the overarching theory/philosophy of the plan. May include the rationale for the name, the population where the plan first came to prominence, etc." .

schema:ownedFrom a rdf:Property ;
	rdfs:label "ownedFrom" ;
	schema:domainIncludes schema:OwnershipInfo ;
	schema:rangeIncludes schema:DateTime ;
	rdfs:comment "The date and time of obtaining the product." .

schema:ownedThrough a rdf:Property ;
	rdfs:label "ownedThrough" ;
	schema:domainIncludes schema:OwnershipInfo ;
	schema:rangeIncludes schema:DateTime ;
	rdfs:comment "The date and time of giving up ownership on the product." .

schema:owns a rdf:Property ;
	rdfs:label "owns" ;
	schema:domainIncludes schema:Organization , schema:Person ;
	schema:rangeIncludes schema:OwnershipInfo , schema:Product ;
	rdfs:comment "Products owned by the organization or person." .

schema:parent a rdf:Property ;
	rdfs:label "parent" ;
	schema:domainIncludes schema:Person ;
	schema:rangeIncludes schema:Person ;
	rdfs:comment "A parent of this person." .

schema:parents a rdf:Property ;
	rdfs:label "parents" ;
	schema:domainIncludes schema:Person ;
	schema:rangeIncludes schema:Person ;
	rdfs:comment "A parents of the person (legacy spelling; see singular form, parent)." .

schema:partOfSeason a rdf:Property ;
	rdfs:label "partOfSeason" ;
	schema:domainIncludes schema:TVEpisode ;
	schema:rangeIncludes schema:TVSeason ;
	rdfs:comment "The season to which this episode belongs." .

schema:partOfSystem a rdf:Property ;
	rdfs:label "partOfSystem" ;
	schema:domainIncludes schema:AnatomicalStructure ;
	schema:rangeIncludes schema:AnatomicalSystem ;
	rdfs:comment "The anatomical or organ system that this structure is part of." .

schema:partOfTVSeries a rdf:Property ;
	rdfs:label "partOfTVSeries" ;
	schema:domainIncludes schema:TVEpisode , schema:TVSeason ;
	schema:rangeIncludes schema:TVSeries ;
	rdfs:comment "The TV series to which this episode or season belongs." .

schema:participant a rdf:Property ;
	rdfs:label "participant" ;
	schema:domainIncludes schema:Action ;
	schema:rangeIncludes schema:Organization , schema:Person ;
	rdfs:comment "Other co-agents that participated in the action indirectly. e.g. John wrote a book with *Steve*." .

schema:pathophysiology a rdf:Property ;
	rdfs:label "pathophysiology" ;
	schema:domainIncludes schema:MedicalCondition , schema:PhysicalActivity ;
	schema:rangeIncludes schema:Text ;
	rdfs:comment "Changes in the normal mechanical, physical, and biochemical functions that are associated with this activity or condition." .

schema:paymentAccepted a rdf:Property ;
	rdfs:label "paymentAccepted" ;
	schema:domainIncludes schema:LocalBusiness ;
	schema:rangeIncludes schema:Text ;
	rdfs:comment "Cash, credit card, etc." .

schema:performer a rdf:Property ;
	rdfs:label "performer" ;
	schema:domainIncludes schema:Event ;
	schema:rangeIncludes schema:Organization , schema:Person ;
	rdfs:comment "A performer at the event&#x2014;for example, a presenter, musician, musical group or actor." .

schema:performerIn a rdf:Property ;
	rdfs:label "performerIn" ;
	schema:domainIncludes schema:Person ;
	schema:rangeIncludes schema:Event ;
	rdfs:comment "Event that this person is a performer or participant in." .

schema:performers a rdf:Property ;
	rdfs:label "performers" ;
	schema:domainIncludes schema:Event ;
	schema:rangeIncludes schema:Organization , schema:Person ;
	rdfs:comment "The main performer or performers of the event&#x2014;for example, a presenter, musician, or actor (legacy spelling; see singular form, performer)." .

schema:permissions a rdf:Property ;
	rdfs:label "permissions" ;
	schema:domainIncludes schema:SoftwareApplication ;
	schema:rangeIncludes schema:Text ;
	rdfs:comment "Permission(s) required to run the app (for example, a mobile app may require full internet access or may run only on wifi)." .

schema:phase a rdf:Property ;
	rdfs:label "phase" ;
	schema:domainIncludes schema:MedicalTrial ;
	schema:rangeIncludes schema:Text ;
	rdfs:comment "The phase of the trial." .

schema:photo a rdf:Property ;
	rdfs:label "photo" ;
	schema:domainIncludes schema:Place ;
	schema:rangeIncludes schema:ImageObject , schema:Photograph ;
	rdfs:comment "A photograph of this place." .

schema:photos a rdf:Property ;
	rdfs:label "photos" ;
	schema:domainIncludes schema:Place ;
	schema:rangeIncludes schema:ImageObject , schema:Photograph ;
	rdfs:comment "Photographs of this place (legacy spelling; see singular form, photo)." .

schema:physiologicalBenefits a rdf:Property ;
	rdfs:label "physiologicalBenefits" ;
	schema:domainIncludes schema:Diet ;
	schema:rangeIncludes schema:Text ;
	rdfs:comment "Specific physiologic benefits associated to the plan." .

schema:playerType a rdf:Property ;
	rdfs:label "playerType" ;
	schema:domainIncludes schema:MediaObject ;
	schema:rangeIncludes schema:Text ;
	rdfs:comment "Player type required&#x2014;for example, Flash or Silverlight." .

schema:polygon a rdf:Property ;
	rdfs:label "polygon" ;
	schema:domainIncludes schema:GeoShape ;
	schema:rangeIncludes schema:Text ;
	rdfs:comment "A polygon is the area enclosed by a point-to-point path for which the starting and ending points are the same. A polygon is expressed as a series of four or more spacedelimited points where the first and final points are identical." .

schema:population a rdf:Property ;
	rdfs:label "population" ;
	schema:domainIncludes schema:MedicalStudy ;
	schema:rangeIncludes schema:Text ;
	rdfs:comment "Any characteristics of the population used in the study, e.g. 'males under 65'." .

schema:possibleComplication a rdf:Property ;
	rdfs:label "possibleComplication" ;
	schema:domainIncludes schema:MedicalCondition ;
	schema:rangeIncludes schema:Text ;
	rdfs:comment "A possible unexpected and unfavorable evolution of a medical condition. Complications may include worsening of the signs or symptoms of the disease, extension of the condition to other organ systems, etc." .

schema:possibleTreatment a rdf:Property ;
	rdfs:label "possibleTreatment" ;
	schema:domainIncludes schema:MedicalCondition , schema:MedicalSignOrSymptom ;
	schema:rangeIncludes schema:MedicalTherapy ;
	rdfs:comment "A possible treatment to address this condition, sign or symptom." .

schema:postOfficeBoxNumber a rdf:Property ;
	rdfs:label "postOfficeBoxNumber" ;
	schema:domainIncludes schema:PostalAddress ;
	schema:rangeIncludes schema:Text ;
	rdfs:comment "The post offce box number for PO box addresses." .

schema:postOp a rdf:Property ;
	rdfs:label "postOp" ;
	schema:domainIncludes schema:MedicalDevice ;
	schema:rangeIncludes schema:Text ;
	rdfs:comment "A description of the postoperative procedures, care, and/or followups for this device." .

schema:postalCode a rdf:Property ;
	rdfs:label "postalCode" ;
	schema:domainIncludes schema:PostalAddress ;
	schema:rangeIncludes schema:Text ;
	rdfs:comment "The postal code. For example, 94043." .

schema:preOp a rdf:Property ;
	rdfs:label "preOp" ;
	schema:domainIncludes schema:MedicalDevice ;
	schema:rangeIncludes schema:Text ;
	rdfs:comment "A description of the workup, testing, and other preparations required before implanting this device." .

schema:predecessorOf a rdf:Property ;
	rdfs:label "predecessorOf" ;
	schema:domainIncludes schema:ProductModel ;
	schema:rangeIncludes schema:ProductModel ;
	rdfs:comment "A pointer from a previous, often discontinued variant of the product to its newer variant." .

schema:pregnancyCategory a rdf:Property ;
	rdfs:label "pregnancyCategory" ;
	schema:domainIncludes schema:Drug ;
	schema:rangeIncludes schema:DrugPregnancyCategory ;
	rdfs:comment "Pregnancy category of this drug." .

schema:pregnancyWarning a rdf:Property ;
	rdfs:label "pregnancyWarning" ;
	schema:domainIncludes schema:Drug ;
	schema:rangeIncludes schema:Text ;
	rdfs:comment "Any precaution, guidance, contraindication, etc. related to this drug's use during pregnancy." .

schema:prepTime a rdf:Property ;
	rdfs:label "prepTime" ;
	schema:domainIncludes schema:Recipe ;
	schema:rangeIncludes schema:Duration ;
	rdfs:comment "The length of time it takes to prepare the recipe, in <a href='http://en.wikipedia.org/wiki/ISO_8601'>ISO 8601 duration format</a>." .

schema:preparation a rdf:Property ;
	rdfs:label "preparation" ;
	schema:domainIncludes schema:MedicalProcedure ;
	schema:rangeIncludes schema:Text ;
	rdfs:comment "Typical preparation that a patient must undergo before having the procedure performed." .

schema:prescribingInfo a rdf:Property ;
	rdfs:label "prescribingInfo" ;
	schema:domainIncludes schema:Drug ;
	schema:rangeIncludes schema:URL ;
	rdfs:comment "Link to prescribing information for the drug." .

schema:prescriptionStatus a rdf:Property ;
	rdfs:label "prescriptionStatus" ;
	schema:domainIncludes schema:Drug ;
	schema:rangeIncludes schema:DrugPrescriptionStatus ;
	rdfs:comment "Indicates whether this drug is available by prescription or over-the-counter." .

schema:price a rdf:Property ;
	rdfs:label "price" ;
	schema:domainIncludes schema:Offer , schema:PriceSpecification , schema:TradeAction ;
	schema:rangeIncludes schema:Number , schema:Text ;
	rdfs:comment "The offer price of a product, or of a price component when attached to PriceSpecification and its subtypes." .

schema:priceCurrency a rdf:Property ;
	rdfs:label "priceCurrency" ;
	schema:domainIncludes schema:Offer , schema:PriceSpecification ;
	schema:rangeIncludes schema:Text ;
	rdfs:comment "The currency (in 3-letter ISO 4217 format) of the offer price or a price component, when attached to PriceSpecification and its subtypes." .

schema:priceRange a rdf:Property ;
	rdfs:label "priceRange" ;
	schema:domainIncludes schema:LocalBusiness ;
	schema:rangeIncludes schema:Text ;
	rdfs:comment "The price range of the business, for example <code>$$$</code>." .

schema:priceSpecification a rdf:Property ;
	rdfs:label "priceSpecification" ;
	schema:domainIncludes schema:Demand , schema:Offer ;
	schema:rangeIncludes schema:PriceSpecification ;
	rdfs:comment "One or more detailed price specifications, indicating the unit price and delivery or payment charges." .

schema:priceType a rdf:Property ;
	rdfs:label "priceType" ;
	schema:domainIncludes schema:UnitPriceSpecification ;
	schema:rangeIncludes schema:Text ;
	rdfs:comment "A short text or acronym indicating multiple price specifications for the same offer, e.g. SRP for the suggested retail price or INVOICE for the invoice price, mostly used in the car industry." .

schema:priceValidUntil a rdf:Property ;
	rdfs:label "priceValidUntil" ;
	schema:domainIncludes schema:Offer ;
	schema:rangeIncludes schema:Date ;
	rdfs:comment "The date after which the price is no longer available." .

schema:primaryImageOfPage a rdf:Property ;
	rdfs:label "primaryImageOfPage" ;
	schema:domainIncludes schema:WebPage ;
	schema:rangeIncludes schema:ImageObject ;
	rdfs:comment "Indicates the main image on the page" .

schema:primaryPrevention a rdf:Property ;
	rdfs:label "primaryPrevention" ;
	schema:domainIncludes schema:MedicalCondition ;
	schema:rangeIncludes schema:MedicalTherapy ;
	rdfs:comment "A preventative therapy used to prevent an initial occurrence of the medical condition, such as vaccination." .

schema:printColumn a rdf:Property ;
	rdfs:label "printColumn" ;
	schema:domainIncludes schema:NewsArticle ;
	schema:rangeIncludes schema:Text ;
	rdfs:comment "The number of the column in which the NewsArticle appears in the print edition." .

schema:printEdition a rdf:Property ;
	rdfs:label "printEdition" ;
	schema:domainIncludes schema:NewsArticle ;
	schema:rangeIncludes schema:Text ;
	rdfs:comment "The edition of the print product in which the NewsArticle appears." .

schema:printPage a rdf:Property ;
	rdfs:label "printPage" ;
	schema:domainIncludes schema:NewsArticle ;
	schema:rangeIncludes schema:Text ;
	rdfs:comment "If this NewsArticle appears in print, this field indicates the name of the page on which the article is found. Please note that this field is intended for the exact page name (e.g. A5, B18)." .

schema:printSection a rdf:Property ;
	rdfs:label "printSection" ;
	schema:domainIncludes schema:NewsArticle ;
	schema:rangeIncludes schema:Text ;
	rdfs:comment "If this NewsArticle appears in print, this field indicates the print section in which the article appeared." .

schema:procedure a rdf:Property ;
	rdfs:label "procedure" ;
	schema:domainIncludes schema:MedicalDevice ;
	schema:rangeIncludes schema:Text ;
	rdfs:comment "A description of the procedure involved in setting up, using, and/or installing the device." .

schema:procedureType a rdf:Property ;
	rdfs:label "procedureType" ;
	schema:domainIncludes schema:MedicalProcedure ;
	schema:rangeIncludes schema:MedicalProcedureType ;
	rdfs:comment "The type of procedure, for example Surgical, Noninvasive, or Percutaneous." .

schema:processorRequirements a rdf:Property ;
	rdfs:label "processorRequirements" ;
	schema:domainIncludes schema:SoftwareApplication ;
	schema:rangeIncludes schema:Text ;
	rdfs:comment "Processor architecture required to run the application (e.g. IA64)." .

schema:producer a rdf:Property ;
	rdfs:label "producer" ;
	schema:domainIncludes schema:Movie , schema:TVEpisode , schema:TVSeries ;
	schema:rangeIncludes schema:Person ;
	rdfs:comment "The producer of the movie, TV series, season, or episode, or video." .

schema:productID a rdf:Property ;
	rdfs:label "productID" ;
	schema:domainIncludes schema:Product ;
	schema:rangeIncludes schema:Text ;
	rdfs:comment "The product identifier, such as ISBN. For example: <code>&lt;meta itemprop='productID' content='isbn:123-456-789'/&gt;</code>." .

schema:productionCompany a rdf:Property ;
	rdfs:label "productionCompany" ;
	schema:domainIncludes schema:Movie , schema:TVEpisode , schema:TVSeries , schema:VideoObject ;
	schema:rangeIncludes schema:Organization ;
	rdfs:comment "The production company or studio that made the movie, TV series, season, or episode, or video." .

schema:proficiencyLevel a rdf:Property ;
	rdfs:label "proficiencyLevel" ;
	schema:domainIncludes schema:TechArticle ;
	schema:rangeIncludes schema:Text ;
	rdfs:comment "Proficiency needed for this content; expected values: 'Beginner', 'Expert'." .

schema:programmingLanguage a rdf:Property ;
	rdfs:label "programmingLanguage" ;
	schema:domainIncludes schema:Code ;
	schema:rangeIncludes schema:Thing ;
	rdfs:comment "The computer programming language." .

schema:programmingModel a rdf:Property ;
	rdfs:label "programmingModel" ;
	schema:domainIncludes schema:APIReference ;
	schema:rangeIncludes schema:Text ;
	rdfs:comment "Indicates whether API is managed or unmanaged." .

schema:proprietaryName a rdf:Property ;
	rdfs:label "proprietaryName" ;
	schema:domainIncludes schema:Diet ;
	schema:rangeIncludes schema:Text ;
	rdfs:comment "Proprietary name given to the diet plan, typically by its originator or creator." .

schema:proteinContent a rdf:Property ;
	rdfs:label "proteinContent" ;
	schema:domainIncludes schema:NutritionInformation ;
	schema:rangeIncludes schema:Mass ;
	rdfs:comment "The number of grams of protein." .

schema:provider a rdf:Property ;
	rdfs:label "provider" ;
	schema:domainIncludes schema:CreativeWork ;
	schema:rangeIncludes schema:Organization , schema:Person ;
	rdfs:comment "Specifies the Person or Organization that distributed the CreativeWork." .

schema:publicationType a rdf:Property ;
	rdfs:label "publicationType" ;
	schema:domainIncludes schema:MedicalScholarlyArticle ;
	schema:rangeIncludes schema:Text ;
	rdfs:comment "The type of the medical article, taken from the US NLM MeSH <a href=http://www.nlm.nih.gov/mesh/pubtypes.html>publication type catalog." .

schema:publisher a rdf:Property ;
	rdfs:label "publisher" ;
	schema:domainIncludes schema:CreativeWork ;
	schema:rangeIncludes schema:Organization ;
	rdfs:comment "The publisher of the creative work." .

schema:publishingPrinciples a rdf:Property ;
	rdfs:label "publishingPrinciples" ;
	schema:domainIncludes schema:CreativeWork ;
	schema:rangeIncludes schema:URL ;
	rdfs:comment "Link to page describing the editorial principles of the organization primarily responsible for the creation of the CreativeWork." .

schema:purpose a rdf:Property ;
	rdfs:label "purpose" ;
	schema:domainIncludes schema:AllocateAction , schema:MedicalDevice , schema:PayAction ;
	schema:rangeIncludes schema:MedicalDevicePurpose , schema:Thing ;
	rdfs:comment "A goal towards an action is taken. Can be concrete or abstract." .

schema:qualifications a rdf:Property ;
	rdfs:label "qualifications" ;
	schema:domainIncludes schema:JobPosting ;
	schema:rangeIncludes schema:Text ;
	rdfs:comment "Specific qualifications required for this role." .

schema:query a rdf:Property ;
	rdfs:label "query" ;
	schema:domainIncludes schema:SearchAction ;
	schema:rangeIncludes schema:Class , schema:Text ;
	rdfs:comment "A sub property of instrument. The query used on this action." .

schema:question a rdf:Property ;
	rdfs:label "question" ;
	schema:domainIncludes schema:AskAction ;
	schema:rangeIncludes schema:Text ;
	rdfs:comment "A sub property of object. A question." .

schema:rangeIncludes a rdf:Property ;
	rdfs:label "rangeIncludes" ;
	schema:domainIncludes schema:Property ;
	schema:rangeIncludes schema:Class ;
	rdfs:comment "Relates a property to a class that constitutes (one of) the expected type(s) for values of the property." .

schema:ratingCount a rdf:Property ;
	rdfs:label "ratingCount" ;
	schema:domainIncludes schema:AggregateRating ;
	schema:rangeIncludes schema:Number ;
	rdfs:comment "The count of total number of ratings." .

schema:ratingValue a rdf:Property ;
	rdfs:label "ratingValue" ;
	schema:domainIncludes schema:Rating ;
	schema:rangeIncludes schema:Text ;
	rdfs:comment "The rating for the content." .

schema:realEstateAgent a rdf:Property ;
	rdfs:label "realEstateAgent" ;
	schema:domainIncludes schema:RentAction ;
	schema:rangeIncludes schema:RealEstateAgent ;
	rdfs:comment "A sub property of participant. The real estate agent involved in the action." .

schema:recipe a rdf:Property ;
	rdfs:label "recipe" ;
	schema:domainIncludes schema:CookAction ;
	schema:rangeIncludes schema:Recipe ;
	rdfs:comment "A sub property of instrument. The recipe/instructions used to perform the action." .

schema:recipeCategory a rdf:Property ;
	rdfs:label "recipeCategory" ;
	schema:domainIncludes schema:Recipe ;
	schema:rangeIncludes schema:Text ;
	rdfs:comment "The category of the recipe&#x2014;for example, appetizer, entree, etc." .

schema:recipeCuisine a rdf:Property ;
	rdfs:label "recipeCuisine" ;
	schema:domainIncludes schema:Recipe ;
	schema:rangeIncludes schema:Text ;
	rdfs:comment "The cuisine of the recipe (for example, French or Ethopian)." .

schema:recipeInstructions a rdf:Property ;
	rdfs:label "recipeInstructions" ;
	schema:domainIncludes schema:Recipe ;
	schema:rangeIncludes schema:Text ;
	rdfs:comment "The steps to make the dish." .

schema:recipeYield a rdf:Property ;
	rdfs:label "recipeYield" ;
	schema:domainIncludes schema:Recipe ;
	schema:rangeIncludes schema:Text ;
	rdfs:comment "The quantity produced by the recipe (for example, number of people served, number of servings, etc)." .

schema:recipient a rdf:Property ;
	rdfs:label "recipient" ;
	schema:domainIncludes schema:AuthorizeAction , schema:CommunicateAction , schema:DonateAction , schema:GiveAction , schema:PayAction , schema:ReturnAction , schema:SendAction , schema:TipAction ;
	schema:rangeIncludes schema:Audience , schema:Organization , schema:Person ;
	rdfs:comment "A sub property of participant. The participant who is at the receiving end of the action." .

schema:recognizingAuthority a rdf:Property ;
	rdfs:label "recognizingAuthority" ;
	schema:domainIncludes schema:MedicalEntity ;
	schema:rangeIncludes schema:Organization ;
	rdfs:comment "If applicable, the organization that officially recognizes this entity as part of its endorsed system of medicine." .

schema:recommendationStrength a rdf:Property ;
	rdfs:label "recommendationStrength" ;
	schema:domainIncludes schema:MedicalGuidelineRecommendation ;
	schema:rangeIncludes schema:Text ;
	rdfs:comment "Strength of the guideline's recommendation (e.g. 'class I')." .

schema:recommendedIntake a rdf:Property ;
	rdfs:label "recommendedIntake" ;
	schema:domainIncludes schema:DietarySupplement ;
	schema:rangeIncludes schema:RecommendedDoseSchedule ;
	rdfs:comment "Recommended intake of this supplement for a given population as defined by a specific recommending authority." .

schema:regionDrained a rdf:Property ;
	rdfs:label "regionDrained" ;
	schema:domainIncludes schema:LymphaticVessel , schema:Vein ;
	schema:rangeIncludes schema:AnatomicalStructure , schema:AnatomicalSystem ;
	rdfs:comment "The anatomical or organ system drained by this vessel; generally refers to a specific part of an organ." .

schema:regionsAllowed a rdf:Property ;
	rdfs:label "regionsAllowed" ;
	schema:domainIncludes schema:MediaObject ;
	schema:rangeIncludes schema:Place ;
	rdfs:comment "The regions where the media is allowed. If not specified, then it's assumed to be allowed everywhere. Specify the countries in <a href='http://en.wikipedia.org/wiki/ISO_3166'>ISO 3166 format</a>." .

schema:relatedAnatomy a rdf:Property ;
	rdfs:label "relatedAnatomy" ;
	schema:domainIncludes schema:SuperficialAnatomy ;
	schema:rangeIncludes schema:AnatomicalStructure , schema:AnatomicalSystem ;
	rdfs:comment "Anatomical systems or structures that relate to the superficial anatomy." .

schema:relatedCondition a rdf:Property ;
	rdfs:label "relatedCondition" ;
	schema:domainIncludes schema:AnatomicalStructure , schema:AnatomicalSystem , schema:SuperficialAnatomy ;
	schema:rangeIncludes schema:MedicalCondition ;
	rdfs:comment "A medical condition associated with this anatomy." .

schema:relatedDrug a rdf:Property ;
	rdfs:label "relatedDrug" ;
	schema:domainIncludes schema:Drug ;
	schema:rangeIncludes schema:Drug ;
	rdfs:comment "Any other drug related to this one, for example commonly-prescribed alternatives." .

schema:relatedLink a rdf:Property ;
	rdfs:label "relatedLink" ;
	schema:domainIncludes schema:WebPage ;
	schema:rangeIncludes schema:URL ;
	rdfs:comment "A link related to this web page, for example to other related web pages." .

schema:relatedStructure a rdf:Property ;
	rdfs:label "relatedStructure" ;
	schema:domainIncludes schema:AnatomicalSystem ;
	schema:rangeIncludes schema:AnatomicalStructure ;
	rdfs:comment "Related anatomical structure(s) that are not part of the system but relate or connect to it, such as vascular bundles associated with an organ system." .

schema:relatedTherapy a rdf:Property ;
	rdfs:label "relatedTherapy" ;
	schema:domainIncludes schema:AnatomicalStructure , schema:AnatomicalSystem , schema:SuperficialAnatomy ;
	schema:rangeIncludes schema:MedicalTherapy ;
	rdfs:comment "A medical therapy related to this anatomy." .

schema:relatedTo a rdf:Property ;
	rdfs:label "relatedTo" ;
	schema:domainIncludes schema:Person ;
	schema:rangeIncludes schema:Person ;
	rdfs:comment "The most generic familial relation." .

schema:releaseDate a rdf:Property ;
	rdfs:label "releaseDate" ;
	schema:domainIncludes schema:Product ;
	schema:rangeIncludes schema:Date ;
	rdfs:comment "The release date of a product or product model. This can be used to distinguish the exact variant of a product." .

schema:releaseNotes a rdf:Property ;
	rdfs:label "releaseNotes" ;
	schema:domainIncludes schema:SoftwareApplication ;
	schema:rangeIncludes schema:Text , schema:URL ;
	rdfs:comment "Description of what changed in this version." .

schema:relevantSpecialty a rdf:Property ;
	rdfs:label "relevantSpecialty" ;
	schema:domainIncludes schema:MedicalEntity ;
	schema:rangeIncludes schema:MedicalSpecialty ;
	rdfs:comment "If applicable, a medical specialty in which this entity is relevant." .

schema:repetitions a rdf:Property ;
	rdfs:label "repetitions" ;
	schema:domainIncludes schema:ExercisePlan ;
	schema:rangeIncludes schema:Number ;
	rdfs:comment "Number of times one should repeat the activity." .

schema:replacee a rdf:Property ;
	rdfs:label "replacee" ;
	schema:domainIncludes schema:ReplaceAction ;
	schema:rangeIncludes schema:Thing ;
	rdfs:comment "A sub property of object. The object that is being replaced." .

schema:replacer a rdf:Property ;
	rdfs:label "replacer" ;
	schema:domainIncludes schema:ReplaceAction ;
	schema:rangeIncludes schema:Thing ;
	rdfs:comment "A sub property of object. The object that replaces." .

schema:replyToUrl a rdf:Property ;
	rdfs:label "replyToUrl" ;
	schema:domainIncludes schema:UserComments ;
	schema:rangeIncludes schema:URL ;
	rdfs:comment "The URL at which a reply may be posted to the specified UserComment." .

schema:representativeOfPage a rdf:Property ;
	rdfs:label "representativeOfPage" ;
	schema:domainIncludes schema:ImageObject ;
	schema:rangeIncludes schema:Boolean ;
	rdfs:comment "Indicates whether this image is representative of the content of the page." .

schema:requirements a rdf:Property ;
	rdfs:label "requirements" ;
	schema:domainIncludes schema:SoftwareApplication ;
	schema:rangeIncludes schema:Text , schema:URL ;
	rdfs:comment "Component dependency requirements for application. This includes runtime environments and shared libraries that are not included in the application distribution package, but required to run the application (Examples: DirectX, Java or .NET runtime)." .

schema:requiresSubscription a rdf:Property ;
	rdfs:label "requiresSubscription" ;
	schema:domainIncludes schema:MediaObject ;
	schema:rangeIncludes schema:Boolean ;
	rdfs:comment "Indicates if use of the media require a subscription  (either paid or free). Allowed values are <code>true</code> or <code>false</code> (note that an earlier version had 'yes', 'no')." .

schema:responsibilities a rdf:Property ;
	rdfs:label "responsibilities" ;
	schema:domainIncludes schema:JobPosting ;
	schema:rangeIncludes schema:Text ;
	rdfs:comment "Responsibilities associated with this role." .

schema:restPeriods a rdf:Property ;
	rdfs:label "restPeriods" ;
	schema:domainIncludes schema:ExercisePlan ;
	schema:rangeIncludes schema:Text ;
	rdfs:comment "How often one should break from the activity." .

schema:result a rdf:Property ;
	rdfs:label "result" ;
	schema:domainIncludes schema:Action ;
	schema:rangeIncludes schema:Thing ;
	rdfs:comment "The result produced in the action. e.g. John wrote *a book*." .

schema:resultReview a rdf:Property ;
	rdfs:label "resultReview" ;
	schema:domainIncludes schema:ReviewAction ;
	schema:rangeIncludes schema:Review ;
	rdfs:comment "A sub property of result. The review that resulted in the performing of the action." .

schema:review a rdf:Property ;
	rdfs:label "review" ;
	schema:domainIncludes schema:CreativeWork , schema:Offer , schema:Organization , schema:Place , schema:Product ;
	schema:rangeIncludes schema:Review ;
	rdfs:comment "A review of the item." .

schema:reviewBody a rdf:Property ;
	rdfs:label "reviewBody" ;
	schema:domainIncludes schema:Review ;
	schema:rangeIncludes schema:Text ;
	rdfs:comment "The actual body of the review" .

schema:reviewCount a rdf:Property ;
	rdfs:label "reviewCount" ;
	schema:domainIncludes schema:AggregateRating ;
	schema:rangeIncludes schema:Number ;
	rdfs:comment "The count of total number of reviews." .

schema:reviewRating a rdf:Property ;
	rdfs:label "reviewRating" ;
	schema:domainIncludes schema:Review ;
	schema:rangeIncludes schema:Rating ;
	rdfs:comment "The rating given in this review. Note that reviews can themselves be rated. The <code>reviewRating</code> applies to rating given by the review. The <code>aggregateRating</code> property applies to the review itself, as a creative work." .

schema:reviewedBy a rdf:Property ;
	rdfs:label "reviewedBy" ;
	schema:domainIncludes schema:WebPage ;
	schema:rangeIncludes schema:Organization , schema:Person ;
	rdfs:comment "People or organizations that have reviewed the content on this web page for accuracy and/or completeness." .

schema:reviews a rdf:Property ;
	rdfs:label "reviews" ;
	schema:domainIncludes schema:CreativeWork , schema:Offer , schema:Organization , schema:Place , schema:Product ;
	schema:rangeIncludes schema:Review ;
	rdfs:comment "Review of the item (legacy spelling; see singular form, review)." .

schema:riskFactor a rdf:Property ;
	rdfs:label "riskFactor" ;
	schema:domainIncludes schema:MedicalCondition ;
	schema:rangeIncludes schema:MedicalRiskFactor ;
	rdfs:comment "A modifiable or non-modifiable factor that increases the risk of a patient contracting this condition, e.g. age,  coexisting condition." .

schema:risks a rdf:Property ;
	rdfs:label "risks" ;
	schema:domainIncludes schema:Diet ;
	schema:rangeIncludes schema:Text ;
	rdfs:comment "Specific physiologic risks associated to the plan." .

schema:runsTo a rdf:Property ;
	rdfs:label "runsTo" ;
	schema:domainIncludes schema:LymphaticVessel ;
	schema:rangeIncludes schema:Vessel ;
	rdfs:comment "The vasculature the lymphatic structure runs, or efferents, to." .

schema:runtime a rdf:Property ;
	rdfs:label "runtime" ;
	schema:domainIncludes schema:Code ;
	schema:rangeIncludes schema:Text ;
	rdfs:comment "Runtime platform or script interpreter dependencies (Example - Java v1, Python2.3, .Net Framework 3.0)" .

schema:safetyConsideration a rdf:Property ;
	rdfs:label "safetyConsideration" ;
	schema:domainIncludes schema:DietarySupplement ;
	schema:rangeIncludes schema:Text ;
	rdfs:comment "Any potential safety concern associated with the supplement. May include interactions with other drugs and foods, pregnancy, breastfeeding, known adverse reactions, and documented efficacy of the supplement." .

schema:salaryCurrency a rdf:Property ;
	rdfs:label "salaryCurrency" ;
	schema:domainIncludes schema:JobPosting ;
	schema:rangeIncludes schema:Text ;
	rdfs:comment "The currency (coded using ISO 4217, http://en.wikipedia.org/wiki/ISO_4217 used for the main salary information in this job posting." .

schema:sameAs a rdf:Property ;
	rdfs:label "sameAs" ;
	schema:domainIncludes schema:Thing ;
	schema:rangeIncludes schema:URL ;
	rdfs:comment "URL of a reference Web page that unambiguously indicates the item's identity. E.g. the URL of the item's Wikipedia page, Freebase page, or official website." .

schema:sampleType a rdf:Property ;
	rdfs:label "sampleType" ;
	schema:domainIncludes schema:Code ;
	schema:rangeIncludes schema:Text ;
	rdfs:comment "Full (compile ready) solution, code snippet, inline code, scripts, template." .

schema:saturatedFatContent a rdf:Property ;
	rdfs:label "saturatedFatContent" ;
	schema:domainIncludes schema:NutritionInformation ;
	schema:rangeIncludes schema:Mass ;
	rdfs:comment "The number of grams of saturated fat." .

schema:scheduledTime a rdf:Property ;
	rdfs:label "scheduledTime" ;
	schema:domainIncludes schema:PlanAction , schema:ReserveAction ;
	schema:rangeIncludes schema:DateTime ;
	rdfs:comment "The time the object is scheduled to." .

schema:screenshot a rdf:Property ;
	rdfs:label "screenshot" ;
	schema:domainIncludes schema:SoftwareApplication ;
	schema:rangeIncludes schema:ImageObject , schema:URL ;
	rdfs:comment "A link to a screenshot image of the app." .

schema:season a rdf:Property ;
	rdfs:label "season" ;
	schema:domainIncludes schema:TVSeries ;
	schema:rangeIncludes schema:TVSeason ;
	rdfs:comment "A season of a TV series." .

schema:seasonNumber a rdf:Property ;
	rdfs:label "seasonNumber" ;
	schema:domainIncludes schema:TVSeason ;
	schema:rangeIncludes schema:Integer ;
	rdfs:comment "The season number." .

schema:seasons a rdf:Property ;
	rdfs:label "seasons" ;
	schema:domainIncludes schema:TVSeries ;
	schema:rangeIncludes schema:TVSeason ;
	rdfs:comment "The seasons of the TV series (legacy spelling; see singular form, season)." .

schema:secondaryPrevention a rdf:Property ;
	rdfs:label "secondaryPrevention" ;
	schema:domainIncludes schema:MedicalCondition ;
	schema:rangeIncludes schema:MedicalTherapy ;
	rdfs:comment "A preventative therapy used to prevent reoccurrence of the medical condition after an initial episode of the condition." .

schema:seeks a rdf:Property ;
	rdfs:label "seeks" ;
	schema:domainIncludes schema:Organization , schema:Person ;
	schema:rangeIncludes schema:Demand ;
	rdfs:comment "A pointer to products or services sought by the organization or person (demand)." .

schema:seller a rdf:Property ;
	rdfs:label "seller" ;
	schema:domainIncludes schema:Demand , schema:Offer ;
	schema:rangeIncludes schema:Organization , schema:Person ;
	rdfs:comment "The seller." .

schema:sender a rdf:Property ;
	rdfs:label "sender" ;
	schema:domainIncludes schema:ReceiveAction ;
	schema:rangeIncludes schema:Audience , schema:Organization , schema:Person ;
	rdfs:comment "A sub property of participant. The participant who is at the sending end of the action." .

schema:sensoryUnit a rdf:Property ;
	rdfs:label "sensoryUnit" ;
	schema:domainIncludes schema:Nerve ;
	schema:rangeIncludes schema:AnatomicalStructure , schema:SuperficialAnatomy ;
	rdfs:comment "The neurological pathway extension that inputs and sends information to the brain or spinal cord." .

schema:serialNumber a rdf:Property ;
	rdfs:label "serialNumber" ;
	schema:domainIncludes schema:Demand , schema:IndividualProduct , schema:Offer ;
	schema:rangeIncludes schema:Text ;
	rdfs:comment "The serial number or any alphanumeric identifier of a particular product. When attached to an offer, it is a shortcut for the serial number of the product included in the offer." .

schema:seriousAdverseOutcome a rdf:Property ;
	rdfs:label "seriousAdverseOutcome" ;
	schema:domainIncludes schema:MedicalDevice , schema:MedicalTherapy ;
	schema:rangeIncludes schema:MedicalEntity ;
	rdfs:comment "A possible serious complication and/or serious side effect of this therapy. Serious adverse outcomes include those that are life-threatening; result in death, disability, or permanent damage; require hospitalization or prolong existing hospitalization; cause congenital anomalies or birth defects; or jeopardize the patient and may require medical or surgical intervention to prevent one of the outcomes in this definition." .

schema:servesCuisine a rdf:Property ;
	rdfs:label "servesCuisine" ;
	schema:domainIncludes schema:FoodEstablishment ;
	schema:rangeIncludes schema:Text ;
	rdfs:comment "The cuisine of the restaurant." .

schema:servingSize a rdf:Property ;
	rdfs:label "servingSize" ;
	schema:domainIncludes schema:NutritionInformation ;
	schema:rangeIncludes schema:Text ;
	rdfs:comment "The serving size, in terms of the number of volume or mass" .

schema:sibling a rdf:Property ;
	rdfs:label "sibling" ;
	schema:domainIncludes schema:Person ;
	schema:rangeIncludes schema:Person ;
	rdfs:comment "A sibling of the person." .

schema:siblings a rdf:Property ;
	rdfs:label "siblings" ;
	schema:domainIncludes schema:Person ;
	schema:rangeIncludes schema:Person ;
	rdfs:comment "A sibling of the person (legacy spelling; see singular form, sibling)." .

schema:signDetected a rdf:Property ;
	rdfs:label "signDetected" ;
	schema:domainIncludes schema:MedicalTest ;
	schema:rangeIncludes schema:MedicalSign ;
	rdfs:comment "A sign detected by the test." .

schema:signOrSymptom a rdf:Property ;
	rdfs:label "signOrSymptom" ;
	schema:domainIncludes schema:MedicalCondition ;
	schema:rangeIncludes schema:MedicalSignOrSymptom ;
	rdfs:comment "A sign or symptom of this condition. Signs are objective or physically observable manifestations of the medical condition while symptoms are the subjective experienceof the medical condition." .

schema:significance a rdf:Property ;
	rdfs:label "significance" ;
	schema:domainIncludes schema:SuperficialAnatomy ;
	schema:rangeIncludes schema:Text ;
	rdfs:comment "The significance associated with the superficial anatomy; as an example, how characteristics of the superficial anatomy can suggest underlying medical conditions or courses of treatment." .

schema:significantLink a rdf:Property ;
	rdfs:label "significantLink" ;
	schema:domainIncludes schema:WebPage ;
	schema:rangeIncludes schema:URL ;
	rdfs:comment "One of the more significant URLs on the page. Typically, these are the non-navigation links that are clicked on the most." .

schema:significantLinks a rdf:Property ;
	rdfs:label "significantLinks" ;
	schema:domainIncludes schema:WebPage ;
	schema:rangeIncludes schema:URL ;
	rdfs:comment "The most significant URLs on the page. Typically, these are the non-navigation links that are clicked on the most (legacy spelling; see singular form, significantLink)." .

schema:skills a rdf:Property ;
	rdfs:label "skills" ;
	schema:domainIncludes schema:JobPosting ;
	schema:rangeIncludes schema:Text ;
	rdfs:comment "Skills required to fulfill this role." .

schema:sku a rdf:Property ;
	rdfs:label "sku" ;
	schema:domainIncludes schema:Demand , schema:Offer , schema:Product ;
	schema:rangeIncludes schema:Text ;
	rdfs:comment "The Stock Keeping Unit (SKU), i.e. a merchant-specific identifier for a product or service, or the product to which the offer refers." .

schema:sodiumContent a rdf:Property ;
	rdfs:label "sodiumContent" ;
	schema:domainIncludes schema:NutritionInformation ;
	schema:rangeIncludes schema:Mass ;
	rdfs:comment "The number of milligrams of sodium." .

schema:softwareVersion a rdf:Property ;
	rdfs:label "softwareVersion" ;
	schema:domainIncludes schema:SoftwareApplication ;
	schema:rangeIncludes schema:Text ;
	rdfs:comment "Version of the software instance." .

schema:source a rdf:Property ;
	rdfs:label "source" ;
	schema:domainIncludes schema:Artery ;
	schema:rangeIncludes schema:AnatomicalStructure ;
	rdfs:comment "The anatomical or organ system that the artery originates from." .

schema:sourceOrganization a rdf:Property ;
	rdfs:label "sourceOrganization" ;
	schema:domainIncludes schema:CreativeWork ;
	schema:rangeIncludes schema:Organization ;
	rdfs:comment "The Organization on whose behalf the creator was working." .

schema:sourcedFrom a rdf:Property ;
	rdfs:label "sourcedFrom" ;
	schema:domainIncludes schema:Nerve ;
	schema:rangeIncludes schema:BrainStructure ;
	rdfs:comment "The neurological pathway that originates the neurons." .

schema:spatial a rdf:Property ;
	rdfs:label "spatial" ;
	schema:domainIncludes schema:Dataset ;
	schema:rangeIncludes schema:Place ;
	rdfs:comment "The range of spatial applicability of a dataset, e.g. for a dataset of New York weather, the state of New York." .

schema:specialCommitments a rdf:Property ;
	rdfs:label "specialCommitments" ;
	schema:domainIncludes schema:JobPosting ;
	schema:rangeIncludes schema:Text ;
	rdfs:comment "Any special commitments associated with this job posting. Valid entries include VeteranCommit, MilitarySpouseCommit, etc." .

schema:specialty a rdf:Property ;
	rdfs:label "specialty" ;
	schema:domainIncludes schema:WebPage ;
	schema:rangeIncludes schema:Specialty ;
	rdfs:comment "One of the domain specialities to which this web page's content applies." .

schema:sponsor a rdf:Property ;
	rdfs:label "sponsor" ;
	schema:domainIncludes schema:MedicalStudy ;
	schema:rangeIncludes schema:Organization ;
	rdfs:comment "Sponsor of the study." .

schema:sportsActivityLocation a rdf:Property ;
	rdfs:label "sportsActivityLocation" ;
	schema:domainIncludes schema:ExerciseAction ;
	schema:rangeIncludes schema:SportsActivityLocation ;
	rdfs:comment "A sub property of location. The sports activity location where this action occurred." .

schema:sportsEvent a rdf:Property ;
	rdfs:label "sportsEvent" ;
	schema:domainIncludes schema:ExerciseAction ;
	schema:rangeIncludes schema:SportsEvent ;
	rdfs:comment "A sub property of location. The sports event where this action occurred." .

schema:sportsTeam a rdf:Property ;
	rdfs:label "sportsTeam" ;
	schema:domainIncludes schema:ExerciseAction ;
	schema:rangeIncludes schema:SportsTeam ;
	rdfs:comment "A sub property of participant. The sports team that participated on this action." .

schema:spouse a rdf:Property ;
	rdfs:label "spouse" ;
	schema:domainIncludes schema:Person ;
	schema:rangeIncludes schema:Person ;
	rdfs:comment "The person's spouse." .

schema:stage a rdf:Property ;
	rdfs:label "stage" ;
	schema:domainIncludes schema:MedicalCondition ;
	schema:rangeIncludes schema:MedicalConditionStage ;
	rdfs:comment "The stage of the condition, if applicable." .

schema:stageAsNumber a rdf:Property ;
	rdfs:label "stageAsNumber" ;
	schema:domainIncludes schema:MedicalConditionStage ;
	schema:rangeIncludes schema:Number ;
	rdfs:comment "The stage represented as a number, e.g. 3." .

schema:startDate a rdf:Property ;
	rdfs:label "startDate" ;
	schema:domainIncludes schema:Event , schema:TVSeason , schema:TVSeries ;
	schema:rangeIncludes schema:Date ;
	rdfs:comment "The start date and time of the event (in <a href='http://en.wikipedia.org/wiki/ISO_8601'>ISO 8601 date format</a>)." .

schema:startTime a rdf:Property ;
	rdfs:label "startTime" ;
	schema:domainIncludes schema:Action ;
	schema:rangeIncludes schema:DateTime ;
	rdfs:comment "When the Action was performed: start time. This is for actions that span a period of time. e.g. John wrote a book from *January* to December." .

schema:status a rdf:Property ;
	rdfs:label "status" ;
	schema:domainIncludes schema:MedicalStudy ;
	schema:rangeIncludes schema:MedicalStudyStatus ;
	rdfs:comment "The status of the study (enumerated)." .

schema:storageRequirements a rdf:Property ;
	rdfs:label "storageRequirements" ;
	schema:domainIncludes schema:SoftwareApplication ;
	schema:rangeIncludes schema:Text , schema:URL ;
	rdfs:comment "Storage requirements (free space required)." .

schema:streetAddress a rdf:Property ;
	rdfs:label "streetAddress" ;
	schema:domainIncludes schema:PostalAddress ;
	schema:rangeIncludes schema:Text ;
	rdfs:comment "The street address. For example, 1600 Amphitheatre Pkwy." .

schema:strengthUnit a rdf:Property ;
	rdfs:label "strengthUnit" ;
	schema:domainIncludes schema:DrugStrength ;
	schema:rangeIncludes schema:Text ;
	rdfs:comment "The units of an active ingredient's strength, e.g. mg." .

schema:strengthValue a rdf:Property ;
	rdfs:label "strengthValue" ;
	schema:domainIncludes schema:DrugStrength ;
	schema:rangeIncludes schema:Number ;
	rdfs:comment "The value of an active ingredient's strength, e.g. 325." .

schema:structuralClass a rdf:Property ;
	rdfs:label "structuralClass" ;
	schema:domainIncludes schema:Joint ;
	schema:rangeIncludes schema:Text ;
	rdfs:comment "The name given to how bone physically connects to each other." .

schema:study a rdf:Property ;
	rdfs:label "study" ;
	schema:domainIncludes schema:MedicalEntity ;
	schema:rangeIncludes schema:MedicalStudy ;
	rdfs:comment "A medical study or trial related to this entity." .

schema:studyDesign a rdf:Property ;
	rdfs:label "studyDesign" ;
	schema:domainIncludes schema:MedicalObservationalStudy ;
	schema:rangeIncludes schema:MedicalObservationalStudyDesign ;
	rdfs:comment "Specifics about the observational study design (enumerated)." .

schema:studyLocation a rdf:Property ;
	rdfs:label "studyLocation" ;
	schema:domainIncludes schema:MedicalStudy ;
	schema:rangeIncludes schema:AdministrativeArea ;
	rdfs:comment "The location in which the study is taking/took place." .

schema:studySubject a rdf:Property ;
	rdfs:label "studySubject" ;
	schema:domainIncludes schema:MedicalStudy ;
	schema:rangeIncludes schema:MedicalEntity ;
	rdfs:comment "A subject of the study, i.e. one of the medical conditions, therapies, devices, drugs, etc. investigated by the study." .

schema:subEvent a rdf:Property ;
	rdfs:label "subEvent" ;
	schema:domainIncludes schema:Event ;
	schema:rangeIncludes schema:Event ;
	rdfs:comment "An Event that is part of this event. For example, a conference event includes many presentations, each are a subEvent of the conference." .

schema:subEvents a rdf:Property ;
	rdfs:label "subEvents" ;
	schema:domainIncludes schema:Event ;
	schema:rangeIncludes schema:Event ;
	rdfs:comment "Events that are a part of this event. For example, a conference event includes many presentations, each are subEvents of the conference (legacy spelling; see singular form, subEvent)." .

schema:subStageSuffix a rdf:Property ;
	rdfs:label "subStageSuffix" ;
	schema:domainIncludes schema:MedicalConditionStage ;
	schema:rangeIncludes schema:Text ;
	rdfs:comment "The substage, e.g. 'a' for Stage IIIa." .

schema:subStructure a rdf:Property ;
	rdfs:label "subStructure" ;
	schema:domainIncludes schema:AnatomicalStructure ;
	schema:rangeIncludes schema:AnatomicalStructure ;
	rdfs:comment "Component (sub-)structure(s) that comprise this anatomical structure." .

schema:subTest a rdf:Property ;
	rdfs:label "subTest" ;
	schema:domainIncludes schema:MedicalTestPanel ;
	schema:rangeIncludes schema:MedicalTest ;
	rdfs:comment "A component test of the panel." .

schema:subtype a rdf:Property ;
	rdfs:label "subtype" ;
	schema:domainIncludes schema:MedicalCondition ;
	schema:rangeIncludes schema:Text ;
	rdfs:comment "A more specific type of the condition, where applicable, for example 'Type 1 Diabetes', 'Type 2 Diabetes', or 'Gestational Diabetes' for Diabetes." .

schema:successorOf a rdf:Property ;
	rdfs:label "successorOf" ;
	schema:domainIncludes schema:ProductModel ;
	schema:rangeIncludes schema:ProductModel ;
	rdfs:comment "A pointer from a newer variant of a product  to its previous, often discontinued predecessor." .

schema:sugarContent a rdf:Property ;
	rdfs:label "sugarContent" ;
	schema:domainIncludes schema:NutritionInformation ;
	schema:rangeIncludes schema:Mass ;
	rdfs:comment "The number of grams of sugar." .

schema:suggestedGender a rdf:Property ;
	rdfs:label "suggestedGender" ;
	schema:domainIncludes schema:PeopleAudience ;
	schema:rangeIncludes schema:Text ;
	rdfs:comment "The gender of the person or audience." .

schema:suggestedMaxAge a rdf:Property ;
	rdfs:label "suggestedMaxAge" ;
	schema:domainIncludes schema:PeopleAudience ;
	schema:rangeIncludes schema:Number ;
	rdfs:comment "Maximal age recommended for viewing content" .

schema:suggestedMinAge a rdf:Property ;
	rdfs:label "suggestedMinAge" ;
	schema:domainIncludes schema:PeopleAudience ;
	schema:rangeIncludes schema:Number ;
	rdfs:comment "Minimal age recommended for viewing content" .

schema:superEvent a rdf:Property ;
	rdfs:label "superEvent" ;
	schema:domainIncludes schema:Event ;
	schema:rangeIncludes schema:Event ;
	rdfs:comment "An event that this event is a part of. For example, a collection of individual music performances might each have a music festival as their superEvent." .

schema:supplyTo a rdf:Property ;
	rdfs:label "supplyTo" ;
	schema:domainIncludes schema:Artery ;
	schema:rangeIncludes schema:AnatomicalStructure ;
	rdfs:comment "The area to which the artery supplies blood to." .

schema:targetDescription a rdf:Property ;
	rdfs:label "targetDescription" ;
	schema:domainIncludes schema:AlignmentObject ;
	schema:rangeIncludes schema:Text ;
	rdfs:comment "The description of a node in an established educational framework." .

schema:targetName a rdf:Property ;
	rdfs:label "targetName" ;
	schema:domainIncludes schema:AlignmentObject ;
	schema:rangeIncludes schema:Text ;
	rdfs:comment "The name of a node in an established educational framework." .

schema:targetPlatform a rdf:Property ;
	rdfs:label "targetPlatform" ;
	schema:domainIncludes schema:APIReference ;
	schema:rangeIncludes schema:Text ;
	rdfs:comment "Type of app development: phone, Metro style, desktop, XBox, etc." .

schema:targetPopulation a rdf:Property ;
	rdfs:label "targetPopulation" ;
	schema:domainIncludes schema:DietarySupplement , schema:DoseSchedule ;
	schema:rangeIncludes schema:Text ;
	rdfs:comment "Characteristics of the population for which this is intended, or which typically uses it, e.g. 'adults'." .

schema:targetProduct a rdf:Property ;
	rdfs:label "targetProduct" ;
	schema:domainIncludes schema:Code ;
	schema:rangeIncludes schema:SoftwareApplication ;
	rdfs:comment "Target Operating System / Product to which the code applies.  If applies to several versions, just the product name can be used." .

schema:targetUrl a rdf:Property ;
	rdfs:label "targetUrl" ;
	schema:domainIncludes schema:AlignmentObject ;
	schema:rangeIncludes schema:URL ;
	rdfs:comment "The URL of a node in an established educational framework." .

schema:taxID a rdf:Property ;
	rdfs:label "taxID" ;
	schema:domainIncludes schema:Organization , schema:Person ;
	schema:rangeIncludes schema:Text ;
	rdfs:comment "The Tax / Fiscal ID of the organization or person, e.g. the TIN in the US or the CIF/NIF in Spain." .

schema:telephone a rdf:Property ;
	rdfs:label "telephone" ;
	schema:domainIncludes schema:ContactPoint , schema:Organization , schema:Person , schema:Place ;
	schema:rangeIncludes schema:Text ;
	rdfs:comment "The telephone number." .

schema:temporal a rdf:Property ;
	rdfs:label "temporal" ;
	schema:domainIncludes schema:Dataset ;
	schema:rangeIncludes schema:DateTime ;
	rdfs:comment "The range of temporal applicability of a dataset, e.g. for a 2011 census dataset, the year 2011 (in ISO 8601 time interval format)." .

schema:text a rdf:Property ;
	rdfs:label "text" ;
	schema:domainIncludes schema:CreativeWork ;
	schema:rangeIncludes schema:Text ;
	rdfs:comment "The textual content of this CreativeWork." .

schema:thumbnail a rdf:Property ;
	rdfs:label "thumbnail" ;
	schema:domainIncludes schema:ImageObject , schema:VideoObject ;
	schema:rangeIncludes schema:ImageObject ;
	rdfs:comment "Thumbnail image for an image or video." .

schema:thumbnailUrl a rdf:Property ;
	rdfs:label "thumbnailUrl" ;
	schema:domainIncludes schema:CreativeWork ;
	schema:rangeIncludes schema:URL ;
	rdfs:comment "A thumbnail image relevant to the Thing." .

schema:tickerSymbol a rdf:Property ;
	rdfs:label "tickerSymbol" ;
	schema:domainIncludes schema:Corporation ;
	schema:rangeIncludes schema:Text ;
	rdfs:comment "The exchange traded instrument associated with a Corporation object. The tickerSymbol is expressed as an exchange and an instrument name separated by a space character. For the exchange component of the tickerSymbol attribute, we reccommend using the controlled vocaulary of Market Identifier Codes (MIC) specified in ISO15022." .

schema:timeRequired a rdf:Property ;
	rdfs:label "timeRequired" ;
	schema:domainIncludes schema:CreativeWork ;
	schema:rangeIncludes schema:Duration ;
	rdfs:comment "Approximate or typical time it takes to work with or through this learning resource for the typical intended target audience, e.g. 'P30M', 'P1H25M'." .

schema:tissueSample a rdf:Property ;
	rdfs:label "tissueSample" ;
	schema:domainIncludes schema:PathologyTest ;
	schema:rangeIncludes schema:Text ;
	rdfs:comment "The type of tissue sample required for the test." .

schema:title a rdf:Property ;
	rdfs:label "title" ;
	schema:domainIncludes schema:JobPosting ;
	schema:rangeIncludes schema:Text ;
	rdfs:comment "The title of the job." .

schema:toLocation a rdf:Property ;
	rdfs:label "toLocation" ;
	schema:domainIncludes schema:ExerciseAction , schema:InsertAction , schema:MoveAction , schema:TransferAction ;
	schema:rangeIncludes schema:Number , schema:Place ;
	rdfs:comment "A sub property of location. The final location of the object or the agent after the action." .

schema:totalTime a rdf:Property ;
	rdfs:label "totalTime" ;
	schema:domainIncludes schema:Recipe ;
	schema:rangeIncludes schema:Duration ;
	rdfs:comment "The total time it takes to prepare and cook the recipe, in <a href='http://en.wikipedia.org/wiki/ISO_8601'>ISO 8601 duration format</a>." .

schema:track a rdf:Property ;
	rdfs:label "track" ;
	schema:domainIncludes schema:MusicGroup , schema:MusicPlaylist ;
	schema:rangeIncludes schema:MusicRecording ;
	rdfs:comment "A music recording (track)&#x2014;usually a single song." .

schema:tracks a rdf:Property ;
	rdfs:label "tracks" ;
	schema:domainIncludes schema:MusicGroup , schema:MusicPlaylist ;
	schema:rangeIncludes schema:MusicRecording ;
	rdfs:comment "A music recording (track)&#x2014;usually a single song (legacy spelling; see singular form, track)." .

schema:trailer a rdf:Property ;
	rdfs:label "trailer" ;
	schema:domainIncludes schema:Movie , schema:TVEpisode , schema:TVSeason , schema:TVSeries ;
	schema:rangeIncludes schema:VideoObject ;
	rdfs:comment "The trailer of the movie or TV series, season, or episode." .

schema:transFatContent a rdf:Property ;
	rdfs:label "transFatContent" ;
	schema:domainIncludes schema:NutritionInformation ;
	schema:rangeIncludes schema:Mass ;
	rdfs:comment "The number of grams of trans fat." .

schema:transcript a rdf:Property ;
	rdfs:label "transcript" ;
	schema:domainIncludes schema:AudioObject , schema:VideoObject ;
	schema:rangeIncludes schema:Text ;
	rdfs:comment "If this MediaObject is an AudioObject or VideoObject, the transcript of that object." .

schema:transmissionMethod a rdf:Property ;
	rdfs:label "transmissionMethod" ;
	schema:domainIncludes schema:InfectiousDisease ;
	schema:rangeIncludes schema:Text ;
	rdfs:comment "How the disease spreads, either as a route or vector, for example 'direct contact', 'Aedes aegypti', etc." .

schema:trialDesign a rdf:Property ;
	rdfs:label "trialDesign" ;
	schema:domainIncludes schema:MedicalTrial ;
	schema:rangeIncludes schema:MedicalTrialDesign ;
	rdfs:comment "Specifics about the trial design (enumerated)." .

schema:tributary a rdf:Property ;
	rdfs:label "tributary" ;
	schema:domainIncludes schema:Vein ;
	schema:rangeIncludes schema:AnatomicalStructure ;
	rdfs:comment "The anatomical or organ system that the vein flows into; a larger structure that the vein connects to." .

schema:typeOfGood a rdf:Property ;
	rdfs:label "typeOfGood" ;
	schema:domainIncludes schema:OwnershipInfo , schema:TypeAndQuantityNode ;
	schema:rangeIncludes schema:Product ;
	rdfs:comment "The product that this structured value is referring to." .

schema:typicalAgeRange a rdf:Property ;
	rdfs:label "typicalAgeRange" ;
	schema:domainIncludes schema:CreativeWork ;
	schema:rangeIncludes schema:Text ;
	rdfs:comment "The typical range of ages the content's intendedEndUser, for example '7-9', '11-'." .

schema:typicalTest a rdf:Property ;
	rdfs:label "typicalTest" ;
	schema:domainIncludes schema:MedicalCondition ;
	schema:rangeIncludes schema:MedicalTest ;
	rdfs:comment "A medical test typically performed given this condition." .

schema:unitCode a rdf:Property ;
	rdfs:label "unitCode" ;
	schema:domainIncludes schema:QuantitativeValue , schema:TypeAndQuantityNode , schema:UnitPriceSpecification ;
	schema:rangeIncludes schema:Text ;
	rdfs:comment "The unit of measurement given using the UN/CEFACT Common Code (3 characters)." .

schema:unsaturatedFatContent a rdf:Property ;
	rdfs:label "unsaturatedFatContent" ;
	schema:domainIncludes schema:NutritionInformation ;
	schema:rangeIncludes schema:Mass ;
	rdfs:comment "The number of grams of unsaturated fat." .

schema:uploadDate a rdf:Property ;
	rdfs:label "uploadDate" ;
	schema:domainIncludes schema:MediaObject ;
	schema:rangeIncludes schema:Date ;
	rdfs:comment "Date when this media object was uploaded to this site." .

schema:url a rdf:Property ;
	rdfs:label "url" ;
	schema:domainIncludes schema:Thing ;
	schema:rangeIncludes schema:URL ;
	rdfs:comment "URL of the item." .

schema:usedToDiagnose a rdf:Property ;
	rdfs:label "usedToDiagnose" ;
	schema:domainIncludes schema:MedicalTest ;
	schema:rangeIncludes schema:MedicalCondition ;
	rdfs:comment "A condition the test is used to diagnose." .

schema:usesDevice a rdf:Property ;
	rdfs:label "usesDevice" ;
	schema:domainIncludes schema:MedicalTest ;
	schema:rangeIncludes schema:MedicalDevice ;
	rdfs:comment "Device used to perform the test." .

schema:validFrom a rdf:Property ;
	rdfs:label "validFrom" ;
	schema:domainIncludes schema:Demand , schema:Offer , schema:OpeningHoursSpecification , schema:PriceSpecification ;
	schema:rangeIncludes schema:DateTime ;
	rdfs:comment "The beginning of the validity of offer, price specification, or opening hours data." .

schema:validThrough a rdf:Property ;
	rdfs:label "validThrough" ;
	schema:domainIncludes schema:Demand , schema:Offer , schema:OpeningHoursSpecification , schema:PriceSpecification ;
	schema:rangeIncludes schema:DateTime ;
	rdfs:comment "The end of the validity of offer, price specification, or opening hours data." .

schema:value a rdf:Property ;
	rdfs:label "value" ;
	schema:domainIncludes schema:QuantitativeValue ;
	schema:rangeIncludes schema:Number ;
	rdfs:comment "The value of the product characteristic." .

schema:valueAddedTaxIncluded a rdf:Property ;
	rdfs:label "valueAddedTaxIncluded" ;
	schema:domainIncludes schema:PriceSpecification ;
	schema:rangeIncludes schema:Boolean ;
	rdfs:comment "Specifies whether the applicable value-added tax (VAT) is included in the price specification or not." .

schema:valueReference a rdf:Property ;
	rdfs:label "valueReference" ;
	schema:domainIncludes schema:QualitativeValue , schema:QuantitativeValue ;
	schema:rangeIncludes schema:Enumeration , schema:StructuredValue ;
	rdfs:comment "A pointer to a secondary value that provides additional information on the original value, e.g. a reference temperature." .

schema:vatID a rdf:Property ;
	rdfs:label "vatID" ;
	schema:domainIncludes schema:Organization , schema:Person ;
	schema:rangeIncludes schema:Text ;
	rdfs:comment "The Value-added Tax ID of the organisation or person." .

schema:vendor a rdf:Property ;
	rdfs:label "vendor" ;
	schema:domainIncludes schema:BuyAction ;
	schema:rangeIncludes schema:Organization , schema:Person ;
	rdfs:comment "A sub property of participant. The seller.The participant/person/organization that sold the object." .

schema:version a rdf:Property ;
	rdfs:label "version" ;
	schema:domainIncludes schema:CreativeWork ;
	schema:rangeIncludes schema:Number ;
	rdfs:comment "The version of the CreativeWork embodied by a specified resource." .

schema:video a rdf:Property ;
	rdfs:label "video" ;
	schema:domainIncludes schema:CreativeWork ;
	schema:rangeIncludes schema:VideoObject ;
	rdfs:comment "An embedded video object." .

schema:videoFrameSize a rdf:Property ;
	rdfs:label "videoFrameSize" ;
	schema:domainIncludes schema:VideoObject ;
	schema:rangeIncludes schema:Text ;
	rdfs:comment "The frame size of the video." .

schema:videoQuality a rdf:Property ;
	rdfs:label "videoQuality" ;
	schema:domainIncludes schema:VideoObject ;
	schema:rangeIncludes schema:Text ;
	rdfs:comment "The quality of the video." .

schema:warning a rdf:Property ;
	rdfs:label "warning" ;
	schema:domainIncludes schema:Drug ;
	schema:rangeIncludes schema:Text , schema:URL ;
	rdfs:comment "Any FDA or other warnings about the drug (text or URL)." .

schema:warranty a rdf:Property ;
	rdfs:label "warranty" ;
	schema:domainIncludes schema:Demand , schema:Offer ;
	schema:rangeIncludes schema:WarrantyPromise ;
	rdfs:comment "The warranty promise(s) included in the offer." .

schema:warrantyPromise a rdf:Property ;
	rdfs:label "warrantyPromise" ;
	schema:domainIncludes schema:BuyAction , schema:SellAction ;
	schema:rangeIncludes schema:WarrantyPromise ;
	rdfs:comment "The warranty promise(s) included in the offer." .

schema:warrantyScope a rdf:Property ;
	rdfs:label "warrantyScope" ;
	schema:domainIncludes schema:WarrantyPromise ;
	schema:rangeIncludes schema:WarrantyScope ;
	rdfs:comment "The scope of the warranty promise." .

schema:weight a rdf:Property ;
	rdfs:label "weight" ;
	schema:domainIncludes schema:Product ;
	schema:rangeIncludes schema:QuantitativeValue ;
	rdfs:comment "The weight of the product." .

schema:width a rdf:Property ;
	rdfs:label "width" ;
	schema:domainIncludes schema:MediaObject , schema:Product ;
	schema:rangeIncludes schema:Distance , schema:QuantitativeValue ;
	rdfs:comment "The width of the item." .

schema:winner a rdf:Property ;
	rdfs:label "winner" ;
	schema:domainIncludes schema:LoseAction ;
	schema:rangeIncludes schema:Person ;
	rdfs:comment "A sub property of participant. The winner of the action." .

schema:wordCount a rdf:Property ;
	rdfs:label "wordCount" ;
	schema:domainIncludes schema:Article ;
	schema:rangeIncludes schema:Integer ;
	rdfs:comment "The number of words in the text of the Article." .

schema:workHours a rdf:Property ;
	rdfs:label "workHours" ;
	schema:domainIncludes schema:JobPosting ;
	schema:rangeIncludes schema:Text ;
	rdfs:comment "The typical working hours for this job (e.g. 1st shift, night shift, 8am-5pm)." .

schema:workLocation a rdf:Property ;
	rdfs:label "workLocation" ;
	schema:domainIncludes schema:Person ;
	schema:rangeIncludes schema:ContactPoint , schema:Place ;
	rdfs:comment "A contact location for a person's place of work." .

schema:workload a rdf:Property ;
	rdfs:label "workload" ;
	schema:domainIncludes schema:ExercisePlan ;
	schema:rangeIncludes schema:Energy ;
	rdfs:comment "Quantitative measure of the physiologic output of the exercise; also referred to as energy expenditure." .

schema:worksFor a rdf:Property ;
	rdfs:label "worksFor" ;
	schema:domainIncludes schema:Person ;
	schema:rangeIncludes schema:Organization ;
	rdfs:comment "Organizations that the person works for." .

schema:worstRating a rdf:Property ;
	rdfs:label "worstRating" ;
	schema:domainIncludes schema:Rating ;
	schema:rangeIncludes schema:Number , schema:Text ;
	rdfs:comment "The lowest value allowed in this rating system. If worstRating is omitted, 1 is assumed." .

<http://www.w3.org/wiki/WebSchemas/SchemaDotOrgSources#source_GoodRelationsProperties> a schema:Organization ;
	rdfs:label "GoodRelationsProperties" ;
	rdfs:comment "This class contains derivatives of properties from the GoodRelations Vocabulary for E-Commerce, created by Martin Hepp. GoodRelations is a data model for sharing e-commerce data on the Web that can be expressed in a variety of syntaxes, including RDFa and HTML5 Microdata. More information about GoodRelations can be found at <a href=\"http://purl.org/goodrelations/\">http://purl.org/goodrelations/</a>." .

<http://www.w3.org/wiki/WebSchemas/SchemaDotOrgSources#source_LRMIClass> a schema:Organization ;
	rdfs:label "LRMIClass" ;
	rdfs:comment "This class is based on the work of the LRMI project, see lrmi.net for details." .

<http://www.w3.org/wiki/WebSchemas/SchemaDotOrgSources#source_DatasetClass> a schema:Organization ;
	rdfs:label "DatasetClass" ;
	rdfs:comment "This class is based upon W3C DCAT work, and benefits from collaboration around the DCAT, ADMS and VoID vocabularies. See http://www.w3.org/wiki/WebSchemas/Datasets for full details and mappings." .

<http://www.w3.org/wiki/WebSchemas/SchemaDotOrgSources#source_rNews> a schema:Organization ;
	rdfs:label "rNews" ;
	rdfs:comment "This class contains derivatives of IPTC rNews properties. rNews is a data model of publishing metadata with serializations currently available for RDFa as well as HTML5 Microdata. More information about the IPTC and rNews can be found at <a href=http://rnews.org>rnews.org</a>." .

<http://www.w3.org/wiki/WebSchemas/SchemaDotOrgSources#source_GoodRelationsClass> a schema:Organization ;
	rdfs:label "GoodRelationsClass" ;
	rdfs:comment "This class is derived from the GoodRelations Vocabulary for E-Commerce, created by Martin Hepp. GoodRelations is a data model for sharing e-commerce data on the Web that can be expressed in a variety of syntaxes, including RDFa and HTML5 Microdata. More information about GoodRelations can be found at <a href=\"http://purl.org/goodrelations/\">http://purl.org/goodrelations/</a>." .

<http://www.w3.org/wiki/WebSchemas/SchemaDotOrgSources#source_WikiDoc> a schema:Organization ;
	rdfs:label "WikiDoc" ;
	rdfs:comment "This class contains information contributed by <a href=http://wikidoc.org>WikiDoc</a>." .
