@prefix dc: <http://purl.org/dc/elements/1.1/> .
@prefix adms: <http://www.w3.org/ns/adms#> .
@prefix rdfs: <http://www.w3.org/2000/01/rdf-schema#> .
@prefix cogs: <http://vocab.deri.ie/cogs#> .
@prefix foaf: <http://xmlns.com/foaf/0.1/> .
@prefix xsd: <http://www.w3.org/2001/XMLSchema#> .
@prefix owl: <http://www.w3.org/2002/07/owl#> .
@prefix vann: <http://purl.org/vocab/vann/> .
@prefix rdf: <http://www.w3.org/1999/02/22-rdf-syntax-ns#> .
@prefix dcterms: <http://purl.org/dc/terms/> .

<http://vocab.deri.ie/cogs> a owl:Ontology , adms:SemanticAsset ;
	dcterms:title "COGS Vocabulary" ;
	dcterms:description "COGS: Vocabulary for describing ETL and data transformation activities." ;
	dcterms:modified "2013-12-08"^^xsd:date ;
	vann:preferredNamespaceUri "http://vocab.deri.ie/cogs#" ;
	vann:preferredNamespacePrefix "cogs" ;
	foaf:homepage <http://vocab.deri.ie/cogs.html> ;
	dcterms:created "2013-12-08"^^xsd:date ;
	dcterms:publisher "http://vocab.deri.ie/cogs#DERI%2C%20NUI%20Galway" ;
	dcterms:partOf <http://vocab.deri.ie> ;
	dcterms:type <http://purl.org/adms/assettype/Ontology> ;
	dcterms:status <http://purl.org/adms/status/UnderDevelopment> ;
	dc:creator cogs:andfre , cogs:benkam .

cogs:ttl a adms:SemanticDistribution ;
	dcterms:FileFormat <http://www.w3.org/1999/02/22-rdf-syntax-ns> ;
	adms:accessURL "http://vocab.deri.ie/cogs.ttl" ;
	adms:status <http://purl.org/adms/status/Completed> .

cogs:rdf a adms:SemanticDistribution ;
	dcterms:FileFormat <http://www.w3.org/1999/02/22-rdf-syntax-ns> ;
	adms:accessURL "http://vocab.deri.ie/cogs.rdf" ;
	adms:status <http://purl.org/adms/status/Completed> .

cogs:andfre a foaf:Person ;
	foaf:name "André Freitas" ;
	foaf:homepage <http://www.w3.org/1999/02/22-rdf-syntax-ns> .

cogs:DERI%2C%20NUI%20Galway a dcterms:Agent ;
	foaf:member cogs:andfre ;
	foaf:name "DERI, NUI Galway" ;
	foaf:homepage <http://www.deri.ie/> .

cogs:benkam a foaf:Person ;
	foaf:name "Benedikt Kämpgen" ;
	foaf:homepage <http://www.w3.org/1999/02/22-rdf-syntax-ns> .

cogs:AIFB%2FKIT a dcterms:Agent ;
	foaf:member cogs:benkam ;
	foaf:name "AIFB/KIT" ;
	foaf:homepage <http://www.kit.edu/> .

cogs:WebServiceLookup a rdfs:Class , owl:Class ;
	rdfs:label "WebServiceLookup" ;
	rdfs:comment "Allows the retrieving of data from a web service and uses this during the form filling process.  @en-us" ;
	rdfs:subClassOf cogs:Lookup .

cogs:View a rdfs:Class , owl:Class ;
	rdfs:label "View" ;
	rdfs:comment "Consists of a stored query accessible as a virtual table composed of the result set of a query. @en-us" ;
	rdfs:subClassOf cogs:Object .

cogs:ValueOperation a rdfs:Class , owl:Class ;
	rdfs:label "ValueOperation" ;
	rdfs:comment "Evaluate a selected function for a particular value of x. @en-us" ;
	rdfs:subClassOf cogs:Operation .

cogs:ValueCalculation a rdfs:Class , owl:Class ;
	rdfs:label "ValueCalculation" ;
	rdfs:comment "A value that results from some sort of calculation performed on a specified input value. " ;
	rdfs:subClassOf cogs:ValueOperation .

cogs:Validation a rdfs:Class , owl:Class ;
	rdfs:label "Validation" ;
	rdfs:comment "The act of validating; finding or testing the truth of something. @en-us" ;
	rdfs:subClassOf cogs:Transformation .

cogs:Uppercase a rdfs:Class , owl:Class ;
	rdfs:label "Uppercase" ;
	rdfs:comment "String operation for converting a string to uppercase. @en-us" ;
	rdfs:subClassOf cogs:StringOperation .

cogs:UpdateQueryObject a rdfs:Class , owl:Class ;
	rdfs:label "UpdateQuery" ;
	rdfs:comment "Query that changes the data of one or more records in a table.  @en-us" ;
	rdfs:subClassOf cogs:QueryObject .

cogs:UnitConversion a rdfs:Class , owl:Class ;
	rdfs:label "UnitConversion" ;
	rdfs:comment "Units of measurement. @en-us" ;
	rdfs:subClassOf cogs:ValueOperation .

cogs:Triple a rdfs:Class , owl:Class ;
	rdfs:label "Triple" ;
	rdfs:comment "A basic RDF statement resembling the English-Language construct of (subject, predicate, object). @en-us" ;
	rdfs:subClassOf cogs:Object .

cogs:Trim a rdfs:Class , owl:Class ;
	rdfs:label "Trim" ;
	rdfs:comment "String operation for removing leading and trailing whitespace from a string. @en-us" ;
	rdfs:subClassOf cogs:StringOperation .

cogs:Trigger a rdfs:Class , owl:Class ;
	rdfs:label "Trigger" ;
	rdfs:comment "A procedural code that is automatically executed in response to certain events on a particular table or view in a database.  @en-us" ;
	rdfs:subClassOf cogs:Object .

cogs:TransformationProcess a rdfs:Class , owl:Class ;
	rdfs:label "TransformationProcess" ;
	rdfs:comment "Process that applies a series of rules or functions to the extracted data from the source to derive the data for loading into the end target. @en-us" ;
	rdfs:subClassOf cogs:Transformation .

cogs:Transformation a rdfs:Class , owl:Class ;
	rdfs:label "Transformation" ;
	rdfs:comment "The process of manipulating data. @en-us" ;
	rdfs:subClassOf owl:Thing .

cogs:TerminologicalMapping a rdfs:Class , owl:Class ;
	rdfs:label "TerminologicalMapping" ;
	rdfs:comment "Maps terminological-level (schema-level) entities. @en-us" ;
	rdfs:subClassOf cogs:Mapping .

cogs:TableLookup a rdfs:Class , owl:Class ;
	rdfs:label "TableLookup" ;
	rdfs:comment "Process of using a known value to search for data on a table. @en-us" ;
	rdfs:subClassOf cogs:Lookup .

cogs:Table a rdfs:Class , owl:Class ;
	rdfs:label "Table" ;
	rdfs:comment "A predefined format of rows and columns that define a database entity. @en-us" ;
	rdfs:subClassOf cogs:Object .

cogs:Success a rdfs:Class , owl:Class ;
	rdfs:label "Success" ;
	rdfs:comment "Status of a job that had successful  performance. @en-us" ;
	rdfs:subClassOf cogs:ExecutionStatus .

cogs:StringSimilarity a rdfs:Class , owl:Class ;
	rdfs:label "StringSimilarity" ;
	rdfs:comment "Matching based on string similarity measures. @en-us" ;
	rdfs:subClassOf cogs:SimilarityMatching .

cogs:StringOperation a rdfs:Class , owl:Class ;
	rdfs:label "StringOperation" ;
	rdfs:comment "Operations for manipulating strings. @en-us" ;
	rdfs:subClassOf cogs:ValueOperation .

cogs:StringFilter a rdfs:Class , owl:Class ;
	rdfs:label "StringFilter" ;
	rdfs:comment "Provides means for matching strings of text, such as particular characters, words, or patterns of characters. @en-us" ;
	rdfs:subClassOf cogs:Filter .

cogs:StoredProcedure a rdfs:Class , owl:Class ;
	rdfs:label "StoredProcedure" ;
	rdfs:comment "A transformation used to create unique primary key values or cycle through a sequential range of numbers to replace missing keys. @en-us" ;
	rdfs:subClassOf cogs:Object .

cogs:StagingAreaArtifact a rdfs:Class , owl:Class ;
	rdfs:label "StagingAreaArtifact" ;
	rdfs:comment "The final product; what the end users see. @en-us" ;
	rdfs:subClassOf cogs:Object .

cogs:StaggingArea a rdfs:Class , owl:Class ;
	rdfs:label "StaggingArea" ;
	rdfs:comment "A place where data can be processed before entering the warehouse area. @en-us" ;
	rdfs:subClassOf cogs:DataManagementLayer .

cogs:SplitColumn a rdfs:Class , owl:Class ;
	rdfs:label "SplitColumn" ;
	rdfs:comment "Divides a column in one or more other columns. @en-us" ;
	rdfs:subClassOf cogs:ColumnOperation .

cogs:Split a rdfs:Class , owl:Class ;
	rdfs:label "Split" ;
	rdfs:comment "String operation that returns a zero-based, one-dimensional array containing a specified number of substrings. @en-us" ;
	rdfs:subClassOf cogs:StringOperation .

cogs:Source a rdfs:Class , owl:Class ;
	rdfs:label "Source" ;
	rdfs:comment "A database, application, file or other storage facility from which the data is derived. @en-us" ;
	rdfs:subClassOf cogs:DataManagementLayer .

cogs:SortRow a rdfs:Class , owl:Class ;
	rdfs:label "SortRow" ;
	rdfs:comment "Row Operation that sorts rows based on a specified fields and on whether they should be sorted in ascending or descending order. @en-us" ;
	rdfs:subClassOf cogs:RowOperation .

cogs:SimilarityMatching a rdfs:Class , owl:Class ;
	rdfs:label "SimilarityMatching" ;
	rdfs:comment "The process of matching two objects by a similarity measure. @en-us" ;
	rdfs:subClassOf cogs:AutomatedMatching .

cogs:Service a rdfs:Class , owl:Class ;
	rdfs:label "Service" ;
	rdfs:comment "Action done by a device or user with the function of giving good by providing usefulness. @en-us" ;
	rdfs:subClassOf cogs:Object .

cogs:Server a rdfs:Class , owl:Class ;
	rdfs:label "Server" ;
	rdfs:comment "Software program, or the computer on which that program runs, that provides a specific kind of service to a client software. @en-us" ;
	rdfs:subClassOf cogs:Object .

cogs:Sensor a rdfs:Class , owl:Class ;
	rdfs:label "Sensor" ;
	rdfs:comment "Device that measures or detects a real-world condition and converts the condition into an analog or digital representation. @en-us" ;
	rdfs:subClassOf cogs:Object .

cogs:SemanticSimilarity a rdfs:Class , owl:Class ;
	rdfs:label "SemanticSimilarity" ;
	rdfs:comment "Matching by a measure of semantic similarity. @en-us" ;
	rdfs:subClassOf cogs:SimilarityMatching .

cogs:SelectQueryObject a rdfs:Class , owl:Class ;
	rdfs:label "SelectQuery" ;
	rdfs:comment "Query that locates and displays information requested. @en-us" ;
	rdfs:subClassOf cogs:QueryObject .

cogs:Script a rdfs:Class , owl:Class ;
	rdfs:label "Script" ;
	rdfs:comment "A program or sequence of instructions that is interpreted or carried out by another program rather than by the computer processor. @en-us" ;
	rdfs:subClassOf cogs:Object .

cogs:Schema a rdfs:Class , owl:Class ;
	rdfs:label "Schema" ;
	rdfs:comment "The structure of a database system described in a formal language supported by the database management system. Describes tables, for example. @en-us" ;
	rdfs:subClassOf cogs:Object .

cogs:ScheduledJob a rdfs:Class , owl:Class ;
	rdfs:label "ScheduledJob" ;
	rdfs:comment "Job that owns information on when and how often it has to execute operations. @en-us" ;
	rdfs:subClassOf cogs:Job .

cogs:Running a rdfs:Class , owl:Class ;
	rdfs:label "Running" ;
	rdfs:comment "Status of a job that is in the state of being operated. @en-us" ;
	rdfs:subClassOf cogs:ExecutionStatus .

cogs:RulesBasedMatching a rdfs:Class , owl:Class ;
	rdfs:label "RulesBasedMatching" ;
	rdfs:comment "Matching of data based on a rule or group of rules. @en-us" ;
	rdfs:subClassOf cogs:AutomatedMatching .

cogs:Rule a rdfs:Class , owl:Class ;
	rdfs:label "Rule" ;
	rdfs:comment "A principle or formula. @en-us" ;
	rdfs:subClassOf cogs:Object .

cogs:RowOperation a rdfs:Class , owl:Class ;
	rdfs:label "RowOperation" ;
	rdfs:comment "Instructions executed on rows of a table or file. @en-us" ;
	rdfs:subClassOf cogs:Operation .

cogs:Row a rdfs:Class , owl:Class ;
	rdfs:label "Row" ;
	rdfs:comment "A serie of objects placed in line. @en-us" ;
	rdfs:subClassOf cogs:Object .

cogs:Round a rdfs:Class , owl:Class ;
	rdfs:label "Round" ;
	rdfs:comment "Round a numeric value to a close number by following a specific rounding criteria. @en-us" ;
	rdfs:subClassOf cogs:NumericOperation .

cogs:Replace a rdfs:Class , owl:Class ;
	rdfs:label "Replace" ;
	rdfs:comment "String operation for updating the content of a string. @en-us" ;
	rdfs:subClassOf cogs:StringOperation .

cogs:RenameColumn a rdfs:Class , owl:Class ;
	rdfs:label "RenameColumn" ;
	rdfs:comment "Changes the name of a certain column. @en-us" ;
	rdfs:subClassOf cogs:ColumnOperation .

cogs:RejectedData a rdfs:Class , owl:Class ;
	rdfs:label "RejectedData" ;
	rdfs:comment "Data that contain database violations and are forbidden to get inserted into a table. @en-us" ;
	rdfs:subClassOf cogs:Object .

cogs:RegexFilter a rdfs:Class , owl:Class ;
	rdfs:label "RegexFilter" ;
	rdfs:comment "Filter written in a formal language that can be interpreted by a regular expression processor. @en-us" ;
	rdfs:subClassOf cogs:Filter .

cogs:RESTLookup a rdfs:Class , owl:Class ;
	rdfs:label "RESTLookup" ;
	rdfs:comment "Lookup on a REST service. @en-us" ;
	rdfs:subClassOf cogs:Lookup .

cogs:RDFObjectPropertyMapping a rdfs:Class , owl:Class ;
	rdfs:label "RDFObjectPropertyMapping" ;
	rdfs:subClassOf cogs:TerminologicalMapping .

cogs:RDFNamedGraph a rdfs:Class , owl:Class ;
	rdfs:label "RDFNamedGraph" ;
	rdfs:comment "Multiple RDF graphs in a single document/repository and naming them with URIs. @en-us" ;
	rdfs:subClassOf cogs:Object .

cogs:RDFInstanceMapping a rdfs:Class , owl:Class ;
	rdfs:label "RDFInstanceMapping" ;
	rdfs:comment "Maps an instance-level element from a source to an instance-level element in a target dataset. " ;
	rdfs:subClassOf cogs:Mapping .

cogs:RDFGraph a rdfs:Class , owl:Class ;
	rdfs:label "RDFGraph" ;
	rdfs:comment "A set of RDF triples. @en-us" ;
	rdfs:subClassOf cogs:Object .

cogs:RDFDataPropertyMapping a rdfs:Class , owl:Class ;
	rdfs:label "RDFDataPropertyMapping" ;
	rdfs:subClassOf cogs:TerminologicalMapping .

cogs:QueryObject a rdfs:Class , owl:Class ;
	rdfs:label "Query" ;
	rdfs:comment "A structured object which is used to request information or perform an action in a database. @en-us" ;
	rdfs:subClassOf cogs:Object .

cogs:Query a rdfs:Class , owl:Class ;
	rdfs:label "Query" ;
	rdfs:subClassOf cogs:Operation .

cogs:Publication a rdfs:Class , owl:Class ;
	rdfs:label "Publication" ;
	rdfs:comment "The output of an ETL process which is made available to a certain public. @en-us" .

cogs:Program a rdfs:Class , owl:Class ;
	rdfs:label "Program" ;
	rdfs:comment "A sequence of instructions written to perform a specified task for a computer. @en-us" ;
	rdfs:subClassOf cogs:Object .

cogs:PresentationArea a rdfs:Class , owl:Class ;
	rdfs:label "PresentationArea" ;
	rdfs:comment "What the user sees. @en-us" ;
	rdfs:subClassOf cogs:DataAccessLayer .

cogs:Prefiltering a rdfs:Class , owl:Class ;
	rdfs:label "Prefiltering" ;
	rdfs:comment "Preliminary filtering during the extraction phase." ;
	rdfs:subClassOf cogs:Extraction .

cogs:PredefinedMatching a rdfs:Class , owl:Class ;
	rdfs:label "PredefinedMatching" ;
	rdfs:comment "Forces a matching under a certain criteria.  @en-us" ;
	rdfs:subClassOf cogs:MappingProcess .

cogs:PerformanceIndicator a rdfs:Class , owl:Class ;
	rdfs:label "PerformanceIndicator" ;
	rdfs:comment "Measures used used to evaluate the success of a particular activity. " ;
	rdfs:subClassOf cogs:Execution .

cogs:Paste a rdfs:Class , owl:Class ;
	rdfs:label "Paste" ;
	rdfs:comment "To copy an object from a buffer  or clipboard to a file. @en-us" ;
	rdfs:subClassOf cogs:Operation .

cogs:Parsing a rdfs:Class , owl:Class ;
	rdfs:label "Parsing" ;
	rdfs:comment "Process of analyzing text or data, checking for correct syntax and building a  implicit in the input tokens. @en-us" ;
	rdfs:subClassOf cogs:Extraction .

cogs:Output a rdfs:Class , owl:Class ;
	rdfs:label "Output" ;
	rdfs:comment "Information, resulting from computer processing, that is delivered to a user. @en-us" ;
	rdfs:subClassOf cogs:Object .

cogs:Order a rdfs:Class , owl:Class ;
	rdfs:label "Order" ;
	rdfs:comment "Application of a specific order to a set of elemetns.  @en-us" ;
	rdfs:subClassOf cogs:Operation .

cogs:Operator a rdfs:Class , owl:Class ;
	rdfs:label "Operator" ;
	rdfs:comment "A symbol or function representing a mathematical operation. @en-us" ;
	rdfs:subClassOf cogs:Object .

cogs:Operation a rdfs:Class , owl:Class ;
	rdfs:label "Operation" ;
	rdfs:comment "Functional operations that can be done by a computer. " ;
	rdfs:subClassOf cogs:Transformation .

cogs:ObjectRepresentation a rdfs:Class , owl:Class ;
	rdfs:label "ObjectRepresentation" ;
	rdfs:comment "Internal representation of an object suitable for matching its features. @en-us" ;
	rdfs:subClassOf cogs:Object .

cogs:ObjectReference a rdfs:Class , owl:Class ;
	rdfs:label "ObjectReference" ;
	rdfs:comment "Value that enables a program to indirectly access a particular object. @en-us" ;
	rdfs:subClassOf cogs:Object .

cogs:Object a rdfs:Class , owl:Class ;
	rdfs:label "Object" ;
	rdfs:comment "Any entity that can be manipulated by the commands of a programming language, such as a value, variable, function, or data structure. " .

cogs:NumericOperation a rdfs:Class , owl:Class ;
	rdfs:label "NumericOperation" ;
	rdfs:comment "Manipulate and manage numeric data. @en-us" ;
	rdfs:subClassOf cogs:ValueOperation .

cogs:NumericCast a rdfs:Class , owl:Class ;
	rdfs:label "NumericCast" ;
	rdfs:comment "Converts an expression of one numeric data type to another. @en-us" ;
	rdfs:subClassOf cogs:NumericOperation .

cogs:Move a rdfs:Class , owl:Class ;
	rdfs:label "Move" ;
	rdfs:comment "To change in position from one point to another. @en-us" ;
	rdfs:subClassOf cogs:Operation .

cogs:Method a rdfs:Class , owl:Class ;
	rdfs:label "Method" ;
	rdfs:comment "A subroutine that is exclusively associated with a object. @en-us" ;
	rdfs:subClassOf cogs:Object .

cogs:Metadata a rdfs:Class , owl:Class ;
	rdfs:label "Metadata" ;
	rdfs:comment "Data that describe data and other structures, such as objects, business rules and processes. @en-us" ;
	rdfs:subClassOf cogs:Object .

cogs:MergeRow a rdfs:Class , owl:Class ;
	rdfs:label "MergeRow" ;
	rdfs:comment "Row Operation that allows the comparison of two streams of rows. It is often used in situations where the source system of a data warehouse does not contain a date of last update. @en-us" ;
	rdfs:subClassOf cogs:RowOperation .

cogs:MappingProcess a rdfs:Class , owl:Class ;
	rdfs:label "MappingProcess" ;
	rdfs:comment "The process of mapping information in a source format to a destination format. @en-us" ;
	rdfs:subClassOf cogs:Mapping .

cogs:MappingFile a rdfs:Class , owl:Class ;
	rdfs:label "MappingFile" ;
	rdfs:comment "The specification of a mapping between source and target fields (e.g. RDB2RDF)." ;
	rdfs:subClassOf cogs:Object .

cogs:Mapping a rdfs:Class , owl:Class ;
	rdfs:label "Mapping" ;
	rdfs:comment "The definition of relationship and data flow between source and target objects. @en-us" ;
	rdfs:subClassOf cogs:Transformation .

cogs:ManuallyStartedJob a rdfs:Class , owl:Class ;
	rdfs:label "ManuallyStartedJob" ;
	rdfs:comment "Job that was initialized by an user. @en-us" ;
	rdfs:subClassOf cogs:Job .

cogs:ManualAdHocProcess a rdfs:Class , owl:Class ;
	rdfs:label "ManualAdHocProcess" ;
	rdfs:comment "A non-recurrent, not-frequent manual process." ;
	rdfs:subClassOf cogs:AdHocProcess .

cogs:Lowercase a rdfs:Class , owl:Class ;
	rdfs:label "Lowercase" ;
	rdfs:comment "String operation for converting a string to lowercase.@en-us" ;
	rdfs:subClassOf cogs:StringOperation .

cogs:Lookup a rdfs:Class , owl:Class ;
	rdfs:label "Lookup" ;
	rdfs:comment "A process used to look up data in a relational table, view or synonym. @en-us" ;
	rdfs:subClassOf cogs:Transformation .

cogs:Log a rdfs:Class , owl:Class ;
	rdfs:label "Log" ;
	rdfs:comment "A record of computer activity. @en-us" ;
	rdfs:subClassOf cogs:Object .

cogs:LoadingType a rdfs:Class , owl:Class ;
	rdfs:label "LoadingType" ;
	rdfs:comment "Techniques required for the movement of data from the operational environment to the data warehouse environment. @en-us" ;
	rdfs:subClassOf cogs:Loading .

cogs:LoadingProcess a rdfs:Class , owl:Class ;
	rdfs:label "LoadingProcess" ;
	rdfs:comment "Information from data sources are loaded and stored in the target data model. " ;
	rdfs:subClassOf cogs:Loading .

cogs:Loading a rdfs:Class , owl:Class ;
	rdfs:label "Loading" ;
	rdfs:comment "Stage that is responsible for loading data into the end target. @en-us" .

cogs:Layer a rdfs:Class , owl:Class ;
	rdfs:label "Layer" ;
	rdfs:comment "Each individual level. @en-us" .

cogs:LastError a rdfs:Class , owl:Class ;
	rdfs:label "LastError" ;
	rdfs:comment "Final error on a execution workflow. @en-us" ;
	rdfs:subClassOf cogs:Object .

cogs:KeyRestructuring a rdfs:Class , owl:Class ;
	rdfs:label "KeyRestructuring" ;
	rdfs:comment "Transformation of keys with built-in meanings into generic keys. @en-us" ;
	rdfs:subClassOf cogs:RowOperation .

cogs:KeyGeneration a rdfs:Class , owl:Class ;
	rdfs:label "KeyGeneration" ;
	rdfs:comment "Process of generating keys for cryptography. @en-us" ;
	rdfs:subClassOf cogs:Operation .

cogs:JoinRows a rdfs:Class , owl:Class ;
	rdfs:label "JoinRows" ;
	rdfs:comment "Row Operation that allows combinations (Cartesian product) of all rows in the input streams.@en-us" ;
	rdfs:subClassOf cogs:RowOperation .

cogs:Job a rdfs:Class , owl:Class ;
	rdfs:label "Job" ;
	rdfs:comment "The instance of a process or group of processes (workflow)." ;
	rdfs:subClassOf cogs:Execution .

cogs:InsertTriple a rdfs:Class , owl:Class ;
	rdfs:label "InsertTriple" ;
	rdfs:comment "Includes one or more triple into the store. @en-us" ;
	rdfs:subClassOf cogs:GraphOperation .

cogs:InsertRow a rdfs:Class , owl:Class ;
	rdfs:label "InsertRow" ;
	rdfs:comment "Inclusion of a row on a table. @en-us" ;
	rdfs:subClassOf cogs:RowOperation .

cogs:InsertQueryObject a rdfs:Class , owl:Class ;
	rdfs:label "InsertQuery" ;
	rdfs:comment "Query that inserts data into the database. @en-us" ;
	rdfs:subClassOf cogs:QueryObject .

cogs:InsertColumn a rdfs:Class , owl:Class ;
	rdfs:label "InsertColumn" ;
	rdfs:comment "Inserts one or more columns according to a certain criteria to a table. @en-us" ;
	rdfs:subClassOf cogs:ColumnOperation .

cogs:Input a rdfs:Class , owl:Class ;
	rdfs:label "Input" ;
	rdfs:comment "Any data entered into a computer.@en-us" ;
	rdfs:subClassOf cogs:Object .

cogs:InitialLoad a rdfs:Class , owl:Class ;
	rdfs:label "InitialLoad" ;
	rdfs:comment "Populates the tables in the data warehouse schema and verifies if the data is ready for use. @en-us" ;
	rdfs:subClassOf cogs:LoadingType .

cogs:IncrementalLoad a rdfs:Class , owl:Class ;
	rdfs:label "IncrementalLoad" ;
	rdfs:comment "Applies ongoing changes to one or more tables based on a predefined schedule. @en-us" ;
	rdfs:subClassOf cogs:LoadingType .

cogs:HumanValidation a rdfs:Class , owl:Class ;
	rdfs:label "HumanValidation" ;
	rdfs:comment "Validation performed by a person:  an user or admin. @en-us" ;
	rdfs:subClassOf cogs:Validation .

cogs:HumanMatching a rdfs:Class , owl:Class ;
	rdfs:label "HumanMatching" ;
	rdfs:subClassOf cogs:MappingProcess .

cogs:GraphOperation a rdfs:Class , owl:Class ;
	rdfs:label "GraphOperation" ;
	rdfs:comment "Instructions performed on graphs. @en-us" ;
	rdfs:subClassOf cogs:Operation .

cogs:FullRefresh a rdfs:Class , owl:Class ;
	rdfs:label "FullRefresh" ;
	rdfs:comment "Truncates all the tables and data gets loaded again. @en-us" ;
	rdfs:subClassOf cogs:LoadingType .

cogs:Formula a rdfs:Class , owl:Class ;
	rdfs:label "Formula" ;
	rdfs:comment "A rule or principle. @en-us" ;
	rdfs:subClassOf cogs:Object .

cogs:FormatRevision a rdfs:Class , owl:Class ;
	rdfs:label "FormatRevision" ;
	rdfs:comment "Reviews the file format. @en-us" ;
	rdfs:subClassOf cogs:ValueOperation .

cogs:Filter a rdfs:Class , owl:Class ;
	rdfs:label "Filter" ;
	rdfs:comment "An operation that can be used to retain rows in a mapping that do not meet specific conditions. @en-us" ;
	rdfs:subClassOf cogs:Operation .

cogs:FillDown a rdfs:Class , owl:Class ;
	rdfs:label "FillDown" ;
	rdfs:comment "Copy the contents of the topmost cells of a selected range into the cells below.@en-us" ;
	rdfs:subClassOf cogs:ColumnOperation .

cogs:FileLookup a rdfs:Class , owl:Class ;
	rdfs:label "FileLookup" ;
	rdfs:comment "The process of looking up for information in a file. @en-us" ;
	rdfs:subClassOf cogs:Lookup .

cogs:File a rdfs:Class , owl:Class ;
	rdfs:label "File" ;
	rdfs:comment "A block of arbitrary information, or resource for storing information, which is available to a computer program. @en-us" ;
	rdfs:subClassOf cogs:Object .

cogs:FieldDecoding a rdfs:Class , owl:Class ;
	rdfs:label "FieldDecoding" ;
	rdfs:comment "Performs decoding operations when you specify field-encoding function. @en-us" ;
	rdfs:subClassOf cogs:ValueOperation .

cogs:Fail a rdfs:Class , owl:Class ;
	rdfs:label "Fail" ;
	rdfs:comment "Status of a job that stops operating or functioning. @en-us" ;
	rdfs:subClassOf cogs:ExecutionStatus .

cogs:FactTable a rdfs:Class , owl:Class ;
	rdfs:label "FactTable" ;
	rdfs:comment "A table that consists of the measurements, metrics or facts of a  process. @en-us" ;
	rdfs:subClassOf cogs:Table .

cogs:Extraction a rdfs:Class , owl:Class ;
	rdfs:label "Extraction" ;
	rdfs:comment "The first part of an ETL process which involves extracting the data from source systems. @en-us" .

cogs:ExecutionStatus a rdfs:Class , owl:Class ;
	rdfs:label "ExecutionStatus" ;
	rdfs:comment "Provides the current execution status of a running process instance (a job). e.g. : fail, running, success. @en-us" ;
	rdfs:subClassOf cogs:Execution .

cogs:Execution a rdfs:Class , owl:Class ;
	rdfs:label "Execution" ;
	rdfs:comment "A carrying into effect or to completion.@en-us" .

cogs:Exception a rdfs:Class , owl:Class ;
	rdfs:label "Exception" ;
	rdfs:comment "An event, which occurs during the execution of a program, which disrupts the normal flow of the program's instructions. @en-us" ;
	rdfs:subClassOf cogs:Object .

cogs:Event a rdfs:Class , owl:Class ;
	rdfs:label "Event" ;
	rdfs:comment "An action that is usually initiated outside the scope of a program and that is handled by a piece of code inside the program. @en-us" ;
	rdfs:subClassOf cogs:Object .

cogs:Endpoint a rdfs:Class , owl:Class ;
	rdfs:label "Endpoint" ;
	rdfs:comment "Database access point as a web service (SPARQL Endpoint) . @en-us" ;
	rdfs:subClassOf cogs:Object .

cogs:DimensionTable a rdfs:Class , owl:Class ;
	rdfs:label "DimensionTable" ;
	rdfs:comment "One of the set of companion tables to a fact table. @en-us" ;
	rdfs:subClassOf cogs:Table .

cogs:Device a rdfs:Class , owl:Class ;
	rdfs:label "Device" ;
	rdfs:comment "A machine designed for a purpose. E.g.: Unit of hardware.  @en-us" ;
	rdfs:subClassOf cogs:Object .

cogs:DestructiveMerge a rdfs:Class , owl:Class ;
	rdfs:label "DestructiveMerge" ;
	rdfs:comment "Applies the incoming data to the target data and if the primary key of an incoming record marches with the key of an existing record updates the matching target record. If the incoming record is a new record without a match with any existing record, adds the incoming record to the target table. @en-us" ;
	rdfs:subClassOf cogs:LoadingType .

cogs:DeleteTriple a rdfs:Class , owl:Class ;
	rdfs:label "DeleteTriple" ;
	rdfs:comment "Deletes on or more triples into the store.@en-us" ;
	rdfs:subClassOf cogs:GraphOperation .

cogs:DeleteRow a rdfs:Class , owl:Class ;
	rdfs:label "DeleteRow" ;
	rdfs:comment "Exclusion of a single or group of rows by a certain criteria on a table. @en-us" ;
	rdfs:subClassOf cogs:RowOperation .

cogs:DeleteQueryObject a rdfs:Class , owl:Class ;
	rdfs:label "DeleteQuery" ;
	rdfs:comment "Query that does a delete operation on a row, column, table for example. @en-us" ;
	rdfs:subClassOf cogs:QueryObject .

cogs:DeleteColumn a rdfs:Class , owl:Class ;
	rdfs:label "DeleteColumn" ;
	rdfs:comment "Deletes one or more columns according to a certain criteria to a table. @en-us" ;
	rdfs:subClassOf cogs:ColumnOperation .

cogs:Deduplication a rdfs:Class , owl:Class ;
	rdfs:label "Deduplication" ;
	rdfs:comment "Data compression technique for eliminating redundant data. @en-us" ;
	rdfs:subClassOf cogs:RowOperation .

cogs:DatetimeConversion a rdfs:Class , owl:Class ;
	rdfs:label "DatetimeConversion" ;
	rdfs:subClassOf cogs:ValueOperation .

cogs:Dataset a rdfs:Class , owl:Class ;
	rdfs:label "Dataset" ;
	rdfs:comment "A collection of data, usually presented in tabular form where each column represents a particular variable and each row corresponds to a given member of the data set in question. @en-us" ;
	rdfs:subClassOf cogs:Object .

cogs:Database a rdfs:Class , owl:Class ;
	rdfs:label "Database" ;
	rdfs:comment "A database is a collection of information organized into interrelated tables of data and specifications of data objects. @en-us" ;
	rdfs:subClassOf cogs:Object .

cogs:DataStream a rdfs:Class , owl:Class ;
	rdfs:label "DataStream" ;
	rdfs:comment "A sequence of digitally encoded coherent signals (packets of data) used to transmit or receive information that is in the process of being transmitted. @en-us" ;
	rdfs:subClassOf cogs:Object .

cogs:DataMart a rdfs:Class , owl:Class ;
	rdfs:label "DataMart" ;
	rdfs:comment "Data mart is a process-oriented subset of the overall organization’s data based on a foundation of atomic data, and that depends only on the physics of the data-measurement events, not on the anticipated user’s questions." ;
	rdfs:subClassOf cogs:Object .

cogs:DataManagementLayer a rdfs:Class , owl:Class ;
	rdfs:label "DataManagementLayer" ;
	rdfs:comment "Layer responsible for the development, execution and supervision of plans, policies, programs and practices that control, protect, deliver and enhance the value of data and information assets. @en-us" ;
	rdfs:subClassOf cogs:Layer .

cogs:DataAccessLayer a rdfs:Class , owl:Class ;
	rdfs:label "DataAccessLayer" ;
	rdfs:comment "Layer that controls access to data in a computer-based information system. @en-us" ;
	rdfs:subClassOf cogs:Layer .

cogs:DSN a rdfs:Class , owl:Class ;
	rdfs:label "DSN" ;
	rdfs:comment "Data Source Name (DSN) is a data structure that contains the information about a specific database. @en-us" ;
	rdfs:subClassOf cogs:Object .

cogs:Cube a rdfs:Class , owl:Class ;
	rdfs:label "Cube" ;
	rdfs:comment "A multidimensional database that holds data. @en-us" ;
	rdfs:subClassOf cogs:Object .

cogs:Copy a rdfs:Class , owl:Class ;
	rdfs:label "Copy" ;
	rdfs:comment "A piece of data that was duplicated. @en-us" ;
	rdfs:subClassOf cogs:Operation .

cogs:ConstructiveMerge a rdfs:Class , owl:Class ;
	rdfs:label "ConstructiveMerge" ;
	rdfs:comment "If the primary key of an incoming record matches with the key of an existing Record, leaves the existing Record, adds the incoming record and marks the added record as superseding the old record. @en-us" ;
	rdfs:subClassOf cogs:LoadingType .

cogs:ColumnOperation a rdfs:Class , owl:Class ;
	rdfs:label "ColumnOperation" ;
	rdfs:comment "Instructions applied on one or more columns. @en-us" ;
	rdfs:subClassOf cogs:Operation .

cogs:Column a rdfs:Class , owl:Class ;
	rdfs:label "Column" ;
	rdfs:comment "Database tables are composed of individual columns corresponding to the attributes of the object. @en-us" ;
	rdfs:subClassOf cogs:Object .

cogs:Class a rdfs:Class , owl:Class ;
	rdfs:label "Class" ;
	rdfs:comment "A construct that is used as a blueprint to create instances of the class. @en-us" ;
	rdfs:subClassOf cogs:Object .

cogs:CharacterSetConversion a rdfs:Class , owl:Class ;
	rdfs:label "CharacterSetConversion" ;
	rdfs:comment "Converts strings between different character sets. @en-us" ;
	rdfs:subClassOf cogs:ValueOperation .

cogs:Ceil a rdfs:Class , owl:Class ;
	rdfs:label "Ceil" ;
	rdfs:comment "Returns the smallest integer greater than or equal to n. @en-us" ;
	rdfs:subClassOf cogs:NumericOperation .

cogs:AutomatedValidation a rdfs:Class , owl:Class ;
	rdfs:label "AutomatedValidation" ;
	rdfs:comment "Validation performed by a computer. @en-us" ;
	rdfs:subClassOf cogs:Validation .

cogs:AutomatedMatching a rdfs:Class , owl:Class ;
	rdfs:label "AutomatedMatching" ;
	rdfs:comment "Task of finding entries that refer to the same entity across different data sources using computer resources. @en-us" ;
	rdfs:subClassOf cogs:MappingProcess .

cogs:AutomatedAdHocProcess a rdfs:Class , owl:Class ;
	rdfs:label "AutomatedAdHocProcess" ;
	rdfs:comment "A non-recurrent, not frequent automated process." ;
	rdfs:subClassOf cogs:AdHocProcess .

cogs:Assignment a rdfs:Class , owl:Class ;
	rdfs:label "Assignment" ;
	rdfs:comment "Sets or re-sets the value stored in the storage location(s) denoted by a variable name. @en-us" ;
	rdfs:subClassOf cogs:ValueOperation .

cogs:ApplyScript a rdfs:Class , owl:Class ;
	rdfs:label "ApplyScript" ;
	rdfs:comment "Execution of a scriptt. @en-us" ;
	rdfs:subClassOf cogs:Operation .

cogs:ApplyFormula a rdfs:Class , owl:Class ;
	rdfs:label "ApplyFormula" ;
	rdfs:comment "New data are computed based on the user-defined formula. @en-us" ;
	rdfs:subClassOf cogs:NumericOperation .

cogs:Append a rdfs:Class , owl:Class ;
	rdfs:label "Append" ;
	rdfs:comment "String operation for concatenating lists or arrays. @en-us" ;
	rdfs:subClassOf cogs:StringOperation .

cogs:AggregateRows a rdfs:Class , owl:Class ;
	rdfs:label "AggregateRows" ;
	rdfs:comment " Functions which return a single result row based on groups of rows. @en-us" ;
	rdfs:subClassOf cogs:RowOperation .

cogs:AdHocProcess a rdfs:Class , owl:Class ;
	rdfs:label "AdHocProcess" ;
	rdfs:comment "Process that seeks a solution designed for a specific problem or task, non-generalizable, and not intended to be able to be adapted to other purposes. @en-us" ;
	rdfs:subClassOf cogs:Execution .

cogs:hasStartPoint a rdf:Property ;
	rdfs:label "hasStartPoint" ;
	rdfs:comment "First process in a transformation workflow." ;
	rdfs:domain cogs:Transformation ;
	rdfs:range cogs:Transformation .

cogs:hasEndPoint a rdf:Property ;
	rdfs:label "hasEndPoint" ;
	rdfs:comment "Last process in a transformation workflow." ;
	rdfs:domain cogs:Transformation ;
	rdfs:range cogs:Transformation .

cogs:dependsOn a rdf:Property ;
	rdfs:label "dependsOn" ;
	rdfs:domain cogs:Job ;
	rdfs:range cogs:Job .

cogs:associatedGraph a rdf:Property ;
	rdfs:label "associatedGraph" ;
	rdfs:range cogs:RDFNamedGraph .

cogs:associatedEndpoint a rdf:Property ;
	rdfs:label "associatedEndpoint" ;
	rdfs:range cogs:Endpoint .

cogs:isExpressedBy a rdf:Property ;
	rdfs:label "isExpressedBy" ;
	rdfs:comment "This property allows the association between an abstract representation of a Transformation and an encapsulated computational artifact artifact (e.g. code, binary)." ;
	rdfs:domain cogs:Transformation .

cogs:precededBy a rdf:Property ;
	rdfs:label "precededBy" ;
	rdfs:comment "Defines the ordering among two processes" ;
	rdfs:subPropertyOf owl:topObjectProperty .

cogs:isPartOf a rdf:Property ;
	rdfs:label "isPartOf" ;
	rdfs:subPropertyOf owl:topObjectProperty .
