@prefix dc: <http://purl.org/dc/terms/> .
@prefix rdfs: <http://www.w3.org/2000/01/rdf-schema#> .
@prefix ns1: <http://schema.org/> .
@prefix owl: <http://www.w3.org/2002/07/owl#> .
@prefix rdf: <http://www.w3.org/1999/02/22-rdf-syntax-ns#> .

ns1:APIReference a rdfs:Class ;
	rdfs:label "APIReference" ;
	rdfs:comment "Reference documentation for application programming interfaces (APIs)." ;
	rdfs:subClassOf ns1:TechArticle .

ns1:AboutPage a rdfs:Class ;
	rdfs:label "AboutPage" ;
	rdfs:comment "Web page type: About page." ;
	rdfs:subClassOf ns1:WebPage .

ns1:AcceptAction a rdfs:Class ;
	rdfs:label "AcceptAction" ;
	rdfs:comment "The act of committing to/adopting an object.<p>Related actions:</p><ul><li><a href=\"http://schema.org/RejectAction\">RejectAction</a>: The antagonym of AcceptAction.</li></ul>" ;
	rdfs:subClassOf ns1:AllocateAction .

ns1:AccountingService a rdfs:Class ;
	rdfs:label "AccountingService" ;
	rdfs:comment "Accountancy business." ;
	rdfs:subClassOf ns1:FinancialService , ns1:ProfessionalService .

ns1:AchieveAction a rdfs:Class ;
	rdfs:label "AchieveAction" ;
	rdfs:comment "The act of accomplishing something via     previous efforts. It is an instantaneous action rather than an ongoing     process." ;
	rdfs:subClassOf ns1:Action .

ns1:Action a rdfs:Class ;
	rdfs:label "Action" ;
	dc:source <http://www.w3.org/wiki/WebSchemas/SchemaDotOrgSources#source_ActionCollabClass> ;
	rdfs:comment "An action performed by a direct agent and indirect     participants upon a direct object. Optionally happens at a location     with the help of an inanimate instrument. The execution of the action     may produce a result. Specific action sub-type documentation specifies     the exact expectation of each argument/role." ;
	rdfs:subClassOf ns1:Thing .

ns1:ActionStatusType a rdfs:Class ;
	rdfs:label "ActionStatusType" ;
	rdfs:comment "The status of an Action." ;
	rdfs:subClassOf ns1:Enumeration .

ns1:AddAction a rdfs:Class ;
	rdfs:label "AddAction" ;
	rdfs:comment "The act of editing by adding an object to a collection." ;
	rdfs:subClassOf ns1:UpdateAction .

ns1:AdministrativeArea a rdfs:Class ;
	rdfs:label "AdministrativeArea" ;
	rdfs:comment "A geographical region under the jurisdiction of a particular government." ;
	rdfs:subClassOf ns1:Place .

ns1:AdultEntertainment a rdfs:Class ;
	rdfs:label "AdultEntertainment" ;
	rdfs:comment "An adult entertainment establishment." ;
	rdfs:subClassOf ns1:EntertainmentBusiness .

ns1:AggregateOffer a rdfs:Class ;
	rdfs:label "AggregateOffer" ;
	rdfs:comment "When a single product is associated with multiple offers (for example, the same pair of shoes is offered by different merchants), then AggregateOffer can be used." ;
	rdfs:subClassOf ns1:Offer .

ns1:AggregateRating a rdfs:Class ;
	rdfs:label "AggregateRating" ;
	rdfs:comment "The average rating based on multiple ratings or reviews." ;
	rdfs:subClassOf ns1:Rating .

ns1:AgreeAction a rdfs:Class ;
	rdfs:label "AgreeAction" ;
	rdfs:comment "The act of expressing a consistency of opinion with the object. An agent agrees to/about an object (a proposition, topic or theme) with participants." ;
	rdfs:subClassOf ns1:ReactAction .

ns1:Airline a rdfs:Class ;
	rdfs:label "Airline" ;
	rdfs:comment "An organization that provides flights for passengers." ;
	rdfs:subClassOf ns1:Organization .

ns1:Airport a rdfs:Class ;
	rdfs:label "Airport" ;
	rdfs:comment "An airport." ;
	rdfs:subClassOf ns1:CivicStructure .

ns1:AlignmentObject a rdfs:Class ;
	rdfs:label "AlignmentObject" ;
	dc:source <http://www.w3.org/wiki/WebSchemas/SchemaDotOrgSources#source_LRMIClass> ;
	rdfs:comment "An intangible item that describes an alignment between a learning resource and a node in an educational framework." ;
	rdfs:subClassOf ns1:Intangible .

ns1:AllocateAction a rdfs:Class ;
	rdfs:label "AllocateAction" ;
	rdfs:comment "The act of organizing tasks/objects/events by associating resources to it." ;
	rdfs:subClassOf ns1:OrganizeAction .

ns1:AmusementPark a rdfs:Class ;
	rdfs:label "AmusementPark" ;
	rdfs:comment "An amusement park." ;
	rdfs:subClassOf ns1:EntertainmentBusiness .

ns1:AnatomicalStructure a rdfs:Class ;
	rdfs:label "AnatomicalStructure" ;
	dc:source <http://www.w3.org/wiki/WebSchemas/SchemaDotOrgSources#source_WikiDoc> ;
	rdfs:comment "Any part of the human body, typically a component of an anatomical system. Organs, tissues, and cells are all anatomical structures." ;
	rdfs:subClassOf ns1:MedicalEntity .

ns1:AnatomicalSystem a rdfs:Class ;
	rdfs:label "AnatomicalSystem" ;
	dc:source <http://www.w3.org/wiki/WebSchemas/SchemaDotOrgSources#source_WikiDoc> ;
	rdfs:comment "An anatomical system is a group of anatomical structures that work together to perform a certain task. Anatomical systems, such as organ systems, are one organizing principle of anatomy, and can includes circulatory, digestive, endocrine, integumentary, immune, lymphatic, muscular, nervous, reproductive, respiratory, skeletal, urinary, vestibular, and other systems." ;
	rdfs:subClassOf ns1:MedicalEntity .

ns1:AnimalShelter a rdfs:Class ;
	rdfs:label "AnimalShelter" ;
	rdfs:comment "Animal shelter." ;
	rdfs:subClassOf ns1:LocalBusiness .

ns1:Answer a rdfs:Class ;
	rdfs:label "Answer" ;
	dc:source <http://www.w3.org/wiki/WebSchemas/SchemaDotOrgSources#source_QAStackExchange> ;
	rdfs:comment "An answer offered to a question; perhaps correct, perhaps opinionated or wrong." ;
	rdfs:subClassOf ns1:CreativeWork .

ns1:ApartmentComplex a rdfs:Class ;
	rdfs:label "ApartmentComplex" ;
	rdfs:comment "Residence type: Apartment complex." ;
	rdfs:subClassOf ns1:Residence .

ns1:AppendAction a rdfs:Class ;
	rdfs:label "AppendAction" ;
	rdfs:comment "The act of inserting at the end if an ordered collection." ;
	rdfs:subClassOf ns1:InsertAction .

ns1:ApplyAction a rdfs:Class ;
	rdfs:label "ApplyAction" ;
	rdfs:comment "The act of registering to an organization/service without the guarantee to receive it. NOTE(goto): should this be under InteractAction instead?<p>Related actions:</p><ul><li><a href=\"http://schema.org/RegisterAction\">RegisterAction</a>: Unlike RegisterAction, ApplyAction has no guarantees that the application will be accepted.</li></ul>" ;
	rdfs:subClassOf ns1:OrganizeAction .

ns1:ApprovedIndication a rdfs:Class ;
	rdfs:label "ApprovedIndication" ;
	dc:source <http://www.w3.org/wiki/WebSchemas/SchemaDotOrgSources#source_WikiDoc> ;
	rdfs:comment "An indication for a medical therapy that has been formally specified or approved by a regulatory body that regulates use of the therapy; for example, the US FDA approves indications for most drugs in the US." ;
	rdfs:subClassOf ns1:MedicalIndication .

ns1:Aquarium a rdfs:Class ;
	rdfs:label "Aquarium" ;
	rdfs:comment "Aquarium." ;
	rdfs:subClassOf ns1:CivicStructure .

ns1:ArriveAction a rdfs:Class ;
	rdfs:label "ArriveAction" ;
	rdfs:comment "The act of arriving at a place. An agent arrives at a destination from an fromLocation, optionally with participants." ;
	rdfs:subClassOf ns1:MoveAction .

ns1:ArtGallery a rdfs:Class ;
	rdfs:label "ArtGallery" ;
	rdfs:comment "An art gallery." ;
	rdfs:subClassOf ns1:EntertainmentBusiness .

ns1:Artery a rdfs:Class ;
	rdfs:label "Artery" ;
	dc:source <http://www.w3.org/wiki/WebSchemas/SchemaDotOrgSources#source_WikiDoc> ;
	rdfs:comment "A type of blood vessel that specifically carries blood away from the heart." ;
	rdfs:subClassOf ns1:Vessel .

ns1:Article a rdfs:Class ;
	rdfs:label "Article" ;
	dc:source <http://www.w3.org/wiki/WebSchemas/SchemaDotOrgSources#source_rNews> ;
	rdfs:comment "An article, such as a news article or piece of investigative report. Newspapers and magazines have articles of many different types and this is intended to cover them all." ;
	rdfs:subClassOf ns1:CreativeWork .

ns1:AskAction a rdfs:Class ;
	rdfs:label "AskAction" ;
	rdfs:comment "The act of posing a question / favor to someone.<p>Related actions:</p><ul><li><a href=\"http://schema.org/ReplyAction\">ReplyAction</a>: Appears generally as a response to AskAction.</li></ul>" ;
	rdfs:subClassOf ns1:CommunicateAction .

ns1:AssessAction a rdfs:Class ;
	rdfs:label "AssessAction" ;
	rdfs:comment "The act of forming one's opinion, reaction or sentiment." ;
	rdfs:subClassOf ns1:Action .

ns1:AssignAction a rdfs:Class ;
	rdfs:label "AssignAction" ;
	rdfs:comment "The act of allocating an action/event/task to some destination (someone or something)." ;
	rdfs:subClassOf ns1:AllocateAction .

ns1:Attorney a rdfs:Class ;
	rdfs:label "Attorney" ;
	rdfs:comment "Professional service: Attorney." ;
	rdfs:subClassOf ns1:ProfessionalService .

ns1:Audience a rdfs:Class ;
	rdfs:label "Audience" ;
	rdfs:comment "Intended audience for an item, i.e. the group for whom the item was created." ;
	rdfs:subClassOf ns1:Intangible .

ns1:AudioObject a rdfs:Class ;
	rdfs:label "AudioObject" ;
	dc:source <http://www.w3.org/wiki/WebSchemas/SchemaDotOrgSources#source_rNews> ;
	rdfs:comment "An audio file." ;
	rdfs:subClassOf ns1:MediaObject .

ns1:AuthorizeAction a rdfs:Class ;
	rdfs:label "AuthorizeAction" ;
	rdfs:comment "The act of granting permission to an object." ;
	rdfs:subClassOf ns1:AllocateAction .

ns1:AutoBodyShop a rdfs:Class ;
	rdfs:label "AutoBodyShop" ;
	rdfs:comment "Auto body shop." ;
	rdfs:subClassOf ns1:AutomotiveBusiness .

ns1:AutoDealer a rdfs:Class ;
	rdfs:label "AutoDealer" ;
	rdfs:comment "An car dealership." ;
	rdfs:subClassOf ns1:AutomotiveBusiness .

ns1:AutoPartsStore a rdfs:Class ;
	rdfs:label "AutoPartsStore" ;
	rdfs:comment "An auto parts store." ;
	rdfs:subClassOf ns1:AutomotiveBusiness , ns1:Store .

ns1:AutoRental a rdfs:Class ;
	rdfs:label "AutoRental" ;
	rdfs:comment "A car rental business." ;
	rdfs:subClassOf ns1:AutomotiveBusiness .

ns1:AutoRepair a rdfs:Class ;
	rdfs:label "AutoRepair" ;
	rdfs:comment "Car repair business." ;
	rdfs:subClassOf ns1:AutomotiveBusiness .

ns1:AutoWash a rdfs:Class ;
	rdfs:label "AutoWash" ;
	rdfs:comment "A car wash business." ;
	rdfs:subClassOf ns1:AutomotiveBusiness .

ns1:AutomatedTeller a rdfs:Class ;
	rdfs:label "AutomatedTeller" ;
	rdfs:comment "ATM/cash machine." ;
	rdfs:subClassOf ns1:FinancialService .

ns1:AutomotiveBusiness a rdfs:Class ;
	rdfs:label "AutomotiveBusiness" ;
	rdfs:comment "Car repair, sales, or parts." ;
	rdfs:subClassOf ns1:LocalBusiness .

ns1:Bakery a rdfs:Class ;
	rdfs:label "Bakery" ;
	rdfs:comment "A bakery." ;
	rdfs:subClassOf ns1:FoodEstablishment .

ns1:BankOrCreditUnion a rdfs:Class ;
	rdfs:label "BankOrCreditUnion" ;
	rdfs:comment "Bank or credit union." ;
	rdfs:subClassOf ns1:FinancialService .

ns1:BarOrPub a rdfs:Class ;
	rdfs:label "BarOrPub" ;
	rdfs:comment "A bar or pub." ;
	rdfs:subClassOf ns1:FoodEstablishment .

ns1:Beach a rdfs:Class ;
	rdfs:label "Beach" ;
	rdfs:comment "Beach." ;
	rdfs:subClassOf ns1:CivicStructure .

ns1:BeautySalon a rdfs:Class ;
	rdfs:label "BeautySalon" ;
	rdfs:comment "Beauty salon." ;
	rdfs:subClassOf ns1:HealthAndBeautyBusiness .

ns1:BedAndBreakfast a rdfs:Class ;
	rdfs:label "BedAndBreakfast" ;
	rdfs:comment "Bed and breakfast." ;
	rdfs:subClassOf ns1:LodgingBusiness .

ns1:BefriendAction a rdfs:Class ;
	rdfs:label "BefriendAction" ;
	rdfs:comment "The act of forming a personal connection with someone (object) mutually/bidirectionally/symmetrically.<p>Related actions:</p><ul><li><a href=\"http://schema.org/FollowAction\">FollowAction</a>: Unlike FollowAction, BefriendAction implies that the connection is reciprocal.</li></ul>" ;
	rdfs:subClassOf ns1:InteractAction .

ns1:BikeStore a rdfs:Class ;
	rdfs:label "BikeStore" ;
	rdfs:comment "A bike store." ;
	rdfs:subClassOf ns1:Store .

ns1:Blog a rdfs:Class ;
	rdfs:label "Blog" ;
	rdfs:comment "A blog" ;
	rdfs:subClassOf ns1:CreativeWork .

ns1:BlogPosting a rdfs:Class ;
	rdfs:label "BlogPosting" ;
	rdfs:comment "A blog post." ;
	rdfs:subClassOf ns1:Article .

ns1:BloodTest a rdfs:Class ;
	rdfs:label "BloodTest" ;
	dc:source <http://www.w3.org/wiki/WebSchemas/SchemaDotOrgSources#source_WikiDoc> ;
	rdfs:comment "A medical test performed on a sample of a patient's blood." ;
	rdfs:subClassOf ns1:MedicalTest .

ns1:BodyOfWater a rdfs:Class ;
	rdfs:label "BodyOfWater" ;
	rdfs:comment "A body of water, such as a sea, ocean, or lake." ;
	rdfs:subClassOf ns1:Landform .

ns1:Bone a rdfs:Class ;
	rdfs:label "Bone" ;
	dc:source <http://www.w3.org/wiki/WebSchemas/SchemaDotOrgSources#source_WikiDoc> ;
	rdfs:comment "Rigid connective tissue that comprises up the skeletal structure of the human body." ;
	rdfs:subClassOf ns1:AnatomicalStructure .

ns1:Book a rdfs:Class ;
	rdfs:label "Book" ;
	rdfs:comment "A book." ;
	rdfs:subClassOf ns1:CreativeWork .

ns1:BookFormatType a rdfs:Class ;
	rdfs:label "BookFormatType" ;
	rdfs:comment "The publication format of the book." ;
	rdfs:subClassOf ns1:Enumeration .

ns1:BookStore a rdfs:Class ;
	rdfs:label "BookStore" ;
	rdfs:comment "A bookstore." ;
	rdfs:subClassOf ns1:Store .

ns1:BookmarkAction a rdfs:Class ;
	rdfs:label "BookmarkAction" ;
	rdfs:comment "An agent bookmarks/flags/labels/tags/marks an object." ;
	rdfs:subClassOf ns1:OrganizeAction .

ns1:Boolean a rdfs:Class ;
	rdfs:label "Boolean" ;
	rdfs:comment "Boolean: True or False." ;
	rdfs:subClassOf ns1:DataType .

ns1:BorrowAction a rdfs:Class ;
	rdfs:label "BorrowAction" ;
	rdfs:comment "The act of obtaining an object under an agreement to return it at a later date. Reciprocal of LendAction.<p>Related actions:</p><ul><li><a href=\"http://schema.org/LendAction\">LendAction</a>: Reciprocal of BorrowAction.</li></ul>" ;
	rdfs:subClassOf ns1:TransferAction .

ns1:BowlingAlley a rdfs:Class ;
	rdfs:label "BowlingAlley" ;
	rdfs:comment "A bowling alley." ;
	rdfs:subClassOf ns1:SportsActivityLocation .

ns1:BrainStructure a rdfs:Class ;
	rdfs:label "BrainStructure" ;
	dc:source <http://www.w3.org/wiki/WebSchemas/SchemaDotOrgSources#source_WikiDoc> ;
	rdfs:comment "Any anatomical structure which pertains to the soft nervous tissue functioning as the coordinating center of sensation and intellectual and nervous activity." ;
	rdfs:subClassOf ns1:AnatomicalStructure .

ns1:Brand a rdfs:Class ;
	rdfs:label "Brand" ;
	dc:source <http://www.w3.org/wiki/WebSchemas/SchemaDotOrgSources#source_GoodRelationsClass> ;
	rdfs:comment "A brand is a name used by an organization or business person for labeling a product, product group, or similar." ;
	rdfs:subClassOf ns1:Intangible .

ns1:Brewery a rdfs:Class ;
	rdfs:label "Brewery" ;
	rdfs:comment "Brewery." ;
	rdfs:subClassOf ns1:FoodEstablishment .

ns1:BroadcastEvent a rdfs:Class ;
	rdfs:label "BroadcastEvent" ;
	rdfs:comment "An over the air or online broadcast event." ;
	rdfs:subClassOf ns1:PublicationEvent .

ns1:BroadcastService a rdfs:Class ;
	rdfs:label "BroadcastService" ;
	rdfs:comment "A delivery service through which content is provided via broadcast over the air or online." ;
	rdfs:subClassOf ns1:Thing .

ns1:BuddhistTemple a rdfs:Class ;
	rdfs:label "BuddhistTemple" ;
	rdfs:comment "A Buddhist temple." ;
	rdfs:subClassOf ns1:PlaceOfWorship .

ns1:BusReservation a rdfs:Class ;
	rdfs:label "BusReservation" ;
	rdfs:comment "A reservation for bus travel.Note: This type is for information about actual reservations, e.g. in confirmation emails or HTML pages with individual confirmations of reservations. For offers of tickets, use http://schema.org/Offer." ;
	rdfs:subClassOf ns1:Reservation .

ns1:BusStation a rdfs:Class ;
	rdfs:label "BusStation" ;
	rdfs:comment "A bus station." ;
	rdfs:subClassOf ns1:CivicStructure .

ns1:BusStop a rdfs:Class ;
	rdfs:label "BusStop" ;
	rdfs:comment "A bus stop." ;
	rdfs:subClassOf ns1:CivicStructure .

ns1:BusTrip a rdfs:Class ;
	rdfs:label "Bus Trip" ;
	rdfs:comment "A trip on a commercial bus line." ;
	rdfs:subClassOf ns1:Intangible .

ns1:BusinessAudience a rdfs:Class ;
	rdfs:label "BusinessAudience" ;
	rdfs:comment "A set of characteristics belonging to businesses, e.g. who compose an item's target audience." ;
	rdfs:subClassOf ns1:Audience .

ns1:BusinessEntityType a rdfs:Class ;
	rdfs:label "BusinessEntityType" ;
	dc:source <http://www.w3.org/wiki/WebSchemas/SchemaDotOrgSources#source_GoodRelationsClass> ;
	rdfs:comment """A business entity type is a conceptual entity representing the legal form, the size, the main line of business, the position in the value chain, or any combination thereof, of an organization or business person.

    Commonly used values:

    http://purl.org/goodrelations/v1#Business
    http://purl.org/goodrelations/v1#Enduser
    http://purl.org/goodrelations/v1#PublicInstitution
    http://purl.org/goodrelations/v1#Reseller

    		""" ;
	rdfs:subClassOf ns1:Enumeration .

ns1:BusinessEvent a rdfs:Class ;
	rdfs:label "BusinessEvent" ;
	rdfs:comment "Event type: Business event." ;
	rdfs:subClassOf ns1:Event .

ns1:BusinessFunction a rdfs:Class ;
	rdfs:label "BusinessFunction" ;
	dc:source <http://www.w3.org/wiki/WebSchemas/SchemaDotOrgSources#source_GoodRelationsClass> ;
	rdfs:comment """The business function specifies the type of activity or access (i.e., the bundle of rights) offered by the organization or business person through the offer. Typical are sell, rental or lease, maintenance or repair, manufacture / produce, recycle / dispose, engineering / construction, or installation. Proprietary specifications of access rights are also instances of this class.

    Commonly used values:

    http://purl.org/goodrelations/v1#ConstructionInstallation
    http://purl.org/goodrelations/v1#Dispose
    http://purl.org/goodrelations/v1#LeaseOut
    http://purl.org/goodrelations/v1#Maintain
    http://purl.org/goodrelations/v1#ProvideService
    http://purl.org/goodrelations/v1#Repair
    http://purl.org/goodrelations/v1#Sell
    http://purl.org/goodrelations/v1#Buy
    		""" ;
	rdfs:subClassOf ns1:Enumeration .

ns1:BuyAction a rdfs:Class ;
	rdfs:label "BuyAction" ;
	rdfs:comment "The act of giving money to a seller in exchange for goods or services rendered. An agent buys an object, product, or service from a seller for a price. Reciprocal of SellAction." ;
	rdfs:subClassOf ns1:TradeAction .

ns1:CafeOrCoffeeShop a rdfs:Class ;
	rdfs:label "CafeOrCoffeeShop" ;
	rdfs:comment "A cafe or coffee shop." ;
	rdfs:subClassOf ns1:FoodEstablishment .

ns1:Campground a rdfs:Class ;
	rdfs:label "Campground" ;
	rdfs:comment "A campground." ;
	rdfs:subClassOf ns1:CivicStructure .

ns1:Canal a rdfs:Class ;
	rdfs:label "Canal" ;
	rdfs:comment "A canal, like the Panama Canal" ;
	rdfs:subClassOf ns1:BodyOfWater .

ns1:CancelAction a rdfs:Class ;
	rdfs:label "CancelAction" ;
	rdfs:comment "The act of asserting that a future event/action is no longer going to happen.<p>Related actions:</p><ul><li><a href=\"http://schema.org/ConfirmAction\">ConfirmAction</a>: The antagonym of CancelAction.</li></ul>" ;
	rdfs:subClassOf ns1:PlanAction .

ns1:Car a rdfs:Class ;
	rdfs:label "Car" ;
	rdfs:comment "An automobile." ;
	rdfs:subClassOf ns1:Vehicle .

ns1:Casino a rdfs:Class ;
	rdfs:label "Casino" ;
	rdfs:comment "A casino." ;
	rdfs:subClassOf ns1:EntertainmentBusiness .

ns1:CatholicChurch a rdfs:Class ;
	rdfs:label "CatholicChurch" ;
	rdfs:comment "A Catholic church." ;
	rdfs:subClassOf ns1:PlaceOfWorship .

ns1:Cemetery a rdfs:Class ;
	rdfs:label "Cemetery" ;
	rdfs:comment "A graveyard." ;
	rdfs:subClassOf ns1:CivicStructure .

ns1:CheckAction a rdfs:Class ;
	rdfs:label "CheckAction" ;
	rdfs:comment "An agent inspects/determines/investigates/inquire or examine an object's accuracy/quality/condition or state." ;
	rdfs:subClassOf ns1:FindAction .

ns1:CheckInAction a rdfs:Class ;
	rdfs:label "CheckInAction" ;
	rdfs:comment "The act of an agent communicating (service provider, social media, etc) their arrival by registering/confirming for a previously reserved service (e.g. flight check in) or at a place (e.g. hotel), possibly resulting in a result (boarding pass, etc).<p>Related actions:</p><ul><li><a href=\"http://schema.org/CheckOutAction\">CheckOutAction</a>: The antagonym of CheckInAction.</li><li><a href=\"http://schema.org/ArriveAction\">ArriveAction</a>: Unlike ArriveAction, CheckInAction implies that the agent is informing/confirming the start of a previously reserved service.</li><li><a href=\"http://schema.org/ConfirmAction\">ConfirmAction</a>: Unlike ConfirmAction, CheckInAction implies that the agent is informing/confirming the *start* of a previously reserved service rather than its validity/existence.</li></ul>" ;
	rdfs:subClassOf ns1:CommunicateAction .

ns1:CheckOutAction a rdfs:Class ;
	rdfs:label "CheckOutAction" ;
	rdfs:comment "The act of an agent communicating (service provider, social media, etc) their departure of a previously reserved service (e.g. flight check in) or place (e.g. hotel).<p>Related actions:</p><ul><li><a href=\"http://schema.org/CheckInAction\">CheckInAction</a>: The antagonym of CheckOutAction.</li><li><a href=\"http://schema.org/DepartAction\">DepartAction</a>: Unlike DepartAction, CheckOutAction implies that the agent is informing/confirming the end of a previously reserved service.</li><li><a href=\"http://schema.org/CancelAction\">CancelAction</a>: Unlike CancelAction, CheckOutAction implies that the agent is informing/confirming the end of a previously reserved service.</li></ul>" ;
	rdfs:subClassOf ns1:CommunicateAction .

ns1:CheckoutPage a rdfs:Class ;
	rdfs:label "CheckoutPage" ;
	rdfs:comment "Web page type: Checkout page." ;
	rdfs:subClassOf ns1:WebPage .

ns1:ChildCare a rdfs:Class ;
	rdfs:label "ChildCare" ;
	rdfs:comment "A Childcare center." ;
	rdfs:subClassOf ns1:LocalBusiness .

ns1:ChildrensEvent a rdfs:Class ;
	rdfs:label "ChildrensEvent" ;
	rdfs:comment "Event type: Children's event." ;
	rdfs:subClassOf ns1:Event .

ns1:ChooseAction a rdfs:Class ;
	rdfs:label "ChooseAction" ;
	rdfs:comment "The act of expressing a preference from a set of options or a large or unbounded set of choices/options." ;
	rdfs:subClassOf ns1:AssessAction .

ns1:Church a rdfs:Class ;
	rdfs:label "Church" ;
	rdfs:comment "A church." ;
	rdfs:subClassOf ns1:PlaceOfWorship .

ns1:City a rdfs:Class ;
	rdfs:label "City" ;
	rdfs:comment "A city or town." ;
	rdfs:subClassOf ns1:AdministrativeArea .

ns1:CityHall a rdfs:Class ;
	rdfs:label "CityHall" ;
	rdfs:comment "A city hall." ;
	rdfs:subClassOf ns1:GovernmentBuilding .

ns1:CivicStructure a rdfs:Class ;
	rdfs:label "CivicStructure" ;
	rdfs:comment "A public structure, such as a town hall or concert hall." ;
	rdfs:subClassOf ns1:Place .

ns1:Class a rdfs:Class ;
	rdfs:label "Class" ;
	rdfs:comment "A class, also often called a 'Type'; equivalent to rdfs:Class." ;
	rdfs:subClassOf ns1:Intangible .

ns1:Clip a rdfs:Class ;
	rdfs:label "Clip" ;
	rdfs:comment "A short TV or radio program or a segment/part of a program." ;
	rdfs:subClassOf ns1:CreativeWork .

ns1:ClothingStore a rdfs:Class ;
	rdfs:label "ClothingStore" ;
	rdfs:comment "A clothing store." ;
	rdfs:subClassOf ns1:Store .

ns1:Code a rdfs:Class ;
	rdfs:label "Code" ;
	rdfs:comment "Computer programming source code. Example: Full (compile ready) solutions, code snippet samples, scripts, templates." ;
	rdfs:subClassOf ns1:CreativeWork .

ns1:CollectionPage a rdfs:Class ;
	rdfs:label "CollectionPage" ;
	rdfs:comment "Web page type: Collection page." ;
	rdfs:subClassOf ns1:WebPage .

ns1:CollegeOrUniversity a rdfs:Class ;
	rdfs:label "CollegeOrUniversity" ;
	rdfs:comment "A college, university, or other third-level educational institution." ;
	rdfs:subClassOf ns1:EducationalOrganization .

ns1:ComedyClub a rdfs:Class ;
	rdfs:label "ComedyClub" ;
	rdfs:comment "A comedy club." ;
	rdfs:subClassOf ns1:EntertainmentBusiness .

ns1:ComedyEvent a rdfs:Class ;
	rdfs:label "ComedyEvent" ;
	rdfs:comment "Event type: Comedy event." ;
	rdfs:subClassOf ns1:Event .

ns1:Comment a rdfs:Class ;
	rdfs:label "Comment" ;
	rdfs:comment "A comment on an item - for example, a comment on a blog post. The comment's content is expressed via the \"text\" property, and its topic via \"about\", properties shared with all CreativeWorks." ;
	rdfs:subClassOf ns1:CreativeWork .

ns1:CommentAction a rdfs:Class ;
	rdfs:label "CommentAction" ;
	rdfs:comment "The act of generating a comment about a subject." ;
	rdfs:subClassOf ns1:CommunicateAction .

ns1:CommunicateAction a rdfs:Class ;
	rdfs:label "CommunicateAction" ;
	rdfs:comment "The act of conveying information to another person via a communication medium (instrument) such as speech, email, or telephone conversation." ;
	rdfs:subClassOf ns1:InteractAction .

ns1:ComputerStore a rdfs:Class ;
	rdfs:label "ComputerStore" ;
	rdfs:comment "A computer store." ;
	rdfs:subClassOf ns1:Store .

ns1:ConfirmAction a rdfs:Class ;
	rdfs:label "ConfirmAction" ;
	rdfs:comment "The act of notifying someone that a future event/action is going to happen as expected.<p>Related actions:</p><ul><li><a href=\"http://schema.org/CancelAction\">CancelAction</a>: The antagonym of ConfirmAction.</li></ul>" ;
	rdfs:subClassOf ns1:InformAction .

ns1:ConsumeAction a rdfs:Class ;
	rdfs:label "ConsumeAction" ;
	rdfs:comment "The act of ingesting information/resources/food." ;
	rdfs:subClassOf ns1:Action .

ns1:ContactPage a rdfs:Class ;
	rdfs:label "ContactPage" ;
	rdfs:comment "Web page type: Contact page." ;
	rdfs:subClassOf ns1:WebPage .

ns1:ContactPoint a rdfs:Class ;
	rdfs:label "ContactPoint" ;
	rdfs:comment "A contact point&#x2014;for example, a Customer Complaints department." ;
	rdfs:subClassOf ns1:StructuredValue .

ns1:ContactPointOption a rdfs:Class ;
	rdfs:label "ContactPointOption" ;
	rdfs:comment "Enumerated options related to a ContactPoint" ;
	rdfs:subClassOf ns1:Enumeration .

ns1:Continent a rdfs:Class ;
	rdfs:label "Continent" ;
	rdfs:comment "One of the continents (for example, Europe or Africa)." ;
	rdfs:subClassOf ns1:Landform .

ns1:ConvenienceStore a rdfs:Class ;
	rdfs:label "ConvenienceStore" ;
	rdfs:comment "A convenience store." ;
	rdfs:subClassOf ns1:Store .

ns1:CookAction a rdfs:Class ;
	rdfs:label "CookAction" ;
	rdfs:comment "The act of producing/preparing food." ;
	rdfs:subClassOf ns1:CreateAction .

ns1:Corporation a rdfs:Class ;
	rdfs:label "Corporation" ;
	dc:source <http://www.w3.org/wiki/WebSchemas/SchemaDotOrgSources#source_rNews> ;
	rdfs:comment "Organization: A business corporation." ;
	rdfs:subClassOf ns1:Organization .

ns1:Country a rdfs:Class ;
	rdfs:label "Country" ;
	rdfs:comment "A country." ;
	rdfs:subClassOf ns1:AdministrativeArea .

ns1:Courthouse a rdfs:Class ;
	rdfs:label "Courthouse" ;
	rdfs:comment "A courthouse." ;
	rdfs:subClassOf ns1:GovernmentBuilding .

ns1:CreateAction a rdfs:Class ;
	rdfs:label "CreateAction" ;
	rdfs:comment "The act of deliberately creating/producing/generating/building a result out of the agent." ;
	rdfs:subClassOf ns1:Action .

ns1:CreativeWork a rdfs:Class ;
	rdfs:label "CreativeWork" ;
	dc:source <http://www.w3.org/wiki/WebSchemas/SchemaDotOrgSources#source_rNews> ;
	rdfs:comment "The most generic kind of creative work, including books, movies, photographs, software programs, etc." ;
	rdfs:subClassOf ns1:Thing .

ns1:CreditCard a rdfs:Class ;
	rdfs:label "CreditCard" ;
	dc:source <http://www.w3.org/wiki/WebSchemas/SchemaDotOrgSources#source_GoodRelationsClass> ;
	rdfs:comment """A credit or debit card type as a standardized procedure for transferring the monetary amount for a purchase.

    Commonly used values:

    http://purl.org/goodrelations/v1#AmericanExpress
    http://purl.org/goodrelations/v1#DinersClub
    http://purl.org/goodrelations/v1#Discover
    http://purl.org/goodrelations/v1#JCB
    http://purl.org/goodrelations/v1#MasterCard
    http://purl.org/goodrelations/v1#VISA
    		""" ;
	rdfs:subClassOf ns1:PaymentMethod .

ns1:Crematorium a rdfs:Class ;
	rdfs:label "Crematorium" ;
	rdfs:comment "A crematorium." ;
	rdfs:subClassOf ns1:CivicStructure .

ns1:DDxElement a rdfs:Class ;
	rdfs:label "DDxElement" ;
	dc:source <http://www.w3.org/wiki/WebSchemas/SchemaDotOrgSources#source_WikiDoc> ;
	rdfs:comment "An alternative, closely-related condition typically considered later in the differential diagnosis process along with the signs that are used to distinguish it." ;
	rdfs:subClassOf ns1:MedicalIntangible .

ns1:DanceEvent a rdfs:Class ;
	rdfs:label "DanceEvent" ;
	rdfs:comment "Event type: A social dance." ;
	rdfs:subClassOf ns1:Event .

ns1:DanceGroup a rdfs:Class ;
	rdfs:label "DanceGroup" ;
	rdfs:comment "A dance group&#x2014;for example, the Alvin Ailey Dance Theater or Riverdance." ;
	rdfs:subClassOf ns1:PerformingGroup .

ns1:DataCatalog a rdfs:Class ;
	rdfs:label "DataCatalog" ;
	dc:source <http://www.w3.org/wiki/WebSchemas/SchemaDotOrgSources#source_DatasetClass> ;
	rdfs:comment "A collection of datasets." ;
	rdfs:subClassOf ns1:CreativeWork ;
	owl:equivalentClass <dcat:DataCatalog> .

ns1:DataDownload a rdfs:Class ;
	rdfs:label "DataDownload" ;
	dc:source <http://www.w3.org/wiki/WebSchemas/SchemaDotOrgSources#source_DatasetClass> ;
	rdfs:comment "A dataset in downloadable form." ;
	rdfs:subClassOf ns1:MediaObject ;
	owl:equivalentClass <dcat:Distribution> .

ns1:DataType a rdfs:Class ;
	rdfs:label "DataType" ;
	rdfs:comment "The basic data types such as Integers, Strings, etc." .

ns1:Dataset a rdfs:Class ;
	rdfs:label "Dataset" ;
	dc:source <http://www.w3.org/wiki/WebSchemas/SchemaDotOrgSources#source_DatasetClass> ;
	rdfs:comment "A body of structured information describing some topic(s) of interest." ;
	rdfs:subClassOf ns1:CreativeWork ;
	owl:equivalentClass <dc:Dataset> , <dcat:Dataset> , <void:Dataset> .

ns1:Date a rdfs:Class ;
	rdfs:label "Date" ;
	rdfs:comment "A date value in <a href='http://en.wikipedia.org/wiki/ISO_8601'>ISO 8601 date format</a>." ;
	rdfs:subClassOf ns1:DataType .

ns1:DateTime a rdfs:Class ;
	rdfs:label "DateTime" ;
	rdfs:comment "A combination of date and time of day in the form [-]CCYY-MM-DDThh:mm:ss[Z|(+|-)hh:mm] (see Chapter 5.4 of ISO 8601)." ;
	rdfs:subClassOf ns1:DataType .

ns1:DayOfWeek a rdfs:Class ;
	rdfs:label "DayOfWeek" ;
	dc:source <http://www.w3.org/wiki/WebSchemas/SchemaDotOrgSources#source_GoodRelationsClass> ;
	rdfs:comment """The day of the week, e.g. used to specify to which day the opening hours of an OpeningHoursSpecification refer.

    Commonly used values:

    http://purl.org/goodrelations/v1#Monday
    http://purl.org/goodrelations/v1#Tuesday
    http://purl.org/goodrelations/v1#Wednesday
    http://purl.org/goodrelations/v1#Thursday
    http://purl.org/goodrelations/v1#Friday
    http://purl.org/goodrelations/v1#Saturday
    http://purl.org/goodrelations/v1#Sunday
    http://purl.org/goodrelations/v1#PublicHolidays
    		""" ;
	rdfs:subClassOf ns1:Enumeration .

ns1:DaySpa a rdfs:Class ;
	rdfs:label "DaySpa" ;
	rdfs:comment "A day spa." ;
	rdfs:subClassOf ns1:HealthAndBeautyBusiness .

ns1:DefenceEstablishment a rdfs:Class ;
	rdfs:label "DefenceEstablishment" ;
	rdfs:comment "A defence establishment, such as an army or navy base." ;
	rdfs:subClassOf ns1:GovernmentBuilding .

ns1:DeleteAction a rdfs:Class ;
	rdfs:label "DeleteAction" ;
	rdfs:comment "The act of editing a recipient by removing one of its objects." ;
	rdfs:subClassOf ns1:UpdateAction .

ns1:DeliveryChargeSpecification a rdfs:Class ;
	rdfs:label "DeliveryChargeSpecification" ;
	dc:source <http://www.w3.org/wiki/WebSchemas/SchemaDotOrgSources#source_GoodRelationsClass> ;
	rdfs:comment "The price for the delivery of an offer using a particular delivery method." ;
	rdfs:subClassOf ns1:PriceSpecification .

ns1:DeliveryEvent a rdfs:Class ;
	rdfs:label "DeliveryEvent" ;
	rdfs:comment "An event involving the delivery of an item." ;
	rdfs:subClassOf ns1:Event .

ns1:DeliveryMethod a rdfs:Class ;
	rdfs:label "DeliveryMethod" ;
	dc:source <http://www.w3.org/wiki/WebSchemas/SchemaDotOrgSources#source_GoodRelationsClass> ;
	rdfs:comment """A delivery method is a standardized procedure for transferring the product or service to the destination of fulfillment chosen by the customer. Delivery methods are characterized by the means of transportation used, and by the organization or group that is the contracting party for the sending organization or person.

    Commonly used values:

    http://purl.org/goodrelations/v1#DeliveryModeDirectDownload
    http://purl.org/goodrelations/v1#DeliveryModeFreight
    http://purl.org/goodrelations/v1#DeliveryModeMail
    http://purl.org/goodrelations/v1#DeliveryModeOwnFleet
    http://purl.org/goodrelations/v1#DeliveryModePickUp
    http://purl.org/goodrelations/v1#DHL
    http://purl.org/goodrelations/v1#FederalExpress
    http://purl.org/goodrelations/v1#UPS
    		""" ;
	rdfs:subClassOf ns1:Enumeration .

ns1:Demand a rdfs:Class ;
	rdfs:label "Demand" ;
	dc:source <http://www.w3.org/wiki/WebSchemas/SchemaDotOrgSources#source_GoodRelationsClass> ;
	rdfs:comment "A demand entity represents the public, not necessarily binding, not necessarily exclusive, announcement by an organization or person to seek a certain type of goods or services. For describing demand using this type, the very same properties used for Offer apply." ;
	rdfs:subClassOf ns1:Intangible .

ns1:Dentist a rdfs:Class ;
	rdfs:label "Dentist" ;
	rdfs:comment "A dentist." ;
	rdfs:subClassOf ns1:MedicalOrganization , ns1:ProfessionalService .

ns1:DepartAction a rdfs:Class ;
	rdfs:label "DepartAction" ;
	rdfs:comment "The act of  departing from a place. An agent departs from an fromLocation for a destination, optionally with participants." ;
	rdfs:subClassOf ns1:MoveAction .

ns1:DepartmentStore a rdfs:Class ;
	rdfs:label "DepartmentStore" ;
	rdfs:comment "A department store." ;
	rdfs:subClassOf ns1:Store .

ns1:DiagnosticLab a rdfs:Class ;
	rdfs:label "DiagnosticLab" ;
	rdfs:comment "A medical laboratory that offers on-site or off-site diagnostic services." ;
	rdfs:subClassOf ns1:MedicalOrganization .

ns1:DiagnosticProcedure a rdfs:Class ;
	rdfs:label "DiagnosticProcedure" ;
	dc:source <http://www.w3.org/wiki/WebSchemas/SchemaDotOrgSources#source_WikiDoc> ;
	rdfs:comment "A medical procedure intended primarily for diagnostic, as opposed to therapeutic, purposes." ;
	rdfs:subClassOf ns1:MedicalProcedure , ns1:MedicalTest .

ns1:Diet a rdfs:Class ;
	rdfs:label "Diet" ;
	dc:source <http://www.w3.org/wiki/WebSchemas/SchemaDotOrgSources#source_WikiDoc> ;
	rdfs:comment "A strategy of regulating the intake of food to achieve or maintain a specific health-related goal." ;
	rdfs:subClassOf ns1:CreativeWork , ns1:LifestyleModification .

ns1:DietarySupplement a rdfs:Class ;
	rdfs:label "DietarySupplement" ;
	dc:source <http://www.w3.org/wiki/WebSchemas/SchemaDotOrgSources#source_WikiDoc> ;
	rdfs:comment "A product taken by mouth that contains a dietary ingredient intended to supplement the diet. Dietary ingredients may include vitamins, minerals, herbs or other botanicals, amino acids, and substances such as enzymes, organ tissues, glandulars and metabolites." ;
	rdfs:subClassOf ns1:MedicalTherapy .

ns1:DisagreeAction a rdfs:Class ;
	rdfs:label "DisagreeAction" ;
	rdfs:comment "The act of expressing a difference of opinion with the object. An agent disagrees to/about an object (a proposition, topic or theme) with participants." ;
	rdfs:subClassOf ns1:ReactAction .

ns1:DiscoverAction a rdfs:Class ;
	rdfs:label "DiscoverAction" ;
	rdfs:comment "The act of discovering/finding an object." ;
	rdfs:subClassOf ns1:FindAction .

ns1:DislikeAction a rdfs:Class ;
	rdfs:label "DislikeAction" ;
	rdfs:comment "The act of expressing a negative sentiment about the object. An agent dislikes an object (a proposition, topic or theme) with participants." ;
	rdfs:subClassOf ns1:ReactAction .

ns1:Distance a rdfs:Class ;
	rdfs:label "Distance" ;
	rdfs:comment "Properties that take Distances as values are of the form '&lt;Number&gt; &lt;Length unit of measure&gt;'. E.g., '7 ft'" ;
	rdfs:subClassOf ns1:Quantity .

ns1:DonateAction a rdfs:Class ;
	rdfs:label "DonateAction" ;
	rdfs:comment "The act of providing goods, services, or money without compensation, often for philanthropic reasons." ;
	rdfs:subClassOf ns1:TradeAction .

ns1:DoseSchedule a rdfs:Class ;
	rdfs:label "DoseSchedule" ;
	rdfs:comment "A specific dosing schedule for a drug or supplement." ;
	rdfs:subClassOf ns1:MedicalIntangible .

ns1:DownloadAction a rdfs:Class ;
	rdfs:label "DownloadAction" ;
	rdfs:comment "The act of downloading an object." ;
	rdfs:subClassOf ns1:TransferAction .

ns1:DrawAction a rdfs:Class ;
	rdfs:label "DrawAction" ;
	rdfs:comment "The act of producing a visual/graphical representation of an object, typically with a pen/pencil and paper as instruments." ;
	rdfs:subClassOf ns1:CreateAction .

ns1:DrinkAction a rdfs:Class ;
	rdfs:label "DrinkAction" ;
	rdfs:comment "The act of swallowing liquids." ;
	rdfs:subClassOf ns1:ConsumeAction .

ns1:Drug a rdfs:Class ;
	rdfs:label "Drug" ;
	dc:source <http://www.w3.org/wiki/WebSchemas/SchemaDotOrgSources#source_WikiDoc> ;
	rdfs:comment "A chemical or biologic substance, used as a medical therapy, that has a physiological effect on an organism." ;
	rdfs:subClassOf ns1:MedicalTherapy .

ns1:DrugClass a rdfs:Class ;
	rdfs:label "DrugClass" ;
	dc:source <http://www.w3.org/wiki/WebSchemas/SchemaDotOrgSources#source_WikiDoc> ;
	rdfs:comment "A class of medical drugs, e.g., statins. Classes can represent general pharmacological class, common mechanisms of action, common physiological effects, etc." ;
	rdfs:subClassOf ns1:MedicalTherapy .

ns1:DrugCost a rdfs:Class ;
	rdfs:label "DrugCost" ;
	rdfs:comment "The cost per unit of a medical drug. Note that this type is not meant to represent the price in an offer of a drug for sale; see the Offer type for that. This type will typically be used to tag wholesale or average retail cost of a drug, or maximum reimbursable cost. Costs of medical drugs vary widely depending on how and where they are paid for, so while this type captures some of the variables, costs should be used with caution by consumers of this schema's markup." ;
	rdfs:subClassOf ns1:MedicalIntangible .

ns1:DrugCostCategory a rdfs:Class ;
	rdfs:label "DrugCostCategory" ;
	rdfs:comment "Enumerated categories of medical drug costs." ;
	rdfs:subClassOf ns1:Enumeration , ns1:MedicalEnumeration .

ns1:DrugLegalStatus a rdfs:Class ;
	rdfs:label "DrugLegalStatus" ;
	dc:source <http://www.w3.org/wiki/WebSchemas/SchemaDotOrgSources#source_WikiDoc> ;
	rdfs:comment "The legal availability status of a medical drug." ;
	rdfs:subClassOf ns1:MedicalIntangible .

ns1:DrugPregnancyCategory a rdfs:Class ;
	rdfs:label "DrugPregnancyCategory" ;
	rdfs:comment "Categories that represent an assessment of the risk of fetal injury due to a drug or pharmaceutical used as directed by the mother during pregnancy." ;
	rdfs:subClassOf ns1:Enumeration , ns1:MedicalEnumeration .

ns1:DrugPrescriptionStatus a rdfs:Class ;
	rdfs:label "DrugPrescriptionStatus" ;
	rdfs:comment "Indicates whether this drug is available by prescription or over-the-counter." ;
	rdfs:subClassOf ns1:Enumeration , ns1:MedicalEnumeration .

ns1:DrugStrength a rdfs:Class ;
	rdfs:label "DrugStrength" ;
	dc:source <http://www.w3.org/wiki/WebSchemas/SchemaDotOrgSources#source_WikiDoc> ;
	rdfs:comment "A specific strength in which a medical drug is available in a specific country." ;
	rdfs:subClassOf ns1:MedicalIntangible .

ns1:DryCleaningOrLaundry a rdfs:Class ;
	rdfs:label "DryCleaningOrLaundry" ;
	rdfs:comment "A dry-cleaning business." ;
	rdfs:subClassOf ns1:LocalBusiness .

ns1:Duration a rdfs:Class ;
	rdfs:label "Duration" ;
	rdfs:comment "Quantity: Duration (use  <a href='http://en.wikipedia.org/wiki/ISO_8601'>ISO 8601 duration format</a>)." ;
	rdfs:subClassOf ns1:Quantity .

ns1:EatAction a rdfs:Class ;
	rdfs:label "EatAction" ;
	rdfs:comment "The act of swallowing solid objects." ;
	rdfs:subClassOf ns1:ConsumeAction .

ns1:EducationEvent a rdfs:Class ;
	rdfs:label "EducationEvent" ;
	rdfs:comment "Event type: Education event." ;
	rdfs:subClassOf ns1:Event .

ns1:EducationalAudience a rdfs:Class ;
	rdfs:label "EducationalAudience" ;
	dc:source <http://www.w3.org/wiki/WebSchemas/SchemaDotOrgSources#source_LRMIClass> ;
	rdfs:comment "An EducationalAudience" ;
	rdfs:subClassOf ns1:Audience .

ns1:EducationalOrganization a rdfs:Class ;
	rdfs:label "EducationalOrganization" ;
	rdfs:comment "An educational organization." ;
	rdfs:subClassOf ns1:Organization .

ns1:Electrician a rdfs:Class ;
	rdfs:label "Electrician" ;
	rdfs:comment "An electrician." ;
	rdfs:subClassOf ns1:HomeAndConstructionBusiness , ns1:ProfessionalService .

ns1:ElectronicsStore a rdfs:Class ;
	rdfs:label "ElectronicsStore" ;
	rdfs:comment "An electronics store." ;
	rdfs:subClassOf ns1:Store .

ns1:ElementarySchool a rdfs:Class ;
	rdfs:label "ElementarySchool" ;
	rdfs:comment "An elementary school." ;
	rdfs:subClassOf ns1:EducationalOrganization .

ns1:EmailMessage a rdfs:Class ;
	rdfs:label "EmailMessage" ;
	rdfs:comment "An email message." ;
	rdfs:subClassOf ns1:CreativeWork .

ns1:Embassy a rdfs:Class ;
	rdfs:label "Embassy" ;
	rdfs:comment "An embassy." ;
	rdfs:subClassOf ns1:GovernmentBuilding .

ns1:EmergencyService a rdfs:Class ;
	rdfs:label "EmergencyService" ;
	rdfs:comment "An emergency service, such as a fire station or ER." ;
	rdfs:subClassOf ns1:LocalBusiness .

ns1:EmploymentAgency a rdfs:Class ;
	rdfs:label "EmploymentAgency" ;
	rdfs:comment "An employment agency." ;
	rdfs:subClassOf ns1:LocalBusiness .

ns1:EndorseAction a rdfs:Class ;
	rdfs:label "EndorseAction" ;
	rdfs:comment "An agent approves/certifies/likes/supports/sanction an object." ;
	rdfs:subClassOf ns1:ReactAction .

ns1:Energy a rdfs:Class ;
	rdfs:label "Energy" ;
	rdfs:comment "Properties that take Energy as values are of the form '&lt;Number&gt; &lt;Energy unit of measure&gt;'" ;
	rdfs:subClassOf ns1:Quantity .

ns1:EntertainmentBusiness a rdfs:Class ;
	rdfs:label "EntertainmentBusiness" ;
	rdfs:comment "A business providing entertainment." ;
	rdfs:subClassOf ns1:LocalBusiness .

ns1:EntryPoint a rdfs:Class ;
	rdfs:label "EntryPoint" ;
	dc:source <http://www.w3.org/wiki/WebSchemas/SchemaDotOrgSources#source_ActionCollabClass> ;
	rdfs:comment "An entry point, within some Web-based protocol." ;
	rdfs:subClassOf ns1:Intangible .

ns1:Enumeration a rdfs:Class ;
	rdfs:label "Enumeration" ;
	rdfs:comment "Lists or enumerations&#x2014;for example, a list of cuisines or music genres, etc." ;
	rdfs:subClassOf ns1:Intangible .

ns1:Episode a rdfs:Class ;
	rdfs:label "Episode" ;
	rdfs:comment "A TV or radio episode which can be part of a series or season." ;
	rdfs:subClassOf ns1:CreativeWork .

ns1:Event a rdfs:Class ;
	rdfs:label "Event" ;
	rdfs:comment "An event happening at a certain time and location, such as a concert, lecture, or festival. Ticketing information may be added via the 'offers' property. Repeated events may be structured as separate Event objects." ;
	rdfs:subClassOf ns1:Thing ;
	owl:equivalentClass <dc:Event> .

ns1:EventReservation a rdfs:Class ;
	rdfs:label "EventReservation" ;
	rdfs:comment "A reservation for an event like a concert, sporting event, or lecture.Note: This type is for information about actual reservations, e.g. in confirmation emails or HTML pages with individual confirmations of reservations. For offers of tickets, use http://schema.org/Offer." ;
	rdfs:subClassOf ns1:Reservation .

ns1:EventStatusType a rdfs:Class ;
	rdfs:label "EventStatusType" ;
	rdfs:comment "EventStatusType is an enumeration type whose instances represent several states that an Event may be in." ;
	rdfs:subClassOf ns1:Enumeration .

ns1:EventVenue a rdfs:Class ;
	rdfs:label "EventVenue" ;
	rdfs:comment "An event venue." ;
	rdfs:subClassOf ns1:CivicStructure .

ns1:ExerciseAction a rdfs:Class ;
	rdfs:label "ExerciseAction" ;
	rdfs:comment "The act of participating in exertive activity for the purposes of improving health and fitness" ;
	rdfs:subClassOf ns1:PlayAction .

ns1:ExerciseGym a rdfs:Class ;
	rdfs:label "ExerciseGym" ;
	rdfs:comment "A gym." ;
	rdfs:subClassOf ns1:SportsActivityLocation .

ns1:ExercisePlan a rdfs:Class ;
	rdfs:label "ExercisePlan" ;
	dc:source <http://www.w3.org/wiki/WebSchemas/SchemaDotOrgSources#source_WikiDoc> ;
	rdfs:comment "Fitness-related activity designed for a specific health-related purpose, including defined exercise routines as well as activity prescribed by a clinician." ;
	rdfs:subClassOf ns1:CreativeWork , ns1:PhysicalActivity .

ns1:FastFoodRestaurant a rdfs:Class ;
	rdfs:label "FastFoodRestaurant" ;
	rdfs:comment "A fast-food restaurant." ;
	rdfs:subClassOf ns1:FoodEstablishment .

ns1:Festival a rdfs:Class ;
	rdfs:label "Festival" ;
	rdfs:comment "Event type: Festival." ;
	rdfs:subClassOf ns1:Event .

ns1:FilmAction a rdfs:Class ;
	rdfs:label "FilmAction" ;
	rdfs:comment "The act of capturing sound and moving images on film, video, or digitally." ;
	rdfs:subClassOf ns1:CreateAction .

ns1:FinancialService a rdfs:Class ;
	rdfs:label "FinancialService" ;
	rdfs:comment "Financial services business." ;
	rdfs:subClassOf ns1:LocalBusiness .

ns1:FindAction a rdfs:Class ;
	rdfs:label "FindAction" ;
	rdfs:comment "The act of finding an object.<p>Related actions:</p><ul><li><a href=\"http://schema.org/SearchAction\">SearchAction</a>: FindAction is generally lead by a SearchAction, but not necessarily.</li></ul>" ;
	rdfs:subClassOf ns1:Action .

ns1:FireStation a rdfs:Class ;
	rdfs:label "FireStation" ;
	rdfs:comment "A fire station. With firemen." ;
	rdfs:subClassOf ns1:CivicStructure , ns1:EmergencyService .

ns1:Flight a rdfs:Class ;
	rdfs:label "Flight" ;
	rdfs:comment "An airline flight." ;
	rdfs:subClassOf ns1:Intangible .

ns1:FlightReservation a rdfs:Class ;
	rdfs:label "FlightReservation" ;
	rdfs:comment "A reservation for air travel.Note: This type is for information about actual reservations, e.g. in confirmation emails or HTML pages with individual confirmations of reservations. For offers of tickets, use http://schema.org/Offer." ;
	rdfs:subClassOf ns1:Reservation .

ns1:Float a rdfs:Class ;
	rdfs:label "Float" ;
	rdfs:comment "Data type: Floating number." ;
	rdfs:subClassOf ns1:Number .

ns1:Florist a rdfs:Class ;
	rdfs:label "Florist" ;
	rdfs:comment "A florist." ;
	rdfs:subClassOf ns1:Store .

ns1:FollowAction a rdfs:Class ;
	rdfs:label "FollowAction" ;
	rdfs:comment "The act of forming a personal connection with someone/something (object) unidirectionally/asymmetrically to get updates polled from.<p>Related actions:</p><ul><li><a href=\"http://schema.org/BefriendAction\">BefriendAction</a>: Unlike BefriendAction, FollowAction implies that the connection is *not* necessarily reciprocal.</li><li><a href=\"http://schema.org/SubscribeAction\">SubscribeAction</a>: Unlike SubscribeAction, FollowAction implies that the follower acts as an active agent constantly/actively polling for updates.</li><li><a href=\"http://schema.org/RegisterAction\">RegisterAction</a>: Unlike RegisterAction, FollowAction implies that the agent is interested in continuing receiving updates from the object.</li><li><a href=\"http://schema.org/JoinAction\">JoinAction</a>: Unlike JoinAction, FollowAction implies that the agent is interested in getting updates from the object.</li><li><a href=\"http://schema.org/TrackAction\">TrackAction</a>: Unlike TrackAction, FollowAction refers to the polling of updates of all aspects of animate objects rather than the location of inanimate objects (e.g. you track a package, but you don't follow it).</li></ul>" ;
	rdfs:subClassOf ns1:InteractAction .

ns1:FoodEstablishment a rdfs:Class ;
	rdfs:label "FoodEstablishment" ;
	rdfs:comment "A food-related business." ;
	rdfs:subClassOf ns1:LocalBusiness .

ns1:FoodEstablishmentReservation a rdfs:Class ;
	rdfs:label "FoodEstablishmentReservation" ;
	rdfs:comment "A reservation to dine at a food-related business.Note: This type is for information about actual reservations, e.g. in confirmation emails or HTML pages with individual confirmations of reservations." ;
	rdfs:subClassOf ns1:Reservation .

ns1:FoodEvent a rdfs:Class ;
	rdfs:label "FoodEvent" ;
	rdfs:comment "Event type: Food event." ;
	rdfs:subClassOf ns1:Event .

ns1:FurnitureStore a rdfs:Class ;
	rdfs:label "FurnitureStore" ;
	rdfs:comment "A furniture store." ;
	rdfs:subClassOf ns1:Store .

ns1:GardenStore a rdfs:Class ;
	rdfs:label "GardenStore" ;
	rdfs:comment "A garden store." ;
	rdfs:subClassOf ns1:Store .

ns1:GasStation a rdfs:Class ;
	rdfs:label "GasStation" ;
	rdfs:comment "A gas station." ;
	rdfs:subClassOf ns1:AutomotiveBusiness .

ns1:GatedResidenceCommunity a rdfs:Class ;
	rdfs:label "GatedResidenceCommunity" ;
	rdfs:comment "Residence type: Gated community." ;
	rdfs:subClassOf ns1:Residence .

ns1:GeneralContractor a rdfs:Class ;
	rdfs:label "GeneralContractor" ;
	rdfs:comment "A general contractor." ;
	rdfs:subClassOf ns1:HomeAndConstructionBusiness , ns1:ProfessionalService .

ns1:GeoCoordinates a rdfs:Class ;
	rdfs:label "GeoCoordinates" ;
	rdfs:comment "The geographic coordinates of a place or event." ;
	rdfs:subClassOf ns1:StructuredValue .

ns1:GeoShape a rdfs:Class ;
	rdfs:label "GeoShape" ;
	dc:source <http://www.w3.org/wiki/WebSchemas/SchemaDotOrgSources#source_rNews> ;
	rdfs:comment "The geographic shape of a place." ;
	rdfs:subClassOf ns1:StructuredValue .

ns1:GiveAction a rdfs:Class ;
	rdfs:label "GiveAction" ;
	rdfs:comment "The act of transferring ownership of an object to a destination. Reciprocal of TakeAction.<p>Related actions:</p><ul><li><a href=\"http://schema.org/TakeAction\">TakeAction</a>: Reciprocal of GiveAction.</li><li><a href=\"http://schema.org/SendAction\">SendAction</a>: Unlike SendAction, GiveAction implies that ownership is being transferred (e.g. I may send my laptop to you, but that doesn't mean I'm giving it to you).</li></ul>" ;
	rdfs:subClassOf ns1:TransferAction .

ns1:GolfCourse a rdfs:Class ;
	rdfs:label "GolfCourse" ;
	rdfs:comment "A golf course." ;
	rdfs:subClassOf ns1:SportsActivityLocation .

ns1:GovernmentBuilding a rdfs:Class ;
	rdfs:label "GovernmentBuilding" ;
	rdfs:comment "A government building." ;
	rdfs:subClassOf ns1:CivicStructure .

ns1:GovernmentOffice a rdfs:Class ;
	rdfs:label "GovernmentOffice" ;
	rdfs:comment "A government office&#x2014;for example, an IRS or DMV office." ;
	rdfs:subClassOf ns1:LocalBusiness .

ns1:GovernmentOrganization a rdfs:Class ;
	rdfs:label "GovernmentOrganization" ;
	rdfs:comment "A governmental organization or agency." ;
	rdfs:subClassOf ns1:Organization .

ns1:GovernmentPermit a rdfs:Class ;
	rdfs:label "GovernmentPermit" ;
	rdfs:comment "A permit issued by a government agency." ;
	rdfs:subClassOf ns1:Permit .

ns1:GovernmentService a rdfs:Class ;
	rdfs:label "GovernmentService" ;
	rdfs:comment "A service provided by a government organization, e.g. food stamps, veterans benefits, etc." ;
	rdfs:subClassOf ns1:Service .

ns1:GroceryStore a rdfs:Class ;
	rdfs:label "GroceryStore" ;
	rdfs:comment "A grocery store." ;
	rdfs:subClassOf ns1:Store .

ns1:HVACBusiness a rdfs:Class ;
	rdfs:label "HVACBusiness" ;
	rdfs:comment "An HVAC service." ;
	rdfs:subClassOf ns1:HomeAndConstructionBusiness .

ns1:HairSalon a rdfs:Class ;
	rdfs:label "HairSalon" ;
	rdfs:comment "A hair salon." ;
	rdfs:subClassOf ns1:HealthAndBeautyBusiness .

ns1:HardwareStore a rdfs:Class ;
	rdfs:label "HardwareStore" ;
	rdfs:comment "A hardware store." ;
	rdfs:subClassOf ns1:Store .

ns1:HealthAndBeautyBusiness a rdfs:Class ;
	rdfs:label "HealthAndBeautyBusiness" ;
	rdfs:comment "Health and beauty." ;
	rdfs:subClassOf ns1:LocalBusiness .

ns1:HealthClub a rdfs:Class ;
	rdfs:label "HealthClub" ;
	rdfs:comment "A health club." ;
	rdfs:subClassOf ns1:HealthAndBeautyBusiness , ns1:SportsActivityLocation .

ns1:HighSchool a rdfs:Class ;
	rdfs:label "HighSchool" ;
	rdfs:comment "A high school." ;
	rdfs:subClassOf ns1:EducationalOrganization .

ns1:HinduTemple a rdfs:Class ;
	rdfs:label "HinduTemple" ;
	rdfs:comment "A Hindu temple." ;
	rdfs:subClassOf ns1:PlaceOfWorship .

ns1:HobbyShop a rdfs:Class ;
	rdfs:label "HobbyShop" ;
	rdfs:comment "A hobby store." ;
	rdfs:subClassOf ns1:Store .

ns1:HomeAndConstructionBusiness a rdfs:Class ;
	rdfs:label "HomeAndConstructionBusiness" ;
	rdfs:comment "A construction business." ;
	rdfs:subClassOf ns1:LocalBusiness .

ns1:HomeGoodsStore a rdfs:Class ;
	rdfs:label "HomeGoodsStore" ;
	rdfs:comment "A home goods store." ;
	rdfs:subClassOf ns1:Store .

ns1:Hospital a rdfs:Class ;
	rdfs:label "Hospital" ;
	rdfs:comment "A hospital." ;
	rdfs:subClassOf ns1:CivicStructure , ns1:EmergencyService , ns1:MedicalOrganization .

ns1:Hostel a rdfs:Class ;
	rdfs:label "Hostel" ;
	rdfs:comment "A hostel." ;
	rdfs:subClassOf ns1:LodgingBusiness .

ns1:Hotel a rdfs:Class ;
	rdfs:label "Hotel" ;
	rdfs:comment "A hotel." ;
	rdfs:subClassOf ns1:LodgingBusiness .

ns1:HousePainter a rdfs:Class ;
	rdfs:label "HousePainter" ;
	rdfs:comment "A house painting service." ;
	rdfs:subClassOf ns1:HomeAndConstructionBusiness , ns1:ProfessionalService .

ns1:IceCreamShop a rdfs:Class ;
	rdfs:label "IceCreamShop" ;
	rdfs:comment "An ice cream shop" ;
	rdfs:subClassOf ns1:FoodEstablishment .

ns1:IgnoreAction a rdfs:Class ;
	rdfs:label "IgnoreAction" ;
	rdfs:comment "The act of intentionally disregarding the object. An agent ignores an object." ;
	rdfs:subClassOf ns1:AssessAction .

ns1:ImageGallery a rdfs:Class ;
	rdfs:label "ImageGallery" ;
	rdfs:comment "Web page type: Image gallery page." ;
	rdfs:subClassOf ns1:CollectionPage .

ns1:ImageObject a rdfs:Class ;
	rdfs:label "ImageObject" ;
	rdfs:comment "An image file." ;
	rdfs:subClassOf ns1:MediaObject ;
	owl:equivalentClass <dc:Image> .

ns1:ImagingTest a rdfs:Class ;
	rdfs:label "ImagingTest" ;
	dc:source <http://www.w3.org/wiki/WebSchemas/SchemaDotOrgSources#source_WikiDoc> ;
	rdfs:comment "Any medical imaging modality typically used for diagnostic purposes." ;
	rdfs:subClassOf ns1:MedicalTest .

ns1:IndividualProduct a rdfs:Class ;
	rdfs:label "IndividualProduct" ;
	dc:source <http://www.w3.org/wiki/WebSchemas/SchemaDotOrgSources#source_GoodRelationsClass> ;
	rdfs:comment "A single, identifiable product instance (e.g. a laptop with a particular serial number)." ;
	rdfs:subClassOf ns1:Product .

ns1:InfectiousAgentClass a rdfs:Class ;
	rdfs:label "InfectiousAgentClass" ;
	dc:source <http://www.w3.org/wiki/WebSchemas/SchemaDotOrgSources#source_WikiDoc> ;
	rdfs:comment "Classes of agents or pathogens that transmit infectious diseases. Enumerated type." ;
	rdfs:subClassOf ns1:Enumeration , ns1:MedicalEnumeration .

ns1:InfectiousDisease a rdfs:Class ;
	rdfs:label "InfectiousDisease" ;
	dc:source <http://www.w3.org/wiki/WebSchemas/SchemaDotOrgSources#source_WikiDoc> ;
	rdfs:comment "An infectious disease is a clinically evident human disease resulting from the presence of pathogenic microbial agents, like pathogenic viruses, pathogenic bacteria, fungi, protozoa, multicellular parasites, and prions. To be considered an infectious disease, such pathogens are known to be able to cause this disease." ;
	rdfs:subClassOf ns1:MedicalCondition .

ns1:InformAction a rdfs:Class ;
	rdfs:label "InformAction" ;
	rdfs:comment "The act of notifying someone of information pertinent to them, with no expectation of a response." ;
	rdfs:subClassOf ns1:CommunicateAction .

ns1:InsertAction a rdfs:Class ;
	rdfs:label "InsertAction" ;
	rdfs:comment "The act of adding at a specific location in an ordered collection." ;
	rdfs:subClassOf ns1:AddAction .

ns1:InstallAction a rdfs:Class ;
	rdfs:label "InstallAction" ;
	rdfs:comment "The act of installing an application." ;
	rdfs:subClassOf ns1:ConsumeAction .

ns1:InsuranceAgency a rdfs:Class ;
	rdfs:label "InsuranceAgency" ;
	rdfs:comment "Insurance agency." ;
	rdfs:subClassOf ns1:FinancialService .

ns1:Intangible a rdfs:Class ;
	rdfs:label "Intangible" ;
	rdfs:comment "A utility class that serves as the umbrella for a number of 'intangible' things such as quantities, structured values, etc." ;
	rdfs:subClassOf ns1:Thing .

ns1:Integer a rdfs:Class ;
	rdfs:label "Integer" ;
	rdfs:comment "Data type: Integer." ;
	rdfs:subClassOf ns1:Number .

ns1:InteractAction a rdfs:Class ;
	rdfs:label "InteractAction" ;
	rdfs:comment "The act of interacting with another person or organization." ;
	rdfs:subClassOf ns1:Action .

ns1:InternetCafe a rdfs:Class ;
	rdfs:label "InternetCafe" ;
	rdfs:comment "An internet cafe." ;
	rdfs:subClassOf ns1:LocalBusiness .

ns1:InviteAction a rdfs:Class ;
	rdfs:label "InviteAction" ;
	rdfs:comment "The act of asking someone to attend an event. Reciprocal of RsvpAction." ;
	rdfs:subClassOf ns1:CommunicateAction .

ns1:ItemAvailability a rdfs:Class ;
	rdfs:label "ItemAvailability" ;
	rdfs:comment "A list of possible product availability options." ;
	rdfs:subClassOf ns1:Enumeration .

ns1:ItemList a rdfs:Class ;
	rdfs:label "ItemList" ;
	rdfs:comment "A list of items of any sort&#x2014;for example, Top 10 Movies About Weathermen, or Top 100 Party Songs. Not to be confused with HTML lists, which are often used only for formatting." ;
	rdfs:subClassOf ns1:CreativeWork .

ns1:ItemPage a rdfs:Class ;
	rdfs:label "ItemPage" ;
	rdfs:comment "A page devoted to a single item, such as a particular product or hotel." ;
	rdfs:subClassOf ns1:WebPage .

ns1:JewelryStore a rdfs:Class ;
	rdfs:label "JewelryStore" ;
	rdfs:comment "A jewelry store." ;
	rdfs:subClassOf ns1:Store .

ns1:JobPosting a rdfs:Class ;
	rdfs:label "JobPosting" ;
	rdfs:comment "A listing that describes a job opening in a certain organization." ;
	rdfs:subClassOf ns1:Intangible .

ns1:JoinAction a rdfs:Class ;
	rdfs:label "JoinAction" ;
	rdfs:comment "An agent joins an event/group with participants/friends at a location.<p>Related actions:</p><ul><li><a href=\"http://schema.org/RegisterAction\">RegisterAction</a>: Unlike RegisterAction, JoinAction refers to joining a group/team of people.</li><li><a href=\"http://schema.org/SubscribeAction\">SubscribeAction</a>: Unlike SubscribeAction, JoinAction does not imply that you'll be receiving updates.</li><li><a href=\"http://schema.org/FollowAction\">FollowAction</a>: Unlike FollowAction, JoinAction does not imply that you'll be polling for updates.</li></ul>" ;
	rdfs:subClassOf ns1:InteractAction .

ns1:Joint a rdfs:Class ;
	rdfs:label "Joint" ;
	dc:source <http://www.w3.org/wiki/WebSchemas/SchemaDotOrgSources#source_WikiDoc> ;
	rdfs:comment "The anatomical location at which two or more bones make contact." ;
	rdfs:subClassOf ns1:AnatomicalStructure .

ns1:LakeBodyOfWater a rdfs:Class ;
	rdfs:label "LakeBodyOfWater" ;
	rdfs:comment "A lake (for example, Lake Pontrachain)." ;
	rdfs:subClassOf ns1:BodyOfWater .

ns1:Landform a rdfs:Class ;
	rdfs:label "Landform" ;
	rdfs:comment "A landform or physical feature.  Landform elements include mountains, plains, lakes, rivers, seascape and oceanic waterbody interface features such as bays, peninsulas, seas and so forth, including sub-aqueous terrain features such as submersed mountain ranges, volcanoes, and the great ocean basins." ;
	rdfs:subClassOf ns1:Place .

ns1:LandmarksOrHistoricalBuildings a rdfs:Class ;
	rdfs:label "LandmarksOrHistoricalBuildings" ;
	rdfs:comment "An historical landmark or building." ;
	rdfs:subClassOf ns1:Place .

ns1:Language a rdfs:Class ;
	rdfs:label "Language" ;
	rdfs:comment "Natural languages such as Spanish, Tamil, Hindi, English, etc. and programming languages such as Scheme and Lisp." ;
	rdfs:subClassOf ns1:Intangible .

ns1:LeaveAction a rdfs:Class ;
	rdfs:label "LeaveAction" ;
	rdfs:comment "An agent leaves an event / group with participants/friends at a location.<p>Related actions:</p><ul><li><a href=\"http://schema.org/JoinAction\">JoinAction</a>: The antagonym of LeaveAction.</li><li><a href=\"http://schema.org/UnRegisterAction\">UnRegisterAction</a>: Unlike UnRegisterAction, LeaveAction implies leaving a group/team of people rather than a service.</li></ul>" ;
	rdfs:subClassOf ns1:InteractAction .

ns1:LegislativeBuilding a rdfs:Class ;
	rdfs:label "LegislativeBuilding" ;
	rdfs:comment "A legislative building&#x2014;for example, the state capitol." ;
	rdfs:subClassOf ns1:GovernmentBuilding .

ns1:LendAction a rdfs:Class ;
	rdfs:label "LendAction" ;
	rdfs:comment "The act of providing an object under an agreement that it will be returned at a later date. Reciprocal of BorrowAction.<p>Related actions:</p><ul><li><a href=\"http://schema.org/BorrowAction\">BorrowAction</a>: Reciprocal of LendAction.</li></ul>" ;
	rdfs:subClassOf ns1:TransferAction .

ns1:Library a rdfs:Class ;
	rdfs:label "Library" ;
	rdfs:comment "A library." ;
	rdfs:subClassOf ns1:LocalBusiness .

ns1:LifestyleModification a rdfs:Class ;
	rdfs:label "LifestyleModification" ;
	dc:source <http://www.w3.org/wiki/WebSchemas/SchemaDotOrgSources#source_WikiDoc> ;
	rdfs:comment "A process of care involving exercise, changes to diet, fitness routines, and other lifestyle changes aimed at improving a health condition." ;
	rdfs:subClassOf ns1:MedicalTherapy .

ns1:Ligament a rdfs:Class ;
	rdfs:label "Ligament" ;
	dc:source <http://www.w3.org/wiki/WebSchemas/SchemaDotOrgSources#source_WikiDoc> ;
	rdfs:comment "A short band of tough, flexible, fibrous connective tissue that functions to connect multiple bones, cartilages, and structurally support joints." ;
	rdfs:subClassOf ns1:AnatomicalStructure .

ns1:LikeAction a rdfs:Class ;
	rdfs:label "LikeAction" ;
	rdfs:comment "The act of expressing a positive sentiment about the object. An agent likes an object (a proposition, topic or theme) with participants." ;
	rdfs:subClassOf ns1:ReactAction .

ns1:LiquorStore a rdfs:Class ;
	rdfs:label "LiquorStore" ;
	rdfs:comment "A liquor store." ;
	rdfs:subClassOf ns1:Store .

ns1:ListenAction a rdfs:Class ;
	rdfs:label "ListenAction" ;
	rdfs:comment "The act of consuming audio content." ;
	rdfs:subClassOf ns1:ConsumeAction .

ns1:LiteraryEvent a rdfs:Class ;
	rdfs:label "LiteraryEvent" ;
	rdfs:comment "Event type: Literary event." ;
	rdfs:subClassOf ns1:Event .

ns1:LocalBusiness a rdfs:Class ;
	rdfs:label "LocalBusiness" ;
	rdfs:comment "A particular physical business or branch of an organization. Examples of LocalBusiness include a restaurant, a particular branch of a restaurant chain, a branch of a bank, a medical practice, a club, a bowling alley, etc." ;
	rdfs:subClassOf ns1:Organization , ns1:Place .

ns1:LockerDelivery a rdfs:Class ;
	rdfs:label "LockerDelivery" ;
	rdfs:comment "A DeliveryMethod in which an item is made available via locker." ;
	rdfs:subClassOf ns1:DeliveryMethod .

ns1:Locksmith a rdfs:Class ;
	rdfs:label "Locksmith" ;
	rdfs:comment "A locksmith." ;
	rdfs:subClassOf ns1:HomeAndConstructionBusiness , ns1:ProfessionalService .

ns1:LodgingBusiness a rdfs:Class ;
	rdfs:label "LodgingBusiness" ;
	rdfs:comment "A lodging business, such as a motel, hotel, or inn." ;
	rdfs:subClassOf ns1:LocalBusiness .

ns1:LodgingReservation a rdfs:Class ;
	rdfs:label "LodgingReservation" ;
	rdfs:comment "A reservation for lodging at a hotel, motel, inn, etc.Note: This type is for information about actual reservations, e.g. in confirmation emails or HTML pages with individual confirmations of reservations." ;
	rdfs:subClassOf ns1:Reservation .

ns1:LoseAction a rdfs:Class ;
	rdfs:label "LoseAction" ;
	rdfs:comment "The act of being defeated in a competitive activity." ;
	rdfs:subClassOf ns1:AchieveAction .

ns1:LymphaticVessel a rdfs:Class ;
	rdfs:label "LymphaticVessel" ;
	dc:source <http://www.w3.org/wiki/WebSchemas/SchemaDotOrgSources#source_WikiDoc> ;
	rdfs:comment "A type of blood vessel that specifically carries lymph fluid unidirectionally toward the heart." ;
	rdfs:subClassOf ns1:Vessel .

ns1:Map a rdfs:Class ;
	rdfs:label "Map" ;
	rdfs:comment "A map." ;
	rdfs:subClassOf ns1:CreativeWork .

ns1:MarryAction a rdfs:Class ;
	rdfs:label "MarryAction" ;
	rdfs:comment "The act of marrying a person." ;
	rdfs:subClassOf ns1:InteractAction .

ns1:Mass a rdfs:Class ;
	rdfs:label "Mass" ;
	rdfs:comment "Properties that take Mass as values are of the form '&lt;Number&gt; &lt;Mass unit of measure&gt;'. E.g., '7 kg'" ;
	rdfs:subClassOf ns1:Quantity .

ns1:MaximumDoseSchedule a rdfs:Class ;
	rdfs:label "MaximumDoseSchedule" ;
	rdfs:comment "The maximum dosing schedule considered safe for a drug or supplement as recommended by an authority or by the drug/supplement's manufacturer. Capture the recommending authority in the recognizingAuthority property of MedicalEntity." ;
	rdfs:subClassOf ns1:DoseSchedule .

ns1:MediaObject a rdfs:Class ;
	rdfs:label "MediaObject" ;
	rdfs:comment "An image, video, or audio object embedded in a web page. Note that a creative work may have many media objects associated with it on the same web page. For example, a page about a single song (MusicRecording) may have a music video (VideoObject), and a high and low bandwidth audio stream (2 AudioObject's)." ;
	rdfs:subClassOf ns1:CreativeWork .

ns1:MedicalAudience a rdfs:Class ;
	rdfs:label "MedicalAudience" ;
	dc:source <http://www.w3.org/wiki/WebSchemas/SchemaDotOrgSources#source_WikiDoc> ;
	rdfs:comment "Target audiences for medical web pages. Enumerated type." ;
	rdfs:subClassOf ns1:Audience , ns1:Enumeration , ns1:MedicalEnumeration , ns1:PeopleAudience .

ns1:MedicalCause a rdfs:Class ;
	rdfs:label "MedicalCause" ;
	dc:source <http://www.w3.org/wiki/WebSchemas/SchemaDotOrgSources#source_WikiDoc> ;
	rdfs:comment "The causative agent(s) that are responsible for the pathophysiologic process that eventually results in a medical condition, symptom or sign. In this schema, unless otherwise specified this is meant to be the proximate cause of the medical condition, symptom or sign. The proximate cause is defined as the causative agent that most directly results in the medical condition, symptom or sign. For example, the HIV virus could be considered a cause of AIDS. Or in a diagnostic context, if a patient fell and sustained a hip fracture and two days later sustained a pulmonary embolism which eventuated in a cardiac arrest, the cause of the cardiac arrest (the proximate cause) would be the pulmonary embolism and not the fall. <p>Medical causes can include cardiovascular, chemical, dermatologic, endocrine, environmental, gastroenterologic, genetic, hematologic, gynecologic, iatrogenic, infectious, musculoskeletal, neurologic, nutritional, obstetric, oncologic, otolaryngologic, pharmacologic, psychiatric, pulmonary, renal, rheumatologic, toxic, traumatic, or urologic causes; medical conditions can be causes as well." ;
	rdfs:subClassOf ns1:MedicalEntity .

ns1:MedicalClinic a rdfs:Class ;
	rdfs:label "MedicalClinic" ;
	rdfs:comment "A medical clinic." ;
	rdfs:subClassOf ns1:MedicalOrganization .

ns1:MedicalCode a rdfs:Class ;
	rdfs:label "MedicalCode" ;
	dc:source <http://www.w3.org/wiki/WebSchemas/SchemaDotOrgSources#source_WikiDoc> ;
	rdfs:comment "A code for a medical entity." ;
	rdfs:subClassOf ns1:MedicalIntangible .

ns1:MedicalCondition a rdfs:Class ;
	rdfs:label "MedicalCondition" ;
	dc:source <http://www.w3.org/wiki/WebSchemas/SchemaDotOrgSources#source_WikiDoc> ;
	rdfs:comment "Any condition of the human body that affects the normal functioning of a person, whether physically or mentally. Includes diseases, injuries, disabilities, disorders, syndromes, etc." ;
	rdfs:subClassOf ns1:MedicalEntity .

ns1:MedicalConditionStage a rdfs:Class ;
	rdfs:label "MedicalConditionStage" ;
	dc:source <http://www.w3.org/wiki/WebSchemas/SchemaDotOrgSources#source_WikiDoc> ;
	rdfs:comment "A stage of a medical condition, such as 'Stage IIIa'." ;
	rdfs:subClassOf ns1:MedicalIntangible .

ns1:MedicalContraindication a rdfs:Class ;
	rdfs:label "MedicalContraindication" ;
	dc:source <http://www.w3.org/wiki/WebSchemas/SchemaDotOrgSources#source_WikiDoc> ;
	rdfs:comment "A condition or factor that serves as a reason to withhold a certain medical therapy. Contraindications can be absolute (there are no reasonable circumstances for undertaking a course of action) or relative (the patient is at higher risk of complications, but that these risks may be outweighed by other considerations or mitigated by other measures)." ;
	rdfs:subClassOf ns1:MedicalEntity .

ns1:MedicalDevice a rdfs:Class ;
	rdfs:label "MedicalDevice" ;
	dc:source <http://www.w3.org/wiki/WebSchemas/SchemaDotOrgSources#source_WikiDoc> ;
	rdfs:comment "Any object used in a medical capacity, such as to diagnose or treat a patient." ;
	rdfs:subClassOf ns1:MedicalEntity .

ns1:MedicalDevicePurpose a rdfs:Class ;
	rdfs:label "MedicalDevicePurpose" ;
	dc:source <http://www.w3.org/wiki/WebSchemas/SchemaDotOrgSources#source_WikiDoc> ;
	rdfs:comment "Categories of medical devices, organized by the purpose or intended use of the device." ;
	rdfs:subClassOf ns1:Enumeration , ns1:MedicalEnumeration .

ns1:MedicalEntity a rdfs:Class ;
	rdfs:label "MedicalEntity" ;
	dc:source <http://www.w3.org/wiki/WebSchemas/SchemaDotOrgSources#source_WikiDoc> ;
	rdfs:comment "The most generic type of entity related to health and the practice of medicine." ;
	rdfs:subClassOf ns1:Thing .

ns1:MedicalEnumeration a rdfs:Class ;
	rdfs:label "MedicalEnumeration" ;
	rdfs:comment "Enumerations related to health and the practice of medicine." ;
	rdfs:subClassOf ns1:Enumeration , ns1:MedicalIntangible .

ns1:MedicalEvidenceLevel a rdfs:Class ;
	rdfs:label "MedicalEvidenceLevel" ;
	dc:source <http://www.w3.org/wiki/WebSchemas/SchemaDotOrgSources#source_WikiDoc> ;
	rdfs:comment "Level of evidence for a medical guideline. Enumerated type." ;
	rdfs:subClassOf ns1:Enumeration , ns1:MedicalEnumeration .

ns1:MedicalGuideline a rdfs:Class ;
	rdfs:label "MedicalGuideline" ;
	dc:source <http://www.w3.org/wiki/WebSchemas/SchemaDotOrgSources#source_WikiDoc> ;
	rdfs:comment "Any recommendation made by a standard society (e.g. ACC/AHA) or consensus statement that denotes how to diagnose and treat a particular condition. Note: this type should be used to tag the actual guideline recommendation; if the guideline recommendation occurs in a larger scholarly article, use MedicalScholarlyArticle to tag the overall article, not this type. Note also: the organization making the recommendation should be captured in the recognizingAuthority base property of MedicalEntity." ;
	rdfs:subClassOf ns1:MedicalEntity .

ns1:MedicalGuidelineContraindication a rdfs:Class ;
	rdfs:label "MedicalGuidelineContraindication" ;
	dc:source <http://www.w3.org/wiki/WebSchemas/SchemaDotOrgSources#source_WikiDoc> ;
	rdfs:comment "A guideline contraindication that designates a process as harmful and where quality of the data supporting the contraindication is sound." ;
	rdfs:subClassOf ns1:MedicalGuideline .

ns1:MedicalGuidelineRecommendation a rdfs:Class ;
	rdfs:label "MedicalGuidelineRecommendation" ;
	dc:source <http://www.w3.org/wiki/WebSchemas/SchemaDotOrgSources#source_WikiDoc> ;
	rdfs:comment "A guideline recommendation that is regarded as efficacious and where quality of the data supporting the recommendation is sound." ;
	rdfs:subClassOf ns1:MedicalGuideline .

ns1:MedicalImagingTechnique a rdfs:Class ;
	rdfs:label "MedicalImagingTechnique" ;
	dc:source <http://www.w3.org/wiki/WebSchemas/SchemaDotOrgSources#source_WikiDoc> ;
	rdfs:comment "Any medical imaging modality typically used for diagnostic purposes. Enumerated type." ;
	rdfs:subClassOf ns1:Enumeration , ns1:MedicalEnumeration .

ns1:MedicalIndication a rdfs:Class ;
	rdfs:label "MedicalIndication" ;
	dc:source <http://www.w3.org/wiki/WebSchemas/SchemaDotOrgSources#source_WikiDoc> ;
	rdfs:comment "A condition or factor that indicates use of a medical therapy, including signs, symptoms, risk factors, anatomical states, etc." ;
	rdfs:subClassOf ns1:MedicalEntity .

ns1:MedicalIntangible a rdfs:Class ;
	rdfs:label "MedicalIntangible" ;
	rdfs:comment "A utility class that serves as the umbrella for a number of 'intangible' things in the medical space." ;
	rdfs:subClassOf ns1:MedicalEntity .

ns1:MedicalObservationalStudy a rdfs:Class ;
	rdfs:label "MedicalObservationalStudy" ;
	dc:source <http://www.w3.org/wiki/WebSchemas/SchemaDotOrgSources#source_WikiDoc> ;
	rdfs:comment "An observational study is a type of medical study that attempts to infer the possible effect of a treatment through observation of a cohort of subjects over a period of time. In an observational study, the assignment of subjects into treatment groups versus control groups is outside the control of the investigator. This is in contrast with controlled studies, such as the randomized controlled trials represented by MedicalTrial, where each subject is randomly assigned to a treatment group or a control group before the start of the treatment." ;
	rdfs:subClassOf ns1:MedicalStudy .

ns1:MedicalObservationalStudyDesign a rdfs:Class ;
	rdfs:label "MedicalObservationalStudyDesign" ;
	dc:source <http://www.w3.org/wiki/WebSchemas/SchemaDotOrgSources#source_WikiDoc> ;
	rdfs:comment "Design models for observational medical studies. Enumerated type." ;
	rdfs:subClassOf ns1:Enumeration , ns1:MedicalEnumeration .

ns1:MedicalOrganization a rdfs:Class ;
	rdfs:label "MedicalOrganization" ;
	rdfs:comment "A medical organization, such as a doctor's office or clinic." ;
	rdfs:subClassOf ns1:LocalBusiness .

ns1:MedicalProcedure a rdfs:Class ;
	rdfs:label "MedicalProcedure" ;
	dc:source <http://www.w3.org/wiki/WebSchemas/SchemaDotOrgSources#source_WikiDoc> ;
	rdfs:comment "A process of care used in either a diagnostic, therapeutic, or palliative capacity that relies on invasive (surgical), non-invasive, or percutaneous techniques." ;
	rdfs:subClassOf ns1:MedicalEntity .

ns1:MedicalProcedureType a rdfs:Class ;
	rdfs:label "MedicalProcedureType" ;
	dc:source <http://www.w3.org/wiki/WebSchemas/SchemaDotOrgSources#source_WikiDoc> ;
	rdfs:comment "An enumeration that describes different types of medical procedures." ;
	rdfs:subClassOf ns1:Enumeration , ns1:MedicalEnumeration .

ns1:MedicalRiskCalculator a rdfs:Class ;
	rdfs:label "MedicalRiskCalculator" ;
	dc:source <http://www.w3.org/wiki/WebSchemas/SchemaDotOrgSources#source_WikiDoc> ;
	rdfs:comment "A complex mathematical calculation requiring an online calculator, used to assess prognosis. Note: use the url property of Thing to record any URLs for online calculators." ;
	rdfs:subClassOf ns1:MedicalRiskEstimator .

ns1:MedicalRiskEstimator a rdfs:Class ;
	rdfs:label "MedicalRiskEstimator" ;
	dc:source <http://www.w3.org/wiki/WebSchemas/SchemaDotOrgSources#source_WikiDoc> ;
	rdfs:comment "Any rule set or interactive tool for estimating the risk of developing a complication or condition." ;
	rdfs:subClassOf ns1:MedicalEntity .

ns1:MedicalRiskFactor a rdfs:Class ;
	rdfs:label "MedicalRiskFactor" ;
	dc:source <http://www.w3.org/wiki/WebSchemas/SchemaDotOrgSources#source_WikiDoc> ;
	rdfs:comment "A risk factor is anything that increases a person's likelihood of developing or contracting a disease, medical condition, or complication." ;
	rdfs:subClassOf ns1:MedicalEntity .

ns1:MedicalRiskScore a rdfs:Class ;
	rdfs:label "MedicalRiskScore" ;
	dc:source <http://www.w3.org/wiki/WebSchemas/SchemaDotOrgSources#source_WikiDoc> ;
	rdfs:comment "A simple system that adds up the number of risk factors to yield a score that is associated with prognosis, e.g. CHAD score, TIMI risk score." ;
	rdfs:subClassOf ns1:MedicalRiskEstimator .

ns1:MedicalScholarlyArticle a rdfs:Class ;
	rdfs:label "MedicalScholarlyArticle" ;
	rdfs:comment "A scholarly article in the medical domain." ;
	rdfs:subClassOf ns1:ScholarlyArticle .

ns1:MedicalSign a rdfs:Class ;
	rdfs:label "MedicalSign" ;
	dc:source <http://www.w3.org/wiki/WebSchemas/SchemaDotOrgSources#source_WikiDoc> ;
	rdfs:comment "Any physical manifestation of a person's medical condition discoverable by objective diagnostic tests or physical examination." ;
	rdfs:subClassOf ns1:MedicalSignOrSymptom .

ns1:MedicalSignOrSymptom a rdfs:Class ;
	rdfs:label "MedicalSignOrSymptom" ;
	dc:source <http://www.w3.org/wiki/WebSchemas/SchemaDotOrgSources#source_WikiDoc> ;
	rdfs:comment "Any indication of the existence of a medical condition or disease." ;
	rdfs:subClassOf ns1:MedicalEntity .

ns1:MedicalSpecialty a rdfs:Class ;
	rdfs:label "MedicalSpecialty" ;
	dc:source <http://www.w3.org/wiki/WebSchemas/SchemaDotOrgSources#source_WikiDoc> ;
	rdfs:comment "Any specific branch of medical science or practice. Medical specialities include clinical specialties that pertain to particular organ systems and their respective disease states, as well as allied health specialties. Enumerated type." ;
	rdfs:subClassOf ns1:Enumeration , ns1:MedicalEnumeration , ns1:Specialty .

ns1:MedicalStudy a rdfs:Class ;
	rdfs:label "MedicalStudy" ;
	dc:source <http://www.w3.org/wiki/WebSchemas/SchemaDotOrgSources#source_WikiDoc> ;
	rdfs:comment "A medical study is an umbrella type covering all kinds of research studies relating to human medicine or health, including observational studies and interventional trials and registries, randomized, controlled or not. When the specific type of study is known, use one of the extensions of this type, such as MedicalTrial or MedicalObservationalStudy. Also, note that this type should be used to mark up data that describes the study itself; to tag an article that publishes the results of a study, use MedicalScholarlyArticle. Note: use the code property of MedicalEntity to store study IDs, e.g. clinicaltrials.gov ID." ;
	rdfs:subClassOf ns1:MedicalEntity .

ns1:MedicalStudyStatus a rdfs:Class ;
	rdfs:label "MedicalStudyStatus" ;
	dc:source <http://www.w3.org/wiki/WebSchemas/SchemaDotOrgSources#source_WikiDoc> ;
	rdfs:comment "The status of a medical study. Enumerated type." ;
	rdfs:subClassOf ns1:Enumeration , ns1:MedicalEnumeration .

ns1:MedicalSymptom a rdfs:Class ;
	rdfs:label "MedicalSymptom" ;
	dc:source <http://www.w3.org/wiki/WebSchemas/SchemaDotOrgSources#source_WikiDoc> ;
	rdfs:comment "Any indication of the existence of a medical condition or disease that is apparent to the patient." ;
	rdfs:subClassOf ns1:MedicalSignOrSymptom .

ns1:MedicalTest a rdfs:Class ;
	rdfs:label "MedicalTest" ;
	dc:source <http://www.w3.org/wiki/WebSchemas/SchemaDotOrgSources#source_WikiDoc> ;
	rdfs:comment "Any medical test, typically performed for diagnostic purposes." ;
	rdfs:subClassOf ns1:MedicalEntity .

ns1:MedicalTestPanel a rdfs:Class ;
	rdfs:label "MedicalTestPanel" ;
	dc:source <http://www.w3.org/wiki/WebSchemas/SchemaDotOrgSources#source_WikiDoc> ;
	rdfs:comment "Any collection of tests commonly ordered together." ;
	rdfs:subClassOf ns1:MedicalTest .

ns1:MedicalTherapy a rdfs:Class ;
	rdfs:label "MedicalTherapy" ;
	dc:source <http://www.w3.org/wiki/WebSchemas/SchemaDotOrgSources#source_WikiDoc> ;
	rdfs:comment "Any medical intervention designed to prevent, treat, and cure human diseases and medical conditions, including both curative and palliative therapies. Medical therapies are typically processes of care relying upon pharmacotherapy, behavioral therapy, supportive therapy (with fluid or nutrition for example), or detoxification (e.g. hemodialysis) aimed at improving or preventing a health condition." ;
	rdfs:subClassOf ns1:MedicalEntity .

ns1:MedicalTrial a rdfs:Class ;
	rdfs:label "MedicalTrial" ;
	dc:source <http://www.w3.org/wiki/WebSchemas/SchemaDotOrgSources#source_WikiDoc> ;
	rdfs:comment "A medical trial is a type of medical study that uses scientific process used to compare the safety and efficacy of medical therapies or medical procedures. In general, medical trials are controlled and subjects are allocated at random to the different treatment and/or control groups." ;
	rdfs:subClassOf ns1:MedicalStudy .

ns1:MedicalTrialDesign a rdfs:Class ;
	rdfs:label "MedicalTrialDesign" ;
	dc:source <http://www.w3.org/wiki/WebSchemas/SchemaDotOrgSources#source_WikiDoc> ;
	rdfs:comment "Design models for medical trials. Enumerated type." ;
	rdfs:subClassOf ns1:Enumeration , ns1:MedicalEnumeration .

ns1:MedicalWebPage a rdfs:Class ;
	rdfs:label "MedicalWebPage" ;
	rdfs:comment "A web page that provides medical information." ;
	rdfs:subClassOf ns1:WebPage .

ns1:MedicineSystem a rdfs:Class ;
	rdfs:label "MedicineSystem" ;
	rdfs:comment "Systems of medical practice." ;
	rdfs:subClassOf ns1:Enumeration , ns1:MedicalEnumeration .

ns1:MensClothingStore a rdfs:Class ;
	rdfs:label "MensClothingStore" ;
	rdfs:comment "A men's clothing store." ;
	rdfs:subClassOf ns1:Store .

ns1:MiddleSchool a rdfs:Class ;
	rdfs:label "MiddleSchool" ;
	rdfs:comment "A middle school." ;
	rdfs:subClassOf ns1:EducationalOrganization .

ns1:MobileApplication a rdfs:Class ;
	rdfs:label "MobileApplication" ;
	rdfs:comment "A mobile software application." ;
	rdfs:subClassOf ns1:SoftwareApplication .

ns1:MobilePhoneStore a rdfs:Class ;
	rdfs:label "MobilePhoneStore" ;
	rdfs:comment "A mobile-phone store." ;
	rdfs:subClassOf ns1:Store .

ns1:Mosque a rdfs:Class ;
	rdfs:label "Mosque" ;
	rdfs:comment "A mosque." ;
	rdfs:subClassOf ns1:PlaceOfWorship .

ns1:Motel a rdfs:Class ;
	rdfs:label "Motel" ;
	rdfs:comment "A motel." ;
	rdfs:subClassOf ns1:LodgingBusiness .

ns1:MotorcycleDealer a rdfs:Class ;
	rdfs:label "MotorcycleDealer" ;
	rdfs:comment "A motorcycle dealer." ;
	rdfs:subClassOf ns1:AutomotiveBusiness .

ns1:MotorcycleRepair a rdfs:Class ;
	rdfs:label "MotorcycleRepair" ;
	rdfs:comment "A motorcycle repair shop." ;
	rdfs:subClassOf ns1:AutomotiveBusiness .

ns1:Mountain a rdfs:Class ;
	rdfs:label "Mountain" ;
	rdfs:comment "A mountain, like Mount Whitney or Mount Everest" ;
	rdfs:subClassOf ns1:Landform .

ns1:MoveAction a rdfs:Class ;
	rdfs:label "MoveAction" ;
	rdfs:comment "The act of an agent relocating to a place.<p>Related actions:</p><ul><li><a href=\"http://schema.org/TransferAction\">TransferAction</a>: Unlike TransferAction, the subject of the move is a living Person or Organization rather than an inanimate object.</li></ul>" ;
	rdfs:subClassOf ns1:Action .

ns1:Movie a rdfs:Class ;
	rdfs:label "Movie" ;
	rdfs:comment "A movie." ;
	rdfs:subClassOf ns1:CreativeWork .

ns1:MovieRentalStore a rdfs:Class ;
	rdfs:label "MovieRentalStore" ;
	rdfs:comment "A movie rental store." ;
	rdfs:subClassOf ns1:Store .

ns1:MovieTheater a rdfs:Class ;
	rdfs:label "MovieTheater" ;
	rdfs:comment "A movie theater." ;
	rdfs:subClassOf ns1:CivicStructure , ns1:EntertainmentBusiness .

ns1:MovingCompany a rdfs:Class ;
	rdfs:label "MovingCompany" ;
	rdfs:comment "A moving company." ;
	rdfs:subClassOf ns1:HomeAndConstructionBusiness .

ns1:Muscle a rdfs:Class ;
	rdfs:label "Muscle" ;
	dc:source <http://www.w3.org/wiki/WebSchemas/SchemaDotOrgSources#source_WikiDoc> ;
	rdfs:comment "A muscle is an anatomical structure consisting of a contractile form of tissue that animals use to effect movement." ;
	rdfs:subClassOf ns1:AnatomicalStructure .

ns1:Museum a rdfs:Class ;
	rdfs:label "Museum" ;
	rdfs:comment "A museum." ;
	rdfs:subClassOf ns1:CivicStructure .

ns1:MusicAlbum a rdfs:Class ;
	rdfs:label "MusicAlbum" ;
	rdfs:comment "A collection of music tracks." ;
	rdfs:subClassOf ns1:MusicPlaylist .

ns1:MusicEvent a rdfs:Class ;
	rdfs:label "MusicEvent" ;
	rdfs:comment "Event type: Music event." ;
	rdfs:subClassOf ns1:Event .

ns1:MusicGroup a rdfs:Class ;
	rdfs:label "MusicGroup" ;
	rdfs:comment "A musical group, such as a band, an orchestra, or a choir. Can also be a solo musician." ;
	rdfs:subClassOf ns1:PerformingGroup .

ns1:MusicPlaylist a rdfs:Class ;
	rdfs:label "MusicPlaylist" ;
	rdfs:comment "A collection of music tracks in playlist form." ;
	rdfs:subClassOf ns1:CreativeWork .

ns1:MusicRecording a rdfs:Class ;
	rdfs:label "MusicRecording" ;
	rdfs:comment "A music recording (track), usually a single song." ;
	rdfs:subClassOf ns1:CreativeWork .

ns1:MusicStore a rdfs:Class ;
	rdfs:label "MusicStore" ;
	rdfs:comment "A music store." ;
	rdfs:subClassOf ns1:Store .

ns1:MusicVenue a rdfs:Class ;
	rdfs:label "MusicVenue" ;
	rdfs:comment "A music venue." ;
	rdfs:subClassOf ns1:CivicStructure .

ns1:MusicVideoObject a rdfs:Class ;
	rdfs:label "MusicVideoObject" ;
	rdfs:comment "A music video file." ;
	rdfs:subClassOf ns1:MediaObject .

ns1:NGO a rdfs:Class ;
	rdfs:label "NGO" ;
	rdfs:comment "Organization: Non-governmental Organization." ;
	rdfs:subClassOf ns1:Organization .

ns1:NailSalon a rdfs:Class ;
	rdfs:label "NailSalon" ;
	rdfs:comment "A nail salon." ;
	rdfs:subClassOf ns1:HealthAndBeautyBusiness .

ns1:Nerve a rdfs:Class ;
	rdfs:label "Nerve" ;
	dc:source <http://www.w3.org/wiki/WebSchemas/SchemaDotOrgSources#source_WikiDoc> ;
	rdfs:comment "A common pathway for the electrochemical nerve impulses that are transmitted along each of the axons." ;
	rdfs:subClassOf ns1:AnatomicalStructure .

ns1:NewsArticle a rdfs:Class ;
	rdfs:label "NewsArticle" ;
	dc:source <http://www.w3.org/wiki/WebSchemas/SchemaDotOrgSources#source_rNews> ;
	rdfs:comment "A news article" ;
	rdfs:subClassOf ns1:Article .

ns1:NightClub a rdfs:Class ;
	rdfs:label "NightClub" ;
	rdfs:comment "A nightclub or discotheque." ;
	rdfs:subClassOf ns1:EntertainmentBusiness .

ns1:Notary a rdfs:Class ;
	rdfs:label "Notary" ;
	rdfs:comment "A notary." ;
	rdfs:subClassOf ns1:ProfessionalService .

ns1:Number a rdfs:Class ;
	rdfs:label "Number" ;
	rdfs:comment "Data type: Number." ;
	rdfs:subClassOf ns1:DataType .

ns1:NutritionInformation a rdfs:Class ;
	rdfs:label "NutritionInformation" ;
	rdfs:comment "Nutritional information about the recipe." ;
	rdfs:subClassOf ns1:StructuredValue .

ns1:OceanBodyOfWater a rdfs:Class ;
	rdfs:label "OceanBodyOfWater" ;
	rdfs:comment "An ocean (for example, the Pacific)." ;
	rdfs:subClassOf ns1:BodyOfWater .

ns1:Offer a rdfs:Class ;
	rdfs:label "Offer" ;
	dc:source <http://www.w3.org/wiki/WebSchemas/SchemaDotOrgSources#source_GoodRelationsProperties> ;
	rdfs:comment "An offer to transfer some rights to an item or to provide a service&#x2014;for example, an offer to sell tickets to an event, to rent the DVD of a movie, to stream a TV show over the internet, to repair a motorcycle, or to loan a book." ;
	rdfs:subClassOf ns1:Intangible .

ns1:OfferItemCondition a rdfs:Class ;
	rdfs:label "OfferItemCondition" ;
	rdfs:comment "A list of possible conditions for the item." ;
	rdfs:subClassOf ns1:Enumeration .

ns1:OfficeEquipmentStore a rdfs:Class ;
	rdfs:label "OfficeEquipmentStore" ;
	rdfs:comment "An office equipment store." ;
	rdfs:subClassOf ns1:Store .

ns1:OnDemandEvent a rdfs:Class ;
	rdfs:label "OnDemandEvent" ;
	rdfs:comment "A publication event e.g. catch-up TV or radio podcast, during which a program is available on-demand." ;
	rdfs:subClassOf ns1:PublicationEvent .

ns1:OpeningHoursSpecification a rdfs:Class ;
	rdfs:label "OpeningHoursSpecification" ;
	dc:source <http://www.w3.org/wiki/WebSchemas/SchemaDotOrgSources#source_GoodRelationsClass> ;
	rdfs:comment "A structured value providing information about the opening hours of a place or a certain service inside a place." ;
	rdfs:subClassOf ns1:StructuredValue .

ns1:Optician a rdfs:Class ;
	rdfs:label "Optician" ;
	rdfs:comment "An optician's store." ;
	rdfs:subClassOf ns1:MedicalOrganization .

ns1:Order a rdfs:Class ;
	rdfs:label "Order" ;
	rdfs:comment "An order is a confirmation of a transaction (a receipt), which can contain multiple line items, each represented by an Offer that has been accepted by the customer." ;
	rdfs:subClassOf ns1:Intangible .

ns1:OrderAction a rdfs:Class ;
	rdfs:label "OrderAction" ;
	rdfs:comment "An agent orders an object/product/service to be delivered/sent." ;
	rdfs:subClassOf ns1:TradeAction .

ns1:OrderStatus a rdfs:Class ;
	rdfs:label "OrderStatus" ;
	rdfs:comment "Enumerated status values for Order." ;
	rdfs:subClassOf ns1:Enumeration .

ns1:Organization a rdfs:Class ;
	rdfs:label "Organization" ;
	rdfs:comment "An organization such as a school, NGO, corporation, club, etc." ;
	rdfs:subClassOf ns1:Thing .

ns1:OrganizationRole a rdfs:Class ;
	rdfs:label "OrganizationRole" ;
	rdfs:comment "A subclass of Role used to describe roles within organizations." ;
	rdfs:subClassOf ns1:Role .

ns1:OrganizeAction a rdfs:Class ;
	rdfs:label "OrganizeAction" ;
	rdfs:comment "The act of manipulating/administering/supervising/controlling one or more objects." ;
	rdfs:subClassOf ns1:Action .

ns1:OutletStore a rdfs:Class ;
	rdfs:label "OutletStore" ;
	rdfs:comment "An outlet store." ;
	rdfs:subClassOf ns1:Store .

ns1:OwnershipInfo a rdfs:Class ;
	rdfs:label "OwnershipInfo" ;
	dc:source <http://www.w3.org/wiki/WebSchemas/SchemaDotOrgSources#source_GoodRelationsClass> ;
	rdfs:comment "A structured value providing information about when a certain organization or person owned a certain product." ;
	rdfs:subClassOf ns1:StructuredValue .

ns1:PaintAction a rdfs:Class ;
	rdfs:label "PaintAction" ;
	rdfs:comment "The act of producing a painting, typically with paint and canvas as instruments." ;
	rdfs:subClassOf ns1:CreateAction .

ns1:Painting a rdfs:Class ;
	rdfs:label "Painting" ;
	rdfs:comment "A painting." ;
	rdfs:subClassOf ns1:CreativeWork .

ns1:PalliativeProcedure a rdfs:Class ;
	rdfs:label "PalliativeProcedure" ;
	dc:source <http://www.w3.org/wiki/WebSchemas/SchemaDotOrgSources#source_WikiDoc> ;
	rdfs:comment "A medical procedure intended primarily for palliative purposes, aimed at relieving the symptoms of an underlying health condition." ;
	rdfs:subClassOf ns1:MedicalProcedure , ns1:MedicalTherapy .

ns1:ParcelDelivery a rdfs:Class ;
	rdfs:label "ParcelDelivery" ;
	rdfs:comment "The delivery of a parcel either via the postal service or a commercial service." ;
	rdfs:subClassOf ns1:Intangible .

ns1:ParcelService a rdfs:Class ;
	rdfs:label "ParcelService" ;
	dc:source <http://www.w3.org/wiki/WebSchemas/SchemaDotOrgSources#source_GoodRelationsClass> ;
	rdfs:comment """A private parcel service as the delivery mode available for a certain offer.

    Commonly used values:

    http://purl.org/goodrelations/v1#DHL
    http://purl.org/goodrelations/v1#FederalExpress
    http://purl.org/goodrelations/v1#UPS
    	""" ;
	rdfs:subClassOf ns1:DeliveryMethod .

ns1:ParentAudience a rdfs:Class ;
	rdfs:label "ParentAudience" ;
	rdfs:comment "A set of characteristics describing parents, who can be interested in viewing some content" ;
	rdfs:subClassOf ns1:PeopleAudience .

ns1:Park a rdfs:Class ;
	rdfs:label "Park" ;
	rdfs:comment "A park." ;
	rdfs:subClassOf ns1:CivicStructure .

ns1:ParkingFacility a rdfs:Class ;
	rdfs:label "ParkingFacility" ;
	rdfs:comment "A parking lot or other parking facility." ;
	rdfs:subClassOf ns1:CivicStructure .

ns1:PathologyTest a rdfs:Class ;
	rdfs:label "PathologyTest" ;
	dc:source <http://www.w3.org/wiki/WebSchemas/SchemaDotOrgSources#source_WikiDoc> ;
	rdfs:comment "A medical test performed by a laboratory that typically involves examination of a tissue sample by a pathologist." ;
	rdfs:subClassOf ns1:MedicalTest .

ns1:PawnShop a rdfs:Class ;
	rdfs:label "PawnShop" ;
	rdfs:comment "A pawn store." ;
	rdfs:subClassOf ns1:Store .

ns1:PayAction a rdfs:Class ;
	rdfs:label "PayAction" ;
	rdfs:comment "An agent pays a price to a participant." ;
	rdfs:subClassOf ns1:TradeAction .

ns1:PaymentChargeSpecification a rdfs:Class ;
	rdfs:label "PaymentChargeSpecification" ;
	dc:source <http://www.w3.org/wiki/WebSchemas/SchemaDotOrgSources#source_GoodRelationsClass> ;
	rdfs:comment "The costs of settling the payment using a particular payment method." ;
	rdfs:subClassOf ns1:PriceSpecification .

ns1:PaymentMethod a rdfs:Class ;
	rdfs:label "PaymentMethod" ;
	dc:source <http://www.w3.org/wiki/WebSchemas/SchemaDotOrgSources#source_GoodRelationsClass> ;
	rdfs:comment """A payment method is a standardized procedure for transferring the monetary amount for a purchase. Payment methods are characterized by the legal and technical structures used, and by the organization or group carrying out the transaction.

    Commonly used values:

    http://purl.org/goodrelations/v1#ByBankTransferInAdvance
    http://purl.org/goodrelations/v1#ByInvoice
    http://purl.org/goodrelations/v1#Cash
    http://purl.org/goodrelations/v1#CheckInAdvance
    http://purl.org/goodrelations/v1#COD
    http://purl.org/goodrelations/v1#DirectDebit
    http://purl.org/goodrelations/v1#GoogleCheckout
    http://purl.org/goodrelations/v1#PayPal
    http://purl.org/goodrelations/v1#PaySwarm
    		""" ;
	rdfs:subClassOf ns1:Enumeration .

ns1:PeopleAudience a rdfs:Class ;
	rdfs:label "PeopleAudience" ;
	rdfs:comment "A set of characteristics belonging to people, e.g. who compose an item's target audience." ;
	rdfs:subClassOf ns1:Audience .

ns1:PerformAction a rdfs:Class ;
	rdfs:label "PerformAction" ;
	rdfs:comment "The act of participating in performance arts." ;
	rdfs:subClassOf ns1:PlayAction .

ns1:PerformanceRole a rdfs:Class ;
	rdfs:label "PerformanceRole" ;
	rdfs:comment "A PerformanceRole is a Role that some entity places with regard to a theatrical performance, e.g. in a Movie, TVSeries etc." ;
	rdfs:subClassOf ns1:Role .

ns1:PerformingArtsTheater a rdfs:Class ;
	rdfs:label "PerformingArtsTheater" ;
	rdfs:comment "A theater or other performing art center." ;
	rdfs:subClassOf ns1:CivicStructure .

ns1:PerformingGroup a rdfs:Class ;
	rdfs:label "PerformingGroup" ;
	rdfs:comment "A performance group, such as a band, an orchestra, or a circus." ;
	rdfs:subClassOf ns1:Organization .

ns1:Permit a rdfs:Class ;
	rdfs:label "Permit" ;
	rdfs:comment "A permit issued by an organization, e.g. a parking pass." ;
	rdfs:subClassOf ns1:Intangible .

ns1:Person a rdfs:Class ;
	rdfs:label "Person" ;
	dc:source <http://www.w3.org/wiki/WebSchemas/SchemaDotOrgSources#source_rNews> ;
	rdfs:comment "A person (alive, dead, undead, or fictional)." ;
	rdfs:subClassOf ns1:Thing ;
	owl:equivalentClass <foaf:Person> .

ns1:PetStore a rdfs:Class ;
	rdfs:label "PetStore" ;
	rdfs:comment "A pet store." ;
	rdfs:subClassOf ns1:Store .

ns1:Pharmacy a rdfs:Class ;
	rdfs:label "Pharmacy" ;
	rdfs:comment "A pharmacy or drugstore." ;
	rdfs:subClassOf ns1:MedicalOrganization .

ns1:Photograph a rdfs:Class ;
	rdfs:label "Photograph" ;
	rdfs:comment "A photograph." ;
	rdfs:subClassOf ns1:CreativeWork .

ns1:PhotographAction a rdfs:Class ;
	rdfs:label "PhotographAction" ;
	rdfs:comment "The act of capturing still images of objects using a camera." ;
	rdfs:subClassOf ns1:CreateAction .

ns1:PhysicalActivity a rdfs:Class ;
	rdfs:label "PhysicalActivity" ;
	dc:source <http://www.w3.org/wiki/WebSchemas/SchemaDotOrgSources#source_WikiDoc> ;
	rdfs:comment "Any bodily activity that enhances or maintains physical fitness and overall health and wellness. Includes activity that is part of daily living and routine, structured exercise, and exercise prescribed as part of a medical treatment or recovery plan." ;
	rdfs:subClassOf ns1:LifestyleModification .

ns1:PhysicalActivityCategory a rdfs:Class ;
	rdfs:label "PhysicalActivityCategory" ;
	dc:source <http://www.w3.org/wiki/WebSchemas/SchemaDotOrgSources#source_WikiDoc> ;
	rdfs:comment "Categories of physical activity, organized by physiologic classification." ;
	rdfs:subClassOf ns1:Enumeration , ns1:MedicalEnumeration .

ns1:PhysicalExam a rdfs:Class ;
	rdfs:label "PhysicalExam" ;
	dc:source <http://www.w3.org/wiki/WebSchemas/SchemaDotOrgSources#source_WikiDoc> ;
	rdfs:comment "A type of physical examination of a patient performed by a physician. Enumerated type." ;
	rdfs:subClassOf ns1:Enumeration , ns1:MedicalEnumeration .

ns1:PhysicalTherapy a rdfs:Class ;
	rdfs:label "PhysicalTherapy" ;
	dc:source <http://www.w3.org/wiki/WebSchemas/SchemaDotOrgSources#source_WikiDoc> ;
	rdfs:comment "A process of progressive physical care and rehabilitation aimed at improving a health condition." ;
	rdfs:subClassOf ns1:MedicalTherapy .

ns1:Physician a rdfs:Class ;
	rdfs:label "Physician" ;
	rdfs:comment "A doctor's office." ;
	rdfs:subClassOf ns1:MedicalOrganization .

ns1:Place a rdfs:Class ;
	rdfs:label "Place" ;
	rdfs:comment "Entities that have a somewhat fixed, physical extension." ;
	rdfs:subClassOf ns1:Thing .

ns1:PlaceOfWorship a rdfs:Class ;
	rdfs:label "PlaceOfWorship" ;
	rdfs:comment "Place of worship, such as a church, synagogue, or mosque." ;
	rdfs:subClassOf ns1:CivicStructure .

ns1:PlanAction a rdfs:Class ;
	rdfs:label "PlanAction" ;
	rdfs:comment "The act of planning the execution of an event/task/action/reservation/plan to a future date." ;
	rdfs:subClassOf ns1:OrganizeAction .

ns1:PlayAction a rdfs:Class ;
	rdfs:label "PlayAction" ;
	rdfs:comment "The act of playing/exercising/training/performing for enjoyment, leisure, recreation, Competition or exercise.<p>Related actions:</p><ul><li><a href=\"http://schema.org/ListenAction\">ListenAction</a>: Unlike ListenAction (which is under ConsumeAction), PlayAction refers to performing for an audience or at an event, rather than consuming music.</li><li><a href=\"http://schema.org/WatchAction\">WatchAction</a>: Unlike WatchAction (which is under ConsumeAction), PlayAction refers to showing/displaying for an audience or at an event, rather than consuming visual content.</li></ul>" ;
	rdfs:subClassOf ns1:Action .

ns1:Playground a rdfs:Class ;
	rdfs:label "Playground" ;
	rdfs:comment "A playground." ;
	rdfs:subClassOf ns1:CivicStructure .

ns1:Plumber a rdfs:Class ;
	rdfs:label "Plumber" ;
	rdfs:comment "A plumbing service." ;
	rdfs:subClassOf ns1:HomeAndConstructionBusiness , ns1:ProfessionalService .

ns1:PoliceStation a rdfs:Class ;
	rdfs:label "PoliceStation" ;
	rdfs:comment "A police station." ;
	rdfs:subClassOf ns1:CivicStructure , ns1:EmergencyService .

ns1:Pond a rdfs:Class ;
	rdfs:label "Pond" ;
	rdfs:comment "A pond" ;
	rdfs:subClassOf ns1:BodyOfWater .

ns1:PostOffice a rdfs:Class ;
	rdfs:label "PostOffice" ;
	rdfs:comment "A post office." ;
	rdfs:subClassOf ns1:GovernmentOffice .

ns1:PostalAddress a rdfs:Class ;
	rdfs:label "PostalAddress" ;
	rdfs:comment "The mailing address." ;
	rdfs:subClassOf ns1:ContactPoint .

ns1:PrependAction a rdfs:Class ;
	rdfs:label "PrependAction" ;
	rdfs:comment "The act of inserting at the beginning if an ordered collection." ;
	rdfs:subClassOf ns1:InsertAction .

ns1:Preschool a rdfs:Class ;
	rdfs:label "Preschool" ;
	rdfs:comment "A preschool." ;
	rdfs:subClassOf ns1:EducationalOrganization .

ns1:PreventionIndication a rdfs:Class ;
	rdfs:label "PreventionIndication" ;
	dc:source <http://www.w3.org/wiki/WebSchemas/SchemaDotOrgSources#source_WikiDoc> ;
	rdfs:comment "An indication for preventing an underlying condition, symptom, etc." ;
	rdfs:subClassOf ns1:MedicalIndication .

ns1:PriceSpecification a rdfs:Class ;
	rdfs:label "PriceSpecification" ;
	dc:source <http://www.w3.org/wiki/WebSchemas/SchemaDotOrgSources#source_GoodRelationsClass> ;
	rdfs:comment "A structured value representing a monetary amount. Typically, only the subclasses of this type are used for markup." ;
	rdfs:subClassOf ns1:StructuredValue .

ns1:Product a rdfs:Class ;
	rdfs:label "Product" ;
	dc:source <http://www.w3.org/wiki/WebSchemas/SchemaDotOrgSources#source_GoodRelationsProperties> ;
	rdfs:comment "Any offered product or service. For example: a pair of shoes; a concert ticket; the rental of a car; a haircut; or an episode of a TV show streamed online." ;
	rdfs:subClassOf ns1:Thing .

ns1:ProductModel a rdfs:Class ;
	rdfs:label "ProductModel" ;
	dc:source <http://www.w3.org/wiki/WebSchemas/SchemaDotOrgSources#source_GoodRelationsClass> ;
	rdfs:comment "A datasheet or vendor specification of a product (in the sense of a prototypical description)." ;
	rdfs:subClassOf ns1:Product .

ns1:ProfessionalService a rdfs:Class ;
	rdfs:label "ProfessionalService" ;
	rdfs:comment "Provider of professional services." ;
	rdfs:subClassOf ns1:LocalBusiness .

ns1:ProfilePage a rdfs:Class ;
	rdfs:label "ProfilePage" ;
	rdfs:comment "Web page type: Profile page." ;
	rdfs:subClassOf ns1:WebPage .

ns1:ProgramMembership a rdfs:Class ;
	rdfs:label "Program Membership" ;
	rdfs:comment "Used to describe membership in a loyalty programs (e.g. \"StarAliance\"), traveler clubs (e.g. \"AAA\"), purchase clubs (\"Safeway Club\"), etc." ;
	rdfs:subClassOf ns1:Intangible .

ns1:Property a rdfs:Class ;
	rdfs:label "Property" ;
	rdfs:comment "A property, used to indicate attributes and relationships of some Thing; equivalent to rdf:Property." ;
	rdfs:subClassOf ns1:Intangible .

ns1:PropertyValueSpecification a rdfs:Class ;
	rdfs:label "PropertyValueSpecification" ;
	dc:source <http://www.w3.org/wiki/WebSchemas/SchemaDotOrgSources#source_ActionCollabClass> ;
	rdfs:comment "A Property value specification." ;
	rdfs:subClassOf ns1:Intangible .

ns1:PsychologicalTreatment a rdfs:Class ;
	rdfs:label "PsychologicalTreatment" ;
	dc:source <http://www.w3.org/wiki/WebSchemas/SchemaDotOrgSources#source_WikiDoc> ;
	rdfs:comment "A process of care relying upon counseling, dialogue, communication, verbalization aimed at improving a mental health condition." ;
	rdfs:subClassOf ns1:MedicalTherapy .

ns1:PublicSwimmingPool a rdfs:Class ;
	rdfs:label "PublicSwimmingPool" ;
	rdfs:comment "A public swimming pool." ;
	rdfs:subClassOf ns1:SportsActivityLocation .

ns1:PublicationEvent a rdfs:Class ;
	rdfs:label "PublicationEvent" ;
	rdfs:comment "A PublicationEvent corresponds indifferently to the event of publication for a CreativeWork of any type e.g. a broadcast event, an on-demand event, a book/journal publication via a variety of delivery media." ;
	rdfs:subClassOf ns1:Event .

ns1:QAPage a rdfs:Class ;
	rdfs:label "QAPage" ;
	rdfs:comment "A QAPage is a WebPage focussed on a specific Question and its Answer(s), e.g. in a question answering site or documenting Frequently Asked Questions (FAQs)." ;
	rdfs:subClassOf ns1:WebPage .

ns1:QualitativeValue a rdfs:Class ;
	rdfs:label "QualitativeValue" ;
	dc:source <http://www.w3.org/wiki/WebSchemas/SchemaDotOrgSources#source_GoodRelationsClass> ;
	rdfs:comment "A predefined value for a product characteristic, e.g. the the power cord plug type \"US\" or the garment sizes \"S\", \"M\", \"L\", and \"XL\"" ;
	rdfs:subClassOf ns1:Enumeration .

ns1:QuantitativeValue a rdfs:Class ;
	rdfs:label "QuantitativeValue" ;
	dc:source <http://www.w3.org/wiki/WebSchemas/SchemaDotOrgSources#source_GoodRelationsClass> ;
	rdfs:comment " A point value or interval for product characteristics and other purposes." ;
	rdfs:subClassOf ns1:StructuredValue .

ns1:Quantity a rdfs:Class ;
	rdfs:label "Quantity" ;
	rdfs:comment "Quantities such as distance, time, mass, weight, etc. Particular instances of say Mass are entities like '3 Kg' or '4 milligrams'." ;
	rdfs:subClassOf ns1:Intangible .

ns1:Question a rdfs:Class ;
	rdfs:label "Question" ;
	dc:source <http://www.w3.org/wiki/WebSchemas/SchemaDotOrgSources#source_QAStackExchange> ;
	rdfs:comment "A specific question - e.g. from a user seeking answers online, or collected in a Frequently Asked Questions (FAQ) document." ;
	rdfs:subClassOf ns1:CreativeWork .

ns1:QuoteAction a rdfs:Class ;
	rdfs:label "QuoteAction" ;
	rdfs:comment "An agent quotes/estimates/appraises an object/product/service with a price at a location/store." ;
	rdfs:subClassOf ns1:TradeAction .

ns1:RVPark a rdfs:Class ;
	rdfs:label "RVPark" ;
	rdfs:comment "An RV park." ;
	rdfs:subClassOf ns1:CivicStructure .

ns1:RadiationTherapy a rdfs:Class ;
	rdfs:label "RadiationTherapy" ;
	dc:source <http://www.w3.org/wiki/WebSchemas/SchemaDotOrgSources#source_WikiDoc> ;
	rdfs:comment "A process of care using radiation aimed at improving a health condition." ;
	rdfs:subClassOf ns1:MedicalTherapy .

ns1:RadioClip a rdfs:Class ;
	rdfs:label "RadioClip" ;
	rdfs:comment "A short radio program or a segment/part of a radio program." ;
	rdfs:subClassOf ns1:Clip .

ns1:RadioEpisode a rdfs:Class ;
	rdfs:label "RadioEpisode" ;
	rdfs:comment "A radio episode which can be part of a series or season." ;
	rdfs:subClassOf ns1:Episode .

ns1:RadioSeason a rdfs:Class ;
	rdfs:label "RadioSeason" ;
	rdfs:comment "Season dedicated to radio broadcast and associated online delivery." ;
	rdfs:subClassOf ns1:Season .

ns1:RadioSeries a rdfs:Class ;
	rdfs:label "RadioSeries" ;
	rdfs:comment "Series dedicated to radio broadcast and associated online delivery." ;
	rdfs:subClassOf ns1:Series .

ns1:RadioStation a rdfs:Class ;
	rdfs:label "RadioStation" ;
	rdfs:comment "A radio station." ;
	rdfs:subClassOf ns1:LocalBusiness .

ns1:Rating a rdfs:Class ;
	rdfs:label "Rating" ;
	rdfs:comment "The rating of the video." ;
	rdfs:subClassOf ns1:Intangible .

ns1:ReactAction a rdfs:Class ;
	rdfs:label "ReactAction" ;
	rdfs:comment "The act of responding instinctively and emotionally to an object, expressing a sentiment." ;
	rdfs:subClassOf ns1:AssessAction .

ns1:ReadAction a rdfs:Class ;
	rdfs:label "ReadAction" ;
	rdfs:comment "The act of consuming written content." ;
	rdfs:subClassOf ns1:ConsumeAction .

ns1:RealEstateAgent a rdfs:Class ;
	rdfs:label "RealEstateAgent" ;
	rdfs:comment "A real-estate agent." ;
	rdfs:subClassOf ns1:LocalBusiness .

ns1:ReceiveAction a rdfs:Class ;
	rdfs:label "ReceiveAction" ;
	rdfs:comment "The act of physically/electronically taking delivery of an object thathas been transferred from an origin to a destination. Reciprocal of SendAction.<p>Related actions:</p><ul><li><a href=\"http://schema.org/SendAction\">SendAction</a>: The reciprocal of ReceiveAction.</li><li><a href=\"http://schema.org/TakeAction\">TakeAction</a>: Unlike TakeAction, ReceiveAction does not imply that the ownership has been transfered (e.g. I can receive a package, but it does not mean the package is now mine).</li></ul>" ;
	rdfs:subClassOf ns1:TransferAction .

ns1:Recipe a rdfs:Class ;
	rdfs:label "Recipe" ;
	rdfs:comment "A recipe." ;
	rdfs:subClassOf ns1:CreativeWork .

ns1:RecommendedDoseSchedule a rdfs:Class ;
	rdfs:label "RecommendedDoseSchedule" ;
	rdfs:comment "A recommended dosing schedule for a drug or supplement as prescribed or recommended by an authority or by the drug/supplement's manufacturer. Capture the recommending authority in the recognizingAuthority property of MedicalEntity." ;
	rdfs:subClassOf ns1:DoseSchedule .

ns1:RecyclingCenter a rdfs:Class ;
	rdfs:label "RecyclingCenter" ;
	rdfs:comment "A recycling center." ;
	rdfs:subClassOf ns1:LocalBusiness .

ns1:RegisterAction a rdfs:Class ;
	rdfs:label "RegisterAction" ;
	rdfs:comment "The act of registering to be a user of a service, product or web page.<p>Related actions:</p><ul><li><a href=\"http://schema.org/JoinAction\">JoinAction</a>: Unlike JoinAction, RegisterAction implies you are registering to be a user of a service, *not* a group/team of people.</li><li><a href=\"http://schema.org/FollowAction\">FollowAction</a>: Unlike FollowAction, RegisterAction doesn't imply that the agent is expecting to poll for updates from the object.</li><li><a href=\"http://schema.org/SubscribeAction\">SubscribeAction</a>: Unlike SubscribeAction, RegisterAction doesn't imply that the agent is expecting updates from the object.</li></ul>" ;
	rdfs:subClassOf ns1:InteractAction .

ns1:RejectAction a rdfs:Class ;
	rdfs:label "RejectAction" ;
	rdfs:comment "The act of rejecting to/adopting an object.<p>Related actions:</p><ul><li><a href=\"http://schema.org/AcceptAction\">AcceptAction</a>: The antagonym of RejectAction.</li></ul>" ;
	rdfs:subClassOf ns1:AllocateAction .

ns1:RentAction a rdfs:Class ;
	rdfs:label "RentAction" ;
	rdfs:comment "The act of giving money in return for temporary use, but not ownership, of an object such as a vehicle or property. For example, an agent rents a property from a landlord in exchange for a periodic payment." ;
	rdfs:subClassOf ns1:TradeAction .

ns1:RentalCarReservation a rdfs:Class ;
	rdfs:label "RentalCarReservation" ;
	rdfs:comment "A reservation for a rental car.Note: This type is for information about actual reservations, e.g. in confirmation emails or HTML pages with individual confirmations of reservations." ;
	rdfs:subClassOf ns1:Reservation .

ns1:ReplaceAction a rdfs:Class ;
	rdfs:label "ReplaceAction" ;
	rdfs:comment "The act of editing a recipient by replacing an old object with a new object." ;
	rdfs:subClassOf ns1:UpdateAction .

ns1:ReplyAction a rdfs:Class ;
	rdfs:label "ReplyAction" ;
	rdfs:comment "The act of responding to a question/message asked/sent by the object. Related to <a href=\"AskAction\">AskAction</a>.<p>Related actions:</p><ul><li><a href=\"http://schema.org/AskAction\">AskAction</a>: Appears generally as an origin of a ReplyAction.</li></ul>" ;
	rdfs:subClassOf ns1:CommunicateAction .

ns1:ReportedDoseSchedule a rdfs:Class ;
	rdfs:label "ReportedDoseSchedule" ;
	rdfs:comment "A patient-reported or observed dosing schedule for a drug or supplement." ;
	rdfs:subClassOf ns1:DoseSchedule .

ns1:Reservation a rdfs:Class ;
	rdfs:label "Reservation" ;
	rdfs:comment "Describes a reservation for travel, dining or an event. Some reservations require tickets.Note: This type is for information about actual reservations, e.g. in confirmation emails or HTML pages with individual confirmations of reservations. For offers of tickets, restaurant reservations, flights, or rental cars, use http://schema.org/Offer." ;
	rdfs:subClassOf ns1:Intangible .

ns1:ReservationPackage a rdfs:Class ;
	rdfs:label "ReservationPackage" ;
	rdfs:comment "A group of multiple reservations with common values for all sub-reservations." ;
	rdfs:subClassOf ns1:Reservation .

ns1:ReservationStatusType a rdfs:Class ;
	rdfs:label "ReservationStatusType" ;
	rdfs:comment "Enumerated status values for Reservation." ;
	rdfs:subClassOf ns1:Enumeration .

ns1:ReserveAction a rdfs:Class ;
	rdfs:label "ReserveAction" ;
	rdfs:comment "Reserving a concrete object.<p>Related actions:</p><ul><li><a href=\"http://schema.org/ScheduleAction\">ScheduleAction</a>: Unlike ScheduleAction, ReserveAction reserves concrete objects (e.g. a table, a hotel) towards a time slot / spatial allocation.</li></ul>" ;
	rdfs:subClassOf ns1:PlanAction .

ns1:Reservoir a rdfs:Class ;
	rdfs:label "Reservoir" ;
	rdfs:comment "A reservoir, like the Lake Kariba reservoir." ;
	rdfs:subClassOf ns1:BodyOfWater .

ns1:Residence a rdfs:Class ;
	rdfs:label "Residence" ;
	rdfs:comment "The place where a person lives." ;
	rdfs:subClassOf ns1:Place .

ns1:Restaurant a rdfs:Class ;
	rdfs:label "Restaurant" ;
	rdfs:comment "A restaurant." ;
	rdfs:subClassOf ns1:FoodEstablishment .

ns1:ReturnAction a rdfs:Class ;
	rdfs:label "ReturnAction" ;
	rdfs:comment "The act of returning to the origin that which was previously received (concrete objects) or taken (ownership)." ;
	rdfs:subClassOf ns1:TransferAction .

ns1:Review a rdfs:Class ;
	rdfs:label "Review" ;
	rdfs:comment "A review of an item - for example, a restaurant, movie, or store." ;
	rdfs:subClassOf ns1:CreativeWork .

ns1:ReviewAction a rdfs:Class ;
	rdfs:label "ReviewAction" ;
	rdfs:comment "The act of producing a balanced opinion about the object for an audience. An agent reviews an object with participants resulting in a review." ;
	rdfs:subClassOf ns1:AssessAction .

ns1:RiverBodyOfWater a rdfs:Class ;
	rdfs:label "RiverBodyOfWater" ;
	rdfs:comment "A river (for example, the broad majestic Shannon)." ;
	rdfs:subClassOf ns1:BodyOfWater .

ns1:Role a rdfs:Class ;
	rdfs:label "Role" ;
	rdfs:comment """Represents additional information about a relationship or property. For example a Role can be used to say that a 'member' role linking some SportsTeam to a player occured during a particular time period. Or that a Person's 'actor' role in a Movie was for some particular characterName. Such properties can be attached to a Role entity, which is then associated with the main entities using ordinary properties like 'member' or 'actor'.
    """ ;
	rdfs:subClassOf ns1:Intangible .

ns1:RoofingContractor a rdfs:Class ;
	rdfs:label "RoofingContractor" ;
	rdfs:comment "A roofing contractor." ;
	rdfs:subClassOf ns1:HomeAndConstructionBusiness , ns1:ProfessionalService .

ns1:RsvpAction a rdfs:Class ;
	rdfs:label "RsvpAction" ;
	rdfs:comment "The act of notifying an event organizer as to whether you expect to attend the event." ;
	rdfs:subClassOf ns1:InformAction .

ns1:SaleEvent a rdfs:Class ;
	rdfs:label "SaleEvent" ;
	rdfs:comment "Event type: Sales event." ;
	rdfs:subClassOf ns1:Event .

ns1:ScheduleAction a rdfs:Class ;
	rdfs:label "ScheduleAction" ;
	rdfs:comment "Scheduling future actions, events, or tasks.<p>Related actions:</p><ul><li><a href=\"http://schema.org/ReserveAction\">ReserveAction</a>: Unlike ReserveAction, ScheduleAction allocates future actions (e.g. an event, a task, etc) towards a time slot / spatial allocation.</li></ul>" ;
	rdfs:subClassOf ns1:PlanAction .

ns1:ScholarlyArticle a rdfs:Class ;
	rdfs:label "ScholarlyArticle" ;
	rdfs:comment "A scholarly article." ;
	rdfs:subClassOf ns1:Article .

ns1:School a rdfs:Class ;
	rdfs:label "School" ;
	rdfs:comment "A school." ;
	rdfs:subClassOf ns1:EducationalOrganization .

ns1:Sculpture a rdfs:Class ;
	rdfs:label "Sculpture" ;
	rdfs:comment "A piece of sculpture." ;
	rdfs:subClassOf ns1:CreativeWork .

ns1:SeaBodyOfWater a rdfs:Class ;
	rdfs:label "SeaBodyOfWater" ;
	rdfs:comment "A sea (for example, the Caspian sea)." ;
	rdfs:subClassOf ns1:BodyOfWater .

ns1:SearchAction a rdfs:Class ;
	rdfs:label "SearchAction" ;
	rdfs:comment "The act of searching for an object.<p>Related actions:</p><ul><li><a href=\"http://schema.org/FindAction\">FindAction</a>: SearchAction generally leads to a FindAction, but not necessarily.</li></ul>" ;
	rdfs:subClassOf ns1:Action .

ns1:SearchResultsPage a rdfs:Class ;
	rdfs:label "SearchResultsPage" ;
	rdfs:comment "Web page type: Search results page." ;
	rdfs:subClassOf ns1:WebPage .

ns1:Season a rdfs:Class ;
	rdfs:label "Season" ;
	rdfs:comment "A TV or radio season." ;
	rdfs:subClassOf ns1:CreativeWork .

ns1:Seat a rdfs:Class ;
	rdfs:label "Seat" ;
	rdfs:comment "Used to describe a seat, such as a reserved seat in an event reservation." ;
	rdfs:subClassOf ns1:Intangible .

ns1:SelfStorage a rdfs:Class ;
	rdfs:label "SelfStorage" ;
	rdfs:comment "Self-storage facility." ;
	rdfs:subClassOf ns1:LocalBusiness .

ns1:SellAction a rdfs:Class ;
	rdfs:label "SellAction" ;
	rdfs:comment "The act of taking money from a buyer in exchange for goods or services rendered. An agent sells an object, product, or service to a buyer for a price. Reciprocal of BuyAction." ;
	rdfs:subClassOf ns1:TradeAction .

ns1:SendAction a rdfs:Class ;
	rdfs:label "SendAction" ;
	rdfs:comment "The act of physically/electronically dispatching an object for transfer from an origin to a destination.<p>Related actions:</p><ul><li><a href=\"http://schema.org/ReceiveAction\">ReceiveAction</a>: The reciprocal of SendAction.</li><li><a href=\"http://schema.org/GiveAction\">GiveAction</a>: Unlike GiveAction, SendAction does not imply the transfer of ownership (e.g. I can send you my laptop, but I'm not necessarily giving it to you).</li></ul>" ;
	rdfs:subClassOf ns1:TransferAction .

ns1:Series a rdfs:Class ;
	rdfs:label "Series" ;
	rdfs:comment "A TV or radio series." ;
	rdfs:subClassOf ns1:CreativeWork .

ns1:Service a rdfs:Class ;
	rdfs:label "Service" ;
	rdfs:comment "A service provided by an organization, e.g. delivery service, print services, etc." ;
	rdfs:subClassOf ns1:Intangible .

ns1:ServiceChannel a rdfs:Class ;
	rdfs:label "ServiceChannel" ;
	rdfs:comment "A means for accessing a service, e.g. a government office location, web site, or phone number." ;
	rdfs:subClassOf ns1:Intangible .

ns1:ShareAction a rdfs:Class ;
	rdfs:label "ShareAction" ;
	rdfs:comment "The act of distributing content to people for their amusement or edification." ;
	rdfs:subClassOf ns1:CommunicateAction .

ns1:ShoeStore a rdfs:Class ;
	rdfs:label "ShoeStore" ;
	rdfs:comment "A shoe store." ;
	rdfs:subClassOf ns1:Store .

ns1:ShoppingCenter a rdfs:Class ;
	rdfs:label "ShoppingCenter" ;
	rdfs:comment "A shopping center or mall." ;
	rdfs:subClassOf ns1:LocalBusiness .

ns1:SingleFamilyResidence a rdfs:Class ;
	rdfs:label "SingleFamilyResidence" ;
	rdfs:comment "Residence type: Single-family home." ;
	rdfs:subClassOf ns1:Residence .

ns1:SiteNavigationElement a rdfs:Class ;
	rdfs:label "SiteNavigationElement" ;
	rdfs:comment "A navigation element of the page." ;
	rdfs:subClassOf ns1:WebPageElement .

ns1:SkiResort a rdfs:Class ;
	rdfs:label "SkiResort" ;
	rdfs:comment "A ski resort." ;
	rdfs:subClassOf ns1:SportsActivityLocation .

ns1:SocialEvent a rdfs:Class ;
	rdfs:label "SocialEvent" ;
	rdfs:comment "Event type: Social event." ;
	rdfs:subClassOf ns1:Event .

ns1:SoftwareApplication a rdfs:Class ;
	rdfs:label "SoftwareApplication" ;
	rdfs:comment "A software application." ;
	rdfs:subClassOf ns1:CreativeWork .

ns1:SomeProducts a rdfs:Class ;
	rdfs:label "SomeProducts" ;
	dc:source <http://www.w3.org/wiki/WebSchemas/SchemaDotOrgSources#source_GoodRelationsClass> ;
	rdfs:comment "A placeholder for multiple similar products of the same kind." ;
	rdfs:subClassOf ns1:Product .

ns1:Specialty a rdfs:Class ;
	rdfs:label "Specialty" ;
	rdfs:comment "Any branch of a field in which people typically develop specific expertise, usually after significant study, time, and effort." ;
	rdfs:subClassOf ns1:Enumeration .

ns1:SportingGoodsStore a rdfs:Class ;
	rdfs:label "SportingGoodsStore" ;
	rdfs:comment "A sporting goods store." ;
	rdfs:subClassOf ns1:Store .

ns1:SportsActivityLocation a rdfs:Class ;
	rdfs:label "SportsActivityLocation" ;
	rdfs:comment "A sports location, such as a playing field." ;
	rdfs:subClassOf ns1:LocalBusiness .

ns1:SportsClub a rdfs:Class ;
	rdfs:label "SportsClub" ;
	rdfs:comment "A sports club." ;
	rdfs:subClassOf ns1:SportsActivityLocation .

ns1:SportsEvent a rdfs:Class ;
	rdfs:label "SportsEvent" ;
	rdfs:comment "Event type: Sports event." ;
	rdfs:subClassOf ns1:Event .

ns1:SportsTeam a rdfs:Class ;
	rdfs:label "SportsTeam" ;
	rdfs:comment "Organization: Sports team." ;
	rdfs:subClassOf ns1:Organization .

ns1:StadiumOrArena a rdfs:Class ;
	rdfs:label "StadiumOrArena" ;
	rdfs:comment "A stadium." ;
	rdfs:subClassOf ns1:CivicStructure , ns1:SportsActivityLocation .

ns1:State a rdfs:Class ;
	rdfs:label "State" ;
	rdfs:comment "A state or province." ;
	rdfs:subClassOf ns1:AdministrativeArea .

ns1:Store a rdfs:Class ;
	rdfs:label "Store" ;
	rdfs:comment "A retail good store." ;
	rdfs:subClassOf ns1:LocalBusiness .

ns1:StructuredValue a rdfs:Class ;
	rdfs:label "StructuredValue" ;
	rdfs:comment "Structured values are strings&#x2014;for example, addresses&#x2014;that have certain constraints on their structure." ;
	rdfs:subClassOf ns1:Intangible .

ns1:SubscribeAction a rdfs:Class ;
	rdfs:label "SubscribeAction" ;
	rdfs:comment "The act of forming a personal connection with someone/something (object) unidirectionally/asymmetrically to get updates pushed to.<p>Related actions:</p><ul><li><a href=\"http://schema.org/FollowAction\">FollowAction</a>: Unlike FollowAction, SubscribeAction implies that the subscriber acts as a passive agent being constantly/actively pushed for updates.</li><li><a href=\"http://schema.org/RegisterAction\">RegisterAction</a>: Unlike RegisterAction, SubscribeAction implies that the agent is interested in continuing receiving updates from the object.</li><li><a href=\"http://schema.org/JoinAction\">JoinAction</a>: Unlike JoinAction, SubscribeAction implies that the agent is interested in continuing receiving updates from the object.</li></ul>" ;
	rdfs:subClassOf ns1:InteractAction .

ns1:SubwayStation a rdfs:Class ;
	rdfs:label "SubwayStation" ;
	rdfs:comment "A subway station." ;
	rdfs:subClassOf ns1:CivicStructure .

ns1:SuperficialAnatomy a rdfs:Class ;
	rdfs:label "SuperficialAnatomy" ;
	dc:source <http://www.w3.org/wiki/WebSchemas/SchemaDotOrgSources#source_WikiDoc> ;
	rdfs:comment "Anatomical features that can be observed by sight (without dissection), including the form and proportions of the human body as well as surface landmarks that correspond to deeper subcutaneous structures. Superficial anatomy plays an important role in sports medicine, phlebotomy, and other medical specialties as underlying anatomical structures can be identified through surface palpation. For example, during back surgery, superficial anatomy can be used to palpate and count vertebrae to find the site of incision. Or in phlebotomy, superficial anatomy can be used to locate an underlying vein; for example, the median cubital vein can be located by palpating the borders of the cubital fossa (such as the epicondyles of the humerus) and then looking for the superficial signs of the vein, such as size, prominence, ability to refill after depression, and feel of surrounding tissue support. As another example, in a subluxation (dislocation) of the glenohumeral joint, the bony structure becomes pronounced with the deltoid muscle failing to cover the glenohumeral joint allowing the edges of the scapula to be superficially visible. Here, the superficial anatomy is the visible edges of the scapula, implying the underlying dislocation of the joint (the related anatomical structure)." ;
	rdfs:subClassOf ns1:MedicalEntity .

ns1:Synagogue a rdfs:Class ;
	rdfs:label "Synagogue" ;
	rdfs:comment "A synagogue." ;
	rdfs:subClassOf ns1:PlaceOfWorship .

ns1:TVClip a rdfs:Class ;
	rdfs:label "TVClip" ;
	rdfs:comment "A short TV program or a segment/part of a TV program." ;
	rdfs:subClassOf ns1:Clip .

ns1:TVEpisode a rdfs:Class ;
	rdfs:label "TVEpisode" ;
	rdfs:comment "A TV episode which can be part of a series or season." ;
	rdfs:subClassOf ns1:Episode .

ns1:TVSeason a rdfs:Class ;
	rdfs:label "TVSeason" ;
	rdfs:comment "Season dedicated to TV broadcast and associated online delivery." ;
	rdfs:subClassOf ns1:CreativeWork , ns1:Season .

ns1:TVSeries a rdfs:Class ;
	rdfs:label "TVSeries" ;
	rdfs:comment "Series dedicated to TV broadcast and associated online delivery." ;
	rdfs:subClassOf ns1:CreativeWork , ns1:Series .

ns1:Table a rdfs:Class ;
	rdfs:label "Table" ;
	rdfs:comment "A table on the page." ;
	rdfs:subClassOf ns1:WebPageElement .

ns1:TakeAction a rdfs:Class ;
	rdfs:label "TakeAction" ;
	rdfs:comment "The act of gaining ownership of an object from an origin. Reciprocal of GiveAction.<p>Related actions:</p><ul><li><a href=\"http://schema.org/GiveAction\">GiveAction</a>: The reciprocal of TakeAction.</li><li><a href=\"http://schema.org/ReceiveAction\">ReceiveAction</a>: Unlike ReceiveAction, TakeAction implies that ownership has been transfered.</li></ul>" ;
	rdfs:subClassOf ns1:TransferAction .

ns1:TattooParlor a rdfs:Class ;
	rdfs:label "TattooParlor" ;
	rdfs:comment "A tattoo parlor." ;
	rdfs:subClassOf ns1:HealthAndBeautyBusiness .

ns1:Taxi a rdfs:Class ;
	rdfs:label "Taxi" ;
	rdfs:comment "A taxi." ;
	rdfs:subClassOf ns1:Service .

ns1:TaxiReservation a rdfs:Class ;
	rdfs:label " TaxiReservation" ;
	rdfs:comment "A reservation for a taxi.Note: This type is for information about actual reservations, e.g. in confirmation emails or HTML pages with individual confirmations of reservations. For offers of tickets, use http://schema.org/Offer." ;
	rdfs:subClassOf ns1:Reservation .

ns1:TaxiStand a rdfs:Class ;
	rdfs:label "TaxiStand" ;
	rdfs:comment "A taxi stand." ;
	rdfs:subClassOf ns1:CivicStructure .

ns1:TechArticle a rdfs:Class ;
	rdfs:label "TechArticle" ;
	rdfs:comment "A technical article - Example: How-to (task) topics, step-by-step, procedural troubleshooting, specifications, etc." ;
	rdfs:subClassOf ns1:Article .

ns1:TelevisionStation a rdfs:Class ;
	rdfs:label "TelevisionStation" ;
	rdfs:comment "A television station." ;
	rdfs:subClassOf ns1:LocalBusiness .

ns1:TennisComplex a rdfs:Class ;
	rdfs:label "TennisComplex" ;
	rdfs:comment "A tennis complex." ;
	rdfs:subClassOf ns1:SportsActivityLocation .

ns1:Text a rdfs:Class ;
	rdfs:label "Text" ;
	rdfs:comment "Data type: Text." ;
	rdfs:subClassOf ns1:DataType .

ns1:TheaterEvent a rdfs:Class ;
	rdfs:label "TheaterEvent" ;
	rdfs:comment "Event type: Theater performance." ;
	rdfs:subClassOf ns1:Event .

ns1:TheaterGroup a rdfs:Class ;
	rdfs:label "TheaterGroup" ;
	rdfs:comment "A theater group or company&#x2014;for example, the Royal Shakespeare Company or Druid Theatre." ;
	rdfs:subClassOf ns1:PerformingGroup .

ns1:TherapeuticProcedure a rdfs:Class ;
	rdfs:label "TherapeuticProcedure" ;
	dc:source <http://www.w3.org/wiki/WebSchemas/SchemaDotOrgSources#source_WikiDoc> ;
	rdfs:comment "A medical procedure intended primarily for therapeutic purposes, aimed at improving a health condition." ;
	rdfs:subClassOf ns1:MedicalProcedure , ns1:MedicalTherapy .

ns1:Thing a rdfs:Class ;
	rdfs:label "Thing" ;
	rdfs:comment "The most generic type of item." .

ns1:Ticket a rdfs:Class ;
	rdfs:label "Ticket" ;
	rdfs:comment "Used to describe a ticket to an event, a flight, a bus ride, etc." ;
	rdfs:subClassOf ns1:Intangible .

ns1:TieAction a rdfs:Class ;
	rdfs:label "TieAction" ;
	rdfs:comment "The act of reaching a draw in a competitive activity." ;
	rdfs:subClassOf ns1:AchieveAction .

ns1:Time a rdfs:Class ;
	rdfs:label "Time" ;
	rdfs:comment "A point in time recurring on multiple days in the form hh:mm:ss[Z|(+|-)hh:mm] (see <a href=\"http://www.w3.org/TR/xmlschema-2/#time\">XML schema for details</a>)." ;
	rdfs:subClassOf ns1:DataType .

ns1:TipAction a rdfs:Class ;
	rdfs:label "TipAction" ;
	rdfs:comment "The act of giving money voluntarily to a beneficiary in recognition of services rendered." ;
	rdfs:subClassOf ns1:TradeAction .

ns1:TireShop a rdfs:Class ;
	rdfs:label "TireShop" ;
	rdfs:comment "A tire shop." ;
	rdfs:subClassOf ns1:Store .

ns1:TouristAttraction a rdfs:Class ;
	rdfs:label "TouristAttraction" ;
	rdfs:comment "A tourist attraction." ;
	rdfs:subClassOf ns1:Place .

ns1:TouristInformationCenter a rdfs:Class ;
	rdfs:label "TouristInformationCenter" ;
	rdfs:comment "A tourist information center." ;
	rdfs:subClassOf ns1:LocalBusiness .

ns1:ToyStore a rdfs:Class ;
	rdfs:label "ToyStore" ;
	rdfs:comment "A toy store." ;
	rdfs:subClassOf ns1:Store .

ns1:TrackAction a rdfs:Class ;
	rdfs:label "TrackAction" ;
	rdfs:comment "An agent tracks an object for updates.<p>Related actions:</p><ul><li><a href=\"http://schema.org/FollowAction\">FollowAction</a>: Unlike FollowAction, TrackAction refers to the interest on the location of innanimates objects.</li><li><a href=\"http://schema.org/SubscribeAction\">SubscribeAction</a>: Unlike SubscribeAction, TrackAction refers to  the interest on the location of innanimate objects.</li></ul>" ;
	rdfs:subClassOf ns1:FindAction .

ns1:TradeAction a rdfs:Class ;
	rdfs:label "TradeAction" ;
	rdfs:comment "The act of participating in an exchange of goods and services for monetary compensation. An agent trades an object, product or service with a participant in exchange for a one time or periodic payment." ;
	rdfs:subClassOf ns1:Action .

ns1:TrainReservation a rdfs:Class ;
	rdfs:label " TrainReservation" ;
	rdfs:comment "A reservation for train travel.Note: This type is for information about actual reservations, e.g. in confirmation emails or HTML pages with individual confirmations of reservations. For offers of tickets, use http://schema.org/Offer." ;
	rdfs:subClassOf ns1:Reservation .

ns1:TrainStation a rdfs:Class ;
	rdfs:label "TrainStation" ;
	rdfs:comment "A train station." ;
	rdfs:subClassOf ns1:CivicStructure .

ns1:TrainTrip a rdfs:Class ;
	rdfs:label "Train Trip" ;
	rdfs:comment "A trip on a commercial train line." ;
	rdfs:subClassOf ns1:Intangible .

ns1:TransferAction a rdfs:Class ;
	rdfs:label "TransferAction" ;
	rdfs:comment "The act of transferring/moving (abstract or concrete) animate or inanimate objects from one place to another." ;
	rdfs:subClassOf ns1:Action .

ns1:TravelAction a rdfs:Class ;
	rdfs:label "TravelAction" ;
	rdfs:comment "The act of traveling from an fromLocation to a destination by a specified mode of transport, optionally with participants." ;
	rdfs:subClassOf ns1:MoveAction .

ns1:TravelAgency a rdfs:Class ;
	rdfs:label "TravelAgency" ;
	rdfs:comment "A travel agency." ;
	rdfs:subClassOf ns1:LocalBusiness .

ns1:TreatmentIndication a rdfs:Class ;
	rdfs:label "TreatmentIndication" ;
	dc:source <http://www.w3.org/wiki/WebSchemas/SchemaDotOrgSources#source_WikiDoc> ;
	rdfs:comment "An indication for treating an underlying condition, symptom, etc." ;
	rdfs:subClassOf ns1:MedicalIndication .

ns1:TypeAndQuantityNode a rdfs:Class ;
	rdfs:label "TypeAndQuantityNode" ;
	dc:source <http://www.w3.org/wiki/WebSchemas/SchemaDotOrgSources#source_GoodRelationsClass> ;
	rdfs:comment "A structured value indicating the quantity, unit of measurement, and business function of goods included in a bundle offer." ;
	rdfs:subClassOf ns1:StructuredValue .

ns1:URL a rdfs:Class ;
	rdfs:label "URL" ;
	rdfs:comment "Data type: URL." ;
	rdfs:subClassOf ns1:Text .

ns1:UnRegisterAction a rdfs:Class ;
	rdfs:label "UnRegisterAction" ;
	rdfs:comment "The act of un-registering from a service.<p>Related actions:</p><ul><li><a href=\"http://schema.org/RegisterAction\">RegisterAction</a>: Antagonym of UnRegisterAction.</li><li><a href=\"http://schema.org/Leave\">Leave</a>: Unlike LeaveAction, UnRegisterAction implies that you are unregistering from a service you werer previously registered, rather than leaving a team/group of people.</li></ul>" ;
	rdfs:subClassOf ns1:InteractAction .

ns1:UnitPriceSpecification a rdfs:Class ;
	rdfs:label "UnitPriceSpecification" ;
	dc:source <http://www.w3.org/wiki/WebSchemas/SchemaDotOrgSources#source_GoodRelationsClass> ;
	rdfs:comment "The price asked for a given offer by the respective organization or person." ;
	rdfs:subClassOf ns1:PriceSpecification .

ns1:UpdateAction a rdfs:Class ;
	rdfs:label "UpdateAction" ;
	rdfs:comment "The act of managing by changing/editing the state of the object." ;
	rdfs:subClassOf ns1:Action .

ns1:UseAction a rdfs:Class ;
	rdfs:label "UseAction" ;
	rdfs:comment "The act of applying an object to its intended purpose." ;
	rdfs:subClassOf ns1:ConsumeAction .

ns1:UserBlocks a rdfs:Class ;
	rdfs:label "UserBlocks" ;
	rdfs:comment "User interaction: Block this content." ;
	rdfs:subClassOf ns1:UserInteraction .

ns1:UserCheckins a rdfs:Class ;
	rdfs:label "UserCheckins" ;
	rdfs:comment "User interaction: Check-in at a place." ;
	rdfs:subClassOf ns1:UserInteraction .

ns1:UserComments a rdfs:Class ;
	rdfs:label "UserComments" ;
	dc:source <http://www.w3.org/wiki/WebSchemas/SchemaDotOrgSources#source_rNews> ;
	rdfs:comment "The UserInteraction event in which a user comments on an item." ;
	rdfs:subClassOf ns1:UserInteraction .

ns1:UserDownloads a rdfs:Class ;
	rdfs:label "UserDownloads" ;
	rdfs:comment "User interaction: Download of an item." ;
	rdfs:subClassOf ns1:UserInteraction .

ns1:UserInteraction a rdfs:Class ;
	rdfs:label "UserInteraction" ;
	rdfs:comment "A user interacting with a page" ;
	rdfs:subClassOf ns1:Event .

ns1:UserLikes a rdfs:Class ;
	rdfs:label "UserLikes" ;
	rdfs:comment "User interaction: Like an item." ;
	rdfs:subClassOf ns1:UserInteraction .

ns1:UserPageVisits a rdfs:Class ;
	rdfs:label "UserPageVisits" ;
	rdfs:comment "User interaction: Visit to a web page." ;
	rdfs:subClassOf ns1:UserInteraction .

ns1:UserPlays a rdfs:Class ;
	rdfs:label "UserPlays" ;
	rdfs:comment "User interaction: Play count of an item, for example a video or a song." ;
	rdfs:subClassOf ns1:UserInteraction .

ns1:UserPlusOnes a rdfs:Class ;
	rdfs:label "UserPlusOnes" ;
	rdfs:comment "User interaction: +1." ;
	rdfs:subClassOf ns1:UserInteraction .

ns1:UserTweets a rdfs:Class ;
	rdfs:label "UserTweets" ;
	rdfs:comment "User interaction: Tweets." ;
	rdfs:subClassOf ns1:UserInteraction .

ns1:Vehicle a rdfs:Class ;
	rdfs:label "Vehicle" ;
	rdfs:comment "A vehicle." ;
	rdfs:subClassOf ns1:Product .

ns1:Vein a rdfs:Class ;
	rdfs:label "Vein" ;
	dc:source <http://www.w3.org/wiki/WebSchemas/SchemaDotOrgSources#source_WikiDoc> ;
	rdfs:comment "A type of blood vessel that specifically carries blood to the heart." ;
	rdfs:subClassOf ns1:Vessel .

ns1:Vessel a rdfs:Class ;
	rdfs:label "Vessel" ;
	dc:source <http://www.w3.org/wiki/WebSchemas/SchemaDotOrgSources#source_WikiDoc> ;
	rdfs:comment "A component of the human body circulatory system comprised of an intricate network of hollow tubes that transport blood throughout the entire body." ;
	rdfs:subClassOf ns1:AnatomicalStructure .

ns1:VeterinaryCare a rdfs:Class ;
	rdfs:label "VeterinaryCare" ;
	rdfs:comment "A vet's office." ;
	rdfs:subClassOf ns1:MedicalOrganization .

ns1:VideoGallery a rdfs:Class ;
	rdfs:label "VideoGallery" ;
	rdfs:comment "Web page type: Video gallery page." ;
	rdfs:subClassOf ns1:CollectionPage .

ns1:VideoObject a rdfs:Class ;
	rdfs:label "VideoObject" ;
	dc:source <http://www.w3.org/wiki/WebSchemas/SchemaDotOrgSources#source_rNews> ;
	rdfs:comment "A video file." ;
	rdfs:subClassOf ns1:MediaObject .

ns1:ViewAction a rdfs:Class ;
	rdfs:label "ViewAction" ;
	rdfs:comment "The act of consuming static visual content." ;
	rdfs:subClassOf ns1:ConsumeAction .

ns1:VisualArtsEvent a rdfs:Class ;
	rdfs:label "VisualArtsEvent" ;
	rdfs:comment "Event type: Visual arts event." ;
	rdfs:subClassOf ns1:Event .

ns1:Volcano a rdfs:Class ;
	rdfs:label "Volcano" ;
	rdfs:comment "A volcano, like Fuji san." ;
	rdfs:subClassOf ns1:Landform .

ns1:VoteAction a rdfs:Class ;
	rdfs:label "VoteAction" ;
	rdfs:comment "The act of expressing a preference from a fixed/finite/structured set of choices/options." ;
	rdfs:subClassOf ns1:ChooseAction .

ns1:WPAdBlock a rdfs:Class ;
	rdfs:label "WPAdBlock" ;
	rdfs:comment "An advertising section of the page." ;
	rdfs:subClassOf ns1:WebPageElement .

ns1:WPFooter a rdfs:Class ;
	rdfs:label "WPFooter" ;
	rdfs:comment "The footer section of the page." ;
	rdfs:subClassOf ns1:WebPageElement .

ns1:WPHeader a rdfs:Class ;
	rdfs:label "WPHeader" ;
	rdfs:comment "The header section of the page." ;
	rdfs:subClassOf ns1:WebPageElement .

ns1:WPSideBar a rdfs:Class ;
	rdfs:label "WPSideBar" ;
	rdfs:comment "A sidebar section of the page." ;
	rdfs:subClassOf ns1:WebPageElement .

ns1:WantAction a rdfs:Class ;
	rdfs:label "WantAction" ;
	rdfs:comment "The act of expressing a desire about the object. An agent wants an object." ;
	rdfs:subClassOf ns1:ReactAction .

ns1:WarrantyPromise a rdfs:Class ;
	rdfs:label "WarrantyPromise" ;
	dc:source <http://www.w3.org/wiki/WebSchemas/SchemaDotOrgSources#source_GoodRelationsClass> ;
	rdfs:comment "A structured value representing the duration and scope of services that will be provided to a customer free of charge in case of a defect or malfunction of a product." ;
	rdfs:subClassOf ns1:StructuredValue .

ns1:WarrantyScope a rdfs:Class ;
	rdfs:label "WarrantyScope" ;
	dc:source <http://www.w3.org/wiki/WebSchemas/SchemaDotOrgSources#source_GoodRelationsClass> ;
	rdfs:comment """A range of of services that will be provided to a customer free of charge in case of a defect or malfunction of a product.

    Commonly used values:

    http://purl.org/goodrelations/v1#Labor-BringIn
    http://purl.org/goodrelations/v1#PartsAndLabor-BringIn
    http://purl.org/goodrelations/v1#PartsAndLabor-PickUp
    	""" ;
	rdfs:subClassOf ns1:Enumeration .

ns1:WatchAction a rdfs:Class ;
	rdfs:label "WatchAction" ;
	rdfs:comment "The act of consuming dynamic/moving visual content." ;
	rdfs:subClassOf ns1:ConsumeAction .

ns1:Waterfall a rdfs:Class ;
	rdfs:label "Waterfall" ;
	rdfs:comment "A waterfall, like Niagara" ;
	rdfs:subClassOf ns1:BodyOfWater .

ns1:WearAction a rdfs:Class ;
	rdfs:label "WearAction" ;
	rdfs:comment "The act of dressing oneself in clothing." ;
	rdfs:subClassOf ns1:UseAction .

ns1:WebApplication a rdfs:Class ;
	rdfs:label "WebApplication" ;
	rdfs:comment "Web applications." ;
	rdfs:subClassOf ns1:SoftwareApplication .

ns1:WebPage a rdfs:Class ;
	rdfs:label "WebPage" ;
	rdfs:comment "A web page. Every web page is implicitly assumed to be declared to be of type WebPage, so the various properties about that webpage, such as <code>breadcrumb</code> may be used. We recommend explicit declaration if these properties are specified, but if they are found outside of an itemscope, they will be assumed to be about the page" ;
	rdfs:subClassOf ns1:CreativeWork .

ns1:WebPageElement a rdfs:Class ;
	rdfs:label "WebPageElement" ;
	rdfs:comment "A web page element, like a table or an image" ;
	rdfs:subClassOf ns1:CreativeWork .

ns1:WholesaleStore a rdfs:Class ;
	rdfs:label "WholesaleStore" ;
	rdfs:comment "A wholesale store." ;
	rdfs:subClassOf ns1:Store .

ns1:WinAction a rdfs:Class ;
	rdfs:label "WinAction" ;
	rdfs:comment "The act of achieving victory in a competitive activity." ;
	rdfs:subClassOf ns1:AchieveAction .

ns1:Winery a rdfs:Class ;
	rdfs:label "Winery" ;
	rdfs:comment "A winery." ;
	rdfs:subClassOf ns1:FoodEstablishment .

ns1:WriteAction a rdfs:Class ;
	rdfs:label "WriteAction" ;
	rdfs:comment "The act of authoring written creative content." ;
	rdfs:subClassOf ns1:CreateAction .

ns1:Zoo a rdfs:Class ;
	rdfs:label "Zoo" ;
	rdfs:comment "A zoo." ;
	rdfs:subClassOf ns1:CivicStructure .

ns1:Abdomen a ns1:PhysicalExam ;
	rdfs:label "Abdomen" ;
	rdfs:comment "Abdomen" .

ns1:ActiveActionStatus a ns1:ActionStatusType ;
	rdfs:label "ActiveActionStatus" ;
	rdfs:comment "An in-progress action (e.g, while watching the movie, or driving to a location)." .

ns1:ActiveNotRecruiting a ns1:MedicalStudyStatus ;
	rdfs:label "ActiveNotRecruiting" ;
	rdfs:comment "Active, but not recruiting new participants." .

ns1:AerobicActivity a ns1:PhysicalActivityCategory ;
	rdfs:label "AerobicActivity" ;
	rdfs:comment "Physical activity of relatively low intensity that depends primarily on the aerobic energy-generating process; during activity, the aerobic metabolism uses oxygen to adequately meet energy demands during exercise." .

ns1:AnaerobicActivity a ns1:PhysicalActivityCategory ;
	rdfs:label "AnaerobicActivity" ;
	rdfs:comment "Physical activity that is of high-intensity which utilizes the anaerobic metabolism of the body." .

ns1:Anesthesia a ns1:MedicalSpecialty ;
	rdfs:label "Anesthesia" ;
	rdfs:comment "A specific branch of medical science that pertains to study of anesthetics and their application." .

ns1:Appearance a ns1:PhysicalExam ;
	rdfs:label "Appearance" ;
	rdfs:comment "Appearance" .

ns1:Ayurvedic a ns1:MedicineSystem ;
	rdfs:label "Ayurvedic" ;
	rdfs:comment "A system of medicine that originated in India over thousands of years and that focuses on integrating and balancing the body, mind, and spirit." .

ns1:Bacteria a ns1:InfectiousAgentClass ;
	rdfs:label "Bacteria" ;
	rdfs:comment "Pathogenic bacteria that cause bacterial infection." .

ns1:Balance a ns1:PhysicalActivityCategory ;
	rdfs:label "Balance" ;
	rdfs:comment "Physical activity that is engaged to help maintain posture and balance." .

ns1:CT a ns1:MedicalImagingTechnique ;
	rdfs:label "CT" ;
	rdfs:comment "X-ray computed tomography imaging." .

ns1:Cardiovascular a ns1:MedicalSpecialty ;
	rdfs:label "Cardiovascular" ;
	rdfs:comment "A specific branch of medical science that pertains to diagnosis and treatment of disorders of heart and vasculature." .

ns1:CardiovascularExam a ns1:PhysicalExam ;
	rdfs:label "CardiovascularExam" ;
	rdfs:comment "Cardiovascular" .

ns1:CaseSeries a ns1:MedicalObservationalStudyDesign ;
	rdfs:label "CaseSeries" ;
	rdfs:comment "A case series (also known as a clinical series) is a medical research study that tracks patients with a known exposure given similar treatment or examines their medical records for exposure and outcome. A case series can be retrospective or prospective and usually involves a smaller number of patients than the more powerful case-control studies or randomized controlled trials. Case series may be consecutive or non-consecutive, depending on whether all cases presenting to the reporting authors over a period of time were included, or only a selection." .

ns1:Chiropractic a ns1:MedicineSystem ;
	rdfs:label "Chiropractic" ;
	rdfs:comment "A system of medicine focused on the relationship between the body's structure, mainly the spine, and its functioning." .

ns1:Clinician a ns1:MedicalAudience ;
	rdfs:label "Clinician" ;
	rdfs:comment "Medical clinicians, including practicing physicians and other medical professionals involved in clinical practice." .

ns1:CohortStudy a ns1:MedicalObservationalStudyDesign ;
	rdfs:label "CohortStudy" ;
	rdfs:comment "Also known as a panel study. A cohort study is a form of longitudinal study used in medicine and social science. It is one type of study design and should be compared with a cross-sectional study.  A cohort is a group of people who share a common characteristic or experience within a defined period (e.g., are born, leave school, lose their job, are exposed to a drug or a vaccine, etc.). The comparison group may be the general population from which the cohort is drawn, or it may be another cohort of persons thought to have had little or no exposure to the substance under investigation, but otherwise similar. Alternatively, subgroups within the cohort may be compared with each other." .

ns1:CommunityHealth a ns1:MedicalSpecialty ;
	rdfs:label "CommunityHealth" ;
	rdfs:comment "Community health." .

ns1:Completed a ns1:MedicalStudyStatus ;
	rdfs:label "Completed" ;
	rdfs:comment "Completed." .

ns1:CompletedActionStatus a ns1:ActionStatusType ;
	rdfs:label "CompletedActionStatus" ;
	rdfs:comment "An action that has already taken place." .

ns1:CrossSectional a ns1:MedicalObservationalStudyDesign ;
	rdfs:label "CrossSectional" ;
	rdfs:comment "Studies carried out on pre-existing data (usually from 'snapshot' surveys), such as that collected by the Census Bureau. Sometimes called Prevalence Studies." .

ns1:DamagedCondition a ns1:OfferItemCondition ;
	rdfs:label "DamagedCondition" ;
	rdfs:comment "Indicates that the item is damaged." .

ns1:Dentistry a ns1:MedicalSpecialty ;
	rdfs:label "Dentistry" ;
	rdfs:comment "Dentistry." .

ns1:Dermatologic a ns1:MedicalSpecialty ;
	rdfs:label "Dermatologic" ;
	rdfs:comment "A specific branch of medical science that pertains to diagnosis and treatment of disorders of skin." .

ns1:Diagnostic a ns1:MedicalDevicePurpose ;
	rdfs:label "Diagnostic" ;
	rdfs:comment "A medical device used for diagnostic purposes." .

ns1:DietNutrition a ns1:MedicalSpecialty ;
	rdfs:label "DietNutrition" ;
	rdfs:comment "Diet and nutrition." .

ns1:Discontinued a ns1:ItemAvailability ;
	rdfs:label "Discontinued" ;
	rdfs:comment "Indicates that the item has been discontinued." .

ns1:DoubleBlindedTrial a ns1:MedicalTrialDesign ;
	rdfs:label "DoubleBlindedTrial" ;
	rdfs:comment "A trial design in which neither the researcher nor the patient knows the details of the treatment the patient was randomly assigned to." .

ns1:EBook a ns1:BookFormatType ;
	rdfs:label "EBook" ;
	rdfs:comment "Book format: Ebook." .

ns1:Ear a ns1:PhysicalExam ;
	rdfs:label "Ear" ;
	rdfs:comment "Ear" .

ns1:Emergency a ns1:MedicalSpecialty ;
	rdfs:label "Emergency" ;
	rdfs:comment "A specific branch of medical science that is deals with the evaluation and initial treatment of medical conditions caused by trauma or sudden illness." .

ns1:Endocrine a ns1:MedicalSpecialty ;
	rdfs:label "Endocrine" ;
	rdfs:comment "A specific branch of medical science that pertains to diagnosis and treatment of disorders of endocrine glands and their secretions." .

ns1:EnrollingByInvitation a ns1:MedicalStudyStatus ;
	rdfs:label "EnrollingByInvitation" ;
	rdfs:comment "Enrolling participants by invitation only." .

ns1:EventCancelled a ns1:EventStatusType ;
	rdfs:label "EventCancelled" ;
	rdfs:comment "The event has been cancelled. If the event has multiple startDate values, all are assumed to be cancelled. Either startDate or previousStartDate may be used to specify the events cancelled date(s)." .

ns1:EventPostponed a ns1:EventStatusType ;
	rdfs:label "EventPostponed" ;
	rdfs:comment "The event has been postponed and no new date has been set. The events previousStartDate should be set." .

ns1:EventRescheduled a ns1:EventStatusType ;
	rdfs:label "EventRescheduled" ;
	rdfs:comment "The event has been rescheduled. The events previousStartDate should be set to the old date and the startDate should be set to the events new date. (If the event has been rescheduled multiple times, the previousStartDate property may be repeated.)" .

ns1:EventScheduled a ns1:EventStatusType ;
	rdfs:label "EventScheduled" ;
	rdfs:comment "The event is taking place or has taken place on the startDate as scheduled. Use of this value is optional, as it is assumed by default." .

ns1:EvidenceLevelA a ns1:MedicalEvidenceLevel ;
	rdfs:label "EvidenceLevelA" ;
	rdfs:comment "Data derived from multiple randomized clinical trials or meta-analyses." .

ns1:EvidenceLevelB a ns1:MedicalEvidenceLevel ;
	rdfs:label "EvidenceLevelB" ;
	rdfs:comment "Data derived from a single randomized trial, or nonrandomized studies." .

ns1:EvidenceLevelC a ns1:MedicalEvidenceLevel ;
	rdfs:label "EvidenceLevelC" ;
	rdfs:comment "Only consensus opinion of experts, case studies, or standard-of-care." .

ns1:Eye a ns1:PhysicalExam ;
	rdfs:label "Eye" ;
	rdfs:comment "Eye" .

ns1:FDAcategoryA a ns1:DrugPregnancyCategory ;
	rdfs:label "FDAcategoryA" ;
	rdfs:comment "A designation by the US FDA signifying that adequate and well-controlled studies have failed to demonstrate a risk to the fetus in the first trimester of pregnancy (and there is no evidence of risk in later trimesters)." .

ns1:FDAcategoryB a ns1:DrugPregnancyCategory ;
	rdfs:label "FDAcategoryB" ;
	rdfs:comment "A designation by the US FDA signifying that animal reproduction studies have failed to demonstrate a risk to the fetus and there are no adequate and well-controlled studies in pregnant women." .

ns1:FDAcategoryC a ns1:DrugPregnancyCategory ;
	rdfs:label "FDAcategoryC" ;
	rdfs:comment "A designation by the US FDA signifying that animal reproduction studies have shown an adverse effect on the fetus and there are no adequate and well-controlled studies in humans, but potential benefits may warrant use of the drug in pregnant women despite potential risks." .

ns1:FDAcategoryD a ns1:DrugPregnancyCategory ;
	rdfs:label "FDAcategoryD" ;
	rdfs:comment "A designation by the US FDA signifying that there is positive evidence of human fetal risk based on adverse reaction data from investigational or marketing experience or studies in humans, but potential benefits may warrant use of the drug in pregnant women despite potential risks." .

ns1:FDAcategoryX a ns1:DrugPregnancyCategory ;
	rdfs:label "FDAcategoryX" ;
	rdfs:comment "A designation by the US FDA signifying that studies in animals or humans have demonstrated fetal abnormalities and/or there is positive evidence of human fetal risk based on adverse reaction data from investigational or marketing experience, and the risks involved in use of the drug in pregnant women clearly outweigh potential benefits." .

ns1:FDAnotEvaluated a ns1:DrugPregnancyCategory ;
	rdfs:label "FDAnotEvaluated" ;
	rdfs:comment "A designation that the drug in question has not been assigned a pregnancy category designation by the US FDA." .

ns1:False a ns1:Boolean ;
	rdfs:label "False" ;
	rdfs:comment "The boolean value false" ;
	rdfs:subClassOf ns1:Boolean .

ns1:Flexibility a ns1:PhysicalActivityCategory ;
	rdfs:label "Flexibility" ;
	rdfs:comment "Physical activity that is engaged in to improve joint and muscle flexibility." .

ns1:Fungus a ns1:InfectiousAgentClass ;
	rdfs:label "Fungus" ;
	rdfs:comment "Pathogenic fungus." .

ns1:Gastroenterologic a ns1:MedicalSpecialty ;
	rdfs:label "Gastroenterologic" ;
	rdfs:comment "A specific branch of medical science that pertains to diagnosis and treatment of disorders of digestive system." .

ns1:Genetic a ns1:MedicalSpecialty ;
	rdfs:label "Genetic" ;
	rdfs:comment "A specific branch of medical science that pertains to hereditary transmission and the variation of inherited characteristics and disorders." .

ns1:Genitourinary a ns1:PhysicalExam ;
	rdfs:label "Genitourinary" ;
	rdfs:comment "Genitourinary" .

ns1:Geriatric a ns1:MedicalSpecialty ;
	rdfs:label "Geriatric" ;
	rdfs:comment "A specific branch of medical science that is concerned with the diagnosis and treatment of diseases, debilities and provision of care to the aged." .

ns1:Gynecologic a ns1:MedicalSpecialty ;
	rdfs:label "Gynecologic" ;
	rdfs:comment "A specific branch of medical science that pertains to the health care of women, particularly in the diagnosis and treatment of disorders affecting the female reproductive system." .

ns1:Hardcover a ns1:BookFormatType ;
	rdfs:label "Hardcover" ;
	rdfs:comment "Book format: Hardcover." .

ns1:Head a ns1:PhysicalExam ;
	rdfs:label "Head" ;
	rdfs:comment "Head" .

ns1:HearingImpairedSupported a ns1:ContactPointOption ;
	rdfs:label "HearingImpairedSupported" ;
	rdfs:comment "Uses devices to support users with hearing impairments." .

ns1:Hematologic a ns1:MedicalSpecialty ;
	rdfs:label "Hematologic" ;
	rdfs:comment "A specific branch of medical science that pertains to diagnosis and treatment of disorders of blood and blood producing organs." .

ns1:Homeopathic a ns1:MedicineSystem ;
	rdfs:label "Homeopathic" ;
	rdfs:comment "A system of medicine based on the principle that a disease can be cured by a substance that produces similar symptoms in healthy people." .

ns1:InStock a ns1:ItemAvailability ;
	rdfs:label "InStock" ;
	rdfs:comment "Indicates that the item is in stock." .

ns1:InStoreOnly a ns1:ItemAvailability ;
	rdfs:label "InStoreOnly" ;
	rdfs:comment "Indicates that the item is available only at physical locations." .

ns1:Infectious a ns1:MedicalSpecialty ;
	rdfs:label "Infectious" ;
	rdfs:comment "A specific branch of medical science that pertains to diagnosis and treatment of bacterial, viral, fungal and parasitic infections." .

ns1:InternationalTrial a ns1:MedicalTrialDesign ;
	rdfs:label "InternationalTrial" ;
	rdfs:comment "An international trial." .

ns1:LaboratoryScience a ns1:MedicalSpecialty ;
	rdfs:label "LaboratoryScience" ;
	rdfs:comment "Laboratory science." .

ns1:LeisureTimeActivity a ns1:PhysicalActivityCategory ;
	rdfs:label "LeisureTimeActivity" ;
	rdfs:comment "Any physical activity engaged in for recreational purposes. Examples may include ballroom dancing, roller skating, canoeing, fishing, etc." .

ns1:LimitedAvailability a ns1:ItemAvailability ;
	rdfs:label "LimitedAvailability" ;
	rdfs:comment "Indicates that the item has limited availability." .

ns1:Longitudinal a ns1:MedicalObservationalStudyDesign ;
	rdfs:label "Longitudinal" ;
	rdfs:comment "Unlike cross-sectional studies, longitudinal studies track the same people, and therefore the differences observed in those people are less likely to be the result of cultural differences across generations. Longitudinal studies are also used in medicine to uncover predictors of certain diseases." .

ns1:Lung a ns1:PhysicalExam ;
	rdfs:label "Lung" ;
	rdfs:comment "Lung" .

ns1:MRI a ns1:MedicalImagingTechnique ;
	rdfs:label "MRI" ;
	rdfs:comment "Magnetic resonance imaging." .

ns1:MedicalResearcher a ns1:MedicalAudience ;
	rdfs:label "MedicalResearcher" ;
	rdfs:comment "Medical researchers." .

ns1:Midwifery a ns1:MedicalSpecialty ;
	rdfs:label "Midwifery" ;
	rdfs:comment "Midwifery." .

ns1:MultiCenterTrial a ns1:MedicalTrialDesign ;
	rdfs:label "MultiCenterTrial" ;
	rdfs:comment "A trial that takes place at multiple centers." .

ns1:MulticellularParasite a ns1:InfectiousAgentClass ;
	rdfs:label "MulticellularParasite" ;
	rdfs:comment "Multicellular parasite that causes an infection." .

ns1:Musculoskeletal a ns1:MedicalSpecialty ;
	rdfs:label "Musculoskeletal" ;
	rdfs:comment "A specific branch of medical science that pertains to diagnosis and treatment of disorders of muscles, ligaments and skeletal system." .

ns1:MusculoskeletalExam a ns1:PhysicalExam ;
	rdfs:label "MusculoskeletalExam" ;
	rdfs:comment "Musculoskeletal" .

ns1:Neck a ns1:PhysicalExam ;
	rdfs:label "Neck" ;
	rdfs:comment "Neck" .

ns1:Neuro a ns1:PhysicalExam ;
	rdfs:label "Neuro" ;
	rdfs:comment "Neuro" .

ns1:Neurologic a ns1:MedicalSpecialty ;
	rdfs:label "Neurologic" ;
	rdfs:comment "A specific branch of medical science that studies the nerves and nervous system and its respective disease states." .

ns1:NewCondition a ns1:OfferItemCondition ;
	rdfs:label "NewCondition" ;
	rdfs:comment "Indicates that the item is new." .

ns1:NoninvasiveProcedure a ns1:MedicalProcedureType ;
	rdfs:label "NoninvasiveProcedure" ;
	rdfs:comment "A type of medical procedure that involves noninvasive techniques." .

ns1:Nose a ns1:PhysicalExam ;
	rdfs:label "Nose" ;
	rdfs:comment "Nose" .

ns1:NotYetRecruiting a ns1:MedicalStudyStatus ;
	rdfs:label "NotYetRecruiting" ;
	rdfs:comment "Not yet recruiting." .

ns1:Nursing a ns1:MedicalSpecialty ;
	rdfs:label "Nursing" ;
	rdfs:comment "Nursing." .

ns1:OTC a ns1:DrugPrescriptionStatus ;
	rdfs:label "OTC" ;
	rdfs:comment "Available over the counter." .

ns1:Observational a ns1:MedicalObservationalStudyDesign ;
	rdfs:label "Observational" ;
	rdfs:comment "An observational study design." .

ns1:Obstetric a ns1:MedicalSpecialty ;
	rdfs:label "Obstetric" ;
	rdfs:comment "A specific branch of medical science that specializes in the care of women during the prenatal and postnatal care and with the delivery of the child." .

ns1:OccupationalActivity a ns1:PhysicalActivityCategory ;
	rdfs:label "OccupationalActivity" ;
	rdfs:comment "Any physical activity engaged in for job-related purposes. Examples may include waiting tables, maid service, carrying a mailbag, picking fruits or vegetables, construction work, etc." .

ns1:OccupationalTherapy a ns1:MedicalSpecialty ;
	rdfs:label "OccupationalTherapy" ;
	rdfs:comment "Occupational therapy." .

ns1:OnSitePickup a ns1:DeliveryMethod ;
	rdfs:label "OnSitePickup" ;
	rdfs:comment "A DeliveryMethod in which an item is collected on site, e.g. in a store or at a box office." .

ns1:Oncologic a ns1:MedicalSpecialty ;
	rdfs:label "Oncologic" ;
	rdfs:comment "A specific branch of medical science that deals with benign and malignant tumors, including the study of their development, diagnosis, treatment and prevention." .

ns1:OnlineOnly a ns1:ItemAvailability ;
	rdfs:label "OnlineOnly" ;
	rdfs:comment "Indicates that the item is available only online." .

ns1:OpenTrial a ns1:MedicalTrialDesign ;
	rdfs:label "OpenTrial" ;
	rdfs:comment "A trial design in which the researcher knows the full details of the treatment, and so does the patient." .

ns1:Optometic a ns1:MedicalSpecialty ;
	rdfs:label "Optometic" ;
	rdfs:comment "Optometry." .

ns1:OrderCancelled a ns1:OrderStatus ;
	rdfs:label "OrderCancelled" ;
	rdfs:comment "OrderStatus representing cancellation of an order." .

ns1:OrderDelivered a ns1:OrderStatus ;
	rdfs:label "OrderDelivered" ;
	rdfs:comment "OrderStatus representing successful delivery of an order." .

ns1:OrderInTransit a ns1:OrderStatus ;
	rdfs:label "OrderInTransit" ;
	rdfs:comment "OrderStatus representing that an order is in transit." .

ns1:OrderPaymentDue a ns1:OrderStatus ;
	rdfs:label "OrderPaymentDue" ;
	rdfs:comment "OrderStatus representing that payment is due on an order." .

ns1:OrderPickupAvailable a ns1:OrderStatus ;
	rdfs:label "OrderPickupAvailable" ;
	rdfs:comment "OrderStatus representing availability of an order for pickup." .

ns1:OrderProblem a ns1:OrderStatus ;
	rdfs:label "OrderProblem" ;
	rdfs:comment "OrderStatus representing that there is a problem with the order." .

ns1:OrderProcessing a ns1:OrderStatus ;
	rdfs:label "OrderProcessing" ;
	rdfs:comment "OrderStatus representing that an order is being processed." .

ns1:OrderReturned a ns1:OrderStatus ;
	rdfs:label "OrderReturned" ;
	rdfs:comment "OrderStatus representing that an order has been returned." .

ns1:Osteopathic a ns1:MedicineSystem ;
	rdfs:label "Osteopathic" ;
	rdfs:comment "A system of medicine focused on promoting the body's innate ability to heal itself." .

ns1:Otolaryngologic a ns1:MedicalSpecialty ;
	rdfs:label "Otolaryngologic" ;
	rdfs:comment "A specific branch of medical science that is concerned with the ear, nose and throat and their respective disease states." .

ns1:OutOfStock a ns1:ItemAvailability ;
	rdfs:label "OutOfStock" ;
	rdfs:comment "Indicates that the item is out of stock." .

ns1:PET a ns1:MedicalImagingTechnique ;
	rdfs:label "PET" ;
	rdfs:comment "Positron emission tomography imaging." .

ns1:Paperback a ns1:BookFormatType ;
	rdfs:label "Paperback" ;
	rdfs:comment "Book format: Paperback." .

ns1:Pathology a ns1:MedicalSpecialty ;
	rdfs:label "Pathology" ;
	rdfs:comment "A specific branch of medical science that is concerned with the study of the cause, origin and nature of a disease state, including its consequences as a result of manifestation of the disease. In clinical care, the term is used to designate a branch of medicine using laboratory tests to diagnose and determine the prognostic significance of illness." .

ns1:Patient a ns1:MedicalAudience ;
	rdfs:label "Patient" ;
	rdfs:comment "Patients." .

ns1:Pediatric a ns1:MedicalSpecialty ;
	rdfs:label "Pediatric" ;
	rdfs:comment "A specific branch of medical science that specializes in the care of infants, children and adolescents." .

ns1:PercutaneousProcedure a ns1:MedicalProcedureType ;
	rdfs:label "PercutaneousProcedure" ;
	rdfs:comment "A type of medical procedure that involves percutaneous techniques, where access to organs or tissue is achieved via needle-puncture of the skin. For example, catheter-based procedures like stent delivery." .

ns1:PharmacySpecialty a ns1:MedicalSpecialty ;
	rdfs:label "PharmacySpecialty" ;
	rdfs:comment "Pharmacy." .

ns1:Physiotherapy a ns1:MedicalSpecialty ;
	rdfs:label "Physiotherapy" ;
	rdfs:comment "Physiotherapy." .

ns1:PlaceboControlledTrial a ns1:MedicalTrialDesign ;
	rdfs:label "PlaceboControlledTrial" ;
	rdfs:comment "A placebo-controlled trial design." .

ns1:PlasticSurgery a ns1:MedicalSpecialty ;
	rdfs:label "PlasticSurgery" ;
	rdfs:comment "A specific branch of medical science that pertains to therapeutic or cosmetic repair or re-formation of missing, injured or malformed tissues or body parts by manual and instrumental means." .

ns1:Podiatric a ns1:MedicalSpecialty ;
	rdfs:label "Podiatric" ;
	rdfs:comment "Podiatry." .

ns1:PotentialActionStatus a ns1:ActionStatusType ;
	rdfs:label "PotentialActionStatus" ;
	rdfs:comment "A description of an action that is supported." .

ns1:PreOrder a ns1:ItemAvailability ;
	rdfs:label "PreOrder" ;
	rdfs:comment "Indicates that the item is available for pre-order." .

ns1:PrescriptionOnly a ns1:DrugPrescriptionStatus ;
	rdfs:label "PrescriptionOnly" ;
	rdfs:comment "Available by prescription only." .

ns1:PrimaryCare a ns1:MedicalSpecialty ;
	rdfs:label "PrimaryCare" ;
	rdfs:comment "Primary care." .

ns1:Prion a ns1:InfectiousAgentClass ;
	rdfs:label "Prion" ;
	rdfs:comment "A prion is an infectious agent composed of protein in a misfolded form." .

ns1:Protozoa a ns1:InfectiousAgentClass ;
	rdfs:label "Protozoa" ;
	rdfs:comment "Single-celled organism that causes an infection." .

ns1:Psychiatric a ns1:MedicalSpecialty ;
	rdfs:label "Psychiatric" ;
	rdfs:comment "A specific branch of medical science that is concerned with the study, treatment, and prevention of mental illness, using both medical and psychological therapies." .

ns1:PublicHealth a ns1:MedicalSpecialty ;
	rdfs:label "PublicHealth" ;
	rdfs:comment "Environment and public health." .

ns1:Pulmonary a ns1:MedicalSpecialty ;
	rdfs:label "Pulmonary" ;
	rdfs:comment "A specific branch of medical science that pertains to the study of the respiratory system and its respective disease states." .

ns1:Radiograpy a ns1:MedicalSpecialty ;
	rdfs:label "Radiograpy" ;
	rdfs:comment "Radiography." .

ns1:RandomizedTrial a ns1:MedicalTrialDesign ;
	rdfs:label "RandomizedTrial" ;
	rdfs:comment "A randomized trial design." .

ns1:Recruiting a ns1:MedicalStudyStatus ;
	rdfs:label "Recruiting" ;
	rdfs:comment "Recruiting participants." .

ns1:RefurbishedCondition a ns1:OfferItemCondition ;
	rdfs:label "RefurbishedCondition" ;
	rdfs:comment "Indicates that the item is refurbished." .

ns1:Registry a ns1:MedicalObservationalStudyDesign ;
	rdfs:label "Registry" ;
	rdfs:comment "A registry-based study design." .

ns1:ReimbursementCap a ns1:DrugCostCategory ;
	rdfs:label "ReimbursementCap" ;
	rdfs:comment "The drug's cost represents the maximum reimbursement paid by an insurer for the drug." .

ns1:Renal a ns1:MedicalSpecialty ;
	rdfs:label "Renal" ;
	rdfs:comment "A specific branch of medical science that pertains to the study of the kidneys and its respective disease states." .

ns1:Researcher a ns1:Audience ;
	rdfs:label "Researcher" ;
	rdfs:comment "Researchers." .

ns1:ReservationCancelled a ns1:ReservationStatusType ;
	rdfs:label "ReservationCancelled" ;
	rdfs:comment "The status for a previously confirmed reservation that is now cancelled." .

ns1:ReservationConfirmed a ns1:ReservationStatusType ;
	rdfs:label "ReservationConfirmed" ;
	rdfs:comment "The status of a confirmed reservation." .

ns1:ReservationHold a ns1:ReservationStatusType ;
	rdfs:label "ReservationHold" ;
	rdfs:comment "The status of a reservation on hold pending an update like credit card number or flight changes." .

ns1:ReservationPending a ns1:ReservationStatusType ;
	rdfs:label "ReservationPending" ;
	rdfs:comment "The status of a reservation when a request has been sent, but not confirmed." .

ns1:RespiratoryTherapy a ns1:MedicalSpecialty ;
	rdfs:label "RespiratoryTherapy" ;
	rdfs:comment "Respiratory therapy." .

ns1:ResultsAvailable a ns1:MedicalStudyStatus ;
	rdfs:label "ResultsAvailable" ;
	rdfs:comment "Results are available." .

ns1:ResultsNotAvailable a ns1:MedicalStudyStatus ;
	rdfs:label "ResultsNotAvailable" ;
	rdfs:comment "Results are not available." .

ns1:Retail a ns1:DrugCostCategory ;
	rdfs:label "Retail" ;
	rdfs:comment "The drug's cost represents the retail cost of the drug." .

ns1:Rheumatologic a ns1:MedicalSpecialty ;
	rdfs:label "Rheumatologic" ;
	rdfs:comment "A specific branch of medical science that deals with the study and treatment of rheumatic, autoimmune or joint diseases." .

ns1:SingleBlindedTrial a ns1:MedicalTrialDesign ;
	rdfs:label "SingleBlindedTrial" ;
	rdfs:comment "A trial design in which the researcher knows which treatment the patient was randomly assigned to but the patient does not." .

ns1:SingleCenterTrial a ns1:MedicalTrialDesign ;
	rdfs:label "SingleCenterTrial" ;
	rdfs:comment "A trial that takes place at a single center." .

ns1:Skin a ns1:PhysicalExam ;
	rdfs:label "Skin" ;
	rdfs:comment "Skin" .

ns1:SoldOut a ns1:ItemAvailability ;
	rdfs:label "SoldOut" ;
	rdfs:comment "Indicates that the item has sold out." .

ns1:SpeechPathology a ns1:MedicalSpecialty ;
	rdfs:label "SpeechPathology" ;
	rdfs:comment "Speech pathology." .

ns1:StrengthTraining a ns1:PhysicalActivityCategory ;
	rdfs:label "StrengthTraining" ;
	rdfs:comment "Physical activity that is engaged in to improve muscle and bone strength. Also referred to as resistance training." .

ns1:Surgical a ns1:MedicalSpecialty ;
	rdfs:label "Surgical" ;
	rdfs:comment "A specific branch of medical science that pertains to treating diseases, injuries and deformities by manual and instrumental means." .

ns1:SurgicalProcedure a ns1:MedicalProcedureType ;
	rdfs:label "SurgicalProcedure" ;
	rdfs:comment "A type of medical procedure that involves invasive surgical techniques." .

ns1:Suspended a ns1:MedicalStudyStatus ;
	rdfs:label "Suspended" ;
	rdfs:comment "Suspended." .

ns1:Terminated a ns1:MedicalStudyStatus ;
	rdfs:label "Terminated" ;
	rdfs:comment "Terminated." .

ns1:Therapeutic a ns1:MedicalDevicePurpose ;
	rdfs:label "Therapeutic" ;
	rdfs:comment "A medical device used for therapeutic purposes." .

ns1:Throat a ns1:PhysicalExam ;
	rdfs:label "Throat" ;
	rdfs:comment "Throat" .

ns1:TollFree a ns1:ContactPointOption ;
	rdfs:label "TollFree" ;
	rdfs:comment "The associated telephone number is toll free." .

ns1:Toxicologic a ns1:MedicalSpecialty ;
	rdfs:label "Toxicologic" ;
	rdfs:comment "A specific branch of medical science that is concerned with poisons, their nature, effects and detection and involved in the treatment of poisoning." .

ns1:TraditionalChinese a ns1:MedicineSystem ;
	rdfs:label "TraditionalChinese" ;
	rdfs:comment "A system of medicine based on common theoretical concepts that originated in China and evolved over thousands of years, that uses herbs, acupuncture, exercise, massage, dietary therapy, and other methods to treat a wide range of conditions." .

ns1:TripleBlindedTrial a ns1:MedicalTrialDesign ;
	rdfs:label "TripleBlindedTrial" ;
	rdfs:comment "A trial design in which neither the researcher, the person administering the therapy nor the patient knows the details of the treatment the patient was randomly assigned to." .

ns1:True a ns1:Boolean ;
	rdfs:label "True" ;
	rdfs:comment "The boolean value true" ;
	rdfs:subClassOf ns1:Boolean .

ns1:Ultrasound a ns1:MedicalImagingTechnique ;
	rdfs:label "Ultrasound" ;
	rdfs:comment "Ultrasound imaging." .

ns1:Urologic a ns1:MedicalSpecialty ;
	rdfs:label "Urologic" ;
	rdfs:comment "A specific branch of medical science that is concerned with the diagnosis and treatment of diseases pertaining to the urinary tract and the urogenital system." .

ns1:UsedCondition a ns1:OfferItemCondition ;
	rdfs:label "UsedCondition" ;
	rdfs:comment "Indicates that the item is used." .

ns1:Virus a ns1:InfectiousAgentClass ;
	rdfs:label "Virus" ;
	rdfs:comment "Pathogenic virus that causes viral infection." .

ns1:VitalSign a ns1:PhysicalExam ;
	rdfs:label "VitalSign" ;
	rdfs:comment "VitalSign" .

ns1:WesternConventional a ns1:MedicineSystem ;
	rdfs:label "WesternConventional" ;
	rdfs:comment "The conventional Western system of medicine, that aims to apply the best available evidence gained from the scientific method to clinical decision making. Also known as conventional or Western medicine." .

ns1:Wholesale a ns1:DrugCostCategory ;
	rdfs:label "Wholesale" ;
	rdfs:comment "The drug's cost represents the wholesale acquisition cost of the drug." .

ns1:Withdrawn a ns1:MedicalStudyStatus ;
	rdfs:label "Withdrawn" ;
	rdfs:comment "Withdrawn." .

ns1:XRay a ns1:MedicalImagingTechnique ;
	rdfs:label "XRay" ;
	rdfs:comment "X-ray imaging." .

ns1:about a rdf:Property ;
	rdfs:label "about" ;
	ns1:domainIncludes ns1:CommunicateAction , ns1:CreativeWork ;
	ns1:rangeIncludes ns1:Thing ;
	rdfs:comment "The subject matter of the content." .

ns1:acceptedAnswer a rdf:Property ;
	rdfs:label "acceptedAnswer" ;
	ns1:domainIncludes ns1:Question ;
	ns1:rangeIncludes ns1:Answer ;
	rdfs:comment "The answer that has been accepted as best, typically on a Question/Answer site. Sites vary in their selection mechanisms, e.g. drawing on community opinion and/or the view of the Question author." ;
	rdfs:subPropertyOf ns1:suggestedAnswer .

ns1:acceptedOffer a rdf:Property ;
	rdfs:label "acceptedOffer" ;
	ns1:domainIncludes ns1:Order ;
	ns1:rangeIncludes ns1:Offer ;
	rdfs:comment "The offer(s) -- e.g., product, quantity and price combinations -- included in the order." .

ns1:acceptedPaymentMethod a rdf:Property ;
	rdfs:label "acceptedPaymentMethod" ;
	ns1:domainIncludes ns1:Demand , ns1:Offer ;
	ns1:rangeIncludes ns1:PaymentMethod ;
	rdfs:comment "The payment method(s) accepted by seller for this offer." .

ns1:acceptsReservations a rdf:Property ;
	rdfs:label "acceptsReservations" ;
	ns1:domainIncludes ns1:FoodEstablishment ;
	ns1:rangeIncludes ns1:Boolean , ns1:Text , ns1:URL ;
	rdfs:comment "Indicates whether a FoodEstablishment accepts reservations. Values can be Boolean, an URL at which reservations can be made or (for backwards compatibility) the strings <code>Yes</code> or <code>No</code>." .

ns1:accessCode a rdf:Property ;
	rdfs:label "accessCode" ;
	ns1:domainIncludes ns1:DeliveryEvent ;
	ns1:rangeIncludes ns1:Text ;
	rdfs:comment "Password, PIN, or access code needed for delivery (e.g. from a locker)." .

ns1:accessibilityAPI a rdf:Property ;
	rdfs:label "accessibilityAPI" ;
	ns1:domainIncludes ns1:CreativeWork ;
	ns1:rangeIncludes ns1:Text ;
	rdfs:comment """Indicates that the resource is compatible with the referenced accessibility API (<a href=\"http://www.w3.org/wiki/WebSchemas/Accessibility\">WebSchemas wiki lists possible values</a>).
         """ .

ns1:accessibilityControl a rdf:Property ;
	rdfs:label "accessibilityControl" ;
	ns1:domainIncludes ns1:CreativeWork ;
	ns1:rangeIncludes ns1:Text ;
	rdfs:comment "Identifies input methods that are sufficient to fully control the described resource (<a href=\"http://www.w3.org/wiki/WebSchemas/Accessibility\">WebSchemas wiki lists possible values</a>)." .

ns1:accessibilityFeature a rdf:Property ;
	rdfs:label "accessibilityFeature" ;
	ns1:domainIncludes ns1:CreativeWork ;
	ns1:rangeIncludes ns1:Text ;
	rdfs:comment "Content features of the resource, such as accessible media, alternatives and supported enhancements for accessibility (<a href=\"http://www.w3.org/wiki/WebSchemas/Accessibility\">WebSchemas wiki lists possible values</a>)." .

ns1:accessibilityHazard a rdf:Property ;
	rdfs:label "accessibilityHazard" ;
	ns1:domainIncludes ns1:CreativeWork ;
	ns1:rangeIncludes ns1:Text ;
	rdfs:comment "A characteristic of the described resource that is physiologically dangerous to some users. Related to WCAG 2.0 guideline 2.3. (<a href=\"http://www.w3.org/wiki/WebSchemas/Accessibility\">WebSchemas wiki lists possible values</a>)" .

ns1:accountablePerson a rdf:Property ;
	rdfs:label "accountablePerson" ;
	ns1:domainIncludes ns1:CreativeWork ;
	ns1:rangeIncludes ns1:Person ;
	rdfs:comment "Specifies the Person that is legally accountable for the CreativeWork." .

ns1:acquiredFrom a rdf:Property ;
	rdfs:label "acquiredFrom" ;
	ns1:domainIncludes ns1:OwnershipInfo ;
	ns1:rangeIncludes ns1:Organization , ns1:Person ;
	rdfs:comment "The organization or person from which the product was acquired." .

ns1:action a rdf:Property ;
	rdfs:label "action" ;
	ns1:domainIncludes ns1:Muscle ;
	ns1:rangeIncludes ns1:Text ;
	ns1:supercededBy ns1:muscleAction ;
	rdfs:comment "The movement the muscle generates." .

ns1:actionStatus a rdf:Property ;
	rdfs:label "actionStatus" ;
	ns1:domainIncludes ns1:Action ;
	ns1:rangeIncludes ns1:ActionStatusType ;
	rdfs:comment "Indicates the current disposition of the Action." .

ns1:activeIngredient a rdf:Property ;
	rdfs:label "activeIngredient" ;
	ns1:domainIncludes ns1:DietarySupplement , ns1:Drug , ns1:DrugStrength ;
	ns1:rangeIncludes ns1:Text ;
	rdfs:comment "An active ingredient, typically chemical compounds and/or biologic substances." .

ns1:activityDuration a rdf:Property ;
	rdfs:label "activityDuration" ;
	ns1:domainIncludes ns1:ExercisePlan ;
	ns1:rangeIncludes ns1:Duration ;
	rdfs:comment "Length of time to engage in the activity." .

ns1:activityFrequency a rdf:Property ;
	rdfs:label "activityFrequency" ;
	ns1:domainIncludes ns1:ExercisePlan ;
	ns1:rangeIncludes ns1:Text ;
	rdfs:comment "How often one should engage in the activity." .

ns1:actors a rdf:Property ;
	rdfs:label "actors" ;
	ns1:domainIncludes ns1:Episode , ns1:Movie , ns1:RadioEpisode , ns1:RadioSeries , ns1:Series , ns1:TVEpisode , ns1:TVSeries ;
	ns1:rangeIncludes ns1:Person ;
	ns1:supercededBy ns1:actor ;
	rdfs:comment "A cast member of the movie, tv/radio series, season, episode, or video. (legacy spelling; see singular form, actor)" .

ns1:addOn a rdf:Property ;
	rdfs:label "addOn" ;
	ns1:domainIncludes ns1:Offer ;
	ns1:rangeIncludes ns1:Offer ;
	rdfs:comment "An additional offer that can only be obtained in combination with the first base offer (e.g. supplements and extensions that are available for a surcharge)." .

ns1:additionalName a rdf:Property ;
	rdfs:label "additionalName" ;
	ns1:domainIncludes ns1:Person ;
	ns1:rangeIncludes ns1:Text ;
	rdfs:comment "An additional name for a Person, can be used for a middle name." .

ns1:additionalType a rdf:Property ;
	rdfs:label "additionalType" ;
	ns1:domainIncludes ns1:Thing ;
	ns1:rangeIncludes ns1:URL ;
	rdfs:comment "An additional type for the item, typically used for adding more specific types from external vocabularies in microdata syntax. This is a relationship between something and a class that the thing is in. In RDFa syntax, it is better to use the native RDFa syntax - the 'typeof' attribute - for multiple types. Schema.org tools may have only weaker understanding of extra types, in particular those defined externally." .

ns1:additionalVariable a rdf:Property ;
	rdfs:label "additionalVariable" ;
	ns1:domainIncludes ns1:ExercisePlan ;
	ns1:rangeIncludes ns1:Text ;
	rdfs:comment "Any additional component of the exercise prescription that may need to be articulated to the patient. This may include the order of exercises, the number of repetitions of movement, quantitative distance, progressions over time, etc." .

ns1:address a rdf:Property ;
	rdfs:label "address" ;
	ns1:domainIncludes ns1:Organization , ns1:Person , ns1:Place ;
	ns1:rangeIncludes ns1:PostalAddress ;
	rdfs:comment "Physical address of the item." .

ns1:addressCountry a rdf:Property ;
	rdfs:label "addressCountry" ;
	ns1:domainIncludes ns1:PostalAddress ;
	ns1:rangeIncludes ns1:Country ;
	rdfs:comment "The country. For example, USA. You can also provide the two-letter <a href='http://en.wikipedia.org/wiki/ISO_3166-1'>ISO 3166-1 alpha-2 country code</a>." .

ns1:addressLocality a rdf:Property ;
	rdfs:label "addressLocality" ;
	ns1:domainIncludes ns1:PostalAddress ;
	ns1:rangeIncludes ns1:Text ;
	rdfs:comment "The locality. For example, Mountain View." .

ns1:addressRegion a rdf:Property ;
	rdfs:label "addressRegion" ;
	ns1:domainIncludes ns1:PostalAddress ;
	ns1:rangeIncludes ns1:Text ;
	rdfs:comment "The region. For example, CA." .

ns1:administrationRoute a rdf:Property ;
	rdfs:label "administrationRoute" ;
	ns1:domainIncludes ns1:Drug ;
	ns1:rangeIncludes ns1:Text ;
	rdfs:comment "A route by which this drug may be administered, e.g. 'oral'." .

ns1:advanceBookingRequirement a rdf:Property ;
	rdfs:label "advanceBookingRequirement" ;
	ns1:domainIncludes ns1:Demand , ns1:Offer ;
	ns1:rangeIncludes ns1:QuantitativeValue ;
	rdfs:comment "The amount of time that is required between accepting the offer and the actual usage of the resource or service." .

ns1:adverseOutcome a rdf:Property ;
	rdfs:label "adverseOutcome" ;
	ns1:domainIncludes ns1:MedicalDevice , ns1:MedicalTherapy ;
	ns1:rangeIncludes ns1:MedicalEntity ;
	rdfs:comment "A possible complication and/or side effect of this therapy. If it is known that an adverse outcome is serious (resulting in death, disability, or permanent damage; requiring hospitalization; or is otherwise life-threatening or requires immediate medical attention), tag it as a seriouseAdverseOutcome instead." .

ns1:affectedBy a rdf:Property ;
	rdfs:label "affectedBy" ;
	ns1:domainIncludes ns1:MedicalTest ;
	ns1:rangeIncludes ns1:Drug ;
	rdfs:comment "Drugs that affect the test's results." .

ns1:affiliation a rdf:Property ;
	rdfs:label "affiliation" ;
	ns1:domainIncludes ns1:Person ;
	ns1:rangeIncludes ns1:Organization ;
	rdfs:comment "An organization that this person is affiliated with. For example, a school/university, a club, or a team." .

ns1:agent a rdf:Property ;
	rdfs:label "agent" ;
	ns1:domainIncludes ns1:Action ;
	ns1:rangeIncludes ns1:Organization , ns1:Person ;
	rdfs:comment "The direct performer or driver of the action (animate or inanimate). e.g. *John* wrote a book." .

ns1:aggregateRating a rdf:Property ;
	rdfs:label "aggregateRating" ;
	ns1:domainIncludes ns1:CreativeWork , ns1:Offer , ns1:Organization , ns1:Place , ns1:Product ;
	ns1:rangeIncludes ns1:AggregateRating ;
	rdfs:comment "The overall rating, based on a collection of reviews or ratings, of the item." .

ns1:aircraft a rdf:Property ;
	rdfs:label "aircraft" ;
	ns1:domainIncludes ns1:Flight ;
	ns1:rangeIncludes ns1:Text , ns1:Vehicle ;
	rdfs:comment "The kind of aircraft (e.g., \"Boeing 747\")." .

ns1:albums a rdf:Property ;
	rdfs:label "albums" ;
	ns1:domainIncludes ns1:MusicGroup ;
	ns1:rangeIncludes ns1:MusicAlbum ;
	ns1:supercededBy ns1:album ;
	rdfs:comment "A collection of music albums (legacy spelling; see singular form, album)." .

ns1:alcoholWarning a rdf:Property ;
	rdfs:label "alcoholWarning" ;
	ns1:domainIncludes ns1:Drug ;
	ns1:rangeIncludes ns1:Text ;
	rdfs:comment "Any precaution, guidance, contraindication, etc. related to consumption of alcohol while taking this drug." .

ns1:algorithm a rdf:Property ;
	rdfs:label "algorithm" ;
	ns1:domainIncludes ns1:MedicalRiskScore ;
	ns1:rangeIncludes ns1:Text ;
	rdfs:comment "The algorithm or rules to follow to compute the score." .

ns1:alignmentType a rdf:Property ;
	rdfs:label "alignmentType" ;
	ns1:domainIncludes ns1:AlignmentObject ;
	ns1:rangeIncludes ns1:Text ;
	rdfs:comment "A category of alignment between the learning resource and the framework node. Recommended values include: 'assesses', 'teaches', 'requires', 'textComplexity', 'readingLevel', 'educationalSubject', and 'educationLevel'." .

ns1:alternateName a rdf:Property ;
	rdfs:label "alternateName" ;
	ns1:domainIncludes ns1:MedicalEntity , ns1:Thing ;
	ns1:rangeIncludes ns1:Text ;
	rdfs:comment "An alias for the item." .

ns1:alternativeHeadline a rdf:Property ;
	rdfs:label "alternativeHeadline" ;
	ns1:domainIncludes ns1:CreativeWork ;
	ns1:rangeIncludes ns1:Text ;
	rdfs:comment "A secondary title of the CreativeWork." .

ns1:amountOfThisGood a rdf:Property ;
	rdfs:label "amountOfThisGood" ;
	ns1:domainIncludes ns1:TypeAndQuantityNode ;
	ns1:rangeIncludes ns1:Number ;
	rdfs:comment "The quantity of the goods included in the offer." .

ns1:answerCount a rdf:Property ;
	rdfs:label "answerCount" ;
	ns1:domainIncludes ns1:Question ;
	ns1:rangeIncludes ns1:Integer ;
	rdfs:comment "The number of answers this question has received." .

ns1:antagonist a rdf:Property ;
	rdfs:label "antagonist" ;
	ns1:domainIncludes ns1:Muscle ;
	ns1:rangeIncludes ns1:Muscle ;
	rdfs:comment "The muscle whose action counteracts the specified muscle." .

ns1:applicableLocation a rdf:Property ;
	rdfs:label "applicableLocation" ;
	ns1:domainIncludes ns1:DrugCost , ns1:DrugLegalStatus ;
	ns1:rangeIncludes ns1:AdministrativeArea ;
	rdfs:comment "The location in which the status applies." .

ns1:application a rdf:Property ;
	rdfs:label "application" ;
	ns1:domainIncludes ns1:EntryPoint ;
	ns1:rangeIncludes ns1:SoftwareApplication ;
	rdfs:comment "An application that can complete the request." .

ns1:applicationCategory a rdf:Property ;
	rdfs:label "applicationCategory" ;
	ns1:domainIncludes ns1:SoftwareApplication ;
	ns1:rangeIncludes ns1:Text , ns1:URL ;
	rdfs:comment "Type of software application, e.g. \"Game, Multimedia\"." .

ns1:applicationSubCategory a rdf:Property ;
	rdfs:label "applicationSubCategory" ;
	ns1:domainIncludes ns1:SoftwareApplication ;
	ns1:rangeIncludes ns1:Text , ns1:URL ;
	rdfs:comment "Subcategory of the application, e.g. \"Arcade Game\"." .

ns1:applicationSuite a rdf:Property ;
	rdfs:label "applicationSuite" ;
	ns1:domainIncludes ns1:SoftwareApplication ;
	ns1:rangeIncludes ns1:Text ;
	rdfs:comment "The name of the application suite to which the application belongs (e.g. Excel belongs to Office)" .

ns1:appliesToDeliveryMethod a rdf:Property ;
	rdfs:label "appliesToDeliveryMethod" ;
	ns1:domainIncludes ns1:DeliveryChargeSpecification , ns1:PaymentChargeSpecification ;
	ns1:rangeIncludes ns1:DeliveryMethod ;
	rdfs:comment "The delivery method(s) to which the delivery charge or payment charge specification applies." .

ns1:appliesToPaymentMethod a rdf:Property ;
	rdfs:label "appliesToPaymentMethod" ;
	ns1:domainIncludes ns1:PaymentChargeSpecification ;
	ns1:rangeIncludes ns1:PaymentMethod ;
	rdfs:comment "The payment method(s) to which the payment charge specification applies." .

ns1:area a rdf:Property ;
	rdfs:label "area" ;
	ns1:domainIncludes ns1:BroadcastService ;
	ns1:rangeIncludes ns1:Place ;
	rdfs:comment "The area within which users can expect to reach the broadcast service." .

ns1:areaServed a rdf:Property ;
	rdfs:label "areaServed" ;
	ns1:domainIncludes ns1:ContactPoint ;
	ns1:rangeIncludes ns1:AdministrativeArea ;
	rdfs:comment "The location served by this contact point (e.g., a phone number intended for Europeans vs. North Americans or only within the United States.)" .

ns1:arrivalAirport a rdf:Property ;
	rdfs:label "departureAirport" ;
	ns1:domainIncludes ns1:Flight ;
	ns1:rangeIncludes ns1:Airport ;
	rdfs:comment "The airport where the flight terminates." .

ns1:arrivalBusStop a rdf:Property ;
	rdfs:label "arrivalBusStop" ;
	ns1:domainIncludes ns1:BusTrip ;
	ns1:rangeIncludes ns1:BusStation , ns1:BusStop ;
	rdfs:comment "The stop or station from which the bus arrives." .

ns1:arrivalGate a rdf:Property ;
	rdfs:label "arrivalGate" ;
	ns1:domainIncludes ns1:Flight ;
	ns1:rangeIncludes ns1:Text ;
	rdfs:comment "Identifier of the flight's arrival gate." .

ns1:arrivalPlatform a rdf:Property ;
	rdfs:label "arrivalPlatform" ;
	ns1:domainIncludes ns1:TrainTrip ;
	ns1:rangeIncludes ns1:Text ;
	rdfs:comment "The platform where the train arrives." .

ns1:arrivalStation a rdf:Property ;
	rdfs:label "arrivalStation" ;
	ns1:domainIncludes ns1:TrainTrip ;
	ns1:rangeIncludes ns1:TrainStation ;
	rdfs:comment "The station where the train trip ends." .

ns1:arrivalTerminal a rdf:Property ;
	rdfs:label "arrivalTerminal" ;
	ns1:domainIncludes ns1:Flight ;
	ns1:rangeIncludes ns1:Text ;
	rdfs:comment "Identifier of the flight's arrival terminal." .

ns1:arrivalTime a rdf:Property ;
	rdfs:label "arrivalTime" ;
	ns1:domainIncludes ns1:BusTrip , ns1:Flight , ns1:TrainTrip ;
	ns1:rangeIncludes ns1:DateTime ;
	rdfs:comment "The expected arrival time." .

ns1:arterialBranch a rdf:Property ;
	rdfs:label "arterialBranch" ;
	ns1:domainIncludes ns1:Artery ;
	ns1:rangeIncludes ns1:AnatomicalStructure ;
	rdfs:comment "The branches that comprise the arterial structure." .

ns1:articleBody a rdf:Property ;
	rdfs:label "articleBody" ;
	ns1:domainIncludes ns1:Article ;
	ns1:rangeIncludes ns1:Text ;
	rdfs:comment "The actual body of the article." .

ns1:articleSection a rdf:Property ;
	rdfs:label "articleSection" ;
	ns1:domainIncludes ns1:Article ;
	ns1:rangeIncludes ns1:Text ;
	rdfs:comment "Articles may belong to one or more 'sections' in a magazine or newspaper, such as Sports, Lifestyle, etc." .

ns1:aspect a rdf:Property ;
	rdfs:label "aspect" ;
	ns1:domainIncludes ns1:MedicalWebPage ;
	ns1:rangeIncludes ns1:Text ;
	rdfs:comment "An aspect of medical practice that is considered on the page, such as 'diagnosis', 'treatment', 'causes', 'prognosis', 'etiology', 'epidemiology', etc." .

ns1:assembly a rdf:Property ;
	rdfs:label "assembly" ;
	ns1:domainIncludes ns1:APIReference ;
	ns1:rangeIncludes ns1:Text ;
	rdfs:comment "Library file name e.g., mscorlib.dll, system.web.dll" .

ns1:assemblyVersion a rdf:Property ;
	rdfs:label "assemblyVersion" ;
	ns1:domainIncludes ns1:APIReference ;
	ns1:rangeIncludes ns1:Text ;
	rdfs:comment "Associated product/technology version. e.g., .NET Framework 4.5" .

ns1:associatedAnatomy a rdf:Property ;
	rdfs:label "associatedAnatomy" ;
	ns1:domainIncludes ns1:MedicalCondition , ns1:PhysicalActivity ;
	ns1:rangeIncludes ns1:AnatomicalStructure , ns1:AnatomicalSystem , ns1:SuperficialAnatomy ;
	rdfs:comment "The anatomy of the underlying organ system or structures associated with this entity." .

ns1:associatedArticle a rdf:Property ;
	rdfs:label "associatedArticle" ;
	ns1:domainIncludes ns1:MediaObject ;
	ns1:rangeIncludes ns1:NewsArticle ;
	rdfs:comment "A NewsArticle associated with the Media Object." .

ns1:associatedMedia a rdf:Property ;
	rdfs:label "associatedMedia" ;
	ns1:domainIncludes ns1:CreativeWork ;
	ns1:rangeIncludes ns1:MediaObject ;
	rdfs:comment "The media objects that encode this creative work. This property is a synonym for encodings." .

ns1:associatedPathophysiology a rdf:Property ;
	rdfs:label "associatedPathophysiology" ;
	ns1:domainIncludes ns1:AnatomicalStructure , ns1:AnatomicalSystem , ns1:SuperficialAnatomy ;
	ns1:rangeIncludes ns1:Text ;
	rdfs:comment "If applicable, a description of the pathophysiology associated with the anatomical system, including potential abnormal changes in the mechanical, physical, and biochemical functions of the system." .

ns1:attendee a rdf:Property ;
	rdfs:label "attendee" ;
	ns1:domainIncludes ns1:Event ;
	ns1:rangeIncludes ns1:Organization , ns1:Person ;
	rdfs:comment "A person or organization attending the event." .

ns1:audience a rdf:Property ;
	rdfs:label "audience" ;
	ns1:domainIncludes ns1:CreativeWork , ns1:PlayAction , ns1:Product ;
	ns1:rangeIncludes ns1:Audience ;
	rdfs:comment "The intended audience of the item, i.e. the group for whom the item was created." .

ns1:audienceType a rdf:Property ;
	rdfs:label "audienceType" ;
	ns1:domainIncludes ns1:Audience ;
	ns1:rangeIncludes ns1:Text ;
	rdfs:comment """The target group associated with a given audience (e.g. veterans, car owners, musicians, etc.)
          domain: Audience
          Range: Text
        """ .

ns1:audio a rdf:Property ;
	rdfs:label "audio" ;
	ns1:domainIncludes ns1:CreativeWork ;
	ns1:rangeIncludes ns1:AudioObject ;
	rdfs:comment "An embedded audio object." .

ns1:author a rdf:Property ;
	rdfs:label "author" ;
	ns1:domainIncludes ns1:CreativeWork ;
	ns1:rangeIncludes ns1:Organization , ns1:Person ;
	rdfs:comment "The author of this content. Please note that author is special in that HTML 5 provides a special mechanism for indicating authorship via the rel tag. That is equivalent to this and may be used interchangeably." .

ns1:availability a rdf:Property ;
	rdfs:label "availability" ;
	ns1:domainIncludes ns1:Demand , ns1:Offer ;
	ns1:rangeIncludes ns1:ItemAvailability ;
	rdfs:comment "The availability of this item&#x2014;for example In stock, Out of stock, Pre-order, etc." .

ns1:availabilityEnds a rdf:Property ;
	rdfs:label "availabilityEnds" ;
	ns1:domainIncludes ns1:Demand , ns1:Offer ;
	ns1:rangeIncludes ns1:DateTime ;
	rdfs:comment "The end of the availability of the product or service included in the offer." .

ns1:availabilityStarts a rdf:Property ;
	rdfs:label "availabilityStarts" ;
	ns1:domainIncludes ns1:Demand , ns1:Offer ;
	ns1:rangeIncludes ns1:DateTime ;
	rdfs:comment "The beginning of the availability of the product or service included in the offer." .

ns1:availableAtOrFrom a rdf:Property ;
	rdfs:label "availableAtOrFrom" ;
	ns1:domainIncludes ns1:Demand , ns1:Offer ;
	ns1:rangeIncludes ns1:Place ;
	rdfs:comment "The place(s) from which the offer can be obtained (e.g. store locations)." .

ns1:availableChannel a rdf:Property ;
	rdfs:label "availableChannel" ;
	ns1:domainIncludes ns1:Service ;
	ns1:rangeIncludes ns1:ServiceChannel ;
	rdfs:comment "A means of accessing the service (e.g. a phone bank, a web site, a location, etc.)" .

ns1:availableDeliveryMethod a rdf:Property ;
	rdfs:label "availableDeliveryMethod" ;
	ns1:domainIncludes ns1:Demand , ns1:Offer ;
	ns1:rangeIncludes ns1:DeliveryMethod ;
	rdfs:comment "The delivery method(s) available for this offer." .

ns1:availableFrom a rdf:Property ;
	rdfs:label "availableFrom" ;
	ns1:domainIncludes ns1:DeliveryEvent ;
	ns1:rangeIncludes ns1:DateTime ;
	rdfs:comment "When the item is available for pickup from the store, locker, etc." .

ns1:availableIn a rdf:Property ;
	rdfs:label "availableIn" ;
	ns1:domainIncludes ns1:DrugStrength ;
	ns1:rangeIncludes ns1:AdministrativeArea ;
	rdfs:comment "The location in which the strength is available." .

ns1:availableLanguage a rdf:Property ;
	rdfs:label "availableLanguage" ;
	ns1:domainIncludes ns1:ContactPoint , ns1:ServiceChannel ;
	ns1:rangeIncludes ns1:Language ;
	rdfs:comment "A language someone may use with the item." .

ns1:availableService a rdf:Property ;
	rdfs:label "availableService" ;
	ns1:domainIncludes ns1:Hospital , ns1:MedicalClinic , ns1:Physician ;
	ns1:rangeIncludes ns1:MedicalProcedure , ns1:MedicalTest , ns1:MedicalTherapy ;
	rdfs:comment "A medical service available from this provider." .

ns1:availableStrength a rdf:Property ;
	rdfs:label "availableStrength" ;
	ns1:domainIncludes ns1:Drug ;
	ns1:rangeIncludes ns1:DrugStrength ;
	rdfs:comment "An available dosage strength for the drug." .

ns1:availableTest a rdf:Property ;
	rdfs:label "availableTest" ;
	ns1:domainIncludes ns1:DiagnosticLab ;
	ns1:rangeIncludes ns1:MedicalTest ;
	rdfs:comment "A diagnostic test or procedure offered by this lab." .

ns1:availableThrough a rdf:Property ;
	rdfs:label "availableThrough" ;
	ns1:domainIncludes ns1:DeliveryEvent ;
	ns1:rangeIncludes ns1:DateTime ;
	rdfs:comment "After this date, the item will no longer be available for pickup." .

ns1:awards a rdf:Property ;
	rdfs:label "awards" ;
	ns1:domainIncludes ns1:CreativeWork , ns1:Person ;
	ns1:rangeIncludes ns1:Text ;
	ns1:supercededBy ns1:award ;
	rdfs:comment "Awards won by this person or for this creative work. (legacy spelling; see singular form, award)" .

ns1:background a rdf:Property ;
	rdfs:label "background" ;
	ns1:domainIncludes ns1:DietarySupplement ;
	ns1:rangeIncludes ns1:Text ;
	rdfs:comment "Descriptive information establishing a historical perspective on the supplement. May include the rationale for the name, the population where the supplement first came to prominence, etc." .

ns1:baseSalary a rdf:Property ;
	rdfs:label "baseSalary" ;
	ns1:domainIncludes ns1:JobPosting ;
	ns1:rangeIncludes ns1:Number ;
	rdfs:comment "The base salary of the job." .

ns1:benefits a rdf:Property ;
	rdfs:label "benefits" ;
	ns1:domainIncludes ns1:JobPosting ;
	ns1:rangeIncludes ns1:Text ;
	rdfs:comment "Description of benefits associated with the job." .

ns1:bestRating a rdf:Property ;
	rdfs:label "bestRating" ;
	ns1:domainIncludes ns1:Rating ;
	ns1:rangeIncludes ns1:Number , ns1:Text ;
	rdfs:comment "The highest value allowed in this rating system. If bestRating is omitted, 5 is assumed." .

ns1:billingAddress a rdf:Property ;
	rdfs:label "billingAddress" ;
	ns1:domainIncludes ns1:Order ;
	ns1:rangeIncludes ns1:PostalAddress ;
	rdfs:comment "The billing address for the order." .

ns1:billingIncrement a rdf:Property ;
	rdfs:label "billingIncrement" ;
	ns1:domainIncludes ns1:UnitPriceSpecification ;
	ns1:rangeIncludes ns1:Number ;
	rdfs:comment "This property specifies the minimal quantity and rounding increment that will be the basis for the billing. The unit of measurement is specified by the unitCode property." .

ns1:biomechnicalClass a rdf:Property ;
	rdfs:label "biomechnicalClass" ;
	ns1:domainIncludes ns1:Joint ;
	ns1:rangeIncludes ns1:Text ;
	rdfs:comment "The biomechanical properties of the bone." .

ns1:birthDate a rdf:Property ;
	rdfs:label "birthDate" ;
	ns1:domainIncludes ns1:Person ;
	ns1:rangeIncludes ns1:Date ;
	rdfs:comment "Date of birth." .

ns1:bitrate a rdf:Property ;
	rdfs:label "bitrate" ;
	ns1:domainIncludes ns1:MediaObject ;
	ns1:rangeIncludes ns1:Text ;
	rdfs:comment "The bitrate of the media object." .

ns1:blogPosts a rdf:Property ;
	rdfs:label "blogPosts" ;
	ns1:domainIncludes ns1:Blog ;
	ns1:rangeIncludes ns1:BlogPosting ;
	ns1:supercededBy ns1:blogPost ;
	rdfs:comment "The postings that are part of this blog (legacy spelling; see singular form, blogPost)." .

ns1:bloodSupply a rdf:Property ;
	rdfs:label "bloodSupply" ;
	ns1:domainIncludes ns1:Muscle ;
	ns1:rangeIncludes ns1:Vessel ;
	rdfs:comment "The blood vessel that carries blood from the heart to the muscle." .

ns1:boardingGroup a rdf:Property ;
	rdfs:label "boardingGroup" ;
	ns1:domainIncludes ns1:FlightReservation ;
	ns1:rangeIncludes ns1:Text ;
	rdfs:comment "The airline-specific indicator of boarding order / preference." .

ns1:bodyLocation a rdf:Property ;
	rdfs:label "bodyLocation" ;
	ns1:domainIncludes ns1:AnatomicalStructure ;
	ns1:rangeIncludes ns1:Text ;
	rdfs:comment "Location in the body of the anatomical structure." .

ns1:bookEdition a rdf:Property ;
	rdfs:label "bookEdition" ;
	ns1:domainIncludes ns1:Book ;
	ns1:rangeIncludes ns1:Text ;
	rdfs:comment "The edition of the book." .

ns1:bookFormat a rdf:Property ;
	rdfs:label "bookFormat" ;
	ns1:domainIncludes ns1:Book ;
	ns1:rangeIncludes ns1:BookFormatType ;
	rdfs:comment "The format of the book." .

ns1:bookingAgent a rdf:Property ;
	rdfs:label "bookingAgent" ;
	ns1:domainIncludes ns1:Reservation ;
	ns1:rangeIncludes ns1:Organization , ns1:Person ;
	rdfs:comment "If the reservation was not booked directly through the provider, the third-party booking agent can be recorded through this property." .

ns1:bookingTime a rdf:Property ;
	rdfs:label "bookingTime" ;
	ns1:domainIncludes ns1:Reservation ;
	ns1:rangeIncludes ns1:DateTime ;
	rdfs:comment "The date and time the reservation was booked." .

ns1:borrower a rdf:Property ;
	rdfs:label "borrower" ;
	ns1:domainIncludes ns1:LendAction ;
	ns1:rangeIncludes ns1:Person ;
	rdfs:comment "A sub property of participant. The person that borrows the object being lent." ;
	rdfs:subPropertyOf ns1:participant .

ns1:box a rdf:Property ;
	rdfs:label "box" ;
	ns1:domainIncludes ns1:GeoShape ;
	ns1:rangeIncludes ns1:Text ;
	rdfs:comment "A polygon is the area enclosed by a point-to-point path for which the starting and ending points are the same. A polygon is expressed as a series of four or more space delimited points where the first and final points are identical." .

ns1:branch a rdf:Property ;
	rdfs:label "branch" ;
	ns1:domainIncludes ns1:Nerve ;
	ns1:rangeIncludes ns1:AnatomicalStructure , ns1:Nerve ;
	rdfs:comment "The branches that delineate from the nerve bundle." .

ns1:branchOf a rdf:Property ;
	rdfs:label "branchOf" ;
	ns1:domainIncludes ns1:LocalBusiness ;
	ns1:rangeIncludes ns1:Organization ;
	rdfs:comment "The larger organization that this local business is a branch of, if any." .

ns1:brand a rdf:Property ;
	rdfs:label "brand" ;
	ns1:domainIncludes ns1:Organization , ns1:Person , ns1:Product ;
	ns1:rangeIncludes ns1:Brand , ns1:Organization ;
	rdfs:comment "The brand(s) associated with a product or service, or the brand(s) maintained by an organization or business person." .

ns1:breadcrumb a rdf:Property ;
	rdfs:label "breadcrumb" ;
	ns1:domainIncludes ns1:WebPage ;
	ns1:rangeIncludes ns1:Text ;
	rdfs:comment "A set of links that can help a user understand and navigate a website hierarchy." .

ns1:breastfeedingWarning a rdf:Property ;
	rdfs:label "breastfeedingWarning" ;
	ns1:domainIncludes ns1:Drug ;
	ns1:rangeIncludes ns1:Text ;
	rdfs:comment "Any precaution, guidance, contraindication, etc. related to this drug's use by breastfeeding mothers." .

ns1:broadcaster a rdf:Property ;
	rdfs:label "broadcaster" ;
	ns1:domainIncludes ns1:BroadcastService ;
	ns1:rangeIncludes ns1:Organization ;
	rdfs:comment "The organization owning or operating the broadcast service." .

ns1:browserRequirements a rdf:Property ;
	rdfs:label "browserRequirements" ;
	ns1:domainIncludes ns1:WebApplication ;
	ns1:rangeIncludes ns1:Text ;
	rdfs:comment "Specifies browser requirements in human-readable text. For example,\"requires HTML5 support\"." .

ns1:busName a rdf:Property ;
	rdfs:label "busName" ;
	ns1:domainIncludes ns1:BusTrip ;
	ns1:rangeIncludes ns1:Text ;
	rdfs:comment "The name of the bus (e.g. Bolt Express)." .

ns1:busNumber a rdf:Property ;
	rdfs:label "busNumber" ;
	ns1:domainIncludes ns1:BusTrip ;
	ns1:rangeIncludes ns1:Text ;
	rdfs:comment "The unique identifier for the bus." .

ns1:businessFunction a rdf:Property ;
	rdfs:label "businessFunction" ;
	ns1:domainIncludes ns1:Demand , ns1:Offer , ns1:TypeAndQuantityNode ;
	ns1:rangeIncludes ns1:BusinessFunction ;
	rdfs:comment "The business function (e.g. sell, lease, repair, dispose) of the offer or component of a bundle (TypeAndQuantityNode). The default is http://purl.org/goodrelations/v1#Sell." .

ns1:buyer a rdf:Property ;
	rdfs:label "buyer" ;
	ns1:domainIncludes ns1:SellAction ;
	ns1:rangeIncludes ns1:Person ;
	rdfs:comment "A sub property of participant. The participant/person/organization that bought the object." ;
	rdfs:subPropertyOf ns1:participant .

ns1:byArtist a rdf:Property ;
	rdfs:label "byArtist" ;
	ns1:domainIncludes ns1:MusicAlbum , ns1:MusicRecording ;
	ns1:rangeIncludes ns1:MusicGroup ;
	rdfs:comment "The artist that performed this album or recording." .

ns1:calories a rdf:Property ;
	rdfs:label "calories" ;
	ns1:domainIncludes ns1:NutritionInformation ;
	ns1:rangeIncludes ns1:Energy ;
	rdfs:comment "The number of calories" .

ns1:candidate a rdf:Property ;
	rdfs:label "candidate" ;
	ns1:domainIncludes ns1:VoteAction ;
	ns1:rangeIncludes ns1:Person ;
	rdfs:comment "A sub property of object. The candidate subject of this action." ;
	rdfs:subPropertyOf ns1:object .

ns1:caption a rdf:Property ;
	rdfs:label "caption" ;
	ns1:domainIncludes ns1:ImageObject , ns1:VideoObject ;
	ns1:rangeIncludes ns1:Text ;
	rdfs:comment "The caption for this object." .

ns1:carbohydrateContent a rdf:Property ;
	rdfs:label "carbohydrateContent" ;
	ns1:domainIncludes ns1:NutritionInformation ;
	ns1:rangeIncludes ns1:Mass ;
	rdfs:comment "The number of grams of carbohydrates." .

ns1:carrier a rdf:Property ;
	rdfs:label "carrier" ;
	ns1:domainIncludes ns1:Flight , ns1:ParcelDelivery ;
	ns1:rangeIncludes ns1:Organization ;
	rdfs:comment "The party responsible for the parcel delivery." .

ns1:carrierRequirements a rdf:Property ;
	rdfs:label "carrierRequirements" ;
	ns1:domainIncludes ns1:MobileApplication ;
	ns1:rangeIncludes ns1:Text ;
	rdfs:comment "Specifies specific carrier(s) requirements for the application (e.g. an application may only work on a specific carrier network)." .

ns1:catalog a rdf:Property ;
	rdfs:label "catalog" ;
	ns1:domainIncludes ns1:Dataset ;
	ns1:rangeIncludes ns1:DataCatalog ;
	rdfs:comment "A data catalog which contains a dataset." .

ns1:category a rdf:Property ;
	rdfs:label "category" ;
	ns1:domainIncludes ns1:Offer , ns1:PhysicalActivity ;
	ns1:rangeIncludes ns1:PhysicalActivityCategory , ns1:Text , ns1:Thing ;
	rdfs:comment "A category for the item. Greater signs or slashes can be used to informally indicate a category hierarchy." .

ns1:cause a rdf:Property ;
	rdfs:label "cause" ;
	ns1:domainIncludes ns1:MedicalCondition , ns1:MedicalSignOrSymptom ;
	ns1:rangeIncludes ns1:MedicalCause ;
	rdfs:comment "An underlying cause. More specifically, one of the causative agent(s) that are most directly responsible for the pathophysiologic process that eventually results in the occurrence." .

ns1:causeOf a rdf:Property ;
	rdfs:label "causeOf" ;
	ns1:domainIncludes ns1:MedicalCause ;
	ns1:rangeIncludes ns1:MedicalEntity ;
	rdfs:comment "The condition, complication, symptom, sign, etc. caused." .

ns1:characterName a rdf:Property ;
	rdfs:label "characterName" ;
	ns1:domainIncludes ns1:PerformanceRole ;
	ns1:rangeIncludes ns1:Text ;
	rdfs:comment "The name of a character played in some acting or performing role, i.e. in a PerformanceRole." .

ns1:checkinTime a rdf:Property ;
	rdfs:label "checkinTime" ;
	ns1:domainIncludes ns1:LodgingReservation ;
	ns1:rangeIncludes ns1:DateTime ;
	rdfs:comment "The earliest someone may check into a lodging establishment." .

ns1:checkoutTime a rdf:Property ;
	rdfs:label "checkoutTime" ;
	ns1:domainIncludes ns1:LodgingReservation ;
	ns1:rangeIncludes ns1:DateTime ;
	rdfs:comment "The latest someone may check out of a lodging establishment." .

ns1:childMaxAge a rdf:Property ;
	rdfs:label "childMaxAge" ;
	ns1:domainIncludes ns1:ParentAudience ;
	ns1:rangeIncludes ns1:Number ;
	rdfs:comment "Maximal age of the child" .

ns1:childMinAge a rdf:Property ;
	rdfs:label "childMinAge" ;
	ns1:domainIncludes ns1:ParentAudience ;
	ns1:rangeIncludes ns1:Number ;
	rdfs:comment "Minimal age of the child" .

ns1:children a rdf:Property ;
	rdfs:label "children" ;
	ns1:domainIncludes ns1:Person ;
	ns1:rangeIncludes ns1:Person ;
	rdfs:comment "A child of the person." .

ns1:cholesterolContent a rdf:Property ;
	rdfs:label "cholesterolContent" ;
	ns1:domainIncludes ns1:NutritionInformation ;
	ns1:rangeIncludes ns1:Mass ;
	rdfs:comment "The number of milligrams of cholesterol." .

ns1:circle a rdf:Property ;
	rdfs:label "circle" ;
	ns1:domainIncludes ns1:GeoShape ;
	ns1:rangeIncludes ns1:Text ;
	rdfs:comment "A circle is the circular region of a specified radius centered at a specified latitude and longitude. A circle is expressed as a pair followed by a radius in meters." .

ns1:citation a rdf:Property ;
	rdfs:label "citation" ;
	ns1:domainIncludes ns1:CreativeWork ;
	ns1:rangeIncludes ns1:CreativeWork , ns1:Text ;
	rdfs:comment "A citation or reference to another creative work, such as another publication, web page, scholarly article, etc." .

ns1:clincalPharmacology a rdf:Property ;
	rdfs:label "clincalPharmacology" ;
	ns1:domainIncludes ns1:Drug ;
	ns1:rangeIncludes ns1:Text ;
	rdfs:comment "Description of the absorption and elimination of drugs, including their concentration (pharmacokinetics, pK) and biological effects (pharmacodynamics, pD)." .

ns1:clipNumber a rdf:Property ;
	rdfs:label "clipNumber" ;
	ns1:domainIncludes ns1:Clip ;
	ns1:rangeIncludes ns1:Integer ;
	rdfs:comment "Position of the clip within an ordered group of clips." .

ns1:closes a rdf:Property ;
	rdfs:label "closes" ;
	ns1:domainIncludes ns1:OpeningHoursSpecification ;
	ns1:rangeIncludes ns1:Time ;
	rdfs:comment "The closing hour of the place or service on the given day(s) of the week." .

ns1:code a rdf:Property ;
	rdfs:label "code" ;
	ns1:domainIncludes ns1:MedicalEntity ;
	ns1:rangeIncludes ns1:MedicalCode ;
	rdfs:comment "A medical code for the entity, taken from a controlled vocabulary or ontology such as ICD-9, DiseasesDB, MeSH, SNOMED-CT, RxNorm, etc." .

ns1:codeRepository a rdf:Property ;
	rdfs:label "codeRepository" ;
	ns1:domainIncludes ns1:Code ;
	ns1:rangeIncludes ns1:URL ;
	rdfs:comment "Link to the repository where the un-compiled, human readable code and related code is located (SVN, github, CodePlex)" .

ns1:codeValue a rdf:Property ;
	rdfs:label "codeValue" ;
	ns1:domainIncludes ns1:MedicalCode ;
	ns1:rangeIncludes ns1:Text ;
	rdfs:comment "The actual code." .

ns1:codingSystem a rdf:Property ;
	rdfs:label "codingSystem" ;
	ns1:domainIncludes ns1:MedicalCode ;
	ns1:rangeIncludes ns1:Text ;
	rdfs:comment "The coding system, e.g. 'ICD-10'." .

ns1:colleagues a rdf:Property ;
	rdfs:label "colleagues" ;
	ns1:domainIncludes ns1:Person ;
	ns1:rangeIncludes ns1:Person ;
	ns1:supercededBy ns1:colleague ;
	rdfs:comment "A colleague of the person (legacy spelling; see singular form, colleague)." .

ns1:collection a rdf:Property ;
	rdfs:label "collection" ;
	ns1:domainIncludes ns1:UpdateAction ;
	ns1:rangeIncludes ns1:Thing ;
	rdfs:comment "A sub property of object. The collection target of the action." ;
	rdfs:subPropertyOf ns1:object .

ns1:color a rdf:Property ;
	rdfs:label "color" ;
	ns1:domainIncludes ns1:Product ;
	ns1:rangeIncludes ns1:Text ;
	rdfs:comment "The color of the product." .

ns1:comment a rdf:Property ;
	rdfs:label "comment" ;
	ns1:domainIncludes ns1:CreativeWork ;
	ns1:rangeIncludes ns1:Comment , ns1:UserComments ;
	rdfs:comment "Comments, typically from users, on this CreativeWork." .

ns1:commentCount a rdf:Property ;
	rdfs:label "commentCount" ;
	ns1:domainIncludes ns1:CreativeWork ;
	ns1:rangeIncludes ns1:Integer ;
	rdfs:comment "The number of comments this CreativeWork (e.g. Article, Question or Answer) has received. This is most applicable to works published in Web sites with commenting system; additional comments may exist elsewhere." .

ns1:commentText a rdf:Property ;
	rdfs:label "commentText" ;
	ns1:domainIncludes ns1:UserComments ;
	ns1:rangeIncludes ns1:Text ;
	rdfs:comment "The text of the UserComment." .

ns1:commentTime a rdf:Property ;
	rdfs:label "commentTime" ;
	ns1:domainIncludes ns1:UserComments ;
	ns1:rangeIncludes ns1:Date ;
	rdfs:comment "The time at which the UserComment was made." .

ns1:comprisedOf a rdf:Property ;
	rdfs:label "comprisedOf" ;
	ns1:domainIncludes ns1:AnatomicalSystem ;
	ns1:rangeIncludes ns1:AnatomicalStructure , ns1:AnatomicalSystem ;
	rdfs:comment "The underlying anatomical structures, such as organs, that comprise the anatomical system." .

ns1:confirmationNumber a rdf:Property ;
	rdfs:label "confirmationNumber" ;
	ns1:domainIncludes ns1:Order ;
	ns1:rangeIncludes ns1:Text ;
	rdfs:comment "A number that confirms the given order." .

ns1:connectedTo a rdf:Property ;
	rdfs:label "connectedTo" ;
	ns1:domainIncludes ns1:AnatomicalStructure ;
	ns1:rangeIncludes ns1:AnatomicalStructure ;
	rdfs:comment "Other anatomical structures to which this structure is connected." .

ns1:contactOption a rdf:Property ;
	rdfs:label "contactOption" ;
	ns1:domainIncludes ns1:ContactPoint ;
	ns1:rangeIncludes ns1:ContactPointOption ;
	rdfs:comment "An option available on this contact point (e.g. a toll-free number or support for hearing-impaired callers.)" .

ns1:contactPoints a rdf:Property ;
	rdfs:label "contactPoints" ;
	ns1:domainIncludes ns1:Organization , ns1:Person ;
	ns1:rangeIncludes ns1:ContactPoint ;
	ns1:supercededBy ns1:contactPoint ;
	rdfs:comment "A contact point for a person or organization (legacy spelling; see singular form, contactPoint)." .

ns1:contactType a rdf:Property ;
	rdfs:label "contactType" ;
	ns1:domainIncludes ns1:ContactPoint ;
	ns1:rangeIncludes ns1:Text ;
	rdfs:comment "A person or organization can have different contact points, for different purposes. For example, a sales contact point, a PR contact point and so on. This property is used to specify the kind of contact point." .

ns1:containedIn a rdf:Property ;
	rdfs:label "containedIn" ;
	ns1:domainIncludes ns1:Place ;
	ns1:rangeIncludes ns1:Place ;
	rdfs:comment "The basic containment relation between places." .

ns1:contentLocation a rdf:Property ;
	rdfs:label "contentLocation" ;
	ns1:domainIncludes ns1:CreativeWork ;
	ns1:rangeIncludes ns1:Place ;
	rdfs:comment "The location of the content." .

ns1:contentRating a rdf:Property ;
	rdfs:label "contentRating" ;
	ns1:domainIncludes ns1:CreativeWork ;
	ns1:rangeIncludes ns1:Text ;
	rdfs:comment "Official rating of a piece of content&#x2014;for example,'MPAA PG-13'." .

ns1:contentSize a rdf:Property ;
	rdfs:label "contentSize" ;
	ns1:domainIncludes ns1:MediaObject ;
	ns1:rangeIncludes ns1:Text ;
	rdfs:comment "File size in (mega/kilo) bytes." .

ns1:contentType a rdf:Property ;
	rdfs:label "contentType" ;
	ns1:domainIncludes ns1:EntryPoint ;
	ns1:rangeIncludes ns1:Text ;
	rdfs:comment "The supported content type(s) for an EntryPoint response." .

ns1:contentUrl a rdf:Property ;
	rdfs:label "contentUrl" ;
	ns1:domainIncludes ns1:MediaObject ;
	ns1:rangeIncludes ns1:URL ;
	rdfs:comment "Actual bytes of the media object, for example the image file or video file. (previous spelling: contentURL)" .

ns1:contraindication a rdf:Property ;
	rdfs:label "contraindication" ;
	ns1:domainIncludes ns1:MedicalDevice , ns1:MedicalTherapy ;
	ns1:rangeIncludes ns1:MedicalContraindication ;
	rdfs:comment "A contraindication for this therapy." .

ns1:contributor a rdf:Property ;
	rdfs:label "contributor" ;
	ns1:domainIncludes ns1:CreativeWork ;
	ns1:rangeIncludes ns1:Organization , ns1:Person ;
	rdfs:comment "A secondary contributor to the CreativeWork." .

ns1:cookTime a rdf:Property ;
	rdfs:label "cookTime" ;
	ns1:domainIncludes ns1:Recipe ;
	ns1:rangeIncludes ns1:Duration ;
	rdfs:comment "The time it takes to actually cook the dish, in <a href='http://en.wikipedia.org/wiki/ISO_8601'>ISO 8601 duration format</a>." .

ns1:cookingMethod a rdf:Property ;
	rdfs:label "cookingMethod" ;
	ns1:domainIncludes ns1:Recipe ;
	ns1:rangeIncludes ns1:Text ;
	rdfs:comment "The method of cooking, such as Frying, Steaming, ..." .

ns1:copyrightHolder a rdf:Property ;
	rdfs:label "copyrightHolder" ;
	ns1:domainIncludes ns1:CreativeWork ;
	ns1:rangeIncludes ns1:Organization , ns1:Person ;
	rdfs:comment "The party holding the legal copyright to the CreativeWork." .

ns1:copyrightYear a rdf:Property ;
	rdfs:label "copyrightYear" ;
	ns1:domainIncludes ns1:CreativeWork ;
	ns1:rangeIncludes ns1:Number ;
	rdfs:comment "The year during which the claimed copyright for the CreativeWork was first asserted." .

ns1:cost a rdf:Property ;
	rdfs:label "cost" ;
	ns1:domainIncludes ns1:Drug ;
	ns1:rangeIncludes ns1:DrugCost ;
	rdfs:comment "Cost per unit of the drug, as reported by the source being tagged." .

ns1:costCategory a rdf:Property ;
	rdfs:label "costCategory" ;
	ns1:domainIncludes ns1:DrugCost ;
	ns1:rangeIncludes ns1:DrugCostCategory ;
	rdfs:comment "The category of cost, such as wholesale, retail, reimbursement cap, etc." .

ns1:costCurrency a rdf:Property ;
	rdfs:label "costCurrency" ;
	ns1:domainIncludes ns1:DrugCost ;
	ns1:rangeIncludes ns1:Text ;
	rdfs:comment "The currency (in 3-letter <a href=http://en.wikipedia.org/wiki/ISO_4217>ISO 4217 format</a>) of the drug cost." .

ns1:costOrigin a rdf:Property ;
	rdfs:label "costOrigin" ;
	ns1:domainIncludes ns1:DrugCost ;
	ns1:rangeIncludes ns1:Text ;
	rdfs:comment "Additional details to capture the origin of the cost data. For example, 'Medicare Part B'." .

ns1:costPerUnit a rdf:Property ;
	rdfs:label "costPerUnit" ;
	ns1:domainIncludes ns1:DrugCost ;
	ns1:rangeIncludes ns1:Number , ns1:Text ;
	rdfs:comment "The cost per unit of the drug." .

ns1:countriesNotSupported a rdf:Property ;
	rdfs:label "countriesNotSupported" ;
	ns1:domainIncludes ns1:SoftwareApplication ;
	ns1:rangeIncludes ns1:Text ;
	rdfs:comment "Countries for which the application is not supported. You can also provide the two-letter ISO 3166-1 alpha-2 country code." .

ns1:countriesSupported a rdf:Property ;
	rdfs:label "countriesSupported" ;
	ns1:domainIncludes ns1:SoftwareApplication ;
	ns1:rangeIncludes ns1:Text ;
	rdfs:comment "Countries for which the application is supported. You can also provide the two-letter ISO 3166-1 alpha-2 country code." .

ns1:course a rdf:Property ;
	rdfs:label "course" ;
	ns1:domainIncludes ns1:ExerciseAction ;
	ns1:rangeIncludes ns1:Place ;
	rdfs:comment "A sub property of location. The course where this action was taken." ;
	rdfs:subPropertyOf ns1:location .

ns1:creator a rdf:Property ;
	rdfs:label "creator" ;
	ns1:domainIncludes ns1:CreativeWork , ns1:UserComments ;
	ns1:rangeIncludes ns1:Organization , ns1:Person ;
	rdfs:comment "The creator/author of this CreativeWork or UserComments. This is the same as the Author property for CreativeWork." .

ns1:currenciesAccepted a rdf:Property ;
	rdfs:label "currenciesAccepted" ;
	ns1:domainIncludes ns1:LocalBusiness ;
	ns1:rangeIncludes ns1:Text ;
	rdfs:comment "The currency accepted (in <a href='http://en.wikipedia.org/wiki/ISO_4217'>ISO 4217 currency format</a>)." .

ns1:customer a rdf:Property ;
	rdfs:label "customer" ;
	ns1:domainIncludes ns1:Order ;
	ns1:rangeIncludes ns1:Organization , ns1:Person ;
	rdfs:comment "Party placing the order." .

ns1:dataset a rdf:Property ;
	rdfs:label "dataset" ;
	ns1:domainIncludes ns1:DataCatalog ;
	ns1:rangeIncludes ns1:Dataset ;
	rdfs:comment "A dataset contained in a catalog." .

ns1:dateCreated a rdf:Property ;
	rdfs:label "dateCreated" ;
	ns1:domainIncludes ns1:CreativeWork ;
	ns1:rangeIncludes ns1:Date ;
	rdfs:comment "The date on which the CreativeWork was created." .

ns1:dateIssued a rdf:Property ;
	rdfs:label "dateIssued" ;
	ns1:domainIncludes ns1:Ticket ;
	ns1:rangeIncludes ns1:DateTime ;
	rdfs:comment "The date the ticket was issued." .

ns1:dateModified a rdf:Property ;
	rdfs:label "dateModified" ;
	ns1:domainIncludes ns1:CreativeWork ;
	ns1:rangeIncludes ns1:Date ;
	rdfs:comment "The date on which the CreativeWork was most recently modified." .

ns1:datePosted a rdf:Property ;
	rdfs:label "datePosted" ;
	ns1:domainIncludes ns1:JobPosting ;
	ns1:rangeIncludes ns1:Date ;
	rdfs:comment "Publication date for the job posting." .

ns1:datePublished a rdf:Property ;
	rdfs:label "datePublished" ;
	ns1:domainIncludes ns1:CreativeWork ;
	ns1:rangeIncludes ns1:Date ;
	rdfs:comment "Date of first broadcast/publication." .

ns1:dateline a rdf:Property ;
	rdfs:label "dateline" ;
	ns1:domainIncludes ns1:NewsArticle ;
	ns1:rangeIncludes ns1:Text ;
	rdfs:comment "The location where the NewsArticle was produced." .

ns1:dayOfWeek a rdf:Property ;
	rdfs:label "dayOfWeek" ;
	ns1:domainIncludes ns1:OpeningHoursSpecification ;
	ns1:rangeIncludes ns1:DayOfWeek ;
	rdfs:comment "The day of the week for which these opening hours are valid." .

ns1:deathDate a rdf:Property ;
	rdfs:label "deathDate" ;
	ns1:domainIncludes ns1:Person ;
	ns1:rangeIncludes ns1:Date ;
	rdfs:comment "Date of death." .

ns1:defaultValue a rdf:Property ;
	rdfs:label "defaultValue" ;
	ns1:domainIncludes ns1:PropertyValueSpecification ;
	ns1:rangeIncludes ns1:Text , ns1:Thing ;
	rdfs:comment "The default value of the input.  For properties that expect a literal, the default is a literal value, for properties that expect an object, it's an ID reference to one of the current values." .

ns1:deliveryAddress a rdf:Property ;
	rdfs:label "deliveryAddress" ;
	ns1:domainIncludes ns1:ParcelDelivery ;
	ns1:rangeIncludes ns1:PostalAddress ;
	rdfs:comment "Destination address." .

ns1:deliveryLeadTime a rdf:Property ;
	rdfs:label "deliveryLeadTime" ;
	ns1:domainIncludes ns1:Demand , ns1:Offer ;
	ns1:rangeIncludes ns1:QuantitativeValue ;
	rdfs:comment "The typical delay between the receipt of the order and the goods leaving the warehouse." .

ns1:deliveryMethod a rdf:Property ;
	rdfs:label "deliveryMethod" ;
	ns1:domainIncludes ns1:ReceiveAction , ns1:SendAction , ns1:TrackAction ;
	ns1:rangeIncludes ns1:DeliveryMethod ;
	rdfs:comment "A sub property of instrument. The method of delivery" ;
	rdfs:subPropertyOf ns1:instrument .

ns1:deliveryStatus a rdf:Property ;
	rdfs:label "deliveryStatus" ;
	ns1:domainIncludes ns1:ParcelDelivery ;
	ns1:rangeIncludes ns1:DeliveryEvent ;
	rdfs:comment "New entry added as the package passes through each leg of its journey (from shipment to final delivery)." .

ns1:department a rdf:Property ;
	rdfs:label "department" ;
	ns1:domainIncludes ns1:Organization ;
	ns1:rangeIncludes ns1:Organization ;
	rdfs:comment "A relationship between an organization and a department of that organization, also described as an organization (allowing different urls, logos, opening hours). For example: a store with a pharmacy, or a bakery with a cafe." .

ns1:departureAirport a rdf:Property ;
	rdfs:label "departureAirport" ;
	ns1:domainIncludes ns1:Flight ;
	ns1:rangeIncludes ns1:Airport ;
	rdfs:comment "The airport where the flight originates." .

ns1:departureBusStop a rdf:Property ;
	rdfs:label "departureBusStop" ;
	ns1:domainIncludes ns1:BusTrip ;
	ns1:rangeIncludes ns1:BusStation , ns1:BusStop ;
	rdfs:comment "The stop or station from which the bus departs." .

ns1:departureGate a rdf:Property ;
	rdfs:label "departureGate" ;
	ns1:domainIncludes ns1:Flight ;
	ns1:rangeIncludes ns1:Text ;
	rdfs:comment "Identifier of the flight's departure gate." .

ns1:departurePlatform a rdf:Property ;
	rdfs:label "departurePlatform" ;
	ns1:domainIncludes ns1:TrainTrip ;
	ns1:rangeIncludes ns1:Text ;
	rdfs:comment "The platform from which the train departs." .

ns1:departureStation a rdf:Property ;
	rdfs:label "departureStation" ;
	ns1:domainIncludes ns1:TrainTrip ;
	ns1:rangeIncludes ns1:TrainStation ;
	rdfs:comment "The station from which the train departs." .

ns1:departureTerminal a rdf:Property ;
	rdfs:label "departureTerminal" ;
	ns1:domainIncludes ns1:Flight ;
	ns1:rangeIncludes ns1:Text ;
	rdfs:comment "Identifier of the flight's departure terminal." .

ns1:departureTime a rdf:Property ;
	rdfs:label "departureTime" ;
	ns1:domainIncludes ns1:BusTrip , ns1:Flight , ns1:TrainTrip ;
	ns1:rangeIncludes ns1:DateTime ;
	rdfs:comment "The expected departure time." .

ns1:dependencies a rdf:Property ;
	rdfs:label "dependencies" ;
	ns1:domainIncludes ns1:TechArticle ;
	ns1:rangeIncludes ns1:Text ;
	rdfs:comment "Prerequisites needed to fulfill steps in article." .

ns1:depth a rdf:Property ;
	rdfs:label "depth" ;
	ns1:domainIncludes ns1:Product ;
	ns1:rangeIncludes ns1:Distance , ns1:QuantitativeValue ;
	rdfs:comment "The depth of the product." .

ns1:description a rdf:Property ;
	rdfs:label "description" ;
	ns1:domainIncludes ns1:Thing ;
	ns1:rangeIncludes ns1:Text ;
	rdfs:comment "A short description of the item." .

ns1:device a rdf:Property ;
	rdfs:label "device" ;
	ns1:domainIncludes ns1:SoftwareApplication ;
	ns1:rangeIncludes ns1:Text ;
	rdfs:comment "Device required to run the application. Used in cases where a specific make/model is required to run the application." .

ns1:diagnosis a rdf:Property ;
	rdfs:label "diagnosis" ;
	ns1:domainIncludes ns1:DDxElement ;
	ns1:rangeIncludes ns1:MedicalCondition ;
	rdfs:comment "One or more alternative conditions considered in the differential diagnosis process." .

ns1:diagram a rdf:Property ;
	rdfs:label "diagram" ;
	ns1:domainIncludes ns1:AnatomicalStructure ;
	ns1:rangeIncludes ns1:ImageObject ;
	rdfs:comment "An image containing a diagram that illustrates the structure and/or its component substructures and/or connections with other structures." .

ns1:diet a rdf:Property ;
	rdfs:label "diet" ;
	ns1:domainIncludes ns1:ExerciseAction ;
	ns1:rangeIncludes ns1:Diet ;
	rdfs:comment "A sub property of instrument. The diet used in this action." ;
	rdfs:subPropertyOf ns1:instrument .

ns1:dietFeatures a rdf:Property ;
	rdfs:label "dietFeatures" ;
	ns1:domainIncludes ns1:Diet ;
	ns1:rangeIncludes ns1:Text ;
	rdfs:comment "Nutritional information specific to the dietary plan. May include dietary recommendations on what foods to avoid, what foods to consume, and specific alterations/deviations from the USDA or other regulatory body's approved dietary guidelines." .

ns1:differentialDiagnosis a rdf:Property ;
	rdfs:label "differentialDiagnosis" ;
	ns1:domainIncludes ns1:MedicalCondition ;
	ns1:rangeIncludes ns1:DDxElement ;
	rdfs:comment "One of a set of differential diagnoses for the condition. Specifically, a closely-related or competing diagnosis typically considered later in the cognitive process whereby this medical condition is distinguished from others most likely responsible for a similar collection of signs and symptoms to reach the most parsimonious diagnosis or diagnoses in a patient." .

ns1:directors a rdf:Property ;
	rdfs:label "directors" ;
	ns1:domainIncludes ns1:Episode , ns1:Movie , ns1:RadioEpisode , ns1:RadioSeries , ns1:Series , ns1:TVEpisode , ns1:TVSeries ;
	ns1:rangeIncludes ns1:Person ;
	ns1:supercededBy ns1:director ;
	rdfs:comment "The director of the movie, tv/radio episode or series. (legacy spelling; see singular form, director)" .

ns1:discount a rdf:Property ;
	rdfs:label "discount" ;
	ns1:domainIncludes ns1:Order ;
	ns1:rangeIncludes ns1:Number , ns1:Text ;
	rdfs:comment "Any discount applied (to an Order)." .

ns1:discountCode a rdf:Property ;
	rdfs:label "discountCode" ;
	ns1:domainIncludes ns1:Order ;
	ns1:rangeIncludes ns1:Text ;
	rdfs:comment "Code used to redeem a discount." .

ns1:discountCurrency a rdf:Property ;
	rdfs:label "discountCurrency" ;
	ns1:domainIncludes ns1:Order ;
	ns1:rangeIncludes ns1:Text ;
	rdfs:comment "The currency (in 3-letter ISO 4217 format) of the discount." .

ns1:discusses a rdf:Property ;
	rdfs:label "discusses" ;
	ns1:domainIncludes ns1:UserComments ;
	ns1:rangeIncludes ns1:CreativeWork ;
	rdfs:comment "Specifies the CreativeWork associated with the UserComment." .

ns1:discussionUrl a rdf:Property ;
	rdfs:label "discussionUrl" ;
	ns1:domainIncludes ns1:CreativeWork ;
	ns1:rangeIncludes ns1:URL ;
	rdfs:comment "A link to the page containing the comments of the CreativeWork." .

ns1:dissolutionDate a rdf:Property ;
	rdfs:label "dissolutionDate" ;
	ns1:domainIncludes ns1:Organization ;
	ns1:rangeIncludes ns1:Date ;
	rdfs:comment "The date that this organization was dissolved." .

ns1:distance a rdf:Property ;
	rdfs:label "distance" ;
	ns1:domainIncludes ns1:ExerciseAction , ns1:TravelAction ;
	ns1:rangeIncludes ns1:Distance ;
	rdfs:comment "The distance travelled, e.g. exercising or travelling." .

ns1:distinguishingSign a rdf:Property ;
	rdfs:label "distinguishingSign" ;
	ns1:domainIncludes ns1:DDxElement ;
	ns1:rangeIncludes ns1:MedicalSignOrSymptom ;
	rdfs:comment "One of a set of signs and symptoms that can be used to distinguish this diagnosis from others in the differential diagnosis." .

ns1:distribution a rdf:Property ;
	rdfs:label "distribution" ;
	ns1:domainIncludes ns1:Dataset ;
	ns1:rangeIncludes ns1:DataDownload ;
	rdfs:comment "A downloadable form of this dataset, at a specific location, in a specific format." .

ns1:domainIncludes a rdf:Property ;
	rdfs:label "domainIncludes" ;
	ns1:domainIncludes ns1:Property ;
	ns1:rangeIncludes ns1:Class ;
	rdfs:comment "Relates a property to a class that is (one of) the type(s) the property is expected to be used on." .

ns1:doorTime a rdf:Property ;
	rdfs:label "doorTime" ;
	ns1:domainIncludes ns1:Event ;
	ns1:rangeIncludes ns1:DateTime ;
	rdfs:comment "The time admission will commence." .

ns1:dosageForm a rdf:Property ;
	rdfs:label "dosageForm" ;
	ns1:domainIncludes ns1:DietarySupplement , ns1:Drug ;
	ns1:rangeIncludes ns1:Text ;
	rdfs:comment "A dosage form in which this drug/supplement is available, e.g. 'tablet', 'suspension', 'injection'." .

ns1:doseSchedule a rdf:Property ;
	rdfs:label "doseSchedule" ;
	ns1:domainIncludes ns1:Drug ;
	ns1:rangeIncludes ns1:DoseSchedule ;
	rdfs:comment "A dosing schedule for the drug for a given population, either observed, recommended, or maximum dose based on the type used." .

ns1:doseUnit a rdf:Property ;
	rdfs:label "doseUnit" ;
	ns1:domainIncludes ns1:DoseSchedule ;
	ns1:rangeIncludes ns1:Text ;
	rdfs:comment "The unit of the dose, e.g. 'mg'." .

ns1:doseValue a rdf:Property ;
	rdfs:label "doseValue" ;
	ns1:domainIncludes ns1:DoseSchedule ;
	ns1:rangeIncludes ns1:Number ;
	rdfs:comment "The value of the dose, e.g. 500." .

ns1:downloadUrl a rdf:Property ;
	rdfs:label "downloadUrl" ;
	ns1:domainIncludes ns1:SoftwareApplication ;
	ns1:rangeIncludes ns1:URL ;
	rdfs:comment "If the file can be downloaded, URL to download the binary." .

ns1:downvoteCount a rdf:Property ;
	rdfs:label "downvoteCount" ;
	ns1:domainIncludes ns1:Answer , ns1:Comment , ns1:Question ;
	ns1:rangeIncludes ns1:Integer ;
	rdfs:comment "The number of downvotes this question has received from the community." .

ns1:drainsTo a rdf:Property ;
	rdfs:label "drainsTo" ;
	ns1:domainIncludes ns1:Vein ;
	ns1:rangeIncludes ns1:Vessel ;
	rdfs:comment "The vasculature that the vein drains into." .

ns1:dropoffLocation a rdf:Property ;
	rdfs:label "dropoffLocation" ;
	ns1:domainIncludes ns1:RentalCarReservation ;
	ns1:rangeIncludes ns1:Place ;
	rdfs:comment "Where a rental car can be dropped off." .

ns1:dropoffTime a rdf:Property ;
	rdfs:label "dropoffTime" ;
	ns1:domainIncludes ns1:RentalCarReservation ;
	ns1:rangeIncludes ns1:DateTime ;
	rdfs:comment "When a rental car can be dropped off." .

ns1:drug a rdf:Property ;
	rdfs:label "drug" ;
	ns1:domainIncludes ns1:DrugClass ;
	ns1:rangeIncludes ns1:Drug ;
	rdfs:comment "A drug in this drug class." .

ns1:drugClass a rdf:Property ;
	rdfs:label "drugClass" ;
	ns1:domainIncludes ns1:Drug ;
	ns1:rangeIncludes ns1:DrugClass ;
	rdfs:comment "The class of drug this belongs to (e.g., statins)." .

ns1:drugUnit a rdf:Property ;
	rdfs:label "drugUnit" ;
	ns1:domainIncludes ns1:DrugCost ;
	ns1:rangeIncludes ns1:Text ;
	rdfs:comment "The unit in which the drug is measured, e.g. '5 mg tablet'." .

ns1:duns a rdf:Property ;
	rdfs:label "duns" ;
	ns1:domainIncludes ns1:Organization , ns1:Person ;
	ns1:rangeIncludes ns1:Text ;
	rdfs:comment "The Dun & Bradstreet DUNS number for identifying an organization or business person." .

ns1:duplicateTherapy a rdf:Property ;
	rdfs:label "duplicateTherapy" ;
	ns1:domainIncludes ns1:MedicalTherapy ;
	ns1:rangeIncludes ns1:MedicalTherapy ;
	rdfs:comment "A therapy that duplicates or overlaps this one." .

ns1:duration a rdf:Property ;
	rdfs:label "duration" ;
	ns1:domainIncludes ns1:Event , ns1:MediaObject , ns1:Movie , ns1:MusicRecording ;
	ns1:rangeIncludes ns1:Duration ;
	rdfs:comment "The duration of the item (movie, audio recording, event, etc.) in <a href='http://en.wikipedia.org/wiki/ISO_8601'>ISO 8601 date format</a>." .

ns1:durationOfWarranty a rdf:Property ;
	rdfs:label "durationOfWarranty" ;
	ns1:domainIncludes ns1:WarrantyPromise ;
	ns1:rangeIncludes ns1:QuantitativeValue ;
	rdfs:comment "The duration of the warranty promise. Common unitCode values are ANN for year, MON for months, or DAY for days." .

ns1:editor a rdf:Property ;
	rdfs:label "editor" ;
	ns1:domainIncludes ns1:CreativeWork ;
	ns1:rangeIncludes ns1:Person ;
	rdfs:comment "Specifies the Person who edited the CreativeWork." .

ns1:educationRequirements a rdf:Property ;
	rdfs:label "educationRequirements" ;
	ns1:domainIncludes ns1:JobPosting ;
	ns1:rangeIncludes ns1:Text ;
	rdfs:comment "Educational background needed for the position." .

ns1:educationalAlignment a rdf:Property ;
	rdfs:label "educationalAlignment" ;
	ns1:domainIncludes ns1:CreativeWork ;
	ns1:rangeIncludes ns1:AlignmentObject ;
	rdfs:comment "An alignment to an established educational framework." .

ns1:educationalFramework a rdf:Property ;
	rdfs:label "educationalFramework" ;
	ns1:domainIncludes ns1:AlignmentObject ;
	ns1:rangeIncludes ns1:Text ;
	rdfs:comment "The framework to which the resource being described is aligned." .

ns1:educationalRole a rdf:Property ;
	rdfs:label "educationalRole" ;
	ns1:domainIncludes ns1:EducationalAudience ;
	ns1:rangeIncludes ns1:Text ;
	rdfs:comment "An educationalRole of an EducationalAudience" .

ns1:educationalUse a rdf:Property ;
	rdfs:label "educationalUse" ;
	ns1:domainIncludes ns1:CreativeWork ;
	ns1:rangeIncludes ns1:Text ;
	rdfs:comment "The purpose of a work in the context of education; for example, 'assignment', 'group work'." .

ns1:elevation a rdf:Property ;
	rdfs:label "elevation" ;
	ns1:domainIncludes ns1:GeoCoordinates , ns1:GeoShape ;
	ns1:rangeIncludes ns1:Number , ns1:Text ;
	rdfs:comment "The elevation of a location." .

ns1:eligibleCustomerType a rdf:Property ;
	rdfs:label "eligibleCustomerType" ;
	ns1:domainIncludes ns1:Demand , ns1:Offer ;
	ns1:rangeIncludes ns1:BusinessEntityType ;
	rdfs:comment "The type(s) of customers for which the given offer is valid." .

ns1:eligibleDuration a rdf:Property ;
	rdfs:label "eligibleDuration" ;
	ns1:domainIncludes ns1:Demand , ns1:Offer ;
	ns1:rangeIncludes ns1:QuantitativeValue ;
	rdfs:comment "The duration for which the given offer is valid." .

ns1:eligibleQuantity a rdf:Property ;
	rdfs:label "eligibleQuantity" ;
	ns1:domainIncludes ns1:Demand , ns1:Offer , ns1:PriceSpecification ;
	ns1:rangeIncludes ns1:QuantitativeValue ;
	rdfs:comment "The interval and unit of measurement of ordering quantities for which the offer or price specification is valid. This allows e.g. specifying that a certain freight charge is valid only for a certain quantity." .

ns1:eligibleRegion a rdf:Property ;
	rdfs:label "eligibleRegion" ;
	ns1:domainIncludes ns1:DeliveryChargeSpecification , ns1:Demand , ns1:Offer ;
	ns1:rangeIncludes ns1:GeoShape , ns1:Text ;
	rdfs:comment "The ISO 3166-1 (ISO 3166-1 alpha-2) or ISO 3166-2 code, or the GeoShape for the geo-political region(s) for which the offer or delivery charge specification is valid." .

ns1:eligibleTransactionVolume a rdf:Property ;
	rdfs:label "eligibleTransactionVolume" ;
	ns1:domainIncludes ns1:Demand , ns1:Offer , ns1:PriceSpecification ;
	ns1:rangeIncludes ns1:PriceSpecification ;
	rdfs:comment "The transaction volume, in a monetary unit, for which the offer or price specification is valid, e.g. for indicating a minimal purchasing volume, to express free shipping above a certain order volume, or to limit the acceptance of credit cards to purchases to a certain minimal amount." .

ns1:email a rdf:Property ;
	rdfs:label "email" ;
	ns1:domainIncludes ns1:ContactPoint , ns1:Organization , ns1:Person ;
	ns1:rangeIncludes ns1:Text ;
	rdfs:comment "Email address." .

ns1:embedUrl a rdf:Property ;
	rdfs:label "embedUrl" ;
	ns1:domainIncludes ns1:MediaObject ;
	ns1:rangeIncludes ns1:URL ;
	rdfs:comment "A URL pointing to a player for a specific video. In general, this is the information in the <code>src</code> element of an <code>embed</code> tag and should not be the same as the content of the <code>loc</code> tag. (previous spelling: embedURL)" .

ns1:employees a rdf:Property ;
	rdfs:label "employees" ;
	ns1:domainIncludes ns1:Organization ;
	ns1:rangeIncludes ns1:Person ;
	ns1:supercededBy ns1:employee ;
	rdfs:comment "People working for this organization. (legacy spelling; see singular form, employee)" .

ns1:employmentType a rdf:Property ;
	rdfs:label "employmentType" ;
	ns1:domainIncludes ns1:JobPosting ;
	ns1:rangeIncludes ns1:Text ;
	rdfs:comment "Type of employment (e.g. full-time, part-time, contract, temporary, seasonal, internship)." .

ns1:encodesCreativeWork a rdf:Property ;
	rdfs:label "encodesCreativeWork" ;
	ns1:domainIncludes ns1:MediaObject ;
	ns1:rangeIncludes ns1:CreativeWork ;
	rdfs:comment "The creative work encoded by this media object" .

ns1:encodingFormat a rdf:Property ;
	rdfs:label "encodingFormat" ;
	ns1:domainIncludes ns1:MediaObject ;
	ns1:rangeIncludes ns1:Text ;
	rdfs:comment "mp3, mpeg4, etc." .

ns1:encodingType a rdf:Property ;
	rdfs:label "encodingType" ;
	ns1:domainIncludes ns1:EntryPoint ;
	ns1:rangeIncludes ns1:Text ;
	rdfs:comment "The supported encoding type(s) for an EntryPoint request." .

ns1:encodings a rdf:Property ;
	rdfs:label "encodings" ;
	ns1:domainIncludes ns1:CreativeWork ;
	ns1:rangeIncludes ns1:MediaObject ;
	ns1:supercededBy ns1:encoding ;
	rdfs:comment "The media objects that encode this creative work (legacy spelling; see singular form, encoding)." .

ns1:endDate a rdf:Property ;
	rdfs:label "endDate" ;
	ns1:domainIncludes ns1:Event , ns1:Role , ns1:Season , ns1:Series , ns1:TVSeason , ns1:TVSeries ;
	ns1:rangeIncludes ns1:Date ;
	rdfs:comment "The end date and time of the role, event or item (in <a href='http://en.wikipedia.org/wiki/ISO_8601'>ISO 8601 date format</a>)." .

ns1:endTime a rdf:Property ;
	rdfs:label "endTime" ;
	ns1:domainIncludes ns1:Action , ns1:FoodEstablishmentReservation ;
	ns1:rangeIncludes ns1:DateTime ;
	rdfs:comment """The endTime of something. For a reserved event or service (e.g. FoodEstablishmentReservation), the time that it is expected to end. For actions that span a period of time, when the action was performed. e.g. John wrote a book from January to *December*.

Note that Event uses startDate/endDate instead of startTime/endTime, even when describing dates with times. This situation may be clarified in future revisions.
""" .

ns1:endorsee a rdf:Property ;
	rdfs:label "endorsee" ;
	ns1:domainIncludes ns1:EndorseAction ;
	ns1:rangeIncludes ns1:Organization , ns1:Person ;
	rdfs:comment "A sub property of participant. The person/organization being supported." ;
	rdfs:subPropertyOf ns1:participant .

ns1:endorsers a rdf:Property ;
	rdfs:label "endorsers" ;
	ns1:domainIncludes ns1:Diet ;
	ns1:rangeIncludes ns1:Organization , ns1:Person ;
	rdfs:comment "People or organizations that endorse the plan." .

ns1:entertainmentBusiness a rdf:Property ;
	rdfs:label "entertainmentBusiness" ;
	ns1:domainIncludes ns1:PerformAction ;
	ns1:rangeIncludes ns1:EntertainmentBusiness ;
	rdfs:comment "A sub property of location. The entertainment business where the action occurred." ;
	rdfs:subPropertyOf ns1:location .

ns1:epidemiology a rdf:Property ;
	rdfs:label "epidemiology" ;
	ns1:domainIncludes ns1:MedicalCondition , ns1:PhysicalActivity ;
	ns1:rangeIncludes ns1:Text ;
	rdfs:comment "The characteristics of associated patients, such as age, gender, race etc." .

ns1:episodeNumber a rdf:Property ;
	rdfs:label "episodeNumber" ;
	ns1:domainIncludes ns1:Episode ;
	ns1:rangeIncludes ns1:Integer ;
	rdfs:comment "Position of the episode within an ordered group of episodes." .

ns1:episodes a rdf:Property ;
	rdfs:label "episodes" ;
	ns1:domainIncludes ns1:RadioSeason , ns1:RadioSeries , ns1:Season , ns1:Series , ns1:TVSeason , ns1:TVSeries ;
	ns1:rangeIncludes ns1:Episode ;
	ns1:supercededBy ns1:episode ;
	rdfs:comment "An episode of a TV/radio series or season (legacy spelling; see singular form, episode)" .

ns1:equal a rdf:Property ;
	rdfs:label "equal" ;
	ns1:domainIncludes ns1:QualitativeValue ;
	ns1:rangeIncludes ns1:QualitativeValue ;
	rdfs:comment "This ordering relation for qualitative values indicates that the subject is equal to the object." .

ns1:estimatedFlightDuration a rdf:Property ;
	rdfs:label "estimatedFlightDuration" ;
	ns1:domainIncludes ns1:Flight ;
	ns1:rangeIncludes ns1:Duration , ns1:Text ;
	rdfs:comment "The estimated time the flight will take." .

ns1:estimatesRiskOf a rdf:Property ;
	rdfs:label "estimatesRiskOf" ;
	ns1:domainIncludes ns1:MedicalRiskEstimator ;
	ns1:rangeIncludes ns1:MedicalEntity ;
	rdfs:comment "The condition, complication, or symptom whose risk is being estimated." .

ns1:eventStatus a rdf:Property ;
	rdfs:label "eventStatus" ;
	ns1:domainIncludes ns1:Event ;
	ns1:rangeIncludes ns1:EventStatusType ;
	rdfs:comment "An eventStatus of an event represents its status; particularly useful when an event is cancelled or rescheduled." .

ns1:events a rdf:Property ;
	rdfs:label "events" ;
	ns1:domainIncludes ns1:Organization , ns1:Place ;
	ns1:rangeIncludes ns1:Event ;
	ns1:supercededBy ns1:event ;
	rdfs:comment "Upcoming or past events associated with this place or organization (legacy spelling; see singular form, event)." .

ns1:evidenceLevel a rdf:Property ;
	rdfs:label "evidenceLevel" ;
	ns1:domainIncludes ns1:MedicalGuideline ;
	ns1:rangeIncludes ns1:MedicalEvidenceLevel ;
	rdfs:comment "Strength of evidence of the data used to formulate the guideline (enumerated)." .

ns1:evidenceOrigin a rdf:Property ;
	rdfs:label "evidenceOrigin" ;
	ns1:domainIncludes ns1:MedicalGuideline ;
	ns1:rangeIncludes ns1:Text ;
	rdfs:comment "Source of the data used to formulate the guidance, e.g. RCT, consensus opinion, etc." .

ns1:exercisePlan a rdf:Property ;
	rdfs:label "exercisePlan" ;
	ns1:domainIncludes ns1:ExerciseAction ;
	ns1:rangeIncludes ns1:ExercisePlan ;
	rdfs:comment "A sub property of instrument. The exercise plan used on this action." ;
	rdfs:subPropertyOf ns1:instrument .

ns1:exerciseType a rdf:Property ;
	rdfs:label "exerciseType" ;
	ns1:domainIncludes ns1:ExerciseAction , ns1:ExercisePlan ;
	ns1:rangeIncludes ns1:Text ;
	rdfs:comment "Type(s) of exercise or activity, such as strength training, flexibility training, aerobics, cardiac rehabilitation, etc." .

ns1:exifData a rdf:Property ;
	rdfs:label "exifData" ;
	ns1:domainIncludes ns1:ImageObject ;
	ns1:rangeIncludes ns1:Text ;
	rdfs:comment "exif data for this object." .

ns1:expectedArrivalFrom a rdf:Property ;
	rdfs:label "expectedArrivalFrom" ;
	ns1:domainIncludes ns1:ParcelDelivery ;
	ns1:rangeIncludes ns1:DateTime ;
	rdfs:comment "The earliest date the package may arrive." .

ns1:expectedArrivalUntil a rdf:Property ;
	rdfs:label "expectedArrivalUntil" ;
	ns1:domainIncludes ns1:ParcelDelivery ;
	ns1:rangeIncludes ns1:DateTime ;
	rdfs:comment "The latest date the package may arrive." .

ns1:expectedPrognosis a rdf:Property ;
	rdfs:label "expectedPrognosis" ;
	ns1:domainIncludes ns1:MedicalCondition ;
	ns1:rangeIncludes ns1:Text ;
	rdfs:comment "The likely outcome in either the short term or long term of the medical condition." .

ns1:experienceRequirements a rdf:Property ;
	rdfs:label "experienceRequirements" ;
	ns1:domainIncludes ns1:JobPosting ;
	ns1:rangeIncludes ns1:Text ;
	rdfs:comment "Description of skills and experience needed for the position." .

ns1:expertConsiderations a rdf:Property ;
	rdfs:label "expertConsiderations" ;
	ns1:domainIncludes ns1:Diet ;
	ns1:rangeIncludes ns1:Text ;
	rdfs:comment "Medical expert advice related to the plan." .

ns1:expires a rdf:Property ;
	rdfs:label "expires" ;
	ns1:domainIncludes ns1:MediaObject ;
	ns1:rangeIncludes ns1:Date ;
	rdfs:comment "Date the content expires and is no longer useful or available. Useful for videos." .

ns1:familyName a rdf:Property ;
	rdfs:label "familyName" ;
	ns1:domainIncludes ns1:Person ;
	ns1:rangeIncludes ns1:Text ;
	rdfs:comment "Family name. In the U.S., the last name of an Person. This can be used along with givenName instead of the Name property." .

ns1:fatContent a rdf:Property ;
	rdfs:label "fatContent" ;
	ns1:domainIncludes ns1:NutritionInformation ;
	ns1:rangeIncludes ns1:Mass ;
	rdfs:comment "The number of grams of fat." .

ns1:faxNumber a rdf:Property ;
	rdfs:label "faxNumber" ;
	ns1:domainIncludes ns1:ContactPoint , ns1:Organization , ns1:Person , ns1:Place ;
	ns1:rangeIncludes ns1:Text ;
	rdfs:comment "The fax number." .

ns1:featureList a rdf:Property ;
	rdfs:label "featureList" ;
	ns1:domainIncludes ns1:SoftwareApplication ;
	ns1:rangeIncludes ns1:Text , ns1:URL ;
	rdfs:comment "Features or modules provided by this application (and possibly required by other applications)." .

ns1:fiberContent a rdf:Property ;
	rdfs:label "fiberContent" ;
	ns1:domainIncludes ns1:NutritionInformation ;
	ns1:rangeIncludes ns1:Mass ;
	rdfs:comment "The number of grams of fiber." .

ns1:fileFormat a rdf:Property ;
	rdfs:label "fileFormat" ;
	ns1:domainIncludes ns1:SoftwareApplication ;
	ns1:rangeIncludes ns1:Text ;
	rdfs:comment "MIME format of the binary (e.g. application/zip)." .

ns1:fileSize a rdf:Property ;
	rdfs:label "fileSize" ;
	ns1:domainIncludes ns1:SoftwareApplication ;
	ns1:rangeIncludes ns1:Integer ;
	rdfs:comment "Size of the application / package (e.g. 18MB). In the absence of a unit (MB, KB etc.), KB will be assumed." .

ns1:flightDistance a rdf:Property ;
	rdfs:label "flightDistance" ;
	ns1:domainIncludes ns1:Flight ;
	ns1:rangeIncludes ns1:Distance , ns1:Text ;
	rdfs:comment "The distance of the flight." .

ns1:flightNumber a rdf:Property ;
	rdfs:label "flightNumber" ;
	ns1:domainIncludes ns1:Flight ;
	ns1:rangeIncludes ns1:Text ;
	rdfs:comment "The unique identifier for a flight, not including the airline IATA code. For example, if describing United flight 110, the flightNumber is '110'. The IATA code can be set on the Airline." .

ns1:followee a rdf:Property ;
	rdfs:label "followee" ;
	ns1:domainIncludes ns1:FollowAction ;
	ns1:rangeIncludes ns1:Organization , ns1:Person ;
	rdfs:comment "A sub property of object. The person or organization being followed." ;
	rdfs:subPropertyOf ns1:object .

ns1:follows a rdf:Property ;
	rdfs:label "follows" ;
	ns1:domainIncludes ns1:Person ;
	ns1:rangeIncludes ns1:Person ;
	rdfs:comment "The most generic uni-directional social relation." .

ns1:followup a rdf:Property ;
	rdfs:label "followup" ;
	ns1:domainIncludes ns1:MedicalProcedure ;
	ns1:rangeIncludes ns1:Text ;
	rdfs:comment "Typical or recommended followup care after the procedure is performed." .

ns1:foodEstablishment a rdf:Property ;
	rdfs:label "foodEstablishment" ;
	ns1:domainIncludes ns1:CookAction ;
	ns1:rangeIncludes ns1:FoodEstablishment , ns1:Place ;
	rdfs:comment "A sub property of location. The specific food establishment where the action occurred." ;
	rdfs:subPropertyOf ns1:location .

ns1:foodEvent a rdf:Property ;
	rdfs:label "foodEvent" ;
	ns1:domainIncludes ns1:CookAction ;
	ns1:rangeIncludes ns1:FoodEvent ;
	rdfs:comment "A sub property of location. The specific food event where the action occurred." ;
	rdfs:subPropertyOf ns1:location .

ns1:foodWarning a rdf:Property ;
	rdfs:label "foodWarning" ;
	ns1:domainIncludes ns1:Drug ;
	ns1:rangeIncludes ns1:Text ;
	rdfs:comment "Any precaution, guidance, contraindication, etc. related to consumption of specific foods while taking this drug." .

ns1:founders a rdf:Property ;
	rdfs:label "founders" ;
	ns1:domainIncludes ns1:Organization ;
	ns1:rangeIncludes ns1:Person ;
	ns1:supercededBy ns1:founder ;
	rdfs:comment "A person who founded this organization (legacy spelling; see singular form, founder)." .

ns1:foundingDate a rdf:Property ;
	rdfs:label "foundingDate" ;
	ns1:domainIncludes ns1:Organization ;
	ns1:rangeIncludes ns1:Date ;
	rdfs:comment "The date that this organization was founded." .

ns1:free a rdf:Property ;
	rdfs:label "free" ;
	ns1:domainIncludes ns1:PublicationEvent ;
	ns1:rangeIncludes ns1:Boolean ;
	rdfs:comment "A flag to signal that the publication is accessible for free." .

ns1:frequency a rdf:Property ;
	rdfs:label "frequency" ;
	ns1:domainIncludes ns1:DoseSchedule ;
	ns1:rangeIncludes ns1:Text ;
	rdfs:comment "How often the dose is taken, e.g. 'daily'." .

ns1:fromLocation a rdf:Property ;
	rdfs:label "fromLocation" ;
	ns1:domainIncludes ns1:ExerciseAction , ns1:MoveAction , ns1:TransferAction ;
	ns1:rangeIncludes ns1:Number , ns1:Place ;
	rdfs:comment "A sub property of location. The original location of the object or the agent before the action." ;
	rdfs:subPropertyOf ns1:location .

ns1:function a rdf:Property ;
	rdfs:label "function" ;
	ns1:domainIncludes ns1:AnatomicalStructure ;
	ns1:rangeIncludes ns1:Text ;
	rdfs:comment "Function of the anatomical structure." .

ns1:functionalClass a rdf:Property ;
	rdfs:label "functionalClass" ;
	ns1:domainIncludes ns1:Joint ;
	ns1:rangeIncludes ns1:Text ;
	rdfs:comment "The degree of mobility the joint allows." .

ns1:gender a rdf:Property ;
	rdfs:label "gender" ;
	ns1:domainIncludes ns1:Person ;
	ns1:rangeIncludes ns1:Text ;
	rdfs:comment "Gender of the person." .

ns1:genre a rdf:Property ;
	rdfs:label "genre" ;
	ns1:domainIncludes ns1:CreativeWork ;
	ns1:rangeIncludes ns1:Text ;
	rdfs:comment "Genre of the creative work" .

ns1:geo a rdf:Property ;
	rdfs:label "geo" ;
	ns1:domainIncludes ns1:Place ;
	ns1:rangeIncludes ns1:GeoCoordinates , ns1:GeoShape ;
	rdfs:comment "The geo coordinates of the place." .

ns1:geographicArea a rdf:Property ;
	rdfs:label "geographicArea" ;
	ns1:domainIncludes ns1:Audience ;
	ns1:rangeIncludes ns1:AdministrativeArea ;
	rdfs:comment "The geographic area associated with the audience." .

ns1:givenName a rdf:Property ;
	rdfs:label "givenName" ;
	ns1:domainIncludes ns1:Person ;
	ns1:rangeIncludes ns1:Text ;
	rdfs:comment "Given name. In the U.S., the first name of a Person. This can be used along with familyName instead of the Name property." .

ns1:globalLocationNumber a rdf:Property ;
	rdfs:label "globalLocationNumber" ;
	ns1:domainIncludes ns1:Organization , ns1:Person , ns1:Place ;
	ns1:rangeIncludes ns1:Text ;
	rdfs:comment "The Global Location Number (GLN, sometimes also referred to as International Location Number or ILN) of the respective organization, person, or place. The GLN is a 13-digit number used to identify parties and physical locations." .

ns1:greater a rdf:Property ;
	rdfs:label "greater" ;
	ns1:domainIncludes ns1:QualitativeValue ;
	ns1:rangeIncludes ns1:QualitativeValue ;
	rdfs:comment "This ordering relation for qualitative values indicates that the subject is greater than the object." .

ns1:greaterOrEqual a rdf:Property ;
	rdfs:label "greaterOrEqual" ;
	ns1:domainIncludes ns1:QualitativeValue ;
	ns1:rangeIncludes ns1:QualitativeValue ;
	rdfs:comment "This ordering relation for qualitative values indicates that the subject is greater than or equal to the object." .

ns1:gtin13 a rdf:Property ;
	rdfs:label "gtin13" ;
	ns1:domainIncludes ns1:Demand , ns1:Offer , ns1:Product ;
	ns1:rangeIncludes ns1:Text ;
	rdfs:comment "The GTIN-13 code of the product, or the product to which the offer refers. This is equivalent to 13-digit ISBN codes and EAN UCC-13. Former 12-digit UPC codes can be converted into a GTIN-13 code by simply adding a preceeding zero." .

ns1:gtin14 a rdf:Property ;
	rdfs:label "gtin14" ;
	ns1:domainIncludes ns1:Demand , ns1:Offer , ns1:Product ;
	ns1:rangeIncludes ns1:Text ;
	rdfs:comment "The GTIN-14 code of the product, or the product to which the offer refers." .

ns1:gtin8 a rdf:Property ;
	rdfs:label "gtin8" ;
	ns1:domainIncludes ns1:Demand , ns1:Offer , ns1:Product ;
	ns1:rangeIncludes ns1:Text ;
	rdfs:comment "The GTIN-8 code of the product, or the product to which the offer refers. This code is also known as EAN/UCC-8 or 8-digit EAN." .

ns1:guideline a rdf:Property ;
	rdfs:label "guideline" ;
	ns1:domainIncludes ns1:MedicalEntity ;
	ns1:rangeIncludes ns1:MedicalGuideline ;
	rdfs:comment "A medical guideline related to this entity." .

ns1:guidelineDate a rdf:Property ;
	rdfs:label "guidelineDate" ;
	ns1:domainIncludes ns1:MedicalGuideline ;
	ns1:rangeIncludes ns1:Date ;
	rdfs:comment "Date on which this guideline's recommendation was made." .

ns1:guidelineSubject a rdf:Property ;
	rdfs:label "guidelineSubject" ;
	ns1:domainIncludes ns1:MedicalGuideline ;
	ns1:rangeIncludes ns1:MedicalEntity ;
	rdfs:comment "The medical conditions, treatments, etc. that are the subject of the guideline." .

ns1:hasDeliveryMethod a rdf:Property ;
	rdfs:label "hasDeliveryMethod" ;
	ns1:domainIncludes ns1:DeliveryEvent , ns1:ParcelDelivery ;
	ns1:rangeIncludes ns1:DeliveryMethod ;
	rdfs:comment "Method used for delivery or shipping." .

ns1:hasPOS a rdf:Property ;
	rdfs:label "hasPOS" ;
	ns1:domainIncludes ns1:Organization , ns1:Person ;
	ns1:rangeIncludes ns1:Place ;
	rdfs:comment "Points-of-Sales operated by the organization or person." .

ns1:headline a rdf:Property ;
	rdfs:label "headline" ;
	ns1:domainIncludes ns1:CreativeWork ;
	ns1:rangeIncludes ns1:Text ;
	rdfs:comment "Headline of the article" .

ns1:healthCondition a rdf:Property ;
	rdfs:label "healthCondition" ;
	ns1:domainIncludes ns1:PeopleAudience ;
	ns1:rangeIncludes ns1:MedicalCondition ;
	rdfs:comment "Expectations for health conditions of target audience" .

ns1:height a rdf:Property ;
	rdfs:label "height" ;
	ns1:domainIncludes ns1:MediaObject , ns1:Product ;
	ns1:rangeIncludes ns1:Distance , ns1:QuantitativeValue ;
	rdfs:comment "The height of the item." .

ns1:highPrice a rdf:Property ;
	rdfs:label "highPrice" ;
	ns1:domainIncludes ns1:AggregateOffer ;
	ns1:rangeIncludes ns1:Number , ns1:Text ;
	rdfs:comment "The highest price of all offers available." .

ns1:hiringOrganization a rdf:Property ;
	rdfs:label "hiringOrganization" ;
	ns1:domainIncludes ns1:JobPosting ;
	ns1:rangeIncludes ns1:Organization ;
	rdfs:comment "Organization offering the job position." .

ns1:homeLocation a rdf:Property ;
	rdfs:label "homeLocation" ;
	ns1:domainIncludes ns1:Person ;
	ns1:rangeIncludes ns1:ContactPoint , ns1:Place ;
	rdfs:comment "A contact location for a person's residence." .

ns1:honorificPrefix a rdf:Property ;
	rdfs:label "honorificPrefix" ;
	ns1:domainIncludes ns1:Person ;
	ns1:rangeIncludes ns1:Text ;
	rdfs:comment "An honorific prefix preceding a Person's name such as Dr/Mrs/Mr." .

ns1:honorificSuffix a rdf:Property ;
	rdfs:label "honorificSuffix" ;
	ns1:domainIncludes ns1:Person ;
	ns1:rangeIncludes ns1:Text ;
	rdfs:comment "An honorific suffix preceding a Person's name such as M.D. /PhD/MSCSW." .

ns1:hospitalAffiliation a rdf:Property ;
	rdfs:label "hospitalAffiliation" ;
	ns1:domainIncludes ns1:Physician ;
	ns1:rangeIncludes ns1:Hospital ;
	rdfs:comment "A hospital with which the physician or office is affiliated." .

ns1:hostingOrganization a rdf:Property ;
	rdfs:label "hostingOrganization" ;
	ns1:domainIncludes ns1:ProgramMembership ;
	ns1:rangeIncludes ns1:Organization ;
	rdfs:comment "The organization (airline, travelers' club, etc.) the membership is made with." .

ns1:hoursAvailable a rdf:Property ;
	rdfs:label "hoursAvailable" ;
	ns1:domainIncludes ns1:ContactPoint ;
	ns1:rangeIncludes ns1:OpeningHoursSpecification ;
	rdfs:comment "The hours during which this contact point is available." .

ns1:howPerformed a rdf:Property ;
	rdfs:label "howPerformed" ;
	ns1:domainIncludes ns1:MedicalProcedure ;
	ns1:rangeIncludes ns1:Text ;
	rdfs:comment "How the procedure is performed." .

ns1:httpMethod a rdf:Property ;
	rdfs:label "httpMethod" ;
	ns1:domainIncludes ns1:EntryPoint ;
	ns1:rangeIncludes ns1:Text ;
	rdfs:comment "An HTTP method that specifies the appropriate HTTP method for a request to an HTTP EntryPoint. Values are capitalized strings as used in HTTP." .

ns1:iataCode a rdf:Property ;
	rdfs:label "iataCode" ;
	ns1:domainIncludes ns1:Airline , ns1:Airport ;
	ns1:rangeIncludes ns1:Text ;
	rdfs:comment "IATA identifier for an airline or airport" .

ns1:icaoCode a rdf:Property ;
	rdfs:label "iacoCode" ;
	ns1:domainIncludes ns1:Airport ;
	ns1:rangeIncludes ns1:Text ;
	rdfs:comment "IACO identifier for an airport." .

ns1:identifyingExam a rdf:Property ;
	rdfs:label "identifyingExam" ;
	ns1:domainIncludes ns1:MedicalSign ;
	ns1:rangeIncludes ns1:PhysicalExam ;
	rdfs:comment "A physical examination that can identify this sign." .

ns1:identifyingTest a rdf:Property ;
	rdfs:label "identifyingTest" ;
	ns1:domainIncludes ns1:MedicalSign ;
	ns1:rangeIncludes ns1:MedicalTest ;
	rdfs:comment "A diagnostic test that can identify this sign." .

ns1:illustrator a rdf:Property ;
	rdfs:label "illustrator" ;
	ns1:domainIncludes ns1:Book ;
	ns1:rangeIncludes ns1:Person ;
	rdfs:comment "The illustrator of the book." .

ns1:image a rdf:Property ;
	rdfs:label "image" ;
	ns1:domainIncludes ns1:Thing ;
	ns1:rangeIncludes ns1:URL ;
	rdfs:comment "URL of an image of the item." .

ns1:imagingTechnique a rdf:Property ;
	rdfs:label "imagingTechnique" ;
	ns1:domainIncludes ns1:ImagingTest ;
	ns1:rangeIncludes ns1:MedicalImagingTechnique ;
	rdfs:comment "Imaging technique used." .

ns1:inAlbum a rdf:Property ;
	rdfs:label "inAlbum" ;
	ns1:domainIncludes ns1:MusicRecording ;
	ns1:rangeIncludes ns1:MusicAlbum ;
	rdfs:comment "The album to which this recording belongs." .

ns1:inLanguage a rdf:Property ;
	rdfs:label "inLanguage" ;
	ns1:domainIncludes ns1:CreativeWork ;
	ns1:rangeIncludes ns1:Text ;
	rdfs:comment "The language of the content. please use one of the language codes from the <a href='http://tools.ietf.org/html/bcp47'>IETF BCP 47 standard.</a>" .

ns1:inPlaylist a rdf:Property ;
	rdfs:label "inPlaylist" ;
	ns1:domainIncludes ns1:MusicRecording ;
	ns1:rangeIncludes ns1:MusicPlaylist ;
	rdfs:comment "The playlist to which this recording belongs." .

ns1:incentives a rdf:Property ;
	rdfs:label "incentives" ;
	ns1:domainIncludes ns1:JobPosting ;
	ns1:rangeIncludes ns1:Text ;
	rdfs:comment "Description of bonus and commission compensation aspects of the job." .

ns1:includedRiskFactor a rdf:Property ;
	rdfs:label "includedRiskFactor" ;
	ns1:domainIncludes ns1:MedicalRiskEstimator ;
	ns1:rangeIncludes ns1:MedicalRiskFactor ;
	rdfs:comment "A modifiable or non-modifiable risk factor included in the calculation, e.g. age, coexisting condition." .

ns1:includesObject a rdf:Property ;
	rdfs:label "includesObject" ;
	ns1:domainIncludes ns1:Demand , ns1:Offer ;
	ns1:rangeIncludes ns1:TypeAndQuantityNode ;
	rdfs:comment "This links to a node or nodes indicating the exact quantity of the products included in the offer." .

ns1:increasesRiskOf a rdf:Property ;
	rdfs:label "increasesRiskOf" ;
	ns1:domainIncludes ns1:MedicalRiskFactor ;
	ns1:rangeIncludes ns1:MedicalEntity ;
	rdfs:comment "The condition, complication, etc. influenced by this factor." .

ns1:indication a rdf:Property ;
	rdfs:label "indication" ;
	ns1:domainIncludes ns1:MedicalDevice , ns1:MedicalTherapy ;
	ns1:rangeIncludes ns1:MedicalIndication ;
	rdfs:comment "A factor that indicates use of this therapy for treatment and/or prevention of a condition, symptom, etc. For therapies such as drugs, indications can include both officially-approved indications as well as off-label uses. These can be distinguished by using the ApprovedIndication subtype of MedicalIndication." .

ns1:industry a rdf:Property ;
	rdfs:label "industry" ;
	ns1:domainIncludes ns1:JobPosting ;
	ns1:rangeIncludes ns1:Text ;
	rdfs:comment "The industry associated with the job position." .

ns1:infectiousAgent a rdf:Property ;
	rdfs:label "infectiousAgent" ;
	ns1:domainIncludes ns1:InfectiousDisease ;
	ns1:rangeIncludes ns1:Text ;
	rdfs:comment "The actual infectious agent, such as a specific bacterium." .

ns1:infectiousAgentClass a rdf:Property ;
	rdfs:label "infectiousAgentClass" ;
	ns1:domainIncludes ns1:InfectiousDisease ;
	ns1:rangeIncludes ns1:InfectiousAgentClass ;
	rdfs:comment "The class of infectious agent (bacteria, prion, etc.) that causes the disease." .

ns1:ingredients a rdf:Property ;
	rdfs:label "ingredients" ;
	ns1:domainIncludes ns1:Recipe ;
	ns1:rangeIncludes ns1:Text ;
	rdfs:comment "An ingredient used in the recipe." .

ns1:insertion a rdf:Property ;
	rdfs:label "insertion" ;
	ns1:domainIncludes ns1:Muscle ;
	ns1:rangeIncludes ns1:AnatomicalStructure ;
	rdfs:comment "The place of attachment of a muscle, or what the muscle moves." .

ns1:installUrl a rdf:Property ;
	rdfs:label "installUrl" ;
	ns1:domainIncludes ns1:SoftwareApplication ;
	ns1:rangeIncludes ns1:URL ;
	rdfs:comment "URL at which the app may be installed, if different from the URL of the item." .

ns1:intensity a rdf:Property ;
	rdfs:label "intensity" ;
	ns1:domainIncludes ns1:ExercisePlan ;
	ns1:rangeIncludes ns1:Text ;
	rdfs:comment "Quantitative measure gauging the degree of force involved in the exercise, for example, heartbeats per minute. May include the velocity of the movement." .

ns1:interactingDrug a rdf:Property ;
	rdfs:label "interactingDrug" ;
	ns1:domainIncludes ns1:Drug ;
	ns1:rangeIncludes ns1:Drug ;
	rdfs:comment "Another drug that is known to interact with this drug in a way that impacts the effect of this drug or causes a risk to the patient. Note: disease interactions are typically captured as contraindications." .

ns1:interactionCount a rdf:Property ;
	rdfs:label "interactionCount" ;
	ns1:domainIncludes ns1:CreativeWork , ns1:MediaObject , ns1:Organization , ns1:Person , ns1:Place ;
	ns1:rangeIncludes ns1:Text ;
	rdfs:comment "A count of a specific user interactions with this item&#x2014;for example, <code>20 UserLikes</code>, <code>5 UserComments</code>, or <code>300 UserDownloads</code>. The user interaction type should be one of the sub types of <a href='UserInteraction'>UserInteraction</a>." .

ns1:interactivityType a rdf:Property ;
	rdfs:label "interactivityType" ;
	ns1:domainIncludes ns1:CreativeWork ;
	ns1:rangeIncludes ns1:Text ;
	rdfs:comment "The predominant mode of learning supported by the learning resource. Acceptable values are 'active', 'expositive', or 'mixed'." .

ns1:inventoryLevel a rdf:Property ;
	rdfs:label "inventoryLevel" ;
	ns1:domainIncludes ns1:Demand , ns1:Offer , ns1:SomeProducts ;
	ns1:rangeIncludes ns1:QuantitativeValue ;
	rdfs:comment "The current approximate inventory level for the item or items." .

ns1:inverseOf a rdf:Property ;
	rdfs:label "inverseOf" ;
	ns1:domainIncludes ns1:Property ;
	ns1:rangeIncludes ns1:Property ;
	rdfs:comment "Relates a property to a property that is its inverse. Inverse properties relate the same pairs of items to each other, but in reversed direction. For example, the 'alumni' and 'alumniOf' properties are inverseOf each other. Some properties don't have explicit inverses; in these situations RDFa and JSON-LD syntax for reverse properties can be used." .

ns1:isAccessoryOrSparePartFor a rdf:Property ;
	rdfs:label "isAccessoryOrSparePartFor" ;
	ns1:domainIncludes ns1:Product ;
	ns1:rangeIncludes ns1:Product ;
	rdfs:comment "A pointer to another product (or multiple products) for which this product is an accessory or spare part." .

ns1:isAvailableGenerically a rdf:Property ;
	rdfs:label "isAvailableGenerically" ;
	ns1:domainIncludes ns1:Drug ;
	ns1:rangeIncludes ns1:Boolean ;
	rdfs:comment "True if the drug is available in a generic form (regardless of name)." .

ns1:isBasedOnUrl a rdf:Property ;
	rdfs:label "isBasedOnUrl" ;
	ns1:domainIncludes ns1:CreativeWork ;
	ns1:rangeIncludes ns1:URL ;
	rdfs:comment "A resource that was used in the creation of this resource. This term can be repeated for multiple sources. For example, http://example.com/great-multiplication-intro.html" .

ns1:isConsumableFor a rdf:Property ;
	rdfs:label "isConsumableFor" ;
	ns1:domainIncludes ns1:Product ;
	ns1:rangeIncludes ns1:Product ;
	rdfs:comment "A pointer to another product (or multiple products) for which this product is a consumable." .

ns1:isFamilyFriendly a rdf:Property ;
	rdfs:label "isFamilyFriendly" ;
	ns1:domainIncludes ns1:CreativeWork ;
	ns1:rangeIncludes ns1:Boolean ;
	rdfs:comment "Indicates whether this content is family friendly." .

ns1:isGift a rdf:Property ;
	rdfs:label "isGift" ;
	ns1:domainIncludes ns1:Order ;
	ns1:rangeIncludes ns1:Boolean ;
	rdfs:comment "Was the offer accepted as a gift for someone other than the buyer." .

ns1:isPartOf a rdf:Property ;
	rdfs:label "isPartOf" ;
	ns1:domainIncludes ns1:WebPage ;
	ns1:rangeIncludes ns1:CollectionPage ;
	rdfs:comment "Indicates the collection or gallery to which the item belongs." .

ns1:isProprietary a rdf:Property ;
	rdfs:label "isProprietary" ;
	ns1:domainIncludes ns1:DietarySupplement , ns1:Drug ;
	ns1:rangeIncludes ns1:Boolean ;
	rdfs:comment "True if this item's name is a proprietary/brand name (vs. generic name)." .

ns1:isRelatedTo a rdf:Property ;
	rdfs:label "isRelatedTo" ;
	ns1:domainIncludes ns1:Product ;
	ns1:rangeIncludes ns1:Product ;
	rdfs:comment "A pointer to another, somehow related product (or multiple products)." .

ns1:isSimilarTo a rdf:Property ;
	rdfs:label "isSimilarTo" ;
	ns1:domainIncludes ns1:Product ;
	ns1:rangeIncludes ns1:Product ;
	rdfs:comment "A pointer to another, functionally similar product (or multiple products)." .

ns1:isVariantOf a rdf:Property ;
	rdfs:label "isVariantOf" ;
	ns1:domainIncludes ns1:ProductModel ;
	ns1:rangeIncludes ns1:ProductModel ;
	rdfs:comment "A pointer to a base product from which this product is a variant. It is safe to infer that the variant inherits all product features from the base model, unless defined locally. This is not transitive." .

ns1:isbn a rdf:Property ;
	rdfs:label "isbn" ;
	ns1:domainIncludes ns1:Book ;
	ns1:rangeIncludes ns1:Text ;
	rdfs:comment "The ISBN of the book." .

ns1:isicV4 a rdf:Property ;
	rdfs:label "isicV4" ;
	ns1:domainIncludes ns1:Organization , ns1:Person , ns1:Place ;
	ns1:rangeIncludes ns1:Text ;
	rdfs:comment "The International Standard of Industrial Classification of All Economic Activities (ISIC), Revision 4 code for a particular organization, business person, or place." .

ns1:issuedBy a rdf:Property ;
	rdfs:label "issuedBy" ;
	ns1:domainIncludes ns1:Permit , ns1:Ticket ;
	ns1:rangeIncludes ns1:Organization ;
	rdfs:comment "The organization issuing the ticket or permit." .

ns1:issuedThrough a rdf:Property ;
	rdfs:label "issuedThrough" ;
	ns1:domainIncludes ns1:Permit ;
	ns1:rangeIncludes ns1:Service ;
	rdfs:comment "The service through with the permit was granted." .

ns1:itemCondition a rdf:Property ;
	rdfs:label "itemCondition" ;
	ns1:domainIncludes ns1:Demand , ns1:Offer , ns1:Product ;
	ns1:rangeIncludes ns1:OfferItemCondition ;
	rdfs:comment "A predefined value from OfferItemCondition or a textual description of the condition of the product or service, or the products or services included in the offer." .

ns1:itemListElement a rdf:Property ;
	rdfs:label "itemListElement" ;
	ns1:domainIncludes ns1:ItemList ;
	ns1:rangeIncludes ns1:Text ;
	rdfs:comment "A single list item." .

ns1:itemListOrder a rdf:Property ;
	rdfs:label "itemListOrder" ;
	ns1:domainIncludes ns1:ItemList ;
	ns1:rangeIncludes ns1:Text ;
	rdfs:comment "Type of ordering (e.g. Ascending, Descending, Unordered)." .

ns1:itemOffered a rdf:Property ;
	rdfs:label "itemOffered" ;
	ns1:domainIncludes ns1:Demand , ns1:Offer ;
	ns1:rangeIncludes ns1:Product ;
	rdfs:comment "The item being offered." .

ns1:itemReviewed a rdf:Property ;
	rdfs:label "itemReviewed" ;
	ns1:domainIncludes ns1:AggregateRating , ns1:Review ;
	ns1:rangeIncludes ns1:Thing ;
	rdfs:comment "The item that is being reviewed/rated." .

ns1:itemShipped a rdf:Property ;
	rdfs:label "itemShipped" ;
	ns1:domainIncludes ns1:ParcelDelivery ;
	ns1:rangeIncludes ns1:Product ;
	rdfs:comment "Item(s) being shipped." .

ns1:jobLocation a rdf:Property ;
	rdfs:label "jobLocation" ;
	ns1:domainIncludes ns1:JobPosting ;
	ns1:rangeIncludes ns1:Place ;
	rdfs:comment "A (typically single) geographic location associated with the job position." .

ns1:jobTitle a rdf:Property ;
	rdfs:label "jobTitle" ;
	ns1:domainIncludes ns1:Person ;
	ns1:rangeIncludes ns1:Text ;
	rdfs:comment "The job title of the person (for example, Financial Manager)." .

ns1:keywords a rdf:Property ;
	rdfs:label "keywords" ;
	ns1:domainIncludes ns1:CreativeWork ;
	ns1:rangeIncludes ns1:Text ;
	rdfs:comment "Keywords or tags used to describe this content. Multiple entries in a keywords list are typically delimited by commas." .

ns1:knows a rdf:Property ;
	rdfs:label "knows" ;
	ns1:domainIncludes ns1:Person ;
	ns1:rangeIncludes ns1:Person ;
	rdfs:comment "The most generic bi-directional social/work relation." .

ns1:labelDetails a rdf:Property ;
	rdfs:label "labelDetails" ;
	ns1:domainIncludes ns1:Drug ;
	ns1:rangeIncludes ns1:URL ;
	rdfs:comment "Link to the drug's label details." .

ns1:landlord a rdf:Property ;
	rdfs:label "landlord" ;
	ns1:domainIncludes ns1:RentAction ;
	ns1:rangeIncludes ns1:Organization , ns1:Person ;
	rdfs:comment "A sub property of participant. The owner of the real estate property." ;
	rdfs:subPropertyOf ns1:participant .

ns1:language a rdf:Property ;
	rdfs:label "language" ;
	ns1:domainIncludes ns1:CommunicateAction , ns1:WriteAction ;
	ns1:rangeIncludes ns1:Language ;
	rdfs:comment "A sub property of instrument. The language used on this action." ;
	rdfs:subPropertyOf ns1:instrument .

ns1:lastReviewed a rdf:Property ;
	rdfs:label "lastReviewed" ;
	ns1:domainIncludes ns1:WebPage ;
	ns1:rangeIncludes ns1:Date ;
	rdfs:comment "Date on which the content on this web page was last reviewed for accuracy and/or completeness." .

ns1:latitude a rdf:Property ;
	rdfs:label "latitude" ;
	ns1:domainIncludes ns1:GeoCoordinates ;
	ns1:rangeIncludes ns1:Number , ns1:Text ;
	rdfs:comment "The latitude of a location. For example <code>37.42242</code>." .

ns1:learningResourceType a rdf:Property ;
	rdfs:label "learningResourceType" ;
	ns1:domainIncludes ns1:CreativeWork ;
	ns1:rangeIncludes ns1:Text ;
	rdfs:comment "The predominant type or kind characterizing the learning resource. For example, 'presentation', 'handout'." .

ns1:legalName a rdf:Property ;
	rdfs:label "legalName" ;
	ns1:domainIncludes ns1:Organization ;
	ns1:rangeIncludes ns1:Text ;
	rdfs:comment "The official name of the organization, e.g. the registered company name." .

ns1:legalStatus a rdf:Property ;
	rdfs:label "legalStatus" ;
	ns1:domainIncludes ns1:DietarySupplement , ns1:Drug ;
	ns1:rangeIncludes ns1:DrugLegalStatus ;
	rdfs:comment "The drug or supplement's legal status, including any controlled substance schedules that apply." .

ns1:lender a rdf:Property ;
	rdfs:label "lender" ;
	ns1:domainIncludes ns1:BorrowAction ;
	ns1:rangeIncludes ns1:Person ;
	rdfs:comment "A sub property of participant. The person that lends the object being borrowed." ;
	rdfs:subPropertyOf ns1:participant .

ns1:lesser a rdf:Property ;
	rdfs:label "lesser" ;
	ns1:domainIncludes ns1:QualitativeValue ;
	ns1:rangeIncludes ns1:QualitativeValue ;
	rdfs:comment "This ordering relation for qualitative values indicates that the subject is lesser than the object." .

ns1:lesserOrEqual a rdf:Property ;
	rdfs:label "lesserOrEqual" ;
	ns1:domainIncludes ns1:QualitativeValue ;
	ns1:rangeIncludes ns1:QualitativeValue ;
	rdfs:comment "This ordering relation for qualitative values indicates that the subject is lesser than or equal to the object." .

ns1:license a rdf:Property ;
	rdfs:label "license" ;
	ns1:domainIncludes ns1:CreativeWork ;
	ns1:rangeIncludes ns1:CreativeWork , ns1:URL ;
	rdfs:comment "A license document that applies to this content, typically indicated by URL." .

ns1:line a rdf:Property ;
	rdfs:label "line" ;
	ns1:domainIncludes ns1:GeoShape ;
	ns1:rangeIncludes ns1:Text ;
	rdfs:comment "A line is a point-to-point path consisting of two or more points. A line is expressed as a series of two or more point objects separated by space." .

ns1:lodgingUnitDescription a rdf:Property ;
	rdfs:label "lodgingUnitDescription" ;
	ns1:domainIncludes ns1:LodgingReservation ;
	ns1:rangeIncludes ns1:Text ;
	rdfs:comment "A full description of the lodging unit." .

ns1:lodgingUnitType a rdf:Property ;
	rdfs:label "lodgingUnitType" ;
	ns1:domainIncludes ns1:LodgingReservation ;
	ns1:rangeIncludes ns1:QualitativeValue , ns1:Text ;
	rdfs:comment "Textual description of the unit type (including suite vs. room, size of bed, etc.)." .

ns1:logo a rdf:Property ;
	rdfs:label "logo" ;
	ns1:domainIncludes ns1:Brand , ns1:Organization , ns1:Place , ns1:Product ;
	ns1:rangeIncludes ns1:ImageObject , ns1:URL ;
	rdfs:comment "A logo associated with an organization." .

ns1:longitude a rdf:Property ;
	rdfs:label "longitude" ;
	ns1:domainIncludes ns1:GeoCoordinates ;
	ns1:rangeIncludes ns1:Number , ns1:Text ;
	rdfs:comment "The longitude of a location. For example <code>-122.08585</code>." .

ns1:loser a rdf:Property ;
	rdfs:label "loser" ;
	ns1:domainIncludes ns1:WinAction ;
	ns1:rangeIncludes ns1:Person ;
	rdfs:comment "A sub property of participant. The loser of the action." ;
	rdfs:subPropertyOf ns1:participant .

ns1:lowPrice a rdf:Property ;
	rdfs:label "lowPrice" ;
	ns1:domainIncludes ns1:AggregateOffer ;
	ns1:rangeIncludes ns1:Number , ns1:Text ;
	rdfs:comment "The lowest price of all offers available." .

ns1:mainContentOfPage a rdf:Property ;
	rdfs:label "mainContentOfPage" ;
	ns1:domainIncludes ns1:WebPage ;
	ns1:rangeIncludes ns1:WebPageElement ;
	rdfs:comment "Indicates if this web page element is the main subject of the page." .

ns1:makesOffer a rdf:Property ;
	rdfs:label "makesOffer" ;
	ns1:domainIncludes ns1:Organization , ns1:Person ;
	ns1:rangeIncludes ns1:Offer ;
	rdfs:comment "A pointer to products or services offered by the organization or person." .

ns1:manufacturer a rdf:Property ;
	rdfs:label "manufacturer" ;
	ns1:domainIncludes ns1:DietarySupplement , ns1:Drug , ns1:Product ;
	ns1:rangeIncludes ns1:Organization ;
	rdfs:comment "The manufacturer of the product." .

ns1:maps a rdf:Property ;
	rdfs:label "maps" ;
	ns1:domainIncludes ns1:Place ;
	ns1:rangeIncludes ns1:URL ;
	ns1:supercededBy ns1:map ;
	rdfs:comment "A URL to a map of the place (legacy spelling; see singular form, map)." .

ns1:maxPrice a rdf:Property ;
	rdfs:label "maxPrice" ;
	ns1:domainIncludes ns1:PriceSpecification ;
	ns1:rangeIncludes ns1:Number ;
	rdfs:comment "The highest price if the price is a range." .

ns1:maxValue a rdf:Property ;
	rdfs:label "maxValue" ;
	ns1:domainIncludes ns1:PropertyValueSpecification , ns1:QuantitativeValue ;
	ns1:rangeIncludes ns1:Number ;
	rdfs:comment "The upper value of some characteristic or property." .

ns1:maximumIntake a rdf:Property ;
	rdfs:label "maximumIntake" ;
	ns1:domainIncludes ns1:DietarySupplement ;
	ns1:rangeIncludes ns1:MaximumDoseSchedule ;
	rdfs:comment "Recommended intake of this supplement for a given population as defined by a specific recommending authority." .

ns1:mealService a rdf:Property ;
	rdfs:label "mealService" ;
	ns1:domainIncludes ns1:Flight ;
	ns1:rangeIncludes ns1:Text ;
	rdfs:comment "Description of the meals that will be provided or available for purchase." .

ns1:mechanismOfAction a rdf:Property ;
	rdfs:label "mechanismOfAction" ;
	ns1:domainIncludes ns1:DietarySupplement , ns1:Drug ;
	ns1:rangeIncludes ns1:Text ;
	rdfs:comment "The specific biochemical interaction through which this drug or supplement produces its pharmacological effect." .

ns1:medicalSpecialty a rdf:Property ;
	rdfs:label "medicalSpecialty" ;
	ns1:domainIncludes ns1:Hospital , ns1:MedicalClinic , ns1:Physician ;
	ns1:rangeIncludes ns1:MedicalSpecialty ;
	rdfs:comment "A medical specialty of the provider." .

ns1:medicineSystem a rdf:Property ;
	rdfs:label "medicineSystem" ;
	ns1:domainIncludes ns1:MedicalEntity ;
	ns1:rangeIncludes ns1:MedicineSystem ;
	rdfs:comment "The system of medicine that includes this MedicalEntity, for example 'evidence-based', 'homeopathic', 'chiropractic', etc." .

ns1:members a rdf:Property ;
	rdfs:label "members" ;
	ns1:domainIncludes ns1:Organization , ns1:ProgramMembership ;
	ns1:rangeIncludes ns1:Organization , ns1:Person ;
	ns1:supercededBy ns1:member ;
	rdfs:comment "A member of this organization (legacy spelling; see singular form, member)." .

ns1:membershipNumber a rdf:Property ;
	rdfs:label "membershipNumber" ;
	ns1:domainIncludes ns1:ProgramMembership ;
	ns1:rangeIncludes ns1:Text ;
	rdfs:comment "A unique identifier for the membership." .

ns1:memoryRequirements a rdf:Property ;
	rdfs:label "memoryRequirements" ;
	ns1:domainIncludes ns1:SoftwareApplication ;
	ns1:rangeIncludes ns1:Text , ns1:URL ;
	rdfs:comment "Minimum memory requirements." .

ns1:mentions a rdf:Property ;
	rdfs:label "mentions" ;
	ns1:domainIncludes ns1:CreativeWork ;
	ns1:rangeIncludes ns1:Thing ;
	rdfs:comment "Indicates that the CreativeWork contains a reference to, but is not necessarily about a concept." .

ns1:menu a rdf:Property ;
	rdfs:label "menu" ;
	ns1:domainIncludes ns1:FoodEstablishment ;
	ns1:rangeIncludes ns1:Text , ns1:URL ;
	rdfs:comment "Either the actual menu or a URL of the menu." .

ns1:merchant a rdf:Property ;
	rdfs:label "merchant" ;
	ns1:domainIncludes ns1:Order ;
	ns1:rangeIncludes ns1:Organization , ns1:Person ;
	rdfs:comment "The party taking the order (e.g. Amazon.com is a merchant for many sellers)." .

ns1:minPrice a rdf:Property ;
	rdfs:label "minPrice" ;
	ns1:domainIncludes ns1:PriceSpecification ;
	ns1:rangeIncludes ns1:Number ;
	rdfs:comment "The lowest price if the price is a range." .

ns1:minValue a rdf:Property ;
	rdfs:label "minValue" ;
	ns1:domainIncludes ns1:PropertyValueSpecification , ns1:QuantitativeValue ;
	ns1:rangeIncludes ns1:Number ;
	rdfs:comment "The lower value of some characteristic or property." .

ns1:model a rdf:Property ;
	rdfs:label "model" ;
	ns1:domainIncludes ns1:Product ;
	ns1:rangeIncludes ns1:ProductModel , ns1:Text ;
	rdfs:comment "The model of the product. Use with the URL of a ProductModel or a textual representation of the model identifier. The URL of the ProductModel can be from an external source. It is recommended to additionally provide strong product identifiers via the gtin8/gtin13/gtin14 and mpn properties." .

ns1:modifiedTime a rdf:Property ;
	rdfs:label "modifiedTime" ;
	ns1:domainIncludes ns1:Reservation ;
	ns1:rangeIncludes ns1:DateTime ;
	rdfs:comment "The date and time the reservation was modified." .

ns1:mpn a rdf:Property ;
	rdfs:label "mpn" ;
	ns1:domainIncludes ns1:Demand , ns1:Offer , ns1:Product ;
	ns1:rangeIncludes ns1:Text ;
	rdfs:comment "The Manufacturer Part Number (MPN) of the product, or the product to which the offer refers." .

ns1:multipleValues a rdf:Property ;
	rdfs:label "multipleValues" ;
	ns1:domainIncludes ns1:PropertyValueSpecification ;
	ns1:rangeIncludes ns1:Boolean ;
	rdfs:comment "Whether multiple values are allowed for the property.  Default is false." .

ns1:musicBy a rdf:Property ;
	rdfs:label "musicBy" ;
	ns1:domainIncludes ns1:Episode , ns1:Movie , ns1:RadioEpisode , ns1:RadioSeries , ns1:Series , ns1:TVEpisode , ns1:TVSeries ;
	ns1:rangeIncludes ns1:MusicGroup , ns1:Person ;
	rdfs:comment "The composer of the movie or TV/radio soundtrack." .

ns1:musicGroupMember a rdf:Property ;
	rdfs:label "musicGroupMember" ;
	ns1:domainIncludes ns1:MusicGroup ;
	ns1:rangeIncludes ns1:Person ;
	ns1:supercededBy ns1:member ;
	rdfs:comment "A member of a music group&#x2014;for example, John, Paul, George, or Ringo." .

ns1:naics a rdf:Property ;
	rdfs:label "naics" ;
	ns1:domainIncludes ns1:Organization , ns1:Person ;
	ns1:rangeIncludes ns1:Text ;
	rdfs:comment "The North American Industry Classification System (NAICS) code for a particular organization or business person." .

ns1:name a rdf:Property ;
	rdfs:label "name" ;
	ns1:domainIncludes ns1:Thing ;
	ns1:rangeIncludes ns1:Text ;
	rdfs:comment "The name of the item." .

ns1:namedPosition a rdf:Property ;
	rdfs:label "namedPosition" ;
	ns1:domainIncludes ns1:OrganizationRole ;
	ns1:rangeIncludes ns1:Text , ns1:URL ;
	rdfs:comment "A position played, performed or filled by a person or organization, as part of an organization. For example, an athlete in a SportsTeam might play in the position named 'Quarterback'." .

ns1:nationality a rdf:Property ;
	rdfs:label "nationality" ;
	ns1:domainIncludes ns1:Person ;
	ns1:rangeIncludes ns1:Country ;
	rdfs:comment "Nationality of the person." .

ns1:naturalProgression a rdf:Property ;
	rdfs:label "naturalProgression" ;
	ns1:domainIncludes ns1:MedicalCondition ;
	ns1:rangeIncludes ns1:Text ;
	rdfs:comment "The expected progression of the condition if it is not treated and allowed to progress naturally." .

ns1:nerve a rdf:Property ;
	rdfs:label "nerve" ;
	ns1:domainIncludes ns1:Muscle ;
	ns1:rangeIncludes ns1:Nerve ;
	rdfs:comment "The underlying innervation associated with the muscle." .

ns1:nerveMotor a rdf:Property ;
	rdfs:label "nerveMotor" ;
	ns1:domainIncludes ns1:Nerve ;
	ns1:rangeIncludes ns1:Muscle ;
	rdfs:comment "The neurological pathway extension that involves muscle control." .

ns1:nonEqual a rdf:Property ;
	rdfs:label "nonEqual" ;
	ns1:domainIncludes ns1:QualitativeValue ;
	ns1:rangeIncludes ns1:QualitativeValue ;
	rdfs:comment "This ordering relation for qualitative values indicates that the subject is not equal to the object." .

ns1:nonProprietaryName a rdf:Property ;
	rdfs:label "nonProprietaryName" ;
	ns1:domainIncludes ns1:DietarySupplement , ns1:Drug ;
	ns1:rangeIncludes ns1:Text ;
	rdfs:comment "The generic name of this drug or supplement." .

ns1:normalRange a rdf:Property ;
	rdfs:label "normalRange" ;
	ns1:domainIncludes ns1:MedicalTest ;
	ns1:rangeIncludes ns1:Text ;
	rdfs:comment "Range of acceptable values for a typical patient, when applicable." .

ns1:numAdults a rdf:Property ;
	rdfs:label "numAdults" ;
	ns1:domainIncludes ns1:LodgingReservation ;
	ns1:rangeIncludes ns1:Number , ns1:QuantitativeValue ;
	rdfs:comment "The number of adults staying in the unit." .

ns1:numChildren a rdf:Property ;
	rdfs:label "numChildren" ;
	ns1:domainIncludes ns1:LodgingReservation ;
	ns1:rangeIncludes ns1:Number , ns1:QuantitativeValue ;
	rdfs:comment "The number of children staying in the unit." .

ns1:numTracks a rdf:Property ;
	rdfs:label "numTracks" ;
	ns1:domainIncludes ns1:MusicPlaylist ;
	ns1:rangeIncludes ns1:Integer ;
	rdfs:comment "The number of tracks in this album or playlist." .

ns1:numberOfEpisodes a rdf:Property ;
	rdfs:label "numberOfEpisodes" ;
	ns1:domainIncludes ns1:RadioSeason , ns1:RadioSeries , ns1:Season , ns1:Series , ns1:TVSeason , ns1:TVSeries ;
	ns1:rangeIncludes ns1:Number ;
	rdfs:comment "The number of episodes in this season or series." .

ns1:numberOfPages a rdf:Property ;
	rdfs:label "numberOfPages" ;
	ns1:domainIncludes ns1:Book ;
	ns1:rangeIncludes ns1:Integer ;
	rdfs:comment "The number of pages in the book." .

ns1:numberOfSeasons a rdf:Property ;
	rdfs:label "numberOfSeasons" ;
	ns1:domainIncludes ns1:Series ;
	ns1:rangeIncludes ns1:Number ;
	rdfs:comment "The number of seasons in this series." .

ns1:numberofEmployees a rdf:Property ;
	rdfs:label "numberofEmployees" ;
	ns1:domainIncludes ns1:BusinessAudience ;
	ns1:rangeIncludes ns1:QuantitativeValue ;
	rdfs:comment "The size of business by number of employees." .

ns1:nutrition a rdf:Property ;
	rdfs:label "nutrition" ;
	ns1:domainIncludes ns1:Recipe ;
	ns1:rangeIncludes ns1:NutritionInformation ;
	rdfs:comment "Nutrition information about the recipe." .

ns1:occupationalCategory a rdf:Property ;
	rdfs:label "occupationalCategory" ;
	ns1:domainIncludes ns1:JobPosting ;
	ns1:rangeIncludes ns1:Text ;
	rdfs:comment "Category or categories describing the job. Use BLS O*NET-SOC taxonomy: http://www.onetcenter.org/taxonomy.html. Ideally includes textual label and formal code, with the property repeated for each applicable value." .

ns1:offerCount a rdf:Property ;
	rdfs:label "offerCount" ;
	ns1:domainIncludes ns1:AggregateOffer ;
	ns1:rangeIncludes ns1:Integer ;
	rdfs:comment "The number of offers for the product." .

ns1:offers a rdf:Property ;
	rdfs:label "offers" ;
	ns1:domainIncludes ns1:CreativeWork , ns1:Event , ns1:MediaObject , ns1:Product ;
	ns1:rangeIncludes ns1:Offer ;
	rdfs:comment "An offer to provide this item&#x2014;for example, an offer to sell a product, rent the DVD of a movie, or give away tickets to an event." .

ns1:openingHours a rdf:Property ;
	rdfs:label "openingHours" ;
	ns1:domainIncludes ns1:CivicStructure , ns1:LocalBusiness ;
	ns1:rangeIncludes ns1:Duration ;
	rdfs:comment "The opening hours for a business. Opening hours can be specified as a weekly time range, starting with days, then times per day. Multiple days can be listed with commas ',' separating each day. Day or time ranges are specified using a hyphen '-'.<br />- Days are specified using the following two-letter combinations: <code>Mo</code>, <code>Tu</code>, <code>We</code>, <code>Th</code>, <code>Fr</code>, <code>Sa</code>, <code>Su</code>.<br />- Times are specified using 24:00 time. For example, 3pm is specified as <code>15:00</code>. <br />- Here is an example: <code>&lt;time itemprop=&quot;openingHours&quot; datetime=&quot;Tu,Th 16:00-20:00&quot;&gt;Tuesdays and Thursdays 4-8pm&lt;/time&gt;</code>. <br />- If a business is open 7 days a week, then it can be specified as <code>&lt;time itemprop=&quot;openingHours&quot; datetime=&quot;Mo-Su&quot;&gt;Monday through Sunday, all day&lt;/time&gt;</code>." .

ns1:openingHoursSpecification a rdf:Property ;
	rdfs:label "openingHoursSpecification" ;
	ns1:domainIncludes ns1:Place ;
	ns1:rangeIncludes ns1:OpeningHoursSpecification ;
	rdfs:comment "The opening hours of a certain place." .

ns1:opens a rdf:Property ;
	rdfs:label "opens" ;
	ns1:domainIncludes ns1:OpeningHoursSpecification ;
	ns1:rangeIncludes ns1:Time ;
	rdfs:comment "The opening hour of the place or service on the given day(s) of the week." .

ns1:operatingSystem a rdf:Property ;
	rdfs:label "operatingSystem" ;
	ns1:domainIncludes ns1:SoftwareApplication ;
	ns1:rangeIncludes ns1:Text ;
	rdfs:comment "Operating systems supported (Windows 7, OSX 10.6, Android 1.6)." .

ns1:opponent a rdf:Property ;
	rdfs:label "opponent" ;
	ns1:domainIncludes ns1:ExerciseAction ;
	ns1:rangeIncludes ns1:Person ;
	rdfs:comment "A sub property of participant. The opponent on this action." ;
	rdfs:subPropertyOf ns1:participant .

ns1:option a rdf:Property ;
	rdfs:label "option" ;
	ns1:domainIncludes ns1:ChooseAction ;
	ns1:rangeIncludes ns1:Text , ns1:Thing ;
	rdfs:comment "A sub property of object. The options subject to this action." ;
	rdfs:subPropertyOf ns1:object .

ns1:orderDate a rdf:Property ;
	rdfs:label "orderDate" ;
	ns1:domainIncludes ns1:Order ;
	ns1:rangeIncludes ns1:DateTime ;
	rdfs:comment "Date order was placed." .

ns1:orderNumber a rdf:Property ;
	rdfs:label "orderNumber" ;
	ns1:domainIncludes ns1:Order ;
	ns1:rangeIncludes ns1:Text ;
	rdfs:comment "The identifier of the transaction." .

ns1:orderStatus a rdf:Property ;
	rdfs:label "orderStatus" ;
	ns1:domainIncludes ns1:Order ;
	ns1:rangeIncludes ns1:OrderStatus ;
	rdfs:comment "The current status of the order." .

ns1:orderedItem a rdf:Property ;
	rdfs:label "orderedItem" ;
	ns1:domainIncludes ns1:Order ;
	ns1:rangeIncludes ns1:Product ;
	rdfs:comment "The item ordered." .

ns1:origin a rdf:Property ;
	rdfs:label "origin" ;
	ns1:domainIncludes ns1:Muscle ;
	ns1:rangeIncludes ns1:AnatomicalStructure ;
	rdfs:comment "The place or point where a muscle arises." .

ns1:originAddress a rdf:Property ;
	rdfs:label "originAddress" ;
	ns1:domainIncludes ns1:ParcelDelivery ;
	ns1:rangeIncludes ns1:PostalAddress ;
	rdfs:comment "Shipper's address." .

ns1:originatesFrom a rdf:Property ;
	rdfs:label "originatesFrom" ;
	ns1:domainIncludes ns1:LymphaticVessel ;
	ns1:rangeIncludes ns1:Vessel ;
	rdfs:comment "The vasculature the lymphatic structure originates, or afferents, from." .

ns1:outcome a rdf:Property ;
	rdfs:label "outcome" ;
	ns1:domainIncludes ns1:MedicalStudy ;
	ns1:rangeIncludes ns1:Text ;
	rdfs:comment "Expected or actual outcomes of the study." .

ns1:overdosage a rdf:Property ;
	rdfs:label "overdosage" ;
	ns1:domainIncludes ns1:Drug ;
	ns1:rangeIncludes ns1:Text ;
	rdfs:comment "Any information related to overdose on a drug, including signs or symptoms, treatments, contact information for emergency response." .

ns1:overview a rdf:Property ;
	rdfs:label "overview" ;
	ns1:domainIncludes ns1:Diet ;
	ns1:rangeIncludes ns1:Text ;
	rdfs:comment "Descriptive information establishing the overarching theory/philosophy of the plan. May include the rationale for the name, the population where the plan first came to prominence, etc." .

ns1:ownedFrom a rdf:Property ;
	rdfs:label "ownedFrom" ;
	ns1:domainIncludes ns1:OwnershipInfo ;
	ns1:rangeIncludes ns1:DateTime ;
	rdfs:comment "The date and time of obtaining the product." .

ns1:ownedThrough a rdf:Property ;
	rdfs:label "ownedThrough" ;
	ns1:domainIncludes ns1:OwnershipInfo ;
	ns1:rangeIncludes ns1:DateTime ;
	rdfs:comment "The date and time of giving up ownership on the product." .

ns1:owns a rdf:Property ;
	rdfs:label "owns" ;
	ns1:domainIncludes ns1:Organization , ns1:Person ;
	ns1:rangeIncludes ns1:OwnershipInfo , ns1:Product ;
	rdfs:comment "Products owned by the organization or person." .

ns1:parentItem a rdf:Property ;
	rdfs:label "parentItem" ;
	ns1:domainIncludes ns1:Answer , ns1:Comment ;
	ns1:rangeIncludes ns1:Question ;
	rdfs:comment "The parent of a question, answer or item in general." .

ns1:parentService a rdf:Property ;
	rdfs:label "parentService" ;
	ns1:domainIncludes ns1:BroadcastService ;
	ns1:rangeIncludes ns1:BroadcastService ;
	rdfs:comment "A broadcast service to which the broadcast service may belong to such as regional variations of a national channel." .

ns1:parents a rdf:Property ;
	rdfs:label "parents" ;
	ns1:domainIncludes ns1:Person ;
	ns1:rangeIncludes ns1:Person ;
	ns1:supercededBy ns1:parent ;
	rdfs:comment "A parents of the person (legacy spelling; see singular form, parent)." .

ns1:partOfEpisode a rdf:Property ;
	rdfs:label "partOfEpisode" ;
	ns1:domainIncludes ns1:Clip ;
	ns1:rangeIncludes ns1:Episode ;
	rdfs:comment "The episode to which this clip belongs." .

ns1:partOfOrder a rdf:Property ;
	rdfs:label "partOfOrder" ;
	ns1:domainIncludes ns1:ParcelDelivery ;
	ns1:rangeIncludes ns1:Order ;
	rdfs:comment "The overall order the items in this delivery were included in." .

ns1:partOfSeason a rdf:Property ;
	rdfs:label "partOfSeason" ;
	ns1:domainIncludes ns1:Clip , ns1:Episode , ns1:RadioClip , ns1:RadioEpisode , ns1:TVClip , ns1:TVEpisode ;
	ns1:rangeIncludes ns1:Season ;
	rdfs:comment "The season to which this episode belongs." .

ns1:partOfSystem a rdf:Property ;
	rdfs:label "partOfSystem" ;
	ns1:domainIncludes ns1:AnatomicalStructure ;
	ns1:rangeIncludes ns1:AnatomicalSystem ;
	rdfs:comment "The anatomical or organ system that this structure is part of." .

ns1:partOfTVSeries a rdf:Property ;
	rdfs:label "partOfTVSeries" ;
	ns1:domainIncludes ns1:TVClip , ns1:TVEpisode , ns1:TVSeason ;
	ns1:rangeIncludes ns1:TVSeries ;
	ns1:supercededBy ns1:partOfSeries ;
	rdfs:comment "The TV series to which this episode or season belongs. (legacy form; partOfSeries is preferred)" .

ns1:partySize a rdf:Property ;
	rdfs:label "partySize" ;
	ns1:domainIncludes ns1:FoodEstablishmentReservation , ns1:TaxiReservation ;
	ns1:rangeIncludes ns1:Number , ns1:QuantitativeValue ;
	rdfs:comment "Number of people the reservation should accommodate." .

ns1:pathophysiology a rdf:Property ;
	rdfs:label "pathophysiology" ;
	ns1:domainIncludes ns1:MedicalCondition , ns1:PhysicalActivity ;
	ns1:rangeIncludes ns1:Text ;
	rdfs:comment "Changes in the normal mechanical, physical, and biochemical functions that are associated with this activity or condition." .

ns1:paymentAccepted a rdf:Property ;
	rdfs:label "paymentAccepted" ;
	ns1:domainIncludes ns1:LocalBusiness ;
	ns1:rangeIncludes ns1:Text ;
	rdfs:comment "Cash, credit card, etc." .

ns1:paymentDue a rdf:Property ;
	rdfs:label "paymentDue" ;
	ns1:domainIncludes ns1:Order ;
	ns1:rangeIncludes ns1:DateTime ;
	rdfs:comment "The date that payment is due." .

ns1:paymentMethod a rdf:Property ;
	rdfs:label "paymentMethod" ;
	ns1:domainIncludes ns1:Order ;
	ns1:rangeIncludes ns1:PaymentMethod ;
	rdfs:comment "The name of the credit card or other method of payment for the order." .

ns1:paymentMethodId a rdf:Property ;
	rdfs:label "paymentMethodId" ;
	ns1:domainIncludes ns1:Order ;
	ns1:rangeIncludes ns1:Text ;
	rdfs:comment "An identifier for the method of payment used (e.g. the last 4 digits of the credit card)." .

ns1:paymentUrl a rdf:Property ;
	rdfs:label "paymentUrl" ;
	ns1:domainIncludes ns1:Order ;
	ns1:rangeIncludes ns1:URL ;
	rdfs:comment "The URL for sending a payment." .

ns1:performerIn a rdf:Property ;
	rdfs:label "performerIn" ;
	ns1:domainIncludes ns1:Person ;
	ns1:rangeIncludes ns1:Event ;
	rdfs:comment "Event that this person is a performer or participant in." .

ns1:performers a rdf:Property ;
	rdfs:label "performers" ;
	ns1:domainIncludes ns1:Event ;
	ns1:rangeIncludes ns1:Organization , ns1:Person ;
	ns1:supercededBy ns1:performer ;
	rdfs:comment "The main performer or performers of the event&#x2014;for example, a presenter, musician, or actor (legacy spelling; see singular form, performer)." .

ns1:permissions a rdf:Property ;
	rdfs:label "permissions" ;
	ns1:domainIncludes ns1:SoftwareApplication ;
	ns1:rangeIncludes ns1:Text ;
	rdfs:comment "Permission(s) required to run the app (for example, a mobile app may require full internet access or may run only on wifi)." .

ns1:permitAudience a rdf:Property ;
	rdfs:label "permitAudience" ;
	ns1:domainIncludes ns1:Permit ;
	ns1:rangeIncludes ns1:Audience ;
	rdfs:comment "The target audience for this permit." .

ns1:phase a rdf:Property ;
	rdfs:label "phase" ;
	ns1:domainIncludes ns1:MedicalTrial ;
	ns1:rangeIncludes ns1:Text ;
	rdfs:comment "The phase of the trial." .

ns1:photos a rdf:Property ;
	rdfs:label "photos" ;
	ns1:domainIncludes ns1:Place ;
	ns1:rangeIncludes ns1:ImageObject , ns1:Photograph ;
	ns1:supercededBy ns1:photo ;
	rdfs:comment "Photographs of this place (legacy spelling; see singular form, photo)." .

ns1:physiologicalBenefits a rdf:Property ;
	rdfs:label "physiologicalBenefits" ;
	ns1:domainIncludes ns1:Diet ;
	ns1:rangeIncludes ns1:Text ;
	rdfs:comment "Specific physiologic benefits associated to the plan." .

ns1:pickupLocation a rdf:Property ;
	rdfs:label "pickupLocation" ;
	ns1:domainIncludes ns1:RentalCarReservation , ns1:TaxiReservation ;
	ns1:rangeIncludes ns1:Place ;
	rdfs:comment "Where a taxi will pick up a passenger or a rental car can be picked up." .

ns1:pickupTime a rdf:Property ;
	rdfs:label "pickupTime" ;
	ns1:domainIncludes ns1:RentalCarReservation , ns1:TaxiReservation ;
	ns1:rangeIncludes ns1:DateTime ;
	rdfs:comment "When a taxi will pickup a passenger or a rental car can be picked up." .

ns1:playerType a rdf:Property ;
	rdfs:label "playerType" ;
	ns1:domainIncludes ns1:MediaObject ;
	ns1:rangeIncludes ns1:Text ;
	rdfs:comment "Player type required&#x2014;for example, Flash or Silverlight." .

ns1:polygon a rdf:Property ;
	rdfs:label "polygon" ;
	ns1:domainIncludes ns1:GeoShape ;
	ns1:rangeIncludes ns1:Text ;
	rdfs:comment "A polygon is the area enclosed by a point-to-point path for which the starting and ending points are the same. A polygon is expressed as a series of four or more space delimited points where the first and final points are identical." .

ns1:population a rdf:Property ;
	rdfs:label "population" ;
	ns1:domainIncludes ns1:MedicalStudy ;
	ns1:rangeIncludes ns1:Text ;
	rdfs:comment "Any characteristics of the population used in the study, e.g. 'males under 65'." .

ns1:position a rdf:Property ;
	rdfs:label "position" ;
	ns1:domainIncludes ns1:Clip , ns1:Episode , ns1:Season ;
	ns1:rangeIncludes ns1:Text ;
	rdfs:comment "Free text to define other than pure numerical ranking of an episode or a season in an ordered list of items (further formatting restrictions may apply within particular user groups)." .

ns1:possibleComplication a rdf:Property ;
	rdfs:label "possibleComplication" ;
	ns1:domainIncludes ns1:MedicalCondition ;
	ns1:rangeIncludes ns1:Text ;
	rdfs:comment "A possible unexpected and unfavorable evolution of a medical condition. Complications may include worsening of the signs or symptoms of the disease, extension of the condition to other organ systems, etc." .

ns1:possibleTreatment a rdf:Property ;
	rdfs:label "possibleTreatment" ;
	ns1:domainIncludes ns1:MedicalCondition , ns1:MedicalSignOrSymptom ;
	ns1:rangeIncludes ns1:MedicalTherapy ;
	rdfs:comment "A possible treatment to address this condition, sign or symptom." .

ns1:postOfficeBoxNumber a rdf:Property ;
	rdfs:label "postOfficeBoxNumber" ;
	ns1:domainIncludes ns1:PostalAddress ;
	ns1:rangeIncludes ns1:Text ;
	rdfs:comment "The post office box number for PO box addresses." .

ns1:postOp a rdf:Property ;
	rdfs:label "postOp" ;
	ns1:domainIncludes ns1:MedicalDevice ;
	ns1:rangeIncludes ns1:Text ;
	rdfs:comment "A description of the postoperative procedures, care, and/or followups for this device." .

ns1:postalCode a rdf:Property ;
	rdfs:label "postalCode" ;
	ns1:domainIncludes ns1:PostalAddress ;
	ns1:rangeIncludes ns1:Text ;
	rdfs:comment "The postal code. For example, 94043." .

ns1:potentialAction a rdf:Property ;
	rdfs:label "potentialAction" ;
	ns1:domainIncludes ns1:Thing ;
	ns1:rangeIncludes ns1:Action ;
	rdfs:comment "Indicates a potential Action, which describes an idealized action in which this thing would play an 'object' role." .

ns1:preOp a rdf:Property ;
	rdfs:label "preOp" ;
	ns1:domainIncludes ns1:MedicalDevice ;
	ns1:rangeIncludes ns1:Text ;
	rdfs:comment "A description of the workup, testing, and other preparations required before implanting this device." .

ns1:predecessorOf a rdf:Property ;
	rdfs:label "predecessorOf" ;
	ns1:domainIncludes ns1:ProductModel ;
	ns1:rangeIncludes ns1:ProductModel ;
	rdfs:comment "A pointer from a previous, often discontinued variant of the product to its newer variant." .

ns1:pregnancyCategory a rdf:Property ;
	rdfs:label "pregnancyCategory" ;
	ns1:domainIncludes ns1:Drug ;
	ns1:rangeIncludes ns1:DrugPregnancyCategory ;
	rdfs:comment "Pregnancy category of this drug." .

ns1:pregnancyWarning a rdf:Property ;
	rdfs:label "pregnancyWarning" ;
	ns1:domainIncludes ns1:Drug ;
	ns1:rangeIncludes ns1:Text ;
	rdfs:comment "Any precaution, guidance, contraindication, etc. related to this drug's use during pregnancy." .

ns1:prepTime a rdf:Property ;
	rdfs:label "prepTime" ;
	ns1:domainIncludes ns1:Recipe ;
	ns1:rangeIncludes ns1:Duration ;
	rdfs:comment "The length of time it takes to prepare the recipe, in <a href='http://en.wikipedia.org/wiki/ISO_8601'>ISO 8601 duration format</a>." .

ns1:preparation a rdf:Property ;
	rdfs:label "preparation" ;
	ns1:domainIncludes ns1:MedicalProcedure ;
	ns1:rangeIncludes ns1:Text ;
	rdfs:comment "Typical preparation that a patient must undergo before having the procedure performed." .

ns1:prescribingInfo a rdf:Property ;
	rdfs:label "prescribingInfo" ;
	ns1:domainIncludes ns1:Drug ;
	ns1:rangeIncludes ns1:URL ;
	rdfs:comment "Link to prescribing information for the drug." .

ns1:prescriptionStatus a rdf:Property ;
	rdfs:label "prescriptionStatus" ;
	ns1:domainIncludes ns1:Drug ;
	ns1:rangeIncludes ns1:DrugPrescriptionStatus ;
	rdfs:comment "Indicates whether this drug is available by prescription or over-the-counter." .

ns1:previousStartDate a rdf:Property ;
	rdfs:label "previousStartDate" ;
	ns1:domainIncludes ns1:Event ;
	ns1:rangeIncludes ns1:Date ;
	rdfs:comment "Used in conjunction with eventStatus for rescheduled or cancelled events. This property contains the previously scheduled start date. For rescheduled events, the startDate property should be used for the newly scheduled start date. In the (rare) case of an event that has been postponed and rescheduled multiple times, this field may be repeated." .

ns1:price a rdf:Property ;
	rdfs:label "price" ;
	ns1:domainIncludes ns1:Offer , ns1:PriceSpecification , ns1:TradeAction ;
	ns1:rangeIncludes ns1:Number , ns1:Text ;
	rdfs:comment "The offer price of a product, or of a price component when attached to PriceSpecification and its subtypes." .

ns1:priceCurrency a rdf:Property ;
	rdfs:label "priceCurrency" ;
	ns1:domainIncludes ns1:Offer , ns1:PriceSpecification , ns1:Reservation , ns1:Ticket ;
	ns1:rangeIncludes ns1:Text ;
	rdfs:comment "The currency (in 3-letter ISO 4217 format) of the price or a price component, when attached to PriceSpecification and its subtypes." .

ns1:priceRange a rdf:Property ;
	rdfs:label "priceRange" ;
	ns1:domainIncludes ns1:LocalBusiness ;
	ns1:rangeIncludes ns1:Text ;
	rdfs:comment "The price range of the business, for example <code>$$$</code>." .

ns1:priceSpecification a rdf:Property ;
	rdfs:label "priceSpecification" ;
	ns1:domainIncludes ns1:Demand , ns1:Offer ;
	ns1:rangeIncludes ns1:PriceSpecification ;
	rdfs:comment "One or more detailed price specifications, indicating the unit price and delivery or payment charges." .

ns1:priceType a rdf:Property ;
	rdfs:label "priceType" ;
	ns1:domainIncludes ns1:UnitPriceSpecification ;
	ns1:rangeIncludes ns1:Text ;
	rdfs:comment "A short text or acronym indicating multiple price specifications for the same offer, e.g. SRP for the suggested retail price or INVOICE for the invoice price, mostly used in the car industry." .

ns1:priceValidUntil a rdf:Property ;
	rdfs:label "priceValidUntil" ;
	ns1:domainIncludes ns1:Offer ;
	ns1:rangeIncludes ns1:Date ;
	rdfs:comment "The date after which the price is no longer available." .

ns1:primaryImageOfPage a rdf:Property ;
	rdfs:label "primaryImageOfPage" ;
	ns1:domainIncludes ns1:WebPage ;
	ns1:rangeIncludes ns1:ImageObject ;
	rdfs:comment "Indicates the main image on the page." .

ns1:primaryPrevention a rdf:Property ;
	rdfs:label "primaryPrevention" ;
	ns1:domainIncludes ns1:MedicalCondition ;
	ns1:rangeIncludes ns1:MedicalTherapy ;
	rdfs:comment "A preventative therapy used to prevent an initial occurrence of the medical condition, such as vaccination." .

ns1:printColumn a rdf:Property ;
	rdfs:label "printColumn" ;
	ns1:domainIncludes ns1:NewsArticle ;
	ns1:rangeIncludes ns1:Text ;
	rdfs:comment "The number of the column in which the NewsArticle appears in the print edition." .

ns1:printEdition a rdf:Property ;
	rdfs:label "printEdition" ;
	ns1:domainIncludes ns1:NewsArticle ;
	ns1:rangeIncludes ns1:Text ;
	rdfs:comment "The edition of the print product in which the NewsArticle appears." .

ns1:printPage a rdf:Property ;
	rdfs:label "printPage" ;
	ns1:domainIncludes ns1:NewsArticle ;
	ns1:rangeIncludes ns1:Text ;
	rdfs:comment "If this NewsArticle appears in print, this field indicates the name of the page on which the article is found. Please note that this field is intended for the exact page name (e.g. A5, B18)." .

ns1:printSection a rdf:Property ;
	rdfs:label "printSection" ;
	ns1:domainIncludes ns1:NewsArticle ;
	ns1:rangeIncludes ns1:Text ;
	rdfs:comment "If this NewsArticle appears in print, this field indicates the print section in which the article appeared." .

ns1:procedure a rdf:Property ;
	rdfs:label "procedure" ;
	ns1:domainIncludes ns1:MedicalDevice ;
	ns1:rangeIncludes ns1:Text ;
	rdfs:comment "A description of the procedure involved in setting up, using, and/or installing the device." .

ns1:procedureType a rdf:Property ;
	rdfs:label "procedureType" ;
	ns1:domainIncludes ns1:MedicalProcedure ;
	ns1:rangeIncludes ns1:MedicalProcedureType ;
	rdfs:comment "The type of procedure, for example Surgical, Noninvasive, or Percutaneous." .

ns1:processingTime a rdf:Property ;
	rdfs:label "processingTime" ;
	ns1:domainIncludes ns1:ServiceChannel ;
	ns1:rangeIncludes ns1:Duration ;
	rdfs:comment "Estimated processing time for the service using this channel." .

ns1:processorRequirements a rdf:Property ;
	rdfs:label "processorRequirements" ;
	ns1:domainIncludes ns1:SoftwareApplication ;
	ns1:rangeIncludes ns1:Text ;
	rdfs:comment "Processor architecture required to run the application (e.g. IA64)." .

ns1:producer a rdf:Property ;
	rdfs:label "producer" ;
	ns1:domainIncludes ns1:Episode , ns1:Movie , ns1:RadioEpisode , ns1:RadioSeries , ns1:Season , ns1:Series , ns1:TVEpisode , ns1:TVSeries ;
	ns1:rangeIncludes ns1:Person ;
	rdfs:comment "The producer of the movie, tv/radio series, season, or episode, or video." .

ns1:produces a rdf:Property ;
	rdfs:label "produces" ;
	ns1:domainIncludes ns1:Service ;
	ns1:rangeIncludes ns1:Thing ;
	rdfs:comment "The tangible thing generated by the service, e.g. a passport, permit, etc." .

ns1:productID a rdf:Property ;
	rdfs:label "productID" ;
	ns1:domainIncludes ns1:Product ;
	ns1:rangeIncludes ns1:Text ;
	rdfs:comment "The product identifier, such as ISBN. For example: <code>&lt;meta itemprop='productID' content='isbn:123-456-789'/&gt;</code>." .

ns1:productSupported a rdf:Property ;
	rdfs:label "productSupported" ;
	ns1:domainIncludes ns1:ContactPoint ;
	ns1:rangeIncludes ns1:Product , ns1:Text ;
	rdfs:comment "The product or service this support contact point is related to (such as product support for a particular product line). This can be a specific product or product line (e.g. \"iPhone\") or a general category of products or services (e.g. \"smartphones\")." .

ns1:productionCompany a rdf:Property ;
	rdfs:label "productionCompany" ;
	ns1:domainIncludes ns1:Episode , ns1:MediaObject , ns1:Movie , ns1:RadioEpisode , ns1:RadioSeries , ns1:Season , ns1:Series , ns1:TVEpisode , ns1:TVSeries , ns1:VideoObject ;
	ns1:rangeIncludes ns1:Organization ;
	rdfs:comment "The production company or studio that made the movie, tv/radio series, season, or episode, or media object." .

ns1:proficiencyLevel a rdf:Property ;
	rdfs:label "proficiencyLevel" ;
	ns1:domainIncludes ns1:TechArticle ;
	ns1:rangeIncludes ns1:Text ;
	rdfs:comment "Proficiency needed for this content; expected values: 'Beginner', 'Expert'." .

ns1:programMembershipUsed a rdf:Property ;
	rdfs:label "programMembershipUsed" ;
	ns1:domainIncludes ns1:Reservation ;
	ns1:rangeIncludes ns1:ProgramMembership ;
	rdfs:comment "Any membership in a frequent flyer, hotel loyalty program, etc. being applied to the reservation." .

ns1:programName a rdf:Property ;
	rdfs:label "programName" ;
	ns1:domainIncludes ns1:ProgramMembership ;
	ns1:rangeIncludes ns1:Text ;
	rdfs:comment "The program providing the membership." .

ns1:programmingLanguage a rdf:Property ;
	rdfs:label "programmingLanguage" ;
	ns1:domainIncludes ns1:Code ;
	ns1:rangeIncludes ns1:Thing ;
	rdfs:comment "The computer programming language." .

ns1:programmingModel a rdf:Property ;
	rdfs:label "programmingModel" ;
	ns1:domainIncludes ns1:APIReference ;
	ns1:rangeIncludes ns1:Text ;
	rdfs:comment "Indicates whether API is managed or unmanaged." .

ns1:proprietaryName a rdf:Property ;
	rdfs:label "proprietaryName" ;
	ns1:domainIncludes ns1:Diet ;
	ns1:rangeIncludes ns1:Text ;
	rdfs:comment "Proprietary name given to the diet plan, typically by its originator or creator." .

ns1:proteinContent a rdf:Property ;
	rdfs:label "proteinContent" ;
	ns1:domainIncludes ns1:NutritionInformation ;
	ns1:rangeIncludes ns1:Mass ;
	rdfs:comment "The number of grams of protein." .

ns1:provider a rdf:Property ;
	rdfs:label "provider" ;
	ns1:domainIncludes ns1:BusTrip , ns1:CreativeWork , ns1:Flight , ns1:Reservation , ns1:Service , ns1:TrainTrip ;
	ns1:rangeIncludes ns1:Organization , ns1:Person ;
	rdfs:comment "The person or organization providing the service, reservation, or creative work. The provider may subcontract out the service." .

ns1:providesService a rdf:Property ;
	rdfs:label "providesService" ;
	ns1:domainIncludes ns1:ServiceChannel ;
	ns1:rangeIncludes ns1:Service ;
	rdfs:comment "The service provided by this channel." .

ns1:publication a rdf:Property ;
	rdfs:label "publication" ;
	ns1:domainIncludes ns1:Clip , ns1:Episode , ns1:MediaObject ;
	ns1:rangeIncludes ns1:PublicationEvent ;
	rdfs:comment "A publication event associated with the episode, clip or media object." .

ns1:publicationType a rdf:Property ;
	rdfs:label "publicationType" ;
	ns1:domainIncludes ns1:MedicalScholarlyArticle ;
	ns1:rangeIncludes ns1:Text ;
	rdfs:comment "The type of the medical article, taken from the US NLM MeSH <a href=http://www.nlm.nih.gov/mesh/pubtypes.html>publication type catalog." .

ns1:publishedOn a rdf:Property ;
	rdfs:label "publishedOn" ;
	ns1:domainIncludes ns1:PublicationEvent ;
	ns1:rangeIncludes ns1:BroadcastService ;
	rdfs:comment "A broadcast service associated with the publication event." .

ns1:publisher a rdf:Property ;
	rdfs:label "publisher" ;
	ns1:domainIncludes ns1:CreativeWork ;
	ns1:rangeIncludes ns1:Organization ;
	rdfs:comment "The publisher of the creative work." .

ns1:publishingPrinciples a rdf:Property ;
	rdfs:label "publishingPrinciples" ;
	ns1:domainIncludes ns1:CreativeWork ;
	ns1:rangeIncludes ns1:URL ;
	rdfs:comment "Link to page describing the editorial principles of the organization primarily responsible for the creation of the CreativeWork." .

ns1:purpose a rdf:Property ;
	rdfs:label "purpose" ;
	ns1:domainIncludes ns1:AllocateAction , ns1:MedicalDevice , ns1:PayAction ;
	ns1:rangeIncludes ns1:MedicalDevicePurpose , ns1:Thing ;
	rdfs:comment "A goal towards an action is taken. Can be concrete or abstract." .

ns1:qualifications a rdf:Property ;
	rdfs:label "qualifications" ;
	ns1:domainIncludes ns1:JobPosting ;
	ns1:rangeIncludes ns1:Text ;
	rdfs:comment "Specific qualifications required for this role." .

ns1:query a rdf:Property ;
	rdfs:label "query" ;
	ns1:domainIncludes ns1:SearchAction ;
	ns1:rangeIncludes ns1:Class , ns1:Text ;
	rdfs:comment "A sub property of instrument. The query used on this action." ;
	rdfs:subPropertyOf ns1:instrument .

ns1:question a rdf:Property ;
	rdfs:label "question" ;
	ns1:domainIncludes ns1:AskAction ;
	ns1:rangeIncludes ns1:Text ;
	rdfs:comment "A sub property of object. A question." ;
	rdfs:subPropertyOf ns1:object .

ns1:rangeIncludes a rdf:Property ;
	rdfs:label "rangeIncludes" ;
	ns1:domainIncludes ns1:Property ;
	ns1:rangeIncludes ns1:Class ;
	rdfs:comment "Relates a property to a class that constitutes (one of) the expected type(s) for values of the property." .

ns1:ratingCount a rdf:Property ;
	rdfs:label "ratingCount" ;
	ns1:domainIncludes ns1:AggregateRating ;
	ns1:rangeIncludes ns1:Number ;
	rdfs:comment "The count of total number of ratings." .

ns1:ratingValue a rdf:Property ;
	rdfs:label "ratingValue" ;
	ns1:domainIncludes ns1:Rating ;
	ns1:rangeIncludes ns1:Text ;
	rdfs:comment "The rating for the content." .

ns1:readonlyValue a rdf:Property ;
	rdfs:label "readonlyValue" ;
	ns1:domainIncludes ns1:PropertyValueSpecification ;
	ns1:rangeIncludes ns1:Boolean ;
	rdfs:comment "Whether or not a property is mutable.  Default is false. Specifying this for a property that also has a value makes it act similar to a \"hidden\" input in an HTML form." .

ns1:realEstateAgent a rdf:Property ;
	rdfs:label "realEstateAgent" ;
	ns1:domainIncludes ns1:RentAction ;
	ns1:rangeIncludes ns1:RealEstateAgent ;
	rdfs:comment "A sub property of participant. The real estate agent involved in the action." ;
	rdfs:subPropertyOf ns1:participant .

ns1:recipe a rdf:Property ;
	rdfs:label "recipe" ;
	ns1:domainIncludes ns1:CookAction ;
	ns1:rangeIncludes ns1:Recipe ;
	rdfs:comment "A sub property of instrument. The recipe/instructions used to perform the action." ;
	rdfs:subPropertyOf ns1:instrument .

ns1:recipeCategory a rdf:Property ;
	rdfs:label "recipeCategory" ;
	ns1:domainIncludes ns1:Recipe ;
	ns1:rangeIncludes ns1:Text ;
	rdfs:comment "The category of the recipe&#x2014;for example, appetizer, entree, etc." .

ns1:recipeCuisine a rdf:Property ;
	rdfs:label "recipeCuisine" ;
	ns1:domainIncludes ns1:Recipe ;
	ns1:rangeIncludes ns1:Text ;
	rdfs:comment "The cuisine of the recipe (for example, French or Ethiopian)." .

ns1:recipeInstructions a rdf:Property ;
	rdfs:label "recipeInstructions" ;
	ns1:domainIncludes ns1:Recipe ;
	ns1:rangeIncludes ns1:Text ;
	rdfs:comment "The steps to make the dish." .

ns1:recipeYield a rdf:Property ;
	rdfs:label "recipeYield" ;
	ns1:domainIncludes ns1:Recipe ;
	ns1:rangeIncludes ns1:Text ;
	rdfs:comment "The quantity produced by the recipe (for example, number of people served, number of servings, etc)." .

ns1:recipient a rdf:Property ;
	rdfs:label "recipient" ;
	ns1:domainIncludes ns1:AuthorizeAction , ns1:CommunicateAction , ns1:DonateAction , ns1:GiveAction , ns1:PayAction , ns1:ReturnAction , ns1:SendAction , ns1:TipAction ;
	ns1:rangeIncludes ns1:Audience , ns1:Organization , ns1:Person ;
	rdfs:comment "A sub property of participant. The participant who is at the receiving end of the action." ;
	rdfs:subPropertyOf ns1:participant .

ns1:recognizingAuthority a rdf:Property ;
	rdfs:label "recognizingAuthority" ;
	ns1:domainIncludes ns1:MedicalEntity ;
	ns1:rangeIncludes ns1:Organization ;
	rdfs:comment "If applicable, the organization that officially recognizes this entity as part of its endorsed system of medicine." .

ns1:recommendationStrength a rdf:Property ;
	rdfs:label "recommendationStrength" ;
	ns1:domainIncludes ns1:MedicalGuidelineRecommendation ;
	ns1:rangeIncludes ns1:Text ;
	rdfs:comment "Strength of the guideline's recommendation (e.g. 'class I')." .

ns1:recommendedIntake a rdf:Property ;
	rdfs:label "recommendedIntake" ;
	ns1:domainIncludes ns1:DietarySupplement ;
	ns1:rangeIncludes ns1:RecommendedDoseSchedule ;
	rdfs:comment "Recommended intake of this supplement for a given population as defined by a specific recommending authority." .

ns1:regionDrained a rdf:Property ;
	rdfs:label "regionDrained" ;
	ns1:domainIncludes ns1:LymphaticVessel , ns1:Vein ;
	ns1:rangeIncludes ns1:AnatomicalStructure , ns1:AnatomicalSystem ;
	rdfs:comment "The anatomical or organ system drained by this vessel; generally refers to a specific part of an organ." .

ns1:regionsAllowed a rdf:Property ;
	rdfs:label "regionsAllowed" ;
	ns1:domainIncludes ns1:MediaObject ;
	ns1:rangeIncludes ns1:Place ;
	rdfs:comment "The regions where the media is allowed. If not specified, then it's assumed to be allowed everywhere. Specify the countries in <a href='http://en.wikipedia.org/wiki/ISO_3166'>ISO 3166 format</a>." .

ns1:relatedAnatomy a rdf:Property ;
	rdfs:label "relatedAnatomy" ;
	ns1:domainIncludes ns1:SuperficialAnatomy ;
	ns1:rangeIncludes ns1:AnatomicalStructure , ns1:AnatomicalSystem ;
	rdfs:comment "Anatomical systems or structures that relate to the superficial anatomy." .

ns1:relatedCondition a rdf:Property ;
	rdfs:label "relatedCondition" ;
	ns1:domainIncludes ns1:AnatomicalStructure , ns1:AnatomicalSystem , ns1:SuperficialAnatomy ;
	ns1:rangeIncludes ns1:MedicalCondition ;
	rdfs:comment "A medical condition associated with this anatomy." .

ns1:relatedDrug a rdf:Property ;
	rdfs:label "relatedDrug" ;
	ns1:domainIncludes ns1:Drug ;
	ns1:rangeIncludes ns1:Drug ;
	rdfs:comment "Any other drug related to this one, for example commonly-prescribed alternatives." .

ns1:relatedLink a rdf:Property ;
	rdfs:label "relatedLink" ;
	ns1:domainIncludes ns1:WebPage ;
	ns1:rangeIncludes ns1:URL ;
	rdfs:comment "A link related to this web page, for example to other related web pages." .

ns1:relatedStructure a rdf:Property ;
	rdfs:label "relatedStructure" ;
	ns1:domainIncludes ns1:AnatomicalSystem ;
	ns1:rangeIncludes ns1:AnatomicalStructure ;
	rdfs:comment "Related anatomical structure(s) that are not part of the system but relate or connect to it, such as vascular bundles associated with an organ system." .

ns1:relatedTherapy a rdf:Property ;
	rdfs:label "relatedTherapy" ;
	ns1:domainIncludes ns1:AnatomicalStructure , ns1:AnatomicalSystem , ns1:SuperficialAnatomy ;
	ns1:rangeIncludes ns1:MedicalTherapy ;
	rdfs:comment "A medical therapy related to this anatomy." .

ns1:relatedTo a rdf:Property ;
	rdfs:label "relatedTo" ;
	ns1:domainIncludes ns1:Person ;
	ns1:rangeIncludes ns1:Person ;
	rdfs:comment "The most generic familial relation." .

ns1:releaseDate a rdf:Property ;
	rdfs:label "releaseDate" ;
	ns1:domainIncludes ns1:Product ;
	ns1:rangeIncludes ns1:Date ;
	rdfs:comment "The release date of a product or product model. This can be used to distinguish the exact variant of a product." .

ns1:releaseNotes a rdf:Property ;
	rdfs:label "releaseNotes" ;
	ns1:domainIncludes ns1:SoftwareApplication ;
	ns1:rangeIncludes ns1:Text , ns1:URL ;
	rdfs:comment "Description of what changed in this version." .

ns1:relevantSpecialty a rdf:Property ;
	rdfs:label "relevantSpecialty" ;
	ns1:domainIncludes ns1:MedicalEntity ;
	ns1:rangeIncludes ns1:MedicalSpecialty ;
	rdfs:comment "If applicable, a medical specialty in which this entity is relevant." .

ns1:repetitions a rdf:Property ;
	rdfs:label "repetitions" ;
	ns1:domainIncludes ns1:ExercisePlan ;
	ns1:rangeIncludes ns1:Number ;
	rdfs:comment "Number of times one should repeat the activity." .

ns1:replacee a rdf:Property ;
	rdfs:label "replacee" ;
	ns1:domainIncludes ns1:ReplaceAction ;
	ns1:rangeIncludes ns1:Thing ;
	rdfs:comment "A sub property of object. The object that is being replaced." ;
	rdfs:subPropertyOf ns1:object .

ns1:replacer a rdf:Property ;
	rdfs:label "replacer" ;
	ns1:domainIncludes ns1:ReplaceAction ;
	ns1:rangeIncludes ns1:Thing ;
	rdfs:comment "A sub property of object. The object that replaces." ;
	rdfs:subPropertyOf ns1:object .

ns1:replyToUrl a rdf:Property ;
	rdfs:label "replyToUrl" ;
	ns1:domainIncludes ns1:UserComments ;
	ns1:rangeIncludes ns1:URL ;
	rdfs:comment "The URL at which a reply may be posted to the specified UserComment." .

ns1:representativeOfPage a rdf:Property ;
	rdfs:label "representativeOfPage" ;
	ns1:domainIncludes ns1:ImageObject ;
	ns1:rangeIncludes ns1:Boolean ;
	rdfs:comment "Indicates whether this image is representative of the content of the page." .

ns1:requiredGender a rdf:Property ;
	rdfs:label "requiredGender" ;
	ns1:domainIncludes ns1:PeopleAudience ;
	ns1:rangeIncludes ns1:Text ;
	rdfs:comment "Audiences defined by a person's gender." .

ns1:requiredMaxAge a rdf:Property ;
	rdfs:label "requiredMaxAge" ;
	ns1:domainIncludes ns1:PeopleAudience ;
	ns1:rangeIncludes ns1:Integer ;
	rdfs:comment "Audiences defined by a person's maximum age." .

ns1:requiredMinAge a rdf:Property ;
	rdfs:label "requiredMinAge" ;
	ns1:domainIncludes ns1:PeopleAudience ;
	ns1:rangeIncludes ns1:Integer ;
	rdfs:comment "Audiences defined by a person's minimum age." .

ns1:requirements a rdf:Property ;
	rdfs:label "requirements" ;
	ns1:domainIncludes ns1:SoftwareApplication ;
	ns1:rangeIncludes ns1:Text , ns1:URL ;
	rdfs:comment "Component dependency requirements for application. This includes runtime environments and shared libraries that are not included in the application distribution package, but required to run the application (Examples: DirectX, Java or .NET runtime)." .

ns1:requiresSubscription a rdf:Property ;
	rdfs:label "requiresSubscription" ;
	ns1:domainIncludes ns1:MediaObject ;
	ns1:rangeIncludes ns1:Boolean ;
	rdfs:comment "Indicates if use of the media require a subscription  (either paid or free). Allowed values are <code>true</code> or <code>false</code> (note that an earlier version had 'yes', 'no')." .

ns1:reservationFor a rdf:Property ;
	rdfs:label "reservationFor" ;
	ns1:domainIncludes ns1:Reservation ;
	ns1:rangeIncludes ns1:Thing ;
	rdfs:comment "The thing -- flight, event, restaurant,etc. being reserved." .

ns1:reservationId a rdf:Property ;
	rdfs:label "reservationId" ;
	ns1:domainIncludes ns1:Reservation ;
	ns1:rangeIncludes ns1:Text ;
	rdfs:comment "A unique identifier for the reservation." .

ns1:reservationStatus a rdf:Property ;
	rdfs:label "reservationStatus" ;
	ns1:domainIncludes ns1:Reservation ;
	ns1:rangeIncludes ns1:ReservationStatusType ;
	rdfs:comment "The current status of the reservation." .

ns1:reservedTicket a rdf:Property ;
	rdfs:label "reservedTicket" ;
	ns1:domainIncludes ns1:Reservation ;
	ns1:rangeIncludes ns1:Ticket ;
	rdfs:comment "A ticket associated with the reservation." .

ns1:responsibilities a rdf:Property ;
	rdfs:label "responsibilities" ;
	ns1:domainIncludes ns1:JobPosting ;
	ns1:rangeIncludes ns1:Text ;
	rdfs:comment "Responsibilities associated with this role." .

ns1:restPeriods a rdf:Property ;
	rdfs:label "restPeriods" ;
	ns1:domainIncludes ns1:ExercisePlan ;
	ns1:rangeIncludes ns1:Text ;
	rdfs:comment "How often one should break from the activity." .

ns1:resultReview a rdf:Property ;
	rdfs:label "resultReview" ;
	ns1:domainIncludes ns1:ReviewAction ;
	ns1:rangeIncludes ns1:Review ;
	rdfs:comment "A sub property of result. The review that resulted in the performing of the action." ;
	rdfs:subPropertyOf ns1:result .

ns1:reviewBody a rdf:Property ;
	rdfs:label "reviewBody" ;
	ns1:domainIncludes ns1:Review ;
	ns1:rangeIncludes ns1:Text ;
	rdfs:comment "The actual body of the review." .

ns1:reviewCount a rdf:Property ;
	rdfs:label "reviewCount" ;
	ns1:domainIncludes ns1:AggregateRating ;
	ns1:rangeIncludes ns1:Number ;
	rdfs:comment "The count of total number of reviews." .

ns1:reviewRating a rdf:Property ;
	rdfs:label "reviewRating" ;
	ns1:domainIncludes ns1:Review ;
	ns1:rangeIncludes ns1:Rating ;
	rdfs:comment "The rating given in this review. Note that reviews can themselves be rated. The <code>reviewRating</code> applies to rating given by the review. The <code>aggregateRating</code> property applies to the review itself, as a creative work." .

ns1:reviewedBy a rdf:Property ;
	rdfs:label "reviewedBy" ;
	ns1:domainIncludes ns1:WebPage ;
	ns1:rangeIncludes ns1:Organization , ns1:Person ;
	rdfs:comment "People or organizations that have reviewed the content on this web page for accuracy and/or completeness." .

ns1:reviews a rdf:Property ;
	rdfs:label "reviews" ;
	ns1:domainIncludes ns1:CreativeWork , ns1:Offer , ns1:Organization , ns1:Place , ns1:Product ;
	ns1:rangeIncludes ns1:Review ;
	ns1:supercededBy ns1:review ;
	rdfs:comment "Review of the item (legacy spelling; see singular form, review)." .

ns1:riskFactor a rdf:Property ;
	rdfs:label "riskFactor" ;
	ns1:domainIncludes ns1:MedicalCondition ;
	ns1:rangeIncludes ns1:MedicalRiskFactor ;
	rdfs:comment "A modifiable or non-modifiable factor that increases the risk of a patient contracting this condition, e.g. age,  coexisting condition." .

ns1:risks a rdf:Property ;
	rdfs:label "risks" ;
	ns1:domainIncludes ns1:Diet ;
	ns1:rangeIncludes ns1:Text ;
	rdfs:comment "Specific physiologic risks associated to the plan." .

ns1:runsTo a rdf:Property ;
	rdfs:label "runsTo" ;
	ns1:domainIncludes ns1:LymphaticVessel ;
	ns1:rangeIncludes ns1:Vessel ;
	rdfs:comment "The vasculature the lymphatic structure runs, or efferents, to." .

ns1:runtime a rdf:Property ;
	rdfs:label "runtime" ;
	ns1:domainIncludes ns1:Code ;
	ns1:rangeIncludes ns1:Text ;
	rdfs:comment "Runtime platform or script interpreter dependencies (Example - Java v1, Python2.3, .Net Framework 3.0)" .

ns1:safetyConsideration a rdf:Property ;
	rdfs:label "safetyConsideration" ;
	ns1:domainIncludes ns1:DietarySupplement ;
	ns1:rangeIncludes ns1:Text ;
	rdfs:comment "Any potential safety concern associated with the supplement. May include interactions with other drugs and foods, pregnancy, breastfeeding, known adverse reactions, and documented efficacy of the supplement." .

ns1:salaryCurrency a rdf:Property ;
	rdfs:label "salaryCurrency" ;
	ns1:domainIncludes ns1:JobPosting ;
	ns1:rangeIncludes ns1:Text ;
	rdfs:comment "The currency (coded using ISO 4217, http://en.wikipedia.org/wiki/ISO_4217 used for the main salary information in this job posting." .

ns1:sameAs a rdf:Property ;
	rdfs:label "sameAs" ;
	ns1:domainIncludes ns1:Thing ;
	ns1:rangeIncludes ns1:URL ;
	rdfs:comment "URL of a reference Web page that unambiguously indicates the item's identity. E.g. the URL of the item's Wikipedia page, Freebase page, or official website." .

ns1:sampleType a rdf:Property ;
	rdfs:label "sampleType" ;
	ns1:domainIncludes ns1:Code ;
	ns1:rangeIncludes ns1:Text ;
	rdfs:comment "Full (compile ready) solution, code snippet, inline code, scripts, template." .

ns1:saturatedFatContent a rdf:Property ;
	rdfs:label "saturatedFatContent" ;
	ns1:domainIncludes ns1:NutritionInformation ;
	ns1:rangeIncludes ns1:Mass ;
	rdfs:comment "The number of grams of saturated fat." .

ns1:scheduledTime a rdf:Property ;
	rdfs:label "scheduledTime" ;
	ns1:domainIncludes ns1:PlanAction , ns1:ReserveAction ;
	ns1:rangeIncludes ns1:DateTime ;
	rdfs:comment "The time the object is scheduled to." .

ns1:screenshot a rdf:Property ;
	rdfs:label "screenshot" ;
	ns1:domainIncludes ns1:SoftwareApplication ;
	ns1:rangeIncludes ns1:ImageObject , ns1:URL ;
	rdfs:comment "A link to a screenshot image of the app." .

ns1:seasonNumber a rdf:Property ;
	rdfs:label "seasonNumber" ;
	ns1:domainIncludes ns1:Season , ns1:TVSeason ;
	ns1:rangeIncludes ns1:Integer ;
	rdfs:comment "Position of the season within an ordered group of seasons." .

ns1:seasons a rdf:Property ;
	rdfs:label "seasons" ;
	ns1:domainIncludes ns1:RadioSeries , ns1:Series , ns1:TVSeries ;
	ns1:rangeIncludes ns1:Season ;
	ns1:supercededBy ns1:season ;
	rdfs:comment "A season in a tv/radio series. (legacy spelling; see singular form, season)" .

ns1:seatNumber a rdf:Property ;
	rdfs:label "seatNumber" ;
	ns1:domainIncludes ns1:Seat ;
	ns1:rangeIncludes ns1:Text ;
	rdfs:comment "The location of the reserved seat (e.g., 27)." .

ns1:seatRow a rdf:Property ;
	rdfs:label "seatRow" ;
	ns1:domainIncludes ns1:Seat ;
	ns1:rangeIncludes ns1:Text ;
	rdfs:comment "The row location of the reserved seat (e.g., B)." .

ns1:seatSection a rdf:Property ;
	rdfs:label "seatSection" ;
	ns1:domainIncludes ns1:Seat ;
	ns1:rangeIncludes ns1:Text ;
	rdfs:comment "The section location of the reserved seat (e.g. Orchestra)." .

ns1:seatingType a rdf:Property ;
	rdfs:label "seatingType" ;
	ns1:domainIncludes ns1:Seat ;
	ns1:rangeIncludes ns1:QualitativeValue , ns1:Text ;
	rdfs:comment "The type/class of the seat." .

ns1:secondaryPrevention a rdf:Property ;
	rdfs:label "secondaryPrevention" ;
	ns1:domainIncludes ns1:MedicalCondition ;
	ns1:rangeIncludes ns1:MedicalTherapy ;
	rdfs:comment "A preventative therapy used to prevent reoccurrence of the medical condition after an initial episode of the condition." .

ns1:seeks a rdf:Property ;
	rdfs:label "seeks" ;
	ns1:domainIncludes ns1:Organization , ns1:Person ;
	ns1:rangeIncludes ns1:Demand ;
	rdfs:comment "A pointer to products or services sought by the organization or person (demand)." .

ns1:seller a rdf:Property ;
	rdfs:label "seller" ;
	ns1:domainIncludes ns1:Demand , ns1:Offer ;
	ns1:rangeIncludes ns1:Organization , ns1:Person ;
	rdfs:comment "The organization or person making the offer." .

ns1:sender a rdf:Property ;
	rdfs:label "sender" ;
	ns1:domainIncludes ns1:ReceiveAction ;
	ns1:rangeIncludes ns1:Audience , ns1:Organization , ns1:Person ;
	rdfs:comment "A sub property of participant. The participant who is at the sending end of the action." ;
	rdfs:subPropertyOf ns1:participant .

ns1:sensoryUnit a rdf:Property ;
	rdfs:label "sensoryUnit" ;
	ns1:domainIncludes ns1:Nerve ;
	ns1:rangeIncludes ns1:AnatomicalStructure , ns1:SuperficialAnatomy ;
	rdfs:comment "The neurological pathway extension that inputs and sends information to the brain or spinal cord." .

ns1:serialNumber a rdf:Property ;
	rdfs:label "serialNumber" ;
	ns1:domainIncludes ns1:Demand , ns1:IndividualProduct , ns1:Offer ;
	ns1:rangeIncludes ns1:Text ;
	rdfs:comment "The serial number or any alphanumeric identifier of a particular product. When attached to an offer, it is a shortcut for the serial number of the product included in the offer." .

ns1:seriousAdverseOutcome a rdf:Property ;
	rdfs:label "seriousAdverseOutcome" ;
	ns1:domainIncludes ns1:MedicalDevice , ns1:MedicalTherapy ;
	ns1:rangeIncludes ns1:MedicalEntity ;
	rdfs:comment "A possible serious complication and/or serious side effect of this therapy. Serious adverse outcomes include those that are life-threatening; result in death, disability, or permanent damage; require hospitalization or prolong existing hospitalization; cause congenital anomalies or birth defects; or jeopardize the patient and may require medical or surgical intervention to prevent one of the outcomes in this definition." .

ns1:servesCuisine a rdf:Property ;
	rdfs:label "servesCuisine" ;
	ns1:domainIncludes ns1:FoodEstablishment ;
	ns1:rangeIncludes ns1:Text ;
	rdfs:comment "The cuisine of the restaurant." .

ns1:serviceArea a rdf:Property ;
	rdfs:label "serviceArea" ;
	ns1:domainIncludes ns1:Service ;
	ns1:rangeIncludes ns1:AdministrativeArea ;
	rdfs:comment "The geographic area where the service is provided." .

ns1:serviceAudience a rdf:Property ;
	rdfs:label "serviceAudience" ;
	ns1:domainIncludes ns1:Service ;
	ns1:rangeIncludes ns1:Audience ;
	rdfs:comment "The audience eligible for this service." .

ns1:serviceLocation a rdf:Property ;
	rdfs:label "serviceLocation" ;
	ns1:domainIncludes ns1:ServiceChannel ;
	ns1:rangeIncludes ns1:Place ;
	rdfs:comment "The location (e.g. civic structure, local business, etc.) where a person can go to access the service." .

ns1:serviceOperator a rdf:Property ;
	rdfs:label "serviceOperator" ;
	ns1:domainIncludes ns1:GovernmentService ;
	ns1:rangeIncludes ns1:Organization ;
	rdfs:comment "The operating organization, if different from the provider.  This enables the representation of services that are provided by an organization, but operated by another organization like a subcontractor." .

ns1:servicePhone a rdf:Property ;
	rdfs:label "servicePhone" ;
	ns1:domainIncludes ns1:ServiceChannel ;
	ns1:rangeIncludes ns1:ContactPoint ;
	rdfs:comment "The phone number to use to access the service." .

ns1:servicePostalAddress a rdf:Property ;
	rdfs:label "servicePostalAddress" ;
	ns1:domainIncludes ns1:ServiceChannel ;
	ns1:rangeIncludes ns1:PostalAddress ;
	rdfs:comment "The address for accessing the service by mail." .

ns1:serviceSmsNumber a rdf:Property ;
	rdfs:label "serviceSmsNumber" ;
	ns1:domainIncludes ns1:ServiceChannel ;
	ns1:rangeIncludes ns1:ContactPoint ;
	rdfs:comment "The number to access the service by text message." .

ns1:serviceType a rdf:Property ;
	rdfs:label "serviceType" ;
	ns1:domainIncludes ns1:Service ;
	ns1:rangeIncludes ns1:Text ;
	rdfs:comment "The type of service being offered, e.g. veterans' benefits, emergency relief, etc." .

ns1:serviceUrl a rdf:Property ;
	rdfs:label "serviceUrl" ;
	ns1:domainIncludes ns1:ServiceChannel ;
	ns1:rangeIncludes ns1:URL ;
	rdfs:comment "The website to access the service." .

ns1:servingSize a rdf:Property ;
	rdfs:label "servingSize" ;
	ns1:domainIncludes ns1:NutritionInformation ;
	ns1:rangeIncludes ns1:Text ;
	rdfs:comment "The serving size, in terms of the number of volume or mass." .

ns1:siblings a rdf:Property ;
	rdfs:label "siblings" ;
	ns1:domainIncludes ns1:Person ;
	ns1:rangeIncludes ns1:Person ;
	ns1:supercededBy ns1:sibling ;
	rdfs:comment "A sibling of the person (legacy spelling; see singular form, sibling)." .

ns1:signDetected a rdf:Property ;
	rdfs:label "signDetected" ;
	ns1:domainIncludes ns1:MedicalTest ;
	ns1:rangeIncludes ns1:MedicalSign ;
	rdfs:comment "A sign detected by the test." .

ns1:signOrSymptom a rdf:Property ;
	rdfs:label "signOrSymptom" ;
	ns1:domainIncludes ns1:MedicalCondition ;
	ns1:rangeIncludes ns1:MedicalSignOrSymptom ;
	rdfs:comment "A sign or symptom of this condition. Signs are objective or physically observable manifestations of the medical condition while symptoms are the subjective experience of the medical condition." .

ns1:significance a rdf:Property ;
	rdfs:label "significance" ;
	ns1:domainIncludes ns1:SuperficialAnatomy ;
	ns1:rangeIncludes ns1:Text ;
	rdfs:comment "The significance associated with the superficial anatomy; as an example, how characteristics of the superficial anatomy can suggest underlying medical conditions or courses of treatment." .

ns1:significantLinks a rdf:Property ;
	rdfs:label "significantLinks" ;
	ns1:domainIncludes ns1:WebPage ;
	ns1:rangeIncludes ns1:URL ;
	ns1:supercededBy ns1:significantLink ;
	rdfs:comment "The most significant URLs on the page. Typically, these are the non-navigation links that are clicked on the most (legacy spelling; see singular form, significantLink)." .

ns1:skills a rdf:Property ;
	rdfs:label "skills" ;
	ns1:domainIncludes ns1:JobPosting ;
	ns1:rangeIncludes ns1:Text ;
	rdfs:comment "Skills required to fulfill this role." .

ns1:sku a rdf:Property ;
	rdfs:label "sku" ;
	ns1:domainIncludes ns1:Demand , ns1:Offer , ns1:Product ;
	ns1:rangeIncludes ns1:Text ;
	rdfs:comment "The Stock Keeping Unit (SKU), i.e. a merchant-specific identifier for a product or service, or the product to which the offer refers." .

ns1:sodiumContent a rdf:Property ;
	rdfs:label "sodiumContent" ;
	ns1:domainIncludes ns1:NutritionInformation ;
	ns1:rangeIncludes ns1:Mass ;
	rdfs:comment "The number of milligrams of sodium." .

ns1:softwareVersion a rdf:Property ;
	rdfs:label "softwareVersion" ;
	ns1:domainIncludes ns1:SoftwareApplication ;
	ns1:rangeIncludes ns1:Text ;
	rdfs:comment "Version of the software instance." .

ns1:source a rdf:Property ;
	rdfs:label "source" ;
	ns1:domainIncludes ns1:Artery ;
	ns1:rangeIncludes ns1:AnatomicalStructure ;
	rdfs:comment "The anatomical or organ system that the artery originates from." .

ns1:sourceOrganization a rdf:Property ;
	rdfs:label "sourceOrganization" ;
	ns1:domainIncludes ns1:CreativeWork ;
	ns1:rangeIncludes ns1:Organization ;
	rdfs:comment "The Organization on whose behalf the creator was working." .

ns1:sourcedFrom a rdf:Property ;
	rdfs:label "sourcedFrom" ;
	ns1:domainIncludes ns1:Nerve ;
	ns1:rangeIncludes ns1:BrainStructure ;
	rdfs:comment "The neurological pathway that originates the neurons." .

ns1:spatial a rdf:Property ;
	rdfs:label "spatial" ;
	ns1:domainIncludes ns1:Dataset ;
	ns1:rangeIncludes ns1:Place ;
	rdfs:comment "The range of spatial applicability of a dataset, e.g. for a dataset of New York weather, the state of New York." .

ns1:specialCommitments a rdf:Property ;
	rdfs:label "specialCommitments" ;
	ns1:domainIncludes ns1:JobPosting ;
	ns1:rangeIncludes ns1:Text ;
	rdfs:comment "Any special commitments associated with this job posting. Valid entries include VeteranCommit, MilitarySpouseCommit, etc." .

ns1:specialty a rdf:Property ;
	rdfs:label "specialty" ;
	ns1:domainIncludes ns1:WebPage ;
	ns1:rangeIncludes ns1:Specialty ;
	rdfs:comment "One of the domain specialities to which this web page's content applies." .

ns1:sponsor a rdf:Property ;
	rdfs:label "sponsor" ;
	ns1:domainIncludes ns1:MedicalStudy ;
	ns1:rangeIncludes ns1:Organization ;
	rdfs:comment "Sponsor of the study." .

ns1:sportsActivityLocation a rdf:Property ;
	rdfs:label "sportsActivityLocation" ;
	ns1:domainIncludes ns1:ExerciseAction ;
	ns1:rangeIncludes ns1:SportsActivityLocation ;
	rdfs:comment "A sub property of location. The sports activity location where this action occurred." ;
	rdfs:subPropertyOf ns1:location .

ns1:sportsEvent a rdf:Property ;
	rdfs:label "sportsEvent" ;
	ns1:domainIncludes ns1:ExerciseAction ;
	ns1:rangeIncludes ns1:SportsEvent ;
	rdfs:comment "A sub property of location. The sports event where this action occurred." ;
	rdfs:subPropertyOf ns1:location .

ns1:sportsTeam a rdf:Property ;
	rdfs:label "sportsTeam" ;
	ns1:domainIncludes ns1:ExerciseAction ;
	ns1:rangeIncludes ns1:SportsTeam ;
	rdfs:comment "A sub property of participant. The sports team that participated on this action." ;
	rdfs:subPropertyOf ns1:participant .

ns1:spouse a rdf:Property ;
	rdfs:label "spouse" ;
	ns1:domainIncludes ns1:Person ;
	ns1:rangeIncludes ns1:Person ;
	rdfs:comment "The person's spouse." .

ns1:stage a rdf:Property ;
	rdfs:label "stage" ;
	ns1:domainIncludes ns1:MedicalCondition ;
	ns1:rangeIncludes ns1:MedicalConditionStage ;
	rdfs:comment "The stage of the condition, if applicable." .

ns1:stageAsNumber a rdf:Property ;
	rdfs:label "stageAsNumber" ;
	ns1:domainIncludes ns1:MedicalConditionStage ;
	ns1:rangeIncludes ns1:Number ;
	rdfs:comment "The stage represented as a number, e.g. 3." .

ns1:startDate a rdf:Property ;
	rdfs:label "startDate" ;
	ns1:domainIncludes ns1:Event , ns1:Role , ns1:Season , ns1:Series , ns1:TVSeason , ns1:TVSeries ;
	ns1:rangeIncludes ns1:Date ;
	rdfs:comment "The start date and time of the event, role or item (in <a href='http://en.wikipedia.org/wiki/ISO_8601'>ISO 8601 date format</a>)." .

ns1:startTime a rdf:Property ;
	rdfs:label "startTime" ;
	ns1:domainIncludes ns1:Action , ns1:FoodEstablishmentReservation ;
	ns1:rangeIncludes ns1:DateTime ;
	rdfs:comment """The startTime of something. For a reserved event or service (e.g. FoodEstablishmentReservation), the time that it is expected to start. For actions that span a period of time, when the action was performed. e.g. John wrote a book from *January* to December.

Note that Event uses startDate/endDate instead of startTime/endTime, even when describing dates with times. This situation may be clarified in future revisions.
""" .

ns1:status a rdf:Property ;
	rdfs:label "status" ;
	ns1:domainIncludes ns1:MedicalStudy ;
	ns1:rangeIncludes ns1:MedicalStudyStatus ;
	rdfs:comment "The status of the study (enumerated)." .

ns1:stepValue a rdf:Property ;
	rdfs:label "stepValue" ;
	ns1:domainIncludes ns1:PropertyValueSpecification ;
	ns1:rangeIncludes ns1:Number ;
	rdfs:comment "The stepValue attribute indicates the granularity that is expected (and required) of the value in a PropertyValueSpecification." .

ns1:storageRequirements a rdf:Property ;
	rdfs:label "storageRequirements" ;
	ns1:domainIncludes ns1:SoftwareApplication ;
	ns1:rangeIncludes ns1:Text , ns1:URL ;
	rdfs:comment "Storage requirements (free space required)." .

ns1:streetAddress a rdf:Property ;
	rdfs:label "streetAddress" ;
	ns1:domainIncludes ns1:PostalAddress ;
	ns1:rangeIncludes ns1:Text ;
	rdfs:comment "The street address. For example, 1600 Amphitheatre Pkwy." .

ns1:strengthUnit a rdf:Property ;
	rdfs:label "strengthUnit" ;
	ns1:domainIncludes ns1:DrugStrength ;
	ns1:rangeIncludes ns1:Text ;
	rdfs:comment "The units of an active ingredient's strength, e.g. mg." .

ns1:strengthValue a rdf:Property ;
	rdfs:label "strengthValue" ;
	ns1:domainIncludes ns1:DrugStrength ;
	ns1:rangeIncludes ns1:Number ;
	rdfs:comment "The value of an active ingredient's strength, e.g. 325." .

ns1:structuralClass a rdf:Property ;
	rdfs:label "structuralClass" ;
	ns1:domainIncludes ns1:Joint ;
	ns1:rangeIncludes ns1:Text ;
	rdfs:comment "The name given to how bone physically connects to each other." .

ns1:study a rdf:Property ;
	rdfs:label "study" ;
	ns1:domainIncludes ns1:MedicalEntity ;
	ns1:rangeIncludes ns1:MedicalStudy ;
	rdfs:comment "A medical study or trial related to this entity." .

ns1:studyDesign a rdf:Property ;
	rdfs:label "studyDesign" ;
	ns1:domainIncludes ns1:MedicalObservationalStudy ;
	ns1:rangeIncludes ns1:MedicalObservationalStudyDesign ;
	rdfs:comment "Specifics about the observational study design (enumerated)." .

ns1:studyLocation a rdf:Property ;
	rdfs:label "studyLocation" ;
	ns1:domainIncludes ns1:MedicalStudy ;
	ns1:rangeIncludes ns1:AdministrativeArea ;
	rdfs:comment "The location in which the study is taking/took place." .

ns1:studySubject a rdf:Property ;
	rdfs:label "studySubject" ;
	ns1:domainIncludes ns1:MedicalStudy ;
	ns1:rangeIncludes ns1:MedicalEntity ;
	rdfs:comment "A subject of the study, i.e. one of the medical conditions, therapies, devices, drugs, etc. investigated by the study." .

ns1:subEvents a rdf:Property ;
	rdfs:label "subEvents" ;
	ns1:domainIncludes ns1:Event ;
	ns1:rangeIncludes ns1:Event ;
	ns1:supercededBy ns1:subEvent ;
	rdfs:comment "Events that are a part of this event. For example, a conference event includes many presentations, each subEvents of the conference (legacy spelling; see singular form, subEvent)." .

ns1:subOrganization a rdf:Property ;
	rdfs:label "subOrganization" ;
	ns1:domainIncludes ns1:Organization ;
	ns1:rangeIncludes ns1:Organization ;
	rdfs:comment "A relationship between two organizations where the first includes the second, e.g., as a subsidiary. See also: the more specific 'department' property." .

ns1:subReservation a rdf:Property ;
	rdfs:label "subReservation" ;
	ns1:domainIncludes ns1:ReservationPackage ;
	ns1:rangeIncludes ns1:Reservation ;
	rdfs:comment "The individual reservations included in the package. Typically a repeated property." .

ns1:subStageSuffix a rdf:Property ;
	rdfs:label "subStageSuffix" ;
	ns1:domainIncludes ns1:MedicalConditionStage ;
	ns1:rangeIncludes ns1:Text ;
	rdfs:comment "The substage, e.g. 'a' for Stage IIIa." .

ns1:subStructure a rdf:Property ;
	rdfs:label "subStructure" ;
	ns1:domainIncludes ns1:AnatomicalStructure ;
	ns1:rangeIncludes ns1:AnatomicalStructure ;
	rdfs:comment "Component (sub-)structure(s) that comprise this anatomical structure." .

ns1:subTest a rdf:Property ;
	rdfs:label "subTest" ;
	ns1:domainIncludes ns1:MedicalTestPanel ;
	ns1:rangeIncludes ns1:MedicalTest ;
	rdfs:comment "A component test of the panel." .

ns1:subtype a rdf:Property ;
	rdfs:label "subtype" ;
	ns1:domainIncludes ns1:MedicalCondition ;
	ns1:rangeIncludes ns1:Text ;
	rdfs:comment "A more specific type of the condition, where applicable, for example 'Type 1 Diabetes', 'Type 2 Diabetes', or 'Gestational Diabetes' for Diabetes." .

ns1:successorOf a rdf:Property ;
	rdfs:label "successorOf" ;
	ns1:domainIncludes ns1:ProductModel ;
	ns1:rangeIncludes ns1:ProductModel ;
	rdfs:comment "A pointer from a newer variant of a product  to its previous, often discontinued predecessor." .

ns1:sugarContent a rdf:Property ;
	rdfs:label "sugarContent" ;
	ns1:domainIncludes ns1:NutritionInformation ;
	ns1:rangeIncludes ns1:Mass ;
	rdfs:comment "The number of grams of sugar." .

ns1:suggestedGender a rdf:Property ;
	rdfs:label "suggestedGender" ;
	ns1:domainIncludes ns1:PeopleAudience ;
	ns1:rangeIncludes ns1:Text ;
	rdfs:comment "The gender of the person or audience." .

ns1:suggestedMaxAge a rdf:Property ;
	rdfs:label "suggestedMaxAge" ;
	ns1:domainIncludes ns1:PeopleAudience ;
	ns1:rangeIncludes ns1:Number ;
	rdfs:comment "Maximal age recommended for viewing content." .

ns1:suggestedMinAge a rdf:Property ;
	rdfs:label "suggestedMinAge" ;
	ns1:domainIncludes ns1:PeopleAudience ;
	ns1:rangeIncludes ns1:Number ;
	rdfs:comment "Minimal age recommended for viewing content." .

ns1:superEvent a rdf:Property ;
	rdfs:label "superEvent" ;
	ns1:domainIncludes ns1:Event ;
	ns1:rangeIncludes ns1:Event ;
	rdfs:comment "An event that this event is a part of. For example, a collection of individual music performances might each have a music festival as their superEvent." .

ns1:supercededBy a rdf:Property ;
	rdfs:label "supercededBy" ;
	ns1:domainIncludes ns1:Property ;
	ns1:rangeIncludes ns1:Property ;
	rdfs:comment "Relates a property to one that supercedes it." .

ns1:supplyTo a rdf:Property ;
	rdfs:label "supplyTo" ;
	ns1:domainIncludes ns1:Artery ;
	ns1:rangeIncludes ns1:AnatomicalStructure ;
	rdfs:comment "The area to which the artery supplies blood." .

ns1:target a rdf:Property ;
	rdfs:label "target" ;
	ns1:domainIncludes ns1:Action ;
	ns1:rangeIncludes ns1:EntryPoint ;
	rdfs:comment "Indicates a target EntryPoint for an Action." .

ns1:targetDescription a rdf:Property ;
	rdfs:label "targetDescription" ;
	ns1:domainIncludes ns1:AlignmentObject ;
	ns1:rangeIncludes ns1:Text ;
	rdfs:comment "The description of a node in an established educational framework." .

ns1:targetName a rdf:Property ;
	rdfs:label "targetName" ;
	ns1:domainIncludes ns1:AlignmentObject ;
	ns1:rangeIncludes ns1:Text ;
	rdfs:comment "The name of a node in an established educational framework." .

ns1:targetPlatform a rdf:Property ;
	rdfs:label "targetPlatform" ;
	ns1:domainIncludes ns1:APIReference ;
	ns1:rangeIncludes ns1:Text ;
	rdfs:comment "Type of app development: phone, Metro style, desktop, XBox, etc." .

ns1:targetPopulation a rdf:Property ;
	rdfs:label "targetPopulation" ;
	ns1:domainIncludes ns1:DietarySupplement , ns1:DoseSchedule ;
	ns1:rangeIncludes ns1:Text ;
	rdfs:comment "Characteristics of the population for which this is intended, or which typically uses it, e.g. 'adults'." .

ns1:targetProduct a rdf:Property ;
	rdfs:label "targetProduct" ;
	ns1:domainIncludes ns1:Code ;
	ns1:rangeIncludes ns1:SoftwareApplication ;
	rdfs:comment "Target Operating System / Product to which the code applies.  If applies to several versions, just the product name can be used." .

ns1:targetUrl a rdf:Property ;
	rdfs:label "targetUrl" ;
	ns1:domainIncludes ns1:AlignmentObject ;
	ns1:rangeIncludes ns1:URL ;
	rdfs:comment "The URL of a node in an established educational framework." .

ns1:taxID a rdf:Property ;
	rdfs:label "taxID" ;
	ns1:domainIncludes ns1:Organization , ns1:Person ;
	ns1:rangeIncludes ns1:Text ;
	rdfs:comment "The Tax / Fiscal ID of the organization or person, e.g. the TIN in the US or the CIF/NIF in Spain." .

ns1:telephone a rdf:Property ;
	rdfs:label "telephone" ;
	ns1:domainIncludes ns1:ContactPoint , ns1:Organization , ns1:Person , ns1:Place ;
	ns1:rangeIncludes ns1:Text ;
	rdfs:comment "The telephone number." .

ns1:temporal a rdf:Property ;
	rdfs:label "temporal" ;
	ns1:domainIncludes ns1:Dataset ;
	ns1:rangeIncludes ns1:DateTime ;
	rdfs:comment "The range of temporal applicability of a dataset, e.g. for a 2011 census dataset, the year 2011 (in ISO 8601 time interval format)." .

ns1:text a rdf:Property ;
	rdfs:label "text" ;
	ns1:domainIncludes ns1:CreativeWork ;
	ns1:rangeIncludes ns1:Text ;
	rdfs:comment "The textual content of this CreativeWork." .

ns1:thumbnail a rdf:Property ;
	rdfs:label "thumbnail" ;
	ns1:domainIncludes ns1:ImageObject , ns1:VideoObject ;
	ns1:rangeIncludes ns1:ImageObject ;
	rdfs:comment "Thumbnail image for an image or video." .

ns1:thumbnailUrl a rdf:Property ;
	rdfs:label "thumbnailUrl" ;
	ns1:domainIncludes ns1:CreativeWork ;
	ns1:rangeIncludes ns1:URL ;
	rdfs:comment "A thumbnail image relevant to the Thing." .

ns1:tickerSymbol a rdf:Property ;
	rdfs:label "tickerSymbol" ;
	ns1:domainIncludes ns1:Corporation ;
	ns1:rangeIncludes ns1:Text ;
	rdfs:comment "The exchange traded instrument associated with a Corporation object. The tickerSymbol is expressed as an exchange and an instrument name separated by a space character. For the exchange component of the tickerSymbol attribute, we reccommend using the controlled vocaulary of Market Identifier Codes (MIC) specified in ISO15022." .

ns1:ticketNumber a rdf:Property ;
	rdfs:label "ticketNumber" ;
	ns1:domainIncludes ns1:Ticket ;
	ns1:rangeIncludes ns1:Text ;
	rdfs:comment "The unique identifier for the ticket." .

ns1:ticketToken a rdf:Property ;
	rdfs:label "ticketToken" ;
	ns1:domainIncludes ns1:Ticket ;
	ns1:rangeIncludes ns1:Text , ns1:URL ;
	rdfs:comment "Reference to an asset (e.g., Barcode, QR code image or PDF) usable for entrance." .

ns1:ticketedSeat a rdf:Property ;
	rdfs:label "ticketedSeat" ;
	ns1:domainIncludes ns1:Ticket ;
	ns1:rangeIncludes ns1:Seat ;
	rdfs:comment "The seat associated with the ticket." .

ns1:timeRequired a rdf:Property ;
	rdfs:label "timeRequired" ;
	ns1:domainIncludes ns1:CreativeWork ;
	ns1:rangeIncludes ns1:Duration ;
	rdfs:comment "Approximate or typical time it takes to work with or through this learning resource for the typical intended target audience, e.g. 'P30M', 'P1H25M'." .

ns1:tissueSample a rdf:Property ;
	rdfs:label "tissueSample" ;
	ns1:domainIncludes ns1:PathologyTest ;
	ns1:rangeIncludes ns1:Text ;
	rdfs:comment "The type of tissue sample required for the test." .

ns1:title a rdf:Property ;
	rdfs:label "title" ;
	ns1:domainIncludes ns1:JobPosting ;
	ns1:rangeIncludes ns1:Text ;
	rdfs:comment "The title of the job." .

ns1:toLocation a rdf:Property ;
	rdfs:label "toLocation" ;
	ns1:domainIncludes ns1:ExerciseAction , ns1:InsertAction , ns1:MoveAction , ns1:TransferAction ;
	ns1:rangeIncludes ns1:Number , ns1:Place ;
	rdfs:comment "A sub property of location. The final location of the object or the agent after the action." ;
	rdfs:subPropertyOf ns1:location .

ns1:totalPrice a rdf:Property ;
	rdfs:label "totalPrice" ;
	ns1:domainIncludes ns1:Reservation , ns1:Ticket ;
	ns1:rangeIncludes ns1:Number , ns1:PriceSpecification , ns1:Text ;
	rdfs:comment "The total price for the reservation or ticket, including applicable taxes, shipping, etc." .

ns1:totalTime a rdf:Property ;
	rdfs:label "totalTime" ;
	ns1:domainIncludes ns1:Recipe ;
	ns1:rangeIncludes ns1:Duration ;
	rdfs:comment "The total time it takes to prepare and cook the recipe, in <a href='http://en.wikipedia.org/wiki/ISO_8601'>ISO 8601 duration format</a>." .

ns1:trackingNumber a rdf:Property ;
	rdfs:label "trackingNumber" ;
	ns1:domainIncludes ns1:ParcelDelivery ;
	ns1:rangeIncludes ns1:Text ;
	rdfs:comment "Shipper tracking number." .

ns1:trackingUrl a rdf:Property ;
	rdfs:label "trackingUrl" ;
	ns1:domainIncludes ns1:ParcelDelivery ;
	ns1:rangeIncludes ns1:URL ;
	rdfs:comment "Tracking url for the parcel delivery." .

ns1:tracks a rdf:Property ;
	rdfs:label "tracks" ;
	ns1:domainIncludes ns1:MusicGroup , ns1:MusicPlaylist ;
	ns1:rangeIncludes ns1:MusicRecording ;
	ns1:supercededBy ns1:track ;
	rdfs:comment "A music recording (track)&#x2014;usually a single song (legacy spelling; see singular form, track)." .

ns1:trailer a rdf:Property ;
	rdfs:label "trailer" ;
	ns1:domainIncludes ns1:Episode , ns1:Movie , ns1:RadioEpisode , ns1:RadioSeason , ns1:RadioSeries , ns1:Season , ns1:Series , ns1:TVEpisode , ns1:TVSeason , ns1:TVSeries ;
	ns1:rangeIncludes ns1:VideoObject ;
	rdfs:comment "The trailer of a movie or tv/radio series, season, or episode." .

ns1:trainName a rdf:Property ;
	rdfs:label "trainName" ;
	ns1:domainIncludes ns1:TrainTrip ;
	ns1:rangeIncludes ns1:Text ;
	rdfs:comment "The name of the train (e.g. The Orient Express)." .

ns1:trainNumber a rdf:Property ;
	rdfs:label "trainNumber" ;
	ns1:domainIncludes ns1:TrainTrip ;
	ns1:rangeIncludes ns1:Text ;
	rdfs:comment "The unique identifier for the train." .

ns1:transFatContent a rdf:Property ;
	rdfs:label "transFatContent" ;
	ns1:domainIncludes ns1:NutritionInformation ;
	ns1:rangeIncludes ns1:Mass ;
	rdfs:comment "The number of grams of trans fat." .

ns1:transcript a rdf:Property ;
	rdfs:label "transcript" ;
	ns1:domainIncludes ns1:AudioObject , ns1:VideoObject ;
	ns1:rangeIncludes ns1:Text ;
	rdfs:comment "If this MediaObject is an AudioObject or VideoObject, the transcript of that object." .

ns1:transmissionMethod a rdf:Property ;
	rdfs:label "transmissionMethod" ;
	ns1:domainIncludes ns1:InfectiousDisease ;
	ns1:rangeIncludes ns1:Text ;
	rdfs:comment "How the disease spreads, either as a route or vector, for example 'direct contact', 'Aedes aegypti', etc." .

ns1:trialDesign a rdf:Property ;
	rdfs:label "trialDesign" ;
	ns1:domainIncludes ns1:MedicalTrial ;
	ns1:rangeIncludes ns1:MedicalTrialDesign ;
	rdfs:comment "Specifics about the trial design (enumerated)." .

ns1:tributary a rdf:Property ;
	rdfs:label "tributary" ;
	ns1:domainIncludes ns1:Vein ;
	ns1:rangeIncludes ns1:AnatomicalStructure ;
	rdfs:comment "The anatomical or organ system that the vein flows into; a larger structure that the vein connects to." .

ns1:typeOfGood a rdf:Property ;
	rdfs:label "typeOfGood" ;
	ns1:domainIncludes ns1:OwnershipInfo , ns1:TypeAndQuantityNode ;
	ns1:rangeIncludes ns1:Product ;
	rdfs:comment "The product that this structured value is referring to." .

ns1:typicalAgeRange a rdf:Property ;
	rdfs:label "typicalAgeRange" ;
	ns1:domainIncludes ns1:CreativeWork , ns1:Event ;
	ns1:rangeIncludes ns1:Text ;
	rdfs:comment "The typical expected age range, e.g. '7-9', '11-'." .

ns1:typicalTest a rdf:Property ;
	rdfs:label "typicalTest" ;
	ns1:domainIncludes ns1:MedicalCondition ;
	ns1:rangeIncludes ns1:MedicalTest ;
	rdfs:comment "A medical test typically performed given this condition." .

ns1:underName a rdf:Property ;
	rdfs:label "underName" ;
	ns1:domainIncludes ns1:Reservation , ns1:Ticket ;
	ns1:rangeIncludes ns1:Organization , ns1:Person ;
	rdfs:comment "The person or organization the reservation or ticket is for." .

ns1:unitCode a rdf:Property ;
	rdfs:label "unitCode" ;
	ns1:domainIncludes ns1:QuantitativeValue , ns1:TypeAndQuantityNode , ns1:UnitPriceSpecification ;
	ns1:rangeIncludes ns1:Text ;
	rdfs:comment "The unit of measurement given using the UN/CEFACT Common Code (3 characters)." .

ns1:unsaturatedFatContent a rdf:Property ;
	rdfs:label "unsaturatedFatContent" ;
	ns1:domainIncludes ns1:NutritionInformation ;
	ns1:rangeIncludes ns1:Mass ;
	rdfs:comment "The number of grams of unsaturated fat." .

ns1:uploadDate a rdf:Property ;
	rdfs:label "uploadDate" ;
	ns1:domainIncludes ns1:MediaObject ;
	ns1:rangeIncludes ns1:Date ;
	rdfs:comment "Date when this media object was uploaded to this site." .

ns1:upvoteCount a rdf:Property ;
	rdfs:label "upvoteCount" ;
	ns1:domainIncludes ns1:Answer , ns1:Comment , ns1:Question ;
	ns1:rangeIncludes ns1:Integer ;
	rdfs:comment "The number of upvotes this question has received from the community." .

ns1:url a rdf:Property ;
	rdfs:label "url" ;
	ns1:domainIncludes ns1:Thing ;
	ns1:rangeIncludes ns1:URL ;
	rdfs:comment "URL of the item." .

ns1:urlTemplate a rdf:Property ;
	rdfs:label "urlTemplate" ;
	ns1:domainIncludes ns1:EntryPoint ;
	ns1:rangeIncludes ns1:Text ;
	rdfs:comment "An url template (RFC6570) that will be used to construct the target of the execution of the action." .

ns1:usedToDiagnose a rdf:Property ;
	rdfs:label "usedToDiagnose" ;
	ns1:domainIncludes ns1:MedicalTest ;
	ns1:rangeIncludes ns1:MedicalCondition ;
	rdfs:comment "A condition the test is used to diagnose." .

ns1:usesDevice a rdf:Property ;
	rdfs:label "usesDevice" ;
	ns1:domainIncludes ns1:MedicalTest ;
	ns1:rangeIncludes ns1:MedicalDevice ;
	rdfs:comment "Device used to perform the test." .

ns1:validFor a rdf:Property ;
	rdfs:label "validFor" ;
	ns1:domainIncludes ns1:Permit ;
	ns1:rangeIncludes ns1:Duration ;
	rdfs:comment "The time validity of the permit." .

ns1:validFrom a rdf:Property ;
	rdfs:label "validFrom" ;
	ns1:domainIncludes ns1:Demand , ns1:Offer , ns1:OpeningHoursSpecification , ns1:Permit , ns1:PriceSpecification ;
	ns1:rangeIncludes ns1:DateTime ;
	rdfs:comment "The date when the item becomes valid." .

ns1:validIn a rdf:Property ;
	rdfs:label "validIn" ;
	ns1:domainIncludes ns1:Permit ;
	ns1:rangeIncludes ns1:AdministrativeArea ;
	rdfs:comment "The geographic area where the permit is valid." .

ns1:validThrough a rdf:Property ;
	rdfs:label "validThrough" ;
	ns1:domainIncludes ns1:Demand , ns1:Offer , ns1:OpeningHoursSpecification , ns1:PriceSpecification ;
	ns1:rangeIncludes ns1:DateTime ;
	rdfs:comment "The end of the validity of offer, price specification, or opening hours data." .

ns1:validUntil a rdf:Property ;
	rdfs:label "validUntil" ;
	ns1:domainIncludes ns1:Permit ;
	ns1:rangeIncludes ns1:Date ;
	rdfs:comment "The date when the item is no longer valid." .

ns1:value a rdf:Property ;
	rdfs:label "value" ;
	ns1:domainIncludes ns1:QuantitativeValue ;
	ns1:rangeIncludes ns1:Number ;
	rdfs:comment "The value of the product characteristic." .

ns1:valueAddedTaxIncluded a rdf:Property ;
	rdfs:label "valueAddedTaxIncluded" ;
	ns1:domainIncludes ns1:PriceSpecification ;
	ns1:rangeIncludes ns1:Boolean ;
	rdfs:comment "Specifies whether the applicable value-added tax (VAT) is included in the price specification or not." .

ns1:valueMaxLength a rdf:Property ;
	rdfs:label "valueMaxLength" ;
	ns1:domainIncludes ns1:PropertyValueSpecification ;
	ns1:rangeIncludes ns1:Number ;
	rdfs:comment "Specifies the allowed range for number of characters in a literal value." .

ns1:valueMinLength a rdf:Property ;
	rdfs:label "valueMinLength" ;
	ns1:domainIncludes ns1:PropertyValueSpecification ;
	ns1:rangeIncludes ns1:Number ;
	rdfs:comment "Specifies the minimum allowed range for number of characters in a literal value." .

ns1:valueName a rdf:Property ;
	rdfs:label "valueName" ;
	ns1:domainIncludes ns1:PropertyValueSpecification ;
	ns1:rangeIncludes ns1:Text ;
	rdfs:comment "Indicates the name of the PropertyValueSpecification to be used in URL templates and form encoding in a manner analogous to HTML's input@name." .

ns1:valuePattern a rdf:Property ;
	rdfs:label "valuePattern" ;
	ns1:domainIncludes ns1:PropertyValueSpecification ;
	ns1:rangeIncludes ns1:Number ;
	rdfs:comment "Specifies a regular expression for testing literal values according to the HTML spec." .

ns1:valueReference a rdf:Property ;
	rdfs:label "valueReference" ;
	ns1:domainIncludes ns1:QualitativeValue , ns1:QuantitativeValue ;
	ns1:rangeIncludes ns1:Enumeration , ns1:StructuredValue ;
	rdfs:comment "A pointer to a secondary value that provides additional information on the original value, e.g. a reference temperature." .

ns1:valueRequired a rdf:Property ;
	rdfs:label "valueRequired" ;
	ns1:domainIncludes ns1:PropertyValueSpecification ;
	ns1:rangeIncludes ns1:Boolean ;
	rdfs:comment "Whether the property must be filled in to complete the action.  Default is false." .

ns1:vatID a rdf:Property ;
	rdfs:label "vatID" ;
	ns1:domainIncludes ns1:Organization , ns1:Person ;
	ns1:rangeIncludes ns1:Text ;
	rdfs:comment "The Value-added Tax ID of the organization or person." .

ns1:vendor a rdf:Property ;
	rdfs:label "vendor" ;
	ns1:domainIncludes ns1:BuyAction ;
	ns1:rangeIncludes ns1:Organization , ns1:Person ;
	rdfs:comment "A sub property of participant. The seller. The participant/person/organization that sold the object." ;
	rdfs:subPropertyOf ns1:participant .

ns1:version a rdf:Property ;
	rdfs:label "version" ;
	ns1:domainIncludes ns1:CreativeWork ;
	ns1:rangeIncludes ns1:Number ;
	rdfs:comment "The version of the CreativeWork embodied by a specified resource." .

ns1:video a rdf:Property ;
	rdfs:label "video" ;
	ns1:domainIncludes ns1:CreativeWork ;
	ns1:rangeIncludes ns1:VideoObject ;
	rdfs:comment "An embedded video object." .

ns1:videoFrameSize a rdf:Property ;
	rdfs:label "videoFrameSize" ;
	ns1:domainIncludes ns1:VideoObject ;
	ns1:rangeIncludes ns1:Text ;
	rdfs:comment "The frame size of the video." .

ns1:videoQuality a rdf:Property ;
	rdfs:label "videoQuality" ;
	ns1:domainIncludes ns1:VideoObject ;
	ns1:rangeIncludes ns1:Text ;
	rdfs:comment "The quality of the video." .

ns1:warning a rdf:Property ;
	rdfs:label "warning" ;
	ns1:domainIncludes ns1:Drug ;
	ns1:rangeIncludes ns1:Text , ns1:URL ;
	rdfs:comment "Any FDA or other warnings about the drug (text or URL)." .

ns1:warranty a rdf:Property ;
	rdfs:label "warranty" ;
	ns1:domainIncludes ns1:Demand , ns1:Offer ;
	ns1:rangeIncludes ns1:WarrantyPromise ;
	rdfs:comment "The warranty promise(s) included in the offer." .

ns1:warrantyPromise a rdf:Property ;
	rdfs:label "warrantyPromise" ;
	ns1:domainIncludes ns1:BuyAction , ns1:SellAction ;
	ns1:rangeIncludes ns1:WarrantyPromise ;
	rdfs:comment "The warranty promise(s) included in the offer." .

ns1:warrantyScope a rdf:Property ;
	rdfs:label "warrantyScope" ;
	ns1:domainIncludes ns1:WarrantyPromise ;
	ns1:rangeIncludes ns1:WarrantyScope ;
	rdfs:comment "The scope of the warranty promise." .

ns1:webCheckinTime a rdf:Property ;
	rdfs:label "webCheckinTime" ;
	ns1:domainIncludes ns1:Flight ;
	ns1:rangeIncludes ns1:DateTime ;
	rdfs:comment "The time when a passenger can check into the flight online." .

ns1:weight a rdf:Property ;
	rdfs:label "weight" ;
	ns1:domainIncludes ns1:Product ;
	ns1:rangeIncludes ns1:QuantitativeValue ;
	rdfs:comment "The weight of the product." .

ns1:width a rdf:Property ;
	rdfs:label "width" ;
	ns1:domainIncludes ns1:MediaObject , ns1:Product ;
	ns1:rangeIncludes ns1:Distance , ns1:QuantitativeValue ;
	rdfs:comment "The width of the item." .

ns1:winner a rdf:Property ;
	rdfs:label "winner" ;
	ns1:domainIncludes ns1:LoseAction ;
	ns1:rangeIncludes ns1:Person ;
	rdfs:comment "A sub property of participant. The winner of the action." ;
	rdfs:subPropertyOf ns1:participant .

ns1:wordCount a rdf:Property ;
	rdfs:label "wordCount" ;
	ns1:domainIncludes ns1:Article ;
	ns1:rangeIncludes ns1:Integer ;
	rdfs:comment "The number of words in the text of the Article." .

ns1:workHours a rdf:Property ;
	rdfs:label "workHours" ;
	ns1:domainIncludes ns1:JobPosting ;
	ns1:rangeIncludes ns1:Text ;
	rdfs:comment "The typical working hours for this job (e.g. 1st shift, night shift, 8am-5pm)." .

ns1:workLocation a rdf:Property ;
	rdfs:label "workLocation" ;
	ns1:domainIncludes ns1:Person ;
	ns1:rangeIncludes ns1:ContactPoint , ns1:Place ;
	rdfs:comment "A contact location for a person's place of work." .

ns1:workPerformed a rdf:Property ;
	rdfs:label "workPerformed" ;
	ns1:domainIncludes ns1:Event ;
	ns1:rangeIncludes ns1:CreativeWork ;
	rdfs:comment "A work performed in some event, for example a play performed in a TheaterEvent." .

ns1:workload a rdf:Property ;
	rdfs:label "workload" ;
	ns1:domainIncludes ns1:ExercisePlan ;
	ns1:rangeIncludes ns1:Energy ;
	rdfs:comment "Quantitative measure of the physiologic output of the exercise; also referred to as energy expenditure." .

ns1:worksFor a rdf:Property ;
	rdfs:label "worksFor" ;
	ns1:domainIncludes ns1:Person ;
	ns1:rangeIncludes ns1:Organization ;
	rdfs:comment "Organizations that the person works for." .

ns1:worstRating a rdf:Property ;
	rdfs:label "worstRating" ;
	ns1:domainIncludes ns1:Rating ;
	ns1:rangeIncludes ns1:Number , ns1:Text ;
	rdfs:comment "The lowest value allowed in this rating system. If worstRating is omitted, 1 is assumed." .

ns1:yearlyRevenue a rdf:Property ;
	rdfs:label "yearlyRevenue" ;
	ns1:domainIncludes ns1:BusinessAudience ;
	ns1:rangeIncludes ns1:QuantitativeValue ;
	rdfs:comment "The size of the business in annual revenue." .

ns1:yearsInOperation a rdf:Property ;
	rdfs:label "yearsInOperation" ;
	ns1:domainIncludes ns1:BusinessAudience ;
	ns1:rangeIncludes ns1:QuantitativeValue ;
	rdfs:comment "The age of the business." .

ns1:actor a rdf:Property ;
	rdfs:label "actor" ;
	ns1:domainIncludes ns1:Episode , ns1:Movie , ns1:RadioEpisode , ns1:RadioSeries , ns1:Series , ns1:TVEpisode , ns1:TVSeries ;
	ns1:rangeIncludes ns1:Person ;
	rdfs:comment "A cast member of the movie, tv/radio series, season, episode, or video." .

ns1:album a rdf:Property ;
	rdfs:label "album" ;
	ns1:domainIncludes ns1:MusicGroup ;
	ns1:rangeIncludes ns1:MusicAlbum ;
	rdfs:comment "A music album." .

ns1:alumni a rdf:Property ;
	rdfs:label "alumni" ;
	ns1:domainIncludes ns1:EducationalOrganization ;
	ns1:inverseOf ns1:alumniOf ;
	ns1:rangeIncludes ns1:Person ;
	rdfs:comment "Alumni of educational organization." .

ns1:alumniOf a rdf:Property ;
	rdfs:label "alumniOf" ;
	ns1:domainIncludes ns1:Person ;
	ns1:inverseOf ns1:alumni ;
	ns1:rangeIncludes ns1:EducationalOrganization ;
	rdfs:comment "An educational organizations that the person is an alumni of." .

ns1:attendees a rdf:Property ;
	rdfs:label "attendees" ;
	ns1:domainIncludes ns1:Event ;
	ns1:rangeIncludes ns1:Organization , ns1:Person ;
	ns1:supercededBy ns1:attendees ;
	rdfs:comment "A person attending the event (legacy spelling; see singular form, attendee)." .

ns1:award a rdf:Property ;
	rdfs:label "award" ;
	ns1:domainIncludes ns1:CreativeWork , ns1:Person ;
	ns1:rangeIncludes ns1:Text ;
	rdfs:comment "An award won by this person or for this creative work." .

ns1:blogPost a rdf:Property ;
	rdfs:label "blogPost" ;
	ns1:domainIncludes ns1:Blog ;
	ns1:rangeIncludes ns1:BlogPosting ;
	rdfs:comment "A posting that is part of this blog." .

ns1:colleague a rdf:Property ;
	rdfs:label "colleague" ;
	ns1:domainIncludes ns1:Person ;
	ns1:rangeIncludes ns1:Person ;
	rdfs:comment "A colleague of the person." .

ns1:contactPoint a rdf:Property ;
	rdfs:label "contactPoint" ;
	ns1:domainIncludes ns1:Organization , ns1:Person ;
	ns1:rangeIncludes ns1:ContactPoint ;
	rdfs:comment "A contact point for a person or organization." .

ns1:director a rdf:Property ;
	rdfs:label "director" ;
	ns1:domainIncludes ns1:Episode , ns1:Movie , ns1:RadioEpisode , ns1:RadioSeries , ns1:Series , ns1:TVEpisode , ns1:TVSeries ;
	ns1:rangeIncludes ns1:Person ;
	rdfs:comment "The director of the movie, tv/radio episode or series." .

ns1:employee a rdf:Property ;
	rdfs:label "employee" ;
	ns1:domainIncludes ns1:Organization ;
	ns1:rangeIncludes ns1:Person ;
	rdfs:comment "Someone working for this organization." .

ns1:encoding a rdf:Property ;
	rdfs:label "encoding" ;
	ns1:domainIncludes ns1:CreativeWork ;
	ns1:rangeIncludes ns1:MediaObject ;
	rdfs:comment "A media object that encode this CreativeWork." .

ns1:episode a rdf:Property ;
	rdfs:label "episode" ;
	ns1:domainIncludes ns1:RadioSeason , ns1:RadioSeries , ns1:Season , ns1:Series , ns1:TVSeason , ns1:TVSeries ;
	ns1:rangeIncludes ns1:Episode ;
	rdfs:comment "An episode of a TV/radio series or season" .

ns1:event a rdf:Property ;
	rdfs:label "event" ;
	ns1:domainIncludes ns1:InformAction , ns1:InviteAction , ns1:JoinAction , ns1:LeaveAction , ns1:Organization , ns1:Place , ns1:PlayAction ;
	ns1:rangeIncludes ns1:Event ;
	rdfs:comment "Upcoming or past event associated with this place or organization." .

ns1:founder a rdf:Property ;
	rdfs:label "founder" ;
	ns1:domainIncludes ns1:Organization ;
	ns1:rangeIncludes ns1:Person ;
	rdfs:comment "A person who founded this organization." .

ns1:map a rdf:Property ;
	rdfs:label "map" ;
	ns1:domainIncludes ns1:Place ;
	ns1:rangeIncludes ns1:URL ;
	rdfs:comment "A URL to a map of the place." .

ns1:memberOf a rdf:Property ;
	rdfs:label "memberOf" ;
	ns1:domainIncludes ns1:Organization , ns1:Person ;
	ns1:inverseOf ns1:member ;
	ns1:rangeIncludes ns1:Organization , ns1:ProgramMembership ;
	rdfs:comment "An Organization (or ProgramMembership) to which this Person or Organization belongs." .

ns1:muscleAction a rdf:Property ;
	rdfs:label "muscleAction" ;
	ns1:domainIncludes ns1:Muscle ;
	ns1:rangeIncludes ns1:Text ;
	rdfs:comment "The movement the muscle generates." .

ns1:parent a rdf:Property ;
	rdfs:label "parent" ;
	ns1:domainIncludes ns1:Person ;
	ns1:rangeIncludes ns1:Person ;
	rdfs:comment "A parent of this person." .

ns1:partOfSeries a rdf:Property ;
	rdfs:label "partOfSeries" ;
	ns1:domainIncludes ns1:Clip , ns1:Episode , ns1:RadioClip , ns1:RadioEpisode , ns1:RadioSeason , ns1:Season , ns1:TVClip , ns1:TVEpisode , ns1:TVSeason ;
	ns1:rangeIncludes ns1:Series ;
	rdfs:comment "The series to which this episode or season belongs." .

ns1:performer a rdf:Property ;
	rdfs:label "performer" ;
	ns1:domainIncludes ns1:Event ;
	ns1:rangeIncludes ns1:Organization , ns1:Person ;
	rdfs:comment "A performer at the event&#x2014;for example, a presenter, musician, musical group or actor." .

ns1:photo a rdf:Property ;
	rdfs:label "photo" ;
	ns1:domainIncludes ns1:Place ;
	ns1:rangeIncludes ns1:ImageObject , ns1:Photograph ;
	rdfs:comment "A photograph of this place." .

ns1:result a rdf:Property ;
	rdfs:label "result" ;
	ns1:domainIncludes ns1:Action ;
	ns1:rangeIncludes ns1:Thing ;
	rdfs:comment "The result produced in the action. e.g. John wrote *a book*." .

ns1:review a rdf:Property ;
	rdfs:label "review" ;
	ns1:domainIncludes ns1:CreativeWork , ns1:Offer , ns1:Organization , ns1:Place , ns1:Product ;
	ns1:rangeIncludes ns1:Review ;
	rdfs:comment "A review of the item." .

ns1:season a rdf:Property ;
	rdfs:label "season" ;
	ns1:domainIncludes ns1:RadioSeries , ns1:Series , ns1:TVSeries ;
	ns1:rangeIncludes ns1:Season ;
	rdfs:comment "A season in a tv/radio series." .

ns1:sibling a rdf:Property ;
	rdfs:label "sibling" ;
	ns1:domainIncludes ns1:Person ;
	ns1:rangeIncludes ns1:Person ;
	rdfs:comment "A sibling of the person." .

ns1:significantLink a rdf:Property ;
	rdfs:label "significantLink" ;
	ns1:domainIncludes ns1:WebPage ;
	ns1:rangeIncludes ns1:URL ;
	rdfs:comment "One of the more significant URLs on the page. Typically, these are the non-navigation links that are clicked on the most." .

ns1:subEvent a rdf:Property ;
	rdfs:label "subEvent" ;
	ns1:domainIncludes ns1:Event ;
	ns1:rangeIncludes ns1:Event ;
	rdfs:comment "An Event that is part of this event. For example, a conference event includes many presentations, each of which is a subEvent of the conference." .

ns1:suggestedAnswer a rdf:Property ;
	rdfs:label "suggestedAnswer" ;
	ns1:domainIncludes ns1:Question ;
	ns1:rangeIncludes ns1:Answer ;
	rdfs:comment "An answer (possibly one of several, possibly incorrect) to a Question, e.g. on a Question/Answer site." .

ns1:track a rdf:Property ;
	rdfs:label "track" ;
	ns1:domainIncludes ns1:MusicGroup , ns1:MusicPlaylist ;
	ns1:rangeIncludes ns1:MusicRecording ;
	rdfs:comment "A music recording (track)&#x2014;usually a single song." .

<http://www.w3.org/wiki/WebSchemas/SchemaDotOrgSources#source_GoodRelationsProperties> a ns1:Organization ;
	rdfs:label "GoodRelationsProperties" ;
	rdfs:comment "This class contains derivatives of properties from the GoodRelations Vocabulary for E-Commerce, created by Martin Hepp. GoodRelations is a data model for sharing e-commerce data on the Web that can be expressed in a variety of syntaxes, including RDFa and HTML5 Microdata. More information about GoodRelations can be found at <a href=\"http://purl.org/goodrelations/\">http://purl.org/goodrelations/</a>." .

<http://www.w3.org/wiki/WebSchemas/SchemaDotOrgSources#source_LRMIClass> a ns1:Organization ;
	rdfs:label "LRMIClass" ;
	rdfs:comment "This class is based on the work of the LRMI project, see lrmi.net for details." .

<http://www.w3.org/wiki/WebSchemas/SchemaDotOrgSources#source_QAStackExchange> a ns1:Organization ;
	rdfs:label "Stack Exchange" ;
	rdfs:comment "The Question/Answer types were <a href=\"https://www.w3.org/wiki/WebSchemas/QASchemaResearch\">based on</a> the Stack Overflow API." .

ns1:member a rdf:Property ;
	rdfs:label "member" ;
	ns1:domainIncludes ns1:Organization , ns1:ProgramMembership ;
	ns1:inverseOf ns1:memberOf ;
	ns1:rangeIncludes ns1:Organization , ns1:Person ;
	rdfs:comment "A member of an Organization or a ProgramMembership. Organizations can be members of organizations; ProgramMembership is typically for individuals." .

<http://www.w3.org/wiki/WebSchemas/SchemaDotOrgSources#source_ActionCollabClass> a ns1:Organization ;
	rdfs:label "ActionCollabClass" ;
	rdfs:comment "The schema.org Actions mechanism benefited from extensive discussions across the Web standards community around W3C, in particular from the <a href=\"http://purl.org/hydra/\"> Hydra project</a>'s community group." .

<http://www.w3.org/wiki/WebSchemas/SchemaDotOrgSources#source_DatasetClass> a ns1:Organization ;
	rdfs:label "DatasetClass" ;
	rdfs:comment "This class is based upon W3C DCAT work, and benefits from collaboration around the DCAT, ADMS and VoID vocabularies. See http://www.w3.org/wiki/WebSchemas/Datasets for full details and mappings." .

ns1:instrument a rdf:Property ;
	rdfs:label "instrument" ;
	ns1:domainIncludes ns1:Action ;
	ns1:rangeIncludes ns1:Thing ;
	rdfs:comment "The object that helped the agent perform the action. e.g. John wrote a book with *a pen*." .

ns1:object a rdf:Property ;
	rdfs:label "object" ;
	ns1:domainIncludes ns1:Action ;
	ns1:rangeIncludes ns1:Thing ;
	rdfs:comment "The object upon the action is carried out, whose state is kept intact or changed. Also known as the semantic roles patient, affected or undergoer (which change their state) or theme (which doesn't). e.g. John read *a book*." .

ns1:location a rdf:Property ;
	rdfs:label "location" ;
	ns1:domainIncludes ns1:Action , ns1:Event , ns1:Organization ;
	ns1:rangeIncludes ns1:Place , ns1:PostalAddress ;
	rdfs:comment "The location of the event, organization or action." .

<http://www.w3.org/wiki/WebSchemas/SchemaDotOrgSources#source_rNews> a ns1:Organization ;
	rdfs:label "rNews" ;
	rdfs:comment "This class contains derivatives of IPTC rNews properties. rNews is a data model of publishing metadata with serializations currently available for RDFa as well as HTML5 Microdata. More information about the IPTC and rNews can be found at <a href=http://rnews.org>rnews.org</a>." .

ns1:participant a rdf:Property ;
	rdfs:label "participant" ;
	ns1:domainIncludes ns1:Action ;
	ns1:rangeIncludes ns1:Organization , ns1:Person ;
	rdfs:comment "Other co-agents that participated in the action indirectly. e.g. John wrote a book with *Steve*." .

<http://www.w3.org/wiki/WebSchemas/SchemaDotOrgSources#source_GoodRelationsClass> a ns1:Organization ;
	rdfs:label "GoodRelationsClass" ;
	rdfs:comment "This class is derived from the GoodRelations Vocabulary for E-Commerce, created by Martin Hepp. GoodRelations is a data model for sharing e-commerce data on the Web that can be expressed in a variety of syntaxes, including RDFa and HTML5 Microdata. More information about GoodRelations can be found at <a href=\"http://purl.org/goodrelations/\">http://purl.org/goodrelations/</a>." .

<http://www.w3.org/wiki/WebSchemas/SchemaDotOrgSources#source_WikiDoc> a ns1:Organization ;
	rdfs:label "WikiDoc" ;
	rdfs:comment "This class contains information contributed by <a href=http://wikidoc.org>WikiDoc</a>." .
