@prefix : <http://zbw.eu/namespaces/zbw-extensions/> .
@prefix dc: <http://purl.org/dc/elements/1.1/> .
@prefix rdfs: <http://www.w3.org/2000/01/rdf-schema#> .
@prefix owl2xml: <http://www.w3.org/2006/12/owl2-xml#> .
@prefix owl: <http://www.w3.org/2002/07/owl#> .
@prefix xsd: <http://www.w3.org/2001/XMLSchema#> .
@prefix rdf: <http://www.w3.org/1999/02/22-rdf-syntax-ns#> .
@prefix skos: <http://www.w3.org/2004/02/skos/core#> .
@prefix dcterms: <http://purl.org/dc/terms/> .

<http://zbw.eu/namespaces/zbw-extensions/> dc:title "Extensions to SKOS and other standard vocabularies used by the German National Library of Economics (ZBW)"@en ;
	dc:creator "Joachim Neubert" ;
	dc:publisher "German National Library of Economics (ZBW)"@en ;
	dcterms:created "2010-04-28" ;
	dcterms:modified "2012-07-24" .

:Descriptor a owl:Class ;
	rdfs:label "Descriptor"@en ;
	rdfs:isDefinedBy <http://zbw.eu/namespaces/zbw-extensions/zbw-extensions.rdf> ;
	rdfs:subClassOf skos:Concept ;
	skos:definition "The descriptors part of the STW."@en ;
	rdfs:comment """Among themselves, the Descriptor entries are 
    linked in multiple skos:broader/skos:narrower hierarchies and skos:related 
    connections. To Thsys entries, only skos:broader connections are
    allowed."""@en .

:Thsys a owl:Class ;
	rdfs:label "Thsys"@en ;
	rdfs:isDefinedBy <http://zbw.eu/namespaces/zbw-extensions/zbw-extensions.rdf> ;
	rdfs:subClassOf skos:Concept ;
	skos:definition """The systematic part (subject categories) 
    of the STW."""@en ;
	rdfs:comment """Each entry has a rdfs:label property for each 
    supported language and one skos:notation property. skos:prefLabel 
    properties are generated by concatenation of these properties. 
    Among themselves, the thsys entries are linked in several
    skos:broader/skos:narrower mono-hierarchies under a top-level 
    \"Subthesaurus\" Thsys concept. To Descriptor entities, only skos:narrower 
    connections are allowed."""@en .

:useInsteadNote a owl:AnnotationProperty ;
	rdfs:label "useInsteadNote"@en ;
	rdfs:isDefinedBy <http://zbw.eu/namespaces/zbw-extensions/zbw-extensions.rdf> ;
	rdfs:subPropertyOf skos:note ;
	skos:definition """For an aspect of the current concept use the 
    concept to which the note points instead of the current."""@en ;
	rdfs:comment """The note consists of a blank node. It contains 
    a rdfs:value literal which designates the aspect and a rdfs:seeAlso link to 
    the concept which should be used instead."""@en .

:indexedItem a owl:ObjectProperty ;
	rdfs:label "indexedItem"@en ;
	rdfs:isDefinedBy <http://zbw.eu/namespaces/zbw-extensions/zbw-extensions.rdf> ;
	rdfs:subPropertyOf rdfs:seeAlso ;
	skos:definition """The concept is used as an index term or subject 
    for the resource."""@en ;
	rdfs:comment """A substitute for the vanished skos:isSubjectOf. 
    May be used with collections of resources also."""@en .

:econbizCount a owl:FunctionalProperty ;
	rdfs:label "econbizCount"@en ;
	rdfs:isDefinedBy <http://zbw.eu/namespaces/zbw-extensions/zbw-extensions.rdf> ;
	rdfs:subPropertyOf <http://rdf.myexperiment.org/ontologies/base/count> ;
	skos:definition """Count of matching items in EconBiz (virtual library 
    for economics and business studies, http://econbiz.eu)."""@en .
