@prefix rdf: <http://www.w3.org/1999/02/22-rdf-syntax-ns#> .
@prefix vann: <http://purl.org/vocab/vann/> .
@prefix skosxl: <http://www.w3.org/2008/05/skos-xl#> .
@prefix muninn: <http://rdf.muninn-project.org/ontologies/muninn#> .
@prefix foaf: <http://xmlns.com/foaf/0.1/> .
@prefix dbpedia: <http://dbpedia.org/resource/> .
@prefix time: <http://www.w3.org/2006/time#> .
@prefix cc: <http://creativecommons.org/ns#> .
@prefix nif: <http://persistence.uni-leipzig.org/nlp2rdf/ontologies/nif-core#> .
@prefix as: <http://www.w3.org/ns/activitystreams#> .
@prefix oa: <http://www.w3.org/ns/oa#> .
@prefix skos: <http://www.w3.org/2004/02/skos/core#> .
@prefix prov: <http://www.w3.org/ns/prov#> .
@prefix owl: <http://www.w3.org/2002/07/owl#> .
@prefix xsd: <http://www.w3.org/2001/XMLSchema#> .
@prefix vs: <http://www.w3.org/2003/06/sw-vocab-status/ns#> .
@prefix swrl: <http://www.w3.org/2003/11/swrl#> .
@prefix doap: <http://usefulinc.com/ns/doap#> .
@prefix dcterms: <http://purl.org/dc/terms/> .
@prefix void: <http://rdfs.org/ns/void#> .
@prefix swrlb: <http://www.w3.org/2003/11/swrlb#> .
@prefix loc: <http://id.loc.gov/vocabulary/relators/> .
@prefix rdfs: <http://www.w3.org/2000/01/rdf-schema#> .
@prefix cwrc: <http://www.cwrc.ca/ontologies/cwrc#> .

<http://www.cwrc.ca/ontologies/cwrc>
    loc:ctb cwrc:ConstanceCrompton ;
    loc:fnd cwrc:sshrc ;
    loc:pdr cwrc:SusanBrown ;
    dcterms:creator cwrc:AbigelLemak, cwrc:ColinFaulkner, cwrc:JohnSimpson, cwrc:RobWarren ;
    dcterms:date "20170319"^^xsd:date ;
    dcterms:description "L'Ontologie CWRC est l'ontologie maîtresse qui représente tous les éléments de la structure du Collaboratoire scientifique des écrits du Canada."@fr, "The CWRC Ontology is the overall ontology that represents all elements of structure within the Canadian Writing Research Collaboratory."@en ;
    dcterms:publisher cwrc:cwrc ;
    dcterms:rights <http://creativecommons.org/licenses/by-nc/4.0/> ;
    dcterms:subject <http://id.loc.gov/authorities/subjects/sh2009007122>, <http://id.loc.gov/authorities/subjects/sh85013838>, <http://id.loc.gov/authorities/subjects/sh85019388>, <http://id.loc.gov/authorities/subjects/sh85043777>, <http://id.loc.gov/authorities/subjects/sh85077519> ;
    dcterms:title "L'Ontologie CWRC"@fr, "The CWRC Ontology"@en ;
    vann:preferredNamespacePrefix "cwrc" ;
    void:inDataset cwrc:datasetdefinition ;
    a owl:Ontology ;
    rdfs:comment "L'Ontologie CWRC est l'ontologie maîtresse qui représente tous les éléments de la structure du Collaboratoire scientifique des écrits du Canada."@fr, "The CWRC Ontology is the overall ontology that represents all elements of structure within the Canadian Writing Research Collaboratory."@en ;
    rdfs:label "L'Ontologie CWRC"@fr, "The CWRC Ontology"@en ;
    owl:priorVersion <http://www.cwrc.ca/ontologies/cwrc> ;
    owl:versionInfo 0.99 ;
    vs:term_status "Testing"@en ;
    skos:definition "L'Ontologie CWRC est l'ontologie maîtresse qui représente tous les éléments de la structure du Collaboratoire scientifique des écrits du Canada."@fr, "The CWRC Ontology is the overall ontology that represents all elements of structure within the Canadian Writing Research Collaboratory."@en ;
    foaf:logo <http://www.cwrc.ca/wp-content/uploads/2010/11/CWRC_logo_v074.gif> ;
    foaf:name "L'Ontologie CWRC"@fr, "The CWRC Ontology"@en .

cwrc:AbigelLemak
    a foaf:Person ;
    foaf:name "Abigel Lemak" .

cwrc:Actor
    void:inDataset cwrc:datasetdefinition ;
    a owl:Class, skos:Concept ;
    rdfs:comment "A person performing a certain role within an event."@en ;
    rdfs:isDefinedBy <https://raw.githubusercontent.com/cwrc/OrlandoOntology/master/OrlandoOntology#> ;
    rdfs:label "Actor"@en ;
    owl:sameAs <http://erlangen-crm.org/current/E39.Actor> .

cwrc:Address
    void:inDataset cwrc:datasetdefinition ;
    a owl:Class, skos:Concept ;
    rdfs:comment "The postal address is the equivalent of a schema.org address and inherits all of the data from that vocabulary to markup a modern postral address."@en ;
    rdfs:isDefinedBy <http://www.cwrc.ca/ontologies/OrlandoOntology#> ;
    rdfs:label "address"@en, "adresse"@fr ;
    rdfs:subClassOf cwrc:Place ;
    owl:sameAs <http://schema.org/PostalAddress> ;
    skos:definition "A mailling or street address."@en, "Une adresse postale ou de rue."@fr .

cwrc:Androgynous
    void:inDataset cwrc:datasetdefinition ;
    a owl:Class, skos:Concept ;
    rdfs:isDefinedBy <http://www.cwrc.ca/ontologies/cwrc#> ;
    rdfs:label "Androgyne"@fr, "Androgynous"@en .

cwrc:CisGendered
    void:inDataset cwrc:datasetdefinition ;
    a owl:Class, skos:Concept ;
    rdfs:isDefinedBy <http://www.cwrc.ca/ontologies/cwrc#> ;
    rdfs:label "Cisgenre"@fr, "cisGendered"@en ;
    owl:differentFrom cwrc:Transgender ;
    owl:sameAs dbpedia:Cisgender ;
    owl:subClass cwrc:CulturalFormation ;
    skos:definition ""@fr, "Indicates alignment between a person's gender identity and their sex as understood or assigned at birth."@en .

cwrc:ColinFaulkner
    a foaf:Person ;
    foaf:name "Colin Faulkner" .

cwrc:ConstanceCrompton
    a foaf:Person ;
    foaf:name "Constance Crompton" .

cwrc:Context
    void:inDataset cwrc:datasetdefinition ;
    a owl:Class, skos:Concept, oa:Annotation ;
    rdfs:isDefinedBy <http://www.cwrc.ca/ontologies/cwrc#> ;
    rdfs:label "Context"@en, "Contexte"@fr ;
    skos:definition ""@fr, "A context relates.... "@en .

cwrc:CulturalFormation
    void:inDataset cwrc:datasetdefinition ;
    a owl:Class, skos:Concept ;
    rdfs:isDefinedBy <http://www.cwrc.ca/ontologies/cwrc#> ;
    rdfs:label "Cultural Formation"@en, "Formation Culturelle"@fr ;
    skos:definition ""@fr, "Cultural formation refers to the processes of lived social subjectivities of people and is often combined with predicates indicating the identity positions as they relate to the following discursive constructions of Class, Denomination, Ethnicity, Gender, GeographicalHeritage, Language, NationalHeritage, NationalIdentity, PoliticalAffiliation, RaceColour, SexualIdentity. These categories are not understood as transhistorical or isolated categories. Rather, they facilitate analysis of howfor a particular individual. It is our hope that modes of classification never occur without a sense of responsibility, and that the tensions inherently present during the practice of classification are never eased but rather challenged and engaged with critically."@en .

cwrc:EnglishLanguage
    void:inDataset cwrc:datasetdefinition ;
    a cwrc:Language, owl:Thing, skos:Concept ;
    rdfs:isDefinedBy <http://www.cwrc.ca/ontologies/cwrc#> ;
    rdfs:label "Anglais"@fr, "English"@en ;
    skos:definition ""@en, ""@fr .

cwrc:EnglishNationalHeritage
    void:inDataset cwrc:datasetdefinition ;
    a cwrc:NationalHeritage, owl:Thing, skos:Concept ;
    rdfs:isDefinedBy <http://www.cwrc.ca/ontologies/cwrc#> ;
    rdfs:label "Anglaise"@fr, "English"@en ;
    skos:definition ""@en, ""@fr .

cwrc:EnglishNationalIdentity
    void:inDataset cwrc:datasetdefinition ;
    a cwrc:NationalIdentity, owl:Thing, skos:Concept ;
    rdfs:isDefinedBy <http://www.cwrc.ca/ontologies/cwrc#> ;
    rdfs:label "Anglaise"@fr, "English"@en ;
    skos:definition ""@en, ""@fr .

cwrc:Ethnicity
    void:inDataset cwrc:datasetdefinition ;
    a owl:Class, skos:Concept ;
    rdfs:isDefinedBy <http://www.cwrc.ca/ontologies/cwrc#> ;
    rdfs:label "Ethnicity"@en, "Ethnicité"@fr ;
    owl:subClass cwrc:CulturalFormation ;
    skos:definition ""@fr, "Ethnicity is a subclass of CulturalFormation that captures information about a person's ethnic position. Ethnicity is a sub-element within culturalFormation and raceAndEthnicity. See raceAndEthnicity for a detailed description of the complexities of this discursive construction and the social practices surrounding it."@en .

cwrc:EthnicityContext
    dcterms:subject cwrc:Ethnicity, cwrc:RaceColour ;
    void:inDataset cwrc:datasetdefinition ;
    a owl:Class, skos:Concept ;
    rdfs:isDefinedBy <http://www.cwrc.ca/ontologies/cwrc#> ;
    rdfs:label "Contexte Raciale, de Couleur de Peau ou d'ethnicité"@fr, "Racial, Colour or Ethnicity Context"@en ;
    owl:subClass cwrc:Context ;
    skos:definition ""@en, ""@fr .

cwrc:Event
    void:inDataset cwrc:datasetdefinition ;
    a owl:Class, skos:Concept, <http://www.w3.org/2006/time/TemporalEntity> ;
    rdfs:isDefinedBy <https://raw.githubusercontent.com/cwrc/OrlandoOntology/master/OrlandoOntology#> ;
    rdfs:label "Event"@de, "Event (Historical)"@en, "Évenement (Historique)"@fr ;
    owl:sameAs <http://en.wikipedia.org/wiki/Event>, <http://erlangen-crm.org/current/E5.Event>, <http://linkedevents.org/ontology/Event> ;
    skos:definition "An event that occurs in space and time."@en ;
    foaf:name "Event" .

cwrc:FemaleLabel
    void:inDataset cwrc:datasetdefinition ;
    a skos:Concept, skosxl:Label ;
    rdf:value "female" ;
    rdfs:isDefinedBy <http://www.cwrc.ca/ontologies/cwrc#> ;
    rdfs:label "Female"@en, "Femelle"@fr ;
    owl:oneOf (cwrc:genderWomanFemale
        cwrc:femaleSex
    ) ;
    skos:definition ""@en, ""@fr ;
    skos:inScheme cwrc:TextLabels ;
    foaf:name "Female (Label)"@en .

cwrc:FrenchLanguage
    void:inDataset cwrc:datasetdefinition ;
    a cwrc:Language, skos:Concept ;
    rdfs:isDefinedBy <http://www.cwrc.ca/ontologies/cwrc#> ;
    rdfs:label "Français"@fr, "French"@en ;
    skos:definition ""@en, ""@fr .

cwrc:Gender
    void:inDataset cwrc:datasetdefinition ;
    a owl:Class, skos:Concept ;
    rdfs:isDefinedBy <http://www.cwrc.ca/ontologies/cwrc#> ;
    rdfs:label "Gender"@en, "Genre"@fr ;
    owl:subClass cwrc:CulturalFormation ;
    skos:definition ""@fr, "A subclass of culturalForms for noting a person's gender whether attributed or self-defined. Although in popular culture gender and biological sex are conflated and understood to be binary, the concept of gender stresses the relationality, constructedness, and performativity of gendered identities and gendered behaviour, whose categories are historically contingent and shifting, and the boundaries between them blurry. Cf. Simone de Beauvoir: \"One is not born, but rather becomes, a woman,\" along with many other theorists of gender including Judith Butler, 1990. Gender is understood as fluid, situational, and sometimes plural, and it is related to though not commensurate with sexual identity and orientation. It is related to but not defined by specific forms of embodiment. Rather than seeing biological sex as a pre-social or natural given, the body is understood as a site of inscription (cf. Elizabeth Grosz 1994) which is also socially constructed and indeed epigenetically shaped by environmental factors (N. Katherine Hayles 2012). This ontology therefore does not provide separate terms for sex as distinct from gender. Instead, the slashes conjoining terms associated with gender and those conventionally associated with sex indicate the constant slippage between gender and sex in the way that these categories circulate through discourses, actions, and institutions. Far from indicating a universal facet of experience, gender intersects with other identity categories and axes of oppression such as class, race or colour, or geographical heritage to produced quite different interests and experiences among people of the same gender, as with the intersection of religion and white masculine identity in the Muscular Christianity movement in nineteenth-century Britain. Being a woman of colour may thus compound the impacts of gender oppression (Kimberlé Crenshaw 1989)."@en .

cwrc:GenderContext
    dcterms:subject cwrc:Gender ;
    void:inDataset cwrc:datasetdefinition ;
    a owl:Class, skos:Concept ;
    rdfs:isDefinedBy <http://www.cwrc.ca/ontologies/cwrc#> ;
    rdfs:label "Contexte de Gendre"@fr, "Gender Context"@en ;
    owl:subClass cwrc:Context ;
    skos:definition ""@en, ""@fr .

cwrc:GenderQueer
    void:inDataset cwrc:datasetdefinition ;
    a owl:Class, skos:Concept ;
    rdfs:isDefinedBy <http://www.cwrc.ca/ontologies/cwrc#> ;
    rdfs:label "GenderQueer"@en, "Non-binaire"@fr ;
    skos:note "Listed as non-binary? in french" .

cwrc:Genre
    void:inDataset cwrc:datasetdefinition ;
    a owl:Class, skos:ConceptScheme ;
    rdfs:isDefinedBy <http://www.cwrc.ca/ontologies/cwrc#> ;
    rdfs:label "genre littéraire"@fr, "literary genre"@en ;
    owl:sameAs dbpedia:Literary_genre ;
    skos:definition ""@en, ""@fr .

cwrc:GeographicalHeritage
    void:inDataset cwrc:datasetdefinition ;
    a owl:Class, skos:Concept ;
    rdfs:isDefinedBy <http://www.cwrc.ca/ontologies/cwrc#> ;
    rdfs:label "Geographical Heritage"@en, "Héritage Géographique"@fr ;
    owl:subClass cwrc:CulturalFormation ;
    skos:definition "Cette sous-catégorie de raceEthnicityContext décrit l’héritage géographique d’une personne et renseigne sur les origines géographiques de sa famille, ce qui contribue souvent à la compréhension de son contexte  ethnique et racial. Cela permet de saisir l’identité d’individus qui se définissent par exemple comme  “sud-asiatique”, en n’indiquant pas d’héritage national précis. Voir raceEthnicityContext pour un compte-rendu détaillé de la complexité de cette catégorie.."@fr, "GeographicalHeritage is a subclass of CulturalFormation that captures information about the geographical origins of a person's family which often contributes to an understanding of their racial and ethnic background. It offers a way to capture women identified as \"South-Asian,\" for example, when no more precise national heritage is indicated. See raceAndEthnicity for a detailed description of the complexities of this element."@en .

cwrc:JohnSimpson
    a foaf:Person ;
    foaf:name "John Simpson" .

cwrc:Language
    void:inDataset cwrc:datasetdefinition ;
    a owl:Class, skos:Concept ;
    rdfs:isDefinedBy <http://www.cwrc.ca/ontologies/cwrc#> ;
    rdfs:label "Habilité linguistique"@fr, "Linguistic Ability"@en ;
    owl:subClass cwrc:CulturalFormation ;
    skos:definition "Does not differentiate between spoken and/or written."@en, "Écris ou Parlé"@fr ;
    foaf:name "Linguistic Ability"@en .

cwrc:LanguageContext
    dcterms:subject cwrc:Language, cwrc:LinguisticAbility ;
    void:inDataset cwrc:datasetdefinition ;
    a owl:Class, skos:Concept ;
    rdfs:isDefinedBy <http://www.cwrc.ca/ontologies/cwrc#> ;
    rdfs:label "Contexte Linguistique"@fr, "Language Context"@en ;
    owl:subClass cwrc:Context ;
    skos:definition ""@en, ""@fr .

cwrc:LinguisticAbility
    void:inDataset cwrc:datasetdefinition ;
    a owl:Class, skos:Concept ;
    rdfs:isDefinedBy <http://www.cwrc.ca/ontologies/cwrc#> ;
    rdfs:label "Habilité linguistique (Écris ou Parlé)"@fr, "Linguistic Ability (Spoken and/or Writen)"@en ;
    owl:subClass cwrc:CulturalFormation ;
    skos:definition ""@en, ""@fr .

cwrc:NationalHeritage
    void:inDataset cwrc:datasetdefinition ;
    a owl:Class, skos:Concept ;
    rdfs:isDefinedBy <http://www.cwrc.ca/ontologies/cwrc#> ;
    rdfs:label "Héritage Nationale"@fr, "National Heritage"@en ;
    owl:subClass cwrc:CulturalFormation ;
    skos:definition ""@fr, "A subclass of culturalForms, this descrbes a person's national heritage and is not the same as citizenship."@en .

cwrc:NationalIdentity
    void:inDataset cwrc:datasetdefinition ;
    a owl:Class, skos:Concept ;
    rdfs:isDefinedBy <http://www.cwrc.ca/ontologies/cwrc#> ;
    rdfs:label "Identité Nationale"@fr, "National Identity"@en ;
    owl:subClass cwrc:CulturalFormation ;
    skos:definition ""@fr, "A subclass of culturalForms, this descrbes a person's nationality/ies and is not the same as citizenship."@en .

cwrc:NationalityContext
    dcterms:subject cwrc:GeographicalHeritage, cwrc:NationalHeritage, cwrc:NationalIdentity ;
    void:inDataset cwrc:datasetdefinition ;
    a owl:Class, skos:Concept ;
    rdfs:isDefinedBy <http://www.cwrc.ca/ontologies/cwrc#> ;
    rdfs:label "Contexte de Nationalité"@fr, "Nationality Context"@en ;
    owl:subClass cwrc:Context ;
    skos:definition ""@en, ""@fr .

cwrc:Place
    void:inDataset cwrc:datasetdefinition ;
    a owl:Class, skos:Concept ;
    rdfs:comment "Could be a populated place according to Geonames, but not necessarily so. Some places, such as cross-roads are named without having a population or settlement per say. The geonames is incosistent in this regards in that a populated place can be abandonned."@en ;
    rdfs:isDefinedBy <http://www.cwrc.ca/ontologies/OrlandoOntology#> ;
    rdfs:label "Endroit"@fr, "Place"@en ;
    rdfs:subClassOf <http://www.w3.org/2003/01/geo/wgs84_pos#SpatialThing> ;
    owl:equivalentClass <http://dbpedia.org/ontology/Place>, <http://schema.org/Place>, <http://www.geonames.org/ontology#Feature> ;
    owl:sameAs <http://geovocab.org/spatial#Feature>, <http://www.opengis.net/ont/geosparql#Feature> ;
    skos:definition "A named place, wheter incorporated, settled or occupied."@en, "Un endroit nommé, qu'il soit populéé, inc nomméorporer ou abandonné."@en ;
    foaf:name "Endroit"@fr, "Place"@en .

cwrc:PoliticalAffiliation
    void:inDataset cwrc:datasetdefinition ;
    a owl:Class, skos:Concept ;
    rdfs:isDefinedBy <http://www.cwrc.ca/ontologies/cwrc#> ;
    rdfs:label "Affiliation Politique"@fr, "Political Affiliation"@en ;
    owl:subClass cwrc:CulturalFormation ;
    skos:definition ""@fr, "This subclass of CulturalFormation tracks the affiliations, connections and associations which designate a person's political involvement. These affiliations can be both formal connections to a party or organization and informal political positions held by the writer. We hope to point our readers towards women writers associated with different political positions and help researchers make links between political beliefs and writing. For this reason, we are defining political affiliations broadly and include things like \"against capital punishment\" or \"strong supporter of the Empire\" in addition to more straightforward affiliations such as \"marxist\" or \"conservative.\""@en .

cwrc:PoliticalContext
    dcterms:subject cwrc:PoliticalAffiliation ;
    void:inDataset cwrc:datasetdefinition ;
    a owl:Class, skos:Concept ;
    rdfs:isDefinedBy <http://www.cwrc.ca/ontologies/cwrc#> ;
    rdfs:label "Contexte Politique"@fr, "Political Context"@en ;
    owl:subClass cwrc:Context ;
    skos:definition ""@en, ""@fr .

cwrc:RaceColour
    void:inDataset cwrc:datasetdefinition ;
    a owl:Class, skos:Concept ;
    rdfs:isDefinedBy <http://www.cwrc.ca/ontologies/cwrc#> ;
    rdfs:label "Race and/or Colour"@en, "Race et/ou Couleur de Peau"@fr ;
    owl:subClass cwrc:CulturalFormation ;
    skos:definition ""@en, ""@fr .

cwrc:RaceEthnicity
    void:inDataset cwrc:datasetdefinition ;
    a owl:Class, skos:Concept ;
    rdfs:isDefinedBy <http://www.cwrc.ca/ontologies/cwrc#> ;
    rdfs:label "Race and/or Ethnicity"@en, "Race et/ou Ethnicité"@fr ;
    owl:subClass cwrc:CulturalFormation ;
    skos:definition ""@en, ""@fr .

cwrc:RaceEthnicityContext
    dcterms:subject cwrc:Ethnicity, cwrc:RaceColour ;
    void:inDataset cwrc:datasetdefinition ;
    a owl:Class, skos:Concept ;
    rdfs:isDefinedBy <http://www.cwrc.ca/ontologies/cwrc#> ;
    rdfs:label "Contexte raciale et/ou ethnique"@fr, "Race Ethnicity Context"@en ;
    rdfs:subClass cwrc:Context ;
    skos:definition """raceEthnicityContext est une sous-catégorie importante de culturalForms. Elle indique la présence d’informations et de discussions sur le sujet concernant son appartenance raciale et ethnique, fonctionnant conjointement avec les sous-éléments spécifiques au sujet (raceColour, nationalHeritage, geogHeritage, ethnicity). La discussion qui suit s’applique aussi bien au contexte discursif général de raceAndEthnicity qu’aux sous-catégories spécifiques.
Malgré les inquiétudes sur la façon dont les catégories de race et d’ethnicité circulent et nourrissent diverses sortes d’intérêts malvenus, les ignorer ou suivre la voix d’un texte totalement libre est un détour qui ne convient pas pour ce projet, même si cela serait plus aisé et plus simple. Le tour que nous empruntons ici fait émerger la complexité des questions de race et d’ethnicité, en faisant bien comprendre que ces catégories sont changeantes, historiquement constituées, développées de façon intéressée, et que leur utilisation doit être comprise dans son contexte. Nous espérons que la discursivité que nous construirons aidera à présenter ces catégories d’une telle manière, ainsi qu’à apaiser l’inquiétude qu’on éprouve à “étiqueter” dans le vide. En d’autres mots, le projet est étranger à l’idée que nous pouvons ou devons aboutir à un ensemble de catégories exactes, totalement définies ou incompatibles ; l’objectif est plutôt de les faire coïncider. Au sein de ce système, compter per se devient hautement problématique et l’utilisateur/trice doit effectuer un certain travail (de réflexion/de définition active) avant d’arriver à quelque liste ou compte, ce qui lui donnera, nous l’espérons, un aperçu du caractère problématique d’une telle activité. 
Les personnes utilisant cette catégorie devront y appliquer des exemples, ou termes, qui semblent corrects en contexte, en les insérant à la ou les catégories qui semblent convenir, mais sont amenés  à ne pas laisser la race/l’ethnicité devenir invisibles ou un problème seulement pour les marginaux. Et nous devons, comme certains l’ont déjà souligné pour les catégories généralisantes “blancs” et “noirs”, encourager les utilisateurs à atteindre le spécifique par le biais du multiple, c’est-à-dire en essayant d’inclure au moins deux catégories parmi “race/couleur”, “ethnicité, “nationalité”, ou “héritage national”. RaceAndEthnicity est une sous-catégorie de culturalFormation. Elle contient quatre sous-catégories relatives: raceColour, nationalHeritage, geogHeritage et ethnicity. Vous êtes également encouragés à prendre en compte toutes les autres sous-catégories en lien avec la problématique de la la formation culturelle: class, denomination, language, nationality, politicalAffiliation, et sexualIdentity. 
"""@fr, """raceEthnicityContext is a significant sub-class within culturalForms. It indicates the presence of information and discussions of a person's subject position with regards to race and ethnicity by working in conjunction with subject specific sub-elements (raceColour, nationalHeritage, geogHeritage, ethnicity). The following discussion applies to both the general discursive context of raceAndEthnicity as well as the specific sub-class categories.
Despite the anxieties of the ways in which categories of race or ethnicity circulate and serve various kinds of undesirable interests, to ignore or go the totally free-text route is not a responsible solution for this project, though it would certainly be easier and simpler. The trick here is to make the complexities of the question of race and ethnicity emerge, and to make it clear that these are shifting, historically constituted, and interestedly deployed categories whose use must be understood contextually. The discursiveness with which we will present these categories will, hopefully, help to do this and also allay the anxiety we feel about \\\"labelling\\\" in a vacuum. In other words, the project has no notion that we could or should come up with what is in any way an exact, fully defined, or mutually exclusive set of categories: the point is the overlap within them. Within this system, counting per se becomes highly problematic and the user has to do some work (and some thinking/active defining) before arriving at any kind of list or count, and will hopefully arrive at it with a sense of how problematic such an activity is.
People using this class should apply it to instances that seem to be right for the context, applying to the category or categories which seem to fit, but they should be encouraged not to let race/ethnicity become invisible or only an issue in relation to the marginalized. And we should, as stressed by those concerned about \\\"white\\\" and \\\"black\\\" as homogenizing categories, encourage people to reach for specificity through multiplicity: i.e. generally attempt to include at least two of: \\\"race/colour\\\"; \\\"ethnicity\\\"; \\\"nationality\\\" or \\\"national-heritage.\\\" RaceAndEthnicity is a sub-class within culturalFormation. It has four realted content sub-classes: raceColour, nationalHeritage, geogHeritage, and ethnicity. You are also encouraged to consider all of the other subclasses appropriate to the discussion of cultural formation: class, denomination, language, nationality, politicalAffiliation, and sexualIdentity."""@en .

cwrc:Religion
    void:inDataset cwrc:datasetdefinition ;
    a owl:Class, skos:ConceptScheme ;
    rdfs:isDefinedBy <http://www.cwrc.ca/ontologies/cwrc#> ;
    rdfs:label "Religion"@en, "Religion"@fr ;
    owl:subClass cwrc:CulturalFormation ;
    skos:definition ""@fr, "A subclass of CulturalFormation, this describes a person's religion(s) or belief system(s). Note that while atheism denotes the absence of religion, we use the Religion label for convinience."@en .

cwrc:ReligionContext
    dcterms:subject cwrc:Religion ;
    void:inDataset cwrc:datasetdefinition ;
    a owl:Class, skos:Concept ;
    rdfs:isDefinedBy <http://www.cwrc.ca/ontologies/cwrc#> ;
    rdfs:label "Contexte Religieux"@fr, "Religious Context"@en ;
    owl:subClass cwrc:Context ;
    skos:definition ""@en, ""@fr .

cwrc:RobWarren
    a foaf:Person ;
    owl:sameAs <http://rdf.muninn-project.org/ww1/2011/11/11/Person/Warren> ;
    foaf:name "Robert Warren" .

cwrc:SexIdentity
    void:inDataset cwrc:datasetdefinition ;
    a owl:Class, skos:Concept ;
    rdfs:isDefinedBy <http://www.cwrc.ca/ontologies/cwrc#> ;
    rdfs:label "Identité Sexe"@fr, "Sex Identity"@en ;
    owl:subClass cwrc:CulturalFormation ;
    skos:definition ""@fr, "Sex according to birth or census data."@en .

cwrc:SexualIdentity
    void:inDataset cwrc:datasetdefinition ;
    a owl:Class, skos:Concept ;
    rdfs:isDefinedBy <http://www.cwrc.ca/ontologies/cwrc#> ;
    rdfs:label "Identité Sexuelle"@fr, "Sexual Identity"@en ;
    owl:sameAs <http://homosaurus.org/terms/sexualIdentity> ;
    owl:subClass cwrc:CulturalFormation ;
    skos:definition """Ces termes englobent en un mot ou en une phrase, l’identification à des types de sexualité (par exemple “lesbienne”, “monogame”, “hétérosexuel/le”), non pas pour fermer la discussion, mais pour développer l’étude et l’analyse critique de ces identifications. L’association suppose que la sexualité n’est pas vécue de manière essentialiste, mais peut être plurielle et fluide, et ainsi plusieurs désignations peuvent être appliquées à une seule personne. Les affirmations de l’identité sexuelle peuvent venir du sujet elle/lui-même ou bien d’autres personnes. Elles peuvent être en tension ou incompatibles, et refléter différents moments de la vie. Par exemple, lier le terme “lesbienne” à la catégorie sexualIdentiy ne signifie pas que le sujet était définitivement lesbienne, puisqu’une telle identification est souvent impossible à cause des lacunes et silences historiques. En ce qui concerne les personnes toujours en vie, notre pratique est de ne nous appuyer que sur des sources ou des divulgations diffusées au public large par le sujet elle/lui-même afin d’éviter de dévoiler sa sexualité par inadvertance. 
"""@fr, "These terms capture in a word or phrase identifications of sexuality (i.e., \"lesbian,\" \"monogamous,\" \"heterosexual\") not as a means of shutting down but advancing investigation and critical analysis of these identifications. The association assumes that sexual identity does not function in an essentialist manner but can be plural and fluid, so multiple designations can be applied to a single person. Assertions of sexual itentity may come from the subject her/himself or from others. They may be in tension or mutually exclusive, and they may reflect different life stages. Linking to the term \"lesbian\" as a sexualIdentity class, for instance, does not signify that the subject was in any definitive sense a lesbian; such identifications are often impossible for reasons of historical gaps and silences. As far as living persons are concerned, our practice is to draw only on widely circulated public sources or disclosures from the subject her/himself in order to avoid inadvertently outing someone. See Campbell and Cowan 2016"@en .

cwrc:SexualityContext
    dcterms:subject cwrc:Gender, cwrc:SexIdentity, cwrc:SexualIdentity ;
    void:inDataset cwrc:datasetdefinition ;
    a owl:Class, skos:Concept ;
    rdfs:isDefinedBy <http://www.cwrc.ca/ontologies/cwrc#> ;
    rdfs:label "Contexte Sexuel"@fr, "Sexuality Context"@en ;
    owl:subClass cwrc:Context ;
    skos:definition "Ces termes englobent en un mot ou en une phrase l’identification à certains  types de sexualité (par exemple “lesbienne”, “monogame”, “hétérosexuel/le”), non pas pour fermer la discussion, mais pour développer l’étude et l’analyse critique de ces identifications. L’association suppose que la sexualité n’est pas vécue de manière essentialiste, mais peut être plurielle et fluide, et ainsi plusieurs désignations peuvent être appliquées à une seule personne. Les affirmations de l’identité sexuelle peuvent venir du sujet elle/lui-même ou bien d’autres personnes. Elles peuvent être en tension ou incompatibles, et refléter différents moments de la vie. Par exemple, lier le terme “lesbienne” à la catégorie sexualIdentiy ne signifie pas que le sujet était définitivement lesbienne, puisqu’une telle identification est souvent impossible à cause des tabous et lacunes historiques. En ce qui concerne les personnes toujours en vie, notre pratique est de ne nous appuyer que sur des sources ou des divulgations diffusées au public large par le sujet elle/lui-même, afin d’éviter de dévoiler par inadvertance des informations privées sur sa sexualité. "@fr, "hasSexualityContext is a significant sub-class within culturalForms. It indicates the presence of information and discussions of a person's subject position with regards to their sexuality and sexual identity. A subclass of Cultural Formation, hasSexualityContext provides depth to more granual categorizations of a person through hasSexuality or hasSexualIdentity. It is not meant to capture individual sexual experiences and relationships, which are covered by intimateRelationships. Specific relationships may be invoked here to indicate the effect on a subject's life and understanding of her own sexuality. This effort to to contextualize gestures towards some of the complicated issues around sexuality, for example, the politics of outing, the historical specificity of some categories such as \"congenital invert,\" or the multiple forms of relating to one's own sexuality. Capturing discussions of her sexuality within this element, will help users interested in the historical, ideological and gendered constructions of sexuality. There are important politics of privacy with respect to the disclosure of a subject's sexuality, sexual orientation and sexual identity. As far as living persons are concerned, our practice is to draw only on widely circulated public sources or disclosures from the subject her/himself in order to avoid inadvertently outing someone. See Campbell and Cowan 2016"@en .

cwrc:SocialClassContext
    dcterms:subject cwrc:SocialClassIdentity ;
    void:inDataset cwrc:datasetdefinition ;
    a owl:Class, skos:Concept ;
    rdfs:isDefinedBy <http://www.cwrc.ca/ontologies/cwrc#> ;
    rdfs:label "Contexte de Classe Sociale"@fr, "Social Class Context"@en ;
    owl:subClass cwrc:Context ;
    skos:definition ""@en, ""@fr .

cwrc:SocialClassIdentity
    void:inDataset cwrc:datasetdefinition ;
    a owl:Class, skos:Concept, skos:ConceptScheme ;
    rdfs:isDefinedBy <http://www.cwrc.ca/ontologies/cwrc#> ;
    rdfs:label "Identité Classe Sociale"@fr, "Social Class Identity"@en ;
    owl:subClass cwrc:CulturalFormation ;
    skos:definition ""@fr, "A subclass of culturalForms, Social Class terms associate subjects with a specific social group, recognizing that such categories and their application to individuals are contested and can change over time. The association may be or have been embraced by the subject by the subject her/himself or attributed by others. Unlike Notes typed as socialClassContext, which contain detailed discussion of a subject's class position, socialClass links to a word or phrase signifying a particular construction of class, with particular reference to earlier historical periods in the British Isles. Social class has been variously constructed and theorized, and for women is further complicated by the fact that women were understood to take their social status from fathers and/or husbands. The terminology used here reflects quite basic social groupings that intersect with other factors such as wealth."@en .

cwrc:SusanBrown
    a foaf:Person ;
    owl:sameAs <http://orcid.org/0000-0002-0267-7344> ;
    foaf:name "Susan Brown" .

cwrc:TextLabels
    void:inDataset cwrc:datasetdefinition ;
    a skos:ConceptScheme ;
    rdfs:isDefinedBy <http://www.cwrc.ca/ontologies/cwrc#> ;
    rdfs:label "Collection of all ambiguous labels within the TEI markup."@en, "blanc"@fr ;
    skos:definition ""@en, ""@fr .

cwrc:Transgender
    void:inDataset cwrc:datasetdefinition ;
    a owl:Class, skos:Concept ;
    rdfs:isDefinedBy <http://www.cwrc.ca/ontologies/cwrc#> ;
    rdfs:label "Transgender"@en, "Transgenre"@fr ;
    owl:sameAs dbpedia:Transgender ;
    owl:subClass cwrc:CulturalFormation ;
    skos:definition "Transgender is the state of one's gender identity, expression or role not matching one's assigned sex."@en ;
    foaf:name "Transgender"@en, "Transgenre"@fr .

cwrc:abrahamicReligions
    void:inDataset cwrc:datasetdefinition ;
    a cwrc:Religion, skos:Concept ;
    rdfs:isDefinedBy <http://www.cwrc.ca/ontologies/cwrc#> ;
    rdfs:label "Abrahamic Religions"@en, "Religions abrahamique"@fr ;
    skos:broaderTransitive cwrc:occultism .

cwrc:agnosticism
    void:inDataset cwrc:datasetdefinition ;
    a cwrc:Religion, skos:Concept ;
    rdfs:isDefinedBy <http://www.cwrc.ca/ontologies/cwrc#> ;
    rdfs:label "Agnosticism"@en, "l'agnosticisme"@fr ;
    skos:broaderTransitive cwrc:occultism ;
    skos:definition ""@en, ""@fr ;
    skos:inScheme cwrc:Religion .

cwrc:anglicanChurch
    void:inDataset cwrc:datasetdefinition ;
    a cwrc:Religion, skos:Concept, foaf:Organization ;
    rdfs:isDefinedBy <http://www.cwrc.ca/ontologies/cwrc#> ;
    rdfs:label "Church of England"@en, "Iglesia de Inglaterra"@es, "anglicaans (kerk van Engeland)"@nl, "anglicanismo"@es, "ying guo sheng gong hui"@zh-latn-pinyin-x-notone, "ying kuo sheng kung hui"@zh-latn-wadegile, "yīng guó shèng gōng huì"@zh-latn-pinyin-x-hanyu, "Église d'Angleterre"@fr, "英國聖公會 (英國國教)"@zh-hant ;
    skos:broaderTransitive cwrc:christianity ;
    skos:definition ""@fr, "A Christian denomination having both Protestant and Catholic aspects that originated with Henry VIII's break with the Roman Catholic Church (ca. 1532-34). As the official state Church of England, the monarch of England is still formally considered its head. While at first it remained mainly Catholic in character, reforms came under Edward IV and Elizabeth I who introduced doctrine that was more Protestant in nature, namely new editions of the Book of Common Prayer and the Thirty-nine Articles. Although an overall attitude of toleration exists in the modern Anglican Church, tension remains between its Protestant and Catholic inclinations as well as with newer liberal and evangelical influences. Anglicanism is based on episcopal authority and parish structure is fundamental to the organization of the church. The term is used with regard to the Church of England; with regard to the Episcopal Church in America, use \"Episcopal.\" "@en, "Te gebruiken om te verwijzen naar de anglicaanse kerk (Church of England); gebruik 'episcopaal' om te verwijzen naar de episcopale kerk in Amerika. De term verwijst naar een christelijke geloofsrichting met zowel protestantse als katholieke elementen die ontstond na de breuk tussen de Engelse koning Hendrik VIII en de rooms-katholieke kerk (circa 1532-34). Het anglicanisme is de officiële Britse staatsgodsdienst, en de Britse soevereine vorst is nog altijd het officiële hoofd van de anglicaanse kerk. Aanvankelijk droeg de kerk nog een overwegend katholiek karakter, maar onder Edward IV en Elizabeth I werden er hervormingen doorgevoerd en werd een meer protestants georiënteerde geloofsleer geïntroduceerd, met een nieuwe versie van het Book of Common Prayer en de Negenendertig Artikelen. Hoewel de huidige anglicaanse kerk in het algemeen wordt gekenmerkt door een tolerante houding, zijn de spanningen tussen protestants en katholiek gezinde stromingen binnen de kerk nooit verdwenen en heerst er weerstand tegen nieuwe vrijzinnige en evangelische invloeden. Het anglicanisme berust op episcopaal gezag en op een structuur van parochies, welke van fundamenteel belang is voor de kerkelijke organisatie."@nl, "Úsese con referencia a la Iglesia de Inglaterra y también con referencia a la Iglesia Episcopal de Estados Unidos (úsese Iglesia Episcopal). Este término s erefiere a a una denominación cristiana que contiene elementos católicos y protestantes en varios aspectos y que se originó con el rey Enrique VIII quien rompió con la Iglesia Católica Romana (ca. 1532-1534) Es la iglesia oficial de Inglaterra, la Monarquía Inglesa es aún formalmente considerada su cabeza.Mientras en sus comienzos conservaba su carácter católico, con las reformas realizadas bajo Eduardo IV e Isabel I quienes introdujeron una doctrina que está más cerca del protestantismo y que se encuentra contenida en nuevas ediciones del Libro de Oraciones Comunes y en los Treinta y nueve Artículos. Aunque el anglicanismo  tiene actualmente una actitud de total tolerancia, aún persisten tensiones con las iglesias protestantes y católicas así como de últimas influencias liberales y evangélicas.El Anglicanismo está basado en la autoridad episcopal y se sustenta en una estructura de parroquias que resulta fundamental para la organización de la Iglesia. "@es, "英王亨利八世與羅馬天主教教會(西元1532-34年)分裂所創的基督教派別，同時含有新教與天主教元素。作為官方英國國教，其正式教會首腦仍為英國國王。起初較具天主教特色，在愛德華四世與伊莉莎白一世時改革，加入較具新教本質的教條，即：新版的公禱書(Book of Common Prayer)及三十九條信綱(Thirty-nine Articles)。雖然現代的英國聖公會大體上態度已越顯寬容，但教會內的新教派系與天主教派系關係仍緊繃，也仍不樂於接受較新的自由與福音派影響。英國聖公會奠基於主教的權威上，牧師教區的結構對教會組織十分重要。此詞彙用於指稱英國國教；美國區的主教派教會，則稱為「美國聖公會(Episcopal)」。"@zh-hant ;
    skos:inScheme cwrc:Religion ;
    prov:derivedFrom <http://vocab.getty.edu/aat/300153822> .

cwrc:atheism
    void:inDataset cwrc:datasetdefinition ;
    a cwrc:Religion, skos:Concept ;
    rdfs:isDefinedBy <http://www.cwrc.ca/ontologies/cwrc#> ;
    rdfs:label "Atheism"@en, "athéisme"@fr ;
    skos:definition ""@en, ""@fr ;
    skos:inScheme cwrc:Religion .

cwrc:baptistChurch
    void:inDataset cwrc:datasetdefinition ;
    a cwrc:Religion, skos:Concept ;
    rdfs:isDefinedBy <http://www.cwrc.ca/ontologies/cwrc#> ;
    rdfs:label "Baptist"@en, "baptisme"@nl, "baptismo"@es, "baptistas"@es, "baptiste"@fr, "chin li tsung"@zh-latn-wadegile, "jin li zong"@zh-latn-pinyin-x-notone, "jìn lǐ zōng"@zh-latn-pinyin-x-hanyu, "浸信會"@zh-hant, "浸禮宗"@zh-hant, "浸禮派"@zh-hant ;
    skos:broaderTransitive cwrc:christianity ;
    skos:definition ""@fr, "Refers to a Protestant denomination centered around the belief that the sacrament of baptism should only be administered to adult members after a personal profession of belief in Jesus Christ. Baptism in this faith is usually done by full immersion. Emphasis is placed on biblical scripture and preaching. The Baptist denomination is primarily derived from early 17th-century England and Wales where it quickly spread although there are some links with the Anabaptists of the 16th century. Baptist churches very rapidly increased in the late 19th century in the United States."@en, "Se refiere a la religión protestante centrada en torno a la creencia que el sacramento del bautismo debería ser administrado sólo a miembros adultos tras una manifestación personal de creencia en Jesucristo. El bautismo en esta fe es usualmente hecho por inmersión total. El énfasis es puesto en las Escrituras Bíblicas y la oración. La denominación baptista deriva principalmente de la Inglaterra y Gales del siglo XVII en donde rápidamente se difundió a pesar que hay algunas conexiones con los Anabaptistas del siglo XVI. La iglesia baptista creció rápidamente en el siglo XIX en los Estados Unidos."@es, "Verwijst naar een protestantse gezindte waarbij het geloof centraal staat dat het sacrament van de doop alleen moet worden toegediend aan volwassen leden na een persoonlijke belijdenis van geloof in Jezus Christus. De doop vindt bij deze gezindte doorgaans plaats door volledige onderdompeling. De nadruk ligt op Bijbelse geschriften en preken. Het baptisme is in hoofdzaak ontstaan in de vroege 17de eeuw in Engeland en Wales waar het zich snel verspreidde, hoewel er enige verbanden zijn met de anabaptisten van de 16de eeuw. In de late 19de eeuw nam het aantal baptistische kerken in de Verenigde Staten snel toe."@nl, "一支新教派別，相信只有親自聲明信仰基督的成人才可受洗。此教的洗禮通常需全身浸洗。重視聖經經文與佈道。浸信會與十六世紀的重浸派有些淵源，但主要源於十七世紀初的英格蘭與威爾斯，在這兩處快速廣傳。其教會於十九世紀末在美國急速增加。"@zh-hant ;
    skos:inScheme cwrc:Religion ;
    prov:derivedFrom <http://vocab.getty.edu/aat/300153825> .

cwrc:black
    void:inDataset cwrc:datasetdefinition ;
    a cwrc:RaceColour ;
    rdfs:isDefinedBy <http://www.cwrc.ca/ontologies/cwrc#> ;
    rdfs:label "black (Race)"@en, "noir (Race)"@fr ;
    skos:definition ""@en, ""@fr .

cwrc:blackLabel
    void:inDataset cwrc:datasetdefinition ;
    a skos:Concept, skosxl:Label ;
    rdfs:isDefinedBy <http://www.cwrc.ca/ontologies/cwrc#> ;
    rdfs:label "black"@en, "noir"@fr ;
    skos:definition ""@en, ""@fr ;
    skos:inScheme cwrc:TextLabels ;
    foaf:name "black"@en .

cwrc:buddhism
    void:inDataset cwrc:datasetdefinition ;
    a cwrc:Religion, skos:Concept ;
    rdfs:isDefinedBy <http://www.cwrc.ca/ontologies/cwrc#> ;
    rdfs:label "Buddhism"@en, "boeddhisme"@nl, "bouddhisme"@fr, "budismo"@es, "fo chiao"@zh-latn-wadegile, "fo jiao"@zh-latn-pinyin-x-notone, "fó jiào"@zh-latn-pinyin-x-hanyu, "佛教"@zh-hant ;
    skos:altLabel "Buddhist"@en ;
    skos:broaderTransitive cwrc:occultism ;
    skos:definition ""@fr, "Refers to the philosophy and religion based on the enlightenment and teachings of the Buddha Gautama in the early sixth century BCE in the northeastern region of modern India. Playing dominant roles in the art and culture of Southeast Asia and East Asia, this religion is based on the transcendence of human suffering and pain through the acceptance of the limitations of individuality, the surrender of worldly desires and cravings that cause disappointment and sorrow, and the deliverance from the impermanence of living and individual ego based on wealth, social position, or family through the process of enlightenment (nirvana). The religion also centers around 'anatman', or no-self, the idea that the self is in a state of action or a series of changing manifestations rather than in a state of fixed, metaphysical substance. The structure of the religion is based on the Triratna (\"Three Jewels\" of Buddha), a tripartite schematic for living based on three elements: Buddha (the teacher), dharma (the teaching), and sangha (community)."@en, "Se refiere a la filosofía y religión basada en la iluminación y enseñanza del Buddha Gautama en el siglo VI a.C temprano en la región nordeste de la India Moderna. Jugando un rol dominante en el arte y la cultura del Asia Sudeste y Asia Oriental, esta religión está basada en la trascendencia del sufrimiento y dolor humano a través de la aceptación de las limitaciones de individualidad, la rendición de deseos mundanos y anhelos que causan desilusión y aflicción y la liberación desde la transitoriedad of living and individual ego based on wealth, social position, or family through the process of enlightenment (nirvana). The religion also centers around anatman, or no-self, the idea that the self is in a state of action or a series of changing manifestations rather than in a state of fixed, metaphysical substance. The structure of the religion is based on the Triratna (\"Three Jewels\" of Buddha), a tripartite schematic for living based on three elements: Buddha (the teacher), dharma (the teaching), and sangha (community)."@es, "Verwijst naar de filosofie en religie die zijn gebaseerd op de verlichting en leer van Boeddha Gautama in de vroege 6de eeuw v. Chr. in het Noord-Oosten van het moderne India. Deze religie, die een dominante rol speelt in de kunst en cultuur van Zuidoost-Azië en Oost-Azië, is gebaseerd op het overstijgen van menselijk lijden en pijn door het accepteren van de grenzen van de individualiteit, het opgeven van wereldse verlangens en wensen die voor teleurstellingen en verdriet zorgen en het loslaten van het niet-permanente van het leven en het afzonderlijke ego met de bijbehorende welvaart, sociale positie of familierelaties, allemaal door het proces van de verlichting (nirvana). Bij deze religie staat ook 'anatman' centraal, het idee dat 'het zelf' altijd in ontwikkeling is of deel uitmaakt van een reeks veranderende verschijningsvormen in plaats van een vaste, metafysische substantie. De structuur van de religie is gebaseerd op de Triratna ('drie juwelen' van boeddha), een drieledige structuur voor het leven gebaseerd op drie elementen: boeddha (de leraar), dharma (de leer) en sangha (de gemeenschap)."@nl, "根據釋迦牟尼佛之開悟與教誨的哲學和宗教，在西元前六世紀初起源於現今印度東北部。佛教於東南亞及東亞的藝術與文化層面扮演主要角色，相信透過接受自身的局限，以及放棄會引起失望與悲傷的世俗欲求及渴望，能夠使人類的苦痛得以昇華，而在開悟（涅盤）過程中得以從短暫的生命以及建築在財富、社會地位與家庭上的個人自尊中獲得解脫。此宗教的中心思想為「無我」，認為自我是處於活動狀態或是一連串的形式改變，而非固定的形上實體狀態。佛教的架構奠基於「三寶」，即生命三元素：佛(老師)、法(規範)、僧(眾)。"@zh-hant ;
    skos:inScheme cwrc:Religion ;
    prov:derivedFrom <http://vocab.getty.edu/aat/300073738> .

cwrc:catholicChurch
    void:inDataset cwrc:datasetdefinition ;
    a cwrc:Religion, skos:Concept, foaf:Organization ;
    rdfs:isDefinedBy <http://www.cwrc.ca/ontologies/cwrc#> ;
    rdfs:label "Roman Catholic"@en, "catholique"@fr, "catolicismo"@es, "catolicismo romano"@es, "katholicisme"@nl, "katholiek"@nl, "rooms-katholicisme"@nl ;
    skos:broaderTransitive cwrc:christianity ;
    skos:definition ""@fr, "Refers to the branch of Christianity characterized by a uniform, highly developed ritual canon and organizational structure with doctrinal roots based in the teachings of the Apostles of Jesus Christ in the first century, in the Alexandrian school of theology, and in Augustinian thought. In this religious branch, faith is considered an acceptance of revelation; revelation appears as doctrine. In juridical terms, it refers to the branch of Christianity distinguished as a unified, monolithic sacramental system under the governance of papal authority. Throughout much of its history, the seat of the Pope has been in Rome, thus \"Roman Catholicism\" is often used to distinguish this concept from the Orthodox Catholic church."@en, "Se refiere a la rama del cristianismo caracterizada por un canon ritual uniforme y altamente desarrollado y una estructura organizacional con raíces doctrinales basadas en las enseñanzas de los Apostoles de Jesucristo en la primera centuria, en la Escuela Alejandrina de teología, y en el pensamiento agustiniano. En esta rama de la religión, la fe es considerada como una aceptación de revelación; la revelación aparece como doctrina. Se refiere a la rama del cristianismo caracterizada por un canon ritual uniforme y altamente desarrollado y una estructura organizacional con raíces doctrinales basadas en las enseñanzas de los Apóstoles de Jesucristo en el primer siglo, en la Escuela Alejandrina de teología, y en el pensamiento agustiniano. En esta rama de la religión, la fe es considerada como una aceptación de revelación; la revelación aparece como doctrina. En términos jurídicos, se refiere a la rama del Cristianismo distinguido como sistema sacramental unificado, monolítico bajo gobierno de la autoridad papal. A través de la mayor parte de su historia, \"la silla del papal” ha estado en Roma, mediante este concepto el Catolicismo Romano se distingue de la Iglesia Católica Ortodoxa."@es, "Verwijst naar de richting van het christendom die zich kenmerkt door een uniforme, hoogontwikkelde rituele canon en organisatiestructuur met een doctrine die wortelt in de leer van de apostelen van Jezus Christus in de 1ste eeuw, in de theologie van de Alexandrijnse school en in het augustijner gedachtegoed. In deze godsdienstige richting wordt het geloof beschouwd als een aanvaarding van de openbaring; de openbaring heeft de vorm van een doctrine. In juridische zin verwijst de term naar de richting van het christendom die zich onderscheidt als een verenigd, monolithisch sacramenteel systeem onder het bestuur van het pauselijk gezag. Gedurende het grootste deel van de geschiedenis van dit systeem was de paus gevestigd in Rome en daarom wordt 'rooms-katholicisme' vaak gebruikt om dit begrip te onderscheiden van de orthodoxe katholieke kerk."@nl ;
    skos:inScheme cwrc:Religion ;
    prov:derivedFrom <http://vocab.getty.edu/aat/300073730> .

cwrc:christianity
    void:inDataset cwrc:datasetdefinition ;
    a cwrc:Religion, skos:Concept ;
    rdfs:isDefinedBy <http://www.cwrc.ca/ontologies/cwrc#> ;
    rdfs:label "Christianity"@en, "chi tu chiao"@zh-latn-wadegile, "christelijk"@nl, "christendom"@nl, "chrétianisme"@fr, "cristianismo"@es, "ji du jiao"@zh-latn-pinyin-x-notone, "jī dū jiāo"@zh-latn-pinyin-x-hanyu, "基督教"@zh-hant ;
    skos:broaderTransitive cwrc:abrahamicReligions ;
    skos:definition ""@fr, "Refers to the world religion and culture that developed in the first century CE, driven by the teachings of Jesus Christ of Nazareth. Its roots are in the Judaic tradition and the Old Testament. The tenets include a belief in the death and redemptive resurrection of Jesus. The religion incorporates a tradition of faith, ritual, and a form of church authority or leadership."@en, "Se refiere a la religión y cultura que se desarrolló en la primera centuria, guiado por la creencia y reverencia por la vida, enseñanza, muerte y resurrección redentiva de Jesucristo de Nazaret. La religión incorpora una tradición de fe, ritual y una forma de iglesia de autoridad y liderazgo."@es, "Verwijst naar de wereldreligie en -cultuur die in de eerste eeuw n. Chr. tot ontwikkeling kwam op basis van de leer van Jezus Christus van Nazareth. De wortels van deze religie liggen in de joodse traditie en het Oude Testament. Een van de kenmerkende grondbeginselen is het geloof in de dood en wederopstanding van Jezus. De religie omvat een traditie van geloof, rituelen en een vorm van kerkelijke autoriteit of leiderschap."@nl, "發展於西元一世紀的世界宗教與文化，跟隨拿薩勒(Nazareth)耶穌基督的教誨。源於猶太傳統及舊約聖經。教義包括相信耶穌之死與救贖復活。此教融合信仰傳統、儀式，及某種形式的教會權威或領導。"@zh-hant ;
    skos:inScheme cwrc:Religion ;
    prov:derivedFrom <http://vocab.getty.edu/aat/300073711> .

cwrc:churchOfChristianScience
    void:inDataset cwrc:datasetdefinition ;
    a cwrc:Religion, skos:Concept ;
    rdfs:isDefinedBy <http://www.cwrc.ca/ontologies/cwrc#> ;
    rdfs:label "Christian Scientist"@en, "Science chrétienne"@fr, "christenwetenschap"@nl, "ciencia cristiana"@es ;
    skos:broaderTransitive cwrc:christianity ;
    skos:definition ""@fr, "Refers to a Christian denomination and movement founded by Mary Baker Eddy (1821-1910) that seeks to reinstate the Christian message of salvation from all evil, including sickness and disease as well as sin. Eddy, a semi-invalid who was interested in cures not involving medicine, claimed a recovery from a bad injury without medical assistance in 1866. Afterwards, she devoted herself to restoring the healing emphasis of early Christianity. In 1875 she finished writing the first edition of the 'Science and Health with Key to the Scriptures.' This work and the Bible are the principal texts of the movement and importance has been laid on establishing reading rooms where these works can make their own appeal to readers. The 'Christian Science Monitor' is also published by the denomination. Christian Science believes that ignorance is at the root of human unease and thus 'dis-ease.' Instead of seeking medical treatment, special Christian Science healers are to be consulted for spiritual healing. Health, happiness, and holiness can be restored by applying to all aspects of life practices and attitudes in keeping with the principal of divine harmony. The first Church of Christ, Scientist was founded in 1879 in Boston and its headquarters remain there."@en, "Se refiere a una secta y movimiento cristiano fundado por Mary Baker Eddy (1821-1910) que busca reincorporar el mensaje cristiano de salvación de todo mal, incluso la enfermedad y padecimiento así como el pecado. Eddy, un semi-inválido que estaba interesado en curas que no involucraran medicina, afirmó que se había recuperado de una lesión grave sin la ayuda médica en 1866. Después, se consagró a restaurar el énfasis curativo de la primera cristiandad. En 1875 ella terminó escribiendo la primera edición del \"la Ciencia y Salud con Llave a las Escrituras\". Este trabajo y la Biblia son los textos principales del movimiento y importancia se ha puesto en establecer salas de lectura donde estos trabajos pueden hacer su propia apelación a los lectores. El \"Instructivo de ciencia cristiano\" también fue publicado por la secta. La Ciencia Cristiana cree que la ignorancia es la raíz de los padecimientos humanos y por lo tanto de la enfermedad. En lugar de buscar tratamiento médico, los sanadores de la Ciencia Cristiana especiales serán consultados para la curación espiritual. La salud, felicidad, y santidad pueden ser restauradas aplicando a todos los aspectos de la vida prácticas y actitudes en concordancia con la armonía divina. La primera Iglesia Científica de Cristo, se fundó en 1879 en Boston y su centro principal permanece allí."@es, "Verwijst naar een christelijke gezindte en beweging die is gesticht door Mary Baker Eddy (1821-1910) en die streeft naar herbevestiging van de christelijke boodschap van verlossing van al het kwaad, met inbegrip van ziekte en zonde. Eddy, die half invalide was en geïnteresseerd in genezing zonder medicijnen, beweerde dat zij in 1866 zonder medische hulp was hersteld van zwaar letsel. Daarna wijdde zij zich aan het herstel van de nadruk op gebedsgenezing die het vroege christendom had gekenmerkt. In 1875 voltooide zij de eerste editie van haar boek 'Science and Health with Key to the Scriptures'. Dit werk en de Bijbel zijn de voornaamste geschriften van de beweging, die veel belang hecht aan de inrichting van leesruimten waar deze boeken een eigen beroep op de lezers kunnen doen. Ook de 'Christian Science Monitor' wordt door het kerkgenootschap uitgegeven. Volgens de leer van Christian Science is onwetendheid de wortel van het menselijk ongemak, de menselijke ziekte. In plaats van medische behandeling te zoeken moet men gebedsgenezers van Christian Science raadplegen voor spirituele genezing. Gezondheid, geluk en heiligheid kunnen worden hersteld door alle aspecten van de levenspraktijk en -houding aan te spreken in overeenstemming met het beginsel van goddelijke harmonie. De eerste Church of Christ, Scientist werd in 1879 in Boston gesticht en het hoofdkwartier van de beweging is daar nog altijd gevestigd."@nl ;
    skos:inScheme cwrc:Religion ;
    prov:derivedFrom <http://vocab.getty.edu/aat/300264476> .

cwrc:churchOfEngland
    void:inDataset cwrc:datasetdefinition ;
    a cwrc:Religion, skos:Concept, foaf:Organization ;
    rdfs:isDefinedBy <http://www.cwrc.ca/ontologies/cwrc#> ;
    rdfs:label ""@fr, "Church of England"@en ;
    skos:broaderTransitive cwrc:christianity ;
    skos:definition ""@en, ""@fr ;
    skos:inScheme cwrc:Religion .

cwrc:churchOfIreland
    void:inDataset cwrc:datasetdefinition ;
    a cwrc:Religion, skos:Concept ;
    rdfs:isDefinedBy <http://www.cwrc.ca/ontologies/cwrc#> ;
    rdfs:label "Church of Ireland"@en, "l'Église d'Irlande"@fr ;
    skos:broaderTransitive cwrc:christianity ;
    skos:definition ""@en, ""@fr ;
    skos:inScheme cwrc:Religion .

cwrc:congregationalChurch
    void:inDataset cwrc:datasetdefinition ;
    a cwrc:Religion, skos:Concept ;
    rdfs:isDefinedBy <http://www.cwrc.ca/ontologies/cwrc#> ;
    rdfs:label "Congregational Church"@en, "Églises congrégationalistes"@fr ;
    skos:broaderTransitive cwrc:christianity ;
    skos:definition ""@en, ""@fr ;
    skos:inScheme cwrc:Religion .

cwrc:cwrc
    a foaf:Organization ;
    foaf:logo <http://www.cwrc.ca/wp-content/uploads/2010/11/CWRC_logo_v074.gif> ;
    foaf:name "Le Collaboratoire scientifique des écrits du Canada"@fr, "The Canadian Writing Research Collaboratory"@en .

cwrc:datasetdefinition
    cc:Jurisdiction dbpedia:Canada ;
    cc:attributionURL <http://www.cwrc.ca/> ;
    cc:license <http://creativecommons.org/licenses/by-nc/4.0/> ;
    loc:ctb cwrc:ConstanceCrompton, cwrc:originalOrlandoAuthor ;
    loc:fnd cwrc:sshrc ;
    loc:pdr cwrc:SusanBrown ;
    dcterms:creator cwrc:AbiLemak, cwrc:ColinFaulkner, cwrc:JohnSimpson, cwrc:RobWarren ;
    dcterms:description "L'Ontologie CWRC est l'ontologie maîtresse qui représente tous les éléments de la structure du Collaboratoire scientifique des écrits du Canada."@fr, "The CWRC Ontology is the overall ontology that represents all elements of structure within the Canadian Writing Research Collaboratory."@en ;
    dcterms:publisher cwrc:cwrc ;
    dcterms:subject <http://id.loc.gov/authorities/subjects/sh2009007122>, <http://id.loc.gov/authorities/subjects/sh85013838>, <http://id.loc.gov/authorities/subjects/sh85019388>, <http://id.loc.gov/authorities/subjects/sh85043777>, <http://id.loc.gov/authorities/subjects/sh85077519> ;
    dcterms:title "L'Ontologie CWRC"@fr, "The CWRC Ontology"@en ;
    a void:Dataset ;
    rdfs:comment "L'Ontologie CWRC est l'ontologie maîtresse qui représente tous les éléments de la structure du Collaboratoire scientifique des écrits du Canada."@fr, "The CWRC Ontology is the overall ontology that represents all elements of structure within the Canadian Writing Research Collaboratory."@en ;
    rdfs:isDefinedBy <http://www.cwrc.ca/ontologies/cwrc#> ;
    rdfs:label "L'Ontologie CWRC"@fr, "The CWRC Ontology"@en ;
    skos:definition "L'Ontologie CWRC est l'ontologie maîtresse qui représente tous les éléments de la structure du Collaboratoire scientifique des écrits du Canada."@fr, "The CWRC Ontology is the overall ontology that represents all elements of structure within the Canadian Writing Research Collaboratory."@en ;
    foaf:logo <http://www.cwrc.ca/wp-content/uploads/2010/11/CWRC_logo_v074.gif> ;
    foaf:name "L'Ontologie CWRC"@fr, "The CWRC Ontology"@en .

cwrc:dissenters
    void:inDataset cwrc:datasetdefinition ;
    a cwrc:Religion, skos:Concept ;
    rdfs:isDefinedBy <http://www.cwrc.ca/ontologies/cwrc#> ;
    rdfs:label "Dissenters"@en, "dissidents (ou non-conformistes)"@fr ;
    skos:broaderTransitive cwrc:churchOfEngland ;
    skos:definition ""@en, ""@fr ;
    skos:inScheme cwrc:Religion .

cwrc:dissentingChurches
    void:inDataset cwrc:datasetdefinition ;
    a cwrc:Religion, skos:Concept ;
    rdfs:isDefinedBy <http://www.cwrc.ca/ontologies/cwrc#> ;
    rdfs:label "Dissenting Churches"@en, "l'Église dissidents"@fr ;
    skos:broaderTransitive cwrc:churchOfEngland ;
    skos:definition ""@en, ""@fr ;
    skos:inScheme cwrc:Religion .

cwrc:england
    void:inDataset cwrc:datasetdefinition ;
    a cwrc:GeographicalHeritage, owl:Thing ;
    rdfs:isDefinedBy <http://www.cwrc.ca/ontologies/cwrc#> ;
    rdfs:label "angleterre"@fr, "england"@en ;
    rdfs:subClass cwrc:englandLabel ;
    skos:definition ""@en, ""@fr ;
    foaf:name "England (Geographical Heritage)"@en .

cwrc:englandLabel
    void:inDataset cwrc:datasetdefinition ;
    a skos:Concept, skosxl:Label ;
    rdfs:isDefinedBy <http://www.cwrc.ca/ontologies/cwrc#> ;
    rdfs:label "angleterre"@fr, "england"@en ;
    owl:oneOf (cwrc:england
    ) ;
    skos:definition ""@en, ""@fr ;
    skos:inScheme cwrc:TextLabels ;
    foaf:name "England"@en .

cwrc:englishLabel
    void:inDataset cwrc:datasetdefinition ;
    a skos:Concept, skosxl:Label ;
    rdf:value "english" ;
    rdfs:isDefinedBy <http://www.cwrc.ca/ontologies/cwrc#> ;
    rdfs:label "englais"@fr, "english"@en ;
    owl:oneOf (cwrc:EnglishNationalHeritage
        cwrc:EnglishLanguage
        cwrc:EnglishNationalIdentity
    ) ;
    skos:definition ""@en, ""@fr ;
    skos:inScheme cwrc:TextLabels ;
    foaf:name "english"@en .

cwrc:entrepreneurial-industrialism
    void:inDataset cwrc:datasetdefinition ;
    a cwrc:SocialClassIdentity, skos:Concept ;
    rdfs:isDefinedBy <http://www.cwrc.ca/ontologies/cwrc#> ;
    rdfs:label ""@fr, "Entrepreneurial Industrialism"@en ;
    skos:definition ""@en, ""@fr .

cwrc:entrepreneurial-industrialist
    void:inDataset cwrc:datasetdefinition ;
    a cwrc:SocialClass, cwrc:SocialClassIdentity, skos:Concept ;
    rdfs:isDefinedBy <http://www.cwrc.ca/ontologies/cwrc#> ;
    rdfs:label "Entrepreneurial Industrialist"@en, "Entrerpreneur Industrialist"@fr, "entrepreneur industrialist"@fr, "entrepreneurial industrialist"@en ;
    owl:subClass cwrc:CulturalFormation ;
    skos:definition ""@en, ""@fr, "Involves larges-scale enterprises such as running factories, or backing such enterprises through investing money, for instance, Elizabeth Montagu or Beatrice Webb."@en .

cwrc:eurasianRace
    void:inDataset cwrc:datasetdefinition ;
    a cwrc:RaceColour, skos:Concept ;
    rdfs:isDefinedBy <http://www.cwrc.ca/ontologies/cwrc#> ;
    rdfs:label "eurasian"@en, "eurasienne"@fr ;
    skos:definition ""@en, ""@fr ;
    foaf:name "Eurasian (Race Colour)"@en .

cwrc:femaleSex
    void:inDataset cwrc:datasetdefinition ;
    a cwrc:SexIdentity, owl:Thing, skos:Concept ;
    rdfs:isDefinedBy <http://www.cwrc.ca/ontologies/cwrc#> ;
    rdfs:label "Female"@en, "Femelle"@fr ;
    skos:definition ""@en, ""@fr ;
    foaf:name "Female (Sex)"@en .

cwrc:fifthMonarchists
    void:inDataset cwrc:datasetdefinition ;
    a cwrc:Religion, skos:Concept ;
    rdfs:isDefinedBy <http://www.cwrc.ca/ontologies/cwrc#> ;
    rdfs:label "Cinquièmes Monarchistes"@fr, "Fifth Monarchists"@en ;
    skos:broaderTransitive cwrc:dissenters, cwrc:millenarianism ;
    skos:definition ""@en, ""@fr ;
    skos:inScheme cwrc:Religion .

cwrc:genderManMale
    void:inDataset cwrc:datasetdefinition ;
    a cwrc:Gender, owl:Thing, skos:Concept ;
    rdfs:isDefinedBy <http://www.cwrc.ca/ontologies/cwrc#> ;
    rdfs:label "man/male"@en, "woman/female"@fr ;
    skos:definition ""@en ;
    foaf:name "man/male (gender)"@en .

cwrc:genderTransMan
    void:inDataset cwrc:datasetdefinition ;
    a cwrc:Gender, skos:Concept ;
    rdfs:isDefinedBy <http://www.cwrc.ca/ontologies/cwrc#> ;
    rdfs:label "Homme Trans"@fr, "Transman/Transmale"@en ;
    skos:definition ""@en ;
    foaf:name "Transman/Transmale (gender)"@en .

cwrc:genderTransWoman
    void:inDataset cwrc:datasetdefinition ;
    a cwrc:Gender, skos:Concept ;
    rdfs:isDefinedBy <http://www.cwrc.ca/ontologies/cwrc#> ;
    rdfs:label "Femme Trans"@fr, "Transwoman/Transfemale"@en ;
    skos:definition ""@en ;
    foaf:name "Transwoman/Transfemale (gender)"@en .

cwrc:genderWomanFemale
    void:inDataset cwrc:datasetdefinition ;
    a cwrc:Gender, owl:Thing, skos:Concept ;
    rdfs:isDefinedBy <http://www.cwrc.ca/ontologies/cwrc#> ;
    rdfs:label "Femme/Femelle"@fr, "Woman/Female"@en ;
    skos:definition ""@en ;
    foaf:name "Woman/Female (gender)"@en .

cwrc:genreAbridgement
    void:inDataset cwrc:datasetdefinition ;
    a cwrc:Genre, skos:Concept ;
    rdf:value "ABRIDGEMENT" ;
    rdfs:isDefinedBy <http://www.cwrc.ca/ontologies/cwrc#> ;
    rdfs:label ""@fr, "abridgement"@en ;
    owl:comment "This term and its description was created from data gathered from the Getty Art & Architecture Thesaurus."@en ;
    skos:definition "Version einer schriftlichen Arbeit, die durch Verdichtung und Auslassung zustande kommt, aber die eigentliche Bedeutung und Art der Darstellung des Originals beibehält; wird häufig von jemand anderem als dem Autor erstellt. "@de, "Versions of written works produced by condensation and omission but with retention of the general meaning and manner of presentation of the original, often prepared by someone other than the author of the original."@en, "Wordt gebruikt voor sterk ingekorte versies van geschreven werken, waarin, ondanks de vele weglatingen, de algemene inhoud en de indeling van het origineel behouden blijft. De schrijver van deze samenvattingen is vaak niet dezelfde als de auteur van het origineel."@nl, "Úsese para versiones de obras escritas producidas mediante un resumen y omisiones del original pero manteniendo el significado general y su forma de presentación, a menudo preparadas por alguien diferente al autor del original."@es, "書寫作品之濃縮與省略版本，但保留原作的大體意義及呈現方式，常由原作者以外的人編纂。"@zh-hant ;
    skos:inScheme cwrc:Genre ;
    prov:derivedFrom <http://vocab.getty.edu/aat/300202489> .

cwrc:genreAclef
    void:inDataset cwrc:datasetdefinition ;
    a cwrc:Genre, skos:Concept ;
    rdf:value "ACLEF" ;
    rdfs:isDefinedBy <http://www.cwrc.ca/ontologies/cwrc#> ;
    rdfs:label ""@fr, "aclef"@en ;
    skos:inScheme cwrc:Genre .

cwrc:genreAcrostic
    void:inDataset cwrc:datasetdefinition ;
    a cwrc:Genre, skos:Concept ;
    rdf:value "ACROSTIC" ;
    rdfs:isDefinedBy <http://www.cwrc.ca/ontologies/cwrc#> ;
    rdfs:label "acrostic"@en, "acrostiche"@fr ;
    owl:comment "This term and its description was created from data gathered from DBpedia."@en, "This term and its description was created from data gathered from the Getty Art & Architecture Thesaurus."@en ;
    skos:definition "Korte gedichten of stukjes proza waarvan de eerste letters van de opeenvolgende regels samen een woord, een zinsnede of een motto vormen."@nl, "Kurzes Gedicht oder Prosakomposition, bei der der Text so angeordnet ist, dass die ersten Buchstaben jeder Zeile aneinandergereiht ein Wort, einen Satz oder ein Motto ergeben."@de, "Poemas cortos o composiciones en prosa en los que el texto es ordenado de tal manera que las primeras letras de cada línea forman una palabra, frase o máxima."@es, "Short poems or prose compositions in which text is arranged so that the first letters of each line form a word, phrase, or motto."@en, "Un acrostiche, du grec akrostikhos (akros, haut, élevé et stikhos, le vers), est un poème, une strophe ou une série de strophes fondés sur une forme poétique consistant en ce que, lues verticalement de haut en bas, la première lettre ou, parfois, les premiers mots d'une suite de vers composent un mot ou une expression en lien avec le poème."@fr, "各行首字母可組成一個字、詞，或座右銘的短詩或散文作品。"@zh-hant ;
    skos:inScheme cwrc:Genre ;
    prov:derivedFrom dbpedia:Acrostic, <http://vocab.getty.edu/aat/300256198> .

cwrc:genreAdaptation
    void:inDataset cwrc:datasetdefinition ;
    a cwrc:Genre, skos:Concept ;
    rdf:value "ADAPTATION" ;
    rdfs:isDefinedBy <http://www.cwrc.ca/ontologies/cwrc#> ;
    rdfs:label ""@fr, "adaptation"@en ;
    owl:comment "This term and its description was created from data gathered from the Getty Art & Architecture Thesaurus."@en ;
    skos:definition "Written works or works derived from written works, where the second work is an alteration or amendment a text to make it suitable for another purpose. An example of an adaptation is a version of an earlier text made to better agree with a philosophy other than that intended by the original. Other examples are written works adapted for another medium, such as film, broadcasting, or stage production. For visual works adapted from another work, use \"adaptations (derivative objects).\""@en ;
    skos:inScheme cwrc:Genre ;
    prov:derivedFrom <http://vocab.getty.edu/aat/300410356> .

cwrc:genreAdventurewriting
    void:inDataset cwrc:datasetdefinition ;
    a cwrc:Genre, skos:Concept ;
    rdf:value "ADVENTUREWRITING" ;
    rdfs:isDefinedBy <http://www.cwrc.ca/ontologies/cwrc#> ;
    rdfs:label ""@fr, "adventure writing"@en ;
    skos:inScheme cwrc:Genre .

cwrc:genreAdvertisingcopy
    void:inDataset cwrc:datasetdefinition ;
    a cwrc:Genre, skos:Concept ;
    rdf:value "ADVERTISINGCOPY" ;
    rdfs:isDefinedBy <http://www.cwrc.ca/ontologies/cwrc#> ;
    rdfs:label ""@fr, "advertising copy"@en ;
    skos:inScheme cwrc:Genre .

cwrc:genreAfterpiece
    void:inDataset cwrc:datasetdefinition ;
    a cwrc:Genre, skos:Concept ;
    rdf:value "AFTERPIECE" ;
    rdfs:isDefinedBy <http://www.cwrc.ca/ontologies/cwrc#> ;
    rdfs:label ""@fr, "afterpiece"@en ;
    skos:inScheme cwrc:Genre .

cwrc:genreAfterword
    void:inDataset cwrc:datasetdefinition ;
    a cwrc:Genre, skos:Concept ;
    rdf:value "AFTERWORD" ;
    rdfs:isDefinedBy <http://www.cwrc.ca/ontologies/cwrc#> ;
    rdfs:label ""@fr, "afterword"@en ;
    skos:inScheme cwrc:Genre .

cwrc:genreAgitprop
    void:inDataset cwrc:datasetdefinition ;
    a cwrc:Genre, skos:Concept ;
    rdf:value "AGITPROP" ;
    rdfs:isDefinedBy <http://www.cwrc.ca/ontologies/cwrc#> ;
    rdfs:label ""@fr, "agitprop"@en ;
    skos:inScheme cwrc:Genre .

cwrc:genreAllegory
    void:inDataset cwrc:datasetdefinition ;
    a cwrc:Genre, skos:Concept ;
    rdf:value "ALLEGORY" ;
    rdfs:isDefinedBy <http://www.cwrc.ca/ontologies/cwrc#> ;
    rdfs:label ""@fr, "allegory"@en ;
    owl:comment "This term and its description was created from data gathered from DBpedia."@en, "This term and its description was created from data gathered from the Getty Art & Architecture Thesaurus."@en ;
    skos:definition "Literaire werken waarin met behulp van fictionele, symbolische figuren en handelingen waarheden of generalisaties omtrent menselijk gedrag of menselijke ervaringen worden gedebiteerd."@nl, "Literarisches Werk, Kunstwerk oder anderes künstlerisches Werk, das allegorische Darstellungsformen benutzt, um komplexe abstrakte Ideen auszudrücken, zum Beispiel ein Werk, das symbolhafte, fiktionale Bilder und Handlungen verwendet, um Wahrheiten oder Verallgemeinerungen über menschliches Verhalten oder Erfahrungen zum Ausdruck zu bringen."@de, "Literary works, art works, or other creative works that employ allegory to express complex abstract ideas, for example works that employ symbolic, fictional figures and actions to express truths or generalizations about human conduct or experience."@en, "Obras literarias que emplean personajes y acciones ficticias simbólicas para expresar verdades o generalizaciones acerca de conductas o experiencias humanas."@es, "Une allégorie (du grec : ἄλλον / állon, « autre chose », et ἀγορεύειν / agoreúein, « parler en public ») est une forme de représentation indirecte qui emploie une chose (une personne, un être animé ou inanimé, une action) comme signe d'une autre chose, cette dernière étant souvent une idée abstraite ou une notion morale difficile à représenter directement. Elle représente donc une idée abstraite par du concret. En littérature, l'allégorie est une figure rhétorique qui consiste à exprimer une idée en utilisant une histoire ou une représentation qui doit servir de support comparatif. La signification étymologique est : « une autre manière de dire », au moyen d'une image figurative ou figurée."@fr ;
    skos:inScheme cwrc:Genre ;
    prov:derivedFrom dbpedia:Allegory, <http://vocab.getty.edu/aat/300202507> .

cwrc:genreAnagram
    void:inDataset cwrc:datasetdefinition ;
    a cwrc:Genre, skos:Concept ;
    rdf:value "ANAGRAM" ;
    rdfs:isDefinedBy <http://www.cwrc.ca/ontologies/cwrc#> ;
    rdfs:label ""@fr, "anagram"@en ;
    owl:comment "This term and its description was created from data gathered from DBpedia."@en ;
    skos:definition "Anagrammatic poetry is poetry with the constrained form that either each line or each verse is an anagram of all other lines or verses in the poem. A poet that specializes in anagrams is an anagrammarian. Writing anagrammatic poetry is a form of a constrained writing similar to writing pangrams or long alliterations."@en ;
    skos:inScheme cwrc:Genre ;
    prov:derivedFrom dbpedia:Anagrammatic_poem .

cwrc:genreAnnotation
    void:inDataset cwrc:datasetdefinition ;
    a cwrc:Genre, skos:Concept ;
    rdf:value "ANNOTATION" ;
    rdfs:isDefinedBy <http://www.cwrc.ca/ontologies/cwrc#> ;
    rdfs:label ""@fr, "annotation"@en ;
    owl:comment "This term and its description was created from data gathered from the Getty Art & Architecture Thesaurus."@en ;
    skos:definition "Ergänzung, die als Kommentar oder Erklärung hinzugefügt wird, wie beispielsweise jene, die einem Titel in einer Bibliografie, einer Leseliste oder einem Katalog beigefügt ist und die betreffende Publikation beschreiben, erklären oder bewerten soll."@de, "Notas agregadas como comentarios o explicaciones."@es, "Notes added as comment or explanation, such as those accompanying an entry in a bibliography, reading list, or catalogue intended to describe, explain, or evaluate the publication referred to."@en, "Verklarende aantekeningen."@nl ;
    skos:inScheme cwrc:Genre ;
    prov:derivedFrom <http://vocab.getty.edu/aat/300026100> .

cwrc:genreAnswer
    void:inDataset cwrc:datasetdefinition ;
    a cwrc:Genre, skos:Concept ;
    rdf:value "ANSWER" ;
    rdfs:isDefinedBy <http://www.cwrc.ca/ontologies/cwrc#> ;
    rdfs:label ""@fr, "answer"@en ;
    skos:inScheme cwrc:Genre .

cwrc:genreAnthem
    void:inDataset cwrc:datasetdefinition ;
    a cwrc:Genre, skos:Concept ;
    rdf:value "ANTHEM" ;
    rdfs:isDefinedBy <http://www.cwrc.ca/ontologies/cwrc#> ;
    rdfs:label ""@fr, "anthem"@en ;
    skos:inScheme cwrc:Genre .

cwrc:genreAnthology
    void:inDataset cwrc:datasetdefinition ;
    a cwrc:Genre, skos:Concept ;
    rdf:value "ANTHOLOGY" ;
    rdfs:isDefinedBy <http://www.cwrc.ca/ontologies/cwrc#> ;
    rdfs:label "anthologie"@fr, "anthology"@en ;
    skos:inScheme cwrc:Genre .

cwrc:genreAntiromance
    void:inDataset cwrc:datasetdefinition ;
    a cwrc:Genre, skos:Concept ;
    rdf:value "ANTIROMANCE" ;
    rdfs:isDefinedBy <http://www.cwrc.ca/ontologies/cwrc#> ;
    rdfs:label ""@fr, "antiromance"@en ;
    skos:inScheme cwrc:Genre .

cwrc:genreAphorism
    void:inDataset cwrc:datasetdefinition ;
    a cwrc:Genre, skos:Concept ;
    rdf:value "APHORISM" ;
    rdfs:isDefinedBy <http://www.cwrc.ca/ontologies/cwrc#> ;
    rdfs:label ""@fr, "aphorism"@en ;
    owl:comment "This term and its description was created from data gathered from the Getty Art & Architecture Thesaurus."@en ;
    skos:definition "Korte, bondige formuleringen van principes of voorschriften, waarvan de auteur dikwijls bekend is; te onderscheiden van 'spreekwoorden', hetgeen uitdrukkingen zijn die in de omgangstaal zijn ingeburgerd en dikwijls een volkswijsheid van een groep mensen of een volk uitdrukken."@nl, "Kurze, prägnante Erklärung eines Prinzips oder Grundsatzes, häufig mit bekannter Urheberschaft; zu unterscheiden vom \"Sprichwort\", einer in der Alltagssprache wiederholten Äußerung, die häufig Volksweisheiten einer Gruppe oder eines Landes enthält."@de, "Sentencias cortas y concisas de principios o preceptos, a menudo de conocida autoría, diferentes de los \"proverbios\" que son sentencias que se repiten coloquialmente y que a menudo encarnan la sabiduría popular de un grupo o nación."@es, "Short, pithy statements of principle or precepts, often of known authorship; distinguished from \"proverbs\" which are statements repeated colloquially and which often embody the folk wisdom of a group or nation."@en ;
    skos:inScheme cwrc:Genre ;
    prov:derivedFrom <http://vocab.getty.edu/aat/300253001> .

cwrc:genreApology
    void:inDataset cwrc:datasetdefinition ;
    a cwrc:Genre, skos:Concept ;
    rdf:value "APOLOGY" ;
    rdfs:isDefinedBy <http://www.cwrc.ca/ontologies/cwrc#> ;
    rdfs:label ""@fr, "apology"@en ;
    skos:inScheme cwrc:Genre .

cwrc:genreArtcriticism
    void:inDataset cwrc:datasetdefinition ;
    a cwrc:Genre, skos:Concept ;
    rdf:value "ARTCRITICISM" ;
    rdfs:isDefinedBy <http://www.cwrc.ca/ontologies/cwrc#> ;
    rdfs:label ""@fr, "art criticism"@en ;
    skos:inScheme cwrc:Genre .

cwrc:genreAutobiography
    void:inDataset cwrc:datasetdefinition ;
    a cwrc:Genre, skos:Concept ;
    rdf:value "AUTOBIOGRAPHY" ;
    rdfs:isDefinedBy <http://www.cwrc.ca/ontologies/cwrc#> ;
    rdfs:label ""@fr, "autobiography"@en ;
    owl:comment "This term and its description was created from data gathered from the Getty Art & Architecture Thesaurus."@en ;
    skos:definition "Biografieën met de auteur zelf als onderwerp."@nl, "Biografías de individuos escritas por ellos mismos."@es, "Biographie einer Person, die von ihr selbst verfasst wurde."@de, "Documents of any type that are biographies of individuals written by themselves. For the overall genre, use \"autobiography (genre).\""@en ;
    skos:inScheme cwrc:Genre ;
    prov:derivedFrom <http://vocab.getty.edu/aat/300080104> .

cwrc:genreBallade
    void:inDataset cwrc:datasetdefinition ;
    a cwrc:Genre, skos:Concept ;
    rdf:value "BALLAD", "BALLADE" ;
    rdfs:isDefinedBy <http://www.cwrc.ca/ontologies/cwrc#> ;
    rdfs:label "ballade"@en, "ballade"@fr ;
    owl:comment "This term and its description was created from data gathered from DBpedia."@en ;
    skos:definition "A ballade (from French ballade, [baˈlad], and German Ballade, [baˈlaːdə], both being words for \"ballad\"), in classical music since the late 18th century, refers to a setting of a literary ballad, a narrative poem, in the musical tradition of the Lied, or to a one-movement instrumental piece with lyrical and dramatic narrative qualities reminiscent of such a song setting, especially a piano ballad."@en, "Die Ballade ist in der Klaviermusik eine Gattung des 19. Jahrhunderts, die ähnlich wie das Charakterstück oder das Lied ohne Worte formal nicht festgelegt ist. Gelegentlich lassen sich die Komponisten von Dichtungen (z. B. Chopin und Brahms) oder Stimmungen inspirieren. Zu den Vorläufern der Klavierballade zählen die Rhapsodien der beiden tschechischen Komponisten Václav Jan Křtitel Tomášek und Jan Václav Voříšek."@de, "El término balada se ha utilizado de formas muy diferentes en la historia de la música. En los siglos XIV y XV la palabra francesa ballade designaba un tipo de canción, habitualmente con tres estrofas de siete u ocho versos de los que el último servía de estribillo. La forma musical era la denominada \"forma bar\" (AAB): la melodía de los dos primeros versos se repetía en el tercero y cuarto; el resto se cantaban con melodía diferente. Las ballades eran habitualmente polifónicas, a dos o, con más frecuencia, tres voces: la voz superior (cantus) era la melodía principal; las otras voces podían ser cantadas o interpretadas con instrumentos. En Italia, en el Trecento (siglo XIV), el término ballata designaba un tipo diferente de canción, similar al virelay francés: un estribillo alternaba con estrofas divididas en dos secciones: la primera repetía dos veces una melodía, con final abierto y cerrado; la segunda se cantaba con la melodía del estribillo. En el siglo XIX, el título fue dado por Frédéric Chopin a cuatro importantes obras a gran escala para piano (Opus 23, 38, 47 y 52), la primera aplicación significativa del término en la música instrumental. Subsecuentemente otros compositores han usado el título para sus obras para piano: Johannes Brahms (la tercera de sus Klavierstücke opus 118, y las cuatro del opus 10), Edvard Grieg (opus 24, un conjunto de variaciones), Franz Liszt (que escribió dos) y Gabriel Fauré (opus 19, posteriormente arreglada para piano y orquesta). Sin embargo, hay que destacar que también se han escrito baladas para otros instrumentos."@es ;
    skos:inScheme cwrc:Genre ;
    prov:derivedFrom <http://dbpedia.org/resource/Ballade_(classical_music)> .

cwrc:genreBalladopera
    void:inDataset cwrc:datasetdefinition ;
    a cwrc:Genre, skos:Concept ;
    rdf:value "BALLADOPERA" ;
    rdfs:isDefinedBy <http://www.cwrc.ca/ontologies/cwrc#> ;
    rdfs:label ""@fr, "ballad opera"@en ;
    skos:inScheme cwrc:Genre .

cwrc:genreBallet
    void:inDataset cwrc:datasetdefinition ;
    a cwrc:Genre, skos:Concept ;
    rdf:value "BALLET" ;
    rdfs:isDefinedBy <http://www.cwrc.ca/ontologies/cwrc#> ;
    rdfs:label ""@fr, "ballet"@en ;
    skos:inScheme cwrc:Genre .

cwrc:genreBergamasque
    void:inDataset cwrc:datasetdefinition ;
    a cwrc:Genre, skos:Concept ;
    rdf:value "BERGAMASQUE" ;
    rdfs:isDefinedBy <http://www.cwrc.ca/ontologies/cwrc#> ;
    rdfs:label ""@fr, "bergamasque"@en ;
    skos:inScheme cwrc:Genre .

cwrc:genreBestiary
    void:inDataset cwrc:datasetdefinition ;
    a cwrc:Genre, skos:Concept ;
    rdf:value "BESTIARY" ;
    rdfs:isDefinedBy <http://www.cwrc.ca/ontologies/cwrc#> ;
    rdfs:label ""@fr, "bestiary"@en ;
    owl:comment "This term and its description was created from data gathered from the Getty Art & Architecture Thesaurus."@en ;
    skos:definition "Colecciones de fábulas moralizadoras, especialmente como aquellas escritas de la Edad Media, acerca de animales actuales o míticos."@es, "Collections of moralized fables, especially as written in the Middle Ages, about actual or mythical animals."@en, "Sammlung moralischer Fabeln, insbesondere solcher, die im Mittelalter über wirkliche oder mythische Tiere verfasst wurden."@de, "Verzamelingen moraliserende vertellingen, zoals die in de middeleeuwen veel werden geschreven, over bestaande of mythische dieren."@nl, "描寫真實或虛構的動物，具道德教訓的寓言集，尤指中世紀之著作。"@zh-hant ;
    skos:inScheme cwrc:Genre ;
    prov:derivedFrom <http://vocab.getty.edu/aat/300201056> .

cwrc:genreBiblicalparaphrase
    void:inDataset cwrc:datasetdefinition ;
    a cwrc:Genre, skos:Concept ;
    rdf:value "BIBLICALPARAPHRASE" ;
    rdfs:isDefinedBy <http://www.cwrc.ca/ontologies/cwrc#> ;
    rdfs:label ""@fr, "biblical paraphrase"@en ;
    skos:inScheme cwrc:Genre .

cwrc:genreBildungsroman
    void:inDataset cwrc:datasetdefinition ;
    a cwrc:Genre, skos:Concept ;
    rdf:value "BILDUNGSROMAN" ;
    rdfs:isDefinedBy <http://www.cwrc.ca/ontologies/cwrc#> ;
    rdfs:label ""@fr, "bildungsroman"@en ;
    owl:comment "This term and its description was created from data gathered from DBpedia."@en, "This term and its description was created from data gathered from the Getty Art & Architecture Thesaurus."@en ;
    skos:definition "La novela de formación o novela de aprendizaje es un género literario que retrata la transición de la niñez a la vida adulta. El término alemán original, Bildungsroman () significa literalmente novela de formación o novela de educación y fue acuñado por el filólogo Johann Carl Simon Morgenstern en 1819. La temática de esta novela es la evolución y el desarrollo físico, moral, psicológico y social de un personaje, generalmente desde su infancia hasta la madurez. En esta evolución se suelen diferenciar tres etapas: la primera es el aprendizaje de juventud (\"Jugendlehre\"), la segunda son los años de peregrinación (\"Wanderjahre\") y por último el perfeccionamiento (\"Läuterung\"). A pesar de que existen rasgos de la novela de aprendizaje en obras clásicas o medievales (en las obras moralizantes, por ejemplo), es plausible situar en el Renacimiento el embrión de este tipo de novela, especialmente en el género picaresco. Por ejemplo, El lazarillo de Tormes muestra el proceso por el que el protagonista, Lázaro, aprende a defenderse en la vida tras sufrir sirviendo a distintos amos abusivos. Convencionalmente se considera que el género surge dentro de la corriente del Romanticismo alemán con Los años de aprendizaje de Wilhelm Meister (Wilhem Meister Lehrjahre, 1795/1796) de Wolfgang Goethe. La traducción al inglés de esta novela, realizada por Thomas Carlyle, contribuyó a expandir este género nacido en Alemania al resto de Europa y luego al resto del mundo. A medida que ha ido avanzando el género, nos podemos encontrar con negativos Bildungsromane en los que se cuentan los fracasos de los personajes como, por ejemplo, en \"Anton Reiser\" de Karl Philip Moritz y modernos Bildungsromane, como Carta breve para un largo adiós (Der Kurze Brief zum langen Abschied, 1972) de Peter Handke. Muchas de las grandes novelas de los siglos XIX y XX, sin ser estrictamente Bildungsroman, comparten alguna de sus características. Por ejemplo, Marcel Proust en En busca del tiempo perdido narra el proceso de aprendizaje del protagonista, Marcel; lo mismo sucede en Retrato del artista adolescente, de James Joyce, en el Moll Flanders de Defoe o en La montaña mágica, de Thomas Mann. Bajo las ruedas, de Hermann Hesse, es un Bildungsroman en sentido aún más estricto. A pesar de que la novela de aprendizaje parece haber perdido peso desde la segunda mitad del siglo XX, muchos de sus elementos aún perviven en novelas como El guardián entre el centeno de J. D. Salinger o en numerosas películas contemporáneas. La sombra del viento (2001), del barcelonés Carlos Ruiz Zafón, narra el tránsito de la infancia a la madurez de Daniel Sempere a través del misterio y del amor a los libros y podría ser considerado un Bildungsroman del siglo XXI."@es, "Le roman d'apprentissage, appelé aussi roman de formation ou roman d’éducation, est un genre littéraire romanesque né en Allemagne au XVIIIe siècle (à ne pas confondre avec le roman de jeunesse). Il s'oppose cependant à la fonction première du romanesque qui est de nous transporter dans un monde de rêve et d'évasion. On parle ainsi de « roman initiatique » ou de « conte initiatique ». En allemand, le roman de formation est nommé « Bildungsroman ». Ce terme est dû au philologue allemand Johann Carl Simon Morgenstern, qui voyait dans le Bildungsroman « l'essence du roman par opposition au récit épique ». On emploie aussi l'expression « Entwicklungsroman » (roman de développement personnel). Un roman d'apprentissage a pour thème le cheminement évolutif d'un héros, souvent jeune, jusqu'à ce qu'il atteigne l'idéal de l'homme accompli et cultivé. Le héros découvre en général un domaine particulier dans lequel il fait ses armes. Mais en réalité, c'est une conception de la vie en elle-même qu'il se forge progressivement. En effet, derrière l'apprentissage d'un domaine, le jeune héros découvre les grands événements de l'existence (la mort, l'amour, la haine, l'altérité, pour prendre quelques exemples). Ainsi, dans L'Éducation sentimentale (Flaubert, 1869), le jeune Frédéric connaît les premiers émois de l'amour : et réfléchissant sur les sentiments qu'il porte à Mme Arnoux, Frédéric se construit une idée de l'existence. Le roman d'apprentissage est un roman qui décrit la maturation du héros. Il manque d'expérience au départ et traverse des obstacles ou des épreuves afin de mûrir et d'en tirer des leçons."@fr, "Novels of a traditional German genre that focuses on the spiritual development or formative years of an individual. Now in broad use to refer to this type of novel written in any language or in any culture."@en, "Romans van een traditioneel Duits genre met daarin een beschrijving van de geestelijke ontwikkeling of vormende jaren van een persoon. De term gebruikt men nu in algemene zin voor romans van dit type, ongeacht de betreffende taal of cultuur."@nl, "Traditionelle deutsche Romanform, bei der das Hauptaugenmerk auf der geistigen Entwicklung oder die prägenden Jahre einer Person liegt. Wird inzwischen weitgehend für diesen Romantypus verwendet, egal in welcher Sprache er geschrieben wurde oder aus welcher Kultur er stammt. "@de, "傳統德國類型之小說，著重於主角的精神發展或構成的年代。而今廣泛用於指以任何語言或於任何文化背景寫作之此一種類的小說。"@zh-hant ;
    skos:inScheme cwrc:Genre ;
    prov:derivedFrom dbpedia:Bildungsroman, <http://vocab.getty.edu/aat/300297857> .

cwrc:genreBiographicaldictionary
    void:inDataset cwrc:datasetdefinition ;
    a cwrc:Genre, skos:Concept ;
    rdf:value "BIOGRAPHICALDICTIONARY" ;
    rdfs:isDefinedBy <http://www.cwrc.ca/ontologies/cwrc#> ;
    rdfs:label ""@fr, "biographical dictionary"@en ;
    skos:inScheme cwrc:Genre .

cwrc:genreBiography
    void:inDataset cwrc:datasetdefinition ;
    a cwrc:Genre, skos:Concept ;
    rdf:value "BIOGRAPHY" ;
    rdfs:isDefinedBy <http://www.cwrc.ca/ontologies/cwrc#> ;
    rdfs:label ""@fr, "biography"@en ;
    owl:comment "This term and its description was created from data gathered from DBpedia."@en, "This term and its description was created from data gathered from the Getty Art & Architecture Thesaurus."@en ;
    skos:definition "Brief profiles of a people's life or work."@en, "Een biografie (Grieks: βιος leven) is een op schrift gestelde (en doorgaans gepubliceerde) levensbeschrijving van een persoon. De term wordt meestal gebruikt voor non-fictie, dat wil zeggen werken waarin iemand het werkelijke leven van een werkelijk bestaand, veelal beroemd, persoon probeert te beschrijven. Een biografie is wel verhalend en probeert op die manier een beter inzicht te geven in de persoonlijkheid en karakter van de beschreven persoon dan een droge opsomming van feiten zou doen. Een biografie van een heilige heet een hagiografie. Deze term wordt ook gebruikt als de schrijver zijn onderwerp onkritisch behandelt. Als de schrijver van een biografie ook het onderwerp van de biografie is, heet dit een autobiografie."@nl, "Eine Biografie, auch Biographie (griechisch βιογραφία, von βίος, bíos „Leben“ und -graphie von γράφω, gráphō „ritzen, malen, schreiben“) ist die Lebensbeschreibung einer Person. Die Biografie ist die mündliche oder schriftliche Präsentation des Lebenslaufes eines anderen Menschen; ein Sonderfall der Biografie ist die Autobiografie: Sie hat der Betreffende selbst (heute allerdings häufig mit der Unterstützung eines Ghostwriters) über seine eigenen Lebenserfahrungen verfasst. Im Familienverbund werden Autobiografien manchmal dem Testament beigefügt. Es soll vom Leben eine Spur übrig bleiben – die Nachkommen sollen wissen, was war. Den Lebenslauf zu beschreiben, bedeutete auch eine nachträgliche Konstruktion einer bestimmten Sinnhaftigkeit des beschriebenen Lebens. Dies führt weiter zur Frage nach dem subjektiv verstandenen und dem objektiven Leben. Jeder Mensch entwirft seine eigene Biografie in unterschiedlichen Lebenssituationen (beim Bewerbungsgespräch, bei der Aufnahme persönlicher Beziehungen oder allgemeiner bei der eigenen Lebensrückschau, z. B. beim Psychologen oder Psychiater). Biografien bilden auch ein wichtiges Instrument der Erinnerung an andere Personen. Sie sind daher Gegenstand der Literatur- und Geschichtswissenschaft, der Soziologie, der Pädagogik, der Psychologie, der Medizin und der Theologie. Die einzelnen Arbeitsfelder und Arbeitsgegenstände der Biografieforschung sind sehr heterogen und haben eigene Forschungstraditionen entwickelt."@de, "La biografía (del griego βίος [bíos], ‘vida’ y γράφειν [grafein], ‘escribir’) es la historia de la vida de una persona narrada desde su nacimiento hasta su muerte, consignando sus hechos logrados, fracasos, sucesos relevantes de su vida, así como todo lo que pueda interesar de la misma."@es, "Une biographie (une bio), du grec ancien βίος, « la vie » et γραφή, « écrire », est un écrit qui a pour objet l'histoire d'une vie particulière. Elle peut être écrite par la personne elle-même (autobiographie) ou par une autre personne."@fr ;
    skos:inScheme cwrc:Genre ;
    prov:derivedFrom dbpedia:Biography, <http://vocab.getty.edu/aat/300404015> .

cwrc:genreBisexualfiction
    void:inDataset cwrc:datasetdefinition ;
    a cwrc:Genre, skos:Concept ;
    rdf:value "BISEXUALFICTION" ;
    rdfs:isDefinedBy <http://www.cwrc.ca/ontologies/cwrc#> ;
    rdfs:label ""@fr, "bisexual fiction"@en ;
    skos:inScheme cwrc:Genre .

cwrc:genreBlackcomedy
    void:inDataset cwrc:datasetdefinition ;
    a cwrc:Genre, skos:Concept ;
    rdf:value "BLACKCOMEDY" ;
    rdfs:isDefinedBy <http://www.cwrc.ca/ontologies/cwrc#> ;
    rdfs:label ""@fr, "black comedy"@en ;
    owl:comment "This term and its description was created from data gathered from DBpedia."@en ;
    skos:definition "A black comedy (or dark comedy) is a comic work that employs morbid humor, which, in its simplest form, is humor that makes light of subject matter usually considered taboo. Black humor corresponds to the earlier concept of gallows humor. Black comedy is often controversial due to its subject matter.[citation needed]"@en, "Als schwarzer Humor wird Humor bezeichnet, der Verbrechen, Krankheit, Tod und ähnliche Themen, für die gewöhnlich eine Abhandlung in ernster Form erwartet wird, in satirischer oder bewusst verharmlosender Weise verwendet. Oft bezieht er sich auf Zeitthemen. Schwarzer Humor bedient sich häufig paradoxer Stilfiguren. Nicht selten löst er Kontroversen aus darüber, ob man sich über die genannten Dinge lustig machen dürfe und wo die Grenzen des guten Geschmacks lägen; besonders ist dies der Fall, wenn religiöse und sexuelle Themen und tragische Ereignisse zum Gegenstand genommen werden. In der darstellenden Kunst nennt man auf schwarzen Humor setzende Werke schwarze Komödien."@de, "El humor negro es un tipo de humor que se ejerce a propósito de cosas que suscitarían, contempladas desde otra perspectiva, piedad, terror, lástima o emociones parecidas. Cuestiona situaciones sociales que generalmente son serias mediante la sátira. El asunto más recurrente en el humor negro es la muerte y todo lo que está relacionado con ella. Atañe los temas más oscuros y dolorosos para el ser humano y que, por norma general, suelen resultar controvertidos y polémicos para la sociedad porque están relacionados con la moral. Algunos ejemplos pueden ser: las grandes tragedias, las normas sociales, la sexualidad, los asesinatos, el suicidio, las enfermedades, la pobreza, la locura, el terrorismo, el racismo, la drogadicción, la violación, las discapacidades, la guerra, la religión, la política, la discriminación, etc., pero representados en forma cómica."@es, "L’humour noir est une forme d’humour qui souligne avec cruauté, amertume et parfois désespoir l’absurdité du monde, face à laquelle il constitue quelquefois une forme de défense."@fr, "Zwarte humor is een vorm van humor, gebaseerd op het leed van anderen met als doel te spotten en te amuseren. Hierbij is er een zekere overeenkomst met het (psychologisch) cynisme, waarbij een negatieve houding tegenover (een deel van) de maatschappij tot uiting komt. Vaak wordt deze, meestal overdreven, vorm van humor gebruikt om het leed te relativeren of een reactie bij de toeschouwer te ontlokken. Zwarte humor draait vaak rond taboe-onderwerpen die over het algemeen erg gevoelig liggen bij de meeste mensen, zoals dood, geweld, ziekte, moord, zelfmoord, natuurrampen, ongevallen, handicaps, drugs, mishandeling, hongersnood, armoede, kindermisbruik, verkrachting, racisme, discriminatie, genocide, de holocaust en de Tweede Wereldoorlog. In normale omstandigheden wordt humor rond deze deprimerende thema's afgekeurd of bijzonder smakeloos gevonden. Veel mensen die gebruikmaken van zwarte humor proberen hun publiek hiermee dan ook ongemakkelijk te maken of te choqueren. Op het juiste moment en in de juiste omstandigheden kan deze vorm van humor echter ook helpen om spanningen weg te nemen of het leed te relativeren. Doordat echter elk individu zijn eigen morele en ethische grenzen heeft is de reactie bij het publiek niet altijd in te schatten."@nl ;
    skos:inScheme cwrc:Genre ;
    prov:derivedFrom dbpedia:Black_comedy .

cwrc:genreBoutsrimes
    void:inDataset cwrc:datasetdefinition ;
    a cwrc:Genre, skos:Concept ;
    rdf:value "BOUTSRIMES" ;
    rdfs:isDefinedBy <http://www.cwrc.ca/ontologies/cwrc#> ;
    rdfs:label ""@fr, "boutsrimes"@en ;
    skos:inScheme cwrc:Genre .

cwrc:genreBroadside
    void:inDataset cwrc:datasetdefinition ;
    a cwrc:Genre, skos:Concept ;
    rdf:value "BROADSIDE" ;
    rdfs:isDefinedBy <http://www.cwrc.ca/ontologies/cwrc#> ;
    rdfs:label ""@fr, "broadside"@en ;
    skos:inScheme cwrc:Genre .

cwrc:genreBurletta
    void:inDataset cwrc:datasetdefinition ;
    a cwrc:Genre, skos:Concept ;
    rdf:value "BURLETTA" ;
    rdfs:isDefinedBy <http://www.cwrc.ca/ontologies/cwrc#> ;
    rdfs:label ""@fr, "burletta"@en ;
    skos:inScheme cwrc:Genre .

cwrc:genreCabaret
    void:inDataset cwrc:datasetdefinition ;
    a cwrc:Genre, skos:Concept ;
    rdf:value "CABARET" ;
    rdfs:isDefinedBy <http://www.cwrc.ca/ontologies/cwrc#> ;
    rdfs:label ""@fr, "cabaret"@en ;
    skos:inScheme cwrc:Genre .

cwrc:genreCaptivitynarrative
    void:inDataset cwrc:datasetdefinition ;
    a cwrc:Genre, skos:Concept ;
    rdf:value "CAPTIVITYNARRATIVE" ;
    rdfs:isDefinedBy <http://www.cwrc.ca/ontologies/cwrc#> ;
    rdfs:label ""@fr, "captivity narrative"@en ;
    owl:comment "This term and its description was created from data gathered from DBpedia."@en ;
    skos:definition "Captivity narratives are usually stories of people captured by enemies whom they consider uncivilized, or whose beliefs and customs they oppose. The best-known captivity narratives are those concerning the indigenous peoples of North America. These narratives (and questions about their accuracy) have an enduring place in literature, history, ethnography, and the study of Native peoples. However, captivity narratives have also come to play a major role in the study of contemporary religious movements, thanks to scholars of religion like David G. Bromley and James R. Lewis. In this article, both main types of captivity narratives are considered. Traditionally, historians have made limited use of certain captivity narratives. They have regarded the genre with suspicion because of its ideological underpinnings. As a result of new scholarly approaches, historians with a more certain grasp of Native American cultures are distinguishing between plausible statements of fact and value-laden judgements in order to study the narratives as rare sources from \"inside\" Native societies. Contemporary historians such as Linda Colley and anthropologists such as Pauline Turner Strong have also found the narratives useful in analyzing how the colonists constructed the \"other\", as well as what the narratives reveal about the settlers' sense of themselves and their culture, and the experience of crossing the line to another. Colley has studied the long history of English captivity in other cultures, both the Barbary pirate captives who preceded those in North America, and British captives in cultures such as India, after the North American experience. Certain North American captivity narratives involving Native peoples were published from the 18th through the 19th centuries, but they reflected a well-established genre in English literature. There had already been English accounts of captivity by Barbary pirates, or in the Middle East, which established some of the major elements of the form. Following the American experience, additional accounts were written after British people were captured during exploration and settlement in India and East Asia. Other types of captivity narratives, such as those recounted by apostates from religious movements (i.e. \"cult survivor\" tales), have remained an enduring feature of modern media, and currently appear in books, periodicals, film, and television. The unifying factor in most captivity narratives, whether they stem from geopolitical or religious conflicts, is that the captive portrays the captors' way of life as alien, undesirable, and incompatible with the captive's own (typically dominant) culture. This underscores the utility of captivity narratives in garnering support for social control measures, such as removing Native Americans to \"reservations\", or stigmatizing participation in religious movements – whether Catholicism in the nineteenth century, or ISKCON in the twentieth. Captivity narratives tend to be culturally chauvinistic, viewing an \"alien\" culture through the lens of the narrator's preferred culture, thus making (possibly unfair) value judgements like \"Puritans good, Indians bad.\""@en, "Der Ausdruck captivity narrative bezeichnet ein eigenständiges Genre der amerikanischen Literatur, das die Erfahrungen weißer Siedler in Nordamerika, zumeist Frauen, in indianischer Gefangenschaft schildert. Captivity narratives hatten im 17. Jahrhundert einen erheblichen Einfluss sowohl auf die autobiografische Literatur als auch später auf den amerikanischen Roman. Bekannt in diesem Zusammenhang wurden u.a. die Schicksale von Mary Rowlandson (1637–1711), Elizabeth Hanson (1684–1737) oder Cynthia Ann Parker (1826–1870)."@de ;
    skos:inScheme cwrc:Genre ;
    prov:derivedFrom dbpedia:Captivity_narrative .

cwrc:genreCatechism
    void:inDataset cwrc:datasetdefinition ;
    a cwrc:Genre, skos:Concept ;
    rdf:value "CATECHISM" ;
    rdfs:isDefinedBy <http://www.cwrc.ca/ontologies/cwrc#> ;
    rdfs:label ""@fr, "catechism"@en ;
    owl:comment "This term and its description was created from data gathered from DBpedia."@en ;
    skos:definition "A catechism (/ˈkætəˌkizəm/; from Greek: κατηχέω, to teach orally), is a summary or exposition of doctrine and served as a learning introduction to the Sacraments traditionally used in catechesis, or Christian religious teaching of children and adult converts. Catechisms are doctrinal manuals - often in the form of questions followed by answers to be memorised - a format in non-religious or secular contexts as well. The term catechumen refers to the designated recipient of the catechetical work or instruction. In the Catholic Church, catachumens were usually placed separately during Holy Mass from those who received the Sacrament of Baptism. Early catecheticals emerged from Graeco-Roman mystery religions, especially the late cult of Mithras meant to educate their members into the secretive teachings, which competed with the Christian Church as an underground religion in the 1st to 4th centuries CE and allegedly shared its many ritual practices. Today, they are characteristic of Western Christianity but are also present in Eastern Christianity."@en, "Dans la religion chrétienne, le catéchisme désigne l'instruction des doctrines de la foi chrétienne, particulièrement destinée aux enfants. Il prend souvent la forme d'une exposé officiel des articles de la foi, servant d'outil de base pour la catéchèse, qui est l'ensemble des actions destinées à éduquer des enfants, des jeunes et des adultes à la doctrine chrétienne. La catéchèse est une des composantes de la mission évangélique du christianisme."@fr, "Der Katechismus ist seit dem Beginn der Neuzeit ein Handbuch der Unterweisung in den Grundfragen des christlichen Glaubens. Mit dem Wort Katechismus wurde auch die Taufkatechese für die Erwachsenen und seit der Einführung der Kindertaufe das Glaubensexamen der Taufpaten bezeichnet."@de, "Een catechismus (van het Griekse: Κατήχησις, katechesis = onderricht) is een opsomming van de leer van een bepaald kerkgenootschap waarin al zijn dogma's systematisch en voor leken begrijpelijk worden gegeven en uitgelegd. Omdat ze een middel zijn bij de catechese, worden ze vaak in vraag- en antwoordvorm uitgegeven."@nl, "El catecismo (del griego κατηχισμός, de kata [«abajo»] + echein [«sonar»], literalmente «sonar abajo» (dentro de los oídos), es decir, «adoctrinar») es el texto en el que se presenta una exposición orgánica y sintética de los contenidos esenciales y fundamentales de la doctrina cristiana tanto sobre la fe como sobre la moral. A lo largo de la historia han existido diversos tipos de catecismos, y la mayoría de iglesias y denominaciones cristianas cuentan con sus propias ediciones. En el caso de la Iglesia católica, sus catecismos se basan principalmente en la Tradición de la Iglesia interpretada a la luz del Concilio Vaticano II. Sus fuentes principales son la Sagrada Escritura, los Santos Padres, la Liturgia y el Magisterio de la Iglesia. Está destinado a servir \"como un punto de referencia para los catecismos o compendios que sean compuestos en los diversos países\" (Sínodo de los Obispos 1985. Relación final II B A 4). Existe una versión in extenso promulgada el 11 de octubre de 1992 por Juan Pablo II y el Compendio, promulgado por el Papa Benedicto XVI el 28 de junio de 2005, que es una síntesis fiel y segura del Catecismo de la Iglesia católica. Contiene, de modo conciso, todos los elementos esenciales y fundamentales de la fe de la Iglesia, de manera tal que constituye, de acuerdo a lo descrito en su presentación por el Papa \"una especie de vademécum, a través del cual las personas, creyentes o no, pueden abarcar con una sola mirada de conjunto el panorama completo de la fe católica\"."@es ;
    skos:inScheme cwrc:Genre ;
    prov:derivedFrom dbpedia:Catechism .

cwrc:genreChapbook
    void:inDataset cwrc:datasetdefinition ;
    a cwrc:Genre, skos:Concept ;
    rdf:value "CHAPBOOK" ;
    rdfs:isDefinedBy <http://www.cwrc.ca/ontologies/cwrc#> ;
    rdfs:label ""@fr, "chapbook"@en ;
    skos:inScheme cwrc:Genre .

cwrc:genreCharacter
    void:inDataset cwrc:datasetdefinition ;
    a cwrc:Genre, skos:Concept ;
    rdf:value "CHARACTER" ;
    rdfs:isDefinedBy <http://www.cwrc.ca/ontologies/cwrc#> ;
    rdfs:label ""@fr, "character"@en ;
    skos:inScheme cwrc:Genre .

cwrc:genreCharade
    void:inDataset cwrc:datasetdefinition ;
    a cwrc:Genre, skos:Concept ;
    rdf:value "CHARADE" ;
    rdfs:isDefinedBy <http://www.cwrc.ca/ontologies/cwrc#> ;
    rdfs:label "charade"@en, "charade"@fr ;
    skos:inScheme cwrc:Genre .

cwrc:genreChildrensLiterature
    void:inDataset cwrc:datasetdefinition ;
    a cwrc:Genre, skos:Concept ;
    rdf:value "CHILDRENSLITERATURE" ;
    rdfs:isDefinedBy <http://www.cwrc.ca/ontologies/cwrc#> ;
    rdfs:label "childrens literature"@en, "littérature pour l'enfants"@fr ;
    skos:inScheme cwrc:Genre .

cwrc:genreClerihew
    void:inDataset cwrc:datasetdefinition ;
    a cwrc:Genre, skos:Concept ;
    rdf:value "CLERIHEW" ;
    rdfs:isDefinedBy <http://www.cwrc.ca/ontologies/cwrc#> ;
    rdfs:label ""@fr, "clerihew"@en ;
    owl:comment "This term and its description was created from data gathered from DBpedia."@en ;
    skos:definition "A clerihew is a whimsical, four-line biographical poem invented by Edmund Clerihew Bentley. The first line is the name of the poem's subject, usually a famous person put in an absurd light. The rhyme scheme is AABB, and the rhymes are often forced. The line length and metre are irregular. Bentley invented the clerihew in school and then popularized it in books. One of his best known is this (1905):"@en, "De clerihew is een zogenaamd light verse (gedicht) bedacht door Edmund Clerihew Bentley (1875-1956). De volgende regels zijn van toepassing op een clerihew: Voorbeeld in het Engels:Our art teacher, Mr. Shaw, Really knows how to draw. But his awful paintings Have caused many faintings. Voorbeeld van Drs. P:Karel IXWou dat het koppen regendeToen de Bartolomeusnacht werd afgeflotenZei hij zelfs: Ik heb (Hu!) genoten!"@nl, "Ein Clerihew ist ein kurzer scherzhafter pseudobiographischer Vierzeiler, eine Gedichtform, die von Edmund Clerihew Bentley (1875–1956) erfunden wurde. Er besteht aus zwei Reimpaaren mit ungleichmäßiger Länge und mehr oder weniger freiem Rhythmus. Der Name der historischen Person steht dabei meist am Ende der ersten oder der zweiten Verszeile. Der Clerihew ist eher wunderlich und schrullig als satirisch.Die Verszeilen sind auf komische Weise irregulär (unregelmäßige Verslänge, unregelmäßiger – nicht aber freier – Rhythmus)."@de ;
    skos:inScheme cwrc:Genre ;
    prov:derivedFrom dbpedia:Clerihew .

cwrc:genreClosetdrama
    void:inDataset cwrc:datasetdefinition ;
    a cwrc:Genre, skos:Concept ;
    rdf:value "CLOSETDRAMA" ;
    rdfs:isDefinedBy <http://www.cwrc.ca/ontologies/cwrc#> ;
    rdfs:label ""@fr, "closetdrama"@en ;
    skos:inScheme cwrc:Genre .

cwrc:genreColouringbook
    void:inDataset cwrc:datasetdefinition ;
    a cwrc:Genre, skos:Concept ;
    rdf:value "COLOURINGBOOK" ;
    rdfs:isDefinedBy <http://www.cwrc.ca/ontologies/cwrc#> ;
    rdfs:label ""@fr, "colouring book"@en ;
    owl:comment "This term and its description was created from data gathered from the Getty Art & Architecture Thesaurus."@en ;
    skos:definition "Boeken met omtrektekeningen die kunnen worden ingekleurd met tekenstiften, aquarelverf, kleurpotloden of andere middelen, gewoonlijk bedoeld voor kinderen."@nl, "Books containing outline drawings, for coloring in with crayons, watercolor, colored pencils, or other media, usually intended for use by children."@en, "Buch mit Umrisszeichnungen zum farbigen Ausmalen mit Wachsstiften, Wasserfarben, Buntstiften oder anderen Medien, in der Regel für Kinder gedacht."@de, "Libros que contienen dibujos de contornos, para ser coloreados con lápices de cera, acuarelas, lápices de colores, u otros medios, generalmente destinados a niños."@es, "內含圖畫輪廓的書本，可用蠟筆、水彩、彩色鉛筆、或其他材料，加以著色，使用對象通常為兒童。"@zh-hant ;
    skos:inScheme cwrc:Genre ;
    prov:derivedFrom <http://vocab.getty.edu/aat/300026449> .

cwrc:genreComedy
    void:inDataset cwrc:datasetdefinition ;
    a cwrc:Genre, skos:Concept ;
    rdf:value "COMEDY" ;
    rdfs:isDefinedBy <http://www.cwrc.ca/ontologies/cwrc#> ;
    rdfs:label "comedy"@en, "comédie"@fr ;
    owl:comment "This term and its description was created from data gathered from the Getty Art & Architecture Thesaurus."@en ;
    skos:definition "Historias livianas y entretenidas."@es, "Leichte und amüsante Geschichte."@de, "Lichte en amusante verhalen."@nl, "Light and amusing stories."@en ;
    skos:inScheme cwrc:Genre ;
    prov:derivedFrom <http://vocab.getty.edu/aat/300201014> .

cwrc:genreComedyofintrigue
    void:inDataset cwrc:datasetdefinition ;
    a cwrc:Genre, skos:Concept ;
    rdf:value "COMEDYOFINTRIGUE" ;
    rdfs:isDefinedBy <http://www.cwrc.ca/ontologies/cwrc#> ;
    rdfs:label ""@fr, "comedy of intrigue"@en ;
    skos:broaderTransitive cwrc:genreComedy ;
    skos:inScheme cwrc:Genre .

cwrc:genreComedyofmanners
    void:inDataset cwrc:datasetdefinition ;
    a cwrc:Genre, skos:Concept ;
    rdf:value "COMEDYOFMANNERS" ;
    rdfs:isDefinedBy <http://www.cwrc.ca/ontologies/cwrc#> ;
    rdfs:label ""@fr, "comedy of manners"@en ;
    owl:comment "This term and its description was created from data gathered from DBpedia."@en ;
    skos:broaderTransitive cwrc:genreComedy ;
    skos:definition "Ein Konversationsstück, auch Gesellschaftsstück, ist eine Form der Komödie. Im Vordergrund eines Konversationsstückes steht der geistreiche, witzig-pointierte Dialog. Theaterstücke, die als Konversationsstücke gelten, entstanden vor allem in der zweiten Hälfte des 19. Jahrhunderts, seltener im 20. Jahrhundert in England und Frankreich. Der Literaturwissenschaftler Péter Szondi beschrieb den Begriff, indem er das Konversationsstück als „Rettungsversuch des Dramas durch die Rettung des Dialogs, der allerdings zur bloßen Konvention wird“ charakterisierte. Die Handlung, die in den höheren Gesellschaftskreisen spielt, wird durch von außen kommende Ereignisse vorangetrieben. Themen sind unter anderem das Frauenstimmrecht, die freie Liebe, die Mesalliance oder der Sozialismus. Bedeutende Vertreter des Konversationsstückes sind in Frankreich Eugène Scribe, Victorien Sardou und Sacha Guitry, in Großbritannien Oscar Wilde, George Bernhard Shaw und Thomas Stearns Eliot. Im deutschsprachigen Raum fehlte für die Ausbildung typischer Konversationsstücke weitgehend der gesellschaftliche Hintergrund. Werke von Hermann Bahr und Arthur Schnitzler können dem Genre noch am ehesten zugerechnet werden. Hugo von Hofmannsthal schuf 1921 mit Der Schwierige, wo die inhaltsleere Konversation selbst zum Thema wird, ein Zerrbild des Konversationsstücks."@de, "La comedia de costumbres es un subgénero dramático que describe con ironía y agudeza la vida cotidiana de una época o de una clase social concreta, por lo general la clase media o burguesa. El Diccionario Oxford la describe como \"Comedia cuyo asunto principal es la presentación de la forma de conducta de los personajes y la descripción de ambientes de la vida social cotidiana\". Trata siempre de los actos comunes de la vida social ordinaria, tanto en el plano egocéntrico (familia, amistades, centro de trabajo...) como en el sociocéntrico (vida política, relaciones institucionales...). Se halla emparentada con el llamado costumbrismo literario o cuadro de costumbres y se destina a un público que suele ser el mismo que aparece caricaturizado, reflejando la destreza o torpeza con que ciertos personajes siguen las pautas convencionales de comportamiento de su entorno, pautas que pueden ser tan rigurosas o banales moralmente cuanto su público pueda soportar, ya que su crítica social suele ser y de hecho es superficial, no toca a los pilares fundamentales de la sociedad y se suele desvanecer fácilmente. Lope de Vega (El perro del hortelano), Molière (Las preciosas ridículas, La escuela de las mujeres), Manuel Bretón de los Herreros (El pelo de la dehesa) y Jacinto Benavente (Pepa Doncel) destacaron escribiendo este tipo de comedias. La trama suele ser algún romance no permitido o algún otro asunto escandaloso, pero es menos importante que los diálogos ingeniosos, los comentarios punzantes sobre las flaquezas humanas y la atmósfera llena de susceptibilidades de la obra. Lope de Vega, Tirso de Molina, Agustín Moreto y otros dramaturgos del s. XVII español fueron los primeros creadores de este tipo de comedias que fueron imitadas y desarrolladas en el XVIII por los franceses (Molière especialmente) e italianos (Carlo Goldoni, quien la imbricó con la Commedia dell'Arte); en Inglaterra se desarrolló a través de las piezas de William Congreve, Oliver Goldsmith y Richard Brinsley Sheridan, y ya en el XIX con las de Óscar Wilde; en el siglo XX destacan las de Noël Coward. En Francia siguieron el género en el XIX Dumas hijo, Eugène Scribe y Victorien Sardou entre otros y, ya en el siglo XX, Sacha Guitry."@es, "La comédie de mœurs est un sous-genre de la comédie qui se développe à partir du XVIe siècle. Y sont dénoncés les travers d'une époque, d'un groupe ou d'une classe sociale, généralement dominante. La comédie de mœurs est souvent caractérisée par une critique sociale qui reste superficielle. Généralement la dimension satirique ne vise qu'un travers particulier ou une convention risible très ciblée de la communauté dépeinte. En ce sens, la comédie de mœurs ne remet souvent rien de fondamental en cause dans la structure sociale ni dans la représentation dominante de l'époque. La critique s'efface vite et devient récupérable par l'ordre en place, comme dans les pièces d'Émile Augier ou d'Alexandre Dumas fils. Cependant, le dénouement peut aussi être impressionnant, comme celui des Affaires sont les affaires du libertaire Octave Mirbeau (1903), parfois qualifié de \"shakespearien\". Plusieurs comédies très connues de Molière sont des comédies de mœurs : Les Précieuses ridicules ou encore Les Femmes savantes mais aussi L'École des femmes. Pour Molière, la comédie de mœurs représente un lieu privilégié pour la satire sociale."@fr, "The comedy of manners is an entertainment form which satirizes the manners and affectations of a social class or of multiple classes, often represented by stereotypical stock characters. For example, the miles gloriosus (\"boastful soldier\") in ancient times, the fop and the rake during the English Restoration, or an old person pretending to be young. Restoration comedy is used as a synonym for \"comedy of manners\". The plot of the comedy, often concerned with scandal, is generally less important than its witty dialogue. A great writer of comedies of manners was Oscar Wilde, his most famous play being The Importance of Being Earnest. The comedy of manners was first developed in the new comedy of the Ancient Greek playwright Menander. His style, elaborate plots, and stock characters were imitated by the Roman playwrights Plautus and Terence, whose comedies were widely known and copied during the Renaissance. The best-known comedies of manners, however, may well be those of the French playwright Molière, who satirized the hypocrisy and pretension of the ancien régime in such plays as L'École des femmes (The School for Wives, 1662), Le Misanthrope (The Misanthrope, 1666), and most famously Tartuffe (1664)."@en ;
    skos:inScheme cwrc:Genre ;
    prov:derivedFrom dbpedia:Comedy_of_manners .

cwrc:genreComedyofmenace
    void:inDataset cwrc:datasetdefinition ;
    a cwrc:Genre, skos:Concept ;
    rdf:value "COMEDYOFMENACE" ;
    rdfs:isDefinedBy <http://www.cwrc.ca/ontologies/cwrc#> ;
    rdfs:label ""@fr, "comedy of menace"@en ;
    skos:broaderTransitive cwrc:genreComedy ;
    skos:inScheme cwrc:Genre .

cwrc:genreComicbook
    void:inDataset cwrc:datasetdefinition ;
    a cwrc:Genre, skos:Concept ;
    rdf:value "COMICBOOK" ;
    rdfs:isDefinedBy <http://www.cwrc.ca/ontologies/cwrc#> ;
    rdfs:label ""@fr, "comicbook"@en ;
    skos:inScheme cwrc:Genre .

cwrc:genreComingout
    void:inDataset cwrc:datasetdefinition ;
    a cwrc:Genre, skos:Concept ;
    rdf:value "COMINGOUT" ;
    rdfs:isDefinedBy <http://www.cwrc.ca/ontologies/cwrc#> ;
    rdfs:label ""@fr, "coming out"@en ;
    skos:inScheme cwrc:Genre .

cwrc:genreCommonplacebook
    void:inDataset cwrc:datasetdefinition ;
    a cwrc:Genre, skos:Concept ;
    rdf:value "COMMONPLACEBOOK" ;
    rdfs:isDefinedBy <http://www.cwrc.ca/ontologies/cwrc#> ;
    rdfs:label ""@fr, "common place book"@en ;
    skos:inScheme cwrc:Genre .

cwrc:genreCompanion
    void:inDataset cwrc:datasetdefinition ;
    a cwrc:Genre, skos:Concept ;
    rdf:value "COMPANION" ;
    rdfs:isDefinedBy <http://www.cwrc.ca/ontologies/cwrc#> ;
    rdfs:label ""@fr, "companion"@en ;
    skos:inScheme cwrc:Genre .

cwrc:genreComputerprogram
    void:inDataset cwrc:datasetdefinition ;
    a cwrc:Genre, skos:Concept ;
    rdf:value "COMPUTERPROGRAM" ;
    rdfs:isDefinedBy <http://www.cwrc.ca/ontologies/cwrc#> ;
    rdfs:label ""@fr, "computer program"@en ;
    skos:inScheme cwrc:Genre .

cwrc:genreConditionofenglandnovel
    void:inDataset cwrc:datasetdefinition ;
    a cwrc:Genre, skos:Concept ;
    rdf:value "CONDITIONOFENGLANDNOVEL" ;
    rdfs:isDefinedBy <http://www.cwrc.ca/ontologies/cwrc#> ;
    rdfs:label ""@fr, "condition of england novel"@en ;
    skos:broaderTransitive cwrc:genreNovel ;
    skos:inScheme cwrc:Genre .

cwrc:genreConductliterature
    void:inDataset cwrc:datasetdefinition ;
    a cwrc:Genre, skos:Concept ;
    rdf:value "CONDUCTLITERATURE" ;
    rdfs:isDefinedBy <http://www.cwrc.ca/ontologies/cwrc#> ;
    rdfs:label ""@fr, "conduct literature"@en ;
    skos:inScheme cwrc:Genre .

cwrc:genreCookbook
    void:inDataset cwrc:datasetdefinition ;
    a cwrc:Genre, skos:Concept ;
    rdf:value "COOKBOOK" ;
    rdfs:isDefinedBy <http://www.cwrc.ca/ontologies/cwrc#> ;
    rdfs:label ""@fr, "cookbook"@en ;
    owl:comment "This term and its description was created from data gathered from DBpedia."@en ;
    skos:definition "A cookbook (sometimes cookery book in Commonwealth English or cook book) is a kitchen reference publication that typically contains a collection of recipes. Modern versions may also include colorful illustrations and advice on purchasing quality ingredients or making substitutions. Cookbooks can also cover a wide variety of topics, including cooking techniques for the home, recipes and commentary from famous chefs, institutional kitchen manuals, and cultural commentary."@en, "El libro de cocina (también recetario) es una colección de recetas de cocina elaboradas por un cocinero famoso que suele exponer algunos trucos culinarios y diferentes experiencias personales. Uno de los más antiguos en lengua europea distinta del latín es el Llibre de Sent Soví, del que se conserva un manuscrito de 1313 o antes, pudiendo ser de 1024. También hay otros, como el escrito por Guillaume Tirel (1326 - 1395) durante la Gastronomía de la Edad Media, cuyo alias fue Taillevent."@es, "In een kookboek vindt men recepten voor de bereiding van voedsel, en informatie over het bereiden van voedsel in het algemeen. Kookboeken worden soms ware bestsellers, zoals de boeken van Jamie Oliver. In een kookboek staan, behalve recepten, informatie over het gebruik van een oven, definities of omschrijvingen van bereidingstechnieken en gewichtstabellen. Kookboeken zijn meestal opgedeeld in verschillende hoofdstukken, die ieder een andere gerechtsoort behandelen (voorgerechten, hoofdgerechten, nagerechten). Westerse kookboeken categoriseren de recepten voor hoofdgerechten meestal op basis van ingrediënten. In Japanse kookboeken worden de gerechten vaak gegroepeerd per kooktechniek (bijvoorbeeld braden, grillen en stomen)."@nl, "Kochbücher beschreiben in Rezepten die Zubereitung von Speisen. Sie sind grob in drei Kategorien zu unterteilen: Der Begriff „Rezept“ für die Kochanweisung weist auf die Verbindung zwischen Heilkunst und Ernährung hin. Auch in der chemischen Industrie steht „Rezeptur“ für eine Liste chemischer Stoffe zur Bereitung eines anderen chemischen Stoffes. So schrieben Ärzte im alten Griechenland nicht nur Rezepte für Medikamente, sondern auch für Gerichte (Diät)."@de, "Un livre de cuisine est un recueil de recettes ou de considérations gastronomiques."@fr ;
    skos:inScheme cwrc:Genre ;
    prov:derivedFrom dbpedia:Cookbook .

cwrc:genreCourtshipfiction
    void:inDataset cwrc:datasetdefinition ;
    a cwrc:Genre, skos:Concept ;
    rdf:value "COURTSHIPFICTION" ;
    rdfs:isDefinedBy <http://www.cwrc.ca/ontologies/cwrc#> ;
    rdfs:label ""@fr, "courtshipfiction"@en ;
    skos:inScheme cwrc:Genre .

cwrc:genreCriminology
    void:inDataset cwrc:datasetdefinition ;
    a cwrc:Genre, skos:Concept ;
    rdf:value "CRIMINOLOGY" ;
    rdfs:isDefinedBy <http://www.cwrc.ca/ontologies/cwrc#> ;
    rdfs:label ""@fr, "criminology"@en ;
    skos:inScheme cwrc:Genre .

cwrc:genreDedication
    void:inDataset cwrc:datasetdefinition ;
    a cwrc:Genre, skos:Concept ;
    rdf:value "DEDICATION" ;
    rdfs:isDefinedBy <http://www.cwrc.ca/ontologies/cwrc#> ;
    rdfs:label ""@fr, "dedication"@en ;
    skos:inScheme cwrc:Genre .

cwrc:genreDetective
    void:inDataset cwrc:datasetdefinition ;
    a cwrc:Genre, skos:Concept ;
    rdf:value "DETECTIVE" ;
    rdfs:isDefinedBy <http://www.cwrc.ca/ontologies/cwrc#> ;
    rdfs:label ""@fr, "detective"@en ;
    owl:comment "This term and its description was created from data gathered from DBpedia."@en ;
    skos:definition "Detective Comics es un comic book publicado por DC Comics desde 1937. Es, junto con Action Comics (donde apareció por primera vez Superman), uno de los títulos más conocidos de la empresa; de hecho, el nombre de ésta (DC) proviene de Detective Comics. Con más de 800 números es el comic book de más larga publicación continua en EE. UU. Mantiene, como en sus orígenes, una periodicidad mensual. En este comic book hicieron su aparición decenas de superhéroes, siendo el más reconocido Batman, en Detective Comics #27, de mayo de 1939. El 26 de febrero de 2010, un coleccionista anónimo, pagó $1.075.000 dólares (789.077 euros) por este número 27, tratándose de una de las cantidades más altas pagadas por un comic book hasta el momento."@es, "Detective Comics est un comics publié par DC Comics depuis mars 1937. C'est l'un des titres les plus connus de la société (avec Action Comics qui vit naître Superman). En fait, le « DC » de l'éditeur vient des initiales de Detective Comics. C'est aussi le comics à la plus grande longévité puisqu'il est toujours publié aux États-Unis en 2011. Cependant, à l'occasion de la recréation de l'univers DC après les évènements racontés dans la minisérie Flashpoint, Detective Comics a commencé une nouvelle numérotation en septembre 2011. À l'origine le comics publiait diverses histoires, principalement de détectives (genre le plus populaire de l'époque). Le premier numéro comportait des histoires avec les personnages « Ching Lung » (un méchant oriental dans le style Fu Manchu), Slam Bradley (créé par Jerry Siegel et Joe Shuster), et Speed Saunders, parmi d'autres. La gloire de Detective Comics fut assurée lors des débuts en ses pages de Batman (appelé tout d'abord « The Bat-Man ») dans le numéro #27 (le numéro de Mai 1939, publié en mars 1939). Il devint le héros principal de la publication. Des exemplaires en bon état de ce numéro ont atteint les valeurs de 80 000 $ en 1992 et 300 000 $ en 2003, d'après Stephen Fishler. Le compagnon de Batman, Robin, fit ses débuts dans le numéro #38 (d'avril 1940). Son apparence (et les ventes croissantes du périodique) conduisirent rapidement à l'essor des justiciers costumés et leurs jeunes compagnons dans les comics de cette époque. En plus des aventures de Batman, Detective Comics publia aussi Martian Manhunter (apparu dans une histoire complémentaire (back-up) de Detective Comics #225 en 1955). À la fin des années 1970s, il ajouta des séries dérivées comme Robin: the Teen Wonder, Batgirl (apparue dans Detective Comics #359 en 1967), The Human Target et les anthologies Tales of Gotham City (des histoires d'habitants ordinaires de Gotham City)."@fr, "Detective Comics is de naam van de comicreeks waarin een personage genaamd Batman in 1939 voor de allereerste keer opdook. Bedenker Bob Kane introduceerde Vleermuisman, zoals hij in Nederland eerst genoemd werd, in deel 27. De serie loopt anno 2016 nog steeds. Behalve Batman zagen ook veel van de personages die tegenwoordig de cast vormen van de vele Batmancomics, -films, -series en tekenfilms in Detective Comics voor het eerst het levenslicht. Bijvoorbeeld Robin (in deel 38), Penguin (deel 58), Two-Face (deel 66), en de Riddler (deel 140). Mits in goede staat, zijn deze delen van Detective Comics tegenwoordig voor veel speculanten en verzamelaars vele duizenden dollars waard. Detective Comics 27 is de op-één-na meest waardevolle comic ter wereld, na Action Comics 1."@nl, "Detective Comics is the title used for two American comic book series published by DC Comics. The first, published from 1937 to 2011, was best known for introducing the superhero Batman in Detective Comics #27 (cover dated May 1939). A second series of the same title was launched in the fall of 2011. The original series is the source of its publishing company's name and with Action Comics, the comic book launched with the debut of Superman, one of the medium's signature series. The original series published 881 issues between 1937 and 2011 and was the longest continuously published comic book in the United States."@en ;
    skos:inScheme cwrc:Genre ;
    prov:derivedFrom dbpedia:Detective_Comics .

cwrc:genreDevotional
    void:inDataset cwrc:datasetdefinition ;
    a cwrc:Genre, skos:Concept ;
    rdf:value "DEVOTIONAL" ;
    rdfs:isDefinedBy <http://www.cwrc.ca/ontologies/cwrc#> ;
    rdfs:label "devotional"@en, "dévotional"@fr ;
    owl:comment "This term and its description was created from data gathered from DBpedia."@en ;
    skos:definition "Christian devotional literature (also called devotionals or Christian living literature) is religious writing that is neither doctrinal nor theological, but designed for individuals to read for their personal edification and spiritual formation. Theologian Karl Holl has suggested that devotional literature came into full development at the time of Pietism during the second half of the 17th century."@en, "Der Begriff Erbauungsliteratur, der erstmals um das 14. Jahrhundert erwähnt wird, beschreibt ursprünglich volksnahe Schriften mit religiöser Motivation. Bei der Erbauungsliteratur handelt es sich nicht um theologische Literatur, da sie keine wissenschaftlichen Diskurse verfolgt und keine dogmatischen Absichten besitzt. Vielmehr war mit den Veränderungen der Neuzeit eine Konzentration auf die Innerlichkeit zu verzeichnen, die sich im Bereich der Religion in der Beobachtung der Frömmigkeit Gestalt schuf. Es handelte sich um eine Anleitung für ein tugendhaftes Leben, die emotional den Geist erbauen sollte. Eine Wurzel hat die Erbauungsliteratur in der Heiligenlegende. Weitere Formen sind Andachtsbuch, Gebetbuch, Stundenbuch oder Sammlungen von Predigten. Erbauungsliteratur war jahrhundertelang weit verbreitet, einzelne Ausgaben wurden sogar über Konfessionsgrenzen hinweg gelesen. Sie trat anfänglich auf in Gestalt religiöser Biografien oder Bekehrungsgeschichten, aber auch in Gestalt von Kirchenliedern, die nicht selten zu diesem Zweck geschaffen wurden. Das 17. Jahrhundert schuf zahlreiche literarisch bedeutende Schriften von bekannten Barockdichtern wie Johann Arndt, Johann Michael Dilherr, Jeremias Drexel, Paul Gerhardt, Johannes Lassenius, Joachim Meichel, Martin Moller, Heinrich Müller und Christian Scriver. Aufgrund der bewussten Schlichtheit der Inhalte wurde der Begriff in späterer Zeit auch negativ wertend gebraucht. Im 19. Jahrhundert verstand man deshalb unter Erbauungsliteratur auch kitschige oder einfältige Literatur. Mit der Industrialisierung des Buchdrucks erwuchs zunächst in den 100.000-fach vertriebenen erbaulichen Traktaten eine eigene Literaturform. Begonnen mit den im angelsächsischen Bereich entstehenden Traktatgesellschaften, verbunden mit dem Aufkommen des Kolportagehandels setzte sich diese Vertriebsform rasch im gesamten europäischen Raum durch. Bahnbrecher des Vertriebs von Erbauungsliteratur im deutschsprachigen Raum waren damals u.a. das Haus Bertelsmann sowie der Christliche Verein im nördlichen Deutschland. Im 19. Jahrhundert wurde Erbauungsliteratur zunehmend durch die Unterhaltungsliteratur verdrängt."@de ;
    skos:inScheme cwrc:Genre ;
    prov:derivedFrom dbpedia:Christian_devotional_literature .

cwrc:genreDialogueofthedead
    void:inDataset cwrc:datasetdefinition ;
    a cwrc:Genre, skos:Concept ;
    rdf:value "DIALOGUEOFTHEDEAD" ;
    rdfs:isDefinedBy <http://www.cwrc.ca/ontologies/cwrc#> ;
    rdfs:label ""@fr, "dialogue of the dead"@en ;
    skos:inScheme cwrc:Genre .

cwrc:genreDialogueordebate
    void:inDataset cwrc:datasetdefinition ;
    a cwrc:Genre, skos:Concept ;
    rdf:value "DIALOGUEORDEBATE" ;
    rdfs:isDefinedBy <http://www.cwrc.ca/ontologies/cwrc#> ;
    rdfs:label ""@fr, "dialogue or debate"@en ;
    skos:inScheme cwrc:Genre .

cwrc:genreDiary
    void:inDataset cwrc:datasetdefinition ;
    a cwrc:Genre, skos:Concept ;
    rdf:value "DIARY" ;
    rdfs:isDefinedBy <http://www.cwrc.ca/ontologies/cwrc#> ;
    rdfs:label ""@fr, "diary"@en ;
    owl:comment "This term and its description was created from data gathered from the Getty Art & Architecture Thesaurus."@en ;
    skos:definition "Refers to books containing the daily, personal accounts of the writer's own experiences, attitudes, and observations. Use \"journals (accounts)\" when referring to an individual's or an organization's account of occurrences or transactions."@en, "Wordt gebruikt voor boeken die het dagelijkse, persoonlijke verslag bevatten van de eigen ervaringen, standpunten en observaties van de schrijver. Gebruik `journalen (verslagen)' wanneer het gaat om het verslag van de activiteiten of de transacties van personen of organisaties."@nl, "Úsese para libros que contienen los relatos personales diarios de las experiencias, actitudes y observaciones del escritor. Use \"jornal (cuenta)\" para referirse al relato de los acontecimientos o transacciones de un individuo u organización."@es, "指內含筆者每日自身經驗、態度，與觀察之個人記述的本子。記述個人或組織所發生的事件或業務進行時，稱為「日誌（記述）」。"@zh-hant ;
    skos:inScheme cwrc:Genre ;
    prov:derivedFrom <http://vocab.getty.edu/aat/300027112> .

cwrc:genreDictionary
    void:inDataset cwrc:datasetdefinition ;
    a cwrc:Genre, skos:Concept ;
    rdf:value "DICTIONARY" ;
    rdfs:isDefinedBy <http://www.cwrc.ca/ontologies/cwrc#> ;
    rdfs:label ""@fr, "dictionary"@en ;
    owl:comment "This term and its description was created from data gathered from the Getty Art & Architecture Thesaurus."@en ;
    skos:definition "Bibliothekskatalog, in dem die Einträge in einer einzigen alphabetischen Folge verzeichnet sind, ohne Berücksichtigung ihres Typs, so dass Autoren, Titel und andere Indexierungsstichworte zusammenhängend alphabetisch geordnet werden, anstatt sie je nach Typ getrennt zu gruppieren."@de, "Library catalog in which the entries are arranged in a single alphabetical sequence, regardless of their type, so that authors, titles, and other indexing terms are all alphabetized together alphabetically instead of in separate groupings by type. "@en, "所有資料皆依照單一字母順序排列的圖書館目錄，不管是作者、書名或任何可據以分類的索引詞彙，不依類型區分，一律按照字母順序混合編列。"@zh-hant ;
    skos:inScheme cwrc:Genre ;
    prov:derivedFrom <http://vocab.getty.edu/aat/300026631> .

cwrc:genreDidactic
    void:inDataset cwrc:datasetdefinition ;
    a cwrc:Genre, skos:Concept ;
    rdf:value "DIDACTIC" ;
    rdfs:isDefinedBy <http://www.cwrc.ca/ontologies/cwrc#> ;
    rdfs:label ""@fr, "didactic"@en ;
    skos:inScheme cwrc:Genre .

cwrc:genreDirectory
    void:inDataset cwrc:datasetdefinition ;
    a cwrc:Genre, skos:Concept ;
    rdf:value "DIRECTORY" ;
    rdfs:isDefinedBy <http://www.cwrc.ca/ontologies/cwrc#> ;
    rdfs:label ""@fr, "directory"@en ;
    skos:inScheme cwrc:Genre .

cwrc:genreDissertation
    void:inDataset cwrc:datasetdefinition ;
    a cwrc:Genre, skos:Concept ;
    rdf:value "DISSERTATION" ;
    rdfs:isDefinedBy <http://www.cwrc.ca/ontologies/cwrc#> ;
    rdfs:label ""@fr, "dissertation"@en ;
    skos:inScheme cwrc:Genre .

cwrc:genreDocumentary
    void:inDataset cwrc:datasetdefinition ;
    a cwrc:Genre, skos:Concept ;
    rdf:value "DOCUMENTARY" ;
    rdfs:isDefinedBy <http://www.cwrc.ca/ontologies/cwrc#> ;
    rdfs:label ""@fr, "documentary"@en ;
    skos:inScheme cwrc:Genre .

cwrc:genreDomestic
    void:inDataset cwrc:datasetdefinition ;
    a cwrc:Genre, skos:Concept ;
    rdf:value "DOMESTIC" ;
    rdfs:isDefinedBy <http://www.cwrc.ca/ontologies/cwrc#> ;
    rdfs:label ""@fr, "domestic"@en ;
    owl:comment "This term and its description was created from data gathered from DBpedia."@en ;
    skos:definition "Domestic realism normally refers to the genre of nineteenth-century novels popular with women readers. This body of writing is also known as \"sentimental fiction\" or \"woman's fiction\". The genre is mainly reflected in the novel though short-stories and non-fiction works such as Harriet Beecher Stowe's \"Our Country Neighbors\" and The New Housekeeper's Manual written by Stowe and her sister-in-law Catharine Beecher are works of domestic realism. The style's particular characteristics are: \"1. Plot focuses on a heroine who embodies one of two types of exemplar: the angel and the practical woman (Reynolds) who sometimes exist in the same work. Baym says that this heroine is contrasted with the passive woman (incompetent, cowardly, ignorant; often the heroine's mother is this type) and the \"belle,\" who is deprived of a proper education. 2. The heroine struggles for self-mastery, learning the pain of conquering her own passions (Tompkins, Sensational Designs, 172). 3. The heroine learns to balance society's demands for self-denial with her own desire for autonomy, a struggle often addressed in terms of religion. 4. She suffers at the hands of abusers of power before establishing a network of surrogate kin. 5. The plots \"repeatedly identify immersion in feeling as one of the great temptations and dangers for a developing woman. They show that feeling must be controlled. . . \" (Baym 25). Frances Cogan notes that the heroines thus undergo a full education within which to realize feminine obligations (The All-American Girl). 6. The tales generally end with marriage, usually one of two possible kinds: A. Reforming the bad or \"wild\" male, as in Augusta Evans's St. Elmo (1867) B. Marrying the solid male who already meets her qualifications.Examples: Maria Cummins, The Lamplighter (1854) and Susan Warner, The Wide, Wide World (1850) 7. The novels may use a \"language of tears\" that evokes sympathy from the readers. 8. Richard Brodhead (Cultures of Letters) sees class as an important issue, as the ideal family or heroine is poised between a lower-class family exemplifying poverty and domestic disorganization and upper-class characters exemplifying an idle, frivolous existence (94).\" An example of this style of novel is Jane Smiley's A Thousand Acres in which the main character's confinement is emphasized in such a way. Some early exponents of the genre of domestic realism were Jane Austen and Elizabeth Barrett Browning."@en ;
    skos:inScheme cwrc:Genre ;
    prov:derivedFrom dbpedia:Domestic_realism .

cwrc:genreDrama
    void:inDataset cwrc:datasetdefinition ;
    a cwrc:Genre, skos:Concept ;
    rdf:value "DRAMA" ;
    rdfs:isDefinedBy <http://www.cwrc.ca/ontologies/cwrc#> ;
    rdfs:label "drama"@en, "drame"@fr ;
    skos:inScheme cwrc:Genre .

cwrc:genreDramaticmonologue
    void:inDataset cwrc:datasetdefinition ;
    a cwrc:Genre, skos:Concept ;
    rdf:value "DRAMATICMONOLOGUE" ;
    rdfs:isDefinedBy <http://www.cwrc.ca/ontologies/cwrc#> ;
    rdfs:label ""@fr, "dramatic monologue"@en ;
    owl:comment "This term and its description was created from data gathered from DBpedia."@en ;
    skos:definition "Dramatic monologue, also known as a persona poem, is a type of poetry written in the form of a speech of an individual character. M.H. Abrams notes the following three features of the dramatic monologue as it applies to poetry"@en, "El monólogo dramático puede ser dos cosas:"@es, "Un monologue dramatique est en France, à la fin du Moyen Âge, un type de poème comique à vocation scénique. À l’instar des jongleurs, l’acteur seul en scène incarnait plusieurs personnages stéréotypés. Il est considéré comme un des quatre grands genres comiques de la fin du Moyen Âge avec la sotie, le sermon joyeux et la farce. Dans l'Angleterre du XIXe siècle, le terme monologue dramatique (dramatic mononologue) désignait un type de poème, fort apprécié par de nombreux poètes de l'époque victorienne, dans lequel un personnage, de fiction ou historique, exprime ses sentiments, ses actions ou ses motifs dans un monologue. Celui-ci, dont les paroles sont souvent influencées par le contexte critique dans lequel elles sont prononcées, s'adresse en général à un auditoire silencieux.Des exemples de monologues dramatiques sont My Last Duchess de Robert Browning, The Captain of the 1984 Top of the Form Team de Carol Ann Duffy, ou encore Lady Lazarus de Sylvia Plath."@fr ;
    skos:inScheme cwrc:Genre ;
    prov:derivedFrom dbpedia:Dramatic_monologue .

cwrc:genreDreamvision
    void:inDataset cwrc:datasetdefinition ;
    a cwrc:Genre, skos:Concept ;
    rdf:value "DREAMVISION" ;
    rdfs:isDefinedBy <http://www.cwrc.ca/ontologies/cwrc#> ;
    rdfs:label ""@fr, "dreamvision"@en ;
    skos:inScheme cwrc:Genre .

cwrc:genreDystopia
    void:inDataset cwrc:datasetdefinition ;
    a cwrc:Genre, skos:Concept ;
    rdf:value "DYSTOPIA" ;
    rdfs:isDefinedBy <http://www.cwrc.ca/ontologies/cwrc#> ;
    rdfs:label ""@fr, "dystopia"@en ;
    skos:inScheme cwrc:Genre .

cwrc:genreEclogue
    void:inDataset cwrc:datasetdefinition ;
    a cwrc:Genre, skos:Concept ;
    rdf:value "ECLOGUE" ;
    rdfs:isDefinedBy <http://www.cwrc.ca/ontologies/cwrc#> ;
    rdfs:label ""@fr, "eclogue"@en ;
    owl:comment "This term and its description was created from data gathered from DBpedia."@en ;
    skos:definition "An eclogue is a poem in a classical style on a pastoral subject. Poems in the genre are sometimes also called bucolics."@en, "Die Ekloge (griechisch ἐκλογή eklogḗ „Auswahl“ oder „Wahl“, latinisiert ecloga) ist ein Begriff aus der antiken Literatur. Die Grundbedeutung ist „Auswahl“, das heißt „das Ausgewählte“. Gemeint ist ursprünglich ein ausgewähltes Stück (Auszug, Zitat) aus einem längeren literarischen Text oder ein einzelnes Gedicht von mäßiger Länge, das aus einer Sammlung von Gedichten oder aus dem Werk eines Dichters herausgegriffen wurde. Der Begriff Ekloge bezeichnet im eigentlichen Wortsinn ein „ausgewähltes“ Gedicht, wurde aber im Humanismus als Gattungsbezeichnung missverstanden. Im Plural bezeichnet eclogae in der römischen Lyrik ursprünglich nur „ausgewählte“ Gedichte, in späterem Sprachgebrauch sind gewöhnlich ländliche oder Hirtengedichte (bukolische Dichtung) gemeint. Daher wird der Begriff Ekloge oft als Synonym von „bukolisches Gedicht“ verwendet. Die bekanntesten Gedichte, für die heute die Bezeichnung Eklogen (Eclogae) gängig ist, sind die Eclogae (oder auch Bucolica) von Vergil. Bereits im 1. Jahrhundert bezeichnet Statius einzelne Gedichte aus seinen Silvae mit dem Ausdruck egloga; er ist der erste römische Dichter, der den Begriff für seine eigenen Werke verwendet. In der deutschen Literatur waren bis ins 18. Jahrhundert Ekloge, Schäfer- bzw. Hirtengedicht und Idylle synonym verwendete Begriffe und bezeichneten lyrisch-dramatische Hirtengesänge oder allgemein kürzere Hirtendichtung, siehe etwa Georg Rodolf Weckherlin Eclogen oder Hürtengedichte (1641) oder Johann Christoph Gottscheds Von Idyllen, Eklogen oder Schäfergedichten (in Critische Dichtkunst, 1730).Durch den Erfolg von Salomon Gessners Idyllen (1756) wurde aber Idylle der gebräuchliche Begriff für diese Gattung."@de, "Ecloge – ook wel: ekloge (Griekse spelling) en ecloga (Latijnse spelling) - is een benaming voor een herdersdicht en maakt deel uit van de bucolische poëzie. Het woord ecloge kennen we vooral van de tien herdersdichten (Bucolica) die Vergilius in 38 v.Chr. publiceerde en die doorgaans Eclogae worden genoemd. Het uit het Grieks afkomstige woord ekloge (ἑκλογή) betekent eigenlijk ‘keus’. Het is waarschijnlijk dat Vergilius niet zelf de naam ecloga gebruikte, maar dat die door latere grammatici aan zijn gedichten is gegeven. De Eclogae of Eclogen van Vergilius zijn tien herdersdichten, die Vergilius dichtte naar het voorbeeld van Theocritus, de uitvinder van het herdersdicht. Ze zijn geschreven in dactylische hexameters en variëren in lengte van 63 tot 111 regels. De meeste zijn gesprekken tussen herders. Sinds Vergilius is de naam ecloge een algemeen gebruikte naam voor dit soort gedichten. We kennen verder zeven eclogen die ene Calpurnius Siculus schreef in de tijd van Nero, en van de derde-eeuwse dichter Nemesianus zijn vier eclogen overgeleverd. Zeer invloedrijk werd in later eeuwen Vergilius’ vierde ecloge, waarin de komst van een bijzonder kind wordt aangekondigd die een nieuwe tijd zal inluiden. Dit werd al snel uitgelegd als een aankondiging van de geboorte van Christus. In de middeleeuwse Latijnse literatuur werd het genre van het herdersdicht niet altijd begrepen. Zo schreef bisschop Radboud ca. 900 een Ecloga pro St. Lebuino, waarin hij de kerstenende activiteiten van Lebuïnus beschrijft. In de Neolatijnse literatuur werd het genre van de ecloga veel beoefend. Het woord werd door de neolatinisten ook wel gespeld als (a)egloga, omdat men dacht dat het verwant was met αἱγ- (aeg), het Griekse woord voor ‘geit’. Geleidelijk ontstonden er enkele varianten op het genre. Zo schreef Iacopo Sannazaro (1458-1530) vijf Eclogae piscatoriae, waarin hij de herders verving door vissers, en schreef de Franse jezuïet René Rapin christelijke eclogen: Eclogae Sacrae (1659)."@nl, "La égloga es un subgénero de la poesía lírica que se dialoga a veces como una pequeña pieza teatral en un acto. De tema amoroso, uno o varios pastores lo desarrollan contándolo en un ambiente campesino donde la naturaleza es paradisíaca y tiene un gran protagonismo la música. Como subgénero lírico se desarrolla a veces mediante un monólogo pastoril o, más frecuentemente, con un diálogo. La égloga es una composición en la que el poeta, encarnado en uno o varios pastores, expresa su amor en un marco idealizado, lleno de belleza y amor. Las primeras églogas fueron los Idilios (en griego, \"poemitas\" o \"pequeños cantos\") de Teócrito; luego los escribieron Mosco, Bión de Esmirna y otros autores bajo su influencia. El escritor latino Virgilio (siglo I a. C.) con sus Églogas (en griego, \"selecciones\") o Bucólicas añadió elementos autobiográficos, haciendo de cada pastor un personaje imaginario que encubría a un personaje real: Cayo Cilnio Mecenas, Augusto, etc. Algunas de ellas llegaron a escenificarse en Roma. Otros autores latinos escribieron también églogas, como Nemesiano, Calpurnio Sículo o Ausonio. Esta innovación pasó a la bucólica posterior, de forma que algunas veces los personajes de las églogas representaban personajes reales. A través de Giovanni Boccaccio y con el Renacimiento y la Arcadia de Jacopo Sannazaro el género se volvió a recuperar mezclándose las composiciones en verso en un marco narrativo en prosa, y se difundió por todo el mundo occidental, bien en verso, bien como églogas intercaladas en una novela pastoril cualquiera. En la literatura castellana, escribieron églogas Juan del Encina, Lucas Fernández, Garcilaso de la Vega, Juan Boscán, Lope de Vega, Pedro Soto de Rojas, Bernardo de Balbuena y Juan Meléndez Valdés."@es, "Une églogue est un poème de style classique consacré à un sujet pastoral. Les poèmes de ce genre littéraire sont parfois qualifiés de « bucoliques »."@fr ;
    skos:inScheme cwrc:Genre ;
    prov:derivedFrom dbpedia:Eclogue .

cwrc:genreElegy
    void:inDataset cwrc:datasetdefinition ;
    a cwrc:Genre, skos:Concept ;
    rdf:value "ELEGY" ;
    rdfs:isDefinedBy <http://www.cwrc.ca/ontologies/cwrc#> ;
    rdfs:label "elegy"@en, "élégie"@fr ;
    owl:comment "This term and its description was created from data gathered from DBpedia."@en, "This term and its description was created from data gathered from the Getty Art & Architecture Thesaurus."@en ;
    skos:definition "L’élégie (en grec ancien ἐλεγεία / elegeía, signifiant « chant de mort ») fut une forme de poème dans l'Antiquité, avant de devenir un genre poétique à partir de la Renaissance. Dans l’Antiquité, était appelé « élégie » tout poème alternant hexamètres et pentamètres en distiques : ce sont les vers élégiaques. De nos jours, l’élégie est considérée comme un genre au sein de la poésie lyrique, en tant que poème de longueur et de forme variables caractérisé par son ton plaintif particulièrement adapté à l’évocation d’un mort ou à l’expression d’une souffrance amoureuse due à un abandon ou à une absence."@fr, "Mournful, melancholy, or plaintive poems, especially funeral songs or laments for the dead."@en, "Poemas tristes, melancólicos o quejumbrosos, especialmente cantos fúnebres o lamentos por los muertos."@es, "Schwermütiges, melancholisches oder trauriges Gedicht, insbesondere Begräbnislied oder Totenklage."@de, "Sombere, melancholieke of treurige gedichten, met name klaagliederen of liederen die bij een begrafenisplechtigheid ten gehore worden gebracht."@nl ;
    skos:inScheme cwrc:Genre ;
    prov:derivedFrom dbpedia:Elegy, <http://vocab.getty.edu/aat/300026285> .

cwrc:genreEncyclopaedia
    void:inDataset cwrc:datasetdefinition ;
    a cwrc:Genre, skos:Concept ;
    rdf:value "ENCYCLOPAEDIA" ;
    rdfs:isDefinedBy <http://www.cwrc.ca/ontologies/cwrc#> ;
    rdfs:label ""@fr, "encyclopaedia"@en ;
    skos:inScheme cwrc:Genre .

cwrc:genreEpic
    void:inDataset cwrc:datasetdefinition ;
    a cwrc:Genre, skos:Concept ;
    rdf:value "EPIC" ;
    rdfs:isDefinedBy <http://www.cwrc.ca/ontologies/cwrc#> ;
    rdfs:label ""@fr, "epic"@en ;
    owl:comment "This term and its description was created from data gathered from the Getty Art & Architecture Thesaurus."@en ;
    skos:definition "Meaning extended from \"epic poetry,\" in modern usage refers to literary art forms, such as prose, poetry, plays, films, and other works where the story has a theme of grandeur and heroism. "@en ;
    skos:inScheme cwrc:Genre ;
    prov:derivedFrom <http://vocab.getty.edu/aat/300404209> .

cwrc:genreEpigram
    void:inDataset cwrc:datasetdefinition ;
    a cwrc:Genre, skos:Concept ;
    rdf:value "EPIGRAM" ;
    rdfs:isDefinedBy <http://www.cwrc.ca/ontologies/cwrc#> ;
    rdfs:label ""@fr, "epigram"@en ;
    owl:comment "This term and its description was created from data gathered from DBpedia."@en, "This term and its description was created from data gathered from the Getty Art & Architecture Thesaurus."@en ;
    skos:definition "Bezeichnet ein kurzes satirisches Gedicht oder jede ähnlich pointierte Redensart."@de, "Refers to short satiric poems or any similar pointed sayings."@en, "Wordt gebruikt voor korte, satirische gedichten of vergelijkbare puntige gezegdes."@nl, "À l’origine, une épigramme, du grec ancien ἐπίγραμμα (epígramma), « inscription », est une inscription, d’abord en prose, puis en vers, qu’on gravait sur les monuments, les statues, les tombeaux et les trophées, pour perpétuer le souvenir d’un héros ou d’un événement. À partir du IVe siècleav. J.-C., l’épigramme devient une petite pièce de poésie sur un sujet quelconque, imitant par sa brièveté les inscriptions, offrant une pensée ingénieuse ou délicate exprimée avec grâce et précision. Enfin, à partir du XVIe siècle, le genre se spécialise dans le mot d’esprit : l’épigramme renferme généralement une pointe grivoise ou assassine. Les plus anciennes épigrammes ne revêtent qu'un caractère pratique, visant à identifier le propriétaire ou la personne dédiant l’objet. Le premier auteur d’épigrammes, selon la tradition grecque, est Simonide de Céos (Hérodote, VII, 228, 4), qui vit à la fin du VIe siècleav. J.-C. C'est de cette même époque que date la première épigramme signée connue ; il s'agit d’une dédicace d’Ion de Chios à Delphes."@fr, "Úsese para poemas satíricos cortos u otros refranes mordaces similares."@es ;
    skos:inScheme cwrc:Genre ;
    prov:derivedFrom dbpedia:Epigram, <http://vocab.getty.edu/aat/300202533> .

cwrc:genreEpilogue
    void:inDataset cwrc:datasetdefinition ;
    a cwrc:Genre, skos:Concept ;
    rdf:value "EPILOGUE" ;
    rdfs:isDefinedBy <http://www.cwrc.ca/ontologies/cwrc#> ;
    rdfs:label "epilogue"@en, "épilogue"@fr ;
    skos:inScheme cwrc:Genre .

cwrc:genreEpistle
    void:inDataset cwrc:datasetdefinition ;
    a cwrc:Genre, skos:Concept ;
    rdf:value "EPISTLE" ;
    rdfs:isDefinedBy <http://www.cwrc.ca/ontologies/cwrc#> ;
    rdfs:label "epistle"@en, "épître>"@fr ;
    owl:comment "This term and its description was created from data gathered from DBpedia."@en, "This term and its description was created from data gathered from the Getty Art & Architecture Thesaurus."@en ;
    skos:definition "Een epistel is een schrijven gericht aan een persoon of een groep personen, meestal in de vorm van een erg formele brief, vaak didactisch van aard en elegant geformuleerd. De brieven van de apostelen aan verscheidene joodse gemeenschappen in de wereld, opgenomen in het Nieuwe Testament, worden vaak epistels genoemd."@nl, "Epistel (griech. ἐπιστολή, epistolē; lat. epistola, epistula) ist ein über das Lateinische aus dem Griechischen entlehntes Wort für „Brief“, das für Brieftexte gehobenen Anspruchs (Sendschreiben, Versepistel) verwendet wird, insbesondere für die Apostelbriefe der Bibel. Als liturgische Kurzbezeichnung bezieht sich der Begriff auf bestimmte im Gottesdienst zu lesende Abschnitte der Bibel."@de, "Epístola (del griego: ἐπιστολή, epistolē) es un sinónimo de carta: un texto cuya función principal es la comunicación entre el remitente o emisor (el escritor que la redacta y envía) y el destinatario o receptor que la debe recibir. El uso del término suele implicar un registro culto o un contexto literario (el género epistolar). En la actualidad es un término arcaico, por lo general restringido en su uso a las cartas didáctica sobre ética o religión; y particularmente para referirse a los libros del Nuevo Testamento que reciben el nombre de \"epístolas\", y donde se recogen las escritas por algunos apóstoles destinadas a las comunidades cristianas primitivas. Las tradicionalmente atribuidas a Pablo de Tarso se conocen como \"epístolas paulinas\" y el resto con el nombre genérico de \"epístolas católicas\" (es decir, \"universales\" o \"generales\"). El género epistolar fue común en el Antiguo Egipto como parte del trabajo de los escribas, y están recogidas bajo el nombre de Sebayt (instrucciones), estando datadas las más antiguas en el siglo XXV a. C. También nos han llegado de la Antigüedad las Epístolas de Horacio, del siglo I a. C. Una de ellas, Epistula ad Pisones, recibe el nombre de Arte poética, y ha sido durante siglos considerada como la normativa de principios literarios."@es, "Le terme épître, issu du latin epistula, du grec επιστολη (epistolē), désigne une lettre (au sens de correspondance).Il a pris le sens aujourd'hui d'un court traité philosophique ou religieux exposé sous forme épistolaire. Ce sont de courts traités le plus souvent philosophiques. Ce peuvent être aussi des « conversations en l'absence » de l'interlocuteur sur des aspects sociaux ou moraux de l'existence. Au fil du temps, l’épître devient, en littérature, un discours en vers du genre académique ou didactique. Elle prend rapidement le sens d’épigramme nettement moins acerbe que la satire.Le mot « épître » est un nom commun féminin. Le Nouveau Testament contient plusieurs épîtres."@fr, "Literary genre taking the form of letters, usually of a literary, formal, or public nature. Examples are the epistles in the Biblical New Testament."@en ;
    skos:inScheme cwrc:Genre ;
    prov:derivedFrom dbpedia:Epistle, <http://vocab.getty.edu/aat/300404697> .

cwrc:genreEpistolary
    void:inDataset cwrc:datasetdefinition ;
    a cwrc:Genre, skos:Concept ;
    rdf:value "EPISTOLARY" ;
    rdfs:isDefinedBy <http://www.cwrc.ca/ontologies/cwrc#> ;
    rdfs:label ""@fr, "epistolary"@en ;
    owl:comment "This term and its description was created from data gathered from DBpedia."@en, "This term and its description was created from data gathered from the Getty Art & Architecture Thesaurus."@en ;
    skos:definition "Briefgedicht ist eine Sammelbezeichnung für alle Arten von in Gedichtform verfassten echten oder fingierten Briefen. Beispiele für Briefgedichte reichen bis in die Antike zurück, am bekanntesten sind Ovids Heroides, in elegischen Distichen verfasste fingierte Briefe mythologischer Frauen an ihre männlichen Partner, in denen sie sich über Vernachlässigung und/oder schlechte Behandlung beklagen, sowie die in Hexametern verfassten Epistulae des Horaz. Aus dem Mittelalter sind spezielle Formen der Minnebrief, ein in Reimpaaren verfasster Liebesgruß an die Geliebte und im Frankreich der Trobadore der Salut d’amour.Im Barock wird von Hofmannswaldau die Ovidsche Form wieder aufgenommen (Helden-Briefe 1664), weitere Beispiele finden sich im französischen Rokoko und der deutschen Anakreontik bei Goeckingk, Gleim, Rabener und Wieland. In der Weimarer Klassik sind die Briefgedichte Goethes an Frau von Stein, Augusta zu Stolberg, Marianne von Willemer und Bettina Brentano die bedeutendsten Beispiele der Gattung in der deutschen Literatur und zugleich Muster einer Gelegenheitsdichtung auf hohem Niveau. Als Beispiel Goethes Gedicht an Charlotte von Stein: Nach der Klassik finden sich vereinzelt Briefgedichte bei Heinrich Heine, Clemens Brentano, Friedrich de la Motte Fouqué, Annette von Droste-Hülshoff, Theodor Fontane, Detlev von Liliencron, Rainer Maria Rilke (Briefwechsel mit Erika Mitterer) und Joachim Ringelnatz. In der französischen Literatur finden sich Briefgedichte bei Clément Marot und in der englischen unter anderem bei John Donne, John Dryden, Alexander Pope und John Keats."@de, "Novels written by using the device of a series of letters, diary entries, newspaper clippings, or other documents."@en ;
    skos:inScheme cwrc:Genre ;
    prov:derivedFrom dbpedia:Epistolary_poem, <http://vocab.getty.edu/aat/300410324> .

cwrc:genreEpitaph
    void:inDataset cwrc:datasetdefinition ;
    a cwrc:Genre, skos:Concept ;
    rdf:value "EPITAPH" ;
    rdfs:isDefinedBy <http://www.cwrc.ca/ontologies/cwrc#> ;
    rdfs:label ""@fr, "epitaph"@en ;
    owl:comment "This term and its description was created from data gathered from the Getty Art & Architecture Thesaurus."@en ;
    skos:definition "Inschrift auf einem Grabmal in Erinnerung an die in der Grabstätte Beerdigten."@de, "Inscripciones en mausoleos en memoria de quienes se encuentran enterrados en la tumba o sepulcro."@es, "Inscripties op grafmonumenten ter nagedachtenis aan personen die in het betreffende graf of de betreffende tombe zijn begraven."@nl, "Inscriptions on sepulchral monuments in the memory of those buried in the tomb or grave."@en, "墓碑上的銘文，以紀念埋葬於墳地或墓穴者。"@zh-hant ;
    skos:inScheme cwrc:Genre ;
    prov:derivedFrom <http://vocab.getty.edu/aat/300028729> .

cwrc:genreEpithalamium
    void:inDataset cwrc:datasetdefinition ;
    a cwrc:Genre, skos:Concept ;
    rdf:value "EPITHALAMIUM" ;
    rdfs:isDefinedBy <http://www.cwrc.ca/ontologies/cwrc#> ;
    rdfs:label ""@fr, "epithalamium"@en ;
    owl:comment "This term and its description was created from data gathered from DBpedia."@en ;
    skos:definition "An epithalamiumLatin form of Greek ἐπιθαλάμιον epithalamion from ἐπί epi \"upon,\" and θάλαμος thalamos nuptial chamber) is a poem written specifically for the bride on the way to her marital chamber. This form continued in popularity through the history of the classical world; the Roman poet Catullus wrote a famous epithalamium, which was translated from or at least inspired by a now-lost work of Sappho. According to Origen, Song of Songs, might be an epithalamium on the marriage of Solomon with Pharaoh’s daughter."@en, "Ein Epithalamion (von griech. έπί epi bei und ϑάλαμος thálamos Schlafgemach; lat. epithalamium; dt. Hochzeitsgedicht, Brautlied; Plural: -ien) ist ein üblicherweise pastorales Gelegenheitsgedicht, verfasst und meist chorisch vorgetragen zur Feier einer Hochzeit."@de, "El epitalamio es una poesía lírica, subgénero lírico griego imitado después por los romanos, consistente en un canto de boda. El nombre epitalamio es griego, compuesto sobre y tálamo (en griego θάλαμος) lecho nupcial. Se cantaba regularmente a la puerta de la habitación de los novios por coros de jóvenes y doncellas acompañados de flautas o de otros instrumentos suaves y armónicos. Entre quienes compusieron epitalamios en la antigüedad, se encuentra los poetas griegos Safo y Calímaco y el romano Catulo."@es, "L'épithalame (en grec ancien ἐπιθαλάμιον / epithalámion) est une sorte de poème lyrique composé chez les Anciens à l'occasion d'un mariage et à la louange des nouveaux époux. En Grèce, il était chanté par un chœur, soit de jeunes vierges seules, soit de jeunes filles[réf. nécessaire] et de jeunes garçons, avec accompagnement de danses. On le nommait aussi catakoemèse (de catakoimân, envoyer dormir)."@fr ;
    skos:inScheme cwrc:Genre ;
    prov:derivedFrom dbpedia:Epithalamium .

cwrc:genreEpyllion
    void:inDataset cwrc:datasetdefinition ;
    a cwrc:Genre, skos:Concept ;
    rdf:value "EPYLLION" ;
    rdfs:isDefinedBy <http://www.cwrc.ca/ontologies/cwrc#> ;
    rdfs:label ""@fr, "epyllion"@en ;
    owl:comment "This term and its description was created from data gathered from the Getty Art & Architecture Thesaurus."@en ;
    skos:definition "Brief narrative poems in dactylic hexameter of ancient Greece, imitated by Romans and others. Usually dealing with mythological and romantic themes. They are characterized by lively description, miniaturistic attitude, scholarly allusion, and an elevated tone similar to that of the elegy."@en ;
    skos:inScheme cwrc:Genre ;
    prov:derivedFrom <http://vocab.getty.edu/aat/300410360> .

cwrc:genreEroticapornography
    void:inDataset cwrc:datasetdefinition ;
    a cwrc:Genre, skos:Concept ;
    rdf:value "EROTICAPORNOGRAPHY" ;
    rdfs:isDefinedBy <http://www.cwrc.ca/ontologies/cwrc#> ;
    rdfs:label ""@fr, "erotica pornography"@en ;
    skos:inScheme cwrc:Genre .

cwrc:genreEssay
    void:inDataset cwrc:datasetdefinition ;
    a cwrc:Genre, skos:Concept ;
    rdf:value "ESSAY" ;
    rdfs:isDefinedBy <http://www.cwrc.ca/ontologies/cwrc#> ;
    rdfs:label "essai"@fr, "essay"@en ;
    owl:comment "This term and its description was created from data gathered from DBpedia."@en, "This term and its description was created from data gathered from the Getty Art & Architecture Thesaurus."@en ;
    skos:definition "Breves composiciones literarias sobre temas específicos, a menudo presentando el punto de vista personal del autor."@es, "En littérature, un essai est une œuvre de réflexion portant sur les sujets les plus divers et exposée de manière personnelle, voire subjective par l'auteur. Contrairement à l'étude, l'essai peut être polémique ou partisan. C'est un texte littéraire qui se prête bien à la réflexion philosophique, mais aussi à d'autres domaines : essais historiques, essais scientifiques, essais politiques, etc. L'auteur d’un essai est appelé « essayiste ». Le terme « essai » est dérivé du latin exagium, un poids ou appareil de mesure."@fr, "Korte literaire verhandelingen over één onderwerp, waarin de auteur dikwijls een persoonlijk standpunt verwoordt."@nl, "Kurzer literarischer Aufsatz über ein Einzelthema, gibt häufig die persönliche Meinung des Autors wieder."@de, "Short literary compositions on single subjects, often presenting the personal view of the author."@en, "單一主題的簡短文學作品，常表述作者之個人觀點。"@zh-hant ;
    skos:inScheme cwrc:Genre ;
    prov:derivedFrom dbpedia:Essay, <http://vocab.getty.edu/aat/300026291> .

cwrc:genreEulogy
    void:inDataset cwrc:datasetdefinition ;
    a cwrc:Genre, skos:Concept ;
    rdf:value "EULOGY" ;
    rdfs:isDefinedBy <http://www.cwrc.ca/ontologies/cwrc#> ;
    rdfs:label ""@fr, "eulogy"@en ;
    owl:comment "This term and its description was created from data gathered from DBpedia."@en ;
    skos:definition "A eulogy (from εὐλογία, eulogia, Classical Greek for \"praise\") is a speech or writing in praise of a person(s) or thing(s), especially one who recently died or retired or as a term of endearment. Eulogies may be given as part of funeral services. They take place in a funeral home during or after a wake. However, some denominations either discourage or do not permit eulogies at services to maintain respect for traditions. Eulogies can also praise people who are still alive. This normally takes place on special occasions like birthdays, office parties, retirement celebrations, etc. Eulogies should not be confused with elegies, which are poems written in tribute to the dead; nor with obituaries, which are published biographies recounting the lives of those who have recently died; nor with obsequies, which refer generally to the rituals surrounding funerals. Catholic priests are prohibited by the rubrics of the Mass from presenting a eulogy for the deceased in place of a homily during a funeral Mass. The modern use of the word eulogy was first documented in the 15th century and came from the Medieval Latin term “eulogium” (Merriam-Webster 2012). “Eulogium” at that time has since turned into the shorter “eulogy” of today. Eulogies are usually delivered by a family member or a close family friend in the case of a dead person. For a living eulogy given in such cases as a retirement, a senior colleague could perhaps deliver it. On occasions, eulogies are given to those who are severely ill or elderly in order to express words of love and gratitude before they die. Eulogies are not limited to merely people, however; Places or things can also be given eulogies (which anyone can deliver), but these are less common than those delivered to people, whether living or deceased."@en, "Een eulogie (uit het Grieks εὐλογία, letterlijk: goed woord) is een lofrede of lofdicht uitgesproken bij een speciale gelegenheid zoals een verjaardag. Het begrip moet niet verward worden met een elegie, die geschreven wordt als eerbetoon aan een overleden persoon."@nl, "El encomio es un texto de alabanza en honor a algo o alguien. Junto a su opuesto, que es el vituperio, textos insultantes, compone el género epidíctico cuyo objetivo práctico es argumentar y que se incluye dentro de la retórica. Podía realizarse en lírica o prosa, según el tono deseado. El encomio era un importante ejercicio de oratoria."@es, "L’éloge (masculin du latin elogium, avec l’influence du grec εὐλογία) est un genre littéraire hérité de l'Antiquité, où il est très présent, qui consiste à vanter les mérites d'un individu ou d'une institution. Il s'agit d'un discours public ou donné comme tel, destiné à l'édification commune ; à cette fin, il recourt à l'exploitation des ressources du discours épidictique héritées de la rhétorique classique. Il existe plusieurs sortes d'éloges:"@fr ;
    skos:inScheme cwrc:Genre ;
    prov:derivedFrom dbpedia:Eulogy .

cwrc:genreExhibitioncatalogue
    void:inDataset cwrc:datasetdefinition ;
    a cwrc:Genre, skos:Concept ;
    rdf:value "EXHIBITIONCATALOGUE" ;
    rdfs:isDefinedBy <http://www.cwrc.ca/ontologies/cwrc#> ;
    rdfs:label ""@fr, "exhibition catalogue"@en ;
    owl:comment "This term and its description was created from data gathered from the Getty Art & Architecture Thesaurus."@en ;
    skos:definition "Druckwerk, das die in einer Ausstellung gezeigten Werke dokumentiert."@de, "Publications that document the works displayed in an exhibition."@en ;
    skos:inScheme cwrc:Genre ;
    prov:derivedFrom <http://vocab.getty.edu/aat/300026096> .

cwrc:genreFable
    void:inDataset cwrc:datasetdefinition ;
    a cwrc:Genre, skos:Concept ;
    rdf:value "FABLE" ;
    rdfs:isDefinedBy <http://www.cwrc.ca/ontologies/cwrc#> ;
    rdfs:label ""@fr, "fable"@en ;
    owl:comment "This term and its description was created from data gathered from the Getty Art & Architecture Thesaurus."@en ;
    skos:definition "Fictitious narratives usually with animals or inanimate objects as protagonists, intended to convey a hidden meaning regarding human conduct."@en, "Fiktionale Erzählung, deren Protagonisten in der Regel Tiere oder unbelebte Objekte sind, mit dem Ziel, unterschwellig menschliches Verhalten darzustellen."@de, "Narraciones imaginarias que generalmente tienen como protagonistas a animales u objetos inanimados, destinadas a transmitir un mensaje oculto relativo a la conducta humana."@es, "Verzonnen verhalen, meestal met dieren of levenloze voorwerpen als hoofdpersonen, waarin gewoonlijk een boodschap met betrekking tot menselijk gedrag wordt verborgen."@nl ;
    skos:inScheme cwrc:Genre ;
    prov:derivedFrom <http://vocab.getty.edu/aat/300055917> .

cwrc:genreFabliau
    void:inDataset cwrc:datasetdefinition ;
    a cwrc:Genre, skos:Concept ;
    rdf:value "FABLIAU" ;
    rdfs:isDefinedBy <http://www.cwrc.ca/ontologies/cwrc#> ;
    rdfs:label ""@fr, "fabliau"@en ;
    skos:inScheme cwrc:Genre .

cwrc:genreFairytale
    void:inDataset cwrc:datasetdefinition ;
    a cwrc:Genre, skos:Concept ;
    rdf:value "FAIRYTALE" ;
    rdfs:isDefinedBy <http://www.cwrc.ca/ontologies/cwrc#> ;
    rdfs:label ""@fr, "fairytale"@en ;
    owl:comment "This term and its description was created from data gathered from DBpedia."@en ;
    skos:definition "Fairytale fantasy is distinguished from other subgenres of fantasy by the works' heavy use of motifs, and often plots, from folklore."@en ;
    skos:inScheme cwrc:Genre ;
    prov:derivedFrom dbpedia:Fairytale_fantasy .

cwrc:genreFantasy
    void:inDataset cwrc:datasetdefinition ;
    a cwrc:Genre, skos:Concept ;
    rdf:value "FANTASY" ;
    rdfs:isDefinedBy <http://www.cwrc.ca/ontologies/cwrc#> ;
    rdfs:label ""@fr, "fantasy"@en ;
    owl:comment "This term and its description was created from data gathered from DBpedia."@en, "This term and its description was created from data gathered from the Getty Art & Architecture Thesaurus."@en ;
    skos:definition "El género fantástico, comúnmente llamado fantasía, es un género artístico en el cual los elementos principales del argumento son imaginarios, irreales y sobrenaturales. En su sentido más amplio, el género fantástico se halla presente en la literatura, cinematografía, historieta, videojuegos, juegos de rol, pintura, escultura, drama y, sobre todo, en la mitología y relatos antiguos, donde tuvo su origen. Se caracteriza por no dar prioridad a una representación realista que respete las leyes de funcionamiento del mundo real. En ese sentido se suele decir que el género fantástico es subversivo, pues viola las normas de la realidad. Generalmente se lo distingue de otras formas artísticas como la ciencia ficción –en la que también se subvierten los mecanismos de funcionamiento de la realidad conocida– aduciendo que la causa de los fenómenos observados en obras de corte fantástico siempre tienen que ver con fuerzas sobrenaturales mientras que en la ciencia ficción hay causas “cientifizadas”, con explicaciones que buscan la racionalidad dentro de su ruptura con el orden conocido. Por eso, algunos autores opinan que la diferencia entre el relato fantástico y el de ciencia-ficción radica no tanto en los hechos sobrenaturales sino en el modo en que el autor presenta y explica los mismos."@es, "Fantasy (von engl. fantasy „Phantasie“) ist ein Genre der Phantastik, dessen Wurzeln sich in der Mythologie und den Sagen finden. Ähnlich wie die benachbarten Genres Science-Fiction und Horror, findet Fantasy ihre wichtigsten Ausprägungen in Literatur und Film, außerdem aber auch in Musik und bildender Kunst sowie im Bereich der Gesellschaftsspiele, Computerspiele sowie Pen-&-Paper- und Live-Rollenspiele."@de, "Fantasy is een apart genre binnen diverse media-, kunst- en cultuurvormen zoals films, televisie, literatuur, computerspellen, festivals, muziek, en dergelijke. Het is een genre dat zich kenmerkt door het gebruik van fictieve verhalen, verzonnen wezens en imaginaire werelden. Bovendien spelen magie en andere bovennatuurlijke elementen veelal een belangrijke rol in het genre. Toch is fantasy meestal duidelijk te onderscheiden van aanverwante genres als sciencefiction en horror, die de meeste van de bovenstaande kenmerken ook kunnen bezitten. Dit onderscheid is vooral te vinden in de toon, de stijl en de manier waarop diverse thema's behandeld worden. Daarnaast focussen sciencefiction en horror zich respectievelijk op bepaalde elementen als 'toekomst en techniek' en 'angst en mysterie', terwijl in fantasy de bovengenoemde kenmerken centraal staan. Vaak lijken fantasy-verhalen zich af te spelen in een onbestemd en mythisch verleden, waarin \"bovennatuurlijke\" verschijnselen of een daarmee samenhangende sfeer alledaags lijken (zoals tovenarij), terwijl het met name bij sciencefiction daarentegen veelal gaat om een setting in een al dan niet onbestemd \"futuristisch\" verschiet, waarin technisch vernuft een belangrijke rol speelt (zoals ruimtereizen)."@nl, "La fantasy, ou fantasie (terme issu de l’anglais fantasy : « imagination » ; à ne pas confondre avec la fantaisie musicale, ni avec le terme allemand phantasie qui désigne le concept psychologique de fantasme), est un genre littéraire présentant un ou plusieurs éléments surnaturels qui relèvent souvent du mythe et qui sont souvent incarnés par l’irruption ou l’utilisation de la magie. La fantasy fait partie des littératures de l'imaginaire. Dans la fantasy comme dans le merveilleux, le surnaturel est généralement accepté, voire utilisé pour définir les règles d'un monde imaginaire, et n'est pas nécessairement objet de doute ou de peur. Cela distingue la fantasy du fantastique où le surnaturel fait intrusion dans les règles du monde habituel, et de l'horreur où il suscite peur et angoisse. Par extension, à partir du genre littéraire, on parle aussi de fantasy à propos d'illustrations, de bandes dessinées, de films, de jeux, etc."@fr, "Literary genre in which works are of a whimsical or visionary nature, having suppositions that are speculation or resting on no solid grounds."@en ;
    skos:inScheme cwrc:Genre ;
    prov:derivedFrom dbpedia:Fantasy, <http://vocab.getty.edu/aat/300380290> .

cwrc:genreFarce
    void:inDataset cwrc:datasetdefinition ;
    a cwrc:Genre, skos:Concept ;
    rdf:value "FARCE" ;
    rdfs:isDefinedBy <http://www.cwrc.ca/ontologies/cwrc#> ;
    rdfs:label ""@fr, "farce"@en ;
    skos:inScheme cwrc:Genre .

cwrc:genreFeminist
    void:inDataset cwrc:datasetdefinition ;
    a cwrc:Genre, skos:Concept ;
    rdf:value "FEMINIST" ;
    rdfs:isDefinedBy <http://www.cwrc.ca/ontologies/cwrc#> ;
    rdfs:label ""@fr, "feminist"@en ;
    skos:inScheme cwrc:Genre .

cwrc:genreFeministtheory
    void:inDataset cwrc:datasetdefinition ;
    a cwrc:Genre, skos:Concept ;
    rdf:value "FEMINISTTHEORY" ;
    rdfs:isDefinedBy <http://www.cwrc.ca/ontologies/cwrc#> ;
    rdfs:label ""@fr, "feminist theory"@en ;
    skos:inScheme cwrc:Genre .

cwrc:genreFiction
    void:inDataset cwrc:datasetdefinition ;
    a cwrc:Genre, skos:Concept ;
    rdf:value "FICTION" ;
    rdfs:isDefinedBy <http://www.cwrc.ca/ontologies/cwrc#> ;
    rdfs:label "fiction"@en, "fiction"@fr ;
    owl:comment "This term and its description was created from data gathered from the Getty Art & Architecture Thesaurus."@en ;
    skos:definition "Narraciones en verso o prosa que relatan sucesos heroicos, fantásticos o sobrenaturales que a menudo transcurren en tiempos medievales."@es, "Poetic or prosaic literary forms derived from medieval narratives of love, legendary or heroic adventures, and chivalry. Extends to narratives about important religious figures, or fantastic or supernatural events."@en, "Vertellingen in proza of versvorm, zich vaak afspelend in de middeleeuwen, waarin grootse, fantastische of bovennatuurlijke gebeurtenissen worden beschreven."@nl, "描述英雄事蹟、幻想，或超自然事件的詩文或散文體記敘文，常設定於中世紀時期。"@zh-hant ;
    skos:inScheme cwrc:Genre ;
    prov:derivedFrom <http://vocab.getty.edu/aat/300191065> .

cwrc:genreFilmtvscript
    void:inDataset cwrc:datasetdefinition ;
    a cwrc:Genre, skos:Concept ;
    rdf:value "FILMTVSCRIPT" ;
    rdfs:isDefinedBy <http://www.cwrc.ca/ontologies/cwrc#> ;
    rdfs:label ""@fr, "film tv script"@en ;
    skos:inScheme cwrc:Genre .

cwrc:genreFolksong
    void:inDataset cwrc:datasetdefinition ;
    a cwrc:Genre, skos:Concept ;
    rdf:value "FOLKSONG" ;
    rdfs:isDefinedBy <http://www.cwrc.ca/ontologies/cwrc#> ;
    rdfs:label ""@fr, "folksong"@en ;
    skos:inScheme cwrc:Genre .

cwrc:genreGardeningbook
    void:inDataset cwrc:datasetdefinition ;
    a cwrc:Genre, skos:Concept ;
    rdf:value "GARDENINGBOOK" ;
    rdfs:isDefinedBy <http://www.cwrc.ca/ontologies/cwrc#> ;
    rdfs:label ""@fr, "gardening book"@en ;
    skos:inScheme cwrc:Genre .

cwrc:genreGenealogy
    void:inDataset cwrc:datasetdefinition ;
    a cwrc:Genre, skos:Concept ;
    rdf:value "GENEALOGY" ;
    rdfs:isDefinedBy <http://www.cwrc.ca/ontologies/cwrc#> ;
    rdfs:label ""@fr, "genealogy"@en ;
    owl:comment "This term and its description was created from data gathered from the Getty Art & Architecture Thesaurus."@en ;
    skos:definition "Accounts or histories of the descent of persons, families, or other groups, from an ancestor or ancestors; enumerations of ancestors and their descendants in the natural order of succession."@en, "Bericht oder Chronik über die Abstammung von Personen, Familien oder anderen Gruppen von einem oder mehreren Vorfahren; Auflistung der Vorfahren und ihrer Nachkommen in natürlicher Abfolge."@de, "Documentos o historias de la ascendencia de personas, familias u otros grupos, desde un antepasado o antepasados, enumeraciones de antepasados y su descendencia en el orden natural de sucesión."@es, "Verslagen van of verhalen over de afkomst van personen, families of andere groepen mensen beginnende bij één of meer gemeenschappelijke voorouders; opsommingen van voorouders en hun afstammelingen in volgorde van nakomelingschap."@nl, "從一位祖先或諸位祖先開始的個人、家庭，或其他群體之記述或歷史；依繼承自然順序列舉祖先與其後裔。"@zh-hant ;
    skos:inScheme cwrc:Genre ;
    prov:derivedFrom <http://vocab.getty.edu/aat/300027015> .

cwrc:genreGeorgic
    void:inDataset cwrc:datasetdefinition ;
    a cwrc:Genre, skos:Concept ;
    rdf:value "GEORGIC" ;
    rdfs:isDefinedBy <http://www.cwrc.ca/ontologies/cwrc#> ;
    rdfs:label ""@fr, "georgic"@en ;
    skos:inScheme cwrc:Genre .

cwrc:genreGhoststory
    void:inDataset cwrc:datasetdefinition ;
    a cwrc:Genre, skos:Concept ;
    rdf:value "GHOSTSTORY" ;
    rdfs:isDefinedBy <http://www.cwrc.ca/ontologies/cwrc#> ;
    rdfs:label ""@fr, "ghost story"@en ;
    owl:comment "This term and its description was created from data gathered from DBpedia."@en, "This term and its description was created from data gathered from the Getty Art & Architecture Thesaurus."@en ;
    skos:definition "Cuentos sobrenaturales en prosa en los que seres vivos tienen encuentros con manifestaciones de los espíritus de los muertos."@es, "Les histoires de fantôme sont un sous-genre du fantastique. Dans ces histoires, le fantôme est souvent le héros et a une personnalité et une identité bien à lui. Le genre peut aussi donner lieu à des récits centrés uniquement sur les fantômes ou les morts."@fr, "Prosaerzählung vom Übernatürlichen, in der die Lebenden den Geistern der Toten begegnen."@de, "Prose tales of the supernatural in which the living encounter manifestations of the spirits of the dead."@en, "Prozavertellingen over het bovennatuurlijke, waarin levende figuren in aanraking komen met verschijningen van de geesten van doden."@nl, "超自然的散文體故事，敘述活人與死者現形的靈魂相遇。"@zh-hant ;
    skos:inScheme cwrc:Genre ;
    prov:derivedFrom dbpedia:Ghost_story, <http://vocab.getty.edu/aat/300254823> .

cwrc:genreGiftbook
    void:inDataset cwrc:datasetdefinition ;
    a cwrc:Genre, skos:Concept ;
    rdf:value "GIFTBOOK" ;
    rdfs:isDefinedBy <http://www.cwrc.ca/ontologies/cwrc#> ;
    rdfs:label ""@fr, "giftbook"@en ;
    skos:inScheme cwrc:Genre .

cwrc:genreGothic
    void:inDataset cwrc:datasetdefinition ;
    a cwrc:Genre, skos:Concept ;
    rdf:value "GOTHIC" ;
    rdfs:isDefinedBy <http://www.cwrc.ca/ontologies/cwrc#> ;
    rdfs:label "gothic"@en, "gothique"@fr ;
    owl:comment "This term and its description was created from data gathered from the Getty Art & Architecture Thesaurus."@en ;
    skos:definition "Romans met een combinatie van mystery, romantiek en horror. Dit genre ontstond in circa 1765 in Engeland, maar werd ook elders in Europa al snel populair, met het hoogtepunt in de jaren negentig van de achttiende eeuw. Het genre beleefde in de daaropvolgende eeuwen regelmatig een wederopbloei. Men noemde dit soort romans ���gotisch' omdat ze zich aanvankelijk vaak gedeeltelijk afspeelden in middeleeuwse ruïnes en gebouwen, zoals kastelen en kloosters."@nl, "Romantic fictions having a prevailing atmosphere of mystery and terror, often combined with a love story. The genre was introduced in England ca. 1765, but soon became popular elsewhere in Europe, reaching its heyday in the 1790s. The genre has undergone frequent revivals in subsequent centuries. It is called \"Gothic\" because the early examples were often set in part among medieval buildings and ruins, such as castles or monasteries."@en, "Romantische Prosa, die in einer Atmosphäre des Mysteriösen und Schreckensvollen spielt, häufig im Zusammenhang mit einer Liebesgeschichte. Das Genre wurde ca. 1765 in England entwickelt, wurde aber bald in ganz Europa beliebt und erreichte in den 1790er Jahren seine Blütezeit. In den nachfolgenden Jahrhunderten hat das Genre viele Wiederbelebungen erfahren. Es wird im Emglischen \"Gothic\" genannt, weil die frühen Beispiele oftmals zu Teilen in mittelalterlichen Bauten und Ruinen spielten, wie beispielsweise in Burgen oder Klöstern."@de, "瀰漫神秘與恐怖氛圍的浪漫小說，常與愛情故事結合。此一文類約於1765年始自英國，但迅即在歐洲其他地區流行，於1790年代達到顛峰。爾後本類型文體經歷頻繁的復興。稱「哥德體」係因早期作品常有部份設定於城堡或修道院之類的中世紀建築與遺跡裡。"@zh-hant ;
    skos:inScheme cwrc:Genre ;
    prov:derivedFrom <http://vocab.getty.edu/aat/300266777> .

cwrc:genreGovernmentreport
    void:inDataset cwrc:datasetdefinition ;
    a cwrc:Genre, skos:Concept ;
    rdf:value "GOVERNMENTREPORT" ;
    rdfs:isDefinedBy <http://www.cwrc.ca/ontologies/cwrc#> ;
    rdfs:label ""@fr, "government report"@en ;
    skos:inScheme cwrc:Genre .

cwrc:genreGrammar
    void:inDataset cwrc:datasetdefinition ;
    a cwrc:Genre, skos:Concept ;
    rdf:value "GRAMMAR" ;
    rdfs:isDefinedBy <http://www.cwrc.ca/ontologies/cwrc#> ;
    rdfs:label ""@fr, "grammar"@en ;
    skos:inScheme cwrc:Genre .

cwrc:genreGraveyardpoetry
    void:inDataset cwrc:datasetdefinition ;
    a cwrc:Genre, skos:Concept ;
    rdf:value "GRAVEYARDPOETRY" ;
    rdfs:isDefinedBy <http://www.cwrc.ca/ontologies/cwrc#> ;
    rdfs:label ""@fr, "graveyard poetry"@en ;
    skos:broaderTransitive cwrc:genrePoetry ;
    skos:inScheme cwrc:Genre .

cwrc:genreGuidebook
    void:inDataset cwrc:datasetdefinition ;
    a cwrc:Genre, skos:Concept ;
    rdf:value "GUIDEBOOK" ;
    rdfs:isDefinedBy <http://www.cwrc.ca/ontologies/cwrc#> ;
    rdfs:label ""@fr, "guidebook"@en ;
    skos:inScheme cwrc:Genre .

cwrc:genreHagiography
    void:inDataset cwrc:datasetdefinition ;
    a cwrc:Genre, skos:Concept ;
    rdf:value "HAGIOGRAPHY" ;
    rdfs:isDefinedBy <http://www.cwrc.ca/ontologies/cwrc#> ;
    rdfs:label ""@fr, "hagiography"@en ;
    owl:comment "This term and its description was created from data gathered from DBpedia."@en, "This term and its description was created from data gathered from the Getty Art & Architecture Thesaurus."@en ;
    skos:definition "Biografie eines Heiligen."@de, "Biografieën van heiligen."@nl, "Biografías de santos."@es, "Biographies of saints, usually written, but includes oral or visual works as well."@en, "L’hagiographie (du grec ancien ἅγιος / hágios (« saint ») et γράφειν / gráphein (« écrire »)) est l'écriture de la vie et / ou de l'œuvre des saints. Pour un texte particulier, on ne parle que rarement d'« une hagiographie » (sauf dans le sens figuré), mais plutôt d'un texte hagiographique ou tout simplement d'une vie de saint. Le texte hagiographique étant destiné à être lu, soit lors de l'office des moines soit en public dans le cadre de la prédication, on lui donne souvent le nom de légende (du latin legenda, « ce qui doit être lu », terme utilisé dans son acception la plus littérale et non dans son sens péjoratif actuel de récit dépourvu de tout enracinement dans l'histoire événementielle). Un texte hagiographique recouvre plusieurs genres littéraires ou artistiques parmi lesquels on compte en premier lieu la vita, c'est-à-dire le récit biographique de la vie du saint. Une fresque à épisode est également une hagiographie, de même qu'une simple notice résumant la vie du bienheureux. Par rapport à une biographie, l'hagiographie est un genre littéraire qui veut mettre en avant le caractère de sainteté du personnage dont on raconte la vie. L'écrivain, l'hagiographe n'a pas d'abord une démarche d'historien, surtout lorsque le genre hagiographique s'est déployé. Aussi les hagiographies anciennes sont parsemées de passages merveilleux à l'historicité douteuse. De plus, des typologies de saints existaient au Moyen Âge, ce qui a conduit les hagiographes à se conformer à ces modèles et à faire de nombreux emprunts à des récits antérieurs. L'hagiographie est ainsi un récit fortement stéréotypé dont la fonction pastorale est de servir à l'instruction et l'édification religieuse, mais qui peut avoir aussi une fonction normative, politique et de propagande religieuse. D'une manière plus polémique, on parle aussi d'hagiographie pour désigner un écrit (une biographie, l'analyse d'un système philosophique, etc.) trop favorable à son objet, c'est-à-dire manquant de recul et/ou ne laissant guère de place à la critique."@fr ;
    skos:inScheme cwrc:Genre ;
    prov:derivedFrom dbpedia:Hagiography, <http://vocab.getty.edu/aat/300201063> .

cwrc:genreHaiku
    void:inDataset cwrc:datasetdefinition ;
    a cwrc:Genre, skos:Concept ;
    rdf:value "HAIKU" ;
    rdfs:isDefinedBy <http://www.cwrc.ca/ontologies/cwrc#> ;
    rdfs:label ""@fr, "haiku"@en ;
    skos:inScheme cwrc:Genre .

cwrc:genreHarlequinade
    void:inDataset cwrc:datasetdefinition ;
    a cwrc:Genre, skos:Concept ;
    rdf:value "HARLEQUINADE" ;
    rdfs:isDefinedBy <http://www.cwrc.ca/ontologies/cwrc#> ;
    rdfs:label ""@fr, "harlequinade"@en ;
    skos:inScheme cwrc:Genre .

cwrc:genreHeroic
    void:inDataset cwrc:datasetdefinition ;
    a cwrc:Genre, skos:Concept ;
    rdf:value "HEROIC" ;
    rdfs:isDefinedBy <http://www.cwrc.ca/ontologies/cwrc#> ;
    rdfs:label ""@fr, "heroic"@en ;
    skos:inScheme cwrc:Genre .

cwrc:genreHistorical
    void:inDataset cwrc:datasetdefinition ;
    a cwrc:Genre, skos:Concept ;
    rdf:value "HISTORICAL" ;
    rdfs:isDefinedBy <http://www.cwrc.ca/ontologies/cwrc#> ;
    rdfs:label "historical"@en, "historique"@fr ;
    skos:inScheme cwrc:Genre .

cwrc:genreHistory
    void:inDataset cwrc:datasetdefinition ;
    a cwrc:Genre, skos:Concept ;
    rdf:value "HISTORY" ;
    rdfs:isDefinedBy <http://www.cwrc.ca/ontologies/cwrc#> ;
    rdfs:label ""@fr, "history"@en ;
    owl:comment "This term and its description was created from data gathered from the Getty Art & Architecture Thesaurus."@en ;
    skos:definition "Accounts of the chronological development of cases of disease or conditions of individuals, with details of symptoms."@en ;
    skos:inScheme cwrc:Genre ;
    prov:derivedFrom <http://vocab.getty.edu/aat/300026359> .

cwrc:genreHymn
    void:inDataset cwrc:datasetdefinition ;
    a cwrc:Genre, skos:Concept ;
    rdf:value "HYMN" ;
    rdfs:isDefinedBy <http://www.cwrc.ca/ontologies/cwrc#> ;
    rdfs:label ""@fr, "hymn"@en ;
    skos:inScheme cwrc:Genre .

cwrc:genreImitation
    void:inDataset cwrc:datasetdefinition ;
    a cwrc:Genre, skos:Concept ;
    rdf:value "IMITATION" ;
    rdfs:isDefinedBy <http://www.cwrc.ca/ontologies/cwrc#> ;
    rdfs:label ""@fr, "imitation"@en ;
    skos:inScheme cwrc:Genre .

cwrc:genreIndustrialnovel
    void:inDataset cwrc:datasetdefinition ;
    a cwrc:Genre, skos:Concept ;
    rdf:value "INDUSTRIALNOVEL" ;
    rdfs:isDefinedBy <http://www.cwrc.ca/ontologies/cwrc#> ;
    rdfs:label ""@fr, "industrial novel"@en ;
    skos:broaderTransitive cwrc:genreNovel ;
    skos:inScheme cwrc:Genre .

cwrc:genreIntroduction
    void:inDataset cwrc:datasetdefinition ;
    a cwrc:Genre, skos:Concept ;
    rdf:value "INTRODUCTION" ;
    rdfs:isDefinedBy <http://www.cwrc.ca/ontologies/cwrc#> ;
    rdfs:label ""@fr, "introduction"@en ;
    skos:inScheme cwrc:Genre .

cwrc:genreJournalism
    void:inDataset cwrc:datasetdefinition ;
    a cwrc:Genre, skos:Concept ;
    rdf:value "JOURNALISM" ;
    rdfs:isDefinedBy <http://www.cwrc.ca/ontologies/cwrc#> ;
    rdfs:label ""@fr, "journalism"@en ;
    skos:inScheme cwrc:Genre .

cwrc:genreJuvenilia
    void:inDataset cwrc:datasetdefinition ;
    a cwrc:Genre, skos:Concept ;
    rdf:value "JUVENILIA" ;
    rdfs:isDefinedBy <http://www.cwrc.ca/ontologies/cwrc#> ;
    rdfs:label ""@fr, "juvenilia"@en ;
    skos:inScheme cwrc:Genre .

cwrc:genreKitchensinkdrama
    void:inDataset cwrc:datasetdefinition ;
    a cwrc:Genre, skos:Concept ;
    rdf:value "KITCHENSINKDRAMA" ;
    rdfs:isDefinedBy <http://www.cwrc.ca/ontologies/cwrc#> ;
    rdfs:label ""@fr, "kitchensink drama"@en ;
    skos:inScheme cwrc:Genre .

cwrc:genreKunstlerroman
    void:inDataset cwrc:datasetdefinition ;
    a cwrc:Genre, skos:Concept ;
    rdf:value "KUNSTLERROMAN" ;
    rdfs:isDefinedBy <http://www.cwrc.ca/ontologies/cwrc#> ;
    rdfs:label ""@fr, "kunstlerroman"@en ;
    skos:inScheme cwrc:Genre .

cwrc:genreLais
    void:inDataset cwrc:datasetdefinition ;
    a cwrc:Genre, skos:Concept ;
    rdf:value "LAIS" ;
    rdfs:isDefinedBy <http://www.cwrc.ca/ontologies/cwrc#> ;
    rdfs:label ""@fr, "lais"@en ;
    owl:comment "This term and its description was created from data gathered from DBpedia."@en ;
    skos:definition "A laisse is a type of stanza, of varying length, found in medieval French literature, specifically medieval French epic poetry (the chanson de geste), such as The Song of Roland. In early works, each laisse was made up of (mono) assonanced verses, although the appearance of (mono) rhymed laisses was increasingly common in later poems. Within a poem, the length of each separate laisse is variable (whereas the metric length of the verses is invariable, each verse having the same syllable length, typically decasyllables or, occasionally, alexandrines. The laisse is characterized by stereotyped phrases and formulas and frequently repeated themes and motifs, including repetitions of material from one laisse to another. Such repetitions and formulaic structures are common of orality and oral-formulaic composition. When medieval poets repeated content (with different wording or assonance/rhyme) from one laisse to another, such \"similar\" laisses are called laisses similaires in French."@en ;
    skos:inScheme cwrc:Genre ;
    prov:derivedFrom dbpedia:Laisse .

cwrc:genreLampoon
    void:inDataset cwrc:datasetdefinition ;
    a cwrc:Genre, skos:Concept ;
    rdf:value "LAMPOON" ;
    rdfs:isDefinedBy <http://www.cwrc.ca/ontologies/cwrc#> ;
    rdfs:label ""@fr, "lampoon"@en ;
    skos:inScheme cwrc:Genre .

cwrc:genreLegalwriting
    void:inDataset cwrc:datasetdefinition ;
    a cwrc:Genre, skos:Concept ;
    rdf:value "LEGALWRITING" ;
    rdfs:isDefinedBy <http://www.cwrc.ca/ontologies/cwrc#> ;
    rdfs:label ""@fr, "legal writing"@en ;
    skos:inScheme cwrc:Genre .

cwrc:genreLegendFolktale
    void:inDataset cwrc:datasetdefinition ;
    a cwrc:Genre, skos:Concept ;
    rdf:value "LEGENDFOLKTALE" ;
    rdfs:isDefinedBy <http://www.cwrc.ca/ontologies/cwrc#> ;
    rdfs:label "legend folktale"@en, "légende et conte de fée"@fr ;
    skos:inScheme cwrc:Genre .

cwrc:genreLesbian
    void:inDataset cwrc:datasetdefinition ;
    a cwrc:Genre, skos:Concept ;
    rdf:value "LESBIAN" ;
    rdfs:isDefinedBy <http://www.cwrc.ca/ontologies/cwrc#> ;
    rdfs:label ""@fr, "lesbian"@en ;
    owl:comment "This term and its description was created from data gathered from DBpedia."@en ;
    skos:definition "Azalea: A Magazine by Third World Lesbians was a quarterly periodical for black, Asian, Latina, and Native American lesbians published between 1977 and 1983 by the Salsa Soul Sisters, Third World Wimmin Inc Collective. The Collective also published the Salsa Soul Sisters/Third World Women's Gay-zette (c. 1982)."@en ;
    skos:inScheme cwrc:Genre ;
    prov:derivedFrom <http://dbpedia.org/resource/Azalea:_A_Magazine_by_Third_World_Lesbians> .

cwrc:genreLetter
    void:inDataset cwrc:datasetdefinition ;
    a cwrc:Genre, skos:Concept ;
    rdf:value "LETTER" ;
    rdfs:isDefinedBy <http://www.cwrc.ca/ontologies/cwrc#> ;
    rdfs:label ""@fr, "letter"@en ;
    owl:comment "This term and its description was created from data gathered from the Getty Art & Architecture Thesaurus."@en ;
    skos:definition "Letters written to a newspaper or magazine to present a position, make a correction, or respond to another story or letter."@en-gb ;
    skos:inScheme cwrc:Genre ;
    prov:derivedFrom <http://vocab.getty.edu/aat/300343729> .

cwrc:genreLettersfromthedeadtotheliving
    void:inDataset cwrc:datasetdefinition ;
    a cwrc:Genre, skos:Concept ;
    rdf:value "LETTERSFROMTHEDEADTOTHELIVING" ;
    rdfs:isDefinedBy <http://www.cwrc.ca/ontologies/cwrc#> ;
    rdfs:label ""@fr, "letters from the dead to the living"@en ;
    skos:inScheme cwrc:Genre .

cwrc:genreLibretto
    void:inDataset cwrc:datasetdefinition ;
    a cwrc:Genre, skos:Concept ;
    rdf:value "LIBRETTO" ;
    rdfs:isDefinedBy <http://www.cwrc.ca/ontologies/cwrc#> ;
    rdfs:label ""@fr, "libretto"@en ;
    skos:inScheme cwrc:Genre .

cwrc:genreLiteraryCriticism
    void:inDataset cwrc:datasetdefinition ;
    a cwrc:Genre, skos:Concept ;
    rdf:value "LITERARYCRITICISM" ;
    rdfs:isDefinedBy <http://www.cwrc.ca/ontologies/cwrc#> ;
    rdfs:label "critiquelittéraire"@fr, "literary criticism"@en ;
    skos:inScheme cwrc:Genre .

cwrc:genreLiturgy
    void:inDataset cwrc:datasetdefinition ;
    a cwrc:Genre, skos:Concept ;
    rdf:value "LITURGY" ;
    rdfs:isDefinedBy <http://www.cwrc.ca/ontologies/cwrc#> ;
    rdfs:label ""@fr, "liturgy"@en ;
    skos:inScheme cwrc:Genre .

cwrc:genreLove
    void:inDataset cwrc:datasetdefinition ;
    a cwrc:Genre, skos:Concept ;
    rdf:value "LOVE" ;
    rdfs:isDefinedBy <http://www.cwrc.ca/ontologies/cwrc#> ;
    rdfs:label ""@fr, "love"@en ;
    owl:comment "This term and its description was created from data gathered from DBpedia."@en ;
    skos:inScheme cwrc:Genre ;
    prov:derivedFrom dbpedia:Christo .

cwrc:genreLyric
    void:inDataset cwrc:datasetdefinition ;
    a cwrc:Genre, skos:Concept ;
    rdf:value "LYRIC" ;
    rdfs:isDefinedBy <http://www.cwrc.ca/ontologies/cwrc#> ;
    rdfs:label "lyric"@en, "lyrique"@fr ;
    owl:comment "This term and its description was created from data gathered from DBpedia."@en ;
    skos:definition "Lyric Essay is a subgenre of essay writing, which combines qualities of poetry, essay, memoir, and research writing. The lyric essay is considered high art, and often requires work and association on behalf of the reader. Proponents of the lyric essay classification insist it differs from prose poetry in its reliance on association rather than line breaks and juxtaposition."@en ;
    skos:inScheme cwrc:Genre ;
    prov:derivedFrom dbpedia:Lyric_essay .

cwrc:genreMagicrealist
    void:inDataset cwrc:datasetdefinition ;
    a cwrc:Genre, skos:Concept ;
    rdf:value "MAGICREALIST" ;
    rdfs:isDefinedBy <http://www.cwrc.ca/ontologies/cwrc#> ;
    rdfs:label ""@fr, "magic realist"@en ;
    skos:inScheme cwrc:Genre .

cwrc:genreManifesto
    void:inDataset cwrc:datasetdefinition ;
    a cwrc:Genre, skos:Concept ;
    rdf:value "MANIFESTO" ;
    rdfs:isDefinedBy <http://www.cwrc.ca/ontologies/cwrc#> ;
    rdfs:label ""@fr, "manifesto"@en ;
    skos:inScheme cwrc:Genre .

cwrc:genreManual
    void:inDataset cwrc:datasetdefinition ;
    a cwrc:Genre, skos:Concept ;
    rdf:value "MANUAL" ;
    rdfs:isDefinedBy <http://www.cwrc.ca/ontologies/cwrc#> ;
    rdfs:label ""@fr, "manual"@en ;
    skos:inScheme cwrc:Genre .

cwrc:genreMap
    void:inDataset cwrc:datasetdefinition ;
    a cwrc:Genre, skos:Concept ;
    rdf:value "MAP" ;
    rdfs:isDefinedBy <http://www.cwrc.ca/ontologies/cwrc#> ;
    rdfs:label ""@fr, "map"@en ;
    skos:inScheme cwrc:Genre .

cwrc:genreMasque
    void:inDataset cwrc:datasetdefinition ;
    a cwrc:Genre, skos:Concept ;
    rdf:value "MASQUE" ;
    rdfs:isDefinedBy <http://www.cwrc.ca/ontologies/cwrc#> ;
    rdfs:label ""@fr, "masque"@en ;
    skos:inScheme cwrc:Genre .

cwrc:genreMedicalwriting
    void:inDataset cwrc:datasetdefinition ;
    a cwrc:Genre, skos:Concept ;
    rdf:value "MEDICALWRITING" ;
    rdfs:isDefinedBy <http://www.cwrc.ca/ontologies/cwrc#> ;
    rdfs:label ""@fr, "medical writing"@en ;
    skos:inScheme cwrc:Genre .

cwrc:genreMelodrama
    void:inDataset cwrc:datasetdefinition ;
    a cwrc:Genre, skos:Concept ;
    rdf:value "MELODRAMA" ;
    rdfs:isDefinedBy <http://www.cwrc.ca/ontologies/cwrc#> ;
    rdfs:label ""@fr, "melodrama"@en ;
    skos:inScheme cwrc:Genre .

cwrc:genreMixedmedia
    void:inDataset cwrc:datasetdefinition ;
    a cwrc:Genre, skos:Concept ;
    rdf:value "MIXEDMEDIA" ;
    rdfs:isDefinedBy <http://www.cwrc.ca/ontologies/cwrc#> ;
    rdfs:label ""@fr, "mixed media"@en ;
    skos:inScheme cwrc:Genre .

cwrc:genreMockforms
    void:inDataset cwrc:datasetdefinition ;
    a cwrc:Genre, skos:Concept ;
    rdf:value "MOCKFORMS" ;
    rdfs:isDefinedBy <http://www.cwrc.ca/ontologies/cwrc#> ;
    rdfs:label ""@fr, "mockforms"@en ;
    skos:inScheme cwrc:Genre .

cwrc:genreMonologue
    void:inDataset cwrc:datasetdefinition ;
    a cwrc:Genre, skos:Concept ;
    rdf:value "MONOLOGUE" ;
    rdfs:isDefinedBy <http://www.cwrc.ca/ontologies/cwrc#> ;
    rdfs:label ""@fr, "monologue"@en ;
    owl:comment "This term and its description was created from data gathered from DBpedia."@en ;
    skos:definition "Der Monolog (gr. μόνος mónos „allein“ und -log; lat. Soliloquium) ist im Gegensatz zum Dialog ein Selbstgespräch und findet vor allem im Drama Verwendung. Er richtet sich nicht direkt an einen Zuhörer, sondern an eine imaginäre Person. Faktisch ist das Publikum Adressat des Monologisierenden. Eine Sonderform des Monologs ist der Innere Monolog in der Erzählprosa. Der Ausdruck Monolog bezeichnet auch eine Rede, die so formuliert ist, als sei sie nicht an einen Zuhörer oder Gesprächspartner gerichtet. Oftmals wird damit nicht das alltägliche Selbstgespräch bezeichnet, sondern der bewusste Einsatz des alleinigen Redens, in der Kunst, vor allem im Theater und in der Literatur, zusammen mit Gesten. Dort dient der Monolog häufig dazu, Gedanken und seelische Vorgänge einer Person hörbar oder lesbar nach außen zu tragen und damit für Zuschauer oder Leser deutlich werden zu lassen. In vielen Theaterstücken bilden Monologe einen dramatischen Höhepunkt oder bezeichnen einen Wendepunkt der Handlung. Ein bekanntes Beispiel dafür ist der Hamlet-Monolog von Shakespeare. Im Englischen, Französischen und anderen Sprachen wird in der Literaturwissenschaft noch eine wichtige Sonderform des Monologs unterschieden. Diese Sonderform wird als (engl.) Soliloquy bezeichnet und erlaubt im Drama – im Gegensatz zum Monolog – Zuhörer. in gewisser Weise handelt es sich um ein meist dramatisches Selbstgespräch."@de, "Een monoloog is alleenspraak; een betoog van één persoon die aan het woord is (en blijft), vaak zonder dat er toehoorders zijn. Monoloog komt van het Grieks, waar μονος (monos) één en alleen betekent, en λογος (logos) woord of idee betekent. In het theater is het een toneeloptreden van één acteur binnen een toneelstuk. Daarvoor wordt vaak de term soliloque gebruikt. In een gesprek op een bijeenkomst betekent een monoloog dat de andere aanwezigen niet aan het woord kunnen of mogen komen. Een toespraak dus. Het is het tegengestelde van een dialoog."@nl, "In theatre, a monologue (from Greek μονόλογος from μόνος mónos, \"alone, solitary\" and λόγος lógos, \"speech\") is a speech presented by a single character, most often to express their mental thoughts aloud, though sometimes also to directly address another character or the audience. Monologues are common across the range of dramatic media (plays, films, etc.), as well as in non-dramatic media such as poetry. Monologues share much in common with several other literary devices including soliloquies, apostrophes, and aside. There are, however, distinctions between each of these devices."@en, "Monólogo (del griego mono: uno; y logo: palabra) es un discurso que emite una sola persona tanto para un solo ente receptor como para hacia otros receptores (personajes, lectores, auditorio, a una cosa, a un personaje o a un narrador). El monólogo es un recurso utilizado en todos los géneros literarios que puede encontrarse tanto en poesía, cuento, periodismo, discusión, teatro, como en novela."@es, "Un monologue (du grec mono : \"un seul\", et logos : \"discours\") est une ou plusieurs phrases auto-adressées à haute voix, rapportant les pensées du locuteur au style direct.Il faut distinguer le véritable monologue non seulement, cela va de soi, du roman autobiographique à la première personne, qui suppose un décalage de temps, même minime (\"Aujourd'hui maman est morte\") entre la narration et le narré, mais aussi d'une forme d'écriture fictionnelle moderne, la représentation du flux intérieur sous la forme je ou tu."@fr ;
    skos:inScheme cwrc:Genre ;
    prov:derivedFrom dbpedia:Monologue .

cwrc:genreMoralitymysteryplay
    void:inDataset cwrc:datasetdefinition ;
    a cwrc:Genre, skos:Concept ;
    rdf:value "MORALITYMYSTERYPLAY" ;
    rdfs:isDefinedBy <http://www.cwrc.ca/ontologies/cwrc#> ;
    rdfs:label ""@fr, "morality mystery play"@en ;
    skos:inScheme cwrc:Genre .

cwrc:genreMultimedia
    void:inDataset cwrc:datasetdefinition ;
    a cwrc:Genre, skos:Concept ;
    rdf:value "MULTIMEDIA" ;
    rdfs:isDefinedBy <http://www.cwrc.ca/ontologies/cwrc#> ;
    rdfs:label ""@fr, "multimedia"@en ;
    skos:inScheme cwrc:Genre .

cwrc:genreMusicology
    void:inDataset cwrc:datasetdefinition ;
    a cwrc:Genre, skos:Concept ;
    rdf:value "MUSICOLOGY" ;
    rdfs:isDefinedBy <http://www.cwrc.ca/ontologies/cwrc#> ;
    rdfs:label ""@fr, "musicology"@en ;
    skos:inScheme cwrc:Genre .

cwrc:genreMystery
    void:inDataset cwrc:datasetdefinition ;
    a cwrc:Genre, skos:Concept ;
    rdf:value "MYSTERY" ;
    rdfs:isDefinedBy <http://www.cwrc.ca/ontologies/cwrc#> ;
    rdfs:label ""@fr, "mystery"@en ;
    skos:inScheme cwrc:Genre .

cwrc:genreMyth
    void:inDataset cwrc:datasetdefinition ;
    a cwrc:Genre, skos:Concept ;
    rdf:value "MYTH" ;
    rdfs:isDefinedBy <http://www.cwrc.ca/ontologies/cwrc#> ;
    rdfs:label ""@fr, "myth"@en ;
    owl:comment "This term and its description was created from data gathered from DBpedia."@en, "This term and its description was created from data gathered from the Getty Art & Architecture Thesaurus."@en ;
    skos:definition "Legendary stories without a determinable basis of fact or natural explanation, typically concerning a being, hero, deity, or event and explains some practice, rite, or phenomenon of nature."@en, "Mythe (Grieks: mythos; μυθος) betekende oorspronkelijk in het Grieks gesproken woord, verhaal.De betekenis is afhankelijk van de context: In tegenstelling tot wat bij sagen, sprookjes en fabels meestal het geval is, gaan mythen in hoofdzaak over goden en halfgoden."@nl, "Sagenhafte Geschichte ohne bestimmbare Faktengrundlage oder natürliche Erklärung, die in der Regel ein Wesen, einen Helden, eine Gottheit oder ein Ereignis zum Thema hat und eine bestimmte Praxis, einen Ritus oder ein Naturphänomen erklärt."@de, "Un mito (del griego μῦθος, mythos, «relato», «cuento») es un relato tradicional que se refiere a acontecimientos prodigiosos, protagonizados por seres sobrenaturales o extraordinarios, tales como dioses, semidioses, héroes, monstruos o personajes fantásticos, los cuales buscan dar una explicación a un hecho o fenómeno."@es, "Un mythe est un récit qui se veut explicatif et surtout fondateur d'une pratique sociale. Il est porté à l'origine par une tradition orale, qui propose une explication pour certains aspects fondamentaux du monde et de la société qui a forgé ou qui véhicule ces mythes : L'étude des mythes est appelée mythologie. Le terme mythe est souvent employé pour désigner une croyance manifestement erronée au premier abord, mais qui peut se rapporter à des éléments concrets exprimés de façon symbolique et partagée par un nombre significatif de personnes. Le mythe se distingue de la légende (qui suppose quelques faits historiques identifiables), du conte (qui se veut inventif sans expliquer), et du roman (qui \"explique\" avec peu de fondements)."@fr ;
    skos:inScheme cwrc:Genre ;
    prov:derivedFrom dbpedia:Myth, <http://vocab.getty.edu/aat/300201023> .

cwrc:genreNarrativepoetry
    void:inDataset cwrc:datasetdefinition ;
    a cwrc:Genre, skos:Concept ;
    rdf:value "NARRATIVEPOETRY" ;
    rdfs:isDefinedBy <http://www.cwrc.ca/ontologies/cwrc#> ;
    rdfs:label ""@fr, "narrative poetry"@en ;
    owl:comment "This term and its description was created from data gathered from DBpedia."@en ;
    skos:broaderTransitive cwrc:genrePoetry ;
    skos:definition "La narrativa poética o poesía narrativa es aquella que narra una historia. La longitud del poema y la complejidad de la historia varía de un poema a otro, no hay un criterio establecido. Por norma general, no suelen ser dramáticos, presentan versos objetivos y un esquema métrico y rima regular. Entre los poemas narrativos se encuentran la poesía épica, la poesía lírica, la balada y la égloga. Los poemas narrativos son una forma de arte. La poesía narrativa es uno de los más antiguos géneros dentro de la poesía. En la mayoría de las primeras obras literarias que se conocen, desde la epopeya de Gilgamesh hasta los poemas homéricos, tanto en la literatura en inglés antiguo como en la poesía en nórdico antiguo, así como la epopeya en sánscrito titulada Mahábharata, aparecen poemas narrativos. Muchos estudiosos de Homero, desde Quinto de Esmirna en adelante, han llegado a la conclusión de que los cuentos de la Ilíada y la Odisea fueron creados a partir de recopilaciones de poemas narrativos cortos que narraban historias individuales, las cuales resultaban más adecuadas para ser contadas alrededor de una hoguera. Algunos poemas narrativos deben ser considerados novelas en verso, como el extenso poema The Ring and the Book de Robert Browning. En cuanto a la poesía narrativa, un romance es un poema narrativo que cuentan historias de caballería. Algunos ejemplos son el Roman de la Rose, de Guillaume de Lorris, o los Idilios del rey, de Lord Tennyson. Aunque estos ejemplos describen historias medievales y leyendas artúricas, los romances también puede contar historias basadas en la [[mitología clásica. Los poemas narrativos más cortos tener un estilo literario similar al de los cuentos. A veces, estas narraciones breves se recogen compilaciones, como los Los cuentos de Canterbury de Chaucer. Algunas obras literarias contienen prosa narrativa, en la que se incluyen poemas e interludios poéticos.Un ejemplo de esta modalidad es la Vita Nuova de Dante Alighierl. pero el existió pero hace mucho mucho tiempo"@es, "La poésie narrative est un courant de la poésie italienne contemporaine dont les principaux représentants sont Carlo Bordini, Mauro Fabi et Andrea di Consoli. Cette poésie, qui sans renoncer à sa dimension expérimentale ou à une certaine forme de lyrisme exploite des matériaux divers - en usant du collage ou en incluant des fragments discursifs ou narratifs - et s'appuie sur le rythme et l'oralité non pour cacher le sens, mais pour le révéler."@fr, "Narratieve poëzie (ook verhalende dichtkunst of epische poëzie genoemd) is poëzie die een verhaal vertelt. Het is een poëziegenre waartoe zowel korte als langere gedichten kunnen behoren en waarbij het verhaal eenvoudig of complex kan zijn. Meestal wordt een regelmatig rijmschema en metrum gehanteerd. Voorbeelden van verhalende gedichten zijn heldendichten, balladen, idylles en lays. Het oudste overgeleverd verhalend gedicht is het Babylonische epos van Gilgamesj dat dateert uit het 2e millennium v.Chr. In de Middelnederlandse literatuur zijn de ballade 'Heer Halewijn zong een liedekijn' en het Arthurverhaal Ferguut bekende voorbeelden. In sommige gevallen wordt verhalende poëzie gepresenteerd in de vorm van een roman in verzen. Een voorbeeld hiervan is The Ring and the Book van Robert Browning. Een romance is een verhalend gedicht dat een verhaal vertelt over ridderlijkheid. Voorbeelden hiervan zijn Romance of the Rose van Alfred Tennyson. Romancedichters behandelen vaak idyllisch voorgestelde taferelen uit de middeleeuwen en uit de klassieke mythologie of inspireren zich op verhalen over de legendarische koning Arthur. Kortere verhalende gedichten vertonen vaak stilistische gelijkenissen met korte verhalen. Soms zijn deze korte verhalen verzameld in aan elkaar verwante groepen, zoals bij Chaucers Canterbury Tales. Sommige vormen van literatuur bevatten prozaverhalen waarin ook gedichten en poëtische intermezzo's zijn opgenomen. Zo is veel oude Ierse poëzie opgenomen in prozaverhalen, en de oude Noordse sagen omvatten zowel incidentele poëzie als biografieën van dichters. Een voorbeeld is \"The Cremation of Sam McGee\" door Robert Service."@nl, "Narrative Poesie ist dadurch gekennzeichnet, dass in ihr Handlung eine wesentliche Rolle spielt und dass sie weitgehend in Versen geschrieben ist. In der Poetik des Aristoteles war dieser Bereich allein durch das Epos abgedeckt, heute rechnen eine große Zahl von Mischformen dazu. In der Ballade finden sich oft Elemente aus allen drei Dichtungsgattungen erzählende, lyrische und dramatische. Idyllen und Lais haben meist primär erzählenden Charakter. Versromane unterscheiden sich vom modernen Roman nicht nur durch die Verwendung des Metrums, sondern haben auch inhaltliche Gemeinsamkeiten mit dem antiken Epos (Heldenreise). Das gilt auch für die Romanzen. In der Versnovelle, Beispiele sind Meier Helmbrecht und insbesondere Chaucers Canterbury Tales, sind dagegen kaum Unterschiede zu der zeitlich parallelen Prosa zu finden. Bei Chaucer stehen Prosa und Verserzählung nebeneinander. In manchen Dichtungsformen ist die Prosaerzählung stark von Versen durchsetzt, so in den altnordischen Sagas und in der Dichtung irischer Barden."@de, "Narrative poetry is a form of poetry that tells a story, often making use of the voices of a narrator and characters as well; the entire story is usually written in metred verse. Narrative poems do not have to follow rhythmic patterns. The poems that make up this genre may be short or long, and the story it relates to may be complex. It is usually well it normally dramatic, with objectives, diverse characters, and metre. Narrative poems include epics, ballads, idylls, and lays. Some narrative poetry takes the form of a novel in verse. An example of this is The Ring and the Book by Robert Browning. In terms of narrative poetry, a romance is a narrative poem that tells a story of chivalry. Examples include the Romance of the Rose or Tennyson's Idylls of the King. Although these examples use medieval and Arthurian materials, romances may also tell stories from classical mythology. Shorter narrative poems are often similar in style to the short story. Sometimes these short narratives are collected into interrelated groups, as with Chaucer's The Canterbury Tales. Some literatures contain prose naose narratives, and the Old Norse sagas include both incidental poetry and the biographies of poets. An example is \"The Cremation of Sam McGee\" by Robert Service."@en ;
    skos:inScheme cwrc:Genre ;
    prov:derivedFrom dbpedia:Narrative_poetry .

cwrc:genreNationaltale
    void:inDataset cwrc:datasetdefinition ;
    a cwrc:Genre, skos:Concept ;
    rdf:value "NATIONALTALE" ;
    rdfs:isDefinedBy <http://www.cwrc.ca/ontologies/cwrc#> ;
    rdfs:label ""@fr, "national tale"@en ;
    skos:inScheme cwrc:Genre .

cwrc:genreNotebook
    void:inDataset cwrc:datasetdefinition ;
    a cwrc:Genre, skos:Concept ;
    rdf:value "NOTEBOOK" ;
    rdfs:isDefinedBy <http://www.cwrc.ca/ontologies/cwrc#> ;
    rdfs:label ""@fr, "notebook"@en ;
    owl:comment "This term and its description was created from data gathered from DBpedia."@en ;
    skos:definition "Notebook is a style of writing where people jot down what they have thought or heard at the spur of moment. The contents of a notebook are unorganized, and the number of subjects covered in a notebook are unlimited: a paragraph of autobiography can be followed immediately by one on astronomy or one on history. Some famous authors are also famous for the notebooks they left. The Italian poet Giacomo Leopardi kept a notebook, called Zibaldone, from 1817 to 1832. The idea of keeping that, which contains no fewer than 4,526 pages, was possibly suggested by a priest who fled from the French Revolution and came to live in the poet's hometown. The priest suggested that \"every literary man should have a written chaos such as this: notebook containing sottiseries, adrersa, excerpta, pugillares, commentaria... the store-house out of which fine literature of every kind may come, as the sun, moon, and stars issued out of chaos.\" There are writers who earned their posthumous fame solely by their notebooks, such as the German scientist and humorous writer Georg Lichtenberg. He called his notebooks \"waste book,\" using the English book-keeping term. He explains the purpose of his \"waste book\" in his notebook E: The notebooks of scientists, such as those of Michael Faraday and Charles Darwin, can reveal the development of their scientific theories. On the other hand, the notebooks used by scientists for recording their experiments are called lab notebooks. The notebooks used by artists are usually referred as sketchbooks, which may contain more than sketches. Leonardo da Vinci's notebooks contain his writings on painting, sculpture, architecture, anatomy, mining, inventions and music, as well as his sketches, his grocery lists and the names of people who owed him money. In Chinese literature, \"notebook\" or biji is a distinct genre, and has a broader meaning."@en, "Pinselnotizen oder Pinselaufzeichnungen (chinesisch 筆記 / 笔记, Pinyin bǐjì) sind eine schwer abgrenzbare Gattung von Kurzprosa überwiegend aus der klassischen chinesischen Literatur. Das Wort lässt sich grob mit „Notizbuch“ oder „Aufzeichnungen“ übersetzen (als Schreibmaterial diente der Schreibpinsel). Pinselnotizen bestehen meist aus kurzen Gedankenskizzen, Literaturkritik, Tagebuchaufzeichnungen, Anekdoten, Zitaten, auch Reiseberichten, Abenteuer- und Geistergeschichten, Witzen, Rätseln und Kleinprosa jeglicher Art. Das Genre bildete sich während der Wei- und Jin-Dynastie in der Zeit der Sechs Dynastien heraus und reifte in der Zeit der Tang-Dynastie heran. In voller Blüte stand die Biji-Literatur während der Zeit der Song-Dynastie. Auch in späteren Epochen wurde diese Literaturgattung ausgiebig gepflegt. Die Prosastücke wurden oft in Sammlungen herausgegeben und sind heute als wertvolle kulturgeschichtliche Quellen geschätzt. Berühmte Pinselnotizen sind die Werke Shishuo xinyu (世說新語) von Liu Yiqing (劉義慶) (Song-Dynastie der Südlichen Dynastien), Youyang zazu (酉陽雜俎) von Duan Chengshi (Tang-Dynastie), Song Jingwen biji (宋景文笔记) von Song Qi (宋祁) (Song-Dynastie), Chouchi biji (仇池笔记) von Su Shi (苏轼), Mengxi bitan (夢溪筆談) von Shen Kuo (auch: Shen Gua) (沈括) (Song-Dynastie) und Rongzhai suibi (容齋隨筆) von Hong Mai (Song-Dynastie), Dongjing meng Hua lu (東京夢華錄) von Meng Yuanlao (孟元老) (Südliche Song-Dynastie), Shanju xinhua (山居新话) von Yang Yu (杨瑀) Yuan-Dynastie, Wuli xiaoshi (物理小識) von Fang Yizhi (Ming-Dynastie), Yuewei caotang biji (閱微草堂筆記) von Ji Yun (紀昀) (Qing-Dynastie). Viele Pinselnotizen sind in sogenannten congshu („Sammelwerken“) überliefert, wie beispielsweise dem Shuofu (说郛), oder für spätere Epochen den Sammelwerken Ming Qing biji congkan (明清笔记丛刊) oder „Qingdai biji congkan“ (清代笔记丛刊)."@de ;
    skos:inScheme cwrc:Genre ;
    prov:derivedFrom <http://dbpedia.org/resource/Notebook_(style)> .

cwrc:genreNovel
    void:inDataset cwrc:datasetdefinition ;
    a cwrc:Genre, skos:Concept ;
    rdf:value "NOVEL" ;
    rdfs:isDefinedBy <http://www.cwrc.ca/ontologies/cwrc#> ;
    rdfs:label "novel"@en, "roman"@fr ;
    owl:comment "This term and its description was created from data gathered from the Getty Art & Architecture Thesaurus."@en ;
    skos:definition "Fiktionale Prosaerzählung beträchtlichen Umfangs und einiger Komplexität, die auf fantasievolle Weise menschliche Erfahrungen durch eine verknüpfte Reihe von Ereignissen mit einer Gruppe von Personen in einem bestimmten Umfeld schildert."@de, "Invented prose narratives of considerable length and a certain complexity that deal imaginatively with human experience through a connected sequence of events involving a group of persons in a specific setting."@en, "Narraciones ficticias en prosa de considerable extensión y una cierta complejidad que tratan imaginativamente sobre experiencias humanas a través de una secuencia relacionada de sucesos que involucran a un grupo de personas en un escenario específico."@es, "Verzonnen prozaverhalen van aanzienlijke lengte en een zekere complexiteit die op verbeeldingsrijke wijze de menselijke ervaring behandelen aan de hand van een reeks onderling verbonden gebeurtenissen rond een groep personen in een specifieke omgeving."@nl, "具相當長度與一定程度複雜性的虛構散文體記敘文，藉由與一群人，於一特定背景中相關聯的一連串事件，於想像中處理人類經驗。"@zh-hant ;
    skos:inScheme cwrc:Genre ;
    prov:derivedFrom <http://vocab.getty.edu/aat/300202580> .

cwrc:genreNovella
    void:inDataset cwrc:datasetdefinition ;
    a cwrc:Genre, skos:Concept ;
    rdf:value "NOVELLA" ;
    rdfs:isDefinedBy <http://www.cwrc.ca/ontologies/cwrc#> ;
    rdfs:label ""@fr, "novella"@en ;
    owl:comment "This term and its description was created from data gathered from the Getty Art & Architecture Thesaurus."@en ;
    skos:definition "Kurze, in der Renaissance beliebte Prosageschichte und in späteren Zeiten Prosaerzählung, zwischen Roman und Kurzgeschichte einzuordnen."@de, "Short prose tales popular in the Renaissance and for later prose narratives intermediate between novels and short stories."@en, "Wordt gebruikt voor korte prozaverhalen die in de renaissance populair waren en voor moderne prozavertellingen die korter zijn dan romans maar langer dan korte verhalen."@nl, "Úsese para cuentos cortos en prosa populares en el Renacimiento y para narraciones en prosa posteriores que se ubican entre la novela y el cuento breve."@es, "指文藝復興時期流行的短篇散文體故事，並指後來介於長篇小說與短篇故事之間的散文體記敘文。"@zh-hant ;
    skos:inScheme cwrc:Genre ;
    prov:derivedFrom <http://vocab.getty.edu/aat/300202569> .

cwrc:genreNurseryrhyme
    void:inDataset cwrc:datasetdefinition ;
    a cwrc:Genre, skos:Concept ;
    rdf:value "NURSERYRHYME" ;
    rdfs:isDefinedBy <http://www.cwrc.ca/ontologies/cwrc#> ;
    rdfs:label ""@fr, "nurseryrhyme"@en ;
    skos:inScheme cwrc:Genre .

cwrc:genreObituary
    void:inDataset cwrc:datasetdefinition ;
    a cwrc:Genre, skos:Concept ;
    rdf:value "OBITUARY" ;
    rdfs:isDefinedBy <http://www.cwrc.ca/ontologies/cwrc#> ;
    rdfs:label ""@fr, "obituary"@en ;
    owl:comment "This term and its description was created from data gathered from DBpedia."@en ;
    skos:definition "Obituary poetry, in the broad sense, includes any poem that commemorates a person or group of people's death: an elegy. In its stricter sense, though, it refers to a genre of popular verse or folk poetry that had its greatest popularity in the nineteenth century, especially in the United States of America. The genre consists largely of sentimental narrative verse that tells the story of the demise of its typically named subjects, and seeks to console their mourners with descriptions of their happy afterlife. The genre achieved its peak of popularity in the decade of the 1870s. While usually full chiefly of conventional pious sentiments, the obituary poets in one sense continue the program of meditations on death begun by the eighteenth-century graveyard poets, such as Edward Young's Night Thoughts, and as such continue one of the themes that went into literary Romanticism."@en ;
    skos:inScheme cwrc:Genre ;
    prov:derivedFrom dbpedia:Obituary_poetry .

cwrc:genreOccasionalpoetry
    void:inDataset cwrc:datasetdefinition ;
    a cwrc:Genre, skos:Concept ;
    rdf:value "OCCASIONALPOETRY" ;
    rdfs:isDefinedBy <http://www.cwrc.ca/ontologies/cwrc#> ;
    rdfs:label ""@fr, "occasional poetry"@en ;
    owl:comment "This term and its description was created from data gathered from DBpedia."@en ;
    skos:broaderTransitive cwrc:genrePoetry ;
    skos:definition "Der Ausdruck Gelegenheitsdichtung (Casualpoesie sowie parallele Wortbildungen auf -lyrik) bezeichnet in der Literaturwissenschaft Dichtung, die meist unter kommerziellen Gesichtspunkten auf einen speziellen Anlass hin verfasst wird (Gelegenheitsschrift). Goethe verwendet in Dichtung und Wahrheit und in den Gesprächen mit Eckermann den Ausdruck „Gelegenheitsgedicht“ auch in einem weniger abschätzigen Sinn für Gedichte, die sich der Inspiration eines Augenblicks verdanken, der nun im Gedicht festgehalten ist."@de, "Occasional poetry is poetry composed for a particular occasion. In the history of literature, it is often studied in connection with orality, performance, and patronage."@en ;
    skos:inScheme cwrc:Genre ;
    prov:derivedFrom dbpedia:Occasional_poetry .

cwrc:genreOde
    void:inDataset cwrc:datasetdefinition ;
    a cwrc:Genre, skos:Concept ;
    rdf:value "ODE" ;
    rdfs:isDefinedBy <http://www.cwrc.ca/ontologies/cwrc#> ;
    rdfs:label ""@fr, "ode"@en ;
    owl:comment "This term and its description was created from data gathered from the Getty Art & Architecture Thesaurus."@en ;
    skos:definition "Geëxalteerde lyrische gedichten waarin een verheven onderwerp wordt bezongen, vaak met gebruikmaking van complexe of onregelmatige metrische patronen."@nl, "Lyric poems of exalted emotion devoted to the praise or celebration of its subject; often employing complex or irregular metrical form."@en, "Lyrisches Gedicht von erhabener Haltung zur Ehre oder Feier seines Gegenstandes; häufig in komplexer oder unregelmäßiger metrischer Form."@de, "Poemas líricos de sentimientos elevados destinados al elogio o celebración del tema tratado, a menudo empleando formas métricas complejas o irregulares."@es ;
    skos:inScheme cwrc:Genre ;
    prov:derivedFrom <http://vocab.getty.edu/aat/300253045> .

cwrc:genreOneactplay
    void:inDataset cwrc:datasetdefinition ;
    a cwrc:Genre, skos:Concept ;
    rdf:value "ONEACTPLAY" ;
    rdfs:isDefinedBy <http://www.cwrc.ca/ontologies/cwrc#> ;
    rdfs:label ""@fr, "one act play"@en ;
    skos:inScheme cwrc:Genre .

cwrc:genreOpera
    void:inDataset cwrc:datasetdefinition ;
    a cwrc:Genre, skos:Concept ;
    rdf:value "OPERA" ;
    rdfs:isDefinedBy <http://www.cwrc.ca/ontologies/cwrc#> ;
    rdfs:label ""@fr, "opera"@en ;
    skos:inScheme cwrc:Genre .

cwrc:genreOratorio
    void:inDataset cwrc:datasetdefinition ;
    a cwrc:Genre, skos:Concept ;
    rdf:value "ORATORIO" ;
    rdfs:isDefinedBy <http://www.cwrc.ca/ontologies/cwrc#> ;
    rdfs:label ""@fr, "oratorio"@en ;
    skos:inScheme cwrc:Genre .

cwrc:genreOriental
    void:inDataset cwrc:datasetdefinition ;
    a cwrc:Genre, skos:Concept ;
    rdf:value "ORIENTAL" ;
    rdfs:isDefinedBy <http://www.cwrc.ca/ontologies/cwrc#> ;
    rdfs:label ""@fr, "oriental"@en ;
    skos:inScheme cwrc:Genre .

cwrc:genrePageant
    void:inDataset cwrc:datasetdefinition ;
    a cwrc:Genre, skos:Concept ;
    rdf:value "PAGEANT" ;
    rdfs:isDefinedBy <http://www.cwrc.ca/ontologies/cwrc#> ;
    rdfs:label ""@fr, "pageant"@en ;
    skos:inScheme cwrc:Genre .

cwrc:genrePanegyric
    void:inDataset cwrc:datasetdefinition ;
    a cwrc:Genre, skos:Concept ;
    rdf:value "PANEGYRIC" ;
    rdfs:isDefinedBy <http://www.cwrc.ca/ontologies/cwrc#> ;
    rdfs:label ""@fr, "panegyric"@en ;
    skos:inScheme cwrc:Genre .

cwrc:genrePantomime
    void:inDataset cwrc:datasetdefinition ;
    a cwrc:Genre, skos:Concept ;
    rdf:value "PANTOMIME" ;
    rdfs:isDefinedBy <http://www.cwrc.ca/ontologies/cwrc#> ;
    rdfs:label ""@fr, "pantomime"@en ;
    skos:inScheme cwrc:Genre .

cwrc:genreParable
    void:inDataset cwrc:datasetdefinition ;
    a cwrc:Genre, skos:Concept ;
    rdf:value "PARABLE" ;
    rdfs:isDefinedBy <http://www.cwrc.ca/ontologies/cwrc#> ;
    rdfs:label ""@fr, "parable"@en ;
    owl:comment "This term and its description was created from data gathered from DBpedia."@en, "This term and its description was created from data gathered from the Getty Art & Architecture Thesaurus."@en ;
    skos:definition "Kurze, fiktive Geschichte, die eine moralische Haltung oder ein religiöses Prinzip veranschaulicht."@de, "Short, fictitious stories that illustrate a moral attitude or religious principle."@en, "Une parabole (du grec παραϐολή, « rapprochement, comparaison ») est une des variétés de l’allégorie. La parabole est une figure de rhétorique consistant en une courte histoire qui utilise les événements quotidiens pour illustrer un enseignement, une morale ou une doctrine. Tandis que celle-ci, en général, présente directement le fait qu’elle a en vue, la parabole offre, sous ses couleurs véritables, un fait qui doit servir à la démonstration d’une vérité d’un autre ordre, avec laquelle elle a une relation plus ou moins facile à saisir. « Substituez dans la parabole, dit l’abbé Girard, le véritable fait à celui qu’elle expose, vous changerez le fond du discours : substituez dans l’allégorie les véritables couleurs à celles qu’elle emprunte, vous ne changerez que la forme. » On la trouve également dans le discours argumentatif lorsqu’un récit illustre la thèse défendue pour faciliter la compréhension du lecteur. La parabole est également un récit allégorique qui permet de dispenser un enseignement moral ou religieux. Présente dans la Bible où elle joue le rôle de l’apologue et de la fable, surtout les Évangiles, qui l'ont empruntée au midrash hébreu, la parabole est reprise dans les sermons des orateurs chrétiens. Le Nouveau Testament en contient un très grand nombre : le grain de sénevé ou l’Église, le Bon Samaritain ou l’amour de l’humanité, le levain ou la grâce, les loups ravisseurs sous des peaux d’agneaux ou les instituteurs de fausses doctrines, le travail des ouvriers de la vigne ou les œuvres du salut, le mauvais riche ou l’obligation de l’aumône, le bon pasteur, etc. Les paraboles sont plus fréquentes encore dans la littérature bouddhique ; les Avadanas, le Hitopadekas donnent à peine l’idée des recueils plus vastes dont ils sont extraits et dont l’un s’appelle le Yu-Lin, c’est-à-dire la « Forêt de comparaisons». Dans les littératures modernes, les Allemands ont surtout cultivé la parabole ; Lessing, Herder, Krummacher y ont particulièrement réussi. Dans le Bouc émissaire, page 270, René Girard remarque que « paraballo signifie jeter quelque chose en pâture à la foule pour apaiser son appétit de violence, de préférence une victime, un condamné à mort ; c'est ainsi qu'on se tire soi-même d'une situation épineuse, de toute évidence. C'est pour empêcher la foule de se retourner contre l'orateur que celui-ci recourt à la parabole, c'est-à-dire à la métaphore. »"@fr, "Wordt gebruikt voor korte, verzonnen verhalen waarin een moreel standpunt of religieus principe wordt toegelicht."@nl, "Úsese para relatos cortos imaginarios que ilustran una actitud moral o un principio religioso."@es ;
    skos:inScheme cwrc:Genre ;
    prov:derivedFrom dbpedia:Parable, <http://vocab.getty.edu/aat/300185342> .

cwrc:genreParatexts
    void:inDataset cwrc:datasetdefinition ;
    a cwrc:Genre, skos:Concept ;
    rdf:value "PARATEXTS" ;
    rdfs:isDefinedBy <http://www.cwrc.ca/ontologies/cwrc#> ;
    rdfs:label "paratextes"@fr, "paratexts"@en ;
    skos:inScheme cwrc:Genre .

cwrc:genreParody
    void:inDataset cwrc:datasetdefinition ;
    a cwrc:Genre, skos:Concept ;
    rdf:value "PARODY" ;
    rdfs:isDefinedBy <http://www.cwrc.ca/ontologies/cwrc#> ;
    rdfs:label ""@fr, "parody"@en ;
    owl:comment "This term and its description was created from data gathered from DBpedia."@en ;
    skos:definition "A parody (/ˈpærədi/; also called spoof, send-up, take-off or lampoon), in use, is a work created to imitate, make fun of, or comment on an original work, its subject, author, style, or some other target, by means of satiric or ironic imitation. As the literary theorist Linda Hutcheon puts it, \"parody … is imitation, not always at the expense of the parodied text.\" Another critic, Simon Dentith, defines parody as \"any cultural practice which provides a relatively polemical allusive imitation of another cultural production or practice.\"Parody may be found in art or culture, including literature, music (although \"parody\" in music has an earlier, somewhat different meaning than for other art forms), animation, gaming and film. The writer and critic John Gross observes in his Oxford Book of Parodies, that parody seems to flourish on territory somewhere between pastiche (\"a composition in another artist's manner, without satirical intent\") and burlesque (which \"fools around with the material of high literature and adapts it to low ends\"). Meanwhile, the Encyclopédie of Denis Diderot distinguishes between the parody and the burlesque, \"A good parody is a fine amusement, capable of amusing and instructing the most sensible and polished minds; the burlesque is a miserable buffoonery which can only please the populace.\" Historically, when a formula grows tired, as in the case of the moralistic melodramas in the 1910s, it retains value only as a parody, as demonstrated by the Buster Keaton shorts that mocked that genre. In his 1960 anthology of parody from the 14th through 20th centuries, critic Dwight Macdonald offered this metaphor: \"Parody is making a new wine that tastes like the old but has a slightly lethal effect.\""@en, "Een parodie of persiflage is een spottende nabootsing van een gedicht, lied, film, toneelstuk, verhaal of andere uiting. Vaak worden hierbij herkenbare eigenschappen van het origineel overdreven of uitvergroot."@nl, "Eine Parodie (griechisch παρῳδία parōdía „Gegenlied“ oder „verstellt gesungenes Lied“) ist eine verzerrende, übertreibende oder verspottende Nachahmung."@de, "La parodia (del griego, παρώδïα, παρα, en contra de o al lado de, y ώδή, oda) es una obra satírica que caracteriza o interpreta humorísticamente otra obra de arte, un autor o un tema, mediante la emulación o alusión irónica. Modernamente, la parodia no implica necesariamente la burla del texto parodiado. En el sentido de en contra del canto, la parodia se refiere a imitaciones burlonas de la forma de cantar o recitar, mientras en el real sentido de al lado del canto implica repetición con diferencia, sin necesariamente burla. La parodia existe en todos los géneros, incluyendo la literatura, la música , el cine y la televisión. Un acontecimiento político, social o cultural puede ser asimismo parodiado. La parodia es la recreación de un personaje o un hecho, empleando recursos irónicos para emitir una opinión generalmente transgresora sobre la persona o el acontecimiento parodiado."@es, "La parodie est une forme d'humour qui utilise le cadre, les personnages, le style et le fonctionnement d'une œuvre ou une institution pour s'en moquer. Elle se base entre autres sur l'inversion et l'exagération des caractéristiques appartenant au sujet parodié. Selon Dominique Maingueneau, la parodie constitue une « stratégie de réinvestissement d'un texte ou d'un genre de discours dans d'autres » : il s'agit d'une stratégie de « subversion », visant à disqualifier l'auteur du texte ou du genre source, tandis que la stratégie opposée (la « captation », imitation positive) permet de « transférer sur le discours réinvestisseur l'autorité attachée au texte ou au genre source »."@fr ;
    skos:inScheme cwrc:Genre ;
    prov:derivedFrom dbpedia:Parody .

cwrc:genrePastoral
    void:inDataset cwrc:datasetdefinition ;
    a cwrc:Genre, skos:Concept ;
    rdf:value "PASTORAL" ;
    rdfs:isDefinedBy <http://www.cwrc.ca/ontologies/cwrc#> ;
    rdfs:label ""@fr, "pastoral"@en ;
    skos:inScheme cwrc:Genre .

cwrc:genrePedagogy
    void:inDataset cwrc:datasetdefinition ;
    a cwrc:Genre, skos:Concept ;
    rdf:value "PEDAGOGY" ;
    rdfs:isDefinedBy <http://www.cwrc.ca/ontologies/cwrc#> ;
    rdfs:label ""@fr, "pedagogy"@en ;
    skos:inScheme cwrc:Genre .

cwrc:genrePerformancepoetry
    void:inDataset cwrc:datasetdefinition ;
    a cwrc:Genre, skos:Concept ;
    rdf:value "PERFORMANCEPOETRY" ;
    rdfs:isDefinedBy <http://www.cwrc.ca/ontologies/cwrc#> ;
    rdfs:label ""@fr, "performance poetry"@en ;
    owl:comment "This term and its description was created from data gathered from DBpedia."@en ;
    skos:broaderTransitive cwrc:genrePoetry ;
    skos:definition "La lecture performée ou lecture-performance est une lecture publique de textes poétiques ou littéraires effectuée le plus souvent par son auteur dans un esprit qui s'apparente à celui de la performance et qui peut convoquer tous les arts et techniques du théâtre et de la scène où la poésie et la littérature sont cependant toujours au premier plan. Christian Prigent, Serge Pey et Charles Pennequin en sont les premiers représentants. Édith Azam est aujourd'hui la conseillère lecture-performance au festival Voix de la Méditerranée de Lodève."@fr, "Performance poetry is poetry that is specifically composed for or during a performance before an audience. During the 1980s, the term came into popular usage to describe poetry written or composed for performance rather than print distribution."@en ;
    skos:inScheme cwrc:Genre ;
    prov:derivedFrom dbpedia:Performance_poetry .

cwrc:genrePeriodical
    void:inDataset cwrc:datasetdefinition ;
    a cwrc:Genre, skos:Concept ;
    rdf:value "PERIODICAL" ;
    rdfs:isDefinedBy <http://www.cwrc.ca/ontologies/cwrc#> ;
    rdfs:label ""@fr, "periodical"@en ;
    skos:inScheme cwrc:Genre .

cwrc:genrePetition
    void:inDataset cwrc:datasetdefinition ;
    a cwrc:Genre, skos:Concept ;
    rdf:value "PETITION" ;
    rdfs:isDefinedBy <http://www.cwrc.ca/ontologies/cwrc#> ;
    rdfs:label ""@fr, "petition"@en ;
    skos:inScheme cwrc:Genre .

cwrc:genrePhilosophical
    void:inDataset cwrc:datasetdefinition ;
    a cwrc:Genre, skos:Concept ;
    rdf:value "PHILOSOPHICAL" ;
    rdfs:isDefinedBy <http://www.cwrc.ca/ontologies/cwrc#> ;
    rdfs:label ""@fr, "philosophical"@en ;
    skos:inScheme cwrc:Genre .

cwrc:genrePhilosophy
    void:inDataset cwrc:datasetdefinition ;
    a cwrc:Genre, skos:Concept ;
    rdf:value "PHILOSOPHY" ;
    rdfs:isDefinedBy <http://www.cwrc.ca/ontologies/cwrc#> ;
    rdfs:label ""@fr, "philosophy"@en ;
    skos:inScheme cwrc:Genre .

cwrc:genrePicaresque
    void:inDataset cwrc:datasetdefinition ;
    a cwrc:Genre, skos:Concept ;
    rdf:value "PICARESQUE" ;
    rdfs:isDefinedBy <http://www.cwrc.ca/ontologies/cwrc#> ;
    rdfs:label ""@fr, "picaresque"@en ;
    owl:comment "This term and its description was created from data gathered from DBpedia."@en ;
    skos:definition "De schelmenroman is een literair genre dat in Spanje ontstond in de 16e en 17e eeuw. Schelmenromans worden ook picareske romans genoemd (naar het Spaanse picaro, dat schelm betekent). De schelmenroman is een subtype van de roman."@nl, "Der Schelmenroman oder pikarischer/pikaresker Roman (aus dem Spanischen: pícaro = Schelm) , dessen Ursprung im 16. Jahrhundert in Spanien liegt, schildert aus der Perspektive seines Helden, wie sich dieser in einer Reihe von Abenteuern durchs Leben schlägt. Der Schelm stammt aus den unteren gesellschaftlichen Schichten, ist deshalb ungebildet, aber „bauernschlau“. Er durchläuft alle gesellschaftlichen Schichten und wird zu deren Spiegel. Der Held hat keinen Einfluss auf die Geschehnisse um ihn herum, schafft es aber immer wieder, sich aus allen brenzligen Situationen zu retten. Traditionell ist der Schelmenroman eine (fingierte) Autobiographie. Sie beginnt oft mit einer Desillusionierung des Helden, der die Schlechtigkeit der Welt erst hier erkennt. Er begibt sich, sei es freiwillig, sei es unfreiwillig, auf Reisen. Die dabei erlebten Abenteuer sind episodenhaft, d. h. sie hängen nicht voneinander ab und können beliebig erweitert werden, was bei Übersetzungen oft der Fall war. Das Ende ist meist eine „Bekehrung“ des Schelms, nach der er zu einem geregelten Leben findet. Es besteht auch die Möglichkeit einer Flucht aus der Welt, also aus der Realität."@de, "Le roman picaresque (de l'espagnol pícaro, « misérable », « futé ») est un genre littéraire né en Espagne au XVIe siècle et qui a connu sa plus florissante époque dans ce pays. Un roman picaresque se compose d'un récit sur le mode autobiographique de l’histoire de héros miséreux, généralement des jeunes gens vivant en marge de la société et à ses dépens. Au cours d’aventures souvent extravagantes supposées plus pittoresques et surtout plus variées que celles des honnêtes gens, qui sont autant de prétextes à présenter des tableaux de la vie vulgaire et des scènes de mœurs, le héros entre en contact avec toutes les couches de la société."@fr, "Novela picaresca es un género literario narrativo en prosa muy característico de la literatura española, aunque trascendió a la europea en general. Surgió en los años de transición entre el Renacimiento y el Barroco, durante el llamado Siglo de Oro de las letras españolas."@es, "The picaresque novel (Spanish: \"picaresca,\" from \"pícaro,\" for \"rogue\" or \"rascal\") is a genre of prose fiction which depicts the adventures of a roguish hero of low social class who lives by his wits in a corrupt society. Picaresque novels typically adopt a realistic style, with elements of comedy and satire. This style of novel originated in 16th-century Spain and flourished throughout Europe in the 17th and 18th centuries. It continues to influence modern literature. According to the traditional view of Thrall and Hibbard (first published in 1936), seven qualities distinguish the picaresque novel or narrative form, all or some of which may be employed for effect by the author. (1) A picaresque narrative is usually written in first person as an autobiographical account. (2) The main character is often of low character or social class. He or she gets by with wit and rarely deigns to hold a job. (3) There is no plot. The story is told in a series of loosely connected adventures or episodes. (4) There is little if any character development in the main character. Once a picaro, always a picaro. His or her circumstances may change but they rarely result in a change of heart. (5) The picaro's story is told with a plainness of language or realism. (6) Satire might sometimes be a prominent element. (7) The behavior of a picaresque hero or heroine stops just short of criminality. Carefree or immoral rascality positions the picaresque hero as a sympathetic outsider, untouched by the false rules of society. However, Trall and Hibbert's thesis has been questioned by scholars[specify] interested in how genre functions, rather than how it looks on the surface."@en ;
    skos:inScheme cwrc:Genre ;
    prov:derivedFrom dbpedia:Picaresque_novel .

cwrc:genrePindaric
    void:inDataset cwrc:datasetdefinition ;
    a cwrc:Genre, skos:Concept ;
    rdf:value "PINDARIC" ;
    rdfs:isDefinedBy <http://www.cwrc.ca/ontologies/cwrc#> ;
    rdfs:label ""@fr, "pindaric"@en ;
    skos:inScheme cwrc:Genre .

cwrc:genrePoetry
    void:inDataset cwrc:datasetdefinition ;
    a cwrc:Genre, skos:Concept ;
    rdf:value "POETRY" ;
    rdfs:isDefinedBy <http://www.cwrc.ca/ontologies/cwrc#> ;
    rdfs:label "poetry"@en, "poésie"@fr ;
    owl:comment "This term and its description was created from data gathered from DBpedia."@en ;
    skos:definition "Das Wort Poesie (von gr. ποίησις poiesis, „Erschaffung“) bezeichnet erstens einen Textbereich, dessen Produktion traditionell nach den poetischen Gattungen geteilt wird. Nach Aristotelischer Poetik (so das Wort für die Theorie der Poesie) sind dies Drama, Epos und kleinere lyrische Gattungen. Im Deutschen wird seit dem 19. Jahrhundert eher von Literatur und literarischen Gattungen gesprochen. Allenfalls kurze Gedichte behielten das Wort, so etwa im Falle des Poesiealbums. Der Begriff bezeichnet im übertragenen Sinn ferner eine bestimmte Qualität. So spricht man etwa von der „Poesie eines Moments“ oder einem „poetischen Film“ und meint damit in der Regel, dass von dem Bezeichneten eine sich der Sprache entziehende, oder über sie hinausgehende Wirkung ausgeht, etwas Stilles, ähnlich wie von einem Gedicht, das eine sich der Alltagssprache entziehende Wirkung entfaltet."@de, "La poesía (del griego ποίησις 'acción, creación; adopción; fabricación; composición, poesía; poema' < ποιέω 'hacer, fabricar; engendrar, dar a luz; obtener; causar; crear') se define como un género literario considerado como una manifestación de la belleza o del sentimiento estético por medio de la palabra, en verso o en prosa. Los griegos entendían que podría haber tres tipos de poesía, la lírica o canción cantada con acompañamiento de lira o arpa de mano, que es el significado que luego se generalizó para la palabra, incluso sin música; la dramática o teatral y la épica o narrativa. Por eso se suele entender generalmente hoy como poesía la poesía lírica. También es encuadrable como una «modalidad textual» (esto es, como un tipo de texto). Es frecuente, en la actualidad, utilizar el término «poesía» como sinónimo de «poesía lírica» o de «lírica», aunque, desde un punto de vista histórico y cultural, esta es un subgénero o subtipo de la poesía."@es, "La poésie est un genre littéraire très ancien aux formes variées, écrites généralement en vers, mais qui admettent aussi la prose, et qui privilégient l'expressivité de la forme, les mots disant plus qu'eux-mêmes par leur choix (sens et sonorités) et leur agencement (rythmes, métrique, figures de style). Sa définition se révèle difficile et varie selon les époques, au point que chaque siècle a pu lui trouver une fonction et une expression différente, à quoi s'ajoute l'approche propre à la personnalité de chaque poète. Le terme « poésie » et ses dérivés viennent du grec ancien ποίησις, et s'écrivait, jusqu'en 1878 poësie (le tréma marquait une disjonction entre les voyelles o et e). ποιεῖν (poiein) signifie « faire, créer » : le poète est donc un créateur, un inventeur de formes expressives, ce que révèlent aussi les termes du Moyen Âge, comme trouvère et troubadour. Le poète, héritier d'une longue tradition orale, privilégie la musicalité et le rythme, d'où, dans la plupart des textes poétiques, le recours à une forme versifiée qui confère de la densité à la langue. Le poète recherche aussi l'expressivité par le poids accordé aux mots comme par l'utilisation des figures de style et au premier chef des images et des figures d'analogie, recherchées pour leur force suggestive. La poésie s'est constamment renouvelée au cours des siècles avec des orientations différentes selon les époques, les civilisations et les individus. On peut par exemple distinguer le poète artiste soucieux d'abord de beauté formelle, le poète « lyrique » qui cultive le « chant de l'âme », le poète prophète, découvreur du monde et « voyant » ou le poète engagé, sans cependant réduire un créateur à une étiquette simplificatrice."@fr, "Poetry is a form of literature that uses aesthetic and rhythmic qualities of language—such as phonaesthetics, sound symbolism, and metre—to evoke meanings in addition to, or in place of, the prosaic ostensible meaning."@en, "Poëzie of dichtkunst (van het Griekse 'poiesis'/ποίησις: maken, scheppen, vormen) is een vorm van literatuur die de esthetische en ritmische eigenschappen van taal zoals metrum en geluidssymboliek benut om betekenissen te genereren ter aanvulling, vervanging of ondermijning van de prozaïsche, ogenschijnlijke betekenis. Poëzie heeft een lange geschiedenis die teruggaat tot het Soemerische epos Gilgamesj. Vroege gedichten ontwikkelden zich uit volksliederen zoals de Chinese Sjijing, of uit de noodzaak om orale epiek steeds opnieuw te vertellen, zoals in de Veda's uit het Sanskriet, het Zoroastrische Gathas en de Homerische epossen Ilias en Odyssee. Antieke pogingen om poëzie te omschrijven, zoals de Poetica van Aristoteles, benadrukten het spraakgebruik in retorica, drama, lied en komedie. Latere pogingen concentreerden zich op kenmerken als herhaling, versvorm en rijm en benadrukten de esthetica die poëzie onderscheidt van meer objectief informatieve, prozaïsche vormen van schrift. Vanaf het midden der twintigste eeuw wordt de dichtkunst soms meer algemeen beschouwd als een wezenlijk creatieve handeling waarbij taal gebruikt wordt. In poëzie worden vormen en conventies gebruikt om een andere interpretatie van woorden te suggereren, of om een gevoelsmatige respons teweeg te brengen. Middelen zoals assonantie, alliteratie, onomatopeeën en ritme worden soms gebruikt om bezwerende of muzikale effecten te bereiken. Het gebruik van ambiguïteit, symboliek, ironie en andere stilistische elementen van de poëtische voordracht maken vaak een veelheid van interpretaties mogelijk. Op dezelfde wijze schept beeldspraak zoals metafoor, vergelijking (al dan niet Homerisch) en metonymie resonantie tussen anderszins ongelijksoortige beelden - een gelaagdheid van betekenissen waarbij niet eerder waargenomen connecties worden gevormd. Tussen individuele versregels kunnen verwante vormen van resonantie aanwezig zijn in hun patronen van rijm of ritme. De genoegens die de poëzie aan lezer of luisteraar verschaft, worden teweeggebracht door de bijzondere combinatie van vorm, klank en betekenis die eigen is aan het vers, en deze genoegens kunnen van emotionele (bijvoorbeeld ontroering of bezwering), intellectuele (bijvoorbeeld inzicht of nuancering) of humoristische aard zijn. Ontvankelijkheid voor poëzie of versgevoeligheid is mede afhankelijk van de mate waarin deze wordt gecultiveerd. Poëzie heeft een lange geschiedenis, vanaf de vroegste mondeling gereciteerde en gezongen verzen tot de hedendaagse schriftelijke, al dan niet gestructureerde vormen van dichtkunst."@nl ;
    skos:inScheme cwrc:Genre ;
    prov:derivedFrom dbpedia:Poetry .

cwrc:genrePolemic
    void:inDataset cwrc:datasetdefinition ;
    a cwrc:Genre, skos:Concept ;
    rdf:value "POLEMIC" ;
    rdfs:isDefinedBy <http://www.cwrc.ca/ontologies/cwrc#> ;
    rdfs:label ""@fr, "polemic"@en ;
    owl:comment "This term and its description was created from data gathered from DBpedia."@en, "This term and its description was created from data gathered from the Getty Art & Architecture Thesaurus."@en ;
    skos:definition "Aggressive, forcefully presented arguments, often disputing a policy or opinion."@en, "Agressieve, scherp geformuleerde twistgeschriften, waarin dikwijls een beleid of een mening wordt betwist."@nl, "Argumentos presentados en forma agresiva y enérgica, a menudo para discutir una política u opinión."@es, "Le terme de polémique (du grec πολεμικός, polêmikôs « qui concerne la guerre », « disposé à la guerre », polêmikon museion, musée de la guerre, « batailleur, querelleur ») désigne une discussion, un débat, une controverse qui traduit de façon violente ou passionnée, et le plus souvent par écrit, des opinions contraires sur toutes espèces de sujets (politique, scientifique, littéraire, religieux, etc.). Il fait aujourd'hui l'objet d'emplois multiples."@fr, "Scharfes und mit Nachdruck vorgebrachtes Argument, das häufig gegen eine bestimmte Politik oder Meinung gerichtet ist."@de ;
    skos:inScheme cwrc:Genre ;
    prov:derivedFrom dbpedia:Polemic, <http://vocab.getty.edu/aat/300252982> .

cwrc:genrePoliticalwriting
    void:inDataset cwrc:datasetdefinition ;
    a cwrc:Genre, skos:Concept ;
    rdf:value "POLITICALWRITING" ;
    rdfs:isDefinedBy <http://www.cwrc.ca/ontologies/cwrc#> ;
    rdfs:label ""@fr, "political writing"@en ;
    skos:inScheme cwrc:Genre .

cwrc:genrePopular
    void:inDataset cwrc:datasetdefinition ;
    a cwrc:Genre, skos:Concept ;
    rdf:value "POPULAR" ;
    rdfs:isDefinedBy <http://www.cwrc.ca/ontologies/cwrc#> ;
    rdfs:label ""@fr, "popular"@en ;
    skos:inScheme cwrc:Genre .

cwrc:genrePrayer
    void:inDataset cwrc:datasetdefinition ;
    a cwrc:Genre, skos:Concept ;
    rdf:value "PRAYER" ;
    rdfs:isDefinedBy <http://www.cwrc.ca/ontologies/cwrc#> ;
    rdfs:label ""@fr, "prayer"@en ;
    owl:comment "This term and its description was created from data gathered from the Getty Art & Architecture Thesaurus."@en ;
    skos:definition "Documents containing prayers that are associated with donning official priestly vestments or transfer of vestments, most commonly in Christian contexts."@en, "Gebed dat de priester uitspreekt bij het aantrekken van een liturgisch gewaad en bij de overhandiging van de liturgische gewaden bij de priesterwijding. Het gebed staat soms ingelijst in de sacristie, bijvoorbeeld op de credens."@nl ;
    skos:inScheme cwrc:Genre ;
    prov:derivedFrom <http://vocab.getty.edu/aat/300391080> .

cwrc:genrePrefatorypiece
    void:inDataset cwrc:datasetdefinition ;
    a cwrc:Genre, skos:Concept ;
    rdf:value "PREFATORYPIECE" ;
    rdfs:isDefinedBy <http://www.cwrc.ca/ontologies/cwrc#> ;
    rdfs:label "prefatory piece"@en, "préfixe"@fr ;
    skos:inScheme cwrc:Genre .

cwrc:genreProletarianwriting
    void:inDataset cwrc:datasetdefinition ;
    a cwrc:Genre, skos:Concept ;
    rdf:value "PROLETARIANWRITING" ;
    rdfs:isDefinedBy <http://www.cwrc.ca/ontologies/cwrc#> ;
    rdfs:label ""@fr, "proletarianwriting"@en ;
    skos:inScheme cwrc:Genre .

cwrc:genrePrologue
    void:inDataset cwrc:datasetdefinition ;
    a cwrc:Genre, skos:Concept ;
    rdf:value "PROLOGUE" ;
    rdfs:isDefinedBy <http://www.cwrc.ca/ontologies/cwrc#> ;
    rdfs:label ""@fr, "prologue"@en ;
    skos:inScheme cwrc:Genre .

cwrc:genrePropaganda
    void:inDataset cwrc:datasetdefinition ;
    a cwrc:Genre, skos:Concept ;
    rdf:value "PROPAGANDA" ;
    rdfs:isDefinedBy <http://www.cwrc.ca/ontologies/cwrc#> ;
    rdfs:label ""@fr, "propaganda"@en ;
    skos:inScheme cwrc:Genre .

cwrc:genreProphecy
    void:inDataset cwrc:datasetdefinition ;
    a cwrc:Genre, skos:Concept ;
    rdf:value "PROPHECY" ;
    rdfs:isDefinedBy <http://www.cwrc.ca/ontologies/cwrc#> ;
    rdfs:label ""@fr, "prophecy"@en ;
    owl:comment "This term and its description was created from data gathered from DBpedia."@en ;
    skos:definition "Als Prophezeiung – auch Weissagung oder Verheißung – bezeichnet man in religiösen Kontexten eine Prognose von Ereignissen in der Zukunft. Der Oberbegriff für gesammelte mündliche oder schriftliche Prophezeiungen, meist einer Einzelperson, ist Prophetie. Dieser Ausdruck stammt vom altgriechischen propheteía für „aussprechen“, „aussagen“ oder „für jemanden sprechen“ (altgriechisch φηµί phēmí „ich spreche“; pro „für, heraus, anstelle“). Prophezeiungen kommen in vielen Religionen in unterschiedlichsten Zusammenhängen, aus verschiedenen Anlässen und aufgrund verschiedener Empfangsweisen der prophezeiten Botschaft vor. Die altorientalischen Kulte kennen vielfältige Arten von Orakeln, regelmäßigen Befragungen an Opferstätten oder vor Schlachten, ekstatischen Ausnahmebotschaften, Traumvisionen, als Prophezeiung gedeuteten Medien wie Tierorganen, Vogelflug, Verzückung oder Audition usw. Die klassische Schriftprophetie im Judentum kennt solche Formen jedoch kaum. Hier bildet in der Regel eine Berufung eines Propheten durch den Gott Israels Ausgangspunkt von Wortbotschaften, die sich auf die Geschichte Gesamtisraels beziehen. Im Christentum werden Prophezeiungen seit der Jerusalemer Urgemeinde erwähnt. In der Folgezeit sind Prophezeiungen ein beliebtes Thema der Literatur geworden. In den Geschichtswissenschaften wird eine Prophezeiung auch als Vatizinium (Plural „Vatizinien“; von lateinisch vates „Weissager“, „Prophet“) bezeichnet. Insbesondere nennt man Prophezeiungen im Nachhinein Vaticinium ex eventu."@de, "Dans les religions abrahamiques, une consiste en des paroles ou des écrits divinement inspirés qu'une personne reçoit par révélation. Pour les chrétiens, le témoignage de Jésus est l'esprit de la prophétie (Apocalypse 19:10). Une prophétie peut avoir trait au passé, au présent ou à l'avenir. Quand une personne prophétise, elle dit ou écrit ce que Dieu veut qu'elle sache, pour son propre bien ou pour le bien des autres. La prophétie n'est pas l'apanage des prophètes. Une personne peut recevoir une prophétie ou une révélation pour sa vie personnelle."@fr, "Het woord profetie is afgeleid van het Griekse woord propheteía, dat uitspreken of voor iemand anders spreken betekent. In algemene zin wordt met 'profetie' gewoonlijk een voorspellende uitspraak over gebeurtenissen in de toekomst bedoeld."@nl, "Prophecy involves a process in which one or more messages allegedly communicated to a prophet are then communicated to other people. Such messages typically involve] inspiration, interpretation, or revelation of events to come (compare divine knowledge). Historically, clairvoyance has been used[by whom?] as an adjunct to prophecy."@en, "Una profecía (del latín prophetīa, y este del griego προφητεία, o quizá del griego φαινος, aparición) es, en la primera acepción del Diccionario de la lengua española de la Real Academia Española, un «don sobrenatural que consiste en conocer por inspiración divina las cosas distantes o futuras». Podría considerarse la existencia de diferencias entre los términos profecía y predicción. El Diccionario de la lengua española de la Real Academia Española no marca límites tan precisos en el sentido de la palabra predicción, al señalar que predecir significa «anunciar por revelación, ciencia o conjetura algo que ha de suceder». Por lo tanto, la predicción puede involucrar un don sobrenatural, un proceso lógico-racional, o un juicio más o menos subjetivo basado en indicios u observaciones. Por el contrario, la mayoría de las acepciones del citado diccionario referidas a la palabra profecía señalan que se trataría de un «don sobrenatural», es decir, que sería «inspirada por Dios». Así, se sitúa a las profecías mayormente en el ámbito de la fe, sin ligarlas necesariamente a un razonamiento en la previsión del resultado predicho. En grados diversos y formas variables, las religiones de la antigüedad hicieron referencia a hombres «inspirados» que afirmaban hablar en nombre de su dios.Pero en las grandes religiones monoteístas (judaísmo, cristianismo, islam), las manifestaciones extraordinarias nunca constituyen lo esencial en los profetas, que se distinguen claramente de otros exaltados o simuladores por tener simplemente carácter de mensajeros. Las profecías eran, pues, consideradas simples indicadores del designio de Dios. Hasta la fecha, más allá de las evidencias científicas que puedan o no resultar suficientes para unos u otros, muchos seguidores de estas grandes religiones históricas afirman que, en buena medida, las profecías de sus libros sagrados se han cumplido."@es ;
    skos:inScheme cwrc:Genre ;
    prov:derivedFrom dbpedia:Prophecy .

cwrc:genrePsalm
    void:inDataset cwrc:datasetdefinition ;
    a cwrc:Genre, skos:Concept ;
    rdf:value "PSALM" ;
    rdfs:isDefinedBy <http://www.cwrc.ca/ontologies/cwrc#> ;
    rdfs:label ""@fr, "psalm"@en ;
    skos:inScheme cwrc:Genre .

cwrc:genrePsychoanalytical
    void:inDataset cwrc:datasetdefinition ;
    a cwrc:Genre, skos:Concept ;
    rdf:value "PSYCHOANALYTICAL" ;
    rdfs:isDefinedBy <http://www.cwrc.ca/ontologies/cwrc#> ;
    rdfs:label ""@fr, "psychoanalytical"@en ;
    skos:inScheme cwrc:Genre .

cwrc:genreQuiz
    void:inDataset cwrc:datasetdefinition ;
    a cwrc:Genre, skos:Concept ;
    rdf:value "QUIZ" ;
    rdfs:isDefinedBy <http://www.cwrc.ca/ontologies/cwrc#> ;
    rdfs:label ""@fr, "quiz"@en ;
    skos:inScheme cwrc:Genre .

cwrc:genreRadiodrama
    void:inDataset cwrc:datasetdefinition ;
    a cwrc:Genre, skos:Concept ;
    rdf:value "RADIODRAMA" ;
    rdfs:isDefinedBy <http://www.cwrc.ca/ontologies/cwrc#> ;
    rdfs:label ""@fr, "radio drama"@en ;
    skos:inScheme cwrc:Genre .

cwrc:genreRealist
    void:inDataset cwrc:datasetdefinition ;
    a cwrc:Genre, skos:Concept ;
    rdf:value "REALIST" ;
    rdfs:isDefinedBy <http://www.cwrc.ca/ontologies/cwrc#> ;
    rdfs:label ""@fr, "realist"@en ;
    skos:inScheme cwrc:Genre .

cwrc:genreRegional
    void:inDataset cwrc:datasetdefinition ;
    a cwrc:Genre, skos:Concept ;
    rdf:value "REGIONAL" ;
    rdfs:isDefinedBy <http://www.cwrc.ca/ontologies/cwrc#> ;
    rdfs:label ""@fr, "regional"@en ;
    skos:inScheme cwrc:Genre .

cwrc:genreReligious
    void:inDataset cwrc:datasetdefinition ;
    a cwrc:Genre, skos:Concept ;
    rdf:value "RELIGIOUS" ;
    rdfs:isDefinedBy <http://www.cwrc.ca/ontologies/cwrc#> ;
    rdfs:label "religieux"@fr, "religious"@en ;
    skos:inScheme cwrc:Genre .

cwrc:genreReview
    void:inDataset cwrc:datasetdefinition ;
    a cwrc:Genre, skos:Concept ;
    rdf:value "REVIEW" ;
    rdfs:isDefinedBy <http://www.cwrc.ca/ontologies/cwrc#> ;
    rdfs:label ""@fr, "review"@en ;
    skos:inScheme cwrc:Genre .

cwrc:genreRevue
    void:inDataset cwrc:datasetdefinition ;
    a cwrc:Genre, skos:Concept ;
    rdf:value "REVUE" ;
    rdfs:isDefinedBy <http://www.cwrc.ca/ontologies/cwrc#> ;
    rdfs:label ""@fr, "revue"@en ;
    skos:inScheme cwrc:Genre .

cwrc:genreRiddle
    void:inDataset cwrc:datasetdefinition ;
    a cwrc:Genre, skos:Concept ;
    rdf:value "RIDDLE" ;
    rdfs:isDefinedBy <http://www.cwrc.ca/ontologies/cwrc#> ;
    rdfs:label "riddle"@en, "énigme"@fr ;
    skos:inScheme cwrc:Genre .

cwrc:genreRomance
    void:inDataset cwrc:datasetdefinition ;
    a cwrc:Genre, skos:Concept ;
    rdf:value "ROMANCE" ;
    rdfs:isDefinedBy <http://www.cwrc.ca/ontologies/cwrc#> ;
    rdfs:label ""@fr, "romance"@en ;
    owl:comment "This term and its description was created from data gathered from the Getty Art & Architecture Thesaurus."@en ;
    skos:definition "Narraciones en verso o prosa que relatan sucesos heroicos, fantásticos o sobrenaturales que a menudo transcurren en tiempos medievales."@es, "Poetic or prosaic literary forms derived from medieval narratives of love, legendary or heroic adventures, and chivalry. Extends to narratives about important religious figures, or fantastic or supernatural events."@en, "Vertellingen in proza of versvorm, zich vaak afspelend in de middeleeuwen, waarin grootse, fantastische of bovennatuurlijke gebeurtenissen worden beschreven."@nl, "描述英雄事蹟、幻想，或超自然事件的詩文或散文體記敘文，常設定於中世紀時期。"@zh-hant ;
    skos:inScheme cwrc:Genre ;
    prov:derivedFrom <http://vocab.getty.edu/aat/300191065> .

cwrc:genreSagewriting
    void:inDataset cwrc:datasetdefinition ;
    a cwrc:Genre, skos:Concept ;
    rdf:value "SAGEWRITING" ;
    rdfs:isDefinedBy <http://www.cwrc.ca/ontologies/cwrc#> ;
    rdfs:label ""@fr, "sage writing"@en ;
    owl:comment "This term and its description was created from data gathered from DBpedia."@en ;
    skos:definition "Sage writing was a genre of creative nonfiction popular in the Victorian era. The concept originates with John Holloway's 1953 book The Victorian Sage: Studies in Argument. Sage writing is a development from ancient wisdom literature in which the writer chastises and instructs the reader about contemporary social issues, often utilizing discourses of philosophy, history, politics, and economics in non-technical ways. Prominent examples of the genre include writings by Thomas Carlyle, Matthew Arnold, John Ruskin, and Henry David Thoreau. Some 20th-century writers, such as Joan Didion and New Journalists such as Norman Mailer and Tom Wolfe, have also been identified as sage writers."@en ;
    skos:inScheme cwrc:Genre ;
    prov:derivedFrom dbpedia:Sage_writing .

cwrc:genreSatire
    void:inDataset cwrc:datasetdefinition ;
    a cwrc:Genre, skos:Concept ;
    rdf:value "SATIRE" ;
    rdfs:isDefinedBy <http://www.cwrc.ca/ontologies/cwrc#> ;
    rdfs:label "satire"@en, "satire"@fr ;
    owl:comment "This term and its description was created from data gathered from DBpedia."@en, "This term and its description was created from data gathered from the Getty Art & Architecture Thesaurus."@en ;
    skos:definition "Composiciones literarias en verso o prosa en las cuales la locura y los vicios humanos son presentados con desprecio, escarnio o burla."@es, "Literaire werken in versvorm of proza waarin menselijke dwaasheden en ondeugden op spottende wijze aan de kaak worden gesteld."@nl, "Literary compositions in verse or prose, or ideas expressed as the subjects of art works, in which human folly and vice are held up to scorn, derision, or ridicule."@en, "Une satire est une œuvre dont l'objectif est une critique moqueuse de son sujet (des individus, des organisations, des États, etc.), souvent dans l'intention de provoquer, prévenir un changement ou de porter à réfléchir. On attribue généralement la paternité de ce genre littéraire (satura, c'est-à-dire pot-pourri) au poète archaïque latin Lucilius."@fr, "Werk der Literatur in Versen oder in Prosa, oder eine in einem Kunstwerk ausgedrückte Idee, in denen menschliche Torheit oder Laster lächerlich gemacht oder mit Hohn und Spott überzogen werden."@de, "指用韻文或散文創作之文學作品，作品凸顯人類的愚蠢與惡習，而加以奚落、嘲弄、或揶揄。"@zh-hant ;
    skos:inScheme cwrc:Genre ;
    prov:derivedFrom dbpedia:Satire, <http://vocab.getty.edu/aat/300251297> .

cwrc:genreScholarship
    void:inDataset cwrc:datasetdefinition ;
    a cwrc:Genre, skos:Concept ;
    rdf:value "SCHOLARSHIP" ;
    rdfs:isDefinedBy <http://www.cwrc.ca/ontologies/cwrc#> ;
    rdfs:label ""@fr, "scholarship"@en ;
    skos:inScheme cwrc:Genre .

cwrc:genreSchoolfiction
    void:inDataset cwrc:datasetdefinition ;
    a cwrc:Genre, skos:Concept ;
    rdf:value "SCHOOLFICTION" ;
    rdfs:isDefinedBy <http://www.cwrc.ca/ontologies/cwrc#> ;
    rdfs:label ""@fr, "school fiction"@en ;
    skos:inScheme cwrc:Genre .

cwrc:genreSciencefiction
    void:inDataset cwrc:datasetdefinition ;
    a cwrc:Genre, skos:Concept ;
    rdf:value "SCIENCEFICTION" ;
    rdfs:isDefinedBy <http://www.cwrc.ca/ontologies/cwrc#> ;
    rdfs:label ""@fr, "science fiction"@en ;
    owl:comment "This term and its description was created from data gathered from DBpedia."@en ;
    skos:definition "Ciencia ficción es la denominación popular con que se conoce a uno de los géneros derivados de la literatura de ficción, junto con la literatura fantástica y la narrativa de terror. Nacida como subgénero literario distinguido en la década de 1920 (aunque hay obras reconocibles muy anteriores) y exportada posteriormente a otros medios, como el cinematográfico, historietístico y televisivo, gozó de un gran auge en la segunda mitad del sigloxx debido al interés popular acerca del futuro que despertó el espectacular avance tanto científico como tecnológico alcanzado durante todos estos años. Es un género especulativo que relata acontecimientos posibles desarrollados en un marco puramente imaginario, cuya verosimilitud se fundamenta narrativamente en los campos de las ciencias físicas, naturales y sociales. La acción puede girar en torno a un abanico grande de posibilidades (viajes interestelares, conquista del espacio, consecuencias de una hecatombe terrestre o cósmica, evolución humana a causa de mutaciones, evolución de los robots, realidad virtual, existencia de civilizaciones alienígenas, etc.). Esta acción puede tener lugar en un tiempo pasado, presente o futuro, o, incluso, en tiempos alternativos ajenos a la realidad conocida, y tener por escenario espacios físicos (reales o imaginarios, terrestres o extraterrestres) o el espacio interno de la mente. Los personajes son igualmente diversos: a partir del patrón natural humano, recorre y explota modelos antropomórficos hasta desembocar en la creación de entidades artificiales de forma humana (robot, androide, cíborg) o en criaturas no antropomórficas"@es, "La science-fiction est un genre narratif, principalement un genre littéraire et un genre cinématographique. Il est structuré par des hypothèses sur ce que pourrait être le futur ou ce qu'aurait pu être le présent voire le passé (planètes éloignées, mondes parallèles, uchronie...), en partant des connaissances actuelles (scientifiques, technologiques, ethnologiques...). Elle se distingue du fantastique qui inclut une dimension inexplicable et de la fantasy qui fait souvent intervenir la magie."@fr, "Science fiction is a genre of speculative fiction dealing with imaginative concepts such as futuristic settings, futuristic science and technology, space travel, time travel, faster than light travel, parallel universes and extraterrestrial life. Science fiction often explores the potential consequences of scientific and other innovations, and has been called a \"literature of ideas.\" It usually eschews the supernatural, and unlike the related genre of fantasy, historically science fiction stories were intended to have at least a faint grounding in science-based fact or theory at the time the story was created, but this connection has become tenuous or non-existent in much of science fiction."@en, "Science-Fiction [ˌsaɪəns ˈfɪkʃən̩] (engl. science „Wissenschaft“, fiction „Fiktion“) ist ein Genre der Literatur und des Films, aber auch anderer Bereiche wie etwa der bildenden Kunst oder der Videospiele, das den Einzelnen, die Gesellschaft oder die Umwelt in (oft radikal) alternativen Konstellationen betrachtet. Science-Fiction entwirft – häufig in die Zukunft verlegte, teilweise auch räumlich entfernte – Konstellationen des Möglichen und beschreibt deren Auswirkungen. Dabei werden reale wissenschaftliche und technische Möglichkeiten mit fiktionalen Spekulationen angereichert."@de, "Sciencefiction (afgekort sf, scifi of essef, in het Engels als science fiction gespeld), is tegenwoordig een belangrijk genre dat vooral opgeld heeft gedaan in literatuur, stripverhalen, films, televisieseries, hoorspelen en computerspellen. Het Engelse \"science fiction\" betekent letterlijk vertaald \"wetenschapsfictie\", en dit is dan ook de betekenis die de bedenker van de term, Hugo Gernsback, eraan heeft willen geven. Voor Gernsback was de sciencefiction vooral bedoeld als een middel tot popularisatie van de wetenschap en van wetenschappelijke ontdekkingen, maar de geschiedenis ervan laat zien dat deze gedachte door latere schrijvers slechts beperkt is nagestreefd. In het genre worden tegenwoordig vooral toekomstbeelden met verzonnen technologische vooruitgang en wetenschappelijke ontwikkelingen gebruikt."@nl ;
    skos:inScheme cwrc:Genre ;
    prov:derivedFrom dbpedia:Science_fiction .

cwrc:genreScientificwriting
    void:inDataset cwrc:datasetdefinition ;
    a cwrc:Genre, skos:Concept ;
    rdf:value "SCIENTIFICWRITING" ;
    rdfs:isDefinedBy <http://www.cwrc.ca/ontologies/cwrc#> ;
    rdfs:label ""@fr, "scientific writing"@en ;
    skos:inScheme cwrc:Genre .

cwrc:genreScrapbook
    void:inDataset cwrc:datasetdefinition ;
    a cwrc:Genre, skos:Concept ;
    rdf:value "SCRAPBOOK" ;
    rdfs:isDefinedBy <http://www.cwrc.ca/ontologies/cwrc#> ;
    rdfs:label ""@fr, "scrapbook"@en ;
    skos:inScheme cwrc:Genre .

cwrc:genreSensationnovel
    void:inDataset cwrc:datasetdefinition ;
    a cwrc:Genre, skos:Concept ;
    rdf:value "SENSATIONNOVEL" ;
    rdfs:isDefinedBy <http://www.cwrc.ca/ontologies/cwrc#> ;
    rdfs:label ""@fr, "sensation novel"@en ;
    owl:comment "This term and its description was created from data gathered from DBpedia."@en ;
    skos:broaderTransitive cwrc:genreNovel ;
    skos:definition "Le roman à sensation est un genre littéraire né dans la deuxième moitié du XIXe siècle en Grande-Bretagne. Ce genre littéraire est une évolution des romans mélodramatiques, qui utilisaient un ensemble de personnages stéréotypés, et des romans Newgate, qui avaient pour thème principal la vie de célèbres criminels. East Lynne de Ellen Wood's, paru en 1861, fut le premier roman à être étiqueté comme roman à sensation par la critique. Le courant comprend trois auteurs majeurs : Ellen Woods, Wilkie Collins (La Femme en blanc, 1859; La Pierre de lune, 1868) et Mary Elizabeth Braddon (Le secret de Lady Audley, 1862). Les romans à sensation avaient pour thèmes des sujets choquants comme l'adultère, le vol, l'enlèvement, la bigamie, la fabrication de fausse monnaie, la séduction et le meurtre. Le genre se distinguait des autres mouvements de l'époque, comme le mouvement Gothique, par l'utilisation de ces thèmes dans un contexte domestique, voire familial, allant ainsi à l'encontre de l'idée largement répandue à l'époque victorienne que les événements sensationnels étaient totalement étrangers à la vie confortable des classes moyennes qui composaient la plus grande partie du lectorat de l'époque. William S. Gilbert fit une satire du genre en 1871 avec son opéra comique A Sensation Novel."@fr, "The sensation novel was a literary genre of fiction popular in Great Britain in the 1860s and 1870s, following on from earlier melodramatic novels and the Newgate novels, which focused on tales woven around criminal biographies. It also drew on the gothic and romantic genres of fiction. The sensation novel's appearance notably follows the Industrial Revolution, which made books available on a mass scale for people of all social standings and increased the sensation novel's popularity. Sensation novels used both modes of romance and realism to the extreme where in the past they had traditionally been contradictory modes of literature. The sensation novelists commonly wrote stories that were allegorical and abstract; the abstract nature of the stories gave the authors room to explore scenarios that wrestled with the social anxieties of the Victorian Era. The loss of identity is seen in many sensation fiction stories because this was a common social anxiety; in Britain, there was an increased use in record keeping and therefore people questioned the meaning and permanence of identity. The social anxiety regarding identity is reflected in stories, such as, The Woman in White and Lady Audley's Secret. The genre of sensation fiction was established by the publications of the following novels The Woman in White by Wilkie Collins in 1859; East Lynne by Ellen Wood in 1861; Lady Audley's Secret by Mary Elizabeth Braddon in 1862. Perhaps the earliest use of the term, sensation fiction, as a name for such novels appears in the 1861 edition of the Saunders, Otley, & co.'s Literary Budget. The neo-Victorian novel of New Zealand author Eleanor Catton, The Luminaries, which won the 2013 Man Booker Prize, has been described as being heavily based on sensation literature, with its plot devices of \"suspect wills and forged documents, secret marriages, illegitimacy and opium\""@en ;
    skos:inScheme cwrc:Genre ;
    prov:derivedFrom dbpedia:Sensation_novel .

cwrc:genreSentimental
    void:inDataset cwrc:datasetdefinition ;
    a cwrc:Genre, skos:Concept ;
    rdf:value "SENTIMENTAL" ;
    rdfs:isDefinedBy <http://www.cwrc.ca/ontologies/cwrc#> ;
    rdfs:label ""@fr, "sentimental"@en ;
    owl:comment "This term and its description was created from data gathered from DBpedia."@en ;
    skos:definition "La novela sentimental es un subgénero literario histórico que se desarrolla entre el Prerrenacimiento del siglo XV y el Renacimiento de la primera mitad del siglo XVI. Se incluye dentro del género épico o narrativo y se compone en prosa con versos intercalados, a veces en forma epistolar; posee temática amorosa, frecuentemente dentro de las leyes del llamado amor cortés."@es, "The sentimental novel or the novel of sensibility is an 18th-century literary genre which celebrates the emotional and intellectual concepts of sentiment, sentimentalism, and sensibility. Sentimentalism, which is to be distinguished from sensibility, was a fashion in both poetry and prose fiction beginning in the eighteenth century in reaction to the rationalism of the Augustan Age. Sentimental novels relied on emotional response, both from their readers and characters. They feature scenes of distress and tenderness, and the plot is arranged to advance both emotions and actions. The result is a valorization of \"fine feeling,\" displaying the characters as a model for refined, sensitive emotional effect. The ability to display feelings was thought to show character and experience, and to shape social life and relations."@en ;
    skos:inScheme cwrc:Genre ;
    prov:derivedFrom dbpedia:Sentimental_novel .

cwrc:genreSequel
    void:inDataset cwrc:datasetdefinition ;
    a cwrc:Genre, skos:Concept ;
    rdf:value "SEQUEL" ;
    rdfs:isDefinedBy <http://www.cwrc.ca/ontologies/cwrc#> ;
    rdfs:label ""@fr, "sequel"@en ;
    skos:inScheme cwrc:Genre .

cwrc:genreSermon
    void:inDataset cwrc:datasetdefinition ;
    a cwrc:Genre, skos:Concept ;
    rdf:value "SERMON" ;
    rdfs:isDefinedBy <http://www.cwrc.ca/ontologies/cwrc#> ;
    rdfs:label ""@fr, "sermon"@en ;
    owl:comment "This term and its description was created from data gathered from DBpedia."@en ;
    skos:definition "A sermon is an oration, lecture, or talk by a member of a religious institution or clergy. Sermons address a Biblical, theological, religious, or moral topic, usually expounding on a type of belief, law or behavior within both past and present contexts. Elements of the sermon often include exposition, exhortation and practical application. In Christianity, a sermon (also known as a homily within some churches) is usually delivered in a place of worship from an elevated architectural feature, variously known as a pulpit, a lectern, or an ambo. The word \"sermon\" comes from a Middle English word which was derived from Old French, which in turn came from the Latin word sermō meaning \"discourse\". The word can mean \"conversation\", which could mean that early sermons were delivered in the form of question and answer, and that only later did it come to mean a monologue. However, the Bible contains many speeches without interlocution, which some take to be sermons: Moses in Deuteronomy 1-33 ; Jesus' sermon on the mount in Matthew 5-7 (though the gospel writers do not specifically call it a sermon; the popular descriptor for Christ's speech there came much later); Peter after Pentecost in Acts 2:14-40 (though this speech was delivered to nonbelievers and as such is not quite parallel to the popular definition of a sermon). In modern language, the word \"sermon\" is used in secular terms, pejoratively, to describe a lengthy or tedious speech delivered with great passion, by any person, to an uninterested audience. A sermonette is a short sermon (usually associated with television broadcasting, as stations would present a sermonette before signing off for the night)."@en, "De preek of prediking is een belangrijk onderdeel van de eredienst in verschillende godsdiensten. De leer van het doordenken, maken en geven van een preek of homilie heet homiletiek."@nl, "Le sermon est un discours de prédication prononcé dans des circonstances religieuses."@fr, "Predigt (lat. praedicatio), auf Englisch und Französisch sermon (von lat. sermo ‚Wechselrede, Gespräch; Vortrag) ist eine Rede mit religiösem Inhalt oder eine Rede im Kontext einer religiösen Feier. Die Predigt hat einen besonderen Stellenwert im Neuen Testament und im christlichen Gottesdienst. In der christlichen Theologie wird die Lehre von der Predigt als Homiletik bezeichnet."@de, "Se denomina sermón u homilía al género de la oratoria que consiste en un discurso de tema religioso, por lo general pronunciado durante el culto cristiano. El sermón se pronunciaba, en la primera liturgia cristiana, en latín, pero después, en vista de que el pueblo ya no entendía el latín culto, empezó a pronunciarse en lengua vernácula, mientras que el resto de la liturgia continuaba pronunciándose en latín. Algunos autores piensan que ese fue el origen de cierto transvase de voces, proverbios y cuentecillos cultos a la lengua vulgar, dando origen a buena parte de la literatura folclórica. El sermón podría ser dogmático, místico, ascético o parenético. Era dogmático si trataba de dogmas; los que explicaban los misterios, eran los sermones místicos; los que trataban sobre las prácticas religiosas, se denominaban ascéticos y los que versaban sobre cuestiones morales, parenéticos. Estos últimos se subdividían a su vez en homilías, pláticas y sermones propiamente dichos. También existe el fervorín (antes de comulgar), la oración fúnebre (glosando las virtudes de un difunto) y el panegírico (en honor de un santo)."@es ;
    skos:inScheme cwrc:Genre ;
    prov:derivedFrom dbpedia:Sermon .

cwrc:genreSexualawakeningfiction
    void:inDataset cwrc:datasetdefinition ;
    a cwrc:Genre, skos:Concept ;
    rdf:value "SEXUALAWAKENINGFICTION" ;
    rdfs:isDefinedBy <http://www.cwrc.ca/ontologies/cwrc#> ;
    rdfs:label ""@fr, "sexual awakening fiction"@en ;
    skos:inScheme cwrc:Genre .

cwrc:genreShortstory
    void:inDataset cwrc:datasetdefinition ;
    a cwrc:Genre, skos:Concept ;
    rdf:value "SHORTSTORY" ;
    rdfs:isDefinedBy <http://www.cwrc.ca/ontologies/cwrc#> ;
    rdfs:label "nouvelle"@fr, "short story"@en ;
    owl:comment "This term and its description was created from data gathered from DBpedia."@en, "This term and its description was created from data gathered from the Getty Art & Architecture Thesaurus."@en ;
    skos:definition "Betrekkelijk korte, verzonnen prozavertellingen."@nl, "Narraciones ficticias en prosa, relativamente breves."@es, "Relatively brief invented prose narratives."@en, "Verhältnismäßig kurze fiktionale Prosaerzählung."@de, "篇幅相對較短的虛構性散文體記敘文。"@zh-hant ;
    skos:inScheme cwrc:Genre ;
    prov:derivedFrom dbpedia:Short_story_cycle, <http://vocab.getty.edu/aat/300202607> .

cwrc:genreSilverforknovel
    void:inDataset cwrc:datasetdefinition ;
    a cwrc:Genre, skos:Concept ;
    rdf:value "SILVERFORKNOVEL" ;
    rdfs:isDefinedBy <http://www.cwrc.ca/ontologies/cwrc#> ;
    rdfs:label ""@fr, "silverfork novel"@en ;
    skos:broaderTransitive cwrc:genreNovel ;
    skos:inScheme cwrc:Genre .

cwrc:genreSketch
    void:inDataset cwrc:datasetdefinition ;
    a cwrc:Genre, skos:Concept ;
    rdf:value "SKETCH" ;
    rdfs:isDefinedBy <http://www.cwrc.ca/ontologies/cwrc#> ;
    rdfs:label ""@fr, "sketch"@en ;
    owl:comment "This term and its description was created from data gathered from the Getty Art & Architecture Thesaurus."@en ;
    skos:definition "Breves composiciones literarias sobre temas específicos, a menudo presentando el punto de vista personal del autor."@es, "Korte literaire verhandelingen over één onderwerp, waarin de auteur dikwijls een persoonlijk standpunt verwoordt."@nl, "Kurzer literarischer Aufsatz über ein Einzelthema, gibt häufig die persönliche Meinung des Autors wieder."@de, "Short literary compositions on single subjects, often presenting the personal view of the author."@en, "單一主題的簡短文學作品，常表述作者之個人觀點。"@zh-hant ;
    skos:inScheme cwrc:Genre ;
    prov:derivedFrom <http://vocab.getty.edu/aat/300026291> .

cwrc:genreSketchbook
    void:inDataset cwrc:datasetdefinition ;
    a cwrc:Genre, skos:Concept ;
    rdf:value "SKETCHBOOK" ;
    rdfs:isDefinedBy <http://www.cwrc.ca/ontologies/cwrc#> ;
    rdfs:label ""@fr, "sketch book"@en ;
    skos:inScheme cwrc:Genre .

cwrc:genreSlavenarrative
    void:inDataset cwrc:datasetdefinition ;
    a cwrc:Genre, skos:Concept ;
    rdf:value "SLAVENARRATIVE" ;
    rdfs:isDefinedBy <http://www.cwrc.ca/ontologies/cwrc#> ;
    rdfs:label ""@fr, "slave narrative"@en ;
    skos:inScheme cwrc:Genre .

cwrc:genreSocialscience
    void:inDataset cwrc:datasetdefinition ;
    a cwrc:Genre, skos:Concept ;
    rdf:value "SOCIALSCIENCE" ;
    rdfs:isDefinedBy <http://www.cwrc.ca/ontologies/cwrc#> ;
    rdfs:label ""@fr, "social science"@en ;
    skos:inScheme cwrc:Genre .

cwrc:genreSong
    void:inDataset cwrc:datasetdefinition ;
    a cwrc:Genre, skos:Concept ;
    rdf:value "SONG" ;
    rdfs:isDefinedBy <http://www.cwrc.ca/ontologies/cwrc#> ;
    rdfs:label ""@fr, "song"@en ;
    skos:inScheme cwrc:Genre .

cwrc:genreSonnet
    void:inDataset cwrc:datasetdefinition ;
    a cwrc:Genre, skos:Concept ;
    rdf:value "SONNET" ;
    rdfs:isDefinedBy <http://www.cwrc.ca/ontologies/cwrc#> ;
    rdfs:label ""@fr, "sonnet"@en ;
    owl:comment "This term and its description was created from data gathered from the Getty Art & Architecture Thesaurus."@en ;
    skos:definition "Gedicht van veertien regels met tien lettergrepen, vaak met een rijmschema. Men denkt dat het sonnet oorspronkelijk uit Italië komt. De eerste sonnetten verschenen in de dertiende eeuw op Sicilië. Daarna verspreidden ze zich naar Toscane, waar Petrarca de vorm perfectioneerde in zijn Canzioniere, een serie van 317 sonnetten voor zijn geïdealiseerde geliefde Laura. Het petrarkische sonnet is historisch gezien het meest gebruikte sonnet, hoewel het shakespearesonnet (drie kwatrijnen en twee slotregels met gepaard rijm) ook veel voorkomt."@nl, "Gedicht, das aus 14 zehnsilbigen Verszeilen besteht, häufig mit Reimschema. Die Sonettform stammt vermutlich aus Italien, wo sie im 13. Jahrhundert in Sizilien aufkam und sich dann bis in die Toskana ausbreitete, wo Petrarca sie mit seinem Canzoniere perfektionierte, einer Sammlung aus 317 Sonetten, die an Laura, seine idealisierte Geliebte, gerichtet sind. Das petrarkische Sonett ist die historisch am weitesten verbreitete Form, obwohl die elisabethanische Form (3 Quartette mit einem Paarreim am Schluss) ebenfalls häufig anzutreffen ist."@de, "Poems consisting of 14 decasyllabic lines, often in a rhyming scheme. The sonnet form is considered to be of Italian origin, appearing in the 13th century in Sicily, after which it spread to Tuscany, where Petrarch perfected the form with his Canzioniere, a series of 317 sonnets to his idealized love, Laura. The Petrarchian sonnet has historically been the most widely used of the form, although the Elizabethan form (3 quatrains, with a final rhyming couplet) is also common."@en, "由十四行十音節詩行所組成的詩，常押韻。十四行詩形式被認為源於義大利，13世紀於西西里島出現，爾後傳播至多斯加尼(或譯托斯卡尼)，佩脫拉克在此完成Canzioniere集，一系列共317首十四行詩，獻給其理想愛人蘿拉，將此一形式臻於完美。史上該形式最廣為使用佩脫拉克式十四行詩，但伊莉莎白式十四行詩（3段四行詩，加上最後押韻的對句）也很常見。"@zh-hant ;
    skos:inScheme cwrc:Genre ;
    prov:derivedFrom <http://vocab.getty.edu/aat/300266382> .

cwrc:genreSpeech
    void:inDataset cwrc:datasetdefinition ;
    a cwrc:Genre, skos:Concept ;
    rdf:value "SPEECH" ;
    rdfs:isDefinedBy <http://www.cwrc.ca/ontologies/cwrc#> ;
    rdfs:label ""@fr, "speech"@en ;
    skos:inScheme cwrc:Genre .

cwrc:genreTestimony
    void:inDataset cwrc:datasetdefinition ;
    a cwrc:Genre, skos:Concept ;
    rdf:value "TESTIMONY" ;
    rdfs:isDefinedBy <http://www.cwrc.ca/ontologies/cwrc#> ;
    rdfs:label ""@fr, "testimony"@en ;
    skos:inScheme cwrc:Genre .

cwrc:genreTextbook
    void:inDataset cwrc:datasetdefinition ;
    a cwrc:Genre, skos:Concept ;
    rdf:value "TEXTBOOK" ;
    rdfs:isDefinedBy <http://www.cwrc.ca/ontologies/cwrc#> ;
    rdfs:label ""@fr, "textbook"@en ;
    skos:inScheme cwrc:Genre .

cwrc:genreTheatreofcruelty
    void:inDataset cwrc:datasetdefinition ;
    a cwrc:Genre, skos:Concept ;
    rdf:value "THEATREOFCRUELTY" ;
    rdfs:isDefinedBy <http://www.cwrc.ca/ontologies/cwrc#> ;
    rdfs:label ""@fr, "theatre of cruelty"@en ;
    skos:inScheme cwrc:Genre .

cwrc:genreTheatreoftheabsurd
    void:inDataset cwrc:datasetdefinition ;
    a cwrc:Genre, skos:Concept ;
    rdf:value "THEATREOFTHEABSURD" ;
    rdfs:isDefinedBy <http://www.cwrc.ca/ontologies/cwrc#> ;
    rdfs:label ""@fr, "theatre of the absurd"@en ;
    skos:inScheme cwrc:Genre .

cwrc:genreTheology
    void:inDataset cwrc:datasetdefinition ;
    a cwrc:Genre, skos:Concept ;
    rdf:value "THEOLOGY" ;
    rdfs:isDefinedBy <http://www.cwrc.ca/ontologies/cwrc#> ;
    rdfs:label ""@fr, "theology"@en ;
    skos:inScheme cwrc:Genre .

cwrc:genreThesaurus
    void:inDataset cwrc:datasetdefinition ;
    a cwrc:Genre, skos:Concept ;
    rdf:value "THESAURUS" ;
    rdfs:isDefinedBy <http://www.cwrc.ca/ontologies/cwrc#> ;
    rdfs:label ""@fr, "thesaurus"@en ;
    skos:inScheme cwrc:Genre .

cwrc:genreThriller
    void:inDataset cwrc:datasetdefinition ;
    a cwrc:Genre, skos:Concept ;
    rdf:value "THRILLER" ;
    rdfs:isDefinedBy <http://www.cwrc.ca/ontologies/cwrc#> ;
    rdfs:label ""@fr, "thriller"@en ;
    skos:inScheme cwrc:Genre .

cwrc:genreTopographicalpoetry
    void:inDataset cwrc:datasetdefinition ;
    a cwrc:Genre, skos:Concept ;
    rdf:value "TOPOGRAPHICALPOETRY" ;
    rdfs:isDefinedBy <http://www.cwrc.ca/ontologies/cwrc#> ;
    rdfs:label ""@fr, "topographical poetry"@en ;
    owl:comment "This term and its description was created from data gathered from DBpedia."@en ;
    skos:broaderTransitive cwrc:genrePoetry ;
    skos:definition "Topographical poetry or loco-descriptive poetry is a genre of poetry that describes, and often praises, a landscape or place. John Denham's 1642 poem \"Cooper's Hill\" established the genre, which peaked in popularity in 18th-century England. Examples of topographical verse date, however, to the late classical period, and can be found throughout the medieval era and during the Renaissance. Though the earliest examples come mostly from continental Europe, the topographical poetry in the tradition originating with Denham concerns itself with the classics, and many of the various types of topographical verse, such as river, ruin, or hilltop poems were established by the early 17th century. Alexander Pope's \"Windsor Forest\" (1713) and John Dyer's \"Grongar Hill' (1762) are two other oft-mentioned examples. More recently, Matthew Arnold's \"The Scholar Gipsy\" (1853) praises the Oxfordshire countryside, and W. H. Auden's \"In Praise of Limestone\" (1948) uses a limestone landscape as an allegory. Subgenres of topographical poetry include the country house poem, written in 17th-century England to compliment a wealthy patron, and the prospect poem, describing the view from a distance or a temporal view into the future, with the sense of opportunity or expectation. When understood broadly as landscape poetry and when assessed from its establishment to the present, topographical poetry can take on many formal situations and types of places. Kenneth Baker identifies 37 varieties and compiles poems from the 16th through the 20th centuries—from Edmund Spenser to Sylvia Plath—correspondent to each type, from \"Walks and Surveys,\" to \"Mountains, Hills, and the View from Above,\" to \"Violation of Nature and the Landscape,\" to \"Spirits and Ghosts.\" Common aesthetic registers of which topographical poetry make use include pastoral imagery, the sublime, and the picturesque. These latter two registers subsume imagery of rivers, ruins, moonlight, birdsong, and clouds, peasants, mountains, caves, and waterscapes."@en ;
    skos:inScheme cwrc:Genre ;
    prov:derivedFrom dbpedia:Topographical_poetry .

cwrc:genreTractpamphlet
    void:inDataset cwrc:datasetdefinition ;
    a cwrc:Genre, skos:Concept ;
    rdf:value "TRACTPAMPHLET" ;
    rdfs:isDefinedBy <http://www.cwrc.ca/ontologies/cwrc#> ;
    rdfs:label ""@fr, "tract pamphlet"@en ;
    skos:inScheme cwrc:Genre .

cwrc:genreTragedy
    void:inDataset cwrc:datasetdefinition ;
    a cwrc:Genre, skos:Concept ;
    rdf:value "TRAGEDY" ;
    rdfs:isDefinedBy <http://www.cwrc.ca/ontologies/cwrc#> ;
    rdfs:label "tragedy"@en, "tragédie"@fr ;
    owl:comment "This term and its description was created from data gathered from DBpedia."@en, "This term and its description was created from data gathered from the Getty Art & Architecture Thesaurus."@en ;
    skos:definition "La tragédie est un genre théâtral dont l’origine remonte au théâtre grec antique. Contrairement à la comédie, elle met en scène des personnages de rangs élevés et se dénoue très souvent par la mort d’un ou de plusieurs personnages.Elle a un rôle cathartique (prévenir les gens de ne pas faire le Mal en suscitant terreur et pitié)."@fr, "Literaire werken met een ernstig en plechtig karakter die toewerken naar een rampzalig of droevig slot."@nl, "Literarisches Werk mit ernstem und würdevollem Charakter, das katastrophal oder unglücklich endet."@de, "Literary works of serious and dignified character that reach disastrous or sorrowful conclusions."@en, "Trabajos literarios de carácter serio y solemne que terminan en desenlaces funestos o lamentables."@es ;
    skos:inScheme cwrc:Genre ;
    prov:derivedFrom dbpedia:Tragedy, <http://vocab.getty.edu/aat/300201026> .

cwrc:genreTragicomedy
    void:inDataset cwrc:datasetdefinition ;
    a cwrc:Genre, skos:Concept ;
    rdf:value "TRAGICOMEDY" ;
    rdfs:isDefinedBy <http://www.cwrc.ca/ontologies/cwrc#> ;
    rdfs:label ""@fr, "tragicomedy"@en ;
    owl:comment "This term and its description was created from data gathered from DBpedia."@en ;
    skos:definition "Een tragikomedie is een dramavorm die zowel in het theater als in zijn afgeleide, de film, een vermenging hanteert van tragische en komische verhaalelementen. Eén van de eerste auteurs die deze mengvorm beheersten, was Plautus, zo ongeveer in 210 v.Chr., met zijn stuk Amphitruo, dat in de 17e eeuw Molière inspireerde tot het schrijven van zijn Amphitrion (1668). De samenstelling tragikomedie geeft aan dat komedie de hoofdbedoeling is, maar dat er enkele tragische gegevens doorheen lopen. Het begrip is pas tegen het einde van de 16e eeuw echt doorgebroken. De theoreticus van dienst is een zekere Italiaan Battista Guarini met zijn verhandelingen die gebundeld zijn als Compendio della poesia tragicomica (1601). Rond dezelfde tijd vinden we in Shakespeares drama's een hele variëteit clowneske figuren terug: de clown is de tragikomische mens bij uitstek. Een typisch voorbeeld is Le Cid van Pierre Corneille. Enkele van de nevenpersonages sterven hierin, maar voor de twee hoofdpersonages kent het verhaal een gunstige afloop. Aangezien de combinatie tragiek en komedie ook scherp wordt aangevoeld door auteurs die ironie, satire en cynisme gepast kunnen hanteren, vind je in het absurde theater van Samuel Beckett, Eugène Ionesco en Harold Pinter ook veel tragikomische situaties en personages. In de film denke men aan Charlie Chaplin, de hoofdfiguur in zijn eigen stomme films."@nl, "Eine Tragikomödie beschreibt ein Drama in der Literatur und im Theater, in dem die Merkmale der Tragödie wie auch der Komödie eng miteinander verknüpft sind. Im weiteren Sinne bezeichnet der Begriff eine Tragödie, welche neben den tragischen auch komische Bestandteile enthält, wie z. B. die alten spanischen und englischen Tragödien."@de, "La tragi-comédie est une forme théâtrale caractérisée par une action romanesque, des personnages de haute extraction, un dénouement heureux et un refus des règles de la tragédie. Le terme est apparu en France chez le dramaturge Robert Garnier vers la fin du XVIe siècle, orthographié tragecomedie ; le terme nous vient de Plaute, qui désigne son Amphitryon comme une \"tragi-comoedia\" (au vers 59). Ce genre a connu un très grand succès en France dans les années 1630-1640. Il est assez difficile de définir les limites de la tragi-comédie à cette époque parce que les auteurs revendiquaient le refus de toute règle. On pouvait alors voir dans la tragi-comédie une sorte de tragédie à fin heureuse parce que la tragédie n'était définie que par son personnel noble et mythologique. Dans les années 1640, les partisans d'un théâtre beaucoup plus normé prennent de plus en plus d'importance et la tragédie répondant aux règles classiques prend le dessus sur la tragi-comédie. Le cas du Le Cid de Corneille est un exemple intéressant à cet égard car il a été publié en 1637 en tant que tragi-comédie et requalifié en tragédie dès 1648 alors que Corneille n'avait pas encore effectué de modification majeure de la pièce. On peut donc considérer que ce n'est pas la pièce mais la perception qu'on avait des différents genres théâtraux qui a évolué entre ces deux dates. En effet, l'intrigue du Cid comporte de nombreux éléments caractéristiques d'une tragi-comédie : il raconte une histoire d'amour dans laquelle un obstacle empêche à un moment donné la réunion des deux amants. À la fin de la pièce, cet obstacle sera levé et le dénouement sera heureux et nuptial ce qui est à l'époque une caractéristique des comédies et des tragi-comédies. La Querelle du Cid aura contribué à fixer les règles de la tragédie même si Le Cid conserve ses caractéristiques à savoir l'accumulation des événements , les coups de théâtre, les changements de décor successif et le dénouement heureux. On a beaucoup reproché à Corneille l'invraisemblance de la fin et un respect très discutable des trois unités. De fait, même s'il est déjà influencé par les règles qui commencent à s'imposer à la fin des années 1630, Corneille conserve dans cette pièce une liberté de composition héritée de la tragi-comédie et que l'on ne trouvera plus dans ses tragédies ultérieures. Pour autant, la pièce annonce la dramaturgie classique parce que les conflits omniprésents qui la constituent ne se manifestent pas à travers de combats spectaculaires sur scène mais à travers le travail du langage. Ainsi le duel entre Rodrigue et Don Gomes s'achève très vite alors que les célébrissimes stances du Cid rendent compte longuement du conflit intérieur qui travaille Rodrigue. Ce refus du spectaculaire au profit d'un travail sur le discours et les sentiments des personnages sera caractéristique de l'esthétique classique et explique que le Cid en soit resté un exemple majeur alors qu'il est encore très influencé par le genre de la tragi-comédie qui s'oppose aux caractéristiques de l'écriture classique. Philippe Quinault , poète et librettiste français, a aussi contribué au succès de ce genre en participant à la création de la tragédie-ballet Psyché en 1671 écrit par Molière aidé de Corneille. Le mélange des genres fut peu représenté par la suite dans le théâtre français, tout au plus trouve-t-on des pièces ou les genres s'alternent sans se mêler. Victor Hugo tente pourtant d'imposer avec son théâtre romantique une écriture entre sublime et grotesque, mais il faudra attendre le XXe siècle et le théâtre de l'absurde pour que le public accepte de concevoir que le rire ne nuit pas obligatoirement à la profondeur dramatique."@fr, "Tragicomedy is a literary genre that blends aspects of both tragic and comic forms. Most often seen in dramatic literature, the term can variously describe either a tragic play which contains enough comic elements to lighten the overall mood or a serious play with a happy ending."@en, "Una tragicomedia es una gran obra dramática en la que se mezclan los elementos trágicos y cómicos, aunque también hay lugar para el sarcasmo y parodia. También se le conoce como pieza, porque se parece a dicho concepto; generalmente en estos están sintetizadas las características de una clase social, por lo que también se le denomina género psicológico. Una pieza es una obra literaria del tipo realista, en donde la situación y los personajes están claramente presentados. Si bien en lo que se relata y expone hay cambios inesperados, ellos son lógicos y explicables, y el suspenso va en continuo aumento, llegando por momentos a clímax con intensas emociones. La resolución o conclusión de la obra es consecuencia de los actos y de las situaciones planteadas con bastante claridad y sin ambigüedades, donde los actos de los personajes son verosímiles. En la Grecia clásica, el drama satírico o la tragicomedia suele tratar un tema legendario, aunque con efectos cómicos protagonizados, fundamentalmente, por el coro. Los dioses no intervienen en la muerte de los hombres y puede haber más de una acción al mismo tiempo. La tragicomedia principalmente va a mostrar la trayectoria del héroe tragicómico, que tiene un objetivo que perseguir (el amor, la justicia, la ambición, un trono, etc) y de cómo éste lo consigue o no pasando por una serie de obstáculos para llegar a su fin. Si los obstáculos se presentan como positivos, es decir que parece que lo acercan cada vez más a su objetivo, más que obstáculos son como pruebas superadas. Por su parte el final será negativo, si los obstáculos son negativos, y parece que le impiden llegar a su objetivo, aunque por lo general el final será positivo y aunque sea a último minuto alcanzará su objetivo. Su creador fue Lope de Vega cuando rompió las estructuras del teatro aristotélico. Lope se negaba a obedecer las unidades, y entonces creó la tragicomedia."@es ;
    skos:inScheme cwrc:Genre ;
    prov:derivedFrom dbpedia:Tragicomedy .

cwrc:genreTranslation
    void:inDataset cwrc:datasetdefinition ;
    a cwrc:Genre, skos:Concept ;
    rdf:value "TRANSLATION" ;
    rdfs:isDefinedBy <http://www.cwrc.ca/ontologies/cwrc#> ;
    rdfs:label ""@fr, "translation"@en ;
    owl:comment "This term and its description was created from data gathered from the Getty Art & Architecture Thesaurus."@en ;
    skos:definition "Translated versions of a text."@en, "Versiones traducidas de un texto."@es, "Vertaalde versies van een tekst."@nl, "Übersetzte Version eines Textes."@de, "一文本之翻譯版本。"@zh-hant ;
    skos:inScheme cwrc:Genre ;
    prov:derivedFrom <http://vocab.getty.edu/aat/300027389> .

cwrc:genreTravelwriting
    void:inDataset cwrc:datasetdefinition ;
    a cwrc:Genre, skos:Concept ;
    rdf:value "TRAVELWRITING" ;
    rdfs:isDefinedBy <http://www.cwrc.ca/ontologies/cwrc#> ;
    rdfs:label ""@fr, "travel writing"@en ;
    skos:inScheme cwrc:Genre .

cwrc:genreTreatise
    void:inDataset cwrc:datasetdefinition ;
    a cwrc:Genre, skos:Concept ;
    rdf:value "TREATISE" ;
    rdfs:isDefinedBy <http://www.cwrc.ca/ontologies/cwrc#> ;
    rdfs:label ""@fr, "treatise"@en ;
    owl:comment "This term and its description was created from data gathered from DBpedia."@en, "This term and its description was created from data gathered from the Getty Art & Architecture Thesaurus."@en ;
    skos:definition "Exposiciones escritas, formales y sistemáticas de las ideas fundamentales de un tema, generalmente más largas y más detalladas que los ensayos."@es, "Formal and systematic written expositions of the principles of a subject, generally longer and more detailed than essays."@en, "Formale und systematische schriftliche Darstellung der Grundgedanken zu einem Thema, im Allgemeinen länger und detaillierter als Essays."@de, "Schriftelijke documenten waarin een bepaald onderwerp volgens een erkende methode systematisch wordt behandeld. Over het algemeen zijn verhandelingen langer en meer gedetailleerd dan essays."@nl, "Un traité est un manuel d'instructions ou un livre standard dans n'importe quelle branche qui forme un sujet d'études. Ils se différencient les uns des autres, aussi bien par le public ciblé que par le sujet abordé. Les traités sont habituellement édités par des imprimeurs spécialisés, dans le but de répondre aux besoins de formation, sur n'importe quel thème susceptible de faire l'objet d'un enseignement. Il s'agit d'un important commerce qui nécessite des ventes massives, afin de rendre ces publications rentables. Bien que la plupart des traités soient uniquement édités sous forme de livres reliés, certains sont désormais consultables sur internet. Les traités sont apparus avec le développement de l'imprimerie de Johannes Gutenberg, sous la forme de méthodes d'enseignement."@fr ;
    skos:inScheme cwrc:Genre ;
    prov:derivedFrom dbpedia:Treatise, <http://vocab.getty.edu/aat/300026681> .

cwrc:genreUtopia
    void:inDataset cwrc:datasetdefinition ;
    a cwrc:Genre, skos:Concept ;
    rdf:value "UTOPIA" ;
    rdfs:isDefinedBy <http://www.cwrc.ca/ontologies/cwrc#> ;
    rdfs:label ""@fr, "utopia"@en ;
    skos:inScheme cwrc:Genre .

cwrc:genreVersenovel
    void:inDataset cwrc:datasetdefinition ;
    a cwrc:Genre, skos:Concept ;
    rdf:value "VERSENOVEL" ;
    rdfs:isDefinedBy <http://www.cwrc.ca/ontologies/cwrc#> ;
    rdfs:label ""@fr, "verse novel"@en ;
    owl:comment "This term and its description was created from data gathered from DBpedia."@en ;
    skos:broaderTransitive cwrc:genreNovel ;
    skos:definition "A verse novel is a type of narrative poetry in which a novel-length narrative is told through the medium of poetry rather than prose. Either simple or complex stanzaic verse-forms may be used, but there will usually be a large cast, multiple voices, dialogue, narration, description, and action in a novelistic manner."@en, "Der Versroman ist eine als Roman geschriebene Erzählung in Vers­form; in erster Linie der Ritterroman der höfischen Dichtung des Mittelalters. Dazu zählen beispielsweise:"@de ;
    skos:inScheme cwrc:Genre ;
    prov:derivedFrom dbpedia:Verse_novel .

cwrc:genreVignette
    void:inDataset cwrc:datasetdefinition ;
    a cwrc:Genre, skos:Concept ;
    rdf:value "VIGNETTE" ;
    rdfs:isDefinedBy <http://www.cwrc.ca/ontologies/cwrc#> ;
    rdfs:label ""@fr, "vignette"@en ;
    owl:comment "This term and its description was created from data gathered from DBpedia."@en ;
    skos:definition "In proza en poëzie is een vignet een kort, impressionistisch tafereel dat een beeld schetst van een bepaald moment en een bepaalde plaats. Typisch is het de bedoeling om een scherp beeld van een personage, een idee, of een omgeving te geven. Dit type scène komt vaker voor bij het recente postmoderne theater, dat de naleving van de conventies en structuur van een verhaal ter discussie stelt. De manier waarop een scène wordt weergegeven is duidelijk beïnvloed door de hedendaagse snelle beeldcultuur van film, video en televisie."@nl, "In theatrical script writing, sketch stories, and poetry, a vignette is a short impressionistic scene that focuses on one moment or gives a trenchant impression about a character, idea, setting, or object.[citation needed] This type of scene is more common in recent postmodern theater, where less emphasis is placed on adhering to the conventions of theatrical structure and story development. Vignettes have been particularly influenced by contemporary notions of a scene as shown in film, video and television scripting. It is also a part of something bigger than itself: for example, a vignette about a house belonging to a collection of vignettes or a whole story, such as The House On Mango Street, by Sandra Cisneros. A blog can provide a form of vignette."@en ;
    skos:inScheme cwrc:Genre ;
    prov:derivedFrom <http://dbpedia.org/resource/Vignette_(literature)> .

cwrc:genreVillanelle
    void:inDataset cwrc:datasetdefinition ;
    a cwrc:Genre, skos:Concept ;
    rdf:value "VILLANELLE" ;
    rdfs:isDefinedBy <http://www.cwrc.ca/ontologies/cwrc#> ;
    rdfs:label ""@fr, "villanelle"@en ;
    skos:inScheme cwrc:Genre .

cwrc:genreYoungadultwriting
    void:inDataset cwrc:datasetdefinition ;
    a cwrc:Genre, skos:Concept ;
    rdf:value "YOUNGADULTWRITING" ;
    rdfs:isDefinedBy <http://www.cwrc.ca/ontologies/cwrc#> ;
    rdfs:label ""@fr, "young adult writing"@en ;
    skos:inScheme cwrc:Genre .

cwrc:gentry
    void:inDataset cwrc:datasetdefinition ;
    a cwrc:SocialClass, cwrc:SocialClassIdentity, skos:Concept ;
    rdfs:isDefinedBy <http://www.cwrc.ca/ontologies/cwrc#> ;
    rdfs:label "Gentry"@en, "Gentry"@fr, "gentry"@en, "noblesse non titrée"@fr ;
    owl:sameAs dbpedia:Gentry ;
    owl:subClass cwrc:CulturalFormation ;
    skos:definition ""@en, ""@fr, "Gentry indicates someone who is property-owning or related to the same; property can be land or stocks and bonds. It begins in the idea of owning arms and having a coat of arms. but is distinguished from nobility in so far as money is not necessarily related to blood and title. Disinterested gentlemen are of this class (i.e. Mr. Bennett in Jane Austen). Gentlewomen belong to this class, even thought they may not themselves own much property but instead be supported by a father or brother, or they may be distressed, which is to say, impoverished gentlewomen, as in the case of Jane Eyre or Austen's Jane Fairfax."@en .

cwrc:hasActor
    void:inDataset cwrc:datasetdefinition ;
    a owl:ObjectProperty, skos:Concept ;
    rdfs:comment "An Actor in this event."@en ;
    rdfs:domain cwrc:Event ;
    rdfs:isDefinedBy <https://raw.githubusercontent.com/cwrc/OrlandoOntology/master/OrlandoOntology#> ;
    rdfs:label "hasActor"@en ;
    rdfs:range cwrc:Actor .

cwrc:hasCulturalForms
    void:inDataset cwrc:datasetdefinition ;
    a owl:ObjectProperty ;
    rdfs:isDefinedBy <http://www.cwrc.ca/ontologies/cwrc#> ;
    rdfs:label "a une formation culturelle"@fr, "has a cultural form"@en ;
    skos:definition "Cette sous-catégorie de culturalFormation associe des concepts et des catégories spécifiques au processus de formation identitaire à travers les processus culturels. Le sujet elle/lui-même peut ou a pu s’approprier de telles associations, ou d’autres personnes les lui ont attribuées. Les concepts et les catégories classés dans culturalForms se chevauchent en termes de concepts et d’étiquettes utilisées."@fr, "This sub-class of culturalFormation associates specific concepts and categories with the process of identity formation through cultural processes. Such associations may be or have been embraced by the subject her/himself or attributed by others. The concepts and categories classed as culturalForms are understood to overlap with each other conceptually and in terms of the labels used."@en .

cwrc:hasEthnicity
    void:inDataset cwrc:datasetdefinition ;
    a owl:ObjectProperty ;
    rdfs:domain cwrc:Ethnicity ;
    rdfs:isDefinedBy <http://www.cwrc.ca/ontologies/cwrc#> ;
    rdfs:label "D'Ethnicité"@fr, "has Ethnicity"@en ;
    rdfs:subPropertyOf cwrc:personalProperty ;
    skos:definition ""@en, ""@fr .

cwrc:hasEthnicitySelfDefined
    void:inDataset cwrc:datasetdefinition ;
    a owl:ObjectProperty ;
    rdfs:domain cwrc:Ethnicity ;
    rdfs:isDefinedBy <http://www.cwrc.ca/ontologies/cwrc#> ;
    rdfs:label "D'Ethnicité (Autodéclarés)"@fr, "has Ethnicity (Self Defined)"@en ;
    rdfs:subPropertyOf cwrc:personalPropertySelfDefined ;
    skos:definition ""@en, ""@fr .

cwrc:hasGender
    void:inDataset cwrc:datasetdefinition ;
    a owl:ObjectProperty ;
    rdfs:domain cwrc:Gender ;
    rdfs:isDefinedBy <http://www.cwrc.ca/ontologies/cwrc#> ;
    rdfs:label "A le Genre"@fr, "has Gender"@en ;
    rdfs:subPropertyOf cwrc:personalProperty ;
    skos:definition ""@en, ""@fr .

cwrc:hasGenderSelfDeclared
    void:inDataset cwrc:datasetdefinition ;
    a owl:ObjectProperty ;
    rdfs:domain cwrc:Gender ;
    rdfs:isDefinedBy <http://www.cwrc.ca/ontologies/cwrc#> ;
    rdfs:label "A le Genre (Autodéclarés)"@fr, "has Gender (Self Declared)"@en ;
    rdfs:subPropertyOf cwrc:personalPropertySelfDeclared ;
    skos:definition ""@en, ""@fr .

cwrc:hasGenre
    void:inDataset cwrc:datasetdefinition ;
    a owl:ObjectProperty ;
    rdfs:isDefinedBy <http://www.cwrc.ca/ontologies/cwrc#> ;
    rdfs:label "a un genre"@fr, "has genre"@en ;
    skos:definition ""@en, ""@fr .

cwrc:hasGeographicHeritage
    void:inDataset cwrc:datasetdefinition ;
    a owl:ObjectProperty ;
    rdfs:domain cwrc:GeographicHeritage ;
    rdfs:isDefinedBy <http://www.cwrc.ca/ontologies/cwrc#> ;
    rdfs:label "A un héritage géographique"@fr, "has Geographic Heritage"@en ;
    rdfs:subPropertyOf cwrc:personalProperty ;
    skos:definition ""@en, ""@fr .

cwrc:hasGeographicHeritageSelfDeclared
    void:inDataset cwrc:datasetdefinition ;
    a owl:ObjectProperty ;
    rdfs:domain cwrc:GeographicHeritage ;
    rdfs:isDefinedBy <http://www.cwrc.ca/ontologies/cwrc#> ;
    rdfs:label "A un héritage géographique (Self Declared)"@fr, "has Geographic Heritage (Self Declared)"@en ;
    rdfs:subPropertyOf cwrc:personalProperty ;
    skos:definition ""@en, ""@fr .

cwrc:hasLanguage
    void:inDataset cwrc:datasetdefinition ;
    a owl:ObjectProperty ;
    rdfs:domain cwrc:Language ;
    rdfs:isDefinedBy <http://www.cwrc.ca/ontologies/cwrc#> ;
    rdfs:label "Connait la langue"@fr, "Knowns Language"@en ;
    rdfs:subPropertyOf cwrc:personalProperty ;
    skos:definition ""@fr, "Knowleage about the language in writing or reading."@en .

cwrc:hasLanguageSelfDeclared
    void:inDataset cwrc:datasetdefinition ;
    a owl:ObjectProperty ;
    rdfs:domain cwrc:Language ;
    rdfs:isDefinedBy <http://www.cwrc.ca/ontologies/cwrc#> ;
    rdfs:label "Connait la langue (Autodéclarés)"@fr, "Knowns Language (Self Declared)"@en ;
    rdfs:subPropertyOf cwrc:personalPropertySelfDeclared ;
    skos:definition ""@en, ""@fr .

cwrc:hasNationality
    void:inDataset cwrc:datasetdefinition ;
    a owl:ObjectProperty ;
    rdfs:domain cwrc:NationalIdentity ;
    rdfs:isDefinedBy <http://www.cwrc.ca/ontologies/cwrc#> ;
    rdfs:label "de Nationalité"@fr, "has Nationality"@en ;
    rdfs:subPropertyOf cwrc:personalProperty ;
    skos:definition ""@en, ""@fr .

cwrc:hasNationalitySelfDeclared
    void:inDataset cwrc:datasetdefinition ;
    a owl:ObjectProperty ;
    rdfs:domain cwrc:NationalIdentity ;
    rdfs:isDefinedBy <http://www.cwrc.ca/ontologies/cwrc#> ;
    rdfs:label "de Nationalité (Autodéclarés)"@fr, "has Nationality (Self Declared)"@en ;
    rdfs:subPropertyOf cwrc:personalPropertySelfDeclared ;
    skos:definition ""@en, ""@fr .

cwrc:hasNativeLanguage
    void:inDataset cwrc:datasetdefinition ;
    a owl:ObjectProperty ;
    rdfs:domain cwrc:Language ;
    rdfs:isDefinedBy <http://www.cwrc.ca/ontologies/cwrc#> ;
    rdfs:label "A une langue native"@fr, "Knowns Language Natively"@en ;
    rdfs:subPropertyOf cwrc:hasLanguage ;
    skos:definition ""@fr, "Knowleage about the language in writing or reading."@en .

cwrc:hasNativeLanguageSelfDeclared
    void:inDataset cwrc:datasetdefinition ;
    a owl:ObjectProperty ;
    rdfs:domain cwrc:Language ;
    rdfs:isDefinedBy <http://www.cwrc.ca/ontologies/cwrc#> ;
    rdfs:label "A une langue native (Autodéclarés)"@fr, "Knowns Language Natively (Self Declared)"@en ;
    rdfs:subPropertyOf cwrc:hasLanguageSelfDeclared ;
    skos:definition ""@en, ""@fr .

cwrc:hasRaceColour
    void:inDataset cwrc:datasetdefinition ;
    a owl:ObjectProperty ;
    rdfs:domain cwrc:RaceColour ;
    rdfs:isDefinedBy <http://www.cwrc.ca/ontologies/cwrc#> ;
    rdfs:label "Est de Race"@fr, "has Race"@en ;
    rdfs:subPropertyOf cwrc:personalProperty ;
    skos:definition ""@fr, "A subclass of raceEthnicityContext, this describes a person's racial identity."@en .

cwrc:hasRaceColourSelfDeclared
    void:inDataset cwrc:datasetdefinition ;
    a owl:ObjectProperty ;
    rdfs:domain cwrc:Race ;
    rdfs:isDefinedBy <http://www.cwrc.ca/ontologies/cwrc#> ;
    rdfs:label "Est de Race (Autodéclarés)"@fr, "has Race (Self Declared)"@en ;
    rdfs:subPropertyOf cwrc:personalPropertySelfDeclared ;
    skos:definition ""@fr, "A subclass of raceEthnicityContext, this describes a person's self-reported racial identity."@en .

cwrc:hasReligion
    void:inDataset cwrc:datasetdefinition ;
    a owl:ObjectProperty ;
    rdfs:domain cwrc:Religion ;
    rdfs:isDefinedBy <http://www.cwrc.ca/ontologies/cwrc#> ;
    rdfs:label "Religion"@fr, "has Religious Affiliation"@en ;
    rdfs:subPropertyOf cwrc:personalProperty ;
    skos:definition ""@en, ""@fr .

cwrc:hasReligionSelfDefined
    void:inDataset cwrc:datasetdefinition ;
    a owl:ObjectProperty ;
    rdfs:domain cwrc:Religion ;
    rdfs:isDefinedBy <http://www.cwrc.ca/ontologies/cwrc#> ;
    rdfs:label "Religion (Autodéclarés)"@fr, "has Religious Affilication (Self Defined)"@en ;
    rdfs:subPropertyOf cwrc:personalPropertySelfDefined ;
    skos:definition ""@en, ""@fr .

cwrc:hasSexuality
    void:inDataset cwrc:datasetdefinition ;
    a owl:ObjectProperty ;
    rdfs:domain cwrc:Sexuality ;
    rdfs:isDefinedBy <http://www.cwrc.ca/ontologies/cwrc#> ;
    rdfs:label "A une Orientation Sexuelle"@fr, "has Sexual Orientation"@en ;
    rdfs:subPropertyOf cwrc:personalProperty ;
    skos:definition ""@en, ""@fr .

cwrc:hasSexualitySelfDeclared
    void:inDataset cwrc:datasetdefinition ;
    a owl:ObjectProperty ;
    rdfs:domain cwrc:Sexuality ;
    rdfs:isDefinedBy <http://www.cwrc.ca/ontologies/cwrc#> ;
    rdfs:label "A une Orientation Sexuelle (Autodéclarés)"@fr, "has Sexual Orientation (Self Declared)"@en ;
    rdfs:subPropertyOf cwrc:personalPropertySelfDeclared ;
    skos:definition ""@en, ""@fr .

cwrc:hasSocialClass
    void:inDataset cwrc:datasetdefinition ;
    a owl:ObjectProperty ;
    rdfs:domain cwrc:SocialClass ;
    rdfs:isDefinedBy <http://www.cwrc.ca/ontologies/cwrc#> ;
    rdfs:label "De Classe Sociale"@fr, "has Social Class"@en ;
    rdfs:subPropertyOf cwrc:personalProperty ;
    skos:definition ""@en, ""@fr .

cwrc:hasSocialClassSelfDefined
    void:inDataset cwrc:datasetdefinition ;
    a owl:ObjectProperty ;
    rdfs:domain cwrc:SocialClass ;
    rdfs:isDefinedBy <http://www.cwrc.ca/ontologies/cwrc#> ;
    rdfs:label "De Classe Sociale (Autodéclarés)"@fr, "has Social Class (Self Defined)"@en ;
    rdfs:subPropertyOf cwrc:personalPropertySelfDefined ;
    skos:definition ""@en, ""@fr .

cwrc:heterosexual
    void:inDataset cwrc:datasetdefinition ;
    a cwrc:SexualIdentity, skos:Concept ;
    rdfs:isDefinedBy <http://www.cwrc.ca/ontologies/cwrc#> ;
    rdfs:label "Heterosexual"@en, "Hétérosexuelle"@fr ;
    owl:sameAs <http://homosaurus.org/terms/heterosexualIdentity> ;
    skos:definition ""@en, ""@fr ;
    foaf:name "Heterosexual (Sexual Identity)"@en .

cwrc:hinduism
    void:inDataset cwrc:datasetdefinition ;
    a cwrc:Religion, skos:Concept ;
    rdfs:isDefinedBy <http://www.cwrc.ca/ontologies/cwrc#> ;
    rdfs:label "Hindou"@fr, "Hinduism"@en, "hindoeïsme"@nl, "hinduismo"@es, "l'hindouisme"@fr, "yin du jiao"@zh-latn-pinyin-x-notone, "yin tu chiao"@zh-latn-wadegile, "yìn dù jiào"@zh-latn-pinyin-x-hanyu, "印度教"@zh-hant ;
    skos:broaderTransitive cwrc:occultism ;
    skos:definition ""@fr, "General term for the set of intellectual and philosophical tenets and highly diverse beliefs and practices that define the civilization, art, literature, society, and politics of the Indian subcontinent. Hinduism is not a common set of rigid beliefs , but varies significantly between different regions; it includes Shaivism, Vaishnavism, Srauta, and numerous other traditions. Among other practices and philosophies, Hinduism includes a wide spectrum of laws and prescriptions of \"daily morality\" based on karma, dharma, and societal norms. The highest divine powers are seen as complementary to one another and not exclusive. Hinduism does not have a particular founder or central authority. Hindu literature is rich and varied, with no one text considered uniquely authoritative. The Vedas, dating to the Vedic period (ca. 1200-500 BCE), are the earliest extant writings. Religious law books and epics such as the Ramayana and the Mahabharata have been and continue to be highly influential."@en, "Se refiere al conjunto de creencias y prácticas altamente diversas que generalmente denotan la civilización y cultura India de los dos mil últimos años. La religión influye fuertemente en el arte, la literatura, la política y al sociedad hinduista. Presenta la creencia y la práctica de ritos mágicos, cultos animales, creencia en demonios, cultos a deidades, incluyendo dioses locales y dioses centrales, misticismo, ascetismo y una apreciación y respeto por otras formas de cultos o creencias religiosas. La verdad de la religión no esta concebida como un término dogmático, sino que la verdad supera toda definición verbal. En vez de un sistema de doctrinas, el énfasis se pone en la manera correcta de vivir (dharma). Hay variaciones significativas entre diversas regiones. La mayoría de las formas de hinduismo enfatizan el concepto del reencarnación o de la transmigración; la liberación (moksha) desde el ciclo del samsara es la última meta espiritual del hindú. Brahma, Vishnu y Shiva son las deidades hindúes principales, juntos forman la tríada, el Trimurti. Existen muchos otros deidades de menor rango. El Hinduismo no tiene un fundador en particular o un iniciado, allí no hay una autoridad central. La literatura hindú es rica y variada, sin un texto considerado únicamente autoritario. El Vedas, fechando en el período de Vedic (ca. 1200-500 a. C), es la escritura más temprana existente. Los libros de ley y las epopeyas religiosas tales como el Ramayana y el Mahabharata han sido y continúan siendo altamente influyentes."@es, "Verwijst naar de reeks uiterst diverse geloven en gebruiken die in het algemeen verwijzen naar de Indiase beschaving en cultuur van de afgelopen tweeduizend jaar. De religie heeft een sterke invloed op de Indiase kunst, literatuur, maatschappij en politiek. Het hindoeïsme omvat diverse religieuze geloven en gebruiken en in plaats van andere goden, andere godsdiensten en andere religieuze concepten als fout of onverenigbaar te zien, worden de hoogste goddelijke machten gezien als elkaar aanvullend. De religieuze waarheid wordt niet gezien in dogmatische termen aangezien wordt geloofd dat de waarheid alle woordelijke definities overstijgt. In plaats van op een reeks doctrines ligt de nadruk op de juiste manier van leven (dharma). Er zijn aanzienlijke verschillen per regio. In de meeste vormen van het hindoeïsme ligt de nadruk op het concept van reïncarnatie of zielsverhuizing; de bevrijding (moksha) van de cyclus van samsara is het uiteindelijke spirituele doel van hindoes. Brahma, Visjnoe en Shiva zijn de belangrijkste hindoeïstische godheden en vormen gezamenlijk een drie-eenheid, de Trimurti. Verder is er een groot aantal lagere goden. Het hindoeïsme heeft geen specifieke oprichter of ontstaansmoment en er is geen centrale autoriteit. De hindoeïstische literatuur is erg rijk en gevarieerd en geen enkele specifieke tekst wordt als gezaghebbend beschouwd. De Veda's, die afkomstig zijn uit de Vedische periode (ca. 1200-500 v. Chr.), zijn de oudste overgebleven geschriften. Religieuze wetboeken en heldendichten zoals de Ramayana en de Mahabharata zijn altijd erg invloedrijk geweest."@nl, "代表過去兩千年來印度文明與文化的一套極多樣的信仰與實踐方式。此宗教對印度藝術、文學、社會與政治有極大影響。印度教包含多元的宗教信仰及實踐方式，因此不會認為其他的神明、其他形式的敬拜及宗教觀是錯誤或者互不相容，反而認為最高的神力是彼此互補的。他們相信真理超越所有言語定義，因此不應武斷認定何謂宗教真理。重視生活的正確方式(法)，而非一連串的教條。不同宗教之間差異甚鉅。大部分的印度教形式強調輪迴觀念；從生死疾苦等輪迴中解脫是印度教徒最終的心靈目標。婆羅摩、毗濕奴、濕婆是印度教主要的三個神明(三相神) 。還有很多其他小神。印度教沒有確切的建立者及開始時間，也沒有中央權威。印度教文學豐富且多樣，但沒有哪一部作品被認為是權威。追溯自吠陀時期(西元前500年到西元1200年)的吠陀經是現存最早的經典。宗教法律典籍及史詩如《羅摩耶那史詩》及《摩訶婆羅達》仍舊極具影響力。"@zh-hant ;
    skos:inScheme cwrc:Religion ;
    prov:derivedFrom <http://vocab.getty.edu/aat/300073727> .

cwrc:homosexual
    void:inDataset cwrc:datasetdefinition ;
    a cwrc:SexualIdentity, skos:Concept ;
    rdfs:isDefinedBy <http://www.cwrc.ca/ontologies/cwrc#> ;
    rdfs:label "Homosexual"@en, "Homosexuel"@fr ;
    skos:definition ""@en, ""@fr ;
    foaf:name "Homosexual (Sexual Identity)"@en .

cwrc:identity
    void:inDataset cwrc:datasetdefinition ;
    a owl:ObjectProperty, skos:Concept ;
    rdfs:comment "The identity of the person who committed the act."@en ;
    rdfs:domain cwrc:Actor ;
    rdfs:isDefinedBy <https://raw.githubusercontent.com/cwrc/OrlandoOntology/master/OrlandoOntology#> ;
    rdfs:label "Identity"@en ;
    rdfs:range cwrc:Person .

cwrc:inRole
    void:inDataset cwrc:datasetdefinition ;
    a owl:ObjectProperty, skos:Concept ;
    rdfs:comment "The role taken on by this actor."@en ;
    rdfs:domain cwrc:Actor ;
    rdfs:isDefinedBy <https://raw.githubusercontent.com/cwrc/OrlandoOntology/master/OrlandoOntology#> ;
    rdfs:label "In Role"@en ;
    rdfs:range cwrc:Role .

cwrc:indigent
    void:inDataset cwrc:datasetdefinition ;
    a cwrc:SocialClass, cwrc:SocialClassIdentity, skos:Concept ;
    rdfs:isDefinedBy <http://www.cwrc.ca/ontologies/cwrc#> ;
    rdfs:label "Indigent"@en, "Pauvre"@fr, "indigent"@en, "indigents"@fr ;
    owl:subClass cwrc:CulturalFormation ;
    skos:definition ""@en, ""@fr, "This social group is poor, destitute, unemployed, supported by charity, or on social security."@en .

cwrc:islam
    void:inDataset cwrc:datasetdefinition ;
    a cwrc:Religion, skos:Concept ;
    rdfs:isDefinedBy <http://www.cwrc.ca/ontologies/cwrc#> ;
    rdfs:label "Islamism"@en, "Religion Mahométane"@fr, "i ssu lan chiao"@zh-latn-wadegile, "islam"@es, "islam"@nl, "islamismo"@es, "l'islam"@fr, "mahométisme"@fr, "yi si lan jiao"@zh-latn-pinyin-x-notone, "yī sī lán jiāo"@zh-latn-pinyin-x-hanyu, "伊斯蘭教"@zh-hant, "回教"@zh-hant ;
    skos:broaderTransitive cwrc:abrahamicReligions ;
    skos:definition ""@fr, "Refers to the religious beliefs and social practices founded in the seventh century by the Arabian Prophet Muhammad, held to be the last of a series of major prophets, which include, according to Islamic dogma, Adam, Noah, and Jesus. It later spread throughout the Middle East, Africa, Europe, and parts of Asia. It is characterized by the belief in the fundamental idea that a devotee 'surrenders' and submits his will to Allah, the prime creator and sustainer of the universe and all creation. In Islam, God is unique and has no partner or intermediary as in the Christian Trinity. Social service and the active alleviation of suffering in others is considered the only path to salvation and prayer and sacred ritual alone are inadequate forms of submission to Allah. The Qur'an (Koran), the sacred text of the religion, is a compilation of revelations from Allah believed to have been received by Muhammad."@en, "Se refiere a creencias religiosas y prácticas sociales fundadas en el siglo VII por el Profeta árabe Mahoma, supuestamente el último de una serie de grandes profetas, incluídos, de acuerdo al dogma Islámico, Adán, Noé y Jesús. Posteriormente se difundió a través del Medio Oriente, África, Europa y parte de Asia. Se caracteriza por la creencia en la idea fundamental que un devoto se \"rinde\" y somete la voluntad de Alá, el principal creador y mantenedor del universo y toda creación. En el Islam, Dios es único y no tiene parentesco o intermediario como la trinidad cristiana. El servicio social y las actividades que alivian el sufrimiento de otros es considerado el único camino a la salvación y la oración y ritual sagrado a solas es una inadecuado forma de sumisión para Alá. El Coran (Koran), consagrado el texto de las religiones, es una compilación relevante de las creencias de Alá que fueron recibidas de Mahoma."@es, "Verwijst naar het samenstel van religieuze overtuigingen en sociale gebruiken dat in de 7de eeuw is ontstaan op basis van de leer van de Arabische profeet Mohammed, die wordt beschouwd als de laatste in een reeks van grote profeten; volgens de islamitische leer zijn dit onder anderen Adam, Noach en Jezus. De islam heeft zich later verspreid in het Midden-Oosten, Afrika, Europa en delen van Azië. De islam wordt gekenmerkt door het geloof in het fundamentele idee dat een gelovige zich 'overgeeft' en zich onderwerpt aan Allah, de schepper van het universum en de schepping als geheel. God is uniek en heeft geen partner of tussenpersoon zoals bij de christelijke drie-eenheid. Maatschappelijke dienstbaarheid en het actief verlichten van het lijden van anderen wordt beschouwd als de enige weg naar verlossing en gebeden en heilige rituelen zijn op zichzelf onvoldoende vormen van overgave aan Allah. De Qur'an (Koran), het heilige geschrift van de religie, is een verzameling onthullingen die, zo gelooft men, door Allah aan Mohammed zijn geopenbaard."@nl, "由阿拉伯先知穆罕默德於七世紀創建的宗教信仰與社會實踐方式。根據伊斯蘭教條，穆罕默德是繼亞當、挪亞、耶穌後最後一個主要的先知。此教之後廣傳中東、非洲、歐洲、及部份亞洲。基本思想為信徒交出自己的意志給阿拉(宇宙及所有創造物的最高造物者與支撐者)。就伊斯蘭教而言，神是獨一無二的，且并非如基督教三位一體的觀點般有夥伴或是媒介。社會服務及積極幫助受苦者被認為是通往救贖的唯一路徑，若只有祈禱及神聖儀式則不算完全奉獻予阿拉。可蘭經是此教的聖典，記載穆罕默德從阿拉得來的神示。"@zh-hant ;
    skos:inScheme cwrc:Religion ;
    prov:derivedFrom <http://vocab.getty.edu/aat/300073715> .

cwrc:jewish
    a owl:Thing .

cwrc:jewishLabel
    void:inDataset cwrc:datasetdefinition ;
    a skos:Concept, skosxl:Label ;
    rdfs:isDefinedBy <http://www.cwrc.ca/ontologies/cwrc#> ;
    rdfs:label "jewish"@en, "juif"@fr ;
    owl:oneOf (cwrc:jewish
    ) ;
    skos:definition ""@en, ""@fr ;
    skos:inScheme cwrc:TextLabels ;
    foaf:name "jewish"@en .

cwrc:judaism
    void:inDataset cwrc:datasetdefinition ;
    a cwrc:Religion, skos:Concept ;
    rdfs:isDefinedBy <http://www.cwrc.ca/ontologies/cwrc#> ;
    rdfs:label "Jewish"@en, "Judaísmo"@es, "jodendom"@nl, "joods"@nl, "judaïsme"@fr, "you tai jiao"@zh-latn-pinyin-x-notone, "yu t'ai chiao"@zh-latn-wadegile, "yóu tài jiāo"@zh-latn-pinyin-x-hanyu, "猶太教"@zh-hant ;
    skos:broaderTransitive cwrc:abrahamicReligions ;
    skos:definition ""@fr, "Refers to the monotheistic religion of the Jewish people, central to which is the belief that the ancient Israelites experienced God's presence in human events. Jews believe that the one God delivered the Israelites out of bondage in Egypt, revealed the structure of communal and individual life to them, and chose them to be a holy nation of people able to set an example for all humankind. The Hebrew Bible and Talmud are the two primary sources for Judaism's spiritual and ethical principles. The religion, which traces its origins to Abraham, places more emphasis on expressing beliefs through ritual rather than through abstract doctrine. The Sabbath, beginning on sunset on Friday and ending at sunset on Saturday, is the central religious observance; there is also an annual cycle of religious festivals and days of fasting. Judaism has had a diverse history of development over almost 4000 years, with a number of resulting branches in modern times, namely Orthodox, Conservative, and Reform."@en, "Se refiere a la religión monoteista del pueblo judío, para los cuales es central la creencia que los antiguos israelitas experimentaron la presencia de Dios en los eventos humanos. Los judíos creen que el Dios único salvó los israelistas de la esclavitud en Egipto, revelándoles la estructura de la vida comunal e individual y eligiéndolos para ser una nación sagrada de personas capaces de dar un ejemplo para toda la humanidad. La Biblia Hebrea y el Talmud son dos fuentes primarias de la espiritualidad judía y de los principios éticos.Los orígenes de la religión se remontan a los tiempos de Abraham, poniendo mayor énfasis en expresar la creencia con rituales más bien que con doctrinas abstractas. El Shabbat, que comienza con la puesta de sol del viernes y termina con la puesta de sol del sábado, es la observancia religiosa central; hay también un ciclo anual de fiestas religiosas y días de ayuno. El judaísmo ha tenido un desarrollo diverso a lo largo de la historia de casi 4.000 años, con un gran número de ramas resultantes en épocas modernas, concretamente ortodoxas, conservadoras, y reformistas."@es, "Verwijst naar de monotheïstische religie van het joodse volk, waarbij het geloof centraal staat dat de oude Israëlieten de aanwezigheid van God ervoeren in menselijke gebeurtenissen. Joden geloven dat één God de Israëlieten uit hun gevangenschap in Egypte heeft bevrijd, de structuur van een gemeenschappelijk en individueel leven aan hen heeft onthuld en hen heeft uitverkoren als een heilig volk dat als voorbeeld moest dienen voor de gehele mensheid. De Hebreeuwse bijbel en de Talmoed zijn de belangrijkste bronnen voor de spirituele en ethische principes van het jodendom. Deze religie, waarvan de oorsprong teruggaat naar de tijd van Abraham, legt meer de nadruk op het tot uitdrukking brengen van het geloof in de vorm van rituelen dan in de vorm van abstracte doctrines. De sabbat, die begint bij zonsondergang op vrijdag en eindigt bij zonsondergang op zaterdag, is een centraal element van de religie; er is ook een jaarlijkse cyclus van religieuze feestdagen en vastendagen. Het jodendom heeft een zeer uiteenlopende ontwikkelingsgeschiedenis die bijna 4000 jaar beslaat en is uitgemond in diverse stromingen: de orthodoxe, conservatieve en reformistische stroming."@nl, "猶太人的一神論宗教，相信古代以色列人於人類事件中體驗到神的存在。猶太人相信這唯一的神使他們脫離埃及的奴役，向他們揭示公共及個人生活的結構，並選擇他們為聖國子民，以為全人類樹立榜樣。《希伯來聖經(Hebrew Bible)》與《塔爾穆德(Talmud)》為猶太教精神與道德原則的兩大來源。猶太教源於亞伯拉罕，較強調以儀式而非抽象的教條表達信仰。遵循信仰的重心為安息日，從週五的日落開始到週日的日出結束；另外每年還有宗教節慶和齋戒日。猶太教經過將近四千年的發展，衍生出許多現代的分支，即正統派猶太教(Orthodox)、保守派猶太教(Conservative)，與改革派猶太教(Reform.)。"@zh-hant ;
    skos:inScheme cwrc:Religion ;
    prov:derivedFrom <http://vocab.getty.edu/aat/300073723> .

cwrc:lesbian
    void:inDataset cwrc:datasetdefinition ;
    a cwrc:SexualIdentity, skos:Concept ;
    rdfs:isDefinedBy <http://www.cwrc.ca/ontologies/cwrc#> ;
    rdfs:label "Lesbian"@en, "Lesbienne"@fr ;
    owl:sameAs <http://homosaurus.org/terms/lesbianIdentity> ;
    skos:definition ""@en, ""@fr ;
    foaf:name "Lesbian (Sexual Identity)"@en .

cwrc:lollards
    void:inDataset cwrc:datasetdefinition ;
    a cwrc:Religion, skos:Concept ;
    rdfs:isDefinedBy <http://www.cwrc.ca/ontologies/cwrc#> ;
    rdfs:label "Lollards"@en, "Lollards"@fr ;
    skos:broaderTransitive cwrc:catholicChurch ;
    skos:definition ""@en, ""@fr ;
    skos:inScheme cwrc:Religion .

cwrc:lowerMiddleClass
    void:inDataset cwrc:datasetdefinition ;
    a cwrc:SocialClassIdentity, skos:Concept ;
    rdfs:isDefinedBy <http://www.cwrc.ca/ontologies/cwrc#> ;
    rdfs:label "This includes employees, clerical workers, teachers, and governesses. Note, however, that some teachers go into Professional (Mr. Chips) and women starting schools and then managing them also go into Professional."@en, "classe basse moyenne"@fr ;
    owl:subClass cwrc:CulturalFormation ;
    skos:definition ""@fr, "Employees, clerical workers, teachers, governesses. Note, however, that some teachers go into Professional (Mr. Chips) and women starting schools and then managing them also go into Professional."@en .

cwrc:maleLabel
    void:inDataset cwrc:datasetdefinition ;
    a skos:Concept, skosxl:Label ;
    rdf:value "male" ;
    rdfs:isDefinedBy <http://www.cwrc.ca/ontologies/cwrc#> ;
    rdfs:label "Male"@en, "Male"@fr ;
    owl:oneOf (cwrc:genderManMale
        cwrc:maleSex
    ) ;
    skos:definition ""@en, ""@fr ;
    skos:inScheme cwrc:TextLabels ;
    foaf:name "Male (Label)"@en .

cwrc:maleSex
    void:inDataset cwrc:datasetdefinition ;
    a cwrc:SexIdentity, owl:Thing, skos:Concept ;
    rdfs:isDefinedBy <http://www.cwrc.ca/ontologies/cwrc#> ;
    rdfs:label "Male"@en, "Male"@fr ;
    skos:definition ""@en, ""@fr ;
    foaf:name "Male (Sex)"@en .

cwrc:manLabel
    void:inDataset cwrc:datasetdefinition ;
    a skos:Concept, skosxl:Label ;
    rdf:value "man" ;
    rdfs:isDefinedBy <http://www.cwrc.ca/ontologies/cwrc#> ;
    rdfs:label "Homme"@fr, "Man"@en ;
    owl:oneOf (cwrc:genderManMale
    ) ;
    skos:definition ""@en, ""@fr ;
    skos:inScheme cwrc:TextLabels ;
    foaf:name "Man (Label)"@en .

cwrc:managerial
    void:inDataset cwrc:datasetdefinition ;
    a cwrc:SocialClassIdentity, skos:Concept ;
    rdfs:isDefinedBy <http://www.cwrc.ca/ontologies/cwrc#> ;
    rdfs:label "gestionnaire"@fr, "managerial"@en ;
    owl:subClass cwrc:CulturalFormation ;
    skos:definition ""@fr, "Someone whose station in life comes from the fact that they are running something but not putting their money into it, e.g. salaried civil service, bankers, hospital administrators."@en .

cwrc:methodistChurch
    void:inDataset cwrc:datasetdefinition ;
    a cwrc:Religion, skos:Concept ;
    rdfs:isDefinedBy <http://www.cwrc.ca/ontologies/cwrc#> ;
    rdfs:label "Methodist Church"@en, "l'Église méthodiste"@fr ;
    skos:broaderTransitive cwrc:christianity ;
    skos:definition ""@en, ""@fr ;
    skos:inScheme cwrc:Religion .

cwrc:millenarianism
    void:inDataset cwrc:datasetdefinition ;
    a cwrc:Religion, skos:Concept ;
    rdfs:isDefinedBy <http://www.cwrc.ca/ontologies/cwrc#> ;
    rdfs:label "Millenarianism"@en, "millénarisme, ou chiliasme"@fr ;
    skos:broaderTransitive cwrc:occultism ;
    skos:definition ""@en, ""@fr ;
    skos:inScheme cwrc:Religion .

cwrc:neo-thomism
    void:inDataset cwrc:datasetdefinition ;
    a cwrc:Religion, skos:Concept ;
    rdfs:isDefinedBy <http://www.cwrc.ca/ontologies/cwrc#> ;
    rdfs:label "Neo-thomism"@en, "néothomisme"@fr ;
    skos:broaderTransitive cwrc:catholicChurch ;
    skos:definition ""@en, ""@fr ;
    skos:inScheme cwrc:Religion .

cwrc:nobility
    void:inDataset cwrc:datasetdefinition ;
    a cwrc:SocialClassIdentity, skos:Concept ;
    rdfs:isDefinedBy <http://www.cwrc.ca/ontologies/cwrc#> ;
    rdfs:label "nobility"@en, "nobilitée"@fr ;
    owl:subClass cwrc:CulturalFormation ;
    skos:definition ""@fr, "This group refers to those holding a title or of close family relation to someone holding a title (such as Lady Mary Wortley Montagu, Lord Byron, or Nancy Mitford)."@en .

cwrc:occultism
    void:inDataset cwrc:datasetdefinition ;
    a cwrc:Religion, skos:Concept ;
    rdfs:isDefinedBy <http://www.cwrc.ca/ontologies/cwrc#> ;
    rdfs:label "Occultism/Theosophism"@en, "occultisme"@fr ;
    skos:definition ""@fr, "Any religious or philosophic ideology based on mystical insight into the nature of God and/or divine truth. This insight is attained only through direct experience of the divine. The term is sometimes used to specifically refer to the principles of the Theosophical Society founded in New York in 1875 by Madame Blavatsky and H. S. Olcott which incorporated aspects of Buddhism and Brahmanism."@en ;
    skos:inScheme cwrc:Religion .

cwrc:originalOrlandoAuthor
    void:entities "405" ;
    void:inDataset cwrc:datasetdefinition ;
    void:triples "4072" ;
    a skos:Concept, foaf:Group ;
    rdfs:isDefinedBy <http://www.cwrc.ca/ontologies/cwrc#> ;
    rdfs:label "Les membres du project Orlando"@fr, "Members of the Orlando Project"@en ;
    skos:definition "La collection de tout les auteurs du Project Orlando."@fr, "The collection of all persons having written entries for The Orlando Project."@en ;
    foaf:homepage <http://orlando.cambridge.org/public/svDocumentation?formname=t&d_id=CREDITSANDACKNOWLEDGEMENTS> ;
    foaf:name "Members of the Orlando Project."@en .

cwrc:pagan
    void:inDataset cwrc:datasetdefinition ;
    a cwrc:Religion, skos:Concept ;
    rdfs:isDefinedBy <http://www.cwrc.ca/ontologies/cwrc#> ;
    rdfs:label "Pagan"@en, "païen (ou payen)"@fr ;
    skos:broaderTransitive cwrc:occultism ;
    skos:definition ""@en, ""@fr ;
    skos:inScheme cwrc:Religion .

cwrc:personalProperty
    void:inDataset cwrc:datasetdefinition ;
    a owl:ObjectProperty ;
    rdfs:isDefinedBy <http://www.cwrc.ca/ontologies/cwrc#> ;
    rdfs:label "Personal Property"@en, "Propriété de la Personne"@fr ;
    skos:definition ""@en, ""@fr .

cwrc:personalPropertySelfDeclared
    void:inDataset cwrc:datasetdefinition ;
    a owl:ObjectProperty ;
    rdfs:isDefinedBy <http://www.cwrc.ca/ontologies/cwrc#> ;
    rdfs:label "Personal Property (Self Reported)"@en, "Propriété de la Personne (Autodéclarés)"@fr ;
    rdfs:subPropertyOf cwrc:personalProperty ;
    skos:definition ""@en, ""@fr .

cwrc:plymouthBrethren
    void:inDataset cwrc:datasetdefinition ;
    a cwrc:Religion, skos:Concept ;
    rdfs:isDefinedBy <http://www.cwrc.ca/ontologies/cwrc#> ;
    rdfs:label "Frères de Schwarzenau"@fr, "Plymouth Brethren"@en ;
    skos:broaderTransitive cwrc:anglicanChurch ;
    skos:definition ""@en, ""@fr ;
    skos:inScheme cwrc:Religion .

cwrc:presbyterianism
    void:inDataset cwrc:datasetdefinition ;
    a cwrc:Religion, skos:Concept ;
    rdfs:isDefinedBy <http://www.cwrc.ca/ontologies/cwrc#> ;
    rdfs:label "Presbyterian"@en, "chang lao tsung"@zh-latn-wadegile, "prebyteriaan"@nl, "presbiterianismo"@es, "presbyterianisme"@nl, "presbytérien"@fr, "zhang lao zong"@zh-latn-pinyin-x-notone, "zhǎng lǎo zōng"@zh-latn-pinyin-x-hanyu, "長老制"@zh-hant, "長老宗"@zh-hant, "長老教會"@zh-hant ;
    skos:broaderTransitive cwrc:christianity ;
    skos:definition ""@fr, "Een van de belangrijkste protestantse groeperingen die voortkwamen uit de 16de-eeuwse Reformatie. In het algemeen hebben moderne presbyteriaanse kerken hun oorsprong in de calvinistische kerken op de Britse eilanden, waarvan de Europese tegenhangers bekend zijn geworden onder de meer algemene naam 'gereformeerden'. De term 'presbyteriaans' verwijst ook naar een collegiaal type kerkbestuur onder leiding van pastors en leken die ouderlingen of presbyters worden genoemd. Strikt genomen maken alle presbyteriaanse kerken deel uit van de gereformeerde of calvinistische traditie, maar zijn niet alle gereformeerde kerken presbyteriaans in hun bestuursvorm."@nl, "One of the main Protestant groups that arose out of the 16th-century Reformation. Generally speaking, modern Presbyterian churches trace their origins to the Calvinist churches of the British Isles, the European counterparts of which came to be known by the more inclusive name of Reformed. The term presbyterian also denotes a collegiate type of church government led by pastors and lay leaders called elders or presbyters. Strictly speaking, all Presbyterian churches are a part of the Reformed, or Calvinist, tradition, although not all Reformed churches are presbyterian in their form of government."@en, "Uno de los principales grupos protestantes que surgió de la Reforma del siglo XVI. Hablando en general, las Iglesias Presbiterianas modernas señalan sus orígenes en las iglesias calvinistas de las Islas Británicas, la contraparte Europea la que fue conocida por el nombre más global de \"Reformada\". El término presbiterianismo también denota un tipo colegiado de gobierno de iglesia liderado por el pastor y lideres laicos llamados ancianos o presbiteros. Estrictamente hablando, todas las iglesias presbiterianas son parte de la Iglesia .El término presbiterianismo también denota un tipo colegiado de gobierno de iglesia liderado por el pastor y lideres laicos llamados ancianos o presbiteros. Estrictamente hablando, todas las iglesias presbiterianas son parte de la Reforma o Calvinismo, tradición, aunque no todas las iglesias Reformadas son presbiterianas en su gubernamentalidad."@es, "自十六世紀宗教改革興起的主要新教團體的一派。一般說來，現代的長老教會可追溯至不列顛群島的喀爾文(Calvinis)教派，其在歐洲的對應教派則被稱為較具涵蓋性的歸正派(Reformed)。長老教會一詞，亦表示其管理方式如同大學，由稱作長老或教士的牧師及信徒領導。嚴格來說，所有長老教會皆為歸正派或喀爾文教派傳統的一部分，但並非所有歸正教會的管理方式皆如同長老教會一般。"@zh-hant ;
    skos:inScheme cwrc:Religion ;
    prov:derivedFrom <http://vocab.getty.edu/aat/300153854> .

cwrc:professional
    void:inDataset cwrc:datasetdefinition ;
    a cwrc:SocialClassIdentity, skos:Concept ;
    rdfs:isDefinedBy <http://www.cwrc.ca/ontologies/cwrc#> ;
    rdfs:label "professional"@en, "professionnel"@fr ;
    owl:subClass cwrc:CulturalFormation ;
    skos:definition ""@fr, "Includes doctors, lawyers, guild members, and those of high calling such as members of the clergy (Church of England). It implies social respect and intellectual requirements. Examples are Ann Hunter, who was married to a surgeon, and Virginia Woolf, daughter of an intellectual."@en .

cwrc:protestantism
    void:inDataset cwrc:datasetdefinition ;
    a cwrc:Religion, skos:Concept ;
    rdfs:isDefinedBy <http://www.cwrc.ca/ontologies/cwrc#> ;
    rdfs:label "Protestantism"@en, "hsin chiao"@zh-latn-wadegile, "protestant"@nl, "protestantisme"@fr, "protestantisme"@nl, "protestantismo"@es, "xin jiao"@zh-latn-pinyin-x-notone, "xīn jiāo"@zh-latn-pinyin-x-hanyu, "抗羅宗"@zh-hant, "新教"@zh-hant ;
    skos:broaderTransitive cwrc:christianity ;
    skos:definition ""@fr, "De algemene term voor typen christelijk geloof die zijn ontstaan tijdens de Reformatie. Hoewel de vroegste vormen van protestantisme werden beoefend door de volgelingen van Luther, Calvijn en Zwingli, wordt de term tegenwoordig gebruikt voor de meeste overtuigingen die niet rooms-katholiek of orthodox zijn. Protestanten willen dichter bij de geloofsstijl van de vroege kerk staan, die volgens hen in de katholieke praktijk overschaduwd is geraakt. De term is afkomstig van het woord 'protestari', wat niet alleen 'protesteren' betekent, maar ook 'belijden'. Enkele algemene kenmerken van het protestantisme zijn: rechtvaardiging door het geloof alleen, de berusting van alle gezag bij de Bijbel en de leer dat alle gelovigen zelf hun zonden aan God kunnen belijden, waarbij het aanhoren van de biecht niet alleen aan priesters is voorbehouden."@nl, "El término general para tipos de fe cristiana originadas a partir de la Reforma. Aunque las formas tempranas del protestantismo fueron aquellas que obedecían a Lutero, Calvino y Zwinglio, el término ahora incluye la mayoría de las denominaciones no Romanas o no Ortodoxas. El caracter común de los protestantes incluye la justificación de la fe por la fe, la autoridad de la sagrada escritura  y el sacerdocio de todos los fieles, por el que cada creyente puede oir la confesión de los pecados, no siendo exclusivo del clero. protestantes quieren estar cerca al estilo de fe de la primera Iglesia el cual sienten ha sido opacado en las prácticas católicas. El término deriva desde la palabra \"protestari\" que significa no sólo protestar sino que reconocer o confesar. Característica común."@es, "The general term for types of Christian faith originating from the Reformation. Although the early forms of Protestantism were those who followed Luther, Calvin, and Zwingli, the term now includes most non-Roman Catholic or non-Orthodox denominations. Protestants want to be closer to the style of faith of the early Church which they feel has been obscured in Catholic practices. The term derives from the word 'protestari' which means not only to protest but to avow or confess. Common characteristics of Protestantism include the justification by faith alone, the authority of scripture, and the priesthood of all believers, in which not only the clergy are able to hear the confession of sin."@en, "泛稱源自宗教改革的各式基督信仰。雖然早期的新教形式是指遵循路德(Luther)、喀爾文(Calvin)，以及茨溫利(Zwingli)的派別，但現在新教這個詞彙包含了大部分非羅馬天主教或非正教的派別。新教徒希望能更接近早期教會信仰，認為天主教將之變得晦澀難解。本詞彙衍生自”protestari”，不僅意指抗議，更要坦白或懺悔。新教的常見特色包括因純信而稱義、經典的權威性、信徒皆牧師，所以不是只有牧師才能聽取認罪懺悔。 "@zh-hant ;
    skos:inScheme cwrc:Religion ;
    prov:derivedFrom <http://vocab.getty.edu/aat/300073735> .

cwrc:quakers
    void:inDataset cwrc:datasetdefinition ;
    a cwrc:Religion, skos:Concept ;
    rdfs:isDefinedBy <http://www.cwrc.ca/ontologies/cwrc#> ;
    rdfs:label "Quaker"@en, "quaker"@fr ;
    skos:broaderTransitive cwrc:churchOfEngland, cwrc:dissenters ;
    skos:definition "Het Religieus Genootschap der Vrienden, beter bekend als quakers, verouderd Nederlands kwakers, vormt een groep ondogmatische gelovigen, die zijn wortels vindt in de christelijke traditie. Het leven en de overgeleverde uitspraken van Jezus vormen een belangrijke inspiratiebron."@nl, "La Société religieuse des Amis est un mouvement religieux fondé en Angleterre au XVIIe siècle par des dissidents de l'Église anglicane. Les membres de ce mouvement sont communément connus sous le nom de quakers () mais ils se nomment entre eux « Amis » et « Amies ». Le mouvement est souvent nommé simplement Société des Amis et le surnom de « quaker » apparaît le plus souvent dans la dénomination officielle, sous la forme Société religieuse des Amis (quakers). Les historiens s'accordent à désigner George Fox comme le principal fondateur ou le plus important meneur des débuts du mouvement. Depuis sa création en Angleterre, le mouvement s'est d'abord répandu dans les pays de colonisation anglo-saxonne. Au XXe siècle, des missionnaires quakers ont propagé leur religion en Amérique latine et en Afrique. Aujourd'hui, les quakers déclarent être au nombre d'environ 350 000 dans le monde. La Société des Amis se différencie de la plupart des autres groupes issus du christianisme par l'absence de credo et de toute structure hiérarchique. Pour les quakers, la croyance religieuse appartient à la sphère personnelle et chacun est libre de ses convictions. Le concept de « lumière intérieure » (inner light) est cependant partagé par la plupart d'entre eux, quelle que soit la signification donnée à ces mots. De nombreux quakers reconnaissent le christianisme mais ne ressentent pas leur foi comme entrant dans les catégories chrétiennes traditionnelles. On trouve aujourd'hui dans la Société des Amis des pratiques très diverses, y compris un large courant évangélique."@fr, "Quakers (or Friends) are members of a group of religious Christian movements which is known as the Religious Society of Friends in Europe, Australia, New Zealand and parts of North America; and known as the Friends Church in Africa, Asia, South America and parts of the US. The movements were originally, and are still predominantly based on Christianity. Members of the movements profess the priesthood of all believers, a doctrine derived from the First Epistle of Peter. They include those with evangelical, holiness, liberal, and traditional Quaker understandings of Christianity. To differing extents, the different movements that make up the Religious Society of Friends/Friends Church avoid creeds and hierarchical structures. In 2007, there were approximately 359,000 adult Quakers."@en ;
    skos:inScheme cwrc:Religion ;
    prov:derivedFrom <http://dbpedia.org/page/Quakers> .

cwrc:rationalDissenter
    void:inDataset cwrc:datasetdefinition ;
    a cwrc:Religion, skos:Concept ;
    rdfs:isDefinedBy <http://www.cwrc.ca/ontologies/cwrc#> ;
    rdfs:label ""@fr, "Rational Dissenter"@en ;
    skos:broaderTransitive cwrc:dissenters ;
    skos:definition ""@en, ""@fr ;
    skos:inScheme cwrc:Religion .

cwrc:rural-unskilled
    void:inDataset cwrc:datasetdefinition ;
    a cwrc:SocialClassIdentity, skos:Concept ;
    rdfs:isDefinedBy <http://www.cwrc.ca/ontologies/cwrc#> ;
    rdfs:label "rural - journalier"@fr, "rural-unskilled"@en ;
    owl:subClass cwrc:CulturalFormation ;
    skos:definition ""@fr, "This generally indicates farm laborers, mostly male in earlier periods, and includes migrant farm workers."@en .

cwrc:servants
    void:inDataset cwrc:datasetdefinition ;
    a cwrc:SocialClassIdentity, skos:Concept ;
    rdfs:isDefinedBy <http://www.cwrc.ca/ontologies/cwrc#> ;
    rdfs:label "servant"@fr, "servants"@en ;
    owl:subClass cwrc:CulturalFormation ;
    skos:definition ""@fr, "Domestic servants typically live in the home with the family or institution that employs them, although the lowest class of servants might work only casually and hence not receive room and board. This type of labour, very common before the twentieth century, is distinct from that of service positions such as shop assistants, flight attendances, and restaurant workers."@en .

cwrc:shopkeepers
    void:inDataset cwrc:datasetdefinition ;
    a cwrc:SocialClassIdentity, skos:Concept ;
    rdfs:isDefinedBy <http://www.cwrc.ca/ontologies/cwrc#> ;
    rdfs:label "Typically applied to someonw who owns and runs a pub or shop, but not on the scale of an entrepreneur or industrialist."@en, "détaillant"@fr ;
    owl:subClass cwrc:CulturalFormation ;
    skos:definition ""@fr, "Owns and runs a pub or shop. Similar to an industrialist but to a lesser degree of magnitude."@en .

cwrc:skilledCraftpersonArtisan
    void:inDataset cwrc:datasetdefinition ;
    a cwrc:SocialClassIdentity, skos:Concept ;
    rdfs:isDefinedBy <http://www.cwrc.ca/ontologies/cwrc#> ;
    rdfs:label "Artisan"@fr, "This category includes such trades as goldsmith, tailor, shoemaker, milliner, and dressmaker."@en ;
    owl:subClass cwrc:CulturalFormation ;
    skos:definition ""@fr, "Goldsmith, tailor, shoemaker, milliner, dressmaker."@en .

cwrc:societyOfFriends
    void:inDataset cwrc:datasetdefinition ;
    a cwrc:Religion, skos:Concept ;
    rdfs:isDefinedBy <http://www.cwrc.ca/ontologies/cwrc#> ;
    rdfs:label "Society of Friends"@en, "Société religieuse des Amis"@fr ;
    skos:broaderTransitive cwrc:christianity ;
    skos:definition ""@en, ""@fr ;
    skos:inScheme cwrc:Religion .

cwrc:spiritualism
    void:inDataset cwrc:datasetdefinition ;
    a cwrc:Religion, skos:Concept ;
    rdfs:isDefinedBy <http://www.cwrc.ca/ontologies/cwrc#> ;
    rdfs:label "Spiritualism"@en, "spiritualisme"@fr ;
    rdfs:subClassOf <http://dbpedia.org/page/Spiritualism> ;
    skos:broaderTransitive cwrc:occultism ;
    skos:definition ""@en, ""@fr ;
    skos:inScheme cwrc:Religion .

cwrc:sshrc
    a foaf:Organization ;
    foaf:name "Conseil de recherches en sciences humaines"@fr, "Social Sciences and Humanities Research Council"@en ;
    foaf:nick "SSHRC" .

cwrc:tractarianMovement
    void:inDataset cwrc:datasetdefinition ;
    a cwrc:Religion, skos:Concept ;
    rdfs:isDefinedBy <http://www.cwrc.ca/ontologies/cwrc#> ;
    rdfs:label "Tractarian Movement"@en, "tractarianisme"@fr ;
    rdfs:subClassOf <http://dbpedia.org/page/Oxford_Movement> ;
    skos:broaderTransitive cwrc:churchOfEngland ;
    skos:definition ""@en, ""@fr ;
    skos:inScheme cwrc:Religion .

cwrc:unitarianChurch
    void:inDataset cwrc:datasetdefinition ;
    a cwrc:Religion, skos:Concept ;
    rdf:value "unitarianChurch" ;
    rdfs:isDefinedBy <http://www.cwrc.ca/ontologies/cwrc#> ;
    rdfs:label "Unitarian Church"@en, "l'Église unitarienne"@fr ;
    skos:broaderTransitive cwrc:christianity ;
    skos:definition ""@en, ""@fr .

cwrc:unitarianism
    void:inDataset cwrc:datasetdefinition ;
    a cwrc:Religion, skos:Concept ;
    rdf:value "unitarianMovement" ;
    rdfs:isDefinedBy <http://www.cwrc.ca/ontologies/cwrc#> ;
    rdfs:label "Unitarianism"@en, "l'unitarisme"@fr, "unitarios"@es, "unitarisme"@nl, "unitarismo"@es ;
    rdfs:subClassOf <http://dbpedia.org/page/Unitarianism> ;
    skos:altLabel "Unitarian"@en, "Unitarian Movement"@en ;
    skos:broaderTransitive cwrc:protestantism ;
    skos:definition ""@fr, "In het bijzonder te gebruiken voor de vrijzinnig protestantse beweging die in Europa opkwam tijdens de Reformatie in de 16de eeuw, werd belichaamd door een kerk in Transsylvanië en een confessionele status verkreeg in Groot-Brittannië, de Verenigde Staten en Canada tijdens de 19de eeuw. De beweging wordt gekenmerkt door de afwijzing van de orthodox christelijke leer van de Drie-eenheid en de goddelijke Christus, het vrije gebruik van de rede in religieuze zaken en het geloof dat God bestaat in één persoon. In 1961 fuseerde deze beweging in de Verenigde Staten en Canada met de universalistische beweging, waardoor het ‘unitaristisch universalisme’ ontstond. Ook in het algemeen te gebruiken voor de theologische leer van de eenheid van God en het mens-zijn van Jezus, zoals voor het eerst verwoord in het monarchisme van de 2de en 3de eeuw en in de leer van Arius in de 3de en 4de eeuw, en later in de leer van de radicale neoplatonisten uit de Reformatie zoals Michael Servetus, Faustus Socinus en Ferenc David."@nl, "The liberal Protestant movement that arose in Europe during the 16th century Reformation, was embodied in a church in Transylvania, and achieved denominational status in the 19th century in the United Kingdom, the United States, and Canada. It is characterized by a denial of the orthodox Christian doctrines of the Trinity and the divinity of Jesus, the free use of reason in religion, and the belief that God exists in one person. In 1961, in the United States and Canada, it merged with the Universalist denomination to form \"Unitarian Universalism.\"  Use also generally for the theological doctrines of the unified nature of God and the humanity of Jesus, first expressed in second- and third-century monarchism and in the teachings of Arius in the third and fourth centuries, and later in the radical Neoplatonist thinkers of the Reformation such as Michael Servetus, Faustus Socinus, and Ferenc David."@en, "Úsese específicamente para el movimiento protestante liberal que surgió en Europa durante la Reforma del siglo XVI, que tuvo su manifestación en una iglesia en Transilvania, y que logró un estatus confesional en el siglo XIX en el Reino Unido, los Estados Unidos y Canadá. Es caracterizado por una desaprobación de las doctrinas cristianas ortodoxas de la Trinidad y la divinidad de Jesús, el libre uso de la razón en la religión y la creencia que Dios existe en una persona. En 1961, en los Estados Unidos y Canadá s"@es ;
    skos:inScheme cwrc:Religion ;
    prov:derivedFrom <http://vocab.getty.edu/aat/300263305> .

cwrc:unknownSex
    void:inDataset cwrc:datasetdefinition ;
    a cwrc:SexIdentity, skos:Concept ;
    rdfs:isDefinedBy <http://www.cwrc.ca/ontologies/cwrc#> ;
    rdfs:label "Inconnue"@fr, "Unknown"@en ;
    skos:definition ""@en, ""@fr ;
    foaf:name "Unknown (Sex)"@en .

cwrc:upper-middleClass
    void:inDataset cwrc:datasetdefinition ;
    a cwrc:SocialClassIdentity, skos:Concept ;
    rdfs:isDefinedBy <http://www.cwrc.ca/ontologies/cwrc#> ;
    rdfs:label "classe haute moyenne"@fr, "upper middle class"@en ;
    owl:comment "This term is a CWRC specific addition not in the original Orlando tag set."@en ;
    owl:subClass cwrc:CulturalFormation ;
    skos:definition ""@en, ""@fr .

cwrc:urban-industrialUnskilled
    void:inDataset cwrc:datasetdefinition ;
    a cwrc:SocialClassIdentity, skos:Concept ;
    rdfs:isDefinedBy <http://www.cwrc.ca/ontologies/cwrc#> ;
    rdfs:label "This category includes factory workers and workers in urban or large-scale industries without defined trades or professional qualifications, and those in low-wage and low-status service sector jobs, such as the restaurant or fast-food industry, in industrial or post-industrial societies."@en, "Urbain - industriel - ouvrier non spécialisé"@fr ;
    owl:subClass cwrc:CulturalFormation ;
    skos:definition ""@en, ""@fr .

cwrc:whiteEthnicity
    void:inDataset cwrc:datasetdefinition ;
    a cwrc:Ethnicity, owl:Thing ;
    rdfs:isDefinedBy <http://www.cwrc.ca/ontologies/cwrc#> ;
    rdfs:label "blanc"@fr, "white"@en ;
    rdfs:subClass cwrc:whiteLabel ;
    skos:definition ""@en, ""@fr ;
    foaf:name "White (Ethnicity)"@en .

cwrc:whiteLabel
    void:inDataset cwrc:datasetdefinition ;
    a skos:Concept, skosxl:Label ;
    rdfs:isDefinedBy <http://www.cwrc.ca/ontologies/cwrc#> ;
    rdfs:label "blanc"@fr, "white"@en ;
    owl:oneOf (cwrc:whiteEthnicity
        cwrc:whiteRace
    ) ;
    skos:definition ""@en, ""@fr ;
    skos:inScheme cwrc:TextLabels ;
    foaf:name "white"@en .

cwrc:whiteRace
    void:inDataset cwrc:datasetdefinition ;
    a cwrc:RaceColour, owl:Thing, skos:Concept ;
    rdfs:isDefinedBy <http://www.cwrc.ca/ontologies/cwrc#> ;
    rdfs:label "blanc"@fr, "white"@en ;
    rdfs:subClass cwrc:whiteLabel ;
    skos:definition ""@en, ""@fr ;
    foaf:name "White (Race Colour)"@en .

cwrc:womanLabel
    void:inDataset cwrc:datasetdefinition ;
    a skos:Concept, skosxl:Label ;
    rdf:value "woman" ;
    rdfs:isDefinedBy <http://www.cwrc.ca/ontologies/cwrc#> ;
    rdfs:label "Femme"@fr, "Woman"@en ;
    owl:oneOf (cwrc:genderWomanFemale
    ) ;
    skos:definition ""@en, ""@fr ;
    skos:inScheme cwrc:TextLabels ;
    foaf:name "Woman (Label)"@en .

cwrc:yeoman-farmer
    void:inDataset cwrc:datasetdefinition ;
    a cwrc:SocialClassIdentity, skos:Concept ;
    rdfs:isDefinedBy <http://www.cwrc.ca/ontologies/cwrc#> ;
    rdfs:label "Members of this historica class owned just enough land to support themselves if they did most of the work themselves. Examples include Elizabeth Ham and Mary Webb."@en, "agriculteur vivrier"@fr ;
    owl:subClass cwrc:CulturalFormation ;
    skos:definition ""@fr, "Own just enough land to support themselves if they do most of the work themselves (ie Elizabeth Ham, Mary Webb)."@en .

prov:derivedFrom
    rdfs:range cwrc:Context .

[]
    a rdf:value .

