@prefix dc: <http://purl.org/dc/elements/1.1/> .
@prefix geo: <http://www.w3.org/2003/01/geo/wgs84_pos#> .
@prefix mo: <http://purl.org/ontology/mo/> .
@prefix foaf: <http://xmlns.com/foaf/0.1/> .
@prefix frbr: <http://purl.org/vocab/frbr/core#> .
@prefix keys: <http://purl.org/NET/c4dm/keys.owl#> .
@prefix vs: <http://www.w3.org/2003/06/sw-vocab-status/ns#> .
@prefix dcterms: <http://purl.org/dc/terms/> .
@prefix wot: <http://xmlns.com/wot/0.1/> .
@prefix rdfs: <http://www.w3.org/2000/01/rdf-schema#> .
@prefix time: <http://www.w3.org/2006/time#> .
@prefix ao: <http://purl.org/ontology/ao/core#> .
@prefix bio: <http://purl.org/vocab/bio/0.1/> .
@prefix event: <http://purl.org/NET/c4dm/event.owl#> .
@prefix xsd: <http://www.w3.org/2001/XMLSchema#> .
@prefix owl: <http://www.w3.org/2002/07/owl#> .
@prefix rdf: <http://www.w3.org/1999/02/22-rdf-syntax-ns#> .
@prefix cc: <http://web.resource.org/cc/> .

<http://purl.org/ontology/mo/> a owl:Ontology ;
	dc:created "2006/12/21 12:00:00" ;
	dc:date "2013/07/22 16:54:19" ;
	dc:description "\n        The Music Ontology Specification provides main concepts and \n        properties fo describing music (i.e. artists, albums and tracks) \n        on the Semantic Web. \n    " ;
	dc:title "The Music Ontology" ;
	owl:imports <http://purl.org/vocab/bio/0.1/> , <http://purl.org/NET/c4dm/event.owl> , <http://purl.org/ontology/ao/core> , <http://www.w3.org/2006/time> , <http://xmlns.com/foaf/0.1/> , <http://purl.org/dc/terms/> , <http://purl.org/NET/c4dm/keys.owl> , <http://purl.org/vocab/frbr/core> ;
	owl:versionInfo "Revision: 2.1.5" ;
	foaf:maker <http://raimond.me.uk/foaf.rdf#moustaki> , <http://foaf.me/zazi#me> , <http://www.talkdigger.com/foaf/fgiasson> , <http://kurtisrandom.com/foaf.rdf#kurtjx> .

_:node1866aqtmex163 foaf:name "George Fazekas" .

<http://purl.org/ontology/mo/> foaf:maker _:node1866aqtmex163 .

_:node1866aqtmex164 foaf:name "Simon Reinhardt" ;
	foaf:homepage <http://simon-reinhardt.de/> .

<http://purl.org/ontology/mo/> foaf:maker _:node1866aqtmex164 .

_:node1866aqtmex165 foaf:name "Alexandre Passant" ;
	foaf:homepage <http://apassant.net/> .

<http://purl.org/ontology/mo/> foaf:maker _:node1866aqtmex165 .

<http://raimond.me.uk/foaf.rdf#moustaki> foaf:name "Yves Raimond" ;
	foaf:homepage <http://raimond.me.uk/> .

<http://foaf.me/zazi#me> foaf:name "Thomas Gängler" ;
	foaf:homepage <http://smiy.wordpress.com/> .

<http://www.talkdigger.com/foaf/fgiasson> foaf:name "Frédérick Giasson" ;
	foaf:homepage <http://fgiasson.com/> .

<http://kurtisrandom.com/foaf.rdf#kurtjx> foaf:name "Kurt Jacobson" ;
	foaf:homepage <http://kurtisrandom.com/> .

mo:Activity a owl:Class ;
	rdfs:comment "\n        An activity period, defining when an artist was musically active.\n    " ;
	rdfs:isDefinedBy <http://purl.org/ontology/mo/> ;
	rdfs:label "activity" ;
	rdfs:subClassOf event:Event ;
	mo:level "1" ;
	vs:term_status "testing" .

mo:AnalogSignal a owl:Class ;
	rdfs:comment "\n        An analog signal.\n    " ;
	rdfs:isDefinedBy <http://purl.org/ontology/mo/> ;
	rdfs:label "analogue signal" ;
	rdfs:subClassOf mo:Signal ;
	mo:level "2" ;
	owl:disjointWith mo:DigitalSignal ;
	vs:term_status "stable" .

mo:Arrangement a owl:Class ;
	rdfs:comment "\n        An arrangement event.\n        Takes as agent the arranger, and produces a score (informational object, not the actually published score).\n    " ;
	rdfs:isDefinedBy <http://purl.org/ontology/mo/> ;
	rdfs:label "arrangement" ;
	rdfs:subClassOf event:Event ;
	mo:level "2" ;
	vs:term_status "stable" .

mo:Arranger a owl:Class ;
	rdfs:label "arranger" ;
	rdfs:subClassOf foaf:Agent ;
	mo:level "2" .

_:node1866aqtmex166 a owl:Restriction ;
	owl:onProperty event:isAgentIn ;
	owl:someValuesFrom mo:Arrangement .

mo:Arranger owl:equivalentClass _:node1866aqtmex166 ;
	vs:term_status "unstable" .

mo:AudioFile a owl:Class ;
	rdfs:comment "An audio file, which may be available on a local file system or through http, ftp, etc." ;
	rdfs:isDefinedBy <http://purl.org/ontology/mo/> ;
	rdfs:label "audio file" ;
	rdfs:subClassOf mo:Medium , foaf:Document ;
	mo:level "1" ;
	vs:term_status "unstable" .

mo:CD a owl:Class ;
	rdfs:comment "Compact Disc used as medium to record a musical manifestation." ;
	rdfs:isDefinedBy <http://purl.org/ontology/mo/> ;
	rdfs:label "CD" ;
	rdfs:subClassOf mo:Medium ;
	mo:level "1" ;
	vs:term_status "unstable" .

mo:Composer a owl:Class ;
	rdfs:label "composer" ;
	rdfs:subClassOf foaf:Agent ;
	mo:level "2" .

_:node1866aqtmex167 a owl:Restriction ;
	owl:onProperty event:isAgentIn ;
	owl:someValuesFrom mo:Composition .

mo:Composer owl:equivalentClass _:node1866aqtmex167 ;
	vs:term_status "unstable" .

mo:Composition a owl:Class ;
	rdfs:comment "\n        A composition event.\n        Takes as agent the composer himself.\n        It produces a MusicalWork, or a MusicalExpression (when the initial \"product\" is a score, for example), or both...\n    " ;
	rdfs:isDefinedBy <http://purl.org/ontology/mo/> ;
	rdfs:label "composition" ;
	rdfs:subClassOf event:Event ;
	mo:level "2" ;
	vs:term_status "stable" .

mo:Conductor a owl:Class ;
	rdfs:label "conductor" ;
	rdfs:subClassOf foaf:Agent ;
	mo:level "2" .

_:node1866aqtmex168 a owl:Restriction ;
	owl:onProperty mo:conducted ;
	owl:someValuesFrom mo:Performance .

mo:Conductor owl:equivalentClass _:node1866aqtmex168 ;
	vs:term_status "unstable" .

mo:CorporateBody a owl:Class ;
	rdfs:comment "Organization or group of individuals and/or other organizations involved in the music market." ;
	rdfs:isDefinedBy <http://purl.org/ontology/mo/> ;
	rdfs:label "corporate body" ;
	rdfs:subClassOf foaf:Organization ;
	mo:level "1" ;
	vs:term_status "stable" .

mo:DAT a owl:Class ;
	rdfs:comment "Digital Audio Tape used as medium to record a musical manifestation." ;
	rdfs:isDefinedBy <http://purl.org/ontology/mo/> ;
	rdfs:label "DAT" ;
	rdfs:subClassOf mo:Medium ;
	mo:level "1" ;
	vs:term_status "unstable" .

mo:DCC a owl:Class ;
	rdfs:comment "Digital Compact Cassette used as medium to record a musical manifestation." ;
	rdfs:isDefinedBy <http://purl.org/ontology/mo/> ;
	rdfs:label "DCC" ;
	rdfs:subClassOf mo:Medium ;
	mo:level "1" ;
	vs:term_status "unstable" .

mo:DVDA a owl:Class ;
	rdfs:comment "DVD-Audio used as medium to record a musical manifestation." ;
	rdfs:isDefinedBy <http://purl.org/ontology/mo/> ;
	rdfs:label "DVDA" ;
	rdfs:subClassOf mo:Medium ;
	mo:level "1" ;
	vs:term_status "unstable" .

mo:DigitalSignal a owl:Class ;
	rdfs:comment "\n        A digital signal\n    " ;
	rdfs:isDefinedBy <http://purl.org/ontology/mo/> ;
	rdfs:label "digital signal" ;
	rdfs:subClassOf mo:Signal ;
	mo:level "2" ;
	owl:disjointWith mo:AnalogSignal ;
	vs:term_status "stable" .

mo:ED2K a owl:Class ;
	rdfs:comment "Something available on the E-Donkey peer-2-peer filesharing network" ;
	rdfs:isDefinedBy <http://purl.org/ontology/mo/> ;
	rdfs:label "ED2K" ;
	rdfs:subClassOf mo:Medium ;
	mo:level "1" ;
	vs:term_status "unstable" .

mo:Festival a owl:Class ;
	rdfs:comment "\n        A festival - musical/artistic event lasting several days, like Glastonbury, Rock Am Ring...\n        We migth decompose this event (which is in fact just a classification of the space/time region related to \n        a particular festival) using hasSubEvent in several performances at different space/time.\n    " ;
	rdfs:isDefinedBy <http://purl.org/ontology/mo/> ;
	rdfs:label "Festival" ;
	rdfs:subClassOf event:Event ;
	mo:level "2" ;
	vs:term_status "stable" .

mo:Genre a owl:Class ;
	rdfs:comment "\n        An expressive style of music.\n        \n        Any taxonomy can be plug-in here. You can either define a genre by yourself, like this:\n\n        :mygenre a mo:Genre; dc:title \"electro rock\".\n\n        Or you can refer to a DBPedia genre (such as http://dbpedia.org/resource/Baroque_music), allowing semantic web\n        clients to access easily really detailed structured information about the genre you are refering to.\n    " ;
	rdfs:isDefinedBy <http://purl.org/ontology/mo/> ;
	rdfs:label "Genre" ;
	mo:level "2" ;
	vs:term_status "stable" .

mo:Instrument a owl:Class ;
	rdfs:comment "\n        Any of various devices or contrivances that can be used to produce musical tones or sound.\n        \n        Any taxonomy can be used to subsume this concept. The default one is one extracted by Ivan Herman\n        from the Musicbrainz instrument taxonomy, conforming to SKOS. This concept holds a seeAlso link \n        towards this taxonomy.\n    " ;
	rdfs:isDefinedBy <http://purl.org/ontology/mo/> ;
	rdfs:label "Instrument" ;
	rdfs:seeAlso <http://purl.org/ontology/mo/mit#> ;
	mo:level "2" ;
	vs:term_status "stable" .

mo:Instrumentation a owl:Class ;
	rdfs:comment "\n        Instrumentation deals with the techniques of writing music for a specific instrument, \n        including the limitations of the instrument, playing techniques and idiomatic handling of the instrument.\n    " ;
	rdfs:isDefinedBy <http://purl.org/ontology/mo/> ;
	rdfs:label "instrumentation" ;
	rdfs:subClassOf mo:Arrangement ;
	mo:level "2" ;
	vs:term_status "stable" .

mo:Label a owl:Class ;
	rdfs:comment "Trade name of a company that produces musical works or expression of musical works." ;
	rdfs:isDefinedBy <http://purl.org/ontology/mo/> ;
	rdfs:label "label" ;
	rdfs:subClassOf mo:CorporateBody ;
	mo:level "1" ;
	vs:term_status "stable" .

mo:Libretto a owl:Class ;
	rdfs:comment "\n                Libretto\n        " ;
	rdfs:isDefinedBy <http://purl.org/ontology/mo/> ;
	rdfs:label "libretto" ;
	rdfs:subClassOf mo:MusicalExpression ;
	mo:level "2" ;
	vs:term_status "stable" .

mo:Listener a owl:Class ;
	rdfs:label "listened" ;
	rdfs:subClassOf foaf:Agent ;
	mo:level "2" .

_:node1866aqtmex169 a owl:Restriction ;
	owl:onProperty mo:listened ;
	owl:someValuesFrom mo:Performance .

mo:Listener owl:equivalentClass _:node1866aqtmex169 ;
	vs:term_status "unstable" .

mo:Lyrics a owl:Class ;
	rdfs:comment "\n        Lyrics\n    " ;
	rdfs:isDefinedBy <http://purl.org/ontology/mo/> ;
	rdfs:label "lyrics" ;
	rdfs:subClassOf mo:MusicalExpression ;
	mo:level "2" ;
	vs:term_status "stable" .

mo:MD a owl:Class ;
	rdfs:comment "Mini Disc used as medium to record a musical manifestation." ;
	rdfs:isDefinedBy <http://purl.org/ontology/mo/> ;
	rdfs:label "MD" ;
	rdfs:subClassOf mo:Medium ;
	mo:level "1" ;
	vs:term_status "unstable" .

mo:MagneticTape a owl:Class ;
	rdfs:comment "Magnetic analogue tape used as medium to record a musical manifestation." ;
	rdfs:isDefinedBy <http://purl.org/ontology/mo/> ;
	rdfs:label "MagneticTape" ;
	rdfs:subClassOf mo:Medium ;
	mo:level "1" ;
	vs:term_status "unstable" .

mo:Medium a owl:Class ;
	rdfs:comment "A means or instrumentality for storing or communicating musical manifestation." ;
	rdfs:isDefinedBy <http://purl.org/ontology/mo/> ;
	rdfs:label "Medium" ;
	rdfs:subClassOf mo:MusicalItem ;
	mo:level "1" ;
	vs:term_status "unstable" .

mo:Membership a owl:Class ;
	rdfs:comment "A membership event, where one or several people belongs to a group during a particular time period." ;
	rdfs:isDefinedBy <http://purl.org/ontology/mo/> ;
	rdfs:label "membership" ;
	rdfs:subClassOf event:Event ;
	mo:level "1" ;
	vs:term_status "testing" .

mo:Movement a owl:Class ;
	rdfs:comment """A movement is a self-contained part of a musical work. While individual or selected movements from a composition are sometimes performed separately, a performance of the complete work requires all the movements to be performed in succession.

Often a composer attempts to interrelate the movements thematically, or sometimes in more subtle ways, in order that the individual
movements exert a cumulative effect. In some forms, composers sometimes link the movements, or ask for them to be played without a
pause between them.
    """ ;
	rdfs:isDefinedBy <http://purl.org/ontology/mo/> ;
	rdfs:label "movement" ;
	rdfs:subClassOf mo:MusicalWork ;
	mo:level "2" ;
	vs:term_status "unstable" .

mo:MusicArtist a owl:Class ;
	rdfs:comment "\n        A person or a group of people (or a computer :-) ), whose musical \n        creative work shows sensitivity and imagination \n    " ;
	rdfs:isDefinedBy <http://purl.org/ontology/mo/> ;
	rdfs:label "music artist" ;
	rdfs:subClassOf foaf:Agent ;
	mo:level "1" ;
	vs:term_status "stable" .

mo:MusicGroup a owl:Class ;
	rdfs:comment "Group of musicians, or musical ensemble, usually popular or folk, playing parts of or improvising off of a musical arrangement. " ;
	rdfs:isDefinedBy <http://purl.org/ontology/mo/> ;
	rdfs:label "music group" ;
	rdfs:subClassOf foaf:Group , mo:MusicArtist ;
	mo:level "1" ;
	vs:term_status "stable" .

mo:MusicalExpression a owl:Class ;
	rdfs:comment "\nThe intellectual or artistic realization of a work in the form of alpha-numeric, musical, or choreographic notation, sound, etc., or any combination of such forms.    \n\n\nFor example:\n\nWork #1 Franz Schubert's Trout quintet\n\n    * Expression #1 the composer's score\n    * Expression #2 sound issued from the performance by the Amadeus Quartet and Hephzibah Menuhin on piano\n    * Expression #3 sound issued from the performance by the Cleveland Quartet and Yo-Yo Ma on the cello\n    * . . . . \n\nThe Music Ontology defines the following sub-concepts of a MusicalExpression, which should be used instead of MusicalExpression itself: Score (the\nresult of an arrangement), Sound (produced during a performance), Signal. However, it is possible to stick to FRBR and bypass the worflow\nmechanism this ontology defines by using the core FRBR properties on such objects. But it is often better to use events to interconnect such \nexpressions (allowing to go deeply into the production process - `this performer was playing this particular instrument at that\nparticular time').\n    \n    " ;
	rdfs:isDefinedBy <http://purl.org/ontology/mo/> ;
	rdfs:label "musical expression" ;
	rdfs:subClassOf frbr:Expression ;
	mo:level "1" ;
	vs:term_status "unstable" .

mo:MusicalItem a owl:Class ;
	rdfs:comment """A single exemplar of a musical expression.
    
For example, it could be a single exemplar of a CD. This is normally an single object (a CD) possessed by somebody.

From the FRBR final report: The entity defined as item is a concrete entity. It is in many instances a single physical object (e.g., a copy of a one-volume monograph, a single audio cassette, etc.). There are instances, however, where the entity defined as item comprises more than one physical object (e.g., a monograph issued as two separately bound volumes, a recording issued on three separate compact discs, etc.).

In terms of intellectual content and physical form, an item exemplifying a manifestation is normally the same as the manifestation itself. However, variations may occur from one item to another, even when the items exemplify the same manifestation, where those variations are the result of actions external to the intent of the producer of the manifestation (e.g., damage occurring after the item was produced, binding performed by a library, etc.). 
    """ ;
	rdfs:isDefinedBy <http://purl.org/ontology/mo/> ;
	rdfs:label "MusicalItem" ;
	mo:level "1" ;
	vs:term_status "unstable" .

mo:MusicalManifestation a owl:Class ;
	rdfs:comment "\n\nThis entity is related to the edition/production/publication of a musical expression (musical manifestation are closely related with the music industry (their terms, concepts, definitions, methods (production, publication, etc.), etc.)\n    \nFrom the FRBR final report: The entity defined as manifestation encompasses a wide range of materials, including manuscripts, books, periodicals, maps, posters, sound recordings, films, video recordings, CD-ROMs, multimedia kits, etc. As an entity, manifestation represents all the physical objects that bear the same characteristics, in respect to both intellectual content and physical form.\n\n\nWork #1 J. S. Bach's Six suites for unaccompanied cello\n\n    * Expression #1 sound issued during the performance by Janos Starker recorded in 1963 and 1965\n          o Manifestation #1 recordings released on 33 1/3 rpm sound discs in 1965 by Mercury\n          o Manifestation #2 recordings re-released on compact disc in 1991 by Mercury \n    * Expression #2 sound issued during the performances by Yo-Yo Ma recorded in 1983\n          o Manifestation #1 recordings released on 33 1/3 rpm sound discs in 1983 by CBS Records\n          o Manifestation #2 recordings re-released on compact disc in 1992 by CBS Records \n\n          \nChanges that occur deliberately or even inadvertently in the production process that affect the copies result, strictly speaking, in a new manifestation. A manifestation resulting from such a change may be identified as a particular \"state\" or \"issue\" of the publication.\n\nChanges that occur to an individual copy after the production process is complete (e.g., the loss of a page, rebinding, etc.) are not considered to result in a new manifestation. That copy is simply considered to be an exemplar (or item) of the manifestation that deviates from the copy as produced.\n\nWith the entity defined as manifestation we can describe the physical characteristics of a set of items and the characteristics associated with the production and distribution of that set of items that may be important factors in enabling users to choose a manifestation appropriate to their physical needs and constraints, and to identify and acquire a copy of that manifestation.\n\nDefining manifestation as an entity also enables us to draw relationships between specific manifestations of a work. We can use the relationships between manifestations to identify, for example, the specific publication that was used to create a microreproduction.          \n\n" ;
	rdfs:isDefinedBy <http://purl.org/ontology/mo/> ;
	rdfs:label "musical manifestation" ;
	rdfs:subClassOf frbr:Manifestation ;
	mo:level "1" ;
	vs:term_status "stable" .

mo:MusicalWork a owl:Class ;
	rdfs:comment "\n    Distinct intellectual or artistic musical creation.\n    \nFrom the FRBR final report: A work is an abstract entity; there is no single material object one can point to as the work. We recognize the work through individual realizations or expressions of the work, but the work itself exists only in the commonality of\ncontent between and among the various expressions of the work. When we speak of Homer's Iliad as a work, our point of reference is not a particular recitation or text of the work, but the intellectual creation that lies behind all the various expressions of the work.     \n\nFor example:\n\nwork #1 J. S. Bach's The art of the fugue\n\n    \n    " ;
	rdfs:isDefinedBy <http://purl.org/ontology/mo/> ;
	rdfs:label "musical work" ;
	rdfs:subClassOf frbr:Work ;
	mo:level "2" ;
	vs:term_status "stable" .

mo:Orchestration a owl:Class ;
	rdfs:comment "\n            Orchestration includes, in addition to instrumentation, the handling of groups of instruments and their balance and interaction.\n    " ;
	rdfs:isDefinedBy <http://purl.org/ontology/mo/> ;
	rdfs:label "orchestration" ;
	rdfs:subClassOf mo:Arrangement ;
	mo:level "2" ;
	vs:term_status "stable" .

mo:Performance a owl:Class ;
	rdfs:comment "\n        A performance event. \n        It might include as agents performers, engineers, conductors, or even listeners.\n        It might include as factors a score, a MusicalWork, musical instruments. \n        It might produce a sound:-)\n    " ;
	rdfs:isDefinedBy <http://purl.org/ontology/mo/> ;
	rdfs:label "performance" ;
	rdfs:subClassOf event:Event ;
	mo:level "2" ;
	vs:term_status "stable" .

mo:Performer a owl:Class ;
	rdfs:label "performer" ;
	rdfs:subClassOf foaf:Agent ;
	mo:level "2" .

_:node1866aqtmex170 a owl:Restriction ;
	owl:onProperty mo:performed ;
	owl:someValuesFrom mo:Performance .

mo:Performer owl:equivalentClass _:node1866aqtmex170 ;
	vs:term_status "unstable" .

mo:PublishedLibretto a owl:Class ;
	rdfs:comment "A published libretto" ;
	rdfs:isDefinedBy <http://purl.org/ontology/mo/> ;
	rdfs:label "published libretto" ;
	rdfs:subClassOf mo:MusicalManifestation ;
	mo:level "2" ;
	vs:term_status "stable" .

mo:PublishedLyrics a owl:Class ;
	rdfs:comment "Published lyrics, as a book or as a text file, for example" ;
	rdfs:isDefinedBy <http://purl.org/ontology/mo/> ;
	rdfs:label "published lyrics" ;
	rdfs:subClassOf mo:MusicalManifestation ;
	mo:level "2" ;
	vs:term_status "stable" .

mo:PublishedScore a owl:Class ;
	rdfs:comment "A published score (subclass of MusicalManifestation)" ;
	rdfs:isDefinedBy <http://purl.org/ontology/mo/> ;
	rdfs:label "published score" ;
	rdfs:subClassOf mo:MusicalManifestation ;
	mo:level "2" ;
	vs:term_status "stable" .

mo:Record a owl:Class ;
	rdfs:comment "A published record (manifestation which first aim is to render the product of a recording)" ;
	rdfs:isDefinedBy <http://purl.org/ontology/mo/> ;
	rdfs:label "record" ;
	rdfs:subClassOf mo:MusicalManifestation ;
	mo:level "1" ;
	vs:term_status "stable" .

mo:Recording a owl:Class ;
	rdfs:comment "\n        A recording event.\n        Takes a sound as a factor to produce a signal (analog or digital).\n        The location of such events (if any) is the actual location of the corresponding\n        microphone or the \"recording device\".\n    " ;
	rdfs:isDefinedBy <http://purl.org/ontology/mo/> ;
	rdfs:label "recording" ;
	rdfs:subClassOf event:Event ;
	mo:level "2" ;
	vs:term_status "stable" .

mo:RecordingSession a owl:Class ;
	rdfs:comment "A set of performances/recordings/mastering events. This event can be decomposed in its constituent events using event:sub_event" ;
	rdfs:isDefinedBy <http://purl.org/ontology/mo/> ;
	rdfs:label "recording session" ;
	rdfs:subClassOf event:Event ;
	mo:level "2" ;
	vs:term_status "testing" .

mo:Release a owl:Class ;
	rdfs:comment "A specific release, with barcode, box, liner notes, cover art, and a number of records" ;
	rdfs:isDefinedBy <http://purl.org/ontology/mo/> ;
	rdfs:label "release" ;
	rdfs:subClassOf mo:MusicalManifestation ;
	mo:level "1" ;
	vs:term_status "testing" .

mo:ReleaseEvent a owl:Class ;
	rdfs:comment "A release event, in a particular place (e.g. a country) at a particular time. Other factors of this event might include cover art, liner notes, box, etc. or a release grouping all these." ;
	rdfs:isDefinedBy <http://purl.org/ontology/mo/> ;
	rdfs:label "release event" ;
	rdfs:subClassOf event:Event ;
	mo:level "1" ;
	vs:term_status "testing" .

mo:ReleaseStatus a owl:Class ;
	rdfs:comment "Musical manifestation release status." ;
	rdfs:isDefinedBy <http://purl.org/ontology/mo/> ;
	rdfs:label "release status" ;
	mo:level "1" ;
	vs:term_status "stable" .

mo:ReleaseType a owl:Class ;
	rdfs:comment "\n        Release type of a particular manifestation, such as \"album\" or \"interview\"...\n    " ;
	rdfs:isDefinedBy <http://purl.org/ontology/mo/> ;
	rdfs:label "Release type" ;
	mo:level "1" ;
	vs:term_status "stable" .

mo:SACD a owl:Class ;
	rdfs:comment "Super Audio Compact Disc used as medium to record a musical manifestation." ;
	rdfs:isDefinedBy <http://purl.org/ontology/mo/> ;
	rdfs:label "SACD" ;
	rdfs:subClassOf mo:Medium ;
	mo:level "1" ;
	vs:term_status "unstable" .

mo:Score a owl:Class ;
	rdfs:comment "\n        Here, we are dealing with the informational object (the MusicalExpression), not the actually \"published\" score.\n        This may be, for example, the product of an arrangement process.\n    " ;
	rdfs:isDefinedBy <http://purl.org/ontology/mo/> ;
	rdfs:label "score" ;
	rdfs:subClassOf mo:MusicalExpression ;
	mo:level "2" ;
	vs:term_status "stable" .

mo:Show a owl:Class ;
	rdfs:comment "\n        A show - a musical event lasting several days, in a particular venue. Examples can be\n        \"The Magic Flute\" at the Opera Bastille, August 2005, or a musical in the west end...\n    " ;
	rdfs:isDefinedBy <http://purl.org/ontology/mo/> ;
	rdfs:label "Show" ;
	rdfs:subClassOf event:Event ;
	mo:level "2" ;
	vs:term_status "stable" .

mo:Signal a owl:Class ;
	rdfs:comment "\n        A subclass of MusicalExpression, representing a signal, for example a master signal produced by a performance and a recording.\n    " ;
	rdfs:isDefinedBy <http://purl.org/ontology/mo/> ;
	rdfs:label "signal" ;
	rdfs:subClassOf mo:MusicalExpression ;
	mo:level "1" ;
	vs:term_status "stable" .

mo:SignalGroup a owl:Class ;
	rdfs:comment "\n        A musical expression representing a group of signals, for example a set of masters resulting from a whole recording/mastering session.\n    " ;
	rdfs:isDefinedBy <http://purl.org/ontology/mo/> ;
	rdfs:label "signal group" ;
	rdfs:subClassOf mo:MusicalExpression ;
	mo:level "1" ;
	vs:term_status "testing" .

mo:SoloMusicArtist a owl:Class ;
	rdfs:comment "Single person whose musical creative work shows sensitivity and imagination." ;
	rdfs:isDefinedBy <http://purl.org/ontology/mo/> ;
	rdfs:label "solo music artist" ;
	rdfs:subClassOf foaf:Person , mo:MusicArtist ;
	mo:level "1" ;
	vs:term_status "stable" .

mo:Sound a owl:Class ;
	rdfs:comment "\n        A subclass of MusicalExpression, representing a sound. Realisation of a MusicalWork during a musical Performance.\n    " ;
	rdfs:isDefinedBy <http://purl.org/ontology/mo/> ;
	rdfs:label "sound" ;
	rdfs:subClassOf event:Event , mo:MusicalExpression ;
	mo:level "2" ;
	vs:term_status "stable" .

mo:SoundEngineer a owl:Class ;
	rdfs:label "sound engineer" ;
	rdfs:subClassOf foaf:Agent ;
	mo:level "2" .

_:node1866aqtmex171 a owl:Restriction ;
	owl:onProperty mo:engineered ;
	owl:someValuesFrom mo:Performance .

mo:SoundEngineer owl:equivalentClass _:node1866aqtmex171 ;
	vs:term_status "unstable" .

mo:Stream a owl:Class ;
	rdfs:comment "Transmission over a network  used as medium to broadcast a musical manifestation" ;
	rdfs:isDefinedBy <http://purl.org/ontology/mo/> ;
	rdfs:label "Stream" ;
	rdfs:subClassOf mo:Medium ;
	mo:level "1" ;
	vs:term_status "unstable" .

mo:Torrent a owl:Class ;
	rdfs:comment "Something available on the Bittorrent peer-2-peer filesharing network" ;
	rdfs:isDefinedBy <http://purl.org/ontology/mo/> ;
	rdfs:label "Torrent" ;
	rdfs:subClassOf mo:Medium ;
	mo:level "1" ;
	vs:term_status "unstable" .

mo:Track a owl:Class ;
	rdfs:comment "A track on a particular record" ;
	rdfs:isDefinedBy <http://purl.org/ontology/mo/> ;
	rdfs:label "track" ;
	rdfs:subClassOf mo:MusicalManifestation ;
	mo:level "1" ;
	vs:term_status "stable" .

mo:Transcription a owl:Class ;
	rdfs:comment "Transcription event" ;
	rdfs:isDefinedBy <http://purl.org/ontology/mo/> ;
	rdfs:label "transcription" ;
	rdfs:subClassOf event:Event ;
	mo:level "2" ;
	vs:term_status "testing" .

mo:Vinyl a owl:Class ;
	rdfs:comment "Vinyl used as medium to record a musical manifestation" ;
	rdfs:isDefinedBy <http://purl.org/ontology/mo/> ;
	rdfs:label "Vinyl" ;
	rdfs:subClassOf mo:Medium ;
	mo:level "1" ;
	vs:term_status "unstable" .

mo:activity a owl:ObjectProperty ;
	rdfs:comment "Relates an artist to an activity period" ;
	rdfs:domain mo:MusicArtist ;
	rdfs:range mo:Activity ;
	rdfs:isDefinedBy <http://purl.org/ontology/mo/> ;
	rdfs:label "activity" ;
	mo:level "1" ;
	vs:term_status "testing" .

mo:activity_end a owl:DatatypeProperty ;
	rdfs:comment "Relates an artist to a date at which its activity ended" ;
	rdfs:domain mo:MusicArtist ;
	rdfs:range xsd:date ;
	rdfs:isDefinedBy <http://purl.org/ontology/mo/> ;
	rdfs:label "activity end" ;
	mo:level "1" ;
	vs:term_status "testing" .

mo:activity_start a owl:DatatypeProperty ;
	rdfs:comment "Relates an artist to a date at which its activity started" ;
	rdfs:domain mo:MusicArtist ;
	rdfs:range xsd:date ;
	rdfs:isDefinedBy <http://purl.org/ontology/mo/> ;
	rdfs:label "activity start" ;
	mo:level "1" ;
	vs:term_status "testing" .

mo:album a mo:ReleaseType ;
	rdfs:isDefinedBy <http://purl.org/ontology/mo/> ;
	dc:description "\n        One or more track issued together.\n            This is a type of MusicalManifestation defined by the musical industry.\n    " ;
	dc:title "album" ;
	mo:level "1" .

mo:amazon_asin a owl:ObjectProperty ;
	rdfs:comment "Used to link a work or the expression of a work to its corresponding Amazon ASINs page." .

_:node1866aqtmex172 a owl:Class .

_:node1866aqtmex173 rdf:first frbr:Work ;
	rdf:rest _:node1866aqtmex174 .

_:node1866aqtmex174 rdf:first frbr:Expression ;
	rdf:rest _:node1866aqtmex175 .

_:node1866aqtmex175 rdf:first frbr:Manifestation ;
	rdf:rest _:node1866aqtmex176 .

_:node1866aqtmex176 rdf:first frbr:Item ;
	rdf:rest rdf:nil .

_:node1866aqtmex172 owl:unionOf _:node1866aqtmex173 .

mo:amazon_asin rdfs:domain _:node1866aqtmex172 ;
	rdfs:isDefinedBy <http://purl.org/ontology/mo/> ;
	rdfs:label "amazon_asin" ;
	rdfs:range foaf:Document ;
	rdfs:subPropertyOf foaf:isPrimaryTopicOf ;
	mo:level "1" ;
	vs:term_status "stable" .

mo:arranged_in a owl:ObjectProperty ;
	rdfs:comment "\n        Associates a work to an arrangement event where it was arranged\n    " ;
	rdfs:domain mo:MusicalWork ;
	rdfs:isDefinedBy <http://purl.org/ontology/mo/> ;
	rdfs:label "arranged in" ;
	rdfs:range mo:Arrangement ;
	rdfs:subPropertyOf event:isFactorOf ;
	mo:level "2" ;
	owl:inverseOf mo:arrangement_of ;
	vs:term_status "unstable" .

mo:arrangement_of a owl:ObjectProperty ;
	rdfs:comment "\n                Associates an arrangement event to a work\n        " ;
	rdfs:domain mo:Arrangement ;
	rdfs:isDefinedBy <http://purl.org/ontology/mo/> ;
	rdfs:label "arrangement of" ;
	rdfs:range mo:MusicalWork ;
	rdfs:subPropertyOf event:factor ;
	mo:level "2" ;
	owl:inverseOf mo:arranged_in ;
	vs:term_status "unstable" .

mo:artist a owl:ObjectProperty ;
	rdfs:comment "Relates a membership event with the corresponding artist" ;
	rdfs:domain mo:Membership ;
	rdfs:isDefinedBy <http://purl.org/ontology/mo/> ;
	rdfs:label "artist" ;
	rdfs:range foaf:Agent ;
	mo:level "1" ;
	vs:term_status "testing" .

mo:audiobook a mo:ReleaseType ;
	rdfs:isDefinedBy <http://purl.org/ontology/mo/> ;
	dc:description "\n        Book read by a narrator without music.\n        This is a type of MusicalManifestation defined by the musical industry.\n    " ;
	dc:title "audio book" ;
	mo:level "1" .

mo:availableAs a owl:ObjectProperty ;
	owl:equivalentProperty mo:available_as ;
	vs:term_status "deprecated" .

mo:available_as a owl:ObjectProperty ;
	rdfs:comment "\n        Relates a musical manifestation to a musical item (this album, and my particular cd). By using\n        this property, there is no assumption on wether the full content is available on the linked item.\n        To be explicit about this, you can use a sub-property, such as mo:item (the full manifestation\n        is available on that item) or mo:preview (only a part of the manifestation is available on\n        that item).\n\n        This is a subproperty of frbr:examplar.\n    " ;
	rdfs:domain mo:MusicalManifestation ;
	rdfs:isDefinedBy <http://purl.org/ontology/mo/> ;
	rdfs:range mo:MusicalItem ;
	rdfs:subPropertyOf frbr:exemplar ;
	mo:level "1" ;
	vs:term_status "stable" .

mo:biography a owl:ObjectProperty ;
	rdfs:comment "Used to link an artist to their online biography." ;
	rdfs:domain mo:MusicArtist ;
	rdfs:isDefinedBy <http://purl.org/ontology/mo/> ;
	rdfs:label "biography" ;
	rdfs:range foaf:Document ;
	rdfs:subPropertyOf foaf:isPrimaryTopicOf ;
	mo:level "1" ;
	vs:term_status "stable" .

mo:bitsPerSample a owl:FunctionalProperty , owl:DatatypeProperty ;
	rdfs:comment "\n        Associates a digital signal to the number a bits used to encode one sample. Range is xsd:int.\n    " ;
	rdfs:domain mo:DigitalSignal ;
	rdfs:isDefinedBy <http://purl.org/ontology/mo/> ;
	rdfs:range xsd:int ;
	mo:level "1" ;
	vs:term_status "stable" .

mo:bootleg a mo:ReleaseStatus ;
	rdfs:isDefinedBy <http://purl.org/ontology/mo/> ;
	dc:description "An unofficial/underground musical work or the expression of a musical work that was not sanctioned by the artist and/or the corporate body. " ;
	dc:title "bootleg" ;
	mo:level "1" .

mo:bpm a owl:DatatypeProperty ;
	rdfs:comment "\n        Indicates the BPM of a MusicalWork or a particular Performance \n        Beats per minute: the pace of music measured by the number of beats occurring in 60 seconds.\n    " .

_:node1866aqtmex177 a owl:Class .

_:node1866aqtmex178 rdf:first mo:MusicalWork ;
	rdf:rest _:node1866aqtmex179 .

_:node1866aqtmex179 rdf:first mo:Performance ;
	rdf:rest _:node1866aqtmex180 .

_:node1866aqtmex180 rdf:first mo:Signal ;
	rdf:rest rdf:nil .

_:node1866aqtmex177 owl:unionOf _:node1866aqtmex178 .

mo:bpm rdfs:domain _:node1866aqtmex177 ;
	rdfs:isDefinedBy <http://purl.org/ontology/mo/> ;
	rdfs:label "bpm" ;
	rdfs:range xsd:float ;
	mo:level "2" ;
	vs:term_status "stable" .

mo:catalogue_number a owl:DatatypeProperty ;
	rdfs:comment "Links a release with the corresponding catalogue number" ;
	rdfs:domain mo:Release ;
	rdfs:isDefinedBy <http://purl.org/ontology/mo/> ;
	rdfs:label "catalogue number" ;
	rdfs:range xsd:string ;
	rdfs:subPropertyOf mo:uuid ;
	mo:level "1" ;
	vs:term_status "testing" .

mo:channels a owl:FunctionalProperty , owl:DatatypeProperty ;
	rdfs:comment "\n        Associates a signal to the number of channels it holds (mono --> 1, stereo --> 2). Range is xsd:int.\n    " ;
	rdfs:domain mo:Signal ;
	rdfs:isDefinedBy <http://purl.org/ontology/mo/> ;
	rdfs:range xsd:int ;
	mo:level "1" ;
	vs:term_status "stable" .

mo:collaborated_with a owl:SymmetricProperty , owl:ObjectProperty ;
	rdfs:comment "Used to relate two collaborating people on a work." ;
	rdfs:domain foaf:Agent ;
	rdfs:isDefinedBy <http://purl.org/ontology/mo/> ;
	rdfs:label "collaborated_with" ;
	rdfs:range foaf:Agent ;
	mo:level "1" ;
	vs:term_status "unstable" .

mo:compilation a mo:ReleaseType ;
	rdfs:isDefinedBy <http://purl.org/ontology/mo/> ;
	dc:description "\n        Collection of previously released manifestations of a musical expression by one or more artists.\n        This is a type of MusicalManifestation defined by the musical industry.\n    " ;
	dc:title "compilation" ;
	mo:level "1" .

mo:compilation_of a owl:ObjectProperty ;
	rdfs:comment "Indicates that a musical manifestation is a compilation of several Signals." ;
	rdfs:domain mo:MusicalManifestation ;
	rdfs:isDefinedBy <http://purl.org/ontology/mo/> ;
	rdfs:label "compilation_of" ;
	rdfs:range mo:Signal ;
	mo:level "1" ;
	vs:term_status "unstable" .

mo:compiled a owl:ObjectProperty ;
	rdfs:comment "Used to relate an person or a group of person who compiled the manifestation of a musical work." ;
	rdfs:domain mo:MusicArtist ;
	rdfs:isDefinedBy <http://purl.org/ontology/mo/> ;
	rdfs:label "compiled" ;
	rdfs:range mo:MusicalManifestation ;
	mo:level "1" ;
	owl:inverseOf mo:compiler ;
	vs:term_status "unstable" .

mo:compiler a owl:ObjectProperty ;
	rdfs:comment "Used to relate the manifestation of a musical work to a person or a group of person who compiled it." ;
	rdfs:domain mo:MusicalManifestation ;
	rdfs:isDefinedBy <http://purl.org/ontology/mo/> ;
	rdfs:label "compiler" ;
	rdfs:range mo:MusicArtist ;
	mo:level "1" ;
	owl:inverseOf mo:compiled ;
	vs:term_status "unstable" .

mo:composed_in a owl:ObjectProperty ;
	rdfs:comment "\n        Associates a MusicalWork to the Composition event pertaining\n        to its creation. For example, I might use this property to associate\n        the Magic Flute to its composition event, occuring during 1782 and having as\n        a mo:composer Mozart.\n    " ;
	rdfs:domain mo:MusicalWork ;
	rdfs:isDefinedBy <http://purl.org/ontology/mo/> ;
	rdfs:label "composed in" ;
	rdfs:range mo:Composition ;
	rdfs:subPropertyOf event:producedIn ;
	mo:level "2" ;
	owl:inverseOf mo:produced_work ;
	vs:term_status "unstable" .

mo:composer a owl:ObjectProperty ;
	rdfs:comment "\n        Associates a composition event to the actual composer. For example,\n        this property could link the event corresponding to the composition of the\n        Magic Flute in 1782 to Mozart himself (who obviously has a FOAF profile:-) ).\n    " ;
	rdfs:domain mo:Composition ;
	rdfs:isDefinedBy <http://purl.org/ontology/mo/> ;
	rdfs:label "composer" ;
	rdfs:range foaf:Agent ;
	rdfs:subPropertyOf event:agent ;
	mo:level "2" ;
	vs:term_status "stable" .

mo:conducted a owl:ObjectProperty ;
	rdfs:comment "Relates agents to the performances they were conducting" ;
	rdfs:domain foaf:Agent ;
	rdfs:isDefinedBy <http://purl.org/ontology/mo/> ;
	rdfs:label "conducted" ;
	rdfs:range mo:Performance ;
	rdfs:subPropertyOf bio:event , event:isAgentIn ;
	mo:level "2" ;
	owl:inverseOf mo:conductor ;
	vs:term_status "unstable" .

mo:conductor a owl:ObjectProperty ;
	rdfs:comment "Relates a performance to the conductor involved" ;
	rdfs:domain mo:Performance ;
	rdfs:isDefinedBy <http://purl.org/ontology/mo/> ;
	rdfs:range foaf:Agent ;
	rdfs:subPropertyOf event:agent ;
	mo:level "2" ;
	owl:inverseOf mo:conducted ;
	vs:term_status "stable" .

mo:contains_sample_from a owl:ObjectProperty ;
	rdfs:comment "\n        Relates a signal to another signal, which has been sampled.\n        " ;
	rdfs:isDefinedBy <http://purl.org/ontology/mo/> ;
	rdfs:label "contains_sample_from" ;
	rdfs:subPropertyOf mo:derived_from ;
	mo:level "1" ;
	vs:term_status "unstable" .

mo:derived_from a owl:ObjectProperty ;
	rdfs:comment "A related signal from which the described signal is derived." ;
	rdfs:domain mo:Signal ;
	rdfs:isDefinedBy <http://purl.org/ontology/mo/> ;
	rdfs:label "derived from" ;
	rdfs:range mo:Signal ;
	rdfs:subPropertyOf dcterms:source ;
	mo:level "1" ;
	vs:term_status "testing" .

mo:discography a owl:ObjectProperty ;
	rdfs:comment "Used to links an artist to an online discography of their musical works. The discography should provide a summary of each released musical work of the artist." ;
	rdfs:domain mo:MusicArtist ;
	rdfs:isDefinedBy <http://purl.org/ontology/mo/> ;
	rdfs:label "discography" ;
	rdfs:range foaf:Document ;
	rdfs:subPropertyOf foaf:isPrimaryTopicOf ;
	mo:level "1" ;
	vs:term_status "stable" .

mo:discogs a owl:ObjectProperty ;
	rdfs:comment "Used to link a musical work or the expression of a musical work, an artist or a corporate body to to its corresponding Discogs page." .

_:node1866aqtmex181 a owl:Class .

_:node1866aqtmex182 rdf:first mo:MusicalWork ;
	rdf:rest _:node1866aqtmex183 .

_:node1866aqtmex183 rdf:first mo:MusicalExpression ;
	rdf:rest _:node1866aqtmex184 .

_:node1866aqtmex184 rdf:first mo:MusicalManifestation ;
	rdf:rest _:node1866aqtmex185 .

_:node1866aqtmex185 rdf:first mo:MusicArtist ;
	rdf:rest _:node1866aqtmex186 .

_:node1866aqtmex186 rdf:first mo:CorporateBody ;
	rdf:rest rdf:nil .

_:node1866aqtmex181 owl:unionOf _:node1866aqtmex182 .

mo:discogs rdfs:domain _:node1866aqtmex181 ;
	rdfs:isDefinedBy <http://purl.org/ontology/mo/> ;
	rdfs:label "discogs" ;
	rdfs:range foaf:Document ;
	rdfs:subPropertyOf foaf:isPrimaryTopicOf ;
	mo:level "1" ;
	vs:term_status "stable" .

mo:djmix_of a owl:ObjectProperty ;
	rdfs:comment """Indicates that all (or most of) the tracks of a musical work or the expression of a musical work were mixed together from all (or most of) the tracks from another musical work or the expression of a musical work to form a so called DJ-Mix. 
    
The tracks might have been altered by pitching (so that the tempo of one track matches the tempo of the following track) and fading (so that one track blends in smoothly with the other). If the tracks have been more substantially altered, the \"mo:remix\" relationship type is more appropriate. """ ;
	rdfs:isDefinedBy <http://purl.org/ontology/mo/> ;
	rdfs:label "djmix_of" ;
	rdfs:subPropertyOf mo:derived_from ;
	mo:level "1" ;
	vs:term_status "unstable" .

mo:djmixed a owl:ObjectProperty ;
	rdfs:comment """Used to relate an artist who djmixed a musical work or the expression of a musical work. 
    
The artist usually selected the tracks, chose their sequence, and slightly changed them by fading (so that one track blends in smoothly with the other) or pitching (so that the tempo of one track matches the tempo of the following track). This applies to a 'Mixtape' in which all tracks were DJ-mixed together into one single long track. """ ;
	rdfs:domain mo:MusicArtist ;
	rdfs:isDefinedBy <http://purl.org/ontology/mo/> ;
	rdfs:label "djmixed" ;
	rdfs:range mo:Signal ;
	mo:level "1" ;
	owl:inverseOf mo:djmixed_by ;
	vs:term_status "unstable" .

mo:djmixed_by a owl:ObjectProperty ;
	rdfs:comment """Used to relate a work or the expression of a work to an artist who djmixed it. 
    
The artist usually selected the tracks, chose their sequence, and slightly changed them by fading (so that one track blends in smoothly with the other) or pitching (so that the tempo of one track matches the tempo of the following track). This applies to a 'Mixtape' in which all tracks were DJ-mixed together into one single long track. """ ;
	rdfs:domain mo:Signal ;
	rdfs:isDefinedBy <http://purl.org/ontology/mo/> ;
	rdfs:label "djmixed_by" ;
	rdfs:range mo:MusicArtist ;
	mo:level "1" ;
	owl:inverseOf mo:djmixed ;
	vs:term_status "unstable" .

mo:download a owl:ObjectProperty ;
	rdfs:comment "\n                This property can be used to link from a person to the website where they make their works available, or from\n                a manifestation (a track or an album, for example) to a web page where it is available for\n                download.\n        \n        It is better to use one of the three sub-properties instead of this one in order to specify wether the\n        content can be accessed for free (mo:freedownload), if it is just free preview material (mo:previewdownload), or\n        if it can be accessed for some money (mo:paiddownload) (this includes links to the Amazon store, for example).\n\n                This property MUST be used only if the content is just available through a web page (holding, for example\n                a Flash application) - it is better to link to actual content directly through the use of mo:available_as and\n                mo:Stream, mo:Torrent or mo:ED2K, etc. Therefore, Semantic Web user agents that don't know how to read HTML and even\n                less to rip streams from Flash applications can still access the audio content.\n        " .

_:node1866aqtmex187 a owl:Class .

_:node1866aqtmex188 rdf:first frbr:Manifestation ;
	rdf:rest _:node1866aqtmex189 .

_:node1866aqtmex189 rdf:first foaf:Agent ;
	rdf:rest _:node1866aqtmex190 .

_:node1866aqtmex190 rdf:first mo:CorporateBody ;
	rdf:rest rdf:nil .

_:node1866aqtmex187 owl:unionOf _:node1866aqtmex188 .

mo:download rdfs:domain _:node1866aqtmex187 ;
	rdfs:isDefinedBy <http://purl.org/ontology/mo/> ;
	rdfs:label "download" ;
	rdfs:range foaf:Document ;
	rdfs:subPropertyOf foaf:isPrimaryTopicOf ;
	mo:level "1" ;
	vs:term_status "stable" .

mo:ean a owl:DatatypeProperty ;
	rdfs:comment "The European Article Number (EAN) is a universal identifier for products, commonly printed in form of barcodes on them. The numbers represented by those codes can either be 8 or 13 digits long, with the 13-digit-version being most common. EANs form a superset of the North American Universal Product Code (UPC) as every UPC can be made an EAN by adding a leading zero to it. Additionally every EAN is also a Japanese Article Number (JAN). The identifiers were formerly assigned by EAN International which merged with Uniform Code Council (UCC, the guys behind the UPCs) and Electronic Commerce Council of Canada (ECCC) to become GS1. " ;
	rdfs:domain mo:Release ;
	rdfs:isDefinedBy <http://purl.org/ontology/mo/> ;
	rdfs:label "ean" ;
	rdfs:range xsd:string ;
	rdfs:subPropertyOf mo:gtin ;
	mo:level "1" ;
	vs:term_status "testing" .

mo:encodes a owl:ObjectProperty ;
	rdfs:comment "\n        Relates a MusicalItem (a track on a particular CD, an audio file, a stream somewhere) to the signal it encodes.\n\n        This is usually a lower-resolution version of the master signal (issued from a Recording event).\n    " ;
	rdfs:domain mo:MusicalItem ;
	rdfs:isDefinedBy <http://purl.org/ontology/mo/> ;
	rdfs:label "encodes" ;
	rdfs:range mo:Signal ;
	mo:level "1" ;
	vs:term_status "unstable" .

mo:encoding a owl:DatatypeProperty ;
	rdfs:comment "Method used to convert analog electronic signals into digital format such as \"MP3 CBR @ 128kbps\", \"OGG @ 160kbps\", \"FLAC\", etc." ;
	rdfs:domain mo:AudioFile ;
	rdfs:isDefinedBy <http://purl.org/ontology/mo/> ;
	rdfs:label "encoding" ;
	rdfs:range rdfs:Literal ;
	mo:level "1" ;
	vs:term_status "unstable" .

mo:duration a owl:DatatypeProperty ;
	rdfs:comment "The duration of a track or a signal in ms" .

_:node1866aqtmex191 a owl:Class .

_:node1866aqtmex192 rdf:first mo:Track ;
	rdf:rest _:node1866aqtmex193 .

_:node1866aqtmex193 rdf:first mo:Signal ;
	rdf:rest rdf:nil .

_:node1866aqtmex191 owl:unionOf _:node1866aqtmex192 .

mo:duration rdfs:domain _:node1866aqtmex191 ;
	rdfs:isDefinedBy <http://purl.org/ontology/mo/> ;
	rdfs:range xsd:float ;
	mo:level "1" ;
	vs:term_status "testing" .

mo:engineer a owl:ObjectProperty ;
	rdfs:comment "Relates a performance or a recording to the engineer involved" .

_:node1866aqtmex194 a owl:Class .

_:node1866aqtmex195 rdf:first mo:Performance ;
	rdf:rest _:node1866aqtmex196 .

_:node1866aqtmex196 rdf:first mo:Recording ;
	rdf:rest _:node1866aqtmex197 .

_:node1866aqtmex197 rdf:first mo:RecordingSession ;
	rdf:rest rdf:nil .

_:node1866aqtmex194 owl:unionOf _:node1866aqtmex195 .

mo:engineer rdfs:domain _:node1866aqtmex194 ;
	rdfs:isDefinedBy <http://purl.org/ontology/mo/> ;
	rdfs:range foaf:Agent ;
	rdfs:subPropertyOf event:agent ;
	mo:level "2" ;
	owl:inverseOf mo:engineered ;
	vs:term_status "stable" .

mo:engineered a owl:ObjectProperty ;
	rdfs:comment "Relates agents to the performances/recordings they were engineering in" ;
	rdfs:domain foaf:Agent ;
	rdfs:isDefinedBy <http://purl.org/ontology/mo/> ;
	rdfs:label "engineered" .

_:node1866aqtmex198 a owl:Class .

_:node1866aqtmex199 rdf:first mo:Performance ;
	rdf:rest _:node1866aqtmex200 .

_:node1866aqtmex200 rdf:first mo:Recording ;
	rdf:rest _:node1866aqtmex201 .

_:node1866aqtmex201 rdf:first mo:RecordingSession ;
	rdf:rest rdf:nil .

_:node1866aqtmex198 owl:unionOf _:node1866aqtmex199 .

mo:engineered rdfs:range _:node1866aqtmex198 ;
	rdfs:subPropertyOf bio:event , event:isAgentIn ;
	mo:level "2" ;
	owl:inverseOf mo:engineer ;
	vs:term_status "unstable" .

mo:ep a mo:ReleaseType ;
	rdfs:isDefinedBy <http://purl.org/ontology/mo/> ;
	dc:description "\n            An EP\n    " ;
	dc:title "ep" ;
	mo:level "1" .

mo:eventHomePage a owl:ObjectProperty ;
	owl:equivalentProperty mo:event_homepage ;
	vs:term_status "deprecated" .

mo:event_homepage a owl:ObjectProperty ;
	rdfs:comment "Links a particular event to a web page" ;
	rdfs:domain event:Event ;
	rdfs:isDefinedBy <http://purl.org/ontology/mo/> ;
	rdfs:label "event homepage" ;
	rdfs:range foaf:Document ;
	rdfs:subPropertyOf foaf:isPrimaryTopicOf ;
	mo:level "2" ;
	vs:term_status "stable" .

mo:exchange_item a owl:ObjectProperty ;
	rdfs:comment "A person, a group of person or an organization exchanging an exemplar of a single manifestation." ;
	rdfs:domain foaf:Agent ;
	rdfs:isDefinedBy <http://purl.org/ontology/mo/> ;
	rdfs:label "exchange_item" ;
	rdfs:range frbr:Item ;
	mo:level "1" ;
	vs:term_status "stable" .

mo:fanpage a owl:ObjectProperty ;
	rdfs:comment "Used to link an artist to a fan-created webpage devoted to that artist." ;
	rdfs:domain mo:MusicArtist ;
	rdfs:isDefinedBy <http://purl.org/ontology/mo/> ;
	rdfs:label "fanpage" ;
	rdfs:range foaf:Document ;
	rdfs:subPropertyOf foaf:isPrimaryTopicOf ;
	mo:level "1" ;
	vs:term_status "stable" .

mo:free_download a owl:ObjectProperty ;
	rdfs:comment "\n        This property can be used to link from a person to the website where they make their works available, or from\n        a manifestation (a track or an album, for example) to a web page where it is available for free \n        download.\n\n        This property MUST be used only if the content is just available through a web page (holding, for example\n        a Flash application) - it is better to link to actual content directly through the use of mo:available_as and \n        mo:Stream, mo:Torrent or mo:ED2K, etc. Therefore, Semantic Web user agents that don't know how to read HTML and even\n        less to rip streams from Flash applications can still access the audio content.\n    " .

_:node1866aqtmex202 a owl:Class .

_:node1866aqtmex203 rdf:first frbr:Manifestation ;
	rdf:rest _:node1866aqtmex204 .

_:node1866aqtmex204 rdf:first foaf:Agent ;
	rdf:rest _:node1866aqtmex205 .

_:node1866aqtmex205 rdf:first mo:CorporateBody ;
	rdf:rest rdf:nil .

_:node1866aqtmex202 owl:unionOf _:node1866aqtmex203 .

mo:free_download rdfs:domain _:node1866aqtmex202 ;
	rdfs:isDefinedBy <http://purl.org/ontology/mo/> ;
	rdfs:label "free download" ;
	rdfs:range foaf:Document ;
	rdfs:subPropertyOf mo:download , foaf:isPrimaryTopicOf ;
	mo:level "1" ;
	vs:term_status "stable" .

mo:freedownload a owl:ObjectProperty ;
	rdfs:isDefinedBy <http://purl.org/ontology/mo/> ;
	owl:equivalentProperty mo:free_download ;
	vs:term_status "deprecated" .

mo:genre a owl:ObjectProperty ;
	rdfs:comment "\n        Associates an event (like a performance or a recording) to a particular musical genre.\n        Further version of this property may also include works and scores in the domain.\n    " .

_:node1866aqtmex206 a owl:Class .

_:node1866aqtmex207 rdf:first foaf:Agent ;
	rdf:rest _:node1866aqtmex208 .

_:node1866aqtmex208 rdf:first mo:Performance ;
	rdf:rest _:node1866aqtmex209 .

_:node1866aqtmex209 rdf:first mo:Arrangement ;
	rdf:rest _:node1866aqtmex210 .

_:node1866aqtmex210 rdf:first mo:Composition ;
	rdf:rest _:node1866aqtmex211 .

_:node1866aqtmex211 rdf:first mo:Recording ;
	rdf:rest _:node1866aqtmex212 .

_:node1866aqtmex212 rdf:first mo:RecordingSession ;
	rdf:rest _:node1866aqtmex213 .

_:node1866aqtmex213 rdf:first mo:MusicalWork ;
	rdf:rest _:node1866aqtmex214 .

_:node1866aqtmex214 rdf:first mo:MusicalExpression ;
	rdf:rest _:node1866aqtmex215 .

_:node1866aqtmex215 rdf:first mo:MusicalManifestation ;
	rdf:rest _:node1866aqtmex216 .

_:node1866aqtmex216 rdf:first mo:MusicalItem ;
	rdf:rest rdf:nil .

_:node1866aqtmex206 owl:unionOf _:node1866aqtmex207 .

mo:genre rdfs:domain _:node1866aqtmex206 ;
	rdfs:isDefinedBy <http://purl.org/ontology/mo/> ;
	rdfs:label "genre" ;
	rdfs:range mo:Genre ;
	rdfs:subPropertyOf ao:genre ;
	mo:level "2" ;
	vs:term_status "stable" .

mo:grid a owl:DatatypeProperty ;
	rdfs:comment "The Global Release Identifier (GRid) is a system for uniquely identifying Releases of music over electronic networks (that is, online stores where you can buy music as digital files). As that it can be seen as the equivalent of the BarCode (or more correctly the GTIN) as found on physical releases of music. Like the ISRC (a code for identifying single recordings as found on releases) it was developed by the IFPI but it does not appear to be a standard of the ISO." ;
	rdfs:domain mo:Release ;
	rdfs:isDefinedBy <http://purl.org/ontology/mo/> ;
	rdfs:label "GRid" ;
	rdfs:range xsd:string ;
	rdfs:subPropertyOf mo:uuid ;
	mo:level "1" ;
	vs:term_status "testing" .

mo:group a owl:ObjectProperty ;
	rdfs:comment "Relates a membership event with the corresponding group" ;
	rdfs:domain mo:Membership ;
	rdfs:isDefinedBy <http://purl.org/ontology/mo/> ;
	rdfs:label "group" ;
	rdfs:range foaf:Group ;
	mo:level "1" ;
	vs:term_status "testing" .

mo:origin a owl:ObjectProperty ;
	rdfs:comment "Relates an artist to its geographic origin" ;
	rdfs:domain mo:MusicArtist ;
	rdfs:range geo:SpatialThing ;
	rdfs:isDefinedBy <http://purl.org/ontology/mo/> ;
	rdfs:label "origin" ;
	mo:level "1" ;
	vs:term_status "testing" .

mo:gtin a owl:DatatypeProperty ;
	rdfs:comment "GTIN is a grouping term for EANs and UPCs. In common speech those are called barcodes although the barcodes are just a representation of those identifying numbers." ;
	rdfs:domain mo:Release ;
	rdfs:isDefinedBy <http://purl.org/ontology/mo/> ;
	rdfs:label "gtin" ;
	rdfs:range xsd:string ;
	mo:level "1" ;
	vs:term_status "testing" .

mo:has_track a owl:ObjectProperty ;
	rdfs:isDefinedBy <http://purl.org/ontology/mo/> ;
	owl:equivalentProperty mo:track ;
	vs:term_status "deprecated" .

mo:headliner a owl:ObjectProperty ;
	rdfs:comment "Relates a performance to the headliner(s) involved" ;
	rdfs:isDefinedBy <http://purl.org/ontology/mo/> ;
	rdfs:label "headliner" ;
	rdfs:subPropertyOf mo:performer ;
	mo:level "2" ;
	vs:term_status "testing" .

mo:homepage a owl:ObjectProperty ;
	rdfs:comment "Links an artist, a record, etc. to a corresponding web page" .

_:node1866aqtmex217 a owl:Class .

_:node1866aqtmex218 rdf:first mo:MusicalWork ;
	rdf:rest _:node1866aqtmex219 .

_:node1866aqtmex219 rdf:first mo:MusicArtist ;
	rdf:rest _:node1866aqtmex220 .

_:node1866aqtmex220 rdf:first mo:MusicalExpression ;
	rdf:rest _:node1866aqtmex221 .

_:node1866aqtmex221 rdf:first mo:MusicalManifestation ;
	rdf:rest _:node1866aqtmex222 .

_:node1866aqtmex222 rdf:first mo:MusicalItem ;
	rdf:rest rdf:nil .

_:node1866aqtmex217 owl:unionOf _:node1866aqtmex218 .

mo:homepage rdfs:domain _:node1866aqtmex217 ;
	rdfs:isDefinedBy <http://purl.org/ontology/mo/> ;
	rdfs:label "homepage" ;
	rdfs:range foaf:Document ;
	rdfs:subPropertyOf foaf:isPrimaryTopicOf ;
	mo:level "1" ;
	vs:term_status "stable" .

mo:image a owl:ObjectProperty ;
	rdfs:comment "Indicates a pictorial image (JPEG, GIF, PNG, Etc.) of a musical work, the expression of a musical work, the manifestation of a work or the examplar of a manifestation." .

_:node1866aqtmex223 a owl:Class .

_:node1866aqtmex224 rdf:first mo:MusicalWork ;
	rdf:rest _:node1866aqtmex225 .

_:node1866aqtmex225 rdf:first mo:MusicArtist ;
	rdf:rest _:node1866aqtmex226 .

_:node1866aqtmex226 rdf:first mo:MusicalExpression ;
	rdf:rest _:node1866aqtmex227 .

_:node1866aqtmex227 rdf:first mo:MusicalManifestation ;
	rdf:rest _:node1866aqtmex228 .

_:node1866aqtmex228 rdf:first mo:MusicalItem ;
	rdf:rest rdf:nil .

_:node1866aqtmex223 owl:unionOf _:node1866aqtmex224 .

mo:image rdfs:domain _:node1866aqtmex223 ;
	rdfs:isDefinedBy <http://purl.org/ontology/mo/> ;
	rdfs:label "image" ;
	rdfs:range foaf:Image ;
	rdfs:subPropertyOf foaf:depiction ;
	mo:level "1" ;
	vs:term_status "stable" .

mo:imdb a owl:ObjectProperty ;
	rdfs:comment "Used to link an artist, a musical work or the expression of a musical work to their equivalent page on IMDb, the InternetMovieDatabase." .

_:node1866aqtmex229 a owl:Class .

_:node1866aqtmex230 rdf:first mo:MusicalWork ;
	rdf:rest _:node1866aqtmex231 .

_:node1866aqtmex231 rdf:first mo:MusicalExpression ;
	rdf:rest _:node1866aqtmex232 .

_:node1866aqtmex232 rdf:first mo:MusicalManifestation ;
	rdf:rest _:node1866aqtmex233 .

_:node1866aqtmex233 rdf:first mo:MusicArtist ;
	rdf:rest _:node1866aqtmex234 .

_:node1866aqtmex234 rdf:first mo:CorporateBody ;
	rdf:rest rdf:nil .

_:node1866aqtmex229 owl:unionOf _:node1866aqtmex230 .

mo:imdb rdfs:domain _:node1866aqtmex229 ;
	rdfs:isDefinedBy <http://purl.org/ontology/mo/> ;
	rdfs:label "imdb" ;
	rdfs:range foaf:Document ;
	rdfs:subPropertyOf foaf:isPrimaryTopicOf ;
	mo:level "1" ;
	vs:term_status "stable" .

mo:instrument a owl:ObjectProperty ;
	rdfs:comment "Relates a performance to a musical instrument involved" ;
	rdfs:domain mo:Performance ;
	rdfs:isDefinedBy <http://purl.org/ontology/mo/> ;
	rdfs:range mo:Instrument ;
	rdfs:subPropertyOf event:factor ;
	mo:level "2" ;
	vs:term_status "stable" .

mo:interpreter a owl:ObjectProperty ;
	rdfs:comment "Adds an involved music artist, who interpreted, remixed, or otherwise modified an existing signal, which resulted in the signal that is here the subject of this relation." ;
	rdfs:domain mo:Signal ;
	rdfs:isDefinedBy <http://purl.org/ontology/mo/> ;
	rdfs:label "has interpeter" ;
	rdfs:range mo:MusicArtist ;
	mo:level "1" ;
	vs:term_status "testing" .

mo:interview a mo:ReleaseType ;
	rdfs:isDefinedBy <http://purl.org/ontology/mo/> ;
	dc:description "\n        Recording of the questioning of a person.\n        This is a type of MusicalManifestation defined by the musical industry.\n    " ;
	dc:title "interview" ;
	mo:level "1" .

mo:ipi a owl:DatatypeProperty ;
	rdfs:comment "The Interested Parties Information Code (IPI) is an ISO standard similar to ISBNs for identifying the people or groups with some involvement with a particular musical work / compositions." ;
	rdfs:domain mo:MusicArtist ;
	rdfs:isDefinedBy <http://purl.org/ontology/mo/> ;
	rdfs:label "ipi" ;
	rdfs:range xsd:string ;
	rdfs:subPropertyOf mo:uuid ;
	mo:level "1" ;
	vs:term_status "testing" .

mo:ismn a owl:DatatypeProperty ;
	rdfs:comment "The International Standard Music Number (ISMN) is an ISO standard similar to ISBNs for identifying printed music publications" .

_:node1866aqtmex235 a owl:Class .

_:node1866aqtmex236 rdf:first mo:PublishedLyrics ;
	rdf:rest _:node1866aqtmex237 .

_:node1866aqtmex237 rdf:first mo:PublishedLibretto ;
	rdf:rest _:node1866aqtmex238 .

_:node1866aqtmex238 rdf:first mo:PublishedScore ;
	rdf:rest rdf:nil .

_:node1866aqtmex235 owl:unionOf _:node1866aqtmex236 .

mo:ismn rdfs:domain _:node1866aqtmex235 ;
	rdfs:isDefinedBy <http://purl.org/ontology/mo/> ;
	rdfs:label "ismn" ;
	rdfs:range xsd:string ;
	rdfs:subPropertyOf mo:uuid ;
	mo:level "1" ;
	vs:term_status "testing" .

mo:isrc a owl:DatatypeProperty ;
	rdfs:comment "\n    The ISRC (International Standard Recording Code) is the international identification system for sound recordings and music videorecordings. \n    Each ISRC is a unique and permanent identifier for a specific recording which can be permanently encoded into a product as its digital fingerprint. \n    Encoded ISRC provide the means to automatically identify recordings for royalty payments.\n    " ;
	rdfs:domain mo:Signal ;
	rdfs:isDefinedBy <http://purl.org/ontology/mo/> ;
	rdfs:label "isrc" ;
	rdfs:range xsd:string ;
	rdfs:subPropertyOf mo:uuid ;
	mo:level "1" ;
	vs:term_status "stable" .

mo:iswc a owl:DatatypeProperty ;
	rdfs:comment "Links a musical work to the corresponding ISWC number" ;
	rdfs:domain mo:MusicalWork ;
	rdfs:isDefinedBy <http://purl.org/ontology/mo/> ;
	rdfs:label "iswc" ;
	rdfs:range xsd:string ;
	rdfs:subPropertyOf mo:uuid ;
	mo:level "1" ;
	vs:term_status "testing" .

mo:item a owl:ObjectProperty ;
	rdfs:comment "\n                Relates a musical manifestation to a musical item (this album, and my particular cd) holding the\n                entire manifestation, and not just a part of it.\n        " ;
	rdfs:domain mo:MusicalManifestation ;
	rdfs:isDefinedBy <http://purl.org/ontology/mo/> ;
	rdfs:range mo:MusicalItem ;
	rdfs:subPropertyOf mo:available_as ;
	mo:level "1" ;
	vs:term_status "testing" .

mo:key a owl:ObjectProperty ;
	rdfs:comment "\n        Indicated the key used by the musicians during a performance, or the key of a MusicalWork.\n        Any of 24 major or minor diatonic scales that provide the tonal framework for a piece of music." .

_:node1866aqtmex239 a owl:Class .

_:node1866aqtmex240 rdf:first mo:MusicalWork ;
	rdf:rest _:node1866aqtmex241 .

_:node1866aqtmex241 rdf:first mo:Performance ;
	rdf:rest _:node1866aqtmex242 .

_:node1866aqtmex242 rdf:first mo:Signal ;
	rdf:rest rdf:nil .

_:node1866aqtmex239 owl:unionOf _:node1866aqtmex240 .

mo:key rdfs:domain _:node1866aqtmex239 ;
	rdfs:isDefinedBy <http://purl.org/ontology/mo/> ;
	rdfs:label "key" ;
	rdfs:range keys:Key ;
	mo:level "2" ;
	vs:term_status "stable" .

mo:label a owl:ObjectProperty ;
	rdfs:comment "Associates a release event with the label releasing the record" .

_:node1866aqtmex243 a owl:Class .

_:node1866aqtmex244 rdf:first mo:Release ;
	rdf:rest _:node1866aqtmex245 .

_:node1866aqtmex245 rdf:first mo:MusicArtist ;
	rdf:rest rdf:nil .

_:node1866aqtmex243 owl:unionOf _:node1866aqtmex244 .

mo:label rdfs:domain _:node1866aqtmex243 ;
	rdfs:isDefinedBy <http://purl.org/ontology/mo/> ;
	rdfs:label "label" ;
	rdfs:range mo:Label ;
	mo:level "1" ;
	vs:term_status "testing" .

mo:lc a owl:DatatypeProperty ;
	rdfs:comment "The Label Code (LC) was introduced in 1977 by the IFPI (International Federation of Phonogram and Videogram Industries) in order to unmistakably identify the different record labels (see Introduction, Record labels) for rights purposes. The Label Code consists historically of 4 figures, presently being extended to 5 figures, preceded by LC and a dash (e.g. LC-0193 = Electrola; LC-0233 = His Master's Voice). Note that the number of countries using the LC is limited, and that the code given on the item is not always accurate." ;
	rdfs:domain mo:Label ;
	rdfs:isDefinedBy <http://purl.org/ontology/mo/> ;
	rdfs:label "lc" ;
	rdfs:range xsd:string ;
	rdfs:subPropertyOf mo:uuid ;
	mo:level "1" ;
	vs:term_status "testing" .

mo:level a owl:AnnotationProperty ;
	rdfs:comment "\n        This annotation property associates to a particular Music Ontology term the corresponding\n        expressiveness level. These levels can be:\n\n            - 1: Only editorial/Musicbrainz type information\n            - 2: Workflow information\n            - 3: Even decomposition\n        \n        This property is mainly used for specification generation.\n    " ;
	rdfs:isDefinedBy <http://purl.org/ontology/mo/> ;
	rdfs:label "level" .

mo:licence a owl:ObjectProperty ;
	rdfs:comment """Used to link a work or the expression of a work to the license under which they can be manipulated (downloaded, modified, etc). 
    
This is usually used to link to a Creative Commons licence.""" .

_:node1866aqtmex246 a owl:Class .

_:node1866aqtmex247 rdf:first frbr:Work ;
	rdf:rest _:node1866aqtmex248 .

_:node1866aqtmex248 rdf:first frbr:Expression ;
	rdf:rest _:node1866aqtmex249 .

_:node1866aqtmex249 rdf:first frbr:Manifestation ;
	rdf:rest rdf:nil .

_:node1866aqtmex246 owl:unionOf _:node1866aqtmex247 .

mo:licence rdfs:domain _:node1866aqtmex246 ;
	rdfs:isDefinedBy <http://purl.org/ontology/mo/> ;
	rdfs:label "licence" ;
	rdfs:range cc:License ;
	mo:level "1" ;
	vs:term_status "stable" .

mo:listened a owl:ObjectProperty ;
	rdfs:comment "Relates agents to the performances they were listening in" ;
	rdfs:domain foaf:Agent ;
	rdfs:isDefinedBy <http://purl.org/ontology/mo/> ;
	rdfs:label "listened" ;
	rdfs:range mo:Performance ;
	rdfs:subPropertyOf bio:event , event:isAgentIn ;
	mo:level "2" ;
	owl:inverseOf mo:listener ;
	vs:term_status "unstable" .

mo:listener a owl:ObjectProperty ;
	rdfs:comment "Relates a performance to the listener involved" ;
	rdfs:domain mo:Performance ;
	rdfs:isDefinedBy <http://purl.org/ontology/mo/> ;
	rdfs:range foaf:Agent ;
	rdfs:subPropertyOf event:agent ;
	mo:level "2" ;
	owl:inverseOf mo:listened ;
	vs:term_status "stable" .

mo:live a mo:ReleaseType ;
	rdfs:isDefinedBy <http://purl.org/ontology/mo/> ;
	dc:description "\n        A musical manifestation that was recorded live.\n        This is a type of MusicalManifestation defined by the musical industry." ;
	dc:title "live" ;
	mo:level "1" .

mo:mailorder a owl:ObjectProperty ;
	rdfs:comment "Used to link a musical work or the expression of a musical work to a website where people can buy a copy of the musical manifestation." .

_:node1866aqtmex250 a owl:Class .

_:node1866aqtmex251 rdf:first frbr:Manifestation ;
	rdf:rest _:node1866aqtmex252 .

_:node1866aqtmex252 rdf:first mo:MusicArtist ;
	rdf:rest _:node1866aqtmex253 .

_:node1866aqtmex253 rdf:first mo:CorporateBody ;
	rdf:rest rdf:nil .

_:node1866aqtmex250 owl:unionOf _:node1866aqtmex251 .

mo:mailorder rdfs:domain _:node1866aqtmex250 ;
	rdfs:isDefinedBy <http://purl.org/ontology/mo/> ;
	rdfs:label "mailorder" ;
	rdfs:range foaf:Document ;
	rdfs:subPropertyOf foaf:isPrimaryTopicOf ;
	mo:level "1" ;
	vs:term_status "stable" .

mo:mashup_of a owl:ObjectProperty ;
	rdfs:comment """Indicates that musical works or the expressions of a musical work were mashed up on this album or track. 
    
This means that two musical works or the expressions of a musical work by different artists are mixed together, over each other, or otherwise combined into a single musical work (usually by a third artist, the remixer).""" ;
	rdfs:isDefinedBy <http://purl.org/ontology/mo/> ;
	rdfs:label "mashup_of" ;
	rdfs:subPropertyOf mo:derived_from ;
	mo:level "1" ;
	vs:term_status "unstable" .

mo:media_type a owl:ObjectProperty ;
	rdfs:comment "The mediatype (file format or MIME type, or physical medium) of a musical manifestation, e.g. a MP3, CD or vinyl." ;
	rdfs:domain mo:MusicalManifestation ;
	rdfs:isDefinedBy <http://purl.org/ontology/mo/> ;
	rdfs:label "has media type" ;
	rdfs:range dcterms:MediaType ;
	rdfs:subPropertyOf dcterms:format ;
	mo:level "1" ;
	vs:term_status "testing" .

mo:medley_of a owl:ObjectProperty ;
	rdfs:comment """Indicates that a musical expression is a medley of several other musical expressions. 
    
This means that the orignial musical expression were rearranged to create a new musical expression in the form of a medley. """ ;
	rdfs:isDefinedBy <http://purl.org/ontology/mo/> ;
	rdfs:label "medley_of" ;
	rdfs:subPropertyOf mo:derived_from ;
	mo:level "1" ;
	vs:term_status "unstable" .

mo:member a owl:ObjectProperty ;
	rdfs:comment "\n        Indicates a member of a musical group\n    " ;
	rdfs:domain mo:MusicGroup ;
	rdfs:isDefinedBy <http://purl.org/ontology/mo/> ;
	rdfs:label "member" ;
	rdfs:range foaf:Agent ;
	rdfs:subPropertyOf foaf:member ;
	mo:level "1" ;
	vs:term_status "stable" .

mo:member_of a owl:ObjectProperty ;
	rdfs:comment "Inverse of the foaf:member property" ;
	rdfs:domain foaf:Agent ;
	rdfs:isDefinedBy <http://purl.org/ontology/mo/> ;
	rdfs:label "member_of" ;
	rdfs:range foaf:Group ;
	mo:level "1" ;
	owl:inverseOf foaf:member ;
	vs:term_status "unstable" .

mo:membership a owl:ObjectProperty ;
	rdfs:comment "Relates an agent with related membership events" ;
	rdfs:domain foaf:Agent ;
	rdfs:isDefinedBy <http://purl.org/ontology/mo/> ;
	rdfs:label "membership" ;
	rdfs:range mo:Membership ;
	mo:level "1" ;
	vs:term_status "testing" .

mo:meter a owl:DatatypeProperty ;
	rdfs:comment "Associates a musical work or a score with its meter" .

_:node1866aqtmex254 a owl:Class .

_:node1866aqtmex255 rdf:first mo:MusicalWork ;
	rdf:rest _:node1866aqtmex256 .

_:node1866aqtmex256 rdf:first mo:Score ;
	rdf:rest rdf:nil .

_:node1866aqtmex254 owl:unionOf _:node1866aqtmex255 .

mo:meter rdfs:domain _:node1866aqtmex254 ;
	rdfs:isDefinedBy <http://purl.org/ontology/mo/> ;
	rdfs:label "meter" ;
	mo:level "2" ;
	vs:term_status "testing" .

mo:movement a owl:ObjectProperty ;
	rdfs:comment "Indicates that a musical work has movements" ;
	rdfs:domain mo:MusicalWork ;
	rdfs:isDefinedBy <http://purl.org/ontology/mo/> ;
	rdfs:label "has_movement" ;
	rdfs:range mo:Movement ;
	mo:level "2" ;
	vs:term_status "unstable" .

mo:movementNum a owl:DatatypeProperty ;
	owl:equivalentProperty mo:movement_number .

mo:movement_number a owl:DatatypeProperty ;
	rdfs:comment "Indicates the position of a movement in a musical work." ;
	rdfs:domain mo:Movement ;
	rdfs:isDefinedBy <http://purl.org/ontology/mo/> ;
	rdfs:label "movement number" ;
	rdfs:range xsd:int ;
	mo:level "2" ;
	vs:term_status "unstable" .

mo:musicbrainz a owl:ObjectProperty ;
	rdfs:comment "\n        Linking an agent, a track or a record to its corresponding Musicbrainz page.\n        " .

_:node1866aqtmex257 a owl:Class .

_:node1866aqtmex258 rdf:first mo:MusicalWork ;
	rdf:rest _:node1866aqtmex259 .

_:node1866aqtmex259 rdf:first mo:MusicalManifestation ;
	rdf:rest _:node1866aqtmex260 .

_:node1866aqtmex260 rdf:first foaf:Agent ;
	rdf:rest _:node1866aqtmex261 .

_:node1866aqtmex261 rdf:first mo:Signal ;
	rdf:rest rdf:nil .

_:node1866aqtmex257 owl:unionOf _:node1866aqtmex258 .

mo:musicbrainz rdfs:domain _:node1866aqtmex257 ;
	rdfs:isDefinedBy <http://purl.org/ontology/mo/> ;
	rdfs:label "musicbrainz" ;
	rdfs:range foaf:Document ;
	rdfs:subPropertyOf foaf:isPrimaryTopicOf ;
	mo:level "1" ;
	vs:term_status "stable" .

mo:musicbrainz_guid a owl:DatatypeProperty ;
	rdfs:comment "Links an object to the corresponding Musicbrainz identifier" .

_:node1866aqtmex262 a owl:Class .

_:node1866aqtmex263 rdf:first mo:MusicArtist ;
	rdf:rest _:node1866aqtmex264 .

_:node1866aqtmex264 rdf:first mo:Track ;
	rdf:rest _:node1866aqtmex265 .

_:node1866aqtmex265 rdf:first mo:Record ;
	rdf:rest _:node1866aqtmex266 .

_:node1866aqtmex266 rdf:first mo:SignalGroup ;
	rdf:rest _:node1866aqtmex267 .

_:node1866aqtmex267 rdf:first mo:Signal ;
	rdf:rest _:node1866aqtmex268 .

_:node1866aqtmex268 rdf:first mo:ReleaseEvent ;
	rdf:rest _:node1866aqtmex269 .

_:node1866aqtmex269 rdf:first mo:Label ;
	rdf:rest rdf:nil .

_:node1866aqtmex262 owl:unionOf _:node1866aqtmex263 .

mo:musicbrainz_guid rdfs:domain _:node1866aqtmex262 ;
	rdfs:isDefinedBy <http://purl.org/ontology/mo/> ;
	rdfs:label "Musicbrainz GUID" ;
	rdfs:subPropertyOf mo:uuid ;
	mo:level "1" ;
	vs:term_status "testing" .

mo:musicmoz a owl:ObjectProperty ;
	rdfs:comment "Used to link an artist, a musical work or the expression of a musical work to its corresponding MusicMoz page." .

_:node1866aqtmex270 a owl:Class .

_:node1866aqtmex271 rdf:first mo:MusicArtist ;
	rdf:rest _:node1866aqtmex272 .

_:node1866aqtmex272 rdf:first mo:MusicalWork ;
	rdf:rest _:node1866aqtmex273 .

_:node1866aqtmex273 rdf:first mo:MusicalExpression ;
	rdf:rest _:node1866aqtmex274 .

_:node1866aqtmex274 rdf:first mo:MusicalManifestation ;
	rdf:rest rdf:nil .

_:node1866aqtmex270 owl:unionOf _:node1866aqtmex271 .

mo:musicmoz rdfs:domain _:node1866aqtmex270 ;
	rdfs:isDefinedBy <http://purl.org/ontology/mo/> ;
	rdfs:label "musicmoz" ;
	rdfs:range foaf:Document ;
	rdfs:subPropertyOf foaf:isPrimaryTopicOf ;
	mo:level "1" ;
	vs:term_status "stable" .

mo:myspace a owl:ObjectProperty ;
	rdfs:comment "Used to link a person to its corresponding MySpace page." ;
	rdfs:domain foaf:Agent ;
	rdfs:isDefinedBy <http://purl.org/ontology/mo/> ;
	rdfs:label "myspace" ;
	rdfs:range foaf:Document ;
	rdfs:subPropertyOf foaf:isPrimaryTopicOf ;
	mo:level "1" ;
	vs:term_status "stable" .

mo:official a mo:ReleaseStatus ;
	rdfs:isDefinedBy <http://purl.org/ontology/mo/> ;
	dc:description "Any musical work or the expression of a musical work officially sanctioned by the artist and/or their corporate body." ;
	dc:title "official" ;
	mo:level "1" .

mo:olga a owl:ObjectProperty ;
	rdfs:comment "Used to link a track to a tabulature file for track in the On-Line Guitar Archive." ;
	rdfs:domain mo:Track ;
	rdfs:isDefinedBy <http://purl.org/ontology/mo/> ;
	rdfs:label "olga" ;
	rdfs:range foaf:Document ;
	rdfs:subPropertyOf foaf:isPrimaryTopicOf ;
	mo:level "1" ;
	vs:term_status "stable" .

mo:onlinecommunity a owl:ObjectProperty ;
	rdfs:comment "Used to link a person with an online community web page like a blog, a wiki, a forum, a livejournal page, Etc." ;
	rdfs:domain foaf:Agent ;
	rdfs:isDefinedBy <http://purl.org/ontology/mo/> ;
	rdfs:label "onlinecommunity" ;
	rdfs:range foaf:Document ;
	rdfs:subPropertyOf foaf:isPrimaryTopicOf ;
	mo:level "1" ;
	vs:term_status "stable" .

mo:opus a owl:DatatypeProperty ;
	rdfs:comment "\n        Used to define a creative work, especially a musical composition numbered to designate the order of a composer's works.\n    " ;
	rdfs:domain mo:MusicalWork ;
	rdfs:isDefinedBy <http://purl.org/ontology/mo/> ;
	rdfs:label "opus" ;
	rdfs:range rdfs:Literal ;
	mo:level "2" ;
	vs:term_status "stable" .

mo:other_release_of a owl:SymmetricProperty , owl:ObjectProperty ;
	rdfs:comment "Indicates that two musical manifestations are essentially the same." ;
	rdfs:domain mo:MusicalManifestation ;
	rdfs:isDefinedBy <http://purl.org/ontology/mo/> ;
	rdfs:label "other_release_of" ;
	rdfs:range mo:MusicalManifestation ;
	mo:level "1" ;
	vs:term_status "unstable" .

mo:paid_download a owl:ObjectProperty ;
	rdfs:comment "\n                Provide a link from an artist to a web page where all of that artist's musical work is available for some money,\n                or a link from a manifestation (record/track, for example) to a web page providing a paid access to this manifestation.\n        " .

_:node1866aqtmex275 a owl:Class .

_:node1866aqtmex276 rdf:first frbr:Manifestation ;
	rdf:rest _:node1866aqtmex277 .

_:node1866aqtmex277 rdf:first mo:MusicArtist ;
	rdf:rest _:node1866aqtmex278 .

_:node1866aqtmex278 rdf:first mo:CorporateBody ;
	rdf:rest rdf:nil .

_:node1866aqtmex275 owl:unionOf _:node1866aqtmex276 .

mo:paid_download rdfs:domain _:node1866aqtmex275 ;
	rdfs:isDefinedBy <http://purl.org/ontology/mo/> ;
	rdfs:label "paid download" ;
	rdfs:range foaf:Document ;
	rdfs:subPropertyOf mo:download , foaf:isPrimaryTopicOf ;
	mo:level "1" ;
	vs:term_status "stable" .

mo:paiddownload a owl:ObjectProperty ;
	rdfs:isDefinedBy <http://purl.org/ontology/mo/> ;
	owl:equivalentProperty mo:paid_download ;
	vs:term_status "deprecated" .

mo:performance_of a owl:ObjectProperty ;
	rdfs:comment "\n        Associates a Performance to a musical work or an arrangement that is being used as a factor in it.\n        For example, I might use this property to attach the Magic Flute musical work to \n        a particular Performance.\n    " ;
	rdfs:domain mo:Performance ;
	rdfs:isDefinedBy <http://purl.org/ontology/mo/> ;
	rdfs:label "performance of" .

_:node1866aqtmex279 a owl:Class .

_:node1866aqtmex280 rdf:first mo:Score ;
	rdf:rest _:node1866aqtmex281 .

_:node1866aqtmex281 rdf:first mo:MusicalWork ;
	rdf:rest rdf:nil .

_:node1866aqtmex279 owl:unionOf _:node1866aqtmex280 .

mo:performance_of rdfs:range _:node1866aqtmex279 ;
	rdfs:subPropertyOf event:factor ;
	mo:level "2" ;
	owl:inverseOf mo:performed_in ;
	vs:term_status "unstable" .

mo:performed a owl:ObjectProperty ;
	rdfs:comment "Relates agents to the performances they were performing in" ;
	rdfs:domain foaf:Agent ;
	rdfs:isDefinedBy <http://purl.org/ontology/mo/> ;
	rdfs:label "performed" ;
	rdfs:range mo:Performance ;
	rdfs:subPropertyOf bio:event , event:isAgentIn ;
	mo:level "2" ;
	owl:inverseOf mo:performer ;
	vs:term_status "unstable" .

mo:performed_in a owl:ObjectProperty ;
	rdfs:comment "\n        Associates a Musical Work or an Score to Performances in which they were\n        a factor. For example, I might use this property in order to \n        associate the Magic Flute to a particular performance at the Opera\n        Bastille last year." .

_:node1866aqtmex282 a owl:Class .

_:node1866aqtmex283 rdf:first mo:Score ;
	rdf:rest _:node1866aqtmex284 .

_:node1866aqtmex284 rdf:first mo:MusicalWork ;
	rdf:rest rdf:nil .

_:node1866aqtmex282 owl:unionOf _:node1866aqtmex283 .

mo:performed_in rdfs:domain _:node1866aqtmex282 ;
	rdfs:isDefinedBy <http://purl.org/ontology/mo/> ;
	rdfs:label "performed in" ;
	rdfs:range mo:Performance ;
	rdfs:subPropertyOf event:isFactorOf ;
	mo:level "2" ;
	owl:inverseOf mo:performance_of ;
	vs:term_status "unstable" .

mo:performer a owl:ObjectProperty ;
	rdfs:comment "Relates a performance to the performers involved" ;
	rdfs:domain mo:Performance ;
	rdfs:isDefinedBy <http://purl.org/ontology/mo/> ;
	rdfs:range foaf:Agent ;
	rdfs:subPropertyOf event:agent ;
	mo:level "2" ;
	owl:inverseOf mo:performed ;
	vs:term_status "stable" .

mo:possess_item a owl:ObjectProperty ;
	rdfs:comment "A person, a group of person or an organization possessing an exemplar of a single manifestation." ;
	rdfs:domain foaf:Agent ;
	rdfs:isDefinedBy <http://purl.org/ontology/mo/> ;
	rdfs:label "possess_item" ;
	rdfs:range frbr:Item ;
	mo:level "1" ;
	vs:term_status "stable" .

mo:preview a owl:ObjectProperty ;
	rdfs:comment "\n                Relates a musical manifestation to a musical item (this album, and my particular cd), which holds\n                a preview of the manifestation (eg. one track for an album, or a snippet for a track)\n        " ;
	rdfs:domain mo:MusicalManifestation ;
	rdfs:isDefinedBy <http://purl.org/ontology/mo/> ;
	rdfs:range mo:MusicalItem ;
	rdfs:subPropertyOf mo:available_as ;
	mo:level "1" ;
	vs:term_status "testing" .

mo:preview_download a owl:ObjectProperty ;
	rdfs:comment "\n                This property can be used to link from a person to the website where they make previews of their works available, or from\n                a manifestation (a track or an album, for example) to a web page where a preview download is available.\n\n                This property MUST be used only if the content is just available through a web page (holding, for example\n                a Flash application) - it is better to link to actual content directly through the use of mo:available_as and\n                mo:Stream, mo:Torrent or mo:ED2K, etc. Therefore, Semantic Web user agents that don't know how to read HTML and even\n                less to rip streams from Flash applications can still access the audio content.\n        " .

_:node1866aqtmex285 a owl:Class .

_:node1866aqtmex286 rdf:first frbr:Manifestation ;
	rdf:rest _:node1866aqtmex287 .

_:node1866aqtmex287 rdf:first foaf:Agent ;
	rdf:rest _:node1866aqtmex288 .

_:node1866aqtmex288 rdf:first mo:CorporateBody ;
	rdf:rest rdf:nil .

_:node1866aqtmex285 owl:unionOf _:node1866aqtmex286 .

mo:preview_download rdfs:domain _:node1866aqtmex285 ;
	rdfs:isDefinedBy <http://purl.org/ontology/mo/> ;
	rdfs:label "preview download" ;
	rdfs:range foaf:Document ;
	rdfs:subPropertyOf foaf:isPrimaryTopicOf , mo:download ;
	mo:level "1" ;
	vs:term_status "stable" .

mo:primary_instrument a owl:ObjectProperty ;
	rdfs:comment "Indicates that an artist primarily plays an instrument, or that a member was primarily playing a particular instrument during his membership" .

_:node1866aqtmex289 a owl:Class .

_:node1866aqtmex290 rdf:first mo:Membership ;
	rdf:rest _:node1866aqtmex291 .

_:node1866aqtmex291 rdf:first foaf:Agent ;
	rdf:rest rdf:nil .

_:node1866aqtmex289 owl:unionOf _:node1866aqtmex290 .

mo:primary_instrument rdfs:domain _:node1866aqtmex289 ;
	rdfs:isDefinedBy <http://purl.org/ontology/mo/> ;
	rdfs:label "primary instrument" ;
	rdfs:range mo:Instrument ;
	mo:level "1" ;
	vs:term_status "testing" .

mo:produced a owl:ObjectProperty ;
	rdfs:comment "Used to relate an person or a group of person who produced the manifestation of a work." ;
	rdfs:domain foaf:Agent ;
	rdfs:isDefinedBy <http://purl.org/ontology/mo/> ;
	rdfs:label "produced" ;
	rdfs:range mo:MusicalManifestation ;
	mo:level "1" ;
	owl:inverseOf mo:producer ;
	vs:term_status "stable" .

mo:produced_score a owl:ObjectProperty ;
	rdfs:comment "\n        Associates an arrangement or a composition event to a score product (score here does not refer to a published score, but more\n        an abstract arrangement of a particular work).\n    " .

_:node1866aqtmex292 a owl:Class .

_:node1866aqtmex293 rdf:first mo:Composition ;
	rdf:rest _:node1866aqtmex294 .

_:node1866aqtmex294 rdf:first mo:Arrangement ;
	rdf:rest rdf:nil .

_:node1866aqtmex292 owl:unionOf _:node1866aqtmex293 .

mo:produced_score rdfs:domain _:node1866aqtmex292 ;
	rdfs:isDefinedBy <http://purl.org/ontology/mo/> ;
	rdfs:label "produced score" ;
	rdfs:range mo:Score ;
	rdfs:subPropertyOf event:product ;
	mo:level "2" ;
	vs:term_status "unstable" .

mo:produced_signal a owl:ObjectProperty ;
	rdfs:comment "\n                Associates a Recording to the outputted signal.\n        " ;
	rdfs:domain mo:Recording ;
	rdfs:isDefinedBy <http://purl.org/ontology/mo/> ;
	rdfs:label "produced signal" ;
	rdfs:range mo:Signal ;
	rdfs:subPropertyOf event:product ;
	mo:level "2" ;
	vs:term_status "stable" .

mo:produced_signal_group a owl:ObjectProperty ;
	rdfs:comment "Associates a recording session with a group of master signals produced by it." ;
	rdfs:domain mo:RecordingSession ;
	rdfs:isDefinedBy <http://purl.org/ontology/mo/> ;
	rdfs:label "produced signal group" ;
	rdfs:range mo:SignalGroup ;
	rdfs:subPropertyOf event:product ;
	mo:level "2" ;
	vs:term_status "testing" .

mo:produced_sound a owl:ObjectProperty ;
	rdfs:comment "\n                Associates a Performance to a physical Sound that is being produced by it.\n        " ;
	rdfs:domain mo:Performance ;
	rdfs:isDefinedBy <http://purl.org/ontology/mo/> ;
	rdfs:label "produced sound" ;
	rdfs:range mo:Sound ;
	rdfs:subPropertyOf event:product ;
	mo:level "2" ;
	vs:term_status "stable" .

mo:produced_work a owl:ObjectProperty ;
	rdfs:comment "\n                Associates a composition event to the produced MusicalWork. For example,\n                this property could link the event corresponding to the composition of the\n                Magic Flute in 1782 to the Magic Flute musical work itself. This musical work\n                can then be used in particular performances.\n        " ;
	rdfs:domain mo:Composition ;
	rdfs:isDefinedBy <http://purl.org/ontology/mo/> ;
	rdfs:label "produced work" ;
	rdfs:range mo:MusicalWork ;
	rdfs:subPropertyOf event:product ;
	mo:level "2" ;
	owl:inverseOf mo:composed_in ;
	vs:term_status "stable" .

mo:producer a owl:ObjectProperty ;
	rdfs:comment "Used to relate the manifestation of a work to a person or a group of person who produced it." ;
	rdfs:domain mo:MusicalManifestation ;
	rdfs:isDefinedBy <http://purl.org/ontology/mo/> ;
	rdfs:label "producer" ;
	rdfs:range foaf:Agent ;
	mo:level "1" ;
	owl:inverseOf mo:produced ;
	vs:term_status "stable" .

mo:producesSignal a owl:ObjectProperty ;
	rdfs:isDefinedBy <http://purl.org/ontology/mo/> ;
	owl:equivalentProperty mo:produced_signal ;
	vs:term_status "deprecated" .

mo:producesSound a owl:ObjectProperty ;
	rdfs:isDefinedBy <http://purl.org/ontology/mo/> ;
	owl:equivalentProperty mo:produced_sound ;
	vs:term_status "deprecated" .

mo:producesWork a owl:ObjectProperty ;
	owl:equivalentProperty mo:produced_work .

mo:productOfComposition a owl:ObjectProperty ;
	rdfs:isDefinedBy <http://purl.org/ontology/mo/> ;
	owl:equivalentProperty mo:composed_in ;
	vs:term_status "deprecated" .

mo:promotion a mo:ReleaseStatus ;
	rdfs:isDefinedBy <http://purl.org/ontology/mo/> ;
	dc:description "A giveaway musical work or the expression of a musical work intended to promote an upcoming official musical work or the expression of a musical work." ;
	dc:title "promotion" ;
	mo:level "1" .

mo:publicationOf a owl:ObjectProperty ;
	owl:equivalentProperty mo:publication_of ;
	vs:term_status "deprecated" .

mo:publication_of a owl:ObjectProperty ;
	rdfs:comment "Link a particular manifestation to the related signal, score, libretto, or lyrics" ;
	rdfs:domain mo:MusicalManifestation ;
	rdfs:isDefinedBy <http://purl.org/ontology/mo/> ;
	rdfs:label "publication of" ;
	rdfs:range mo:MusicalExpression ;
	mo:level "1" ;
	owl:inverseOf mo:published_as ;
	vs:term_status "unstable" .

mo:published a owl:ObjectProperty ;
	rdfs:comment "Used to relate an person or a group of person who published the manifestation of a work." ;
	rdfs:domain foaf:Agent ;
	rdfs:isDefinedBy <http://purl.org/ontology/mo/> ;
	rdfs:label "published" ;
	rdfs:range mo:MusicalManifestation ;
	mo:level "1" ;
	owl:inverseOf mo:publisher ;
	vs:term_status "unstable" .

mo:publishedAs a owl:ObjectProperty ;
	owl:equivalentProperty mo:published_as ;
	vs:term_status "deprecated" .

mo:published_as a owl:ObjectProperty ;
	rdfs:comment "\n        Links a musical expression (e.g. a signal or a score) to one of its manifestations (e.g. a track on a particular record or a published score).\n    " ;
	rdfs:domain mo:MusicalExpression ;
	rdfs:isDefinedBy <http://purl.org/ontology/mo/> ;
	rdfs:label "published as" ;
	rdfs:range mo:MusicalManifestation ;
	rdfs:subPropertyOf frbr:embodiment ;
	mo:level "1" ;
	owl:inverseOf mo:publication_of ;
	vs:term_status "stable" .

mo:publisher a owl:ObjectProperty ;
	rdfs:comment "Used to relate a musical manifestation to a person or a group of person who published it." ;
	rdfs:domain mo:MusicalManifestation ;
	rdfs:isDefinedBy <http://purl.org/ontology/mo/> ;
	rdfs:label "publisher" ;
	rdfs:range foaf:Agent ;
	mo:level "1" ;
	owl:inverseOf mo:published ;
	vs:term_status "unstable" .

mo:publishingLocation a owl:ObjectProperty ;
	owl:equivalentProperty mo:publishing_location ;
	vs:term_status "deprecated" .

mo:publishing_location a owl:ObjectProperty ;
	rdfs:comment "\n        Relates a musical manifestation to its publication location.\n        " ;
	rdfs:domain mo:MusicalManifestation ;
	rdfs:isDefinedBy <http://purl.org/ontology/mo/> ;
	rdfs:label "publishingLocation" ;
	rdfs:range geo:SpatialThing ;
	mo:level "1" ;
	vs:term_status "stable" .

mo:puid a owl:DatatypeProperty ;
	rdfs:comment "\n        Link a signal to the PUIDs associated with it, that is, PUID computed from MusicalItems (mo:AudioFile) \n        derived from this signal.\n        PUIDs (Portable Unique IDentifier) are the IDs used in the \n        proprietary MusicDNS AudioFingerprinting system which is operated by MusicIP.\n\n        Using PUIDs, one (with some luck) can identify the Signal object associated with a particular audio file, therefore allowing\n        to access further information (on which release this track is featured? etc.). Using some more metadata one can identify\n        the particular Track corresponding to the audio file (a track on a particular release)." ;
	rdfs:domain mo:Signal ;
	rdfs:isDefinedBy <http://purl.org/ontology/mo/> ;
	rdfs:label "puid" ;
	rdfs:range xsd:string ;
	mo:level "1" ;
	vs:term_status "stable" .

mo:record a owl:ObjectProperty ;
	rdfs:comment "Associates a release with the records it contains. A single release can be associated with multiple records, for example for a multi-disc release." ;
	rdfs:domain mo:Release ;
	rdfs:isDefinedBy <http://purl.org/ontology/mo/> ;
	rdfs:label "released record" ;
	rdfs:range mo:Record ;
	mo:level "1" ;
	vs:term_status "testing" .

mo:record_count a owl:DatatypeProperty ;
	rdfs:comment "Associates a release with the number of records it contains, e.g. the number of discs it contains in the case of a multi-disc release." ;
	rdfs:domain mo:Release ;
	rdfs:isDefinedBy <http://purl.org/ontology/mo/> ;
	rdfs:label "record count" ;
	rdfs:range xsd:int ;
	mo:level "1" ;
	vs:term_status "testing" .

mo:record_number a owl:DatatypeProperty ;
	rdfs:comment "Indicates the position of a record in a release (e.g. a 2xLP, etc.)." ;
	rdfs:domain mo:Record ;
	rdfs:isDefinedBy <http://purl.org/ontology/mo/> ;
	rdfs:label "has record number" ;
	rdfs:range xsd:nonNegativeInteger ;
	mo:level "1" ;
	vs:term_status "testing" .

mo:record_side a owl:DatatypeProperty ;
	rdfs:comment """Associates the side on a vinyl record, where a track is located, e.g. A, B, C, etc. This property can then also be used 
in conjunction with mo:track_number, so that one can infer e.g. \"A1\", that means, track number 1 on side A.""" ;
	rdfs:domain mo:Track ;
	rdfs:isDefinedBy <http://purl.org/ontology/mo/> ;
	rdfs:label "has record side" ;
	rdfs:range xsd:string ;
	mo:level "1" ;
	vs:term_status "testing" .

mo:recordedAs a owl:ObjectProperty ;
	owl:equivalentProperty mo:recorded_as .

mo:recorded_as a owl:ObjectProperty ;
	rdfs:comment "\n        This is a shortcut property, allowing to bypass all the Sound/Recording steps. This property\n        allows to directly link a Performance to the recorded Signal. This is recommended for \"normal\"\n        users. However, advanced users wanting to express things such as the location of the microphone will\n        have to create this shortcut as well as the whole workflow, in order to let the \"normal\" users access\n        simply the, well, simple information:-) .\n    " ;
	rdfs:domain mo:Performance ;
	rdfs:isDefinedBy <http://purl.org/ontology/mo/> ;
	rdfs:label "recorded as" ;
	rdfs:range mo:Signal ;
	mo:level "2" ;
	owl:inverseOf mo:records ;
	vs:term_status "stable" .

mo:recorded_in a owl:ObjectProperty ;
	rdfs:comment "\n            Associates a physical Sound to a Recording event where it is being used \n        in order to produce a signal. For example, I might use this property to \n        associate the sound produced by a particular performance of the magic flute\n        to a given recording, done using my cell-phone.\n    " ;
	rdfs:domain mo:Sound ;
	rdfs:isDefinedBy <http://purl.org/ontology/mo/> ;
	rdfs:label "recorded in" ;
	rdfs:range mo:Recording ;
	rdfs:subPropertyOf event:isFactorOf ;
	mo:level "2" ;
	owl:inverseOf mo:recording_of ;
	vs:term_status "unstable" .

mo:recording_of a owl:ObjectProperty ;
	rdfs:comment "\n            Associates a Recording event to a physical Sound being recorded.\n                For example, I might use this property to\n                associate a given recording, done using my cell phone, to the \n        sound produced by a particular performance of the magic flute.\n    " ;
	rdfs:domain mo:Recording ;
	rdfs:isDefinedBy <http://purl.org/ontology/mo/> ;
	rdfs:label "recorded sound" ;
	rdfs:range mo:Sound ;
	rdfs:subPropertyOf event:factor ;
	mo:level "2" ;
	owl:inverseOf mo:recorded_in ;
	vs:term_status "stable" .

mo:records a owl:ObjectProperty ;
	rdfs:comment "\n        This is the inverse of the shortcut property recordedAs, allowing to relate directly a performance\n        to a signal.\n    " ;
	rdfs:domain mo:Signal ;
	rdfs:isDefinedBy <http://purl.org/ontology/mo/> ;
	rdfs:label "records" ;
	rdfs:range mo:Performance ;
	mo:level "2" ;
	owl:inverseOf mo:recordedAs ;
	vs:term_status "unstable" .

mo:release a owl:ObjectProperty ;
	rdfs:comment "Associates a release with the corresponding release event" ;
	rdfs:domain mo:ReleaseEvent ;
	rdfs:isDefinedBy <http://purl.org/ontology/mo/> ;
	rdfs:label "release" ;
	rdfs:range mo:Release ;
	rdfs:subPropertyOf event:product ;
	mo:level "1" ;
	vs:term_status "testing" .

mo:releaseStatus a owl:ObjectProperty ;
	owl:equivalentProperty mo:release_status ;
	vs:term_status "deprecated" .

mo:releaseType a owl:ObjectProperty ;
	owl:equivalentProperty mo:release_type ;
	vs:term_status "deprecated" .

mo:release_status a owl:ObjectProperty ;
	rdfs:comment "\n                Relates a musical manifestation to its release status (bootleg, ...)\n        " ;
	rdfs:domain mo:MusicalManifestation ;
	rdfs:isDefinedBy <http://purl.org/ontology/mo/> ;
	rdfs:range mo:ReleaseStatus ;
	mo:level "1" ;
	vs:term_status "stable" .

mo:release_type a owl:ObjectProperty ;
	rdfs:comment "\n        Relates a musical manifestation to its release type (interview, spoken word, album, ...)\n    " ;
	rdfs:domain mo:MusicalManifestation ;
	rdfs:isDefinedBy <http://purl.org/ontology/mo/> ;
	rdfs:range mo:ReleaseType ;
	mo:level "1" ;
	vs:term_status "stable" .

mo:remaster_of a owl:ObjectProperty ;
	rdfs:comment """This relates two musical work or the expression of a musical work, where one is a remaster of the other. 
    
A remaster is a new version made for release from source recordings that were earlier released separately. This is usually done to improve the audio quality or adjust for more modern playback equipment. The process generally doesn't involve changing the music in any artistically important way. It may, however, result in tracks that are a few seconds longer or shorter.""" ;
	rdfs:isDefinedBy <http://purl.org/ontology/mo/> ;
	rdfs:label "remaster_of" ;
	rdfs:subPropertyOf mo:derived_from ;
	mo:level "1" ;
	vs:term_status "unstable" .

mo:remix a mo:ReleaseType ;
	rdfs:isDefinedBy <http://purl.org/ontology/mo/> ;
	dc:description "\n        Musical manifestation that primarily contains remixed material. \n        This is a type of MusicalManifestation defined by the musical industry.\n    " ;
	dc:title "remix" ;
	mo:level "1" .

mo:remix_of a owl:ObjectProperty ;
	rdfs:comment "Used to relate the remix of a musical work in a substantially altered version produced by mixing together individual tracks or segments of an original musical source work." ;
	rdfs:isDefinedBy <http://purl.org/ontology/mo/> ;
	rdfs:label "remix_of" ;
	rdfs:subPropertyOf mo:derived_from ;
	mo:level "1" ;
	vs:term_status "unstable" .

mo:remixed a owl:ObjectProperty ;
	rdfs:comment """Used to relate an artist who remixed a musical work or the expression of a musical work. 
    
This involves taking just one other musical work and using audio editing to make it sound like a significantly different, but usually still recognisable, song. It can be used to link an artist to a single song that they remixed, or, if they remixed an entire musical work.""" ;
	rdfs:domain mo:MusicArtist ;
	rdfs:isDefinedBy <http://purl.org/ontology/mo/> ;
	rdfs:label "remixed" ;
	rdfs:range mo:Signal ;
	mo:level "1" ;
	owl:inverseOf mo:remixer ;
	vs:term_status "unstable" .

mo:remixer a owl:ObjectProperty ;
	rdfs:comment """Used to relate a musical work or the expression of a musical work to an artist who remixed it. 
    
This involves taking just one other musical work and using audio editing to make it sound like a significantly different, but usually still recognisable, song. It can be used to link an artist to a single song that they remixed, or, if they remixed an entire musical work.""" ;
	rdfs:isDefinedBy <http://purl.org/ontology/mo/> ;
	rdfs:label "remixer" ;
	rdfs:subPropertyOf mo:interpreter ;
	mo:level "1" ;
	owl:inverseOf mo:remixed ;
	vs:term_status "unstable" .

mo:review a owl:ObjectProperty ;
	rdfs:comment """Used to link a work or the expression of a work to a review. 
    
The review does not have to be open content, as long as it is accessible to the general internet population.""" .

_:node1866aqtmex295 a owl:Class .

_:node1866aqtmex296 rdf:first frbr:Work ;
	rdf:rest _:node1866aqtmex297 .

_:node1866aqtmex297 rdf:first frbr:Expression ;
	rdf:rest _:node1866aqtmex298 .

_:node1866aqtmex298 rdf:first frbr:Manifestation ;
	rdf:rest rdf:nil .

_:node1866aqtmex295 owl:unionOf _:node1866aqtmex296 .

mo:review rdfs:domain _:node1866aqtmex295 ;
	rdfs:isDefinedBy <http://purl.org/ontology/mo/> ;
	rdfs:label "review" ;
	rdfs:range foaf:Document ;
	rdfs:subPropertyOf foaf:isPrimaryTopicOf ;
	mo:level "1" ;
	vs:term_status "stable" .

mo:sampleRate a owl:DatatypeProperty ;
	owl:equivalentProperty mo:sample_rate ;
	vs:term_status "deprecated" .

mo:sample_rate a owl:FunctionalProperty , owl:DatatypeProperty ;
	rdfs:comment "\n        Associates a digital signal to its sample rate. It might be easier to express it this way instead of\n        defining a timeline map:-) Range is xsd:float.\n    " ;
	rdfs:domain mo:DigitalSignal ;
	rdfs:isDefinedBy <http://purl.org/ontology/mo/> ;
	rdfs:range xsd:float ;
	mo:level "1" ;
	vs:term_status "stable" .

mo:sampled a owl:ObjectProperty ;
	rdfs:comment "Used to relate an artist who sampled a Signal." ;
	rdfs:domain mo:MusicArtist ;
	rdfs:isDefinedBy <http://purl.org/ontology/mo/> ;
	rdfs:label "sampled" ;
	rdfs:range mo:Signal ;
	mo:level "1" ;
	owl:inverseOf mo:sampler ;
	vs:term_status "unstable" .

mo:sampledVersionOf a owl:ObjectProperty ;
	rdfs:isDefinedBy <http://purl.org/ontology/mo/> ;
	owl:equivalentProperty mo:sampled_version_of ;
	vs:term_status "deprecated" .

mo:sampled_version a owl:ObjectProperty ;
	rdfs:comment "\n        Associates an analog signal with a sampled version of it\n    " ;
	rdfs:domain mo:AnalogSignal ;
	rdfs:isDefinedBy <http://purl.org/ontology/mo/> ;
	rdfs:label "sampled version" ;
	rdfs:range mo:DigitalSignal ;
	mo:level "2" ;
	owl:inverseOf mo:sampled_version_of ;
	vs:term_status "stable" .

mo:sampled_version_of a owl:FunctionalProperty , owl:ObjectProperty ;
	rdfs:comment "\n        Associates a digital signal with the analog version of it\n    " ;
	rdfs:domain mo:DigitalSignal ;
	rdfs:isDefinedBy <http://purl.org/ontology/mo/> ;
	rdfs:label "sampled version of" ;
	rdfs:range mo:AnalogSignal ;
	rdfs:subPropertyOf mo:derived_from ;
	mo:level "2" ;
	owl:inverseOf mo:sampled_version ;
	vs:term_status "stable" .

mo:sampler a owl:ObjectProperty ;
	rdfs:comment "Used to relate the signal of a musical work to an artist who sampled it." ;
	rdfs:isDefinedBy <http://purl.org/ontology/mo/> ;
	rdfs:label "sampler" ;
	rdfs:subPropertyOf mo:interpreter ;
	mo:level "1" ;
	owl:inverseOf mo:sampled ;
	vs:term_status "unstable" .

mo:sell_item a owl:ObjectProperty ;
	rdfs:comment "A person, a group of person or an organization selling an exemplar of a single manifestation." ;
	rdfs:domain foaf:Agent ;
	rdfs:isDefinedBy <http://purl.org/ontology/mo/> ;
	rdfs:label "sell_item" ;
	rdfs:range frbr:Item ;
	mo:level "1" ;
	vs:term_status "stable" .

mo:signal a owl:ObjectProperty ;
	rdfs:comment "Associates a group of signals with one of the signals it contains" ;
	rdfs:domain mo:SignalGroup ;
	rdfs:isDefinedBy <http://purl.org/ontology/mo/> ;
	rdfs:label "signal" ;
	rdfs:range mo:Signal ;
	mo:level "1" ;
	vs:term_status "testing" .

mo:signalTime a owl:ObjectProperty ;
	rdfs:isDefinedBy <http://purl.org/ontology/mo/> ;
	owl:equivalentProperty mo:time ;
	vs:term_status "deprecated" .

mo:similar_to a owl:ObjectProperty ;
	rdfs:comment "\n            A similarity relationships between two objects (so far, either an agent, a signal or a genre, but\n        this could grow).\n        This relationship is pretty general and doesn't make any assumptions on how the similarity claim\n        was derived.\n        Such similarity statements can come from a range of different sources (Musicbrainz similarities between\n        artists, or coming from some automatic content analysis).\n        However, the origin of such statements should be kept using a named graph approach - and ultimately, the \n        documents providing such statements should attach some metadata to themselves (confidence of the claim, etc.).\n        " .

_:node1866aqtmex299 a owl:Class .

_:node1866aqtmex300 rdf:first foaf:Agent ;
	rdf:rest _:node1866aqtmex301 .

_:node1866aqtmex301 rdf:first mo:MusicalWork ;
	rdf:rest _:node1866aqtmex302 .

_:node1866aqtmex302 rdf:first mo:MusicalExpression ;
	rdf:rest _:node1866aqtmex303 .

_:node1866aqtmex303 rdf:first mo:MusicalManifestation ;
	rdf:rest _:node1866aqtmex304 .

_:node1866aqtmex304 rdf:first mo:MusicalItem ;
	rdf:rest _:node1866aqtmex305 .

_:node1866aqtmex305 rdf:first mo:Genre ;
	rdf:rest rdf:nil .

_:node1866aqtmex299 owl:unionOf _:node1866aqtmex300 .

mo:similar_to rdfs:domain _:node1866aqtmex299 ;
	rdfs:isDefinedBy <http://purl.org/ontology/mo/> ;
	rdfs:label "similar_to" .

_:node1866aqtmex306 a owl:Class .

_:node1866aqtmex307 rdf:first foaf:Agent ;
	rdf:rest _:node1866aqtmex308 .

_:node1866aqtmex308 rdf:first mo:MusicalWork ;
	rdf:rest _:node1866aqtmex309 .

_:node1866aqtmex309 rdf:first mo:MusicalExpression ;
	rdf:rest _:node1866aqtmex310 .

_:node1866aqtmex310 rdf:first mo:MusicalManifestation ;
	rdf:rest _:node1866aqtmex311 .

_:node1866aqtmex311 rdf:first mo:MusicalItem ;
	rdf:rest _:node1866aqtmex312 .

_:node1866aqtmex312 rdf:first mo:Genre ;
	rdf:rest rdf:nil .

_:node1866aqtmex306 owl:unionOf _:node1866aqtmex307 .

mo:similar_to rdfs:range _:node1866aqtmex306 ;
	mo:level "1" ;
	vs:term_status "unstable" .

mo:singer a owl:ObjectProperty ;
	rdfs:comment "Relates a performance to an involved singer" ;
	rdfs:domain mo:Performance ;
	rdfs:isDefinedBy <http://purl.org/ontology/mo/> ;
	rdfs:range foaf:Agent ;
	rdfs:subPropertyOf mo:performer ;
	mo:level "2" ;
	vs:term_status "stable" .

mo:single a mo:ReleaseType ;
	rdfs:isDefinedBy <http://purl.org/ontology/mo/> ;
	dc:description "A single or record single is a type of release, typically a recording of two tracks. In most cases, the single is a song that is released separately from an album, but it can still appear on an album." ;
	dc:title "single" ;
	mo:level "1" .

mo:soundtrack a mo:ReleaseType ;
	rdfs:isDefinedBy <http://purl.org/ontology/mo/> ;
	dc:description "\n        Sound recording on a narrow strip of a motion picture film.\n        This is a type of MusicalManifestation defined by the musical industry.\n    " ;
	dc:title "soundtrack" ;
	mo:level "1" .

mo:spokenword a mo:ReleaseType ;
	rdfs:isDefinedBy <http://purl.org/ontology/mo/> ;
	dc:description "\n        Spoken word is a form of music or artistic performance in which lyrics, poetry, or stories are spoken rather than sung. \n        Spoken-word is often done with a musical background, but emphasis is kept on the speaker.\n        This is a type of MusicalManifestation defined by the musical industry.\n    " ;
	dc:title "spoken word" ;
	mo:level "1" .

mo:supporting_musician a owl:ObjectProperty ;
	rdfs:comment "Used to relate an artist doing long-time instrumental or vocal support for another artist." ;
	rdfs:domain mo:MusicArtist ;
	rdfs:isDefinedBy <http://purl.org/ontology/mo/> ;
	rdfs:label "supporting_musician" ;
	rdfs:range mo:MusicArtist ;
	mo:level "1" ;
	vs:term_status "unstable" .

mo:tempo a owl:DatatypeProperty ;
	rdfs:comment "\n        Rate of speed or pace of music. Tempo markings are traditionally given in Italian; \n        common markings include: grave (solemn; very, very slow); largo (broad; very slow); \n        adagio (quite slow); andante (a walking pace); moderato (moderate); allegro (fast; cheerful); \n        vivace (lively); presto (very fast); accelerando (getting faster); ritardando (getting slower); \n        and a tempo (in time; returning to the original pace).\n    " .

_:node1866aqtmex313 a owl:Class .

_:node1866aqtmex314 rdf:first mo:MusicalWork ;
	rdf:rest _:node1866aqtmex315 .

_:node1866aqtmex315 rdf:first mo:Performance ;
	rdf:rest _:node1866aqtmex316 .

_:node1866aqtmex316 rdf:first mo:Signal ;
	rdf:rest rdf:nil .

_:node1866aqtmex313 owl:unionOf _:node1866aqtmex314 .

mo:tempo rdfs:domain _:node1866aqtmex313 ;
	rdfs:isDefinedBy <http://purl.org/ontology/mo/> ;
	rdfs:label "tempo" ;
	rdfs:range xsd:string ;
	mo:level "2" ;
	vs:term_status "stable" .

mo:lyrics a owl:ObjectProperty ;
	rdfs:comment "Associates lyrics with a musical work" ;
	rdfs:domain mo:MusicalWork ;
	rdfs:range mo:Lyrics ;
	rdfs:isDefinedBy <http://purl.org/ontology/mo/> ;
	rdfs:label "lyrics" ;
	mo:level "2" ;
	vs:term_status "testing" .

mo:text a owl:DatatypeProperty ;
	rdfs:comment "Associates lyrics with their text." ;
	rdfs:domain mo:Lyrics ;
	rdfs:isDefinedBy <http://purl.org/ontology/mo/> ;
	rdfs:label "text" ;
	mo:level "2" ;
	vs:term_status "testing" .

mo:time a owl:FunctionalProperty , owl:ObjectProperty ;
	rdfs:comment "\n        Associates a Signal to a time object - its actual domain\n    " ;
	rdfs:domain mo:Signal ;
	rdfs:isDefinedBy <http://purl.org/ontology/mo/> ;
	rdfs:label "time" ;
	rdfs:range time:TemporalEntity ;
	mo:level "1" ;
	vs:term_status "stable" .

mo:track a owl:ObjectProperty ;
	rdfs:comment "Indicates a part of a musical manifestation - in this particular case, a track." ;
	rdfs:domain mo:Record ;
	rdfs:isDefinedBy <http://purl.org/ontology/mo/> ;
	rdfs:label "track" ;
	rdfs:range mo:Track ;
	mo:level "1" ;
	vs:term_status "stable" .

mo:trackNum a owl:DatatypeProperty ;
	rdfs:isDefinedBy <http://purl.org/ontology/mo/> ;
	owl:equivalentProperty mo:track_number ;
	vs:term_status "deprecated" .

mo:track_count a owl:DatatypeProperty ;
	rdfs:comment "The track count of a record" ;
	rdfs:domain mo:Record ;
	rdfs:isDefinedBy <http://purl.org/ontology/mo/> ;
	rdfs:label "track count" ;
	rdfs:range xsd:int ;
	mo:level "1" ;
	vs:term_status "testing" .

mo:track_number a owl:DatatypeProperty ;
	rdfs:comment "Indicates the position of a track on a record medium (a CD, etc.)." ;
	rdfs:domain mo:Track ;
	rdfs:isDefinedBy <http://purl.org/ontology/mo/> ;
	rdfs:label "track number" ;
	rdfs:range xsd:nonNegativeInteger ;
	mo:level "1" ;
	vs:term_status "stable" .

mo:translation_of a owl:ObjectProperty ;
	rdfs:comment "Indicates that a work or the expression of a work has translated or transliterated into another expression of a work." ;
	rdfs:domain frbr:Expression ;
	rdfs:isDefinedBy <http://purl.org/ontology/mo/> ;
	rdfs:label "translation_of" ;
	rdfs:range frbr:Expression ;
	mo:level "1" ;
	vs:term_status "unstable" .

mo:tribute_to a owl:ObjectProperty ;
	rdfs:comment "Indicates a musical work or the expression of a musical work that is a tribute to an artist - normally consisting of music being composed by the artist but performed by other artists. " ;
	rdfs:domain mo:MusicalManifestation ;
	rdfs:isDefinedBy <http://purl.org/ontology/mo/> ;
	rdfs:label "tribute_to" ;
	rdfs:range mo:MusicArtist ;
	mo:level "1" ;
	vs:term_status "unstable" .

mo:trmid a owl:DatatypeProperty ;
	rdfs:comment "\n        Indicates the TRMID of a track.\n        TRM IDs are MusicBrainz' old AudioFingerprinting system. \n        TRM (TRM Recognizes Music) IDs are (somewhat) unique ids that represent \n        the audio signature of a musical piece (see AudioFingerprint).\n    " ;
	rdfs:domain mo:Signal ;
	rdfs:isDefinedBy <http://purl.org/ontology/mo/> ;
	rdfs:label "trmid" ;
	rdfs:range xsd:string ;
	mo:level "1" ;
	vs:term_status "stable" .

mo:upc a owl:DatatypeProperty ;
	rdfs:comment "UPC stands for \"Universal Product Code\", which was the original barcode used in the United States and Canada. The UPC (now officially EAN.UCC-12 is a numerical method of identifying products without redundancy worldwide for all types of products in the retail sector. The EAN is a superset of the original UPC increasing the digits to 13 with the prefix 0 reserved for UPC. As of 2005, manufacturers are only allowed to use the new 13-digit codes on their items, rather than having two separate numbers." ;
	rdfs:domain mo:Release ;
	rdfs:isDefinedBy <http://purl.org/ontology/mo/> ;
	rdfs:label "upc" ;
	rdfs:range xsd:string ;
	rdfs:subPropertyOf mo:gtin ;
	mo:level "1" ;
	vs:term_status "testing" .

mo:usedInPerformance a owl:ObjectProperty ;
	rdfs:isDefinedBy <http://purl.org/ontology/mo/> ;
	owl:equivalentProperty mo:performed_in ;
	vs:term_status "deprecated" .

mo:usedInRecording a owl:ObjectProperty ;
	rdfs:isDefinedBy <http://purl.org/ontology/mo/> ;
	owl:equivalentProperty mo:recorded_in ;
	vs:term_status "deprecated" .

mo:usesSound a owl:ObjectProperty ;
	rdfs:isDefinedBy <http://purl.org/ontology/mo/> ;
	owl:equivalentProperty mo:recording_of ;
	vs:term_status "deprecated" .

mo:usesWork a owl:ObjectProperty ;
	rdfs:isDefinedBy <http://purl.org/ontology/mo/> ;
	owl:equivalentProperty mo:performance_of ;
	vs:term_status "deprecated" .

mo:uuid a owl:DatatypeProperty ;
	rdfs:comment "\n            Links an object to an universally unique identifier for it.\n    " ;
	rdfs:domain owl:Thing ;
	rdfs:label "universally unique identifier" ;
	rdfs:subPropertyOf dcterms:identifier ;
	mo:level "1" ;
	vs:term_status "testing" .

mo:want_item a owl:ObjectProperty ;
	rdfs:comment "A person, a group of person or an organization wanting an exemplar of a single manifestation." ;
	rdfs:domain foaf:Agent ;
	rdfs:isDefinedBy <http://purl.org/ontology/mo/> ;
	rdfs:label "want_item" ;
	rdfs:range frbr:Item ;
	mo:level "1" ;
	vs:term_status "stable" .

mo:wikipedia a owl:ObjectProperty ;
	rdfs:comment "\n        Used to link an work, an expression of a work, a manifestation of a work, \n        a person, an instrument or a musical genre to its corresponding WikiPedia page. \n        The full URL should be used, not just the WikiName.\n    " .

_:node1866aqtmex317 a owl:Class .

_:node1866aqtmex318 rdf:first frbr:Work ;
	rdf:rest _:node1866aqtmex319 .

_:node1866aqtmex319 rdf:first frbr:Expression ;
	rdf:rest _:node1866aqtmex320 .

_:node1866aqtmex320 rdf:first frbr:Manifestation ;
	rdf:rest _:node1866aqtmex321 .

_:node1866aqtmex321 rdf:first frbr:Item ;
	rdf:rest _:node1866aqtmex322 .

_:node1866aqtmex322 rdf:first foaf:Agent ;
	rdf:rest _:node1866aqtmex323 .

_:node1866aqtmex323 rdf:first mo:Instrument ;
	rdf:rest _:node1866aqtmex324 .

_:node1866aqtmex324 rdf:first mo:Genre ;
	rdf:rest rdf:nil .

_:node1866aqtmex317 owl:unionOf _:node1866aqtmex318 .

mo:wikipedia rdfs:domain _:node1866aqtmex317 ;
	rdfs:isDefinedBy <http://purl.org/ontology/mo/> ;
	rdfs:label "wikipedia" ;
	rdfs:range foaf:Document ;
	rdfs:subPropertyOf foaf:isPrimaryTopicOf ;
	mo:level "1" ;
	vs:term_status "stable" .

vs:term_status a owl:AnnotationProperty .
