@prefix dc: <http://purl.org/dc/elements/1.1/> .
@prefix rdfs: <http://www.w3.org/2000/01/rdf-schema#> .
@prefix co: <http://purl.org/ontology/co/core#> .
@prefix event: <http://purl.org/NET/c4dm/event.owl#> .
@prefix xsd: <http://www.w3.org/2001/XMLSchema#> .
@prefix owl: <http://www.w3.org/2002/07/owl#> .
@prefix rdf: <http://www.w3.org/1999/02/22-rdf-syntax-ns#> .
@prefix vs: <http://www.w3.org/2003/06/sw-vocab-status/ns#> .

<http://purl.org/ontology/co/core#> a owl:Ontology ;
	dc:creator <http://foaf.me/zazi#me> , <http://moustaki.org/foaf.rdf#moustaki> , <http://foaf.me/intrz#me> ;
	dc:date "2010-08-04T14:24:52+01:00"^^xsd:dateTime ;
	dc:description """The Counter Ontology specification provides basic concepts and properties 
for describing a general counter concept and some important sub counters, e.g. an event counter, on/ for 
the Semantic Web. This document contains a RDF description of the Counter Ontology."""@en ;
	dc:title "The Counter Ontology"@en ;
	owl:imports <http://purl.org/dc/elements/1.1/> , <http://www.w3.org/2003/06/sw-vocab-status/ns> , <http://purl.org/NET/c4dm/event.owl> ;
	owl:versionInfo "0.8"^^xsd:decimal .

co:Counter a owl:Class , rdfs:Class ;
	rdfs:comment "Counter of a given object/ given objects, which are related to that counter."@en ;
	rdfs:isDefinedBy <http://purl.org/ontology/co/core#> ;
	rdfs:label "Counter"@en ;
	rdfs:subClassOf owl:Thing .

_:node171gub6bex1 a owl:Restriction ;
	owl:cardinality "1"^^xsd:nonNegativeInteger ;
	owl:onProperty co:count .

co:Counter rdfs:subClassOf _:node171gub6bex1 ;
	vs:term_status "stable"@en .

co:ScrobbleEvent a owl:Class , rdfs:Class ;
	rdfs:comment """An event corresponding to a scrobbling (counting an activity, which includes at least a specific factor and 
a specific agent), e.g. a track being played by someone, a video watched by someone, a book read by 
someone, a sporting activity by someone, ..."""@en ;
	rdfs:isDefinedBy <http://purl.org/ontology/co/core#> ;
	rdfs:label "Scrobble Event"@en ;
	rdfs:subClassOf event:Event ;
	vs:term_status "unstable"@en .

co:application a rdf:Property , owl:ObjectProperty ;
	rdfs:comment "An application that is related to a scrobble event, e.g. a iTunes to a play back event of a music track."@en ;
	rdfs:domain co:ScrobbleEvent ;
	rdfs:isDefinedBy <http://purl.org/ontology/co/core#> ;
	rdfs:label "has application"@en ;
	rdfs:subPropertyOf event:factor ;
	vs:term_status "unstable"@en .

co:count a owl:DatatypeProperty , owl:FunctionalProperty , rdf:Property ;
	rdfs:comment "Links a counter resource to the actual count"@en ;
	rdfs:domain co:Counter ;
	rdfs:isDefinedBy <http://purl.org/ontology/co/core#> ;
	rdfs:label "has count"@en ;
	rdfs:range xsd:integer ;
	vs:term_status "stable"@en .

co:counter a owl:ObjectProperty , rdf:Property ;
	rdfs:comment "Links an object to a counter resource. Please feel free to create further sub properties with more restricted domains."@en ;
	rdfs:isDefinedBy <http://purl.org/ontology/co/core#> ;
	rdfs:label "has counter"@en ;
	rdfs:range co:Counter ;
	vs:term_status "stable"@en .

co:device a rdf:Property , owl:ObjectProperty ;
	rdfs:comment "A device that is related to a scrobble event, e.g. a MP3 player to a play back event of a music track."@en ;
	rdfs:domain co:ScrobbleEvent ;
	rdfs:isDefinedBy <http://purl.org/ontology/co/core#> ;
	rdfs:label "has device"@en ;
	rdfs:subPropertyOf event:factor ;
	vs:term_status "unstable"@en .

co:event a owl:ObjectProperty , rdf:Property ;
	rdfs:comment "Links counter resources to related events."@en ;
	rdfs:isDefinedBy <http://purl.org/ontology/co/core#> ;
	rdfs:label "has event"@en ;
	rdfs:range event:Event ;
	rdfs:subPropertyOf co:object ;
	owl:inverseOf co:event_counter ;
	vs:term_status "testing"@en .

co:event_counter a owl:ObjectProperty , rdf:Property ;
	rdfs:comment "Links events to a counter resource, where they where counted in."@en ;
	rdfs:domain event:Event ;
	rdfs:isDefinedBy <http://purl.org/ontology/co/core#> ;
	rdfs:label "has event counter"@en ;
	rdfs:subPropertyOf co:counter ;
	vs:term_status "unstable"@en .

co:object a owl:ObjectProperty , rdf:Property ;
	rdfs:comment "Links a counter resource to an object. Please feel free to create further sub properties with more restricted ranges."@en ;
	rdfs:domain co:Counter ;
	rdfs:isDefinedBy <http://purl.org/ontology/co/core#> ;
	rdfs:label "has object"@en ;
	owl:inverseOf co:counter ;
	vs:term_status "testing"@en .

co:scrobble_object a owl:ObjectProperty , rdf:Property ;
	rdfs:comment "A scrobble object of a scrobble event, e.g. a music track, a video or a described activity. That means a specific thing that is involved in this scrobbling action."@en ;
	rdfs:domain co:ScrobbleEvent ;
	rdfs:isDefinedBy <http://purl.org/ontology/co/core#> ;
	rdfs:label "has scrobble object"@en ;
	rdfs:subPropertyOf event:factor ;
	vs:term_status "unstable"@en .

_:node171gub6bex2 a owl:Restriction ;
	owl:cardinality "1"^^xsd:nonNegativeInteger ;
	owl:onProperty co:count .

co:Counter rdfs:subClassOf _:node171gub6bex2 .
