@prefix : <http://www.w3.org/ns/adms#> .
@prefix wdrs: <http://www.w3.org/2007/05/powder-s#> .
@prefix xh: <http://www.w3.org/1999/xhtml> .
@prefix foaf: <http://xmlns.com/foaf/0.1/> .
@prefix vann: <http://purl.org/vocab/vann/> .
@prefix vcard: <http://www.w3.org/2006/vcard/ns#> .
@prefix dcterms: <http://purl.org/dc/terms/> .
@prefix sioc: <http://rdfs.org/sioc/ns#> .
@prefix schema: <http://schema.org/> .
@prefix rdfs: <http://www.w3.org/2000/01/rdf-schema#> .
@prefix voaf: <http://labs.mondeca.com/vocab/voaf#> .
@prefix dcat: <http://www.w3.org/ns/dcat#> .
@prefix owl: <http://www.w3.org/2002/07/owl#> .
@prefix xsd: <http://www.w3.org/2001/XMLSchema#> .
@prefix rdf: <http://www.w3.org/1999/02/22-rdf-syntax-ns#> .
@prefix xhv: <http://www.w3.org/1999/xhtml/vocab#> .
@prefix skos: <http://www.w3.org/2004/02/skos/core#> .
@prefix cc: <http://creativecommons.org/ns#> .
@prefix rad: <http://www.w3.org/ns/rad#> .

<http://www.w3.org/ns/adms#> a owl:Ontology ;
	rdfs:label "Asset Description Metadata Schema (ADMS)"@en ;
	rdfs:comment "This file specifies the set of RDF classes and properties used in ADMS"@en ;
	owl:versionInfo "25 June 2012"@en ;
	dcterms:modified "2012-06-25"^^xsd:date ;
	a voaf:Vocabulary ;
	voaf:specializes <http://www.w3.org/ns/rad#> ;
	vann:preferredNamespaceUri "http://www.w3.org/ns/adms#"@en-gb ;
	vann:preferredNamespacePrefix "adms"@en-gb ;
	dcterms:creator _:node1719vfjk8x1 .

_:node1719vfjk8x1 rdfs:seeAlso <http://makxdekkers.com/makxdekkers.rdf#me> ;
	foaf:name "Makx Dekkers"@en-gb ;
	foaf:homepage <http://makxdekkers.com/> .

<http://www.w3.org/ns/adms#> dcterms:creator _:node1719vfjk8x2 .

_:node1719vfjk8x2 rdfs:seeAlso <http://andrea-perego.name/foaf/#me> ;
	foaf:name "Andrea Perego"@en-gb ;
	foaf:homepage <http://andrea-perego.name/> ;
	schema:affiliation _:node1719vfjk8x3 .

_:node1719vfjk8x3 foaf:name "European Commission, Joint Research Centre"@en-gb ;
	foaf:homepage <http://ies.jrc.ec.europa.eu/DE> .

<http://www.w3.org/ns/adms#> dcterms:creator _:node1719vfjk8x4 .

_:node1719vfjk8x4 rdfs:seeAlso <http://philarcher.org/foaf.rdf#me> ;
	foaf:name "Phil Archer"@en-gb ;
	foaf:homepage <http://www.w3.org/People/all#phila> ;
	schema:affiliation _:node1719vfjk8x5 .

_:node1719vfjk8x5 foaf:name "W3C/ERCIM"@en-gb ;
	foaf:homepage <http://www.w3.org/> .

<http://www.w3.org/ns/adms#> foaf:maker _:node1719vfjk8x6 .

_:node1719vfjk8x6 foaf:name "ADMS Working Group"@en-gb ;
	foaf:page <http://joinup.ec.europa.eu/asset/adms/home> .

<http://www.w3.org/ns/adms#> dcterms:description """This is the RDF encoding of the Asset Description 
      Metadata Schema, developed under the European Union's ISA Programme,
      specifically under SEMIC Phase II, directed by Vassilios Peristeras of
      DG DIGIT. It re-uses terms from several other vocabularues, notably Dublin Core with elements of SKOS, FOAF 
      and more. The ADMS Concept Scheme, available at http://www.w3.org/ns/adms.html, defines
      its own lexical terms for its classes, properties and relationships."""@en-gb ;
	foaf:depiction <http://www.w3.org/2012/05/ADMS_Conceptual_Model.png> .

<http://www.w3.org/2012/05/ADMS_Conceptual_Model.png> rdfs:label "Asset Description Metadata Schema (ADMS) UML Class Diagram"@en-gb .

<http://www.w3.org/ns/adms#> dcterms:abstract """ADMS is intended as a model that facilitates federation 
    and co-operation. It is not the primary intention that repository owners 
    redesign or convert their current systems and data to conform to ADMS, but 
    rather that ADMS can act as a common layer among repositories that want to 
    exchange data. A change log for this namespace document is maintained in the
    HTML representation of this document, available at http://www.w3.org/ns/adms.html."""@en-gb ;
	wdrs:describedby <https://joinup.ec.europa.eu/system/files/project/ADMS_Specification_v1.00.zip> .

<https://joinup.ec.europa.eu/system/files/project/ADMS_Specification_v1.00.zip> dcterms:title "ADMS Specification"@en-gb .

<http://www.w3.org/ns/adms#> dcterms:conformsTo <https://joinup.ec.europa.eu/elibrary/document/isa-deliverable-process-and-methodology-developing-core-vocabularies> .

<https://joinup.ec.europa.eu/elibrary/document/isa-deliverable-process-and-methodology-developing-core-vocabularies> dcterms:title "Process and Methodology for Developing Core Vocabularies"@en-gb .

<http://www.w3.org/ns/adms#> dcterms:relation <https://joinup.ec.europa.eu/asset/adms/topic/public-comments-adms-specification-v10> .

<https://joinup.ec.europa.eu/asset/adms/topic/public-comments-adms-specification-v10> a sioc:Forum ;
	dcterms:title "Public comments on ADMS Specification v1.0"@en-gb .

<http://www.w3.org/ns/adms#> dcterms:publisher <http://dbpedia.org/resource/European_Commission> .

<http://dbpedia.org/resource/European_Commission> foaf:name "European Commission"@en-gb ;
	foaf:homepage <http://ec.europa.eu/> .

<http://www.w3.org/ns/adms#> dcterms:rights "Copyright © 2012 European Commission."@en-gb ;
	dcterms:license <https://joinup.ec.europa.eu/category/licence/isa-open-metadata-licence-v10> .

<https://joinup.ec.europa.eu/category/licence/isa-open-metadata-licence-v10> dcterms:title "ISA Open Metadata Licence v1.0"@en-gb ;
	cc:attributionName "European Commission"@en-gb ;
	cc:attributionURL <http://ec.europa.eu/> .

<http://www.w3.org/ns/adms#> cc:attributionName "European Commission"@en-gb ;
	cc:attributionURL <http://ec.europa.eu/> .

skos:Concept rdfs:label "Asset Type"@en ;
	rdfs:comment "The skos:Concept class fully represents the ADMS class of Asset Type (see section on the <xh:a xh:href=\"#Code\" xmlns:xh=\"http://www.w3.org/1999/xhtml\">Code</xh:a> datatype for details)."^^rdf:XMLLiteral ;
	vann:usageNote "Used in ADMS to provide a classification of a Semantic Asset according to a controlled vocabulary, e.g. code list, metadata schema."@en ;
	rdfs:isDefinedBy <http://www.w3.org/TR/skos-primer/> ;
	dcterms:identifier "skos:Concept"@en-gb ;
	rdfs:label "Code"@en ;
	rdfs:comment """<xh:p xmlns:xh=\"http://www.w3.org/1999/xhtml\">The Conceptual Model includes a 'Code' datatype that 
      is used by several classes. This is expressed using the <xh:a xh:href=\"http://www.w3.org/TR/skos-primer/\">SKOS vocabulary</xh:a> with
      a particular 'code' usually being a skos:Concept thatis part of a scheme. 
      The intention is that the skos:Concept class be used as follows;</xh:p><xh:ul>
      <xh:li>for the content property, use skos:notation</xh:li>
      <xh:li>the 'list' property will be taken care of by means of the skos:inScheme property;</xh:li>
      <xh:li>the list agency property is likely to be applied to the scheme as a whole for which dcterms:creator is appropriate;</xh:li>
      <xh:li>the list version property can be fulfilled using schema:version (see <xh:a xh:href=\"http://schema.org/CreativeWork\">http://schema.org/CreativeWork</xh:a>)</xh:li></xh:ul>
    """^^rdf:XMLLiteral .

vcard:VCard rdfs:label "Contact Information"@en ;
	rdfs:comment "VCard fully represents the ADMS class of Contact Information"@en ;
	vann:usageNote "ADMS uses VCard to provide contact information regarding a Semantic Asset, including e-mail, address, name and associated Web page information. See <xh:a xh:href=\"http://www.w3.org/TR/vcard-rdf/\" xmlns:xh=\"http://www.w3.org/1999/xhtml\">Representing vCard Objects in RDF</xh:a> for details of this widely used specification."^^rdf:XMLLiteral ;
	rdfs:isDefinedBy <http://www.w3.org/TR/vcard-rdf/> ;
	dcterms:identifier "vcard:VCard"@en-gb .

foaf:Document rdfs:label "Documentation"@en ;
	rdfs:comment "The foaf:Document class fully represents the ADMS concept of documentation."@en ;
	vann:usageNote "Used in ADMS specifically for the class of documents that further describe a Semantic Asset or give guidelines for its use. ADMS expects all documents to have a title (use <xh:a xh:href=\"http://purl.org/dc/terms/title\" xmlns:xh=\"http://www.w3.org/1999/xhtml\">dcterms:title</xh:a>)."^^rdf:XMLLiteral ;
	rdfs:isDefinedBy <http://xmlns.com/foaf/spec/> ;
	dcterms:identifier "foaf:Documentation"@en-gb .

dcterms:FileFormat rdfs:label "File Format"@en ;
	rdfs:comment "The dcterms:FileFormat class fully represents the ADMS concept of a file format."@en ;
	vann:usageNote "Used in ADMS to provide the technical format that a Distribution is available in, e.g. PDF for a document, XML for a schema."@en ;
	rdfs:isDefinedBy <http://dublincore.org/documents/dcmi-terms/> ;
	dcterms:identifier "dcterms:FileFormat"@en-gb .

:Identifier a rdfs:Class ;
	rdfs:label "Identifier"@en ;
	rdfs:comment """<xh:p xmlns:xh=\"http://www.w3.org/1999/xhtml\">This class is based on 
      the UN/CEFACT Identifier complex type defined in See Section 5.8 of <xh:a xh:href=\"http://www.unece.org/fileadmin/DAM/cefact/codesfortrade/CCTS/CCTS-DTCatalogueVersion3p1.pdf\">Core Components Data Type Catalogue Version 3.1</xh:a></xh:p>
      <xh:p>The various properties can be fulfilled as follows:</xh:p><xh:ul>
      <xh:li>use <xh:a xh:href=\"http://www.w3.org/2004/02/skos/core#notation\">skos:notation</xh:a> to provide the actual identifier (the Identifier class is effectively meaningless without this property and conceptually it is mandatory);</xh:li>
      <xh:li>use <xh:a xh:href=\"http://purl.org/dc/terms/type\">dcterms:type</xh:a> to provide an identifier for the type of identifier issued (the identifier scheme);</xh:li>
      <xh:li>use <xh:a xh:href=\"#schemeversion\">adms:schemeVersion</xh:a> to identify the version of the identifier scheme;</xh:li>
      <xh:li>use <xh:a xh:href=\"#schemeagency\">adms:schemeAgency</xh:a> to provide the name of the agency that created the identifier (as an rdfs:Literal).</xh:li></xh:ul>
      <xh:p>Although not part of the ADMS conceptual model, it may be useful to provide further properties to the Identifier class:</xh:p><xh:ul>
      <xh:li>use <xh:a xh:href=\"http://purl.org/dc/terms/creator\">dcterms:creator</xh:a> to link to a URI of an Agent class describing the issuing Agency;</xh:li>
      <xh:li>use <xh:a xh:href=\"http://purl.org/dc/terms/created\">dcterms:created</xh:a> to provide the date on which the identifier was issued.</xh:li></xh:ul>
    """^^rdf:XMLLiteral ;
	rdfs:isDefinedBy <https://joinup.ec.europa.eu/system/files/project/ADMS_Specification_v1.00.zip> ;
	dcterms:identifier "adms:Identifier"@en-gb .

skos:Concept rdfs:label "Interoperability Level"@en ;
	rdfs:comment "The skos:Concept class fully represents the ADMS class of Interoperability Level (see section on the <xh:a xh:href=\"#Code\" xmlns:xh=\"http://www.w3.org/1999/xhtml\">Code</xh:a> datatype for details)."^^rdf:XMLLiteral ;
	vann:usageNote "ADMS uses SKOS Concepts to provide the level according to the European Interoperability Framework (EIF 2.0) for which an Asset is relevant."@en .

:Item a rdfs:Class ;
	rdfs:label "Item"@en ;
	rdfs:comment "An item that is contained inside an Asset, e.g. an individual term in a vocabulary, an individual code in a code list or some other ‘atomic’ element of an Asset."@en ;
	rdfs:isDefinedBy <https://joinup.ec.europa.eu/system/files/project/ADMS_Specification_v1.00.zip> ;
	dcterms:identifier "adms:Item"@en-gb .

dcterms:PeriodOfTime rdfs:label "Period Of Time"@en ;
	rdfs:comment "The dcterms:PeriodOfTime class fully represents the ADMS concept of the same name."@en ;
	vann:usageNote "Used in ADMS to provide a time period relevant for an Asset, e.g. for its validity."@en ;
	rdfs:isDefinedBy <http://dublincore.org/documents/dcmi-terms/> ;
	dcterms:identifier "dcterms:PeriodOfTime"@en-gb .

skos:Concept rdfs:label "Representation Technique"@en ;
	rdfs:comment "The skos:Concept class fully represents the ADMS class of Representation Technique (see section on the <xh:a xh:href=\"#Code\" xmlns:xh=\"http://www.w3.org/1999/xhtml\">Code</xh:a> datatype for details)."^^rdf:XMLLiteral ;
	vann:usageNote "ADMS uses SKOS Concepts to represent the machine-readable language in which a Distribution is expressed. This differs from File Format in that, for example, the XML File Format can be used to represent a number of different langauges including UML, RDF and more."@en .

:SemanticAsset rdfs:label "Semantic Asset"@en ;
	rdfs:comment "A Semantic Asset in the model is an abstract entity that reflects the intellectual content of the asset and represents those characteristics of the asset that are independent of its physical embodiment. This abstract entity combines the FRBR entities work (a distinct intellectual or artistic creation) and expression (the intellectual or artistic realization of a work). Assets can be versioned. Every time the intellectual content of an asset changes, the result is considered to be a new asset that can be linked to previous and next versions of the Asset. The physical embodiment of an Asset is called a Distribution. A particular Asset may have zero or more Distributions."@en ;
	rdfs:subClassOf rad:Asset ;
	rdfs:isDefinedBy <https://joinup.ec.europa.eu/system/files/project/ADMS_Specification_v1.00.zip> ;
	dcterms:identifier "adms:SemanticAsset"@en-gb .

:SemanticAssetDistribution a rdfs:Class ;
	rdfs:label "Semantic Asset Distribution"@en ;
	rdfs:comment "A Semantic Asset Distribution in the model represents a particular physical embodiment of a Semantic Asset, which is an example of the FRBR entity manifestation (the physical embodiment of an expression of a work). A Distribution is typically a downloadable computer file (but in principle it could also be a paper document) that implements the intellectual content of an Asset. A particular Distribution is associated with one and only one Asset, while all Distributions of an Asset share the same intellectual content in different physical formats. Distributions themselves are not versioned."@en ;
	rdfs:subClassOf rad:Distribution ;
	rdfs:isDefinedBy <https://joinup.ec.europa.eu/system/files/project/ADMS_Specification_v1.00.zip> ;
	dcterms:identifier "adms:SemanticAssetDistribution"@en-gb .

:SemanticAssetRepository a rdfs:Class ;
	rdfs:label "Semantic Asset Repository"@en ;
	rdfs:comment "A Semantic Asset Repository is a system or service that provides facilities for storage and maintenance of descriptions of Semantic Assets and Semantic Asset Distributions, and functionality that allows users to search and access these descriptions. A Semantic Asset Repository will typically contain descriptions of several Semantic Assets and related Semantic Asset Distributions."@en ;
	rdfs:isDefinedBy <https://joinup.ec.europa.eu/system/files/project/ADMS_Specification_v1.00.zip> ;
	rdfs:subClassOf rad:Repository ;
	dcterms:identifier "adms:SemanticAssetRepository"@en-gb .

skos:Concept rdfs:label "Status"@en ;
	rdfs:comment "The skos:Concept class fully represents the ADMS class of Status (see section on the <xh:a xh:href=\"#Code\" xmlns:xh=\"http://www.w3.org/1999/xhtml\">Code</xh:a> datatype for details)."^^rdf:XMLLiteral ;
	vann:usageNote "ADMS uses SKOS Concepts to provide an indication of the maturity of an Asset or Distribution."@en .

:accessURL a rdf:Property ;
	rdfs:label "access URL"@en ;
	rdfs:comment "The URL of the Repository or Distribution. The range of adms:accessURL is xsd:anyURI"@en ;
	rdfs:isDefinedBy <https://joinup.ec.europa.eu/system/files/project/ADMS_Specification_v1.00.zip> ;
	rdfs:range xsd:anyURI ;
	dcterms:identifier "adms:accessURL"@en-gb .

:contactPoint a rdf:Property ;
	rdfs:label "contact point"@en ;
	rdfs:comment "Links a Semantic Asset to relevant <xh:a xh:href=\"#ContactInformation\" xmlns:xh=\"http://www.w3.org/1999/xhtml\">Contact Information</xh:a> which is provided using VCard."^^rdf:XMLLiteral ;
	rdfs:isDefinedBy <https://joinup.ec.europa.eu/system/files/project/ADMS_Specification_v1.00.zip> ;
	rdfs:range vcard:VCard ;
	dcterms:identifier "adms:contactPoint"@en-gb .

wdrs:describedby rdfs:label "documentation"@en ;
	rdfs:comment "The <xh:a xh:href=\"http://www.w3.org/2007/05/powder-s#describedby\" xmlns:xh=\"http://www.w3.org/1999/xhtml\">wdrs:describedby</xh:a> property fully represents the ADMS relationship of main documentation."^^rdf:XMLLiteral ;
	vann:usageNote "Used in ADMS to link to the main documentation or specification of the Asset."@en ;
	rdfs:isDefinedBy <http://www.w3.org/2007/05/powder-s#> ;
	dcterms:identifier "wdrs:describedby"@en-gb .

schema:endDate a rdf:Property ;
	rdfs:label "end"@en ;
	rdfs:comment "The schema:endDate fully represents the ADMS property that gives the end of the <xh:a xh:href=\"#PeriodOfTime\" xmlns:xh=\"http://www.w3.org/1999/xhtml\">Period of Time</xh:a>."^^rdf:XMLLiteral ;
	rdfs:isDefinedBy schema:Event ;
	dcterms:identifier "schema:endDate"@en-gb .

foaf:homepage rdfs:label "homepage"@en ;
	rdfs:comment "The foaf:homepage property fully represents the ADMS relationship of the same name."@en ;
	vann:usageNote "Used in ADMS to link to a Web page that is fully dedicated to the Asset."@en ;
	rdfs:isDefinedBy <http://xmlns.com/foaf/spec/> ;
	dcterms:identifier "foaf:homepage"@en-gb .

:identifier rdfs:label "identifier"@en ;
	rdfs:comment "adms:identifier is used to link any resource to an instance of adms:Identifier which is its range. N.B. it is not appropriate to use dcterms:identifer to link to the Identifier class as its range is rdfs:Literal."@en ;
	vann:usageNote "ADMS uses this to provide any identifier for the Asset."@en ;
	rdfs:isDefinedBy <https://joinup.ec.europa.eu/system/files/project/ADMS_Specification_v1.00.zip> ;
	rdfs:range :Identifier ;
	dcterms:identifier "adms:identifier"@en-gb .

:identifies a rdf:Property ;
	rdfs:label "identifies"@en ;
	rdfs:comment "The identifies relation is used to link an adms:Identifier class to whatever resource it identifies."@en ;
	rdfs:domain :Identifier ;
	rdfs:isDefinedBy <https://joinup.ec.europa.eu/system/files/project/ADMS_Specification_v1.00.zip> ;
	dcterms:identifier "adms:identifies"@en-gb .

:includedAsset a rdf:Property ;
	rdfs:label "included asset"@en ;
	rdfs:comment "Links to a Semantic Asset that is contained in the Asset being described, e.g. when there are several vocabularies defined in a single document."@en ;
	rdfs:isDefinedBy <https://joinup.ec.europa.eu/system/files/project/ADMS_Specification_v1.00.zip> ;
	rdfs:range :Asset ;
	dcterms:identifier "adms:includedAsset"@en-gb .

:includedItem a rdf:Property ;
	rdfs:label "included item"@en ;
	rdfs:comment "Links a Semantic Asset to an item that is contained within it (e.g. a concept in a controlled vocabulary). The range of adms:includedItem is <xh:a xh:href=\"#Item\" xmlns:xh=\"http://www.w3.org/1999/xhtml\">adms:Item</xh:a>."^^rdf:XMLLiteral ;
	rdfs:isDefinedBy <https://joinup.ec.europa.eu/system/files/project/ADMS_Specification_v1.00.zip> ;
	rdfs:range :Item ;
	dcterms:identifier "adms:includedItem"@en-gb .

:interoperabilityLevel a rdf:Property ;
	rdfs:label "interoperability level"@en ;
	rdfs:comment "Links a resource to its <xh:a xh:href=\"#InteroperabilityLevel\" xmlns:xh=\"http://www.w3.org/1999/xhtml\">adms:InteroperabilityLevel</xh:a>. Since this is encoded using skos:Concept, that is the defined range for this property."^^rdf:XMLLiteral ;
	rdfs:isDefinedBy <https://joinup.ec.europa.eu/system/files/project/ADMS_Specification_v1.00.zip> ;
	rdfs:range skos:Concept ;
	dcterms:identifier "adms:interoperabilityLevel"@en-gb .

:metadataDate a rdf:Property ;
	rdfs:label "metadata date"@en ;
	rdfs:comment "The date of the most recent update of the metadata for the Asset."@en ;
	rdfs:isDefinedBy <https://joinup.ec.europa.eu/system/files/project/ADMS_Specification_v1.00.zip> ;
	rdfs:range rdfs:Literal ;
	dcterms:identifier "adms:metadataDate"@en-gb .

:metadataLanguage a rdf:Property ;
	rdfs:label "metadata language"@en ;
	rdfs:comment "Links to the language of the metadata for the Asset. The range of adms:metadataLanguage is dcterms:LinguisticSystem which is used by RADion (and therefore ADMS) to represent the Language class."@en ;
	rdfs:isDefinedBy <https://joinup.ec.europa.eu/system/files/project/ADMS_Specification_v1.00.zip> ;
	rdfs:range dcterms:LinguisticSystem ;
	dcterms:identifier "adms:metadataLanguage"@en-gb .

:metadataPublisher a rdf:Property ;
	rdfs:label "metadata publisher"@en ;
	rdfs:comment "Links to the organisation making the metadata for the Asset available. The range of adms:metadataPublisher as dcterms:Agent which is used by RADion, and therefore ADMS, for the Publisher class."@en ;
	rdfs:isDefinedBy <https://joinup.ec.europa.eu/system/files/project/ADMS_Specification_v1.00.zip> ;
	rdfs:range dcterms:Agent ;
	dcterms:identifier "adms:metadataPublisher"@en-gb .

:relatedDocumentation a rdf:Property ;
	rdfs:label "related documentation"@en ;
	rdfs:comment "Links to documentation that contains information related to the asset. The range of adms:relatedDocumentation is foaf:Document"@en ;
	rdfs:isDefinedBy <https://joinup.ec.europa.eu/system/files/project/ADMS_Specification_v1.00.zip> ;
	rdfs:range foaf:Document ;
	dcterms:identifier "adms:relatedDocumentation"@en-gb .

:relatedWebPage a rdf:Property ;
	rdfs:label "related web page"@en ;
	rdfs:comment "Links to a Web page that contains information related to the asset. The range of adms:relatedWebPage is foaf:Document"@en ;
	rdfs:isDefinedBy <https://joinup.ec.europa.eu/system/files/project/ADMS_Specification_v1.00.zip> ;
	rdfs:range foaf:Document ;
	dcterms:identifier "adms:relatedWebPage"@en-gb .

:representationTechnique a rdf:Property ;
	rdfs:label "representation technique"@en ;
	rdfs:comment "Links an adms:Distribution to a skos:Concept that is its <xh:a xh:href=\"#RepresentationTechnique\" xmlns:xh=\"http://www.w3.org/1999/xhtml\">Representation Technique</xh:a>."^^rdf:XMLLiteral ;
	rdfs:isDefinedBy <https://joinup.ec.europa.eu/system/files/project/ADMS_Specification_v1.00.zip> ;
	rdfs:range skos:Concept ;
	dcterms:identifier "adms:representationTechnique"@en-gb .

:sample a rdf:Property ;
	rdfs:label "sample"@en ;
	rdfs:comment "Links to a sample of the Semantic Asset (which is itself a Semantic Asset, i.e the range is adms:Asset)."@en ;
	rdfs:isDefinedBy <https://joinup.ec.europa.eu/system/files/project/ADMS_Specification_v1.00.zip> ;
	rdfs:range :Asset ;
	dcterms:identifier "adms:sample"@en-gb .

:schemeAgency a rdf:Property ;
	rdfs:label "scheme agency"@en ;
	rdfs:comment "The name of the agency responsible for issuing the identifier"@en ;
	rdfs:isDefinedBy <https://joinup.ec.europa.eu/system/files/project/ADMS_Specification_v1.00.zip> ;
	rdfs:domain :Identifier ;
	rdfs:range rdfs:Literal ;
	dcterms:identifier "adms:schemeAgency"@en-gb .

:schemeVersion a rdf:Property ;
	rdfs:label "scheme version"@en ;
	rdfs:comment "The version number of the identifier for the scheme used to create the identifier"@en ;
	rdfs:isDefinedBy <https://joinup.ec.europa.eu/system/files/project/ADMS_Specification_v1.00.zip> ;
	rdfs:domain :Identifier ;
	rdfs:range rdfs:Literal ;
	dcterms:identifier "adms:schemeVersion"@en-gb .

schema:startDate a rdf:Property ;
	rdfs:label "start"@en ;
	rdfs:comment "The schema:startDate fully represents the ADMS property of start."@en ;
	vann:usageNote "Used in ADMS to provide the beginning of the <xh:a xh:href=\"#PeriodOfTime\" xmlns:xh=\"http://www.w3.org/1999/xhtml\">Period of Time</xh:a> relevant to a Semantic Asset. The term is defined as part of schema.org's <xh:a xh:href=\"http://schema.org/Event\">Event vocabulary</xh:a> but has no defined domain and range and so is suitable for use in this context."^^rdf:XMLLiteral ;
	rdfs:isDefinedBy schema:Event ;
	dcterms:identifier "schema:startDate"@en-gb .

:status a rdf:Property ;
	rdfs:label "status"@en ;
	rdfs:comment "Links to the status of the Asset or Distribution in the context of a particular workflow process. Since <xh:a xh:href=\"#Status\" xmlns:xh=\"http://www.w3.org/1999/xhtml\">Status</xh:a> is defined using a skos:Concept, that is the defined range for this property."^^rdf:XMLLiteral ;
	rdfs:isDefinedBy <https://joinup.ec.europa.eu/system/files/project/ADMS_Specification_v1.00.zip> ;
	rdfs:range skos:Concept ;
	dcterms:identifier "adms:status"@en-gb .

:supportedSchema a rdf:Property ;
	rdfs:label "supported schema"@en ;
	rdfs:comment "A schema according to which the Repository can provide data about its content, e.g. ADMS"@en ;
	rdfs:isDefinedBy <https://joinup.ec.europa.eu/system/files/project/ADMS_Specification_v1.00.zip> ;
	rdfs:range rdfs:Literal ;
	dcterms:identifier "adms:supportedSchema"@en-gb .

dcterms:temporal rdfs:label "temporal coverage"@en ;
	rdfs:comment "The <xh:a xh:href=\"http://purl.org/dc/terms/temporal\" xmlns:xh=\"http://www.w3.org/1999/xhtml\">dcterms:temporal</xh:a> property fully represents the ADMS relationship of temporal coverage."^^rdf:XMLLiteral ;
	vann:usageNote "Used in ADMS to link to the Period of Time class. Note that the range is dcterms:PeriodOfTime"@en ;
	rdfs:isDefinedBy <http://dublincore.org/documents/dcmi-terms/> ;
	dcterms:identifier "dcterms:temporal"@en-gb .

:translation a rdf:Property ;
	rdfs:label "translation"@en ;
	rdfs:comment "Links to a translation of the Semantic Asset (which is itself a Semantic Asset, i.e the range is adms:Asset)."@en ;
	rdfs:isDefinedBy <https://joinup.ec.europa.eu/system/files/project/ADMS_Specification_v1.00.zip> ;
	rdfs:range :Asset ;
	dcterms:identifier "adms:translation"@en-gb .

dcterms:type a rdf:Property ;
	rdfs:label "type"@en ;
	rdfs:comment "The <xh:a xh:href=\"http://purl.org/dc/terms/type\" xmlns:xh=\"http://www.w3.org/1999/xhtml\">dcterms:type</xh:a> property fully represents the ADMS property of asset type, and the type properties of both the Licence and Publisher classes. The range of dcterms:type is rdfs:Class."^^rdf:XMLLiteral ;
	vann:usageNote "Used in ADMS to link an Asset to its Asset Type."@en ;
	rdfs:isDefinedBy <http://dublincore.org/documents/dcmi-terms/> ;
	dcterms:identifier "dcterms:type"@en-gb .

<http://www.w3.org/ns/adms#> dcterms:creator _:node1719vfjk8x7 .

_:node1719vfjk8x7 rdfs:seeAlso <http://makxdekkers.com/makxdekkers.rdf#me> ;
	foaf:name "Makx Dekkers"@en-gb ;
	foaf:homepage <http://makxdekkers.com/> .

<http://www.w3.org/ns/adms#> dcterms:creator _:node1719vfjk8x8 .

_:node1719vfjk8x8 rdfs:seeAlso <http://andrea-perego.name/foaf/#me> ;
	foaf:name "Andrea Perego"@en-gb ;
	foaf:homepage <http://andrea-perego.name/> ;
	schema:affiliation _:node1719vfjk8x9 .

_:node1719vfjk8x9 foaf:name "European Commission, Joint Research Centre"@en-gb ;
	foaf:homepage <http://ies.jrc.ec.europa.eu/DE> .

<http://www.w3.org/ns/adms#> dcterms:creator _:node1719vfjk8x10 .

_:node1719vfjk8x10 rdfs:seeAlso <http://philarcher.org/foaf.rdf#me> ;
	foaf:name "Phil Archer"@en-gb ;
	foaf:homepage <http://www.w3.org/People/all#phila> ;
	schema:affiliation _:node1719vfjk8x11 .

_:node1719vfjk8x11 foaf:name "W3C/ERCIM"@en-gb ;
	foaf:homepage <http://www.w3.org/> .

<http://www.w3.org/ns/adms#> foaf:maker _:node1719vfjk8x12 .

_:node1719vfjk8x12 foaf:name "ADMS Working Group"@en-gb ;
	foaf:page <http://joinup.ec.europa.eu/asset/adms/home> .
