<?xml version="1.0" encoding="utf-8"?><rdf:RDF xml:base="http://dbpedia.org/ontology/" xmlns:foaf="http://xmlns.com/foaf/0.1/" xmlns:cc="http://creativecommons.org/ns#" xmlns:vann="http://purl.org/vocab/vann/" xmlns:dcterms="http://purl.org/dc/terms/" xmlns:dc="http://purl.org/dc/elements/1.1/" xmlns:wgs84pos="http://www.w3.org/2003/01/geo/wgs84_pos#" xmlns:cidoccrm="http://purl.org/NET/cidoc-crm/core#" xmlns:wikidata="http://www.wikidata.org/entity/" xmlns:dul="http://www.ontologydesignpatterns.org/ont/dul/DUL.owl#" xmlns:d0="http://www.ontologydesignpatterns.org/ont/d0.owl#" xmlns:owl="http://www.w3.org/2002/07/owl#" xmlns:xsd="http://www.w3.org/2001/XMLSchema#" xmlns:rdf="http://www.w3.org/1999/02/22-rdf-syntax-ns#" xmlns:rdfs="http://www.w3.org/2000/01/rdf-schema#" xmlns:prov="http://www.w3.org/ns/prov#" xmlns="http://dbpedia.org/ontology/">

          <owl:Ontology rdf:about="http://dbpedia.org/ontology/">
            <rdf:type rdf:resource="http://purl.org/vocommons/voaf#Vocabulary"/>
            <vann:preferredNamespacePrefix>dbo</vann:preferredNamespacePrefix>
            <vann:preferredNamespaceUri>http://dbpedia.org/ontology/</vann:preferredNamespaceUri>
            <dcterms:title xml:lang="en">The DBpedia Ontology</dcterms:title>
            <dcterms:description xml:lang="en">
              The DBpedia ontology provides the classes and properties used in the DBpedia data set.
            </dcterms:description>
            <foaf:homepage rdf:resource="http://wiki.dbpedia.org/Ontology"/>
            <dcterms:source rdf:resource="http://mappings.dbpedia.org"/>
            <dcterms:publisher>DBpedia Maintainers</dcterms:publisher>
            <dcterms:creator>DBpedia Maintainers and Contributors</dcterms:creator>
            <dcterms:issued>2008-11-17T12:00Z</dcterms:issued>
            <owl:versionInfo xml:lang="en">latest-snapshot</owl:versionInfo>
            <rdfs:comment xml:lang="en">
              This ontology is generated from the manually created specifications in the DBpedia Mappings
              Wiki. Each release of this ontology corresponds to a new release of the DBpedia data set which
              contains instance data extracted from the different language versions of Wikipedia. For
              information regarding changes in this ontology, please refer to the DBpedia Mappings Wiki.
            </rdfs:comment>
            <cc:license rdf:resource="http://creativecommons.org/licenses/by-sa/3.0/"/>
            <dcterms:license rdf:resource="http://creativecommons.org/licenses/by-sa/3.0/"/>
          </owl:Ontology>
        <owl:Class rdf:about="http://dbpedia.org/ontology/BasketballLeague">
        <rdfs:label xml:lang="nl">basketbal competitie</rdfs:label><rdfs:label xml:lang="el">Ομοσπονδία Καλαθοσφαίρισης</rdfs:label><rdfs:label xml:lang="ko">농구 리그</rdfs:label><rdfs:label xml:lang="ur">باسکٹ بال کی انجمن</rdfs:label><rdfs:label xml:lang="ga">sraith cispheile</rdfs:label><rdfs:label xml:lang="fr">ligue de basketball</rdfs:label><rdfs:label xml:lang="es">liga de baloncesto</rdfs:label><rdfs:label xml:lang="it">lega di pallacanestro</rdfs:label><rdfs:label xml:lang="en">basketball league</rdfs:label><rdfs:label xml:lang="ja">バスケットボールリーグ</rdfs:label><rdfs:label xml:lang="de">Basketball-Liga</rdfs:label><rdfs:comment xml:lang="en">a group of sports teams that compete against each other in Basketball</rdfs:comment><rdfs:comment xml:lang="ur">کھیلوں کی ٹیموں کا ایک گروپ جو باسکٹ بال میں ایک دوسرے سے مقابلہ کرتا ہے</rdfs:comment><rdfs:subClassOf rdf:resource="http://dbpedia.org/ontology/SportsLeague"/><prov:wasDerivedFrom rdf:resource="http://mappings.dbpedia.org/index.php/OntologyClass:BasketballLeague"/>
        </owl:Class><owl:Class rdf:about="http://dbpedia.org/ontology/NaturalEvent">
        <rdfs:label xml:lang="nl">gebeurtenis in de natuur</rdfs:label><rdfs:label xml:lang="el">φυσικό γεγονός</rdfs:label><rdfs:label xml:lang="ur">قدرتی واقعہ</rdfs:label><rdfs:label xml:lang="fr">événement naturel</rdfs:label><rdfs:label xml:lang="it">evento naturale</rdfs:label><rdfs:label xml:lang="en">natural event</rdfs:label><rdfs:label xml:lang="de">Naturereignis</rdfs:label><rdfs:comment xml:lang="el">Το φυσικό γεγονός χρησιμοποιείται για να περιγράψει ένα συμβάν που πραγματοποιείται φυσικά</rdfs:comment><rdfs:comment xml:lang="ur">مادی تقریب کا استعمال قدرتی طور پر رونما ہونے والے واقعے کو بیان کرنے کے لیے کیا جاتا ہے۔</rdfs:comment><rdfs:subClassOf rdf:resource="http://dbpedia.org/ontology/Event"/><prov:wasDerivedFrom rdf:resource="http://mappings.dbpedia.org/index.php/OntologyClass:NaturalEvent"/>
        </owl:Class><owl:Class rdf:about="http://dbpedia.org/ontology/Province">
        <rdfs:label xml:lang="nl">provincie</rdfs:label><rdfs:label xml:lang="el">επαρχία</rdfs:label><rdfs:label xml:lang="ur">صوبہ</rdfs:label><rdfs:label xml:lang="ga">cúige</rdfs:label><rdfs:label xml:lang="fr">province</rdfs:label><rdfs:label xml:lang="en">province</rdfs:label><rdfs:label xml:lang="ja">英語圏の行政区画</rdfs:label><rdfs:label xml:lang="de">Provinz</rdfs:label><rdfs:comment xml:lang="en">An administrative body governing a territorial unity on the intermediate level, between local and national level</rdfs:comment><rdfs:comment xml:lang="fr">Entité administrative en charge d'une unité territoriale se situant entre le niveau local et national; ex: Province Nord (Nouvelle-Calédonie)</rdfs:comment><rdfs:comment xml:lang="el">Είναι διοικητική δομή του κράτους που διοικεί μια περιοχή που είναι σε έκταση μεγαλύτερη από τοπικό επίπεδο και μικρότερη από εθνικό επίπεδο.</rdfs:comment><rdfs:comment xml:lang="ur">ایک انتظامی ادارہ جو مقامی اور قومی سطح کے درمیان انٹرمیڈیٹ سطح پر علاقائی وحدت کا انتظام کرتا ہے۔</rdfs:comment><rdfs:subClassOf rdf:resource="http://dbpedia.org/ontology/GovernmentalAdministrativeRegion"/><prov:wasDerivedFrom rdf:resource="http://mappings.dbpedia.org/index.php/OntologyClass:Province"/>
        </owl:Class><owl:Class rdf:about="http://dbpedia.org/ontology/TopLevelDomain">
        <rdfs:label xml:lang="en">top level domain</rdfs:label><rdfs:label xml:lang="ur">اوپر سطح کی ڈومین</rdfs:label><rdfs:label xml:lang="de">top level domain</rdfs:label><rdfs:label xml:lang="fr">domaine de premier niveau</rdfs:label><rdfs:subClassOf rdf:resource="http://dbpedia.org/ontology/Identifier"/><owl:equivalentClass rdf:resource="http://www.wikidata.org/entity/Q14296"/><prov:wasDerivedFrom rdf:resource="http://mappings.dbpedia.org/index.php/OntologyClass:TopLevelDomain"/>
        </owl:Class><owl:Class rdf:about="http://dbpedia.org/ontology/LunarCrater">
        <rdfs:label xml:lang="pt">cratera lunar</rdfs:label><rdfs:label xml:lang="nl">maankrater</rdfs:label><rdfs:label xml:lang="el">Σεληνιακός κρατήρας</rdfs:label><rdfs:label xml:lang="ur">قمری گڑھا</rdfs:label><rdfs:label xml:lang="ga">cráitéar gealaí</rdfs:label><rdfs:label xml:lang="fr">cratère lunaire</rdfs:label><rdfs:label xml:lang="en">lunar crater</rdfs:label><rdfs:label xml:lang="de">Mondkrater</rdfs:label><rdfs:subClassOf rdf:resource="http://dbpedia.org/ontology/Crater"/><owl:equivalentClass rdf:resource="http://www.wikidata.org/entity/Q1348589"/><prov:wasDerivedFrom rdf:resource="http://mappings.dbpedia.org/index.php/OntologyClass:LunarCrater"/>
        </owl:Class><owl:Class rdf:about="http://dbpedia.org/ontology/MotorsportSeason">
        <rdfs:label xml:lang="en">motorsport season</rdfs:label><rdfs:label xml:lang="ur">موٹر کھیل کا موسم</rdfs:label><rdfs:label xml:lang="nl">motorsportseizoen</rdfs:label><rdfs:label xml:lang="de">Motorsportsaison</rdfs:label><rdfs:subClassOf rdf:resource="http://dbpedia.org/ontology/SportsSeason"/><prov:wasDerivedFrom rdf:resource="http://mappings.dbpedia.org/index.php/OntologyClass:MotorsportSeason"/>
        </owl:Class><owl:Class rdf:about="http://dbpedia.org/ontology/MilitaryPerson">
        <rdfs:label xml:lang="nl">militair</rdfs:label><rdfs:label xml:lang="el">στρατιωτικός</rdfs:label><rdfs:label xml:lang="ko">군인</rdfs:label><rdfs:label xml:lang="ur">فوجی شخص</rdfs:label><rdfs:label xml:lang="fr">militaire</rdfs:label><rdfs:label xml:lang="it">militare</rdfs:label><rdfs:label xml:lang="en">military person</rdfs:label><rdfs:label xml:lang="ja">軍人</rdfs:label><rdfs:label xml:lang="de">militärische Person</rdfs:label><rdfs:subClassOf rdf:resource="http://dbpedia.org/ontology/Person"/><prov:wasDerivedFrom rdf:resource="http://mappings.dbpedia.org/index.php/OntologyClass:MilitaryPerson"/>
        </owl:Class><owl:Class rdf:about="http://dbpedia.org/ontology/TimePeriod">
        <rdfs:label xml:lang="nl">tijdvak</rdfs:label><rdfs:label xml:lang="el">χρονική περίοδος</rdfs:label><rdfs:label xml:lang="ur">وقت کی مدت</rdfs:label><rdfs:label xml:lang="ga">tréimhse</rdfs:label><rdfs:label xml:lang="fr">période temporelle</rdfs:label><rdfs:label xml:lang="es">periodo temporal</rdfs:label><rdfs:label xml:lang="en">time period</rdfs:label><rdfs:label xml:lang="da">tidsperiode</rdfs:label><rdfs:label xml:lang="de">Zeitraum</rdfs:label><rdfs:subClassOf rdf:resource="http://www.w3.org/2002/07/owl#Thing"/><rdfs:subClassOf rdf:resource="http://www.ontologydesignpatterns.org/ont/dul/DUL.owl#TimeInterval"/><owl:disjointWith rdf:resource="http://dbpedia.org/ontology/Person"/><prov:wasDerivedFrom rdf:resource="http://mappings.dbpedia.org/index.php/OntologyClass:TimePeriod"/>
        </owl:Class><owl:Class rdf:about="http://dbpedia.org/ontology/AutomobileEngine">
        <rdfs:label xml:lang="pt">motor de automóvel</rdfs:label><rdfs:label xml:lang="nl">automotor</rdfs:label><rdfs:label xml:lang="el">κινητήρας αυτοκινήτου</rdfs:label><rdfs:label xml:lang="ko">자동차 엔진</rdfs:label><rdfs:label xml:lang="ur">موٹر گاڑی کا انجن</rdfs:label><rdfs:label xml:lang="ga">inneall gluaisteáin</rdfs:label><rdfs:label xml:lang="fr">moteur d'automobile</rdfs:label><rdfs:label xml:lang="it">motore d'automobile</rdfs:label><rdfs:label xml:lang="en">automobile engine</rdfs:label><rdfs:label xml:lang="ja">内燃機関</rdfs:label><rdfs:label xml:lang="de">Fahrzeugmotor</rdfs:label><rdfs:subClassOf rdf:resource="http://dbpedia.org/ontology/Engine"/><prov:wasDerivedFrom rdf:resource="http://mappings.dbpedia.org/index.php/OntologyClass:AutomobileEngine"/>
        </owl:Class><owl:Class rdf:about="http://dbpedia.org/ontology/Nebula">
        <rdfs:label xml:lang="en">Nebula</rdfs:label><rdfs:label xml:lang="fr">Nébuleuse</rdfs:label><rdfs:label xml:lang="ru">Туманность</rdfs:label><rdfs:label xml:lang="ur">آنکھ کا جالا</rdfs:label><rdfs:subClassOf rdf:resource="http://dbpedia.org/ontology/CelestialBody"/><owl:disjointWith rdf:resource="http://dbpedia.org/ontology/Person"/><prov:wasDerivedFrom rdf:resource="http://mappings.dbpedia.org/index.php/OntologyClass:Nebula"/>
        </owl:Class><owl:Class rdf:about="http://dbpedia.org/ontology/Archeologist">
        <rdfs:label xml:lang="pl">archeolog</rdfs:label><rdfs:label xml:lang="nl">archeoloog</rdfs:label><rdfs:label xml:lang="el">Αρχαιολόγος</rdfs:label><rdfs:label xml:lang="ur">ماہر آثار قدیمہ</rdfs:label><rdfs:label xml:lang="ga">seandálaí</rdfs:label><rdfs:label xml:lang="fr">archéologue</rdfs:label><rdfs:label xml:lang="es">Arqueólogo</rdfs:label><rdfs:label xml:lang="en">archeologist</rdfs:label><rdfs:label xml:lang="ja">考古学者</rdfs:label><rdfs:label xml:lang="de">Archäologe</rdfs:label><rdfs:subClassOf rdf:resource="http://dbpedia.org/ontology/Person"/><owl:equivalentClass rdf:resource="http://www.wikidata.org/entity/Q3621491"/><prov:wasDerivedFrom rdf:resource="http://mappings.dbpedia.org/index.php/OntologyClass:Archeologist"/>
        </owl:Class><owl:Class rdf:about="http://dbpedia.org/ontology/Enzyme">
        <rdfs:label xml:lang="nl">enzym</rdfs:label><rdfs:label xml:lang="el">ένζυμο</rdfs:label><rdfs:label xml:lang="ko">효소</rdfs:label><rdfs:label xml:lang="ur">خامرہ</rdfs:label><rdfs:label xml:lang="ga">einsím</rdfs:label><rdfs:label xml:lang="fr">enzyme</rdfs:label><rdfs:label xml:lang="it">enzima</rdfs:label><rdfs:label xml:lang="en">enzyme</rdfs:label><rdfs:label xml:lang="ja">酵素</rdfs:label><rdfs:label xml:lang="de">Enzym</rdfs:label><rdfs:subClassOf rdf:resource="http://dbpedia.org/ontology/Biomolecule"/><owl:equivalentClass rdf:resource="http://www.wikidata.org/entity/Q8047"/><prov:wasDerivedFrom rdf:resource="http://mappings.dbpedia.org/index.php/OntologyClass:Enzyme"/>
        </owl:Class><owl:Class rdf:about="http://dbpedia.org/ontology/SongWriter">
        <rdfs:label xml:lang="nl">songwriter (tekstdichter)</rdfs:label><rdfs:label xml:lang="ur">نغمہ نگار</rdfs:label><rdfs:label xml:lang="fr">auteur-compositeur</rdfs:label><rdfs:label xml:lang="en">songwriter</rdfs:label><rdfs:label xml:lang="da">sangskriver</rdfs:label><rdfs:label xml:lang="de">Liedschreiber</rdfs:label><rdfs:comment xml:lang="en">a person who writes songs.</rdfs:comment><rdfs:comment xml:lang="nl">een persoon die de muziek en/of de tekst voor populaire muzieknummers schrijft.</rdfs:comment><rdfs:comment xml:lang="ur">ایک شخص جو گانے لکھتا ہے۔</rdfs:comment><rdfs:subClassOf rdf:resource="http://dbpedia.org/ontology/Writer"/><owl:equivalentClass rdf:resource="http://www.wikidata.org/entity/Q753110"/><prov:wasDerivedFrom rdf:resource="http://mappings.dbpedia.org/index.php/OntologyClass:SongWriter"/>
        </owl:Class><owl:Class rdf:about="http://dbpedia.org/ontology/Square">
        <rdfs:label xml:lang="nl">plein</rdfs:label><rdfs:label xml:lang="ur">چوکور</rdfs:label><rdfs:label xml:lang="ga">cearnóg</rdfs:label><rdfs:label xml:lang="fr">place</rdfs:label><rdfs:label xml:lang="en">square</rdfs:label><rdfs:label xml:lang="ja">正方形</rdfs:label><rdfs:label xml:lang="de">Platz</rdfs:label><rdfs:subClassOf rdf:resource="http://dbpedia.org/ontology/ArchitecturalStructure"/><owl:equivalentClass rdf:resource="http://www.wikidata.org/entity/Q174782"/><prov:wasDerivedFrom rdf:resource="http://mappings.dbpedia.org/index.php/OntologyClass:Square"/>
        </owl:Class><owl:Class rdf:about="http://dbpedia.org/ontology/University">
        <rdfs:label xml:lang="pl">uniwersytet</rdfs:label><rdfs:label xml:lang="pt">universidade</rdfs:label><rdfs:label xml:lang="nl">universiteit</rdfs:label><rdfs:label xml:lang="el">πανεπιστήμιο</rdfs:label><rdfs:label xml:lang="ko">대학</rdfs:label><rdfs:label xml:lang="ur">جامع درس گاہ</rdfs:label><rdfs:label xml:lang="ga">ollscoil</rdfs:label><rdfs:label xml:lang="fr">université</rdfs:label><rdfs:label xml:lang="es">universidad</rdfs:label><rdfs:label xml:lang="en">university</rdfs:label><rdfs:label xml:lang="ja">大学</rdfs:label><rdfs:label xml:lang="de">Universität</rdfs:label><rdfs:subClassOf rdf:resource="http://dbpedia.org/ontology/EducationalInstitution"/><rdfs:subClassOf rdf:resource="http://schema.org/CollegeOrUniversity"/><owl:equivalentClass rdf:resource="http://www.wikidata.org/entity/Q3918"/><prov:wasDerivedFrom rdf:resource="http://mappings.dbpedia.org/index.php/OntologyClass:University"/>
        </owl:Class><owl:Class rdf:about="http://dbpedia.org/ontology/AnatomicalStructure">
        <rdfs:label xml:lang="nl">anatomische structuur</rdfs:label><rdfs:label xml:lang="el">ανατομική δομή</rdfs:label><rdfs:label xml:lang="ko">해부학</rdfs:label><rdfs:label xml:lang="ur">جسمانی ساخت</rdfs:label><rdfs:label xml:lang="ga">coirpeog</rdfs:label><rdfs:label xml:lang="fr">structure anatomique</rdfs:label><rdfs:label xml:lang="gl">estrutura anatómica</rdfs:label><rdfs:label xml:lang="it">struttura anatomica</rdfs:label><rdfs:label xml:lang="sl">anatomska struktura</rdfs:label><rdfs:label xml:lang="en">anatomical structure</rdfs:label><rdfs:label xml:lang="ja">解剖構造</rdfs:label><rdfs:label xml:lang="de">anatomischen Struktur</rdfs:label><rdfs:subClassOf rdf:resource="http://www.w3.org/2002/07/owl#Thing"/><owl:equivalentClass rdf:resource="http://www.wikidata.org/entity/Q4936952"/><prov:wasDerivedFrom rdf:resource="http://mappings.dbpedia.org/index.php/OntologyClass:AnatomicalStructure"/>
        </owl:Class><owl:Class rdf:about="http://dbpedia.org/ontology/TelevisionShow">
        <rdfs:label xml:lang="nl">televisie show</rdfs:label><rdfs:label xml:lang="el">τηλεοπτική σειρά</rdfs:label><rdfs:label xml:lang="ur">ٹی وی شو</rdfs:label><rdfs:label xml:lang="ga">clár teilifíse</rdfs:label><rdfs:label xml:lang="fr">émission de télévision</rdfs:label><rdfs:label xml:lang="es">serie de televisión</rdfs:label><rdfs:label xml:lang="ar">معلومات تلفاز</rdfs:label><rdfs:label xml:lang="sl">televizijska oddaja</rdfs:label><rdfs:label xml:lang="en">television show</rdfs:label><rdfs:label xml:lang="ja">テレビ番組</rdfs:label><rdfs:label xml:lang="de">Fernsehsendung</rdfs:label><rdfs:subClassOf rdf:resource="http://dbpedia.org/ontology/Work"/><owl:equivalentClass rdf:resource="http://www.wikidata.org/entity/Q15416"/><prov:wasDerivedFrom rdf:resource="http://mappings.dbpedia.org/index.php/OntologyClass:TelevisionShow"/>
        </owl:Class><owl:Class rdf:about="http://dbpedia.org/ontology/LaunchPad">
        <rdfs:label xml:lang="nl">lanceerbasis</rdfs:label><rdfs:label xml:lang="el">ράμπα φορτώσεως</rdfs:label><rdfs:label xml:lang="ur">میزائل چلانے کی جگہ</rdfs:label><rdfs:label xml:lang="ga">ceap lainseála</rdfs:label><rdfs:label xml:lang="fr">rampe de lancement</rdfs:label><rdfs:label xml:lang="en">launch pad</rdfs:label><rdfs:label xml:lang="de">Startrampe</rdfs:label><rdfs:subClassOf rdf:resource="http://dbpedia.org/ontology/Infrastructure"/><owl:equivalentClass rdf:resource="http://www.wikidata.org/entity/Q1353183"/><prov:wasDerivedFrom rdf:resource="http://mappings.dbpedia.org/index.php/OntologyClass:LaunchPad"/>
        </owl:Class><owl:Class rdf:about="http://dbpedia.org/ontology/CyclingLeague">
        <rdfs:label xml:lang="nl">wielerronde</rdfs:label><rdfs:label xml:lang="el">Ομοσπονδία Ποδηλασίας</rdfs:label><rdfs:label xml:lang="ko">사이클 리그</rdfs:label><rdfs:label xml:lang="ur">سائیکل سوار کی انجمن</rdfs:label><rdfs:label xml:lang="fr">ligue de cyclisme</rdfs:label><rdfs:label xml:lang="es">liga de ciclismo</rdfs:label><rdfs:label xml:lang="en">cycling league</rdfs:label><rdfs:label xml:lang="de">Rad-Liga</rdfs:label><rdfs:comment xml:lang="ur">کھیلوں کی ٹیموں کا ایک گروپ جو سائیکلنگ میں ایک دوسرے کے خلاف مقابلہ کرتا ہے۔</rdfs:comment><rdfs:comment xml:lang="en">a group of sports teams that compete against each other in Cycling</rdfs:comment><rdfs:subClassOf rdf:resource="http://dbpedia.org/ontology/SportsLeague"/><prov:wasDerivedFrom rdf:resource="http://mappings.dbpedia.org/index.php/OntologyClass:CyclingLeague"/>
        </owl:Class><owl:Class rdf:about="http://dbpedia.org/ontology/Territory">
        <rdfs:label xml:lang="nl">territorium</rdfs:label><rdfs:label xml:lang="el">περιοχή</rdfs:label><rdfs:label xml:lang="ur">ماتحت علاقہ</rdfs:label><rdfs:label xml:lang="fr">Territoire</rdfs:label><rdfs:label xml:lang="en">territory</rdfs:label><rdfs:label xml:lang="ja">国土</rdfs:label><rdfs:label xml:lang="de">Territorium</rdfs:label><rdfs:comment xml:lang="en">A territory may refer to a country subdivision, a non-sovereign geographic region.</rdfs:comment><rdfs:comment xml:lang="fr">Un territoire peut désigner une subdivision de pays, une région géographique non souveraine.</rdfs:comment><rdfs:comment xml:lang="ur">ایک ماتحت علاقہ کسی ملک کی ذیلی تقسیم، ایک غیر خودمختار جغرافیائی خطہ کا حوالہ دے سکتا ہے۔</rdfs:comment><rdfs:subClassOf rdf:resource="http://dbpedia.org/ontology/PopulatedPlace"/><prov:wasDerivedFrom rdf:resource="http://mappings.dbpedia.org/index.php/OntologyClass:Territory"/>
        </owl:Class><owl:Class rdf:about="http://dbpedia.org/ontology/Tank">
        <rdfs:label xml:lang="en">Tank</rdfs:label><rdfs:label xml:lang="ur">حوض</rdfs:label><rdfs:label xml:lang="ru">Танк</rdfs:label><rdfs:subClassOf rdf:resource="http://www.w3.org/2002/07/owl#Thing"/><prov:wasDerivedFrom rdf:resource="http://mappings.dbpedia.org/index.php/OntologyClass:Tank"/>
        </owl:Class><owl:Class rdf:about="http://dbpedia.org/ontology/CurlingLeague">
        <rdfs:label xml:lang="nl">curling competitie</rdfs:label><rdfs:label xml:lang="el">πρωτάθλημα curling</rdfs:label><rdfs:label xml:lang="ko">컬링 리그</rdfs:label><rdfs:label xml:lang="ur">پتھر کنڈلی کھيل کی انجمن</rdfs:label><rdfs:label xml:lang="ga">sraith curlála</rdfs:label><rdfs:label xml:lang="fr">ligue de curling</rdfs:label><rdfs:label xml:lang="es">liga de curling</rdfs:label><rdfs:label xml:lang="en">curling league</rdfs:label><rdfs:label xml:lang="de">Curling-Liga</rdfs:label><rdfs:comment xml:lang="en">a group of sports teams that compete against each other in Curling</rdfs:comment><rdfs:comment xml:lang="ur">کھیلوں کی ٹیموں کا ایک گروپ جو کرلنگ میں ایک دوسرے کے خلاف مقابلہ کرتے ہیں۔</rdfs:comment><rdfs:subClassOf rdf:resource="http://dbpedia.org/ontology/SportsLeague"/><prov:wasDerivedFrom rdf:resource="http://mappings.dbpedia.org/index.php/OntologyClass:CurlingLeague"/>
        </owl:Class><owl:Class rdf:about="http://dbpedia.org/ontology/GatedCommunity">
        <rdfs:label xml:lang="en">Gated community</rdfs:label><rdfs:label xml:lang="nl">Hofje / gebouw met woongemeenschap</rdfs:label><rdfs:label xml:lang="de">bewachte Wohnanlage / Siedlung</rdfs:label><rdfs:label xml:lang="ur">مسدود برادری</rdfs:label><rdfs:subClassOf rdf:resource="http://dbpedia.org/ontology/PopulatedPlace"/><prov:wasDerivedFrom rdf:resource="http://mappings.dbpedia.org/index.php/OntologyClass:GatedCommunity"/>
        </owl:Class><owl:Class rdf:about="http://dbpedia.org/ontology/MusicFestival">
        <rdfs:label xml:lang="nl">muziekfestival</rdfs:label><rdfs:label xml:lang="el">φεστιβάλ μουσικής</rdfs:label><rdfs:label xml:lang="ko">음악제</rdfs:label><rdfs:label xml:lang="ur">موسیقی میلہ</rdfs:label><rdfs:label xml:lang="fr">festival de musique</rdfs:label><rdfs:label xml:lang="es">festival de música</rdfs:label><rdfs:label xml:lang="en">music festival</rdfs:label><rdfs:label xml:lang="de">Musikfestival</rdfs:label><rdfs:subClassOf rdf:resource="http://dbpedia.org/ontology/SocietalEvent"/><owl:equivalentClass rdf:resource="http://www.wikidata.org/entity/Q868557"/><owl:equivalentClass rdf:resource="http://schema.org/Festival"/><prov:wasDerivedFrom rdf:resource="http://mappings.dbpedia.org/index.php/OntologyClass:MusicFestival"/>
        </owl:Class><owl:Class rdf:about="http://dbpedia.org/ontology/Tax">
        <rdfs:label xml:lang="nl">belasting</rdfs:label><rdfs:label xml:lang="el">φόρος</rdfs:label><rdfs:label xml:lang="ur">محصول</rdfs:label><rdfs:label xml:lang="ga">cáin</rdfs:label><rdfs:label xml:lang="fr">taxe</rdfs:label><rdfs:label xml:lang="es">impuesto</rdfs:label><rdfs:label xml:lang="en">tax</rdfs:label><rdfs:label xml:lang="ja">租税</rdfs:label><rdfs:label xml:lang="de">Steuer</rdfs:label><rdfs:subClassOf rdf:resource="http://dbpedia.org/ontology/TopicalConcept"/><owl:equivalentClass rdf:resource="http://www.wikidata.org/entity/Q8161"/><prov:wasDerivedFrom rdf:resource="http://mappings.dbpedia.org/index.php/OntologyClass:Tax"/>
        </owl:Class><owl:Class rdf:about="http://dbpedia.org/ontology/Racecourse">
        <rdfs:label xml:lang="nl">renbaan</rdfs:label><rdfs:label xml:lang="el">ιππόδρομος</rdfs:label><rdfs:label xml:lang="ur">بھاگنے والا رستہ</rdfs:label><rdfs:label xml:lang="ga">ráschúrsa</rdfs:label><rdfs:label xml:lang="it">ippodromo</rdfs:label><rdfs:label xml:lang="en">racecourse</rdfs:label><rdfs:label xml:lang="ja">競馬場</rdfs:label><rdfs:label xml:lang="de">Rennbahn</rdfs:label><rdfs:comment xml:lang="en">A racecourse is an alternate term for a horse racing track, found in countries such as the United Kingdom, Australia, Hong Kong, and the United Arab Emirates.</rdfs:comment><rdfs:comment xml:lang="ur">ریس کورس ہارس ریسنگ ٹریک کے لیے ایک متبادل اصطلاح ہے، جو برطانیہ، آسٹریلیا، ہانگ کانگ اور متحدہ عرب امارات جیسے ممالک میں پائی جاتی ہے۔</rdfs:comment><rdfs:comment xml:lang="el">Ο ιππόδρομος,εναλλακτικός όρος για την πίστα διεξαγωγής αγώνων μεταξύ ίππων,συναντάται σε χώρες όπως η Αγγλία, Αυστραλία, Χονγκ Κονγκ και τα Ηνωμένα Αραβικά Εμιράτα.</rdfs:comment><rdfs:subClassOf rdf:resource="http://dbpedia.org/ontology/RaceTrack"/><owl:equivalentClass rdf:resource="http://www.wikidata.org/entity/Q1777138"/><prov:wasDerivedFrom rdf:resource="http://mappings.dbpedia.org/index.php/OntologyClass:Racecourse"/>
        </owl:Class><owl:Class rdf:about="http://dbpedia.org/ontology/Dancer">
        <rdfs:label xml:lang="pl">tancerz</rdfs:label><rdfs:label xml:lang="nl">danser</rdfs:label><rdfs:label xml:lang="el">χορευτής</rdfs:label><rdfs:label xml:lang="ur">رقص کرنے والا</rdfs:label><rdfs:label xml:lang="ga">damhsóir</rdfs:label><rdfs:label xml:lang="fr">danceur</rdfs:label><rdfs:label xml:lang="it">ballerino</rdfs:label><rdfs:label xml:lang="en">dancer</rdfs:label><rdfs:label xml:lang="ja">ダンサー</rdfs:label><rdfs:label xml:lang="de">Tänzer</rdfs:label><rdfs:subClassOf rdf:resource="http://dbpedia.org/ontology/Artist"/><prov:wasDerivedFrom rdf:resource="http://mappings.dbpedia.org/index.php/OntologyClass:Dancer"/>
        </owl:Class><owl:Class rdf:about="http://dbpedia.org/ontology/IceHockeyPlayer">
        <rdfs:label xml:lang="nl">ijshockeyspeler</rdfs:label><rdfs:label xml:lang="el">παίκτης χόκεϋ</rdfs:label><rdfs:label xml:lang="ko">아이스하키 선수</rdfs:label><rdfs:label xml:lang="ur">برفانی ہاکی کا کھلاڑی</rdfs:label><rdfs:label xml:lang="fr">joueur de hockey sur glace</rdfs:label><rdfs:label xml:lang="en">ice hockey player</rdfs:label><rdfs:label xml:lang="de">Eishockeyspieler</rdfs:label><rdfs:subClassOf rdf:resource="http://dbpedia.org/ontology/WinterSportPlayer"/><owl:equivalentClass rdf:resource="http://www.wikidata.org/entity/Q11774891"/><prov:wasDerivedFrom rdf:resource="http://mappings.dbpedia.org/index.php/OntologyClass:IceHockeyPlayer"/>
        </owl:Class><owl:Class rdf:about="http://dbpedia.org/ontology/PublicTransitSystem">
        <rdfs:label xml:lang="nl">openbaar vervoer systeem</rdfs:label><rdfs:label xml:lang="el">μέσα μαζικής μεταφοράς</rdfs:label><rdfs:label xml:lang="ur">عوامی راہداری کا نظام</rdfs:label><rdfs:label xml:lang="fr">Système de transport public</rdfs:label><rdfs:label xml:lang="es">Sistema de Transporte Público</rdfs:label><rdfs:label xml:lang="en">public transit system</rdfs:label><rdfs:label xml:lang="de">Öffentliches Personenverkehrssystem</rdfs:label><rdfs:comment xml:lang="el">Τα μέσα μαζικής μεταφοράς (συντομογραφία ΜΜΜ) είναι τα δημόσια συγκοινωνιακά μέσα, που περιλαμβάνουν τα λεωφορεία, τα τρόλεϊ, τα τραμ, τα τρένα, το μετρό, τα πλοία. Υπάρχουν και τα ταχεία μέσα συγκοινωνίας που περιλαμβάνουν τα αεροπλάνα, υπερταχεία τρένα.</rdfs:comment><rdfs:comment xml:lang="ur">عوامی راہداری کا نظام ایک مشترکہ عوامی نقل و حمل کی سروس ہے جو عام لوگوں کے استعمال کے لیے دستیاب ہے۔عوامی نقل و حمل کے طریقوں میں بسیں ، ٹرالی بسیں ، ٹرام اور ٹرینیں ، 'تیز رفتارراہداری' (میٹرو/زمین دوز برقی ریل/زیر زمین وغیرہ) اور فیری شامل ہیں۔</rdfs:comment><rdfs:comment xml:lang="fr">Un système de transport en commun est un service de transport partagé de passagers mis à la disposition du grand public. Les modes de transport public comprennent les bus, les trolleybus, les tramways et les trains, le « transport en commun rapide » (métro, TGV, etc.) et les ferries. Les transports publics interurbains sont dominés par les compagnies aériennes, les autocars et le rail intercité. (http://en.wikipedia.org/wiki/Public_transit).</rdfs:comment><rdfs:comment xml:lang="en">A public transit system is a shared passenger transportation service which is available for use by the general public. Public transport modes include buses, trolleybuses, trams and trains, 'rapid transit' (metro/subways/undergrounds etc) and ferries. Intercity public transport is dominated by airlines, coaches, and intercity rail. (http://en.wikipedia.org/wiki/Public_transit).</rdfs:comment><rdfs:comment xml:lang="de">Ein System des Öffentlichen Personenverkehrs auf Straße, Schiene oder Wasser.</rdfs:comment><rdfs:subClassOf rdf:resource="http://dbpedia.org/ontology/Company"/><prov:wasDerivedFrom rdf:resource="http://mappings.dbpedia.org/index.php/OntologyClass:PublicTransitSystem"/>
        </owl:Class><owl:Class rdf:about="http://dbpedia.org/ontology/BloodVessel">
        <rdfs:label xml:lang="en">blood vessel</rdfs:label><rdfs:label xml:lang="nl">bloedvat</rdfs:label><rdfs:label xml:lang="fr">vaisseau sanguin</rdfs:label><rdfs:label xml:lang="ur">خون کی شریان</rdfs:label><rdfs:subClassOf rdf:resource="http://dbpedia.org/ontology/AnatomicalStructure"/><prov:wasDerivedFrom rdf:resource="http://mappings.dbpedia.org/index.php/OntologyClass:BloodVessel"/>
        </owl:Class><owl:Class rdf:about="http://dbpedia.org/ontology/FootballMatch">
        <rdfs:label xml:lang="pl">mecz piłki nożnej</rdfs:label><rdfs:label xml:lang="nl">voetbal wedstrijd</rdfs:label><rdfs:label xml:lang="el">αγώνας ποδοσφαίρου</rdfs:label><rdfs:label xml:lang="ur">فٹ بال مقابلہ</rdfs:label><rdfs:label xml:lang="ga">cluiche peile</rdfs:label><rdfs:label xml:lang="es">partido de fútbol</rdfs:label><rdfs:label xml:lang="en">football match</rdfs:label><rdfs:label xml:lang="de">Fußballspiel</rdfs:label><rdfs:comment xml:lang="en">a competition between two football teams</rdfs:comment><rdfs:comment xml:lang="ur">دو فٹ بال ٹیموں کے درمیان مقابلہ</rdfs:comment><rdfs:subClassOf rdf:resource="http://dbpedia.org/ontology/SportsEvent"/><prov:wasDerivedFrom rdf:resource="http://mappings.dbpedia.org/index.php/OntologyClass:FootballMatch"/>
        </owl:Class><owl:Class rdf:about="http://dbpedia.org/ontology/MouseGeneLocation">
        <rdfs:label xml:lang="nl">muisgenoom locatie</rdfs:label><rdfs:label xml:lang="ur">چوہے کے نَسبہ کا مقام</rdfs:label><rdfs:label xml:lang="en">MouseGeneLocation</rdfs:label><rdfs:label xml:lang="ja">マウス遺伝子座</rdfs:label><rdfs:label xml:lang="de">Mausgenom Lokation</rdfs:label><rdfs:subClassOf rdf:resource="http://dbpedia.org/ontology/GeneLocation"/><prov:wasDerivedFrom rdf:resource="http://mappings.dbpedia.org/index.php/OntologyClass:MouseGeneLocation"/>
        </owl:Class><owl:Class rdf:about="http://dbpedia.org/ontology/MilitaryConflict">
        <rdfs:label xml:lang="nl">militair conflict</rdfs:label><rdfs:label xml:lang="el">στρατιωτική σύγκρουση</rdfs:label><rdfs:label xml:lang="ko">전쟁</rdfs:label><rdfs:label xml:lang="ur">فوجی تنازعہ</rdfs:label><rdfs:label xml:lang="fr">conflit militaire</rdfs:label><rdfs:label xml:lang="en">military conflict</rdfs:label><rdfs:label xml:lang="da">militær konflikt</rdfs:label><rdfs:label xml:lang="de">militärischer Konflikt</rdfs:label><rdfs:subClassOf rdf:resource="http://dbpedia.org/ontology/SocietalEvent"/><prov:wasDerivedFrom rdf:resource="http://mappings.dbpedia.org/index.php/OntologyClass:MilitaryConflict"/>
        </owl:Class><owl:Class rdf:about="http://dbpedia.org/ontology/StatedResolution">
        <rdfs:label xml:lang="nl">Aangenomen Besluit</rdfs:label><rdfs:label xml:lang="ur">ریاستی قرارداد</rdfs:label><rdfs:label xml:lang="fr">Résolution adoptée</rdfs:label><rdfs:label xml:lang="en">Stated Resolution</rdfs:label><rdfs:label xml:lang="de">Angenommen Beschluß</rdfs:label><rdfs:comment xml:lang="en">A Resolution describes a formal statement adopted by a meeting or convention.</rdfs:comment><rdfs:comment xml:lang="ur">ایک قرارداد میٹنگ یا کنونشن کے ذریعہ اختیار کردہ ایک رسمی بیان کی وضاحت کرتی ہے</rdfs:comment><rdfs:comment xml:lang="fr">Une résolution décrit une déclaration officielle adoptée par une réunion ou une convention.</rdfs:comment><rdfs:comment xml:lang="nl">Een Besluit of Verklaring beschrijft een formeel besluit of formele aanbeveling aangenomen door een vergadering.</rdfs:comment><rdfs:subClassOf rdf:resource="http://dbpedia.org/ontology/WrittenWork"/><prov:wasDerivedFrom rdf:resource="http://mappings.dbpedia.org/index.php/OntologyClass:StatedResolution"/>
        </owl:Class><owl:Class rdf:about="http://dbpedia.org/ontology/Tram">
        <rdfs:label xml:lang="nl">tram</rdfs:label><rdfs:label xml:lang="ur">ٹرام گاڑی</rdfs:label><rdfs:label xml:lang="fr">tramway</rdfs:label><rdfs:label xml:lang="en">streetcar</rdfs:label><rdfs:label xml:lang="ja">路面電車</rdfs:label><rdfs:label xml:lang="de">Straßenbahn</rdfs:label><rdfs:subClassOf rdf:resource="http://dbpedia.org/ontology/MeanOfTransportation"/><prov:wasDerivedFrom rdf:resource="http://mappings.dbpedia.org/index.php/OntologyClass:Tram"/>
        </owl:Class><owl:Class rdf:about="http://dbpedia.org/ontology/FilmFestival">
        <rdfs:label xml:lang="pl">festiwal filmowy</rdfs:label><rdfs:label xml:lang="nl">filmfestival</rdfs:label><rdfs:label xml:lang="el">φεστιβάλ κινηματογράφου</rdfs:label><rdfs:label xml:lang="ko">영화제</rdfs:label><rdfs:label xml:lang="ur">فلمی میلہ</rdfs:label><rdfs:label xml:lang="ga">féile scannán</rdfs:label><rdfs:label xml:lang="fr">festival du film</rdfs:label><rdfs:label xml:lang="en">film festival</rdfs:label><rdfs:label xml:lang="da">filmfestival</rdfs:label><rdfs:label xml:lang="ja">映画祭</rdfs:label><rdfs:label xml:lang="de">Filmfestival</rdfs:label><rdfs:subClassOf rdf:resource="http://dbpedia.org/ontology/SocietalEvent"/><rdfs:subClassOf rdf:resource="http://schema.org/Festival"/><owl:equivalentClass rdf:resource="http://www.wikidata.org/entity/Q220505"/><prov:wasDerivedFrom rdf:resource="http://mappings.dbpedia.org/index.php/OntologyClass:FilmFestival"/>
        </owl:Class><owl:Class rdf:about="http://dbpedia.org/ontology/MonoclonalAntibody">
        <rdfs:label xml:lang="de">monoklonaler Antikörper</rdfs:label><rdfs:label xml:lang="en">monoclonal antibody</rdfs:label><rdfs:label xml:lang="ur">مونوکلونل دافِع جِسم</rdfs:label><rdfs:label xml:lang="fr">monoclonal anticorps</rdfs:label><rdfs:comment xml:lang="en">Medikamente welche monoklonale Antikörper sind</rdfs:comment><rdfs:comment xml:lang="ur">وہ دوائیں جو ایک مونوکلونل دافِع جِسم ہیں۔‎‎</rdfs:comment><rdfs:subClassOf rdf:resource="http://dbpedia.org/ontology/Drug"/><prov:wasDerivedFrom rdf:resource="http://mappings.dbpedia.org/index.php/OntologyClass:MonoclonalAntibody"/>
        </owl:Class><owl:Class rdf:about="http://dbpedia.org/ontology/TheatreDirector">
        <rdfs:label xml:lang="nl">theaterdirecteur</rdfs:label><rdfs:label xml:lang="ur">تھیٹر ہدایت کار</rdfs:label><rdfs:label xml:lang="fr">directeur de théâtre</rdfs:label><rdfs:label xml:lang="en">Theatre director</rdfs:label><rdfs:label xml:lang="de">Theaterdirektor</rdfs:label><rdfs:comment xml:lang="en">A director in the theatre field who oversees and orchestrates the mounting of a theatre production.</rdfs:comment><rdfs:comment xml:lang="ur">تھیٹر کے میدان میں ایک ڈائریکٹر جو تھیٹر پروڈکشن کے بڑھتے ہوئے کام کی نگرانی اور آرکیسٹریٹ کرتا ہے</rdfs:comment><rdfs:subClassOf rdf:resource="http://dbpedia.org/ontology/Person"/><owl:equivalentClass rdf:resource="http://www.wikidata.org/entity/Q3387717"/><prov:wasDerivedFrom rdf:resource="http://mappings.dbpedia.org/index.php/OntologyClass:TheatreDirector"/>
        </owl:Class><owl:Class rdf:about="http://dbpedia.org/ontology/Beverage">
        <rdfs:label xml:lang="nl">drank</rdfs:label><rdfs:label xml:lang="el">αναψυκτικό</rdfs:label><rdfs:label xml:lang="ko">음료</rdfs:label><rdfs:label xml:lang="ur">مشروب</rdfs:label><rdfs:label xml:lang="ga">deoch</rdfs:label><rdfs:label xml:lang="fr">boisson</rdfs:label><rdfs:label xml:lang="es">bebida</rdfs:label><rdfs:label xml:lang="it">bevanda</rdfs:label><rdfs:label xml:lang="en">beverage</rdfs:label><rdfs:label xml:lang="da">drik</rdfs:label><rdfs:label xml:lang="ja">飲料</rdfs:label><rdfs:label xml:lang="de">Getränk</rdfs:label><rdfs:comment xml:lang="en">A drink, or beverage, is a liquid which is specifically prepared for human consumption.</rdfs:comment><rdfs:comment xml:lang="de">Ein Getränk ist eine zum Trinken zubereitete Flüssigkeit. Getränke werden entweder zum Stillen von Durst und damit zur Wasseraufnahme des Körpers, als Nahrungsmittel oder auch als reine Genussmittel aufgenommen.</rdfs:comment><rdfs:comment xml:lang="el">Ένα πόσιμο υγρό ρόφημα, συνήθως με μηδενική ή ελάχιστη περιεκτικότητα αλκοόλης.</rdfs:comment><rdfs:comment xml:lang="ur">یک مشروب مائع ہے جو خاص طور پر انسانی استعمال کے لیے تیار کیا جاتا ہے۔</rdfs:comment><rdfs:subClassOf rdf:resource="http://dbpedia.org/ontology/Food"/><prov:wasDerivedFrom rdf:resource="http://mappings.dbpedia.org/index.php/OntologyClass:Beverage"/>
        </owl:Class><owl:Class rdf:about="http://dbpedia.org/ontology/SpaceShuttle">
        <rdfs:label xml:lang="nl">ruimteveer</rdfs:label><rdfs:label xml:lang="el">διαστημικό λεωφορείο</rdfs:label><rdfs:label xml:lang="ko">우주 왕복선</rdfs:label><rdfs:label xml:lang="ur">خلائی جہاز</rdfs:label><rdfs:label xml:lang="ga">spástointeáil</rdfs:label><rdfs:label xml:lang="fr">navette spatiale</rdfs:label><rdfs:label xml:lang="en">space shuttle</rdfs:label><rdfs:label xml:lang="de">Raumfähre</rdfs:label><rdfs:subClassOf rdf:resource="http://dbpedia.org/ontology/MeanOfTransportation"/><owl:equivalentClass rdf:resource="http://www.wikidata.org/entity/Q48806"/><prov:wasDerivedFrom rdf:resource="http://mappings.dbpedia.org/index.php/OntologyClass:SpaceShuttle"/>
        </owl:Class><owl:Class rdf:about="http://dbpedia.org/ontology/EmployersOrganisation">
        <rdfs:label xml:lang="nl">werkgeversorganisatie</rdfs:label><rdfs:label xml:lang="ur">آجروں کی تنظیم</rdfs:label><rdfs:label xml:lang="fr">syndicat de patrons</rdfs:label><rdfs:label xml:lang="en">Employers' Organisation</rdfs:label><rdfs:label xml:lang="de">Arbeitgeberverbände</rdfs:label><rdfs:comment xml:lang="ur">ملازمین کی تنظیم تاجروں کی ایک تنظیم ہے جو مزدور تعلقات کے میدان میں اپنے اعمال کو مربوط کرنے کے لیے مل کر کام کرتی ہے۔</rdfs:comment><rdfs:comment xml:lang="en">An employers' organisation is an organisation of entrepreneurs who work together to coordinate their actions in the field of labour relations</rdfs:comment><rdfs:subClassOf rdf:resource="http://dbpedia.org/ontology/Organisation"/><prov:wasDerivedFrom rdf:resource="http://mappings.dbpedia.org/index.php/OntologyClass:EmployersOrganisation"/>
        </owl:Class><owl:Class rdf:about="http://dbpedia.org/ontology/Prison">
        <rdfs:label xml:lang="nl">gevangenis</rdfs:label><rdfs:label xml:lang="el">φυλακή</rdfs:label><rdfs:label xml:lang="ur">جیل</rdfs:label><rdfs:label xml:lang="ga">príosún</rdfs:label><rdfs:label xml:lang="fr">prison</rdfs:label><rdfs:label xml:lang="it">prigione</rdfs:label><rdfs:label xml:lang="en">prison</rdfs:label><rdfs:label xml:lang="ja">刑務所</rdfs:label><rdfs:label xml:lang="de">gefängnis</rdfs:label><rdfs:subClassOf rdf:resource="http://dbpedia.org/ontology/Building"/><owl:equivalentClass rdf:resource="http://www.wikidata.org/entity/Q40357"/><prov:wasDerivedFrom rdf:resource="http://mappings.dbpedia.org/index.php/OntologyClass:Prison"/>
        </owl:Class><owl:Class rdf:about="http://dbpedia.org/ontology/Archaea">
        <rdfs:label xml:lang="nl">Archaea (oerbacteriën)</rdfs:label><rdfs:label xml:lang="el">αρχαία</rdfs:label><rdfs:label xml:lang="ko">고세균</rdfs:label><rdfs:label xml:lang="ur">آثار قدیمہ</rdfs:label><rdfs:label xml:lang="fr">archées</rdfs:label><rdfs:label xml:lang="it">archei</rdfs:label><rdfs:label xml:lang="en">archaea</rdfs:label><rdfs:label xml:lang="ja">古細菌</rdfs:label><rdfs:label xml:lang="de">Archaeen</rdfs:label><rdfs:subClassOf rdf:resource="http://dbpedia.org/ontology/Species"/><prov:wasDerivedFrom rdf:resource="http://mappings.dbpedia.org/index.php/OntologyClass:Archaea"/>
        </owl:Class><owl:Class rdf:about="http://dbpedia.org/ontology/HandballPlayer">
        <rdfs:label xml:lang="nl">handballer</rdfs:label><rdfs:label xml:lang="el">παίκτης του handball</rdfs:label><rdfs:label xml:lang="ur">ہینڈ بال کا کھلاڑی</rdfs:label><rdfs:label xml:lang="ga">imreoir liathróid láimhe</rdfs:label><rdfs:label xml:lang="fr">joueur de handball</rdfs:label><rdfs:label xml:lang="es">jugador de balonmano</rdfs:label><rdfs:label xml:lang="en">handball player</rdfs:label><rdfs:label xml:lang="da">håndboldspiller</rdfs:label><rdfs:label xml:lang="de">Handballspieler</rdfs:label><rdfs:comment xml:lang="ur">ایک کھیل جِس میں دو یا چار کھِلاڑی بَند احاطے میں ربَڑ کی چھوٹی گیند کو ہاتھوں سے دیوار پَر مارتے ہیں</rdfs:comment><rdfs:subClassOf rdf:resource="http://dbpedia.org/ontology/Athlete"/><owl:equivalentClass rdf:resource="http://www.wikidata.org/entity/Q13365117"/><prov:wasDerivedFrom rdf:resource="http://mappings.dbpedia.org/index.php/OntologyClass:HandballPlayer"/>
        </owl:Class><owl:Class rdf:about="http://dbpedia.org/ontology/Man">
        <rdfs:label xml:lang="pl">Mężczyzna</rdfs:label><rdfs:label xml:lang="nl">Mens</rdfs:label><rdfs:label xml:lang="ko">남자</rdfs:label><rdfs:label xml:lang="ur">آدمی</rdfs:label><rdfs:label xml:lang="fr">Homme</rdfs:label><rdfs:label xml:lang="it">Uomo</rdfs:label><rdfs:label xml:lang="ru">мужчина</rdfs:label><rdfs:label xml:lang="en">man</rdfs:label><rdfs:label xml:lang="da">Mand</rdfs:label><rdfs:label xml:lang="ja">おとこ</rdfs:label><rdfs:label xml:lang="de">Mann</rdfs:label><rdfs:subClassOf rdf:resource="http://dbpedia.org/ontology/Person"/><owl:equivalentClass rdf:resource="http://www.wikidata.org/entity/Q8441"/><prov:wasDerivedFrom rdf:resource="http://mappings.dbpedia.org/index.php/OntologyClass:Man"/>
        </owl:Class><owl:Class rdf:about="http://dbpedia.org/ontology/Covid19">
        <rdfs:label xml:lang="en">COVID-19 pandemic</rdfs:label><rdfs:label xml:lang="fr">Pandémie COVID-19</rdfs:label><rdfs:label xml:lang="zh">2019冠状病毒病疫情</rdfs:label><rdfs:label xml:lang="ur">کورونا وائرس2019</rdfs:label><rdfs:comment xml:lang="ur">کورونا وائرس کی بیماری 2019 کی جاری وبائی بیماری۔</rdfs:comment><rdfs:comment xml:lang="en">Ongoing pandemic of coronavirus disease 2019</rdfs:comment><rdfs:comment xml:lang="fr">Pandémie actuelle de maladie coronavirus 2019</rdfs:comment><rdfs:comment xml:lang="zh">2019冠狀病毒病疫情是一次由严重急性呼吸系统综合征冠状病毒导致的2019冠状病毒病所引發的全球大流行疫情</rdfs:comment><rdfs:subClassOf rdf:resource="http://www.w3.org/2002/07/owl#Thing"/><owl:equivalentClass rdf:resource="http://www.wikidata.org/entity/Q84263196"/><prov:wasDerivedFrom rdf:resource="http://mappings.dbpedia.org/index.php/OntologyClass:Covid19"/>
        </owl:Class><owl:Class rdf:about="http://dbpedia.org/ontology/Woman">
        <rdfs:label xml:lang="pl">kobieta</rdfs:label><rdfs:label xml:lang="nl">vrouw</rdfs:label><rdfs:label xml:lang="ko">여자</rdfs:label><rdfs:label xml:lang="ur">عورت</rdfs:label><rdfs:label xml:lang="fr">femme</rdfs:label><rdfs:label xml:lang="it">donna</rdfs:label><rdfs:label xml:lang="ru">женщина</rdfs:label><rdfs:label xml:lang="en">woman</rdfs:label><rdfs:label xml:lang="da">kvinde</rdfs:label><rdfs:label xml:lang="ja">女性</rdfs:label><rdfs:label xml:lang="de">Frauen</rdfs:label><rdfs:subClassOf rdf:resource="http://dbpedia.org/ontology/Person"/><owl:equivalentClass rdf:resource="http://www.wikidata.org/entity/Q467"/><prov:wasDerivedFrom rdf:resource="http://mappings.dbpedia.org/index.php/OntologyClass:Woman"/>
        </owl:Class><owl:Class rdf:about="http://dbpedia.org/ontology/Religious">
        <rdfs:label xml:lang="nl">religieus</rdfs:label><rdfs:label xml:lang="el">θρησκευτικός</rdfs:label><rdfs:label xml:lang="ur">مذہبی</rdfs:label><rdfs:label xml:lang="fr">religieux</rdfs:label><rdfs:label xml:lang="en">religious</rdfs:label><rdfs:label xml:lang="de">religiös</rdfs:label><rdfs:subClassOf rdf:resource="http://dbpedia.org/ontology/Person"/><owl:equivalentClass rdf:resource="http://www.wikidata.org/entity/Q2566598"/><prov:wasDerivedFrom rdf:resource="http://mappings.dbpedia.org/index.php/OntologyClass:Religious"/>
        </owl:Class><owl:Class rdf:about="http://dbpedia.org/ontology/Arachnid">
        <rdfs:label xml:lang="pt">aracnídeos</rdfs:label><rdfs:label xml:lang="nl">spinachtigen</rdfs:label><rdfs:label xml:lang="el">αραχνοειδές</rdfs:label><rdfs:label xml:lang="ko">거미강</rdfs:label><rdfs:label xml:lang="ur">عنکبات</rdfs:label><rdfs:label xml:lang="ga">araicnid</rdfs:label><rdfs:label xml:lang="fr">arachnides</rdfs:label><rdfs:label xml:lang="es">arácnido</rdfs:label><rdfs:label xml:lang="it">aracnide</rdfs:label><rdfs:label xml:lang="en">arachnid</rdfs:label><rdfs:label xml:lang="ja">クモ綱</rdfs:label><rdfs:label xml:lang="de">Spinnentier</rdfs:label><rdfs:comment xml:lang="ur">حیوانیات میں اِس خاندان کا نام جِس میں مکڑی اور بچھو وغیرہ شامِل ہیں</rdfs:comment><rdfs:subClassOf rdf:resource="http://dbpedia.org/ontology/Animal"/><prov:wasDerivedFrom rdf:resource="http://mappings.dbpedia.org/index.php/OntologyClass:Arachnid"/>
        </owl:Class><owl:Class rdf:about="http://dbpedia.org/ontology/Department">
        <rdfs:label xml:lang="nl">departement</rdfs:label><rdfs:label xml:lang="el">τμήμα</rdfs:label><rdfs:label xml:lang="ko">부서</rdfs:label><rdfs:label xml:lang="ur">شعبہ</rdfs:label><rdfs:label xml:lang="ga">roinn</rdfs:label><rdfs:label xml:lang="fr">département</rdfs:label><rdfs:label xml:lang="es">Distrito</rdfs:label><rdfs:label xml:lang="en">department</rdfs:label><rdfs:label xml:lang="de">Distrikt</rdfs:label><rdfs:subClassOf rdf:resource="http://dbpedia.org/ontology/GovernmentalAdministrativeRegion"/><prov:wasDerivedFrom rdf:resource="http://mappings.dbpedia.org/index.php/OntologyClass:Department"/>
        </owl:Class><owl:Class rdf:about="http://dbpedia.org/ontology/CardinalDirection">
        <rdfs:label xml:lang="nl">windrichting</rdfs:label><rdfs:label xml:lang="ur">ہوا کی سمت</rdfs:label><rdfs:label xml:lang="fr">direction cardinale</rdfs:label><rdfs:label xml:lang="en">Cardinal direction</rdfs:label><rdfs:label xml:lang="de">Windrichtung</rdfs:label><rdfs:comment xml:lang="en">One of the four main directions on a compass or any other system to determine a geographical position</rdfs:comment><rdfs:comment xml:lang="fr">Une des 4 principales directions d'un compas ou  de tout autre système pour déterminer une position geographique</rdfs:comment><rdfs:comment xml:lang="ur">جغرافیائی پوزیشن کا تعین کرنے کے لیے کمپاس یا کسی دوسرے نظام پر چار اہم سمتوں میں سے ایک</rdfs:comment><rdfs:subClassOf rdf:resource="http://dbpedia.org/ontology/TopicalConcept"/><prov:wasDerivedFrom rdf:resource="http://mappings.dbpedia.org/index.php/OntologyClass:CardinalDirection"/>
        </owl:Class><owl:Class rdf:about="http://dbpedia.org/ontology/Chief">
        <rdfs:label xml:lang="en">Chief</rdfs:label><rdfs:label xml:lang="ur">چیف(سردار)</rdfs:label><rdfs:label xml:lang="fr">Chef</rdfs:label><rdfs:subClassOf rdf:resource="http://dbpedia.org/ontology/Politician"/><owl:equivalentClass rdf:resource="http://www.wikidata.org/entity/Q1259323"/><prov:wasDerivedFrom rdf:resource="http://mappings.dbpedia.org/index.php/OntologyClass:Chief"/>
        </owl:Class><owl:Class rdf:about="http://dbpedia.org/ontology/Painter">
        <rdfs:label xml:lang="nl">schilder</rdfs:label><rdfs:label xml:lang="el">ζωγράφος</rdfs:label><rdfs:label xml:lang="ur">رنگ ساز</rdfs:label><rdfs:label xml:lang="fr">peintre</rdfs:label><rdfs:label xml:lang="en">painter</rdfs:label><rdfs:label xml:lang="da">maler</rdfs:label><rdfs:label xml:lang="ja">画家</rdfs:label><rdfs:label xml:lang="de">Maler</rdfs:label><rdfs:subClassOf rdf:resource="http://dbpedia.org/ontology/Artist"/><owl:equivalentClass rdf:resource="http://www.wikidata.org/entity/Q1028181"/><prov:wasDerivedFrom rdf:resource="http://mappings.dbpedia.org/index.php/OntologyClass:Painter"/>
        </owl:Class><owl:Class rdf:about="http://dbpedia.org/ontology/LineOfFashion">
        <rdfs:label xml:lang="nl">modelijn</rdfs:label><rdfs:label xml:lang="ur">قطار رائج</rdfs:label><rdfs:label xml:lang="fr">type de couture</rdfs:label><rdfs:label xml:lang="en">line of fashion</rdfs:label><rdfs:label xml:lang="de">Modelinie</rdfs:label><rdfs:comment xml:lang="en">A coherent type of clothing or dressing following a particular fashion</rdfs:comment><rdfs:comment xml:lang="ur">ایک مربوط قسم کا لباس یا لباس کسی خاص فیشن کے بعد</rdfs:comment><rdfs:comment xml:lang="nl">Een samenhangend geheel van kleding in een bepaalde stijl volgens een bepaalde mode.</rdfs:comment><rdfs:subClassOf rdf:resource="http://dbpedia.org/ontology/Work"/><prov:wasDerivedFrom rdf:resource="http://mappings.dbpedia.org/index.php/OntologyClass:LineOfFashion"/>
        </owl:Class><owl:Class rdf:about="http://dbpedia.org/ontology/Sailor">
        <rdfs:label xml:lang="hi">नाविक</rdfs:label><rdfs:label xml:lang="ur">ملاح</rdfs:label><rdfs:label xml:lang="fr">Navigatrice</rdfs:label><rdfs:label xml:lang="ar">بحار</rdfs:label><rdfs:label xml:lang="en">Sailor</rdfs:label><rdfs:label xml:lang="da">Sømand</rdfs:label><rdfs:label xml:lang="eu">Marinela</rdfs:label><rdfs:subClassOf rdf:resource="http://dbpedia.org/ontology/Athlete"/><prov:wasDerivedFrom rdf:resource="http://mappings.dbpedia.org/index.php/OntologyClass:Sailor"/>
        </owl:Class><owl:Class rdf:about="http://dbpedia.org/ontology/Park">
        <rdfs:label xml:lang="pt">parque</rdfs:label><rdfs:label xml:lang="nl">park</rdfs:label><rdfs:label xml:lang="el">πάρκο</rdfs:label><rdfs:label xml:lang="ko">공원</rdfs:label><rdfs:label xml:lang="ur">تفریح گاہ</rdfs:label><rdfs:label xml:lang="ga">páirc</rdfs:label><rdfs:label xml:lang="fr">parc</rdfs:label><rdfs:label xml:lang="en">park</rdfs:label><rdfs:label xml:lang="ja">公園</rdfs:label><rdfs:label xml:lang="de">Park</rdfs:label><rdfs:comment xml:lang="en">A park is an area of open space provided for recreational use. http://en.wikipedia.org/wiki/Park</rdfs:comment><rdfs:comment xml:lang="ur">پارک کھلی جگہ کا ایک علاقہ ہے جو تفریحی استعمال کے لیے فراہم کی جاتی ہے۔</rdfs:comment><rdfs:subClassOf rdf:resource="http://dbpedia.org/ontology/Place"/><owl:equivalentClass rdf:resource="http://schema.org/Park"/><prov:wasDerivedFrom rdf:resource="http://mappings.dbpedia.org/index.php/OntologyClass:Park"/>
        </owl:Class><owl:Class rdf:about="http://dbpedia.org/ontology/CyclingTeam">
        <rdfs:label xml:lang="nl">wielerploeg</rdfs:label><rdfs:label xml:lang="el">ομάδα ποδηλασίας</rdfs:label><rdfs:label xml:lang="ko">사이클 팀</rdfs:label><rdfs:label xml:lang="ur">سائیکلنگ جماعت</rdfs:label><rdfs:label xml:lang="ga">foireann rothaíochta</rdfs:label><rdfs:label xml:lang="fr">équipe cycliste</rdfs:label><rdfs:label xml:lang="it">squadra di ciclismo</rdfs:label><rdfs:label xml:lang="en">cycling team</rdfs:label><rdfs:label xml:lang="da">cykelhold</rdfs:label><rdfs:label xml:lang="de">Radsportteam</rdfs:label><rdfs:subClassOf rdf:resource="http://dbpedia.org/ontology/SportsTeam"/><prov:wasDerivedFrom rdf:resource="http://mappings.dbpedia.org/index.php/OntologyClass:CyclingTeam"/>
        </owl:Class><owl:Class rdf:about="http://dbpedia.org/ontology/GrossDomesticProduct">
        <rdfs:label xml:lang="nl">bruto nationaal product</rdfs:label><rdfs:label xml:lang="el">ακαθάριστο εγχώριο προϊόν</rdfs:label><rdfs:label xml:lang="ur">مجموعی ملکی پیداوار</rdfs:label><rdfs:label xml:lang="ga">olltáirgeacht intíre</rdfs:label><rdfs:label xml:lang="en">gross domestic product</rdfs:label><rdfs:label xml:lang="de">Bruttoinlandsprodukt</rdfs:label><rdfs:subClassOf rdf:resource="http://www.w3.org/2002/07/owl#Thing"/><prov:wasDerivedFrom rdf:resource="http://mappings.dbpedia.org/index.php/OntologyClass:GrossDomesticProduct"/>
        </owl:Class><owl:Class rdf:about="http://dbpedia.org/ontology/WaterRide">
        <rdfs:label xml:lang="nl">waterbaan</rdfs:label><rdfs:label xml:lang="ur">پانی کی سواری</rdfs:label><rdfs:label xml:lang="ga">marcaíocht uisce</rdfs:label><rdfs:label xml:lang="en">water ride</rdfs:label><rdfs:label xml:lang="de">Wasserbahn</rdfs:label><rdfs:subClassOf rdf:resource="http://dbpedia.org/ontology/AmusementParkAttraction"/><owl:equivalentClass rdf:resource="http://www.wikidata.org/entity/Q2870166"/><prov:wasDerivedFrom rdf:resource="http://mappings.dbpedia.org/index.php/OntologyClass:WaterRide"/>
        </owl:Class><owl:Class rdf:about="http://dbpedia.org/ontology/MilitaryVehicle">
        <rdfs:label xml:lang="nl">legervoertuig</rdfs:label><rdfs:label xml:lang="ur">فوجی گاڑی</rdfs:label><rdfs:label xml:lang="fr">véhicule militaire</rdfs:label><rdfs:label xml:lang="en">military vehicle</rdfs:label><rdfs:label xml:lang="de">Militärfahrzeug</rdfs:label><rdfs:subClassOf rdf:resource="http://dbpedia.org/ontology/MeanOfTransportation"/><rdfs:subClassOf rdf:resource="http://schema.org/Product"/><prov:wasDerivedFrom rdf:resource="http://mappings.dbpedia.org/index.php/OntologyClass:MilitaryVehicle"/>
        </owl:Class><owl:Class rdf:about="http://dbpedia.org/ontology/ArtisticGenre">
        <rdfs:label xml:lang="nl">kunstsoort</rdfs:label><rdfs:label xml:lang="ur">فنکارانہ صنف</rdfs:label><rdfs:label xml:lang="fr">genre artistique</rdfs:label><rdfs:label xml:lang="en">artistic genre</rdfs:label><rdfs:label xml:lang="de">Kunstgattung</rdfs:label><rdfs:comment xml:lang="en">Genres of art, e.g. Pointillist, Modernist</rdfs:comment><rdfs:comment xml:lang="de">Gattung nennt man in den Kunstwissenschaften die auf das künstlerische Ausdrucksmedium bezogenen Formen der Kunst.</rdfs:comment><rdfs:comment xml:lang="fr">genre d'art, ex: Pointillisme, Modernisme</rdfs:comment><rdfs:comment xml:lang="ur">فن کی انواع</rdfs:comment><rdfs:subClassOf rdf:resource="http://dbpedia.org/ontology/Genre"/><prov:wasDerivedFrom rdf:resource="http://mappings.dbpedia.org/index.php/OntologyClass:ArtisticGenre"/>
        </owl:Class><owl:Class rdf:about="http://dbpedia.org/ontology/SportsSeason">
        <rdfs:label xml:lang="nl">sportseizoen</rdfs:label><rdfs:label xml:lang="el">περίοδος αθλημάτων</rdfs:label><rdfs:label xml:lang="ur">کھیلوں کا موسم</rdfs:label><rdfs:label xml:lang="en">sports season</rdfs:label><rdfs:label xml:lang="de">Sportsaison</rdfs:label><rdfs:subClassOf rdf:resource="http://www.w3.org/2002/07/owl#Thing"/><prov:wasDerivedFrom rdf:resource="http://mappings.dbpedia.org/index.php/OntologyClass:SportsSeason"/>
        </owl:Class><owl:Class rdf:about="http://dbpedia.org/ontology/Cricketer">
        <rdfs:label xml:lang="nl">cricketspeler</rdfs:label><rdfs:label xml:lang="el">παίκτης του κρίκετ</rdfs:label><rdfs:label xml:lang="ko">크리켓 선수</rdfs:label><rdfs:label xml:lang="ur">کرکٹ کا کھلاڑی</rdfs:label><rdfs:label xml:lang="ga">imreoir cruicéid</rdfs:label><rdfs:label xml:lang="fr">joueur de cricket</rdfs:label><rdfs:label xml:lang="en">cricketer</rdfs:label><rdfs:label xml:lang="ja">クリケット選手</rdfs:label><rdfs:label xml:lang="de">Cricketspieler</rdfs:label><rdfs:subClassOf rdf:resource="http://dbpedia.org/ontology/Athlete"/><prov:wasDerivedFrom rdf:resource="http://mappings.dbpedia.org/index.php/OntologyClass:Cricketer"/>
        </owl:Class><owl:Class rdf:about="http://dbpedia.org/ontology/FloweringPlant">
        <rdfs:label xml:lang="nl">bedektzadigen</rdfs:label><rdfs:label xml:lang="el">ανθοφόρο φυτό</rdfs:label><rdfs:label xml:lang="ur">پھولوں کا پودا</rdfs:label><rdfs:label xml:lang="fr">angiospermes</rdfs:label><rdfs:label xml:lang="es">angiosperma</rdfs:label><rdfs:label xml:lang="it">magnoliofita</rdfs:label><rdfs:label xml:lang="en">flowering plant</rdfs:label><rdfs:label xml:lang="ja">被子植物</rdfs:label><rdfs:label xml:lang="de">bedecktsamige Pflanze</rdfs:label><rdfs:subClassOf rdf:resource="http://dbpedia.org/ontology/Plant"/><prov:wasDerivedFrom rdf:resource="http://mappings.dbpedia.org/index.php/OntologyClass:FloweringPlant"/>
        </owl:Class><owl:Class rdf:about="http://dbpedia.org/ontology/Spreadsheet">
        <rdfs:label xml:lang="en">Spreadsheet</rdfs:label><rdfs:label xml:lang="ru">Электронная таблица</rdfs:label><rdfs:label xml:lang="ur">سپریڈ شیٹ</rdfs:label><rdfs:label xml:lang="fr">tableur</rdfs:label><rdfs:comment xml:lang="ur">مرتب و شمار یا معلومات کو کام میں لانےوالاایک کمپیوٹر پروگرام</rdfs:comment><rdfs:comment xml:lang="fr">Programme informatique qui utilise des statistiques ou des informations</rdfs:comment><rdfs:subClassOf rdf:resource="http://www.w3.org/2002/07/owl#Thing"/><prov:wasDerivedFrom rdf:resource="http://mappings.dbpedia.org/index.php/OntologyClass:Spreadsheet"/>
        </owl:Class><owl:Class rdf:about="http://dbpedia.org/ontology/TelevisionEpisode">
        <rdfs:label xml:lang="nl">televisie seizoen</rdfs:label><rdfs:label xml:lang="el">επεισόδιο τηλεόρασης</rdfs:label><rdfs:label xml:lang="ko">텔레비전 에피소드</rdfs:label><rdfs:label xml:lang="ur">ٹی وی کی قسط</rdfs:label><rdfs:label xml:lang="ga">eagrán de chlár teilifíse</rdfs:label><rdfs:label xml:lang="fr">épisode télévisé</rdfs:label><rdfs:label xml:lang="es">capítulo de serie de televisión</rdfs:label><rdfs:label xml:lang="en">television episode</rdfs:label><rdfs:label xml:lang="ja">テレビ放送回</rdfs:label><rdfs:label xml:lang="de">Fernsehfolge</rdfs:label><rdfs:comment xml:lang="en">A television episode is a part of serial television program.</rdfs:comment><rdfs:comment xml:lang="ur">ٹیلی ویژن ایپی سوڈ سیریل ٹیلی ویژن پروگرام کا ایک حصہ ہے</rdfs:comment><rdfs:subClassOf rdf:resource="http://dbpedia.org/ontology/Work"/><owl:equivalentClass rdf:resource="http://schema.org/TVEpisode"/><prov:wasDerivedFrom rdf:resource="http://mappings.dbpedia.org/index.php/OntologyClass:TelevisionEpisode"/>
        </owl:Class><owl:Class rdf:about="http://dbpedia.org/ontology/Baronet">
        <rdfs:label xml:lang="nl">baronet</rdfs:label><rdfs:label xml:lang="ur">چھوٹا نواب</rdfs:label><rdfs:label xml:lang="it">baronetto</rdfs:label><rdfs:label xml:lang="en">baronet</rdfs:label><rdfs:label xml:lang="ja">準男爵</rdfs:label><rdfs:label xml:lang="de">Baronet</rdfs:label><rdfs:subClassOf rdf:resource="http://dbpedia.org/ontology/BritishRoyalty"/><prov:wasDerivedFrom rdf:resource="http://mappings.dbpedia.org/index.php/OntologyClass:Baronet"/>
        </owl:Class><owl:Class rdf:about="http://dbpedia.org/ontology/Canton">
        <rdfs:label xml:lang="nl">kanton</rdfs:label><rdfs:label xml:lang="ur">ضِلَع</rdfs:label><rdfs:label xml:lang="fr">canton</rdfs:label><rdfs:label xml:lang="en">canton</rdfs:label><rdfs:label xml:lang="ja">スイス連邦の州またはフランスの群</rdfs:label><rdfs:label xml:lang="de">Kanton</rdfs:label><rdfs:comment xml:lang="en">An administrative (France) or lawcourts (Netherlands) body governing a territorial unity on the municipal level or somewhat above</rdfs:comment><rdfs:comment xml:lang="de">Das Wort Kanton dient zur Bezeichnung verschiedener (niederen) Verwaltungsbezirke in Frankreich, Belgien, Kanada und anderen Ländern</rdfs:comment><rdfs:comment xml:lang="ur">ایک انتظامی (فرانس) یا قانون کی عدالت (نیدرلینڈز) کا ادارہ جو علاقائی وحدت کا انتظام کرتا ہے بلدیاتی سطح پر یا اس سے کچھ اوپر</rdfs:comment><rdfs:subClassOf rdf:resource="http://dbpedia.org/ontology/GovernmentalAdministrativeRegion"/><prov:wasDerivedFrom rdf:resource="http://mappings.dbpedia.org/index.php/OntologyClass:Canton"/>
        </owl:Class><owl:Class rdf:about="http://dbpedia.org/ontology/Cinema">
        <rdfs:label xml:lang="nl">bioscoop</rdfs:label><rdfs:label xml:lang="el">κινηματογράφος</rdfs:label><rdfs:label xml:lang="ur">سنیما</rdfs:label><rdfs:label xml:lang="fr">cinéma</rdfs:label><rdfs:label xml:lang="en">cinema (movie theater)</rdfs:label><rdfs:label xml:lang="de">Theater</rdfs:label><rdfs:comment xml:lang="en">A building for viewing films.</rdfs:comment><rdfs:comment xml:lang="ur">فلم دیکھنے کے لیے ایک عمارت۔</rdfs:comment><rdfs:subClassOf rdf:resource="http://dbpedia.org/ontology/Venue"/><owl:equivalentClass rdf:resource="http://www.wikidata.org/entity/Q41253"/><prov:wasDerivedFrom rdf:resource="http://mappings.dbpedia.org/index.php/OntologyClass:Cinema"/>
        </owl:Class><owl:Class rdf:about="http://dbpedia.org/ontology/Gnetophytes">
        <rdfs:label xml:lang="nl">Gnetales</rdfs:label><rdfs:label xml:lang="el">Gnetophytes</rdfs:label><rdfs:label xml:lang="ur">گمٹیلا پودا</rdfs:label><rdfs:label xml:lang="fr">gnétophytes</rdfs:label><rdfs:label xml:lang="en">Gnetophytes</rdfs:label><rdfs:label xml:lang="ja">グネツム綱</rdfs:label><rdfs:label xml:lang="de">Gnetophyta</rdfs:label><rdfs:subClassOf rdf:resource="http://dbpedia.org/ontology/Plant"/><prov:wasDerivedFrom rdf:resource="http://mappings.dbpedia.org/index.php/OntologyClass:Gnetophytes"/>
        </owl:Class><owl:Class rdf:about="http://dbpedia.org/ontology/Jockey">
        <rdfs:label xml:lang="nl">jockey</rdfs:label><rdfs:label xml:lang="el">αναβάτης αλόγου αγώνων</rdfs:label><rdfs:label xml:lang="ur">پیشہ ور گھڑ سوار</rdfs:label><rdfs:label xml:lang="ga">marcach</rdfs:label><rdfs:label xml:lang="fr">jockey (coureur à cheval)</rdfs:label><rdfs:label xml:lang="en">jockey (horse racer)</rdfs:label><rdfs:label xml:lang="ja">騎手</rdfs:label><rdfs:label xml:lang="de">Jockey (Pferderennprofi)</rdfs:label><rdfs:subClassOf rdf:resource="http://dbpedia.org/ontology/Athlete"/><prov:wasDerivedFrom rdf:resource="http://mappings.dbpedia.org/index.php/OntologyClass:Jockey"/>
        </owl:Class><owl:Class rdf:about="http://dbpedia.org/ontology/ScientificConcept">
        <rdfs:label xml:lang="nl">wetenschappelijke theorie</rdfs:label><rdfs:label xml:lang="ur">سائنسی تصور</rdfs:label><rdfs:label xml:lang="fr">concept scientifique</rdfs:label><rdfs:label xml:lang="en">Scientific concept</rdfs:label><rdfs:label xml:lang="de">wissenschaftliche Theorie</rdfs:label><rdfs:comment xml:lang="en">Scientific concepts, e.g. Theory of relativity, Quantum gravity</rdfs:comment><rdfs:comment xml:lang="fr">Concepts scientifiques tels que la théorie de la relativité, la gravité quantique</rdfs:comment><rdfs:comment xml:lang="ur">سائنسی تصورات، جیسے نظریہ اضافیت، کوانٹم کشش ثقل</rdfs:comment><rdfs:subClassOf rdf:resource="http://dbpedia.org/ontology/TopicalConcept"/><prov:wasDerivedFrom rdf:resource="http://mappings.dbpedia.org/index.php/OntologyClass:ScientificConcept"/>
        </owl:Class><owl:Class rdf:about="http://dbpedia.org/ontology/SportCompetitionResult">
        <rdfs:label xml:lang="nl">uitslag van een sport competitie</rdfs:label><rdfs:label xml:lang="el">αποτελέσματα αθλητικού διαγωνισμού</rdfs:label><rdfs:label xml:lang="ur">کھیلوں کے مقابلے کا نتیجہ</rdfs:label><rdfs:label xml:lang="fr">résultats d'une compétition sportive</rdfs:label><rdfs:label xml:lang="es">resultados de una competición deportiva</rdfs:label><rdfs:label xml:lang="en">results of a sport competition</rdfs:label><rdfs:label xml:lang="de">Ergebnisse eines Sportwettbewerbs</rdfs:label><rdfs:subClassOf rdf:resource="http://www.w3.org/2002/07/owl#Thing"/><prov:wasDerivedFrom rdf:resource="http://mappings.dbpedia.org/index.php/OntologyClass:SportCompetitionResult"/>
        </owl:Class><owl:Class rdf:about="http://dbpedia.org/ontology/Tower">
        <rdfs:label xml:lang="nl">toren</rdfs:label><rdfs:label xml:lang="el">πύργος</rdfs:label><rdfs:label xml:lang="ur">مینار</rdfs:label><rdfs:label xml:lang="ga">túr</rdfs:label><rdfs:label xml:lang="fr">tour</rdfs:label><rdfs:label xml:lang="en">tower</rdfs:label><rdfs:label xml:lang="ja">塔</rdfs:label><rdfs:label xml:lang="de">Turm</rdfs:label><rdfs:comment xml:lang="en">A Tower is a kind of structure (not necessarily a building) that is higher than the rest</rdfs:comment><rdfs:comment xml:lang="ur">مینار ایک قسم کا ڈھانچہ ہے (ضروری نہیں کہ کوئی عمارت) جو باقی سے اونچی ہو</rdfs:comment><rdfs:subClassOf rdf:resource="http://dbpedia.org/ontology/ArchitecturalStructure"/><owl:equivalentClass rdf:resource="http://www.wikidata.org/entity/Q12518"/><owl:disjointWith rdf:resource="http://dbpedia.org/ontology/Person"/><prov:wasDerivedFrom rdf:resource="http://mappings.dbpedia.org/index.php/OntologyClass:Tower"/>
        </owl:Class><owl:Class rdf:about="http://dbpedia.org/ontology/Protein">
        <rdfs:label xml:lang="pt">proteína</rdfs:label><rdfs:label xml:lang="nl">proteïne</rdfs:label><rdfs:label xml:lang="el">πρωτεΐνη</rdfs:label><rdfs:label xml:lang="ko">단백질</rdfs:label><rdfs:label xml:lang="ur">لحمیات</rdfs:label><rdfs:label xml:lang="ga">próitéin</rdfs:label><rdfs:label xml:lang="fr">protéine</rdfs:label><rdfs:label xml:lang="it">proteina</rdfs:label><rdfs:label xml:lang="en">protein</rdfs:label><rdfs:label xml:lang="ja">タンパク質</rdfs:label><rdfs:label xml:lang="de">Protein</rdfs:label><rdfs:subClassOf rdf:resource="http://dbpedia.org/ontology/Biomolecule"/><owl:equivalentClass rdf:resource="http://www.wikidata.org/entity/Q8054"/><prov:wasDerivedFrom rdf:resource="http://mappings.dbpedia.org/index.php/OntologyClass:Protein"/>
        </owl:Class><owl:Class rdf:about="http://dbpedia.org/ontology/HumanGeneLocation">
        <rdfs:label xml:lang="nl">menselijk genoom locatie</rdfs:label><rdfs:label xml:lang="el">τοποθεσία του ανθρώπινου γονιδίου</rdfs:label><rdfs:label xml:lang="ur">انسانی نَسبہ کا مقام</rdfs:label><rdfs:label xml:lang="fr">Position de gène chez l'homme</rdfs:label><rdfs:label xml:lang="en">HumanGeneLocation</rdfs:label><rdfs:label xml:lang="ja">ヒト遺伝子座</rdfs:label><rdfs:label xml:lang="de">Humangen Lokation</rdfs:label><rdfs:subClassOf rdf:resource="http://dbpedia.org/ontology/GeneLocation"/><prov:wasDerivedFrom rdf:resource="http://mappings.dbpedia.org/index.php/OntologyClass:HumanGeneLocation"/>
        </owl:Class><owl:Class rdf:about="http://dbpedia.org/ontology/SpeedwayTeam">
        <rdfs:label xml:lang="pl">klub żużlowy</rdfs:label><rdfs:label xml:lang="nl">speedwayteam</rdfs:label><rdfs:label xml:lang="ur">سپیڈ وے ٹیم</rdfs:label><rdfs:label xml:lang="ga">foireann luasbhealaigh</rdfs:label><rdfs:label xml:lang="en">speedway team</rdfs:label><rdfs:label xml:lang="de">Speedwayteam</rdfs:label><rdfs:subClassOf rdf:resource="http://dbpedia.org/ontology/SportsTeam"/><prov:wasDerivedFrom rdf:resource="http://mappings.dbpedia.org/index.php/OntologyClass:SpeedwayTeam"/>
        </owl:Class><owl:Class rdf:about="http://dbpedia.org/ontology/ChristianPatriarch">
        <rdfs:label xml:lang="pl">patriarcha chrześcijański</rdfs:label><rdfs:label xml:lang="nl">christelijk patriarch</rdfs:label><rdfs:label xml:lang="el">χριστιανός πατριάρχης</rdfs:label><rdfs:label xml:lang="ko">기독교 총대주교</rdfs:label><rdfs:label xml:lang="ur">عیسائی پادری</rdfs:label><rdfs:label xml:lang="fr">patriarche chrétien</rdfs:label><rdfs:label xml:lang="it">patriarca cristiano</rdfs:label><rdfs:label xml:lang="en">Christian Patriarch</rdfs:label><rdfs:label xml:lang="de">christlicher Patriarch</rdfs:label><rdfs:subClassOf rdf:resource="http://dbpedia.org/ontology/Cleric"/><prov:wasDerivedFrom rdf:resource="http://mappings.dbpedia.org/index.php/OntologyClass:ChristianPatriarch"/>
        </owl:Class><owl:Class rdf:about="http://dbpedia.org/ontology/GovernmentType">
        <rdfs:label xml:lang="nl">regeringsvorm</rdfs:label><rdfs:label xml:lang="el">Είδη Διακυβέρνησης</rdfs:label><rdfs:label xml:lang="ur">حکومت کی قسم</rdfs:label><rdfs:label xml:lang="fr">régime politique</rdfs:label><rdfs:label xml:lang="en">Government Type</rdfs:label><rdfs:label xml:lang="de">Regierungsform</rdfs:label><rdfs:comment xml:lang="en">a form of government</rdfs:comment><rdfs:comment xml:lang="ur">حکومت کی ایک شکل</rdfs:comment><rdfs:subClassOf rdf:resource="http://dbpedia.org/ontology/Type"/><prov:wasDerivedFrom rdf:resource="http://mappings.dbpedia.org/index.php/OntologyClass:GovernmentType"/>
        </owl:Class><owl:Class rdf:about="http://dbpedia.org/ontology/Town">
        <rdfs:label xml:lang="pl">miasteczko</rdfs:label><rdfs:label xml:lang="nl">stad</rdfs:label><rdfs:label xml:lang="el">πόλη</rdfs:label><rdfs:label xml:lang="hi">नगर</rdfs:label><rdfs:label xml:lang="ur">قصبہ</rdfs:label><rdfs:label xml:lang="ga">baile</rdfs:label><rdfs:label xml:lang="fr">ville</rdfs:label><rdfs:label xml:lang="en">town</rdfs:label><rdfs:label xml:lang="ja">町</rdfs:label><rdfs:label xml:lang="de">Stadt</rdfs:label><rdfs:comment xml:lang="en">a settlement ranging from a few hundred to several thousand (occasionally hundreds of thousands). The precise meaning varies between countries and is not always a matter of legal definition. Usually, a town is thought of as larger than a village but smaller than a city, though there are exceptions to this rule.</rdfs:comment><rdfs:comment xml:lang="ur">چند سو سے لے کر کئی ہزار (کبھی کبھار سیکڑوں ہزاروں) تک کی تصفیہ۔ درست معنی ممالک کے درمیان مختلف ہوتے ہیں اور یہ ہمیشہ قانونی تعریف کا معاملہ نہیں ہوتا ہے۔ عام طور پر، ایک قصبہ کو گاؤں سے بڑا لیکن شہر سے چھوٹا سمجھا جاتا ہے، حالانکہ اس اصول میں مستثنیات ہیں</rdfs:comment><rdfs:subClassOf rdf:resource="http://dbpedia.org/ontology/Settlement"/><owl:equivalentClass rdf:resource="http://www.wikidata.org/entity/Q3957"/><prov:wasDerivedFrom rdf:resource="http://mappings.dbpedia.org/index.php/OntologyClass:Town"/>
        </owl:Class><owl:Class rdf:about="http://dbpedia.org/ontology/RomanEmperor">
        <rdfs:label xml:lang="nl">Romeinse keizer</rdfs:label><rdfs:label xml:lang="el">ρωμαίος αυτοκράτορας</rdfs:label><rdfs:label xml:lang="ur">رومن شہنشاہ</rdfs:label><rdfs:label xml:lang="fr">empereur romain</rdfs:label><rdfs:label xml:lang="en">roman emperor</rdfs:label><rdfs:label xml:lang="de">römischer Kaiser</rdfs:label><rdfs:subClassOf rdf:resource="http://dbpedia.org/ontology/Person"/><owl:equivalentClass rdf:resource="http://www.wikidata.org/entity/Q842606"/><prov:wasDerivedFrom rdf:resource="http://mappings.dbpedia.org/index.php/OntologyClass:RomanEmperor"/>
        </owl:Class><owl:Class rdf:about="http://dbpedia.org/ontology/ReligiousBuilding">
        <rdfs:label xml:lang="nl">cultusgebouw</rdfs:label><rdfs:label xml:lang="el">θρησκευτικό κτίριο</rdfs:label><rdfs:label xml:lang="ko">종교 건물</rdfs:label><rdfs:label xml:lang="ur">مذہبی عمارت</rdfs:label><rdfs:label xml:lang="fr">édifice religieux</rdfs:label><rdfs:label xml:lang="es">edificio religioso</rdfs:label><rdfs:label xml:lang="it">edificio religioso</rdfs:label><rdfs:label xml:lang="en">religious building</rdfs:label><rdfs:label xml:lang="da">religiøs bygning</rdfs:label><rdfs:label xml:lang="ja">宗教建築</rdfs:label><rdfs:label xml:lang="de">religiöses Gebäude</rdfs:label><rdfs:subClassOf rdf:resource="http://dbpedia.org/ontology/Building"/><owl:equivalentClass rdf:resource="http://www.wikidata.org/entity/Q1370598"/><prov:wasDerivedFrom rdf:resource="http://mappings.dbpedia.org/index.php/OntologyClass:ReligiousBuilding"/>
        </owl:Class><owl:Class rdf:about="http://dbpedia.org/ontology/Minister">
        <rdfs:label xml:lang="nl">minister</rdfs:label><rdfs:label xml:lang="ur">وزیر</rdfs:label><rdfs:label xml:lang="fr">ministre</rdfs:label><rdfs:label xml:lang="en">minister</rdfs:label><rdfs:label xml:lang="de">Minister</rdfs:label><rdfs:subClassOf rdf:resource="http://dbpedia.org/ontology/Politician"/><prov:wasDerivedFrom rdf:resource="http://mappings.dbpedia.org/index.php/OntologyClass:Minister"/>
        </owl:Class><owl:Class rdf:about="http://dbpedia.org/ontology/MotorcycleRider">
        <rdfs:label xml:lang="nl">motorrijder</rdfs:label><rdfs:label xml:lang="el">μοτοσυκλετιστής</rdfs:label><rdfs:label xml:lang="ur">موٹر سائیکل سوار</rdfs:label><rdfs:label xml:lang="en">motorcycle rider</rdfs:label><rdfs:label xml:lang="de">Motorradfahrer</rdfs:label><rdfs:subClassOf rdf:resource="http://dbpedia.org/ontology/MotorsportRacer"/><prov:wasDerivedFrom rdf:resource="http://mappings.dbpedia.org/index.php/OntologyClass:MotorcycleRider"/>
        </owl:Class><owl:Class rdf:about="http://dbpedia.org/ontology/ClericalAdministrativeRegion">
        <rdfs:label xml:lang="nl">kerkelijk bestuurlijk gebied</rdfs:label><rdfs:label xml:lang="ko">사무 관리 지역</rdfs:label><rdfs:label xml:lang="ur">علمی انتظامی علاقہ</rdfs:label><rdfs:label xml:lang="fr">région administrative dans une église</rdfs:label><rdfs:label xml:lang="en">clerical administrative region</rdfs:label><rdfs:label xml:lang="de">klerikale Verwaltungsregion</rdfs:label><rdfs:comment xml:lang="en">An administrative body governing some territorial unity, in this case a clerical administrative body</rdfs:comment><rdfs:comment xml:lang="ur">ایک علمی انتظامی معاملات میں ایک انتظامی ادارہ جو کچھ علاقائی وحدت کو کنٹرول کرتا ہے</rdfs:comment><rdfs:subClassOf rdf:resource="http://dbpedia.org/ontology/AdministrativeRegion"/><prov:wasDerivedFrom rdf:resource="http://mappings.dbpedia.org/index.php/OntologyClass:ClericalAdministrativeRegion"/>
        </owl:Class><owl:Class rdf:about="http://dbpedia.org/ontology/BusCompany">
        <rdfs:label xml:lang="nl">busmaatschappij</rdfs:label><rdfs:label xml:lang="el">εταιρία λεωφορείων</rdfs:label><rdfs:label xml:lang="ur">بس كا تِجارتی اِدارہ</rdfs:label><rdfs:label xml:lang="ga">comhlacht bus</rdfs:label><rdfs:label xml:lang="fr">compagnie d'autobus</rdfs:label><rdfs:label xml:lang="es">compañía de autobuses</rdfs:label><rdfs:label xml:lang="en">bus company</rdfs:label><rdfs:label xml:lang="de">Busunternehmen</rdfs:label><rdfs:subClassOf rdf:resource="http://dbpedia.org/ontology/PublicTransitSystem"/><prov:wasDerivedFrom rdf:resource="http://mappings.dbpedia.org/index.php/OntologyClass:BusCompany"/>
        </owl:Class><owl:Class rdf:about="http://dbpedia.org/ontology/PowerStation">
        <rdfs:label xml:lang="nl">Elektriciteitscentrale</rdfs:label><rdfs:label xml:lang="el">σταθμός παραγωγής ενέργειας</rdfs:label><rdfs:label xml:lang="ur">بجلی گھر</rdfs:label><rdfs:label xml:lang="ga">stáisiún cumhachta</rdfs:label><rdfs:label xml:lang="fr">centrale électrique</rdfs:label><rdfs:label xml:lang="es">central eléctrica</rdfs:label><rdfs:label xml:lang="en">power station</rdfs:label><rdfs:label xml:lang="ja">発電所</rdfs:label><rdfs:label xml:lang="de">Kraftwerk</rdfs:label><rdfs:subClassOf rdf:resource="http://dbpedia.org/ontology/Infrastructure"/><owl:equivalentClass rdf:resource="http://www.wikidata.org/entity/Q159719"/><prov:wasDerivedFrom rdf:resource="http://mappings.dbpedia.org/index.php/OntologyClass:PowerStation"/>
        </owl:Class><owl:Class rdf:about="http://dbpedia.org/ontology/Engineer">
        <rdfs:label xml:lang="nl">ingenieur</rdfs:label><rdfs:label xml:lang="el">μηχανικός</rdfs:label><rdfs:label xml:lang="ko">공학자</rdfs:label><rdfs:label xml:lang="ur">ماہر فنیات</rdfs:label><rdfs:label xml:lang="ga">innealtóir</rdfs:label><rdfs:label xml:lang="fr">ingénieur</rdfs:label><rdfs:label xml:lang="es">ingeniero</rdfs:label><rdfs:label xml:lang="it">ingeniere</rdfs:label><rdfs:label xml:lang="en">engineer</rdfs:label><rdfs:label xml:lang="ja">技術者</rdfs:label><rdfs:label xml:lang="de">Ingenieur</rdfs:label><rdfs:subClassOf rdf:resource="http://dbpedia.org/ontology/Person"/><owl:equivalentClass rdf:resource="http://www.wikidata.org/entity/Q81096"/><prov:wasDerivedFrom rdf:resource="http://mappings.dbpedia.org/index.php/OntologyClass:Engineer"/>
        </owl:Class><owl:Class rdf:about="http://dbpedia.org/ontology/Name">
        <rdfs:label xml:lang="pl">nazwa</rdfs:label><rdfs:label xml:lang="pt">nome</rdfs:label><rdfs:label xml:lang="nl">naam</rdfs:label><rdfs:label xml:lang="el">όνομα</rdfs:label><rdfs:label xml:lang="ur">نام</rdfs:label><rdfs:label xml:lang="ga">ainm</rdfs:label><rdfs:label xml:lang="fr">nom</rdfs:label><rdfs:label xml:lang="en">name</rdfs:label><rdfs:label xml:lang="ja">名前</rdfs:label><rdfs:label xml:lang="de">Name</rdfs:label><rdfs:subClassOf rdf:resource="http://www.w3.org/2002/07/owl#Thing"/><owl:equivalentClass rdf:resource="http://www.wikidata.org/entity/Q82799"/><prov:wasDerivedFrom rdf:resource="http://mappings.dbpedia.org/index.php/OntologyClass:Name"/>
        </owl:Class><owl:Class rdf:about="http://dbpedia.org/ontology/SumoWrestler">
        <rdfs:label xml:lang="nl">sumoworstelaar</rdfs:label><rdfs:label xml:lang="ur">سومو پہلوان</rdfs:label><rdfs:label xml:lang="fr">lutteur de sumo</rdfs:label><rdfs:label xml:lang="en">sumo wrestler</rdfs:label><rdfs:label xml:lang="de">Sumo-Ringer</rdfs:label><rdfs:subClassOf rdf:resource="http://dbpedia.org/ontology/Wrestler"/><prov:wasDerivedFrom rdf:resource="http://mappings.dbpedia.org/index.php/OntologyClass:SumoWrestler"/>
        </owl:Class><owl:Class rdf:about="http://dbpedia.org/ontology/InternationalOrganisation">
        <rdfs:label xml:lang="en">international organisation</rdfs:label><rdfs:label xml:lang="fr">organisation internationale</rdfs:label><rdfs:label xml:lang="nl">internationale organisatie</rdfs:label><rdfs:label xml:lang="ur">بین الاقوامی تنظیم</rdfs:label><rdfs:comment xml:lang="en">An international organisation is either a private or a public organisation seeking to accomplish goals across country borders</rdfs:comment><rdfs:comment xml:lang="ur">ایک بین الاقوامی تنظیم یا تو ایک نجی یا عوامی تنظیم ہے جو ملک کی سرحدوں سے اہداف حاصل کرنے کی کوشش کرتی ہے۔</rdfs:comment><rdfs:subClassOf rdf:resource="http://dbpedia.org/ontology/Organisation"/><prov:wasDerivedFrom rdf:resource="http://mappings.dbpedia.org/index.php/OntologyClass:InternationalOrganisation"/>
        </owl:Class><owl:Class rdf:about="http://dbpedia.org/ontology/HighDiver">
        <rdfs:label xml:lang="de">Turmspringer</rdfs:label><rdfs:label xml:lang="nl">schoonspringer</rdfs:label><rdfs:label xml:lang="en">high diver</rdfs:label><rdfs:label xml:lang="ur">اونچائی سے پانی میں ڈبکی لگانے والا</rdfs:label><rdfs:subClassOf rdf:resource="http://dbpedia.org/ontology/Athlete"/><prov:wasDerivedFrom rdf:resource="http://mappings.dbpedia.org/index.php/OntologyClass:HighDiver"/>
        </owl:Class><owl:Class rdf:about="http://dbpedia.org/ontology/FormulaOneRacer">
        <rdfs:label xml:lang="nl">formule 1-coureur</rdfs:label><rdfs:label xml:lang="el">πιλότος της φόρμουλας ένα</rdfs:label><rdfs:label xml:lang="ur">فارمولا ون ریسر</rdfs:label><rdfs:label xml:lang="fr">pilote de formule 1</rdfs:label><rdfs:label xml:lang="en">Formula One racer</rdfs:label><rdfs:label xml:lang="de">Formel-1 Rennfahrer</rdfs:label><rdfs:subClassOf rdf:resource="http://dbpedia.org/ontology/RacingDriver"/><prov:wasDerivedFrom rdf:resource="http://mappings.dbpedia.org/index.php/OntologyClass:FormulaOneRacer"/>
        </owl:Class><owl:Class rdf:about="http://dbpedia.org/ontology/Conifer">
        <rdfs:label xml:lang="nl">conifeer</rdfs:label><rdfs:label xml:lang="el">κωνοφόρο</rdfs:label><rdfs:label xml:lang="ko">침엽수</rdfs:label><rdfs:label xml:lang="ur">صنوبر کی قِسم کا پودا</rdfs:label><rdfs:label xml:lang="ga">cónaiféar</rdfs:label><rdfs:label xml:lang="fr">conifere</rdfs:label><rdfs:label xml:lang="es">conífera</rdfs:label><rdfs:label xml:lang="en">conifer</rdfs:label><rdfs:label xml:lang="ja">球果植物門</rdfs:label><rdfs:label xml:lang="de">Konifere</rdfs:label><rdfs:comment xml:lang="ur">عروقی (نالی دار)پودے ہیں ، بیج ایک شنک میں موجود ہوتے ہیں۔ وہ لکڑی کے پودے ہیں۔</rdfs:comment><rdfs:comment xml:lang="it">Le conifere sono piante vascolari, con semi contenuti in un cono. Sono piante legnose, perlopiù sono alberi e solo poche sono arbusti.</rdfs:comment><rdfs:comment xml:lang="es">Las coníferas son plantas vasculares, con las semillas contenidas en un cono. Son plantas leñosas.</rdfs:comment><rdfs:subClassOf rdf:resource="http://dbpedia.org/ontology/Plant"/><prov:wasDerivedFrom rdf:resource="http://mappings.dbpedia.org/index.php/OntologyClass:Conifer"/>
        </owl:Class><owl:Class rdf:about="http://dbpedia.org/ontology/SpeedwayLeague">
        <rdfs:label xml:lang="nl">speedway competitie</rdfs:label><rdfs:label xml:lang="el">πρωτάθλημα αυτοκινητοδρόμου</rdfs:label><rdfs:label xml:lang="ur">تیز راہ کی انجمن</rdfs:label><rdfs:label xml:lang="fr">ligue de speedway</rdfs:label><rdfs:label xml:lang="en">speedway league</rdfs:label><rdfs:label xml:lang="de">Speedway Liga</rdfs:label><rdfs:comment xml:lang="en">A group of sports teams that compete against each other in motorcycle speedway racing.</rdfs:comment><rdfs:comment xml:lang="ur">کھیلوں کی ٹیموں کا ایک گروپ جو موٹرسائیکل سپیڈ وے ریسنگ میں ایک دوسرے سے مقابلہ کرتا ہے</rdfs:comment><rdfs:subClassOf rdf:resource="http://dbpedia.org/ontology/SportsLeague"/><prov:wasDerivedFrom rdf:resource="http://mappings.dbpedia.org/index.php/OntologyClass:SpeedwayLeague"/>
        </owl:Class><owl:Class rdf:about="http://dbpedia.org/ontology/Instrumentalist">
        <rdfs:label xml:lang="nl">instrumentalist</rdfs:label><rdfs:label xml:lang="el">μουσικός</rdfs:label><rdfs:label xml:lang="ur">سازندہ</rdfs:label><rdfs:label xml:lang="ga">ionstraimí</rdfs:label><rdfs:label xml:lang="fr">instrumentiste</rdfs:label><rdfs:label xml:lang="en">instrumentalist</rdfs:label><rdfs:label xml:lang="ja">音楽家</rdfs:label><rdfs:label xml:lang="de">Musiker</rdfs:label><rdfs:comment xml:lang="el">Ο μουσικός είναι ένα άτομο το οποίο γράφει, ερμηνεύει, ή κάνει μουσική.</rdfs:comment><rdfs:comment xml:lang="ur">موسیقار وہ شخص ہوتا ہے جو لکھتا ہے، پرفارم کرتا ہے یا موسیقی بناتا ہے۔</rdfs:comment><rdfs:comment xml:lang="fr">Un instrumentiste est quelqu'un qui joue d'un instrument. Tout instrumentiste non-vocal (incluant guitariste, pianiste, saxophoniste, DJ, musicien divers...). Tout artiste solo qui compose et/ou fait partie d'un groupe.</rdfs:comment><rdfs:comment xml:lang="nl">Een instrumentalist is een musicus die een muziekinstrument bespeelt. (https://nl.wikipedia.org/wiki/Instrumentalist)</rdfs:comment><rdfs:subClassOf rdf:resource="http://dbpedia.org/ontology/MusicalArtist"/><prov:wasDerivedFrom rdf:resource="http://mappings.dbpedia.org/index.php/OntologyClass:Instrumentalist"/>
        </owl:Class><owl:Class rdf:about="http://dbpedia.org/ontology/Farmer">
        <rdfs:label xml:lang="nl">boer</rdfs:label><rdfs:label xml:lang="el">αγρότης</rdfs:label><rdfs:label xml:lang="ur">کسان</rdfs:label><rdfs:label xml:lang="ga">feirmeoir</rdfs:label><rdfs:label xml:lang="fr">fermier</rdfs:label><rdfs:label xml:lang="en">farmer</rdfs:label><rdfs:label xml:lang="ja">農家</rdfs:label><rdfs:label xml:lang="de">Bauer</rdfs:label><rdfs:subClassOf rdf:resource="http://dbpedia.org/ontology/Person"/><owl:equivalentClass rdf:resource="http://www.wikidata.org/entity/Q131512"/><prov:wasDerivedFrom rdf:resource="http://mappings.dbpedia.org/index.php/OntologyClass:Farmer"/>
        </owl:Class><owl:Class rdf:about="http://dbpedia.org/ontology/HistoricalSettlement">
        <rdfs:label xml:lang="nl">voormalige stad of dorp</rdfs:label><rdfs:label xml:lang="ur">تاریخی آبادکاری</rdfs:label><rdfs:label xml:lang="ga">áit lonnaithe stairiúil</rdfs:label><rdfs:label xml:lang="fr">ancien ville ou village</rdfs:label><rdfs:label xml:lang="en">Historical settlement</rdfs:label><rdfs:label xml:lang="de">historischer Siedlung</rdfs:label><rdfs:comment xml:lang="en">A place which used to be a city or town or village.</rdfs:comment><rdfs:comment xml:lang="ur">وہ جگہ جو پہلے شہر یا قصبہ یا گاؤں ہوا کرتی تھی</rdfs:comment><rdfs:subClassOf rdf:resource="http://dbpedia.org/ontology/Settlement"/><prov:wasDerivedFrom rdf:resource="http://mappings.dbpedia.org/index.php/OntologyClass:HistoricalSettlement"/>
        </owl:Class><owl:Class rdf:about="http://dbpedia.org/ontology/VideogamesLeague">
        <rdfs:label xml:lang="el">πρωτάθλημα βιντεοπαιχνιδιών</rdfs:label><rdfs:label xml:lang="ur">بصری کھیلوں کی انجمن</rdfs:label><rdfs:label xml:lang="ga">sraith físchluichí</rdfs:label><rdfs:label xml:lang="fr">ligue de jeux vidéo</rdfs:label><rdfs:label xml:lang="en">videogames league</rdfs:label><rdfs:label xml:lang="de">Videospiele-Liga</rdfs:label><rdfs:comment xml:lang="en">A group of sports teams or person that compete against each other in videogames.</rdfs:comment><rdfs:comment xml:lang="ur">کھیلوں کی ٹیموں کا ایک گروپ یا شخص جو بصری کھیلوں میں ایک دوسرے سے مقابلہ کرتا ہے</rdfs:comment><rdfs:comment xml:lang="el">Ένα σύνολο ομάδων ή ατόμων που ανταγωνίζονται σε ηλεκτρονικά παιχνίδια.</rdfs:comment><rdfs:subClassOf rdf:resource="http://dbpedia.org/ontology/SportsLeague"/><prov:wasDerivedFrom rdf:resource="http://mappings.dbpedia.org/index.php/OntologyClass:VideogamesLeague"/>
        </owl:Class><owl:Class rdf:about="http://dbpedia.org/ontology/CricketGround">
        <rdfs:label xml:lang="nl">cricketveld</rdfs:label><rdfs:label xml:lang="ur">کرکٹ کا میدان</rdfs:label><rdfs:label xml:lang="it">campo da cricket</rdfs:label><rdfs:label xml:lang="en">cricket ground</rdfs:label><rdfs:label xml:lang="de">Cricketfeld</rdfs:label><rdfs:subClassOf rdf:resource="http://dbpedia.org/ontology/SportFacility"/><prov:wasDerivedFrom rdf:resource="http://mappings.dbpedia.org/index.php/OntologyClass:CricketGround"/>
        </owl:Class><owl:Class rdf:about="http://dbpedia.org/ontology/DTMRacer">
        <rdfs:label xml:lang="en">DTM racer</rdfs:label><rdfs:label xml:lang="nl">DTM-coureur</rdfs:label><rdfs:label xml:lang="de">DTM Rennfahrer</rdfs:label><rdfs:label xml:lang="ur">جرمن ٹورنگ کار ماسٹرزریسر</rdfs:label><rdfs:subClassOf rdf:resource="http://dbpedia.org/ontology/RacingDriver"/><prov:wasDerivedFrom rdf:resource="http://mappings.dbpedia.org/index.php/OntologyClass:DTMRacer"/>
        </owl:Class><owl:Class rdf:about="http://dbpedia.org/ontology/HistoricalDistrict">
        <rdfs:label xml:lang="nl">voormalig kwartier of district</rdfs:label><rdfs:label xml:lang="ur">تاریخی ضلع</rdfs:label><rdfs:label xml:lang="ga">ceantar stairiúil</rdfs:label><rdfs:label xml:lang="fr">ancien département</rdfs:label><rdfs:label xml:lang="en">Historical district</rdfs:label><rdfs:label xml:lang="de">historischer Kreis / Bezirk</rdfs:label><rdfs:comment xml:lang="en">a place which used to be a district.</rdfs:comment><rdfs:comment xml:lang="ur">یک ایسی جگہ جو پہلے ضلع ہوتی تھی۔</rdfs:comment><rdfs:subClassOf rdf:resource="http://dbpedia.org/ontology/District"/><prov:wasDerivedFrom rdf:resource="http://mappings.dbpedia.org/index.php/OntologyClass:HistoricalDistrict"/>
        </owl:Class><owl:Class rdf:about="http://dbpedia.org/ontology/Company">
        <rdfs:label xml:lang="pt">empresa</rdfs:label><rdfs:label xml:lang="nl">bedrijf</rdfs:label><rdfs:label xml:lang="el">εταιρία</rdfs:label><rdfs:label xml:lang="ko">회사</rdfs:label><rdfs:label xml:lang="ur">تِجارتی اِدارہ</rdfs:label><rdfs:label xml:lang="ga">comhlacht</rdfs:label><rdfs:label xml:lang="fr">entreprise</rdfs:label><rdfs:label xml:lang="es">empresa</rdfs:label><rdfs:label xml:lang="en">company</rdfs:label><rdfs:label xml:lang="da">firma</rdfs:label><rdfs:label xml:lang="ja">会社</rdfs:label><rdfs:label xml:lang="de">Unternehmen</rdfs:label><rdfs:subClassOf rdf:resource="http://dbpedia.org/ontology/Organisation"/><owl:equivalentClass rdf:resource="http://www.wikidata.org/entity/Q4830453"/><prov:wasDerivedFrom rdf:resource="http://mappings.dbpedia.org/index.php/OntologyClass:Company"/>
        </owl:Class><owl:Class rdf:about="http://dbpedia.org/ontology/Locomotive">
        <rdfs:label xml:lang="nl">locomotief</rdfs:label><rdfs:label xml:lang="el">κινητήριος</rdfs:label><rdfs:label xml:lang="ur">ریل گاڑی کا انجن</rdfs:label><rdfs:label xml:lang="ga">traen</rdfs:label><rdfs:label xml:lang="fr">locomotive</rdfs:label><rdfs:label xml:lang="en">locomotive</rdfs:label><rdfs:label xml:lang="ja">機関車</rdfs:label><rdfs:label xml:lang="de">Lokomotive</rdfs:label><rdfs:subClassOf rdf:resource="http://dbpedia.org/ontology/MeanOfTransportation"/><rdfs:subClassOf rdf:resource="http://schema.org/Product"/><owl:equivalentClass rdf:resource="http://www.wikidata.org/entity/Q93301"/><prov:wasDerivedFrom rdf:resource="http://mappings.dbpedia.org/index.php/OntologyClass:Locomotive"/>
        </owl:Class><owl:Class rdf:about="http://dbpedia.org/ontology/MotocycleRacer">
        <rdfs:label xml:lang="nl">motorcoureur</rdfs:label><rdfs:label xml:lang="el">οδηγός αγώνων μοτοσυκλέτας</rdfs:label><rdfs:label xml:lang="ur">موٹر سائیکل دوڑانے والا</rdfs:label><rdfs:label xml:lang="en">motocycle racer</rdfs:label><rdfs:label xml:lang="de">Motorrad-Rennfahrer</rdfs:label><rdfs:subClassOf rdf:resource="http://dbpedia.org/ontology/MotorcycleRider"/><prov:wasDerivedFrom rdf:resource="http://mappings.dbpedia.org/index.php/OntologyClass:MotocycleRacer"/>
        </owl:Class><owl:Class rdf:about="http://dbpedia.org/ontology/Wrestler">
        <rdfs:label xml:lang="nl">worstelaar</rdfs:label><rdfs:label xml:lang="el">παλαιστής</rdfs:label><rdfs:label xml:lang="ur">پہلوان</rdfs:label><rdfs:label xml:lang="ga">coraí</rdfs:label><rdfs:label xml:lang="fr">lutteur</rdfs:label><rdfs:label xml:lang="en">wrestler</rdfs:label><rdfs:label xml:lang="ja">レスラー</rdfs:label><rdfs:label xml:lang="de">Ringer</rdfs:label><rdfs:subClassOf rdf:resource="http://dbpedia.org/ontology/Athlete"/><owl:equivalentClass rdf:resource="http://www.wikidata.org/entity/Q13474373"/><prov:wasDerivedFrom rdf:resource="http://mappings.dbpedia.org/index.php/OntologyClass:Wrestler"/>
        </owl:Class><owl:Class rdf:about="http://dbpedia.org/ontology/GolfTournament">
        <rdfs:label xml:lang="nl">golf toernooi</rdfs:label><rdfs:label xml:lang="ur">گولف کا باہمی مقابلہ</rdfs:label><rdfs:label xml:lang="ga">comórtas gailf</rdfs:label><rdfs:label xml:lang="fr">tournoi de golf</rdfs:label><rdfs:label xml:lang="it">torneo di golf</rdfs:label><rdfs:label xml:lang="en">golf tournament</rdfs:label><rdfs:label xml:lang="de">Golfturnier</rdfs:label><rdfs:subClassOf rdf:resource="http://dbpedia.org/ontology/Tournament"/><owl:equivalentClass rdf:resource="http://www.wikidata.org/entity/Q15061650"/><prov:wasDerivedFrom rdf:resource="http://mappings.dbpedia.org/index.php/OntologyClass:GolfTournament"/>
        </owl:Class><owl:Class rdf:about="http://dbpedia.org/ontology/Treaty">
        <rdfs:label xml:lang="nl">verdrag</rdfs:label><rdfs:label xml:lang="ur">معاہدہ</rdfs:label><rdfs:label xml:lang="fr">traité</rdfs:label><rdfs:label xml:lang="en">treaty</rdfs:label><rdfs:label xml:lang="ja">条約</rdfs:label><rdfs:label xml:lang="de">Vertrag</rdfs:label><rdfs:subClassOf rdf:resource="http://dbpedia.org/ontology/WrittenWork"/><prov:wasDerivedFrom rdf:resource="http://mappings.dbpedia.org/index.php/OntologyClass:Treaty"/>
        </owl:Class><owl:Class rdf:about="http://dbpedia.org/ontology/MotorcycleRacingLeague">
        <rdfs:label xml:lang="ur">موٹر سائیکل ریسنگ لیگ</rdfs:label><rdfs:label xml:lang="en">motorcycle racing league</rdfs:label><rdfs:comment xml:lang="ur">کھیلوں کی ٹیموں یا بائیک سواروں کا ایک گروپ جو موٹر سائیکل ریسنگ میں ایک دوسرے سے مقابلہ کرتے ہیں</rdfs:comment><rdfs:comment xml:lang="en">a group of sports teams or bikerider that compete against each other in Motorcycle Racing</rdfs:comment><rdfs:subClassOf rdf:resource="http://dbpedia.org/ontology/SportsLeague"/><prov:wasDerivedFrom rdf:resource="http://mappings.dbpedia.org/index.php/OntologyClass:MotorcycleRacingLeague"/>
        </owl:Class><owl:Class rdf:about="http://dbpedia.org/ontology/Sales">
        <rdfs:label xml:lang="nl">verkoop</rdfs:label><rdfs:label xml:lang="el">εκπτώσεις</rdfs:label><rdfs:label xml:lang="ur">فروخت</rdfs:label><rdfs:label xml:lang="ga">díolacháin</rdfs:label><rdfs:label xml:lang="fr">vente</rdfs:label><rdfs:label xml:lang="en">sales</rdfs:label><rdfs:label xml:lang="ja">販売</rdfs:label><rdfs:label xml:lang="de">Vertrieb</rdfs:label><rdfs:subClassOf rdf:resource="http://dbpedia.org/ontology/Activity"/><owl:equivalentClass rdf:resource="http://www.wikidata.org/entity/Q194189"/><prov:wasDerivedFrom rdf:resource="http://mappings.dbpedia.org/index.php/OntologyClass:Sales"/>
        </owl:Class><owl:Class rdf:about="http://dbpedia.org/ontology/AdultActor">
        <rdfs:label xml:lang="pl">aktor pornograficzny</rdfs:label><rdfs:label xml:lang="pt">ator adulto</rdfs:label><rdfs:label xml:lang="zh">色情演員</rdfs:label><rdfs:label xml:lang="nl">pornografisch acteur</rdfs:label><rdfs:label xml:lang="el">ενήλικας (πορνογραφικός) ηθοποιός</rdfs:label><rdfs:label xml:lang="ko">성인 배우</rdfs:label><rdfs:label xml:lang="ur">بالغ اداکار</rdfs:label><rdfs:label xml:lang="ga">aisteoir pornagrafaíochta</rdfs:label><rdfs:label xml:lang="fr">acteur porno/acteur adulte</rdfs:label><rdfs:label xml:lang="es">actor porno</rdfs:label><rdfs:label xml:lang="gl">actor porno</rdfs:label><rdfs:label xml:lang="it">attore porno</rdfs:label><rdfs:label xml:lang="en">adult (pornographic) actor</rdfs:label><rdfs:label xml:lang="ja">ポルノ女優</rdfs:label><rdfs:label xml:lang="de">pornographischer Schauspieler</rdfs:label><rdfs:comment xml:lang="en">A pornographic actor or actress or a porn star is a person who performs sex acts in film, normally characterised as a pornographic film.</rdfs:comment><rdfs:comment xml:lang="gl">Un actor ou unha actriz porno ou pornográfico/a, é un actor ou actriz de cine porno que actúa en películas de temática pornográfica..&amp;lt;ref&amp;gt;https://gl.wikipedia.org/wiki/Actor_pornogr%C3%A1fico&amp;lt;/ref&amp;gt;</rdfs:comment><rdfs:comment xml:lang="ur">ایک فحش اداکار یا اداکارہ یا پورن سٹار وہ شخص ہوتا ہے جو فلم میں جنسی حرکتیں کرتا ہے، عام طور پر اسے فحش فلم کے طور پر دیکھا جاتا ہے۔</rdfs:comment><rdfs:subClassOf rdf:resource="http://dbpedia.org/ontology/Actor"/><owl:equivalentClass rdf:resource="http://www.wikidata.org/entity/Q488111"/><prov:wasDerivedFrom rdf:resource="http://mappings.dbpedia.org/index.php/OntologyClass:AdultActor"/>
        </owl:Class><owl:Class rdf:about="http://dbpedia.org/ontology/WikimediaTemplate">
        <rdfs:label xml:lang="en">Wikimedia template</rdfs:label><rdfs:label xml:lang="ur">ویکی میڈیا کا سانچہ</rdfs:label><rdfs:label xml:lang="de">Wikimedia-Vorlage</rdfs:label><rdfs:label xml:lang="fr">modèle de Wikimedia</rdfs:label><rdfs:comment xml:lang="en">DO NOT USE THIS CLASS! This is for internal use only!</rdfs:comment><rdfs:comment xml:lang="ur">!اس کلاس کو استعمال نہ کریں! یہ صرف اندرونی استعمال کے لیے ہے</rdfs:comment><rdfs:comment xml:lang="fr">NE PAS UTILISER CETTE CLASSE! Usage interne réservé uniquement!</rdfs:comment><rdfs:subClassOf rdf:resource="http://dbpedia.org/ontology/Unknown"/><owl:equivalentClass rdf:resource="http://www.wikidata.org/entity/Q11266439"/><prov:wasDerivedFrom rdf:resource="http://mappings.dbpedia.org/index.php/OntologyClass:WikimediaTemplate"/>
        </owl:Class><owl:Class rdf:about="http://dbpedia.org/ontology/GridironFootballPlayer">
        <rdfs:label xml:lang="nl">Gridiron voetballer</rdfs:label><rdfs:label xml:lang="ur">گرڈیرون فٹ بال کھلاڑی</rdfs:label><rdfs:label xml:lang="fr">joueur de football américain gridiron</rdfs:label><rdfs:label xml:lang="en">gridiron football player</rdfs:label><rdfs:label xml:lang="de">Gridiron Footballspieler</rdfs:label><rdfs:comment xml:lang="en">Gradiron football, also called North American football, is a family of soccer team games played primarily in the United States and Canada.</rdfs:comment><rdfs:comment xml:lang="ur">گریڈیرون فٹ بال ، جسے شمالی امریکی فٹ بال بھی کہا جاتا ہے ، فٹ بال ٹیم کھیلوں کا ایک خاندان ہے جو بنیادی طور پر ریاستہائے متحدہ اور کینیڈا میں کھیلا جاتا ہے</rdfs:comment><rdfs:subClassOf rdf:resource="http://dbpedia.org/ontology/Athlete"/><owl:equivalentClass rdf:resource="http://www.wikidata.org/entity/Q14128148"/><prov:wasDerivedFrom rdf:resource="http://mappings.dbpedia.org/index.php/OntologyClass:GridironFootballPlayer"/>
        </owl:Class><owl:Class rdf:about="http://dbpedia.org/ontology/Engine">
        <rdfs:label xml:lang="nl">motor</rdfs:label><rdfs:label xml:lang="ur">انجن</rdfs:label><rdfs:label xml:lang="fr">moteur</rdfs:label><rdfs:label xml:lang="en">engine</rdfs:label><rdfs:label xml:lang="ja">機関 (機械)</rdfs:label><rdfs:label xml:lang="de">Motor</rdfs:label><rdfs:subClassOf rdf:resource="http://dbpedia.org/ontology/Device"/><prov:wasDerivedFrom rdf:resource="http://mappings.dbpedia.org/index.php/OntologyClass:Engine"/>
        </owl:Class><owl:Class rdf:about="http://dbpedia.org/ontology/ChristianDoctrine">
        <rdfs:label xml:lang="nl">Christelijke leer</rdfs:label><rdfs:label xml:lang="el">Χριστιανικό Δόγμα</rdfs:label><rdfs:label xml:lang="ko">기독교 교리</rdfs:label><rdfs:label xml:lang="ur">عیسائی نظریہ</rdfs:label><rdfs:label xml:lang="fr">doctrine chrétienne</rdfs:label><rdfs:label xml:lang="it">dottrina cristiana</rdfs:label><rdfs:label xml:lang="en">Christian Doctrine</rdfs:label><rdfs:label xml:lang="de">Christliche Lehre</rdfs:label><rdfs:comment xml:lang="en">Tenets of the Christian faith, e.g. Trinity, Nicene Creed</rdfs:comment><rdfs:comment xml:lang="ur">عیسائی عقیدے کے اصول، جیسے تثلیث، نیکین عقیدہ</rdfs:comment><rdfs:subClassOf rdf:resource="http://dbpedia.org/ontology/TheologicalConcept"/><prov:wasDerivedFrom rdf:resource="http://mappings.dbpedia.org/index.php/OntologyClass:ChristianDoctrine"/>
        </owl:Class><owl:Class rdf:about="http://dbpedia.org/ontology/Area">
        <rdfs:label xml:lang="nl">gebied</rdfs:label><rdfs:label xml:lang="el">εμβαδόν</rdfs:label><rdfs:label xml:lang="ur">رقبہ</rdfs:label><rdfs:label xml:lang="ga">ceantar</rdfs:label><rdfs:label xml:lang="fr">aire</rdfs:label><rdfs:label xml:lang="en">area</rdfs:label><rdfs:label xml:lang="ja">面積</rdfs:label><rdfs:label xml:lang="de">Bereich</rdfs:label><rdfs:comment xml:lang="en">Area of something. Use &quot;value&quot; for the value, &quot;min&quot; &amp; &quot;max&quot; for a range (if uncertain) and &quot;rank&quot; (integer) for the rank of that thing amongst its siblings (eg regions ordered by area)</rdfs:comment><rdfs:comment xml:lang="ur">کسی چیز کا علاقہ</rdfs:comment><rdfs:comment xml:lang="fr">Mesure d'une surface.</rdfs:comment><rdfs:comment xml:lang="el">Εμβαδόν ή έκταση είναι το μέγεθος μέτρησης των επιφανειών.</rdfs:comment><rdfs:subClassOf rdf:resource="http://www.w3.org/2002/07/owl#Thing"/><prov:wasDerivedFrom rdf:resource="http://mappings.dbpedia.org/index.php/OntologyClass:Area"/>
        </owl:Class><owl:Class rdf:about="http://dbpedia.org/ontology/NationalAnthem">
        <rdfs:label xml:lang="nl">volkslied</rdfs:label><rdfs:label xml:lang="ur">قومی ترانہ</rdfs:label><rdfs:label xml:lang="ga">amhrán náisiúnta</rdfs:label><rdfs:label xml:lang="fr">Hymne national</rdfs:label><rdfs:label xml:lang="en">National anthem</rdfs:label><rdfs:label xml:lang="de">Nationalhymne</rdfs:label><rdfs:comment xml:lang="en">Patriotic musical composition which is the offcial national song.</rdfs:comment><rdfs:comment xml:lang="ur">محب وطن موسیقی کی ساخت جو سرکاری قومی گانا ہے۔</rdfs:comment><rdfs:subClassOf rdf:resource="http://dbpedia.org/ontology/MusicalWork"/><owl:equivalentClass rdf:resource="http://www.wikidata.org/entity/Q23691"/><prov:wasDerivedFrom rdf:resource="http://mappings.dbpedia.org/index.php/OntologyClass:NationalAnthem"/>
        </owl:Class><owl:Class rdf:about="http://dbpedia.org/ontology/SoccerLeague">
        <rdfs:label xml:lang="nl">voetbal competitie</rdfs:label><rdfs:label xml:lang="el">Ομοσπονδία Ποδοσφαίρου</rdfs:label><rdfs:label xml:lang="ur">فٹ بال کی انجمن</rdfs:label><rdfs:label xml:lang="ga">sraith sacair</rdfs:label><rdfs:label xml:lang="fr">ligue de football</rdfs:label><rdfs:label xml:lang="en">soccer league</rdfs:label><rdfs:label xml:lang="ja">サッカーリーグ</rdfs:label><rdfs:label xml:lang="de">Fußball Liga</rdfs:label><rdfs:comment xml:lang="en">A group of sports teams that compete against each other in soccer.</rdfs:comment><rdfs:comment xml:lang="ur">کھیلوں کی ٹیموں کا ایک گروپ جو فٹ بال میں ایک دوسرے کے خلاف مقابلہ کرتا ہے۔</rdfs:comment><rdfs:subClassOf rdf:resource="http://dbpedia.org/ontology/SportsLeague"/><prov:wasDerivedFrom rdf:resource="http://mappings.dbpedia.org/index.php/OntologyClass:SoccerLeague"/>
        </owl:Class><owl:Class rdf:about="http://dbpedia.org/ontology/Battery">
        <rdfs:label xml:lang="pt">bateria</rdfs:label><rdfs:label xml:lang="nl">batterij</rdfs:label><rdfs:label xml:lang="ur">برقی طاقت پیدا کرنے کا آلہ</rdfs:label><rdfs:label xml:lang="fr">pile</rdfs:label><rdfs:label xml:lang="es">batería</rdfs:label><rdfs:label xml:lang="it">batteria</rdfs:label><rdfs:label xml:lang="en">battery</rdfs:label><rdfs:label xml:lang="de">Batterie</rdfs:label><rdfs:comment xml:lang="en">The battery (type) used as energy source in vehicles.</rdfs:comment><rdfs:comment xml:lang="ur">بیٹری (قسم) گاڑیوں میں توانائی کے منبع کے طور پر استعمال ہوتی ہے۔.</rdfs:comment><rdfs:subClassOf rdf:resource="http://dbpedia.org/ontology/Device"/><owl:equivalentClass rdf:resource="http://www.wikidata.org/entity/Q267298"/><prov:wasDerivedFrom rdf:resource="http://mappings.dbpedia.org/index.php/OntologyClass:Battery"/>
        </owl:Class><owl:Class rdf:about="http://dbpedia.org/ontology/AcademicConference">
        <rdfs:label xml:lang="pl">konferencja naukowa</rdfs:label><rdfs:label xml:lang="nl">wetenschappelijke conferentie</rdfs:label><rdfs:label xml:lang="be">навуковая канферэнцыя</rdfs:label><rdfs:label xml:lang="ur">تعلیمی_کانفرنس</rdfs:label><rdfs:label xml:lang="fr">conférence scientifique</rdfs:label><rdfs:label xml:lang="it">congresso scientifico</rdfs:label><rdfs:label xml:lang="ru">научная конференция</rdfs:label><rdfs:label xml:lang="en">academic conference</rdfs:label><rdfs:label xml:lang="ja">学術会議</rdfs:label><rdfs:label xml:lang="de">wissenschaftliche Konferenz</rdfs:label><rdfs:subClassOf rdf:resource="http://dbpedia.org/ontology/SocietalEvent"/><owl:equivalentClass rdf:resource="http://www.wikidata.org/entity/Q2020153"/><prov:wasDerivedFrom rdf:resource="http://mappings.dbpedia.org/index.php/OntologyClass:AcademicConference"/>
        </owl:Class><owl:Class rdf